# baseURI: https://spec.edmcouncil.org/fibo/ontology/master/2021Q4/FND/Relations/Relations/
# imports: https://spec.edmcouncil.org/fibo/ontology/master/2021Q4/FND/AgentsAndPeople/Agents/
# imports: https://spec.edmcouncil.org/fibo/ontology/master/2021Q4/FND/Utilities/AnnotationVocabulary/
# imports: https://www.omg.org/spec/LCC/Countries/CountryRepresentation/
# imports: https://www.omg.org/spec/LCC/Languages/LanguageRepresentation/

@base <https://spec.edmcouncil.org/fibo/ontology/master/2021Q4/FND/Relations/Relations/> .
@prefix dct: <http://purl.org/dc/terms/> .
@prefix fibo-fnd-aap-agt: <https://spec.edmcouncil.org/fibo/ontology/FND/AgentsAndPeople/Agents/> .
@prefix fibo-fnd-rel-rel: <https://spec.edmcouncil.org/fibo/ontology/FND/Relations/Relations/> .
@prefix fibo-fnd-utl-av: <https://spec.edmcouncil.org/fibo/ontology/FND/Utilities/AnnotationVocabulary/> .
@prefix lcc-cr: <https://www.omg.org/spec/LCC/Countries/CountryRepresentation/> .
@prefix lcc-lr: <https://www.omg.org/spec/LCC/Languages/LanguageRepresentation/> .
@prefix owl: <http://www.w3.org/2002/07/owl#> .
@prefix rdf: <http://www.w3.org/1999/02/22-rdf-syntax-ns#> .
@prefix rdfs: <http://www.w3.org/2000/01/rdf-schema#> .
@prefix skos: <http://www.w3.org/2004/02/skos/core#> .
@prefix sm: <http://www.omg.org/techprocess/ab/SpecificationMetadata/> .
@prefix xsd: <http://www.w3.org/2001/XMLSchema#> .

<https://spec.edmcouncil.org/fibo/ontology/FND/Relations/Relations/>
	a owl:Ontology ;
	rdfs:label "Relations Ontology" ;
	dct:abstract "This ontology defines a set of general purpose relations for use in other FIBO ontology elements.  These include a number of properties required for reuse across the foundations and business entities models." ;
	dct:license "http://opensource.org/licenses/MIT"^^xsd:anyURI ;
	sm:contentLanguage <https://www.w3.org/TR/owl2-quick-reference/> ;
	sm:copyright
		"Copyright (c) 2013-2021 EDM Council, Inc." ,
		"Copyright (c) 2013-2021 Object Management Group, Inc."
		;
	sm:dependsOn
		"https://spec.edmcouncil.org/fibo/ontology/FND/AgentsAndPeople/Agents/"^^xsd:anyURI ,
		"https://spec.edmcouncil.org/fibo/ontology/FND/Utilities/AnnotationVocabulary/"^^xsd:anyURI ,
		"https://www.omg.org/spec/LCC/"^^xsd:anyURI
		;
	sm:fileAbbreviation "fibo-fnd-rel-rel" ;
	sm:filename "Relations.rdf" ;
	owl:imports
		<https://spec.edmcouncil.org/fibo/ontology/master/2021Q4/FND/AgentsAndPeople/Agents/> ,
		<https://spec.edmcouncil.org/fibo/ontology/master/2021Q4/FND/Utilities/AnnotationVocabulary/> ,
		<https://www.omg.org/spec/LCC/Countries/CountryRepresentation/> ,
		<https://www.omg.org/spec/LCC/Languages/LanguageRepresentation/>
		;
	owl:versionIRI <https://spec.edmcouncil.org/fibo/ontology/master/2021Q4/FND/Relations/Relations/> ;
	skos:changeNote
		"The http://www.omg.org/spec/EDMC-FIBO/FND/20170201/Relations/Relations.rdf version of this ontology was modified per the FIBO 2.0 RFC to include additional properties and the linkage to LCC." ,
		"""The http://www.omg.org/spec/FIBO/Foundations/20130601/Relations/Relations.owl version of the ontology submitted with the FIBO FND RFC, was revised in advance of the September 2013 New Brunswick, NJ meeting, as follows:
   (1) to use slash style URI/IRIss (also called 303 URIs, vs. hash style) as required to support server side processing 
   (2) to use version-independent IRIs for all definitions internally as opposed to version-specific IRIs
   (3) to change the file suffix from .owl to .rdf to increase usability in RDF tools
   (4) to use 4-level abbreviations and corresponding namespace prefixes for all FIBO ontologies, reflecting a family/specification/module/ontology structure
   (5) to incorporate changes to the specification metadata to support documentation at the family, specification, module, and ontology level, similar to the abbreviations
   (6) to move the ontology from the Utilities module to an independent Relations module
   (7) to revise a number of definitions, per discussion with various stakeholders.
   (8) to augment the definitions to include entity names from Business Entities.""" ,
		"The https://spec.edmcouncil.org/fibo/ontology/FND/Relations/Relations.rdf version of this ontology was modified per the issue resolutions identified in the FIBO FND 1.0 FTF report and in https://spec.edmcouncil.org/fibo/ontology/FND/1.0/AboutFND-1.0/. It was further revised in FTF 2 resulting in https://spec.edmcouncil.org/fibo/ontology/FND/Relations/Relations/." ,
		"The https://spec.edmcouncil.org/fibo/ontology/FND/Relations/Relations.rdf version of this ontology was modified per the issue resolutions identified in the FIBO FND 1.2 RTF report." ,
		"The https://spec.edmcouncil.org/fibo/ontology/FND/Relations/Relations.rdf version of this ontology was modified to add Reference as a superclass of Name and use the hasTextValue property as the superproperty of certain data properties." ,
		"The https://spec.edmcouncil.org/fibo/ontology/FND/Relations/Relations.rdf version of this ontology was modified to clean up references to external dictionaries that don't meet FIBO policies, eliminate ambiguity where possible, eliminate the superproperties of produces and is produced by, whose semantics are different from their parent properties, and improve ISO 704 compliance of definitions." ,
		"The https://spec.edmcouncil.org/fibo/ontology/FND/Relations/Relations.rdf version of this ontology was modified to eliminate deprecated elements." ,
		"The https://spec.edmcouncil.org/fibo/ontology/FND/Relations/Relations.rdf version of this ontology was modified to eliminate duplication with concepts in LCC and remove the unused hasDispositionDate property, whose semantics were unclear at best." ,
		"The https://spec.edmcouncil.org/fibo/ontology/FND/Relations/Relations.rdf version of this ontology was modified to incorporate evaluates and isEvaluatedBy, and to loosen constraints on hasName properties to allow multi-lingual names." ,
		"The https://spec.edmcouncil.org/fibo/ontology/FND/Relations/Relations.rdf version of this ontology was modified to loosen constraints on properties using xsd:dateTime in their range to allow for more flexible representation, and to add properties including produces, isProducedBy." ,
		"The https://spec.edmcouncil.org/fibo/ontology/FND/Relations/Relations.rdf version of this ontology was modified to move hasAcquisitionDate to Financial Dates to improve usability and simplify reasoning, to eliminate circular definitions, to deprecate fibo-fnd-rel-rel;hasTag in favor of the simpler LCC property of the same name, to loosen domain restrictions on some properties which were too narrowly specified, and to add two new properties, describes and isDescribedBy, which are more appropriate for certain cases where we were using characterizes and isCharacterizedBy." ,
		"The https://spec.edmcouncil.org/fibo/ontology/FND/Relations/Relations.rdf version of this ontology was modified to move the property 'exchanges' to FND given that it could be applied more generally than with respect to swaps only." ,
		"The https://spec.edmcouncil.org/fibo/ontology/FND/Relations/Relations.rdf version of this ontology was modified to rename (migrate) the hasDefinition property to isDefinedIn." ,
		"The https://spec.edmcouncil.org/fibo/ontology/FND/Relations/Relations.rdf version of this ontology was revised to add the appliesTo object property in support of the IND RFC."
		;
	fibo-fnd-utl-av:hasMaturityLevel fibo-fnd-utl-av:Release ;
	.

fibo-fnd-aap-agt:Name
	a owl:Class ;
	rdfs:subClassOf fibo-fnd-rel-rel:Reference ;
	.

fibo-fnd-rel-rel:Reference
	a owl:Class ;
	rdfs:label "reference" ;
	rdfs:isDefinedBy <https://spec.edmcouncil.org/fibo/ontology/FND/Relations/Relations/> ;
	skos:definition "concept that stands in for how something may be interpreted/understood in some context" ;
	fibo-fnd-utl-av:explanatoryNote "In linguistics, a reference characterizes, provides context for, or specifies the relationship of one linguistic expression to another, i.e., provides the information necessary to interpret the dependent expression." ;
	.

fibo-fnd-rel-rel:Referent
	a owl:Class ;
	rdfs:label "referent" ;
	rdfs:isDefinedBy <https://spec.edmcouncil.org/fibo/ontology/FND/Relations/Relations/> ;
	skos:definition "something that another concept stands for, exemplifies, symbolizes, or otherwise mentions" ;
	.

fibo-fnd-rel-rel:appliesTo
	a owl:ObjectProperty ;
	rdfs:subPropertyOf fibo-fnd-rel-rel:refersTo ;
	rdfs:label "applies to" ;
	rdfs:isDefinedBy <https://spec.edmcouncil.org/fibo/ontology/FND/Relations/Relations/> ;
	skos:definition "is pertinent, suitable, or relevant to" ;
	.

fibo-fnd-rel-rel:causes
	a owl:ObjectProperty ;
	rdfs:label "causes" ;
	rdfs:isDefinedBy <https://spec.edmcouncil.org/fibo/ontology/FND/Relations/Relations/> ;
	skos:definition "relationship between an event or set of events or factors (the cause) and a second event, phenomenon, situation, or result (the effect), where the second event or outcome is understood as a consequence of the first" ;
	.

fibo-fnd-rel-rel:characterizes
	a owl:ObjectProperty ;
	rdfs:subPropertyOf fibo-fnd-rel-rel:appliesTo ;
	rdfs:label "characterizes" ;
	rdfs:isDefinedBy <https://spec.edmcouncil.org/fibo/ontology/FND/Relations/Relations/> ;
	skos:definition "specifies a discriminating feature or quality of" ;
	.

fibo-fnd-rel-rel:comprises
	a owl:ObjectProperty ;
	rdfs:label "comprises" ;
	rdfs:isDefinedBy <https://spec.edmcouncil.org/fibo/ontology/FND/Relations/Relations/> ;
	skos:definition "includes, especially within a particular scope" ;
	fibo-fnd-utl-av:usageNote "Note that something can be comprised of something(s) that may or may not be understood as separable parts, and thus is not defined as being explicitly transitive." ;
	.

fibo-fnd-rel-rel:confers
	a owl:ObjectProperty ;
	rdfs:label "confers" ;
	rdfs:isDefinedBy <https://spec.edmcouncil.org/fibo/ontology/FND/Relations/Relations/> ;
	skos:definition "grants or bestows by virtue of some authority" ;
	fibo-fnd-utl-av:explanatoryNote "This property should be read as describing the conferral of some legal power or duty, some commitment or some social construct, and is a property of some social construct such as an agreement or some legal authority. These concepts, which would describe the kind of thing of which this is a property, and the kinds of thing in terms of which this property is framed, are outside the scope of this mode land so are not shown." ;
	fibo-fnd-utl-av:synonym "invests with" ;
	.

fibo-fnd-rel-rel:controls
	a owl:ObjectProperty ;
	rdfs:label "controls" ;
	rdfs:isDefinedBy <https://spec.edmcouncil.org/fibo/ontology/FND/Relations/Relations/> ;
	skos:definition "exercises authority or influence over" ;
	.

fibo-fnd-rel-rel:defines
	a owl:ObjectProperty ;
	rdfs:subPropertyOf fibo-fnd-rel-rel:represents ;
	rdfs:label "defines" ;
	rdfs:isDefinedBy <https://spec.edmcouncil.org/fibo/ontology/FND/Relations/Relations/> ;
	skos:definition "identifies the essential qualities of, specifies the meaning of, fixes the limits of, demarcates" ;
	.

fibo-fnd-rel-rel:describes
	a owl:ObjectProperty ;
	rdfs:subPropertyOf fibo-fnd-rel-rel:appliesTo ;
	rdfs:label "describes" ;
	rdfs:isDefinedBy <https://spec.edmcouncil.org/fibo/ontology/FND/Relations/Relations/> ;
	skos:definition "conveys the nature of" ;
	.

fibo-fnd-rel-rel:designates
	a owl:ObjectProperty ;
	rdfs:label "designates" ;
	rdfs:isDefinedBy <https://spec.edmcouncil.org/fibo/ontology/FND/Relations/Relations/> ;
	skos:definition "appoints someone officially" ;
	fibo-fnd-utl-av:explanatoryNote "This property is intended to cover assigning a job or role to someone, selecting or designating someone to fill an office or a position, and fixing or setting by authority or by mutual agreement." ;
	.

fibo-fnd-rel-rel:embodies
	a owl:ObjectProperty ;
	rdfs:label "embodies" ;
	rdfs:isDefinedBy <https://spec.edmcouncil.org/fibo/ontology/FND/Relations/Relations/> ;
	skos:definition "is an expression of, gives a tangible or visible form to (an idea, quality, or feeling), makes concrete and perceptible" ;
	.

fibo-fnd-rel-rel:evaluates
	a owl:ObjectProperty ;
	rdfs:subPropertyOf fibo-fnd-rel-rel:appliesTo ;
	rdfs:label "evaluates" ;
	rdfs:isDefinedBy <https://spec.edmcouncil.org/fibo/ontology/FND/Relations/Relations/> ;
	skos:definition "assesses the nature, quality, or ability of someone or something" ;
	.

fibo-fnd-rel-rel:exchanges
	a owl:ObjectProperty ;
	rdfs:label "exchanges" ;
	rdfs:isDefinedBy <https://spec.edmcouncil.org/fibo/ontology/FND/Relations/Relations/> ;
	skos:definition "gives something in return something else" ;
	.

fibo-fnd-rel-rel:generates
	a owl:ObjectProperty ;
	rdfs:label "generates" ;
	rdfs:isDefinedBy <https://spec.edmcouncil.org/fibo/ontology/FND/Relations/Relations/> ;
	skos:definition "produces through the application of one or more mathematical or logical steps or rules" ;
	.

fibo-fnd-rel-rel:governs
	a owl:ObjectProperty ;
	rdfs:label "governs" ;
	rdfs:isDefinedBy <https://spec.edmcouncil.org/fibo/ontology/FND/Relations/Relations/> ;
	skos:definition "has and exercises authority over, regulates" ;
	.

fibo-fnd-rel-rel:hasAlias
	a owl:DatatypeProperty ;
	rdfs:subPropertyOf
		fibo-fnd-aap-agt:hasTextValue ,
		lcc-lr:hasName
		;
	rdfs:label "has alias" ;
	rdfs:isDefinedBy <https://spec.edmcouncil.org/fibo/ontology/FND/Relations/Relations/> ;
	skos:definition "indicates an alternate name of by which something is known" ;
	.

fibo-fnd-rel-rel:hasCommonName
	a owl:DatatypeProperty ;
	rdfs:subPropertyOf
		fibo-fnd-aap-agt:hasTextValue ,
		lcc-lr:hasName
		;
	rdfs:label "has common name" ;
	rdfs:isDefinedBy <https://spec.edmcouncil.org/fibo/ontology/FND/Relations/Relations/> ;
	skos:definition "indicates a name by which something is frequently referred, without reference to any formal usage or structure" ;
	.

fibo-fnd-rel-rel:hasContext
	a owl:ObjectProperty ;
	rdfs:subPropertyOf lcc-lr:has ;
	rdfs:label "has context" ;
	rdfs:isDefinedBy <https://spec.edmcouncil.org/fibo/ontology/FND/Relations/Relations/> ;
	skos:definition "indicates the setting in which something is defined, expressed, or represented" ;
	.

fibo-fnd-rel-rel:hasDesignation
	a owl:ObjectProperty ;
	rdfs:label "has designation" ;
	rdfs:domain fibo-fnd-aap-agt:AutonomousAgent ;
	rdfs:isDefinedBy <https://spec.edmcouncil.org/fibo/ontology/FND/Relations/Relations/> ;
	skos:definition "relates an individual or organization to a position, role, or other designation" ;
	.

fibo-fnd-rel-rel:hasFormalName
	a owl:DatatypeProperty ;
	rdfs:subPropertyOf
		fibo-fnd-aap-agt:hasTextValue ,
		lcc-lr:hasName
		;
	rdfs:label "has formal name" ;
	rdfs:isDefinedBy <https://spec.edmcouncil.org/fibo/ontology/FND/Relations/Relations/> ;
	skos:definition "indicates a name by which something is known for some official purpose or context, or which is structured in some way such as to always follow the same format regardless of usage" ;
	.

fibo-fnd-rel-rel:hasIdentity
	a owl:ObjectProperty ;
	rdfs:subPropertyOf lcc-lr:has ;
	rdfs:label "has identity" ;
	rdfs:isDefinedBy <https://spec.edmcouncil.org/fibo/ontology/FND/Relations/Relations/> ;
	skos:definition "provides a means for identifying something that fills a particular role" ;
	fibo-fnd-utl-av:explanatoryNote "This property should be read as being a property of some kind of 'relative thing' as defined externality to this ontology. The property is usually but not exclusively framed with reference to some 'independent thing' but may take other forms and so should be regarded as having a target of 'thing'." ;
	.

fibo-fnd-rel-rel:hasLegalName
	a owl:DatatypeProperty ;
	rdfs:subPropertyOf fibo-fnd-rel-rel:hasFormalName ;
	rdfs:label "has legal name" ;
	rdfs:isDefinedBy <https://spec.edmcouncil.org/fibo/ontology/FND/Relations/Relations/> ;
	skos:definition "specifies the name used to refer to a party in legal communications" ;
	.

fibo-fnd-rel-rel:hasRepresentation
	a owl:ObjectProperty ;
	rdfs:subPropertyOf lcc-lr:has ;
	rdfs:label "has representation" ;
	rdfs:isDefinedBy <https://spec.edmcouncil.org/fibo/ontology/FND/Relations/Relations/> ;
	skos:definition "relates a concept to some textual or other symbol which is intended to convey the sense of that concept or to some form of words which sets out the meaning of that concept" ;
	.

fibo-fnd-rel-rel:hasTag
	a owl:DatatypeProperty ;
	rdfs:label "has tag" ;
	rdfs:isDefinedBy <https://spec.edmcouncil.org/fibo/ontology/FND/Relations/Relations/> ;
	rdfs:range [
		a rdfs:Datatype ;
		owl:unionOf (
			xsd:string
			xsd:base64Binary
			xsd:hexBinary
		) ;
	] ;
	owl:deprecated "true"^^xsd:boolean ;
	skos:definition "has a unique combination of alphanumeric characters or binary representation corresponding to the identifier, code, or other element to which it applies" ;
	.

fibo-fnd-rel-rel:holds
	a owl:ObjectProperty ;
	rdfs:label "holds" ;
	rdfs:isDefinedBy <https://spec.edmcouncil.org/fibo/ontology/FND/Relations/Relations/> ;
	skos:definition "is the relationship between a party and something it possesses, or over which it exercises some ownership or control or has at its discretion the ability to dispose of it as it sees fit" ;
	.

fibo-fnd-rel-rel:involves
	a owl:ObjectProperty ;
	rdfs:label "involves" ;
	rdfs:isDefinedBy <https://spec.edmcouncil.org/fibo/ontology/FND/Relations/Relations/> ;
	skos:definition "(of a situation or event) includes (something) as a necessary part or result" ;
	.

fibo-fnd-rel-rel:isCausedBy
	a owl:ObjectProperty ;
	rdfs:label "is caused by" ;
	rdfs:isDefinedBy <https://spec.edmcouncil.org/fibo/ontology/FND/Relations/Relations/> ;
	owl:inverseOf fibo-fnd-rel-rel:causes ;
	skos:definition "is the relationship between an event (the effect) and a second event (the cause), where the first event is understood as a consequence of the second; also, the relationship between a set of factors (causes) and a phenomenon (the effect)" ;
	.

fibo-fnd-rel-rel:isCharacterizedBy
	a owl:ObjectProperty ;
	rdfs:label "is characterized by" ;
	rdfs:isDefinedBy <https://spec.edmcouncil.org/fibo/ontology/FND/Relations/Relations/> ;
	owl:inverseOf fibo-fnd-rel-rel:characterizes ;
	skos:definition "indicates a quality or feature of something, distinguishing it from something else" ;
	.

fibo-fnd-rel-rel:isConferredBy
	a owl:ObjectProperty ;
	rdfs:label "is conferred by" ;
	rdfs:isDefinedBy <https://spec.edmcouncil.org/fibo/ontology/FND/Relations/Relations/> ;
	owl:inverseOf fibo-fnd-rel-rel:confers ;
	skos:definition "a relationship between a right or obligation and the vehicle, such as an agreement or contract, that vests (or confers) said right or obligation" ;
	fibo-fnd-utl-av:explanatoryNote "This property should be read as describing some legal power or duty, some commitment or some social construct being conferred as a result of some social construct such as an agreement or some legal authority. These concepts, which would describe the kind of thing of which this is a property, and the kinds of thing in terms of which this property is framed, are outside the scope of this model and so are not shown." ;
	.

fibo-fnd-rel-rel:isConferredOn
	a owl:ObjectProperty ;
	rdfs:label "is conferred on" ;
	rdfs:isDefinedBy <https://spec.edmcouncil.org/fibo/ontology/FND/Relations/Relations/> ;
	rdfs:range fibo-fnd-aap-agt:AutonomousAgent ;
	skos:definition "that on which the conferred thing is conferred" ;
	.

fibo-fnd-rel-rel:isControlledBy
	a owl:ObjectProperty ;
	rdfs:label "is controlled by" ;
	rdfs:isDefinedBy <https://spec.edmcouncil.org/fibo/ontology/FND/Relations/Relations/> ;
	owl:inverseOf fibo-fnd-rel-rel:controls ;
	skos:definition "is influenced, managed, or directed by" ;
	.

fibo-fnd-rel-rel:isDefinedIn
	a owl:ObjectProperty ;
	rdfs:subPropertyOf fibo-fnd-rel-rel:hasRepresentation ;
	rdfs:label "is defined in" ;
	rdfs:isDefinedBy <https://spec.edmcouncil.org/fibo/ontology/FND/Relations/Relations/> ;
	owl:inverseOf fibo-fnd-rel-rel:defines ;
	skos:definition "indicates something that specifies the meaning associated with the subject" ;
	fibo-fnd-utl-av:explanatoryNote "Typically, a concept, such as a classifier or identifier, will be defined in terms of a scheme, contract, specification, standard, or other reference." ;
	.

fibo-fnd-rel-rel:isDescribedBy
	a owl:ObjectProperty ;
	rdfs:label "is described by" ;
	rdfs:isDefinedBy <https://spec.edmcouncil.org/fibo/ontology/FND/Relations/Relations/> ;
	owl:inverseOf fibo-fnd-rel-rel:describes ;
	skos:definition "has general nature or description" ;
	.

fibo-fnd-rel-rel:isDesignatedBy
	a owl:ObjectProperty ;
	rdfs:label "is designated by" ;
	rdfs:isDefinedBy <https://spec.edmcouncil.org/fibo/ontology/FND/Relations/Relations/> ;
	owl:inverseOf fibo-fnd-rel-rel:designates ;
	skos:definition "indicates the party that has assigned or appointed someone to an office or position" ;
	.

fibo-fnd-rel-rel:isEvaluatedBy
	a owl:ObjectProperty ;
	rdfs:label "is evaluated by" ;
	rdfs:isDefinedBy <https://spec.edmcouncil.org/fibo/ontology/FND/Relations/Relations/> ;
	owl:inverseOf fibo-fnd-rel-rel:evaluates ;
	skos:definition "is ascertained or determined by" ;
	.

fibo-fnd-rel-rel:isGeneratedBy
	a owl:ObjectProperty ;
	rdfs:label "is generated by" ;
	rdfs:isDefinedBy <https://spec.edmcouncil.org/fibo/ontology/FND/Relations/Relations/> ;
	owl:inverseOf fibo-fnd-rel-rel:generates ;
	skos:definition "identifies some party or something that produces something via some equation, logic, or rules" ;
	.

fibo-fnd-rel-rel:isGovernedBy
	a owl:ObjectProperty ;
	rdfs:label "is governed by" ;
	rdfs:isDefinedBy <https://spec.edmcouncil.org/fibo/ontology/FND/Relations/Relations/> ;
	owl:inverseOf fibo-fnd-rel-rel:governs ;
	skos:definition "relates a contract, agreement, jurisdiction, or other legal construct and the regulation, policy, procedure, or legal person that regulates or oversees (governs) it" ;
	fibo-fnd-utl-av:explanatoryNote "This property should be read as being the property of some thing and as referring to a logical union of social construct (in the informative abstractions ontology) and legal person." ;
	.

fibo-fnd-rel-rel:isHeldBy
	a owl:ObjectProperty ;
	rdfs:label "is held by" ;
	rdfs:isDefinedBy <https://spec.edmcouncil.org/fibo/ontology/FND/Relations/Relations/> ;
	owl:inverseOf fibo-fnd-rel-rel:holds ;
	skos:definition "indicates the party that possesses and has at least partial control of something, regardless of ownership" ;
	.

fibo-fnd-rel-rel:isIncludedIn
	a owl:ObjectProperty ;
	rdfs:label "is included in" ;
	rdfs:isDefinedBy <https://spec.edmcouncil.org/fibo/ontology/FND/Relations/Relations/> ;
	owl:inverseOf fibo-fnd-rel-rel:comprises ;
	skos:definition "relates something to something that contains it" ;
	.

fibo-fnd-rel-rel:isIssuedBy
	a owl:ObjectProperty ;
	rdfs:subPropertyOf fibo-fnd-rel-rel:isProvidedBy ;
	rdfs:label "is issued by" ;
	rdfs:isDefinedBy <https://spec.edmcouncil.org/fibo/ontology/FND/Relations/Relations/> ;
	skos:definition "indicates a functional entity or party responsible for circulating, distributing, or publishing something" ;
	.

fibo-fnd-rel-rel:isManagedBy
	a owl:ObjectProperty ;
	rdfs:label "is managed by" ;
	rdfs:isDefinedBy <https://spec.edmcouncil.org/fibo/ontology/FND/Relations/Relations/> ;
	skos:definition "relates something to another thing that has some role in directing its affairs" ;
	fibo-fnd-utl-av:explanatoryNote "The target or range of this property should be read as always being some kind of 'relative thing', that is a thing defined in some context. Generally this will be a 'party in role'. This property is not intended to be used to relate a thing to some independent thing which it is managed by, only to something in the role of being that which manages it." ;
	.

fibo-fnd-rel-rel:isMandatedBy
	a owl:ObjectProperty ;
	rdfs:subPropertyOf fibo-fnd-rel-rel:isConferredBy ;
	rdfs:label "is mandated by" ;
	rdfs:isDefinedBy <https://spec.edmcouncil.org/fibo/ontology/FND/Relations/Relations/> ;
	skos:definition "relates a responsibility, capacity, or action to that which requires it" ;
	.

fibo-fnd-rel-rel:isProducedBy
	a owl:ObjectProperty ;
	rdfs:label "is produced by" ;
	rdfs:isDefinedBy <https://spec.edmcouncil.org/fibo/ontology/FND/Relations/Relations/> ;
	owl:inverseOf fibo-fnd-rel-rel:produces ;
	skos:definition "identifies the producer that fabricates, manufactures or otherwise creates something through some production process" ;
	.

fibo-fnd-rel-rel:isProvidedBy
	a owl:ObjectProperty ;
	rdfs:label "is provided by" ;
	rdfs:isDefinedBy <https://spec.edmcouncil.org/fibo/ontology/FND/Relations/Relations/> ;
	owl:inverseOf fibo-fnd-rel-rel:provides ;
	skos:definition "is made available by" ;
	fibo-fnd-utl-av:explanatoryNote "The target or range of this property should be read as always being some kind of 'relative thing', that is a thing defined in some context. Generally this will be a 'party in role'. This property is not intended to be used to relate a thing to some independent thing which it is provided by, only to something in the role of being that which provides it." ;
	.

fibo-fnd-rel-rel:issues
	a owl:ObjectProperty ;
	rdfs:subPropertyOf fibo-fnd-rel-rel:provides ;
	rdfs:label "issues" ;
	rdfs:isDefinedBy <https://spec.edmcouncil.org/fibo/ontology/FND/Relations/Relations/> ;
	owl:inverseOf fibo-fnd-rel-rel:isIssuedBy ;
	skos:definition "officially makes something available" ;
	.

fibo-fnd-rel-rel:manages
	a owl:ObjectProperty ;
	rdfs:label "manages" ;
	rdfs:isDefinedBy <https://spec.edmcouncil.org/fibo/ontology/FND/Relations/Relations/> ;
	owl:inverseOf fibo-fnd-rel-rel:isManagedBy ;
	skos:definition "relates a party to something that it directs in some way" ;
	.

fibo-fnd-rel-rel:mandates
	a owl:ObjectProperty ;
	rdfs:subPropertyOf fibo-fnd-rel-rel:confers ;
	rdfs:label "mandates" ;
	rdfs:isDefinedBy <https://spec.edmcouncil.org/fibo/ontology/FND/Relations/Relations/> ;
	owl:inverseOf fibo-fnd-rel-rel:isMandatedBy ;
	skos:definition "relates something to a commitment, contract, law, obligation, requirement, regulation, or similar concept that requires it" ;
	.

fibo-fnd-rel-rel:produces
	a owl:ObjectProperty ;
	rdfs:label "produces" ;
	rdfs:isDefinedBy <https://spec.edmcouncil.org/fibo/ontology/FND/Relations/Relations/> ;
	skos:definition "creates through a fabrication, manufacturing or production process" ;
	.

fibo-fnd-rel-rel:provides
	a owl:ObjectProperty ;
	rdfs:label "provides" ;
	rdfs:isDefinedBy <https://spec.edmcouncil.org/fibo/ontology/FND/Relations/Relations/> ;
	skos:definition "makes something available" ;
	.

fibo-fnd-rel-rel:refersTo
	a owl:ObjectProperty ;
	rdfs:label "refers to" ;
	rdfs:isDefinedBy <https://spec.edmcouncil.org/fibo/ontology/FND/Relations/Relations/> ;
	skos:definition "classifies, provides context for, or indicates" ;
	.

fibo-fnd-rel-rel:represents
	a owl:ObjectProperty ;
	rdfs:subPropertyOf fibo-fnd-rel-rel:refersTo ;
	rdfs:label "represents" ;
	rdfs:isDefinedBy <https://spec.edmcouncil.org/fibo/ontology/FND/Relations/Relations/> ;
	owl:inverseOf fibo-fnd-rel-rel:hasRepresentation ;
	skos:definition "illustrates, symbolizes, exemplifies, stands for, or means" ;
	.

fibo-fnd-rel-rel:wasFormerlyKnownAs
	a owl:DatatypeProperty ;
	rdfs:subPropertyOf
		fibo-fnd-aap-agt:hasTextValue ,
		lcc-lr:hasName
		;
	rdfs:label "was formerly known as" ;
	rdfs:isDefinedBy <https://spec.edmcouncil.org/fibo/ontology/FND/Relations/Relations/> ;
	skos:definition "indicates a name by which something was known in the past" ;
	.

lcc-cr:classifies
	a owl:ObjectProperty ;
	rdfs:subPropertyOf fibo-fnd-rel-rel:refersTo ;
	.

lcc-lr:denotes
	a owl:ObjectProperty ;
	rdfs:subPropertyOf fibo-fnd-rel-rel:represents ;
	.

lcc-lr:hasDenotation
	a owl:ObjectProperty ;
	rdfs:subPropertyOf fibo-fnd-rel-rel:hasRepresentation ;
	.

