# baseURI: https://spec.edmcouncil.org/fibo/ontology/master/2021Q4/FND/Places/Addresses/
# imports: https://spec.edmcouncil.org/fibo/ontology/master/2021Q4/FND/Arrangements/ClassificationSchemes/
# imports: https://spec.edmcouncil.org/fibo/ontology/master/2021Q4/FND/Arrangements/IdentifiersAndIndices/
# imports: https://spec.edmcouncil.org/fibo/ontology/master/2021Q4/FND/Places/Locations/
# imports: https://spec.edmcouncil.org/fibo/ontology/master/2021Q4/FND/Relations/Relations/
# imports: https://spec.edmcouncil.org/fibo/ontology/master/2021Q4/FND/Utilities/Analytics/
# imports: https://spec.edmcouncil.org/fibo/ontology/master/2021Q4/FND/Utilities/AnnotationVocabulary/
# imports: https://www.omg.org/spec/LCC/Countries/CountryRepresentation/
# imports: https://www.omg.org/spec/LCC/Languages/LanguageRepresentation/

@base <https://spec.edmcouncil.org/fibo/ontology/master/2021Q4/FND/Places/Addresses/> .
@prefix dct: <http://purl.org/dc/terms/> .
@prefix fibo-fnd-arr-cls: <https://spec.edmcouncil.org/fibo/ontology/FND/Arrangements/ClassificationSchemes/> .
@prefix fibo-fnd-arr-id: <https://spec.edmcouncil.org/fibo/ontology/FND/Arrangements/IdentifiersAndIndices/> .
@prefix fibo-fnd-plc-adr: <https://spec.edmcouncil.org/fibo/ontology/FND/Places/Addresses/> .
@prefix fibo-fnd-plc-loc: <https://spec.edmcouncil.org/fibo/ontology/FND/Places/Locations/> .
@prefix fibo-fnd-rel-rel: <https://spec.edmcouncil.org/fibo/ontology/FND/Relations/Relations/> .
@prefix fibo-fnd-utl-alx: <https://spec.edmcouncil.org/fibo/ontology/FND/Utilities/Analytics/> .
@prefix fibo-fnd-utl-av: <https://spec.edmcouncil.org/fibo/ontology/FND/Utilities/AnnotationVocabulary/> .
@prefix lcc-cr: <https://www.omg.org/spec/LCC/Countries/CountryRepresentation/> .
@prefix lcc-lr: <https://www.omg.org/spec/LCC/Languages/LanguageRepresentation/> .
@prefix owl: <http://www.w3.org/2002/07/owl#> .
@prefix rdf: <http://www.w3.org/1999/02/22-rdf-syntax-ns#> .
@prefix rdfs: <http://www.w3.org/2000/01/rdf-schema#> .
@prefix skos: <http://www.w3.org/2004/02/skos/core#> .
@prefix sm: <http://www.omg.org/techprocess/ab/SpecificationMetadata/> .
@prefix xsd: <http://www.w3.org/2001/XMLSchema#> .

<https://spec.edmcouncil.org/fibo/ontology/FND/Places/Addresses/>
	a owl:Ontology ;
	rdfs:label "Addresses Ontology" ;
	dct:abstract "This ontology provides high level definitions for addresses and address components including elements that are common to addressing standards." ;
	dct:license "http://opensource.org/licenses/MIT"^^xsd:anyURI ;
	sm:contentLanguage "https://www.w3.org/TR/owl2-quick-reference/"^^xsd:anyURI ;
	sm:copyright
		"Copyright (c) 2013-2021 EDM Council, Inc." ,
		"Copyright (c) 2013-2021 Object Management Group, Inc."
		;
	sm:dependsOn
		"https://spec.edmcouncil.org/fibo/ontology/FND/Arrangements/ClassificationSchemes/"^^xsd:anyURI ,
		"https://spec.edmcouncil.org/fibo/ontology/FND/Arrangements/IdentifiersAndIndices/"^^xsd:anyURI ,
		"https://spec.edmcouncil.org/fibo/ontology/FND/Places/Locations/"^^xsd:anyURI ,
		"https://spec.edmcouncil.org/fibo/ontology/FND/Relations/Relations/"^^xsd:anyURI ,
		"https://spec.edmcouncil.org/fibo/ontology/FND/Utilities/Analytics/"^^xsd:anyURI ,
		"https://spec.edmcouncil.org/fibo/ontology/FND/Utilities/AnnotationVocabulary/"^^xsd:anyURI ,
		"https://www.omg.org/spec/LCC/"^^xsd:anyURI
		;
	sm:fileAbbreviation "fibo-fnd-plc-adr" ;
	sm:filename "Addresses.rdf" ;
	owl:imports
		<https://spec.edmcouncil.org/fibo/ontology/master/2021Q4/FND/Arrangements/ClassificationSchemes/> ,
		<https://spec.edmcouncil.org/fibo/ontology/master/2021Q4/FND/Arrangements/IdentifiersAndIndices/> ,
		<https://spec.edmcouncil.org/fibo/ontology/master/2021Q4/FND/Places/Locations/> ,
		<https://spec.edmcouncil.org/fibo/ontology/master/2021Q4/FND/Relations/Relations/> ,
		<https://spec.edmcouncil.org/fibo/ontology/master/2021Q4/FND/Utilities/Analytics/> ,
		<https://spec.edmcouncil.org/fibo/ontology/master/2021Q4/FND/Utilities/AnnotationVocabulary/> ,
		<https://www.omg.org/spec/LCC/Countries/CountryRepresentation/> ,
		<https://www.omg.org/spec/LCC/Languages/LanguageRepresentation/>
		;
	owl:versionIRI <https://spec.edmcouncil.org/fibo/ontology/master/2021Q4/FND/Places/Addresses/> ;
	skos:changeNote
		"The http://www.omg.org/spec/EDMC-FIBO/FND/20141101/Places/Addresses.rdf version of this ontology was modified per the issue resolutions identified in the FIBO FND 1.1 RTF report. Differences from the 1.0 version include the addition of a hasAddress property and PhysicalAddress class as a parent of PostalAddress." ,
		"The http://www.omg.org/spec/EDMC-FIBO/FND/20160201/Places/Addresses.rdf version of this ontology was modified for the FIBO 2.0 RFC to integrate LCC." ,
		"The https://spec.edmcouncil.org/fibo/ontology/FND/Places/Addresses.rdf version of this ontology was modified per the issue resolutions identified in the FIBO FND 1.0 FTF report and in https://spec.edmcouncil.org/fibo/ontology/FND/1.0/AboutFND-1.0/. Primary differences include elimination of data properties in favor of a simple class model,the addition of virtual address, and the addition of addressing scheme." ,
		"The https://spec.edmcouncil.org/fibo/ontology/FND/Places/Addresses.rdf version of this ontology was modified replace hasDefinition with isDefinedIn to clarify intent, and the address hierarchy was simplified to enable extensions for international and national delivery address specification, and to eliminate deprecated elements." ,
		"The https://spec.edmcouncil.org/fibo/ontology/FND/Places/Addresses.rdf version of this ontology was modified to correct a missing imports statement." ,
		"The https://spec.edmcouncil.org/fibo/ontology/FND/Places/Addresses.rdf version of this ontology was modified to eliminate duplication of concepts in LCC, simplify address representation and merge countries with locations." ,
		"The https://spec.edmcouncil.org/fibo/ontology/FND/Places/Addresses.rdf version of this ontology was modified to eliminate unnecessary unions and max 1 restrictions." ,
		"The https://spec.edmcouncil.org/fibo/ontology/FND/Places/Addresses.rdf version of this ontology was modified to make postcode a subclass of geographic region identifier and fix spelling errors." ,
		"The https://spec.edmcouncil.org/fibo/ontology/FND/Places/Addresses.rdf version of this ontology was modified to revise names of address elements that could be construed as referring to multiple concepts." ,
		"""The https://spec.edmcouncil.org/fibo/ontology/Foundations/20130601/Organizations/Addresses.owl version of the ontology was revised in advance of the September 2013 New Brunswick, NJ meeting, as follows:
   (1) to use slash style URI/IRIss (also called 303 URIs, vs. hash style) as required to support server side processing 
   (2) to use version-independent IRIs for all definitions internally as opposed to version-specific IRIs
   (3) to change the file suffix from .owl to .rdf to increase usability in RDF tools
   (4) to use 4-level abbreviations and corresponding namespace prefixes for all FIBO ontologies, reflecting a family/specification/module/ontology structure
   (5) to incorporate changes to the specification metadata to support documentation at the family, specification, module, and ontology level, similar to the abbreviations
   (6) to move this ontology from Organizations to Places and eliminate unnecessary properties and related imports dependencies."""
		;
	fibo-fnd-utl-av:hasMaturityLevel fibo-fnd-utl-av:Release ;
	.

fibo-fnd-plc-adr:Address
	a owl:Class ;
	rdfs:subClassOf
		fibo-fnd-arr-id:Index ,
		[
			a owl:Restriction ;
			owl:onProperty fibo-fnd-rel-rel:isDefinedIn ;
			owl:onClass fibo-fnd-plc-adr:AddressingScheme ;
			owl:minQualifiedCardinality "0"^^xsd:nonNegativeInteger ;
		] ,
		[
			a owl:Restriction ;
			owl:onProperty fibo-fnd-arr-id:isIndexTo ;
			owl:onClass lcc-cr:Location ;
			owl:qualifiedCardinality "1"^^xsd:nonNegativeInteger ;
		]
		;
	rdfs:label "address"@en ;
	rdfs:isDefinedBy <https://spec.edmcouncil.org/fibo/ontology/FND/Places/Addresses/> ;
	skos:definition "index to a location to which communications may be delivered" ;
	.

fibo-fnd-plc-adr:AddressComponent
	a owl:Class ;
	rdfs:subClassOf fibo-fnd-utl-alx:Aspect ;
	rdfs:label "address component" ;
	rdfs:isDefinedBy <https://spec.edmcouncil.org/fibo/ontology/FND/Places/Addresses/> ;
	skos:definition "aspect of an address" ;
	.

fibo-fnd-plc-adr:AddressingScheme
	a owl:Class ;
	rdfs:subClassOf
		fibo-fnd-arr-id:IndexingScheme ,
		[
			a owl:Restriction ;
			owl:onProperty fibo-fnd-rel-rel:defines ;
			owl:allValuesFrom fibo-fnd-plc-adr:Address ;
		]
		;
	rdfs:label "addressing scheme" ;
	rdfs:isDefinedBy <https://spec.edmcouncil.org/fibo/ontology/FND/Places/Addresses/> ;
	skos:definition "system for allocating addresses to objects" ;
	.

fibo-fnd-plc-adr:Apartment
	a
		owl:NamedIndividual ,
		fibo-fnd-plc-adr:SecondaryUnitDesignator
		;
	rdfs:label "apartment"@en ;
	rdfs:isDefinedBy <https://spec.edmcouncil.org/fibo/ontology/FND/Places/Addresses/> ;
	skos:definition "room or a group of related rooms, among similar sets in one building, designed for use as a dwelling" ;
	fibo-fnd-plc-adr:requiresSecondaryUnitRange "true"^^xsd:boolean ;
	.

fibo-fnd-plc-adr:Basement
	a
		owl:NamedIndividual ,
		fibo-fnd-plc-adr:SecondaryUnitDesignator
		;
	rdfs:label "basement"@en ;
	rdfs:isDefinedBy <https://spec.edmcouncil.org/fibo/ontology/FND/Places/Addresses/> ;
	skos:definition "part of a building consisting of rooms that are partly or entirely below ground" ;
	fibo-fnd-plc-adr:requiresSecondaryUnitRange "false"^^xsd:boolean ;
	.

fibo-fnd-plc-adr:Building
	a
		owl:NamedIndividual ,
		fibo-fnd-plc-adr:SecondaryUnitDesignator
		;
	rdfs:label "building"@en ;
	rdfs:isDefinedBy <https://spec.edmcouncil.org/fibo/ontology/FND/Places/Addresses/> ;
	skos:definition "relatively permanent enclosed structure, that has a roof and walls and stands more or less permanently in one place" ;
	fibo-fnd-plc-adr:requiresSecondaryUnitRange "true"^^xsd:boolean ;
	.

fibo-fnd-plc-adr:ConventionalStreetAddress
	a owl:Class ;
	rdfs:subClassOf
		fibo-fnd-plc-adr:PhysicalAddress ,
		[
			a owl:Restriction ;
			owl:onProperty fibo-fnd-plc-adr:hasStreetAddress ;
			owl:onClass fibo-fnd-plc-adr:StreetAddress ;
			owl:maxQualifiedCardinality "1"^^xsd:nonNegativeInteger ;
		] ,
		[
			a owl:Restriction ;
			owl:onProperty fibo-fnd-plc-adr:hasAddressLine1 ;
			owl:maxQualifiedCardinality "1"^^xsd:nonNegativeInteger ;
			owl:onDataRange rdfs:Literal ;
		] ,
		[
			a owl:Restriction ;
			owl:onProperty fibo-fnd-plc-adr:hasAddressLine2 ;
			owl:maxQualifiedCardinality "1"^^xsd:nonNegativeInteger ;
			owl:onDataRange rdfs:Literal ;
		] ,
		[
			a owl:Restriction ;
			owl:onProperty fibo-fnd-plc-adr:hasAddressLine3 ;
			owl:maxQualifiedCardinality "1"^^xsd:nonNegativeInteger ;
			owl:onDataRange rdfs:Literal ;
		]
		;
	rdfs:label "conventional street address" ;
	rdfs:isDefinedBy <https://spec.edmcouncil.org/fibo/ontology/FND/Places/Addresses/> ;
	skos:definition "physical address that identifies a location on a street to which communications may be delivered" ;
	fibo-fnd-utl-av:explanatoryNote "Other unconventional addresses may include rural and highway route addresses, general delivery addresses, post office box addresses, private mail center addresses, and so forth." ;
	.

fibo-fnd-plc-adr:Department
	a
		owl:NamedIndividual ,
		fibo-fnd-plc-adr:SecondaryUnitDesignator
		;
	rdfs:label "department"@en ;
	rdfs:isDefinedBy <https://spec.edmcouncil.org/fibo/ontology/FND/Places/Addresses/> ;
	skos:definition "division of a large organization such as a government, university, business, or shop, dealing with a specific subject, commodity, or area of activity" ;
	fibo-fnd-plc-adr:requiresSecondaryUnitRange "true"^^xsd:boolean ;
	.

fibo-fnd-plc-adr:Floor
	a
		owl:NamedIndividual ,
		fibo-fnd-plc-adr:SecondaryUnitDesignator
		;
	rdfs:label "floor"@en ;
	rdfs:isDefinedBy <https://spec.edmcouncil.org/fibo/ontology/FND/Places/Addresses/> ;
	skos:definition "all of the rooms or areas on the same level of a building; a story" ;
	fibo-fnd-plc-adr:requiresSecondaryUnitRange "true"^^xsd:boolean ;
	fibo-fnd-utl-av:explanatoryNote "Labeling systems for floors vary from country to country, and may be specific to the building, for example, whether or not a 13th floor is identified as such tends to be on a case-by-case basis." ;
	.

fibo-fnd-plc-adr:Front
	a
		owl:NamedIndividual ,
		fibo-fnd-plc-adr:SecondaryUnitDesignator
		;
	rdfs:label "front"@en ;
	rdfs:isDefinedBy <https://spec.edmcouncil.org/fibo/ontology/FND/Places/Addresses/> ;
	skos:definition "side or part of a building that presents itself to view first, that faces the street; the most forward part of a building" ;
	fibo-fnd-plc-adr:requiresSecondaryUnitRange "false"^^xsd:boolean ;
	.

fibo-fnd-plc-adr:GeographicDirectionalSymbol
	a owl:Class ;
	rdfs:subClassOf
		lcc-lr:CodeElement ,
		[
			a owl:Restriction ;
			owl:onProperty lcc-lr:hasTag ;
			owl:someValuesFrom xsd:string ;
		]
		;
	rdfs:label "geographic directional symbol" ;
	rdfs:isDefinedBy <https://spec.edmcouncil.org/fibo/ontology/FND/Places/Addresses/> ;
	skos:definition "code element that gives directional information for postal delivery" ;
	skos:example "In the United States, these include N, S, E, W, NE, NW, SE, SW." ;
	.

fibo-fnd-plc-adr:Hangar
	a
		owl:NamedIndividual ,
		fibo-fnd-plc-adr:SecondaryUnitDesignator
		;
	rdfs:label "hanger"@en ;
	rdfs:isDefinedBy <https://spec.edmcouncil.org/fibo/ontology/FND/Places/Addresses/> ;
	skos:definition "shed or shelter; any relatively wide structure used for housing airplanes or airships" ;
	fibo-fnd-plc-adr:requiresSecondaryUnitRange "true"^^xsd:boolean ;
	.

fibo-fnd-plc-adr:Key
	a
		owl:NamedIndividual ,
		fibo-fnd-plc-adr:SecondaryUnitDesignator
		;
	rdfs:label "key"@en ;
	rdfs:isDefinedBy <https://spec.edmcouncil.org/fibo/ontology/FND/Places/Addresses/> ;
	skos:definition "usually metal instrument by which the bolt of a lock is turned" ;
	fibo-fnd-plc-adr:requiresSecondaryUnitRange "true"^^xsd:boolean ;
	.

fibo-fnd-plc-adr:Lobby
	a
		owl:NamedIndividual ,
		fibo-fnd-plc-adr:SecondaryUnitDesignator
		;
	rdfs:label "lobby"@en ;
	rdfs:isDefinedBy <https://spec.edmcouncil.org/fibo/ontology/FND/Places/Addresses/> ;
	skos:definition "entrance hall, corridor, or vestibule, as in a public building, often serving as an anteroom; foyer" ;
	fibo-fnd-plc-adr:requiresSecondaryUnitRange "false"^^xsd:boolean ;
	.

fibo-fnd-plc-adr:Lot
	a
		owl:NamedIndividual ,
		fibo-fnd-plc-adr:SecondaryUnitDesignator
		;
	rdfs:label "lot"@en ;
	rdfs:isDefinedBy <https://spec.edmcouncil.org/fibo/ontology/FND/Places/Addresses/> ;
	skos:definition "measured parcel of land having fixed boundaries and designated on a plot or survey" ;
	fibo-fnd-plc-adr:requiresSecondaryUnitRange "true"^^xsd:boolean ;
	.

fibo-fnd-plc-adr:Lower
	a
		owl:NamedIndividual ,
		fibo-fnd-plc-adr:SecondaryUnitDesignator
		;
	rdfs:label "lower"@en ;
	rdfs:isDefinedBy <https://spec.edmcouncil.org/fibo/ontology/FND/Places/Addresses/> ;
	skos:definition "floor of a building in a multistory structure that is closer to ground level" ;
	fibo-fnd-plc-adr:requiresSecondaryUnitRange "false"^^xsd:boolean ;
	.

fibo-fnd-plc-adr:Office
	a
		owl:NamedIndividual ,
		fibo-fnd-plc-adr:SecondaryUnitDesignator
		;
	rdfs:label "office"@en ;
	rdfs:isDefinedBy <https://spec.edmcouncil.org/fibo/ontology/FND/Places/Addresses/> ;
	skos:definition "place where a particular kind of business is transacted or a service is supplied" ;
	fibo-fnd-plc-adr:requiresSecondaryUnitRange "false"^^xsd:boolean ;
	.

fibo-fnd-plc-adr:Penthouse
	a
		owl:NamedIndividual ,
		fibo-fnd-plc-adr:SecondaryUnitDesignator
		;
	rdfs:label "penthouse"@en ;
	rdfs:isDefinedBy <https://spec.edmcouncil.org/fibo/ontology/FND/Places/Addresses/> ;
	skos:definition "structure or dwelling on the roof or top floor of a building" ;
	fibo-fnd-plc-adr:requiresSecondaryUnitRange "false"^^xsd:boolean ;
	.

fibo-fnd-plc-adr:PhysicalAddress
	a owl:Class ;
	rdfs:subClassOf
		fibo-fnd-plc-adr:Address ,
		[
			a owl:Restriction ;
			owl:onProperty fibo-fnd-plc-adr:hasIndividualPostcode ;
			owl:onClass fibo-fnd-plc-adr:Postcode ;
			owl:maxQualifiedCardinality "1"^^xsd:nonNegativeInteger ;
		] ,
		[
			a owl:Restriction ;
			owl:onProperty fibo-fnd-plc-loc:hasMunicipality ;
			owl:onClass fibo-fnd-plc-loc:Municipality ;
			owl:maxQualifiedCardinality "1"^^xsd:nonNegativeInteger ;
		] ,
		[
			a owl:Restriction ;
			owl:onProperty fibo-fnd-plc-loc:hasCountry ;
			owl:onClass lcc-cr:Country ;
			owl:maxQualifiedCardinality "1"^^xsd:nonNegativeInteger ;
		] ,
		[
			a owl:Restriction ;
			owl:onProperty fibo-fnd-plc-adr:hasPostalCode ;
			owl:maxQualifiedCardinality "1"^^xsd:nonNegativeInteger ;
			owl:onDataRange rdfs:Literal ;
		] ,
		[
			a owl:Restriction ;
			owl:onProperty fibo-fnd-plc-loc:hasCityName ;
			owl:maxQualifiedCardinality "1"^^xsd:nonNegativeInteger ;
			owl:onDataRange rdfs:Literal ;
		] ,
		[
			a owl:Restriction ;
			owl:onProperty fibo-fnd-arr-id:isIndexTo ;
			owl:onClass fibo-fnd-plc-loc:PhysicalLocation ;
			owl:minQualifiedCardinality "0"^^xsd:nonNegativeInteger ;
		] ,
		[
			a owl:Restriction ;
			owl:onProperty fibo-fnd-plc-loc:hasSubdivision ;
			owl:someValuesFrom lcc-cr:CountrySubdivision ;
		]
		;
	rdfs:label "physical address"@en ;
	rdfs:isDefinedBy <https://spec.edmcouncil.org/fibo/ontology/FND/Places/Addresses/> ;
	skos:definition "physical address where communications can be addressed, papers served or representatives located for any kind of organization or person" ;
	skos:scopeNote "An address may be used as an index to the location of a building, apartment, office within an office block, or other structure or parcel of land, often using political boundaries and street names as references, along with other information such as house or building numbers or names.  Some addresses also contain secondary elements such as apartment or building numbers, or special codes to aid routing of mail and packages." ;
	fibo-fnd-utl-av:usageNote "Typically, addresses will have only one postcode expressed either as a string value or individual, and only a municipality (individual) or city (string value)." ;
	.

fibo-fnd-plc-adr:PhysicalAddressIdentifier
	a owl:Class ;
	rdfs:subClassOf
		lcc-lr:CodeElement ,
		lcc-lr:Identifier ,
		[
			a owl:Restriction ;
			owl:onProperty lcc-lr:identifies ;
			owl:onClass fibo-fnd-plc-adr:PhysicalAddress ;
			owl:qualifiedCardinality "1"^^xsd:nonNegativeInteger ;
		] ,
		[
			a owl:Restriction ;
			owl:onProperty lcc-lr:isMemberOf ;
			owl:onClass fibo-fnd-plc-adr:PhysicalAddressingScheme ;
			owl:qualifiedCardinality "1"^^xsd:nonNegativeInteger ;
		]
		;
	rdfs:label "physical address identifier" ;
	rdfs:isDefinedBy <https://spec.edmcouncil.org/fibo/ontology/FND/Places/Addresses/> ;
	skos:definition "unique identifier for a physical address" ;
	skos:example "Physical address identifiers may include bar codes, QCR codes, and +codes in a number of countries." ;
	.

fibo-fnd-plc-adr:PhysicalAddressingScheme
	a owl:Class ;
	rdfs:subClassOf
		fibo-fnd-plc-adr:AddressingScheme ,
		[
			a owl:Class ;
			owl:unionOf (
				[
					a owl:Restriction ;
					owl:onProperty fibo-fnd-rel-rel:defines ;
					owl:onClass fibo-fnd-plc-adr:PhysicalAddressIdentifier ;
					owl:minQualifiedCardinality "0"^^xsd:nonNegativeInteger ;
				]
				[
					a owl:Restriction ;
					owl:onProperty fibo-fnd-rel-rel:defines ;
					owl:onClass fibo-fnd-plc-adr:PhysicalAddress ;
					owl:minQualifiedCardinality "0"^^xsd:nonNegativeInteger ;
				]
			) ;
		]
		;
	rdfs:label "physical addressing scheme" ;
	rdfs:isDefinedBy <https://spec.edmcouncil.org/fibo/ontology/FND/Places/Addresses/> ;
	rdfs:seeAlso <https://pe.usps.com/cpim/ftp/pubs/Pub28/pub28.pdf> ;
	skos:definition "scheme for specifying physical addresses according to a country specific standard" ;
	.

fibo-fnd-plc-adr:Pier
	a
		owl:NamedIndividual ,
		fibo-fnd-plc-adr:SecondaryUnitDesignator
		;
	rdfs:label "pier"@en ;
	rdfs:isDefinedBy <https://spec.edmcouncil.org/fibo/ontology/FND/Places/Addresses/> ;
	skos:definition "structure extending into navigable water for use as a landing place or promenade" ;
	fibo-fnd-plc-adr:requiresSecondaryUnitRange "true"^^xsd:boolean ;
	.

fibo-fnd-plc-adr:PostCodeArea
	a owl:Class ;
	rdfs:subClassOf lcc-cr:GeographicRegion ;
	rdfs:label "post code area"@en ;
	rdfs:isDefinedBy <https://spec.edmcouncil.org/fibo/ontology/FND/Places/Addresses/> ;
	skos:definition "physical area uniquely identified by some postal code" ;
	.

fibo-fnd-plc-adr:PostOfficeBox
	a owl:Class ;
	rdfs:subClassOf
		fibo-fnd-plc-adr:SupplementalAddressComponent ,
		[
			a owl:Restriction ;
			owl:onProperty fibo-fnd-rel-rel:comprises ;
			owl:onClass fibo-fnd-plc-adr:PostOfficeBoxDesignator ;
			owl:qualifiedCardinality "1"^^xsd:nonNegativeInteger ;
		]
		;
	rdfs:label "post office box" ;
	rdfs:isDefinedBy <https://spec.edmcouncil.org/fibo/ontology/FND/Places/Addresses/> ;
	skos:definition "post office box associated with an address" ;
	fibo-fnd-utl-av:explanatoryNote "Post office box identifiers are only unique to a given jurisdiction, which may be a post office, town, or other region." ;
	.

fibo-fnd-plc-adr:PostOfficeBoxAddress
	a owl:Class ;
	rdfs:subClassOf
		fibo-fnd-plc-adr:PhysicalAddress ,
		[
			a owl:Restriction ;
			owl:onProperty fibo-fnd-rel-rel:comprises ;
			owl:onClass fibo-fnd-plc-adr:PostOfficeBox ;
			owl:qualifiedCardinality "1"^^xsd:nonNegativeInteger ;
		]
		;
	rdfs:label "post office box address" ;
	rdfs:isDefinedBy <https://spec.edmcouncil.org/fibo/ontology/FND/Places/Addresses/> ;
	skos:definition "physical address used to deliver communications to a designated container at a local post office or the local equivalent for the jurisdiction, where mail is held until the recipient collects it, rather than to a given house, building, or other location" ;
	.

fibo-fnd-plc-adr:PostOfficeBoxDesignator
	a owl:Class ;
	rdfs:subClassOf fibo-fnd-plc-adr:SupplementalAddressDesignator ;
	rdfs:label "post office box designator"@en ;
	rdfs:isDefinedBy <https://spec.edmcouncil.org/fibo/ontology/FND/Places/Addresses/> ;
	skos:definition "designator used, together with an identifier, for a post office box" ;
	skos:example "In the U.S., the preferred designator is 'PO BOX'." ;
	.

fibo-fnd-plc-adr:Postcode
	a owl:Class ;
	rdfs:subClassOf
		lcc-cr:GeographicRegionIdentifier ,
		lcc-lr:CodeElement ,
		[
			a owl:Restriction ;
			owl:onProperty lcc-lr:denotes ;
			owl:onClass fibo-fnd-plc-adr:PostCodeArea ;
			owl:qualifiedCardinality "1"^^xsd:nonNegativeInteger ;
		] ,
		[
			a owl:Restriction ;
			owl:onProperty lcc-lr:identifies ;
			owl:onClass fibo-fnd-plc-adr:PostCodeArea ;
			owl:qualifiedCardinality "1"^^xsd:nonNegativeInteger ;
		]
		;
	rdfs:label "postcode"@en ;
	rdfs:isDefinedBy <https://spec.edmcouncil.org/fibo/ontology/FND/Places/Addresses/> ;
	skos:definition "sequence of characters used to assist in the sorting of mail" ;
	fibo-fnd-utl-av:synonym "postal code" ;
	.

fibo-fnd-plc-adr:PostdirectionalSymbol
	a owl:Class ;
	rdfs:subClassOf fibo-fnd-plc-adr:GeographicDirectionalSymbol ;
	rdfs:label "postdirectional symbol" ;
	rdfs:isDefinedBy <https://spec.edmcouncil.org/fibo/ontology/FND/Places/Addresses/> ;
	skos:definition "geographic directional symbol that follows the street name and street suffix in a street address" ;
	.

fibo-fnd-plc-adr:PredirectionalSymbol
	a owl:Class ;
	rdfs:subClassOf fibo-fnd-plc-adr:GeographicDirectionalSymbol ;
	rdfs:label "predirectional symbol" ;
	rdfs:isDefinedBy <https://spec.edmcouncil.org/fibo/ontology/FND/Places/Addresses/> ;
	skos:definition "geographic directional symbol that occurs after the primary street number but before the street name in a street address" ;
	.

fibo-fnd-plc-adr:PrimaryAddressNumber
	a owl:Class ;
	rdfs:subClassOf
		fibo-fnd-plc-adr:AddressComponent ,
		[
			a owl:Restriction ;
			owl:onProperty lcc-lr:hasTag ;
			owl:onDataRange xsd:string ;
			owl:qualifiedCardinality "1"^^xsd:nonNegativeInteger ;
		]
		;
	rdfs:label "primary address number" ;
	rdfs:isDefinedBy <https://spec.edmcouncil.org/fibo/ontology/FND/Places/Addresses/> ;
	skos:definition "address component that identifies a location with respect to a given street" ;
	fibo-fnd-utl-av:explanatoryNote "Although traditionally called a 'number', the street number may consist of alphanumeric characters, for example, '221B'." ;
	fibo-fnd-utl-av:synonym "street number" ;
	.

fibo-fnd-plc-adr:Rear
	a
		owl:NamedIndividual ,
		fibo-fnd-plc-adr:SecondaryUnitDesignator
		;
	rdfs:label "rear"@en ;
	rdfs:isDefinedBy <https://spec.edmcouncil.org/fibo/ontology/FND/Places/Addresses/> ;
	skos:definition "side or part of a building at the back, located opposite its front" ;
	fibo-fnd-plc-adr:requiresSecondaryUnitRange "false"^^xsd:boolean ;
	.

fibo-fnd-plc-adr:RegionSpecificIdentifier
	a owl:Class ;
	rdfs:subClassOf
		lcc-cr:GeographicRegionIdentifier ,
		[
			a owl:Restriction ;
			owl:onProperty lcc-cr:isUsedBy ;
			owl:someValuesFrom lcc-cr:GeopoliticalEntity ;
		]
		;
	rdfs:label "region-specific identifier" ;
	rdfs:isDefinedBy <https://spec.edmcouncil.org/fibo/ontology/FND/Places/Addresses/> ;
	skos:definition "geographic region or subdivision identifier used internally by a country or other region" ;
	.

fibo-fnd-plc-adr:Room
	a
		owl:NamedIndividual ,
		fibo-fnd-plc-adr:SecondaryUnitDesignator
		;
	rdfs:label "room"@en ;
	rdfs:isDefinedBy <https://spec.edmcouncil.org/fibo/ontology/FND/Places/Addresses/> ;
	skos:definition "partitioned part of the inside of a building" ;
	fibo-fnd-plc-adr:requiresSecondaryUnitRange "true"^^xsd:boolean ;
	.

fibo-fnd-plc-adr:SecondaryUnit
	a owl:Class ;
	rdfs:subClassOf
		fibo-fnd-plc-adr:AddressComponent ,
		[
			a owl:Restriction ;
			owl:onProperty fibo-fnd-rel-rel:comprises ;
			owl:onClass fibo-fnd-plc-adr:SecondaryUnitIndicator ;
			owl:minQualifiedCardinality "0"^^xsd:nonNegativeInteger ;
		] ,
		[
			a owl:Restriction ;
			owl:onProperty fibo-fnd-rel-rel:comprises ;
			owl:onClass fibo-fnd-plc-adr:SecondaryUnitDesignator ;
			owl:qualifiedCardinality "1"^^xsd:nonNegativeInteger ;
		]
		;
	rdfs:label "secondary unit" ;
	rdfs:isDefinedBy <https://spec.edmcouncil.org/fibo/ontology/FND/Places/Addresses/> ;
	skos:definition "address component that identifies an individual unit within a larger structure, such as an apartment, office, hangar, slip, mailbox, and so forth, at a given street address" ;
	.

fibo-fnd-plc-adr:SecondaryUnitDesignator
	a owl:Class ;
	rdfs:subClassOf
		fibo-fnd-arr-cls:Classifier ,
		[
			a owl:Restriction ;
			owl:onProperty fibo-fnd-plc-adr:requiresSecondaryUnitRange ;
			owl:onDataRange xsd:boolean ;
			owl:qualifiedCardinality "1"^^xsd:nonNegativeInteger ;
		]
		;
	rdfs:label "secondary unit designator" ;
	rdfs:isDefinedBy <https://spec.edmcouncil.org/fibo/ontology/FND/Places/Addresses/> ;
	skos:definition "classifier for a smaller structure or component within a larger facility, such as an apartment, office, mail stop, or other similar designation" ;
	fibo-fnd-utl-av:explanatoryNote "Note that only certain secondary units require a secondary range, such as an apartment number, to complete a delivery point." ;
	.

fibo-fnd-plc-adr:SecondaryUnitIndicator
	a owl:Class ;
	rdfs:subClassOf
		fibo-fnd-plc-adr:AddressComponent ,
		[
			a owl:Restriction ;
			owl:onProperty lcc-lr:hasTag ;
			owl:onDataRange xsd:string ;
			owl:qualifiedCardinality "1"^^xsd:nonNegativeInteger ;
		]
		;
	rdfs:label "secondary unit indicator" ;
	rdfs:isDefinedBy <https://spec.edmcouncil.org/fibo/ontology/FND/Places/Addresses/> ;
	skos:definition "index to the specific unit within a secondary unit, such as a building or apartment, at a particular street address" ;
	.

fibo-fnd-plc-adr:Side
	a
		owl:NamedIndividual ,
		fibo-fnd-plc-adr:SecondaryUnitDesignator
		;
	rdfs:label "side"@en ;
	rdfs:isDefinedBy <https://spec.edmcouncil.org/fibo/ontology/FND/Places/Addresses/> ;
	skos:definition "place, space, or direction with respect to a center or to a line of division" ;
	fibo-fnd-plc-adr:requiresSecondaryUnitRange "false"^^xsd:boolean ;
	.

fibo-fnd-plc-adr:Slip
	a
		owl:NamedIndividual ,
		fibo-fnd-plc-adr:SecondaryUnitDesignator
		;
	rdfs:label "slip"@en ;
	rdfs:isDefinedBy <https://spec.edmcouncil.org/fibo/ontology/FND/Places/Addresses/> ;
	skos:definition "sloping ramp extending out into the water to serve as a place for landing or repairing ships; ship's or boat's berth between two piers" ;
	fibo-fnd-plc-adr:requiresSecondaryUnitRange "true"^^xsd:boolean ;
	.

fibo-fnd-plc-adr:Space
	a
		owl:NamedIndividual ,
		fibo-fnd-plc-adr:SecondaryUnitDesignator
		;
	rdfs:label "space"@en ;
	rdfs:isDefinedBy <https://spec.edmcouncil.org/fibo/ontology/FND/Places/Addresses/> ;
	skos:definition "extent set apart or available, such as a parking or storage space" ;
	fibo-fnd-plc-adr:requiresSecondaryUnitRange "true"^^xsd:boolean ;
	.

fibo-fnd-plc-adr:Stop
	a
		owl:NamedIndividual ,
		fibo-fnd-plc-adr:SecondaryUnitDesignator
		;
	rdfs:label "stop"@en ;
	rdfs:isDefinedBy <https://spec.edmcouncil.org/fibo/ontology/FND/Places/Addresses/> ;
	skos:definition "stopping place, such as a bus or mail stop" ;
	fibo-fnd-plc-adr:requiresSecondaryUnitRange "true"^^xsd:boolean ;
	.

fibo-fnd-plc-adr:StreetAddress
	a owl:Class ;
	rdfs:subClassOf
		fibo-fnd-plc-adr:AddressComponent ,
		[
			a owl:Restriction ;
			owl:onProperty fibo-fnd-plc-adr:hasPrimaryAddressNumber ;
			owl:onClass fibo-fnd-plc-adr:PrimaryAddressNumber ;
			owl:maxQualifiedCardinality "1"^^xsd:nonNegativeInteger ;
		] ,
		[
			a owl:Restriction ;
			owl:onProperty fibo-fnd-plc-adr:hasPostdirectionalSymbol ;
			owl:onClass fibo-fnd-plc-adr:PostdirectionalSymbol ;
			owl:minQualifiedCardinality "0"^^xsd:nonNegativeInteger ;
		] ,
		[
			a owl:Restriction ;
			owl:onProperty fibo-fnd-plc-adr:hasPredirectionalSymbol ;
			owl:onClass fibo-fnd-plc-adr:PredirectionalSymbol ;
			owl:minQualifiedCardinality "0"^^xsd:nonNegativeInteger ;
		] ,
		[
			a owl:Restriction ;
			owl:onProperty fibo-fnd-plc-adr:hasSecondaryUnit ;
			owl:onClass fibo-fnd-plc-adr:SecondaryUnit ;
			owl:minQualifiedCardinality "0"^^xsd:nonNegativeInteger ;
		] ,
		[
			a owl:Restriction ;
			owl:onProperty fibo-fnd-plc-adr:hasStreetSuffix ;
			owl:onClass fibo-fnd-plc-adr:StreetSuffix ;
			owl:minQualifiedCardinality "0"^^xsd:nonNegativeInteger ;
		] ,
		[
			a owl:Restriction ;
			owl:onProperty fibo-fnd-plc-adr:hasStreetName ;
			owl:someValuesFrom fibo-fnd-plc-adr:StreetName ;
		]
		;
	rdfs:label "street address" ;
	rdfs:isDefinedBy <https://spec.edmcouncil.org/fibo/ontology/FND/Places/Addresses/> ;
	skos:definition "index to a location that consists of a primary address number, predirectional, street name, suffix, postdirectional, and an optional secondary unit" ;
	.

fibo-fnd-plc-adr:StreetName
	a owl:Class ;
	rdfs:subClassOf
		fibo-fnd-plc-adr:AddressComponent ,
		[
			a owl:Restriction ;
			owl:onProperty lcc-lr:hasTag ;
			owl:onDataRange xsd:string ;
			owl:qualifiedCardinality "1"^^xsd:nonNegativeInteger ;
		]
		;
	rdfs:label "street name" ;
	rdfs:isDefinedBy <https://spec.edmcouncil.org/fibo/ontology/FND/Places/Addresses/> ;
	skos:definition "identifier for a street in some context (e.g., city, municipality, geographic region)" ;
	.

fibo-fnd-plc-adr:StreetSuffix
	a owl:Class ;
	rdfs:subClassOf
		fibo-fnd-arr-cls:Classifier ,
		fibo-fnd-plc-adr:AddressComponent
		;
	rdfs:label "street suffix" ;
	rdfs:isDefinedBy <https://spec.edmcouncil.org/fibo/ontology/FND/Places/Addresses/> ;
	skos:definition "classifier for a street or other delivery location, such as a dwelling located along a waterway" ;
	fibo-fnd-utl-av:explanatoryNote "The suffix may provide some insight into the size or length of the street, though not necessarily consistently. In some cities, the suffix differentiates the street from another in the same context, such as 19th Street vs. 19th Avenue in San Francisco." ;
	.

fibo-fnd-plc-adr:StructureName
	a owl:Class ;
	rdfs:subClassOf
		fibo-fnd-plc-adr:AddressComponent ,
		[
			a owl:Restriction ;
			owl:onProperty lcc-lr:hasTag ;
			owl:onDataRange xsd:string ;
			owl:qualifiedCardinality "1"^^xsd:nonNegativeInteger ;
		]
		;
	rdfs:label "structure name" ;
	rdfs:isDefinedBy <https://spec.edmcouncil.org/fibo/ontology/FND/Places/Addresses/> ;
	skos:definition "identifier for a building, house, office complex, shopping center, or other structure or group of structures" ;
	skos:example "Examples include 'McCoy Center', which is the name of the office complex where JPMorgan Chase's Polaris facility is located, 'Apple Park', which is the name of the corporate headquarters of Apple, Inc., and 'Howells Bridge Cottage', which is the name of a very old cottage in Cornwall." ;
	.

fibo-fnd-plc-adr:Suite
	a
		owl:NamedIndividual ,
		fibo-fnd-plc-adr:SecondaryUnitDesignator
		;
	rdfs:label "suite"@en ;
	rdfs:isDefinedBy <https://spec.edmcouncil.org/fibo/ontology/FND/Places/Addresses/> ;
	skos:definition "group of rooms occupied as a unit" ;
	fibo-fnd-plc-adr:requiresSecondaryUnitRange "true"^^xsd:boolean ;
	.

fibo-fnd-plc-adr:SupplementalAddressComponent
	a owl:Class ;
	rdfs:subClassOf
		fibo-fnd-plc-adr:AddressComponent ,
		[
			a owl:Restriction ;
			owl:onProperty fibo-fnd-rel-rel:comprises ;
			owl:onClass fibo-fnd-plc-adr:SupplementalAddressUnit ;
			owl:minQualifiedCardinality "0"^^xsd:nonNegativeInteger ;
		] ,
		[
			a owl:Restriction ;
			owl:onProperty lcc-lr:hasTag ;
			owl:minQualifiedCardinality "0"^^xsd:nonNegativeInteger ;
			owl:onDataRange rdfs:Literal ;
		] ,
		[
			a owl:Restriction ;
			owl:onProperty fibo-fnd-rel-rel:comprises ;
			owl:onClass fibo-fnd-plc-adr:SupplementalAddressDesignator ;
			owl:qualifiedCardinality "1"^^xsd:nonNegativeInteger ;
		]
		;
	rdfs:label "supplemental address component" ;
	rdfs:isDefinedBy <https://spec.edmcouncil.org/fibo/ontology/FND/Places/Addresses/> ;
	skos:definition "address component that provides additional information that is important to ensuring proper delivery of communications" ;
	fibo-fnd-utl-av:explanatoryNote "Supplemental components include post office box information, rural route and highway contract route information, private mailboxes, and so forth, that are not part of a conventional street address." ;
	.

fibo-fnd-plc-adr:SupplementalAddressDesignator
	a owl:Class ;
	rdfs:subClassOf
		fibo-fnd-arr-cls:Classifier ,
		[
			a owl:Restriction ;
			owl:onProperty lcc-cr:classifies ;
			owl:someValuesFrom fibo-fnd-plc-adr:SupplementalAddressComponent ;
		]
		;
	rdfs:label "supplemental address designator" ;
	rdfs:isDefinedBy <https://spec.edmcouncil.org/fibo/ontology/FND/Places/Addresses/> ;
	skos:definition "classifier for supplemental address information, such as a highway contract route, rural route, building complex, shopping center, condominium complex, mail box, or other similar designation" ;
	.

fibo-fnd-plc-adr:SupplementalAddressUnit
	a owl:Class ;
	rdfs:subClassOf
		fibo-fnd-plc-adr:AddressComponent ,
		[
			a owl:Restriction ;
			owl:onProperty lcc-lr:hasTag ;
			owl:onDataRange xsd:string ;
			owl:qualifiedCardinality "1"^^xsd:nonNegativeInteger ;
		]
		;
	rdfs:label "supplemental address unit" ;
	rdfs:isDefinedBy <https://spec.edmcouncil.org/fibo/ontology/FND/Places/Addresses/> ;
	skos:definition "address component that includes a specific route, box, apartment, condominium or other indicator or unit associated with a specific address" ;
	.

fibo-fnd-plc-adr:Trailer
	a
		owl:NamedIndividual ,
		fibo-fnd-plc-adr:SecondaryUnitDesignator
		;
	rdfs:label "trailer"@en ;
	rdfs:isDefinedBy <https://spec.edmcouncil.org/fibo/ontology/FND/Places/Addresses/> ;
	skos:definition "vehicle designed to serve wherever parked as a temporary dwelling or place of business" ;
	fibo-fnd-plc-adr:requiresSecondaryUnitRange "true"^^xsd:boolean ;
	.

fibo-fnd-plc-adr:Unit
	a
		owl:NamedIndividual ,
		fibo-fnd-plc-adr:SecondaryUnitDesignator
		;
	rdfs:label "unit"@en ;
	rdfs:isDefinedBy <https://spec.edmcouncil.org/fibo/ontology/FND/Places/Addresses/> ;
	skos:definition "area in a facility, such as a medical facility or hospital that is specially staffed and equipped to provide a particular service or type of care" ;
	fibo-fnd-plc-adr:requiresSecondaryUnitRange "true"^^xsd:boolean ;
	.

fibo-fnd-plc-adr:Upper
	a
		owl:NamedIndividual ,
		fibo-fnd-plc-adr:SecondaryUnitDesignator
		;
	rdfs:label "upper"@en ;
	rdfs:isDefinedBy <https://spec.edmcouncil.org/fibo/ontology/FND/Places/Addresses/> ;
	skos:definition "floor of a building in a multistory structure that is farther away from the ground level" ;
	fibo-fnd-plc-adr:requiresSecondaryUnitRange "false"^^xsd:boolean ;
	.

fibo-fnd-plc-adr:VirtualAddress
	a owl:Class ;
	rdfs:subClassOf
		fibo-fnd-plc-adr:Address ,
		[
			a owl:Restriction ;
			owl:onProperty lcc-lr:hasTag ;
			owl:onDataRange xsd:string ;
			owl:qualifiedCardinality "1"^^xsd:nonNegativeInteger ;
		]
		;
	rdfs:label "virtual address" ;
	rdfs:isDefinedBy <https://spec.edmcouncil.org/fibo/ontology/FND/Places/Addresses/> ;
	owl:disjointWith fibo-fnd-plc-adr:PhysicalAddress ;
	skos:definition "address identifying a virtual, i.e. non-physical, location" ;
	.

fibo-fnd-plc-adr:hasAddress
	a owl:ObjectProperty ;
	rdfs:subPropertyOf lcc-lr:has ;
	rdfs:label "has address" ;
	rdfs:isDefinedBy <https://spec.edmcouncil.org/fibo/ontology/FND/Places/Addresses/> ;
	rdfs:range fibo-fnd-plc-adr:Address ;
	skos:definition "indicates a means by which something (in the case of a network address) or some entity may be located or contacted or may receive correspondence" ;
	.

fibo-fnd-plc-adr:hasAddressLine1
	a owl:DatatypeProperty ;
	rdfs:label "has address line 1" ;
	rdfs:domain fibo-fnd-plc-adr:PhysicalAddress ;
	rdfs:isDefinedBy <https://spec.edmcouncil.org/fibo/ontology/FND/Places/Addresses/> ;
	skos:definition "the first line of the street address" ;
	fibo-fnd-utl-av:adaptedFrom "https://www.gleif.org/en/about-lei/common-data-file-format/lei-cdf-format/lei-cdf-format-version-2-1"^^xsd:anyURI ;
	.

fibo-fnd-plc-adr:hasAddressLine2
	a owl:DatatypeProperty ;
	rdfs:label "has address line 2" ;
	rdfs:domain fibo-fnd-plc-adr:PhysicalAddress ;
	rdfs:isDefinedBy <https://spec.edmcouncil.org/fibo/ontology/FND/Places/Addresses/> ;
	skos:definition "the second line of the street address" ;
	fibo-fnd-utl-av:adaptedFrom "https://www.gleif.org/en/about-lei/common-data-file-format/lei-cdf-format/lei-cdf-format-version-2-1"^^xsd:anyURI ;
	.

fibo-fnd-plc-adr:hasAddressLine3
	a owl:DatatypeProperty ;
	rdfs:label "has address line 3" ;
	rdfs:domain fibo-fnd-plc-adr:PhysicalAddress ;
	rdfs:isDefinedBy <https://spec.edmcouncil.org/fibo/ontology/FND/Places/Addresses/> ;
	skos:definition "the third line of the street address" ;
	fibo-fnd-utl-av:adaptedFrom "https://www.gleif.org/en/about-lei/common-data-file-format/lei-cdf-format/lei-cdf-format-version-2-1"^^xsd:anyURI ;
	fibo-fnd-utl-av:usageNote "This element SHALL be omitted if address line 2 is omitted." ;
	.

fibo-fnd-plc-adr:hasAttentionLine
	a owl:DatatypeProperty ;
	rdfs:label "has attention line" ;
	rdfs:domain fibo-fnd-plc-adr:PhysicalAddress ;
	rdfs:isDefinedBy <https://spec.edmcouncil.org/fibo/ontology/FND/Places/Addresses/> ;
	skos:definition "an optional, free text address line denoting the intended recipient" ;
	.

fibo-fnd-plc-adr:hasIndividualPostcode
	a owl:ObjectProperty ;
	rdfs:subPropertyOf fibo-fnd-rel-rel:comprises ;
	rdfs:label "has individual postcode" ;
	rdfs:domain fibo-fnd-plc-adr:PhysicalAddress ;
	rdfs:isDefinedBy <https://spec.edmcouncil.org/fibo/ontology/FND/Places/Addresses/> ;
	rdfs:range fibo-fnd-plc-adr:Postcode ;
	skos:definition "indicates the local or international postcode element of a delivery address as specified by the local postal service" ;
	fibo-fnd-utl-av:adaptedFrom "https://www.gleif.org/en/about-lei/common-data-file-format/lei-cdf-format/lei-cdf-format-version-2-1"^^xsd:anyURI ;
	.

fibo-fnd-plc-adr:hasMailRouting
	a owl:DatatypeProperty ;
	rdfs:label "has mail routing" ;
	rdfs:domain fibo-fnd-plc-adr:PhysicalAddress ;
	rdfs:isDefinedBy <https://spec.edmcouncil.org/fibo/ontology/FND/Places/Addresses/> ;
	skos:definition "an optional, free text address line containing explicit routing information (this elements's presence indicates that this address is a routing / 'care of' address)" ;
	fibo-fnd-utl-av:adaptedFrom "https://www.gleif.org/en/about-lei/common-data-file-format/lei-cdf-format/lei-cdf-format-version-2-1"^^xsd:anyURI ;
	.

fibo-fnd-plc-adr:hasPostalCode
	a owl:DatatypeProperty ;
	rdfs:label "has postal code" ;
	rdfs:domain fibo-fnd-plc-adr:PhysicalAddress ;
	rdfs:isDefinedBy <https://spec.edmcouncil.org/fibo/ontology/FND/Places/Addresses/> ;
	skos:definition "the postal code of this address as specified by the local postal service" ;
	fibo-fnd-utl-av:adaptedFrom "https://www.gleif.org/en/about-lei/common-data-file-format/lei-cdf-format/lei-cdf-format-version-2-1"^^xsd:anyURI ;
	.

fibo-fnd-plc-adr:hasPostdirectionalSymbol
	a owl:ObjectProperty ;
	rdfs:subPropertyOf fibo-fnd-rel-rel:comprises ;
	rdfs:label "has postdirectional symbol" ;
	rdfs:domain fibo-fnd-plc-adr:StreetAddress ;
	rdfs:isDefinedBy <https://spec.edmcouncil.org/fibo/ontology/FND/Places/Addresses/> ;
	rdfs:range fibo-fnd-plc-adr:PostdirectionalSymbol ;
	skos:definition "specifies a geographic directional symbol that follows the street name and street suffix in a street address" ;
	.

fibo-fnd-plc-adr:hasPredirectionalSymbol
	a owl:ObjectProperty ;
	rdfs:subPropertyOf fibo-fnd-rel-rel:comprises ;
	rdfs:label "has predirectional symbol" ;
	rdfs:domain fibo-fnd-plc-adr:StreetAddress ;
	rdfs:isDefinedBy <https://spec.edmcouncil.org/fibo/ontology/FND/Places/Addresses/> ;
	rdfs:range fibo-fnd-plc-adr:PredirectionalSymbol ;
	skos:definition "specifies a geographic directional symbol that occurs after the primary street number but before the street name in a street address" ;
	.

fibo-fnd-plc-adr:hasPrimaryAddressNumber
	a owl:ObjectProperty ;
	rdfs:subPropertyOf fibo-fnd-rel-rel:comprises ;
	rdfs:label "has primary address number" ;
	rdfs:domain fibo-fnd-plc-adr:StreetAddress ;
	rdfs:isDefinedBy <https://spec.edmcouncil.org/fibo/ontology/FND/Places/Addresses/> ;
	rdfs:range fibo-fnd-plc-adr:PrimaryAddressNumber ;
	skos:definition "specifies a a location with respect to a given street" ;
	.

fibo-fnd-plc-adr:hasSecondaryUnit
	a owl:ObjectProperty ;
	rdfs:subPropertyOf fibo-fnd-rel-rel:comprises ;
	rdfs:label "has secondary unit" ;
	rdfs:domain fibo-fnd-plc-adr:StreetAddress ;
	rdfs:isDefinedBy <https://spec.edmcouncil.org/fibo/ontology/FND/Places/Addresses/> ;
	rdfs:range fibo-fnd-plc-adr:SecondaryUnit ;
	skos:definition "specifies an individual unit within a larger structure, such as an apartment, office, hangar, slip, mailbox, and so forth, at a given street address" ;
	.

fibo-fnd-plc-adr:hasStreetAddress
	a owl:ObjectProperty ;
	rdfs:subPropertyOf fibo-fnd-rel-rel:comprises ;
	rdfs:label "has street address" ;
	rdfs:domain fibo-fnd-plc-adr:ConventionalStreetAddress ;
	rdfs:isDefinedBy <https://spec.edmcouncil.org/fibo/ontology/FND/Places/Addresses/> ;
	rdfs:range fibo-fnd-plc-adr:StreetAddress ;
	skos:definition "indicates a fully-specified address component that consists of a primary address number, predirectional, street name, suffix, postdirectional, and an optional secondary unit" ;
	.

fibo-fnd-plc-adr:hasStreetName
	a owl:ObjectProperty ;
	rdfs:subPropertyOf fibo-fnd-rel-rel:comprises ;
	rdfs:label "has street name" ;
	rdfs:domain fibo-fnd-plc-adr:StreetAddress ;
	rdfs:isDefinedBy <https://spec.edmcouncil.org/fibo/ontology/FND/Places/Addresses/> ;
	rdfs:range fibo-fnd-plc-adr:StreetName ;
	skos:definition "specifies an identifier for a street in some context (e.g., 'Baker', 'First', 'Main')" ;
	.

fibo-fnd-plc-adr:hasStreetSuffix
	a owl:ObjectProperty ;
	rdfs:subPropertyOf fibo-fnd-rel-rel:comprises ;
	rdfs:label "has street suffix" ;
	rdfs:domain fibo-fnd-plc-adr:StreetAddress ;
	rdfs:isDefinedBy <https://spec.edmcouncil.org/fibo/ontology/FND/Places/Addresses/> ;
	rdfs:range fibo-fnd-plc-adr:StreetSuffix ;
	skos:definition "specifies an additional qualifier for a street or other delivery location, such as a dwelling located along a waterway" ;
	.

fibo-fnd-plc-adr:hasStructureName
	a owl:ObjectProperty ;
	rdfs:subPropertyOf fibo-fnd-rel-rel:comprises ;
	rdfs:label "has structure name" ;
	rdfs:domain fibo-fnd-plc-adr:PhysicalAddress ;
	rdfs:isDefinedBy <https://spec.edmcouncil.org/fibo/ontology/FND/Places/Addresses/> ;
	rdfs:range fibo-fnd-plc-adr:StructureName ;
	skos:definition "specifies an identifier for a building, house, office complex, shopping center, or other structure or group of structures" ;
	.

fibo-fnd-plc-adr:hasTransliteratedAddress
	a owl:ObjectProperty ;
	rdfs:subPropertyOf fibo-fnd-plc-adr:hasAddress ;
	rdfs:label "has transliterated address" ;
	rdfs:isDefinedBy <https://spec.edmcouncil.org/fibo/ontology/FND/Places/Addresses/> ;
	rdfs:range fibo-fnd-plc-adr:Address ;
	skos:definition "identifies a transliterated (i.e., in Latin or Romanized ASCII) address for the registered entity" ;
	fibo-fnd-utl-av:adaptedFrom "https://www.gleif.org/en/about-lei/common-data-file-format/lei-cdf-format/lei-cdf-format-version-2-1"^^xsd:anyURI ;
	.

fibo-fnd-plc-adr:requiresSecondaryUnitRange
	a owl:DatatypeProperty ;
	rdfs:label "requires secondary unit range" ;
	rdfs:isDefinedBy <https://spec.edmcouncil.org/fibo/ontology/FND/Places/Addresses/> ;
	rdfs:range xsd:boolean ;
	rdfs:seeAlso <https://pe.usps.com/cpim/ftp/pubs/Pub28/pub28.pdf> ;
	skos:definition "if true, indicates that an additional qualifier is needed to complete the delivery point description, such as an apartment number" ;
	fibo-fnd-utl-av:explanatoryNote "Note that in some cases, such as for lobby or office, if there are multiple secondary units then a range may be needed to differentiate between them, even if the range is not always required." ;
	.

