# baseURI: https://spec.edmcouncil.org/fibo/ontology/master/2021Q4/DER/RateDerivatives/IRSwaps/
# imports: https://spec.edmcouncil.org/fibo/ontology/master/2021Q4/DER/DerivativesContracts/DerivativesBasics/
# imports: https://spec.edmcouncil.org/fibo/ontology/master/2021Q4/DER/DerivativesContracts/Swaps/
# imports: https://spec.edmcouncil.org/fibo/ontology/master/2021Q4/DER/RateDerivatives/RateDerivatives/
# imports: https://spec.edmcouncil.org/fibo/ontology/master/2021Q4/FBC/DebtAndEquities/Debt/
# imports: https://spec.edmcouncil.org/fibo/ontology/master/2021Q4/FBC/FunctionalEntities/RegistrationAuthorities/
# imports: https://spec.edmcouncil.org/fibo/ontology/master/2021Q4/FBC/ProductsAndServices/FinancialProductsAndServices/
# imports: https://spec.edmcouncil.org/fibo/ontology/master/2021Q4/FND/Accounting/CurrencyAmount/
# imports: https://spec.edmcouncil.org/fibo/ontology/master/2021Q4/FND/Agreements/Contracts/
# imports: https://spec.edmcouncil.org/fibo/ontology/master/2021Q4/FND/DatesAndTimes/BusinessDates/
# imports: https://spec.edmcouncil.org/fibo/ontology/master/2021Q4/FND/DatesAndTimes/FinancialDates/
# imports: https://spec.edmcouncil.org/fibo/ontology/master/2021Q4/FND/ProductsAndServices/PaymentsAndSchedules/
# imports: https://spec.edmcouncil.org/fibo/ontology/master/2021Q4/FND/Quantities/QuantitiesAndUnits/
# imports: https://spec.edmcouncil.org/fibo/ontology/master/2021Q4/FND/Relations/Relations/
# imports: https://spec.edmcouncil.org/fibo/ontology/master/2021Q4/FND/Utilities/Analytics/
# imports: https://spec.edmcouncil.org/fibo/ontology/master/2021Q4/FND/Utilities/AnnotationVocabulary/
# imports: https://spec.edmcouncil.org/fibo/ontology/master/2021Q4/IND/EconomicIndicators/EconomicIndicators/
# imports: https://spec.edmcouncil.org/fibo/ontology/master/2021Q4/IND/InterestRates/InterestRates/
# imports: https://spec.edmcouncil.org/fibo/ontology/master/2021Q4/SEC/Debt/Bonds/
# imports: https://spec.edmcouncil.org/fibo/ontology/master/2021Q4/SEC/Securities/ParametricSchedules/

@base <https://spec.edmcouncil.org/fibo/ontology/master/2021Q4/DER/RateDerivatives/IRSwaps/> .
@prefix dct: <http://purl.org/dc/terms/> .
@prefix fibo-der-drc-bsc: <https://spec.edmcouncil.org/fibo/ontology/DER/DerivativesContracts/DerivativesBasics/> .
@prefix fibo-der-drc-swp: <https://spec.edmcouncil.org/fibo/ontology/DER/DerivativesContracts/Swaps/> .
@prefix fibo-der-rtd-irswp: <https://spec.edmcouncil.org/fibo/ontology/DER/RateDerivatives/IRSwaps/> .
@prefix fibo-der-rtd-rtd: <https://spec.edmcouncil.org/fibo/ontology/DER/RateDerivatives/RateDerivatives/> .
@prefix fibo-fbc-dae-dbt: <https://spec.edmcouncil.org/fibo/ontology/FBC/DebtAndEquities/Debt/> .
@prefix fibo-fbc-fct-ra: <https://spec.edmcouncil.org/fibo/ontology/FBC/FunctionalEntities/RegistrationAuthorities/> .
@prefix fibo-fnd-acc-cur: <https://spec.edmcouncil.org/fibo/ontology/FND/Accounting/CurrencyAmount/> .
@prefix fibo-fnd-dt-bd: <https://spec.edmcouncil.org/fibo/ontology/FND/DatesAndTimes/BusinessDates/> .
@prefix fibo-fnd-dt-fd: <https://spec.edmcouncil.org/fibo/ontology/FND/DatesAndTimes/FinancialDates/> .
@prefix fibo-fnd-pas-psch: <https://spec.edmcouncil.org/fibo/ontology/FND/ProductsAndServices/PaymentsAndSchedules/> .
@prefix fibo-fnd-qt-qtu: <https://spec.edmcouncil.org/fibo/ontology/FND/Quantities/QuantitiesAndUnits/> .
@prefix fibo-fnd-rel-rel: <https://spec.edmcouncil.org/fibo/ontology/FND/Relations/Relations/> .
@prefix fibo-fnd-utl-alx: <https://spec.edmcouncil.org/fibo/ontology/FND/Utilities/Analytics/> .
@prefix fibo-fnd-utl-av: <https://spec.edmcouncil.org/fibo/ontology/FND/Utilities/AnnotationVocabulary/> .
@prefix fibo-ind-ei-ei: <https://spec.edmcouncil.org/fibo/ontology/IND/EconomicIndicators/EconomicIndicators/> .
@prefix fibo-sec-dbt-bnd: <https://spec.edmcouncil.org/fibo/ontology/SEC/Debt/Bonds/> .
@prefix fibo-sec-sec-sch: <https://spec.edmcouncil.org/fibo/ontology/SEC/Securities/ParametricSchedules/> .
@prefix owl: <http://www.w3.org/2002/07/owl#> .
@prefix rdf: <http://www.w3.org/1999/02/22-rdf-syntax-ns#> .
@prefix rdfs: <http://www.w3.org/2000/01/rdf-schema#> .
@prefix skos: <http://www.w3.org/2004/02/skos/core#> .
@prefix sm: <http://www.omg.org/techprocess/ab/SpecificationMetadata/> .
@prefix xsd: <http://www.w3.org/2001/XMLSchema#> .

<https://spec.edmcouncil.org/fibo/ontology/DER/RateDerivatives/IRSwaps/>
	a owl:Ontology ;
	rdfs:label "Interest Rate Swaps Ontology" ;
	dct:abstract "This ontology defines concepts specific to interest rate swap contracts, including but not limited to fixed and floating rate combinations, single and cross-currency contracts, etc." ;
	dct:license "http://opensource.org/licenses/MIT"^^xsd:anyURI ;
	sm:contentLanguage <https://www.w3.org/TR/owl2-quick-reference/> ;
	sm:copyright
		"Copyright (c) 2016-2021 EDM Council, Inc." ,
		"Copyright (c) 2016-2021 Object Management Group, Inc."
		;
	sm:dependsOn
		<https://spec.edmcouncil.org/fibo/ontology/DER/DerivativesContracts/DerivativesBasics/> ,
		<https://spec.edmcouncil.org/fibo/ontology/DER/DerivativesContracts/Swaps/> ,
		<https://spec.edmcouncil.org/fibo/ontology/DER/RateDerivatives/RateDerivatives/> ,
		<https://spec.edmcouncil.org/fibo/ontology/FBC/> ,
		<https://spec.edmcouncil.org/fibo/ontology/FND/> ,
		<https://spec.edmcouncil.org/fibo/ontology/IND/> ,
		<https://spec.edmcouncil.org/fibo/ontology/SEC/>
		;
	sm:fileAbbreviation "fibo-der-rtd-irswp" ;
	sm:filename "IRSwaps.rdf" ;
	owl:imports
		<https://spec.edmcouncil.org/fibo/ontology/master/2021Q4/DER/DerivativesContracts/DerivativesBasics/> ,
		<https://spec.edmcouncil.org/fibo/ontology/master/2021Q4/DER/DerivativesContracts/Swaps/> ,
		<https://spec.edmcouncil.org/fibo/ontology/master/2021Q4/DER/RateDerivatives/RateDerivatives/> ,
		<https://spec.edmcouncil.org/fibo/ontology/master/2021Q4/FBC/DebtAndEquities/Debt/> ,
		<https://spec.edmcouncil.org/fibo/ontology/master/2021Q4/FBC/FunctionalEntities/RegistrationAuthorities/> ,
		<https://spec.edmcouncil.org/fibo/ontology/master/2021Q4/FBC/ProductsAndServices/FinancialProductsAndServices/> ,
		<https://spec.edmcouncil.org/fibo/ontology/master/2021Q4/FND/Accounting/CurrencyAmount/> ,
		<https://spec.edmcouncil.org/fibo/ontology/master/2021Q4/FND/Agreements/Contracts/> ,
		<https://spec.edmcouncil.org/fibo/ontology/master/2021Q4/FND/DatesAndTimes/BusinessDates/> ,
		<https://spec.edmcouncil.org/fibo/ontology/master/2021Q4/FND/DatesAndTimes/FinancialDates/> ,
		<https://spec.edmcouncil.org/fibo/ontology/master/2021Q4/FND/ProductsAndServices/PaymentsAndSchedules/> ,
		<https://spec.edmcouncil.org/fibo/ontology/master/2021Q4/FND/Quantities/QuantitiesAndUnits/> ,
		<https://spec.edmcouncil.org/fibo/ontology/master/2021Q4/FND/Relations/Relations/> ,
		<https://spec.edmcouncil.org/fibo/ontology/master/2021Q4/FND/Utilities/Analytics/> ,
		<https://spec.edmcouncil.org/fibo/ontology/master/2021Q4/FND/Utilities/AnnotationVocabulary/> ,
		<https://spec.edmcouncil.org/fibo/ontology/master/2021Q4/IND/EconomicIndicators/EconomicIndicators/> ,
		<https://spec.edmcouncil.org/fibo/ontology/master/2021Q4/IND/InterestRates/InterestRates/> ,
		<https://spec.edmcouncil.org/fibo/ontology/master/2021Q4/SEC/Debt/Bonds/> ,
		<https://spec.edmcouncil.org/fibo/ontology/master/2021Q4/SEC/Securities/ParametricSchedules/>
		;
	owl:versionIRI <https://spec.edmcouncil.org/fibo/ontology/master/2021Q4/DER/RateDerivatives/IRSwaps/> ;
	skos:changeNote
		"The https://spec.edmcouncil.org/fibo/ontology/DER/RateDerivatives/IRSwaps.rdf version of this ontology was modified to use the generic statistical measures and measurements now in FND." ,
		"The https://spec.edmcouncil.org/fibo/ontology/DER/RateDerivatives/IRSwaps/ version of this ontology was modified take advantage of basic fixed and floating legs as higher level concepts common to many swaps, and to refine definitions to eliminate ambiguity and conform with ISO 704." ,
		"The https://spec.edmcouncil.org/fibo/ontology/DER/RateDerivatives/IRSwaps/ version of this ontology was modified to eliminate the property 'hasPaymentSchedule' from the Swaps ontology in favor of the equivalent property with the same name from FND." ,
		"The https://spec.edmcouncil.org/fibo/ontology/DER/RateDerivatives/IRSwaps/ version of this ontology was modified to enable representation of plain vanilla interest rate swaps as a separate concept, to integrate the concept of an inflation swap and correct spelling." ,
		"The https://spec.edmcouncil.org/fibo/ontology/DER/RateDerivatives/IRSwaps/ version of this ontology was modified to move the property 'exchanges' to FND given that it could be applied more generally than with respect to swaps only."
		;
	fibo-fnd-utl-av:hasMaturityLevel fibo-fnd-utl-av:Release ;
	.

fibo-der-rtd-irswp:CrossCurrencyInterestRateSwap
	a owl:Class ;
	rdfs:subClassOf
		fibo-der-rtd-irswp:InterestRateSwap ,
		[
			a owl:Restriction ;
			owl:onProperty fibo-fbc-fct-ra:specifies ;
			owl:onClass fibo-fnd-acc-cur:Currency ;
			owl:qualifiedCardinality "2"^^xsd:nonNegativeInteger ;
		]
		;
	rdfs:label "cross-currency interest rate swap" ;
	rdfs:isDefinedBy <https://spec.edmcouncil.org/fibo/ontology/DER/RateDerivatives/IRSwaps/> ;
	skos:definition "interest rate swap in which the two streams of interest payments are in different currencies" ;
	.

fibo-der-rtd-irswp:ExplicitInterestAmountCalculationEvent
	a owl:Class ;
	rdfs:subClassOf
		fibo-der-rtd-irswp:InterestRateStreamEvent ,
		fibo-sec-sec-sch:ScheduledCalculationPeriodEndEvent
		;
	rdfs:label "explicit interest amount calculation event" ;
	rdfs:isDefinedBy <https://spec.edmcouncil.org/fibo/ontology/DER/RateDerivatives/IRSwaps/> ;
	skos:definition "the explicit representation of the calculation event in a given period, in which an interest payment is calculated based on the rate (fixed or floating) and the notional amount (in the payment currency, and factored for Fx if necessary), on a given date" ;
	.

fibo-der-rtd-irswp:FixedFloatCrossCurrencyInterestRateSwap
	a owl:Class ;
	rdfs:subClassOf
		fibo-der-rtd-irswp:CrossCurrencyInterestRateSwap ,
		fibo-der-rtd-irswp:FixedFloatInterestRateSwap
		;
	rdfs:label "fixed float cross-currency interest rate swap" ;
	rdfs:isDefinedBy <https://spec.edmcouncil.org/fibo/ontology/DER/RateDerivatives/IRSwaps/> ;
	owl:equivalentClass [
		a owl:Class ;
		owl:intersectionOf (
			fibo-der-rtd-irswp:CrossCurrencyInterestRateSwap
			fibo-der-rtd-irswp:FixedFloatInterestRateSwap
		) ;
	] ;
	skos:definition "interest rate swap in which fixed interest payments on the notional are exchanged for floating interest payments and the two streams of interest payments are in different currencies" ;
	fibo-fnd-utl-av:synonym
		"fixed float cross currency interest rate swap" ,
		"fixed-float cross-currency interest rate swap"
		;
	.

fibo-der-rtd-irswp:FixedFloatInterestRateSwap
	a owl:Class ;
	rdfs:subClassOf
		fibo-der-rtd-irswp:InterestRateSwap ,
		[
			a owl:Class ;
			owl:intersectionOf (
				[
					a owl:Restriction ;
					owl:onProperty fibo-fnd-rel-rel:exchanges ;
					owl:someValuesFrom fibo-der-rtd-irswp:FixedInterestRateLeg ;
				]
				[
					a owl:Restriction ;
					owl:onProperty fibo-fnd-rel-rel:exchanges ;
					owl:someValuesFrom fibo-der-rtd-irswp:FloatingInterestRateLeg ;
				]
			) ;
		]
		;
	rdfs:label "fixed float interest rate swap" ;
	rdfs:isDefinedBy <https://spec.edmcouncil.org/fibo/ontology/DER/RateDerivatives/IRSwaps/> ;
	owl:equivalentClass [
		a owl:Class ;
		owl:intersectionOf (
			fibo-der-rtd-irswp:InterestRateSwap
			[
				a owl:Restriction ;
				owl:onProperty fibo-der-drc-swp:hasLeg ;
				owl:someValuesFrom fibo-der-rtd-irswp:FixedInterestRateLeg ;
			]
			[
				a owl:Restriction ;
				owl:onProperty fibo-der-drc-swp:hasLeg ;
				owl:someValuesFrom fibo-der-rtd-irswp:FloatingInterestRateLeg ;
			]
		) ;
	] ;
	skos:definition "interest rate swap in which fixed interest payments on the notional are exchanged for floating interest payments" ;
	fibo-fnd-utl-av:synonym "fixed-float interest rate swap" ;
	.

fibo-der-rtd-irswp:FixedFloatSingleCurrencyInterestRateSwap
	a owl:Class ;
	rdfs:subClassOf fibo-der-rtd-irswp:FixedFloatInterestRateSwap ;
	rdfs:label "fixed float single currency interest rate swap" ;
	rdfs:isDefinedBy <https://spec.edmcouncil.org/fibo/ontology/DER/RateDerivatives/IRSwaps/> ;
	owl:equivalentClass [
		a owl:Class ;
		owl:intersectionOf (
			fibo-der-rtd-irswp:FixedFloatInterestRateSwap
			fibo-der-rtd-irswp:SingleCurrencyInterestRateSwap
		) ;
	] ;
	skos:definition "interest rate swap in which fixed interest payments on the notional are exchanged for floating interest payments and where both payment streams are expressed in terms of the same currency" ;
	fibo-fnd-utl-av:synonym "fixed-float single-currency interest rate swap" ;
	.

fibo-der-rtd-irswp:FixedInterestRateLeg
	a owl:Class ;
	rdfs:subClassOf
		fibo-der-drc-swp:FixedLeg ,
		fibo-der-rtd-irswp:InterestRateSwapLeg
		;
	rdfs:label "fixed interest rate leg" ;
	rdfs:isDefinedBy <https://spec.edmcouncil.org/fibo/ontology/DER/RateDerivatives/IRSwaps/> ;
	owl:disjointWith fibo-der-rtd-irswp:FloatingInterestRateLeg ;
	owl:equivalentClass [
		a owl:Class ;
		owl:intersectionOf (
			fibo-der-rtd-irswp:InterestRateSwapLeg
			[
				a owl:Restriction ;
				owl:onProperty fibo-fbc-dae-dbt:hasInterestRate ;
				owl:someValuesFrom fibo-fbc-dae-dbt:FixedInterestRate ;
			]
		) ;
	] ;
	skos:definition "fixed leg that specifies fixed interest amounts and terms for the payment of that interest" ;
	fibo-fnd-utl-av:explanatoryNote "This may be the funding leg of some swaps (i.e. one party agrees to pay fixed interest amounts in exchange for whatever is the other leg) or it may be one or both sides of an interest rate swap, where the two parties exchange different interest streams." ;
	fibo-fnd-utl-av:synonym "fixed interest rate swap stream" ;
	.

fibo-der-rtd-irswp:FloatFloatCrossCurrencyInterestRateSwap
	a owl:Class ;
	rdfs:subClassOf fibo-der-rtd-irswp:FloatFloatInterestRateSwap ;
	rdfs:label "float float cross-currency interest rate swap" ;
	rdfs:isDefinedBy <https://spec.edmcouncil.org/fibo/ontology/DER/RateDerivatives/IRSwaps/> ;
	owl:equivalentClass [
		a owl:Class ;
		owl:intersectionOf (
			fibo-der-rtd-irswp:CrossCurrencyInterestRateSwap
			fibo-der-rtd-irswp:FloatFloatInterestRateSwap
		) ;
	] ;
	skos:definition "interest rate swap that exchanges cashflows based on two different interest rates in different currencies" ;
	fibo-fnd-utl-av:synonym "float-float cross-currency interest rate swap" ;
	.

fibo-der-rtd-irswp:FloatFloatInterestRateSwap
	a owl:Class ;
	rdfs:subClassOf
		fibo-der-drc-swp:BasisSwap ,
		fibo-der-rtd-irswp:InterestRateSwap ,
		[
			a owl:Restriction ;
			owl:onProperty fibo-fnd-rel-rel:exchanges ;
			owl:onClass fibo-der-rtd-irswp:FloatingInterestRateLeg ;
			owl:qualifiedCardinality "2"^^xsd:nonNegativeInteger ;
		]
		;
	rdfs:label "float float interest rate swap" ;
	rdfs:isDefinedBy <https://spec.edmcouncil.org/fibo/ontology/DER/RateDerivatives/IRSwaps/> ;
	owl:equivalentClass [
		a owl:Class ;
		owl:intersectionOf (
			fibo-der-rtd-irswp:InterestRateSwap
			[
				a owl:Restriction ;
				owl:onProperty fibo-der-drc-swp:hasLeg ;
				owl:onClass fibo-der-rtd-irswp:FloatingInterestRateLeg ;
				owl:qualifiedCardinality "2"^^xsd:nonNegativeInteger ;
			]
		) ;
	] ;
	skos:definition "interest rate swap that exchanges cashflows based on two different floating interest rates" ;
	fibo-fnd-utl-av:adaptedFrom "http://www.investopedia.com/terms/b/basisrateswap.asp"^^xsd:anyURI ;
	fibo-fnd-utl-av:explanatoryNote "This is a swap in which two parties swap variable interest rates based on different money markets, and this is usually done to limit interest-rate risk that a company faces as a result of having differing lending and borrowing rates." ;
	fibo-fnd-utl-av:synonym
		"basis rate swap" ,
		"float-float interest rate swap"
		;
	.

fibo-der-rtd-irswp:FloatFloatSingleCurrencyInterestRateSwap
	a owl:Class ;
	rdfs:subClassOf fibo-der-rtd-irswp:FloatFloatInterestRateSwap ;
	rdfs:label "float float single currency interest rate swap" ;
	rdfs:isDefinedBy <https://spec.edmcouncil.org/fibo/ontology/DER/RateDerivatives/IRSwaps/> ;
	owl:equivalentClass [
		a owl:Class ;
		owl:intersectionOf (
			fibo-der-rtd-irswp:FloatFloatInterestRateSwap
			fibo-der-rtd-irswp:SingleCurrencyInterestRateSwap
		) ;
	] ;
	skos:definition "interest rate swap that exchanges cashflows based on two different floating interest rates in the same currency" ;
	fibo-fnd-utl-av:synonym "float-float single-currency interest rate swap" ;
	.

fibo-der-rtd-irswp:FloatingInterestRateLeg
	a owl:Class ;
	rdfs:subClassOf
		fibo-der-drc-swp:FloatingLeg ,
		fibo-der-rtd-irswp:InterestRateSwapLeg ,
		[
			a owl:Restriction ;
			owl:onProperty fibo-der-rtd-irswp:hasInterestCalculationSchedule ;
			owl:someValuesFrom fibo-der-rtd-irswp:SwapStreamInterestCalculationSchedule ;
		] ,
		[
			a owl:Restriction ;
			owl:onProperty fibo-der-rtd-irswp:hasInterestRateResetSchedule ;
			owl:someValuesFrom fibo-der-rtd-irswp:SwapStreamInterestRateResetSchedule ;
		] ,
		[
			a owl:Restriction ;
			owl:onProperty fibo-fbc-fct-ra:specifies ;
			owl:someValuesFrom fibo-der-rtd-irswp:SwapStreamInterestRateReset ;
		] ,
		[
			a owl:Restriction ;
			owl:onProperty fibo-fbc-fct-ra:specifies ;
			owl:someValuesFrom fibo-der-rtd-irswp:SwapStreamInterestRateSettingEvent ;
		]
		;
	rdfs:label "floating interest rate leg" ;
	rdfs:isDefinedBy <https://spec.edmcouncil.org/fibo/ontology/DER/RateDerivatives/IRSwaps/> ;
	owl:equivalentClass [
		a owl:Class ;
		owl:intersectionOf (
			fibo-der-rtd-irswp:InterestRateSwapLeg
			[
				a owl:Restriction ;
				owl:onProperty fibo-fbc-dae-dbt:hasInterestRate ;
				owl:someValuesFrom fibo-fbc-dae-dbt:FloatingInterestRate ;
			]
		) ;
	] ;
	skos:definition "floating leg in which variable interest is paid on some notional amount, linked to some underlying interest reference rate" ;
	fibo-fnd-utl-av:explanatoryNote "Instead of an absolute rate you have either a variable reference rate or fixed reference rate and an offset that varies in some way, called a spread (same as margin in floating rate notes)." ;
	fibo-fnd-utl-av:synonym "floating interest rate swap stream" ;
	.

fibo-der-rtd-irswp:InflationLeg
	a owl:Class ;
	rdfs:subClassOf
		fibo-der-drc-swp:FloatingLeg ,
		[
			a owl:Restriction ;
			owl:onProperty fibo-der-drc-bsc:hasUnderlier ;
			owl:someValuesFrom fibo-ind-ei-ei:EconomicIndicator ;
		]
		;
	rdfs:label "inflation leg"@en ;
	rdfs:isDefinedBy <https://spec.edmcouncil.org/fibo/ontology/DER/RateDerivatives/IRSwaps/> ;
	skos:definition "floating rate leg of an inflation swap linked to an inflation index, such as the Consumer Price Index (CPI)"@en ;
	.

fibo-der-rtd-irswp:InflationSwap
	a owl:Class ;
	rdfs:subClassOf
		fibo-der-drc-swp:Swap ,
		fibo-der-rtd-rtd:RateBasedDerivativeInstrument ,
		[
			a owl:Restriction ;
			owl:onProperty fibo-sec-dbt-bnd:isLinkedToFallback ;
			owl:onClass fibo-sec-dbt-bnd:GovernmentBond ;
			owl:maxQualifiedCardinality "1"^^xsd:nonNegativeInteger ;
		] ,
		[
			a owl:Restriction ;
			owl:onProperty fibo-der-drc-swp:hasLeg ;
			owl:someValuesFrom fibo-der-rtd-irswp:InflationLeg ;
		]
		;
	rdfs:label "inflation swap"@en ;
	rdfs:isDefinedBy <https://spec.edmcouncil.org/fibo/ontology/DER/RateDerivatives/IRSwaps/> ;
	skos:definition "rate swap in which one party pays an amount calculated using an inflation rate index, and the other party pays an amount calculated using another inflation rate index, or a fixed or floating interest rate"@en ;
	fibo-fnd-utl-av:adaptedFrom "ISO 10962, Securities and related financial instruments - Classification of financial instruments (CFI) code, Fourth Edition, 2019."@en ;
	.

fibo-der-rtd-irswp:InterestRateStreamEvent
	a owl:Class ;
	rdfs:subClassOf fibo-der-drc-swp:SwapStreamEvent ;
	rdfs:label "interest rate stream event" ;
	rdfs:isDefinedBy <https://spec.edmcouncil.org/fibo/ontology/DER/RateDerivatives/IRSwaps/> ;
	skos:definition "interest-rate specific event occurring with respect to one leg of a swap" ;
	.

fibo-der-rtd-irswp:InterestRateSwap
	a owl:Class ;
	rdfs:subClassOf
		fibo-der-drc-swp:Swap ,
		fibo-der-rtd-rtd:InterestRateDerivativeInstrument ,
		[
			a owl:Restriction ;
			owl:onProperty fibo-fnd-rel-rel:exchanges ;
			owl:onClass fibo-der-rtd-irswp:InterestRateSwapLeg ;
			owl:qualifiedCardinality "2"^^xsd:nonNegativeInteger ;
		]
		;
	rdfs:label "interest rate swap" ;
	rdfs:isDefinedBy <https://spec.edmcouncil.org/fibo/ontology/DER/RateDerivatives/IRSwaps/> ;
	owl:equivalentClass [
		a owl:Class ;
		owl:intersectionOf (
			fibo-der-drc-swp:Swap
			[
				a owl:Restriction ;
				owl:onProperty fibo-der-drc-swp:hasLeg ;
				owl:onClass fibo-der-rtd-irswp:InterestRateSwapLeg ;
				owl:qualifiedCardinality "2"^^xsd:nonNegativeInteger ;
			]
		) ;
	] ;
	skos:definition "swap in which the reference (underlier) for at least one leg is an interest rate" ;
	.

fibo-der-rtd-irswp:InterestRateSwapLeg
	a owl:Class ;
	rdfs:subClassOf
		fibo-der-drc-swp:SwapLeg ,
		[
			a owl:Restriction ;
			owl:onProperty fibo-fbc-fct-ra:specifies ;
			owl:onClass fibo-der-rtd-irswp:NotionalStepChangeEvent ;
			owl:minQualifiedCardinality "0"^^xsd:nonNegativeInteger ;
		] ,
		[
			a owl:Restriction ;
			owl:onProperty fibo-der-rtd-irswp:hasNotionalStepSchedule ;
			owl:onClass fibo-der-rtd-irswp:NotionalStepSchedule ;
			owl:minQualifiedCardinality "0"^^xsd:nonNegativeInteger ;
		] ,
		[
			a owl:Restriction ;
			owl:onProperty fibo-fbc-fct-ra:specifies ;
			owl:onClass fibo-fnd-acc-cur:Currency ;
			owl:qualifiedCardinality "1"^^xsd:nonNegativeInteger ;
		] ,
		[
			a owl:Restriction ;
			owl:onProperty fibo-fbc-fct-ra:specifies ;
			owl:someValuesFrom fibo-der-rtd-irswp:InterestRateStreamEvent ;
		] ,
		[
			a owl:Restriction ;
			owl:onProperty fibo-fbc-fct-ra:specifies ;
			owl:someValuesFrom fibo-der-rtd-irswp:SwapStreamInterestCalculation ;
		] ,
		[
			a owl:Restriction ;
			owl:onProperty fibo-fbc-fct-ra:specifies ;
			owl:someValuesFrom fibo-der-rtd-irswp:SwapStreamInterestPayment ;
		] ,
		[
			a owl:Restriction ;
			owl:onProperty fibo-fnd-dt-bd:hasBusinessRecurrenceIntervalConvention ;
			owl:someValuesFrom fibo-fbc-dae-dbt:DayCountConvention ;
		] ,
		[
			a owl:Restriction ;
			owl:onProperty fibo-fnd-pas-psch:hasPaymentSchedule ;
			owl:someValuesFrom fibo-der-rtd-irswp:SwapStreamInterestPaymentSchedule ;
		]
		;
	rdfs:label "interest rate swap leg" ;
	rdfs:isDefinedBy <https://spec.edmcouncil.org/fibo/ontology/DER/RateDerivatives/IRSwaps/> ;
	owl:equivalentClass [
		a owl:Class ;
		owl:intersectionOf (
			fibo-der-drc-swp:SwapLeg
			[
				a owl:Restriction ;
				owl:onProperty fibo-fbc-dae-dbt:hasInterestRate ;
				owl:someValuesFrom fibo-fnd-acc-cur:InterestRate ;
			]
		) ;
	] ;
	skos:definition "swap leg specifying an interest rate stream, including both a parametric and cashflow representation for the stream of payments" ;
	fibo-fnd-utl-av:synonym "interest rate swap stream" ;
	.

fibo-der-rtd-irswp:NotionalStepAmount
	a owl:Class ;
	rdfs:subClassOf
		fibo-fnd-qt-qtu:QuantityValue ,
		[
			a owl:Restriction ;
			owl:onProperty fibo-fnd-acc-cur:hasNotionalAmount ;
			owl:someValuesFrom [
				a owl:Class ;
				owl:unionOf (
					fibo-fnd-acc-cur:MonetaryAmount
					fibo-fnd-acc-cur:PercentageMonetaryAmount
				) ;
			] ;
		]
		;
	rdfs:label "notional step amount" ;
	rdfs:isDefinedBy <https://spec.edmcouncil.org/fibo/ontology/DER/RateDerivatives/IRSwaps/> ;
	skos:definition "the amount of money that is subtracted from the notional on each step date" ;
	fibo-fnd-utl-av:explanatoryNote "Note that this is an actual concrete sum of money, which may be specified either as a monetary amount (e.g. dollars and cents) or as a percentage of either the original notional amount or the previous notional amount." ;
	.

fibo-der-rtd-irswp:NotionalStepChangeEvent
	a owl:Class ;
	rdfs:subClassOf
		fibo-der-rtd-irswp:InterestRateStreamEvent ,
		[
			a owl:Restriction ;
			owl:onProperty fibo-fnd-dt-fd:hasDate ;
			owl:someValuesFrom fibo-fnd-dt-fd:CalculatedDate ;
		]
		;
	rdfs:label "notional step change event" ;
	rdfs:isDefinedBy <https://spec.edmcouncil.org/fibo/ontology/DER/RateDerivatives/IRSwaps/> ;
	skos:definition "event in which a step change in the notional amount of the swap stream occurs" ;
	fibo-fnd-utl-av:explanatoryNote "This always occurs on a calculation date (that is, one of the calculation period end dates). Therefore the frequency / period length of the steps in the step schedule is a multiple of the calculation period or frequency. For example, if the notional is recalculated on every calculation date, applying a new interest rate to the new notional amount, then the two frequencies are the same. If notional is updated every second calculation period, then the step schedule specifies periods that are twice as long, and so on." ;
	.

fibo-der-rtd-irswp:NotionalStepPercentageAmount
	a owl:Class ;
	rdfs:subClassOf
		fibo-fnd-acc-cur:PercentageMonetaryAmount ,
		[
			a owl:Restriction ;
			owl:onProperty fibo-fnd-qt-qtu:hasQuantityKind ;
			owl:allValuesFrom fibo-fnd-acc-cur:MonetaryMeasure ;
		]
		;
	rdfs:label "notional step percentage amount" ;
	rdfs:isDefinedBy <https://spec.edmcouncil.org/fibo/ontology/DER/RateDerivatives/IRSwaps/> ;
	skos:definition "the percentage amount by which the notional changes on each step date" ;
	fibo-fnd-utl-av:explanatoryNote "The percentage is either a percentage applied to the initial notional amount or the previous outstanding notional, and may be positive or negative." ;
	.

fibo-der-rtd-irswp:NotionalStepPeriodLength
	a owl:Class ;
	rdfs:subClassOf fibo-fnd-dt-fd:RecurrenceInterval ;
	rdfs:label "notional step period length" ;
	rdfs:isDefinedBy <https://spec.edmcouncil.org/fibo/ontology/DER/RateDerivatives/IRSwaps/> ;
	skos:definition "recurrence interval indicating the frequency with which step changes occur, which is a multiple of the calculation period in the calculation schedule" ;
	.

fibo-der-rtd-irswp:NotionalStepSchedule
	a owl:Class ;
	rdfs:subClassOf
		fibo-sec-sec-sch:ParametricSchedule ,
		[
			a owl:Restriction ;
			owl:onProperty fibo-fbc-fct-ra:specifies ;
			owl:someValuesFrom fibo-der-rtd-irswp:NotionalStepAmount ;
		] ,
		[
			a owl:Restriction ;
			owl:onProperty fibo-fnd-rel-rel:refersTo ;
			owl:someValuesFrom fibo-der-rtd-irswp:SwapStreamInterestCalculationSchedule ;
		]
		;
	rdfs:label "notional step schedule" ;
	rdfs:isDefinedBy <https://spec.edmcouncil.org/fibo/ontology/DER/RateDerivatives/IRSwaps/> ;
	skos:definition "schedule of changes in the notional amount on which interest is paid, comprising the regular sequence of step events" ;
	.

fibo-der-rtd-irswp:PlainVanillaInterestRateSwap
	a owl:Class ;
	rdfs:subClassOf
		fibo-der-rtd-irswp:FixedFloatSingleCurrencyInterestRateSwap ,
		[
			a owl:Restriction ;
			owl:onProperty fibo-fnd-acc-cur:hasNotionalAmount ;
			owl:onClass fibo-fnd-acc-cur:MonetaryAmount ;
			owl:qualifiedCardinality "1"^^xsd:nonNegativeInteger ;
		] ,
		[
			a owl:Restriction ;
			owl:onProperty fibo-der-drc-swp:hasLeg ;
			owl:someValuesFrom [
				a owl:Restriction ;
				owl:onProperty fibo-fbc-fct-ra:specifies ;
				owl:onClass fibo-der-rtd-irswp:NotionalStepChangeEvent ;
				owl:qualifiedCardinality "0"^^xsd:nonNegativeInteger ;
			] ;
		] ,
		[
			a owl:Restriction ;
			owl:onProperty fibo-der-drc-swp:hasLeg ;
			owl:someValuesFrom [
				a owl:Restriction ;
				owl:onProperty fibo-der-rtd-irswp:hasNotionalStepSchedule ;
				owl:onClass fibo-der-rtd-irswp:NotionalStepSchedule ;
				owl:qualifiedCardinality "0"^^xsd:nonNegativeInteger ;
			] ;
		]
		;
	rdfs:label "plain vanilla interest rate swap" ;
	rdfs:isDefinedBy <https://spec.edmcouncil.org/fibo/ontology/DER/RateDerivatives/IRSwaps/> ;
	skos:definition "fixed-float single currency interest rate swap in which interest payments are netted, the notional principal does not change, and there are no embedded options" ;
	.

fibo-der-rtd-irswp:SingleCurrencyInterestRateSwap
	a owl:Class ;
	rdfs:subClassOf
		fibo-der-rtd-irswp:InterestRateSwap ,
		[
			a owl:Restriction ;
			owl:onProperty fibo-fbc-fct-ra:specifies ;
			owl:onClass fibo-fnd-acc-cur:Currency ;
			owl:qualifiedCardinality "1"^^xsd:nonNegativeInteger ;
		]
		;
	rdfs:label "single currency interest rate swap" ;
	rdfs:isDefinedBy <https://spec.edmcouncil.org/fibo/ontology/DER/RateDerivatives/IRSwaps/> ;
	skos:definition "interest rate swap in which the two streams of interest payments are in the same currency" ;
	.

fibo-der-rtd-irswp:SwapStreamCalculationRelativeDate
	a owl:Class ;
	rdfs:subClassOf
		fibo-fnd-dt-fd:RelativeDate ,
		[
			a owl:Restriction ;
			owl:onProperty fibo-fnd-dt-fd:isRelativeTo ;
			owl:someValuesFrom fibo-der-rtd-irswp:SwapStreamInterestRateResetSchedule ;
		]
		;
	rdfs:label "swap stream calculation relative date" ;
	rdfs:isDefinedBy <https://spec.edmcouncil.org/fibo/ontology/DER/RateDerivatives/IRSwaps/> ;
	skos:definition "calculation date that is relative to the rate reset schedule" ;
	.

fibo-der-rtd-irswp:SwapStreamInterestCalculation
	a owl:Class ;
	rdfs:subClassOf fibo-fnd-utl-alx:Expression ;
	rdfs:label "swapstream interest calculation" ;
	rdfs:isDefinedBy <https://spec.edmcouncil.org/fibo/ontology/DER/RateDerivatives/IRSwaps/> ;
	skos:definition "expression that specifies the formula for calculation of interest" ;
	.

fibo-der-rtd-irswp:SwapStreamInterestCalculationSchedule
	a owl:Class ;
	rdfs:subClassOf fibo-sec-sec-sch:ParametricSchedule ;
	rdfs:label "swap stream interest calculation schedule" ;
	rdfs:isDefinedBy <https://spec.edmcouncil.org/fibo/ontology/DER/RateDerivatives/IRSwaps/> ;
	skos:definition "parametric schedule that represents the dates on which interest is calculated" ;
	.

fibo-der-rtd-irswp:SwapStreamInterestPayment
	a owl:Class ;
	rdfs:subClassOf fibo-fnd-pas-psch:Payment ;
	rdfs:label "swap stream interest payment" ;
	rdfs:isDefinedBy <https://spec.edmcouncil.org/fibo/ontology/DER/RateDerivatives/IRSwaps/> ;
	skos:definition "event involving the payment of interest for a given swap leg" ;
	.

fibo-der-rtd-irswp:SwapStreamInterestPaymentSchedule
	a owl:Class ;
	rdfs:subClassOf
		fibo-fnd-pas-psch:PaymentSchedule ,
		fibo-sec-sec-sch:ParametricSchedule
		;
	rdfs:label "swap stream interest payment schedule" ;
	rdfs:isDefinedBy <https://spec.edmcouncil.org/fibo/ontology/DER/RateDerivatives/IRSwaps/> ;
	skos:definition "parametric schedule that represents the dates on which interest is due to be paid" ;
	fibo-fnd-utl-av:explanatoryNote "These may more commonly be expressed as an offset of the calculation dates, however the creation of a schedule specifically for payment dates is allowed for." ;
	.

fibo-der-rtd-irswp:SwapStreamInterestRateReset
	a owl:Class ;
	rdfs:subClassOf fibo-der-rtd-irswp:InterestRateStreamEvent ;
	rdfs:label "swap stream interest rate reset" ;
	rdfs:isDefinedBy <https://spec.edmcouncil.org/fibo/ontology/DER/RateDerivatives/IRSwaps/> ;
	skos:definition "event in which an interest rate for a given swap stream changes (resets)" ;
	.

fibo-der-rtd-irswp:SwapStreamInterestRateResetSchedule
	a owl:Class ;
	rdfs:subClassOf fibo-sec-sec-sch:ParametricSchedule ;
	rdfs:label "swapstream interest rate reset schedule" ;
	rdfs:isDefinedBy <https://spec.edmcouncil.org/fibo/ontology/DER/RateDerivatives/IRSwaps/> ;
	skos:definition "parametric schedule of reset dates" ;
	fibo-fnd-utl-av:explanatoryNote "These may more commonly be expressed as an offset of the calculation dates, however the creation of a schedule specifically for reset dates is allowed for." ;
	.

fibo-der-rtd-irswp:SwapStreamInterestRateSettingEvent
	a owl:Class ;
	rdfs:subClassOf
		fibo-der-rtd-irswp:InterestRateStreamEvent ,
		[
			a owl:Restriction ;
			owl:onProperty fibo-fnd-dt-fd:hasDate ;
			owl:someValuesFrom fibo-der-rtd-irswp:SwapStreamInterestSettingRelativeDate ;
		]
		;
	rdfs:label "swap stream interest rate setting event" ;
	rdfs:isDefinedBy <https://spec.edmcouncil.org/fibo/ontology/DER/RateDerivatives/IRSwaps/> ;
	skos:definition "event in which an interest rate for a given swap stream is determined" ;
	.

fibo-der-rtd-irswp:SwapStreamInterestSettingRelativeDate
	a owl:Class ;
	rdfs:subClassOf
		fibo-fnd-dt-fd:RelativeDate ,
		[
			a owl:Restriction ;
			owl:onProperty fibo-fnd-dt-fd:isRelativeTo ;
			owl:someValuesFrom fibo-der-rtd-irswp:SwapStreamInterestRateReset ;
		]
		;
	rdfs:label "swap stream interest setting relative date" ;
	rdfs:isDefinedBy <https://spec.edmcouncil.org/fibo/ontology/DER/RateDerivatives/IRSwaps/> ;
	skos:definition "date on which an interest rate is revised if that date is relative to a rate reset event" ;
	.

fibo-der-rtd-irswp:hasFirstNotionalStepDate
	a owl:ObjectProperty ;
	rdfs:subPropertyOf fibo-fnd-dt-fd:hasStartDate ;
	rdfs:label "has first notional step date" ;
	rdfs:isDefinedBy <https://spec.edmcouncil.org/fibo/ontology/DER/RateDerivatives/IRSwaps/> ;
	rdfs:range fibo-fnd-dt-fd:ExplicitDate ;
	skos:definition "indicates the initial date in a notional step schedule" ;
	.

fibo-der-rtd-irswp:hasFloatingRateCap
	a owl:ObjectProperty ;
	rdfs:subPropertyOf fibo-fbc-dae-dbt:hasInterestRate ;
	rdfs:label "has floating rate cap" ;
	rdfs:isDefinedBy <https://spec.edmcouncil.org/fibo/ontology/DER/RateDerivatives/IRSwaps/> ;
	rdfs:range fibo-fbc-dae-dbt:FloatingInterestRate ;
	skos:definition "indicates an optional ceiling (cap) on interest rates on floating rate debts" ;
	fibo-fnd-utl-av:explanatoryNote "Rate caps can be viewed as insurance, ensuring that the maximum borrowing rate never exceeds the specified cap level." ;
	.

fibo-der-rtd-irswp:hasFloatingRateFloor
	a owl:ObjectProperty ;
	rdfs:subPropertyOf fibo-fbc-dae-dbt:hasInterestRate ;
	rdfs:label "has floating rate floor" ;
	rdfs:isDefinedBy <https://spec.edmcouncil.org/fibo/ontology/DER/RateDerivatives/IRSwaps/> ;
	rdfs:range fibo-fbc-dae-dbt:FloatingInterestRate ;
	skos:definition "indicates an optional lower bound on interest rates on floating rate debts" ;
	.

fibo-der-rtd-irswp:hasFloatingRateSpread
	a owl:DatatypeProperty ;
	rdfs:label "has floating rate spread" ;
	rdfs:isDefinedBy <https://spec.edmcouncil.org/fibo/ontology/DER/RateDerivatives/IRSwaps/> ;
	rdfs:range xsd:decimal ;
	skos:definition "defines the spread rate that can optionally be used to adjust the floating rate" ;
	fibo-fnd-utl-av:explanatoryNote "Such adjustments may be added to or subtracted from the floating rate." ;
	.

fibo-der-rtd-irswp:hasInterestCalculationSchedule
	a owl:ObjectProperty ;
	rdfs:subPropertyOf fibo-fnd-dt-fd:hasSchedule ;
	rdfs:label "has interest calculation schedule" ;
	rdfs:isDefinedBy <https://spec.edmcouncil.org/fibo/ontology/DER/RateDerivatives/IRSwaps/> ;
	rdfs:range fibo-fnd-dt-fd:RegularSchedule ;
	skos:definition "links a set of terms to a corresponding schedule for calculating interest" ;
	.

fibo-der-rtd-irswp:hasInterestRateResetSchedule
	a owl:ObjectProperty ;
	rdfs:subPropertyOf fibo-fnd-dt-fd:hasSchedule ;
	rdfs:label "has interest rate reset schedule" ;
	rdfs:isDefinedBy <https://spec.edmcouncil.org/fibo/ontology/DER/RateDerivatives/IRSwaps/> ;
	rdfs:range fibo-fnd-dt-fd:Schedule ;
	skos:definition "links a set of terms to a corresponding schedule for resetting the interest rate" ;
	.

fibo-der-rtd-irswp:hasLastNotionalStepDate
	a owl:ObjectProperty ;
	rdfs:subPropertyOf fibo-fnd-dt-fd:hasEndDate ;
	rdfs:label "has last notional step date" ;
	rdfs:isDefinedBy <https://spec.edmcouncil.org/fibo/ontology/DER/RateDerivatives/IRSwaps/> ;
	rdfs:range fibo-fnd-dt-fd:ExplicitDate ;
	skos:definition "indicates the final date in a notional step schedule" ;
	.

fibo-der-rtd-irswp:hasNotionalStepSchedule
	a owl:ObjectProperty ;
	rdfs:subPropertyOf fibo-fnd-dt-fd:hasSchedule ;
	rdfs:label "has notional step schedule" ;
	rdfs:isDefinedBy <https://spec.edmcouncil.org/fibo/ontology/DER/RateDerivatives/IRSwaps/> ;
	rdfs:range fibo-fnd-dt-fd:Schedule ;
	skos:definition "links a set of terms to a corresponding notional step schedule" ;
	.

fibo-der-rtd-irswp:hasRateMultiplier
	a owl:DatatypeProperty ;
	rdfs:label "has rate multiplier" ;
	rdfs:isDefinedBy <https://spec.edmcouncil.org/fibo/ontology/DER/RateDerivatives/IRSwaps/> ;
	rdfs:range xsd:decimal ;
	skos:definition "indicates a multiplier applied to the coupon before adding the floating rate spread" ;
	.

