# baseURI: https://spec.edmcouncil.org/fibo/ontology/master/2021Q4/FBC/ProductsAndServices/FinancialProductsAndServices/
# imports: https://spec.edmcouncil.org/fibo/ontology/master/2021Q4/BE/FunctionalEntities/FunctionalEntities/
# imports: https://spec.edmcouncil.org/fibo/ontology/master/2021Q4/BE/FunctionalEntities/Publishers/
# imports: https://spec.edmcouncil.org/fibo/ontology/master/2021Q4/BE/LegalEntities/LEIEntities/
# imports: https://spec.edmcouncil.org/fibo/ontology/master/2021Q4/BE/LegalEntities/LegalPersons/
# imports: https://spec.edmcouncil.org/fibo/ontology/master/2021Q4/BE/OwnershipAndControl/Executives/
# imports: https://spec.edmcouncil.org/fibo/ontology/master/2021Q4/FBC/FunctionalEntities/RegulatoryAgencies/
# imports: https://spec.edmcouncil.org/fibo/ontology/master/2021Q4/FND/Accounting/CurrencyAmount/
# imports: https://spec.edmcouncil.org/fibo/ontology/master/2021Q4/FND/AgentsAndPeople/Agents/
# imports: https://spec.edmcouncil.org/fibo/ontology/master/2021Q4/FND/Agreements/Contracts/
# imports: https://spec.edmcouncil.org/fibo/ontology/master/2021Q4/FND/Arrangements/Arrangements/
# imports: https://spec.edmcouncil.org/fibo/ontology/master/2021Q4/FND/Arrangements/ClassificationSchemes/
# imports: https://spec.edmcouncil.org/fibo/ontology/master/2021Q4/FND/Arrangements/IdentifiersAndIndices/
# imports: https://spec.edmcouncil.org/fibo/ontology/master/2021Q4/FND/Arrangements/Lifecycles/
# imports: https://spec.edmcouncil.org/fibo/ontology/master/2021Q4/FND/DatesAndTimes/BusinessDates/
# imports: https://spec.edmcouncil.org/fibo/ontology/master/2021Q4/FND/DatesAndTimes/FinancialDates/
# imports: https://spec.edmcouncil.org/fibo/ontology/master/2021Q4/FND/DatesAndTimes/Occurrences/
# imports: https://spec.edmcouncil.org/fibo/ontology/master/2021Q4/FND/GoalsAndObjectives/Objectives/
# imports: https://spec.edmcouncil.org/fibo/ontology/master/2021Q4/FND/Law/Jurisdiction/
# imports: https://spec.edmcouncil.org/fibo/ontology/master/2021Q4/FND/Law/LegalCapacity/
# imports: https://spec.edmcouncil.org/fibo/ontology/master/2021Q4/FND/OwnershipAndControl/Ownership/
# imports: https://spec.edmcouncil.org/fibo/ontology/master/2021Q4/FND/Parties/Parties/
# imports: https://spec.edmcouncil.org/fibo/ontology/master/2021Q4/FND/Parties/Roles/
# imports: https://spec.edmcouncil.org/fibo/ontology/master/2021Q4/FND/ProductsAndServices/ProductsAndServices/
# imports: https://spec.edmcouncil.org/fibo/ontology/master/2021Q4/FND/Quantities/QuantitiesAndUnits/
# imports: https://spec.edmcouncil.org/fibo/ontology/master/2021Q4/FND/Relations/Relations/
# imports: https://spec.edmcouncil.org/fibo/ontology/master/2021Q4/FND/Utilities/Analytics/
# imports: https://spec.edmcouncil.org/fibo/ontology/master/2021Q4/FND/Utilities/AnnotationVocabulary/
# imports: https://www.omg.org/spec/LCC/Countries/CountryRepresentation/
# imports: https://www.omg.org/spec/LCC/Languages/LanguageRepresentation/

@base <https://spec.edmcouncil.org/fibo/ontology/master/2021Q4/FBC/ProductsAndServices/FinancialProductsAndServices/> .
@prefix dct: <http://purl.org/dc/terms/> .
@prefix fibo-be-fct-fct: <https://spec.edmcouncil.org/fibo/ontology/BE/FunctionalEntities/FunctionalEntities/> .
@prefix fibo-be-fct-pub: <https://spec.edmcouncil.org/fibo/ontology/BE/FunctionalEntities/Publishers/> .
@prefix fibo-be-le-lei: <https://spec.edmcouncil.org/fibo/ontology/BE/LegalEntities/LEIEntities/> .
@prefix fibo-be-le-lp: <https://spec.edmcouncil.org/fibo/ontology/BE/LegalEntities/LegalPersons/> .
@prefix fibo-be-oac-exec: <https://spec.edmcouncil.org/fibo/ontology/BE/OwnershipAndControl/Executives/> .
@prefix fibo-fbc-fct-rga: <https://spec.edmcouncil.org/fibo/ontology/FBC/FunctionalEntities/RegulatoryAgencies/> .
@prefix fibo-fbc-pas-fpas: <https://spec.edmcouncil.org/fibo/ontology/FBC/ProductsAndServices/FinancialProductsAndServices/> .
@prefix fibo-fnd-aap-agt: <https://spec.edmcouncil.org/fibo/ontology/FND/AgentsAndPeople/Agents/> .
@prefix fibo-fnd-acc-cur: <https://spec.edmcouncil.org/fibo/ontology/FND/Accounting/CurrencyAmount/> .
@prefix fibo-fnd-agr-ctr: <https://spec.edmcouncil.org/fibo/ontology/FND/Agreements/Contracts/> .
@prefix fibo-fnd-arr-arr: <https://spec.edmcouncil.org/fibo/ontology/FND/Arrangements/Arrangements/> .
@prefix fibo-fnd-arr-lif: <https://spec.edmcouncil.org/fibo/ontology/FND/Arrangements/Lifecycles/> .
@prefix fibo-fnd-dt-fd: <https://spec.edmcouncil.org/fibo/ontology/FND/DatesAndTimes/FinancialDates/> .
@prefix fibo-fnd-dt-oc: <https://spec.edmcouncil.org/fibo/ontology/FND/DatesAndTimes/Occurrences/> .
@prefix fibo-fnd-gao-obj: <https://spec.edmcouncil.org/fibo/ontology/FND/GoalsAndObjectives/Objectives/> .
@prefix fibo-fnd-law-jur: <https://spec.edmcouncil.org/fibo/ontology/FND/Law/Jurisdiction/> .
@prefix fibo-fnd-law-lcap: <https://spec.edmcouncil.org/fibo/ontology/FND/Law/LegalCapacity/> .
@prefix fibo-fnd-oac-own: <https://spec.edmcouncil.org/fibo/ontology/FND/OwnershipAndControl/Ownership/> .
@prefix fibo-fnd-pas-pas: <https://spec.edmcouncil.org/fibo/ontology/FND/ProductsAndServices/ProductsAndServices/> .
@prefix fibo-fnd-pty-pty: <https://spec.edmcouncil.org/fibo/ontology/FND/Parties/Parties/> .
@prefix fibo-fnd-pty-rl: <https://spec.edmcouncil.org/fibo/ontology/FND/Parties/Roles/> .
@prefix fibo-fnd-rel-rel: <https://spec.edmcouncil.org/fibo/ontology/FND/Relations/Relations/> .
@prefix fibo-fnd-utl-alx: <https://spec.edmcouncil.org/fibo/ontology/FND/Utilities/Analytics/> .
@prefix fibo-fnd-utl-av: <https://spec.edmcouncil.org/fibo/ontology/FND/Utilities/AnnotationVocabulary/> .
@prefix lcc-cr: <https://www.omg.org/spec/LCC/Countries/CountryRepresentation/> .
@prefix lcc-lr: <https://www.omg.org/spec/LCC/Languages/LanguageRepresentation/> .
@prefix owl: <http://www.w3.org/2002/07/owl#> .
@prefix rdf: <http://www.w3.org/1999/02/22-rdf-syntax-ns#> .
@prefix rdfs: <http://www.w3.org/2000/01/rdf-schema#> .
@prefix skos: <http://www.w3.org/2004/02/skos/core#> .
@prefix sm: <http://www.omg.org/techprocess/ab/SpecificationMetadata/> .
@prefix xsd: <http://www.w3.org/2001/XMLSchema#> .

<https://spec.edmcouncil.org/fibo/ontology/FBC/ProductsAndServices/FinancialProductsAndServices/>
	a owl:Ontology ;
	rdfs:label "Financial Products and Services Ontology" ;
	dct:abstract "This ontology defines concepts that extend the Foundations (FND) Products and Services concepts specifically for the financial industry, including financial product, financial service, and financial service provider." ;
	dct:license "http://opensource.org/licenses/MIT"^^xsd:anyURI ;
	sm:contentLanguage "https://www.w3.org/TR/owl2-quick-reference/"^^xsd:anyURI ;
	sm:copyright
		"Copyright (c) 2015-2021 EDM Council, Inc." ,
		"Copyright (c) 2015-2021 Object Management Group, Inc."
		;
	sm:dependsOn
		"https://spec.edmcouncil.org/fibo/ontology/BE/"^^xsd:anyURI ,
		"https://spec.edmcouncil.org/fibo/ontology/FBC/FunctionalEntities/RegulatoryAgencies/"^^xsd:anyURI ,
		"https://spec.edmcouncil.org/fibo/ontology/FND/"^^xsd:anyURI ,
		"https://www.omg.org/spec/LCC/"^^xsd:anyURI
		;
	sm:fileAbbreviation "fibo-fbc-pas-fpas" ;
	sm:filename "FinancialProductsAndServices.rdf" ;
	owl:imports
		<https://spec.edmcouncil.org/fibo/ontology/master/2021Q4/BE/FunctionalEntities/FunctionalEntities/> ,
		<https://spec.edmcouncil.org/fibo/ontology/master/2021Q4/BE/FunctionalEntities/Publishers/> ,
		<https://spec.edmcouncil.org/fibo/ontology/master/2021Q4/BE/LegalEntities/LEIEntities/> ,
		<https://spec.edmcouncil.org/fibo/ontology/master/2021Q4/BE/LegalEntities/LegalPersons/> ,
		<https://spec.edmcouncil.org/fibo/ontology/master/2021Q4/BE/OwnershipAndControl/Executives/> ,
		<https://spec.edmcouncil.org/fibo/ontology/master/2021Q4/FBC/FunctionalEntities/RegulatoryAgencies/> ,
		<https://spec.edmcouncil.org/fibo/ontology/master/2021Q4/FND/Accounting/CurrencyAmount/> ,
		<https://spec.edmcouncil.org/fibo/ontology/master/2021Q4/FND/AgentsAndPeople/Agents/> ,
		<https://spec.edmcouncil.org/fibo/ontology/master/2021Q4/FND/Agreements/Contracts/> ,
		<https://spec.edmcouncil.org/fibo/ontology/master/2021Q4/FND/Arrangements/Arrangements/> ,
		<https://spec.edmcouncil.org/fibo/ontology/master/2021Q4/FND/Arrangements/ClassificationSchemes/> ,
		<https://spec.edmcouncil.org/fibo/ontology/master/2021Q4/FND/Arrangements/IdentifiersAndIndices/> ,
		<https://spec.edmcouncil.org/fibo/ontology/master/2021Q4/FND/Arrangements/Lifecycles/> ,
		<https://spec.edmcouncil.org/fibo/ontology/master/2021Q4/FND/DatesAndTimes/BusinessDates/> ,
		<https://spec.edmcouncil.org/fibo/ontology/master/2021Q4/FND/DatesAndTimes/FinancialDates/> ,
		<https://spec.edmcouncil.org/fibo/ontology/master/2021Q4/FND/DatesAndTimes/Occurrences/> ,
		<https://spec.edmcouncil.org/fibo/ontology/master/2021Q4/FND/GoalsAndObjectives/Objectives/> ,
		<https://spec.edmcouncil.org/fibo/ontology/master/2021Q4/FND/Law/Jurisdiction/> ,
		<https://spec.edmcouncil.org/fibo/ontology/master/2021Q4/FND/Law/LegalCapacity/> ,
		<https://spec.edmcouncil.org/fibo/ontology/master/2021Q4/FND/OwnershipAndControl/Ownership/> ,
		<https://spec.edmcouncil.org/fibo/ontology/master/2021Q4/FND/Parties/Parties/> ,
		<https://spec.edmcouncil.org/fibo/ontology/master/2021Q4/FND/Parties/Roles/> ,
		<https://spec.edmcouncil.org/fibo/ontology/master/2021Q4/FND/ProductsAndServices/ProductsAndServices/> ,
		<https://spec.edmcouncil.org/fibo/ontology/master/2021Q4/FND/Quantities/QuantitiesAndUnits/> ,
		<https://spec.edmcouncil.org/fibo/ontology/master/2021Q4/FND/Relations/Relations/> ,
		<https://spec.edmcouncil.org/fibo/ontology/master/2021Q4/FND/Utilities/Analytics/> ,
		<https://spec.edmcouncil.org/fibo/ontology/master/2021Q4/FND/Utilities/AnnotationVocabulary/> ,
		<https://www.omg.org/spec/LCC/Countries/CountryRepresentation/> ,
		<https://www.omg.org/spec/LCC/Languages/LanguageRepresentation/>
		;
	owl:versionIRI <https://spec.edmcouncil.org/fibo/ontology/master/2021Q4/FBC/ProductsAndServices/FinancialProductsAndServices/> ;
	skos:changeNote
		"The https://spec.edmcouncil.org/fibo/ontology/FBC/ProductsAndServices/FinancialProductsAndServices/ version of this ontology was modified as a part of organizational hierarchy simplification and to correct a logical inconsistency with respect to the representation of baskets." ,
		"The https://spec.edmcouncil.org/fibo/ontology/FBC/ProductsAndServices/FinancialProductsAndServices/ version of this ontology was modified by the FIBO 2.0 RFC, including, but not limited to, the addition of lifecycle events, concepts related to trade settlement, and the definition of a unique transaction identifier (UTI)." ,
		"The https://spec.edmcouncil.org/fibo/ontology/FBC/ProductsAndServices/FinancialProductsAndServices/ version of this ontology was modified to add a property to describe the criteria for including something in a basket, if that criteria is known, and to point to a party that is responsible for determining that criteria." ,
		"The https://spec.edmcouncil.org/fibo/ontology/FBC/ProductsAndServices/FinancialProductsAndServices/ version of this ontology was modified to add the notion of a weighted basket, whose consituents are weighted." ,
		"The https://spec.edmcouncil.org/fibo/ontology/FBC/ProductsAndServices/FinancialProductsAndServices/ version of this ontology was modified to eliminate deprecated elements." ,
		"The https://spec.edmcouncil.org/fibo/ontology/FBC/ProductsAndServices/FinancialProductsAndServices/ version of this ontology was modified to eliminate duplication with concepts in LCC and eliminated a redundant superclass on FinancialServiceProvider." ,
		"The https://spec.edmcouncil.org/fibo/ontology/FBC/ProductsAndServices/FinancialProductsAndServices/ version of this ontology was modified to eliminate references to external dictionary sites that no longer resolve, eliminate circular and ambiguous definitions, and revise definitions that referenced 'face value' improperly." ,
		"The https://spec.edmcouncil.org/fibo/ontology/FBC/ProductsAndServices/FinancialProductsAndServices/ version of this ontology was modified to fix spelling errors." ,
		"The https://spec.edmcouncil.org/fibo/ontology/FBC/ProductsAndServices/FinancialProductsAndServices/ version of this ontology was modified to reflect issue resolutions detailed in the FIBO FBC 1.0 FTF report." ,
		"The https://spec.edmcouncil.org/fibo/ontology/FBC/ProductsAndServices/FinancialProductsAndServices/ version of this ontology was modified to rename ownership related properties for consistent alignment with the ownership situational pattern, add a definition for trading strategy, and loosen the constraint on offeree for offering to be optional." ,
		"The https://spec.edmcouncil.org/fibo/ontology/FBC/ProductsAndServices/FinancialProductsAndServices/ version of this ontology was modified to replace hasDefinition with isDefinedIn to clarify intent." ,
		"The https://spec.edmcouncil.org/fibo/ontology/FBC/ProductsAndServices/FinancialProductsAndServices/ version of this ontology was modified to replace the property 'characterizes' with 'describes' with respect to restrictions on catalogs, and to correct the label on terminated trade."
		;
	fibo-fnd-utl-av:hasMaturityLevel fibo-fnd-utl-av:Release ;
	.

fibo-fbc-pas-fpas:AgencyAgreement
	a owl:Class ;
	rdfs:subClassOf
		fibo-fnd-agr-ctr:MutualContractualAgreement ,
		[
			a owl:Restriction ;
			owl:onProperty fibo-fnd-agr-ctr:hasContractParty ;
			owl:someValuesFrom fibo-fbc-pas-fpas:RegisteredAgent ;
		]
		;
	rdfs:label "agency agreement" ;
	rdfs:isDefinedBy <https://spec.edmcouncil.org/fibo/ontology/FBC/ProductsAndServices/FinancialProductsAndServices/> ;
	rdfs:seeAlso <http://www.sos.state.tx.us/corp/registeredagents.shtml> ;
	skos:definition "an agreement that designates a party as a registered agent to represent and act on behalf of another party in some, typically legal, financial, or medical capacity" ;
	.

fibo-fbc-pas-fpas:AgentForServiceOfProcess
	a owl:Class ;
	rdfs:subClassOf fibo-fbc-pas-fpas:RegisteredAgent ;
	rdfs:label "agent for service of process" ;
	rdfs:isDefinedBy <https://spec.edmcouncil.org/fibo/ontology/FBC/ProductsAndServices/FinancialProductsAndServices/> ;
	rdfs:seeAlso
		<http://www.law.cornell.edu/wex/agent_for_service_of_process> ,
		<http://www.sos.state.tx.us/corp/registeredagents.shtml>
		;
	skos:definition "a registered agent (person or organization) designated by a business entity, such as a corporation, to receive legal correspondence on behalf of the business entity in the jurisdiction in which the agent's address is located" ;
	fibo-fnd-utl-av:explanatoryNote "The person may be an officer of the corporation or a third party, such as the corporation's attorney, or a company providing such agency services." ;
	.

fibo-fbc-pas-fpas:AmendedTrade
	a
		owl:NamedIndividual ,
		fibo-fbc-pas-fpas:TradeLifecycleStage
		;
	rdfs:label "amended trade" ;
	rdfs:isDefinedBy <https://spec.edmcouncil.org/fibo/ontology/FBC/ProductsAndServices/FinancialProductsAndServices/> ;
	skos:definition "stage in the lifecycle of a trade indicating that a change or addition has been made to the terms of the trade, leaving the original terms largely intact" ;
	.

fibo-fbc-pas-fpas:Basket
	a owl:Class ;
	rdfs:subClassOf
		lcc-lr:Collection ,
		[
			a owl:Restriction ;
			owl:onProperty fibo-fbc-pas-fpas:hasSelectingParty ;
			owl:onClass fibo-fnd-pty-pty:IndependentParty ;
			owl:minQualifiedCardinality "0"^^xsd:nonNegativeInteger ;
		] ,
		[
			a owl:Restriction ;
			owl:onProperty fibo-fbc-pas-fpas:hasSelectionCriteria ;
			owl:minQualifiedCardinality "0"^^xsd:nonNegativeInteger ;
			owl:onDataRange xsd:string ;
		] ,
		[
			a owl:Restriction ;
			owl:onProperty fibo-fnd-arr-arr:hasConstituent ;
			owl:someValuesFrom fibo-fbc-pas-fpas:BasketConstituent ;
		]
		;
	rdfs:label "basket" ;
	rdfs:isDefinedBy <https://spec.edmcouncil.org/fibo/ontology/FBC/ProductsAndServices/FinancialProductsAndServices/> ;
	skos:definition "collection of goods, services, or other things (e.g., financial contracts) that can be purchased and sold in some marketplace" ;
	fibo-fnd-utl-av:explanatoryNote
		"A basket may be associated with a specific market sector, and may be delineated for the purposes of statistical analysis, such as for calculating CPI. According to the US Bureau of Labor Statistics (BLS), with respect to the CPI, a market basket is a package of goods and services that consumers purchase for day-to-day living. The weight of each item is based on the amount of expenditure reported by a sample of households." ,
		"From a securities perspective, a basket is a collection of products or securities that are designated to mimic the performance of a market. For investors, the market basket is the principal idea behind index funds, which are essentially a broad sample of stocks, bonds or other securities in the market; this provides investors with a benchmark against which to compare their investment returns."
		;
	.

fibo-fbc-pas-fpas:BasketConstituent
	a owl:Class ;
	rdfs:subClassOf fibo-fnd-arr-arr:CollectionConstituent ;
	rdfs:label "basket constituent" ;
	rdfs:isDefinedBy <https://spec.edmcouncil.org/fibo/ontology/FBC/ProductsAndServices/FinancialProductsAndServices/> ;
	owl:equivalentClass [
		a owl:Restriction ;
		owl:onProperty fibo-fnd-arr-arr:isConstituentOf ;
		owl:someValuesFrom fibo-fbc-pas-fpas:Basket ;
	] ;
	skos:definition "component of a basket" ;
	.

fibo-fbc-pas-fpas:Broker
	a owl:Class ;
	rdfs:subClassOf
		fibo-fnd-agr-ctr:ContractThirdParty ,
		[
			a owl:Class ;
			owl:unionOf (
				fibo-fbc-pas-fpas:LicensedAgent
				fibo-fbc-pas-fpas:ThirdPartyAgent
			) ;
		]
		;
	rdfs:label "broker" ;
	rdfs:isDefinedBy <https://spec.edmcouncil.org/fibo/ontology/FBC/ProductsAndServices/FinancialProductsAndServices/> ;
	skos:definition "any party that acts as an intermediary between a buyer and a seller, usually charging a commission" ;
	fibo-fnd-utl-av:adaptedFrom "17 CFR 45.1, Definitions - see the definition of agent" ;
	fibo-fnd-utl-av:explanatoryNote "A broker that specializes in stocks, bonds, commodities, or certain derivatives must be registered with the exchange in which the securities are traded." ;
	.

fibo-fbc-pas-fpas:BrokerDealer
	a owl:Class ;
	rdfs:subClassOf
		fibo-be-fct-fct:FunctionalEntity ,
		[
			a owl:Class ;
			owl:unionOf (
				fibo-fbc-pas-fpas:Broker
				fibo-fbc-pas-fpas:Dealer
			) ;
		]
		;
	rdfs:label "broker-dealer" ;
	rdfs:isDefinedBy <https://spec.edmcouncil.org/fibo/ontology/FBC/ProductsAndServices/FinancialProductsAndServices/> ;
	skos:definition "any party in the business of buying and selling securities, operating as both a broker and a dealer, depending on the transaction" ;
	fibo-fnd-utl-av:adaptedFrom "Office of Financial Research (OFR) Annual Report, 2012, Glossary" ;
	.

fibo-fbc-pas-fpas:Catalog
	a owl:Class ;
	rdfs:subClassOf
		fibo-be-fct-pub:Publication ,
		[
			a owl:Restriction ;
			owl:onProperty lcc-lr:isIdentifiedBy ;
			owl:allValuesFrom lcc-lr:Identifier ;
		] ,
		[
			a owl:Restriction ;
			owl:onProperty fibo-fnd-rel-rel:describes ;
			owl:someValuesFrom fibo-fnd-pas-pas:Product ;
		]
		;
	rdfs:label "catalog" ;
	rdfs:isDefinedBy <https://spec.edmcouncil.org/fibo/ontology/FBC/ProductsAndServices/FinancialProductsAndServices/> ;
	skos:definition "publication including a list of products available for sale with their descriptions and possibly prices" ;
	.

fibo-fbc-pas-fpas:ClearedTrade
	a
		owl:NamedIndividual ,
		fibo-fbc-pas-fpas:TradeLifecycleStage
		;
	rdfs:label "cleared trade" ;
	rdfs:isDefinedBy <https://spec.edmcouncil.org/fibo/ontology/FBC/ProductsAndServices/FinancialProductsAndServices/> ;
	skos:definition "stage in the lifecycle of a trade indicating that a third-party clearing house, acting as an intermediary, has reconciled the orders involved in the trade" ;
	fibo-fnd-utl-av:explanatoryNote "Clearing validates the availability of funds, records the transfer, and in the case of securities ensures the delivery of the security to the buyer." ;
	.

fibo-fbc-pas-fpas:ClosedTrade
	a
		owl:NamedIndividual ,
		fibo-fbc-pas-fpas:TradeLifecycleStage
		;
	rdfs:label "closed trade" ;
	rdfs:isDefinedBy <https://spec.edmcouncil.org/fibo/ontology/FBC/ProductsAndServices/FinancialProductsAndServices/> ;
	skos:definition "stage in the lifecycle of a trade indicating that the trade has been finalized, and that there is no longer a corresponding open position on the books of the trader, eliminating any exposure" ;
	.

fibo-fbc-pas-fpas:Dealer
	a owl:Class ;
	rdfs:subClassOf
		fibo-fnd-pas-pas:ServiceProvider ,
		[
			a owl:Class ;
			owl:unionOf (
				fibo-fnd-pas-pas:Buyer
				fibo-fnd-pas-pas:Seller
			) ;
		]
		;
	rdfs:label "dealer" ;
	rdfs:isDefinedBy <https://spec.edmcouncil.org/fibo/ontology/FBC/ProductsAndServices/FinancialProductsAndServices/> ;
	skos:definition "any party that purchases goods or services for resale and acts on their own behalf in a transaction" ;
	fibo-fnd-utl-av:explanatoryNote "A dealer is a counterparty or principal in the transaction with the customer." ;
	.

fibo-fbc-pas-fpas:Exposure
	a owl:Class ;
	rdfs:label "exposure" ;
	rdfs:isDefinedBy <https://spec.edmcouncil.org/fibo/ontology/FBC/ProductsAndServices/FinancialProductsAndServices/> ;
	skos:definition "the extent to which an individual or organization is unprotected and open to damage, danger, risk of suffering a loss, or uncertainty" ;
	skos:example "Examples include financial exposure, credit exposure, legal exposure, credit rating exposure, reputational exposure, and so forth." ;
	.

fibo-fbc-pas-fpas:FinancialExposure
	a owl:Class ;
	rdfs:subClassOf
		fibo-fbc-pas-fpas:Exposure ,
		[
			a owl:Restriction ;
			owl:onProperty fibo-fnd-rel-rel:appliesTo ;
			owl:someValuesFrom fibo-fnd-pty-pty:PartyInRole ;
		]
		;
	rdfs:label "financial exposure" ;
	rdfs:isDefinedBy <https://spec.edmcouncil.org/fibo/ontology/FBC/ProductsAndServices/FinancialProductsAndServices/> ;
	skos:definition "the extent to which an individual or organization is open to risk of suffering a loss in a transaction, or with respect to some investment or set of investments, e.g., some holding; the amount one stands to lose in that transaction or investment" ;
	skos:example "Examples in banking include the total amount of unsecured loans, the amount of loans advanced to a single borrower, group, industry, or country, and the probability of loss from devaluation, revaluation, or foreign exchange fluctuations." ;
	.

fibo-fbc-pas-fpas:FinancialIntermediationService
	a owl:Class ;
	rdfs:subClassOf fibo-fbc-pas-fpas:FinancialService ;
	rdfs:label "financial intermediation service" ;
	rdfs:isDefinedBy <https://spec.edmcouncil.org/fibo/ontology/FBC/ProductsAndServices/FinancialProductsAndServices/> ;
	skos:definition "any financial service in which a third party (the intermediary) matches lenders and investors with entrepreneurs and other borrowers in need of capital" ;
	fibo-fnd-utl-av:definitionOrigin "Office of Financial Research (OFR) Annual Report, 2012, Glossary" ;
	fibo-fnd-utl-av:explanatoryNote "Often investors and borrowers do not have precisely matching needs, and the intermediary's capital is put at risk to transform the credit risk and maturity of the liabilities to meet the needs of investors." ;
	.

fibo-fbc-pas-fpas:FinancialProduct
	a owl:Class ;
	rdfs:subClassOf
		fibo-fnd-pas-pas:Product ,
		[
			a owl:Restriction ;
			owl:onProperty fibo-fnd-rel-rel:isProvidedBy ;
			owl:someValuesFrom fibo-fbc-pas-fpas:FinancialServiceProvider ;
		]
		;
	rdfs:label "financial product" ;
	rdfs:isDefinedBy <https://spec.edmcouncil.org/fibo/ontology/FBC/ProductsAndServices/FinancialProductsAndServices/> ;
	skos:definition "product provided to consumers and businesses by financial institutions such as banks, insurance companies, brokerage firms, consumer finance companies, and investment companies" ;
	.

fibo-fbc-pas-fpas:FinancialProductCatalog
	a owl:Class ;
	rdfs:subClassOf
		fibo-fbc-pas-fpas:Catalog ,
		[
			a owl:Restriction ;
			owl:onProperty fibo-fnd-rel-rel:describes ;
			owl:someValuesFrom fibo-fbc-pas-fpas:FinancialProduct ;
		]
		;
	rdfs:label "financial product catalog" ;
	rdfs:isDefinedBy <https://spec.edmcouncil.org/fibo/ontology/FBC/ProductsAndServices/FinancialProductsAndServices/> ;
	skos:definition "a catalog of financial products and/or services available for sale with their description and other product details" ;
	fibo-fnd-utl-av:adaptedFrom "Nordea Bank" ;
	.

fibo-fbc-pas-fpas:FinancialService
	a owl:Class ;
	rdfs:subClassOf
		fibo-fnd-pas-pas:Service ,
		[
			a owl:Restriction ;
			owl:onProperty fibo-fnd-rel-rel:isProvidedBy ;
			owl:someValuesFrom fibo-fbc-pas-fpas:FinancialServiceProvider ;
		]
		;
	rdfs:label "financial service" ;
	rdfs:isDefinedBy <https://spec.edmcouncil.org/fibo/ontology/FBC/ProductsAndServices/FinancialProductsAndServices/> ;
	skos:definition "service provided to consumers and businesses by financial institutions such as banks, insurance companies, brokerage firms, consumer finance companies, and investment companies" ;
	.

fibo-fbc-pas-fpas:FinancialServiceProvider
	a owl:Class ;
	rdfs:subClassOf
		fibo-fnd-pas-pas:ServiceProvider ,
		[
			a owl:Restriction ;
			owl:onProperty fibo-fnd-rel-rel:hasIdentity ;
			owl:onClass fibo-be-le-lp:LegalEntity ;
			owl:qualifiedCardinality "1"^^xsd:nonNegativeInteger ;
		] ,
		[
			a owl:Restriction ;
			owl:onProperty fibo-fnd-rel-rel:provides ;
			owl:someValuesFrom fibo-fbc-pas-fpas:FinancialService ;
		]
		;
	rdfs:label "financial service provider" ;
	rdfs:isDefinedBy <https://spec.edmcouncil.org/fibo/ontology/FBC/ProductsAndServices/FinancialProductsAndServices/> ;
	skos:definition "functional entity either licensed to provide financial services to consumers and/or businesses or established by law to provide financial services, such as a central bank" ;
	.

fibo-fbc-pas-fpas:Holding
	a owl:Class ;
	rdfs:subClassOf
		fibo-fnd-oac-own:Ownership ,
		[
			a owl:Restriction ;
			owl:onProperty fibo-fnd-oac-own:hasOwnedAsset ;
			owl:someValuesFrom fibo-fnd-oac-own:Asset ;
		]
		;
	rdfs:label "holding" ;
	rdfs:isDefinedBy <https://spec.edmcouncil.org/fibo/ontology/FBC/ProductsAndServices/FinancialProductsAndServices/> ;
	skos:definition "real or personal property (assets), including but not limited to financial assets, to which one holds title and of which one has possession" ;
	fibo-fnd-utl-av:explanatoryNote "Note that a holding may refer to a single asset, such as a piece of real estate, a portfolio of assets, multiple portfolios, and so forth, and is frequently aggregated over multiple assets." ;
	.

fibo-fbc-pas-fpas:LegalAgent
	a owl:Class ;
	rdfs:subClassOf
		fibo-fnd-pty-rl:AgentInRole ,
		[
			a owl:Restriction ;
			owl:onProperty fibo-fnd-pty-rl:isPlayedBy ;
			owl:someValuesFrom [
				a owl:Restriction ;
				owl:onProperty fibo-fnd-law-lcap:hasCapacity ;
				owl:someValuesFrom fibo-fnd-law-lcap:DelegatedLegalAuthority ;
			] ;
		]
		;
	rdfs:label "legal agent" ;
	rdfs:isDefinedBy <https://spec.edmcouncil.org/fibo/ontology/FBC/ProductsAndServices/FinancialProductsAndServices/> ;
	skos:definition "any party that has been legally empowered to act on behalf of another party" ;
	fibo-fnd-utl-av:adaptedFrom "17 CFR 45.1, Definitions - see the definition of agent" ;
	.

fibo-fbc-pas-fpas:LicensedAgent
	a owl:Class ;
	rdfs:subClassOf
		fibo-be-oac-exec:ResponsibleParty ,
		fibo-fbc-pas-fpas:LegalAgent ,
		fibo-fnd-law-lcap:Licensee
		;
	rdfs:label "licensed agent" ;
	rdfs:isDefinedBy <https://spec.edmcouncil.org/fibo/ontology/FBC/ProductsAndServices/FinancialProductsAndServices/> ;
	skos:definition "any individual who is licensed to perform a legally binding function, and who has been legally empowered to act on behalf of another party" ;
	skos:example "Insurance agents, realtors, financial advisors, certain attorneys, and brokers are examples of legal agents." ;
	fibo-fnd-utl-av:adaptedFrom "17 CFR 45.1, Definitions - see the definition of agent" ;
	.

fibo-fbc-pas-fpas:MaturedTrade
	a
		owl:NamedIndividual ,
		fibo-fbc-pas-fpas:TradeLifecycleStage
		;
	rdfs:label "matured trade" ;
	rdfs:isDefinedBy <https://spec.edmcouncil.org/fibo/ontology/FBC/ProductsAndServices/FinancialProductsAndServices/> ;
	skos:definition "stage in the lifecycle of a trade indicating that the trade, and related instrument(s) has ended (expired)" ;
	.

fibo-fbc-pas-fpas:Offeree
	a owl:Class ;
	rdfs:subClassOf
		fibo-fnd-pty-pty:PartyInRole ,
		[
			a owl:Restriction ;
			owl:onProperty fibo-fnd-pty-rl:isPlayedBy ;
			owl:someValuesFrom [
				a owl:Restriction ;
				owl:onProperty fibo-fnd-pty-pty:isAPartyTo ;
				owl:someValuesFrom fibo-fbc-pas-fpas:Offering ;
			] ;
		]
		;
	rdfs:label "offeree" ;
	rdfs:isDefinedBy <https://spec.edmcouncil.org/fibo/ontology/FBC/ProductsAndServices/FinancialProductsAndServices/> ;
	skos:definition "party that receives an offer from something from someone (i.e., an offerer) based on the terms of the offering" ;
	.

fibo-fbc-pas-fpas:Offering
	a owl:Class ;
	rdfs:subClassOf
		[
			a owl:Restriction ;
			owl:onProperty fibo-fnd-pty-pty:hasPartyInRole ;
			owl:onClass fibo-fbc-pas-fpas:Offeree ;
			owl:minQualifiedCardinality "0"^^xsd:nonNegativeInteger ;
		] ,
		[
			a owl:Restriction ;
			owl:onProperty fibo-fnd-pty-pty:hasPartyInRole ;
			owl:someValuesFrom fibo-fbc-pas-fpas:Offeror ;
		] ,
		[
			a owl:Restriction ;
			owl:onProperty fibo-fnd-rel-rel:appliesTo ;
			owl:someValuesFrom owl:Thing ;
		] ,
		[
			a owl:Restriction ;
			owl:onProperty fibo-fnd-rel-rel:isIssuedBy ;
			owl:someValuesFrom fibo-fbc-pas-fpas:Offeror ;
		]
		;
	rdfs:label "offering" ;
	rdfs:isDefinedBy <https://spec.edmcouncil.org/fibo/ontology/FBC/ProductsAndServices/FinancialProductsAndServices/> ;
	skos:definition "expression of interest in providing something to someone that is contingent upon acceptance, forbearance, or some other consideration, as might be desired by an offeree(s)" ;
	fibo-fnd-utl-av:explanatoryNote "The making of an offer is the first of three steps in the traditional process of forming a valid contract: an offer, an acceptance of the offer, and an exchange of consideration. (Consideration is the act of doing something or promising to do something that a person is not legally required to do, or the forbearance or the promise to forbear from doing something that he or she has the legal right to do.)" ;
	.

fibo-fbc-pas-fpas:Offeror
	a owl:Class ;
	rdfs:subClassOf
		fibo-fnd-pty-pty:PartyInRole ,
		[
			a owl:Restriction ;
			owl:onProperty fibo-fnd-pty-rl:isPlayedBy ;
			owl:someValuesFrom [
				a owl:Restriction ;
				owl:onProperty fibo-fnd-pty-pty:isAPartyTo ;
				owl:someValuesFrom fibo-fbc-pas-fpas:Offering ;
			] ;
		] ,
		[
			a owl:Restriction ;
			owl:onProperty fibo-fnd-rel-rel:issues ;
			owl:someValuesFrom fibo-fbc-pas-fpas:Offering ;
		]
		;
	rdfs:label "offeror" ;
	rdfs:isDefinedBy <https://spec.edmcouncil.org/fibo/ontology/FBC/ProductsAndServices/FinancialProductsAndServices/> ;
	skos:definition "a party that proposes to make something available to someone (i.e., an offeree) based on the terms of the offering" ;
	.

fibo-fbc-pas-fpas:OpenTrade
	a
		owl:NamedIndividual ,
		fibo-fbc-pas-fpas:TradeLifecycleStage
		;
	rdfs:label "open trade" ;
	rdfs:isDefinedBy <https://spec.edmcouncil.org/fibo/ontology/FBC/ProductsAndServices/FinancialProductsAndServices/> ;
	skos:definition "stage in the lifecycle of a trade indicating that the trade has been established and there is an associated open position on the books of the trader as a consequence" ;
	.

fibo-fbc-pas-fpas:Position
	a owl:Class ;
	rdfs:subClassOf
		fibo-fbc-pas-fpas:Holding ,
		[
			a owl:Restriction ;
			owl:onProperty fibo-fnd-oac-own:hasOwnedAsset ;
			owl:onClass fibo-fnd-oac-own:Asset ;
			owl:qualifiedCardinality "1"^^xsd:nonNegativeInteger ;
		]
		;
	rdfs:label "position" ;
	rdfs:isDefinedBy <https://spec.edmcouncil.org/fibo/ontology/FBC/ProductsAndServices/FinancialProductsAndServices/> ;
	skos:definition "an investor's stake, i.e., a holding, in a particular asset (such as an individual security)" ;
	fibo-fnd-utl-av:explanatoryNote "A position can be long or short, and it can be in any asset class, such as stocks, bonds, futures, or options. A position can be open (current) or closed (past), but in general use, unless a position is specifically referred to as closed, the assumption is that it references an open position." ;
	.

fibo-fbc-pas-fpas:ProductLifecycle
	a owl:Class ;
	rdfs:subClassOf
		fibo-fnd-arr-lif:Lifecycle ,
		[
			a owl:Restriction ;
			owl:onProperty fibo-fnd-arr-lif:hasStage ;
			owl:someValuesFrom fibo-fbc-pas-fpas:ProductLifecycleStage ;
		] ,
		[
			a owl:Restriction ;
			owl:onProperty fibo-fnd-arr-lif:isLifecycleOf ;
			owl:someValuesFrom fibo-fnd-pas-pas:Product ;
		] ,
		[
			a owl:Restriction ;
			owl:onProperty fibo-fnd-rel-rel:defines ;
			owl:someValuesFrom fibo-fbc-pas-fpas:ProductLifecycleStage ;
		]
		;
	rdfs:label "product lifecycle" ;
	rdfs:isDefinedBy <https://spec.edmcouncil.org/fibo/ontology/FBC/ProductsAndServices/FinancialProductsAndServices/> ;
	skos:definition "a lifecycle specific to a product or product family" ;
	skos:example "The product life cycle describes the period of time over which an item is developed, brought to market and eventually removed from the market. The cycle is broken into four stages: introduction, growth, maturity and decline. The idea of the product life cycle is used in marketing to decide when it is appropriate to advertise, reduce prices, explore new markets or create new packaging." ;
	.

fibo-fbc-pas-fpas:ProductLifecycleEvent
	a owl:Class ;
	rdfs:subClassOf
		fibo-fnd-arr-lif:LifecycleEvent ,
		[
			a owl:Restriction ;
			owl:onProperty fibo-fnd-rel-rel:appliesTo ;
			owl:someValuesFrom fibo-fbc-pas-fpas:ProductLifecycleStage ;
		]
		;
	rdfs:label "product lifecycle event" ;
	rdfs:isDefinedBy <https://spec.edmcouncil.org/fibo/ontology/FBC/ProductsAndServices/FinancialProductsAndServices/> ;
	skos:definition "a kind of event that occurs during one or more stages of a product lifecycle" ;
	skos:example "a call notification or coupon payment as a part of a bond lifecycle" ;
	.

fibo-fbc-pas-fpas:ProductLifecycleEventOccurrence
	a owl:Class ;
	rdfs:subClassOf
		fibo-fnd-arr-lif:LifecycleEventOccurrence ,
		[
			a owl:Restriction ;
			owl:onProperty fibo-fnd-dt-oc:exemplifies ;
			owl:onClass fibo-fbc-pas-fpas:ProductLifecycleEvent ;
			owl:qualifiedCardinality "1"^^xsd:nonNegativeInteger ;
		] ,
		[
			a owl:Restriction ;
			owl:onProperty fibo-fnd-rel-rel:appliesTo ;
			owl:someValuesFrom fibo-fbc-pas-fpas:ProductLifecycleStageOccurrence ;
		]
		;
	rdfs:label "product lifecycle event occurrence" ;
	rdfs:isDefinedBy <https://spec.edmcouncil.org/fibo/ontology/FBC/ProductsAndServices/FinancialProductsAndServices/> ;
	skos:definition "an occurrence of an event that occurs during a specific stage of a specific product lifecycle" ;
	.

fibo-fbc-pas-fpas:ProductLifecycleOccurrence
	a owl:Class ;
	rdfs:subClassOf
		fibo-fnd-arr-lif:LifecycleOccurrence ,
		[
			a owl:Restriction ;
			owl:onProperty fibo-fnd-dt-oc:exemplifies ;
			owl:onClass fibo-fbc-pas-fpas:ProductLifecycle ;
			owl:qualifiedCardinality "1"^^xsd:nonNegativeInteger ;
		] ,
		[
			a owl:Restriction ;
			owl:onProperty fibo-fnd-arr-lif:hasStage ;
			owl:someValuesFrom fibo-fbc-pas-fpas:ProductLifecycleStageOccurrence ;
		]
		;
	rdfs:label "product lifecycle occurrence" ;
	rdfs:isDefinedBy <https://spec.edmcouncil.org/fibo/ontology/FBC/ProductsAndServices/FinancialProductsAndServices/> ;
	skos:definition "a realization of a product lifecycle" ;
	.

fibo-fbc-pas-fpas:ProductLifecycleStage
	a owl:Class ;
	rdfs:subClassOf
		fibo-fnd-arr-lif:LifecycleStage ,
		[
			a owl:Restriction ;
			owl:onProperty fibo-fnd-arr-lif:isStageOf ;
			owl:someValuesFrom fibo-fbc-pas-fpas:ProductLifecycle ;
		] ,
		[
			a owl:Restriction ;
			owl:onProperty fibo-fnd-rel-rel:comprises ;
			owl:someValuesFrom fibo-fbc-pas-fpas:ProductLifecycleEvent ;
		] ,
		[
			a owl:Restriction ;
			owl:onProperty fibo-fnd-rel-rel:isDefinedIn ;
			owl:someValuesFrom fibo-fbc-pas-fpas:ProductLifecycle ;
		] ,
		[
			a owl:Restriction ;
			owl:onProperty lcc-cr:classifies ;
			owl:someValuesFrom fibo-fnd-pas-pas:Product ;
		]
		;
	rdfs:label "product lifecycle stage" ;
	rdfs:isDefinedBy <https://spec.edmcouncil.org/fibo/ontology/FBC/ProductsAndServices/FinancialProductsAndServices/> ;
	skos:definition "a phase in a product lifecycle" ;
	skos:example "a research and development phase of a product lifecycle, the introduction phase in a marketing lifecycle, a growth stage in an economic lifecycle, or the origination phase in the lifecycle of a loan" ;
	.

fibo-fbc-pas-fpas:ProductLifecycleStageOccurrence
	a owl:Class ;
	rdfs:subClassOf
		fibo-fnd-arr-lif:LifecycleStageOccurrence ,
		[
			a owl:Restriction ;
			owl:onProperty fibo-fnd-dt-oc:exemplifies ;
			owl:onClass fibo-fbc-pas-fpas:ProductLifecycleStage ;
			owl:qualifiedCardinality "1"^^xsd:nonNegativeInteger ;
		] ,
		[
			a owl:Restriction ;
			owl:onProperty fibo-fnd-arr-lif:isStageOf ;
			owl:someValuesFrom fibo-fbc-pas-fpas:ProductLifecycleOccurrence ;
		] ,
		[
			a owl:Restriction ;
			owl:onProperty fibo-fnd-rel-rel:comprises ;
			owl:someValuesFrom fibo-fbc-pas-fpas:ProductLifecycleEventOccurrence ;
		]
		;
	rdfs:label "product lifecycle stage occurrence" ;
	rdfs:isDefinedBy <https://spec.edmcouncil.org/fibo/ontology/FBC/ProductsAndServices/FinancialProductsAndServices/> ;
	skos:definition "an instance of a phase in an occurrence of a given product lifecycle" ;
	.

fibo-fbc-pas-fpas:RegisteredAgent
	a owl:Class ;
	rdfs:subClassOf
		fibo-fbc-pas-fpas:LegalAgent ,
		fibo-fnd-agr-ctr:ContractParty ,
		[
			a owl:Restriction ;
			owl:onProperty fibo-fnd-pty-rl:isPlayedBy ;
			owl:someValuesFrom [
				a owl:Class ;
				owl:intersectionOf (
					[
						a owl:Restriction ;
						owl:onProperty fibo-fnd-pty-pty:isAPartyTo ;
						owl:someValuesFrom fibo-fbc-pas-fpas:AgencyAgreement ;
					]
					[
						a owl:Restriction ;
						owl:onProperty fibo-be-le-lp:isRecognizedIn ;
						owl:someValuesFrom fibo-fnd-law-jur:Jurisdiction ;
					]
				) ;
			] ;
		]
		;
	rdfs:label "registered agent" ;
	rdfs:isDefinedBy <https://spec.edmcouncil.org/fibo/ontology/FBC/ProductsAndServices/FinancialProductsAndServices/> ;
	rdfs:seeAlso
		<http://www.sos.state.tx.us/corp/registeredagents.shtml> ,
		<https://thelawdictionary.org/agent/>
		;
	skos:definition "a legal agent designated by another party (person or organization), to represent and acts on their behalf under a formal agency agreement" ;
	fibo-fnd-utl-av:explanatoryNote "Agency capacity, as specified in an agency agreement, may include power of attorney, the ability to act as an agent in certain kinds of transactions such as real estate, tax, audit or other financial or legal transactions, as a fiduciary, including as a trustee or legal guardian, for service of process, and so forth." ;
	fibo-fnd-utl-av:synonym
		"resident agent" ,
		"statutory agent"
		;
	.

fibo-fbc-pas-fpas:RegulatedCommodity
	a owl:Class ;
	rdfs:subClassOf
		fibo-fnd-pas-pas:Commodity ,
		[
			a owl:Restriction ;
			owl:onProperty fibo-fbc-fct-rga:isRegulatedBy ;
			owl:allValuesFrom fibo-fbc-fct-rga:RegulatoryAgency ;
		] ,
		[
			a owl:Restriction ;
			owl:onProperty fibo-fnd-rel-rel:isGovernedBy ;
			owl:someValuesFrom fibo-fnd-law-jur:Jurisdiction ;
		]
		;
	rdfs:label "regulated commodity" ;
	rdfs:isDefinedBy <https://spec.edmcouncil.org/fibo/ontology/FBC/ProductsAndServices/FinancialProductsAndServices/> ;
	skos:definition "a commodity under the jurisdiction of the regulatory agency, such as the Commodities Futures Trading Commission (CFTF), which includes any commodity traded in an organized contracts market" ;
	fibo-fnd-utl-av:explanatoryNote "The CFTC polices matters of information and disclosure, fair trading practices, registration of firms and individuals, protection of customer funds, record keeping, and maintenance of orderly options and futures markets in the United States." ;
	.

fibo-fbc-pas-fpas:SettlementTerms
	a owl:Class ;
	rdfs:subClassOf
		fibo-fnd-agr-ctr:ContractualCommitment ,
		[
			a owl:Restriction ;
			owl:onProperty fibo-fbc-pas-fpas:hasSettlementDate ;
			owl:allValuesFrom fibo-fnd-dt-fd:Date ;
		]
		;
	rdfs:label "settlement terms" ;
	rdfs:isDefinedBy <https://spec.edmcouncil.org/fibo/ontology/FBC/ProductsAndServices/FinancialProductsAndServices/> ;
	skos:definition "contract terms that define the commitment to and mechanism for settling one or more sides of a transaction" ;
	fibo-fnd-utl-av:explanatoryNote "In general, settlement involves arrangement of disposition of property, typically for legal reasons.  With respect to financial transactions, it involves completion of a trade, either between brokers or agents, or between a broker and client. This may include settlement in cash, either for the entire transaction or for the cash leg of a transaction, either now or at some specified time in the future." ;
	.

fibo-fbc-pas-fpas:TerminatedTrade
	a
		owl:NamedIndividual ,
		fibo-fbc-pas-fpas:TradeLifecycleStage
		;
	rdfs:label "terminated trade" ;
	rdfs:isDefinedBy <https://spec.edmcouncil.org/fibo/ontology/FBC/ProductsAndServices/FinancialProductsAndServices/> ;
	skos:definition "stage in the trade lifecycle in which the trade has been terminated early, i.e., prior to maturity" ;
	fibo-fnd-utl-av:explanatoryNote "Early termination may be triggered by a position sell or early termination provision, such as auto call/cancel, knock-out, etc." ;
	.

fibo-fbc-pas-fpas:ThirdPartyAgent
	a owl:Class ;
	rdfs:subClassOf
		fibo-fbc-pas-fpas:LegalAgent ,
		fibo-fnd-law-lcap:Licensee ,
		fibo-fnd-pas-pas:ServiceProvider
		;
	rdfs:label "third-party agent" ;
	rdfs:isDefinedBy <https://spec.edmcouncil.org/fibo/ontology/FBC/ProductsAndServices/FinancialProductsAndServices/> ;
	skos:definition "any service provider that is licensed to perform a legally binding function and has been legally empowered to act on behalf of another party" ;
	fibo-fnd-utl-av:adaptedFrom "17 CFR 45.1, Definitions - see the definition of agent" ;
	fibo-fnd-utl-av:usageNote "Note that third-party agent is defined as a service provider (organization) acting in an agency capacity, such as a law firm, accountancy, or investment bank.  This is distinct from the concept of an individual (licensed agent), for example one who works for a broker-dealer, that is a registered agent licensed to sell securities." ;
	.

fibo-fbc-pas-fpas:Trade
	a owl:Class ;
	rdfs:subClassOf
		fibo-fnd-pas-pas:TransactionEvent ,
		[
			a owl:Restriction ;
			owl:onProperty fibo-fbc-pas-fpas:succeeds ;
			owl:onClass fibo-fbc-pas-fpas:Trade ;
			owl:minQualifiedCardinality "0"^^xsd:nonNegativeInteger ;
		] ,
		[
			a owl:Restriction ;
			owl:onProperty lcc-lr:isIdentifiedBy ;
			owl:onClass fibo-fbc-pas-fpas:TradeIdentifier ;
			owl:minQualifiedCardinality "0"^^xsd:nonNegativeInteger ;
		] ,
		[
			a owl:Restriction ;
			owl:onProperty fibo-fnd-rel-rel:isCharacterizedBy ;
			owl:onClass fibo-fbc-pas-fpas:TradeLifecycle ;
			owl:minQualifiedCardinality "0"^^xsd:nonNegativeInteger ;
		] ,
		[
			a owl:Restriction ;
			owl:onProperty fibo-fbc-pas-fpas:isFacilitatedBy ;
			owl:onClass fibo-fbc-pas-fpas:Trader ;
			owl:minQualifiedCardinality "0"^^xsd:nonNegativeInteger ;
		] ,
		[
			a owl:Restriction ;
			owl:onProperty fibo-fbc-pas-fpas:isEmbodiedIn ;
			owl:someValuesFrom fibo-fnd-agr-ctr:Contract ;
		] ,
		[
			a owl:Restriction ;
			owl:onProperty fibo-fnd-rel-rel:involves ;
			owl:someValuesFrom [
				a owl:Class ;
				owl:unionOf (
					fibo-fnd-pas-pas:Good
					fibo-fnd-pas-pas:Service
					fibo-fnd-agr-ctr:Contract
				) ;
			] ;
		]
		;
	rdfs:label "trade" ;
	rdfs:isDefinedBy <https://spec.edmcouncil.org/fibo/ontology/FBC/ProductsAndServices/FinancialProductsAndServices/> ;
	skos:definition "an agreement between parties participating in a voluntary action of buying and selling goods and services" ;
	fibo-fnd-utl-av:adaptedFrom "Deutsche Bank Presentation on the Lifecycle of a Trade, available at http://www.slideshare.net/ahaline/23512555-tradelifecycle" ;
	fibo-fnd-utl-av:explanatoryNote
		"The advent of money as a medium of exchange has allowed trade to be conducted in a manner that is much simpler and effective compared to earlier forms of trade, such as bartering. In financial markets, trading also can mean performing a transaction that involves the selling and purchasing of a security." ,
		"The seller must deliver the commodity sold to the buyer; the buyer must pay the agreed purchase price, which could be in the form of other goods or services, on the agreed date." ,
		"Trading activities typically include (a) regularly underwriting or dealing in securities; interest rate, foreign exchange rate, commodity, equity, and credit derivative contracts; other financial instruments; and other assets for resale, (b) acquiring or taking positions in such items principally for the purpose of selling in the near term or otherwise with the intent to resell in order to profit from short-term price movements, and (c) acquiring or taking positions in such items as an accommodation to customers or for other trading purposes. (Source: Instructions for Preparation of Consolidated Reports of Condition and Income (FFIEC 031 and 041), Schedule RC-D - Trading Assets and Liabilities, 2013."
		;
	.

fibo-fbc-pas-fpas:TradeIdentifier
	a owl:Class ;
	rdfs:subClassOf
		lcc-lr:Identifier ,
		[
			a owl:Restriction ;
			owl:onProperty lcc-lr:identifies ;
			owl:onClass fibo-fbc-pas-fpas:Trade ;
			owl:qualifiedCardinality "1"^^xsd:nonNegativeInteger ;
		]
		;
	rdfs:label "trade identifier" ;
	rdfs:isDefinedBy <https://spec.edmcouncil.org/fibo/ontology/FBC/ProductsAndServices/FinancialProductsAndServices/> ;
	skos:definition "an identifier for a trade" ;
	.

fibo-fbc-pas-fpas:TradeLifecycle
	a owl:Class ;
	rdfs:subClassOf
		fibo-fnd-arr-lif:Lifecycle ,
		[
			a owl:Restriction ;
			owl:onProperty fibo-fnd-arr-lif:hasStage ;
			owl:someValuesFrom fibo-fbc-pas-fpas:TradeLifecycleStage ;
		] ,
		[
			a owl:Restriction ;
			owl:onProperty fibo-fnd-arr-lif:isLifecycleOf ;
			owl:someValuesFrom fibo-fbc-pas-fpas:Trade ;
		] ,
		[
			a owl:Restriction ;
			owl:onProperty fibo-fnd-rel-rel:defines ;
			owl:someValuesFrom fibo-fbc-pas-fpas:TradeLifecycleStage ;
		]
		;
	rdfs:label "trade lifecycle" ;
	rdfs:isDefinedBy <https://spec.edmcouncil.org/fibo/ontology/FBC/ProductsAndServices/FinancialProductsAndServices/> ;
	skos:definition "a lifecycle that defines the evolution of a trade, from initiation through settlement" ;
	skos:example "The trade life cycle describes the period of time over which a trade is initiated, typically as a part of a broader deal, consumated, processed and executed, settled or closed for other reasons, and reported." ;
	.

fibo-fbc-pas-fpas:TradeLifecycleEvent
	a owl:Class ;
	rdfs:subClassOf
		fibo-fnd-arr-lif:LifecycleEvent ,
		[
			a owl:Restriction ;
			owl:onProperty fibo-fbc-pas-fpas:succeeds ;
			owl:onClass fibo-fbc-pas-fpas:TradeLifecycleEvent ;
			owl:minQualifiedCardinality "0"^^xsd:nonNegativeInteger ;
		] ,
		[
			a owl:Restriction ;
			owl:onProperty fibo-fnd-rel-rel:appliesTo ;
			owl:someValuesFrom fibo-fbc-pas-fpas:TradeLifecycleStage ;
		]
		;
	rdfs:label "trade lifecycle event" ;
	rdfs:isDefinedBy <https://spec.edmcouncil.org/fibo/ontology/FBC/ProductsAndServices/FinancialProductsAndServices/> ;
	skos:definition "a kind of event that occurs during one or more stages of the lifecycle of a trade" ;
	.

fibo-fbc-pas-fpas:TradeLifecycleEventOccurrence
	a owl:Class ;
	rdfs:subClassOf
		fibo-fnd-arr-lif:LifecycleEventOccurrence ,
		[
			a owl:Restriction ;
			owl:onProperty fibo-fbc-pas-fpas:succeeds ;
			owl:onClass fibo-fbc-pas-fpas:TradeLifecycleEventOccurrence ;
			owl:minQualifiedCardinality "0"^^xsd:nonNegativeInteger ;
		] ,
		[
			a owl:Restriction ;
			owl:onProperty fibo-fnd-dt-oc:exemplifies ;
			owl:onClass fibo-fbc-pas-fpas:TradeLifecycleEvent ;
			owl:qualifiedCardinality "1"^^xsd:nonNegativeInteger ;
		] ,
		[
			a owl:Restriction ;
			owl:onProperty fibo-fnd-rel-rel:appliesTo ;
			owl:someValuesFrom fibo-fbc-pas-fpas:TradeLifecycleStageOccurrence ;
		]
		;
	rdfs:label "trade lifecycle event occurrence" ;
	rdfs:isDefinedBy <https://spec.edmcouncil.org/fibo/ontology/FBC/ProductsAndServices/FinancialProductsAndServices/> ;
	skos:definition "an occurrence of an event that occurs during a specific stage of a specific trade lifecycle" ;
	.

fibo-fbc-pas-fpas:TradeLifecycleOccurrence
	a owl:Class ;
	rdfs:subClassOf
		fibo-fnd-arr-lif:LifecycleOccurrence ,
		[
			a owl:Restriction ;
			owl:onProperty fibo-fnd-dt-oc:exemplifies ;
			owl:onClass fibo-fbc-pas-fpas:TradeLifecycle ;
			owl:qualifiedCardinality "1"^^xsd:nonNegativeInteger ;
		] ,
		[
			a owl:Restriction ;
			owl:onProperty fibo-fnd-arr-lif:hasStage ;
			owl:someValuesFrom fibo-fbc-pas-fpas:TradeLifecycleStageOccurrence ;
		]
		;
	rdfs:label "trade lifecycle occurrence" ;
	rdfs:isDefinedBy <https://spec.edmcouncil.org/fibo/ontology/FBC/ProductsAndServices/FinancialProductsAndServices/> ;
	skos:definition "a realization of a trade lifecycle" ;
	.

fibo-fbc-pas-fpas:TradeLifecycleStage
	a owl:Class ;
	rdfs:subClassOf
		fibo-fnd-arr-lif:LifecycleStage ,
		[
			a owl:Restriction ;
			owl:onProperty fibo-fbc-pas-fpas:succeeds ;
			owl:onClass fibo-fbc-pas-fpas:TradeLifecycleStage ;
			owl:minQualifiedCardinality "0"^^xsd:nonNegativeInteger ;
		] ,
		[
			a owl:Restriction ;
			owl:onProperty fibo-fnd-arr-lif:isStageOf ;
			owl:someValuesFrom fibo-fbc-pas-fpas:TradeLifecycle ;
		] ,
		[
			a owl:Restriction ;
			owl:onProperty fibo-fnd-rel-rel:comprises ;
			owl:someValuesFrom fibo-fbc-pas-fpas:TradeLifecycleEvent ;
		] ,
		[
			a owl:Restriction ;
			owl:onProperty fibo-fnd-rel-rel:isDefinedIn ;
			owl:someValuesFrom fibo-fbc-pas-fpas:TradeLifecycle ;
		] ,
		[
			a owl:Restriction ;
			owl:onProperty lcc-cr:classifies ;
			owl:someValuesFrom fibo-fbc-pas-fpas:Trade ;
		]
		;
	rdfs:label "trade lifecycle stage" ;
	rdfs:isDefinedBy <https://spec.edmcouncil.org/fibo/ontology/FBC/ProductsAndServices/FinancialProductsAndServices/> ;
	skos:definition "a phase in the lifecycle of a trade" ;
	.

fibo-fbc-pas-fpas:TradeLifecycleStageOccurrence
	a owl:Class ;
	rdfs:subClassOf
		fibo-fnd-arr-lif:LifecycleStageOccurrence ,
		[
			a owl:Restriction ;
			owl:onProperty fibo-fbc-pas-fpas:succeeds ;
			owl:onClass fibo-fbc-pas-fpas:TradeLifecycleStageOccurrence ;
			owl:minQualifiedCardinality "0"^^xsd:nonNegativeInteger ;
		] ,
		[
			a owl:Restriction ;
			owl:onProperty fibo-fnd-dt-oc:exemplifies ;
			owl:onClass fibo-fbc-pas-fpas:TradeLifecycleStage ;
			owl:qualifiedCardinality "1"^^xsd:nonNegativeInteger ;
		] ,
		[
			a owl:Restriction ;
			owl:onProperty fibo-fnd-arr-lif:isStageOf ;
			owl:someValuesFrom fibo-fbc-pas-fpas:TradeLifecycleOccurrence ;
		] ,
		[
			a owl:Restriction ;
			owl:onProperty fibo-fnd-rel-rel:comprises ;
			owl:someValuesFrom fibo-fbc-pas-fpas:TradeLifecycleEventOccurrence ;
		]
		;
	rdfs:label "trade lifecycle stage occurrence" ;
	rdfs:isDefinedBy <https://spec.edmcouncil.org/fibo/ontology/FBC/ProductsAndServices/FinancialProductsAndServices/> ;
	skos:definition "an instance of a phase in an occurrence of a given trade lifecycle" ;
	.

fibo-fbc-pas-fpas:Trader
	a owl:Class ;
	rdfs:subClassOf
		fibo-fnd-pas-pas:ServiceProvider ,
		[
			a owl:Restriction ;
			owl:onProperty fibo-fbc-pas-fpas:facilitates ;
			owl:someValuesFrom fibo-fbc-pas-fpas:Trade ;
		] ,
		[
			a owl:Restriction ;
			owl:onProperty fibo-fnd-pty-rl:isPlayedBy ;
			owl:someValuesFrom [
				a owl:Restriction ;
				owl:onProperty fibo-fnd-law-lcap:hasCapacity ;
				owl:someValuesFrom fibo-fnd-law-lcap:ContractualCapability ;
			] ;
		]
		;
	rdfs:label "trader" ;
	rdfs:isDefinedBy <https://spec.edmcouncil.org/fibo/ontology/FBC/ProductsAndServices/FinancialProductsAndServices/> ;
	skos:definition "party that engages in the transfer of financial assets in any financial market on behalf of a client or the financial services provider" ;
	.

fibo-fbc-pas-fpas:TradingStrategy
	a owl:Class ;
	rdfs:subClassOf fibo-fnd-gao-obj:Strategy ;
	rdfs:label "trading strategy" ;
	rdfs:isDefinedBy <https://spec.edmcouncil.org/fibo/ontology/FBC/ProductsAndServices/FinancialProductsAndServices/> ;
	skos:definition "approach used for buying and selling in the securities markets" ;
	fibo-fnd-utl-av:explanatoryNote "A trading strategy is a plan whose aim is to make a profit or hedge against risk, based on rules and other criteria used when making trading decisions. A trading strategy may be simple or complex, and involve considerations such as investment style (e.g., value vs. growth), market cap, technical indicators, fundamental analysis, industry sector, level of portfolio diversification, time horizon or holding period, risk tolerance, leverage, tax considerations, and so on." ;
	.

fibo-fbc-pas-fpas:UniqueTransactionIdentifier
	a owl:Class ;
	rdfs:subClassOf
		fibo-fbc-pas-fpas:TradeIdentifier ,
		[
			a owl:Restriction ;
			owl:onProperty fibo-fbc-pas-fpas:hasGeneratingEntityIdentifier ;
			owl:someValuesFrom fibo-be-le-lei:LegalEntityIdentifier ;
		]
		;
	rdfs:label "unique transaction identifier" ;
	rdfs:isDefinedBy <https://spec.edmcouncil.org/fibo/ontology/FBC/ProductsAndServices/FinancialProductsAndServices/> ;
	skos:definition "globally unique identifier for a reportable transaction, whose primary purpose is to uniquely identify individual OTC derivatives transactions in reports to trade repositories" ;
	fibo-fnd-utl-av:abbreviation "UTI" ;
	fibo-fnd-utl-av:adaptedFrom "Harmonization of the Unique Transaction Identifier - Technical Guidance, 20 Feb 2017, described in https://www.bis.org/cpmi/publ/d158.pdf" ;
	fibo-fnd-utl-av:explanatoryNote "In particular, a UTI will help to ensure the consistent aggregation of OTC derivatives transactions by minimising the likelihood that the same transaction will be counted more than once (for instance, because it is reported by more than one counterparty to a transaction, or to more than one trade repository (TR))." ;
	.

fibo-fbc-pas-fpas:WeightedBasket
	a owl:Class ;
	rdfs:subClassOf
		fibo-fbc-pas-fpas:Basket ,
		fibo-fnd-arr-arr:StructuredCollection ,
		[
			a owl:Restriction ;
			owl:onProperty fibo-fnd-arr-arr:hasConstituent ;
			owl:someValuesFrom fibo-fbc-pas-fpas:WeightedBasketConstituent ;
		] ,
		[
			a owl:Restriction ;
			owl:onProperty fibo-fnd-utl-alx:hasExpression ;
			owl:someValuesFrom fibo-fnd-utl-alx:WeightingFunction ;
		]
		;
	rdfs:label "weighted basket" ;
	rdfs:isDefinedBy <https://spec.edmcouncil.org/fibo/ontology/FBC/ProductsAndServices/FinancialProductsAndServices/> ;
	skos:definition "basket whose constituents have some relative importance with respect to one another" ;
	.

fibo-fbc-pas-fpas:WeightedBasketConstituent
	a owl:Class ;
	rdfs:subClassOf
		fibo-fbc-pas-fpas:BasketConstituent ,
		[
			a owl:Restriction ;
			owl:onProperty fibo-fnd-utl-alx:hasWeight ;
			owl:onDataRange xsd:decimal ;
			owl:qualifiedCardinality "1"^^xsd:nonNegativeInteger ;
		]
		;
	rdfs:label "weighted basket constituent" ;
	rdfs:isDefinedBy <https://spec.edmcouncil.org/fibo/ontology/FBC/ProductsAndServices/FinancialProductsAndServices/> ;
	skos:definition "component of a basket whose relative importance with respect to other basket constituents is known" ;
	.

fibo-fbc-pas-fpas:facilitates
	a owl:ObjectProperty ;
	rdfs:label "facilitates" ;
	rdfs:isDefinedBy <https://spec.edmcouncil.org/fibo/ontology/FBC/ProductsAndServices/FinancialProductsAndServices/> ;
	skos:definition "provides the context in which an event, a task, a conversation or something else can occur" ;
	.

fibo-fbc-pas-fpas:hasGeneratingEntity
	a owl:ObjectProperty ;
	rdfs:subPropertyOf fibo-fnd-rel-rel:generates ;
	rdfs:label "has generating entity" ;
	rdfs:isDefinedBy <https://spec.edmcouncil.org/fibo/ontology/FBC/ProductsAndServices/FinancialProductsAndServices/> ;
	rdfs:range fibo-be-le-lp:LegalEntity ;
	skos:definition "specifies a legal entity that generates something" ;
	.

fibo-fbc-pas-fpas:hasGeneratingEntityIdentifier
	a owl:ObjectProperty ;
	rdfs:label "has generating entity identifier" ;
	rdfs:domain fibo-fbc-pas-fpas:UniqueTransactionIdentifier ;
	rdfs:isDefinedBy <https://spec.edmcouncil.org/fibo/ontology/FBC/ProductsAndServices/FinancialProductsAndServices/> ;
	owl:propertyChainAxiom (
		fibo-fbc-pas-fpas:hasGeneratingEntity
		lcc-lr:isIdentifiedBy
	) ;
	skos:definition "specifies an identifier for the entity that generated something" ;
	fibo-fnd-utl-av:explanatoryNote "Note that the range of is identified by must be that entity's LEI in the context of a UTI" ;
	.

fibo-fbc-pas-fpas:hasLegalAgent
	a owl:ObjectProperty ;
	rdfs:subPropertyOf fibo-fnd-pty-pty:hasPartyInRole ;
	rdfs:label "has registered agent" ;
	rdfs:isDefinedBy <https://spec.edmcouncil.org/fibo/ontology/FBC/ProductsAndServices/FinancialProductsAndServices/> ;
	rdfs:range fibo-fbc-pas-fpas:LegalAgent ;
	skos:definition "identifies a party as one that has the legal, medical or financial capacity to act on behalf of someone else under specific circumstances" ;
	.

fibo-fbc-pas-fpas:hasNominalNumberOfUnits
	a owl:DatatypeProperty ;
	rdfs:subPropertyOf fibo-fnd-acc-cur:hasAmount ;
	rdfs:label "has nominal number of units" ;
	rdfs:isDefinedBy <https://spec.edmcouncil.org/fibo/ontology/FBC/ProductsAndServices/FinancialProductsAndServices/> ;
	rdfs:range xsd:integer ;
	skos:definition "indicates the base number of units of something associated with some offering" ;
	.

fibo-fbc-pas-fpas:hasOffering
	a owl:ObjectProperty ;
	rdfs:subPropertyOf lcc-lr:has ;
	rdfs:label "has offering" ;
	rdfs:isDefinedBy <https://spec.edmcouncil.org/fibo/ontology/FBC/ProductsAndServices/FinancialProductsAndServices/> ;
	rdfs:range fibo-fbc-pas-fpas:Offering ;
	owl:inverseOf fibo-fbc-pas-fpas:isOfferingOf ;
	skos:definition "relates something to a voluntary but conditional promise submitted by a buyer or seller (offeror) to another (offeree) for acceptance, and which becomes legally enforceable if accepted by the offeree" ;
	.

fibo-fbc-pas-fpas:hasOfferingAmount
	a owl:ObjectProperty ;
	rdfs:subPropertyOf fibo-fnd-acc-cur:hasNotionalAmount ;
	rdfs:label "has offering amount" ;
	rdfs:isDefinedBy <https://spec.edmcouncil.org/fibo/ontology/FBC/ProductsAndServices/FinancialProductsAndServices/> ;
	rdfs:range fibo-fnd-acc-cur:MonetaryAmount ;
	skos:definition "indicates the notional monetary amount, determined based on reference data, market rates or some other agreed method associated with some offering" ;
	.

fibo-fbc-pas-fpas:hasOfferingPrice
	a owl:ObjectProperty ;
	rdfs:subPropertyOf fibo-fnd-acc-cur:hasPrice ;
	rdfs:label "has offering price" ;
	rdfs:isDefinedBy <https://spec.edmcouncil.org/fibo/ontology/FBC/ProductsAndServices/FinancialProductsAndServices/> ;
	rdfs:range fibo-fnd-acc-cur:MonetaryPrice ;
	skos:definition "indicates the price associated with an offering, which may be an explicit or calculated price" ;
	.

fibo-fbc-pas-fpas:hasOfferingUnits
	a owl:DatatypeProperty ;
	rdfs:subPropertyOf fibo-fnd-acc-cur:hasAmount ;
	rdfs:label "has offering units" ;
	rdfs:isDefinedBy <https://spec.edmcouncil.org/fibo/ontology/FBC/ProductsAndServices/FinancialProductsAndServices/> ;
	rdfs:range xsd:integer ;
	skos:definition "indicates the actual number of units of something, including any premium on the number of units, associated with some offering" ;
	.

fibo-fbc-pas-fpas:hasSelectingParty
	a owl:ObjectProperty ;
	rdfs:subPropertyOf fibo-fnd-pty-pty:hasParty ;
	rdfs:label "has selecting party" ;
	rdfs:isDefinedBy <https://spec.edmcouncil.org/fibo/ontology/FBC/ProductsAndServices/FinancialProductsAndServices/> ;
	rdfs:range fibo-fnd-pty-pty:IndependentParty ;
	skos:definition "indicates the person(s) or organization(s) responsible for determining the contents of a basket" ;
	.

fibo-fbc-pas-fpas:hasSelectionCriteria
	a owl:DatatypeProperty ;
	rdfs:subPropertyOf fibo-fnd-aap-agt:hasTextValue ;
	rdfs:label "has selection criteria" ;
	rdfs:domain lcc-lr:Collection ;
	rdfs:isDefinedBy <https://spec.edmcouncil.org/fibo/ontology/FBC/ProductsAndServices/FinancialProductsAndServices/> ;
	skos:definition "describes the methodology or program used to determine the membership of a collection" ;
	.

fibo-fbc-pas-fpas:hasSettlementDate
	a owl:ObjectProperty ;
	rdfs:subPropertyOf fibo-fnd-dt-fd:hasEndDate ;
	rdfs:label "has settlement date" ;
	rdfs:isDefinedBy <https://spec.edmcouncil.org/fibo/ontology/FBC/ProductsAndServices/FinancialProductsAndServices/> ;
	rdfs:range fibo-fnd-dt-fd:CalculatedDate ;
	skos:definition "indicates the date by which an executed order or transaction must be settled" ;
	fibo-fnd-utl-av:explanatoryNote "Settlement might involve either a buyer paying in cash or a seller delivering the relevant instrument(s) and receiving the proceeds as specified by the terms of a given transaction." ;
	.

fibo-fbc-pas-fpas:hasTradeDate
	a owl:ObjectProperty ;
	rdfs:subPropertyOf fibo-fnd-dt-fd:hasDate ;
	rdfs:label "has trade date" ;
	rdfs:isDefinedBy <https://spec.edmcouncil.org/fibo/ontology/FBC/ProductsAndServices/FinancialProductsAndServices/> ;
	rdfs:range fibo-fnd-dt-fd:Date ;
	skos:definition "indicates the date on which a security or other instrument-specific trade actually takes place" ;
	.

fibo-fbc-pas-fpas:isEmbodiedIn
	a owl:ObjectProperty ;
	rdfs:label "is embodied in" ;
	rdfs:isDefinedBy <https://spec.edmcouncil.org/fibo/ontology/FBC/ProductsAndServices/FinancialProductsAndServices/> ;
	owl:inverseOf fibo-fnd-rel-rel:embodies ;
	skos:definition "identifies the representation or tangible form of something in some context" ;
	.

fibo-fbc-pas-fpas:isFacilitatedBy
	a owl:ObjectProperty ;
	rdfs:label "is facilitated by" ;
	rdfs:isDefinedBy <https://spec.edmcouncil.org/fibo/ontology/FBC/ProductsAndServices/FinancialProductsAndServices/> ;
	owl:inverseOf fibo-fbc-pas-fpas:facilitates ;
	skos:definition "identifies someone or something that expedites some event, transaction, conversation or something else in some context" ;
	.

fibo-fbc-pas-fpas:isOfferingOf
	a owl:ObjectProperty ;
	rdfs:label "is offering of" ;
	rdfs:domain fibo-fbc-pas-fpas:Offering ;
	rdfs:isDefinedBy <https://spec.edmcouncil.org/fibo/ontology/FBC/ProductsAndServices/FinancialProductsAndServices/> ;
	skos:definition "relates an offering to one or things that are the subject of the offer" ;
	.

fibo-fbc-pas-fpas:precedes
	a owl:ObjectProperty ;
	rdfs:subPropertyOf fibo-fbc-pas-fpas:relatesTo ;
	rdfs:label "precedes" ;
	rdfs:isDefinedBy <https://spec.edmcouncil.org/fibo/ontology/FBC/ProductsAndServices/FinancialProductsAndServices/> ;
	skos:definition "relates a product, organization, stage in a lifecycle, an event, or occurrence, such as a trade, to one that occurs before it" ;
	.

fibo-fbc-pas-fpas:relatesTo
	a owl:ObjectProperty ;
	rdfs:label "relates to" ;
	rdfs:isDefinedBy <https://spec.edmcouncil.org/fibo/ontology/FBC/ProductsAndServices/FinancialProductsAndServices/> ;
	skos:definition "has a logical or causal connection with" ;
	.

fibo-fbc-pas-fpas:succeeds
	a owl:ObjectProperty ;
	rdfs:subPropertyOf fibo-fbc-pas-fpas:relatesTo ;
	rdfs:label "succeeds" ;
	rdfs:isDefinedBy <https://spec.edmcouncil.org/fibo/ontology/FBC/ProductsAndServices/FinancialProductsAndServices/> ;
	owl:inverseOf fibo-fbc-pas-fpas:precedes ;
	skos:definition "relates a product, organization, stage in a lifecycle, an event, or occurrence, such as a trade, to one that follows it" ;
	.

fibo-fnd-pas-pas:Product
	a owl:Class ;
	rdfs:subClassOf
		[
			a owl:Restriction ;
			owl:onProperty fibo-fnd-rel-rel:isCharacterizedBy ;
			owl:onClass fibo-fbc-pas-fpas:Catalog ;
			owl:minQualifiedCardinality "0"^^xsd:nonNegativeInteger ;
		] ,
		[
			a owl:Restriction ;
			owl:onProperty fibo-fnd-arr-lif:hasLifecycle ;
			owl:onClass fibo-fbc-pas-fpas:ProductLifecycle ;
			owl:minQualifiedCardinality "0"^^xsd:nonNegativeInteger ;
		]
		;
	.

