# baseURI: http://fundontology.com/fr/form/IAPDSECCompilationReport.ttl
# imports: http://finregont.com/fro/cfr/Code_Federal_Regulations.ttl
# imports: http://fundontology.com/fr/ref/Fund_Legal_Reference.ttl
# imports: http://topbraid.org/sxml
# imports: http://www.linkedmodel.org/schema/dtype
# prefix: iapd-sec-cr

@prefix dct: <http://purl.org/dc/terms/> .
@prefix dtype: <http://www.linkedmodel.org/schema/dtype#> .
@prefix iapd-sec-cr: <http://fundontology.com/fr/form/IAPDSECCompilationReport.ttl#> .
@prefix lkif-action: <http://www.estrellaproject.org/lkif-core/action.owl#> .
@prefix lkif-expr: <http://www.estrellaproject.org/lkif-core/expression.owl#> .
@prefix lkif-proc: <http://www.estrellaproject.org/lkif-core/process.owl#> .
@prefix lkif-top: <http://www.estrellaproject.org/lkif-core/lkif-top.owl#> .
@prefix owl: <http://www.w3.org/2002/07/owl#> .
@prefix rdf: <http://www.w3.org/1999/02/22-rdf-syntax-ns#> .
@prefix rdfs: <http://www.w3.org/2000/01/rdf-schema#> .
@prefix skos: <http://www.w3.org/2004/02/skos/core#> .
@prefix sxml: <http://topbraid.org/sxml#> .
@prefix xsd: <http://www.w3.org/2001/XMLSchema#> .

<http://finregont.com/fro/ref/LegalReference.ttl#LegalForm>
  rdfs:subClassOf [
      rdf:type owl:Class ;
      owl:intersectionOf (
          <http://www.estrellaproject.org/lkif-core/norm.owl#Legal_Document>
          [
            rdf:type owl:Restriction ;
            owl:onProperty lkif-expr:bears ;
            owl:someValuesFrom <http://www.estrellaproject.org/lkif-core/norm.owl#Definitional_Expression> ;
          ]
        ) ;
    ] ;
.
<http://fundontology.com/fr/form/IAPDSECCompilationReport.ttl>
  rdf:type owl:Ontology ;
  dct:license "https://opensource.org/licenses/GPL-3.0"^^xsd:string ;
  dct:license "https://opensource.org/licenses/MIT"^^xsd:string ;
  <http://topbraid.org/sparqlmotion#author> "Jurgen Ziemer"^^xsd:string ;
  <http://topbraid.org/sparqlmotion#copyright> "Securities and Exchange Commission"^^xsd:string ;
  rdfs:comment """The OWL structure underneith the class FirmReport is used in two ways:
1) Included in Investment Adviser instance data files (IA_Firm_SEC_Feed.ttl)
2) To create instances of form ADV for Semantic Compliance."""^^xsd:string ;
  rdfs:isDefinedBy <https://adviserinfo.sec.gov/IAPD/InvestmentAdviserData.aspx> ;
  owl:imports <http://finregont.com/fro/cfr/Code_Federal_Regulations.ttl> ;
  owl:imports <http://fundontology.com/fr/ref/Fund_Legal_Reference.ttl> ;
  owl:imports <http://topbraid.org/sxml> ;
  owl:imports <http://www.linkedmodel.org/schema/dtype> ;
  owl:versionInfo "Created with TopBraid Composer from the XML Schema(s) IAPDSECCompilationReport.xsd"^^xsd:string ;
  skos:definition "The Ontology Web Language (OWL) version of the Securities and Exchange Commission's Investment Adviser Public Disclosure compilation report and form. "^^xsd:string ;
.
iapd-sec-cr:AYNT_N
  rdf:type iapd-sec-cr:AnswerYNType ;
  dtype:order "1"^^xsd:nonNegativeInteger ;
  dtype:value "N"^^xsd:string ;
  rdfs:label "N"^^xsd:string ;
.
iapd-sec-cr:AYNT_Y
  rdf:type iapd-sec-cr:AnswerYNType ;
  dtype:order "0"^^xsd:nonNegativeInteger ;
  dtype:value "Y"^^xsd:string ;
  rdfs:label "Y"^^xsd:string ;
.
iapd-sec-cr:AddrType
  rdf:type owl:Class ;
  sxml:tag "AddrType" ;
  rdfs:label "Addr type"^^xsd:string ;
  rdfs:subClassOf iapd-sec-cr:FirmReport ;
  rdfs:subClassOf [
      rdf:type owl:Restriction ;
      sxml:isAttribute "true"^^xsd:boolean ;
      owl:allValuesFrom iapd-sec-cr:StateCdType ;
      owl:onProperty iapd-sec-cr:state ;
    ] ;
  rdfs:subClassOf [
      rdf:type owl:Restriction ;
      sxml:isAttribute "true"^^xsd:boolean ;
      owl:allValuesFrom iapd-sec-cr:Str11Datatype ;
      owl:onProperty iapd-sec-cr:postlCd ;
    ] ;
  rdfs:subClassOf [
      rdf:type owl:Restriction ;
      sxml:isAttribute "true"^^xsd:boolean ;
      owl:allValuesFrom iapd-sec-cr:Str27Datatype ;
      owl:onProperty iapd-sec-cr:faxNb ;
    ] ;
  rdfs:subClassOf [
      rdf:type owl:Restriction ;
      sxml:isAttribute "true"^^xsd:boolean ;
      owl:allValuesFrom iapd-sec-cr:Str27Datatype ;
      owl:onProperty iapd-sec-cr:phNb ;
    ] ;
  rdfs:subClassOf [
      rdf:type owl:Restriction ;
      sxml:isAttribute "true"^^xsd:boolean ;
      owl:allValuesFrom iapd-sec-cr:Str50Datatype ;
      owl:onProperty iapd-sec-cr:city ;
    ] ;
  rdfs:subClassOf [
      rdf:type owl:Restriction ;
      sxml:isAttribute "true"^^xsd:boolean ;
      owl:allValuesFrom iapd-sec-cr:Str50Datatype ;
      owl:onProperty iapd-sec-cr:cntry ;
    ] ;
  rdfs:subClassOf [
      rdf:type owl:Restriction ;
      sxml:isAttribute "true"^^xsd:boolean ;
      owl:allValuesFrom iapd-sec-cr:Str50Datatype ;
      owl:onProperty iapd-sec-cr:strt1 ;
    ] ;
  rdfs:subClassOf [
      rdf:type owl:Restriction ;
      sxml:isAttribute "true"^^xsd:boolean ;
      owl:allValuesFrom iapd-sec-cr:Str50Datatype ;
      owl:onProperty iapd-sec-cr:strt2 ;
    ] ;
  rdfs:subClassOf [
      rdf:type owl:Restriction ;
      owl:maxCardinality "1"^^xsd:int ;
      owl:onProperty iapd-sec-cr:city ;
    ] ;
  rdfs:subClassOf [
      rdf:type owl:Restriction ;
      owl:maxCardinality "1"^^xsd:int ;
      owl:onProperty iapd-sec-cr:cntry ;
    ] ;
  rdfs:subClassOf [
      rdf:type owl:Restriction ;
      owl:maxCardinality "1"^^xsd:int ;
      owl:onProperty iapd-sec-cr:faxNb ;
    ] ;
  rdfs:subClassOf [
      rdf:type owl:Restriction ;
      owl:maxCardinality "1"^^xsd:int ;
      owl:onProperty iapd-sec-cr:phNb ;
    ] ;
  rdfs:subClassOf [
      rdf:type owl:Restriction ;
      owl:maxCardinality "1"^^xsd:int ;
      owl:onProperty iapd-sec-cr:postlCd ;
    ] ;
  rdfs:subClassOf [
      rdf:type owl:Restriction ;
      owl:maxCardinality "1"^^xsd:int ;
      owl:onProperty iapd-sec-cr:state ;
    ] ;
  rdfs:subClassOf [
      rdf:type owl:Restriction ;
      owl:maxCardinality "1"^^xsd:int ;
      owl:onProperty iapd-sec-cr:strt1 ;
    ] ;
  rdfs:subClassOf [
      rdf:type owl:Restriction ;
      owl:maxCardinality "1"^^xsd:int ;
      owl:onProperty iapd-sec-cr:strt2 ;
    ] ;
  skos:definition "The Address structure for business and mailing addresses including phone and fax number."^^xsd:string ;
.
iapd-sec-cr:AnswerYNType
  rdf:type owl:Class ;
  sxml:tag "answerYNType" ;
  rdfs:label "Answer YNType"^^xsd:string ;
  rdfs:subClassOf iapd-sec-cr:EnumeratedValue ;
  rdfs:subClassOf [
      rdf:type owl:Restriction ;
      sxml:isAttribute "false"^^xsd:boolean ;
      owl:allValuesFrom xsd:string ;
      owl:onProperty dtype:value ;
    ] ;
  rdfs:subClassOf [
      rdf:type owl:Restriction ;
      owl:maxCardinality "1"^^xsd:int ;
      owl:onProperty dtype:value ;
    ] ;
  owl:oneOf (
      iapd-sec-cr:AYNT_N
      iapd-sec-cr:AYNT_Y
    ) ;
.
iapd-sec-cr:Decimal14P2Datatype
  rdf:type rdfs:Datatype ;
  rdfs:label "Decimal14P2Datatype"^^xsd:string ;
  rdfs:subClassOf xsd:decimal ;
  owl:equivalentClass [
      rdf:type rdfs:Datatype ;
      owl:onDatatype xsd:decimal ;
      owl:withRestrictions (
          [
            xsd:fractionDigits "2"^^xsd:decimal ;
          ]
          [
            xsd:totalDigits "14"^^xsd:decimal ;
          ]
        ) ;
    ] ;
.
iapd-sec-cr:Decimal17P2Datatype
  rdf:type rdfs:Datatype ;
  rdfs:label "Decimal17P2Datatype"^^xsd:string ;
  rdfs:subClassOf xsd:decimal ;
  owl:equivalentClass [
      rdf:type rdfs:Datatype ;
      owl:onDatatype xsd:decimal ;
      owl:withRestrictions (
          [
            xsd:fractionDigits "2"^^xsd:decimal ;
          ]
          [
            xsd:totalDigits "17"^^xsd:decimal ;
          ]
        ) ;
    ] ;
.
iapd-sec-cr:EnumeratedValue
  rdf:type owl:Class ;
  rdfs:label "Enumerated value"^^xsd:string ;
  rdfs:subClassOf dtype:EnumeratedValue ;
.
iapd-sec-cr:FCT_ERA
  rdf:type iapd-sec-cr:FirmCdType ;
  dtype:order "1"^^xsd:nonNegativeInteger ;
  dtype:value "ERA"^^xsd:NMTOKEN ;
  rdfs:label "ERA"^^xsd:string ;
.
iapd-sec-cr:FCT_Registered
  rdf:type iapd-sec-cr:FirmCdType ;
  dtype:order "0"^^xsd:nonNegativeInteger ;
  dtype:value "Registered"^^xsd:NMTOKEN ;
  rdfs:label "Registered"^^xsd:string ;
.
iapd-sec-cr:FilingType
  rdf:type owl:Class ;
  sxml:tag "FilingType" ;
  rdfs:label "Filing type"^^xsd:string ;
  rdfs:subClassOf iapd-sec-cr:FirmReport ;
  rdfs:subClassOf [
      rdf:type owl:Restriction ;
      sxml:isAttribute "true"^^xsd:boolean ;
      rdfs:comment "This has the date the organization's most recent Form ADV filing was processed."@en ;
      owl:allValuesFrom xsd:date ;
      owl:onProperty iapd-sec-cr:dt ;
    ] ;
  rdfs:subClassOf [
      rdf:type owl:Restriction ;
      sxml:isAttribute "true"^^xsd:boolean ;
      rdfs:comment "This node has the version of the latest form ADV submitted."@en ;
      owl:allValuesFrom iapd-sec-cr:Str20Datatype ;
      owl:onProperty iapd-sec-cr:formVrsn ;
    ] ;
  rdfs:subClassOf [
      rdf:type owl:Restriction ;
      owl:cardinality "1"^^xsd:int ;
      owl:onProperty iapd-sec-cr:dt ;
    ] ;
  rdfs:subClassOf [
      rdf:type owl:Restriction ;
      owl:cardinality "1"^^xsd:int ;
      owl:onProperty iapd-sec-cr:formVrsn ;
    ] ;
  skos:definition "The Filing Type has the version of the form ADV submitted and the date the organization's most recent Form ADV filing was processed."^^xsd:string ;
.
iapd-sec-cr:FirmCdType
  rdf:type owl:Class ;
  sxml:tag "FirmCdType" ;
  rdfs:comment """Elements of this type represent the business type.
        Allowed values (code-Name) are:
        Registered-Registered Firms.
        ERA-Exempt Reporting Adviser firms."""@en ;
  rdfs:label "Firm cd type"^^xsd:string ;
  rdfs:subClassOf iapd-sec-cr:EnumeratedValue ;
  rdfs:subClassOf [
      rdf:type owl:Restriction ;
      sxml:isAttribute "false"^^xsd:boolean ;
      owl:allValuesFrom xsd:NMTOKEN ;
      owl:onProperty dtype:value ;
    ] ;
  rdfs:subClassOf [
      rdf:type owl:Restriction ;
      owl:maxCardinality "1"^^xsd:int ;
      owl:onProperty dtype:value ;
    ] ;
  owl:oneOf (
      iapd-sec-cr:FCT_ERA
      iapd-sec-cr:FCT_Registered
    ) ;
.
iapd-sec-cr:FirmReport
  rdf:type owl:Class ;
  rdfs:comment "The class structure has been reverse engineered from the IAPDSECCompilationReport.xsd XML schema and integrated into LKIF/FRO Legal Document, Legal Form. We load the XML report data into this structure."^^xsd:string ;
  rdfs:label "CRD Number"^^xsd:string ;
  rdfs:subClassOf <http://fundontology.com/fr/ref/Fund_Legal_Reference.ttl#Form_ADV> ;
  skos:definition "Form ADV filings made by investment adviser firms that register electronically using the Investment Adviser Registration Depository (IARD). All form elements are subclass of FirmReport."^^xsd:string ;
.
iapd-sec-cr:IAPDFirmSECReport
  rdf:type owl:Class ;
  sxml:tag "IAPDFirmSECReport" ;
  rdfs:comment "The Compilation Report contains information for any firm that currently holds an approved-equivalent registration with the SEC, or currently hold an ERA-Active status with the SEC, and has filed a Form ADV.The question numbers correspond to Form ADV version 10/2012."@en ;
  rdfs:label "IAPDFirm SECReport"^^xsd:string ;
  rdfs:subClassOf iapd-sec-cr:IAPDFirmSECReportType ;
.
iapd-sec-cr:IAPDFirmSECReportType
  rdf:type owl:Class ;
  sxml:tag "IAPDFirmSECReportType" ;
  rdfs:label "IAPDFirm SECReport type"^^xsd:string ;
  rdfs:subClassOf iapd-sec-cr:FirmReport ;
  rdfs:subClassOf [
      rdf:type owl:Restriction ;
      sxml:isAttribute "false"^^xsd:boolean ;
      sxml:order "0"^^xsd:int ;
      owl:allValuesFrom iapd-sec-cr:IAPDFirmSECReportType-firms ;
      owl:onProperty iapd-sec-cr:firmsRef ;
    ] ;
  rdfs:subClassOf [
      rdf:type owl:Restriction ;
      sxml:isAttribute "true"^^xsd:boolean ;
      rdfs:comment "This node contains the report generated date information."@en ;
      owl:allValuesFrom xsd:date ;
      owl:onProperty iapd-sec-cr:genOn ;
    ] ;
  rdfs:subClassOf [
      rdf:type owl:Restriction ;
      owl:cardinality "1"^^xsd:int ;
      owl:onProperty iapd-sec-cr:firmsRef ;
    ] ;
  rdfs:subClassOf [
      rdf:type owl:Restriction ;
      owl:cardinality "1"^^xsd:int ;
      owl:onProperty iapd-sec-cr:genOn ;
    ] ;
  skos:definition "This is the root class for the report structure. It has one instance for each report with the generation date. The object property iapd-sec-cr:firmsRef connects to an instance of iapd-sec-cr:IAPDFirmSECReportType-firms, which is root for the list of reporting firms."^^xsd:string ;
.
iapd-sec-cr:IAPDFirmSECReportType-firms
  rdf:type owl:Class ;
  rdfs:comment "There is one instance of this class for each report. The object property iapd-sec-cr:firmRef links to instances of iapd-sec-cr:SECFirmType, which is the root for a firm filing."^^xsd:string ;
  rdfs:label "IAPDFirm SECReport type-firms"^^xsd:string ;
  rdfs:subClassOf iapd-sec-cr:FirmReport ;
  rdfs:subClassOf [
      rdf:type owl:Restriction ;
      sxml:isAttribute "false"^^xsd:boolean ;
      sxml:order "0"^^xsd:int ;
      rdfs:comment "This node contains the list of firms information."@en ;
      owl:allValuesFrom iapd-sec-cr:SECFirmType ;
      owl:onProperty iapd-sec-cr:firmRef ;
    ] ;
  rdfs:subClassOf [
      rdf:type owl:Restriction ;
      owl:minCardinality "1"^^xsd:int ;
      owl:onProperty iapd-sec-cr:firmRef ;
    ] ;
  skos:definition "The class is a list with references to the individual firm reports."^^xsd:string ;
.
iapd-sec-cr:Int10Datatype
  rdf:type rdfs:Datatype ;
  rdfs:label "Int10Datatype"^^xsd:string ;
  rdfs:subClassOf xsd:integer ;
  owl:equivalentClass [
      rdf:type rdfs:Datatype ;
      owl:onDatatype xsd:integer ;
      owl:withRestrictions (
          [
            xsd:totalDigits 10 ;
          ]
        ) ;
    ] ;
.
iapd-sec-cr:Int38Datatype
  rdf:type rdfs:Datatype ;
  rdfs:label "Int38Datatype"^^xsd:string ;
  rdfs:subClassOf xsd:integer ;
  owl:equivalentClass [
      rdf:type rdfs:Datatype ;
      owl:onDatatype xsd:integer ;
      owl:withRestrictions (
          [
            xsd:totalDigits 38 ;
          ]
        ) ;
    ] ;
.
iapd-sec-cr:Int3Datatype
  rdf:type rdfs:Datatype ;
  rdfs:label "Int3Datatype"^^xsd:string ;
  rdfs:subClassOf xsd:integer ;
  owl:equivalentClass [
      rdf:type rdfs:Datatype ;
      owl:onDatatype xsd:integer ;
      owl:withRestrictions (
          [
            xsd:totalDigits 3 ;
          ]
        ) ;
    ] ;
.
iapd-sec-cr:Int8Datatype
  rdf:type rdfs:Datatype ;
  rdfs:label "Int8Datatype"^^xsd:string ;
  rdfs:subClassOf xsd:integer ;
  owl:equivalentClass [
      rdf:type rdfs:Datatype ;
      owl:onDatatype xsd:integer ;
      owl:withRestrictions (
          [
            xsd:totalDigits 8 ;
          ]
        ) ;
    ] ;
.
iapd-sec-cr:Item10AType
  rdf:type owl:Class ;
  sxml:tag "Item10AType" ;
  rdfs:label "Item10AType"^^xsd:string ;
  rdfs:subClassOf iapd-sec-cr:FirmReport ;
  rdfs:subClassOf [
      rdf:type owl:Restriction ;
      sxml:isAttribute "true"^^xsd:boolean ;
      rdfs:comment "This node has Firm's response to Part1A Item 10A -Does any person not named in Item 1.A. or Schedules A, B, or C, directly or indirectly, control your management or policies (Y/N/null)."@en ;
      owl:allValuesFrom iapd-sec-cr:AnswerYNType ;
      owl:onProperty iapd-sec-cr:q10A ;
    ] ;
  rdfs:subClassOf [
      rdf:type owl:Restriction ;
      owl:maxCardinality "1"^^xsd:int ;
      owl:onProperty iapd-sec-cr:q10A ;
    ] ;
  skos:definition "Firm's response to Part1A Item 10A -Does any person not named in Item 1.A. or Schedules A, B, or C, directly or indirectly, control your management or policies (Y/N/null). -->"^^xsd:string ;
.
iapd-sec-cr:Item11AType
  rdf:type owl:Class ;
  sxml:tag "Item11AType" ;
  rdfs:label "Item11AType"^^xsd:string ;
  rdfs:subClassOf iapd-sec-cr:FirmReport ;
  rdfs:subClassOf [
      rdf:type owl:Restriction ;
      sxml:isAttribute "true"^^xsd:boolean ;
      rdfs:comment "This node has Firm's response to Part1A Item 11A(1)-been convicted of or plead guilty or nolo contendere (\"no contest\") in a domestic, foreign, or military court to any felony (Y/N/null)."@en ;
      owl:allValuesFrom iapd-sec-cr:AnswerYNType ;
      owl:onProperty iapd-sec-cr:q11A1 ;
    ] ;
  rdfs:subClassOf [
      rdf:type owl:Restriction ;
      sxml:isAttribute "true"^^xsd:boolean ;
      rdfs:comment "This node has Firm's response to Part1A Item 11A(2)-been charged with any felony (Y/N/null)."@en ;
      owl:allValuesFrom iapd-sec-cr:AnswerYNType ;
      owl:onProperty iapd-sec-cr:q11A2 ;
    ] ;
  rdfs:subClassOf [
      rdf:type owl:Restriction ;
      owl:maxCardinality "1"^^xsd:int ;
      owl:onProperty iapd-sec-cr:q11A1 ;
    ] ;
  rdfs:subClassOf [
      rdf:type owl:Restriction ;
      owl:maxCardinality "1"^^xsd:int ;
      owl:onProperty iapd-sec-cr:q11A2 ;
    ] ;
  skos:definition """Firm's response to Part1A Item 11A(1)-been convicted of or plead guilty or nolo contendere (\"no contest\") in a domestic, foreign, or military court to any felony (Y/N/null).
Firm's response to Part1A Item 11A(2)-been charged with any felony (Y/N/null)."""^^xsd:string ;
.
iapd-sec-cr:Item11BType
  rdf:type owl:Class ;
  sxml:tag "Item11BType" ;
  rdfs:label "Item11BType"^^xsd:string ;
  rdfs:subClassOf iapd-sec-cr:FirmReport ;
  rdfs:subClassOf [
      rdf:type owl:Restriction ;
      sxml:isAttribute "true"^^xsd:boolean ;
      rdfs:comment "This node has Firm's response to Part1A Item 11B(1)-been convicted of or plead guilty or nolo contendere (\"no contest\") in a domestic, foreign, or military court to a misdemeanor involving: investments or an investment-related business, or any fraud, false statements, or omissions, wrongful taking of property, bribery, perjury, forgery, counterfeiting, extortion, or a conspiracy to commit any of these offenses (Y/N/null)."@en ;
      owl:allValuesFrom iapd-sec-cr:AnswerYNType ;
      owl:onProperty iapd-sec-cr:q11B1 ;
    ] ;
  rdfs:subClassOf [
      rdf:type owl:Restriction ;
      sxml:isAttribute "true"^^xsd:boolean ;
      rdfs:comment "This node has Firm's response to Part1A Item 11B(2)-been charged with a misdemeanor listed in 11.B(1) (Y/N/null)."@en ;
      owl:allValuesFrom iapd-sec-cr:AnswerYNType ;
      owl:onProperty iapd-sec-cr:q11B2 ;
    ] ;
  rdfs:subClassOf [
      rdf:type owl:Restriction ;
      owl:maxCardinality "1"^^xsd:int ;
      owl:onProperty iapd-sec-cr:q11B1 ;
    ] ;
  rdfs:subClassOf [
      rdf:type owl:Restriction ;
      owl:maxCardinality "1"^^xsd:int ;
      owl:onProperty iapd-sec-cr:q11B2 ;
    ] ;
  skos:definition """Firm's response to Part1A Item 11B(1)-been convicted of or plead guilty or nolo contendere (\"no contest\") in a domestic, foreign, or military court to a misdemeanor involving: investments or an investment-related business, or any fraud, false statements, or omissions, wrongful taking of property, bribery, perjury, forgery, counterfeiting, extortion, or a conspiracy to commit any of these offenses (Y/N/null).
Firm's response to Part1A Item 11B(2)-been charged with a misdemeanor listed in 11.B(1) (Y/N/null)."""^^xsd:string ;
.
iapd-sec-cr:Item11CType
  rdf:type owl:Class ;
  sxml:tag "Item11CType" ;
  rdfs:comment "The answers are object properties to instances of the anwerYNType class."^^xsd:string ;
  rdfs:label "Item11CType"^^xsd:string ;
  rdfs:subClassOf iapd-sec-cr:FirmReport ;
  rdfs:subClassOf [
      rdf:type owl:Restriction ;
      sxml:isAttribute "true"^^xsd:boolean ;
      rdfs:comment "This node has Firm's response to Part1A Item 11C(1)-found you or any advisory affiliate to have made a false statement or omission (Y/N/null)."@en ;
      owl:allValuesFrom iapd-sec-cr:AnswerYNType ;
      owl:onProperty iapd-sec-cr:q11C1 ;
    ] ;
  rdfs:subClassOf [
      rdf:type owl:Restriction ;
      sxml:isAttribute "true"^^xsd:boolean ;
      rdfs:comment "This node has Firm's response to Part1A Item 11C(2)-found you or any advisory affiliate to have been involved in a violation of SEC or CFTC regulations or statutes (Y/N)."@en ;
      owl:allValuesFrom iapd-sec-cr:AnswerYNType ;
      owl:onProperty iapd-sec-cr:q11C2 ;
    ] ;
  rdfs:subClassOf [
      rdf:type owl:Restriction ;
      sxml:isAttribute "true"^^xsd:boolean ;
      rdfs:comment "This node has Firm's response to Part1A Item 11C(3)-found you or any advisory affiliate to have been a cause of an investment-related business having its authorization to do business denied, suspended, revoked, or restricted (Y/N/null)."@en ;
      owl:allValuesFrom iapd-sec-cr:AnswerYNType ;
      owl:onProperty iapd-sec-cr:q11C3 ;
    ] ;
  rdfs:subClassOf [
      rdf:type owl:Restriction ;
      sxml:isAttribute "true"^^xsd:boolean ;
      rdfs:comment "This node has Firm's response to Part1A Item 11C(4)-entered an order against you or any advisory affiliate in connection with investment-related activity (Y/N/null)."@en ;
      owl:allValuesFrom iapd-sec-cr:AnswerYNType ;
      owl:onProperty iapd-sec-cr:q11C4 ;
    ] ;
  rdfs:subClassOf [
      rdf:type owl:Restriction ;
      sxml:isAttribute "true"^^xsd:boolean ;
      rdfs:comment "This node has Firm's response to Part1A Item 11C(5)-imposed a civil money penalty on you or any advisory affiliate, or ordered you or any advisory affiliate to cease and desist from any activity (Y/N/null)."@en ;
      owl:allValuesFrom iapd-sec-cr:AnswerYNType ;
      owl:onProperty iapd-sec-cr:q11C5 ;
    ] ;
  rdfs:subClassOf [
      rdf:type owl:Restriction ;
      owl:maxCardinality "1"^^xsd:int ;
      owl:onProperty iapd-sec-cr:q11C1 ;
    ] ;
  rdfs:subClassOf [
      rdf:type owl:Restriction ;
      owl:maxCardinality "1"^^xsd:int ;
      owl:onProperty iapd-sec-cr:q11C2 ;
    ] ;
  rdfs:subClassOf [
      rdf:type owl:Restriction ;
      owl:maxCardinality "1"^^xsd:int ;
      owl:onProperty iapd-sec-cr:q11C3 ;
    ] ;
  rdfs:subClassOf [
      rdf:type owl:Restriction ;
      owl:maxCardinality "1"^^xsd:int ;
      owl:onProperty iapd-sec-cr:q11C4 ;
    ] ;
  rdfs:subClassOf [
      rdf:type owl:Restriction ;
      owl:maxCardinality "1"^^xsd:int ;
      owl:onProperty iapd-sec-cr:q11C5 ;
    ] ;
  skos:definition """Firm's response to Part1A Item 11C - Has the SEC or the Commodity Futures Trading Commission (CFTC) ever:
(1) found you or any advisory affiliate to have made a false statement or omission?
(2) found you or any advisory affiliate to have been involved in a violation of SEC
or CFTC regulations or statutes?
(3) found you or any advisory affiliate to have been a cause of an investment-related
business having its authorization to do business denied, suspended, revoked, or
restricted?
(4) entered an order against you or any advisory affiliate in connection with
investment-related activity?
(5) imposed a civil money penalty on you or any advisory affiliate, or ordered you
or any advisory affiliate to cease and desist from any activity?"""^^xsd:string ;
.
iapd-sec-cr:Item11DType
  rdf:type owl:Class ;
  sxml:tag "Item11DType" ;
  rdfs:comment "The answers are object properties to instances of the anwerYNType class."^^xsd:string ;
  rdfs:label "Item11DType"^^xsd:string ;
  rdfs:subClassOf iapd-sec-cr:FirmReport ;
  rdfs:subClassOf [
      rdf:type owl:Restriction ;
      sxml:isAttribute "true"^^xsd:boolean ;
      rdfs:comment "This node has Firm's response to Item 11D(5)-ever denied, suspended, or revoked your or any advisory affiliate's registration or license, or otherwise prevented you or any advisory affiliate, by order, from associating with an investment-related business or restricted your or any advisory affiliate's activity (Y/N/null)."@en ;
      owl:allValuesFrom iapd-sec-cr:AnswerYNType ;
      owl:onProperty iapd-sec-cr:q11D5 ;
    ] ;
  rdfs:subClassOf [
      rdf:type owl:Restriction ;
      sxml:isAttribute "true"^^xsd:boolean ;
      rdfs:comment "This node has Firm's response to Part1A Item 11D(1)-ever found you or any advisory affiliate to have made a false statement or omission, or been dishonest, unfair, or unethical (Y/N/null)."@en ;
      owl:allValuesFrom iapd-sec-cr:AnswerYNType ;
      owl:onProperty iapd-sec-cr:q11D1 ;
    ] ;
  rdfs:subClassOf [
      rdf:type owl:Restriction ;
      sxml:isAttribute "true"^^xsd:boolean ;
      rdfs:comment "This node has Firm's response to Part1A Item 11D(2)-ever found you or any advisory affiliate to have been involved in a violation of investment-related regulations or statutes (Y/N/null)."@en ;
      owl:allValuesFrom iapd-sec-cr:AnswerYNType ;
      owl:onProperty iapd-sec-cr:q11D2 ;
    ] ;
  rdfs:subClassOf [
      rdf:type owl:Restriction ;
      sxml:isAttribute "true"^^xsd:boolean ;
      rdfs:comment "This node has Firm's response to Part1A Item 11D(3)-ever found you or any advisory affiliate to have been a cause of an investment-related business having its authorization to do business denied, suspended, revoked, or restricted (Y/N/null)."@en ;
      owl:allValuesFrom iapd-sec-cr:AnswerYNType ;
      owl:onProperty iapd-sec-cr:q11D3 ;
    ] ;
  rdfs:subClassOf [
      rdf:type owl:Restriction ;
      sxml:isAttribute "true"^^xsd:boolean ;
      rdfs:comment "This node has Firm's response to Part1A Item 11D(4)-in the past ten years, entered an order against you or any advisory affiliate in connection with an investment-related activity (Y/N/null)."@en ;
      owl:allValuesFrom iapd-sec-cr:AnswerYNType ;
      owl:onProperty iapd-sec-cr:q11D4 ;
    ] ;
  rdfs:subClassOf [
      rdf:type owl:Restriction ;
      owl:maxCardinality "1"^^xsd:int ;
      owl:onProperty iapd-sec-cr:q11D1 ;
    ] ;
  rdfs:subClassOf [
      rdf:type owl:Restriction ;
      owl:maxCardinality "1"^^xsd:int ;
      owl:onProperty iapd-sec-cr:q11D2 ;
    ] ;
  rdfs:subClassOf [
      rdf:type owl:Restriction ;
      owl:maxCardinality "1"^^xsd:int ;
      owl:onProperty iapd-sec-cr:q11D3 ;
    ] ;
  rdfs:subClassOf [
      rdf:type owl:Restriction ;
      owl:maxCardinality "1"^^xsd:int ;
      owl:onProperty iapd-sec-cr:q11D4 ;
    ] ;
  rdfs:subClassOf [
      rdf:type owl:Restriction ;
      owl:maxCardinality "1"^^xsd:int ;
      owl:onProperty iapd-sec-cr:q11D5 ;
    ] ;
  skos:definition """Firm's response to Part1A Item 11D - federal regulatory agency, any state regulatory agency, or any foreign financial regulatory authority:
(1) ever found you or any advisory affiliate to have made a false statement or omission, or been dishonest, unfair, or unethical?
(2) ever found you or any advisory affiliate to have been involved in a violation of investment-related regulations or statutes?
(3) ever found you or any advisory affiliate to have been a cause of an investment-related business having its authorization to do business denied, suspended, revoked, or restricted?
(4) in the past ten years, entered an order against you or any advisory affiliate in connection with an investment-related activity?
(5) ever denied, suspended, or revoked your or any advisory affiliate’s registration or license, or otherwise prevented you or any advisory affiliate, by order, from associating with an investment-"""^^xsd:string ;
.
iapd-sec-cr:Item11EType
  rdf:type owl:Class ;
  sxml:tag "Item11EType" ;
  rdfs:comment "The answers are object properties to instances of the anwerYNType class."^^xsd:string ;
  rdfs:label "Item11EType"^^xsd:string ;
  rdfs:subClassOf iapd-sec-cr:FirmReport ;
  rdfs:subClassOf [
      rdf:type owl:Restriction ;
      sxml:isAttribute "true"^^xsd:boolean ;
      rdfs:comment "This node has Firm's response to Item 11E(2)-found you or any advisory affiliate to have been involved in a violation of its rules (other than a violation designated as a \"minor rule violation\" under a plan approved by the SEC) (Y/N/null)."@en ;
      owl:allValuesFrom iapd-sec-cr:AnswerYNType ;
      owl:onProperty iapd-sec-cr:q11E2 ;
    ] ;
  rdfs:subClassOf [
      rdf:type owl:Restriction ;
      sxml:isAttribute "true"^^xsd:boolean ;
      rdfs:comment "This node has Firm's response to Part1A Item 11E(1)-found you or any advisory affiliate to have made a false statement or omission (Y/N/null)."@en ;
      owl:allValuesFrom iapd-sec-cr:AnswerYNType ;
      owl:onProperty iapd-sec-cr:q11E1 ;
    ] ;
  rdfs:subClassOf [
      rdf:type owl:Restriction ;
      sxml:isAttribute "true"^^xsd:boolean ;
      rdfs:comment "This node has Firm's response to Part1A Item 11E(3)-found you or any advisory affiliate to have been the cause of an investment-related business having its authorization to do business denied, suspended, revoked, or restricted (Y/N/null)."@en ;
      owl:allValuesFrom iapd-sec-cr:AnswerYNType ;
      owl:onProperty iapd-sec-cr:q11E3 ;
    ] ;
  rdfs:subClassOf [
      rdf:type owl:Restriction ;
      sxml:isAttribute "true"^^xsd:boolean ;
      rdfs:comment "This node has Firm's response to Part1A Item 11E(4)-disciplined you or any advisory affiliate by expelling or suspending you or the advisory affiliate from membership, barring or suspending you or the advisory affiliate from association with other members, or otherwise restricting your or the advisory affiliate's activities (Y/N/null)."@en ;
      owl:allValuesFrom iapd-sec-cr:AnswerYNType ;
      owl:onProperty iapd-sec-cr:q11E4 ;
    ] ;
  rdfs:subClassOf [
      rdf:type owl:Restriction ;
      owl:maxCardinality "1"^^xsd:int ;
      owl:onProperty iapd-sec-cr:q11E1 ;
    ] ;
  rdfs:subClassOf [
      rdf:type owl:Restriction ;
      owl:maxCardinality "1"^^xsd:int ;
      owl:onProperty iapd-sec-cr:q11E2 ;
    ] ;
  rdfs:subClassOf [
      rdf:type owl:Restriction ;
      owl:maxCardinality "1"^^xsd:int ;
      owl:onProperty iapd-sec-cr:q11E3 ;
    ] ;
  rdfs:subClassOf [
      rdf:type owl:Restriction ;
      owl:maxCardinality "1"^^xsd:int ;
      owl:onProperty iapd-sec-cr:q11E4 ;
    ] ;
  skos:definition """Firm's response to Part1A Item 11E - Has any self-regulatory organization or commodities exchange ever:
(1) found you or any advisory affiliate to have made a false statement or omission?
(2) found you or any advisory affiliate to have been involved in a violation of its rules (other than a violation designated as a “minor rule violation” under a plan approved by the SEC)?
(3) found you or any advisory affiliate to have been the cause of an investment-related business having its authorization to do business denied, suspended, revoked, or restricted?
(4) disciplined you or any advisory affiliate by expelling or suspending you or the advisory affiliate from membership, barring or suspending you or the advisory affiliate from association with other members, or otherwise restricting your or the advisory affiliate’s activities?"""^^xsd:string ;
.
iapd-sec-cr:Item11FType
  rdf:type owl:Class ;
  sxml:tag "Item11FType" ;
  rdfs:label "Item11FType"^^xsd:string ;
  rdfs:subClassOf iapd-sec-cr:FirmReport ;
  rdfs:subClassOf [
      rdf:type owl:Restriction ;
      sxml:isAttribute "true"^^xsd:boolean ;
      rdfs:comment "This node has Firm's response to Part1A Item 11F-Has an authorization to act as an attorney, accountant, or federal contractor granted to you or any advisory affiliate ever been revoked or suspended (Y/N/null)."@en ;
      owl:allValuesFrom iapd-sec-cr:AnswerYNType ;
      owl:onProperty iapd-sec-cr:q11F ;
    ] ;
  rdfs:subClassOf [
      rdf:type owl:Restriction ;
      owl:maxCardinality "1"^^xsd:int ;
      owl:onProperty iapd-sec-cr:q11F ;
    ] ;
  skos:definition "Firm's response to Part1A Item 11F-Has an authorization to act as an attorney, accountant, or federal contractor granted to you or any advisory affiliate ever been revoked or suspended (Y/N/null)."^^xsd:string ;
.
iapd-sec-cr:Item11GType
  rdf:type owl:Class ;
  sxml:tag "Item11GType" ;
  rdfs:label "Item11GType"^^xsd:string ;
  rdfs:subClassOf iapd-sec-cr:FirmReport ;
  rdfs:subClassOf [
      rdf:type owl:Restriction ;
      sxml:isAttribute "true"^^xsd:boolean ;
      rdfs:comment "This node has Firm's response to Part1A Item 11G-Are you or any advisory affiliate now the subject of any regulatory proceeding that could result in a \"yes\" answer to any part of Item 11.C., 11.D., or 11.E. (Y/N/null)."@en ;
      owl:allValuesFrom iapd-sec-cr:AnswerYNType ;
      owl:onProperty iapd-sec-cr:q11G ;
    ] ;
  rdfs:subClassOf [
      rdf:type owl:Restriction ;
      owl:maxCardinality "1"^^xsd:int ;
      owl:onProperty iapd-sec-cr:q11G ;
    ] ;
  skos:definition "Firm's response to Part1A Item 11G-Are you or any advisory affiliate now the subject of any regulatory proceeding that could result in a \"yes\" answer to any part of Item 11.C., 11.D., or 11.E. (Y/N/null)."^^xsd:string ;
.
iapd-sec-cr:Item11HType
  rdf:type owl:Class ;
  sxml:tag "Item11HType" ;
  rdfs:comment "The answers are object properties to instances of the anwerYNType class."^^xsd:string ;
  rdfs:label "Item11HType"^^xsd:string ;
  rdfs:subClassOf iapd-sec-cr:FirmReport ;
  rdfs:subClassOf [
      rdf:type owl:Restriction ;
      sxml:isAttribute "true"^^xsd:boolean ;
      rdfs:comment "This node has Firm's response to Part1A Item 11H(1)(a)-the past ten years, enjoined you or any advisory affiliate in connection with any investment-related activity (Y/N/null)."@en ;
      owl:allValuesFrom iapd-sec-cr:AnswerYNType ;
      owl:onProperty iapd-sec-cr:q11H1A ;
    ] ;
  rdfs:subClassOf [
      rdf:type owl:Restriction ;
      sxml:isAttribute "true"^^xsd:boolean ;
      rdfs:comment "This node has Firm's response to Part1A Item 11H(1)(b)-ever found that you or any advisory affiliate were involved in a violation of investment-related statutes or regulations (Y/N/null)."@en ;
      owl:allValuesFrom iapd-sec-cr:AnswerYNType ;
      owl:onProperty iapd-sec-cr:q11H1B ;
    ] ;
  rdfs:subClassOf [
      rdf:type owl:Restriction ;
      sxml:isAttribute "true"^^xsd:boolean ;
      rdfs:comment "This node has Firm's response to Part1A Item 11H(1)(c)-ever dismissed, pursuant to a settlement agreement, an investment-related civil action brought against you or any advisory affiliate by a state or foreign financial regulatory authority (Y/N/null)."@en ;
      owl:allValuesFrom iapd-sec-cr:AnswerYNType ;
      owl:onProperty iapd-sec-cr:q11H1C ;
    ] ;
  rdfs:subClassOf [
      rdf:type owl:Restriction ;
      sxml:isAttribute "true"^^xsd:boolean ;
      rdfs:comment "This node has Firm's response to Part1A Item 11H(2)-Are you or any advisory affiliate now the subject of any civil proceeding that could result in a \"yes\" answer to any part of Item 11.H(1) (Y/N/null)."@en ;
      owl:allValuesFrom iapd-sec-cr:AnswerYNType ;
      owl:onProperty iapd-sec-cr:q11H2 ;
    ] ;
  rdfs:subClassOf [
      rdf:type owl:Restriction ;
      owl:maxCardinality "1"^^xsd:int ;
      owl:onProperty iapd-sec-cr:q11H1A ;
    ] ;
  rdfs:subClassOf [
      rdf:type owl:Restriction ;
      owl:maxCardinality "1"^^xsd:int ;
      owl:onProperty iapd-sec-cr:q11H1B ;
    ] ;
  rdfs:subClassOf [
      rdf:type owl:Restriction ;
      owl:maxCardinality "1"^^xsd:int ;
      owl:onProperty iapd-sec-cr:q11H1C ;
    ] ;
  rdfs:subClassOf [
      rdf:type owl:Restriction ;
      owl:maxCardinality "1"^^xsd:int ;
      owl:onProperty iapd-sec-cr:q11H2 ;
    ] ;
  skos:definition """Firm's response to Part1A Item 11H
(1) Has any domestic or foreign court:
(a) in the past ten years, enjoined you or any advisory affiliate in connection with any investment-related activity?
(b) ever found that you or any advisory affiliate were involved in a violation of investment-related statutes or regulations?
(c) ever dismissed, pursuant to a settlement agreement, an investment-related civil action brought against you or any advisory affiliate by a state or foreign financial regulatory authority?
(2) Are you or any advisory affiliate now the subject of any civil proceeding that could
result in a “yes” answer to any part of Item 11.H(1)?"""^^xsd:string ;
.
iapd-sec-cr:Item11Type
  rdf:type owl:Class ;
  sxml:tag "Item11Type" ;
  rdfs:label "Item11Type"^^xsd:string ;
  rdfs:subClassOf iapd-sec-cr:FirmReport ;
  rdfs:subClassOf [
      rdf:type owl:Restriction ;
      sxml:isAttribute "true"^^xsd:boolean ;
      rdfs:comment "This node has Firm's response to Part1A Item 11-Do any of the events below involve you or any of your supervised persons (Y/N/null)."@en ;
      owl:allValuesFrom iapd-sec-cr:AnswerYNType ;
      owl:onProperty iapd-sec-cr:q11 ;
    ] ;
  rdfs:subClassOf [
      rdf:type owl:Restriction ;
      owl:maxCardinality "1"^^xsd:int ;
      owl:onProperty iapd-sec-cr:q11 ;
    ] ;
  skos:definition "Firm's response to Part1A Item 11-Do any of the events below involve you or any of your supervised persons (Y/N/null)."^^xsd:string ;
.
iapd-sec-cr:Item1Type
  rdf:type owl:Class ;
  sxml:tag "Item1Type" ;
  rdfs:comment """The answers are to l,M,N, O are object properties to instances of the anwerYNType class. The LEI is an xsd:string
Web addresses are reference to instances of the Item1Type-webAddrs class."""^^xsd:string ;
  rdfs:label "Item1Type"^^xsd:string ;
  rdfs:subClassOf iapd-sec-cr:FirmReport ;
  rdfs:subClassOf [
      rdf:type owl:Restriction ;
      sxml:isAttribute "false"^^xsd:boolean ;
      sxml:order "0"^^xsd:int ;
      rdfs:comment "This node has Firm's response to Schedule D Section 1I Website Address-include all if there are multiple reported."@en ;
      owl:allValuesFrom iapd-sec-cr:Item1Type-webAddrs ;
      owl:onProperty iapd-sec-cr:webAddrsRef ;
    ] ;
  rdfs:subClassOf [
      rdf:type owl:Restriction ;
      sxml:isAttribute "true"^^xsd:boolean ;
      rdfs:comment "This node has Firm's response to Part1A Item 1I-Do you have one or more websites (Y/N/null)."@en ;
      owl:allValuesFrom iapd-sec-cr:AnswerYNType ;
      owl:onProperty iapd-sec-cr:q1I ;
    ] ;
  rdfs:subClassOf [
      rdf:type owl:Restriction ;
      sxml:isAttribute "true"^^xsd:boolean ;
      rdfs:comment "This node has Firm's response to Part1A Item 1M -Are you registered with a foreign financial regulatory authority (Y/N/null)."@en ;
      owl:allValuesFrom iapd-sec-cr:AnswerYNType ;
      owl:onProperty iapd-sec-cr:q1M ;
    ] ;
  rdfs:subClassOf [
      rdf:type owl:Restriction ;
      sxml:isAttribute "true"^^xsd:boolean ;
      rdfs:comment "This node has Firm's response to Part1A Item 1N-Are you a public reporting company under Sections 12 or 15(d) of the Securities Exchange Act of 1934 (Y/N/null)."@en ;
      owl:allValuesFrom iapd-sec-cr:AnswerYNType ;
      owl:onProperty iapd-sec-cr:q1N ;
    ] ;
  rdfs:subClassOf [
      rdf:type owl:Restriction ;
      sxml:isAttribute "true"^^xsd:boolean ;
      rdfs:comment "This node has Firm's response to Part1A Item 1N-If yes, provide your CIK number (Central Index Key number that the SEC assigns to each public reporting company)."@en ;
      owl:allValuesFrom xsd:unsignedInt ;
      owl:onProperty iapd-sec-cr:cIKNb ;
    ] ;
  rdfs:subClassOf [
      rdf:type owl:Restriction ;
      sxml:isAttribute "true"^^xsd:boolean ;
      rdfs:comment "This node has Firm's response to Part1A Item 1O-Did you have $1 billion or more in assets on the last day of your most recent fiscal year."@en ;
      owl:allValuesFrom iapd-sec-cr:AnswerYNType ;
      owl:onProperty iapd-sec-cr:q1O ;
    ] ;
  rdfs:subClassOf [
      rdf:type owl:Restriction ;
      sxml:isAttribute "true"^^xsd:boolean ;
      rdfs:comment "This node has Firm's response to Part1A Item 1P- Legal Entity Identifier."@en ;
      owl:allValuesFrom iapd-sec-cr:Str20Datatype ;
      owl:onProperty iapd-sec-cr:q1P ;
    ] ;
  rdfs:subClassOf [
      rdf:type owl:Restriction ;
      owl:cardinality "1"^^xsd:int ;
      owl:onProperty iapd-sec-cr:webAddrsRef ;
    ] ;
  rdfs:subClassOf [
      rdf:type owl:Restriction ;
      owl:maxCardinality "1"^^xsd:int ;
      owl:onProperty iapd-sec-cr:cIKNb ;
    ] ;
  rdfs:subClassOf [
      rdf:type owl:Restriction ;
      owl:maxCardinality "1"^^xsd:int ;
      owl:onProperty iapd-sec-cr:q1I ;
    ] ;
  rdfs:subClassOf [
      rdf:type owl:Restriction ;
      owl:maxCardinality "1"^^xsd:int ;
      owl:onProperty iapd-sec-cr:q1M ;
    ] ;
  rdfs:subClassOf [
      rdf:type owl:Restriction ;
      owl:maxCardinality "1"^^xsd:int ;
      owl:onProperty iapd-sec-cr:q1N ;
    ] ;
  rdfs:subClassOf [
      rdf:type owl:Restriction ;
      owl:maxCardinality "1"^^xsd:int ;
      owl:onProperty iapd-sec-cr:q1O ;
    ] ;
  rdfs:subClassOf [
      rdf:type owl:Restriction ;
      owl:maxCardinality "1"^^xsd:int ;
      owl:onProperty iapd-sec-cr:q1P ;
    ] ;
  skos:definition """The firm Identifying Information.This maps to Form ADV - Item 1
L. Do you maintain some or all of the books and records you are required to keep under Section 204 of the Advisers Act, or similar state law, somewhere other than your principal office and place of business?
M. Are you registered with a foreign financial regulatory authority?
N. Are you a public reporting company under Sections 12 or 15(d) of the Securities Exchange Act of 1934?
O. Did you have $1 billion or more in assets on the last day of your most recent fiscal year?
P. Provide your Legal Entity Identifier if you have one:"""^^xsd:string ;
.
iapd-sec-cr:Item1Type-webAddrs
  rdf:type owl:Class ;
  rdfs:label "Item1Type-web addrs"^^xsd:string ;
  rdfs:subClassOf iapd-sec-cr:FirmReport ;
  rdfs:subClassOf [
      rdf:type owl:Restriction ;
      sxml:isAttribute "false"^^xsd:boolean ;
      sxml:order "0"^^xsd:int ;
      owl:allValuesFrom iapd-sec-cr:Str128Datatype ;
      owl:onProperty iapd-sec-cr:webAddr ;
    ] ;
  skos:definition "Firm's response to Part1A Item 1I-Do you have one or more websites (xsd:string)."^^xsd:string ;
.
iapd-sec-cr:Item2AType
  rdf:type owl:Class ;
  sxml:tag "Item2AType" ;
  rdfs:comment "Part 1A Item 2A has Yes/No questions about the firms assets, offices, and advisory business. The questions are modeled as object properties with the range of AnswerYNType."^^xsd:string ;
  rdfs:label "Item2AType"^^xsd:string ;
  rdfs:subClassOf iapd-sec-cr:FirmReport ;
  rdfs:subClassOf [
      rdf:type owl:Restriction ;
      sxml:isAttribute "true"^^xsd:boolean ;
      rdfs:comment """This node has Firm's response to Part1A Item 2A(1)- are a large advisory firm that either:
          (a) has regulatory assets under management of $100 million (in U.S. dollars) or more, or
          (b) is SEC-registered and is submitting an annual updating amendment and has regulatory assets under management of $90 million (in U.S. dollars) or more (Y/N) Display a 'Y' when the checkbox is selected.
              Display an 'N' when the checkbox is not selected."""@en ;
      owl:allValuesFrom iapd-sec-cr:AnswerYNType ;
      owl:onProperty iapd-sec-cr:q2A1 ;
    ] ;
  rdfs:subClassOf [
      rdf:type owl:Restriction ;
      sxml:isAttribute "true"^^xsd:boolean ;
      rdfs:comment "This node has Firm's response to Part1A Item 2A(10) are a multi-state adviser that is required to register in 15 or more states and is relying on rule 203A-2(d) (Y/N) Display a 'Y' when the checkbox is selected. Display an 'N' when the checkbox is not selected."@en ;
      owl:allValuesFrom iapd-sec-cr:AnswerYNType ;
      owl:onProperty iapd-sec-cr:q2A10 ;
    ] ;
  rdfs:subClassOf [
      rdf:type owl:Restriction ;
      sxml:isAttribute "true"^^xsd:boolean ;
      rdfs:comment "This node has Firm's response to Part1A Item 2A(11)-are an Internet adviser relying on rule 203A-2(e) (Y/N) Display a 'Y' when the checkbox is selected. Display an 'N' when the checkbox is not selected."@en ;
      owl:allValuesFrom iapd-sec-cr:AnswerYNType ;
      owl:onProperty iapd-sec-cr:q2A11 ;
    ] ;
  rdfs:subClassOf [
      rdf:type owl:Restriction ;
      sxml:isAttribute "true"^^xsd:boolean ;
      rdfs:comment "This node has Firm's response to Part1A Item 2A(12)-have received an SEC order exempting you from the prohibition against registration with the SEC (Y/N) Display a 'Y' when the checkbox is selected. Display an 'N' when the checkbox is not selected."@en ;
      owl:allValuesFrom iapd-sec-cr:AnswerYNType ;
      owl:onProperty iapd-sec-cr:q2A12 ;
    ] ;
  rdfs:subClassOf [
      rdf:type owl:Restriction ;
      sxml:isAttribute "true"^^xsd:boolean ;
      rdfs:comment "This node has Firm's response to Part1A Item 2A(13)-are no longer eligible to remain registered with the SEC (Y/N) Display a 'Y' when the checkbox is selected. Display an 'N' when the checkbox is not selected."@en ;
      owl:allValuesFrom iapd-sec-cr:AnswerYNType ;
      owl:onProperty iapd-sec-cr:q2A13 ;
    ] ;
  rdfs:subClassOf [
      rdf:type owl:Restriction ;
      sxml:isAttribute "true"^^xsd:boolean ;
      rdfs:comment """This node has Firm's response to Part1A Item 2A(2)-are a mid-sized advisory firm that has regulatory assets under management of $25 million (in U.S. dollars) or more but less than $100 million (in U.S. dollars) and you are either:
          (a) not required to be registered as an adviser with the state securities authority of the state where you maintain your principal office and place of business, or
          (b) not subject to examination by the state securities authority of the state where you maintain your principal office and place of business (Y/N) Display a 'Y' when the checkbox is selected. 
              Display an 'N' when the checkbox is not selected."""@en ;
      owl:allValuesFrom iapd-sec-cr:AnswerYNType ;
      owl:onProperty iapd-sec-cr:q2A2 ;
    ] ;
  rdfs:subClassOf [
      rdf:type owl:Restriction ;
      sxml:isAttribute "true"^^xsd:boolean ;
      rdfs:comment "This node has Firm's response to Part1A Item 2A(3)-have your principal office and place of business in Wyoming (which does not regulate advisers) (Y/N) Display a 'Y' when the checkbox is selected. Display an 'N' when the checkbox is not selected."@en ;
      owl:allValuesFrom iapd-sec-cr:AnswerYNType ;
      owl:onProperty iapd-sec-cr:q2A3 ;
    ] ;
  rdfs:subClassOf [
      rdf:type owl:Restriction ;
      sxml:isAttribute "true"^^xsd:boolean ;
      rdfs:comment "This node has Firm's response to Part1A Item 2A(4)-have your principal office and place of business outside the United States (Y/N) Display a 'Y' when the checkbox is selected. Display an 'N' when the checkbox is not selected."@en ;
      owl:allValuesFrom iapd-sec-cr:AnswerYNType ;
      owl:onProperty iapd-sec-cr:q2A4 ;
    ] ;
  rdfs:subClassOf [
      rdf:type owl:Restriction ;
      sxml:isAttribute "true"^^xsd:boolean ;
      rdfs:comment "This node has Firm's response to Part1A Item 2A(5)-are an investment adviser (or sub-adviser) to an investment company registered under the Investment Company Act of 1940 (Y/N) Display a 'Y' when the checkbox is selected. Display an 'N' when the checkbox is not selected."@en ;
      owl:allValuesFrom iapd-sec-cr:AnswerYNType ;
      owl:onProperty iapd-sec-cr:q2A5 ;
    ] ;
  rdfs:subClassOf [
      rdf:type owl:Restriction ;
      sxml:isAttribute "true"^^xsd:boolean ;
      rdfs:comment "This node has Firm's response to Part1A Item 2A(6)-are an investment adviser to a company which has elected to be a business development company pursuant to section 54 of the Investment Company Act of 1940 and has not withdrawn the election, and you have at least $25 million of regulatory assets under management (Y/N)."@en ;
      owl:allValuesFrom iapd-sec-cr:AnswerYNType ;
      owl:onProperty iapd-sec-cr:q2A6 ;
    ] ;
  rdfs:subClassOf [
      rdf:type owl:Restriction ;
      sxml:isAttribute "true"^^xsd:boolean ;
      rdfs:comment "This node has Firm's response to Part1A Item 2A(7)-are a pension consultant with respect to assets of plans having an aggregate value of at least $200,000,000 that qualifies for the exemption in rule 203A-2 (Y/N) Display a 'Y' when the checkbox is selected. Display an 'N' when the checkbox is not selected."@en ;
      owl:allValuesFrom iapd-sec-cr:AnswerYNType ;
      owl:onProperty iapd-sec-cr:q2A7 ;
    ] ;
  rdfs:subClassOf [
      rdf:type owl:Restriction ;
      sxml:isAttribute "true"^^xsd:boolean ;
      rdfs:comment "This node has Firm's response to Part1A Item 2A(8)-are a related adviser under rule 203A-2(b) that controls, is controlled by, or is under common control with, an investment adviser that is registered with the SEC, and your principal office and place of business is the same as the registered adviser (Y/N) Display a 'Y' when the checkbox is selected. Display an 'N' when the checkbox is not selected."@en ;
      owl:allValuesFrom iapd-sec-cr:AnswerYNType ;
      owl:onProperty iapd-sec-cr:q2A8 ;
    ] ;
  rdfs:subClassOf [
      rdf:type owl:Restriction ;
      sxml:isAttribute "true"^^xsd:boolean ;
      rdfs:comment "This node has Firm's response to Part1A Item 2A(9)-are a newly formed adviser relying on rule 203A-2(c) because you expect to be eligible for SEC registration within 120 days (Y/N) Display a 'Y' when the checkbox is selected. Display an 'N' when the checkbox is not selected."@en ;
      owl:allValuesFrom iapd-sec-cr:AnswerYNType ;
      owl:onProperty iapd-sec-cr:q2A9 ;
    ] ;
  rdfs:subClassOf [
      rdf:type owl:Restriction ;
      owl:maxCardinality "1"^^xsd:int ;
      owl:onProperty iapd-sec-cr:q2A1 ;
    ] ;
  rdfs:subClassOf [
      rdf:type owl:Restriction ;
      owl:maxCardinality "1"^^xsd:int ;
      owl:onProperty iapd-sec-cr:q2A10 ;
    ] ;
  rdfs:subClassOf [
      rdf:type owl:Restriction ;
      owl:maxCardinality "1"^^xsd:int ;
      owl:onProperty iapd-sec-cr:q2A11 ;
    ] ;
  rdfs:subClassOf [
      rdf:type owl:Restriction ;
      owl:maxCardinality "1"^^xsd:int ;
      owl:onProperty iapd-sec-cr:q2A12 ;
    ] ;
  rdfs:subClassOf [
      rdf:type owl:Restriction ;
      owl:maxCardinality "1"^^xsd:int ;
      owl:onProperty iapd-sec-cr:q2A13 ;
    ] ;
  rdfs:subClassOf [
      rdf:type owl:Restriction ;
      owl:maxCardinality "1"^^xsd:int ;
      owl:onProperty iapd-sec-cr:q2A2 ;
    ] ;
  rdfs:subClassOf [
      rdf:type owl:Restriction ;
      owl:maxCardinality "1"^^xsd:int ;
      owl:onProperty iapd-sec-cr:q2A3 ;
    ] ;
  rdfs:subClassOf [
      rdf:type owl:Restriction ;
      owl:maxCardinality "1"^^xsd:int ;
      owl:onProperty iapd-sec-cr:q2A4 ;
    ] ;
  rdfs:subClassOf [
      rdf:type owl:Restriction ;
      owl:maxCardinality "1"^^xsd:int ;
      owl:onProperty iapd-sec-cr:q2A5 ;
    ] ;
  rdfs:subClassOf [
      rdf:type owl:Restriction ;
      owl:maxCardinality "1"^^xsd:int ;
      owl:onProperty iapd-sec-cr:q2A6 ;
    ] ;
  rdfs:subClassOf [
      rdf:type owl:Restriction ;
      owl:maxCardinality "1"^^xsd:int ;
      owl:onProperty iapd-sec-cr:q2A7 ;
    ] ;
  rdfs:subClassOf [
      rdf:type owl:Restriction ;
      owl:maxCardinality "1"^^xsd:int ;
      owl:onProperty iapd-sec-cr:q2A8 ;
    ] ;
  rdfs:subClassOf [
      rdf:type owl:Restriction ;
      owl:maxCardinality "1"^^xsd:int ;
      owl:onProperty iapd-sec-cr:q2A9 ;
    ] ;
  skos:definition "Firm's response to Part1A Item 2A."^^xsd:string ;
.
iapd-sec-cr:Item2BType
  rdf:type owl:Class ;
  sxml:tag "Item2BType" ;
  rdfs:label "Item2BType"^^xsd:string ;
  rdfs:subClassOf iapd-sec-cr:FirmReport ;
  rdfs:subClassOf [
      rdf:type owl:Restriction ;
      sxml:isAttribute "true"^^xsd:boolean ;
      rdfs:comment "This node has Firm's response to Item to Part1A 2B(3)-act solely as an adviser to private funds but you are no longer eligible to check box 2.B.(2) because you have assets under management in the United States of $150 million or more (Y/N)."@en ;
      owl:allValuesFrom iapd-sec-cr:AnswerYNType ;
      owl:onProperty iapd-sec-cr:q2B3 ;
    ] ;
  rdfs:subClassOf [
      rdf:type owl:Restriction ;
      sxml:isAttribute "true"^^xsd:boolean ;
      rdfs:comment "This node has Firm's response to Part1A Item 2B(1)-qualify for the exemption from registration as an adviser solely to one or more venture capital funds (Y/N)."@en ;
      owl:allValuesFrom iapd-sec-cr:AnswerYNType ;
      owl:onProperty iapd-sec-cr:q2B1 ;
    ] ;
  rdfs:subClassOf [
      rdf:type owl:Restriction ;
      sxml:isAttribute "true"^^xsd:boolean ;
      rdfs:comment "This node has Firm's response to Part1A Item 2B(2)-qualify for the exemption from registration because you act solely as an adviser to private funds and have assets under management in the United States of less than $150 million (Y/N)."@en ;
      owl:allValuesFrom iapd-sec-cr:AnswerYNType ;
      owl:onProperty iapd-sec-cr:q2B2 ;
    ] ;
  rdfs:subClassOf [
      rdf:type owl:Restriction ;
      owl:maxCardinality "1"^^xsd:int ;
      owl:onProperty iapd-sec-cr:q2B1 ;
    ] ;
  rdfs:subClassOf [
      rdf:type owl:Restriction ;
      owl:maxCardinality "1"^^xsd:int ;
      owl:onProperty iapd-sec-cr:q2B2 ;
    ] ;
  rdfs:subClassOf [
      rdf:type owl:Restriction ;
      owl:maxCardinality "1"^^xsd:int ;
      owl:onProperty iapd-sec-cr:q2B3 ;
    ] ;
  skos:definition "Part 1A Item 2Bs holds Yes/No questions about the firm's potential exemption from registration. The questions are modeled as object properties with the range of AnswerYNType."^^xsd:string ;
.
iapd-sec-cr:Item3AType
  rdf:type owl:Class ;
  sxml:tag "Item3AType" ;
  rdfs:label "Item3AType"^^xsd:string ;
  rdfs:subClassOf iapd-sec-cr:FirmReport ;
  rdfs:subClassOf [
      rdf:type owl:Restriction ;
      sxml:isAttribute "true"^^xsd:boolean ;
      rdfs:comment "This node has Firm's response to Part1A Item 3A Other textbox-How are you organized Other (specify)."@en ;
      owl:allValuesFrom iapd-sec-cr:Str50Datatype ;
      owl:onProperty iapd-sec-cr:orgFormOthNm ;
    ] ;
  rdfs:subClassOf [
      rdf:type owl:Restriction ;
      sxml:isAttribute "true"^^xsd:boolean ;
      rdfs:comment "This node has Firm's response to Part1A Item 3A-How are you organized (Description)."@en ;
      owl:allValuesFrom iapd-sec-cr:Str128Datatype ;
      owl:onProperty iapd-sec-cr:orgFormNm ;
    ] ;
  rdfs:subClassOf [
      rdf:type owl:Restriction ;
      owl:cardinality "1"^^xsd:int ;
      owl:onProperty iapd-sec-cr:orgFormNm ;
    ] ;
  rdfs:subClassOf [
      rdf:type owl:Restriction ;
      owl:maxCardinality "1"^^xsd:int ;
      owl:onProperty iapd-sec-cr:orgFormOthNm ;
    ] ;
  skos:definition "Firm's response to Part1A Item 3A-How are you organized (Description). And Firm's response to other textbox-How are you organized Other (specify)."^^xsd:string ;
.
iapd-sec-cr:Item3BType
  rdf:type owl:Class ;
  sxml:tag "Item3BType" ;
  rdfs:label "Item3BType"^^xsd:string ;
  rdfs:subClassOf iapd-sec-cr:FirmReport ;
  rdfs:subClassOf [
      rdf:type owl:Restriction ;
      sxml:isAttribute "true"^^xsd:boolean ;
      rdfs:comment "This node has Firm's response to Part 1A Item 3B-In what month does your fiscal year end each year?."@en ;
      owl:allValuesFrom iapd-sec-cr:Str128Datatype ;
      owl:onProperty iapd-sec-cr:q3B ;
    ] ;
  rdfs:subClassOf [
      rdf:type owl:Restriction ;
      owl:maxCardinality "1"^^xsd:int ;
      owl:onProperty iapd-sec-cr:q3B ;
    ] ;
  skos:definition "Firm's response to Part 1A Item 3B-In what month does your fiscal year end each year?."^^xsd:string ;
.
iapd-sec-cr:Item3CType
  rdf:type owl:Class ;
  sxml:tag "Item3CType" ;
  rdfs:comment "The class has object properties relating to the SEC state codes and Country names."^^xsd:string ;
  rdfs:label "Item3CType"^^xsd:string ;
  rdfs:subClassOf iapd-sec-cr:FirmReport ;
  rdfs:subClassOf [
      rdf:type owl:Restriction ;
      sxml:isAttribute "true"^^xsd:boolean ;
      rdfs:comment "This node has Firm's response to Part1A Item 3C-Country Drop-down-Under the laws of what state or country are you organized."@en ;
      owl:allValuesFrom iapd-sec-cr:Str50Datatype ;
      owl:onProperty iapd-sec-cr:cntryNm ;
    ] ;
  rdfs:subClassOf [
      rdf:type owl:Restriction ;
      sxml:isAttribute "true"^^xsd:boolean ;
      rdfs:comment "This node has Firm's response to Part1A Item 3C-State Drop-down-Under the laws of what state or country are you organized (Code)."@en ;
      owl:allValuesFrom iapd-sec-cr:StateCdType ;
      owl:onProperty iapd-sec-cr:stateCD ;
    ] ;
  rdfs:subClassOf [
      rdf:type owl:Restriction ;
      owl:maxCardinality "1"^^xsd:int ;
      owl:onProperty iapd-sec-cr:cntryNm ;
    ] ;
  rdfs:subClassOf [
      rdf:type owl:Restriction ;
      owl:maxCardinality "1"^^xsd:int ;
      owl:onProperty iapd-sec-cr:stateCD ;
    ] ;
  skos:definition """Firm's response to Part1A Item 3C-State Drop-down-Under the laws of what state or country are you
organized (Code)."""^^xsd:string ;
.
iapd-sec-cr:Item5AType
  rdf:type owl:Class ;
  sxml:tag "Item5AType" ;
  rdfs:label "Item5AType"^^xsd:string ;
  rdfs:subClassOf iapd-sec-cr:FirmReport ;
  rdfs:subClassOf [
      rdf:type owl:Restriction ;
      sxml:isAttribute "true"^^xsd:boolean ;
      rdfs:comment "This node has Firm's response to Part1A Item 5A-Approximately how many employees do you have."@en ;
      owl:allValuesFrom iapd-sec-cr:Int10Datatype ;
      owl:onProperty iapd-sec-cr:ttlEmp ;
    ] ;
  rdfs:subClassOf [
      rdf:type owl:Restriction ;
      owl:maxCardinality "1"^^xsd:int ;
      owl:onProperty iapd-sec-cr:ttlEmp ;
    ] ;
  skos:definition "Firm's response to Part1A Item 5A-Approximately how many employees do you have."^^xsd:string ;
.
iapd-sec-cr:Item5BType
  rdf:type owl:Class ;
  sxml:tag "Item5BType" ;
  rdfs:comment "The responses are modeled as a xsd:integer (10)"^^xsd:string ;
  rdfs:label "Item5BType"^^xsd:string ;
  rdfs:subClassOf iapd-sec-cr:FirmReport ;
  rdfs:subClassOf [
      rdf:type owl:Restriction ;
      sxml:isAttribute "true"^^xsd:boolean ;
      rdfs:comment "This node has Firm's response to Part1A Item 5B(1)-Approximately how many of the employees reported in 5.A. perform investment advisory functions (including research)."@en ;
      owl:allValuesFrom iapd-sec-cr:Int10Datatype ;
      owl:onProperty iapd-sec-cr:q5B1 ;
    ] ;
  rdfs:subClassOf [
      rdf:type owl:Restriction ;
      sxml:isAttribute "true"^^xsd:boolean ;
      rdfs:comment "This node has Firm's response to Part1A Item 5B(2)-Approximately how many of the employees reported in 5.A. are registered representatives of a broker-dealer."@en ;
      owl:allValuesFrom iapd-sec-cr:Int10Datatype ;
      owl:onProperty iapd-sec-cr:q5B2 ;
    ] ;
  rdfs:subClassOf [
      rdf:type owl:Restriction ;
      sxml:isAttribute "true"^^xsd:boolean ;
      rdfs:comment "This node has Firm's response to Part1A Item 5B(3)-Approximately how many of the employees reported in 5.A. are registered with one or more state securities authorities as investment adviser representatives."@en ;
      owl:allValuesFrom iapd-sec-cr:Int10Datatype ;
      owl:onProperty iapd-sec-cr:q5B3 ;
    ] ;
  rdfs:subClassOf [
      rdf:type owl:Restriction ;
      sxml:isAttribute "true"^^xsd:boolean ;
      rdfs:comment "This node has Firm's response to Part1A Item 5B(4)-Approximately how many of the employees reported in 5.A. are registered with one or more state securities authorities as investment adviser representatives for an investment adviser other than you."@en ;
      owl:allValuesFrom iapd-sec-cr:Int10Datatype ;
      owl:onProperty iapd-sec-cr:q5B4 ;
    ] ;
  rdfs:subClassOf [
      rdf:type owl:Restriction ;
      sxml:isAttribute "true"^^xsd:boolean ;
      rdfs:comment "This node has Firm's response to Part1A Item 5B(5)-Approximately how many of the employees reported in 5.A. are licensed agents of an insurance company or agency."@en ;
      owl:allValuesFrom iapd-sec-cr:Int10Datatype ;
      owl:onProperty iapd-sec-cr:q5B5 ;
    ] ;
  rdfs:subClassOf [
      rdf:type owl:Restriction ;
      sxml:isAttribute "true"^^xsd:boolean ;
      rdfs:comment "This node has Firm's response to Part1A Item 5B(6)-Approximately how many firms or other persons solicit advisory clients on your behalf."@en ;
      owl:allValuesFrom iapd-sec-cr:Int10Datatype ;
      owl:onProperty iapd-sec-cr:q5B6 ;
    ] ;
  rdfs:subClassOf [
      rdf:type owl:Restriction ;
      owl:maxCardinality "1"^^xsd:int ;
      owl:onProperty iapd-sec-cr:q5B1 ;
    ] ;
  rdfs:subClassOf [
      rdf:type owl:Restriction ;
      owl:maxCardinality "1"^^xsd:int ;
      owl:onProperty iapd-sec-cr:q5B2 ;
    ] ;
  rdfs:subClassOf [
      rdf:type owl:Restriction ;
      owl:maxCardinality "1"^^xsd:int ;
      owl:onProperty iapd-sec-cr:q5B3 ;
    ] ;
  rdfs:subClassOf [
      rdf:type owl:Restriction ;
      owl:maxCardinality "1"^^xsd:int ;
      owl:onProperty iapd-sec-cr:q5B4 ;
    ] ;
  rdfs:subClassOf [
      rdf:type owl:Restriction ;
      owl:maxCardinality "1"^^xsd:int ;
      owl:onProperty iapd-sec-cr:q5B5 ;
    ] ;
  rdfs:subClassOf [
      rdf:type owl:Restriction ;
      owl:maxCardinality "1"^^xsd:int ;
      owl:onProperty iapd-sec-cr:q5B6 ;
    ] ;
  skos:definition """Firm's response to Part1A Item 5B:
(1) Approximately how many of the employees reported in 5A perform investment advisory functions (including research).
(2) Approximately how many of the employees reported in 5A are registered representatives of a broker-dealer.
(3) Approximately how many of the employees reported in 5A are registered with one or more state securities authorities as investment adviser representatives.
(4) Approximately how many of the employees reported in 5A are registered with one or more state securities authorities as investment adviser representatives for an investment adviser other than you.
(5) Approximately how many of the employees reported in 5.A. are licensed agents of an insurance company or agency.
(6) Approximately how many firms or other persons solicit advisory
clients on your behalf."""^^xsd:string ;
.
iapd-sec-cr:Item5CType
  rdf:type owl:Class ;
  sxml:tag "Item5CType" ;
  rdfs:comment "Response (1) has a string field and a free from text."^^xsd:string ;
  rdfs:label "Item5CType"^^xsd:string ;
  rdfs:subClassOf iapd-sec-cr:FirmReport ;
  rdfs:subClassOf [
      rdf:type owl:Restriction ;
      sxml:isAttribute "true"^^xsd:boolean ;
      rdfs:comment "This node has Firm's response to Part1A Item 5C(1)-If more than 100, how many (round to the nearest 100)."@en ;
      owl:allValuesFrom iapd-sec-cr:Int10Datatype ;
      owl:onProperty iapd-sec-cr:q5C1Oth ;
    ] ;
  rdfs:subClassOf [
      rdf:type owl:Restriction ;
      sxml:isAttribute "true"^^xsd:boolean ;
      rdfs:comment "This node has Firm's response to Part1A Item 5C(1)-To approximately how many clients did you provide investment advisory services during your most recently completed fiscal year."@en ;
      owl:allValuesFrom iapd-sec-cr:Str128Datatype ;
      owl:onProperty iapd-sec-cr:q5C1 ;
    ] ;
  rdfs:subClassOf [
      rdf:type owl:Restriction ;
      sxml:isAttribute "true"^^xsd:boolean ;
      rdfs:comment "This node has Firm's response to Part1A Item 5C(2)-Approximately what percentage of your clients are non-United States persons."@en ;
      owl:allValuesFrom iapd-sec-cr:Int3Datatype ;
      owl:onProperty iapd-sec-cr:q5C2 ;
    ] ;
  rdfs:subClassOf [
      rdf:type owl:Restriction ;
      owl:maxCardinality "1"^^xsd:int ;
      owl:onProperty iapd-sec-cr:q5C1 ;
    ] ;
  rdfs:subClassOf [
      rdf:type owl:Restriction ;
      owl:maxCardinality "1"^^xsd:int ;
      owl:onProperty iapd-sec-cr:q5C1Oth ;
    ] ;
  rdfs:subClassOf [
      rdf:type owl:Restriction ;
      owl:maxCardinality "1"^^xsd:int ;
      owl:onProperty iapd-sec-cr:q5C2 ;
    ] ;
  skos:definition """Firm's response to Part1A Item 5C
(1) To approximately how many clients did you provide investment advisory services during your most recently completed fiscal year. If more than 100, how many (round to the nearest 100).
(2) Approximately what percentage of your clients are non-United States persons."""^^xsd:string ;
.
iapd-sec-cr:Item5DType
  rdf:type owl:Class ;
  sxml:tag "Item5DType" ;
  rdfs:comment "The information is stored in xsd:string, but can be transformed into semantic of the brackets."^^xsd:string ;
  rdfs:label "Item5DType"^^xsd:string ;
  rdfs:subClassOf iapd-sec-cr:FirmReport ;
  rdfs:subClassOf [
      rdf:type owl:Restriction ;
      sxml:isAttribute "true"^^xsd:boolean ;
      rdfs:comment "This node has Firm's response to Part1A Item 5D(1)(a)-Individuals (other than high net worth individuals)."@en ;
      owl:allValuesFrom iapd-sec-cr:Str128Datatype ;
      owl:onProperty iapd-sec-cr:q5D1A ;
    ] ;
  rdfs:subClassOf [
      rdf:type owl:Restriction ;
      sxml:isAttribute "true"^^xsd:boolean ;
      rdfs:comment "This node has Firm's response to Part1A Item 5D(1)(b)-High net worth individuals."@en ;
      owl:allValuesFrom iapd-sec-cr:Str128Datatype ;
      owl:onProperty iapd-sec-cr:q5D1B ;
    ] ;
  rdfs:subClassOf [
      rdf:type owl:Restriction ;
      sxml:isAttribute "true"^^xsd:boolean ;
      rdfs:comment "This node has Firm's response to Part1A Item 5D(1)(c)-Banking or thrift institutions."@en ;
      owl:allValuesFrom iapd-sec-cr:Str128Datatype ;
      owl:onProperty iapd-sec-cr:q5D1C ;
    ] ;
  rdfs:subClassOf [
      rdf:type owl:Restriction ;
      sxml:isAttribute "true"^^xsd:boolean ;
      rdfs:comment "This node has Firm's response to Part1A Item 5D(1)(d)-Investment companies ."@en ;
      owl:allValuesFrom iapd-sec-cr:Str128Datatype ;
      owl:onProperty iapd-sec-cr:q5D1D ;
    ] ;
  rdfs:subClassOf [
      rdf:type owl:Restriction ;
      sxml:isAttribute "true"^^xsd:boolean ;
      rdfs:comment "This node has Firm's response to Part1A Item 5D(1)(e)-Business development companies."@en ;
      owl:allValuesFrom iapd-sec-cr:Str128Datatype ;
      owl:onProperty iapd-sec-cr:q5D1E ;
    ] ;
  rdfs:subClassOf [
      rdf:type owl:Restriction ;
      sxml:isAttribute "true"^^xsd:boolean ;
      rdfs:comment "This node has Firm's response to Part1A Item 5D(1)(f)-Pooled investment vehicles (other than investment companies)."@en ;
      owl:allValuesFrom iapd-sec-cr:Str128Datatype ;
      owl:onProperty iapd-sec-cr:q5D1F ;
    ] ;
  rdfs:subClassOf [
      rdf:type owl:Restriction ;
      sxml:isAttribute "true"^^xsd:boolean ;
      rdfs:comment "This node has Firm's response to Part1A Item 5D(1)(g)-Pension and profit sharing plans (but not the plan participants)."@en ;
      owl:allValuesFrom iapd-sec-cr:Str128Datatype ;
      owl:onProperty iapd-sec-cr:q5D1G ;
    ] ;
  rdfs:subClassOf [
      rdf:type owl:Restriction ;
      sxml:isAttribute "true"^^xsd:boolean ;
      rdfs:comment "This node has Firm's response to Part1A Item 5D(1)(h)-Charitable organizations."@en ;
      owl:allValuesFrom iapd-sec-cr:Str128Datatype ;
      owl:onProperty iapd-sec-cr:q5D1H ;
    ] ;
  rdfs:subClassOf [
      rdf:type owl:Restriction ;
      sxml:isAttribute "true"^^xsd:boolean ;
      rdfs:comment "This node has Firm's response to Part1A Item 5D(1)(i)-Corporations or other businesses not listed above."@en ;
      owl:allValuesFrom iapd-sec-cr:Str128Datatype ;
      owl:onProperty iapd-sec-cr:q5D1I ;
    ] ;
  rdfs:subClassOf [
      rdf:type owl:Restriction ;
      sxml:isAttribute "true"^^xsd:boolean ;
      rdfs:comment "This node has Firm's response to Part1A Item 5D(1)(j)-State or municipal government entities."@en ;
      owl:allValuesFrom iapd-sec-cr:Str128Datatype ;
      owl:onProperty iapd-sec-cr:q5D1J ;
    ] ;
  rdfs:subClassOf [
      rdf:type owl:Restriction ;
      sxml:isAttribute "true"^^xsd:boolean ;
      rdfs:comment "This node has Firm's response to Part1A Item 5D(1)(k)-Other investment advisers."@en ;
      owl:allValuesFrom iapd-sec-cr:Str128Datatype ;
      owl:onProperty iapd-sec-cr:q5D1K ;
    ] ;
  rdfs:subClassOf [
      rdf:type owl:Restriction ;
      sxml:isAttribute "true"^^xsd:boolean ;
      rdfs:comment "This node has Firm's response to Part1A Item 5D(1)(l)-Insurance companies."@en ;
      owl:allValuesFrom iapd-sec-cr:Str128Datatype ;
      owl:onProperty iapd-sec-cr:q5D1L ;
    ] ;
  rdfs:subClassOf [
      rdf:type owl:Restriction ;
      sxml:isAttribute "true"^^xsd:boolean ;
      rdfs:comment "This node has Firm's response to Part1A Item 5D(1)(m)-Other textbox."@en ;
      owl:allValuesFrom iapd-sec-cr:Str128Datatype ;
      owl:onProperty iapd-sec-cr:q5D1MOth ;
    ] ;
  rdfs:subClassOf [
      rdf:type owl:Restriction ;
      sxml:isAttribute "true"^^xsd:boolean ;
      rdfs:comment "This node has Firm's response to Part1A Item 5D(1)(m)-Other."@en ;
      owl:allValuesFrom iapd-sec-cr:Str128Datatype ;
      owl:onProperty iapd-sec-cr:q5D1M ;
    ] ;
  rdfs:subClassOf [
      rdf:type owl:Restriction ;
      sxml:isAttribute "true"^^xsd:boolean ;
      rdfs:comment "This node has Firm's response to Part1A Item 5D(2)(a)-Individuals (other than high net worth individuals)."@en ;
      owl:allValuesFrom iapd-sec-cr:Str128Datatype ;
      owl:onProperty iapd-sec-cr:q5D2A ;
    ] ;
  rdfs:subClassOf [
      rdf:type owl:Restriction ;
      sxml:isAttribute "true"^^xsd:boolean ;
      rdfs:comment "This node has Firm's response to Part1A Item 5D(2)(b)-High net worth individuals."@en ;
      owl:allValuesFrom iapd-sec-cr:Str128Datatype ;
      owl:onProperty iapd-sec-cr:q5D2B ;
    ] ;
  rdfs:subClassOf [
      rdf:type owl:Restriction ;
      sxml:isAttribute "true"^^xsd:boolean ;
      rdfs:comment "This node has Firm's response to Part1A Item 5D(2)(c)-Banking or thrift institutions."@en ;
      owl:allValuesFrom iapd-sec-cr:Str128Datatype ;
      owl:onProperty iapd-sec-cr:q5D2C ;
    ] ;
  rdfs:subClassOf [
      rdf:type owl:Restriction ;
      sxml:isAttribute "true"^^xsd:boolean ;
      rdfs:comment "This node has Firm's response to Part1A Item 5D(2)(d)-Investment companies."@en ;
      owl:allValuesFrom iapd-sec-cr:Str128Datatype ;
      owl:onProperty iapd-sec-cr:q5D2D ;
    ] ;
  rdfs:subClassOf [
      rdf:type owl:Restriction ;
      sxml:isAttribute "true"^^xsd:boolean ;
      rdfs:comment "This node has Firm's response to Part1A Item 5D(2)(e)-Business development companies."@en ;
      owl:allValuesFrom iapd-sec-cr:Str128Datatype ;
      owl:onProperty iapd-sec-cr:q5D2E ;
    ] ;
  rdfs:subClassOf [
      rdf:type owl:Restriction ;
      sxml:isAttribute "true"^^xsd:boolean ;
      rdfs:comment "This node has Firm's response to Part1A Item 5D(2)(f)-Pooled investment vehicles (other than investment companies)."@en ;
      owl:allValuesFrom iapd-sec-cr:Str128Datatype ;
      owl:onProperty iapd-sec-cr:q5D2F ;
    ] ;
  rdfs:subClassOf [
      rdf:type owl:Restriction ;
      sxml:isAttribute "true"^^xsd:boolean ;
      rdfs:comment "This node has Firm's response to Part1A Item 5D(2)(g)-Pension and profit sharing plans (but not the plan participants)."@en ;
      owl:allValuesFrom iapd-sec-cr:Str128Datatype ;
      owl:onProperty iapd-sec-cr:q5D2G ;
    ] ;
  rdfs:subClassOf [
      rdf:type owl:Restriction ;
      sxml:isAttribute "true"^^xsd:boolean ;
      rdfs:comment "This node has Firm's response to Part1A Item 5D(2)(h)-Charitable organizations."@en ;
      owl:allValuesFrom iapd-sec-cr:Str128Datatype ;
      owl:onProperty iapd-sec-cr:q5D2H ;
    ] ;
  rdfs:subClassOf [
      rdf:type owl:Restriction ;
      sxml:isAttribute "true"^^xsd:boolean ;
      rdfs:comment "This node has Firm's response to Part1A Item 5D(2)(i)-Corporations or other businesses not listed above."@en ;
      owl:allValuesFrom iapd-sec-cr:Str128Datatype ;
      owl:onProperty iapd-sec-cr:q5D2I ;
    ] ;
  rdfs:subClassOf [
      rdf:type owl:Restriction ;
      sxml:isAttribute "true"^^xsd:boolean ;
      rdfs:comment "This node has Firm's response to Part1A Item 5D(2)(j)-State or municipal government entities."@en ;
      owl:allValuesFrom iapd-sec-cr:Str128Datatype ;
      owl:onProperty iapd-sec-cr:q5D2J ;
    ] ;
  rdfs:subClassOf [
      rdf:type owl:Restriction ;
      sxml:isAttribute "true"^^xsd:boolean ;
      rdfs:comment "This node has Firm's response to Part1A Item 5D(2)(k)-Other investment advisers."@en ;
      owl:allValuesFrom iapd-sec-cr:Str128Datatype ;
      owl:onProperty iapd-sec-cr:q5D2K ;
    ] ;
  rdfs:subClassOf [
      rdf:type owl:Restriction ;
      sxml:isAttribute "true"^^xsd:boolean ;
      rdfs:comment "This node has Firm's response to Part1A Item 5D(2)(l)-Insurance companies."@en ;
      owl:allValuesFrom iapd-sec-cr:Str128Datatype ;
      owl:onProperty iapd-sec-cr:q5D2L ;
    ] ;
  rdfs:subClassOf [
      rdf:type owl:Restriction ;
      sxml:isAttribute "true"^^xsd:boolean ;
      rdfs:comment "This node has Firm's response to Part1A Item 5D(2)(m)-Other textbox."@en ;
      owl:allValuesFrom iapd-sec-cr:Str128Datatype ;
      owl:onProperty iapd-sec-cr:q5D2MOth ;
    ] ;
  rdfs:subClassOf [
      rdf:type owl:Restriction ;
      sxml:isAttribute "true"^^xsd:boolean ;
      rdfs:comment "This node has Firm's response to Part1A Item 5D(2)(m)-Other."@en ;
      owl:allValuesFrom iapd-sec-cr:Str128Datatype ;
      owl:onProperty iapd-sec-cr:q5D2M ;
    ] ;
  rdfs:subClassOf [
      rdf:type owl:Restriction ;
      owl:maxCardinality "1"^^xsd:int ;
      owl:onProperty iapd-sec-cr:q5D1A ;
    ] ;
  rdfs:subClassOf [
      rdf:type owl:Restriction ;
      owl:maxCardinality "1"^^xsd:int ;
      owl:onProperty iapd-sec-cr:q5D1B ;
    ] ;
  rdfs:subClassOf [
      rdf:type owl:Restriction ;
      owl:maxCardinality "1"^^xsd:int ;
      owl:onProperty iapd-sec-cr:q5D1C ;
    ] ;
  rdfs:subClassOf [
      rdf:type owl:Restriction ;
      owl:maxCardinality "1"^^xsd:int ;
      owl:onProperty iapd-sec-cr:q5D1D ;
    ] ;
  rdfs:subClassOf [
      rdf:type owl:Restriction ;
      owl:maxCardinality "1"^^xsd:int ;
      owl:onProperty iapd-sec-cr:q5D1E ;
    ] ;
  rdfs:subClassOf [
      rdf:type owl:Restriction ;
      owl:maxCardinality "1"^^xsd:int ;
      owl:onProperty iapd-sec-cr:q5D1F ;
    ] ;
  rdfs:subClassOf [
      rdf:type owl:Restriction ;
      owl:maxCardinality "1"^^xsd:int ;
      owl:onProperty iapd-sec-cr:q5D1G ;
    ] ;
  rdfs:subClassOf [
      rdf:type owl:Restriction ;
      owl:maxCardinality "1"^^xsd:int ;
      owl:onProperty iapd-sec-cr:q5D1H ;
    ] ;
  rdfs:subClassOf [
      rdf:type owl:Restriction ;
      owl:maxCardinality "1"^^xsd:int ;
      owl:onProperty iapd-sec-cr:q5D1I ;
    ] ;
  rdfs:subClassOf [
      rdf:type owl:Restriction ;
      owl:maxCardinality "1"^^xsd:int ;
      owl:onProperty iapd-sec-cr:q5D1J ;
    ] ;
  rdfs:subClassOf [
      rdf:type owl:Restriction ;
      owl:maxCardinality "1"^^xsd:int ;
      owl:onProperty iapd-sec-cr:q5D1K ;
    ] ;
  rdfs:subClassOf [
      rdf:type owl:Restriction ;
      owl:maxCardinality "1"^^xsd:int ;
      owl:onProperty iapd-sec-cr:q5D1L ;
    ] ;
  rdfs:subClassOf [
      rdf:type owl:Restriction ;
      owl:maxCardinality "1"^^xsd:int ;
      owl:onProperty iapd-sec-cr:q5D1M ;
    ] ;
  rdfs:subClassOf [
      rdf:type owl:Restriction ;
      owl:maxCardinality "1"^^xsd:int ;
      owl:onProperty iapd-sec-cr:q5D1MOth ;
    ] ;
  rdfs:subClassOf [
      rdf:type owl:Restriction ;
      owl:maxCardinality "1"^^xsd:int ;
      owl:onProperty iapd-sec-cr:q5D2A ;
    ] ;
  rdfs:subClassOf [
      rdf:type owl:Restriction ;
      owl:maxCardinality "1"^^xsd:int ;
      owl:onProperty iapd-sec-cr:q5D2B ;
    ] ;
  rdfs:subClassOf [
      rdf:type owl:Restriction ;
      owl:maxCardinality "1"^^xsd:int ;
      owl:onProperty iapd-sec-cr:q5D2C ;
    ] ;
  rdfs:subClassOf [
      rdf:type owl:Restriction ;
      owl:maxCardinality "1"^^xsd:int ;
      owl:onProperty iapd-sec-cr:q5D2D ;
    ] ;
  rdfs:subClassOf [
      rdf:type owl:Restriction ;
      owl:maxCardinality "1"^^xsd:int ;
      owl:onProperty iapd-sec-cr:q5D2E ;
    ] ;
  rdfs:subClassOf [
      rdf:type owl:Restriction ;
      owl:maxCardinality "1"^^xsd:int ;
      owl:onProperty iapd-sec-cr:q5D2F ;
    ] ;
  rdfs:subClassOf [
      rdf:type owl:Restriction ;
      owl:maxCardinality "1"^^xsd:int ;
      owl:onProperty iapd-sec-cr:q5D2G ;
    ] ;
  rdfs:subClassOf [
      rdf:type owl:Restriction ;
      owl:maxCardinality "1"^^xsd:int ;
      owl:onProperty iapd-sec-cr:q5D2H ;
    ] ;
  rdfs:subClassOf [
      rdf:type owl:Restriction ;
      owl:maxCardinality "1"^^xsd:int ;
      owl:onProperty iapd-sec-cr:q5D2I ;
    ] ;
  rdfs:subClassOf [
      rdf:type owl:Restriction ;
      owl:maxCardinality "1"^^xsd:int ;
      owl:onProperty iapd-sec-cr:q5D2J ;
    ] ;
  rdfs:subClassOf [
      rdf:type owl:Restriction ;
      owl:maxCardinality "1"^^xsd:int ;
      owl:onProperty iapd-sec-cr:q5D2K ;
    ] ;
  rdfs:subClassOf [
      rdf:type owl:Restriction ;
      owl:maxCardinality "1"^^xsd:int ;
      owl:onProperty iapd-sec-cr:q5D2L ;
    ] ;
  rdfs:subClassOf [
      rdf:type owl:Restriction ;
      owl:maxCardinality "1"^^xsd:int ;
      owl:onProperty iapd-sec-cr:q5D2M ;
    ] ;
  rdfs:subClassOf [
      rdf:type owl:Restriction ;
      owl:maxCardinality "1"^^xsd:int ;
      owl:onProperty iapd-sec-cr:q5D2MOth ;
    ] ;
  skos:definition """Firm's response to Part1A Item 5D about the firms clients.
The number of clients in brackets Up to 25%, Up to 50%, Up to 75%, >75%
(1)(a)-Individuals (other than high net worth individuals).
(1)(b)-High net worth individuals.
(1)(c)-Banking or thrift institutions.
(1)(d)-Investment companies
(1)(e)-Business development companies.
(1)(f)-Pooled investment vehicles (other than investment companies).
(1)(g)-Pension and profit sharing plans (but not the plan participants).
(1)(h)-Charitable organizations.
(1)(i)-Corporations or other businesses not listed above.
(1)(j)-State or municipal government entities.
(1)(k)-Other investment advisers.
(1)(l)-Insurance companies.
(1)(m)-Other.

The share of AUM in brackets Up to 25%, Up to 50%, Up to 75%, >75%
(2)(a)-Individuals (other than high net worth individuals).
(2)(b)-High net worth individuals.
(2)(c)-Banking or thrift institutions.
(2)(d)-Investment companies.
(2)(e)-Business development companies.
(2)(f)-Pooled investment vehicles (other than investment companies).
(2)(g)-Pension and profit sharing plans (but not the plan participants).
(2)(h)-Charitable organizations.
(2)(i)-Corporations or other businesses not listed above.
(2)(j)-State or municipal government entities.
(2)(k)-Other investment advisers.
(2)(l)-Insurance companies.
(2)(m)-Other."""^^xsd:string ;
.
iapd-sec-cr:Item5EType
  rdf:type owl:Class ;
  sxml:tag "Item5EType" ;
  rdfs:comment "The answers are Yes/No fields. Fundontology transforms this into object properties to classification codes that apply. (see FR_IA_Firm.ttl)"^^xsd:string ;
  rdfs:label "Item5EType"^^xsd:string ;
  rdfs:subClassOf iapd-sec-cr:FirmReport ;
  rdfs:subClassOf [
      rdf:type owl:Restriction ;
      sxml:isAttribute "true"^^xsd:boolean ;
      rdfs:comment "This node has Firm's response to Part1A Item 5E(1)-A percentage of assets under your management (Y/N) Display a 'Y' when the checkbox is selected. Display an 'N' when the checkbox is not selected."@en ;
      owl:allValuesFrom iapd-sec-cr:AnswerYNType ;
      owl:onProperty iapd-sec-cr:q5E1 ;
    ] ;
  rdfs:subClassOf [
      rdf:type owl:Restriction ;
      sxml:isAttribute "true"^^xsd:boolean ;
      rdfs:comment "This node has Firm's response to Part1A Item 5E(2)-Hourly charges (Y/N) Display a 'Y' when the checkbox is selected. Display an 'N' when the checkbox is not selected."@en ;
      owl:allValuesFrom iapd-sec-cr:AnswerYNType ;
      owl:onProperty iapd-sec-cr:q5E2 ;
    ] ;
  rdfs:subClassOf [
      rdf:type owl:Restriction ;
      sxml:isAttribute "true"^^xsd:boolean ;
      rdfs:comment "This node has Firm's response to Part1A Item 5E(3)-Subscription fees (for a newsletter or periodical) (Y/N) Display a 'Y' when the checkbox is selected. Display an 'N' when the checkbox is not selected."@en ;
      owl:allValuesFrom iapd-sec-cr:AnswerYNType ;
      owl:onProperty iapd-sec-cr:q5E3 ;
    ] ;
  rdfs:subClassOf [
      rdf:type owl:Restriction ;
      sxml:isAttribute "true"^^xsd:boolean ;
      rdfs:comment "This node has Firm's response to Part1A Item 5E(4)-Fixed fees (other than subscription fees) (Y/N) Display a 'Y' when the checkbox is selected. Display an 'N' when the checkbox is not selected."@en ;
      owl:allValuesFrom iapd-sec-cr:AnswerYNType ;
      owl:onProperty iapd-sec-cr:q5E4 ;
    ] ;
  rdfs:subClassOf [
      rdf:type owl:Restriction ;
      sxml:isAttribute "true"^^xsd:boolean ;
      rdfs:comment "This node has Firm's response to Part1A Item 5E(5)-Commissions (Y/N) Display a 'Y' when the checkbox is selected. Display an 'N' when the checkbox is not selected."@en ;
      owl:allValuesFrom iapd-sec-cr:AnswerYNType ;
      owl:onProperty iapd-sec-cr:q5E5 ;
    ] ;
  rdfs:subClassOf [
      rdf:type owl:Restriction ;
      sxml:isAttribute "true"^^xsd:boolean ;
      rdfs:comment "This node has Firm's response to Part1A Item 5E(6)-Performance-based fees (Y/N) Display a 'Y' when the checkbox is selected. Display an 'N' when the checkbox is not selected."@en ;
      owl:allValuesFrom iapd-sec-cr:AnswerYNType ;
      owl:onProperty iapd-sec-cr:q5E6 ;
    ] ;
  rdfs:subClassOf [
      rdf:type owl:Restriction ;
      sxml:isAttribute "true"^^xsd:boolean ;
      rdfs:comment "This node has Firm's response to Part1A Item 5E(7)-Other (Y/N) Display a 'Y' when the checkbox is selected. Display an 'N' when the checkbox is not selected."@en ;
      owl:allValuesFrom iapd-sec-cr:AnswerYNType ;
      owl:onProperty iapd-sec-cr:q5E7 ;
    ] ;
  rdfs:subClassOf [
      rdf:type owl:Restriction ;
      sxml:isAttribute "true"^^xsd:boolean ;
      rdfs:comment "This node has Firm's response to Part1A Item 5E(7)-Other (specify)."@en ;
      owl:allValuesFrom iapd-sec-cr:Str64Datatype ;
      owl:onProperty iapd-sec-cr:q5E7Oth ;
    ] ;
  rdfs:subClassOf [
      rdf:type owl:Restriction ;
      owl:maxCardinality "1"^^xsd:int ;
      owl:onProperty iapd-sec-cr:q5E1 ;
    ] ;
  rdfs:subClassOf [
      rdf:type owl:Restriction ;
      owl:maxCardinality "1"^^xsd:int ;
      owl:onProperty iapd-sec-cr:q5E2 ;
    ] ;
  rdfs:subClassOf [
      rdf:type owl:Restriction ;
      owl:maxCardinality "1"^^xsd:int ;
      owl:onProperty iapd-sec-cr:q5E3 ;
    ] ;
  rdfs:subClassOf [
      rdf:type owl:Restriction ;
      owl:maxCardinality "1"^^xsd:int ;
      owl:onProperty iapd-sec-cr:q5E4 ;
    ] ;
  rdfs:subClassOf [
      rdf:type owl:Restriction ;
      owl:maxCardinality "1"^^xsd:int ;
      owl:onProperty iapd-sec-cr:q5E5 ;
    ] ;
  rdfs:subClassOf [
      rdf:type owl:Restriction ;
      owl:maxCardinality "1"^^xsd:int ;
      owl:onProperty iapd-sec-cr:q5E6 ;
    ] ;
  rdfs:subClassOf [
      rdf:type owl:Restriction ;
      owl:maxCardinality "1"^^xsd:int ;
      owl:onProperty iapd-sec-cr:q5E7 ;
    ] ;
  rdfs:subClassOf [
      rdf:type owl:Restriction ;
      owl:maxCardinality "1"^^xsd:int ;
      owl:onProperty iapd-sec-cr:q5E7Oth ;
    ] ;
.
iapd-sec-cr:Item5FType
  rdf:type owl:Class ;
  sxml:tag "Item5FType" ;
  rdfs:comment "The answers are stored as object properties to interger (10) for the number and decimal (17,2) for amounts."^^xsd:string ;
  rdfs:label "Item5FType"^^xsd:string ;
  rdfs:subClassOf iapd-sec-cr:FirmReport ;
  rdfs:subClassOf [
      rdf:type owl:Restriction ;
      sxml:isAttribute "true"^^xsd:boolean ;
      rdfs:comment "This node has Firm's response to Part1A Item 5F(1)-Do you provide continuous and regular supervisory or management services to securities portfolios (Y/N/null)."@en ;
      owl:allValuesFrom iapd-sec-cr:AnswerYNType ;
      owl:onProperty iapd-sec-cr:q5F1 ;
    ] ;
  rdfs:subClassOf [
      rdf:type owl:Restriction ;
      sxml:isAttribute "true"^^xsd:boolean ;
      rdfs:comment "This node has Firm's response to Part1A Item 5F2a-Discretionary U.S. Dollar Amount."@en ;
      owl:allValuesFrom iapd-sec-cr:Decimal17P2Datatype ;
      owl:onProperty iapd-sec-cr:q5F2A ;
    ] ;
  rdfs:subClassOf [
      rdf:type owl:Restriction ;
      sxml:isAttribute "true"^^xsd:boolean ;
      rdfs:comment "This node has Firm's response to Part1A Item 5F2b-Non-Discretionary U. S. Dollar Amount."@en ;
      owl:allValuesFrom iapd-sec-cr:Decimal17P2Datatype ;
      owl:onProperty iapd-sec-cr:q5F2B ;
    ] ;
  rdfs:subClassOf [
      rdf:type owl:Restriction ;
      sxml:isAttribute "true"^^xsd:boolean ;
      rdfs:comment "This node has Firm's response to Part1A Item 5F2c-Total U.S. Dollar Amount."@en ;
      owl:allValuesFrom iapd-sec-cr:Decimal17P2Datatype ;
      owl:onProperty iapd-sec-cr:q5F2C ;
    ] ;
  rdfs:subClassOf [
      rdf:type owl:Restriction ;
      sxml:isAttribute "true"^^xsd:boolean ;
      rdfs:comment "This node has Firm's response to Part1A Item 5F2d-Discretionary Total Number of Accounts."@en ;
      owl:allValuesFrom iapd-sec-cr:Int10Datatype ;
      owl:onProperty iapd-sec-cr:q5F2D ;
    ] ;
  rdfs:subClassOf [
      rdf:type owl:Restriction ;
      sxml:isAttribute "true"^^xsd:boolean ;
      rdfs:comment "This node has Firm's response to Part1A Item 5F2e-Non-Discretionary Total Number of Accounts."@en ;
      owl:allValuesFrom iapd-sec-cr:Int10Datatype ;
      owl:onProperty iapd-sec-cr:q5F2E ;
    ] ;
  rdfs:subClassOf [
      rdf:type owl:Restriction ;
      sxml:isAttribute "true"^^xsd:boolean ;
      rdfs:comment "This node has Firm's response to Part1A Item 5F2f-Total Number of Accounts."@en ;
      owl:allValuesFrom iapd-sec-cr:Int10Datatype ;
      owl:onProperty iapd-sec-cr:q5F2F ;
    ] ;
  rdfs:subClassOf [
      rdf:type owl:Restriction ;
      owl:maxCardinality "1"^^xsd:int ;
      owl:onProperty iapd-sec-cr:q5F1 ;
    ] ;
  rdfs:subClassOf [
      rdf:type owl:Restriction ;
      owl:maxCardinality "1"^^xsd:int ;
      owl:onProperty iapd-sec-cr:q5F2A ;
    ] ;
  rdfs:subClassOf [
      rdf:type owl:Restriction ;
      owl:maxCardinality "1"^^xsd:int ;
      owl:onProperty iapd-sec-cr:q5F2B ;
    ] ;
  rdfs:subClassOf [
      rdf:type owl:Restriction ;
      owl:maxCardinality "1"^^xsd:int ;
      owl:onProperty iapd-sec-cr:q5F2C ;
    ] ;
  rdfs:subClassOf [
      rdf:type owl:Restriction ;
      owl:maxCardinality "1"^^xsd:int ;
      owl:onProperty iapd-sec-cr:q5F2D ;
    ] ;
  rdfs:subClassOf [
      rdf:type owl:Restriction ;
      owl:maxCardinality "1"^^xsd:int ;
      owl:onProperty iapd-sec-cr:q5F2E ;
    ] ;
  rdfs:subClassOf [
      rdf:type owl:Restriction ;
      owl:maxCardinality "1"^^xsd:int ;
      owl:onProperty iapd-sec-cr:q5F2F ;
    ] ;
  skos:definition """Firm's response to Part1A Item 5F(1)-Do you provide continuous and regular supervisory or management
services to securities portfolios (Y/N/null).
Discretionnary, Non-Discretionary and Total with USD amount and total number of accounts."""^^xsd:string ;
.
iapd-sec-cr:Item5GType
  rdf:type owl:Class ;
  sxml:tag "Item5GType" ;
  rdfs:comment "The answers are object properties to the anwerYNType class. Fundontology transforms this into object properties to classification codes that apply. (see FR_IA_Firm.ttl)"^^xsd:string ;
  rdfs:label "Item5GType"^^xsd:string ;
  rdfs:subClassOf iapd-sec-cr:FirmReport ;
  rdfs:subClassOf [
      rdf:type owl:Restriction ;
      sxml:isAttribute "true"^^xsd:boolean ;
      rdfs:comment "This node has Firm's response to Part1A Item 5G(1)-Financial planning services (Y/N) Display a 'Y' when the checkbox is selected. Display an 'N' when the checkbox is not selected."@en ;
      owl:allValuesFrom iapd-sec-cr:AnswerYNType ;
      owl:onProperty iapd-sec-cr:q5G1 ;
    ] ;
  rdfs:subClassOf [
      rdf:type owl:Restriction ;
      sxml:isAttribute "true"^^xsd:boolean ;
      rdfs:comment "This node has Firm's response to Part1A Item 5G(10)-Market timing services (Y/N) Display a 'Y' when the checkbox is selected. Display an 'N' when the checkbox is not selected."@en ;
      owl:allValuesFrom iapd-sec-cr:AnswerYNType ;
      owl:onProperty iapd-sec-cr:q5G10 ;
    ] ;
  rdfs:subClassOf [
      rdf:type owl:Restriction ;
      sxml:isAttribute "true"^^xsd:boolean ;
      rdfs:comment "This node has Firm's response to Part1A Item 5G(11)-Educational seminars/workshops (Y/N) Display a 'Y' when the checkbox is selected. Display an 'N' when the checkbox is not selected."@en ;
      owl:allValuesFrom iapd-sec-cr:AnswerYNType ;
      owl:onProperty iapd-sec-cr:q5G11 ;
    ] ;
  rdfs:subClassOf [
      rdf:type owl:Restriction ;
      sxml:isAttribute "true"^^xsd:boolean ;
      rdfs:comment "This node has Firm's response to Part1A Item 5G(12) Other (specify)."@en ;
      owl:allValuesFrom iapd-sec-cr:Str128Datatype ;
      owl:onProperty iapd-sec-cr:q5G12Oth ;
    ] ;
  rdfs:subClassOf [
      rdf:type owl:Restriction ;
      sxml:isAttribute "true"^^xsd:boolean ;
      rdfs:comment "This node has Firm's response to Part1A Item 5G(12)-Other (Y/N) Display a 'Y' when the checkbox is selected. Display an 'N' when the checkbox is not selected."@en ;
      owl:allValuesFrom iapd-sec-cr:AnswerYNType ;
      owl:onProperty iapd-sec-cr:q5G12 ;
    ] ;
  rdfs:subClassOf [
      rdf:type owl:Restriction ;
      sxml:isAttribute "true"^^xsd:boolean ;
      rdfs:comment "This node has Firm's response to Part1A Item 5G(2)-Portfolio management for individuals and/or small businesses (Y/N) Display a 'Y' when the checkbox is selected. Display an 'N' when the checkbox is not selected."@en ;
      owl:allValuesFrom iapd-sec-cr:AnswerYNType ;
      owl:onProperty iapd-sec-cr:q5G2 ;
    ] ;
  rdfs:subClassOf [
      rdf:type owl:Restriction ;
      sxml:isAttribute "true"^^xsd:boolean ;
      rdfs:comment "This node has Firm's response to Part1A Item 5G(3)-Portfolio management for investment companies (Y/N) Display a 'Y' when the checkbox is selected. Display an 'N' when the checkbox is not selected."@en ;
      owl:allValuesFrom iapd-sec-cr:AnswerYNType ;
      owl:onProperty iapd-sec-cr:q5G3 ;
    ] ;
  rdfs:subClassOf [
      rdf:type owl:Restriction ;
      sxml:isAttribute "true"^^xsd:boolean ;
      rdfs:comment "This node has Firm's response to Part1A Item 5G(4)-Portfolio management for pooled investment vehicles (other than investment companies) (Y/N) Display a 'Y' when the checkbox is selected. Display an 'N' when the checkbox is not selected."@en ;
      owl:allValuesFrom iapd-sec-cr:AnswerYNType ;
      owl:onProperty iapd-sec-cr:q5G4 ;
    ] ;
  rdfs:subClassOf [
      rdf:type owl:Restriction ;
      sxml:isAttribute "true"^^xsd:boolean ;
      rdfs:comment "This node has Firm's response to Part1A Item 5G(5)-Portfolio management for businesses (other than small businesses) or institutional clients (other than registered investment companies and other pooled investment vehicles and) (Y/N) Display a 'Y' when the checkbox is selected. Display an 'N' when the checkbox is not selected."@en ;
      owl:allValuesFrom iapd-sec-cr:AnswerYNType ;
      owl:onProperty iapd-sec-cr:q5G5 ;
    ] ;
  rdfs:subClassOf [
      rdf:type owl:Restriction ;
      sxml:isAttribute "true"^^xsd:boolean ;
      rdfs:comment "This node has Firm's response to Part1A Item 5G(6)-Pension consulting services (Y/N) Display a 'Y' when the checkbox is selected. Display an 'N' when the checkbox is not selected."@en ;
      owl:allValuesFrom iapd-sec-cr:AnswerYNType ;
      owl:onProperty iapd-sec-cr:q5G6 ;
    ] ;
  rdfs:subClassOf [
      rdf:type owl:Restriction ;
      sxml:isAttribute "true"^^xsd:boolean ;
      rdfs:comment "This node has Firm's response to Part1A Item 5G(7)-Selection of other advisers (Y/N) Display a 'Y' when the checkbox is selected. Display an 'N' when the checkbox is not selected."@en ;
      owl:allValuesFrom iapd-sec-cr:AnswerYNType ;
      owl:onProperty iapd-sec-cr:q5G7 ;
    ] ;
  rdfs:subClassOf [
      rdf:type owl:Restriction ;
      sxml:isAttribute "true"^^xsd:boolean ;
      rdfs:comment "This node has Firm's response to Part1A Item 5G(8)-Publication of periodicals or newsletters (Y/N) Display a 'Y' when the checkbox is selected. Display an 'N' when the checkbox is not selected."@en ;
      owl:allValuesFrom iapd-sec-cr:AnswerYNType ;
      owl:onProperty iapd-sec-cr:q5G8 ;
    ] ;
  rdfs:subClassOf [
      rdf:type owl:Restriction ;
      sxml:isAttribute "true"^^xsd:boolean ;
      rdfs:comment "This node has Firm's response to Part1A Item 5G(9)-Security ratings or pricing services (Y/N) Display a 'Y' when the checkbox is selected. Display an 'N' when the checkbox is not selected."@en ;
      owl:allValuesFrom iapd-sec-cr:AnswerYNType ;
      owl:onProperty iapd-sec-cr:q5G9 ;
    ] ;
  rdfs:subClassOf [
      rdf:type owl:Restriction ;
      owl:maxCardinality "1"^^xsd:int ;
      owl:onProperty iapd-sec-cr:q5G1 ;
    ] ;
  rdfs:subClassOf [
      rdf:type owl:Restriction ;
      owl:maxCardinality "1"^^xsd:int ;
      owl:onProperty iapd-sec-cr:q5G10 ;
    ] ;
  rdfs:subClassOf [
      rdf:type owl:Restriction ;
      owl:maxCardinality "1"^^xsd:int ;
      owl:onProperty iapd-sec-cr:q5G11 ;
    ] ;
  rdfs:subClassOf [
      rdf:type owl:Restriction ;
      owl:maxCardinality "1"^^xsd:int ;
      owl:onProperty iapd-sec-cr:q5G12 ;
    ] ;
  rdfs:subClassOf [
      rdf:type owl:Restriction ;
      owl:maxCardinality "1"^^xsd:int ;
      owl:onProperty iapd-sec-cr:q5G12Oth ;
    ] ;
  rdfs:subClassOf [
      rdf:type owl:Restriction ;
      owl:maxCardinality "1"^^xsd:int ;
      owl:onProperty iapd-sec-cr:q5G2 ;
    ] ;
  rdfs:subClassOf [
      rdf:type owl:Restriction ;
      owl:maxCardinality "1"^^xsd:int ;
      owl:onProperty iapd-sec-cr:q5G3 ;
    ] ;
  rdfs:subClassOf [
      rdf:type owl:Restriction ;
      owl:maxCardinality "1"^^xsd:int ;
      owl:onProperty iapd-sec-cr:q5G4 ;
    ] ;
  rdfs:subClassOf [
      rdf:type owl:Restriction ;
      owl:maxCardinality "1"^^xsd:int ;
      owl:onProperty iapd-sec-cr:q5G5 ;
    ] ;
  rdfs:subClassOf [
      rdf:type owl:Restriction ;
      owl:maxCardinality "1"^^xsd:int ;
      owl:onProperty iapd-sec-cr:q5G6 ;
    ] ;
  rdfs:subClassOf [
      rdf:type owl:Restriction ;
      owl:maxCardinality "1"^^xsd:int ;
      owl:onProperty iapd-sec-cr:q5G7 ;
    ] ;
  rdfs:subClassOf [
      rdf:type owl:Restriction ;
      owl:maxCardinality "1"^^xsd:int ;
      owl:onProperty iapd-sec-cr:q5G8 ;
    ] ;
  rdfs:subClassOf [
      rdf:type owl:Restriction ;
      owl:maxCardinality "1"^^xsd:int ;
      owl:onProperty iapd-sec-cr:q5G9 ;
    ] ;
  skos:definition """Firm's response to Part1A Item 5G - advisory services
(1) Financial planning services
(2) Portfolio management for individuals and/or small businesses
(3) Portfolio management for investment companies (as well as “business development companies”
that have made an election pursuant to section 54 of the Investment Company Act of 1940)
(4) Portfolio management for pooled investment vehicles (other than investment companies) (5) Portfolio management for businesses (other than small businesses) or institutional clients
(other than registered investment companies and other pooled investment vehicles) (6) Pension consulting services
(7) Selection of other advisers (including private fund managers)
(8) Publication of periodicals or newsletters
(9) Security ratings or pricing services
(10) Market timing services
(11) Educational seminars/workshops (12) Other (specify):"""^^xsd:string ;
.
iapd-sec-cr:Item5HType
  rdf:type owl:Class ;
  sxml:tag "Item5HType" ;
  rdfs:label "Item5HType"^^xsd:string ;
  rdfs:subClassOf iapd-sec-cr:FirmReport ;
  rdfs:subClassOf [
      rdf:type owl:Restriction ;
      sxml:isAttribute "true"^^xsd:boolean ;
      rdfs:comment "This node has Firm's response to Part1A Item 5H-If more than 500, how many (round to the nearest 500)."@en ;
      owl:allValuesFrom iapd-sec-cr:Int10Datatype ;
      owl:onProperty iapd-sec-cr:q5HMT500 ;
    ] ;
  rdfs:subClassOf [
      rdf:type owl:Restriction ;
      sxml:isAttribute "true"^^xsd:boolean ;
      rdfs:comment "This node has Firm's response to Part1A Item 5H-If you provide financial planning services, to how many clients did you provide these services during your last fiscal year."@en ;
      owl:allValuesFrom iapd-sec-cr:Str128Datatype ;
      owl:onProperty iapd-sec-cr:q5H ;
    ] ;
  rdfs:subClassOf [
      rdf:type owl:Restriction ;
      owl:maxCardinality "1"^^xsd:int ;
      owl:onProperty iapd-sec-cr:q5H ;
    ] ;
  rdfs:subClassOf [
      rdf:type owl:Restriction ;
      owl:maxCardinality "1"^^xsd:int ;
      owl:onProperty iapd-sec-cr:q5HMT500 ;
    ] ;
  skos:definition "Firm's response to Part1A Item 5H-If you provide financial planning services, to how many clients did you provide these services during your last fiscal year."^^xsd:string ;
.
iapd-sec-cr:Item5IType
  rdf:type owl:Class ;
  sxml:tag "Item5IType" ;
  rdfs:label "Item5IType"^^xsd:string ;
  rdfs:subClassOf iapd-sec-cr:FirmReport ;
  rdfs:subClassOf [
      rdf:type owl:Restriction ;
      sxml:isAttribute "true"^^xsd:boolean ;
      rdfs:comment "This node has Firm's response to Part1A Item 5I(1)-sponsor the wrap fee program (Y/N) Display a 'Y' when the checkbox is selected. Display an 'N' when the checkbox is not selected."@en ;
      owl:allValuesFrom iapd-sec-cr:AnswerYNType ;
      owl:onProperty iapd-sec-cr:q5I1 ;
    ] ;
  rdfs:subClassOf [
      rdf:type owl:Restriction ;
      sxml:isAttribute "true"^^xsd:boolean ;
      rdfs:comment "This node has Firm's response to Part1A Item 5I(2)-act as a portfolio manager for the wrap fee program (Y/N) Display a 'Y' when the checkbox is selected. Display an 'N' when the checkbox is not selected."@en ;
      owl:allValuesFrom iapd-sec-cr:AnswerYNType ;
      owl:onProperty iapd-sec-cr:q5I2 ;
    ] ;
  rdfs:subClassOf [
      rdf:type owl:Restriction ;
      owl:maxCardinality "1"^^xsd:int ;
      owl:onProperty iapd-sec-cr:q5I1 ;
    ] ;
  rdfs:subClassOf [
      rdf:type owl:Restriction ;
      owl:maxCardinality "1"^^xsd:int ;
      owl:onProperty iapd-sec-cr:q5I2 ;
    ] ;
  skos:definition "Firm's response to Part1A Item 5I(1)-sponsor the wrap fee program (Y/N) and Firm's response to Part1A Item 5I(2)-act as a portfolio manager for the wrap fee program (Y/N)"^^xsd:string ;
.
iapd-sec-cr:Item5JType
  rdf:type owl:Class ;
  sxml:tag "Item5JType" ;
  rdfs:label "Item5JType"^^xsd:string ;
  rdfs:subClassOf iapd-sec-cr:FirmReport ;
  rdfs:subClassOf [
      rdf:type owl:Restriction ;
      sxml:isAttribute "true"^^xsd:boolean ;
      rdfs:comment "This node has Firm's response to Part1A Item 5J-In response to Item 4.B. of Part 2A of Form ADV, do you indicate that you provide investment advice only with respect to limited types of investments (Y/N/null)."@en ;
      owl:allValuesFrom iapd-sec-cr:AnswerYNType ;
      owl:onProperty iapd-sec-cr:q5J ;
    ] ;
  rdfs:subClassOf [
      rdf:type owl:Restriction ;
      owl:maxCardinality "1"^^xsd:int ;
      owl:onProperty iapd-sec-cr:q5J ;
    ] ;
  skos:definition "Firm's response to Part1A Item 5J-In response to Item 4.B. of Part 2A of Form ADV, do you indicate that you provide investment advice only with respect to limited types of investments (Y/N/null)."^^xsd:string ;
.
iapd-sec-cr:Item6AType
  rdf:type owl:Class ;
  sxml:tag "Item6AType" ;
  rdfs:comment "The answers are object properties to instances of the anwerYNType class."^^xsd:string ;
  rdfs:label "Item6AType"^^xsd:string ;
  rdfs:subClassOf iapd-sec-cr:FirmReport ;
  rdfs:subClassOf [
      rdf:type owl:Restriction ;
      sxml:isAttribute "true"^^xsd:boolean ;
      rdfs:comment "This node has Firm's response to Part1A Item 6A(1)- broker-dealer (registered or unregistered) (Y/N) Display a 'Y' when the checkbox is selected. Display an 'N' when the checkbox is not selected."@en ;
      owl:allValuesFrom iapd-sec-cr:AnswerYNType ;
      owl:onProperty iapd-sec-cr:q6A1 ;
    ] ;
  rdfs:subClassOf [
      rdf:type owl:Restriction ;
      sxml:isAttribute "true"^^xsd:boolean ;
      rdfs:comment "This node has Firm's response to Part1A Item 6A(10)-registered security-based swap dealer (Y/N) Display a 'Y' when the checkbox is selected. Display an 'N' when the checkbox is not selected."@en ;
      owl:allValuesFrom iapd-sec-cr:AnswerYNType ;
      owl:onProperty iapd-sec-cr:q6A10 ;
    ] ;
  rdfs:subClassOf [
      rdf:type owl:Restriction ;
      sxml:isAttribute "true"^^xsd:boolean ;
      rdfs:comment "This node has Firm's response to Part1A Item 6A(11)-major security-based swap participant (Y/N) Display a 'Y' when the checkbox is selected. Display an 'N' when the checkbox is not selected."@en ;
      owl:allValuesFrom iapd-sec-cr:AnswerYNType ;
      owl:onProperty iapd-sec-cr:q6A11 ;
    ] ;
  rdfs:subClassOf [
      rdf:type owl:Restriction ;
      sxml:isAttribute "true"^^xsd:boolean ;
      rdfs:comment "This node has Firm's response to Part1A Item 6A(12)-accountant or accounting firm (Y/N) Display a 'Y' when the checkbox is selected. Display an 'N' when the checkbox is not selected."@en ;
      owl:allValuesFrom iapd-sec-cr:AnswerYNType ;
      owl:onProperty iapd-sec-cr:q6A12 ;
    ] ;
  rdfs:subClassOf [
      rdf:type owl:Restriction ;
      sxml:isAttribute "true"^^xsd:boolean ;
      rdfs:comment "This node has Firm's response to Part1A Item 6A(13)-lawyer or law firm (Y/N) Display a 'Y' when the checkbox is selected. Display an 'N' when the checkbox is not selected."@en ;
      owl:allValuesFrom iapd-sec-cr:AnswerYNType ;
      owl:onProperty iapd-sec-cr:q6A13 ;
    ] ;
  rdfs:subClassOf [
      rdf:type owl:Restriction ;
      sxml:isAttribute "true"^^xsd:boolean ;
      rdfs:comment "This node has Firm's response to Part1A Item 6A(14)-Other financial product salesperson Display a 'Y' when the checkbox is selected. Display an 'N' when the checkbox is not selected."@en ;
      owl:allValuesFrom iapd-sec-cr:AnswerYNType ;
      owl:onProperty iapd-sec-cr:q6A14 ;
    ] ;
  rdfs:subClassOf [
      rdf:type owl:Restriction ;
      sxml:isAttribute "true"^^xsd:boolean ;
      rdfs:comment "This node has Firm's response to Part1A Item 6A(14)-Other text when financial product salesperson is selected 'Y'."@en ;
      owl:allValuesFrom iapd-sec-cr:Str50Datatype ;
      owl:onProperty iapd-sec-cr:q6A14Oth ;
    ] ;
  rdfs:subClassOf [
      rdf:type owl:Restriction ;
      sxml:isAttribute "true"^^xsd:boolean ;
      rdfs:comment "This node has Firm's response to Part1A Item 6A(2)-registered representative of a broker-dealer (Y/N) Display a 'Y' when the checkbox is selected. Display an 'N' when the checkbox is not selected."@en ;
      owl:allValuesFrom iapd-sec-cr:AnswerYNType ;
      owl:onProperty iapd-sec-cr:q6A2 ;
    ] ;
  rdfs:subClassOf [
      rdf:type owl:Restriction ;
      sxml:isAttribute "true"^^xsd:boolean ;
      rdfs:comment "This node has Firm's response to Part1A Item 6A(3)- commodity pool operator or commodity trading advisor (whether registered or exempt from registration) (Y/N) Display a 'Y' when the checkbox is selected. Display an 'N' when the checkbox is not selected."@en ;
      owl:allValuesFrom iapd-sec-cr:AnswerYNType ;
      owl:onProperty iapd-sec-cr:q6A3 ;
    ] ;
  rdfs:subClassOf [
      rdf:type owl:Restriction ;
      sxml:isAttribute "true"^^xsd:boolean ;
      rdfs:comment "This node has Firm's response to Part1A Item 6A(4)-futures commission merchant (Y/N) Display a 'Y' when the checkbox is selected. Display an 'N' when the checkbox is not selected."@en ;
      owl:allValuesFrom iapd-sec-cr:AnswerYNType ;
      owl:onProperty iapd-sec-cr:q6A4 ;
    ] ;
  rdfs:subClassOf [
      rdf:type owl:Restriction ;
      sxml:isAttribute "true"^^xsd:boolean ;
      rdfs:comment "This node has Firm's response to Part1A Item 6A(5)-real estate broker, dealer, or agent (Y/N) Display a 'Y' when the checkbox is selected. Display an 'N' when the checkbox is not selected."@en ;
      owl:allValuesFrom iapd-sec-cr:AnswerYNType ;
      owl:onProperty iapd-sec-cr:q6A5 ;
    ] ;
  rdfs:subClassOf [
      rdf:type owl:Restriction ;
      sxml:isAttribute "true"^^xsd:boolean ;
      rdfs:comment "This node has Firm's response to Part1A Item 6A(6)-insurance broker or agent (Y/N) Display a 'Y' when the checkbox is selected. Display an 'N' when the checkbox is not selected."@en ;
      owl:allValuesFrom iapd-sec-cr:AnswerYNType ;
      owl:onProperty iapd-sec-cr:q6A6 ;
    ] ;
  rdfs:subClassOf [
      rdf:type owl:Restriction ;
      sxml:isAttribute "true"^^xsd:boolean ;
      rdfs:comment "This node has Firm's response to Part1A Item 6A(7)-bank (including a separately identifiable department or division of a bank) (Y/N) Display a 'Y' when the checkbox is selected. Display an 'N' when the checkbox is not selected."@en ;
      owl:allValuesFrom iapd-sec-cr:AnswerYNType ;
      owl:onProperty iapd-sec-cr:q6A7 ;
    ] ;
  rdfs:subClassOf [
      rdf:type owl:Restriction ;
      sxml:isAttribute "true"^^xsd:boolean ;
      rdfs:comment "This node has Firm's response to Part1A Item 6A(8)-trust company (Y/N) Display a 'Y' when the checkbox is selected. Display an 'N' when the checkbox is not selected."@en ;
      owl:allValuesFrom iapd-sec-cr:AnswerYNType ;
      owl:onProperty iapd-sec-cr:q6A8 ;
    ] ;
  rdfs:subClassOf [
      rdf:type owl:Restriction ;
      sxml:isAttribute "true"^^xsd:boolean ;
      rdfs:comment "This node has Firm's response to Part1A Item 6A(9)-registered municipal advisor (Y/N) Display a 'Y' when the checkbox is selected. Display an 'N' when the checkbox is not selected."@en ;
      owl:allValuesFrom iapd-sec-cr:AnswerYNType ;
      owl:onProperty iapd-sec-cr:q6A9 ;
    ] ;
  rdfs:subClassOf [
      rdf:type owl:Restriction ;
      owl:maxCardinality "1"^^xsd:int ;
      owl:onProperty iapd-sec-cr:q6A1 ;
    ] ;
  rdfs:subClassOf [
      rdf:type owl:Restriction ;
      owl:maxCardinality "1"^^xsd:int ;
      owl:onProperty iapd-sec-cr:q6A10 ;
    ] ;
  rdfs:subClassOf [
      rdf:type owl:Restriction ;
      owl:maxCardinality "1"^^xsd:int ;
      owl:onProperty iapd-sec-cr:q6A11 ;
    ] ;
  rdfs:subClassOf [
      rdf:type owl:Restriction ;
      owl:maxCardinality "1"^^xsd:int ;
      owl:onProperty iapd-sec-cr:q6A12 ;
    ] ;
  rdfs:subClassOf [
      rdf:type owl:Restriction ;
      owl:maxCardinality "1"^^xsd:int ;
      owl:onProperty iapd-sec-cr:q6A13 ;
    ] ;
  rdfs:subClassOf [
      rdf:type owl:Restriction ;
      owl:maxCardinality "1"^^xsd:int ;
      owl:onProperty iapd-sec-cr:q6A14 ;
    ] ;
  rdfs:subClassOf [
      rdf:type owl:Restriction ;
      owl:maxCardinality "1"^^xsd:int ;
      owl:onProperty iapd-sec-cr:q6A14Oth ;
    ] ;
  rdfs:subClassOf [
      rdf:type owl:Restriction ;
      owl:maxCardinality "1"^^xsd:int ;
      owl:onProperty iapd-sec-cr:q6A2 ;
    ] ;
  rdfs:subClassOf [
      rdf:type owl:Restriction ;
      owl:maxCardinality "1"^^xsd:int ;
      owl:onProperty iapd-sec-cr:q6A3 ;
    ] ;
  rdfs:subClassOf [
      rdf:type owl:Restriction ;
      owl:maxCardinality "1"^^xsd:int ;
      owl:onProperty iapd-sec-cr:q6A4 ;
    ] ;
  rdfs:subClassOf [
      rdf:type owl:Restriction ;
      owl:maxCardinality "1"^^xsd:int ;
      owl:onProperty iapd-sec-cr:q6A5 ;
    ] ;
  rdfs:subClassOf [
      rdf:type owl:Restriction ;
      owl:maxCardinality "1"^^xsd:int ;
      owl:onProperty iapd-sec-cr:q6A6 ;
    ] ;
  rdfs:subClassOf [
      rdf:type owl:Restriction ;
      owl:maxCardinality "1"^^xsd:int ;
      owl:onProperty iapd-sec-cr:q6A7 ;
    ] ;
  rdfs:subClassOf [
      rdf:type owl:Restriction ;
      owl:maxCardinality "1"^^xsd:int ;
      owl:onProperty iapd-sec-cr:q6A8 ;
    ] ;
  rdfs:subClassOf [
      rdf:type owl:Restriction ;
      owl:maxCardinality "1"^^xsd:int ;
      owl:onProperty iapd-sec-cr:q6A9 ;
    ] ;
  skos:definition """Firm's response to Part1A Item 6A - Other Business Activities
(1) broker-dealer (registered or unregistered)
(2) registered representative of a broker-dealer (3) commodity pool operator or commodity trading advisor (whether registered or exempt from
registration) (4) futures commission merchant
(5) real estate broker, dealer, or agent
(6) insurance broker or agent
(7) bank (including a separately identifiable department or division of a bank)
(8) trust company
(9) registered municipal advisor
(10) registered security-based swap dealer
(11) major security-based swap participant
(12) accountant or accounting firm
(13) lawyer or law firm
(14) other financial product salesperson (specify):"""^^xsd:string ;
.
iapd-sec-cr:Item6BType
  rdf:type owl:Class ;
  sxml:tag "Item6BType" ;
  rdfs:label "Item6BType"^^xsd:string ;
  rdfs:subClassOf iapd-sec-cr:FirmReport ;
  rdfs:subClassOf [
      rdf:type owl:Restriction ;
      sxml:isAttribute "true"^^xsd:boolean ;
      rdfs:comment "This node has Firm's response to Part1A Item 6B(1)-Are you actively engaged in any other business not listed in Item 6.A. (other than giving investment advice) (Y/N)."@en ;
      owl:allValuesFrom iapd-sec-cr:AnswerYNType ;
      owl:onProperty iapd-sec-cr:q6B1 ;
    ] ;
  rdfs:subClassOf [
      rdf:type owl:Restriction ;
      sxml:isAttribute "true"^^xsd:boolean ;
      rdfs:comment "This node has Firm's response to Part1A Item 6B(2)-If yes, is this other business your primary business (Y/N/null)."@en ;
      owl:allValuesFrom iapd-sec-cr:AnswerYNType ;
      owl:onProperty iapd-sec-cr:q6B2 ;
    ] ;
  rdfs:subClassOf [
      rdf:type owl:Restriction ;
      sxml:isAttribute "true"^^xsd:boolean ;
      rdfs:comment "This node has Firm's response to Part1A Item 6B(3)-Do you sell products or provide services other than investment advice to your advisory clients (Y/N)."@en ;
      owl:allValuesFrom iapd-sec-cr:AnswerYNType ;
      owl:onProperty iapd-sec-cr:q6B3 ;
    ] ;
  rdfs:subClassOf [
      rdf:type owl:Restriction ;
      owl:maxCardinality "1"^^xsd:int ;
      owl:onProperty iapd-sec-cr:q6B1 ;
    ] ;
  rdfs:subClassOf [
      rdf:type owl:Restriction ;
      owl:maxCardinality "1"^^xsd:int ;
      owl:onProperty iapd-sec-cr:q6B2 ;
    ] ;
  rdfs:subClassOf [
      rdf:type owl:Restriction ;
      owl:maxCardinality "1"^^xsd:int ;
      owl:onProperty iapd-sec-cr:q6B3 ;
    ] ;
  skos:definition """Firm's response to Part1A Item 6B - other business
(1) Are you actively engaged in any other business not listed in Item 6.A. (other than giving investment advice)? Y/N
(2) If yes, is this other business your primary business? Y/N
(3) Do you sell products or provide services other than investment advice to your advisory clients? Y/N"""^^xsd:string ;
.
iapd-sec-cr:Item7AType
  rdf:type owl:Class ;
  sxml:tag "Item7AType" ;
  rdfs:comment "The answers are object properties to instances of the anwerYNType class."^^xsd:string ;
  rdfs:label "Item7AType"^^xsd:string ;
  rdfs:subClassOf iapd-sec-cr:FirmReport ;
  rdfs:subClassOf [
      rdf:type owl:Restriction ;
      sxml:isAttribute "true"^^xsd:boolean ;
      rdfs:comment "This node has Firm's response to Part1A Item 7A(1)-broker-dealer, municipal securities dealer, or government securities broker or dealer (registered or unregistered) (Y/N)."@en ;
      owl:allValuesFrom iapd-sec-cr:AnswerYNType ;
      owl:onProperty iapd-sec-cr:q7A1 ;
    ] ;
  rdfs:subClassOf [
      rdf:type owl:Restriction ;
      sxml:isAttribute "true"^^xsd:boolean ;
      rdfs:comment "This node has Firm's response to Part1A Item 7A(10)-accountant or accounting firm (Y/N)."@en ;
      owl:allValuesFrom iapd-sec-cr:AnswerYNType ;
      owl:onProperty iapd-sec-cr:q7A10 ;
    ] ;
  rdfs:subClassOf [
      rdf:type owl:Restriction ;
      sxml:isAttribute "true"^^xsd:boolean ;
      rdfs:comment "This node has Firm's response to Part1A Item 7A(11)-lawyer or law firm (Y/N)."@en ;
      owl:allValuesFrom iapd-sec-cr:AnswerYNType ;
      owl:onProperty iapd-sec-cr:q7A11 ;
    ] ;
  rdfs:subClassOf [
      rdf:type owl:Restriction ;
      sxml:isAttribute "true"^^xsd:boolean ;
      rdfs:comment "This node has Firm's response to Part1A Item 7A(12)-insurance company or agency (Y/N)."@en ;
      owl:allValuesFrom iapd-sec-cr:AnswerYNType ;
      owl:onProperty iapd-sec-cr:q7A12 ;
    ] ;
  rdfs:subClassOf [
      rdf:type owl:Restriction ;
      sxml:isAttribute "true"^^xsd:boolean ;
      rdfs:comment "This node has Firm's response to Part1A Item 7A(13)-pension consultant (Y/N)."@en ;
      owl:allValuesFrom iapd-sec-cr:AnswerYNType ;
      owl:onProperty iapd-sec-cr:q7A13 ;
    ] ;
  rdfs:subClassOf [
      rdf:type owl:Restriction ;
      sxml:isAttribute "true"^^xsd:boolean ;
      rdfs:comment "This node has Firm's response to Part1A Item 7A(14)-real estate broker or dealer (Y/N)."@en ;
      owl:allValuesFrom iapd-sec-cr:AnswerYNType ;
      owl:onProperty iapd-sec-cr:q7A14 ;
    ] ;
  rdfs:subClassOf [
      rdf:type owl:Restriction ;
      sxml:isAttribute "true"^^xsd:boolean ;
      rdfs:comment "This node has Firm's response to Part1A Item 7A(15)-sponsor or syndicator of limited partnerships (or equivalent), excluding pooled investment vehicles (Y/N)."@en ;
      owl:allValuesFrom iapd-sec-cr:AnswerYNType ;
      owl:onProperty iapd-sec-cr:q7A15 ;
    ] ;
  rdfs:subClassOf [
      rdf:type owl:Restriction ;
      sxml:isAttribute "true"^^xsd:boolean ;
      rdfs:comment "This node has Firm's response to Part1A Item 7A(16)-sponsor, general partner, managing member (or equivalent) of pooled investment vehicles (Y/N)."@en ;
      owl:allValuesFrom iapd-sec-cr:AnswerYNType ;
      owl:onProperty iapd-sec-cr:q7A16 ;
    ] ;
  rdfs:subClassOf [
      rdf:type owl:Restriction ;
      sxml:isAttribute "true"^^xsd:boolean ;
      rdfs:comment "This node has Firm's response to Part1A Item 7A(2)-other investment adviser (including financial planners) (Y/N)."@en ;
      owl:allValuesFrom iapd-sec-cr:AnswerYNType ;
      owl:onProperty iapd-sec-cr:q7A2 ;
    ] ;
  rdfs:subClassOf [
      rdf:type owl:Restriction ;
      sxml:isAttribute "true"^^xsd:boolean ;
      rdfs:comment "This node has Firm's response to Part1A Item 7A(3)-registered municipal advisor."@en ;
      owl:allValuesFrom iapd-sec-cr:AnswerYNType ;
      owl:onProperty iapd-sec-cr:q7A3 ;
    ] ;
  rdfs:subClassOf [
      rdf:type owl:Restriction ;
      sxml:isAttribute "true"^^xsd:boolean ;
      rdfs:comment "This node has Firm's response to Part1A Item 7A(4)-registered security-based swap dealer."@en ;
      owl:allValuesFrom iapd-sec-cr:AnswerYNType ;
      owl:onProperty iapd-sec-cr:q7A4 ;
    ] ;
  rdfs:subClassOf [
      rdf:type owl:Restriction ;
      sxml:isAttribute "true"^^xsd:boolean ;
      rdfs:comment "This node has Firm's response to Part1A Item 7A(5)-major security-based swap participant."@en ;
      owl:allValuesFrom iapd-sec-cr:AnswerYNType ;
      owl:onProperty iapd-sec-cr:q7A5 ;
    ] ;
  rdfs:subClassOf [
      rdf:type owl:Restriction ;
      sxml:isAttribute "true"^^xsd:boolean ;
      rdfs:comment "This node has Firm's response to Part1A Item 7A(6)- commodity pool operator or commodity trading advisor (whether registered or exempt from registration) (Y/N)."@en ;
      owl:allValuesFrom iapd-sec-cr:AnswerYNType ;
      owl:onProperty iapd-sec-cr:q7A6 ;
    ] ;
  rdfs:subClassOf [
      rdf:type owl:Restriction ;
      sxml:isAttribute "true"^^xsd:boolean ;
      rdfs:comment "This node has Firm's response to Part1A Item 7A(7)-futures commission merchant."@en ;
      owl:allValuesFrom iapd-sec-cr:AnswerYNType ;
      owl:onProperty iapd-sec-cr:q7A7 ;
    ] ;
  rdfs:subClassOf [
      rdf:type owl:Restriction ;
      sxml:isAttribute "true"^^xsd:boolean ;
      rdfs:comment "This node has Firm's response to Part1A Item 7A(8)-banking or thrift institution (Y/N)."@en ;
      owl:allValuesFrom iapd-sec-cr:AnswerYNType ;
      owl:onProperty iapd-sec-cr:q7A8 ;
    ] ;
  rdfs:subClassOf [
      rdf:type owl:Restriction ;
      sxml:isAttribute "true"^^xsd:boolean ;
      rdfs:comment "This node has Firm's response to Part1A Item 7A(9)-trust company."@en ;
      owl:allValuesFrom iapd-sec-cr:AnswerYNType ;
      owl:onProperty iapd-sec-cr:q7A9 ;
    ] ;
  rdfs:subClassOf [
      rdf:type owl:Restriction ;
      owl:maxCardinality "1"^^xsd:int ;
      owl:onProperty iapd-sec-cr:q7A1 ;
    ] ;
  rdfs:subClassOf [
      rdf:type owl:Restriction ;
      owl:maxCardinality "1"^^xsd:int ;
      owl:onProperty iapd-sec-cr:q7A10 ;
    ] ;
  rdfs:subClassOf [
      rdf:type owl:Restriction ;
      owl:maxCardinality "1"^^xsd:int ;
      owl:onProperty iapd-sec-cr:q7A11 ;
    ] ;
  rdfs:subClassOf [
      rdf:type owl:Restriction ;
      owl:maxCardinality "1"^^xsd:int ;
      owl:onProperty iapd-sec-cr:q7A12 ;
    ] ;
  rdfs:subClassOf [
      rdf:type owl:Restriction ;
      owl:maxCardinality "1"^^xsd:int ;
      owl:onProperty iapd-sec-cr:q7A13 ;
    ] ;
  rdfs:subClassOf [
      rdf:type owl:Restriction ;
      owl:maxCardinality "1"^^xsd:int ;
      owl:onProperty iapd-sec-cr:q7A14 ;
    ] ;
  rdfs:subClassOf [
      rdf:type owl:Restriction ;
      owl:maxCardinality "1"^^xsd:int ;
      owl:onProperty iapd-sec-cr:q7A15 ;
    ] ;
  rdfs:subClassOf [
      rdf:type owl:Restriction ;
      owl:maxCardinality "1"^^xsd:int ;
      owl:onProperty iapd-sec-cr:q7A16 ;
    ] ;
  rdfs:subClassOf [
      rdf:type owl:Restriction ;
      owl:maxCardinality "1"^^xsd:int ;
      owl:onProperty iapd-sec-cr:q7A2 ;
    ] ;
  rdfs:subClassOf [
      rdf:type owl:Restriction ;
      owl:maxCardinality "1"^^xsd:int ;
      owl:onProperty iapd-sec-cr:q7A3 ;
    ] ;
  rdfs:subClassOf [
      rdf:type owl:Restriction ;
      owl:maxCardinality "1"^^xsd:int ;
      owl:onProperty iapd-sec-cr:q7A4 ;
    ] ;
  rdfs:subClassOf [
      rdf:type owl:Restriction ;
      owl:maxCardinality "1"^^xsd:int ;
      owl:onProperty iapd-sec-cr:q7A5 ;
    ] ;
  rdfs:subClassOf [
      rdf:type owl:Restriction ;
      owl:maxCardinality "1"^^xsd:int ;
      owl:onProperty iapd-sec-cr:q7A6 ;
    ] ;
  rdfs:subClassOf [
      rdf:type owl:Restriction ;
      owl:maxCardinality "1"^^xsd:int ;
      owl:onProperty iapd-sec-cr:q7A7 ;
    ] ;
  rdfs:subClassOf [
      rdf:type owl:Restriction ;
      owl:maxCardinality "1"^^xsd:int ;
      owl:onProperty iapd-sec-cr:q7A8 ;
    ] ;
  rdfs:subClassOf [
      rdf:type owl:Restriction ;
      owl:maxCardinality "1"^^xsd:int ;
      owl:onProperty iapd-sec-cr:q7A9 ;
    ] ;
  skos:definition """Firm's response to Part1A Item 7A - Financial Industry Affiliations and Private Fund Reporting
(1) broker-dealer, municipal securities dealer, or government securities broker or dealer (registered
(2) other investment adviser (including financial planners)
(3) registered municipal advisor (4) registered security-based swap dealer
(5) major security-based swap participant (6) commodity pool operator or commodity trading advisor (whether registered or exempt from registration) 
(7) futures commission merchant
(8) banking or thrift institution (9) trust company
(10) accountant or accounting firm
(11) lawyer or law firm
(12) insurance company or agency
(13) pension consultant
(14) real estate broker or dealer
(15) sponsor or syndicator of limited partnerships (or equivalent), excluding pooled investment vehicles
(16) sponsor, general partner, managing member (or equivalent) of pooled investment vehicles"""^^xsd:string ;
.
iapd-sec-cr:Item7BType
  rdf:type owl:Class ;
  sxml:tag "Item7BType" ;
  rdfs:label "Item7BType"^^xsd:string ;
  rdfs:subClassOf iapd-sec-cr:FirmReport ;
  rdfs:subClassOf [
      rdf:type owl:Restriction ;
      sxml:isAttribute "true"^^xsd:boolean ;
      rdfs:comment "This node has Firm's response to Part1A Item 7B-Are you an adviser to any private fund (Y/N/null)."@en ;
      owl:allValuesFrom iapd-sec-cr:AnswerYNType ;
      owl:onProperty iapd-sec-cr:q7B ;
    ] ;
  rdfs:subClassOf [
      rdf:type owl:Restriction ;
      owl:maxCardinality "1"^^xsd:int ;
      owl:onProperty iapd-sec-cr:q7B ;
    ] ;
  skos:definition "Firm's response to Part1A Item 7B-Are you an adviser to any private fund (Y/N/null)."^^xsd:string ;
.
iapd-sec-cr:Item8AType
  rdf:type owl:Class ;
  sxml:tag "Item8AType" ;
  rdfs:comment "The answers are object properties to instances of the anwerYNType class."^^xsd:string ;
  rdfs:label "Item8AType"^^xsd:string ;
  rdfs:subClassOf iapd-sec-cr:FirmReport ;
  rdfs:subClassOf [
      rdf:type owl:Restriction ;
      sxml:isAttribute "true"^^xsd:boolean ;
      rdfs:comment "This node has Firm's response to Part1A Item 8A(1)-buy securities for yourself from advisory clients, or sell securities you own to advisory clients (principal transactions) (Y/N/null)."@en ;
      owl:allValuesFrom iapd-sec-cr:AnswerYNType ;
      owl:onProperty iapd-sec-cr:q8A1 ;
    ] ;
  rdfs:subClassOf [
      rdf:type owl:Restriction ;
      sxml:isAttribute "true"^^xsd:boolean ;
      rdfs:comment "This node has Firm's response to Part1A Item 8A(2)-buy or sell for yourself securities (other than shares of mutual funds) that you also recommend to advisory clients (Y/N/null)."@en ;
      owl:allValuesFrom iapd-sec-cr:AnswerYNType ;
      owl:onProperty iapd-sec-cr:q8A2 ;
    ] ;
  rdfs:subClassOf [
      rdf:type owl:Restriction ;
      sxml:isAttribute "true"^^xsd:boolean ;
      rdfs:comment "This node has Firm's response to Part1A Item 8A(3)-recommend securities (or other investment products) to advisory clients in which you or any related person has some other proprietary (ownership) interest (other than those mentioned in Items 8.A(1) or (2)) (Y/N/null)."@en ;
      owl:allValuesFrom iapd-sec-cr:AnswerYNType ;
      owl:onProperty iapd-sec-cr:q8A3 ;
    ] ;
  rdfs:subClassOf [
      rdf:type owl:Restriction ;
      owl:maxCardinality "1"^^xsd:int ;
      owl:onProperty iapd-sec-cr:q8A1 ;
    ] ;
  rdfs:subClassOf [
      rdf:type owl:Restriction ;
      owl:maxCardinality "1"^^xsd:int ;
      owl:onProperty iapd-sec-cr:q8A2 ;
    ] ;
  rdfs:subClassOf [
      rdf:type owl:Restriction ;
      owl:maxCardinality "1"^^xsd:int ;
      owl:onProperty iapd-sec-cr:q8A3 ;
    ] ;
  skos:definition """Firm's response to Part1A Item 8A - Participation or Interest in Client Transactions
Do you or any related person:
(1) buy securities for yourself from advisory clients, or sell securities you own to advisory clients (principal transactions)?
(2) buy or sell for yourself securities (other than shares of mutual funds) that you also recommend to advisory clients?
(3) recommend securities (or other investment products) to advisory clients in which you or any related person has some other proprietary (ownership) interest (other than those mentioned in Items 8.A.(1) or (2))?"""^^xsd:string ;
.
iapd-sec-cr:Item8BType
  rdf:type owl:Class ;
  sxml:tag "Item8BType" ;
  rdfs:comment "The answers are object properties to instances of the anwerYNType class."^^xsd:string ;
  rdfs:label "Item8BType"^^xsd:string ;
  rdfs:subClassOf iapd-sec-cr:FirmReport ;
  rdfs:subClassOf [
      rdf:type owl:Restriction ;
      sxml:isAttribute "true"^^xsd:boolean ;
      rdfs:comment "This node has Firm's response to Part1A Item 8B(1)-as a broker-dealer or registered representative of a broker-dealer, execute securities trades for brokerage customers in which advisory client securities are sold to or bought from the brokerage customer (agency cross transactions) (Y/N/null)."@en ;
      owl:allValuesFrom iapd-sec-cr:AnswerYNType ;
      owl:onProperty iapd-sec-cr:q8B1 ;
    ] ;
  rdfs:subClassOf [
      rdf:type owl:Restriction ;
      sxml:isAttribute "true"^^xsd:boolean ;
      rdfs:comment "This node has Firm's response to Part1A Item 8B(2)-recommend purchase of securities to advisory clients for which you or any related person serves as underwriter, general or managing partner, or purchaser representative (Y/N/null)."@en ;
      owl:allValuesFrom iapd-sec-cr:AnswerYNType ;
      owl:onProperty iapd-sec-cr:q8B2 ;
    ] ;
  rdfs:subClassOf [
      rdf:type owl:Restriction ;
      sxml:isAttribute "true"^^xsd:boolean ;
      rdfs:comment "This node has Firm's response to Part1A Item 8B(3)-recommend purchase or sale of securities to advisory clients for which you or any related person has any other sales interest (other than the receipt of sales commissions as a broker or registered representative of a broker-dealer) (Y/N/null)."@en ;
      owl:allValuesFrom iapd-sec-cr:AnswerYNType ;
      owl:onProperty iapd-sec-cr:q8B3 ;
    ] ;
  rdfs:subClassOf [
      rdf:type owl:Restriction ;
      owl:maxCardinality "1"^^xsd:int ;
      owl:onProperty iapd-sec-cr:q8B1 ;
    ] ;
  rdfs:subClassOf [
      rdf:type owl:Restriction ;
      owl:maxCardinality "1"^^xsd:int ;
      owl:onProperty iapd-sec-cr:q8B2 ;
    ] ;
  rdfs:subClassOf [
      rdf:type owl:Restriction ;
      owl:maxCardinality "1"^^xsd:int ;
      owl:onProperty iapd-sec-cr:q8B3 ;
    ] ;
  skos:definition "Firm's response to Part1A Item 8B - Sales Interest in Client Transactions"^^xsd:string ;
.
iapd-sec-cr:Item8CType
  rdf:type owl:Class ;
  sxml:tag "Item8CType" ;
  rdfs:comment "The answers are object properties to instances of the anwerYNType class."^^xsd:string ;
  rdfs:label "Item8CType"^^xsd:string ;
  rdfs:subClassOf iapd-sec-cr:FirmReport ;
  rdfs:subClassOf [
      rdf:type owl:Restriction ;
      sxml:isAttribute "true"^^xsd:boolean ;
      rdfs:comment "This node has Firm's response to Part1A Item 8C(1)-securities to be bought or sold for a client's account (Y/N/null)."@en ;
      owl:allValuesFrom iapd-sec-cr:AnswerYNType ;
      owl:onProperty iapd-sec-cr:q8C1 ;
    ] ;
  rdfs:subClassOf [
      rdf:type owl:Restriction ;
      sxml:isAttribute "true"^^xsd:boolean ;
      rdfs:comment "This node has Firm's response to Part1A Item 8C(2)-amount of securities to be bought or sold for a client's account (Y/N/null)."@en ;
      owl:allValuesFrom iapd-sec-cr:AnswerYNType ;
      owl:onProperty iapd-sec-cr:q8C2 ;
    ] ;
  rdfs:subClassOf [
      rdf:type owl:Restriction ;
      sxml:isAttribute "true"^^xsd:boolean ;
      rdfs:comment "This node has Firm's response to Part1A Item 8C(3)-broker or dealer to be used for a purchase or sale of securities for a client's account (Y/N/null)."@en ;
      owl:allValuesFrom iapd-sec-cr:AnswerYNType ;
      owl:onProperty iapd-sec-cr:q8C3 ;
    ] ;
  rdfs:subClassOf [
      rdf:type owl:Restriction ;
      sxml:isAttribute "true"^^xsd:boolean ;
      rdfs:comment "This node has Firm's response to Part1A Item 8C(4)-commission rates to be paid to a broker or dealer for a client's securities transactions (Y/N/null)."@en ;
      owl:allValuesFrom iapd-sec-cr:AnswerYNType ;
      owl:onProperty iapd-sec-cr:q8C4 ;
    ] ;
  rdfs:subClassOf [
      rdf:type owl:Restriction ;
      owl:maxCardinality "1"^^xsd:int ;
      owl:onProperty iapd-sec-cr:q8C1 ;
    ] ;
  rdfs:subClassOf [
      rdf:type owl:Restriction ;
      owl:maxCardinality "1"^^xsd:int ;
      owl:onProperty iapd-sec-cr:q8C2 ;
    ] ;
  rdfs:subClassOf [
      rdf:type owl:Restriction ;
      owl:maxCardinality "1"^^xsd:int ;
      owl:onProperty iapd-sec-cr:q8C3 ;
    ] ;
  rdfs:subClassOf [
      rdf:type owl:Restriction ;
      owl:maxCardinality "1"^^xsd:int ;
      owl:onProperty iapd-sec-cr:q8C4 ;
    ] ;
  skos:definition """Firm's response to Part1A Item 8C - Investment or Brokerage Discretion
Do you or any related person have discretionary authority to determine the:
(1) securities to be bought or sold for a client’s account?
(2) amount of securities to be bought or sold for a client’s account?
(3) broker or dealer to be used for a purchase or sale of securities for a client’s account?
(4) commission rates to be paid to a broker or dealer for a client’s securities transactions?"""^^xsd:string ;
.
iapd-sec-cr:Item8DType
  rdf:type owl:Class ;
  sxml:tag "Item8DType" ;
  rdfs:label "Item8DType"^^xsd:string ;
  rdfs:subClassOf iapd-sec-cr:FirmReport ;
  rdfs:subClassOf [
      rdf:type owl:Restriction ;
      sxml:isAttribute "true"^^xsd:boolean ;
      rdfs:comment "This node has Firm's response to Part1A Item 8D-If you answer \"yes\" to 8C.(3), are any of the brokers or dealers related persons (Y/N/null)."@en ;
      owl:allValuesFrom iapd-sec-cr:AnswerYNType ;
      owl:onProperty iapd-sec-cr:q8D ;
    ] ;
  rdfs:subClassOf [
      rdf:type owl:Restriction ;
      owl:maxCardinality "1"^^xsd:int ;
      owl:onProperty iapd-sec-cr:q8D ;
    ] ;
  skos:definition "Firm's response to Part1A Item 8D-If you answer \"yes\" to 8C.(3), are any of the brokers or dealers related persons (Y/N/null)."^^xsd:string ;
.
iapd-sec-cr:Item8EType
  rdf:type owl:Class ;
  sxml:tag "Item8EType" ;
  rdfs:label "Item8EType"^^xsd:string ;
  rdfs:subClassOf iapd-sec-cr:FirmReport ;
  rdfs:subClassOf [
      rdf:type owl:Restriction ;
      sxml:isAttribute "true"^^xsd:boolean ;
      rdfs:comment "This node has Firm's response to Part1A Item 8E -Do you or any related person recommend brokers or dealers to clients (Y/N/null)."@en ;
      owl:allValuesFrom iapd-sec-cr:AnswerYNType ;
      owl:onProperty iapd-sec-cr:q8E ;
    ] ;
  rdfs:subClassOf [
      rdf:type owl:Restriction ;
      owl:maxCardinality "1"^^xsd:int ;
      owl:onProperty iapd-sec-cr:q8E ;
    ] ;
  skos:definition "Firm's response to Part1A Item 8E -Do you or any related person recommend brokers or dealers to clients (Y/N/null)."^^xsd:string ;
.
iapd-sec-cr:Item8FType
  rdf:type owl:Class ;
  sxml:tag "Item8FType" ;
  rdfs:label "Item8FType"^^xsd:string ;
  rdfs:subClassOf iapd-sec-cr:FirmReport ;
  rdfs:subClassOf [
      rdf:type owl:Restriction ;
      sxml:isAttribute "true"^^xsd:boolean ;
      rdfs:comment "This node has Firm's response to Part1A Item 8F-If you answer \"yes\" to 8E, are any of the brokers or dealers related persons (Y/N/null)."@en ;
      owl:allValuesFrom iapd-sec-cr:AnswerYNType ;
      owl:onProperty iapd-sec-cr:q8F ;
    ] ;
  rdfs:subClassOf [
      rdf:type owl:Restriction ;
      owl:maxCardinality "1"^^xsd:int ;
      owl:onProperty iapd-sec-cr:q8F ;
    ] ;
  skos:definition "Firm's response to Part1A Item 8F-If you answer \"yes\" to 8E, are any of the brokers or dealers related persons (Y/N/null)."^^xsd:string ;
.
iapd-sec-cr:Item8GType
  rdf:type owl:Class ;
  sxml:tag "Item8GType" ;
  rdfs:label "Item8GType"^^xsd:string ;
  rdfs:subClassOf iapd-sec-cr:FirmReport ;
  rdfs:subClassOf [
      rdf:type owl:Restriction ;
      sxml:isAttribute "true"^^xsd:boolean ;
      rdfs:comment "This node has Firm's response to Part1A Item 8G(1)-Do you or any related person receive research or other products or services other than execution from a broker-dealer or a third party (\"soft dollar benefits\") in connection with client securities transactions (Y/N/null)."@en ;
      owl:allValuesFrom iapd-sec-cr:AnswerYNType ;
      owl:onProperty iapd-sec-cr:q8G1 ;
    ] ;
  rdfs:subClassOf [
      rdf:type owl:Restriction ;
      sxml:isAttribute "true"^^xsd:boolean ;
      rdfs:comment "This node has Firm's response to Part1A Item 8G(2)-If \"yes\" to G.(1), are all the \"soft dollar benefits\" you or any related persons receive eligible \"research or brokerage services\" under section 28(e) of the Securities Exchange Act of 1934 (Y/N/null)."@en ;
      owl:allValuesFrom iapd-sec-cr:AnswerYNType ;
      owl:onProperty iapd-sec-cr:q8G2 ;
    ] ;
  rdfs:subClassOf [
      rdf:type owl:Restriction ;
      owl:maxCardinality "1"^^xsd:int ;
      owl:onProperty iapd-sec-cr:q8G1 ;
    ] ;
  rdfs:subClassOf [
      rdf:type owl:Restriction ;
      owl:maxCardinality "1"^^xsd:int ;
      owl:onProperty iapd-sec-cr:q8G2 ;
    ] ;
  skos:definition """Firm's response to Part1A Item 8G -soft dollars
(1)  Do you or any related person receive research or other products or services other than execution from a broker-dealer or a third party (\"soft dollar benefits\") in onnection with client securities transactions (Y/N/null).
(2) If \"yes\" to G.(1), are all the \"soft dollar benefits\" you or any related persons receive eligible \"research or brokerage services\" under section 28(e) of the Securities Exchange Act of 1934 (Y/N/null)."""^^xsd:string ;
.
iapd-sec-cr:Item8HType
  rdf:type owl:Class ;
  sxml:tag "Item8HType" ;
  rdfs:label "Item8HType"^^xsd:string ;
  rdfs:subClassOf iapd-sec-cr:FirmReport ;
  rdfs:subClassOf [
      rdf:type owl:Restriction ;
      sxml:isAttribute "true"^^xsd:boolean ;
      rdfs:comment "This node has Firm's response to Part1A Item 8H-Do you or any related person, directly or indirectly, compensate any person for client referrals (Y/N/null)."@en ;
      owl:allValuesFrom iapd-sec-cr:AnswerYNType ;
      owl:onProperty iapd-sec-cr:q8H ;
    ] ;
  rdfs:subClassOf [
      rdf:type owl:Restriction ;
      owl:maxCardinality "1"^^xsd:int ;
      owl:onProperty iapd-sec-cr:q8H ;
    ] ;
  skos:definition "Firm's response to Part1A Item 8H-Do you or any related person, directly or indirectly, compensate any person for client referrals (Y/N/null)."^^xsd:string ;
.
iapd-sec-cr:Item8IType
  rdf:type owl:Class ;
  sxml:tag "Item8IType" ;
  rdfs:label "Item8IType"^^xsd:string ;
  rdfs:subClassOf iapd-sec-cr:FirmReport ;
  rdfs:subClassOf [
      rdf:type owl:Restriction ;
      sxml:isAttribute "true"^^xsd:boolean ;
      rdfs:comment "This node has Firm's response to Part1A Item 8I-Do you or any related person, directly or indirectly, receive compensation from any person for client referrals(Y/N/null)."@en ;
      owl:allValuesFrom iapd-sec-cr:AnswerYNType ;
      owl:onProperty iapd-sec-cr:q8I ;
    ] ;
  rdfs:subClassOf [
      rdf:type owl:Restriction ;
      owl:maxCardinality "1"^^xsd:int ;
      owl:onProperty iapd-sec-cr:q8I ;
    ] ;
  skos:definition "Firm's response to Part1A Item 8I-Do you or any related person, directly or indirectly, receive compensation from any person for client referrals(Y/N/null)."^^xsd:string ;
.
iapd-sec-cr:Item9A1Type
  rdf:type owl:Class ;
  sxml:tag "Item9A1Type" ;
  rdfs:comment "The answers to (1) are object properties to instances of the anwerYNType class. Answers to (2) are decimal (17.2) and integer (38)"^^xsd:string ;
  rdfs:label "Item9A1Type"^^xsd:string ;
  rdfs:subClassOf iapd-sec-cr:FirmReport ;
  rdfs:subClassOf [
      rdf:type owl:Restriction ;
      sxml:isAttribute "true"^^xsd:boolean ;
      rdfs:comment "This node has Firm's response to Part1A Item  9A(2)(a)-U.S. Dollar Amount."@en ;
      owl:allValuesFrom iapd-sec-cr:Decimal17P2Datatype ;
      owl:onProperty iapd-sec-cr:q9A2A ;
    ] ;
  rdfs:subClassOf [
      rdf:type owl:Restriction ;
      sxml:isAttribute "true"^^xsd:boolean ;
      rdfs:comment "This node has Firm's response to Part1A Item 9A(1)(a)-cash or bank accounts (Y/N/null)."@en ;
      owl:allValuesFrom iapd-sec-cr:AnswerYNType ;
      owl:onProperty iapd-sec-cr:q9A1A ;
    ] ;
  rdfs:subClassOf [
      rdf:type owl:Restriction ;
      sxml:isAttribute "true"^^xsd:boolean ;
      rdfs:comment "This node has Firm's response to Part1A Item 9A(1)(b)-securities (Y/N/null)."@en ;
      owl:allValuesFrom iapd-sec-cr:AnswerYNType ;
      owl:onProperty iapd-sec-cr:q9A1B ;
    ] ;
  rdfs:subClassOf [
      rdf:type owl:Restriction ;
      sxml:isAttribute "true"^^xsd:boolean ;
      rdfs:comment "This node has Firm's response to Part1A Item 9A(2)(b)-Total Number of Clients."@en ;
      owl:allValuesFrom iapd-sec-cr:Int38Datatype ;
      owl:onProperty iapd-sec-cr:q9A2B ;
    ] ;
  rdfs:subClassOf [
      rdf:type owl:Restriction ;
      owl:maxCardinality "1"^^xsd:int ;
      owl:onProperty iapd-sec-cr:q9A1A ;
    ] ;
  rdfs:subClassOf [
      rdf:type owl:Restriction ;
      owl:maxCardinality "1"^^xsd:int ;
      owl:onProperty iapd-sec-cr:q9A1B ;
    ] ;
  rdfs:subClassOf [
      rdf:type owl:Restriction ;
      owl:maxCardinality "1"^^xsd:int ;
      owl:onProperty iapd-sec-cr:q9A2A ;
    ] ;
  rdfs:subClassOf [
      rdf:type owl:Restriction ;
      owl:maxCardinality "1"^^xsd:int ;
      owl:onProperty iapd-sec-cr:q9A2B ;
    ] ;
  skos:definition """Firm's response to Part1A Item 9A1 
(1) Do you have custody of any advisory clients’: Yes No
(a) cash or bank accounts?
(b) securities?
(2) If you checked “yes” to Item 9.A.(1)(a) or (b), what is the approximate amount of client funds and securities and total number of clients for which you have custody:
(a) U.S. Dollar Amount 
(b) Total Number of Clients"""^^xsd:string ;
.
iapd-sec-cr:Item9BType
  rdf:type owl:Class ;
  sxml:tag "Item9BType" ;
  rdfs:comment "The answers to (1) are object properties to instances of the anwerYNType class. Answers to (2) are xsd:decimal (17.2) and xsd:integer (38)"^^xsd:string ;
  rdfs:label "Item9BType"^^xsd:string ;
  rdfs:subClassOf iapd-sec-cr:FirmReport ;
  rdfs:subClassOf [
      rdf:type owl:Restriction ;
      sxml:isAttribute "true"^^xsd:boolean ;
      rdfs:comment "This node has Firm's response to Part1A Item  9B(2)(a)-U.S. Dollar Amount."@en ;
      owl:allValuesFrom iapd-sec-cr:Decimal17P2Datatype ;
      owl:onProperty iapd-sec-cr:q9B2A ;
    ] ;
  rdfs:subClassOf [
      rdf:type owl:Restriction ;
      sxml:isAttribute "true"^^xsd:boolean ;
      rdfs:comment "This node has Firm's response to Part1A Item 9B(1)(a)-cash or bank accounts (Y/N/null)."@en ;
      owl:allValuesFrom iapd-sec-cr:AnswerYNType ;
      owl:onProperty iapd-sec-cr:q9B1A ;
    ] ;
  rdfs:subClassOf [
      rdf:type owl:Restriction ;
      sxml:isAttribute "true"^^xsd:boolean ;
      rdfs:comment "This node has Firm's response to Part1A Item 9B(1)(b)-securities (Y/N/null)."@en ;
      owl:allValuesFrom iapd-sec-cr:AnswerYNType ;
      owl:onProperty iapd-sec-cr:q9B1B ;
    ] ;
  rdfs:subClassOf [
      rdf:type owl:Restriction ;
      sxml:isAttribute "true"^^xsd:boolean ;
      rdfs:comment "This node has Firm's response to Part1A Item 9B(2)(b)-Total Number of Clients."@en ;
      owl:allValuesFrom iapd-sec-cr:Int38Datatype ;
      owl:onProperty iapd-sec-cr:q9B2B ;
    ] ;
  rdfs:subClassOf [
      rdf:type owl:Restriction ;
      owl:maxCardinality "1"^^xsd:int ;
      owl:onProperty iapd-sec-cr:q9B1A ;
    ] ;
  rdfs:subClassOf [
      rdf:type owl:Restriction ;
      owl:maxCardinality "1"^^xsd:int ;
      owl:onProperty iapd-sec-cr:q9B1B ;
    ] ;
  rdfs:subClassOf [
      rdf:type owl:Restriction ;
      owl:maxCardinality "1"^^xsd:int ;
      owl:onProperty iapd-sec-cr:q9B2A ;
    ] ;
  rdfs:subClassOf [
      rdf:type owl:Restriction ;
      owl:maxCardinality "1"^^xsd:int ;
      owl:onProperty iapd-sec-cr:q9B2B ;
    ] ;
  skos:definition """Firm's response to Part1A Item 9B
(1) In connection with advisory services you provide to clients, do any of your related persons have custody of any of your advisory clients’: Yes No
(a) cash or bank accounts?
(b) securities?
You are required to answer this item regardless of how you answered Item 9.A.(1)(a) or (b).
(2) If you checked “yes” to Item 9.B.(1)(a) or (b), what is the approximate amount of client funds and securities and total number of clients for which your related persons have custody:"""^^xsd:string ;
.
iapd-sec-cr:Item9CType
  rdf:type owl:Class ;
  sxml:tag "Item9CType" ;
  rdfs:comment "The answers are object properties to instances of the anwerYNType class."^^xsd:string ;
  rdfs:label "Item9CType"^^xsd:string ;
  rdfs:subClassOf iapd-sec-cr:FirmReport ;
  rdfs:subClassOf [
      rdf:type owl:Restriction ;
      sxml:isAttribute "true"^^xsd:boolean ;
      rdfs:comment "This node has Firm's response to Part1A Item 9C(1)- A qualified custodian(s) sends account statements at least quarterly to the investors in the pooled investment vehicle(s) you manage."@en ;
      owl:allValuesFrom iapd-sec-cr:AnswerYNType ;
      owl:onProperty iapd-sec-cr:q9C1 ;
    ] ;
  rdfs:subClassOf [
      rdf:type owl:Restriction ;
      sxml:isAttribute "true"^^xsd:boolean ;
      rdfs:comment "This node has Firm's response to Part1A Item 9C(2)- An independent public accountant audits annually the pooled investment vehicle(s) that you manage and the audited financial statements are distributed to the investors in the pools."@en ;
      owl:allValuesFrom iapd-sec-cr:AnswerYNType ;
      owl:onProperty iapd-sec-cr:q9C2 ;
    ] ;
  rdfs:subClassOf [
      rdf:type owl:Restriction ;
      sxml:isAttribute "true"^^xsd:boolean ;
      rdfs:comment "This node has Firm's response to Part1A Item 9C(3)- An independent public accountant conducts an annual surprise examination of client funds and securities."@en ;
      owl:allValuesFrom iapd-sec-cr:AnswerYNType ;
      owl:onProperty iapd-sec-cr:q9C3 ;
    ] ;
  rdfs:subClassOf [
      rdf:type owl:Restriction ;
      sxml:isAttribute "true"^^xsd:boolean ;
      rdfs:comment "This node has Firm's response to Part1A Item 9C(4)- An independent public accountant prepares an internal control report with respect to custodial services when you or your related persons are qualified custodians for client funds and securities."@en ;
      owl:allValuesFrom iapd-sec-cr:AnswerYNType ;
      owl:onProperty iapd-sec-cr:q9C4 ;
    ] ;
  rdfs:subClassOf [
      rdf:type owl:Restriction ;
      owl:maxCardinality "1"^^xsd:int ;
      owl:onProperty iapd-sec-cr:q9C1 ;
    ] ;
  rdfs:subClassOf [
      rdf:type owl:Restriction ;
      owl:maxCardinality "1"^^xsd:int ;
      owl:onProperty iapd-sec-cr:q9C2 ;
    ] ;
  rdfs:subClassOf [
      rdf:type owl:Restriction ;
      owl:maxCardinality "1"^^xsd:int ;
      owl:onProperty iapd-sec-cr:q9C3 ;
    ] ;
  rdfs:subClassOf [
      rdf:type owl:Restriction ;
      owl:maxCardinality "1"^^xsd:int ;
      owl:onProperty iapd-sec-cr:q9C4 ;
    ] ;
  skos:definition """Firm's response to Part1A Item 9C - custody of client funds or securities in connection with advisory services you provide to clients 
(1) A qualified custodian(s) sends account statements at least quarterly to the investors in the pooled investment vehicle(s) you manage.
(2) An independent public accountant audits annually the pooled investment vehicle(s) that you manage and the audited financial statements are distributed to the investors in the pools.
(3) An independent public accountant conducts an annual surprise examination of client funds and securities.
(4) An independent public accountant prepares an internal control report with respect to custodial services when you or your related persons are qualified custodians for client funds and securities."""^^xsd:string ;
.
iapd-sec-cr:Item9DType
  rdf:type owl:Class ;
  sxml:tag "Item9DType" ;
  rdfs:comment "The answers are object properties to instances of the anwerYNType class."^^xsd:string ;
  rdfs:label "Item9DType"^^xsd:string ;
  rdfs:subClassOf iapd-sec-cr:FirmReport ;
  rdfs:subClassOf [
      rdf:type owl:Restriction ;
      sxml:isAttribute "true"^^xsd:boolean ;
      rdfs:comment "This node has Firm's response to Part1A Item 9D(1)-you act as a qualified custodian (Y/N/null)."@en ;
      owl:allValuesFrom iapd-sec-cr:AnswerYNType ;
      owl:onProperty iapd-sec-cr:q9D1 ;
    ] ;
  rdfs:subClassOf [
      rdf:type owl:Restriction ;
      sxml:isAttribute "true"^^xsd:boolean ;
      rdfs:comment "This node has Firm's response to Part1A Item 9D(2)-Do you or your related persons act as qualified custodians for your clients in connection with advisory services you provide to clients your related persons act as qualified custodians (Y/N/null)."@en ;
      owl:allValuesFrom iapd-sec-cr:AnswerYNType ;
      owl:onProperty iapd-sec-cr:q9D2 ;
    ] ;
  rdfs:subClassOf [
      rdf:type owl:Restriction ;
      owl:maxCardinality "1"^^xsd:int ;
      owl:onProperty iapd-sec-cr:q9D1 ;
    ] ;
  rdfs:subClassOf [
      rdf:type owl:Restriction ;
      owl:maxCardinality "1"^^xsd:int ;
      owl:onProperty iapd-sec-cr:q9D2 ;
    ] ;
  skos:definition """Firm's response to Part1A Item 9D - qualified custodian
(1) you act as a qualified custodian
(2) your related person(s) act as qualified custodian(s)"""^^xsd:string ;
.
iapd-sec-cr:Item9EType
  rdf:type owl:Class ;
  sxml:tag "Item9EType" ;
  rdfs:comment "This is stored as an untyped data property. It can be parsed a string."^^xsd:string ;
  rdfs:label "Item9EType"^^xsd:string ;
  rdfs:subClassOf iapd-sec-cr:FirmReport ;
  rdfs:subClassOf [
      rdf:type owl:Restriction ;
      sxml:isAttribute "true"^^xsd:boolean ;
      rdfs:comment "This node has Firm's response to Part1A Item 9E-If you are filing your annual updating amendment and you were subject to a surprise examination by an independent public accountant during your last fiscal year, provide the date (YYYY-MM) the examination commenced."@en ;
      owl:allValuesFrom xsd:gYearMonth ;
      owl:onProperty iapd-sec-cr:q9E ;
    ] ;
  rdfs:subClassOf [
      rdf:type owl:Restriction ;
      owl:maxCardinality "1"^^xsd:int ;
      owl:onProperty iapd-sec-cr:q9E ;
    ] ;
  skos:definition """Firm's response to Part1A Item 9E-If you are filing your annual updating amendment and you were
subject to a surprise examination by an independent public accountant during your last fiscal year, provide the date
(YYYY-MM) the examination commenced."""^^xsd:string ;
.
iapd-sec-cr:Item9FType
  rdf:type owl:Class ;
  sxml:tag "Item9FType" ;
  rdfs:label "Item9FType"^^xsd:string ;
  rdfs:subClassOf iapd-sec-cr:FirmReport ;
  rdfs:subClassOf [
      rdf:type owl:Restriction ;
      sxml:isAttribute "true"^^xsd:boolean ;
      rdfs:comment "This node has Firm's response to Part1A Item 9F-If you or your related persons have custody of client funds or securities, how many persons, including, but not limited to, you and your related persons, act as qualified custodians for your clients in connection with advisory services you provide to clients (Y/N/null)."@en ;
      owl:allValuesFrom iapd-sec-cr:Int38Datatype ;
      owl:onProperty iapd-sec-cr:q9F ;
    ] ;
  rdfs:subClassOf [
      rdf:type owl:Restriction ;
      owl:maxCardinality "1"^^xsd:int ;
      owl:onProperty iapd-sec-cr:q9F ;
    ] ;
  skos:definition "Firm's response to Part1A Item 9F-If you or your related persons have custody of client funds or securities, how many persons, including, but not limited to, you and your related persons, act as qualified custodians for your clients in connection with advisory services you provide to clients (Y/N/null)."^^xsd:string ;
.
iapd-sec-cr:ItemAType
  rdf:type owl:Class ;
  sxml:tag "ItemAType" ;
  rdfs:label "Item AType"^^xsd:string ;
  rdfs:subClassOf iapd-sec-cr:AddrType ;
  rdfs:subClassOf [
      rdf:type owl:Restriction ;
      sxml:isAttribute "true"^^xsd:boolean ;
      owl:allValuesFrom iapd-sec-cr:AnswerYNType ;
      owl:onProperty iapd-sec-cr:prvtAdrsFl ;
    ] ;
  rdfs:subClassOf [
      rdf:type owl:Restriction ;
      sxml:isAttribute "true"^^xsd:boolean ;
      owl:allValuesFrom iapd-sec-cr:Str128Datatype ;
      owl:onProperty iapd-sec-cr:email ;
    ] ;
  rdfs:subClassOf [
      rdf:type owl:Restriction ;
      sxml:isAttribute "true"^^xsd:boolean ;
      owl:allValuesFrom iapd-sec-cr:Str128Datatype ;
      owl:onProperty iapd-sec-cr:nm ;
    ] ;
  rdfs:subClassOf [
      rdf:type owl:Restriction ;
      sxml:isAttribute "true"^^xsd:boolean ;
      owl:allValuesFrom iapd-sec-cr:Str128Datatype ;
      owl:onProperty iapd-sec-cr:titleNm ;
    ] ;
  rdfs:subClassOf [
      rdf:type owl:Restriction ;
      owl:maxCardinality "1"^^xsd:int ;
      owl:onProperty iapd-sec-cr:email ;
    ] ;
  rdfs:subClassOf [
      rdf:type owl:Restriction ;
      owl:maxCardinality "1"^^xsd:int ;
      owl:onProperty iapd-sec-cr:nm ;
    ] ;
  rdfs:subClassOf [
      rdf:type owl:Restriction ;
      owl:maxCardinality "1"^^xsd:int ;
      owl:onProperty iapd-sec-cr:prvtAdrsFl ;
    ] ;
  rdfs:subClassOf [
      rdf:type owl:Restriction ;
      owl:maxCardinality "1"^^xsd:int ;
      owl:onProperty iapd-sec-cr:titleNm ;
    ] ;
.
iapd-sec-cr:NFT_FILED
  rdf:type iapd-sec-cr:NtcFiledType ;
  dtype:order "1"^^xsd:nonNegativeInteger ;
  dtype:value "FILED"^^xsd:NMTOKEN ;
  rdfs:label "FILED"^^xsd:string ;
.
iapd-sec-cr:NFT_PENDSEC
  rdf:type iapd-sec-cr:NtcFiledType ;
  dtype:order "2"^^xsd:nonNegativeInteger ;
  dtype:value "PENDSEC"^^xsd:NMTOKEN ;
  rdfs:label "PENDSEC"^^xsd:string ;
.
iapd-sec-cr:NFT_TRANS
  rdf:type iapd-sec-cr:NtcFiledType ;
  dtype:order "0"^^xsd:nonNegativeInteger ;
  dtype:value "TRANS"^^xsd:NMTOKEN ;
  rdfs:label "TRANS"^^xsd:string ;
.
iapd-sec-cr:NoticeFiledType
  rdf:type owl:Class ;
  sxml:tag "NoticeFiledType" ;
  rdfs:label "Notice filed type"^^xsd:string ;
  rdfs:subClassOf iapd-sec-cr:FirmReport ;
  rdfs:subClassOf [
      rdf:type owl:Restriction ;
      sxml:isAttribute "false"^^xsd:boolean ;
      sxml:order "0"^^xsd:int ;
      rdfs:comment "The States node has the List of states the firm is notice filed in."@en ;
      owl:allValuesFrom iapd-sec-cr:NtcType ;
      owl:onProperty iapd-sec-cr:statesRef ;
    ] ;
  skos:definition "A record of notices filed containg the state code and date."^^xsd:string ;
.
iapd-sec-cr:NtcFiledType
  rdf:type owl:Class ;
  sxml:tag "NtcFiledType" ;
  rdfs:comment """Elements of this type represent the business type.
        Allowed values (code-Name) are:
        TRANS-Transitioning.
        FILED-Notice Filed.
        PENDSEC-Pending."""@en ;
  rdfs:label "Ntc filed type"^^xsd:string ;
  rdfs:subClassOf iapd-sec-cr:EnumeratedValue ;
  rdfs:subClassOf [
      rdf:type owl:Restriction ;
      sxml:isAttribute "false"^^xsd:boolean ;
      owl:allValuesFrom xsd:NMTOKEN ;
      owl:onProperty dtype:value ;
    ] ;
  rdfs:subClassOf [
      rdf:type owl:Restriction ;
      owl:maxCardinality "1"^^xsd:int ;
      owl:onProperty dtype:value ;
    ] ;
  owl:oneOf (
      iapd-sec-cr:NFT_FILED
      iapd-sec-cr:NFT_PENDSEC
      iapd-sec-cr:NFT_TRANS
    ) ;
.
iapd-sec-cr:NtcType
  rdf:type owl:Class ;
  sxml:tag "NtcType" ;
  rdfs:comment "This has regulator, NTC status and date"@en ;
  rdfs:label "Ntc type"^^xsd:string ;
  rdfs:subClassOf iapd-sec-cr:FirmReport ;
  rdfs:subClassOf [
      rdf:type owl:Restriction ;
      sxml:isAttribute "true"^^xsd:boolean ;
      rdfs:comment "The Dt node has the effective date of the notice filed status."@en ;
      owl:allValuesFrom xsd:date ;
      owl:onProperty iapd-sec-cr:dt ;
    ] ;
  rdfs:subClassOf [
      rdf:type owl:Restriction ;
      sxml:isAttribute "true"^^xsd:boolean ;
      rdfs:comment "The st node has the Notice filed status of the state."@en ;
      owl:allValuesFrom iapd-sec-cr:NtcFiledType ;
      owl:onProperty iapd-sec-cr:st ;
    ] ;
  rdfs:subClassOf [
      rdf:type owl:Restriction ;
      sxml:isAttribute "true"^^xsd:boolean ;
      rdfs:comment "This node has the regulator code."@en ;
      owl:allValuesFrom iapd-sec-cr:StateCdType ;
      owl:onProperty iapd-sec-cr:rgltrCd ;
    ] ;
  rdfs:subClassOf [
      rdf:type owl:Restriction ;
      owl:cardinality "1"^^xsd:int ;
      owl:onProperty iapd-sec-cr:rgltrCd ;
    ] ;
  rdfs:subClassOf [
      rdf:type owl:Restriction ;
      owl:maxCardinality "1"^^xsd:int ;
      owl:onProperty iapd-sec-cr:dt ;
    ] ;
  rdfs:subClassOf [
      rdf:type owl:Restriction ;
      owl:maxCardinality "1"^^xsd:int ;
      owl:onProperty iapd-sec-cr:st ;
    ] ;
.
iapd-sec-cr:Part1AType
  rdf:type owl:Class ;
  sxml:tag "Part1AType" ;
  rdfs:comment """Here is a full list of populated references:
Object Property				Range (target class)
iapd-sec-cr:item1Ref	iapd-sec-cr:Item1Type
iapd-sec-cr:item2ARef	iapd-sec-cr:Item2AType
iapd-sec-cr:item2BRef	iapd-sec-cr:Item2BType
iapd-sec-cr:item3ARef	iapd-sec-cr:Item3AType
iapd-sec-cr:item3BRef	iapd-sec-cr:Item3BType
iapd-sec-cr:item3CRef	iapd-sec-cr:Item3CType
iapd-sec-cr:item5ARef	iapd-sec-cr:Item5AType
iapd-sec-cr:item5BRef	iapd-sec-cr:Item5BType
iapd-sec-cr:item5CRef	iapd-sec-cr:Item5CType
iapd-sec-cr:item5DRef	iapd-sec-cr:Item5DType
iapd-sec-cr:item5ERef	iapd-sec-cr:Item5EType
iapd-sec-cr:item5FRef	iapd-sec-cr:Item5FType
iapd-sec-cr:item5GRef	iapd-sec-cr:Item5GType
iapd-sec-cr:item5HRef	iapd-sec-cr:Item5HType
iapd-sec-cr:item5IRef		iapd-sec-cr:Item5IType
iapd-sec-cr:item5JRef		iapd-sec-cr:Item5JType
iapd-sec-cr:item6ARef	iapd-sec-cr:Item6AType
iapd-sec-cr:item6BRef	iapd-sec-cr:Item6BType
iapd-sec-cr:item7ARef	iapd-sec-cr:Item7AType
iapd-sec-cr:item7BRef	iapd-sec-cr:Item7BType
iapd-sec-cr:item8ARef	iapd-sec-cr:Item8AType
iapd-sec-cr:item8BRef	iapd-sec-cr:Item8BType
iapd-sec-cr:item8CRef	iapd-sec-cr:Item8CType
iapd-sec-cr:item8DRef	iapd-sec-cr:Item8DType
iapd-sec-cr:item8ERef	iapd-sec-cr:Item8EType
iapd-sec-cr:item8FRef	iapd-sec-cr:Item8FType
iapd-sec-cr:item8GRef	iapd-sec-cr:Item8GType
iapd-sec-cr:item8HRef	iapd-sec-cr:Item8HType
iapd-sec-cr:item8IRef		iapd-sec-cr:Item8IType
iapd-sec-cr:item9ARef	iapd-sec-cr:Item9A1Type
iapd-sec-cr:item9BRef	iapd-sec-cr:Item9BType
iapd-sec-cr:item9CRef	iapd-sec-cr:Item9CType
iapd-sec-cr:item9DRef	iapd-sec-cr:Item9DType
iapd-sec-cr:item9ERef	iapd-sec-cr:Item9EType
iapd-sec-cr:item9FRef	iapd-sec-cr:Item9FType
iapd-sec-cr:item10ARef	iapd-sec-cr:Item10AType
iapd-sec-cr:item11ARef	iapd-sec-cr:Item11AType
iapd-sec-cr:item11BRef	iapd-sec-cr:Item11BType
iapd-sec-cr:item11CRef	iapd-sec-cr:Item11CType
iapd-sec-cr:item11DRef	iapd-sec-cr:Item11DType
iapd-sec-cr:item11ERef	iapd-sec-cr:Item11EType
iapd-sec-cr:item11FRef	iapd-sec-cr:Item11FType
iapd-sec-cr:item11GRef	iapd-sec-cr:Item11GType
iapd-sec-cr:item11HRef	iapd-sec-cr:Item11HType
iapd-sec-cr:item11Ref	iapd-sec-cr:Item11Type
"""^^xsd:string ;
  rdfs:label "Part1AType"^^xsd:string ;
  rdfs:subClassOf iapd-sec-cr:FirmReport ;
  rdfs:subClassOf [
      rdf:type owl:Restriction ;
      sxml:isAttribute "false"^^xsd:boolean ;
      sxml:order "0"^^xsd:int ;
      rdfs:comment "This node has the firm Identifying Information.This maps to Form ADV - Item 1"@en ;
      owl:allValuesFrom iapd-sec-cr:Item1Type ;
      owl:onProperty iapd-sec-cr:item1Ref ;
    ] ;
  rdfs:subClassOf [
      rdf:type owl:Restriction ;
      sxml:isAttribute "false"^^xsd:boolean ;
      sxml:order "1"^^xsd:int ;
      rdfs:comment "This node has the SEC Registration.This maps to Form ADV - Item 2A"@en ;
      owl:allValuesFrom iapd-sec-cr:Item2AType ;
      owl:onProperty iapd-sec-cr:item2ARef ;
    ] ;
  rdfs:subClassOf [
      rdf:type owl:Restriction ;
      sxml:isAttribute "false"^^xsd:boolean ;
      sxml:order "10"^^xsd:int ;
      rdfs:comment "This node has the Information About Your Advisory Business - Compensation Arrangements.This maps to Form ADV - Item 5 -  Q.E"@en ;
      owl:allValuesFrom iapd-sec-cr:Item5EType ;
      owl:onProperty iapd-sec-cr:item5ERef ;
    ] ;
  rdfs:subClassOf [
      rdf:type owl:Restriction ;
      sxml:isAttribute "false"^^xsd:boolean ;
      sxml:order "11"^^xsd:int ;
      rdfs:comment "This node has the Information About Your Advisory Business - Regulatory Assets Under Management.This maps to Form ADV - Item 5 -  Q.F"@en ;
      owl:allValuesFrom iapd-sec-cr:Item5FType ;
      owl:onProperty iapd-sec-cr:item5FRef ;
    ] ;
  rdfs:subClassOf [
      rdf:type owl:Restriction ;
      sxml:isAttribute "false"^^xsd:boolean ;
      sxml:order "12"^^xsd:int ;
      rdfs:comment "This node has the Information About Your Advisory Business - What type(s) of advisory services do you provide?.This maps to Form ADV - Item 5 -  Q.G"@en ;
      owl:allValuesFrom iapd-sec-cr:Item5GType ;
      owl:onProperty iapd-sec-cr:item5GRef ;
    ] ;
  rdfs:subClassOf [
      rdf:type owl:Restriction ;
      sxml:isAttribute "false"^^xsd:boolean ;
      sxml:order "13"^^xsd:int ;
      rdfs:comment "This node has the Information About Your Advisory Business - If you provide financial planning services, to how many clients did you provide these services during your last fiscal year?.This maps to Form ADV - Item 5 -  Q.H"@en ;
      owl:allValuesFrom iapd-sec-cr:Item5HType ;
      owl:onProperty iapd-sec-cr:item5HRef ;
    ] ;
  rdfs:subClassOf [
      rdf:type owl:Restriction ;
      sxml:isAttribute "false"^^xsd:boolean ;
      sxml:order "14"^^xsd:int ;
      rdfs:comment "This node has the Information About Your Advisory Business - wrap fee program.This maps to Form ADV - Item 5 -  Q.I"@en ;
      owl:allValuesFrom iapd-sec-cr:Item5IType ;
      owl:onProperty iapd-sec-cr:item5IRef ;
    ] ;
  rdfs:subClassOf [
      rdf:type owl:Restriction ;
      sxml:isAttribute "false"^^xsd:boolean ;
      sxml:order "15"^^xsd:int ;
      rdfs:comment "This node has the Information About Your Advisory Business - In response to Item 4.B. of Part 2A of Form ADV, do you indicate that you provide investment advice only with respect to limited types of investments? .This maps to Form ADV - Item 5 -  Q.J"@en ;
      owl:allValuesFrom iapd-sec-cr:Item5JType ;
      owl:onProperty iapd-sec-cr:item5JRef ;
    ] ;
  rdfs:subClassOf [
      rdf:type owl:Restriction ;
      sxml:isAttribute "false"^^xsd:boolean ;
      sxml:order "16"^^xsd:int ;
      rdfs:comment "This node has the Other Business Activities - You are actively engaged in business as a?.This maps to Form ADV - Item 6 -  Q.A"@en ;
      owl:allValuesFrom iapd-sec-cr:Item6AType ;
      owl:onProperty iapd-sec-cr:item6ARef ;
    ] ;
  rdfs:subClassOf [
      rdf:type owl:Restriction ;
      sxml:isAttribute "false"^^xsd:boolean ;
      sxml:order "17"^^xsd:int ;
      rdfs:comment "This node has the Other Business Activities.This maps to Form ADV - Item 6 -  Q.B.1 to  Q.B.3"@en ;
      owl:allValuesFrom iapd-sec-cr:Item6BType ;
      owl:onProperty iapd-sec-cr:item6BRef ;
    ] ;
  rdfs:subClassOf [
      rdf:type owl:Restriction ;
      sxml:isAttribute "false"^^xsd:boolean ;
      sxml:order "18"^^xsd:int ;
      rdfs:comment """This node has the Financial Industry Affiliations -
            This part of Item 7 requires you to provide information about you and your related persons, including foreign affiliates. Your related persons are all of your advisory affiliates and any person that is under common control with you.
            You have a related person that is a?. This maps to Form ADV - Item 7 - Q.A"""@en ;
      owl:allValuesFrom iapd-sec-cr:Item7AType ;
      owl:onProperty iapd-sec-cr:item7ARef ;
    ] ;
  rdfs:subClassOf [
      rdf:type owl:Restriction ;
      sxml:isAttribute "false"^^xsd:boolean ;
      sxml:order "19"^^xsd:int ;
      rdfs:comment """This node has the Financial Industry Affiliations - Are you an adviser to any private fund?
            This maps to Form ADV - Item 7 - Q.B"""@en ;
      owl:allValuesFrom iapd-sec-cr:Item7BType ;
      owl:onProperty iapd-sec-cr:item7BRef ;
    ] ;
  rdfs:subClassOf [
      rdf:type owl:Restriction ;
      sxml:isAttribute "false"^^xsd:boolean ;
      sxml:order "2"^^xsd:int ;
      rdfs:comment "This node has the SEC Registration.This maps to Form ADV - Item 2B"@en ;
      owl:allValuesFrom iapd-sec-cr:Item2BType ;
      owl:onProperty iapd-sec-cr:item2BRef ;
    ] ;
  rdfs:subClassOf [
      rdf:type owl:Restriction ;
      sxml:isAttribute "false"^^xsd:boolean ;
      sxml:order "20"^^xsd:int ;
      rdfs:comment "This node has the Participation or Interest in Client Transactions - Proprietary Interest in Client Transactions. This maps to Form ADV - Item 8 - Q.A.1 to Q.A.3"@en ;
      owl:allValuesFrom iapd-sec-cr:Item8AType ;
      owl:onProperty iapd-sec-cr:item8ARef ;
    ] ;
  rdfs:subClassOf [
      rdf:type owl:Restriction ;
      sxml:isAttribute "false"^^xsd:boolean ;
      sxml:order "21"^^xsd:int ;
      rdfs:comment "This node has the Participation or Interest in Client Transactions - Sales Interest in Client Transactions. This maps to Form ADV - Item 8 - Q.B.1 to Q.B.3"@en ;
      owl:allValuesFrom iapd-sec-cr:Item8BType ;
      owl:onProperty iapd-sec-cr:item8BRef ;
    ] ;
  rdfs:subClassOf [
      rdf:type owl:Restriction ;
      sxml:isAttribute "false"^^xsd:boolean ;
      sxml:order "22"^^xsd:int ;
      rdfs:comment "This node has the Participation or Interest in Client Transactions - Investment or Brokerage Discretion. This maps to Form ADV - Item 8 - Q.C.1 to Q.C.4"@en ;
      owl:allValuesFrom iapd-sec-cr:Item8CType ;
      owl:onProperty iapd-sec-cr:item8CRef ;
    ] ;
  rdfs:subClassOf [
      rdf:type owl:Restriction ;
      sxml:isAttribute "false"^^xsd:boolean ;
      sxml:order "23"^^xsd:int ;
      rdfs:comment "This node has the Participation or Interest in Client Transactions - Investment or Brokerage Discretion. This maps to Form ADV - Item 8 - Q.D"@en ;
      owl:allValuesFrom iapd-sec-cr:Item8DType ;
      owl:onProperty iapd-sec-cr:item8DRef ;
    ] ;
  rdfs:subClassOf [
      rdf:type owl:Restriction ;
      sxml:isAttribute "false"^^xsd:boolean ;
      sxml:order "24"^^xsd:int ;
      rdfs:comment "This node has the Participation or Interest in Client Transactions - Investment or Brokerage Discretion. This maps to Form ADV - Item 8 - Q.E"@en ;
      owl:allValuesFrom iapd-sec-cr:Item8EType ;
      owl:onProperty iapd-sec-cr:item8ERef ;
    ] ;
  rdfs:subClassOf [
      rdf:type owl:Restriction ;
      sxml:isAttribute "false"^^xsd:boolean ;
      sxml:order "25"^^xsd:int ;
      rdfs:comment "This node has the Participation or Interest in Client Transactions - Investment or Brokerage Discretion. This maps to Form ADV - Item 8 - Q.F"@en ;
      owl:allValuesFrom iapd-sec-cr:Item8FType ;
      owl:onProperty iapd-sec-cr:item8FRef ;
    ] ;
  rdfs:subClassOf [
      rdf:type owl:Restriction ;
      sxml:isAttribute "false"^^xsd:boolean ;
      sxml:order "26"^^xsd:int ;
      rdfs:comment "This node has the Participation or Interest in Client Transactions - Investment or Brokerage Discretion. This maps to Form ADV - Item 8 - Q.G.1 to Q.G.2"@en ;
      owl:allValuesFrom iapd-sec-cr:Item8GType ;
      owl:onProperty iapd-sec-cr:item8GRef ;
    ] ;
  rdfs:subClassOf [
      rdf:type owl:Restriction ;
      sxml:isAttribute "false"^^xsd:boolean ;
      sxml:order "27"^^xsd:int ;
      rdfs:comment "This node has the Participation or Interest in Client Transactions- Investment or Brokerage Discretion. This maps to Form ADV - Item 8 - Q.H"@en ;
      owl:allValuesFrom iapd-sec-cr:Item8HType ;
      owl:onProperty iapd-sec-cr:item8HRef ;
    ] ;
  rdfs:subClassOf [
      rdf:type owl:Restriction ;
      sxml:isAttribute "false"^^xsd:boolean ;
      sxml:order "28"^^xsd:int ;
      rdfs:comment "This node has the Participation or Interest in Client Transactions - Investment or Brokerage Discretion. This maps to Form ADV - Item 8 - Q.I"@en ;
      owl:allValuesFrom iapd-sec-cr:Item8IType ;
      owl:onProperty iapd-sec-cr:item8IRef ;
    ] ;
  rdfs:subClassOf [
      rdf:type owl:Restriction ;
      sxml:isAttribute "false"^^xsd:boolean ;
      sxml:order "29"^^xsd:int ;
      rdfs:comment "This node has the Custody.This maps to Form ADV - Item 9 - Q.A.1 and Q.A.2"@en ;
      owl:allValuesFrom iapd-sec-cr:Item9A1Type ;
      owl:onProperty iapd-sec-cr:item9ARef ;
    ] ;
  rdfs:subClassOf [
      rdf:type owl:Restriction ;
      sxml:isAttribute "false"^^xsd:boolean ;
      sxml:order "3"^^xsd:int ;
      rdfs:comment "This node has the Form of Organization - How are you organized?. This maps to Form ADV - Item 3 -  Q.A"@en ;
      owl:allValuesFrom iapd-sec-cr:Item3AType ;
      owl:onProperty iapd-sec-cr:item3ARef ;
    ] ;
  rdfs:subClassOf [
      rdf:type owl:Restriction ;
      sxml:isAttribute "false"^^xsd:boolean ;
      sxml:order "30"^^xsd:int ;
      rdfs:comment "This node has the Custody.This maps to Form ADV - Item 9 - Q.B.1 and Q.B.2"@en ;
      owl:allValuesFrom iapd-sec-cr:Item9BType ;
      owl:onProperty iapd-sec-cr:item9BRef ;
    ] ;
  rdfs:subClassOf [
      rdf:type owl:Restriction ;
      sxml:isAttribute "false"^^xsd:boolean ;
      sxml:order "31"^^xsd:int ;
      rdfs:comment "This node has the Custody.This maps to Form ADV - Item 9 - Q.C.1 to Q.C.4"@en ;
      owl:allValuesFrom iapd-sec-cr:Item9CType ;
      owl:onProperty iapd-sec-cr:item9CRef ;
    ] ;
  rdfs:subClassOf [
      rdf:type owl:Restriction ;
      sxml:isAttribute "false"^^xsd:boolean ;
      sxml:order "32"^^xsd:int ;
      rdfs:comment "This node has the Custody.This maps to Form ADV - Item 9 - Q.D.1 and Q.D.2"@en ;
      owl:allValuesFrom iapd-sec-cr:Item9DType ;
      owl:onProperty iapd-sec-cr:item9DRef ;
    ] ;
  rdfs:subClassOf [
      rdf:type owl:Restriction ;
      sxml:isAttribute "false"^^xsd:boolean ;
      sxml:order "33"^^xsd:int ;
      rdfs:comment "This node has the Custody.This maps to Form ADV - Item 9 - Q.E"@en ;
      owl:allValuesFrom iapd-sec-cr:Item9EType ;
      owl:onProperty iapd-sec-cr:item9ERef ;
    ] ;
  rdfs:subClassOf [
      rdf:type owl:Restriction ;
      sxml:isAttribute "false"^^xsd:boolean ;
      sxml:order "34"^^xsd:int ;
      rdfs:comment "This node has the Custody.This maps to Form ADV - Item 9 - Q.F"@en ;
      owl:allValuesFrom iapd-sec-cr:Item9FType ;
      owl:onProperty iapd-sec-cr:item9FRef ;
    ] ;
  rdfs:subClassOf [
      rdf:type owl:Restriction ;
      sxml:isAttribute "false"^^xsd:boolean ;
      sxml:order "35"^^xsd:int ;
      rdfs:comment "This node has Control Persons details.This maps to Form ADV - Item 10 - Q.A and Q.B"@en ;
      owl:allValuesFrom iapd-sec-cr:Item10AType ;
      owl:onProperty iapd-sec-cr:item10ARef ;
    ] ;
  rdfs:subClassOf [
      rdf:type owl:Restriction ;
      sxml:isAttribute "false"^^xsd:boolean ;
      sxml:order "36"^^xsd:int ;
      rdfs:comment "This node has Disclosure Information.This maps to Form ADV - Item 11"@en ;
      owl:allValuesFrom iapd-sec-cr:Item11Type ;
      owl:onProperty iapd-sec-cr:item11Ref ;
    ] ;
  rdfs:subClassOf [
      rdf:type owl:Restriction ;
      sxml:isAttribute "false"^^xsd:boolean ;
      sxml:order "37"^^xsd:int ;
      rdfs:comment "This node has Disclosure Information - Criminal Action DRP.This maps to Form ADV - Item 11 - Q.A"@en ;
      owl:allValuesFrom iapd-sec-cr:Item11AType ;
      owl:onProperty iapd-sec-cr:item11ARef ;
    ] ;
  rdfs:subClassOf [
      rdf:type owl:Restriction ;
      sxml:isAttribute "false"^^xsd:boolean ;
      sxml:order "38"^^xsd:int ;
      rdfs:comment "This node has Disclosure Information - advisory affiliate.This maps to Form ADV - Item 11 - Q.B"@en ;
      owl:allValuesFrom iapd-sec-cr:Item11BType ;
      owl:onProperty iapd-sec-cr:item11BRef ;
    ] ;
  rdfs:subClassOf [
      rdf:type owl:Restriction ;
      sxml:isAttribute "false"^^xsd:boolean ;
      sxml:order "39"^^xsd:int ;
      rdfs:comment "This node has Disclosure Information - Regulatory Action DRP - Has the SEC or the Commodity Futures Trading Commission (CFTC) ever.This maps to Form ADV - Item 11 - Q.C"@en ;
      owl:allValuesFrom iapd-sec-cr:Item11CType ;
      owl:onProperty iapd-sec-cr:item11CRef ;
    ] ;
  rdfs:subClassOf [
      rdf:type owl:Restriction ;
      sxml:isAttribute "false"^^xsd:boolean ;
      sxml:order "4"^^xsd:int ;
      rdfs:comment "This node has the Form of Organization - In what month does your fiscal year end each year?. This maps to Form ADV - Item 3 -  Q.B"@en ;
      owl:allValuesFrom iapd-sec-cr:Item3BType ;
      owl:onProperty iapd-sec-cr:item3BRef ;
    ] ;
  rdfs:subClassOf [
      rdf:type owl:Restriction ;
      sxml:isAttribute "false"^^xsd:boolean ;
      sxml:order "40"^^xsd:int ;
      rdfs:comment "This node has Disclosure Information - Regulatory Action DRP - Has any other federal regulatory agency, any state regulatory agency, or any foreign financial regulatory authority.This maps to Form ADV - Item 11 - Q.D"@en ;
      owl:allValuesFrom iapd-sec-cr:Item11DType ;
      owl:onProperty iapd-sec-cr:item11DRef ;
    ] ;
  rdfs:subClassOf [
      rdf:type owl:Restriction ;
      sxml:isAttribute "false"^^xsd:boolean ;
      sxml:order "41"^^xsd:int ;
      rdfs:comment "This node has Disclosure Information - Regulatory Action DRP - Has any self-regulatory organization or commodities exchange ever.This maps to Form ADV - Item 11 - Q.E"@en ;
      owl:allValuesFrom iapd-sec-cr:Item11EType ;
      owl:onProperty iapd-sec-cr:item11ERef ;
    ] ;
  rdfs:subClassOf [
      rdf:type owl:Restriction ;
      sxml:isAttribute "false"^^xsd:boolean ;
      sxml:order "42"^^xsd:int ;
      rdfs:comment "This node has Disclosure Information - Regulatory Action DRP - Has an authorization to act as an attorney, accountant, or federal contractor granted to you or any advisory affiliate ever been revoked or suspended.This maps to Form ADV - Item 11 - Q.F"@en ;
      owl:allValuesFrom iapd-sec-cr:Item11FType ;
      owl:onProperty iapd-sec-cr:item11FRef ;
    ] ;
  rdfs:subClassOf [
      rdf:type owl:Restriction ;
      sxml:isAttribute "false"^^xsd:boolean ;
      sxml:order "43"^^xsd:int ;
      rdfs:comment "This node has Disclosure Information - Regulatory Action DRP - advisory affiliate .This maps to Form ADV - Item 11 - Q.G"@en ;
      owl:allValuesFrom iapd-sec-cr:Item11GType ;
      owl:onProperty iapd-sec-cr:item11GRef ;
    ] ;
  rdfs:subClassOf [
      rdf:type owl:Restriction ;
      sxml:isAttribute "false"^^xsd:boolean ;
      sxml:order "44"^^xsd:int ;
      rdfs:comment "This node has Disclosure Information - Civil Judicial Action DRP.This maps to Form ADV - Item 11 - Q.H"@en ;
      owl:allValuesFrom iapd-sec-cr:Item11HType ;
      owl:onProperty iapd-sec-cr:item11HRef ;
    ] ;
  rdfs:subClassOf [
      rdf:type owl:Restriction ;
      sxml:isAttribute "false"^^xsd:boolean ;
      sxml:order "5"^^xsd:int ;
      rdfs:comment "This node has the Form of Organization - Under the laws of what state or country are you organized?. This maps to Form ADV - Item 3 -  Q.C"@en ;
      owl:allValuesFrom iapd-sec-cr:Item3CType ;
      owl:onProperty iapd-sec-cr:item3CRef ;
    ] ;
  rdfs:subClassOf [
      rdf:type owl:Restriction ;
      sxml:isAttribute "false"^^xsd:boolean ;
      sxml:order "6"^^xsd:int ;
      rdfs:comment "This node has the Information About Your Advisory Business - Approximately how many employees do you have? Include full- and part-time employees but do not include any clerical workers. This maps to Form ADV - Item 5 -  Q.A"@en ;
      owl:allValuesFrom iapd-sec-cr:Item5AType ;
      owl:onProperty iapd-sec-cr:item5ARef ;
    ] ;
  rdfs:subClassOf [
      rdf:type owl:Restriction ;
      sxml:isAttribute "false"^^xsd:boolean ;
      sxml:order "7"^^xsd:int ;
      rdfs:comment "This node has the Information About Your Advisory Business - Approximately how many of the employees reported in 5.A.This maps to Form ADV - Item 5 -  Q.B"@en ;
      owl:allValuesFrom iapd-sec-cr:Item5BType ;
      owl:onProperty iapd-sec-cr:item5BRef ;
    ] ;
  rdfs:subClassOf [
      rdf:type owl:Restriction ;
      sxml:isAttribute "false"^^xsd:boolean ;
      sxml:order "8"^^xsd:int ;
      rdfs:comment "This node has the Information About Your Advisory Business - Clients.This maps to Form ADV - Item 5 -  Q.C.1 and Q.C.2"@en ;
      owl:allValuesFrom iapd-sec-cr:Item5CType ;
      owl:onProperty iapd-sec-cr:item5CRef ;
    ] ;
  rdfs:subClassOf [
      rdf:type owl:Restriction ;
      sxml:isAttribute "false"^^xsd:boolean ;
      sxml:order "9"^^xsd:int ;
      rdfs:comment "This node has the Information About Your Advisory Business - Clients.This maps to Form ADV - Item 5 -  Q.D.1 and Q.D.2"@en ;
      owl:allValuesFrom iapd-sec-cr:Item5DType ;
      owl:onProperty iapd-sec-cr:item5DRef ;
    ] ;
  rdfs:subClassOf [
      rdf:type owl:Restriction ;
      owl:maxCardinality "1"^^xsd:int ;
      owl:onProperty iapd-sec-cr:item10ARef ;
    ] ;
  rdfs:subClassOf [
      rdf:type owl:Restriction ;
      owl:maxCardinality "1"^^xsd:int ;
      owl:onProperty iapd-sec-cr:item11ARef ;
    ] ;
  rdfs:subClassOf [
      rdf:type owl:Restriction ;
      owl:maxCardinality "1"^^xsd:int ;
      owl:onProperty iapd-sec-cr:item11BRef ;
    ] ;
  rdfs:subClassOf [
      rdf:type owl:Restriction ;
      owl:maxCardinality "1"^^xsd:int ;
      owl:onProperty iapd-sec-cr:item11CRef ;
    ] ;
  rdfs:subClassOf [
      rdf:type owl:Restriction ;
      owl:maxCardinality "1"^^xsd:int ;
      owl:onProperty iapd-sec-cr:item11DRef ;
    ] ;
  rdfs:subClassOf [
      rdf:type owl:Restriction ;
      owl:maxCardinality "1"^^xsd:int ;
      owl:onProperty iapd-sec-cr:item11ERef ;
    ] ;
  rdfs:subClassOf [
      rdf:type owl:Restriction ;
      owl:maxCardinality "1"^^xsd:int ;
      owl:onProperty iapd-sec-cr:item11FRef ;
    ] ;
  rdfs:subClassOf [
      rdf:type owl:Restriction ;
      owl:maxCardinality "1"^^xsd:int ;
      owl:onProperty iapd-sec-cr:item11GRef ;
    ] ;
  rdfs:subClassOf [
      rdf:type owl:Restriction ;
      owl:maxCardinality "1"^^xsd:int ;
      owl:onProperty iapd-sec-cr:item11HRef ;
    ] ;
  rdfs:subClassOf [
      rdf:type owl:Restriction ;
      owl:maxCardinality "1"^^xsd:int ;
      owl:onProperty iapd-sec-cr:item11Ref ;
    ] ;
  rdfs:subClassOf [
      rdf:type owl:Restriction ;
      owl:maxCardinality "1"^^xsd:int ;
      owl:onProperty iapd-sec-cr:item1Ref ;
    ] ;
  rdfs:subClassOf [
      rdf:type owl:Restriction ;
      owl:maxCardinality "1"^^xsd:int ;
      owl:onProperty iapd-sec-cr:item2ARef ;
    ] ;
  rdfs:subClassOf [
      rdf:type owl:Restriction ;
      owl:maxCardinality "1"^^xsd:int ;
      owl:onProperty iapd-sec-cr:item2BRef ;
    ] ;
  rdfs:subClassOf [
      rdf:type owl:Restriction ;
      owl:maxCardinality "1"^^xsd:int ;
      owl:onProperty iapd-sec-cr:item3ARef ;
    ] ;
  rdfs:subClassOf [
      rdf:type owl:Restriction ;
      owl:maxCardinality "1"^^xsd:int ;
      owl:onProperty iapd-sec-cr:item3BRef ;
    ] ;
  rdfs:subClassOf [
      rdf:type owl:Restriction ;
      owl:maxCardinality "1"^^xsd:int ;
      owl:onProperty iapd-sec-cr:item3CRef ;
    ] ;
  rdfs:subClassOf [
      rdf:type owl:Restriction ;
      owl:maxCardinality "1"^^xsd:int ;
      owl:onProperty iapd-sec-cr:item5ARef ;
    ] ;
  rdfs:subClassOf [
      rdf:type owl:Restriction ;
      owl:maxCardinality "1"^^xsd:int ;
      owl:onProperty iapd-sec-cr:item5BRef ;
    ] ;
  rdfs:subClassOf [
      rdf:type owl:Restriction ;
      owl:maxCardinality "1"^^xsd:int ;
      owl:onProperty iapd-sec-cr:item5CRef ;
    ] ;
  rdfs:subClassOf [
      rdf:type owl:Restriction ;
      owl:maxCardinality "1"^^xsd:int ;
      owl:onProperty iapd-sec-cr:item5DRef ;
    ] ;
  rdfs:subClassOf [
      rdf:type owl:Restriction ;
      owl:maxCardinality "1"^^xsd:int ;
      owl:onProperty iapd-sec-cr:item5ERef ;
    ] ;
  rdfs:subClassOf [
      rdf:type owl:Restriction ;
      owl:maxCardinality "1"^^xsd:int ;
      owl:onProperty iapd-sec-cr:item5FRef ;
    ] ;
  rdfs:subClassOf [
      rdf:type owl:Restriction ;
      owl:maxCardinality "1"^^xsd:int ;
      owl:onProperty iapd-sec-cr:item5GRef ;
    ] ;
  rdfs:subClassOf [
      rdf:type owl:Restriction ;
      owl:maxCardinality "1"^^xsd:int ;
      owl:onProperty iapd-sec-cr:item5HRef ;
    ] ;
  rdfs:subClassOf [
      rdf:type owl:Restriction ;
      owl:maxCardinality "1"^^xsd:int ;
      owl:onProperty iapd-sec-cr:item5IRef ;
    ] ;
  rdfs:subClassOf [
      rdf:type owl:Restriction ;
      owl:maxCardinality "1"^^xsd:int ;
      owl:onProperty iapd-sec-cr:item5JRef ;
    ] ;
  rdfs:subClassOf [
      rdf:type owl:Restriction ;
      owl:maxCardinality "1"^^xsd:int ;
      owl:onProperty iapd-sec-cr:item6ARef ;
    ] ;
  rdfs:subClassOf [
      rdf:type owl:Restriction ;
      owl:maxCardinality "1"^^xsd:int ;
      owl:onProperty iapd-sec-cr:item6BRef ;
    ] ;
  rdfs:subClassOf [
      rdf:type owl:Restriction ;
      owl:maxCardinality "1"^^xsd:int ;
      owl:onProperty iapd-sec-cr:item7ARef ;
    ] ;
  rdfs:subClassOf [
      rdf:type owl:Restriction ;
      owl:maxCardinality "1"^^xsd:int ;
      owl:onProperty iapd-sec-cr:item7BRef ;
    ] ;
  rdfs:subClassOf [
      rdf:type owl:Restriction ;
      owl:maxCardinality "1"^^xsd:int ;
      owl:onProperty iapd-sec-cr:item8ARef ;
    ] ;
  rdfs:subClassOf [
      rdf:type owl:Restriction ;
      owl:maxCardinality "1"^^xsd:int ;
      owl:onProperty iapd-sec-cr:item8BRef ;
    ] ;
  rdfs:subClassOf [
      rdf:type owl:Restriction ;
      owl:maxCardinality "1"^^xsd:int ;
      owl:onProperty iapd-sec-cr:item8CRef ;
    ] ;
  rdfs:subClassOf [
      rdf:type owl:Restriction ;
      owl:maxCardinality "1"^^xsd:int ;
      owl:onProperty iapd-sec-cr:item8DRef ;
    ] ;
  rdfs:subClassOf [
      rdf:type owl:Restriction ;
      owl:maxCardinality "1"^^xsd:int ;
      owl:onProperty iapd-sec-cr:item8ERef ;
    ] ;
  rdfs:subClassOf [
      rdf:type owl:Restriction ;
      owl:maxCardinality "1"^^xsd:int ;
      owl:onProperty iapd-sec-cr:item8FRef ;
    ] ;
  rdfs:subClassOf [
      rdf:type owl:Restriction ;
      owl:maxCardinality "1"^^xsd:int ;
      owl:onProperty iapd-sec-cr:item8GRef ;
    ] ;
  rdfs:subClassOf [
      rdf:type owl:Restriction ;
      owl:maxCardinality "1"^^xsd:int ;
      owl:onProperty iapd-sec-cr:item8HRef ;
    ] ;
  rdfs:subClassOf [
      rdf:type owl:Restriction ;
      owl:maxCardinality "1"^^xsd:int ;
      owl:onProperty iapd-sec-cr:item8IRef ;
    ] ;
  rdfs:subClassOf [
      rdf:type owl:Restriction ;
      owl:maxCardinality "1"^^xsd:int ;
      owl:onProperty iapd-sec-cr:item9ARef ;
    ] ;
  rdfs:subClassOf [
      rdf:type owl:Restriction ;
      owl:maxCardinality "1"^^xsd:int ;
      owl:onProperty iapd-sec-cr:item9BRef ;
    ] ;
  rdfs:subClassOf [
      rdf:type owl:Restriction ;
      owl:maxCardinality "1"^^xsd:int ;
      owl:onProperty iapd-sec-cr:item9CRef ;
    ] ;
  rdfs:subClassOf [
      rdf:type owl:Restriction ;
      owl:maxCardinality "1"^^xsd:int ;
      owl:onProperty iapd-sec-cr:item9DRef ;
    ] ;
  rdfs:subClassOf [
      rdf:type owl:Restriction ;
      owl:maxCardinality "1"^^xsd:int ;
      owl:onProperty iapd-sec-cr:item9ERef ;
    ] ;
  rdfs:subClassOf [
      rdf:type owl:Restriction ;
      owl:maxCardinality "1"^^xsd:int ;
      owl:onProperty iapd-sec-cr:item9FRef ;
    ] ;
  skos:definition """Part 1A has references to the firm's response to items in the form:
1) Identifying information
2) Registration
3) Organization
5) Employees & Advisory business
6) Other business activities and affiliations
7) Related persons
8) Participation or interest in client transactions
9) Custody business
10) Control persons
11) Disclosure information"""^^xsd:string ;
.
iapd-sec-cr:RgstnType
  rdf:type owl:Class ;
  sxml:tag "RgstnType" ;
  rdfs:label "Rgstn type"^^xsd:string ;
  rdfs:subClassOf iapd-sec-cr:FirmReport ;
  rdfs:subClassOf [
      rdf:type owl:Restriction ;
      sxml:isAttribute "true"^^xsd:boolean ;
      rdfs:comment """The FirmType node has the detail if firm is Registered or an ERA. 
          Displays Registered for registered firms. Displays ERA for Exempt Reporting Adviser firms."""@en ;
      owl:allValuesFrom iapd-sec-cr:FirmCdType ;
      owl:onProperty iapd-sec-cr:firmType ;
    ] ;
  rdfs:subClassOf [
      rdf:type owl:Restriction ;
      sxml:isAttribute "true"^^xsd:boolean ;
      rdfs:comment "The dt node has the firm's effective date of their SEC registration or the firm's ERA reporting filing date at the time of report generation."@en ;
      owl:allValuesFrom xsd:date ;
      owl:onProperty iapd-sec-cr:dt ;
    ] ;
  rdfs:subClassOf [
      rdf:type owl:Restriction ;
      sxml:isAttribute "true"^^xsd:boolean ;
      rdfs:comment "The st node has the firm's registration status with the SEC or the firm's ERA 'status' at the time of report generation"@en ;
      owl:allValuesFrom iapd-sec-cr:SecRgstnStType ;
      owl:onProperty iapd-sec-cr:st ;
    ] ;
  rdfs:subClassOf [
      rdf:type owl:Restriction ;
      owl:cardinality "1"^^xsd:int ;
      owl:onProperty iapd-sec-cr:dt ;
    ] ;
  rdfs:subClassOf [
      rdf:type owl:Restriction ;
      owl:cardinality "1"^^xsd:int ;
      owl:onProperty iapd-sec-cr:firmType ;
    ] ;
  rdfs:subClassOf [
      rdf:type owl:Restriction ;
      owl:cardinality "1"^^xsd:int ;
      owl:onProperty iapd-sec-cr:st ;
    ] ;
  skos:definition """The firm's registration status:
Firm code - Registered or Exempt Reporting Adviser
Registration status - APPROVED, ACTIVE, ACTIVE-120, SUSPENDED 
Effective date of registration"""^^xsd:string ;
.
iapd-sec-cr:SCT_AK
  rdf:type iapd-sec-cr:StateCdType ;
  dtype:order "0"^^xsd:nonNegativeInteger ;
  dtype:value "AK"^^xsd:NMTOKEN ;
  rdfs:label "AK"^^xsd:string ;
.
iapd-sec-cr:SCT_AL
  rdf:type iapd-sec-cr:StateCdType ;
  dtype:order "1"^^xsd:nonNegativeInteger ;
  dtype:value "AL"^^xsd:NMTOKEN ;
  rdfs:label "AL"^^xsd:string ;
.
iapd-sec-cr:SCT_AR
  rdf:type iapd-sec-cr:StateCdType ;
  dtype:order "2"^^xsd:nonNegativeInteger ;
  dtype:value "AR"^^xsd:NMTOKEN ;
  rdfs:label "AR"^^xsd:string ;
.
iapd-sec-cr:SCT_AZ
  rdf:type iapd-sec-cr:StateCdType ;
  dtype:order "3"^^xsd:nonNegativeInteger ;
  dtype:value "AZ"^^xsd:NMTOKEN ;
  rdfs:label "AZ"^^xsd:string ;
.
iapd-sec-cr:SCT_CA
  rdf:type iapd-sec-cr:StateCdType ;
  dtype:order "4"^^xsd:nonNegativeInteger ;
  dtype:value "CA"^^xsd:NMTOKEN ;
  rdfs:label "CA"^^xsd:string ;
.
iapd-sec-cr:SCT_CO
  rdf:type iapd-sec-cr:StateCdType ;
  dtype:order "5"^^xsd:nonNegativeInteger ;
  dtype:value "CO"^^xsd:NMTOKEN ;
  rdfs:label "CO"^^xsd:string ;
.
iapd-sec-cr:SCT_CT
  rdf:type iapd-sec-cr:StateCdType ;
  dtype:order "6"^^xsd:nonNegativeInteger ;
  dtype:value "CT"^^xsd:NMTOKEN ;
  rdfs:label "CT"^^xsd:string ;
.
iapd-sec-cr:SCT_DC
  rdf:type iapd-sec-cr:StateCdType ;
  dtype:order "7"^^xsd:nonNegativeInteger ;
  dtype:value "DC"^^xsd:NMTOKEN ;
  rdfs:label "DC"^^xsd:string ;
.
iapd-sec-cr:SCT_DE
  rdf:type iapd-sec-cr:StateCdType ;
  dtype:order "8"^^xsd:nonNegativeInteger ;
  dtype:value "DE"^^xsd:NMTOKEN ;
  rdfs:label "DE"^^xsd:string ;
.
iapd-sec-cr:SCT_FL
  rdf:type iapd-sec-cr:StateCdType ;
  dtype:order "9"^^xsd:nonNegativeInteger ;
  dtype:value "FL"^^xsd:NMTOKEN ;
  rdfs:label "FL"^^xsd:string ;
.
iapd-sec-cr:SCT_GA
  rdf:type iapd-sec-cr:StateCdType ;
  dtype:order "10"^^xsd:nonNegativeInteger ;
  dtype:value "GA"^^xsd:NMTOKEN ;
  rdfs:label "GA"^^xsd:string ;
.
iapd-sec-cr:SCT_GU
  rdf:type iapd-sec-cr:StateCdType ;
  dtype:order "11"^^xsd:nonNegativeInteger ;
  dtype:value "GU"^^xsd:NMTOKEN ;
  rdfs:label "GU"^^xsd:string ;
.
iapd-sec-cr:SCT_HI
  rdf:type iapd-sec-cr:StateCdType ;
  dtype:order "12"^^xsd:nonNegativeInteger ;
  dtype:value "HI"^^xsd:NMTOKEN ;
  rdfs:label "HI"^^xsd:string ;
.
iapd-sec-cr:SCT_IA
  rdf:type iapd-sec-cr:StateCdType ;
  dtype:order "13"^^xsd:nonNegativeInteger ;
  dtype:value "IA"^^xsd:NMTOKEN ;
  rdfs:label "IA"^^xsd:string ;
.
iapd-sec-cr:SCT_ID
  rdf:type iapd-sec-cr:StateCdType ;
  dtype:order "14"^^xsd:nonNegativeInteger ;
  dtype:value "ID"^^xsd:NMTOKEN ;
  rdfs:label "ID"^^xsd:string ;
.
iapd-sec-cr:SCT_IL
  rdf:type iapd-sec-cr:StateCdType ;
  dtype:order "15"^^xsd:nonNegativeInteger ;
  dtype:value "IL"^^xsd:NMTOKEN ;
  rdfs:label "IL"^^xsd:string ;
.
iapd-sec-cr:SCT_IN
  rdf:type iapd-sec-cr:StateCdType ;
  dtype:order "16"^^xsd:nonNegativeInteger ;
  dtype:value "IN"^^xsd:NMTOKEN ;
  rdfs:label "IN"^^xsd:string ;
.
iapd-sec-cr:SCT_KS
  rdf:type iapd-sec-cr:StateCdType ;
  dtype:order "17"^^xsd:nonNegativeInteger ;
  dtype:value "KS"^^xsd:NMTOKEN ;
  rdfs:label "KS"^^xsd:string ;
.
iapd-sec-cr:SCT_KY
  rdf:type iapd-sec-cr:StateCdType ;
  dtype:order "18"^^xsd:nonNegativeInteger ;
  dtype:value "KY"^^xsd:NMTOKEN ;
  rdfs:label "KY"^^xsd:string ;
.
iapd-sec-cr:SCT_LA
  rdf:type iapd-sec-cr:StateCdType ;
  dtype:order "19"^^xsd:nonNegativeInteger ;
  dtype:value "LA"^^xsd:NMTOKEN ;
  rdfs:label "LA"^^xsd:string ;
.
iapd-sec-cr:SCT_MA
  rdf:type iapd-sec-cr:StateCdType ;
  dtype:order "20"^^xsd:nonNegativeInteger ;
  dtype:value "MA"^^xsd:NMTOKEN ;
  rdfs:label "MA"^^xsd:string ;
.
iapd-sec-cr:SCT_MD
  rdf:type iapd-sec-cr:StateCdType ;
  dtype:order "21"^^xsd:nonNegativeInteger ;
  dtype:value "MD"^^xsd:NMTOKEN ;
  rdfs:label "MD"^^xsd:string ;
.
iapd-sec-cr:SCT_ME
  rdf:type iapd-sec-cr:StateCdType ;
  dtype:order "22"^^xsd:nonNegativeInteger ;
  dtype:value "ME"^^xsd:NMTOKEN ;
  rdfs:label "ME"^^xsd:string ;
.
iapd-sec-cr:SCT_MI
  rdf:type iapd-sec-cr:StateCdType ;
  dtype:order "23"^^xsd:nonNegativeInteger ;
  dtype:value "MI"^^xsd:NMTOKEN ;
  rdfs:label "MI"^^xsd:string ;
.
iapd-sec-cr:SCT_MN
  rdf:type iapd-sec-cr:StateCdType ;
  dtype:order "24"^^xsd:nonNegativeInteger ;
  dtype:value "MN"^^xsd:NMTOKEN ;
  rdfs:label "MN"^^xsd:string ;
.
iapd-sec-cr:SCT_MO
  rdf:type iapd-sec-cr:StateCdType ;
  dtype:order "25"^^xsd:nonNegativeInteger ;
  dtype:value "MO"^^xsd:NMTOKEN ;
  rdfs:label "MO"^^xsd:string ;
.
iapd-sec-cr:SCT_MS
  rdf:type iapd-sec-cr:StateCdType ;
  dtype:order "26"^^xsd:nonNegativeInteger ;
  dtype:value "MS"^^xsd:NMTOKEN ;
  rdfs:label "MS"^^xsd:string ;
.
iapd-sec-cr:SCT_MT
  rdf:type iapd-sec-cr:StateCdType ;
  dtype:order "27"^^xsd:nonNegativeInteger ;
  dtype:value "MT"^^xsd:NMTOKEN ;
  rdfs:label "MT"^^xsd:string ;
.
iapd-sec-cr:SCT_NC
  rdf:type iapd-sec-cr:StateCdType ;
  dtype:order "28"^^xsd:nonNegativeInteger ;
  dtype:value "NC"^^xsd:NMTOKEN ;
  rdfs:label "NC"^^xsd:string ;
.
iapd-sec-cr:SCT_ND
  rdf:type iapd-sec-cr:StateCdType ;
  dtype:order "29"^^xsd:nonNegativeInteger ;
  dtype:value "ND"^^xsd:NMTOKEN ;
  rdfs:label "ND"^^xsd:string ;
.
iapd-sec-cr:SCT_NE
  rdf:type iapd-sec-cr:StateCdType ;
  dtype:order "30"^^xsd:nonNegativeInteger ;
  dtype:value "NE"^^xsd:NMTOKEN ;
  rdfs:label "NE"^^xsd:string ;
.
iapd-sec-cr:SCT_NH
  rdf:type iapd-sec-cr:StateCdType ;
  dtype:order "31"^^xsd:nonNegativeInteger ;
  dtype:value "NH"^^xsd:NMTOKEN ;
  rdfs:label "NH"^^xsd:string ;
.
iapd-sec-cr:SCT_NJ
  rdf:type iapd-sec-cr:StateCdType ;
  dtype:order "32"^^xsd:nonNegativeInteger ;
  dtype:value "NJ"^^xsd:NMTOKEN ;
  rdfs:label "NJ"^^xsd:string ;
.
iapd-sec-cr:SCT_NM
  rdf:type iapd-sec-cr:StateCdType ;
  dtype:order "33"^^xsd:nonNegativeInteger ;
  dtype:value "NM"^^xsd:NMTOKEN ;
  rdfs:label "NM"^^xsd:string ;
.
iapd-sec-cr:SCT_NV
  rdf:type iapd-sec-cr:StateCdType ;
  dtype:order "34"^^xsd:nonNegativeInteger ;
  dtype:value "NV"^^xsd:NMTOKEN ;
  rdfs:label "NV"^^xsd:string ;
.
iapd-sec-cr:SCT_NY
  rdf:type iapd-sec-cr:StateCdType ;
  dtype:order "35"^^xsd:nonNegativeInteger ;
  dtype:value "NY"^^xsd:NMTOKEN ;
  rdfs:label "NY"^^xsd:string ;
.
iapd-sec-cr:SCT_OH
  rdf:type iapd-sec-cr:StateCdType ;
  dtype:order "36"^^xsd:nonNegativeInteger ;
  dtype:value "OH"^^xsd:NMTOKEN ;
  rdfs:label "OH"^^xsd:string ;
.
iapd-sec-cr:SCT_OK
  rdf:type iapd-sec-cr:StateCdType ;
  dtype:order "37"^^xsd:nonNegativeInteger ;
  dtype:value "OK"^^xsd:NMTOKEN ;
  rdfs:label "OK"^^xsd:string ;
.
iapd-sec-cr:SCT_OR
  rdf:type iapd-sec-cr:StateCdType ;
  dtype:order "38"^^xsd:nonNegativeInteger ;
  dtype:value "OR"^^xsd:NMTOKEN ;
  rdfs:label "OR"^^xsd:string ;
.
iapd-sec-cr:SCT_PA
  rdf:type iapd-sec-cr:StateCdType ;
  dtype:order "39"^^xsd:nonNegativeInteger ;
  dtype:value "PA"^^xsd:NMTOKEN ;
  rdfs:label "PA"^^xsd:string ;
.
iapd-sec-cr:SCT_PR
  rdf:type iapd-sec-cr:StateCdType ;
  dtype:order "40"^^xsd:nonNegativeInteger ;
  dtype:value "PR"^^xsd:NMTOKEN ;
  rdfs:label "PR"^^xsd:string ;
.
iapd-sec-cr:SCT_RI
  rdf:type iapd-sec-cr:StateCdType ;
  dtype:order "41"^^xsd:nonNegativeInteger ;
  dtype:value "RI"^^xsd:NMTOKEN ;
  rdfs:label "RI"^^xsd:string ;
.
iapd-sec-cr:SCT_SC
  rdf:type iapd-sec-cr:StateCdType ;
  dtype:order "42"^^xsd:nonNegativeInteger ;
  dtype:value "SC"^^xsd:NMTOKEN ;
  rdfs:label "SC"^^xsd:string ;
.
iapd-sec-cr:SCT_SD
  rdf:type iapd-sec-cr:StateCdType ;
  dtype:order "43"^^xsd:nonNegativeInteger ;
  dtype:value "SD"^^xsd:NMTOKEN ;
  rdfs:label "SD"^^xsd:string ;
.
iapd-sec-cr:SCT_TN
  rdf:type iapd-sec-cr:StateCdType ;
  dtype:order "44"^^xsd:nonNegativeInteger ;
  dtype:value "TN"^^xsd:NMTOKEN ;
  rdfs:label "TN"^^xsd:string ;
.
iapd-sec-cr:SCT_TX
  rdf:type iapd-sec-cr:StateCdType ;
  dtype:order "45"^^xsd:nonNegativeInteger ;
  dtype:value "TX"^^xsd:NMTOKEN ;
  rdfs:label "TX"^^xsd:string ;
.
iapd-sec-cr:SCT_UT
  rdf:type iapd-sec-cr:StateCdType ;
  dtype:order "46"^^xsd:nonNegativeInteger ;
  dtype:value "UT"^^xsd:NMTOKEN ;
  rdfs:label "UT"^^xsd:string ;
.
iapd-sec-cr:SCT_VA
  rdf:type iapd-sec-cr:StateCdType ;
  dtype:order "47"^^xsd:nonNegativeInteger ;
  dtype:value "VA"^^xsd:NMTOKEN ;
  rdfs:label "VA"^^xsd:string ;
.
iapd-sec-cr:SCT_VI
  rdf:type iapd-sec-cr:StateCdType ;
  dtype:order "53"^^xsd:nonNegativeInteger ;
  dtype:value "VI"^^xsd:NMTOKEN ;
  rdfs:label "VI"^^xsd:string ;
.
iapd-sec-cr:SCT_VT
  rdf:type iapd-sec-cr:StateCdType ;
  dtype:order "48"^^xsd:nonNegativeInteger ;
  dtype:value "VT"^^xsd:NMTOKEN ;
  rdfs:label "VT"^^xsd:string ;
.
iapd-sec-cr:SCT_WA
  rdf:type iapd-sec-cr:StateCdType ;
  dtype:order "49"^^xsd:nonNegativeInteger ;
  dtype:value "WA"^^xsd:NMTOKEN ;
  rdfs:label "WA"^^xsd:string ;
.
iapd-sec-cr:SCT_WI
  rdf:type iapd-sec-cr:StateCdType ;
  dtype:order "50"^^xsd:nonNegativeInteger ;
  dtype:value "WI"^^xsd:NMTOKEN ;
  rdfs:label "WI"^^xsd:string ;
.
iapd-sec-cr:SCT_WV
  rdf:type iapd-sec-cr:StateCdType ;
  dtype:order "51"^^xsd:nonNegativeInteger ;
  dtype:value "WV"^^xsd:NMTOKEN ;
  rdfs:label "WV"^^xsd:string ;
.
iapd-sec-cr:SCT_WY
  rdf:type iapd-sec-cr:StateCdType ;
  dtype:order "52"^^xsd:nonNegativeInteger ;
  dtype:value "WY"^^xsd:NMTOKEN ;
  rdfs:label "WY"^^xsd:string ;
.
iapd-sec-cr:SECFirmType
  rdf:type owl:Class ;
  sxml:tag "SECFirmType" ;
  rdfs:comment """Per report there is one instance of this class for every fiming firm. Object properties connect the instance to the main filing structures:
iapd-sec-cr:filingRef				iapd-sec-cr:FilingType
iapd-sec-cr:formInfoRef			iapd-sec-cr:SECFormInfoType
iapd-sec-cr:infoRef					iapd-sec-cr:SECOrgInfoType
iapd-sec-cr:mailingAddrRef	iapd-sec-cr:AddrType
iapd-sec-cr:mainAddrRef		iapd-sec-cr:AddrType
iapd-sec-cr:noticeFiledRef		iapd-sec-cr:NoticeFiledType
iapd-sec-cr:rgstnRef				iapd-sec-cr:RgstnType"""^^xsd:string ;
  rdfs:label "SECFirm type"^^xsd:string ;
  rdfs:subClassOf iapd-sec-cr:FirmReport ;
  rdfs:subClassOf [
      rdf:type owl:Restriction ;
      sxml:isAttribute "false"^^xsd:boolean ;
      sxml:order "0"^^xsd:int ;
      rdfs:comment "This node contains the organization's information."@en ;
      owl:allValuesFrom iapd-sec-cr:SECOrgInfoType ;
      owl:onProperty iapd-sec-cr:infoRef ;
    ] ;
  rdfs:subClassOf [
      rdf:type owl:Restriction ;
      sxml:isAttribute "false"^^xsd:boolean ;
      sxml:order "1"^^xsd:int ;
      rdfs:comment "This node has the Item 1F Principal Main office address info."@en ;
      owl:allValuesFrom iapd-sec-cr:AddrType ;
      owl:onProperty iapd-sec-cr:mainAddrRef ;
    ] ;
  rdfs:subClassOf [
      rdf:type owl:Restriction ;
      sxml:isAttribute "false"^^xsd:boolean ;
      sxml:order "2"^^xsd:int ;
      rdfs:comment "This node has the Item 1G mailing address info."@en ;
      owl:allValuesFrom iapd-sec-cr:AddrType ;
      owl:onProperty iapd-sec-cr:mailingAddrRef ;
    ] ;
  rdfs:subClassOf [
      rdf:type owl:Restriction ;
      sxml:isAttribute "false"^^xsd:boolean ;
      sxml:order "3"^^xsd:int ;
      rdfs:comment "This node has the firm registration type."@en ;
      owl:allValuesFrom iapd-sec-cr:RgstnType ;
      owl:onProperty iapd-sec-cr:rgstnRef ;
    ] ;
  rdfs:subClassOf [
      rdf:type owl:Restriction ;
      sxml:isAttribute "false"^^xsd:boolean ;
      sxml:order "4"^^xsd:int ;
      rdfs:comment "This node has the active notice filing statuses."@en ;
      owl:allValuesFrom iapd-sec-cr:NoticeFiledType ;
      owl:onProperty iapd-sec-cr:noticeFiledRef ;
    ] ;
  rdfs:subClassOf [
      rdf:type owl:Restriction ;
      sxml:isAttribute "false"^^xsd:boolean ;
      sxml:order "5"^^xsd:int ;
      rdfs:comment "This node has the firm filing info."@en ;
      owl:allValuesFrom iapd-sec-cr:FilingType ;
      owl:onProperty iapd-sec-cr:filingRef ;
    ] ;
  rdfs:subClassOf [
      rdf:type owl:Restriction ;
      sxml:isAttribute "false"^^xsd:boolean ;
      sxml:order "6"^^xsd:int ;
      rdfs:comment "This node has the firm forminfo."@en ;
      owl:allValuesFrom iapd-sec-cr:SECFormInfoType ;
      owl:onProperty iapd-sec-cr:formInfoRef ;
    ] ;
  rdfs:subClassOf [
      rdf:type owl:Restriction ;
      owl:cardinality "1"^^xsd:int ;
      owl:onProperty iapd-sec-cr:infoRef ;
    ] ;
  rdfs:subClassOf [
      rdf:type owl:Restriction ;
      owl:maxCardinality "1"^^xsd:int ;
      owl:onProperty iapd-sec-cr:formInfoRef ;
    ] ;
  rdfs:subClassOf [
      rdf:type owl:Restriction ;
      owl:maxCardinality "1"^^xsd:int ;
      owl:onProperty iapd-sec-cr:mailingAddrRef ;
    ] ;
  rdfs:subClassOf [
      rdf:type owl:Restriction ;
      owl:maxCardinality "1"^^xsd:int ;
      owl:onProperty iapd-sec-cr:mainAddrRef ;
    ] ;
  rdfs:subClassOf [
      rdf:type owl:Restriction ;
      owl:maxCardinality "1"^^xsd:int ;
      owl:onProperty iapd-sec-cr:noticeFiledRef ;
    ] ;
  rdfs:subClassOf [
      rdf:type owl:Restriction ;
      owl:minCardinality "1"^^xsd:int ;
      owl:onProperty iapd-sec-cr:filingRef ;
    ] ;
  rdfs:subClassOf [
      rdf:type owl:Restriction ;
      owl:minCardinality "1"^^xsd:int ;
      owl:onProperty iapd-sec-cr:rgstnRef ;
    ] ;
  skos:definition "The root class for a firm filing with references to filing type, form, organization, addresses, notice and regristration information."^^xsd:string ;
.
iapd-sec-cr:SECFormInfoType
  rdf:type owl:Class ;
  sxml:tag "SECFormInfoType" ;
  rdfs:comment "The class doesn't have any data properties. It is just in between SEC Firm Type and Part 1A."^^xsd:string ;
  rdfs:label "SECForm info type"^^xsd:string ;
  rdfs:subClassOf iapd-sec-cr:FirmReport ;
  rdfs:subClassOf [
      rdf:type owl:Restriction ;
      sxml:isAttribute "false"^^xsd:boolean ;
      sxml:order "0"^^xsd:int ;
      rdfs:comment "This has the form ADV Part1 details"@en ;
      owl:allValuesFrom iapd-sec-cr:Part1AType ;
      owl:onProperty iapd-sec-cr:part1ARef ;
    ] ;
  rdfs:subClassOf [
      rdf:type owl:Restriction ;
      owl:cardinality "1"^^xsd:int ;
      owl:onProperty iapd-sec-cr:part1ARef ;
    ] ;
  skos:definition "The root class for a firm filing with reference to the form Part  1A"^^xsd:string ;
.
iapd-sec-cr:SECOrgInfoType
  rdf:type owl:Class ;
  sxml:tag "SECOrgInfoType" ;
  rdfs:label "SECOrg info type"^^xsd:string ;
  rdfs:subClassOf iapd-sec-cr:FirmReport ;
  rdfs:subClassOf [
      rdf:type owl:Restriction ;
      sxml:isAttribute "true"^^xsd:boolean ;
      rdfs:comment "This node has the Firm's legal name from the IARD composite record. This maps to Form ADV-Item 1 - Q1.a"@en ;
      owl:allValuesFrom iapd-sec-cr:Str64Datatype ;
      owl:onProperty iapd-sec-cr:legalNm ;
    ] ;
  rdfs:subClassOf [
      rdf:type owl:Restriction ;
      sxml:isAttribute "true"^^xsd:boolean ;
      rdfs:comment "This node has the Firm's primary business name from the IARD composite record. This maps to Form ADV-Item 1 - Q1.b"@en ;
      owl:allValuesFrom iapd-sec-cr:Str64Datatype ;
      owl:onProperty iapd-sec-cr:busNm ;
    ] ;
  rdfs:subClassOf [
      rdf:type owl:Restriction ;
      sxml:isAttribute "true"^^xsd:boolean ;
      rdfs:comment "This node has the SEC Region Acronym."@en ;
      owl:allValuesFrom iapd-sec-cr:SECRgnCdType ;
      owl:onProperty iapd-sec-cr:sECRgnCD ;
    ] ;
  rdfs:subClassOf [
      rdf:type owl:Restriction ;
      sxml:isAttribute "true"^^xsd:boolean ;
      rdfs:comment "This node has the SEC firm's CRD number. This maps to Form ADV-Item 1 - Q1.e"@en ;
      owl:allValuesFrom iapd-sec-cr:Int8Datatype ;
      owl:onProperty iapd-sec-cr:firmCrdNb ;
    ] ;
  rdfs:subClassOf [
      rdf:type owl:Restriction ;
      sxml:isAttribute "true"^^xsd:boolean ;
      rdfs:comment "This node has the firm's 801# or 802# from the IARD composite record. This maps to Form ADV-Item 1 - Q1.d"@en ;
      owl:allValuesFrom iapd-sec-cr:Str10Datatype ;
      owl:onProperty iapd-sec-cr:sECNb ;
    ] ;
  rdfs:subClassOf [
      rdf:type owl:Restriction ;
      owl:cardinality "1"^^xsd:int ;
      owl:onProperty iapd-sec-cr:firmCrdNb ;
    ] ;
  rdfs:subClassOf [
      rdf:type owl:Restriction ;
      owl:cardinality "1"^^xsd:int ;
      owl:onProperty iapd-sec-cr:legalNm ;
    ] ;
  rdfs:subClassOf [
      rdf:type owl:Restriction ;
      owl:maxCardinality "1"^^xsd:int ;
      owl:onProperty iapd-sec-cr:busNm ;
    ] ;
  rdfs:subClassOf [
      rdf:type owl:Restriction ;
      owl:maxCardinality "1"^^xsd:int ;
      owl:onProperty iapd-sec-cr:sECNb ;
    ] ;
  rdfs:subClassOf [
      rdf:type owl:Restriction ;
      owl:maxCardinality "1"^^xsd:int ;
      owl:onProperty iapd-sec-cr:sECRgnCD ;
    ] ;
  skos:definition "SEC information about the filing firm's organization: Business & Legal Name, CRD-, ECN-number and the region code."^^xsd:string ;
.
iapd-sec-cr:SECRCT_ARO
  rdf:type iapd-sec-cr:SECRgnCdType ;
  dtype:order "0"^^xsd:nonNegativeInteger ;
  dtype:value "ARO"^^xsd:NMTOKEN ;
  rdfs:label "ARO"^^xsd:string ;
.
iapd-sec-cr:SECRCT_BRO
  rdf:type iapd-sec-cr:SECRgnCdType ;
  dtype:order "1"^^xsd:nonNegativeInteger ;
  dtype:value "BRO"^^xsd:NMTOKEN ;
  rdfs:label "BRO"^^xsd:string ;
.
iapd-sec-cr:SECRCT_CHRO
  rdf:type iapd-sec-cr:SECRgnCdType ;
  dtype:order "4"^^xsd:nonNegativeInteger ;
  dtype:value "CHRO"^^xsd:NMTOKEN ;
  rdfs:label "CHRO"^^xsd:string ;
.
iapd-sec-cr:SECRCT_DRO
  rdf:type iapd-sec-cr:SECRgnCdType ;
  dtype:order "2"^^xsd:nonNegativeInteger ;
  dtype:value "DRO"^^xsd:NMTOKEN ;
  rdfs:label "DRO"^^xsd:string ;
.
iapd-sec-cr:SECRCT_FWRO
  rdf:type iapd-sec-cr:SECRgnCdType ;
  dtype:order "3"^^xsd:nonNegativeInteger ;
  dtype:value "FWRO"^^xsd:NMTOKEN ;
  rdfs:label "FWRO"^^xsd:string ;
.
iapd-sec-cr:SECRCT_HQ
  rdf:type iapd-sec-cr:SECRgnCdType ;
  dtype:order "10"^^xsd:nonNegativeInteger ;
  dtype:value "HQ"^^xsd:NMTOKEN ;
  rdfs:label "HQ"^^xsd:string ;
.
iapd-sec-cr:SECRCT_LARO
  rdf:type iapd-sec-cr:SECRgnCdType ;
  dtype:order "6"^^xsd:nonNegativeInteger ;
  dtype:value "LARO"^^xsd:NMTOKEN ;
  rdfs:label "LARO"^^xsd:string ;
.
iapd-sec-cr:SECRCT_MIRO
  rdf:type iapd-sec-cr:SECRgnCdType ;
  dtype:order "9"^^xsd:nonNegativeInteger ;
  dtype:value "MIRO"^^xsd:NMTOKEN ;
  rdfs:label "MIRO"^^xsd:string ;
.
iapd-sec-cr:SECRCT_NYRO
  rdf:type iapd-sec-cr:SECRgnCdType ;
  dtype:order "5"^^xsd:nonNegativeInteger ;
  dtype:value "NYRO"^^xsd:NMTOKEN ;
  rdfs:label "NYRO"^^xsd:string ;
.
iapd-sec-cr:SECRCT_PLRO
  rdf:type iapd-sec-cr:SECRgnCdType ;
  dtype:order "7"^^xsd:nonNegativeInteger ;
  dtype:value "PLRO"^^xsd:NMTOKEN ;
  rdfs:label "PLRO"^^xsd:string ;
.
iapd-sec-cr:SECRCT_SFRO
  rdf:type iapd-sec-cr:SECRgnCdType ;
  dtype:order "8"^^xsd:nonNegativeInteger ;
  dtype:value "SFRO"^^xsd:NMTOKEN ;
  rdfs:label "SFRO"^^xsd:string ;
.
iapd-sec-cr:SECRgnCdType
  rdf:type owl:Class ;
  sxml:tag "SECRgnCdType" ;
  rdfs:comment """Elements of this type represent the business type.
        Allowed values (code-Name) are:
        ARO-Atlanta Regional Office.
        BRO-Boston Regional Office.
        DRO-Denver Regional Office.
        FWRO-Fort Worth Regional Office.
        CHRO-Chicago Regional Office.
        NYRO-New York Regional Office.
        LARO-Los Angeles Regional Office.
        PLRO-Philadelphia Regional Office.
        SFRO-San Francisco Regional Office.
        MIRO-Miami Regional Office.
        HQ-Headquarters."""@en ;
  rdfs:label "SECRgn cd type"^^xsd:string ;
  rdfs:subClassOf iapd-sec-cr:EnumeratedValue ;
  rdfs:subClassOf [
      rdf:type owl:Restriction ;
      sxml:isAttribute "false"^^xsd:boolean ;
      owl:allValuesFrom xsd:NMTOKEN ;
      owl:onProperty dtype:value ;
    ] ;
  rdfs:subClassOf [
      rdf:type owl:Restriction ;
      owl:maxCardinality "1"^^xsd:int ;
      owl:onProperty dtype:value ;
    ] ;
  owl:oneOf (
      iapd-sec-cr:SECRCT_ARO
      iapd-sec-cr:SECRCT_BRO
      iapd-sec-cr:SECRCT_CHRO
      iapd-sec-cr:SECRCT_DRO
      iapd-sec-cr:SECRCT_FWRO
      iapd-sec-cr:SECRCT_HQ
      iapd-sec-cr:SECRCT_LARO
      iapd-sec-cr:SECRCT_MIRO
      iapd-sec-cr:SECRCT_NYRO
      iapd-sec-cr:SECRCT_PLRO
      iapd-sec-cr:SECRCT_SFRO
    ) ;
.
iapd-sec-cr:SRST_ACTIVE
  rdf:type iapd-sec-cr:SecRgstnStType ;
  dtype:order "3"^^xsd:nonNegativeInteger ;
  dtype:value "ACTIVE"^^xsd:NMTOKEN ;
  rdfs:label "ACTIVE"^^xsd:string ;
.
iapd-sec-cr:SRST_APPROVED
  rdf:type iapd-sec-cr:SecRgstnStType ;
  dtype:order "0"^^xsd:nonNegativeInteger ;
  dtype:value "APPROVED"^^xsd:NMTOKEN ;
  rdfs:label "APPROVED"^^xsd:string ;
.
iapd-sec-cr:SRST_APPROVED-120
  rdf:type iapd-sec-cr:SecRgstnStType ;
  dtype:order "1"^^xsd:nonNegativeInteger ;
  dtype:value "APPROVED-120"^^xsd:NMTOKEN ;
  rdfs:label "APPROVED-120"^^xsd:string ;
.
iapd-sec-cr:SRST_SUSPENDED
  rdf:type iapd-sec-cr:SecRgstnStType ;
  dtype:order "2"^^xsd:nonNegativeInteger ;
  dtype:value "SUSPENDED"^^xsd:NMTOKEN ;
  rdfs:label "SUSPENDED"^^xsd:string ;
.
iapd-sec-cr:SecRgstnStType
  rdf:type owl:Class ;
  sxml:tag "SecRgstnStType" ;
  rdfs:comment """Elements of this type represent the business type.
        Allowed values (code-Name) are:
        APPROVED-Approved.
        APPROVED-120-120-Day Approval.
        SUSPENDED-Suspended.
        ACTIVE-Active."""@en ;
  rdfs:label "Sec rgstn st type"^^xsd:string ;
  rdfs:subClassOf iapd-sec-cr:EnumeratedValue ;
  rdfs:subClassOf [
      rdf:type owl:Restriction ;
      sxml:isAttribute "false"^^xsd:boolean ;
      owl:allValuesFrom xsd:NMTOKEN ;
      owl:onProperty dtype:value ;
    ] ;
  rdfs:subClassOf [
      rdf:type owl:Restriction ;
      owl:maxCardinality "1"^^xsd:int ;
      owl:onProperty dtype:value ;
    ] ;
  owl:oneOf (
      iapd-sec-cr:SRST_ACTIVE
      iapd-sec-cr:SRST_APPROVED
      iapd-sec-cr:SRST_APPROVED-120
      iapd-sec-cr:SRST_SUSPENDED
    ) ;
.
iapd-sec-cr:StateCdType
  rdf:type owl:Class ;
  sxml:tag "StateCdType" ;
  rdfs:comment """Elements of this type represent the allowed State Codes.
        Allowed values (code-Name) are:
        AK-Alaska
        AL-Alabama
        AR-Arkansas
        AZ-Arizona
        CA-California
        CO-Colorado
        CT-Connecticut
        DC-District of Columbia
        DE-Delaware
        FL-Florida
        GA-Georgia
        GU-Guam
        HI-Hawaii
        IA-Iowa
        ID-Idaho
        IL-Illinois
        IN-Indiana
        KS-Kansas
        KY-Kentucky
        LA-Louisiana
        MA-Massachusetts
        MD-Maryland
        ME-Maine
        MI-Michigan
        MN-Minnesota
        MO-Missouri
        MS-Mississippi
        MT-Montana
        NC-North Carolina
        ND-North Dakota
        NE-Nebraska
        NH-New Hampshire
        NJ-New Jersey
        NM-New Mexico
        NV-Nevada
        NY-New York
        OH-Ohio
        OK-Oklahoma
        OR-Oregon
        PA-Pennsylvania
        PR-Puerto Rico
        RI-Rhode Island
        SC-South Carolina
        SD-South Dakota
        TN-Tennessee
        TX-Texas
        UT-Utah
        VA-Virginia
        VT-Vermont
        WA-Washington
        WI-Wisconsin
        WV-West Virginia
        WY-Wyoming
        VI-Virgin Islands"""@en ;
  rdfs:label "State cd type"^^xsd:string ;
  rdfs:subClassOf iapd-sec-cr:EnumeratedValue ;
  rdfs:subClassOf [
      rdf:type owl:Restriction ;
      sxml:isAttribute "false"^^xsd:boolean ;
      owl:allValuesFrom xsd:NMTOKEN ;
      owl:onProperty dtype:value ;
    ] ;
  rdfs:subClassOf [
      rdf:type owl:Restriction ;
      owl:maxCardinality "1"^^xsd:int ;
      owl:onProperty dtype:value ;
    ] ;
  owl:oneOf (
      iapd-sec-cr:SCT_AK
      iapd-sec-cr:SCT_AL
      iapd-sec-cr:SCT_AR
      iapd-sec-cr:SCT_AZ
      iapd-sec-cr:SCT_CA
      iapd-sec-cr:SCT_CO
      iapd-sec-cr:SCT_CT
      iapd-sec-cr:SCT_DC
      iapd-sec-cr:SCT_DE
      iapd-sec-cr:SCT_FL
      iapd-sec-cr:SCT_GA
      iapd-sec-cr:SCT_GU
      iapd-sec-cr:SCT_HI
      iapd-sec-cr:SCT_IA
      iapd-sec-cr:SCT_ID
      iapd-sec-cr:SCT_IL
      iapd-sec-cr:SCT_IN
      iapd-sec-cr:SCT_KS
      iapd-sec-cr:SCT_KY
      iapd-sec-cr:SCT_LA
      iapd-sec-cr:SCT_MA
      iapd-sec-cr:SCT_MD
      iapd-sec-cr:SCT_ME
      iapd-sec-cr:SCT_MI
      iapd-sec-cr:SCT_MN
      iapd-sec-cr:SCT_MO
      iapd-sec-cr:SCT_MS
      iapd-sec-cr:SCT_MT
      iapd-sec-cr:SCT_NC
      iapd-sec-cr:SCT_ND
      iapd-sec-cr:SCT_NE
      iapd-sec-cr:SCT_NH
      iapd-sec-cr:SCT_NJ
      iapd-sec-cr:SCT_NM
      iapd-sec-cr:SCT_NV
      iapd-sec-cr:SCT_NY
      iapd-sec-cr:SCT_OH
      iapd-sec-cr:SCT_OK
      iapd-sec-cr:SCT_OR
      iapd-sec-cr:SCT_PA
      iapd-sec-cr:SCT_PR
      iapd-sec-cr:SCT_RI
      iapd-sec-cr:SCT_SC
      iapd-sec-cr:SCT_SD
      iapd-sec-cr:SCT_TN
      iapd-sec-cr:SCT_TX
      iapd-sec-cr:SCT_UT
      iapd-sec-cr:SCT_VA
      iapd-sec-cr:SCT_VI
      iapd-sec-cr:SCT_VT
      iapd-sec-cr:SCT_WA
      iapd-sec-cr:SCT_WI
      iapd-sec-cr:SCT_WV
      iapd-sec-cr:SCT_WY
    ) ;
.
iapd-sec-cr:Str10Datatype
  rdf:type rdfs:Datatype ;
  rdfs:label "Str10Datatype"^^xsd:string ;
  rdfs:subClassOf xsd:string ;
  owl:equivalentClass [
      rdf:type rdfs:Datatype ;
      owl:onDatatype xsd:string ;
      owl:withRestrictions (
          [
            xsd:maxLength "10"^^xsd:string ;
          ]
        ) ;
    ] ;
.
iapd-sec-cr:Str11Datatype
  rdf:type rdfs:Datatype ;
  rdfs:label "Str11Datatype"^^xsd:string ;
  rdfs:subClassOf xsd:string ;
  owl:equivalentClass [
      rdf:type rdfs:Datatype ;
      owl:onDatatype xsd:string ;
      owl:withRestrictions (
          [
            xsd:maxLength "11"^^xsd:string ;
          ]
        ) ;
    ] ;
.
iapd-sec-cr:Str128Datatype
  rdf:type rdfs:Datatype ;
  rdfs:label "Str128Datatype"^^xsd:string ;
  rdfs:subClassOf xsd:string ;
  owl:equivalentClass [
      rdf:type rdfs:Datatype ;
      owl:onDatatype xsd:string ;
      owl:withRestrictions (
          [
            xsd:maxLength "128"^^xsd:string ;
          ]
        ) ;
    ] ;
.
iapd-sec-cr:Str20Datatype
  rdf:type rdfs:Datatype ;
  rdfs:label "Str20Datatype"^^xsd:string ;
  rdfs:subClassOf xsd:string ;
  owl:equivalentClass [
      rdf:type rdfs:Datatype ;
      owl:onDatatype xsd:string ;
      owl:withRestrictions (
          [
            xsd:maxLength "20"^^xsd:string ;
          ]
        ) ;
    ] ;
.
iapd-sec-cr:Str27Datatype
  rdf:type rdfs:Datatype ;
  rdfs:label "Str27Datatype"^^xsd:string ;
  rdfs:subClassOf xsd:string ;
  owl:equivalentClass [
      rdf:type rdfs:Datatype ;
      owl:onDatatype xsd:string ;
      owl:withRestrictions (
          [
            xsd:maxLength "27"^^xsd:string ;
          ]
        ) ;
    ] ;
.
iapd-sec-cr:Str4000Datatype
  rdf:type rdfs:Datatype ;
  rdfs:label "Str4000Datatype"^^xsd:string ;
  rdfs:subClassOf xsd:string ;
  owl:equivalentClass [
      rdf:type rdfs:Datatype ;
      owl:onDatatype xsd:string ;
      owl:withRestrictions (
          [
            xsd:maxLength "4000"^^xsd:string ;
          ]
        ) ;
    ] ;
.
iapd-sec-cr:Str50Datatype
  rdf:type rdfs:Datatype ;
  rdfs:label "Str50Datatype"^^xsd:string ;
  rdfs:subClassOf xsd:string ;
  owl:equivalentClass [
      rdf:type rdfs:Datatype ;
      owl:onDatatype xsd:string ;
      owl:withRestrictions (
          [
            xsd:maxLength "50"^^xsd:string ;
          ]
        ) ;
    ] ;
.
iapd-sec-cr:Str512Datatype
  rdf:type rdfs:Datatype ;
  rdfs:label "Str512Datatype"^^xsd:string ;
  rdfs:subClassOf xsd:string ;
  owl:equivalentClass [
      rdf:type rdfs:Datatype ;
      owl:onDatatype xsd:string ;
      owl:withRestrictions (
          [
            xsd:maxLength "512"^^xsd:string ;
          ]
        ) ;
    ] ;
.
iapd-sec-cr:Str64Datatype
  rdf:type rdfs:Datatype ;
  rdfs:label "Str64Datatype"^^xsd:string ;
  rdfs:subClassOf xsd:string ;
  owl:equivalentClass [
      rdf:type rdfs:Datatype ;
      owl:onDatatype xsd:string ;
      owl:withRestrictions (
          [
            xsd:maxLength "64"^^xsd:string ;
          ]
        ) ;
    ] ;
.
iapd-sec-cr:busNm
  rdf:type owl:DatatypeProperty ;
  sxml:attribute "BusNm" ;
  rdfs:label "Business Name"^^xsd:string ;
  rdfs:subPropertyOf iapd-sec-cr:hasFirmReportField ;
.
iapd-sec-cr:cIKNb
  rdf:type owl:DatatypeProperty ;
  sxml:attribute "CIKNb" ;
  rdfs:label "Central Index Key number"^^xsd:string ;
  rdfs:subPropertyOf iapd-sec-cr:hasFirmReportField ;
.
iapd-sec-cr:city
  rdf:type owl:DatatypeProperty ;
  sxml:attribute "City" ;
  rdfs:label "City"^^xsd:string ;
  rdfs:subPropertyOf iapd-sec-cr:hasFirmReportField ;
.
iapd-sec-cr:cntry
  rdf:type owl:DatatypeProperty ;
  sxml:attribute "Cntry" ;
  rdfs:label "Country"^^xsd:string ;
  rdfs:subPropertyOf iapd-sec-cr:hasFirmReportField ;
.
iapd-sec-cr:cntryNm
  rdf:type owl:DatatypeProperty ;
  sxml:attribute "CntryNm" ;
  rdfs:label "Country Name"^^xsd:string ;
  rdfs:subPropertyOf iapd-sec-cr:hasFirmReportField ;
.
iapd-sec-cr:dt
  rdf:type owl:DatatypeProperty ;
  sxml:attribute "Dt" ;
  rdfs:label "Date"^^xsd:string ;
  rdfs:subPropertyOf iapd-sec-cr:hasFirmReportField ;
.
iapd-sec-cr:email
  rdf:type owl:DatatypeProperty ;
  sxml:attribute "Email" ;
  rdfs:label "email"^^xsd:string ;
  rdfs:subPropertyOf iapd-sec-cr:hasFirmReportField ;
.
iapd-sec-cr:faxNb
  rdf:type owl:DatatypeProperty ;
  sxml:attribute "FaxNb" ;
  rdfs:label "Fax number"^^xsd:string ;
  rdfs:subPropertyOf iapd-sec-cr:hasFirmReportField ;
.
iapd-sec-cr:filingRef
  rdf:type owl:ObjectProperty ;
  sxml:tag "Filing" ;
  rdfs:label "filing ref"^^xsd:string ;
  rdfs:subPropertyOf iapd-sec-cr:hasFirmReportReference ;
  skos:definition "Filing reference relates the SEC Firm Type to the Filing Type."^^xsd:string ;
.
iapd-sec-cr:firmCrdNb
  rdf:type owl:DatatypeProperty ;
  sxml:attribute "FirmCrdNb" ;
  rdfs:label "Firm CRD number"^^xsd:string ;
  rdfs:subPropertyOf iapd-sec-cr:hasFirmReportField ;
.
iapd-sec-cr:firmRef
  rdf:type owl:ObjectProperty ;
  sxml:tag "Firm" ;
  rdfs:label "firm ref"^^xsd:string ;
  rdfs:subPropertyOf iapd-sec-cr:hasFirmReportReference ;
  skos:definition "Firm reference relates the IAPD SEC Report Type-firms to SEC Firm Type for each reporting adviser."^^xsd:string ;
.
iapd-sec-cr:firmType
  rdf:type owl:DatatypeProperty ;
  sxml:attribute "FirmType" ;
  rdfs:label "Firm Type"^^xsd:string ;
  rdfs:subPropertyOf iapd-sec-cr:hasFirmReportField ;
.
iapd-sec-cr:firmsRef
  rdf:type owl:ObjectProperty ;
  sxml:tag "Firms" ;
  rdfs:label "firms ref"^^xsd:string ;
  rdfs:subPropertyOf iapd-sec-cr:hasFirmReportReference ;
.
iapd-sec-cr:formInfoRef
  rdf:type owl:ObjectProperty ;
  sxml:tag "FormInfo" ;
  rdfs:label "form info ref"^^xsd:string ;
  rdfs:subPropertyOf iapd-sec-cr:hasFirmReportReference ;
  skos:definition "Form Info reference relates the SEC Firm Type to the Form information."^^xsd:string ;
.
iapd-sec-cr:formVrsn
  rdf:type owl:DatatypeProperty ;
  sxml:attribute "FormVrsn" ;
  rdfs:label "Form Version"^^xsd:string ;
  rdfs:subPropertyOf iapd-sec-cr:hasFirmReportField ;
.
iapd-sec-cr:genOn
  rdf:type owl:DatatypeProperty ;
  sxml:attribute "Generated on date"^^xsd:string ;
  rdfs:label "Generated on date"^^xsd:string ;
  rdfs:subPropertyOf iapd-sec-cr:hasFirmReportField ;
.
iapd-sec-cr:hasFirmReportField
  rdf:type owl:DatatypeProperty ;
  rdfs:label "Firm Report Reference"^^xsd:string ;
.
iapd-sec-cr:hasFirmReportReference
  rdf:type owl:ObjectProperty ;
  rdfs:label "Firm Report Reference"^^xsd:string ;
  skos:definition "The super property for all IDAP SEC compilation report form references."^^xsd:string ;
.
iapd-sec-cr:infoRef
  rdf:type owl:ObjectProperty ;
  sxml:tag "Info" ;
  rdfs:label "info ref"^^xsd:string ;
  rdfs:subPropertyOf iapd-sec-cr:hasFirmReportReference ;
  skos:definition "Info reference relates the SEC Firm Type to the Organization info."^^xsd:string ;
.
iapd-sec-cr:item10ARef
  rdf:type owl:ObjectProperty ;
  sxml:tag "Item10A" ;
  rdfs:label "item10ARef"^^xsd:string ;
  rdfs:subPropertyOf iapd-sec-cr:hasFirmReportReference ;
.
iapd-sec-cr:item11ARef
  rdf:type owl:ObjectProperty ;
  sxml:tag "Item11A" ;
  rdfs:label "item11ARef"^^xsd:string ;
  rdfs:subPropertyOf iapd-sec-cr:hasFirmReportReference ;
.
iapd-sec-cr:item11BRef
  rdf:type owl:ObjectProperty ;
  sxml:tag "Item11B" ;
  rdfs:label "item11BRef"^^xsd:string ;
  rdfs:subPropertyOf iapd-sec-cr:hasFirmReportReference ;
.
iapd-sec-cr:item11CRef
  rdf:type owl:ObjectProperty ;
  sxml:tag "Item11C" ;
  rdfs:label "item11CRef"^^xsd:string ;
  rdfs:subPropertyOf iapd-sec-cr:hasFirmReportReference ;
.
iapd-sec-cr:item11DRef
  rdf:type owl:ObjectProperty ;
  sxml:tag "Item11D" ;
  rdfs:label "item11DRef"^^xsd:string ;
  rdfs:subPropertyOf iapd-sec-cr:hasFirmReportReference ;
.
iapd-sec-cr:item11ERef
  rdf:type owl:ObjectProperty ;
  sxml:tag "Item11E" ;
  rdfs:label "item11ERef"^^xsd:string ;
  rdfs:subPropertyOf iapd-sec-cr:hasFirmReportReference ;
.
iapd-sec-cr:item11FRef
  rdf:type owl:ObjectProperty ;
  sxml:tag "Item11F" ;
  rdfs:label "item11FRef"^^xsd:string ;
  rdfs:subPropertyOf iapd-sec-cr:hasFirmReportReference ;
.
iapd-sec-cr:item11GRef
  rdf:type owl:ObjectProperty ;
  sxml:tag "Item11G" ;
  rdfs:label "item11GRef"^^xsd:string ;
  rdfs:subPropertyOf iapd-sec-cr:hasFirmReportReference ;
.
iapd-sec-cr:item11HRef
  rdf:type owl:ObjectProperty ;
  sxml:tag "Item11H" ;
  rdfs:label "item11HRef"^^xsd:string ;
  rdfs:subPropertyOf iapd-sec-cr:hasFirmReportReference ;
.
iapd-sec-cr:item11Ref
  rdf:type owl:ObjectProperty ;
  sxml:tag "Item11" ;
  rdfs:label "item11Ref"^^xsd:string ;
  rdfs:subPropertyOf iapd-sec-cr:hasFirmReportReference ;
.
iapd-sec-cr:item1Ref
  rdf:type owl:ObjectProperty ;
  sxml:tag "Item1" ;
  rdfs:label "item1Ref"^^xsd:string ;
  rdfs:subPropertyOf iapd-sec-cr:hasFirmReportReference ;
.
iapd-sec-cr:item2ARef
  rdf:type owl:ObjectProperty ;
  sxml:tag "Item2A" ;
  rdfs:label "item2ARef"^^xsd:string ;
  rdfs:subPropertyOf iapd-sec-cr:hasFirmReportReference ;
.
iapd-sec-cr:item2BRef
  rdf:type owl:ObjectProperty ;
  sxml:tag "Item2B" ;
  rdfs:label "item2BRef"^^xsd:string ;
  rdfs:subPropertyOf iapd-sec-cr:hasFirmReportReference ;
.
iapd-sec-cr:item3ARef
  rdf:type owl:ObjectProperty ;
  sxml:tag "Item3A" ;
  rdfs:label "item3ARef"^^xsd:string ;
  rdfs:subPropertyOf iapd-sec-cr:hasFirmReportReference ;
.
iapd-sec-cr:item3BRef
  rdf:type owl:ObjectProperty ;
  sxml:tag "Item3B" ;
  rdfs:label "item3BRef"^^xsd:string ;
  rdfs:subPropertyOf iapd-sec-cr:hasFirmReportReference ;
.
iapd-sec-cr:item3CRef
  rdf:type owl:ObjectProperty ;
  sxml:tag "Item3C" ;
  rdfs:label "item3CRef"^^xsd:string ;
  rdfs:subPropertyOf iapd-sec-cr:hasFirmReportReference ;
.
iapd-sec-cr:item5ARef
  rdf:type owl:ObjectProperty ;
  sxml:tag "Item5A" ;
  rdfs:label "item5ARef"^^xsd:string ;
  rdfs:subPropertyOf iapd-sec-cr:hasFirmReportReference ;
.
iapd-sec-cr:item5BRef
  rdf:type owl:ObjectProperty ;
  sxml:tag "Item5B" ;
  rdfs:label "item5BRef"^^xsd:string ;
  rdfs:subPropertyOf iapd-sec-cr:hasFirmReportReference ;
.
iapd-sec-cr:item5CRef
  rdf:type owl:ObjectProperty ;
  sxml:tag "Item5C" ;
  rdfs:label "item5CRef"^^xsd:string ;
  rdfs:subPropertyOf iapd-sec-cr:hasFirmReportReference ;
.
iapd-sec-cr:item5DRef
  rdf:type owl:ObjectProperty ;
  sxml:tag "Item5D" ;
  rdfs:label "item5DRef"^^xsd:string ;
  rdfs:subPropertyOf iapd-sec-cr:hasFirmReportReference ;
.
iapd-sec-cr:item5ERef
  rdf:type owl:ObjectProperty ;
  sxml:tag "Item5E" ;
  rdfs:label "item5ERef"^^xsd:string ;
  rdfs:subPropertyOf iapd-sec-cr:hasFirmReportReference ;
.
iapd-sec-cr:item5FRef
  rdf:type owl:ObjectProperty ;
  sxml:tag "Item5F" ;
  rdfs:label "item5FRef"^^xsd:string ;
  rdfs:subPropertyOf iapd-sec-cr:hasFirmReportReference ;
.
iapd-sec-cr:item5GRef
  rdf:type owl:ObjectProperty ;
  sxml:tag "Item5G" ;
  rdfs:label "item5GRef"^^xsd:string ;
  rdfs:subPropertyOf iapd-sec-cr:hasFirmReportReference ;
.
iapd-sec-cr:item5HRef
  rdf:type owl:ObjectProperty ;
  sxml:tag "Item5H" ;
  rdfs:label "item5HRef"^^xsd:string ;
  rdfs:subPropertyOf iapd-sec-cr:hasFirmReportReference ;
.
iapd-sec-cr:item5IRef
  rdf:type owl:ObjectProperty ;
  sxml:tag "Item5I" ;
  rdfs:label "item5IRef"^^xsd:string ;
  rdfs:subPropertyOf iapd-sec-cr:hasFirmReportReference ;
.
iapd-sec-cr:item5JRef
  rdf:type owl:ObjectProperty ;
  sxml:tag "Item5J" ;
  rdfs:label "item5JRef"^^xsd:string ;
  rdfs:subPropertyOf iapd-sec-cr:hasFirmReportReference ;
.
iapd-sec-cr:item6ARef
  rdf:type owl:ObjectProperty ;
  sxml:tag "Item6A" ;
  rdfs:label "item6ARef"^^xsd:string ;
  rdfs:subPropertyOf iapd-sec-cr:hasFirmReportReference ;
.
iapd-sec-cr:item6BRef
  rdf:type owl:ObjectProperty ;
  sxml:tag "Item6B" ;
  rdfs:label "item6BRef"^^xsd:string ;
  rdfs:subPropertyOf iapd-sec-cr:hasFirmReportReference ;
.
iapd-sec-cr:item7ARef
  rdf:type owl:ObjectProperty ;
  sxml:tag "Item7A" ;
  rdfs:label "item7ARef"^^xsd:string ;
  rdfs:subPropertyOf iapd-sec-cr:hasFirmReportReference ;
.
iapd-sec-cr:item7BRef
  rdf:type owl:ObjectProperty ;
  sxml:tag "Item7B" ;
  rdfs:label "item7BRef"^^xsd:string ;
  rdfs:subPropertyOf iapd-sec-cr:hasFirmReportReference ;
.
iapd-sec-cr:item8ARef
  rdf:type owl:ObjectProperty ;
  sxml:tag "Item8A" ;
  rdfs:label "item8ARef"^^xsd:string ;
  rdfs:subPropertyOf iapd-sec-cr:hasFirmReportReference ;
.
iapd-sec-cr:item8BRef
  rdf:type owl:ObjectProperty ;
  sxml:tag "Item8B" ;
  rdfs:label "item8BRef"^^xsd:string ;
  rdfs:subPropertyOf iapd-sec-cr:hasFirmReportReference ;
.
iapd-sec-cr:item8CRef
  rdf:type owl:ObjectProperty ;
  sxml:tag "Item8C" ;
  rdfs:label "item8CRef"^^xsd:string ;
  rdfs:subPropertyOf iapd-sec-cr:hasFirmReportReference ;
.
iapd-sec-cr:item8DRef
  rdf:type owl:ObjectProperty ;
  sxml:tag "Item8D" ;
  rdfs:label "item8DRef"^^xsd:string ;
  rdfs:subPropertyOf iapd-sec-cr:hasFirmReportReference ;
.
iapd-sec-cr:item8ERef
  rdf:type owl:ObjectProperty ;
  sxml:tag "Item8E" ;
  rdfs:label "item8ERef"^^xsd:string ;
  rdfs:subPropertyOf iapd-sec-cr:hasFirmReportReference ;
.
iapd-sec-cr:item8FRef
  rdf:type owl:ObjectProperty ;
  sxml:tag "Item8F" ;
  rdfs:label "item8FRef"^^xsd:string ;
  rdfs:subPropertyOf iapd-sec-cr:hasFirmReportReference ;
.
iapd-sec-cr:item8GRef
  rdf:type owl:ObjectProperty ;
  sxml:tag "Item8G" ;
  rdfs:label "item8GRef"^^xsd:string ;
  rdfs:subPropertyOf iapd-sec-cr:hasFirmReportReference ;
.
iapd-sec-cr:item8HRef
  rdf:type owl:ObjectProperty ;
  sxml:tag "Item8H" ;
  rdfs:label "item8HRef"^^xsd:string ;
  rdfs:subPropertyOf iapd-sec-cr:hasFirmReportReference ;
.
iapd-sec-cr:item8IRef
  rdf:type owl:ObjectProperty ;
  sxml:tag "Item8I" ;
  rdfs:label "item8IRef"^^xsd:string ;
  rdfs:subPropertyOf iapd-sec-cr:hasFirmReportReference ;
.
iapd-sec-cr:item9ARef
  rdf:type owl:ObjectProperty ;
  sxml:tag "Item9A" ;
  rdfs:label "item9ARef"^^xsd:string ;
  rdfs:subPropertyOf iapd-sec-cr:hasFirmReportReference ;
.
iapd-sec-cr:item9BRef
  rdf:type owl:ObjectProperty ;
  sxml:tag "Item9B" ;
  rdfs:label "item9BRef"^^xsd:string ;
  rdfs:subPropertyOf iapd-sec-cr:hasFirmReportReference ;
.
iapd-sec-cr:item9CRef
  rdf:type owl:ObjectProperty ;
  sxml:tag "Item9C" ;
  rdfs:label "item9CRef"^^xsd:string ;
  rdfs:subPropertyOf iapd-sec-cr:hasFirmReportReference ;
.
iapd-sec-cr:item9DRef
  rdf:type owl:ObjectProperty ;
  sxml:tag "Item9D" ;
  rdfs:label "item9DRef"^^xsd:string ;
  rdfs:subPropertyOf iapd-sec-cr:hasFirmReportReference ;
.
iapd-sec-cr:item9ERef
  rdf:type owl:ObjectProperty ;
  sxml:tag "Item9E" ;
  rdfs:label "item9ERef"^^xsd:string ;
  rdfs:subPropertyOf iapd-sec-cr:hasFirmReportReference ;
.
iapd-sec-cr:item9FRef
  rdf:type owl:ObjectProperty ;
  sxml:tag "Item9F" ;
  rdfs:label "item9FRef"^^xsd:string ;
  rdfs:subPropertyOf iapd-sec-cr:hasFirmReportReference ;
.
iapd-sec-cr:legalNm
  rdf:type owl:DatatypeProperty ;
  sxml:attribute "LegalNm" ;
  rdfs:label "Legal Name"^^xsd:string ;
  rdfs:subPropertyOf iapd-sec-cr:hasFirmReportField ;
.
iapd-sec-cr:mailingAddrRef
  rdf:type owl:ObjectProperty ;
  sxml:tag "MailingAddr" ;
  rdfs:label "mailing addr ref"^^xsd:string ;
  rdfs:subPropertyOf iapd-sec-cr:hasFirmReportReference ;
  skos:definition "Mailing Address reference relates the SEC Firm Type to the Address Type for the mailing address."^^xsd:string ;
.
iapd-sec-cr:mainAddrRef
  rdf:type owl:ObjectProperty ;
  sxml:tag "MainAddr" ;
  rdfs:label "main addr ref"^^xsd:string ;
  rdfs:subPropertyOf iapd-sec-cr:hasFirmReportReference ;
  skos:definition "Main Address reference relates the SEC Firm Type to the Address Type of the main address."^^xsd:string ;
.
iapd-sec-cr:nm
  rdf:type owl:DatatypeProperty ;
  sxml:attribute "Nm" ;
  rdfs:label "Name"^^xsd:string ;
  rdfs:subPropertyOf iapd-sec-cr:hasFirmReportField ;
.
iapd-sec-cr:noticeFiledRef
  rdf:type owl:ObjectProperty ;
  sxml:tag "NoticeFiled" ;
  rdfs:label "notice filed ref"^^xsd:string ;
  rdfs:subPropertyOf iapd-sec-cr:hasFirmReportReference ;
  skos:definition "Notice Filed reference links the SEC Firm Type to the Notice Filed Type."^^xsd:string ;
.
iapd-sec-cr:orgFormNm
  rdf:type owl:DatatypeProperty ;
  sxml:attribute "OrgFormNm" ;
  rdfs:label "Organization Form Name"^^xsd:string ;
  rdfs:subPropertyOf iapd-sec-cr:hasFirmReportField ;
.
iapd-sec-cr:orgFormOthNm
  rdf:type owl:DatatypeProperty ;
  sxml:attribute "OrgFormOthNm" ;
  rdfs:label "Organization Form other Name"^^xsd:string ;
  rdfs:subPropertyOf iapd-sec-cr:hasFirmReportField ;
.
iapd-sec-cr:part1ARef
  rdf:type owl:ObjectProperty ;
  sxml:tag "Part1A" ;
  rdfs:label "part1ARef"^^xsd:string ;
  rdfs:subPropertyOf iapd-sec-cr:hasFirmReportReference ;
.
iapd-sec-cr:phNb
  rdf:type owl:DatatypeProperty ;
  sxml:attribute "PhNb" ;
  rdfs:label "Phone Number"^^xsd:string ;
  rdfs:subPropertyOf iapd-sec-cr:hasFirmReportField ;
.
iapd-sec-cr:postlCd
  rdf:type owl:DatatypeProperty ;
  sxml:attribute "PostlCd" ;
  rdfs:label "Postal Code"^^xsd:string ;
  rdfs:subPropertyOf iapd-sec-cr:hasFirmReportField ;
.
iapd-sec-cr:prvtAdrsFl
  rdf:type owl:DatatypeProperty ;
  sxml:attribute "PrvtAdrsFl" ;
  rdfs:label "Private Address Field"^^xsd:string ;
  rdfs:subPropertyOf iapd-sec-cr:hasFirmReportField ;
.
iapd-sec-cr:q10A
  rdf:type owl:DatatypeProperty ;
  sxml:attribute "Q10A" ;
  rdfs:label "Question 10A"^^xsd:string ;
  rdfs:subPropertyOf iapd-sec-cr:hasFirmReportField ;
.
iapd-sec-cr:q11
  rdf:type owl:DatatypeProperty ;
  sxml:attribute "Q11" ;
  rdfs:label "Question 11"^^xsd:string ;
  rdfs:subPropertyOf iapd-sec-cr:hasFirmReportField ;
.
iapd-sec-cr:q11A1
  rdf:type owl:DatatypeProperty ;
  sxml:attribute "Q11A1" ;
  rdfs:label "Question 11A1"^^xsd:string ;
  rdfs:subPropertyOf iapd-sec-cr:hasFirmReportField ;
.
iapd-sec-cr:q11A2
  rdf:type owl:DatatypeProperty ;
  sxml:attribute "Q11A2" ;
  rdfs:label "Question 11A2"^^xsd:string ;
  rdfs:subPropertyOf iapd-sec-cr:hasFirmReportField ;
.
iapd-sec-cr:q11B1
  rdf:type owl:DatatypeProperty ;
  sxml:attribute "Q11B1" ;
  rdfs:label "Question 11B1"^^xsd:string ;
  rdfs:subPropertyOf iapd-sec-cr:hasFirmReportField ;
.
iapd-sec-cr:q11B2
  rdf:type owl:DatatypeProperty ;
  sxml:attribute "Q11B2" ;
  rdfs:label "q11B2"^^xsd:string ;
  rdfs:subPropertyOf iapd-sec-cr:hasFirmReportField ;
.
iapd-sec-cr:q11C1
  rdf:type owl:DatatypeProperty ;
  sxml:attribute "Q11C1" ;
  rdfs:label "Question 11C1"^^xsd:string ;
  rdfs:subPropertyOf iapd-sec-cr:hasFirmReportField ;
.
iapd-sec-cr:q11C2
  rdf:type owl:DatatypeProperty ;
  sxml:attribute "Q11C2" ;
  rdfs:label "Question 11C2"^^xsd:string ;
  rdfs:subPropertyOf iapd-sec-cr:hasFirmReportField ;
.
iapd-sec-cr:q11C3
  rdf:type owl:DatatypeProperty ;
  sxml:attribute "Q11C3" ;
  rdfs:label "Question 11C3"^^xsd:string ;
  rdfs:subPropertyOf iapd-sec-cr:hasFirmReportField ;
.
iapd-sec-cr:q11C4
  rdf:type owl:DatatypeProperty ;
  sxml:attribute "Q11C4" ;
  rdfs:label "Question 11C4"^^xsd:string ;
  rdfs:subPropertyOf iapd-sec-cr:hasFirmReportField ;
.
iapd-sec-cr:q11C5
  rdf:type owl:DatatypeProperty ;
  sxml:attribute "Q11C5" ;
  rdfs:label "Question 11C5"^^xsd:string ;
  rdfs:subPropertyOf iapd-sec-cr:hasFirmReportField ;
.
iapd-sec-cr:q11D1
  rdf:type owl:DatatypeProperty ;
  sxml:attribute "Q11D1" ;
  rdfs:label "Question 11D1"^^xsd:string ;
  rdfs:subPropertyOf iapd-sec-cr:hasFirmReportField ;
.
iapd-sec-cr:q11D2
  rdf:type owl:DatatypeProperty ;
  sxml:attribute "Q11D2" ;
  rdfs:label "Question 11D2"^^xsd:string ;
  rdfs:subPropertyOf iapd-sec-cr:hasFirmReportField ;
.
iapd-sec-cr:q11D3
  rdf:type owl:DatatypeProperty ;
  sxml:attribute "Q11D3" ;
  rdfs:label "Question 11D3"^^xsd:string ;
  rdfs:subPropertyOf iapd-sec-cr:hasFirmReportField ;
.
iapd-sec-cr:q11D4
  rdf:type owl:DatatypeProperty ;
  sxml:attribute "Q11D4" ;
  rdfs:label "Question 11D4"^^xsd:string ;
  rdfs:subPropertyOf iapd-sec-cr:hasFirmReportField ;
.
iapd-sec-cr:q11D5
  rdf:type owl:DatatypeProperty ;
  sxml:attribute "Q11D5" ;
  rdfs:label "Question 11D5"^^xsd:string ;
  rdfs:subPropertyOf iapd-sec-cr:hasFirmReportField ;
.
iapd-sec-cr:q11E1
  rdf:type owl:DatatypeProperty ;
  sxml:attribute "Q11E1" ;
  rdfs:label "Question 11E1"^^xsd:string ;
  rdfs:subPropertyOf iapd-sec-cr:hasFirmReportField ;
.
iapd-sec-cr:q11E2
  rdf:type owl:DatatypeProperty ;
  sxml:attribute "Q11E2" ;
  rdfs:label "Question 11E2"^^xsd:string ;
  rdfs:subPropertyOf iapd-sec-cr:hasFirmReportField ;
.
iapd-sec-cr:q11E3
  rdf:type owl:DatatypeProperty ;
  sxml:attribute "Q11E3" ;
  rdfs:label "Question 11E3"^^xsd:string ;
  rdfs:subPropertyOf iapd-sec-cr:hasFirmReportField ;
.
iapd-sec-cr:q11E4
  rdf:type owl:DatatypeProperty ;
  sxml:attribute "Q11E4" ;
  rdfs:label "Question 11E4"^^xsd:string ;
  rdfs:subPropertyOf iapd-sec-cr:hasFirmReportField ;
.
iapd-sec-cr:q11F
  rdf:type owl:DatatypeProperty ;
  sxml:attribute "Q11F" ;
  rdfs:label "Question 11F"^^xsd:string ;
  rdfs:subPropertyOf iapd-sec-cr:hasFirmReportField ;
.
iapd-sec-cr:q11G
  rdf:type owl:DatatypeProperty ;
  sxml:attribute "Q11G" ;
  rdfs:label "Question 11G"^^xsd:string ;
  rdfs:subPropertyOf iapd-sec-cr:hasFirmReportField ;
.
iapd-sec-cr:q11H1A
  rdf:type owl:DatatypeProperty ;
  sxml:attribute "Q11H1A" ;
  rdfs:label "Question 11H1A"^^xsd:string ;
  rdfs:subPropertyOf iapd-sec-cr:hasFirmReportField ;
.
iapd-sec-cr:q11H1B
  rdf:type owl:DatatypeProperty ;
  sxml:attribute "Q11H1B" ;
  rdfs:label "Question 11H1B"^^xsd:string ;
  rdfs:subPropertyOf iapd-sec-cr:hasFirmReportField ;
.
iapd-sec-cr:q11H1C
  rdf:type owl:DatatypeProperty ;
  sxml:attribute "Q11H1C" ;
  rdfs:label "Question 11H1C"^^xsd:string ;
  rdfs:subPropertyOf iapd-sec-cr:hasFirmReportField ;
.
iapd-sec-cr:q11H2
  rdf:type owl:DatatypeProperty ;
  sxml:attribute "Q11H2" ;
  rdfs:label "Question 11H2"^^xsd:string ;
  rdfs:subPropertyOf iapd-sec-cr:hasFirmReportField ;
.
iapd-sec-cr:q1I
  rdf:type owl:DatatypeProperty ;
  sxml:attribute "Q1I" ;
  rdfs:label "Question 1I"^^xsd:string ;
  rdfs:subPropertyOf iapd-sec-cr:hasFirmReportField ;
.
iapd-sec-cr:q1M
  rdf:type owl:DatatypeProperty ;
  sxml:attribute "Q1M" ;
  rdfs:label "Question 1M"^^xsd:string ;
  rdfs:subPropertyOf iapd-sec-cr:hasFirmReportField ;
.
iapd-sec-cr:q1N
  rdf:type owl:DatatypeProperty ;
  sxml:attribute "Q1N" ;
  rdfs:label "Question 1N"^^xsd:string ;
  rdfs:subPropertyOf iapd-sec-cr:hasFirmReportField ;
.
iapd-sec-cr:q1O
  rdf:type owl:DatatypeProperty ;
  sxml:attribute "Q1O" ;
  rdfs:label "Question 1O"^^xsd:string ;
  rdfs:subPropertyOf iapd-sec-cr:hasFirmReportField ;
.
iapd-sec-cr:q1P
  rdf:type owl:DatatypeProperty ;
  sxml:attribute "Q1P" ;
  rdfs:label "Question 1P"^^xsd:string ;
  rdfs:subPropertyOf iapd-sec-cr:hasFirmReportField ;
.
iapd-sec-cr:q2A1
  rdf:type owl:DatatypeProperty ;
  sxml:attribute "Q2A1" ;
  rdfs:label "Question 2A1"^^xsd:string ;
  rdfs:subPropertyOf iapd-sec-cr:hasFirmReportField ;
.
iapd-sec-cr:q2A10
  rdf:type owl:DatatypeProperty ;
  sxml:attribute "Q2A10" ;
  rdfs:label "Question 2A10"^^xsd:string ;
  rdfs:subPropertyOf iapd-sec-cr:hasFirmReportField ;
.
iapd-sec-cr:q2A11
  rdf:type owl:DatatypeProperty ;
  sxml:attribute "Q2A11" ;
  rdfs:label "Question 2A11"^^xsd:string ;
  rdfs:subPropertyOf iapd-sec-cr:hasFirmReportField ;
.
iapd-sec-cr:q2A12
  rdf:type owl:DatatypeProperty ;
  sxml:attribute "Q2A12" ;
  rdfs:label "Question 2A12"^^xsd:string ;
  rdfs:subPropertyOf iapd-sec-cr:hasFirmReportField ;
.
iapd-sec-cr:q2A13
  rdf:type owl:DatatypeProperty ;
  sxml:attribute "Q2A13" ;
  rdfs:label "Question 2A13"^^xsd:string ;
  rdfs:subPropertyOf iapd-sec-cr:hasFirmReportField ;
.
iapd-sec-cr:q2A2
  rdf:type owl:DatatypeProperty ;
  sxml:attribute "Q2A2" ;
  rdfs:label "Question 2A2"^^xsd:string ;
  rdfs:subPropertyOf iapd-sec-cr:hasFirmReportField ;
.
iapd-sec-cr:q2A3
  rdf:type owl:DatatypeProperty ;
  sxml:attribute "Q2A3" ;
  rdfs:label "Question 2A3"^^xsd:string ;
  rdfs:subPropertyOf iapd-sec-cr:hasFirmReportField ;
.
iapd-sec-cr:q2A4
  rdf:type owl:DatatypeProperty ;
  sxml:attribute "Q2A4" ;
  rdfs:label "Question 2A4"^^xsd:string ;
  rdfs:subPropertyOf iapd-sec-cr:hasFirmReportField ;
.
iapd-sec-cr:q2A5
  rdf:type owl:DatatypeProperty ;
  sxml:attribute "Q2A5" ;
  rdfs:label "Question 2A5"^^xsd:string ;
  rdfs:subPropertyOf iapd-sec-cr:hasFirmReportField ;
.
iapd-sec-cr:q2A6
  rdf:type owl:DatatypeProperty ;
  sxml:attribute "Q2A6" ;
  rdfs:label "Question 2A6"^^xsd:string ;
  rdfs:subPropertyOf iapd-sec-cr:hasFirmReportField ;
.
iapd-sec-cr:q2A7
  rdf:type owl:DatatypeProperty ;
  sxml:attribute "Q2A7" ;
  rdfs:label "Question 2A7"^^xsd:string ;
  rdfs:subPropertyOf iapd-sec-cr:hasFirmReportField ;
.
iapd-sec-cr:q2A8
  rdf:type owl:DatatypeProperty ;
  sxml:attribute "Q2A8" ;
  rdfs:label "Question 2A8"^^xsd:string ;
  rdfs:subPropertyOf iapd-sec-cr:hasFirmReportField ;
.
iapd-sec-cr:q2A9
  rdf:type owl:DatatypeProperty ;
  sxml:attribute "Q2A9" ;
  rdfs:label "Question 2A9"^^xsd:string ;
  rdfs:subPropertyOf iapd-sec-cr:hasFirmReportField ;
.
iapd-sec-cr:q2B1
  rdf:type owl:DatatypeProperty ;
  sxml:attribute "Q2B1" ;
  rdfs:label "Question 2B1"^^xsd:string ;
  rdfs:subPropertyOf iapd-sec-cr:hasFirmReportField ;
.
iapd-sec-cr:q2B2
  rdf:type owl:DatatypeProperty ;
  sxml:attribute "Q2B2" ;
  rdfs:label "Question 2B2"^^xsd:string ;
  rdfs:subPropertyOf iapd-sec-cr:hasFirmReportField ;
.
iapd-sec-cr:q2B3
  rdf:type owl:DatatypeProperty ;
  sxml:attribute "Q2B3" ;
  rdfs:label "Question 2B3"^^xsd:string ;
  rdfs:subPropertyOf iapd-sec-cr:hasFirmReportField ;
.
iapd-sec-cr:q3B
  rdf:type owl:DatatypeProperty ;
  sxml:attribute "Q3B" ;
  rdfs:label "Question 3B"^^xsd:string ;
  rdfs:subPropertyOf iapd-sec-cr:hasFirmReportField ;
.
iapd-sec-cr:q5B1
  rdf:type owl:DatatypeProperty ;
  sxml:attribute "Q5B1" ;
  rdfs:label "Question 5B1"^^xsd:string ;
  rdfs:subPropertyOf iapd-sec-cr:hasFirmReportField ;
.
iapd-sec-cr:q5B2
  rdf:type owl:DatatypeProperty ;
  sxml:attribute "Q5B2" ;
  rdfs:label "Question 5B2"^^xsd:string ;
  rdfs:subPropertyOf iapd-sec-cr:hasFirmReportField ;
.
iapd-sec-cr:q5B3
  rdf:type owl:DatatypeProperty ;
  sxml:attribute "Q5B3" ;
  rdfs:label "Question 5B3"^^xsd:string ;
  rdfs:subPropertyOf iapd-sec-cr:hasFirmReportField ;
.
iapd-sec-cr:q5B4
  rdf:type owl:DatatypeProperty ;
  sxml:attribute "Q5B4" ;
  rdfs:label "Question 5B4"^^xsd:string ;
  rdfs:subPropertyOf iapd-sec-cr:hasFirmReportField ;
.
iapd-sec-cr:q5B5
  rdf:type owl:DatatypeProperty ;
  sxml:attribute "Q5B5" ;
  rdfs:label "Question 5B5"^^xsd:string ;
  rdfs:subPropertyOf iapd-sec-cr:hasFirmReportField ;
.
iapd-sec-cr:q5B6
  rdf:type owl:DatatypeProperty ;
  sxml:attribute "Q5B6" ;
  rdfs:label "Question 5B6"^^xsd:string ;
  rdfs:subPropertyOf iapd-sec-cr:hasFirmReportField ;
.
iapd-sec-cr:q5C1
  rdf:type owl:DatatypeProperty ;
  sxml:attribute "Q5C1" ;
  rdfs:label "Question 5C1"^^xsd:string ;
  rdfs:subPropertyOf iapd-sec-cr:hasFirmReportField ;
.
iapd-sec-cr:q5C1Oth
  rdf:type owl:DatatypeProperty ;
  sxml:attribute "Q5C1Oth" ;
  rdfs:label "Question 5C1Oth"^^xsd:string ;
  rdfs:subPropertyOf iapd-sec-cr:hasFirmReportField ;
.
iapd-sec-cr:q5C2
  rdf:type owl:DatatypeProperty ;
  sxml:attribute "Q5C2" ;
  rdfs:label "Question 5C2"^^xsd:string ;
  rdfs:subPropertyOf iapd-sec-cr:hasFirmReportField ;
.
iapd-sec-cr:q5D1A
  rdf:type owl:DatatypeProperty ;
  sxml:attribute "Q5D1A" ;
  rdfs:label "Question 5D1A"^^xsd:string ;
  rdfs:subPropertyOf iapd-sec-cr:hasFirmReportField ;
.
iapd-sec-cr:q5D1B
  rdf:type owl:DatatypeProperty ;
  sxml:attribute "Q5D1B" ;
  rdfs:label "Question 5D1B"^^xsd:string ;
  rdfs:subPropertyOf iapd-sec-cr:hasFirmReportField ;
.
iapd-sec-cr:q5D1C
  rdf:type owl:DatatypeProperty ;
  sxml:attribute "Q5D1C" ;
  rdfs:label "Question 5D1C"^^xsd:string ;
  rdfs:subPropertyOf iapd-sec-cr:hasFirmReportField ;
.
iapd-sec-cr:q5D1D
  rdf:type owl:DatatypeProperty ;
  sxml:attribute "Q5D1D" ;
  rdfs:label "Question 5D1D"^^xsd:string ;
  rdfs:subPropertyOf iapd-sec-cr:hasFirmReportField ;
.
iapd-sec-cr:q5D1E
  rdf:type owl:DatatypeProperty ;
  sxml:attribute "Q5D1E" ;
  rdfs:label "Question 5D1E"^^xsd:string ;
  rdfs:subPropertyOf iapd-sec-cr:hasFirmReportField ;
.
iapd-sec-cr:q5D1F
  rdf:type owl:DatatypeProperty ;
  sxml:attribute "Q5D1F" ;
  rdfs:label "Question 5D1F"^^xsd:string ;
  rdfs:subPropertyOf iapd-sec-cr:hasFirmReportField ;
.
iapd-sec-cr:q5D1G
  rdf:type owl:DatatypeProperty ;
  sxml:attribute "Q5D1G" ;
  rdfs:label "Question 5D1G"^^xsd:string ;
  rdfs:subPropertyOf iapd-sec-cr:hasFirmReportField ;
.
iapd-sec-cr:q5D1H
  rdf:type owl:DatatypeProperty ;
  sxml:attribute "Q5D1H" ;
  rdfs:label "Question 5D1H"^^xsd:string ;
  rdfs:subPropertyOf iapd-sec-cr:hasFirmReportField ;
.
iapd-sec-cr:q5D1I
  rdf:type owl:DatatypeProperty ;
  sxml:attribute "Q5D1I" ;
  rdfs:label "Question 5D1I"^^xsd:string ;
  rdfs:subPropertyOf iapd-sec-cr:hasFirmReportField ;
.
iapd-sec-cr:q5D1J
  rdf:type owl:DatatypeProperty ;
  sxml:attribute "Q5D1J" ;
  rdfs:label "Question 5D1J"^^xsd:string ;
  rdfs:subPropertyOf iapd-sec-cr:hasFirmReportField ;
.
iapd-sec-cr:q5D1K
  rdf:type owl:DatatypeProperty ;
  sxml:attribute "Q5D1K" ;
  rdfs:label "Question 5D1K"^^xsd:string ;
  rdfs:subPropertyOf iapd-sec-cr:hasFirmReportField ;
.
iapd-sec-cr:q5D1L
  rdf:type owl:DatatypeProperty ;
  sxml:attribute "Q5D1L" ;
  rdfs:label "Question 5D1L"^^xsd:string ;
  rdfs:subPropertyOf iapd-sec-cr:hasFirmReportField ;
.
iapd-sec-cr:q5D1M
  rdf:type owl:DatatypeProperty ;
  sxml:attribute "Q5D1M" ;
  rdfs:label "Question 5D1M"^^xsd:string ;
  rdfs:subPropertyOf iapd-sec-cr:hasFirmReportField ;
.
iapd-sec-cr:q5D1MOth
  rdf:type owl:DatatypeProperty ;
  sxml:attribute "Q5D1MOth" ;
  rdfs:label "Question 5D1MOth"^^xsd:string ;
  rdfs:subPropertyOf iapd-sec-cr:hasFirmReportField ;
.
iapd-sec-cr:q5D2A
  rdf:type owl:DatatypeProperty ;
  sxml:attribute "Q5D2A" ;
  rdfs:label "Question 5D2A"^^xsd:string ;
  rdfs:subPropertyOf iapd-sec-cr:hasFirmReportField ;
.
iapd-sec-cr:q5D2B
  rdf:type owl:DatatypeProperty ;
  sxml:attribute "Q5D2B" ;
  rdfs:label "Question 5D2B"^^xsd:string ;
  rdfs:subPropertyOf iapd-sec-cr:hasFirmReportField ;
.
iapd-sec-cr:q5D2C
  rdf:type owl:DatatypeProperty ;
  sxml:attribute "Q5D2C" ;
  rdfs:label "Question 5D2C"^^xsd:string ;
  rdfs:subPropertyOf iapd-sec-cr:hasFirmReportField ;
.
iapd-sec-cr:q5D2D
  rdf:type owl:DatatypeProperty ;
  sxml:attribute "Q5D2D" ;
  rdfs:label "Question 5D2D"^^xsd:string ;
  rdfs:subPropertyOf iapd-sec-cr:hasFirmReportField ;
.
iapd-sec-cr:q5D2E
  rdf:type owl:DatatypeProperty ;
  sxml:attribute "Q5D2E" ;
  rdfs:label "Question 5D2E"^^xsd:string ;
  rdfs:subPropertyOf iapd-sec-cr:hasFirmReportField ;
.
iapd-sec-cr:q5D2F
  rdf:type owl:DatatypeProperty ;
  sxml:attribute "Q5D2F" ;
  rdfs:label "Question 5D2F"^^xsd:string ;
  rdfs:subPropertyOf iapd-sec-cr:hasFirmReportField ;
.
iapd-sec-cr:q5D2G
  rdf:type owl:DatatypeProperty ;
  sxml:attribute "Q5D2G" ;
  rdfs:label "Question 5D2G"^^xsd:string ;
  rdfs:subPropertyOf iapd-sec-cr:hasFirmReportField ;
.
iapd-sec-cr:q5D2H
  rdf:type owl:DatatypeProperty ;
  sxml:attribute "Q5D2H" ;
  rdfs:label "Question 5D2H"^^xsd:string ;
  rdfs:subPropertyOf iapd-sec-cr:hasFirmReportField ;
.
iapd-sec-cr:q5D2I
  rdf:type owl:DatatypeProperty ;
  sxml:attribute "Q5D2I" ;
  rdfs:label "Question 5D2I"^^xsd:string ;
  rdfs:subPropertyOf iapd-sec-cr:hasFirmReportField ;
.
iapd-sec-cr:q5D2J
  rdf:type owl:DatatypeProperty ;
  sxml:attribute "Q5D2J" ;
  rdfs:label "Question 5D2J"^^xsd:string ;
  rdfs:subPropertyOf iapd-sec-cr:hasFirmReportField ;
.
iapd-sec-cr:q5D2K
  rdf:type owl:DatatypeProperty ;
  sxml:attribute "Q5D2K" ;
  rdfs:label "Question 5D2K"^^xsd:string ;
  rdfs:subPropertyOf iapd-sec-cr:hasFirmReportField ;
.
iapd-sec-cr:q5D2L
  rdf:type owl:DatatypeProperty ;
  sxml:attribute "Q5D2L" ;
  rdfs:label "Question 5D2L"^^xsd:string ;
  rdfs:subPropertyOf iapd-sec-cr:hasFirmReportField ;
.
iapd-sec-cr:q5D2M
  rdf:type owl:DatatypeProperty ;
  sxml:attribute "Q5D2M" ;
  rdfs:label "Question 5D2M"^^xsd:string ;
  rdfs:subPropertyOf iapd-sec-cr:hasFirmReportField ;
.
iapd-sec-cr:q5D2MOth
  rdf:type owl:DatatypeProperty ;
  sxml:attribute "Q5D2MOth" ;
  rdfs:label "Question 5D2MOth"^^xsd:string ;
  rdfs:subPropertyOf iapd-sec-cr:hasFirmReportField ;
.
iapd-sec-cr:q5E1
  rdf:type owl:DatatypeProperty ;
  sxml:attribute "Q5E1" ;
  rdfs:label "Question 5E1"^^xsd:string ;
  rdfs:subPropertyOf iapd-sec-cr:hasFirmReportField ;
.
iapd-sec-cr:q5E2
  rdf:type owl:DatatypeProperty ;
  sxml:attribute "Q5E2" ;
  rdfs:label "Question 5E2"^^xsd:string ;
  rdfs:subPropertyOf iapd-sec-cr:hasFirmReportField ;
.
iapd-sec-cr:q5E3
  rdf:type owl:DatatypeProperty ;
  sxml:attribute "Q5E3" ;
  rdfs:label "Question 5E3"^^xsd:string ;
  rdfs:subPropertyOf iapd-sec-cr:hasFirmReportField ;
.
iapd-sec-cr:q5E4
  rdf:type owl:DatatypeProperty ;
  sxml:attribute "Q5E4" ;
  rdfs:label "Question 5E4"^^xsd:string ;
  rdfs:subPropertyOf iapd-sec-cr:hasFirmReportField ;
.
iapd-sec-cr:q5E5
  rdf:type owl:DatatypeProperty ;
  sxml:attribute "Q5E5" ;
  rdfs:label "Question 5E5"^^xsd:string ;
  rdfs:subPropertyOf iapd-sec-cr:hasFirmReportField ;
.
iapd-sec-cr:q5E6
  rdf:type owl:DatatypeProperty ;
  sxml:attribute "Q5E6" ;
  rdfs:label "Question 5E6"^^xsd:string ;
  rdfs:subPropertyOf iapd-sec-cr:hasFirmReportField ;
.
iapd-sec-cr:q5E7
  rdf:type owl:DatatypeProperty ;
  sxml:attribute "Q5E7" ;
  rdfs:label "Question 5E7"^^xsd:string ;
  rdfs:subPropertyOf iapd-sec-cr:hasFirmReportField ;
.
iapd-sec-cr:q5E7Oth
  rdf:type owl:DatatypeProperty ;
  sxml:attribute "Q5E7Oth" ;
  rdfs:label "Question 5E7Oth"^^xsd:string ;
  rdfs:subPropertyOf iapd-sec-cr:hasFirmReportField ;
.
iapd-sec-cr:q5F1
  rdf:type owl:DatatypeProperty ;
  sxml:attribute "Q5F1" ;
  rdfs:label "Question 5F1"^^xsd:string ;
  rdfs:subPropertyOf iapd-sec-cr:hasFirmReportField ;
.
iapd-sec-cr:q5F2A
  rdf:type owl:DatatypeProperty ;
  sxml:attribute "Q5F2A" ;
  rdfs:label "Question 5F2A"^^xsd:string ;
  rdfs:subPropertyOf iapd-sec-cr:hasFirmReportField ;
.
iapd-sec-cr:q5F2B
  rdf:type owl:DatatypeProperty ;
  sxml:attribute "Q5F2B" ;
  rdfs:label "Question 5F2B "^^xsd:string ;
  rdfs:subPropertyOf iapd-sec-cr:hasFirmReportField ;
.
iapd-sec-cr:q5F2C
  rdf:type owl:DatatypeProperty ;
  sxml:attribute "Q5F2C" ;
  rdfs:label "Question 5F2C"^^xsd:string ;
  rdfs:subPropertyOf iapd-sec-cr:hasFirmReportField ;
.
iapd-sec-cr:q5F2D
  rdf:type owl:DatatypeProperty ;
  sxml:attribute "Q5F2D" ;
  rdfs:label "Question 5F2D"^^xsd:string ;
  rdfs:subPropertyOf iapd-sec-cr:hasFirmReportField ;
.
iapd-sec-cr:q5F2E
  rdf:type owl:DatatypeProperty ;
  sxml:attribute "Q5F2E" ;
  rdfs:label "Question 5F2E"^^xsd:string ;
  rdfs:subPropertyOf iapd-sec-cr:hasFirmReportField ;
.
iapd-sec-cr:q5F2F
  rdf:type owl:DatatypeProperty ;
  sxml:attribute "Q5F2F" ;
  rdfs:label "Question 5F2F"^^xsd:string ;
  rdfs:subPropertyOf iapd-sec-cr:hasFirmReportField ;
.
iapd-sec-cr:q5G1
  rdf:type owl:DatatypeProperty ;
  sxml:attribute "Q5G1" ;
  rdfs:label "Question 5G1"^^xsd:string ;
  rdfs:subPropertyOf iapd-sec-cr:hasFirmReportField ;
.
iapd-sec-cr:q5G10
  rdf:type owl:DatatypeProperty ;
  sxml:attribute "Q5G10" ;
  rdfs:label "Question 5G10"^^xsd:string ;
  rdfs:subPropertyOf iapd-sec-cr:hasFirmReportField ;
.
iapd-sec-cr:q5G11
  rdf:type owl:DatatypeProperty ;
  sxml:attribute "Q5G11" ;
  rdfs:label "Question 5G11 "^^xsd:string ;
  rdfs:subPropertyOf iapd-sec-cr:hasFirmReportField ;
.
iapd-sec-cr:q5G12
  rdf:type owl:DatatypeProperty ;
  sxml:attribute "Q5G12" ;
  rdfs:label "Question 5G12"^^xsd:string ;
  rdfs:subPropertyOf iapd-sec-cr:hasFirmReportField ;
.
iapd-sec-cr:q5G12Oth
  rdf:type owl:DatatypeProperty ;
  sxml:attribute "Q5G12Oth" ;
  rdfs:label "Question 5G12Oth"^^xsd:string ;
  rdfs:subPropertyOf iapd-sec-cr:hasFirmReportField ;
.
iapd-sec-cr:q5G2
  rdf:type owl:DatatypeProperty ;
  sxml:attribute "Q5G2" ;
  rdfs:label "Question 5G2"^^xsd:string ;
  rdfs:subPropertyOf iapd-sec-cr:hasFirmReportField ;
.
iapd-sec-cr:q5G3
  rdf:type owl:DatatypeProperty ;
  sxml:attribute "Q5G3" ;
  rdfs:label "Question 5G3"^^xsd:string ;
  rdfs:subPropertyOf iapd-sec-cr:hasFirmReportField ;
.
iapd-sec-cr:q5G4
  rdf:type owl:DatatypeProperty ;
  sxml:attribute "Q5G4" ;
  rdfs:label "Question 5G4"^^xsd:string ;
  rdfs:subPropertyOf iapd-sec-cr:hasFirmReportField ;
.
iapd-sec-cr:q5G5
  rdf:type owl:DatatypeProperty ;
  sxml:attribute "Q5G5" ;
  rdfs:label "Question 5G5"^^xsd:string ;
  rdfs:subPropertyOf iapd-sec-cr:hasFirmReportField ;
.
iapd-sec-cr:q5G6
  rdf:type owl:DatatypeProperty ;
  sxml:attribute "Q5G6" ;
  rdfs:label "Question 5G6"^^xsd:string ;
  rdfs:subPropertyOf iapd-sec-cr:hasFirmReportField ;
.
iapd-sec-cr:q5G7
  rdf:type owl:DatatypeProperty ;
  sxml:attribute "Q5G7" ;
  rdfs:label "Question 5G7"^^xsd:string ;
  rdfs:subPropertyOf iapd-sec-cr:hasFirmReportField ;
.
iapd-sec-cr:q5G8
  rdf:type owl:DatatypeProperty ;
  sxml:attribute "Q5G8" ;
  rdfs:label "Question 5G8"^^xsd:string ;
  rdfs:subPropertyOf iapd-sec-cr:hasFirmReportField ;
.
iapd-sec-cr:q5G9
  rdf:type owl:DatatypeProperty ;
  sxml:attribute "Q5G9" ;
  rdfs:label "Question 5G9"^^xsd:string ;
  rdfs:subPropertyOf iapd-sec-cr:hasFirmReportField ;
.
iapd-sec-cr:q5H
  rdf:type owl:DatatypeProperty ;
  sxml:attribute "Q5H" ;
  rdfs:label "Question 5H"^^xsd:string ;
  rdfs:subPropertyOf iapd-sec-cr:hasFirmReportField ;
.
iapd-sec-cr:q5HMT500
  rdf:type owl:DatatypeProperty ;
  sxml:attribute "Q5HMT500" ;
  rdfs:label "Question 5HMT500"^^xsd:string ;
  rdfs:subPropertyOf iapd-sec-cr:hasFirmReportField ;
.
iapd-sec-cr:q5I1
  rdf:type owl:DatatypeProperty ;
  sxml:attribute "Q5I1" ;
  rdfs:label "Question 5I1"^^xsd:string ;
  rdfs:subPropertyOf iapd-sec-cr:hasFirmReportField ;
.
iapd-sec-cr:q5I2
  rdf:type owl:DatatypeProperty ;
  sxml:attribute "Q5I2" ;
  rdfs:label "Question 5I2"^^xsd:string ;
  rdfs:subPropertyOf iapd-sec-cr:hasFirmReportField ;
.
iapd-sec-cr:q5J
  rdf:type owl:DatatypeProperty ;
  sxml:attribute "Q5J" ;
  rdfs:label "Question 5J"^^xsd:string ;
  rdfs:subPropertyOf iapd-sec-cr:hasFirmReportField ;
.
iapd-sec-cr:q6A1
  rdf:type owl:DatatypeProperty ;
  sxml:attribute "Q6A1" ;
  rdfs:label "Question 6A1"^^xsd:string ;
  rdfs:subPropertyOf iapd-sec-cr:hasFirmReportField ;
.
iapd-sec-cr:q6A10
  rdf:type owl:DatatypeProperty ;
  sxml:attribute "Q6A10" ;
  rdfs:label "Question 6A10"^^xsd:string ;
  rdfs:subPropertyOf iapd-sec-cr:hasFirmReportField ;
.
iapd-sec-cr:q6A11
  rdf:type owl:DatatypeProperty ;
  sxml:attribute "Q6A11" ;
  rdfs:label "Question 6A11"^^xsd:string ;
  rdfs:subPropertyOf iapd-sec-cr:hasFirmReportField ;
.
iapd-sec-cr:q6A12
  rdf:type owl:DatatypeProperty ;
  sxml:attribute "Q6A12" ;
  rdfs:label "Question 6A12"^^xsd:string ;
  rdfs:subPropertyOf iapd-sec-cr:hasFirmReportField ;
.
iapd-sec-cr:q6A13
  rdf:type owl:DatatypeProperty ;
  sxml:attribute "Q6A13" ;
  rdfs:label "Question 6A13"^^xsd:string ;
  rdfs:subPropertyOf iapd-sec-cr:hasFirmReportField ;
.
iapd-sec-cr:q6A14
  rdf:type owl:DatatypeProperty ;
  sxml:attribute "Q6A14" ;
  rdfs:label "Question 6A14"^^xsd:string ;
  rdfs:subPropertyOf iapd-sec-cr:hasFirmReportField ;
.
iapd-sec-cr:q6A14Oth
  rdf:type owl:DatatypeProperty ;
  sxml:attribute "Q6A14Oth" ;
  rdfs:label "Question 6A14Oth"^^xsd:string ;
  rdfs:subPropertyOf iapd-sec-cr:hasFirmReportField ;
.
iapd-sec-cr:q6A2
  rdf:type owl:DatatypeProperty ;
  sxml:attribute "Q6A2" ;
  rdfs:label "Question 6A2"^^xsd:string ;
  rdfs:subPropertyOf iapd-sec-cr:hasFirmReportField ;
.
iapd-sec-cr:q6A3
  rdf:type owl:DatatypeProperty ;
  sxml:attribute "Q6A3" ;
  rdfs:label "Question 6A3"^^xsd:string ;
  rdfs:subPropertyOf iapd-sec-cr:hasFirmReportField ;
.
iapd-sec-cr:q6A4
  rdf:type owl:DatatypeProperty ;
  sxml:attribute "Q6A4" ;
  rdfs:label "Question 6A4"^^xsd:string ;
  rdfs:subPropertyOf iapd-sec-cr:hasFirmReportField ;
.
iapd-sec-cr:q6A5
  rdf:type owl:DatatypeProperty ;
  sxml:attribute "Q6A5" ;
  rdfs:label "Question 6A5"^^xsd:string ;
  rdfs:subPropertyOf iapd-sec-cr:hasFirmReportField ;
.
iapd-sec-cr:q6A6
  rdf:type owl:DatatypeProperty ;
  sxml:attribute "Q6A6" ;
  rdfs:label "Question 6A6"^^xsd:string ;
  rdfs:subPropertyOf iapd-sec-cr:hasFirmReportField ;
.
iapd-sec-cr:q6A7
  rdf:type owl:DatatypeProperty ;
  sxml:attribute "Q6A7" ;
  rdfs:label "Question 6A7"^^xsd:string ;
  rdfs:subPropertyOf iapd-sec-cr:hasFirmReportField ;
.
iapd-sec-cr:q6A8
  rdf:type owl:DatatypeProperty ;
  sxml:attribute "Q6A8" ;
  rdfs:label "Question 6A8"^^xsd:string ;
  rdfs:subPropertyOf iapd-sec-cr:hasFirmReportField ;
.
iapd-sec-cr:q6A9
  rdf:type owl:DatatypeProperty ;
  sxml:attribute "Q6A9" ;
  rdfs:label "Question 6A9"^^xsd:string ;
  rdfs:subPropertyOf iapd-sec-cr:hasFirmReportField ;
.
iapd-sec-cr:q6B1
  rdf:type owl:DatatypeProperty ;
  sxml:attribute "Q6B1" ;
  rdfs:label "Question 6B1"^^xsd:string ;
  rdfs:subPropertyOf iapd-sec-cr:hasFirmReportField ;
.
iapd-sec-cr:q6B2
  rdf:type owl:DatatypeProperty ;
  sxml:attribute "Q6B2" ;
  rdfs:label "Question 6B2"^^xsd:string ;
  rdfs:subPropertyOf iapd-sec-cr:hasFirmReportField ;
.
iapd-sec-cr:q6B3
  rdf:type owl:DatatypeProperty ;
  sxml:attribute "Q6B3" ;
  rdfs:label "Question 6B3"^^xsd:string ;
  rdfs:subPropertyOf iapd-sec-cr:hasFirmReportField ;
.
iapd-sec-cr:q7A1
  rdf:type owl:DatatypeProperty ;
  sxml:attribute "Q7A1" ;
  rdfs:label "Question 7A1"^^xsd:string ;
  rdfs:subPropertyOf iapd-sec-cr:hasFirmReportField ;
.
iapd-sec-cr:q7A10
  rdf:type owl:DatatypeProperty ;
  sxml:attribute "Q7A10" ;
  rdfs:label "Question 7A10"^^xsd:string ;
  rdfs:subPropertyOf iapd-sec-cr:hasFirmReportField ;
.
iapd-sec-cr:q7A11
  rdf:type owl:DatatypeProperty ;
  sxml:attribute "Q7A11" ;
  rdfs:label "Question 7A11"^^xsd:string ;
  rdfs:subPropertyOf iapd-sec-cr:hasFirmReportField ;
.
iapd-sec-cr:q7A12
  rdf:type owl:DatatypeProperty ;
  sxml:attribute "Q7A12" ;
  rdfs:label "Question 7A12"^^xsd:string ;
  rdfs:subPropertyOf iapd-sec-cr:hasFirmReportField ;
.
iapd-sec-cr:q7A13
  rdf:type owl:DatatypeProperty ;
  sxml:attribute "Q7A13" ;
  rdfs:label "Question 7A13"^^xsd:string ;
  rdfs:subPropertyOf iapd-sec-cr:hasFirmReportField ;
.
iapd-sec-cr:q7A14
  rdf:type owl:DatatypeProperty ;
  sxml:attribute "Q7A14" ;
  rdfs:label "Question 7A14"^^xsd:string ;
  rdfs:subPropertyOf iapd-sec-cr:hasFirmReportField ;
.
iapd-sec-cr:q7A15
  rdf:type owl:DatatypeProperty ;
  sxml:attribute "Q7A15" ;
  rdfs:label "Question 7A15"^^xsd:string ;
  rdfs:subPropertyOf iapd-sec-cr:hasFirmReportField ;
.
iapd-sec-cr:q7A16
  rdf:type owl:DatatypeProperty ;
  sxml:attribute "Q7A16" ;
  rdfs:label "Question 7A16"^^xsd:string ;
  rdfs:subPropertyOf iapd-sec-cr:hasFirmReportField ;
.
iapd-sec-cr:q7A2
  rdf:type owl:DatatypeProperty ;
  sxml:attribute "Q7A2" ;
  rdfs:label "Question 7A2"^^xsd:string ;
  rdfs:subPropertyOf iapd-sec-cr:hasFirmReportField ;
.
iapd-sec-cr:q7A3
  rdf:type owl:DatatypeProperty ;
  sxml:attribute "Q7A3" ;
  rdfs:label "Question 7A3"^^xsd:string ;
  rdfs:subPropertyOf iapd-sec-cr:hasFirmReportField ;
.
iapd-sec-cr:q7A4
  rdf:type owl:DatatypeProperty ;
  sxml:attribute "Q7A4" ;
  rdfs:label "Question 7A4"^^xsd:string ;
  rdfs:subPropertyOf iapd-sec-cr:hasFirmReportField ;
.
iapd-sec-cr:q7A5
  rdf:type owl:DatatypeProperty ;
  sxml:attribute "Q7A5" ;
  rdfs:label "Question 7A5"^^xsd:string ;
  rdfs:subPropertyOf iapd-sec-cr:hasFirmReportField ;
.
iapd-sec-cr:q7A6
  rdf:type owl:DatatypeProperty ;
  sxml:attribute "Q7A6" ;
  rdfs:label "Question 7A6"^^xsd:string ;
  rdfs:subPropertyOf iapd-sec-cr:hasFirmReportField ;
.
iapd-sec-cr:q7A7
  rdf:type owl:DatatypeProperty ;
  sxml:attribute "Q7A7" ;
  rdfs:label "Question 7A7"^^xsd:string ;
  rdfs:subPropertyOf iapd-sec-cr:hasFirmReportField ;
.
iapd-sec-cr:q7A8
  rdf:type owl:DatatypeProperty ;
  sxml:attribute "Q7A8" ;
  rdfs:label "Question 7A8"^^xsd:string ;
  rdfs:subPropertyOf iapd-sec-cr:hasFirmReportField ;
.
iapd-sec-cr:q7A9
  rdf:type owl:DatatypeProperty ;
  sxml:attribute "Q7A9" ;
  rdfs:label "Question 7A9"^^xsd:string ;
  rdfs:subPropertyOf iapd-sec-cr:hasFirmReportField ;
.
iapd-sec-cr:q7B
  rdf:type owl:DatatypeProperty ;
  sxml:attribute "Q7B" ;
  rdfs:label "Question 7B"^^xsd:string ;
  rdfs:subPropertyOf iapd-sec-cr:hasFirmReportField ;
.
iapd-sec-cr:q8A1
  rdf:type owl:DatatypeProperty ;
  sxml:attribute "Q8A1" ;
  rdfs:label "Question 8A1"^^xsd:string ;
  rdfs:subPropertyOf iapd-sec-cr:hasFirmReportField ;
.
iapd-sec-cr:q8A2
  rdf:type owl:DatatypeProperty ;
  sxml:attribute "Q8A2" ;
  rdfs:label "Question 8A2"^^xsd:string ;
  rdfs:subPropertyOf iapd-sec-cr:hasFirmReportField ;
.
iapd-sec-cr:q8A3
  rdf:type owl:DatatypeProperty ;
  sxml:attribute "Q8A3" ;
  rdfs:label "Question 8A3"^^xsd:string ;
  rdfs:subPropertyOf iapd-sec-cr:hasFirmReportField ;
.
iapd-sec-cr:q8B1
  rdf:type owl:DatatypeProperty ;
  sxml:attribute "Q8B1" ;
  rdfs:label "Question 8B1"^^xsd:string ;
  rdfs:subPropertyOf iapd-sec-cr:hasFirmReportField ;
.
iapd-sec-cr:q8B2
  rdf:type owl:DatatypeProperty ;
  sxml:attribute "Q8B2" ;
  rdfs:label "Question 8B2"^^xsd:string ;
  rdfs:subPropertyOf iapd-sec-cr:hasFirmReportField ;
.
iapd-sec-cr:q8B3
  rdf:type owl:DatatypeProperty ;
  sxml:attribute "Q8B3" ;
  rdfs:label "Question 8B3"^^xsd:string ;
  rdfs:subPropertyOf iapd-sec-cr:hasFirmReportField ;
.
iapd-sec-cr:q8C1
  rdf:type owl:DatatypeProperty ;
  sxml:attribute "Q8C1" ;
  rdfs:label "Question 8C1"^^xsd:string ;
  rdfs:subPropertyOf iapd-sec-cr:hasFirmReportField ;
.
iapd-sec-cr:q8C2
  rdf:type owl:DatatypeProperty ;
  sxml:attribute "Q8C2" ;
  rdfs:label "Question 8C2"^^xsd:string ;
  rdfs:subPropertyOf iapd-sec-cr:hasFirmReportField ;
.
iapd-sec-cr:q8C3
  rdf:type owl:DatatypeProperty ;
  sxml:attribute "Q8C3" ;
  rdfs:label "Question 8C3"^^xsd:string ;
  rdfs:subPropertyOf iapd-sec-cr:hasFirmReportField ;
.
iapd-sec-cr:q8C4
  rdf:type owl:DatatypeProperty ;
  sxml:attribute "Q8C4" ;
  rdfs:label "Question 8C4"^^xsd:string ;
  rdfs:subPropertyOf iapd-sec-cr:hasFirmReportField ;
.
iapd-sec-cr:q8D
  rdf:type owl:DatatypeProperty ;
  sxml:attribute "Q8D" ;
  rdfs:label "Question 8D"^^xsd:string ;
  rdfs:subPropertyOf iapd-sec-cr:hasFirmReportField ;
.
iapd-sec-cr:q8E
  rdf:type owl:DatatypeProperty ;
  sxml:attribute "Q8E" ;
  rdfs:label "Question 8E"^^xsd:string ;
  rdfs:subPropertyOf iapd-sec-cr:hasFirmReportField ;
.
iapd-sec-cr:q8F
  rdf:type owl:DatatypeProperty ;
  sxml:attribute "Q8F" ;
  rdfs:label "Question 8F"^^xsd:string ;
  rdfs:subPropertyOf iapd-sec-cr:hasFirmReportField ;
.
iapd-sec-cr:q8G1
  rdf:type owl:DatatypeProperty ;
  sxml:attribute "Q8G1" ;
  rdfs:label "Question 8G1"^^xsd:string ;
  rdfs:subPropertyOf iapd-sec-cr:hasFirmReportField ;
.
iapd-sec-cr:q8G2
  rdf:type owl:DatatypeProperty ;
  sxml:attribute "Q8G2" ;
  rdfs:label "Question 8G2"^^xsd:string ;
  rdfs:subPropertyOf iapd-sec-cr:hasFirmReportField ;
.
iapd-sec-cr:q8H
  rdf:type owl:DatatypeProperty ;
  sxml:attribute "Q8H" ;
  rdfs:label "Question 8H"^^xsd:string ;
  rdfs:subPropertyOf iapd-sec-cr:hasFirmReportField ;
.
iapd-sec-cr:q8I
  rdf:type owl:DatatypeProperty ;
  sxml:attribute "Q8I" ;
  rdfs:label "Question 8I"^^xsd:string ;
  rdfs:subPropertyOf iapd-sec-cr:hasFirmReportField ;
.
iapd-sec-cr:q9A1A
  rdf:type owl:DatatypeProperty ;
  sxml:attribute "Q9A1A" ;
  rdfs:label "Question 9A1A"^^xsd:string ;
  rdfs:subPropertyOf iapd-sec-cr:hasFirmReportField ;
.
iapd-sec-cr:q9A1B
  rdf:type owl:DatatypeProperty ;
  sxml:attribute "Q9A1B" ;
  rdfs:label "Question 9A1B"^^xsd:string ;
  rdfs:subPropertyOf iapd-sec-cr:hasFirmReportField ;
.
iapd-sec-cr:q9A2A
  rdf:type owl:DatatypeProperty ;
  sxml:attribute "Q9A2A" ;
  rdfs:label "Question 9A2A"^^xsd:string ;
  rdfs:subPropertyOf iapd-sec-cr:hasFirmReportField ;
.
iapd-sec-cr:q9A2B
  rdf:type owl:DatatypeProperty ;
  sxml:attribute "Q9A2B" ;
  rdfs:label "Question 9A2B"^^xsd:string ;
  rdfs:subPropertyOf iapd-sec-cr:hasFirmReportField ;
.
iapd-sec-cr:q9B1A
  rdf:type owl:DatatypeProperty ;
  sxml:attribute "Q9B1A" ;
  rdfs:label "Question 9B1A"^^xsd:string ;
  rdfs:subPropertyOf iapd-sec-cr:hasFirmReportField ;
.
iapd-sec-cr:q9B1B
  rdf:type owl:DatatypeProperty ;
  sxml:attribute "Q9B1B" ;
  rdfs:label "Question 9B1B"^^xsd:string ;
  rdfs:subPropertyOf iapd-sec-cr:hasFirmReportField ;
.
iapd-sec-cr:q9B2A
  rdf:type owl:DatatypeProperty ;
  sxml:attribute "Q9B2A" ;
  rdfs:label "Question 9B2A"^^xsd:string ;
  rdfs:subPropertyOf iapd-sec-cr:hasFirmReportField ;
.
iapd-sec-cr:q9B2B
  rdf:type owl:DatatypeProperty ;
  sxml:attribute "Q9B2B" ;
  rdfs:label "Question 9B2B"^^xsd:string ;
  rdfs:subPropertyOf iapd-sec-cr:hasFirmReportField ;
.
iapd-sec-cr:q9C1
  rdf:type owl:DatatypeProperty ;
  sxml:attribute "Q9C1" ;
  rdfs:label "Question 9C1"^^xsd:string ;
  rdfs:subPropertyOf iapd-sec-cr:hasFirmReportField ;
.
iapd-sec-cr:q9C2
  rdf:type owl:DatatypeProperty ;
  sxml:attribute "Q9C2" ;
  rdfs:label "Question 9C2"^^xsd:string ;
  rdfs:subPropertyOf iapd-sec-cr:hasFirmReportField ;
.
iapd-sec-cr:q9C3
  rdf:type owl:DatatypeProperty ;
  sxml:attribute "Q9C3" ;
  rdfs:label "Question 9C3"^^xsd:string ;
  rdfs:subPropertyOf iapd-sec-cr:hasFirmReportField ;
.
iapd-sec-cr:q9C4
  rdf:type owl:DatatypeProperty ;
  sxml:attribute "Q9C4" ;
  rdfs:label "Question 9C4"^^xsd:string ;
  rdfs:subPropertyOf iapd-sec-cr:hasFirmReportField ;
.
iapd-sec-cr:q9D1
  rdf:type owl:DatatypeProperty ;
  sxml:attribute "Q9D1" ;
  rdfs:label "Question 9D1"^^xsd:string ;
  rdfs:subPropertyOf iapd-sec-cr:hasFirmReportField ;
.
iapd-sec-cr:q9D2
  rdf:type owl:DatatypeProperty ;
  sxml:attribute "Q9D2" ;
  rdfs:label "Question 9D2"^^xsd:string ;
  rdfs:subPropertyOf iapd-sec-cr:hasFirmReportField ;
.
iapd-sec-cr:q9E
  rdf:type owl:DatatypeProperty ;
  sxml:attribute "Q9E" ;
  rdfs:label "Question 9E"^^xsd:string ;
  rdfs:subPropertyOf iapd-sec-cr:hasFirmReportField ;
.
iapd-sec-cr:q9F
  rdf:type owl:DatatypeProperty ;
  sxml:attribute "Q9F" ;
  rdfs:label "Question 9F"^^xsd:string ;
  rdfs:subPropertyOf iapd-sec-cr:hasFirmReportField ;
.
iapd-sec-cr:rgltrCd
  rdf:type owl:DatatypeProperty ;
  sxml:attribute "RgltrCd" ;
  rdfs:label "Regulator code"^^xsd:string ;
  rdfs:subPropertyOf iapd-sec-cr:hasFirmReportField ;
.
iapd-sec-cr:rgstnRef
  rdf:type owl:ObjectProperty ;
  sxml:tag "Rgstn" ;
  rdfs:label "rgstn ref"^^xsd:string ;
  rdfs:subPropertyOf iapd-sec-cr:hasFirmReportReference ;
  skos:definition "Registration reference links the SEC Firm Type to registrations information."^^xsd:string ;
.
iapd-sec-cr:sECNb
  rdf:type owl:DatatypeProperty ;
  sxml:attribute "SECNb" ;
  rdfs:label "EC number"^^xsd:string ;
  rdfs:subPropertyOf iapd-sec-cr:hasFirmReportField ;
.
iapd-sec-cr:sECRgnCD
  rdf:type owl:DatatypeProperty ;
  sxml:attribute "SECRgnCD" ;
  rdfs:label "EC region code"^^xsd:string ;
  rdfs:subPropertyOf iapd-sec-cr:hasFirmReportField ;
.
iapd-sec-cr:st
  rdf:type owl:DatatypeProperty ;
  sxml:attribute "St" ;
  rdfs:label "State code"^^xsd:string ;
  rdfs:subPropertyOf iapd-sec-cr:hasFirmReportField ;
.
iapd-sec-cr:state
  rdf:type owl:DatatypeProperty ;
  sxml:attribute "State" ;
  rdfs:label "State"^^xsd:string ;
  rdfs:subPropertyOf iapd-sec-cr:hasFirmReportField ;
.
iapd-sec-cr:stateCD
  rdf:type owl:DatatypeProperty ;
  sxml:attribute "StateCD" ;
  rdfs:label "State Code"^^xsd:string ;
  rdfs:subPropertyOf iapd-sec-cr:hasFirmReportField ;
.
iapd-sec-cr:statesRef
  rdf:type owl:ObjectProperty ;
  sxml:tag "States" ;
  rdfs:label "states ref"^^xsd:string ;
  rdfs:subPropertyOf iapd-sec-cr:hasFirmReportReference ;
.
iapd-sec-cr:strt1
  rdf:type owl:DatatypeProperty ;
  sxml:attribute "Strt1" ;
  rdfs:label "Street line 1"^^xsd:string ;
  rdfs:subPropertyOf iapd-sec-cr:hasFirmReportField ;
.
iapd-sec-cr:strt2
  rdf:type owl:DatatypeProperty ;
  sxml:attribute "Strt2" ;
  rdfs:label "Street line 2"^^xsd:string ;
  rdfs:subPropertyOf iapd-sec-cr:hasFirmReportField ;
.
iapd-sec-cr:titleNm
  rdf:type owl:DatatypeProperty ;
  sxml:attribute "TitleNm" ;
  rdfs:label "Title name"^^xsd:string ;
  rdfs:subPropertyOf iapd-sec-cr:hasFirmReportField ;
.
iapd-sec-cr:ttlEmp
  rdf:type owl:DatatypeProperty ;
  sxml:attribute "TtlEmp" ;
  rdfs:label "ttl emp"^^xsd:string ;
  rdfs:subPropertyOf iapd-sec-cr:hasFirmReportField ;
.
iapd-sec-cr:webAddr
  rdf:type owl:DatatypeProperty ;
  sxml:attribute "WebAddr" ;
  rdfs:label "Web address"^^xsd:string ;
  rdfs:subPropertyOf iapd-sec-cr:hasFirmReportField ;
.
iapd-sec-cr:webAddrsRef
  rdf:type owl:ObjectProperty ;
  sxml:tag "WebAddrs" ;
  rdfs:label "web addrs ref"^^xsd:string ;
  rdfs:subPropertyOf iapd-sec-cr:hasFirmReportReference ;
.
<http://fundontology.com/fr/ref/Fund_Legal_Reference.ttl#Form_ADV_gen>
  lkif-expr:bears <http://finregont.com/fro/ref/US_LegalReference.ttl#Definitional_Expression_US_Investment_Adviser_Regulation> ;
.
skos:prefLabel
  rdf:type owl:AnnotationProperty ;
  rdfs:label "pref label"^^xsd:string ;
.
