# baseURI: https://spec.edmcouncil.org/fibo/ontology/master/2021Q4/FBC/FunctionalEntities/Markets/
# imports: https://spec.edmcouncil.org/fibo/ontology/master/2021Q4/FBC/FunctionalEntities/RegistrationAuthorities/
# imports: https://spec.edmcouncil.org/fibo/ontology/master/2021Q4/FBC/FunctionalEntities/RegulatoryAgencies/
# imports: https://spec.edmcouncil.org/fibo/ontology/master/2021Q4/FBC/ProductsAndServices/FinancialProductsAndServices/
# imports: https://spec.edmcouncil.org/fibo/ontology/master/2021Q4/FND/Arrangements/Arrangements/
# imports: https://spec.edmcouncil.org/fibo/ontology/master/2021Q4/FND/Arrangements/Lifecycles/
# imports: https://spec.edmcouncil.org/fibo/ontology/master/2021Q4/FND/Law/Jurisdiction/
# imports: https://spec.edmcouncil.org/fibo/ontology/master/2021Q4/FND/Organizations/FormalOrganizations/
# imports: https://spec.edmcouncil.org/fibo/ontology/master/2021Q4/FND/Organizations/Organizations/
# imports: https://spec.edmcouncil.org/fibo/ontology/master/2021Q4/FND/Parties/Roles/
# imports: https://spec.edmcouncil.org/fibo/ontology/master/2021Q4/FND/Places/Facilities/
# imports: https://spec.edmcouncil.org/fibo/ontology/master/2021Q4/FND/Places/Locations/
# imports: https://spec.edmcouncil.org/fibo/ontology/master/2021Q4/FND/Places/VirtualPlaces/
# imports: https://spec.edmcouncil.org/fibo/ontology/master/2021Q4/FND/Relations/Relations/
# imports: https://spec.edmcouncil.org/fibo/ontology/master/2021Q4/FND/Utilities/AnnotationVocabulary/
# imports: https://www.omg.org/spec/LCC/Countries/CountryRepresentation/
# imports: https://www.omg.org/spec/LCC/Languages/LanguageRepresentation/

@base <https://spec.edmcouncil.org/fibo/ontology/master/2021Q4/FBC/FunctionalEntities/Markets/> .
@prefix dct: <http://purl.org/dc/terms/> .
@prefix fibo-fbc-fct-mkt: <https://spec.edmcouncil.org/fibo/ontology/FBC/FunctionalEntities/Markets/> .
@prefix fibo-fbc-fct-ra: <https://spec.edmcouncil.org/fibo/ontology/FBC/FunctionalEntities/RegistrationAuthorities/> .
@prefix fibo-fbc-fct-rga: <https://spec.edmcouncil.org/fibo/ontology/FBC/FunctionalEntities/RegulatoryAgencies/> .
@prefix fibo-fbc-pas-fpas: <https://spec.edmcouncil.org/fibo/ontology/FBC/ProductsAndServices/FinancialProductsAndServices/> .
@prefix fibo-fnd-arr-arr: <https://spec.edmcouncil.org/fibo/ontology/FND/Arrangements/Arrangements/> .
@prefix fibo-fnd-arr-lif: <https://spec.edmcouncil.org/fibo/ontology/FND/Arrangements/Lifecycles/> .
@prefix fibo-fnd-law-jur: <https://spec.edmcouncil.org/fibo/ontology/FND/Law/Jurisdiction/> .
@prefix fibo-fnd-org-fm: <https://spec.edmcouncil.org/fibo/ontology/FND/Organizations/FormalOrganizations/> .
@prefix fibo-fnd-org-org: <https://spec.edmcouncil.org/fibo/ontology/FND/Organizations/Organizations/> .
@prefix fibo-fnd-plc-fac: <https://spec.edmcouncil.org/fibo/ontology/FND/Places/Facilities/> .
@prefix fibo-fnd-plc-loc: <https://spec.edmcouncil.org/fibo/ontology/FND/Places/Locations/> .
@prefix fibo-fnd-pty-rl: <https://spec.edmcouncil.org/fibo/ontology/FND/Parties/Roles/> .
@prefix fibo-fnd-rel-rel: <https://spec.edmcouncil.org/fibo/ontology/FND/Relations/Relations/> .
@prefix fibo-fnd-utl-av: <https://spec.edmcouncil.org/fibo/ontology/FND/Utilities/AnnotationVocabulary/> .
@prefix lcc-cr: <https://www.omg.org/spec/LCC/Countries/CountryRepresentation/> .
@prefix lcc-lr: <https://www.omg.org/spec/LCC/Languages/LanguageRepresentation/> .
@prefix owl: <http://www.w3.org/2002/07/owl#> .
@prefix rdf: <http://www.w3.org/1999/02/22-rdf-syntax-ns#> .
@prefix rdfs: <http://www.w3.org/2000/01/rdf-schema#> .
@prefix skos: <http://www.w3.org/2004/02/skos/core#> .
@prefix sm: <http://www.omg.org/techprocess/ab/SpecificationMetadata/> .
@prefix xsd: <http://www.w3.org/2001/XMLSchema#> .

<https://spec.edmcouncil.org/fibo/ontology/FBC/FunctionalEntities/Markets/>
	a owl:Ontology ;
	rdfs:label "Markets Ontology" ;
	dct:abstract "This ontology defines the fundamental concepts for markets, exchanges, regulated markets, and multilateral trading facilities." ;
	dct:license "http://opensource.org/licenses/MIT"^^xsd:anyURI ;
	sm:contentLanguage <https://www.w3.org/TR/owl2-quick-reference/> ;
	sm:copyright
		"Copyright (c) 2015-2021 EDM Council, Inc." ,
		"Copyright (c) 2015-2021 Object Management Group, Inc."
		;
	sm:dependsOn
		<https://spec.edmcouncil.org/fibo/ontology/FBC/FunctionalEntities/RegistrationAuthorities/> ,
		<https://spec.edmcouncil.org/fibo/ontology/FBC/FunctionalEntities/RegulatoryAgencies/> ,
		<https://spec.edmcouncil.org/fibo/ontology/FBC/ProductsAndServices/FinancialProductsAndServices/> ,
		<https://spec.edmcouncil.org/fibo/ontology/FND/> ,
		<https://www.omg.org/spec/LCC/>
		;
	sm:fileAbbreviation "fibo-fbc-fct-mkt" ;
	sm:filename "Markets.rdf" ;
	owl:imports
		<https://spec.edmcouncil.org/fibo/ontology/master/2021Q4/FBC/FunctionalEntities/RegistrationAuthorities/> ,
		<https://spec.edmcouncil.org/fibo/ontology/master/2021Q4/FBC/FunctionalEntities/RegulatoryAgencies/> ,
		<https://spec.edmcouncil.org/fibo/ontology/master/2021Q4/FBC/ProductsAndServices/FinancialProductsAndServices/> ,
		<https://spec.edmcouncil.org/fibo/ontology/master/2021Q4/FND/Arrangements/Arrangements/> ,
		<https://spec.edmcouncil.org/fibo/ontology/master/2021Q4/FND/Arrangements/Lifecycles/> ,
		<https://spec.edmcouncil.org/fibo/ontology/master/2021Q4/FND/Law/Jurisdiction/> ,
		<https://spec.edmcouncil.org/fibo/ontology/master/2021Q4/FND/Organizations/FormalOrganizations/> ,
		<https://spec.edmcouncil.org/fibo/ontology/master/2021Q4/FND/Organizations/Organizations/> ,
		<https://spec.edmcouncil.org/fibo/ontology/master/2021Q4/FND/Parties/Roles/> ,
		<https://spec.edmcouncil.org/fibo/ontology/master/2021Q4/FND/Places/Facilities/> ,
		<https://spec.edmcouncil.org/fibo/ontology/master/2021Q4/FND/Places/Locations/> ,
		<https://spec.edmcouncil.org/fibo/ontology/master/2021Q4/FND/Places/VirtualPlaces/> ,
		<https://spec.edmcouncil.org/fibo/ontology/master/2021Q4/FND/Relations/Relations/> ,
		<https://spec.edmcouncil.org/fibo/ontology/master/2021Q4/FND/Utilities/AnnotationVocabulary/> ,
		<https://www.omg.org/spec/LCC/Countries/CountryRepresentation/> ,
		<https://www.omg.org/spec/LCC/Languages/LanguageRepresentation/>
		;
	owl:versionIRI <https://spec.edmcouncil.org/fibo/ontology/master/2021Q4/FBC/FunctionalEntities/Markets/> ;
	skos:changeNote
		"The https://spec.edmcouncil.org/fibo/ontology/FBC/FunctionalEntities/Markets/ version of this ontology was modified per the FIBO 2.0 RFC." ,
		"The https://spec.edmcouncil.org/fibo/ontology/FBC/FunctionalEntities/Markets/ version of this ontology was modified to add the definition of an exchange participant and loosen constraints on the location in which a given exchange operates, given that there are cases when an exchange may operate in multiple locations." ,
		"The https://spec.edmcouncil.org/fibo/ontology/FBC/FunctionalEntities/Markets/ version of this ontology was modified to add: 'off-market', with synonyms of 'off-facility' and 'off-book', 'auction market' for periodic or on-demand auction markets, 'dark pool', and 'quote-driven market' for those that have QUOTE or RFQ in their name excluding QUOTED FUNDS, and other 'alternative trading system's; also moved 'designated contract market' and 'swap execution facility' from DER to the this ontology for use in generating proper classification of the ISO MIC codes." ,
		"The https://spec.edmcouncil.org/fibo/ontology/FBC/FunctionalEntities/Markets/ version of this ontology was modified to eliminate deprecated elements." ,
		"The https://spec.edmcouncil.org/fibo/ontology/FBC/FunctionalEntities/Markets/ version of this ontology was modified to eliminate duplication of concepts in LCC, simplify addresses, merge countries with locations in FND, and correct the declaration of the property 'operates in municipality' to be an object property." ,
		"The https://spec.edmcouncil.org/fibo/ontology/FBC/FunctionalEntities/Markets/ version of this ontology was modified to generalize certain unions where they were no longer required and to move international registration authorities individuals to a separate ontology for better modularity." ,
		"The https://spec.edmcouncil.org/fibo/ontology/FBC/FunctionalEntities/Markets/ version of this ontology was modified to integrated details from the redundant 'securities exchange' concept with 'exchange'." ,
		"The https://spec.edmcouncil.org/fibo/ontology/FBC/FunctionalEntities/Markets/ version of this ontology was modified to reflect issue resolutions detailed in the FIBO FBC 1.0 RTF report." ,
		"The https://spec.edmcouncil.org/fibo/ontology/FBC/FunctionalEntities/Markets/ version of this ontology was modified to replace the hasTag property in Relations with the LCC equivalent on nominals."
		;
	fibo-fnd-utl-av:hasMaturityLevel fibo-fnd-utl-av:Release ;
	.

fibo-fbc-fct-mkt:ActiveMICStatus
	a
		owl:NamedIndividual ,
		fibo-fbc-fct-mkt:MarketIdentifierCodeStatus
		;
	rdfs:label "active MIC status" ;
	rdfs:isDefinedBy <https://spec.edmcouncil.org/fibo/ontology/FBC/FunctionalEntities/Markets/> ;
	skos:definition "as of the last report or update, the exchange code was registered and actively in use" ;
	fibo-fnd-utl-av:adaptedFrom "ISO 10383, Securities and related financial instruments - Codes for exchanges and market identification (MIC), Third edition, 2012-10-01" ;
	lcc-lr:hasTag "ACTIVE" ;
	.

fibo-fbc-fct-mkt:AlternativeTradingSystem
	a owl:Class ;
	rdfs:subClassOf fibo-fbc-fct-mkt:Exchange ;
	rdfs:label "alternative trading system" ;
	rdfs:isDefinedBy <https://spec.edmcouncil.org/fibo/ontology/FBC/FunctionalEntities/Markets/> ;
	skos:definition "trading venue that is more loosely regulated than a regulated exchange" ;
	fibo-fnd-utl-av:abbreviation "ATS" ;
	fibo-fnd-utl-av:explanatoryNote "The SEC formally defines an alternative trading system as any organization, association, person, group of persons, or systems (1) that constitutes, maintains, or provides a market place or facilities for bringing together purchasers and sellers of securities or for otherwise performing with respect to securities the functions commonly performed by a stock exchange within the meaning of Rule 3b-16 under the Exchange Act; and (2) that does not (i) set rules governing the conduct of subscribers other than the conduct of such subscribers' trading on such organization, association, person, group of persons, or system, or (ii) discipline subscribers other than by exclusion from trading." ;
	.

fibo-fbc-fct-mkt:AuctionMarket
	a owl:Class ;
	rdfs:subClassOf fibo-fbc-fct-mkt:Exchange ;
	rdfs:label "auction market" ;
	rdfs:isDefinedBy <https://spec.edmcouncil.org/fibo/ontology/FBC/FunctionalEntities/Markets/> ;
	skos:definition "exchange in which buyers and sellers submit competitive bids that do not involve direct negotiations between parties, as part of an auction scheduled either on demand or on a periodic basis" ;
	.

fibo-fbc-fct-mkt:DarkPool
	a owl:Class ;
	rdfs:subClassOf fibo-fbc-fct-mkt:AlternativeTradingSystem ;
	rdfs:label "dark pool" ;
	rdfs:isDefinedBy <https://spec.edmcouncil.org/fibo/ontology/FBC/FunctionalEntities/Markets/> ;
	skos:definition "privately organized alternative trading system, that allows institutional investors the ability to trade without exposure until after the trade has been executed and reported" ;
	.

fibo-fbc-fct-mkt:DeletedMICStatus
	a
		owl:NamedIndividual ,
		fibo-fbc-fct-mkt:MarketIdentifierCodeStatus
		;
	rdfs:label "deleted MIC status" ;
	rdfs:isDefinedBy <https://spec.edmcouncil.org/fibo/ontology/FBC/FunctionalEntities/Markets/> ;
	skos:definition "as of the last report or update, the exchange code was deleted" ;
	fibo-fnd-utl-av:adaptedFrom "ISO 10383, Securities and related financial instruments - Codes for exchanges and market identification (MIC), Third edition, 2012-10-01" ;
	lcc-lr:hasTag "DELETED" ;
	.

fibo-fbc-fct-mkt:DesignatedContractMarket
	a owl:Class ;
	rdfs:subClassOf fibo-fbc-fct-mkt:Exchange ;
	rdfs:label "designated contract market" ;
	rdfs:isDefinedBy <https://spec.edmcouncil.org/fibo/ontology/FBC/FunctionalEntities/Markets/> ;
	skos:definition "exchange, trading system, or platform that enables listing for trading futures or option contracts based on any underlying commodity, index or instrument" ;
	fibo-fnd-utl-av:abbreviation "DCM" ;
	fibo-fnd-utl-av:adaptedFrom "http://www.cftc.gov/IndustryOversight/TradingOrganizations/DCMs/index.htm"^^xsd:anyURI ;
	.

fibo-fbc-fct-mkt:ElectronicCommunicationNetwork
	a owl:Class ;
	rdfs:subClassOf fibo-fbc-fct-mkt:AlternativeTradingSystem ;
	rdfs:label "electronic communication network" ;
	rdfs:isDefinedBy <https://spec.edmcouncil.org/fibo/ontology/FBC/FunctionalEntities/Markets/> ;
	rdfs:seeAlso <https://www.cfainstitute.org/-/media/documents/issue-brief/dark-pools-internalization-and-equity-market-quality-issue-brief> ;
	owl:disjointWith fibo-fbc-fct-mkt:DarkPool ;
	skos:definition "alternative trading system that automatically matches buy and sell orders for securities in the market" ;
	fibo-fnd-utl-av:abbreviation "ECN" ;
	fibo-fnd-utl-av:explanatoryNote "ECNs allow brokerages and investors in different geographic areas to trade without a third party involved, offering privacy for investors. They also allow after-hours trading, but trading may be subject to commissions and other fees." ;
	.

fibo-fbc-fct-mkt:Exchange
	a owl:Class ;
	rdfs:subClassOf
		fibo-fbc-pas-fpas:FinancialServiceProvider ,
		fibo-fnd-plc-fac:Facility ,
		[
			a owl:Restriction ;
			owl:onProperty fibo-fbc-fct-mkt:hasExchangeAcronym ;
			owl:minQualifiedCardinality "0"^^xsd:nonNegativeInteger ;
			owl:onDataRange rdfs:Literal ;
		] ,
		[
			a owl:Restriction ;
			owl:onProperty fibo-fbc-fct-mkt:hasExchangeName ;
			owl:someValuesFrom rdfs:Literal ;
		] ,
		[
			a owl:Restriction ;
			owl:onProperty fibo-fbc-fct-mkt:operatesInCountry ;
			owl:someValuesFrom lcc-cr:Country ;
		] ,
		[
			a owl:Restriction ;
			owl:onProperty fibo-fbc-fct-mkt:operatesInMunicipality ;
			owl:someValuesFrom fibo-fnd-plc-loc:Municipality ;
		] ,
		[
			a owl:Restriction ;
			owl:onProperty fibo-fnd-rel-rel:hasIdentity ;
			owl:someValuesFrom fibo-fnd-org-fm:FormalOrganization ;
		] ,
		[
			a owl:Restriction ;
			owl:onProperty lcc-lr:isIdentifiedBy ;
			owl:someValuesFrom fibo-fbc-fct-mkt:MarketIdentifier ;
		]
		;
	rdfs:label "exchange" ;
	rdfs:isDefinedBy <https://spec.edmcouncil.org/fibo/ontology/FBC/FunctionalEntities/Markets/> ;
	skos:definition "any organization, association, or group of persons, whether incorporated or unincorporated, which constitutes, maintains, or provides a facility for bringing together purchasers and sellers of financial instruments, commodities, or other products, services, or goods, and includes the market place and facilities maintained by such exchange" ;
	fibo-fnd-utl-av:adaptedFrom
		"ISO 10383, Securities and related financial instruments - Codes for exchanges and market identification (MIC), Third edition, 2012-10-01" ,
		"Securities Exchange Act of 1934, as amended 12 August 2012"
		;
	fibo-fnd-utl-av:explanatoryNote """An exchange is typically a corporation or mutual organization that provides securities trading services, where securities may be bought and sold by third parties. As a facility, an exchange is also a place of trade associated with a particular site, i.e., stock exchange, regulated market such as an Electronic Trading Platform (ECN), or unregulated market, such as an Automated Trading System (ATS) (MIC - ISO 10383). Stock exchanges also provide facilities for the issue and redemption of securities as well as other financial instruments and capital events including the payment of income and dividends.

The securities traded on a stock exchange include: shares issued by companies, unit trusts, derivatives, pooled investment products and bonds. To be able to trade a security on a certain stock exchange, it has to be listed there. Usually there is a central location at least for recordkeeping, but trade is less and less linked to such a physical place, as modern markets are electronic networks, which gives them advantages of speed and cost of transactions. Trade on an exchange is by members only.""" ;
	fibo-fnd-utl-av:synonym "market" ;
	.

fibo-fbc-fct-mkt:ExchangeParticipant
	a owl:Class ;
	rdfs:subClassOf
		fibo-fbc-pas-fpas:RegisteredAgent ,
		fibo-fnd-org-org:OrganizationMember ,
		[
			a owl:Restriction ;
			owl:onProperty fibo-fbc-fct-ra:isRegisteredBy ;
			owl:someValuesFrom fibo-fbc-fct-mkt:Exchange ;
		] ,
		[
			a owl:Restriction ;
			owl:onProperty fibo-fnd-pty-rl:isPlayedBy ;
			owl:someValuesFrom [
				a owl:Restriction ;
				owl:onProperty lcc-lr:isMemberOf ;
				owl:someValuesFrom [
					a owl:Restriction ;
					owl:onProperty fibo-fnd-pty-rl:playsRole ;
					owl:someValuesFrom fibo-fbc-fct-mkt:Exchange ;
				] ;
			] ;
		]
		;
	rdfs:label "exchange participant" ;
	rdfs:isDefinedBy <https://spec.edmcouncil.org/fibo/ontology/FBC/FunctionalEntities/Markets/> ;
	rdfs:seeAlso <https://www.lawinsider.com/dictionary/exchange-participant> ;
	skos:definition "registered agent who, in accordance with the rules of an exchange, may trade on or through the exchange and whose name is entered in a list, register or roll kept by the exchange as an agent who may trade on or through the exchange" ;
	.

fibo-fbc-fct-mkt:MarketIdentifier
	a owl:Class ;
	rdfs:subClassOf
		lcc-lr:Identifier ,
		[
			a owl:Restriction ;
			owl:onProperty lcc-lr:identifies ;
			owl:onClass fibo-fbc-fct-mkt:Exchange ;
			owl:qualifiedCardinality "1"^^xsd:nonNegativeInteger ;
		] ,
		[
			a owl:Restriction ;
			owl:onProperty fibo-fbc-fct-mkt:hasOperatingOrSegmentIndicator ;
			owl:onDataRange xsd:string ;
			owl:qualifiedCardinality "1"^^xsd:nonNegativeInteger ;
		]
		;
	rdfs:label "market identifier" ;
	rdfs:isDefinedBy <https://spec.edmcouncil.org/fibo/ontology/FBC/FunctionalEntities/Markets/> ;
	skos:definition "an identifier and code that specifies a universal method of identifying exchanges, trading platforms and regulated or non-regulated markets as sources of prices and related information in order to facilitate automated processing, i.e., stock exchanges, regulated markets, e.g., Electronic Trading Platforms (ECN), and unregulated markets, e.g., Automated Trading Systems (ATS)" ;
	fibo-fnd-utl-av:abbreviation "MIC" ;
	fibo-fnd-utl-av:adaptedFrom
		"ISO 10383, Securities and related financial instruments - Codes for exchanges and market identification (MIC), Third edition, 2012-10-01" ,
		"https://www.anna-web.org/standards/mic-iso-10383/"^^xsd:anyURI ,
		"https://www.iso20022.org/10383/iso-10383-market-identifier-codes"^^xsd:anyURI
		;
	fibo-fnd-utl-av:explanatoryNote """It is intended for use in any application and communication for identification of places
- where a financial instrument is listed (place of official listing),
- where a related trade is executed (place of trade), and
- where trade details are reported (trade reporting facility).""" ;
	fibo-fnd-utl-av:synonym "Market Identifier Code" ;
	.

fibo-fbc-fct-mkt:MarketIdentifierCodeStatus
	a owl:Class ;
	rdfs:subClassOf fibo-fnd-arr-lif:LifecycleStage ;
	rdfs:label "market indicator code status" ;
	rdfs:isDefinedBy <https://spec.edmcouncil.org/fibo/ontology/FBC/FunctionalEntities/Markets/> ;
	skos:definition "a lifecycle stage indicating the status of the MIC code, as specified by the registration authority" ;
	fibo-fnd-utl-av:adaptedFrom "https://www.iso20022.org/10383/iso-10383-market-identifier-codes"^^xsd:anyURI ;
	.

fibo-fbc-fct-mkt:MarketSegmentLevelMarket
	a owl:Class ;
	rdfs:subClassOf
		fibo-fbc-fct-mkt:Exchange ,
		[
			a owl:Restriction ;
			owl:onProperty lcc-lr:isIdentifiedBy ;
			owl:onClass fibo-fbc-fct-mkt:MarketSegmentLevelMarketIdentifier ;
			owl:minQualifiedCardinality "0"^^xsd:nonNegativeInteger ;
		] ,
		[
			a owl:Restriction ;
			owl:onProperty fibo-fnd-arr-arr:isConstituentOf ;
			owl:onClass fibo-fbc-fct-mkt:OperatingLevelMarket ;
			owl:qualifiedCardinality "1"^^xsd:nonNegativeInteger ;
		]
		;
	rdfs:label "market segment-level market" ;
	rdfs:isDefinedBy <https://spec.edmcouncil.org/fibo/ontology/FBC/FunctionalEntities/Markets/> ;
	skos:definition "an exchange/market/trade reporting facility that specializes in one or more specific instruments or that is regulated uniquely from the operating-level market that manages it" ;
	fibo-fnd-utl-av:adaptedFrom "ISO 10383, Securities and related financial instruments - Codes for exchanges and market identification (MIC), Third edition, 2012-10-01" ;
	.

fibo-fbc-fct-mkt:MarketSegmentLevelMarketIdentifier
	a owl:Class ;
	rdfs:subClassOf
		fibo-fbc-fct-mkt:MarketIdentifier ,
		[
			a owl:Restriction ;
			owl:onProperty fibo-fbc-fct-mkt:hasOperatingOrSegmentIndicator ;
			owl:hasValue "S" ;
		]
		;
	rdfs:label "market segment-level market identifier" ;
	rdfs:isDefinedBy <https://spec.edmcouncil.org/fibo/ontology/FBC/FunctionalEntities/Markets/> ;
	skos:definition "a market identifier that identifies a section of an exchange/market/trade reporting facility that specializes in one or more specific instruments or that is regulated differently" ;
	fibo-fnd-utl-av:adaptedFrom "ISO 10383, Securities and related financial instruments - Codes for exchanges and market identification (MIC), Third edition, 2012-10-01" ;
	.

fibo-fbc-fct-mkt:ModifiedMICStatus
	a
		owl:NamedIndividual ,
		fibo-fbc-fct-mkt:MarketIdentifierCodeStatus
		;
	rdfs:label "modified MIC status" ;
	rdfs:isDefinedBy <https://spec.edmcouncil.org/fibo/ontology/FBC/FunctionalEntities/Markets/> ;
	skos:definition "as of the last report or update, the exchange code was revised" ;
	fibo-fnd-utl-av:adaptedFrom "ISO 10383, Securities and related financial instruments - Codes for exchanges and market identification (MIC), Third edition, 2012-10-01" ;
	lcc-lr:hasTag "MODIFIED" ;
	.

fibo-fbc-fct-mkt:MultilateralTradingFacility
	a owl:Class ;
	rdfs:subClassOf
		fibo-fbc-fct-mkt:AlternativeTradingSystem ,
		[
			a owl:Restriction ;
			owl:onProperty fibo-fnd-rel-rel:isManagedBy ;
			owl:allValuesFrom fibo-fbc-pas-fpas:FinancialServiceProvider ;
		]
		;
	rdfs:label "multilateral trading facility" ;
	rdfs:isDefinedBy <https://spec.edmcouncil.org/fibo/ontology/FBC/FunctionalEntities/Markets/> ;
	skos:definition "trading system that facilitates the exchange of financial instruments between multiple parties" ;
	fibo-fnd-utl-av:abbreviation "MTF" ;
	fibo-fnd-utl-av:adaptedFrom "http://www.investopedia.com/terms/m/multilateral_trading_facility.asp" ;
	fibo-fnd-utl-av:explanatoryNote "Multilateral trading facilities allow eligible contract participants to gather and transfer a variety of securities, especially instruments that may not have an official market. These facilities are often electronic systems controlled by approved market operators or larger investment banks. Traders will usually submit orders electronically, where a matching software engine is used to pair buyers with sellers." ;
	.

fibo-fbc-fct-mkt:OffMarketFacility
	a owl:Class ;
	rdfs:subClassOf fibo-fbc-fct-mkt:Exchange ;
	rdfs:label "off-market facility" ;
	rdfs:isDefinedBy <https://spec.edmcouncil.org/fibo/ontology/FBC/FunctionalEntities/Markets/> ;
	skos:definition "facility used for reporting over-the-counter (OTC) and other direct trades that are not executed by the exchange but are reported through the exchange" ;
	fibo-fnd-utl-av:synonym
		"off-book" ,
		"off-facility"
		;
	.

fibo-fbc-fct-mkt:OperatingLevelMarket
	a owl:Class ;
	rdfs:subClassOf
		fibo-fbc-fct-mkt:Exchange ,
		[
			a owl:Restriction ;
			owl:onProperty lcc-lr:isIdentifiedBy ;
			owl:someValuesFrom fibo-fbc-fct-mkt:OperatingLevelMarketIdentifier ;
		]
		;
	rdfs:label "operating-level market" ;
	rdfs:isDefinedBy <https://spec.edmcouncil.org/fibo/ontology/FBC/FunctionalEntities/Markets/> ;
	skos:definition "exchange/market/trade/reporting facility that operates in a specific market/country" ;
	fibo-fnd-utl-av:adaptedFrom "ISO 10383, Securities and related financial instruments - Codes for exchanges and market identification (MIC), Third edition, 2012-10-01" ;
	.

fibo-fbc-fct-mkt:OperatingLevelMarketIdentifier
	a owl:Class ;
	rdfs:subClassOf
		fibo-fbc-fct-mkt:MarketIdentifier ,
		[
			a owl:Restriction ;
			owl:onProperty fibo-fbc-fct-mkt:hasOperatingOrSegmentIndicator ;
			owl:hasValue "O" ;
		]
		;
	rdfs:label "operating-level market identifier" ;
	rdfs:isDefinedBy <https://spec.edmcouncil.org/fibo/ontology/FBC/FunctionalEntities/Markets/> ;
	skos:definition "market identifier that identifies an entity operating an exchange/market/trade/reporting facility that operates in a specific market/country" ;
	fibo-fnd-utl-av:adaptedFrom "ISO 10383, Securities and related financial instruments - Codes for exchanges and market identification (MIC), Third edition, 2012-10-01" ;
	.

fibo-fbc-fct-mkt:OrganizedTradingFacility
	a owl:Class ;
	rdfs:subClassOf
		fibo-fbc-fct-mkt:AlternativeTradingSystem ,
		[
			a owl:Restriction ;
			owl:onProperty fibo-fnd-rel-rel:isManagedBy ;
			owl:allValuesFrom fibo-fbc-pas-fpas:FinancialServiceProvider ;
		] ,
		[
			a owl:Restriction ;
			owl:onProperty fibo-fnd-rel-rel:isGovernedBy ;
			owl:someValuesFrom fibo-fnd-law-jur:Jurisdiction ;
		]
		;
	rdfs:label "organized trading facility" ;
	rdfs:isDefinedBy <https://spec.edmcouncil.org/fibo/ontology/FBC/FunctionalEntities/Markets/> ;
	rdfs:seeAlso <https://www.financierworldwide.com/organised-trading-facilities-how-they-differ-from-mtfs> ;
	owl:disjointWith
		fibo-fbc-fct-mkt:MultilateralTradingFacility ,
		fibo-fbc-fct-mkt:RegulatedExchange
		;
	skos:definition "multi-lateral system which is not an RM or an MTF and in which multiple third-party buying and selling interests in bonds, structured finance products, emission allowances or derivatives are able to interact in the system in a way that results in a contract in accordance with the provisions of Title II of MiFID II" ;
	fibo-fnd-utl-av:abbreviation "OTF" ;
	fibo-fnd-utl-av:adaptedFrom "http://www.marketswiki.com/mwiki/Organized_Trading_Facility" ;
	fibo-fnd-utl-av:explanatoryNote
		"""OTFs were introduced by the European Commission as part of MiFID II and are focused on non-equities such as derivatives and cash bond markets.

OTFs are intended to be similar in scope to a swap execution facility (SEF), a type of entity created by the Dodd-Frank Act in the U.S. The goal of SEFs and OTFs is to bring transparency and structure to OTC derivatives trading.""" ,
		"Unlike RMs and MTFs, operators of OTFs will have discretion as to how to execute orders, subject to pre-transparency and best execution obligations."
		;
	.

fibo-fbc-fct-mkt:QuoteDrivenMarket
	a owl:Class ;
	rdfs:subClassOf fibo-fbc-fct-mkt:Exchange ;
	rdfs:label "quote-driven market" ;
	rdfs:isDefinedBy <https://spec.edmcouncil.org/fibo/ontology/FBC/FunctionalEntities/Markets/> ;
	skos:definition "exchange in which prices are determined from bid and ask quotations made by market makers, dealers, or specialists" ;
	fibo-fnd-utl-av:explanatoryNote "In a quote-driven market, dealers fill orders from their own inventory or by matching them with other orders. Note that this differs from a typical market, which is order-driven rather than quote-driven." ;
	fibo-fnd-utl-av:synonym "price-driven market" ;
	.

fibo-fbc-fct-mkt:RegisteredMultilateralTradingFacility
	a owl:Class ;
	rdfs:subClassOf
		fibo-fbc-fct-mkt:MultilateralTradingFacility ,
		[
			a owl:Restriction ;
			owl:onProperty fibo-fbc-fct-ra:isRegisteredBy ;
			owl:someValuesFrom fibo-fbc-fct-ra:RegistrationAuthority ;
		] ,
		[
			a owl:Restriction ;
			owl:onProperty fibo-fnd-rel-rel:isGovernedBy ;
			owl:someValuesFrom fibo-fnd-law-jur:Jurisdiction ;
		] ,
		[
			a owl:Restriction ;
			owl:onProperty fibo-fnd-rel-rel:isManagedBy ;
			owl:someValuesFrom fibo-fbc-pas-fpas:FinancialServiceProvider ;
		]
		;
	rdfs:label "registered multilateral trading facility" ;
	rdfs:isDefinedBy <https://spec.edmcouncil.org/fibo/ontology/FBC/FunctionalEntities/Markets/> ;
	skos:definition "multilateral system operated by an investment firm or market operator, which brings together multiple third-party buying and selling interests in financial instruments in the system, in accordance with non-discretionary rules, in a way that results in a contract in accordance with the provisions of Title II of the MiFID II" ;
	.

fibo-fbc-fct-mkt:RegulatedExchange
	a owl:Class ;
	rdfs:subClassOf
		fibo-fbc-fct-mkt:Exchange ,
		[
			a owl:Restriction ;
			owl:onProperty fibo-fbc-fct-rga:isRegulatedBy ;
			owl:someValuesFrom fibo-fbc-fct-rga:RegulatoryAgency ;
		] ,
		[
			a owl:Restriction ;
			owl:onProperty fibo-fnd-rel-rel:isGovernedBy ;
			owl:someValuesFrom fibo-fnd-law-jur:Jurisdiction ;
		]
		;
	rdfs:label "regulated exchange" ;
	rdfs:isDefinedBy <https://spec.edmcouncil.org/fibo/ontology/FBC/FunctionalEntities/Markets/> ;
	skos:definition "regulated market that is operated by and/or managed by a market operator that brings together or facilitates the bringing together of multiple third-party buying and selling interests in financial instruments" ;
	fibo-fnd-utl-av:abbreviation "RM" ;
	fibo-fnd-utl-av:adaptedFrom "http://www.investopedia.com/terms/r/regulated-market.asp" ;
	fibo-fnd-utl-av:explanatoryNote "In the financial community in the EU, such an exchange operates in accordance with its non-discretionary rules in a way that results in a contract, in respect of the financial instruments admitted to trading under its rules and/or systems, and which is authorised and functions regularly and in accordance with the provisions of Title III of MiFID II." ;
	fibo-fnd-utl-av:synonym "regulated market" ;
	.

fibo-fbc-fct-mkt:SwapExecutionFacility
	a owl:Class ;
	rdfs:subClassOf fibo-fbc-fct-mkt:Exchange ;
	rdfs:label "swap execution facility" ;
	rdfs:isDefinedBy <https://spec.edmcouncil.org/fibo/ontology/FBC/FunctionalEntities/Markets/> ;
	skos:definition "exchange that enables participants to execute and trade swaps" ;
	fibo-fnd-utl-av:abbreviation "SEF" ;
	fibo-fnd-utl-av:explanatoryNote "Swap execution facilities, including trading systems and other platforms, allow for greater transparency and represent a significant shift in the way derivative trading has been done. The Dodd-Frank Act lays the foundation for this change of derivative execution." ;
	.

fibo-fbc-fct-mkt:SystematicInternaliser
	a owl:Class ;
	rdfs:subClassOf fibo-fbc-fct-mkt:Exchange ;
	rdfs:label "systematic internaliser" ;
	rdfs:isDefinedBy <https://spec.edmcouncil.org/fibo/ontology/FBC/FunctionalEntities/Markets/> ;
	skos:definition "investment firm that, on an organised, frequent, systematic and substantial basis, deals on its own account by executing client orders outside a regulated exchange, MTF or OTF without operating a multilateral system" ;
	fibo-fnd-utl-av:abbreviation "SI" ;
	fibo-fnd-utl-av:adaptedFrom "https://www.emissions-euets.com/systematic-internaliser" ;
	.

fibo-fbc-fct-mkt:hasExchangeAcronym
	a owl:DatatypeProperty ;
	rdfs:subPropertyOf fibo-fnd-rel-rel:hasAlias ;
	rdfs:label "has exchange acronym" ;
	rdfs:domain fibo-fbc-fct-mkt:Exchange ;
	rdfs:isDefinedBy <https://spec.edmcouncil.org/fibo/ontology/FBC/FunctionalEntities/Markets/> ;
	skos:definition "indicates an acronym for the exchange / institution" ;
	fibo-fnd-utl-av:adaptedFrom "ISO 10383, Securities and related financial instruments - Codes for exchanges and market identification (MIC), Third edition, 2012-10-01" ;
	.

fibo-fbc-fct-mkt:hasExchangeName
	a owl:DatatypeProperty ;
	rdfs:subPropertyOf fibo-fnd-rel-rel:hasFormalName ;
	rdfs:label "has exchange name" ;
	rdfs:domain fibo-fbc-fct-mkt:Exchange ;
	rdfs:isDefinedBy <https://spec.edmcouncil.org/fibo/ontology/FBC/FunctionalEntities/Markets/> ;
	skos:definition "indicates the name or description of the exchange / institution (which may be different from the name of the legal entity)" ;
	fibo-fnd-utl-av:adaptedFrom "ISO 10383, Securities and related financial instruments - Codes for exchanges and market identification (MIC), Third edition, 2012-10-01" ;
	.

fibo-fbc-fct-mkt:hasMarketIdentifierCodeStatus
	a owl:ObjectProperty ;
	rdfs:subPropertyOf fibo-fnd-arr-lif:hasStage ;
	rdfs:label "has market identifier code status" ;
	rdfs:isDefinedBy <https://spec.edmcouncil.org/fibo/ontology/FBC/FunctionalEntities/Markets/> ;
	rdfs:range fibo-fbc-fct-mkt:MarketIdentifierCodeStatus ;
	skos:definition "indicates the status of a specific market identifier code (MIC)" ;
	.

fibo-fbc-fct-mkt:hasOperatingOrSegmentIndicator
	a owl:DatatypeProperty ;
	rdfs:label "has operating or segment indicator" ;
	rdfs:domain fibo-fbc-fct-mkt:MarketIdentifier ;
	rdfs:isDefinedBy <https://spec.edmcouncil.org/fibo/ontology/FBC/FunctionalEntities/Markets/> ;
	rdfs:range xsd:string ;
	skos:definition "indicates whether the market identifier is for an operating exchange or market segment exchange" ;
	fibo-fnd-utl-av:adaptedFrom "ISO 10383, Securities and related financial instruments - Codes for exchanges and market identification (MIC), Third edition, 2012-10-01" ;
	.

fibo-fbc-fct-mkt:operatesInCountry
	a owl:ObjectProperty ;
	rdfs:subPropertyOf fibo-fnd-plc-loc:hasCountry ;
	rdfs:label "operates in country" ;
	rdfs:domain fibo-fbc-fct-mkt:Exchange ;
	rdfs:isDefinedBy <https://spec.edmcouncil.org/fibo/ontology/FBC/FunctionalEntities/Markets/> ;
	rdfs:range lcc-cr:Country ;
	skos:definition "indicates the country in which the exchange is registered and operates" ;
	.

fibo-fbc-fct-mkt:operatesInMunicipality
	a owl:ObjectProperty ;
	rdfs:subPropertyOf fibo-fnd-plc-loc:hasMunicipality ;
	rdfs:label "operates in municipality" ;
	rdfs:isDefinedBy <https://spec.edmcouncil.org/fibo/ontology/FBC/FunctionalEntities/Markets/> ;
	rdfs:range fibo-fnd-plc-loc:Municipality ;
	skos:definition "indicates the municipality or business center in which the exchange is registered and operates" ;
	.

