@prefix rdf: <http://www.w3.org/1999/02/22-rdf-syntax-ns#> .
@prefix rdfs: <http://www.w3.org/2000/01/rdf-schema#> .
@prefix owl: <http://www.w3.org/2002/07/owl#> .
@prefix xsd: <http://www.w3.org/2001/XMLSchema#> .
@prefix dct: <http://purl.org/dc/terms/> .
@prefix skos: <http://www.w3.org/2004/02/skos/core#> .
@prefix sm: <http://www.omg.org/techprocess/ab/SpecificationMetadata/> .
@prefix figi-gii: <http://www.omg.org/spec/FIGI/GlobalInstrumentIdentifiers/> .
@prefix figi-ps: <http://www.omg.org/spec/FIGI/PricingSources/> .
@prefix figi-st: <http://www.omg.org/spec/FIGI/SecurityTypes/> .
@prefix figi-spc: <http://www.omg.org/spec/FIGI/AboutFIGI/> .
@prefix ns1: <http://www.omg.org/spec/FIGI/AboutFIGI-1.0/> .

figi-ps:BAGJ skos:prefLabel "bank artha graha" .

figi-ps:DLAM a figi-gii:PricingSource .

<http://www.omg.org/spec/FIGI/AboutFIGI-1.0/> a owl:Ontology .

_:node1fqlq18m7x15 owl:onProperty figi-gii:isIdentifiedBy .

figi-ps:DLAM skos:prefLabel "dai-ichi life asset" .

<http://www.omg.org/spec/FIGI/AboutFIGI-1.0/> rdfs:label "About the Financial Instrument Global Identifier (FIGI) Specification Version 1.0" .

figi-ps:BAGJ figi-gii:hasUniqueTextIdentifier "BAGJ" .

<http://www.omg.org/spec/FIGI/AboutFIGI-1.0/> dct:license "http://www.omg.org/techprocess/ab/SpecificationMetadata/MITLicense"^^xsd:anyURI .

figi-ps:DLAM figi-gii:hasUniqueTextIdentifier "DLAM" .

_:node1fqlq18m7x15 owl:onClass figi-gii:Ticker .

figi-ps:DLCY a owl:NamedIndividual .

<http://www.omg.org/spec/FIGI/AboutFIGI-1.0/> owl:versionIRI <http://www.omg.org/spec/FIGI/20150501/AboutFIGI-1.0/> .

figi-ps:BAGR a owl:NamedIndividual .

<http://www.omg.org/spec/FIGI/AboutFIGI-1.0/> owl:imports <http://www.omg.org/spec/FIGI/SecurityTypes/> .

figi-ps:DLCY a figi-gii:PricingSource .

<http://www.omg.org/spec/FIGI/AboutFIGI-1.0/> owl:imports <http://www.omg.org/spec/FIGI/PricingSources/> .

_:node1fqlq18m7x15 owl:minQualifiedCardinality "1"^^xsd:nonNegativeInteger .

<http://www.omg.org/spec/FIGI/AboutFIGI-1.0/> owl:imports <http://www.omg.org/spec/FIGI/GlobalInstrumentIdentifiers/> .

figi-ps:DLCY skos:prefLabel "delta lloyd and cyrte" .

figi-ps:BAGR a figi-gii:PricingSource .

figi-ps:DLCY figi-gii:hasUniqueTextIdentifier "DLCY" .

<http://www.omg.org/spec/FIGI/AboutFIGI-1.0/> owl:imports <http://www.omg.org/spec/FIGI/AboutFIGI/> .

_:node1fqlq18m7x16 rdf:first _:node1fqlq18m7x15 .

<http://www.omg.org/spec/FIGI/AboutFIGI-1.0/> sm:copyright """Copyright (c) 2015 Bloomberg LP
Copyright (c) 2015 Object Management Group, Inc.""" .

_:node1fqlq18m7x16 rdf:rest _:node1fqlq18m7x18 .

figi-ps:DLJ a owl:NamedIndividual .

figi-ps:BAGR skos:prefLabel "jsc belagroprombank" .

figi-ps:DLJ a figi-gii:PricingSource .

_:node1fqlq18m7x17 a owl:Restriction .

<http://www.omg.org/spec/FIGI/AboutFIGI-1.0/> sm:filename "AboutFIGI-1.0.rdf" .

_:node1fqlq18m7x17 owl:onProperty figi-gii:has .

figi-ps:DLJ skos:prefLabel "donaldson, luf and jen" .

figi-ps:BAGR figi-gii:hasUniqueTextIdentifier "BAGR" .

figi-ps:DLJ figi-gii:hasUniqueTextIdentifier "DLJ" .

_:node1fqlq18m7x17 owl:onClass figi-gii:ExchangeCode .

<http://www.omg.org/spec/FIGI/AboutFIGI-1.0/> sm:fileAbbreviation "figi-spc-1.0" .

_:node1fqlq18m7x17 owl:maxQualifiedCardinality "1"^^xsd:nonNegativeInteger .

<http://www.omg.org/spec/FIGI/AboutFIGI-1.0/> sm:publicationDate "2015-05-18T18:00:00"^^xsd:dateTime .

figi-ps:DLMN a owl:NamedIndividual .

<http://www.omg.org/spec/FIGI/AboutFIGI-1.0/> sm:contentLanguage "http://www.omg.org/spec/ODM/"^^xsd:anyURI .

figi-st:shortTermBn a owl:NamedIndividual .

<http://www.omg.org/spec/FIGI/AboutFIGI-1.0/> sm:contentLanguage "http://www.w3.org/standards/techs/owl#w3c_all"^^xsd:anyURI .

figi-ps:DLMN a figi-gii:PricingSource .

<http://www.omg.org/spec/FIGI/SecurityTypes/> a owl:Ontology .

_:node1fqlq18m7x18 rdf:first _:node1fqlq18m7x17 .

figi-ps:DLMN skos:prefLabel "dunn loren merrifiel" .

_:node1fqlq18m7x18 rdf:rest rdf:nil .

figi-ps:DLMN figi-gii:hasUniqueTextIdentifier "DLMN" .

_:node1fqlq18m7x19 a owl:Restriction .

figi-ps:DLS a owl:NamedIndividual .

<http://www.omg.org/spec/FIGI/SecurityTypes/> rdfs:label "FIGI Security Types Vocabulary" .

figi-ps:DLS a figi-gii:PricingSource .

_:node1fqlq18m7x19 owl:onProperty figi-gii:hasUniqueTextIdentifier .

figi-ps:DLS skos:prefLabel "dls capital partners" .

<http://www.omg.org/spec/FIGI/SecurityTypes/> dct:license "http://www.omg.org/techprocess/ab/SpecificationMetadata/MITLicense"^^xsd:anyURI .

_:node1fqlq18m7x19 owl:allValuesFrom _:node1fqlq18m7x20 .

figi-ps:DLS figi-gii:hasUniqueTextIdentifier "DLS" .

<http://www.omg.org/spec/FIGI/SecurityTypes/> owl:versionIRI "http://www.omg.org/spec/FIGI/20150501/SecurityTypes/"^^xsd:anyURI .

figi-ps:DMBK a owl:NamedIndividual .

_:node1fqlq18m7x2 a owl:Restriction .

figi-ps:DMBK a figi-gii:PricingSource .

figi-st:shortTermBn a figi-gii:SecurityType .

figi-ps:DMBK skos:prefLabel "d commerce bank" .

<http://www.omg.org/spec/FIGI/SecurityTypes/> skos:changeNote "The http://www.omg.org/spec/FIGI/20140201/SecurityTypes.rdf version of this ontology was modified per the issue resolutions identified in the FIGI 1.0 FTF report." .

figi-st:shortTermBn skos:definition "Short Term Bank Notes" .

figi-ps:DMBK figi-gii:hasUniqueTextIdentifier "DMBK" .

figi-st:shortTermBn skos:prefLabel "short term bn" .

figi-ps:DMEQ a owl:NamedIndividual .

<http://www.omg.org/spec/FIGI/SecurityTypes/> owl:imports <http://www.omg.org/spec/FIGI/GlobalInstrumentIdentifiers/> .

figi-ps:DMEQ a figi-gii:PricingSource .

figi-st:shortTermBn figi-gii:hasUniqueTextIdentifier "SHORT TERM BN" .

figi-ps:DMEQ skos:prefLabel "deutsche bk london" .

<http://www.omg.org/spec/FIGI/SecurityTypes/> rdfs:seeAlso "http://www.omg.org/spec/FIGI/AboutFIGI/"^^xsd:anyURI .

figi-ps:BAHA a owl:NamedIndividual .

figi-ps:DMEQ figi-gii:hasUniqueTextIdentifier "DMEQ" .

figi-ps:BAHA a figi-gii:PricingSource .

<http://www.omg.org/spec/FIGI/SecurityTypes/> sm:copyright """Copyright (c) 2013-2015 Bloomberg LP
Copyright (c) 2013-2015 Object Management Group, Inc.""" .

figi-ps:DMG a owl:NamedIndividual .

figi-ps:BAHA skos:prefLabel "bahana securities" .

figi-ps:DMG a figi-gii:PricingSource .

<http://www.omg.org/spec/FIGI/SecurityTypes/> sm:filename "SecurityTypes.rdf" .

figi-ps:BAHA figi-gii:hasUniqueTextIdentifier "BAHA" .

figi-ps:DMG skos:prefLabel "deutsche bank securi" .

<http://www.omg.org/spec/FIGI/SecurityTypes/> sm:fileAbbreviation "figi-st" .

figi-ps:DMG figi-gii:hasUniqueTextIdentifier "DMG" .

figi-ps:BAHK a owl:NamedIndividual .

_:node1fqlq18m7x2 owl:onProperty figi-gii:has .

figi-ps:DMGA a owl:NamedIndividual .

figi-ps:BAHK a figi-gii:PricingSource .

<http://www.omg.org/spec/FIGI/SecurityTypes/> sm:fileAbstract """The Financial Instrument Global Identifier (FIGI) is a unique, persistent twelve character string that serves to identify financial instruments. Along with the identifier, a number of related data points are identified and defined so as to provide clear context and differentiation of the financial instruments specified by the identifiers.  

This ontology the individuals representing security types for FIGI, and is current as of May 2015.""" .

figi-ps:DMGA a figi-gii:PricingSource .

_:node1fqlq18m7x2 owl:onClass figi-gii:GlobalIdentifier .

figi-ps:DMGA skos:prefLabel "dmg australia" .

<http://www.omg.org/spec/FIGI/SecurityTypes/> sm:contentLanguage "http://www.omg.org/spec/ODM/"^^xsd:anyURI .

figi-ps:DMGA figi-gii:hasUniqueTextIdentifier "DMGA" .

_:node1fqlq18m7x2 owl:minQualifiedCardinality "1"^^xsd:nonNegativeInteger .

figi-ps:DMMU a owl:NamedIndividual .

<http://www.omg.org/spec/FIGI/SecurityTypes/> sm:contentLanguage "http://www.w3.org/standards/techs/owl#w3c_all"^^xsd:anyURI .

_:node1fqlq18m7x20 a rdfs:Datatype .

figi-ps:DMMU a figi-gii:PricingSource .

figi-ps:BAHK skos:prefLabel "ba sec asia limited" .

figi-ps:DMMU skos:prefLabel "di matteo mondino" .

_:node1fqlq18m7x20 owl:onDatatype xsd:string .

figi-ps:DMMU figi-gii:hasUniqueTextIdentifier "DMMU" .

figi-ps:BAHK figi-gii:hasUniqueTextIdentifier "BAHK" .

_:node1fqlq18m7x20 owl:withRestrictions _:node1fqlq18m7x22 .

figi-ps:DMTS a owl:NamedIndividual .

figi-st:shortTermDn a owl:NamedIndividual .

figi-ps:DMTS a figi-gii:PricingSource .

<http://www.omg.org/spec/FIGI/SecurityTypes/> sm:dependsOn "http://www.omg.org/spec/FIGI/GlobalInstrumentIdentifiers/"^^xsd:anyURI .

figi-ps:DMTS skos:prefLabel "denmark mts" .

figi-st:shortTermDn a figi-gii:SecurityType .

<http://www.omg.org/spec/FIGI/SecurityTypes/> sm:dependsOn "http://www.omg.org/techprocess/ab/SpecificationMetadata/"^^xsd:anyURI .

figi-ps:DMTS figi-gii:hasUniqueTextIdentifier "DMTS" .

figi-st:shortTermDn skos:definition "Short Term Deposit Notes- Short-term deposit notes issued directly by the bank. These deposit notes are issued for the bank's own general funding purposes" .

<http://www.omg.org/spec/FIGI/PricingSources/> a owl:Ontology .

figi-ps:DNB a owl:NamedIndividual .

figi-st:shortTermDn skos:prefLabel "short term dn" .

figi-ps:DNB a figi-gii:PricingSource .

<http://www.omg.org/spec/FIGI/PricingSources/> rdfs:label "FIGI Pricing Sources Vocabulary" .

figi-ps:DNB skos:prefLabel "dnb markets" .

figi-st:shortTermDn figi-gii:hasUniqueTextIdentifier "SHORT TERM DN" .

figi-ps:DNB figi-gii:hasUniqueTextIdentifier "DNB" .

<http://www.omg.org/spec/FIGI/PricingSources/> dct:license "http://www.omg.org/techprocess/ab/SpecificationMetadata/MITLicense"^^xsd:anyURI .

figi-ps:DNBB a owl:NamedIndividual .

figi-ps:BAIL a owl:NamedIndividual .

figi-ps:DNBB a figi-gii:PricingSource .

_:node1fqlq18m7x21 xsd:pattern "^(((?!BS|BM|GG|GB|VG|GH|KY)[BCDFGHJKLMNPQRSTVWXZ]{2})G[BCDFGHJKLMNPQRSTVWXYZ\\d]{8}\\d)$" .

figi-ps:BAIL a figi-gii:PricingSource .

figi-ps:DNBB skos:prefLabel "dnb vilnius" .

figi-ps:BAIL skos:prefLabel "banc of america sec" .

_:node1fqlq18m7x22 rdf:first _:node1fqlq18m7x21 .

figi-ps:DNBB figi-gii:hasUniqueTextIdentifier "DNBB" .

_:node1fqlq18m7x22 rdf:rest rdf:nil .

figi-ps:DNBP a owl:NamedIndividual .

<http://www.omg.org/spec/FIGI/PricingSources/> owl:versionIRI "http://www.omg.org/spec/FIGI/20150501/PricingSources/"^^xsd:anyURI .

figi-ps:DNBP a figi-gii:PricingSource .

_:node1fqlq18m7x23 a owl:Restriction .

figi-ps:DNBP skos:prefLabel "den norske bk oslo" .

figi-ps:BAIL figi-gii:hasUniqueTextIdentifier "BAIL" .

_:node1fqlq18m7x23 owl:onProperty figi-gii:identifies .

<http://www.omg.org/spec/FIGI/PricingSources/> skos:changeNote "The http://www.omg.org/spec/FIGI/20131101/PricingSources.rdf version of this ontology was modified per the issue resolutions identified in the FIGI 1.0 FTF report." .

_:node1fqlq18m7x23 owl:qualifiedCardinality "1"^^xsd:nonNegativeInteger .

figi-st:singaporeCP a owl:NamedIndividual .

<http://www.omg.org/spec/FIGI/PricingSources/> owl:imports <http://www.omg.org/spec/FIGI/GlobalInstrumentIdentifiers/> .

figi-st:singaporeCP a figi-gii:SecurityType .

_:node1fqlq18m7x23 owl:onClass figi-gii:FinancialInstrument .

<http://www.omg.org/spec/FIGI/PricingSources/> owl:imports <http://www.omg.org/techprocess/ab/SpecificationMetadata/> .

figi-ps:DNBP figi-gii:hasUniqueTextIdentifier "DNBP" .

<http://www.omg.org/spec/FIGI/PricingSources/> rdfs:seeAlso "http://www.omg.org/spec/FIGI/AboutFIGI/"^^xsd:anyURI .

figi-ps:DNBS a owl:NamedIndividual .

_:node1fqlq18m7x24 a owl:Class .

<http://www.omg.org/spec/FIGI/PricingSources/> sm:copyright """Copyright (c) 2013-2015 Bloomberg LP
Copyright (c) 2013-2015 Object Management Group, Inc.""" .

figi-ps:DNBS a figi-gii:PricingSource .

_:node1fqlq18m7x24 owl:intersectionOf _:node1fqlq18m7x25 .

figi-ps:DNBS skos:prefLabel "dnb bank asa" .

<http://www.omg.org/spec/FIGI/PricingSources/> sm:filename "PricingSources.rdf" .

figi-ps:DNBS figi-gii:hasUniqueTextIdentifier "DNBS" .

_:node1fqlq18m7x25 rdf:first figi-gii:FinancialInstrumentIdentifier .

figi-ps:DNBV a owl:NamedIndividual .

<http://www.omg.org/spec/FIGI/PricingSources/> sm:fileAbbreviation "figi-ps" .

figi-ps:DNBV a figi-gii:PricingSource .

_:node1fqlq18m7x25 rdf:rest _:node1fqlq18m7x27 .

figi-ps:DNBV skos:prefLabel "dnb nor filial asa" .

figi-st:singaporeCP skos:definition "Singapore Commercial Paper" .

figi-ps:DNBV figi-gii:hasUniqueTextIdentifier "DNBV" .

figi-st:singaporeCP skos:prefLabel "singapore cp" .

figi-ps:DNCN a owl:NamedIndividual .

_:node1fqlq18m7x26 a owl:Restriction .

figi-st:singaporeCP figi-gii:hasUniqueTextIdentifier "SINGAPORE CP" .

figi-ps:DNCN a figi-gii:PricingSource .

_:node1fqlq18m7x26 owl:onProperty figi-gii:has .

figi-ps:BAKM a owl:NamedIndividual .

figi-ps:DNCN skos:prefLabel "duncan williams" .

figi-ps:BAKM a figi-gii:PricingSource .

_:node1fqlq18m7x26 owl:onClass figi-gii:CompositeGlobalIdentifier .

figi-ps:BAKM skos:prefLabel "banca akros milan" .

figi-ps:DNCN figi-gii:hasUniqueTextIdentifier "DNCN" .

figi-ps:BAKM figi-gii:hasUniqueTextIdentifier "BAKM" .

_:node1fqlq18m7x26 owl:maxQualifiedCardinality "1"^^xsd:nonNegativeInteger .

figi-ps:DNHR a owl:NamedIndividual .

figi-ps:BAKT a owl:NamedIndividual .

_:node1fqlq18m7x27 rdf:first _:node1fqlq18m7x26 .

figi-ps:BAKT a figi-gii:PricingSource .

_:node1fqlq18m7x27 rdf:rest rdf:nil .

figi-ps:DNHR a figi-gii:PricingSource .

figi-ps:BAKT skos:prefLabel "banka kombetare" .

_:node1fqlq18m7x28 a owl:Restriction .

figi-ps:DNHR skos:prefLabel "danaher oil" .

_:node1fqlq18m7x28 owl:onProperty figi-gii:hasUniqueTextIdentifier .

figi-ps:DNHR figi-gii:hasUniqueTextIdentifier "DNHR" .

_:node1fqlq18m7x28 owl:qualifiedCardinality "1"^^xsd:nonNegativeInteger .

figi-ps:DNLP a owl:NamedIndividual .

<http://www.omg.org/spec/FIGI/PricingSources/> sm:fileAbstract """The Financial Instrument Global Identifier (FIGI) is a unique, persistent twelve character string that serves to identify financial instruments. Along with the identifier, a number of related data points are identified and defined so as to provide clear context and differentiation of the financial instruments specified by the identifiers.  

This ontology the individuals representing pricing sources for FIGI, and is current as of May 2015.""" .

figi-ps:DNLP a figi-gii:PricingSource .

_:node1fqlq18m7x28 owl:onDataRange xsd:token .

figi-ps:DNLP skos:prefLabel "danske bank vilnius" .

<http://www.omg.org/spec/FIGI/PricingSources/> sm:contentLanguage "http://www.omg.org/spec/ODM/"^^xsd:anyURI .

figi-ps:DNLP figi-gii:hasUniqueTextIdentifier "DNLP" .

_:node1fqlq18m7x29 a owl:Restriction .

figi-ps:DOHA a owl:NamedIndividual .

<http://www.omg.org/spec/FIGI/PricingSources/> sm:contentLanguage "http://www.w3.org/standards/techs/owl#w3c_all"^^xsd:anyURI .

figi-ps:DOHA a figi-gii:PricingSource .

_:node1fqlq18m7x29 owl:onProperty figi-gii:isIdentifiedBy .

figi-ps:DOHA skos:prefLabel "doha bank" .

<http://www.omg.org/spec/FIGI/PricingSources/> sm:dependsOn "http://www.omg.org/spec/FIGI/GlobalInstrumentIdentifiers/"^^xsd:anyURI .

figi-ps:DOHA figi-gii:hasUniqueTextIdentifier "DOHA" .

_:node1fqlq18m7x29 owl:qualifiedCardinality "1"^^xsd:nonNegativeInteger .

<http://www.omg.org/spec/FIGI/PricingSources/> sm:dependsOn "http://www.omg.org/techprocess/ab/SpecificationMetadata/"^^xsd:anyURI .

figi-ps:DOLM a owl:NamedIndividual .

_:node1fqlq18m7x29 owl:onClass figi-gii:Identifier .

figi-ps:DOLM a figi-gii:PricingSource .

<http://www.omg.org/spec/FIGI/GlobalInstrumentIdentifiers/> a owl:Ontology .

_:node1fqlq18m7x3 a owl:Class .

figi-ps:DOLM skos:prefLabel "dolmen dublin" .

<http://www.omg.org/spec/FIGI/GlobalInstrumentIdentifiers/> rdfs:label "Financial Industry Global Instrument Identifiers (FIGI) Ontology" .

figi-ps:DOLM figi-gii:hasUniqueTextIdentifier "DOLM" .

_:node1fqlq18m7x3 owl:intersectionOf _:node1fqlq18m7x4 .

figi-ps:DOW a owl:NamedIndividual .

<http://www.omg.org/spec/FIGI/GlobalInstrumentIdentifiers/> dct:license "http://www.omg.org/techprocess/ab/SpecificationMetadata/MITLicense"^^xsd:anyURI .

figi-ps:DOW a figi-gii:PricingSource .

_:node1fqlq18m7x30 a owl:Restriction .

figi-ps:DOW skos:prefLabel "dow chemical company" .

<http://www.omg.org/spec/FIGI/GlobalInstrumentIdentifiers/> owl:versionIRI <http://www.omg.org/spec/FIGI/20150501/GlobalInstrumentIdentifiers/> .

figi-ps:DOW figi-gii:hasUniqueTextIdentifier "DOW" .

_:node1fqlq18m7x30 owl:onProperty figi-gii:has .

figi-ps:DOWL a owl:NamedIndividual .

<http://www.omg.org/spec/FIGI/GlobalInstrumentIdentifiers/> skos:changeNote "The http://www.omg.org/spec/FIGI/20140201/GlobalInstrumentIdentifiers.rdf version of this ontology was modified per the issue resolutions identified in the FIGI 1.0 FTF report." .

figi-ps:DOWL a figi-gii:PricingSource .

_:node1fqlq18m7x30 owl:onClass figi-gii:CompositeGlobalIdentifier .

figi-ps:DOWL skos:prefLabel "dowling partners" .

<http://www.omg.org/spec/FIGI/GlobalInstrumentIdentifiers/> owl:imports <http://www.omg.org/techprocess/ab/SpecificationMetadata/> .

_:node1fqlq18m7x30 owl:minQualifiedCardinality "1"^^xsd:nonNegativeInteger .

figi-ps:DOWL figi-gii:hasUniqueTextIdentifier "DOWL" .

<http://www.omg.org/spec/FIGI/GlobalInstrumentIdentifiers/> rdfs:seeAlso "http://www.omg.org/spec/FIGI/AboutFIGI/"^^xsd:anyURI .

figi-ps:DPA a owl:NamedIndividual .

_:node1fqlq18m7x4 rdf:first figi-gii:FinancialInstrumentIdentifier .

<http://www.omg.org/spec/FIGI/GlobalInstrumentIdentifiers/> sm:copyright """Copyright (c) 2013-2015 Bloomberg LP
Copyright (c) 2013-2015 Object Management Group, Inc.""" .

figi-ps:DPA a figi-gii:PricingSource .

_:node1fqlq18m7x4 rdf:rest _:node1fqlq18m7x6 .

<http://www.omg.org/spec/FIGI/GlobalInstrumentIdentifiers/> sm:filename "GlobalInstrumentIdentifiers.rdf" .

figi-ps:DPA skos:prefLabel "dpa invest" .

_:node1fqlq18m7x5 a owl:Restriction .

figi-ps:DPA figi-gii:hasUniqueTextIdentifier "DPA" .

<http://www.omg.org/spec/FIGI/GlobalInstrumentIdentifiers/> sm:fileAbbreviation "figi-gii" .

figi-ps:DPB a owl:NamedIndividual .

_:node1fqlq18m7x5 owl:onProperty figi-gii:has .

figi-ps:DPB a figi-gii:PricingSource .

figi-ps:BAKT figi-gii:hasUniqueTextIdentifier "BAKT" .

figi-ps:DPB skos:prefLabel "deut postbank int" .

<http://www.omg.org/spec/FIGI/GlobalInstrumentIdentifiers/> sm:fileAbstract """The Financial Instrument Global Identifier (FIGI) is a unique, persistent twelve character string that serves to identify financial instruments. Along with the identifier, a number of related data points are identified and defined so as to provide clear context and differentiation of the financial instruments specified by the identifiers.  

This ontology provides the 'schema' for the identifier and related constructs.  Individuals representing the corresponding security types and pricing sources are provided in separate RDF/XML serialized OWL files.""" .

figi-ps:DPB figi-gii:hasUniqueTextIdentifier "DPB" .

figi-st:singleStockDividendFuture a owl:NamedIndividual .

_:node1fqlq18m7x5 owl:onClass figi-gii:ShareClassGlobalIdentifier .

figi-st:singleStockDividendFuture a figi-gii:SecurityType .

figi-ps:DPH a owl:NamedIndividual .

_:node1fqlq18m7x5 owl:maxQualifiedCardinality "1"^^xsd:nonNegativeInteger .

figi-ps:DPH a figi-gii:PricingSource .

figi-st:singleStockDividendFuture skos:definition "Single Stock Dividend Future. A dividend future is a derivative contract that allows investors to take positions on future dividend payments." .

figi-ps:DPH skos:prefLabel "duff and phelps" .

_:node1fqlq18m7x6 rdf:first _:node1fqlq18m7x5 .

figi-st:singleStockDividendFuture skos:prefLabel "single stock dividend future" .

figi-ps:DPH figi-gii:hasUniqueTextIdentifier "DPH" .

_:node1fqlq18m7x6 rdf:rest rdf:nil .

figi-st:singleStockDividendFuture figi-gii:hasUniqueTextIdentifier "SINGLE STOCK DIVIDEND FUTURE" .

figi-ps:DPI a owl:NamedIndividual .

_:node1fqlq18m7x7 a owl:Restriction .

figi-ps:BAKU a owl:NamedIndividual .

figi-ps:DPI a figi-gii:PricingSource .

_:node1fqlq18m7x7 owl:onProperty figi-gii:isIdentifiedBy .

figi-ps:BAKU a figi-gii:PricingSource .

figi-ps:DPI skos:prefLabel "dupont" .

_:node1fqlq18m7x7 owl:qualifiedCardinality "1"^^xsd:nonNegativeInteger .

figi-ps:BAKU skos:prefLabel "baku stock exchange" .

figi-ps:DPI figi-gii:hasUniqueTextIdentifier "DPI" .

figi-ps:BAKU figi-gii:hasUniqueTextIdentifier "BAKU" .

figi-ps:DPNY a owl:NamedIndividual .

_:node1fqlq18m7x7 owl:onClass figi-gii:FinancialInstrumentIdentifier .

figi-ps:DPNY a figi-gii:PricingSource .

figi-ps:BALN a owl:NamedIndividual .

_:node1fqlq18m7x8 a owl:Class .

figi-ps:DPNY skos:prefLabel "depfa bank" .

figi-ps:BALN a figi-gii:PricingSource .

_:node1fqlq18m7x8 owl:intersectionOf _:node1fqlq18m7x10 .

figi-ps:DPNY figi-gii:hasUniqueTextIdentifier "DPNY" .

figi-ps:BALN skos:prefLabel "bofa-grcc struct inv" .

_:node1fqlq18m7x9 a owl:Restriction .

figi-ps:DRAE a owl:NamedIndividual .

figi-ps:BALN figi-gii:hasUniqueTextIdentifier "BALN" .

figi-ps:DRAE a figi-gii:PricingSource .

_:node1fqlq18m7x9 owl:onProperty figi-gii:has .

figi-st:singleStockForward a owl:NamedIndividual .

figi-ps:DRAE skos:prefLabel "dresdner bank mid" .

figi-st:singleStockForward a figi-gii:SecurityType .

_:node1fqlq18m7x9 owl:onClass figi-gii:PricingSource .

figi-ps:DRAE figi-gii:hasUniqueTextIdentifier "DRAE" .

figi-st:singleStockForward skos:definition "Single Stock Forward. A forward contract is a non-standardized contract between two parties where the price is agreed at the initial trade date. These contracts are not exchange listed." .

_:node1fqlq18m7x9 owl:minQualifiedCardinality "0"^^xsd:nonNegativeInteger .

figi-st:singleStockForward skos:prefLabel "single stock forward" .

<http://www.omg.org/spec/FIGI/GlobalInstrumentIdentifiers/> sm:contentLanguage "http://www.omg.org/spec/ODM/"^^xsd:anyURI .

figi-st:singleStockForward figi-gii:hasUniqueTextIdentifier "SINGLE STOCK FORWARD" .

<http://www.omg.org/spec/FIGI/GlobalInstrumentIdentifiers/> sm:contentLanguage "http://www.w3.org/standards/techs/owl#w3c_all"^^xsd:anyURI .

figi-ps:BALS a owl:NamedIndividual .

figi-ps:DRAG a owl:NamedIndividual .

<http://www.omg.org/spec/FIGI/GlobalInstrumentIdentifiers/> sm:dependsOn "http://www.omg.org/techprocess/ab/SpecificationMetadata/"^^xsd:anyURI .

figi-ps:DRAG a figi-gii:PricingSource .

figi-ps:BALS a figi-gii:PricingSource .

ns1:FIGISpecification-1.0 a owl:NamedIndividual .

figi-ps:DRAG skos:prefLabel "dragon capital" .

ns1:FIGISpecification-1.0 a sm:SpecificationVersion .

figi-ps:BALS skos:prefLabel "bank austria credit." .

figi-ps:DRAG figi-gii:hasUniqueTextIdentifier "DRAG" .

ns1:FIGISpecification-1.0 rdfs:label "Financial Instrument Global Identifier (FIGI) Specification Version 1.0" .

figi-ps:BALS figi-gii:hasUniqueTextIdentifier "BALS" .

figi-ps:DRB a owl:NamedIndividual .

figi-st:singleStockFuture a owl:NamedIndividual .

figi-ps:DRB a figi-gii:PricingSource .

ns1:FIGISpecification-1.0 skos:definition "individual representing metadata about the Financial Instrument Global Identifier (FIGI) Version 1.0 Specification" .

figi-st:singleStockFuture a figi-gii:SecurityType .

figi-ps:DRB skos:prefLabel "dresdner bank ag,fft" ;
	figi-gii:hasUniqueTextIdentifier "DRB" .

figi-st:singleStockFuture skos:definition "All standard equity futures are single stock futures or SSFs. Other possible returns are SSDF, Single Stock Dividend Future, DNSF, Dividend Neutral Stock Future, and CFD, Contract For Difference. These returns only apply to the equity button." .

ns1:FIGISpecification-1.0 skos:historyNote """Revisions to the FIGI specification are managed per the process outlined in the Policies and Procedures for OMG standards, with the intent to maintain backwards compatibility in the ontologies to the degree possible.
  
The RDF/XML serialized OWL for the Foundations ODM/OWL ontologies have been checked for syntactic errors and logical consistency with Protege 4 (http://protege.stanford.edu/) and HermiT 1.3.8 (http://www.hermit-reasoner.com/) and Pellet 2.2 (http://clarkparsia.com/pellet/).  Pellet 2.2 is not able to process the regex string pattern in the data restriction, however. Users who wish to use Pellet due to other advantages should comment out the restriction on the hasUniqueTextIdentifier property in the definition of FinancialInstrumentIdentifier.""" .

figi-st:singleStockFuture skos:prefLabel "single stock future" .

ns1:FIGISpecification-1.0 sm:publicationDate "2015-05-18T18:00:00"^^xsd:dateTime .

figi-st:singleStockFuture figi-gii:hasUniqueTextIdentifier "SINGLE STOCK FUTURE" .

figi-ps:DRBA a owl:NamedIndividual .

ns1:FIGISpecification-1.0 sm:specificationVersionURL "http://www.omg.org/spec/FIGI/1.0/"^^xsd:anyURI .

figi-ps:DRBA a figi-gii:PricingSource .

figi-ps:BALT a owl:NamedIndividual .

ns1:FIGISpecification-1.0 sm:specificationVersionStatus "Formal Specification" .

figi-ps:DRBA skos:prefLabel "dresdner asia" .

figi-ps:BALT a figi-gii:PricingSource .

ns1:FIGISpecification-1.0 sm:isVersionOf figi-spc:FIGISpecification .

figi-ps:DRBA figi-gii:hasUniqueTextIdentifier "DRBA" .

figi-ps:BALT skos:prefLabel "baltic exchange" .

ns1:FIGISpecification-1.0 sm:responsibleTaskForce "http://fdtf.omg.org/"^^xsd:anyURI .

figi-ps:BALT figi-gii:hasUniqueTextIdentifier "BALT" .

figi-ps:DRBZ a owl:NamedIndividual .

ns1:FIGISpecification-1.0 sm:addressForComments "http://www.omg.org/issues/"^^xsd:anyURI .

figi-ps:DRBZ a figi-gii:PricingSource .

figi-ps:BALU a owl:NamedIndividual .

figi-gii:classifies a owl:ObjectProperty .

figi-ps:DRBZ skos:prefLabel "dresdner bk latam" .

figi-ps:BALU a figi-gii:PricingSource .

figi-gii:classifies rdfs:label "classifies" .

figi-ps:DRBZ figi-gii:hasUniqueTextIdentifier "DRBZ" .

figi-gii:classifies skos:definition "arranges in classes; assigns to a category" .

figi-ps:BALU skos:prefLabel "balanz capital usd" .

figi-gii:classifies dct:source "Merriam-Webster Dictionary" .

figi-ps:BALU figi-gii:hasUniqueTextIdentifier "BALU" .

figi-ps:AAAA a owl:NamedIndividual .

figi-ps:DRC a owl:NamedIndividual .

figi-st:sn a owl:NamedIndividual .

figi-ps:AAAA a figi-gii:PricingSource .

figi-st:sn a figi-gii:SecurityType .

figi-ps:DRC a figi-gii:PricingSource .

figi-ps:AAAA skos:prefLabel "asset mgmt consult" .

figi-st:sn skos:definition "Structured Note" .

figi-ps:DRC skos:prefLabel "dahlman rose and co" .

figi-st:sn skos:prefLabel "sn" .

figi-ps:DRC figi-gii:hasUniqueTextIdentifier "DRC" .

figi-ps:AAAA figi-gii:hasUniqueTextIdentifier "AAAA" .

figi-st:sn figi-gii:hasUniqueTextIdentifier "SN" .

figi-gii:PricingSource a owl:Class .

figi-ps:DRCC a owl:NamedIndividual .

figi-ps:BALZ a owl:NamedIndividual .

figi-gii:PricingSource rdfs:label "pricing source" .

figi-ps:BALZ a figi-gii:PricingSource .

figi-ps:DRCC a figi-gii:PricingSource .

figi-gii:PricingSource skos:definition "the pricing source for a security" .

figi-ps:BALZ skos:prefLabel "balanz capital" .

figi-ps:DRCC skos:prefLabel "dresdner kleinwort" .

figi-gii:PricingSource rdfs:subClassOf figi-gii:Code .

figi-ps:BALZ skos:prefLabel "balanz capital ars" .

figi-gii:hasUniqueTextIdentifier a owl:DatatypeProperty .

figi-ps:DRCC figi-gii:hasUniqueTextIdentifier "DRCC" .

figi-ps:BALZ figi-gii:hasUniqueTextIdentifier "BALZ" .

figi-gii:hasUniqueTextIdentifier rdfs:label "has unique text identifier" .

figi-ps:DREG a owl:NamedIndividual .

figi-ps:BAM a owl:NamedIndividual .

figi-ps:DREG a figi-gii:PricingSource .

figi-gii:hasUniqueTextIdentifier skos:definition "links an entity to a unique identifier for that entity; may be associated with anything.  With reference to a given (possibly implicit) set of objects, a unique identifier (UID) is any identifier which is guaranteed to be unique among all identifiers used for those objects and for a specific purpose." .

figi-ps:DREG skos:prefLabel "dresdner bank" .

figi-ps:BAM a figi-gii:PricingSource .

figi-gii:hasUniqueTextIdentifier dct:source "https://en.wikipedia.org/wiki/Unique_identifier"^^xsd:anyURI .

figi-ps:DREG figi-gii:hasUniqueTextIdentifier "DREG" .

figi-ps:BAM skos:prefLabel "brownstone asset mgt" .

figi-ps:DRES a owl:NamedIndividual .

figi-gii:hasUniqueTextIdentifier rdfs:range xsd:string .

figi-ps:DRES a figi-gii:PricingSource .

figi-ps:BAM figi-gii:hasUniqueTextIdentifier "BAM" .

figi-ps:DRES skos:prefLabel "dresdner bank ag" .

figi-gii:has a owl:ObjectProperty .

figi-st:spareNA a owl:NamedIndividual .

figi-ps:DRES figi-gii:hasUniqueTextIdentifier "DRES" .

figi-st:spareNA a figi-gii:SecurityType .

figi-gii:has rdfs:label "has" .

figi-st:spareNA skos:definition "A dummy market issue type entered on mistaked or dummy securities." .

figi-ps:DRET a owl:NamedIndividual .

figi-gii:has skos:definition "indicates that someone (or something) possesses something, as a characteristic, attribute, feature, capability, and so forth" .

figi-st:spareNA skos:prefLabel "spare - n/a" .

figi-ps:DRET a figi-gii:PricingSource .

figi-st:aTUnit a owl:NamedIndividual .

figi-st:spareNA figi-gii:hasUniqueTextIdentifier "SPARE - N/A" .

figi-ps:DRET skos:prefLabel "dresdner kleinwort" .

figi-ps:BAME a owl:NamedIndividual .

figi-ps:DRET figi-gii:hasUniqueTextIdentifier "DRET" .

figi-st:aTUnit a figi-gii:SecurityType .

figi-ps:BAME a figi-gii:PricingSource .

figi-ps:DREU a owl:NamedIndividual .

figi-st:aTUnit skos:definition "Similar to 'Amertst'. This noted an Americus Trust instrument, which are no longer issued." .

figi-ps:DREU a figi-gii:PricingSource .

figi-ps:BAME skos:prefLabel "barclays asset mgt" .

figi-st:aTUnit skos:prefLabel "a/t unit" .

figi-ps:DREU skos:prefLabel "dresdner bank" .

figi-ps:BAME skos:prefLabel "bofa ml london fi" .

figi-st:aTUnit figi-gii:hasUniqueTextIdentifier "A/T Unit" .

figi-ps:DREU figi-gii:hasUniqueTextIdentifier "DREU" .

figi-gii:SecurityType a owl:Class .

figi-ps:BAME figi-gii:hasUniqueTextIdentifier "BAME" .

figi-ps:DREX a owl:NamedIndividual .

figi-gii:SecurityType rdfs:label "security type" .

figi-st:specialLmmkPgm a owl:NamedIndividual .

figi-ps:DREX a figi-gii:PricingSource .

figi-gii:SecurityType skos:definition "the type of security, for example, common stock" .

figi-ps:DREX skos:prefLabel "dresdner bk (mex)" .

figi-gii:SecurityType rdfs:subClassOf _:node1fqlq18m7x29 .

figi-ps:DREX figi-gii:hasUniqueTextIdentifier "DREX" .

figi-st:specialLmmkPgm a figi-gii:SecurityType .

figi-ps:AAAM a owl:NamedIndividual .

figi-ps:DRFR a owl:NamedIndividual .

figi-st:specialLmmkPgm skos:definition "Auxiliary program type setup for linking securities to mmkt ticker" .

figi-ps:DRFR a figi-gii:PricingSource .

figi-ps:AAAM a figi-gii:PricingSource .

figi-st:specialLmmkPgm skos:prefLabel "special lmmk pgm" .

figi-ps:DRFR skos:prefLabel "dresdner bank (frnk)" .

figi-st:specialLmmkPgm figi-gii:hasUniqueTextIdentifier "SPECIAL LMMK PGM" .

figi-ps:DRFR figi-gii:hasUniqueTextIdentifier "DRFR" .

figi-st:spot a owl:NamedIndividual .

figi-ps:AAAM skos:prefLabel "j and t investment co" .

figi-st:spot a figi-gii:SecurityType .

figi-ps:DRFT a owl:NamedIndividual .

figi-ps:AAAM figi-gii:hasUniqueTextIdentifier "AAAM" .

figi-ps:DRFT a figi-gii:PricingSource .

figi-st:spot skos:definition "Spot. Available for immediate delivery" .

figi-gii:identifies a owl:ObjectProperty .

figi-ps:DRFT skos:prefLabel "drkw frankfurt" .

figi-st:spot skos:prefLabel "spot" .

figi-ps:DRFT figi-gii:hasUniqueTextIdentifier "DRFT" .

figi-gii:identifies a owl:FunctionalProperty .

figi-st:spot figi-gii:hasUniqueTextIdentifier "SPOT" .

figi-ps:DRGG a owl:NamedIndividual .

figi-gii:identifies rdfs:label "identifies" .

figi-ps:BAMG a owl:NamedIndividual .

figi-ps:DRGG a figi-gii:PricingSource .

figi-ps:BAMG a figi-gii:PricingSource .

figi-gii:identifies skos:definition "relates an identifier to the entity that it identifies" .

figi-ps:BAMG skos:prefLabel "barclays asset mgt" .

figi-ps:DRGG skos:prefLabel "dragon capital" .

figi-ps:BAMG figi-gii:hasUniqueTextIdentifier "BAMG" .

figi-ps:AAAN a owl:NamedIndividual .

figi-ps:DRGG figi-gii:hasUniqueTextIdentifier "DRGG" .

figi-ps:BAMI a owl:NamedIndividual .

figi-ps:AAAN a figi-gii:PricingSource .

figi-ps:BAMI a figi-gii:PricingSource .

figi-ps:DRGN a owl:NamedIndividual .

figi-ps:AAAN skos:prefLabel "abn amro boom" .

figi-ps:DRGN a figi-gii:PricingSource .

figi-ps:BAMI skos:prefLabel "banque misr" .

figi-ps:AAAN figi-gii:hasUniqueTextIdentifier "AAAN" .

figi-ps:DRGN skos:prefLabel "dragon capital" .

figi-ps:BAMI figi-gii:hasUniqueTextIdentifier "BAMI" .

figi-st:absAuto a owl:NamedIndividual .

figi-ps:DRGN figi-gii:hasUniqueTextIdentifier "DRGN" .

figi-st:absAuto a figi-gii:SecurityType .

figi-st:spotIndex a owl:NamedIndividual .

figi-ps:DRHD a owl:NamedIndividual .

figi-st:spotIndex a figi-gii:SecurityType .

figi-st:absAuto skos:definition "Asset Backed Security (backed by AUTO loans)" .

figi-ps:DRHD a figi-gii:PricingSource .

figi-st:spotIndex skos:definition "Statistical movement of the underlying security as represented by a basket of spot traded securities." .

figi-st:absAuto skos:prefLabel "abs auto" .

figi-st:spotIndex skos:prefLabel "spot index." .

figi-st:absAuto figi-gii:hasUniqueTextIdentifier "ABS Auto" .

figi-st:spotIndex figi-gii:hasUniqueTextIdentifier "Spot index." .

figi-ps:AABA a owl:NamedIndividual .

figi-ps:DRHD skos:prefLabel "banco bhd" .

figi-ps:AABA a figi-gii:PricingSource .

figi-ps:BAML a owl:NamedIndividual .

figi-ps:DRHD figi-gii:hasUniqueTextIdentifier "DRHD" .

figi-ps:AABA skos:prefLabel "abn amro bank (asia)" .

figi-ps:BAML a figi-gii:PricingSource .

figi-ps:DRK a owl:NamedIndividual .

figi-ps:AABA figi-gii:hasUniqueTextIdentifier "AABA" .

figi-ps:DRK a figi-gii:PricingSource .

figi-ps:BAML skos:prefLabel "baml auto ex" .

figi-st:absCard a owl:NamedIndividual .

figi-ps:DRK skos:prefLabel "deutsche bank ag" .

figi-st:absCard a figi-gii:SecurityType .

figi-ps:BAML figi-gii:hasUniqueTextIdentifier "BAML" .

figi-ps:DRK figi-gii:hasUniqueTextIdentifier "DRK" .

figi-st:absCard skos:definition "Asset Backed Security (backed by Other less common loans and receivables) i.e. Charge accounts, Reference Notes, etc." .

figi-st:standby a owl:NamedIndividual .

figi-ps:DRKW a owl:NamedIndividual .

figi-st:standby a figi-gii:SecurityType .

figi-st:absCard skos:prefLabel "abs card" .

figi-ps:DRKW a figi-gii:PricingSource .

figi-st:standby skos:definition "A financial commitment issued on a stand-by basis and borrowed only if and when needed. It is not used alone as a loan type." .

figi-st:absCard figi-gii:hasUniqueTextIdentifier "ABS Card" .

figi-ps:DRKW skos:prefLabel "drkw indicative" .

figi-st:standby skos:prefLabel "standby" .

figi-ps:AABG a owl:NamedIndividual .

figi-ps:DRKW figi-gii:hasUniqueTextIdentifier "DRKW" .

figi-st:standby figi-gii:hasUniqueTextIdentifier "STANDBY" .

figi-ps:AABG a figi-gii:PricingSource .

figi-ps:DRPB a owl:NamedIndividual .

figi-ps:BAMR a owl:NamedIndividual .

figi-ps:AABG skos:prefLabel "abn amro" .

figi-ps:BAMR a figi-gii:PricingSource .

figi-ps:DRPB a figi-gii:PricingSource .

figi-ps:AABG figi-gii:hasUniqueTextIdentifier "AABG" .

figi-ps:DRPB skos:prefLabel "dresdner bank pb" .

figi-ps:BAMR skos:prefLabel "bradford and marzec" .

figi-gii:isClassifiedBy a owl:ObjectProperty .

figi-ps:DRPB figi-gii:hasUniqueTextIdentifier "DRPB" .

figi-ps:BAMR figi-gii:hasUniqueTextIdentifier "BAMR" .

figi-gii:isClassifiedBy a owl:IrreflexiveProperty .

figi-ps:DRRT a owl:NamedIndividual .

figi-st:standbyDelayDrawTerm a owl:NamedIndividual .

figi-ps:DRRT a figi-gii:PricingSource .

figi-st:standbyDelayDrawTerm a figi-gii:SecurityType .

figi-gii:isClassifiedBy rdfs:label "is classified by" .

figi-ps:DRRT skos:prefLabel "dresdner" .

figi-st:standbyDelayDrawTerm skos:definition "A financial commitment issued on a stand-by basis and borrowed only if and when needed. Borrower is allowed to draw down on the loan in one or more drawings within a specified time period after the signing date. Once borrowed, cannot be re-borrowed." .

figi-gii:isClassifiedBy skos:definition "indicates the category or classifier used to classify an entity" .

figi-ps:DRRT figi-gii:hasUniqueTextIdentifier "DRRT" .

figi-st:standbyDelayDrawTerm skos:prefLabel "standby delay-draw term" .

figi-gii:isClassifiedBy owl:inverseOf figi-gii:classifies .

figi-ps:DRWA a owl:NamedIndividual .

figi-st:standbyDelayDrawTerm figi-gii:hasUniqueTextIdentifier "STANDBY DELAY-DRAW TERM" .

figi-ps:AABI a owl:NamedIndividual .

figi-ps:DRWA a figi-gii:PricingSource .

figi-ps:BAMT a owl:NamedIndividual .

figi-ps:AABI a figi-gii:PricingSource .

figi-ps:DRWA skos:prefLabel "kleinwort benson" .

figi-ps:BAMT a figi-gii:PricingSource .

figi-ps:AABI skos:prefLabel "abn amro istanbul" .

figi-ps:DRWA figi-gii:hasUniqueTextIdentifier "DRWA" .

figi-ps:BAMT skos:prefLabel "bofa merrill lynch" .

figi-ps:AABI figi-gii:hasUniqueTextIdentifier "AABI" .

figi-ps:BAMT figi-gii:hasUniqueTextIdentifier "BAMT" .

figi-ps:DSAB a owl:NamedIndividual .

figi-st:absHome a owl:NamedIndividual .

figi-ps:DSAB a figi-gii:PricingSource .

figi-st:standbyLoc a owl:NamedIndividual .

figi-st:absHome a figi-gii:SecurityType .

figi-st:standbyLoc a figi-gii:SecurityType .

figi-ps:DSAB skos:prefLabel "deutsche bank ny" .

figi-st:absHome skos:definition "Asset Backed Security (backed by Other less common loans and receivables) i.e. Charge accounts, Reference Notes, etc." .

figi-st:standbyLoc skos:definition "A financial commitment issued on a stand-by basis and borrowed only if and when needed. Guaranteed by the lender(s) and used for purchase of goods, completion of construction projects, and/or general purposes." .

figi-ps:DSAB figi-gii:hasUniqueTextIdentifier "DSAB" .

figi-st:standbyLoc skos:prefLabel "standby loc" .

figi-st:absHome skos:prefLabel "abs home" .

figi-ps:DSAI a owl:NamedIndividual .

figi-st:standbyLoc figi-gii:hasUniqueTextIdentifier "STANDBY LOC" .

figi-st:absHome figi-gii:hasUniqueTextIdentifier "ABS Home" .

figi-ps:DSAI a figi-gii:PricingSource .

figi-ps:BAMX a owl:NamedIndividual .

figi-gii:isIdentifiedBy a owl:ObjectProperty .

figi-ps:BAMX a figi-gii:PricingSource .

figi-ps:DSAI skos:prefLabel "daiwa capmkts ame" .

figi-ps:BAMX skos:prefLabel "bofa ml london" .

figi-gii:isIdentifiedBy rdfs:label "is identified by" .

figi-ps:DSAI figi-gii:hasUniqueTextIdentifier "DSAI" .

figi-ps:BAMX figi-gii:hasUniqueTextIdentifier "BAMX" .

figi-gii:isIdentifiedBy skos:definition "relates an entity to an identifier or key that identifies it" .

figi-ps:DSAN a owl:NamedIndividual .

figi-st:standbyRev a owl:NamedIndividual .

figi-gii:isIdentifiedBy owl:inverseOf figi-gii:identifies .

figi-ps:DSAN a figi-gii:PricingSource .

figi-st:standbyRev a figi-gii:SecurityType .

figi-ps:AABK a owl:NamedIndividual .

figi-ps:DSAN skos:prefLabel "daiwa sec america ny" .

figi-ps:AABK a figi-gii:PricingSource .

figi-st:standbyRev skos:definition "A financial commitment issued on a stand-by basis and borrowed only if and when needed. Once borrowed, can be borrowed again." .

figi-ps:DSAN figi-gii:hasUniqueTextIdentifier "DSAN" .

figi-ps:AABK skos:prefLabel "abn amro bangkok" .

figi-st:standbyRev skos:prefLabel "standby rev" .

figi-ps:DSAX a owl:NamedIndividual .

figi-st:standbyRev figi-gii:hasUniqueTextIdentifier "STANDBY REV" .

figi-ps:AABK figi-gii:hasUniqueTextIdentifier "AABK" .

figi-ps:DSAX a figi-gii:PricingSource .

figi-ps:BANC a owl:NamedIndividual .

figi-st:absOther a owl:NamedIndividual .

figi-ps:DSAX skos:prefLabel "daiwa smbc axes" .

figi-st:absOther a figi-gii:SecurityType .

figi-ps:BANC a figi-gii:PricingSource .

figi-ps:DSAX figi-gii:hasUniqueTextIdentifier "DSAX" .

figi-st:absOther skos:definition "Asset Backed Security (backed by Home Equity loans)" .

figi-ps:BANC skos:prefLabel "banc one" .

figi-ps:DSBK a owl:NamedIndividual .

figi-st:absOther skos:prefLabel "abs other" .

figi-ps:BANC figi-gii:hasUniqueTextIdentifier "BANC" .

figi-ps:DSBK a figi-gii:PricingSource .

figi-st:absOther figi-gii:hasUniqueTextIdentifier "ABS Other" .

figi-st:standbyTerm a owl:NamedIndividual .

figi-ps:AABN a owl:NamedIndividual .

figi-st:standbyTerm a figi-gii:SecurityType .

figi-ps:DSBK skos:prefLabel "dah sing bank 11:30" .

figi-ps:AABN a figi-gii:PricingSource .

figi-st:standbyTerm skos:definition "A financial commitment issued on a stand-by basis and borrowed only if and when needed. Once borrowed, cannot be re-borrowed." .

figi-ps:DSBK figi-gii:hasUniqueTextIdentifier "DSBK" .

figi-st:standbyTerm skos:prefLabel "standby term" .

figi-ps:AABN skos:prefLabel "abn amro bank nv" .

figi-ps:DSBP a owl:NamedIndividual .

figi-st:standbyTerm figi-gii:hasUniqueTextIdentifier "STANDBY TERM" .

figi-ps:DSBP a figi-gii:PricingSource .

figi-ps:AABN figi-gii:hasUniqueTextIdentifier "AABN" .

figi-ps:DSBP skos:prefLabel "dah sing bank 4:30" .

figi-ps:BANI a owl:NamedIndividual .

figi-st:acceptBancaria a owl:NamedIndividual .

figi-ps:BANI a figi-gii:PricingSource .

figi-ps:DSBP figi-gii:hasUniqueTextIdentifier "DSBP" .

figi-ps:BANI skos:prefLabel "banif investimento" .

figi-st:acceptBancaria a figi-gii:SecurityType .

figi-ps:BANI figi-gii:hasUniqueTextIdentifier "BANI" .

figi-ps:DSBU a owl:NamedIndividual .

figi-st:acceptBancaria skos:definition "Mexico Bankers Acceptances" .

figi-ps:DSBU a figi-gii:PricingSource .

figi-st:sterlingCD a owl:NamedIndividual .

figi-st:acceptBancaria skos:prefLabel "accept bancaria" .

figi-ps:DSBU skos:prefLabel "del sur banco univ." .

figi-st:sterlingCD a figi-gii:SecurityType .

figi-st:acceptBancaria figi-gii:hasUniqueTextIdentifier "ACCEPT BANCARIA" .

figi-ps:DSBU figi-gii:hasUniqueTextIdentifier "DSBU" .

figi-st:sterlingCD skos:definition "Certificates of Deposit issued in British Sterling Market" .

figi-ps:AABP a owl:NamedIndividual .

figi-ps:DSC a owl:NamedIndividual , figi-gii:PricingSource .

figi-ps:AABP a figi-gii:PricingSource .

figi-st:sterlingCD skos:prefLabel "sterling cd" .

figi-ps:DSC skos:prefLabel "dundee securities" .

figi-st:sterlingCD figi-gii:hasUniqueTextIdentifier "STERLING CD" .

figi-ps:DSC figi-gii:hasUniqueTextIdentifier "DSC" .

figi-ps:BANO a owl:NamedIndividual .

figi-ps:AABP skos:prefLabel "abn amro bank ldn" .

figi-ps:DSCM a owl:NamedIndividual .

figi-ps:BANO a figi-gii:PricingSource .

figi-ps:DSCM a figi-gii:PricingSource .

figi-ps:AABP figi-gii:hasUniqueTextIdentifier "AABP" .

figi-ps:BANO skos:prefLabel "banorte" .

figi-ps:DSCM skos:prefLabel "deutsche bank nyc" .

figi-st:adjConvToFixed a owl:NamedIndividual .

figi-ps:BANO figi-gii:hasUniqueTextIdentifier "BANO" .

figi-st:adjConvToFixed a figi-gii:SecurityType .

figi-ps:DSCM skos:prefLabel "deutsche bank nyx" .

figi-st:sterlingCP a owl:NamedIndividual .

figi-st:adjConvToFixed skos:definition "These are bonds that had been adjustable, but were remarketed as Fixed interest rate bonds, and the coupon rate will no longer be subject to change." .

figi-st:sterlingCP a figi-gii:SecurityType .

figi-ps:DSCM figi-gii:hasUniqueTextIdentifier "DSCM" .

figi-st:adjConvToFixed skos:prefLabel "adj conv. to fixed" .

figi-ps:DSCP a owl:NamedIndividual .

figi-st:adjConvToFixed figi-gii:hasUniqueTextIdentifier "ADJ CONV. TO FIXED" .

figi-ps:DSCP a figi-gii:PricingSource .

figi-st:sterlingCP skos:definition "Certificate of Deposit (CD). A debt instrument issued by a bank that will pay interest, periodically or at maturity (set by competitive forces in the marketplace), and principal when it reaches maturity. Maturities range from a few weeks to several years. It may have a fixed or floating rate of interest. Certificate of Deposit Rollover. An investment strategy used to defer taxes on income from a Certificate of Deposit. An individual who has purchased a certificate of deposit on margin expected to mature in the following year, can deduct the interest on the loan in the current year and move the income from the certificate to the up-coming year. - STERLING" .

figi-ps:DSCP skos:prefLabel "descap securities" .

figi-gii:Code a owl:Class .

figi-st:sterlingCP skos:prefLabel "sterling cp" .

figi-ps:DSCP figi-gii:hasUniqueTextIdentifier "DSCP" .

figi-st:sterlingCP figi-gii:hasUniqueTextIdentifier "STERLING CP" .

figi-gii:Code rdfs:label "code" .

figi-ps:BANP a owl:NamedIndividual .

figi-ps:DSEC a owl:NamedIndividual .

figi-ps:BANP a figi-gii:PricingSource .

figi-gii:Code skos:definition "A system of valid symbols that substitute for specified values, such as alpha, numeric, symbols or combinations thereof." .

figi-ps:BANP skos:prefLabel "banco panamericano s" .

figi-gii:Code rdfs:subClassOf _:node1fqlq18m7x1 .

figi-ps:BANP figi-gii:hasUniqueTextIdentifier "BANP" .

figi-ps:DSEC a figi-gii:PricingSource .

figi-gii:Code sm:directSource "ISO/IEC 11179-3, Information technology - Metadata registries (MDR) - Part 3: Registry metamodel and basic attributes" .

figi-st:stermLoanNote a owl:NamedIndividual .

figi-ps:DSEC skos:prefLabel "daiwa sec sbcm" .

figi-ps:AABR a owl:NamedIndividual .

figi-st:stermLoanNote a figi-gii:SecurityType .

figi-ps:AABR a figi-gii:PricingSource .

figi-ps:DSEC figi-gii:hasUniqueTextIdentifier "DSEC" .

figi-st:stermLoanNote skos:definition "Short Term Loan Notes" .

figi-ps:AABR skos:prefLabel "abn amro inc." .

figi-ps:DSEL a owl:NamedIndividual .

figi-st:stermLoanNote skos:prefLabel "s.term loan note" .

figi-ps:AABR figi-gii:hasUniqueTextIdentifier "AABR" .

figi-st:stermLoanNote figi-gii:hasUniqueTextIdentifier "S.TERM LOAN NOTE" .

figi-st:adjConvToFixedOid a owl:NamedIndividual .

figi-ps:DSEL a figi-gii:PricingSource .

figi-st:adjConvToFixedOid a figi-gii:SecurityType .

figi-ps:BANQ a owl:NamedIndividual .

figi-ps:DSEL skos:prefLabel "daiwa smbc" .

figi-ps:BANQ a figi-gii:PricingSource .

figi-st:adjConvToFixedOid skos:definition "These are bonds that had been adjustable, but were remarketed as Fixed interest rate bonds, and the coupon rate will no longer be subject to change. The security is an Original Issue Discount." .

figi-ps:DSEL figi-gii:hasUniqueTextIdentifier "DSEL" .

figi-st:adjConvToFixedOid skos:prefLabel "adj conv. to fixed, oid" .

figi-ps:BANQ skos:prefLabel "banquo credit mgmt" .

figi-st:adjConvToFixedOid figi-gii:hasUniqueTextIdentifier "ADJ CONV. TO FIXED, OID" .

figi-ps:DSHK a owl:NamedIndividual .

figi-ps:BANQ figi-gii:hasUniqueTextIdentifier "BANQ" .

figi-ps:DSHK a figi-gii:PricingSource .

figi-ps:AABS a owl:NamedIndividual .

figi-st:swap a owl:NamedIndividual .

figi-ps:AABS a figi-gii:PricingSource .

figi-ps:DSHK skos:prefLabel "daiwa smbc hk" .

figi-st:swap a figi-gii:SecurityType .

figi-ps:AABS skos:prefLabel "abn amro caracas" .

figi-ps:DSHK figi-gii:hasUniqueTextIdentifier "DSHK" .

figi-ps:AABS figi-gii:hasUniqueTextIdentifier "AABS" .

figi-st:swap skos:definition "Swap Rates. Interest rate swaps are highly customized agreements that possess a wide range of configurations and complexities. However, most are of the generic, or plain vanilla sort. A plain vanilla swap is an agreement of two parties to exchange interest payments with each other during an agreed-upon period of time. In a plain vanilla swap, one of the interest payment streams is fixed, while the other is floating, and no exchange of principle takes place." .

figi-ps:AABV a owl:NamedIndividual .

figi-ps:DSII a owl:NamedIndividual .

figi-ps:AABV a figi-gii:PricingSource .

figi-st:swap skos:prefLabel "swap" .

figi-ps:DSII a figi-gii:PricingSource .

figi-ps:AABV skos:prefLabel "abn amro australia" .

figi-st:swap figi-gii:hasUniqueTextIdentifier "SWAP" .

figi-ps:AABV figi-gii:hasUniqueTextIdentifier "AABV" .

figi-ps:DSII skos:prefLabel "daiwa secs - london" .

figi-ps:BANS a owl:NamedIndividual .

figi-st:adjustable a owl:NamedIndividual .

figi-ps:BANS a figi-gii:PricingSource .

figi-st:adjustable a figi-gii:SecurityType .

figi-ps:DSII figi-gii:hasUniqueTextIdentifier "DSII" .

figi-ps:BANS skos:prefLabel "banortes securities" .

figi-st:adjustable skos:definition "The rate changes throughout the life of the bond. This includes variables and step-coupons." .

figi-ps:BANS figi-gii:hasUniqueTextIdentifier "BANS" .

figi-st:adjustable skos:prefLabel "adjustable" .

figi-st:swapSpread a owl:NamedIndividual .

figi-ps:DSIM a owl:NamedIndividual .

figi-st:swapSpread a figi-gii:SecurityType .

figi-st:adjustable figi-gii:hasUniqueTextIdentifier "ADJUSTABLE" .

figi-ps:DSIM a figi-gii:PricingSource .

figi-st:swapSpread skos:definition "Primarily quoted in basis points, swap spreads take the difference between two different interest rate swaps." .

figi-ps:AABZ a owl:NamedIndividual .

figi-ps:DSIM skos:prefLabel "deutsche sec inc" .

figi-st:swapSpread skos:prefLabel "swap spread" .

figi-ps:AABZ a figi-gii:PricingSource .

figi-ps:DSIM figi-gii:hasUniqueTextIdentifier "DSIM" .

figi-st:swapSpread figi-gii:hasUniqueTextIdentifier "SWAP SPREAD" .

figi-ps:AABZ skos:prefLabel "abn amro bz auto-ex" .

figi-ps:DSKB a owl:NamedIndividual .

figi-ps:BANT a owl:NamedIndividual .

figi-ps:AABZ figi-gii:hasUniqueTextIdentifier "AABZ" .

figi-ps:BANT a figi-gii:PricingSource .

figi-ps:DSKB a figi-gii:PricingSource .

figi-st:adjustableOid a owl:NamedIndividual .

figi-ps:BANT skos:prefLabel "bantleon bank ag" .

figi-st:adjustableOid a figi-gii:SecurityType .

figi-ps:DSKB skos:prefLabel "dsk bank" .

figi-ps:BANT figi-gii:hasUniqueTextIdentifier "BANT" .

figi-st:adjustableOid skos:definition "The rate changes throughout the life of the bond. The security is an Original Issue Discount." .

figi-ps:DSKB figi-gii:hasUniqueTextIdentifier "DSKB" .

figi-st:adjustableOid skos:prefLabel "adjustable, oid" .

figi-st:swaptionVolatility a owl:NamedIndividual .

figi-st:adjustableOid figi-gii:hasUniqueTextIdentifier "ADJUSTABLE, OID" .

figi-st:swaptionVolatility a figi-gii:SecurityType .

figi-ps:DSLZ a owl:NamedIndividual .

figi-ps:AACB a owl:NamedIndividual .

figi-st:swaptionVolatility skos:definition "Volatility of the underlying swap rate" .

figi-ps:DSLZ a figi-gii:PricingSource .

figi-ps:AACB a figi-gii:PricingSource .

figi-st:swaptionVolatility skos:prefLabel "swaption volatility" .

figi-ps:AACB skos:prefLabel "abn amro bank" .

figi-st:swaptionVolatility figi-gii:hasUniqueTextIdentifier "SWAPTION VOLATILITY" .

figi-ps:AACB figi-gii:hasUniqueTextIdentifier "AACB" .

figi-ps:DSLZ skos:prefLabel "deutsche secs japan" .

figi-gii:CompositeGlobalIdentifier a owl:Class .

figi-ps:BANV a owl:NamedIndividual .

figi-ps:DSLZ figi-gii:hasUniqueTextIdentifier "DSLZ" .

figi-gii:CompositeGlobalIdentifier rdfs:label "composite global identifier" .

figi-ps:BANV a figi-gii:PricingSource .

figi-ps:DSP a owl:NamedIndividual .

figi-ps:BANV skos:prefLabel "banvalor" .

figi-ps:DSP a figi-gii:PricingSource .

figi-gii:CompositeGlobalIdentifier skos:definition "A composite global identifier is a global identifier which is differentiated from a 'normal' global identifier in that it serves as a parent in a hierarchy of individual global identifiers.  This parent identifier may also provide a unique, common identifier for a financial instrument within the context of a jurisdiction (e.g., country)." .

figi-ps:BANV figi-gii:hasUniqueTextIdentifier "BANV" .

figi-gii:CompositeGlobalIdentifier rdfs:subClassOf _:node1fqlq18m7x2 .

figi-ps:DSP skos:prefLabel "dalton strategic" .

figi-gii:CompositeGlobalIdentifier rdfs:subClassOf _:node1fqlq18m7x3 .

figi-st:swedishCP a owl:NamedIndividual .

figi-ps:DSP figi-gii:hasUniqueTextIdentifier "DSP" .

figi-st:swedishCP a figi-gii:SecurityType .

figi-gii:CompositeGlobalIdentifier skos:example "AAPL common stock, US Composite" .

figi-ps:DSPL a owl:NamedIndividual .

figi-st:swedishCP skos:definition "Swedish Commercial Paper" .

figi-ps:DSPL a figi-gii:PricingSource .

figi-st:adr a owl:NamedIndividual .

figi-st:swedishCP skos:prefLabel "swedish cp" .

figi-ps:DSPL skos:prefLabel "dsp merrill lynch" .

figi-st:swedishCP figi-gii:hasUniqueTextIdentifier "SWEDISH CP" .

figi-ps:DSPL figi-gii:hasUniqueTextIdentifier "DSPL" .

figi-st:swingline a owl:NamedIndividual .

figi-st:adr a figi-gii:SecurityType .

figi-st:swingline a figi-gii:SecurityType .

figi-ps:DSSE a owl:NamedIndividual , figi-gii:PricingSource ;
	skos:prefLabel "daiwa sec cm seoul" .

figi-st:swingline skos:definition "Short term loan that allows the borrower to draw funds on short notice, usually the same day. It is not used alone as a loan type." .

figi-ps:DSSE figi-gii:hasUniqueTextIdentifier "DSSE" .

figi-st:adr skos:definition "A negotiable certificate issued by a U.S. bank representing a specified number of shares (or one share) in a foreign stock that is traded on a U.S. exchange. ADRs are denominated in U.S. dollars, with the underlying security held by a U.S. financial institution overseas. ADRs help to reduce administration and duty costs that would otherwise be levied on each transaction." .

figi-ps:DSSK a owl:NamedIndividual .

figi-st:adr skos:prefLabel "adr" .

figi-st:swingline skos:prefLabel "swingline" .

figi-ps:DSSK a figi-gii:PricingSource .

figi-st:adr figi-gii:hasUniqueTextIdentifier "ADR" .

figi-st:swingline figi-gii:hasUniqueTextIdentifier "SWINGLINE" .

figi-ps:DSSK skos:prefLabel "daishin securities" .

figi-ps:AACD a owl:NamedIndividual .

figi-ps:BANX a owl:NamedIndividual .

figi-ps:DSSK figi-gii:hasUniqueTextIdentifier "DSSK" .

figi-ps:AACD a figi-gii:PricingSource .

figi-ps:BANX a figi-gii:PricingSource ;
	skos:prefLabel "banamex bond prices" .

figi-ps:DSTA a owl:NamedIndividual .

figi-ps:AACD skos:prefLabel "abn amro credit der." .

figi-ps:DSTA a figi-gii:PricingSource .

figi-ps:BANX figi-gii:hasUniqueTextIdentifier "BANX" .

figi-ps:AACD figi-gii:hasUniqueTextIdentifier "AACD" .

figi-st:swissCert a owl:NamedIndividual .

figi-gii:GlobalIdentifier a owl:Class .

figi-st:swissCert a figi-gii:SecurityType .

figi-ps:DSTA skos:prefLabel "dutch state treasury" .

figi-gii:GlobalIdentifier rdfs:label "global identifier" .

figi-ps:DSTA figi-gii:hasUniqueTextIdentifier "DSTA" .

figi-st:swissCert skos:definition "Swiss Certificate. Original share certificate of a foreign company, mainly originating in the US, the UK or Canada, which is quoted on a Swiss Stock Exchange and is registered in the nominee name of a specified Swiss nominee endorsed in blank. For dividend payments or in corporate actions it must be stamped by the nominee company." .

figi-ps:DSUO a owl:NamedIndividual .

figi-st:swissCert skos:prefLabel "swiss cert" .

figi-ps:DSUO a figi-gii:PricingSource .

figi-gii:GlobalIdentifier skos:definition "A global identifier is the most basic type of identifier that applies to exactly and only one Financial Instrument at the most granular level. For example,  AAPL common stock as traded on NASDAQ Global Select. The granularity of this identifier is found in that which it identifies. In particular, the most basic FIGI identifies a financial instrument, where applicable, at the trading venue level. That is, where applicable, the Global Identifier  identifies a Financial Instrument within the context of an exchange venue." .

figi-st:swissCert figi-gii:hasUniqueTextIdentifier "Swiss Cert" .

figi-gii:GlobalIdentifier rdfs:subClassOf _:node1fqlq18m7x24 .

figi-ps:BAOP a owl:NamedIndividual .

figi-ps:DSUO skos:prefLabel "deutsche bk ny- mtge" .

figi-ps:AACO a owl:NamedIndividual .

figi-ps:BAOP a figi-gii:PricingSource .

figi-ps:DSUO figi-gii:hasUniqueTextIdentifier "DSUO" .

figi-ps:AACO a figi-gii:PricingSource .

figi-ps:BAOP skos:prefLabel "bancofamerica - opus" .

figi-ps:DTBA a owl:NamedIndividual .

figi-ps:AACO skos:prefLabel "abn amro bogota" .

figi-ps:DTBA a figi-gii:PricingSource .

figi-ps:BAOP figi-gii:hasUniqueTextIdentifier "BAOP" .

figi-ps:AACO figi-gii:hasUniqueTextIdentifier "AACO" .

figi-ps:DTBA skos:prefLabel "deutsche mortgages" .

figi-st:synthLoc a owl:NamedIndividual .

figi-st:agncyAbsHome a owl:NamedIndividual .

figi-ps:DTBA figi-gii:hasUniqueTextIdentifier "DTBA" .

figi-st:agncyAbsHome a figi-gii:SecurityType .

figi-st:synthLoc a figi-gii:SecurityType .

figi-ps:DTNE a owl:NamedIndividual .

figi-st:agncyAbsHome skos:definition "Asset Backed Loans issued by an Agency such as SBA" .

figi-ps:DTNE a figi-gii:PricingSource .

figi-st:synthLoc skos:definition "A letter of credit facility which is fully cash collateralized with proceeds of a term loan which has been issued by the same borrower, usually with the same amount and terms." .

figi-st:agncyAbsHome skos:prefLabel "agncy abs home" .

figi-ps:DTNE skos:prefLabel "dtn energy" .

figi-st:agncyAbsHome figi-gii:hasUniqueTextIdentifier "Agncy ABS Home" .

figi-ps:DTNE figi-gii:hasUniqueTextIdentifier "DTNE" .

figi-ps:AADV a owl:NamedIndividual .

figi-st:synthLoc skos:prefLabel "synth loc" .

figi-ps:DTPR a owl:NamedIndividual .

figi-ps:AADV a figi-gii:PricingSource .

figi-ps:DTPR a figi-gii:PricingSource .

figi-st:synthLoc figi-gii:hasUniqueTextIdentifier "SYNTH LOC" .

figi-ps:DTPR skos:prefLabel "debt traders" .

figi-ps:BAP a owl:NamedIndividual .

figi-ps:DTPR figi-gii:hasUniqueTextIdentifier "DTPR" .

figi-ps:BAP a figi-gii:PricingSource .

figi-ps:DTST a owl:NamedIndividual .

figi-ps:BAP skos:prefLabel "ba pension inv mgt" .

figi-ps:DTST a figi-gii:PricingSource .

figi-ps:AADV skos:prefLabel "atlantic advisors" .

figi-ps:DTST skos:prefLabel "dresdner bank" .

figi-ps:BAP figi-gii:hasUniqueTextIdentifier "BAP" .

figi-ps:AADV figi-gii:hasUniqueTextIdentifier "AADV" .

figi-ps:DTST figi-gii:hasUniqueTextIdentifier "DTST" .

figi-gii:FinancialInstrumentIdentifier a owl:Class .

figi-st:synthRev a owl:NamedIndividual .

figi-ps:DUET a owl:NamedIndividual .

figi-st:synthRev a figi-gii:SecurityType .

figi-gii:FinancialInstrumentIdentifier rdfs:label "financial instrument identifier" .

figi-ps:DUET a figi-gii:PricingSource .

figi-st:synthRev skos:definition "A letter of credit facility which is fully cash collateralized with proceeds of a term loan which has been issued by the same borrower, usually with the same amount and terms. Once borrowed, can be borrowed again." .

figi-ps:DUET skos:prefLabel "duet alternative inv" .

figi-st:synthRev skos:prefLabel "synth rev" .

figi-ps:DUET figi-gii:hasUniqueTextIdentifier "DUET" .

figi-st:synthRev figi-gii:hasUniqueTextIdentifier "SYNTH REV" .

figi-ps:DUNN a owl:NamedIndividual .

figi-gii:FinancialInstrumentIdentifier skos:definition "A financial instrument identifier is an identifier that identifies (that is, labels the identity of) a financial instrument with a unique, persistent, semantically meaningless ID. The abbreviation 'ID' often refers to identity, identification (the process of identifying), or an identifier (that is, an instance of identification).  A financial instrument identifier consists of a 12 digit alpha-numeric, randomly generated ID covering active and inactive securities. In total there will be more than 852 billion potential combinations available. The first 3 characters begin with 'xxG'; where 'x' can be any upper-case consonant or 'Y' (with certain restrictions), positions 4-11 are alpha-numeric (excluding vowels) and the last digit is a check digit, which is calculated based on a variation of the Modulus 10 Double Add Double Formula." .

figi-st:synthTerm a owl:NamedIndividual .

figi-ps:DUNN a figi-gii:PricingSource .

figi-gii:FinancialInstrumentIdentifier rdfs:subClassOf figi-gii:Identifier .

figi-st:synthTerm a figi-gii:SecurityType .

figi-ps:DUNN skos:prefLabel "dunmore trading llc" .

figi-gii:FinancialInstrumentIdentifier rdfs:subClassOf _:node1fqlq18m7x23 .

figi-st:synthTerm skos:definition "A letter of credit facility which is fully cash collateralized with proceeds of a term loan which has been issued by the same borrower, usually with the same amount and terms. Once borrowed, cannot be re-borrowed." .

figi-ps:DUNN figi-gii:hasUniqueTextIdentifier "DUNN" .

figi-st:synthTerm skos:prefLabel "synth term" .

figi-ps:DUSS a owl:NamedIndividual .

figi-st:synthTerm figi-gii:hasUniqueTextIdentifier "SYNTH TERM" .

figi-gii:FinancialInstrumentIdentifier skos:scopeNote """Note that not all versions of the various OWL 2 compliant reasoning engines available can process the string pattern properly.

The structure of the identifier includes twelve (12) character string as follows:
Position 1: any upper-case alpha character excluding vowels ('Y' counts as a consonant).
Position 2: any upper-case alpha character exlcuding vowels.
Position 3: the letter 'G'.
Positions 4-11: any alpha numeric charater excluding vowels that, in combination with positions 1 and 2 does not constitute a duplicate of an existing string.
Position 12: check digit (see additional documentation for algorithm)
Qualification: positions 1 and 2 cannot be the following sequences: BS, BM, GG, GB, VG, GH, or KY.""" .

figi-ps:DUSS a figi-gii:PricingSource .

figi-ps:BAPA a owl:NamedIndividual .

figi-gii:FinancialInstrumentIdentifier owl:equivalentClass _:node1fqlq18m7x19 .

figi-ps:BAPA a figi-gii:PricingSource .

figi-ps:DUSS skos:prefLabel "dusseldorf exch" .

figi-st:agncyAbsOther a owl:NamedIndividual .

figi-ps:BAPA skos:prefLabel "bank panin" .

figi-st:agncyAbsOther a figi-gii:SecurityType .

figi-ps:DUSS figi-gii:hasUniqueTextIdentifier "DUSS" .

figi-st:agncyAbsOther skos:definition "Asset Backed Loans issued by an Agency such as SBA" .

figi-ps:BAPA figi-gii:hasUniqueTextIdentifier "BAPA" .

figi-ps:DVBK a owl:NamedIndividual .

figi-st:agncyAbsOther skos:prefLabel "agncy abs other" .

figi-st:taiwanCP a owl:NamedIndividual .

figi-ps:DVBK a figi-gii:PricingSource .

figi-st:agncyAbsOther figi-gii:hasUniqueTextIdentifier "Agncy ABS Other" .

figi-st:taiwanCP a figi-gii:SecurityType .

figi-ps:DVBK skos:prefLabel "cfet ch developmn bk" .

figi-ps:AAEB a owl:NamedIndividual .

figi-st:taiwanCP skos:definition "Taiwan Commercial Paper" .

figi-ps:AAEB a figi-gii:PricingSource .

figi-ps:DVBK figi-gii:hasUniqueTextIdentifier "DVBK" .

figi-st:taiwanCP skos:prefLabel "taiwan cp" .

figi-ps:AAEB skos:prefLabel "abn amro singapore" .

figi-st:taiwanCP figi-gii:hasUniqueTextIdentifier "TAIWAN CP" .

figi-ps:AAEB figi-gii:hasUniqueTextIdentifier "AAEB" .

figi-ps:BAPI a owl:NamedIndividual .

figi-ps:DVP a owl:NamedIndividual .

figi-gii:ShareClassGlobalIdentifier a owl:Class .

figi-ps:BAPI a figi-gii:PricingSource .

figi-ps:DVP a figi-gii:PricingSource .

figi-gii:ShareClassGlobalIdentifier rdfs:label "share class global identifier" .

figi-ps:BAPI skos:prefLabel "bloomberg sapi demo" .

figi-ps:DVP skos:prefLabel "davenport and company" .

figi-ps:BAPI figi-gii:hasUniqueTextIdentifier "BAPI" .

figi-ps:DVP figi-gii:hasUniqueTextIdentifier "DVP" .

figi-gii:ShareClassGlobalIdentifier skos:definition "A share class global identifier is a global identifier that is differentiated from a 'normal' global identifier and a composite global identifier in that it serves as a parent in a hierarchy of individual composite global identifiers. For example, AAPL common stock as traded across the planet presented as a list of ocmposite global identifiers. Similar to a composite global identifier, the share class global identifier identifies a financial instrument within the context of the global perspective, e.g., aapl common stock." .

figi-st:taiwanCPGuar a owl:NamedIndividual .

figi-ps:DW a owl:NamedIndividual .

figi-gii:ShareClassGlobalIdentifier rdfs:subClassOf figi-gii:FinancialInstrumentIdentifier .

figi-st:taiwanCPGuar a figi-gii:SecurityType .

figi-ps:DW a figi-gii:PricingSource .

figi-gii:ShareClassGlobalIdentifier rdfs:subClassOf _:node1fqlq18m7x30 .

figi-st:taiwanCPGuar skos:definition "Taiwan Guaranteed Commercial Paper" .

figi-ps:DW skos:prefLabel "dean witter" .

figi-st:taiwanCPGuar skos:prefLabel "taiwan cp guar" .

figi-st:agncyCmbs a owl:NamedIndividual .

figi-ps:DW figi-gii:hasUniqueTextIdentifier "DW" .

figi-st:taiwanCPGuar figi-gii:hasUniqueTextIdentifier "TAIWAN CP GUAR" .

figi-st:agncyCmbs a figi-gii:SecurityType .

figi-ps:DWAM a owl:NamedIndividual .

figi-st:taiwanNegoCD a owl:NamedIndividual .

figi-ps:DWAM a figi-gii:PricingSource .

figi-st:agncyCmbs skos:definition "Agency Commercial Mortgage security (ie GNR ticker)" .

figi-st:taiwanNegoCD a figi-gii:SecurityType .

figi-ps:DWAM skos:prefLabel "daiwa asset mgmt co" .

figi-st:agncyCmbs skos:prefLabel "agncy cmbs" .

figi-st:taiwanNegoCD skos:definition "Taiwan Negotiable Certificates of Deposit" .

figi-st:agncyCmbs figi-gii:hasUniqueTextIdentifier "Agncy CMBS" .

figi-st:taiwanNegoCD skos:prefLabel "taiwan nego cd" .

figi-ps:AAEM a owl:NamedIndividual .

figi-ps:DWAM figi-gii:hasUniqueTextIdentifier "DWAM" .

figi-st:taiwanNegoCD figi-gii:hasUniqueTextIdentifier "TAIWAN NEGO CD" .

figi-ps:AAEM a figi-gii:PricingSource .

figi-ps:DWEU a owl:NamedIndividual .

figi-ps:AAEM skos:prefLabel "abn amro" .

figi-ps:BAPX a owl:NamedIndividual .

figi-ps:DWEU a figi-gii:PricingSource .

figi-ps:AAEM figi-gii:hasUniqueTextIdentifier "AAEM" .

figi-ps:BAPX a figi-gii:PricingSource .

figi-ps:DWEU skos:prefLabel "daiwa securities" .

figi-ps:AAET a owl:NamedIndividual .

figi-ps:BAPX skos:prefLabel "boa treasury marks" .

figi-ps:AAET a figi-gii:PricingSource .

figi-ps:DWEU figi-gii:hasUniqueTextIdentifier "DWEU" .

figi-ps:BAPX figi-gii:hasUniqueTextIdentifier "BAPX" .

figi-ps:AAET skos:prefLabel "abn amro safrica et" .

figi-ps:DWFN a owl:NamedIndividual .

figi-st:taiwanTimeDepo a owl:NamedIndividual .

figi-ps:AAET figi-gii:hasUniqueTextIdentifier "AAET" .

figi-st:taiwanTimeDepo a figi-gii:SecurityType .

figi-ps:DWFN a figi-gii:PricingSource .

figi-st:taiwanTimeDepo skos:definition "Taiwan Time Deposits" .

figi-st:agncyCmoFlt a owl:NamedIndividual .

figi-ps:DWFN skos:prefLabel "dewaay financial" .

figi-st:agncyCmoFlt a figi-gii:SecurityType .

figi-st:taiwanTimeDepo skos:prefLabel "taiwan time depo" .

figi-st:agncyCmoFlt skos:definition "Agency Floater" .

figi-st:taiwanTimeDepo figi-gii:hasUniqueTextIdentifier "TAIWAN TIME DEPO" .

figi-st:agncyCmoFlt skos:prefLabel "agncy cmo flt" .

figi-ps:BARC a owl:NamedIndividual .

figi-ps:DWFN figi-gii:hasUniqueTextIdentifier "DWFN" .

figi-st:agncyCmoFlt figi-gii:hasUniqueTextIdentifier "Agncy CMO FLT" .

figi-ps:DWM a owl:NamedIndividual .

figi-gii:ExchangeCode a owl:Class .

figi-ps:BARC a figi-gii:PricingSource .

figi-ps:DWM a figi-gii:PricingSource .

figi-gii:ExchangeCode rdfs:label "exchange code" .

figi-ps:DWM skos:prefLabel "dwight asset mgmt" .

figi-ps:BARC skos:prefLabel "barclays capital" .

figi-gii:ExchangeCode skos:definition "a code for the exchange on which the security trades" .

figi-ps:DWM figi-gii:hasUniqueTextIdentifier "DWM" .

figi-ps:BARC figi-gii:hasUniqueTextIdentifier "BARC" .

figi-gii:ExchangeCode rdfs:subClassOf figi-gii:Code .

figi-ps:DWSB a owl:NamedIndividual .

figi-st:taxCredit a owl:NamedIndividual .

figi-ps:AAF a owl:NamedIndividual .

figi-ps:DWSB a figi-gii:PricingSource .

figi-st:taxCredit a figi-gii:SecurityType .

figi-ps:AAF a figi-gii:PricingSource .

figi-ps:DWSB skos:prefLabel "daewoo securities co" .

figi-ps:AAF skos:prefLabel "abn amro luxembourg" .

figi-ps:DWSB figi-gii:hasUniqueTextIdentifier "DWSB" .

figi-st:taxCredit skos:definition "The bond pays little or no interest, but gives a tax credit to bondholders." .

figi-ps:AAF figi-gii:hasUniqueTextIdentifier "AAF" .

figi-ps:DWSP a owl:NamedIndividual .

figi-st:taxCredit skos:prefLabel "tax credit" .

figi-st:agncyCmoInv a owl:NamedIndividual .

figi-ps:DWSP a figi-gii:PricingSource .

figi-st:agncyCmoInv a figi-gii:SecurityType .

figi-st:taxCredit figi-gii:hasUniqueTextIdentifier "TAX CREDIT" .

figi-ps:DWSP skos:prefLabel "dws polska" .

figi-st:agncyCmoInv skos:definition "Agency CMO Inverse Floating Rate security, Fannie Mae, Freddie Mac, Ginnie Mae" .

figi-ps:BARH a owl:NamedIndividual .

figi-ps:DWSP figi-gii:hasUniqueTextIdentifier "DWSP" .

figi-ps:BARH a figi-gii:PricingSource .

figi-st:agncyCmoInv skos:prefLabel "agncy cmo inv" .

figi-ps:BARH skos:prefLabel "barclays capital hk" .

figi-ps:DWZB a owl:NamedIndividual .

figi-st:agncyCmoInv figi-gii:hasUniqueTextIdentifier "Agncy CMO INV" .

figi-ps:BARH figi-gii:hasUniqueTextIdentifier "BARH" .

figi-ps:DWZB a figi-gii:PricingSource .

figi-gii:FinancialInstrument a owl:Class .

figi-st:taxCreditOid a owl:NamedIndividual .

figi-ps:DWZB skos:prefLabel "dwz - berlin fixing" .

figi-st:taxCreditOid a figi-gii:SecurityType .

figi-gii:FinancialInstrument rdfs:label "financial instrument" .

figi-ps:DWZB figi-gii:hasUniqueTextIdentifier "DWZB" .

figi-gii:FinancialInstrument skos:definition "Financial instruments are cash, evidence of an ownership interest in an entity, or a contractual right to receive, or deliver, cash or another financial instrument." .

figi-ps:DWZC a owl:NamedIndividual .

figi-gii:FinancialInstrument rdfs:subClassOf _:node1fqlq18m7x7 .

figi-ps:DWZC a figi-gii:PricingSource .

figi-gii:FinancialInstrument rdfs:subClassOf _:node1fqlq18m7x8 .

figi-ps:DWZC skos:prefLabel "dwz - bremen fixing" ;
	figi-gii:hasUniqueTextIdentifier "DWZC" .

figi-ps:DWZD a owl:NamedIndividual , figi-gii:PricingSource ;
	skos:prefLabel "dwz - dusseldorf fix" .

figi-gii:FinancialInstrument skos:scopeNote """Financial instruments can be categorized by form depending on whether they are cash instruments or derivative instruments.

Cash instruments are financial instruments whose value is determined directly by markets. They can be divided into securities, which are readily transferable, and other cash instruments such as loans and deposits, where both borrower and lender have to agree on a transfer.

Derivative instruments are financial instruments which derive their value from the value and characteristics of one or more underlying assets. They can be divided into exchange-traded derivatives and over-the-counter (OTC) derivatives.

Alternatively, financial instruments can be categorized by 'asset class' depending on whether they are equity based (reflecting ownership of the issuing entity) or debt based (reflecting a loan the investor has made to the issuing entity). If it is debt, it can be further categorized into short term (less than one year) or long term.

Foreign Exchange instruments and transactions are neither debt nor equity based and belong in their own category.""" .

figi-st:taxCreditOid skos:definition "The bond pays little or no interest, but gives a tax credit to bondholders. The security is an Original Issue Discount." .

figi-ps:DWZD figi-gii:hasUniqueTextIdentifier "DWZD" .

figi-ps:AAFI a owl:NamedIndividual .

figi-ps:DWZF a owl:NamedIndividual .

figi-st:taxCreditOid skos:prefLabel "tax credit, oid" .

figi-ps:AAFI a figi-gii:PricingSource .

figi-ps:DWZF a figi-gii:PricingSource .

figi-st:taxCreditOid figi-gii:hasUniqueTextIdentifier "TAX CREDIT, OID" .

figi-ps:AAFI skos:prefLabel "abn amro ldn" .

figi-ps:BARL a owl:NamedIndividual .

figi-ps:AAFI skos:prefLabel "rbs nv ldn" .

figi-ps:BARL a figi-gii:PricingSource .

figi-ps:AAFI figi-gii:hasUniqueTextIdentifier "AAFI" .

figi-ps:BARL skos:prefLabel "barclays bank lnd" .

figi-st:agncyCmoIo a owl:NamedIndividual .

figi-ps:BARL figi-gii:hasUniqueTextIdentifier "BARL" .

figi-st:agncyCmoIo a figi-gii:SecurityType .

figi-st:tdr a owl:NamedIndividual , figi-gii:SecurityType .

figi-st:agncyCmoIo skos:definition "Collateralized Mortgage Obligation (CMO). A security which pools together mortgages and separates them into short-, medium-, and long-term positions (called tranches). Tranches are set up to pay different rates of interest depending upon their maturity." .

figi-st:tdr skos:definition "Taiwan Depository Receipt" .

figi-st:agncyCmoIo skos:prefLabel "agncy cmo io" .

figi-st:tdr skos:prefLabel "tdr" .

figi-st:agncyCmoIo figi-gii:hasUniqueTextIdentifier "Agncy CMO IO" .

figi-st:tdr figi-gii:hasUniqueTextIdentifier "TDR" .

figi-ps:AAGH a owl:NamedIndividual , figi-gii:PricingSource .

figi-ps:BARM a owl:NamedIndividual .

figi-ps:AAGH skos:prefLabel "african alliance" .

figi-ps:BARM a figi-gii:PricingSource .

figi-ps:AAGH figi-gii:hasUniqueTextIdentifier "AAGH" .

figi-ps:BARM skos:prefLabel "barclay's capital" .

figi-st:agncyCmoOther a owl:NamedIndividual , figi-gii:SecurityType .

figi-ps:BARM figi-gii:hasUniqueTextIdentifier "BARM" .

figi-st:agncyCmoOther skos:definition "Agency CMO Other(Less common type of security such as PAC or Sequential) Fannie Mae, Freddie Mac, Ginnie Mae" .

figi-st:term a owl:NamedIndividual .

figi-st:agncyCmoOther skos:prefLabel "agncy cmo other" .

figi-ps:DWZF skos:prefLabel "dwz - frankfurt fix" .

figi-st:agncyCmoOther figi-gii:hasUniqueTextIdentifier "Agncy CMO Other" .

figi-st:term a figi-gii:SecurityType .

figi-ps:DWZF figi-gii:hasUniqueTextIdentifier "DWZF" .

figi-ps:AAHK a owl:NamedIndividual .

figi-st:term skos:definition "A loan with a fixed availability period and often includes some minimum repayment schedule. Once borrowings have been repaid, they cannot be re-borrowed." .

figi-ps:AAHK a figi-gii:PricingSource .

figi-ps:DWZG a owl:NamedIndividual .

figi-st:term skos:prefLabel "term" .

figi-ps:AAHK skos:prefLabel "abn amro bk hk" .

figi-ps:DWZG a figi-gii:PricingSource .

figi-st:term figi-gii:hasUniqueTextIdentifier "TERM" .

figi-ps:DWZG skos:prefLabel "dwz - german fixing" .

figi-ps:AAHK figi-gii:hasUniqueTextIdentifier "AAHK" .

figi-ps:DWZG figi-gii:hasUniqueTextIdentifier "DWZG" .

figi-ps:BARP a owl:NamedIndividual .

figi-st:agncyCmoPo a owl:NamedIndividual .

figi-ps:BARP a figi-gii:PricingSource .

figi-st:agncyCmoPo a figi-gii:SecurityType .

figi-ps:BARP skos:prefLabel "bank america secs." ;
	figi-gii:hasUniqueTextIdentifier "BARP" .

figi-st:termDeposits a owl:NamedIndividual , figi-gii:SecurityType .

figi-ps:DWZH a owl:NamedIndividual .

figi-st:agncyCmoPo skos:definition "Agency collateralized Mortgage Obligations - Principal only" .

figi-ps:DWZH a figi-gii:PricingSource .

figi-st:termDeposits skos:definition "Term Deposits" .

figi-ps:DWZH skos:prefLabel "dwz - hamburg fixing" .

figi-st:agncyCmoPo skos:prefLabel "agncy cmo po" .

figi-ps:DWZH figi-gii:hasUniqueTextIdentifier "DWZH" .

figi-st:agncyCmoPo figi-gii:hasUniqueTextIdentifier "Agncy CMO PO" .

figi-st:termDeposits skos:prefLabel "term deposits" .

figi-ps:AAIL a owl:NamedIndividual .

figi-ps:DWZI a owl:NamedIndividual .

figi-ps:AAIL a figi-gii:PricingSource .

figi-st:termDeposits figi-gii:hasUniqueTextIdentifier "TERM DEPOSITS" .

figi-ps:DWZI a figi-gii:PricingSource .

figi-ps:AAIL skos:prefLabel "abn amro inflation" .

figi-ps:DWZI skos:prefLabel "dwz - hanover fixing" .

figi-ps:BART a owl:NamedIndividual .

figi-ps:AAIL figi-gii:hasUniqueTextIdentifier "AAIL" .

figi-ps:BART a figi-gii:PricingSource .

figi-ps:DWZI figi-gii:hasUniqueTextIdentifier "DWZI" .

figi-st:agncyCmoZ a owl:NamedIndividual .

figi-ps:BART skos:prefLabel "barclays capital ust" .

figi-st:agncyCmoZ a figi-gii:SecurityType .

figi-ps:DWZM a owl:NamedIndividual .

figi-ps:BART figi-gii:hasUniqueTextIdentifier "BART" .

figi-ps:DWZM a figi-gii:PricingSource .

figi-st:agncyCmoZ skos:definition "Agency CMO Z (Accrual Bond), Fannie Mae, Freddie Mac, Ginnie Mae" .

figi-ps:DWZM skos:prefLabel "dwz - munich fixing" .

figi-st:termVatTrnch a owl:NamedIndividual .

figi-st:agncyCmoZ skos:prefLabel "agncy cmo z" .

figi-ps:DWZM figi-gii:hasUniqueTextIdentifier "DWZM" .

figi-st:agncyCmoZ figi-gii:hasUniqueTextIdentifier "Agncy CMO Z" .

figi-ps:DWZS a owl:NamedIndividual .

figi-st:termVatTrnch a figi-gii:SecurityType .

figi-ps:DWZS a figi-gii:PricingSource .

figi-ps:AAKB a owl:NamedIndividual , figi-gii:PricingSource .

figi-ps:DWZS skos:prefLabel "dwz - stuttgart fix" .

figi-ps:AAKB skos:prefLabel "aargauische kant" .

figi-ps:DWZS figi-gii:hasUniqueTextIdentifier "DWZS" .

figi-ps:AAKB figi-gii:hasUniqueTextIdentifier "AAKB" .

figi-ps:DXBB a owl:NamedIndividual .

figi-st:assetBack a owl:NamedIndividual .

figi-st:termVatTrnch skos:definition "A loan with a fixed availability period and often includes some minimum repayment schedule. Once borrowings have been repaid, they cannot be re-borrowed. Given as temporary reimbursement for a VAT credit it has with the state." .

figi-ps:DXBB a figi-gii:PricingSource .

figi-st:assetBack a figi-gii:SecurityType .

figi-st:termVatTrnch skos:prefLabel "term vat-trnch" .

figi-ps:DXBB skos:prefLabel "dexia bank belgium" .

figi-st:termVatTrnch figi-gii:hasUniqueTextIdentifier "TERM VAT-TRNCH" .

figi-st:assetBack skos:definition "A financial security backed by a loan, lease or receivables against assets other than real estate and mortgage-backed securities." .

figi-ps:DXBB figi-gii:hasUniqueTextIdentifier "DXBB" .

figi-ps:BARX a owl:NamedIndividual .

figi-st:assetBack skos:prefLabel "asset back" .

figi-ps:BARX a figi-gii:PricingSource .

figi-ps:DXBU a owl:NamedIndividual .

figi-st:assetBack figi-gii:hasUniqueTextIdentifier "ASSET BACK" .

figi-ps:DXBU a figi-gii:PricingSource .

figi-ps:BARX skos:prefLabel "barclays bank plc" .

figi-ps:DXBU skos:prefLabel "dubai bank" .

figi-ps:BARX skos:prefLabel "barclays bank plc." .

figi-ps:DXBU figi-gii:hasUniqueTextIdentifier "DXBU" .

figi-ps:BARX figi-gii:hasUniqueTextIdentifier "BARX" .

figi-ps:DXSK a owl:NamedIndividual , figi-gii:PricingSource .

figi-gii:FinancialInstrumentName a owl:Class .

figi-ps:DXSK skos:prefLabel "dexia bank slovensko" .

figi-st:thailandCP a owl:NamedIndividual .

figi-gii:FinancialInstrumentName rdfs:label "financial instrument name" .

figi-st:thailandCP a figi-gii:SecurityType .

figi-ps:DXSK figi-gii:hasUniqueTextIdentifier "DXSK" .

figi-st:thailandCP skos:definition "Thailand Commercial Paper" .

figi-gii:FinancialInstrumentName skos:definition "the English language name of the company or the financial instrument, e.g., a particular fund name. It sometimes includes a brief description of the security or a differentiating feature, e.g., the issuance date. The name of an instrument may change in conjunction with corporate actions." .

figi-st:thailandCP skos:prefLabel "thailand cp" .

figi-gii:FinancialInstrumentName rdfs:subClassOf figi-gii:Identifier .

figi-st:thailandCP figi-gii:hasUniqueTextIdentifier "THAILAND CP" .

figi-ps:DYBL a owl:NamedIndividual .

figi-ps:BASH a owl:NamedIndividual .

figi-st:assetBasedBridge a owl:NamedIndividual .

figi-ps:BASH a figi-gii:PricingSource .

figi-st:assetBasedBridge a figi-gii:SecurityType .

figi-ps:DYBL a figi-gii:PricingSource ;
	skos:prefLabel "dyer and blair inv b" .

figi-ps:BASH skos:prefLabel "boa shanghai internl" .

figi-ps:DYBL figi-gii:hasUniqueTextIdentifier "DYBL" .

figi-ps:BASH figi-gii:hasUniqueTextIdentifier "BASH" .

figi-st:assetBasedBridge skos:definition "Event-driven loan intended to provide finance for a short period of time until longer-term financing can be obtained. Fully secured by a specific pool of assets, with availability determined as a percentage of the current value of the collateral assets." .

figi-st:trackingStk a owl:NamedIndividual .

figi-ps:DYNA a owl:NamedIndividual .

figi-st:trackingStk a figi-gii:SecurityType .

figi-ps:DYNA a figi-gii:PricingSource .

figi-st:assetBasedBridge skos:prefLabel "asset-based bridge" .

figi-ps:DYNA skos:prefLabel "dynacapital sa" .

figi-st:assetBasedBridge figi-gii:hasUniqueTextIdentifier "ASSET-BASED BRIDGE" .

figi-st:trackingStk skos:definition "Tracking Stock. Shares issued by a company which pay a dividend determined by the performance of a specific portion of the whole company. Tracking stocks do not represent or require any change in business structure. Holders of tracking stock are considered to hold equity in the parent company and not the specific entity represented by the tracking stock. Tracking stock is often set up by companies that have several diverse divisions, both so that investors can take a share in a division of their interest, and so that the performance of these divisions can be tracked in terms of shareholder interest. A company will sometimes issue a tracking stock when it has a very successful division that it feels is underappreciated by the market and not fully reflected in the company's stock price." .

figi-ps:DYNA figi-gii:hasUniqueTextIdentifier "DYNA" .

figi-st:trackingStk skos:prefLabel "tracking stk" .

figi-ps:DYNC a owl:NamedIndividual .

figi-gii:Ticker a owl:Class .

figi-st:trackingStk figi-gii:hasUniqueTextIdentifier "Tracking Stk" .

figi-ps:DYNC a figi-gii:PricingSource .

figi-gii:Ticker rdfs:label "ticker" .

figi-ps:BASI a owl:NamedIndividual .

figi-ps:DYNC skos:prefLabel "dynacapital" .

figi-gii:Ticker skos:definition "the assigned ticker for a financial instrument; the rules for forming the ticker vary according to security class" .

figi-ps:BASI a figi-gii:PricingSource .

figi-ps:DYNC figi-gii:hasUniqueTextIdentifier "DYNC" .

figi-gii:Ticker rdfs:subClassOf figi-gii:Identifier .

figi-ps:BASI skos:prefLabel "bank of america sec" .

figi-ps:DZ a owl:NamedIndividual .

figi-st:assetBasedBridgeRev a owl:NamedIndividual .

figi-ps:DZ a figi-gii:PricingSource .

figi-ps:BASI figi-gii:hasUniqueTextIdentifier "BASI" .

figi-ps:DZ skos:prefLabel "dz bank intl" .

figi-ps:BASP a owl:NamedIndividual , figi-gii:PricingSource .

figi-st:assetBasedBridgeRev a figi-gii:SecurityType .

figi-ps:DZ figi-gii:hasUniqueTextIdentifier "DZ" .

figi-ps:BASP skos:prefLabel "bank of america-lon" .

figi-ps:DZAB a owl:NamedIndividual .

figi-ps:BASP figi-gii:hasUniqueTextIdentifier "BASP" .

figi-ps:DZAB a figi-gii:PricingSource .

figi-st:assetBasedBridgeRev skos:definition "Event-driven loan intended to provide finance for a short period of time until longer-term financing can be obtained. Fully secured by a specific pool of assets, with availability determined as a percentage of the current value of the collateral assets. Once borrowed funds are repaid they can be borrowed again." .

figi-ps:DZAB skos:prefLabel "dx bank asset backed" .

figi-st:treasuryBill a owl:NamedIndividual .

figi-st:assetBasedBridgeRev skos:prefLabel "asset-based bridge rev" .

figi-ps:DZAB skos:prefLabel "dz bank asset backed" .

figi-st:assetBasedBridgeRev figi-gii:hasUniqueTextIdentifier "ASSET-BASED BRIDGE REV" .

figi-ps:DZAB figi-gii:hasUniqueTextIdentifier "DZAB" .

figi-ps:DZAG a owl:NamedIndividual , figi-gii:PricingSource .

figi-st:treasuryBill a figi-gii:SecurityType .

figi-ps:AAM a owl:NamedIndividual .

figi-ps:DZAG skos:prefLabel "dz bank" .

figi-st:treasuryBill skos:definition "Represents the interest rate of short term bonds issued by governments." .

figi-ps:AAM a figi-gii:PricingSource .

figi-ps:DZAG figi-gii:hasUniqueTextIdentifier "DZAG" .

figi-ps:AAM skos:prefLabel "asset allocation" .

figi-st:treasuryBill skos:prefLabel "treasury bill" .

figi-ps:AAM figi-gii:hasUniqueTextIdentifier "AAM" .

figi-st:treasuryBill figi-gii:hasUniqueTextIdentifier "TREASURY BILL" .

figi-ps:DZBB a owl:NamedIndividual .

figi-ps:AAMT a owl:NamedIndividual .

figi-ps:DZBB a figi-gii:PricingSource .

figi-ps:AAMT a figi-gii:PricingSource .

figi-ps:DZBB skos:prefLabel "dz bank iii" .

figi-ps:BAT a owl:NamedIndividual .

figi-ps:DZBB figi-gii:hasUniqueTextIdentifier "DZBB" .

figi-ps:BAT a figi-gii:PricingSource .

figi-ps:DZF a owl:NamedIndividual .

figi-ps:BAT skos:prefLabel "emsx sqa" .

figi-ps:DZF a figi-gii:PricingSource .

figi-ps:BAT figi-gii:hasUniqueTextIdentifier "BAT" .

figi-ps:DZF skos:prefLabel "dz bank frankfurt" .

figi-st:uit a owl:NamedIndividual , figi-gii:SecurityType .

figi-ps:DZF figi-gii:hasUniqueTextIdentifier "DZF" .

figi-ps:AAMT skos:prefLabel "avenue asset mgmt" .

figi-st:uit skos:definition "Unit Investment Trust. A portfolio made up of a variety of different income securities that are pooled together and sold to investors as units. Each unit represents a fractional, undivided interest in the portfolio's principal and income." .

figi-ps:DZL1 a owl:NamedIndividual .

figi-ps:AAMT figi-gii:hasUniqueTextIdentifier "AAMT" .

figi-st:uit skos:prefLabel "uit" .

figi-ps:DZL1 a figi-gii:PricingSource .

figi-st:assetBasedDip a owl:NamedIndividual .

figi-st:uit figi-gii:hasUniqueTextIdentifier "UIT" .

figi-ps:DZL1 skos:prefLabel "dz bank1 mid" .

figi-st:assetBasedDip a figi-gii:SecurityType .

figi-ps:BATB a owl:NamedIndividual .

figi-ps:DZL1 figi-gii:hasUniqueTextIdentifier "DZL1" .

figi-ps:BATB a figi-gii:PricingSource .

figi-st:assetBasedDip skos:definition "Fully secured by a specific pool of assets, with availability determined as a percentage of the current value of the collateral assets. Issued when a company is in bankruptcy" .

figi-ps:DZL2 a owl:NamedIndividual .

figi-ps:BATB skos:prefLabel "banc of america tbas" .

figi-ps:DZL2 a figi-gii:PricingSource .

figi-st:assetBasedDip skos:prefLabel "asset-based dip" .

figi-ps:DZL2 skos:prefLabel "dz bank 2" .

figi-ps:BATB figi-gii:hasUniqueTextIdentifier "BATB" .

figi-ps:DZL2 figi-gii:hasUniqueTextIdentifier "DZL2" .

figi-st:ukGiltStock a owl:NamedIndividual , figi-gii:SecurityType .

figi-ps:DZL3 a owl:NamedIndividual , figi-gii:PricingSource .

figi-st:ukGiltStock skos:definition "Gilt. A British word used to connote a debt obligation." .

figi-ps:DZL3 skos:prefLabel "dz bank 3" .

figi-st:ukGiltStock skos:prefLabel "uk gilt stock" .

figi-ps:DZL3 figi-gii:hasUniqueTextIdentifier "DZL3" .

figi-st:ukGiltStock figi-gii:hasUniqueTextIdentifier "UK GILT STOCK" .

figi-ps:DZMI a owl:NamedIndividual , figi-gii:PricingSource .

figi-st:assetBasedDip figi-gii:hasUniqueTextIdentifier "ASSET-BASED DIP" .

figi-ps:BATC a owl:NamedIndividual .

figi-ps:DZMI skos:prefLabel "dz bank ag dzmi" .

figi-ps:AAMX a owl:NamedIndividual .

figi-ps:BATC a figi-gii:PricingSource .

figi-ps:AAMX a figi-gii:PricingSource .

figi-ps:DZMI figi-gii:hasUniqueTextIdentifier "DZMI" .

figi-ps:BATC skos:prefLabel "bk america intraday" .

figi-ps:AAMX skos:prefLabel "abn amro mexico" .

figi-ps:DZNY a owl:NamedIndividual .

figi-ps:BATC figi-gii:hasUniqueTextIdentifier "BATC" .

figi-ps:DZNY a figi-gii:PricingSource .

figi-ps:AAMX figi-gii:hasUniqueTextIdentifier "AAMX" .

figi-ps:BATR a owl:NamedIndividual .

figi-ps:DZNY skos:prefLabel "dz bank" .

figi-ps:BATR a figi-gii:PricingSource .

figi-st:assetBasedDipRev a owl:NamedIndividual .

figi-ps:DZNY figi-gii:hasUniqueTextIdentifier "DZNY" .

figi-ps:BATR skos:prefLabel "bk of america london" .

figi-ps:DZSG a owl:NamedIndividual .

figi-st:assetBasedDipRev a figi-gii:SecurityType .

figi-ps:BATR figi-gii:hasUniqueTextIdentifier "BATR" .

figi-ps:DZSG a figi-gii:PricingSource .

figi-st:unit a owl:NamedIndividual .

figi-ps:DZSG skos:prefLabel "dz bank singapore" .

figi-st:assetBasedDipRev skos:definition "Fully secured by a specific pool of assets, with availability determined as a percentage of the current value of the collateral assets. Issued when a company is in bankruptcy. Once borrowed funds are repaid they can be borrowed again." .

figi-st:unit a figi-gii:SecurityType .

figi-ps:DZSG figi-gii:hasUniqueTextIdentifier "DZSG" .

figi-st:assetBasedDipRev skos:prefLabel "asset-based dip rev" .

figi-ps:DZSP a owl:NamedIndividual , figi-gii:PricingSource ;
	skos:prefLabel "dz bank sg" .

figi-st:assetBasedDipRev figi-gii:hasUniqueTextIdentifier "ASSET-BASED DIP REV" .

figi-ps:DZSP figi-gii:hasUniqueTextIdentifier "DZSP" .

figi-ps:AAPL a owl:NamedIndividual .

figi-ps:DZWP a owl:NamedIndividual .

figi-ps:AAPL a figi-gii:PricingSource .

figi-ps:DZWP a figi-gii:PricingSource .

figi-ps:AAPL skos:prefLabel "apple inc" .

figi-ps:DZWP skos:prefLabel "dz bank polska s.a." .

figi-ps:AAPL figi-gii:hasUniqueTextIdentifier "AAPL" .

figi-ps:DZWP figi-gii:hasUniqueTextIdentifier "DZWP" .

figi-st:assetBasedDipTerm a owl:NamedIndividual .

figi-ps:EAAF a owl:NamedIndividual .

figi-st:unit skos:definition "A unit is an exchange traded equity-type investment that is similar to common stock. By owning securities or assets of an underlying business (or businesses), an income trust is structured to distribute cash flows from those businesses to unit holders in a tax efficient manner." .

figi-st:assetBasedDipTerm a figi-gii:SecurityType .

figi-ps:EAAF a figi-gii:PricingSource .

figi-st:unit skos:prefLabel "unit" .

figi-ps:EAAF skos:prefLabel "erste aa1" .

figi-st:assetBasedDipTerm skos:definition "Fully secured by a specific pool of assets, with availability determined as a percentage of the current value of the collateral assets. Issued when a company is in bankruptcy. Once borrowed, cannot be re-borrowed." .

figi-ps:EAAF figi-gii:hasUniqueTextIdentifier "EAAF" .

figi-st:assetBasedDipTerm skos:prefLabel "asset-based dip term" .

figi-ps:EAST a owl:NamedIndividual .

figi-st:assetBasedDipTerm figi-gii:hasUniqueTextIdentifier "ASSET-BASED DIP TERM" .

figi-ps:EAST a figi-gii:PricingSource .

figi-ps:AARB a owl:NamedIndividual .

figi-st:unit figi-gii:hasUniqueTextIdentifier "Unit" .

figi-ps:AARB a figi-gii:PricingSource .

figi-ps:EAST skos:prefLabel "eastern advisors" .

figi-ps:AARB skos:prefLabel "abn amro rbs" .

figi-ps:EAST figi-gii:hasUniqueTextIdentifier "EAST" .

figi-ps:AARB figi-gii:hasUniqueTextIdentifier "AARB" .

figi-ps:EB a owl:NamedIndividual .

figi-st:assetBasedLoc a owl:NamedIndividual .

figi-ps:BATS a owl:NamedIndividual .

figi-st:assetBasedLoc a figi-gii:SecurityType .

figi-ps:BATS a figi-gii:PricingSource .

figi-ps:EB a figi-gii:PricingSource .

figi-ps:BATS skos:prefLabel "bats top market data" .

figi-ps:EB skos:prefLabel "euro brokers" .

figi-st:assetBasedLoc skos:definition "Fully secured by a specific pool of assets, with availability determined as a percentage of the current value of the collateral assets. Guaranteed by the lender(s) and used for purchase of goods, completion of construction projects, and/or general purposes." .

figi-ps:EB figi-gii:hasUniqueTextIdentifier "EB" .

figi-st:assetBasedLoc skos:prefLabel "asset-based loc" .

figi-ps:EBBC a owl:NamedIndividual .

figi-st:assetBasedLoc figi-gii:hasUniqueTextIdentifier "ASSET-BASED LOC" .

figi-ps:EBBC a figi-gii:PricingSource .

figi-ps:AASG a owl:NamedIndividual .

figi-ps:BATS figi-gii:hasUniqueTextIdentifier "BATS" .

figi-ps:AASG a figi-gii:PricingSource .

figi-ps:EBBC skos:prefLabel "cfif ch evrbright bk" .

figi-ps:AASG skos:prefLabel "abn amro singapore" .

figi-st:usCD a owl:NamedIndividual .

figi-ps:EBBC figi-gii:hasUniqueTextIdentifier "EBBC" .

figi-ps:AASG figi-gii:hasUniqueTextIdentifier "AASG" .

figi-st:usCD a figi-gii:SecurityType .

figi-ps:EBCQ a owl:NamedIndividual .

figi-st:assetBasedLocGuaranteeF a owl:NamedIndividual .

figi-st:usCD skos:definition "US Certificates of Deposit" .

figi-ps:EBCQ a figi-gii:PricingSource .

figi-st:assetBasedLocGuaranteeF a figi-gii:SecurityType .

figi-st:usCD skos:prefLabel "u.s. cd" .

figi-ps:EBCQ skos:prefLabel "e-bond composite" .

figi-st:usCD figi-gii:hasUniqueTextIdentifier "U.S. CD" .

figi-st:assetBasedLocGuaranteeF skos:definition "A financial obligation of the borrower which has been guaranteed by the lender(s) to ensure a project is completed. Fully secured by a specific pool of assets, with availability determined as a percentage of the current value of the collateral assets." .

figi-ps:BATY a owl:NamedIndividual .

figi-st:assetBasedLocGuaranteeF skos:prefLabel "asset-based loc guarantee f" .

figi-ps:BATY a figi-gii:PricingSource .

figi-st:assetBasedLocGuaranteeF figi-gii:hasUniqueTextIdentifier "ASSET-BASED LOC GUARANTEE F" .

figi-ps:BATY skos:prefLabel "bank america closes" .

figi-gii:Identifier a owl:Class .

figi-ps:BATY figi-gii:hasUniqueTextIdentifier "BATY" .

figi-gii:Identifier rdfs:label "identifier" .

figi-ps:BAUM a owl:NamedIndividual .

figi-ps:EBCQ figi-gii:hasUniqueTextIdentifier "EBCQ" .

figi-ps:BAUM a figi-gii:PricingSource .

figi-ps:EBCT a owl:NamedIndividual .

figi-ps:BAUM skos:prefLabel "george k. baum and co." .

figi-ps:EBCT a figi-gii:PricingSource .

figi-ps:BAUM figi-gii:hasUniqueTextIdentifier "BAUM" .

figi-gii:Identifier skos:definition """An identifier is a name that identifies (that is, labels the identity of) either a unique object or a unique class of objects, where the 'object' or class may be an idea, physical (countable) object (or class thereof), or physical (noncountable) substance (or class thereof). The abbreviation ID often refers to identity, identification (the process of identifying), or an identifier (that is, an instance of identification). An identifier may be a word, number, letter, symbol, or any combination of those.

The words, numbers, letters, or symbols may follow an encoding system (wherein letters, digits, words, or symbols stand for (represent) ideas or longer names) or they may simply be arbitrary. When an identifier follows an encoding system, it is often referred to as a code or ID code. Identifiers that do not follow any encoding scheme are often said to be arbitrary IDs; they are arbitrarily assigned and have no greater meaning. (Sometimes identifiers are called 'codes' even when they are actually arbitrary, whether because the speaker believes that they have deeper meaning or simply because he is speaking casually and imprecisely.)""" .

figi-ps:EBCT skos:prefLabel "e-bond comp test" .

figi-gii:Identifier rdfs:subClassOf _:node1fqlq18m7x28 .

figi-ps:EBCT figi-gii:hasUniqueTextIdentifier "EBCT" .

figi-gii:Identifier sm:directSource "http://en.wikipedia.org/wiki/Identifier"^^xsd:anyURI .

figi-st:usCP a owl:NamedIndividual .

figi-st:assetBasedRev a owl:NamedIndividual .

figi-ps:EBI a owl:NamedIndividual .

figi-st:assetBasedRev a figi-gii:SecurityType .

figi-st:usCP a figi-gii:SecurityType .

figi-ps:EBI a figi-gii:PricingSource .

figi-st:assetBasedRev skos:definition "Fully secured by a specific pool of assets, with availability determined as a percentage of the current value of the collateral assets. Once borrowed funds are repaid they can be borrowed again." .

figi-st:usCP skos:definition "US Commercial Paper" .

figi-ps:EBI skos:prefLabel "erste bank investmen" .

figi-st:assetBasedRev skos:prefLabel "asset-based rev" .

figi-st:usCP skos:prefLabel "u.s. cp" .

figi-ps:EBI figi-gii:hasUniqueTextIdentifier "EBI" .

figi-st:assetBasedRev figi-gii:hasUniqueTextIdentifier "ASSET-BASED REV" .

figi-st:usCP figi-gii:hasUniqueTextIdentifier "U.S. CP" .

figi-ps:EBII a owl:NamedIndividual .

figi-ps:AASI a owl:NamedIndividual .

figi-ps:BAWG a owl:NamedIndividual .

figi-ps:EBII a figi-gii:PricingSource .

figi-ps:AASI a figi-gii:PricingSource .

figi-ps:BAWG a figi-gii:PricingSource .

figi-ps:AASI skos:prefLabel "abn-amro securities" .

figi-ps:EBII skos:prefLabel "emirates bank intl" .

figi-ps:AASI figi-gii:hasUniqueTextIdentifier "AASI" .

figi-ps:BAWG skos:prefLabel "bawag" .

figi-st:assetBasedTerm a owl:NamedIndividual .

figi-ps:BAWG figi-gii:hasUniqueTextIdentifier "BAWG" .

figi-st:assetBasedTerm a figi-gii:SecurityType .

figi-ps:BAXA a owl:NamedIndividual .

figi-ps:EBII figi-gii:hasUniqueTextIdentifier "EBII" .

figi-ps:BAXA a figi-gii:PricingSource .

figi-ps:EBIQ a owl:NamedIndividual .

figi-st:assetBasedTerm skos:definition "Fully secured by a specific pool of assets, with availability determined as a percentage of the current value of the collateral assets. Once borrowed, cannot be re-borrowed." .

figi-ps:EBIQ a figi-gii:PricingSource .

figi-ps:BAXA skos:prefLabel "bharti axa inv mgrs" .

figi-ps:EBIQ skos:prefLabel "e-bond inside" .

figi-st:assetBasedTerm skos:prefLabel "asset-based term" .

figi-ps:EBIQ figi-gii:hasUniqueTextIdentifier "EBIQ" .

figi-st:assetBasedTerm figi-gii:hasUniqueTextIdentifier "ASSET-BASED TERM" .

figi-ps:EBIT a owl:NamedIndividual .

figi-ps:AATP a owl:NamedIndividual .

figi-ps:BAXA figi-gii:hasUniqueTextIdentifier "BAXA" .

figi-ps:EBIT a figi-gii:PricingSource .

figi-st:usDomestic a owl:NamedIndividual .

figi-ps:EBIT skos:prefLabel "e-bond inside test" .

figi-st:usDomestic a figi-gii:SecurityType .

figi-ps:AATP a figi-gii:PricingSource .

figi-ps:EBIT figi-gii:hasUniqueTextIdentifier "EBIT" .

figi-st:usDomestic skos:definition "US issuer issuing in US dollar in the US market." .

figi-ps:EBLL a owl:NamedIndividual .

figi-ps:AATP skos:prefLabel "abn amro, taiwan" .

figi-st:usDomestic skos:prefLabel "us domestic" .

figi-ps:AATP figi-gii:hasUniqueTextIdentifier "AATP" .

figi-st:usDomestic figi-gii:hasUniqueTextIdentifier "US DOMESTIC" .

figi-ps:AAU2 a owl:NamedIndividual .

figi-ps:EBLL a figi-gii:PricingSource .

figi-ps:AAU2 a figi-gii:PricingSource .

figi-ps:BAYB a owl:NamedIndividual , figi-gii:PricingSource .

figi-ps:EBLL skos:prefLabel "euro broker" .

figi-ps:BAYB skos:prefLabel "bayernlb bills" .

figi-ps:EBLL figi-gii:hasUniqueTextIdentifier "EBLL" .

figi-ps:AAU2 skos:prefLabel "abn amro uruguay" .

figi-ps:BAYB figi-gii:hasUniqueTextIdentifier "BAYB" .

figi-ps:EBLO a owl:NamedIndividual .

figi-ps:AAU2 figi-gii:hasUniqueTextIdentifier "AAU2" .

figi-st:usGovernment a owl:NamedIndividual .

figi-ps:EBLO a figi-gii:PricingSource .

figi-st:usGovernment a figi-gii:SecurityType .

figi-st:australian a owl:NamedIndividual .

figi-ps:EBLO skos:prefLabel "bbg london ebnd" .

figi-st:usGovernment skos:definition "US Government issued security" .

figi-ps:EBLO figi-gii:hasUniqueTextIdentifier "EBLO" .

figi-st:usGovernment skos:prefLabel "us government" .

figi-ps:EBMX a owl:NamedIndividual .

figi-st:australian a figi-gii:SecurityType .

figi-st:usGovernment figi-gii:hasUniqueTextIdentifier "US GOVERNMENT" .

figi-ps:EBMX a figi-gii:PricingSource .

figi-st:australian skos:definition "Market issue type where the issue is an Australian issuer issuing in AUD into the Australian domestic mkt." .

figi-ps:EBMX skos:prefLabel "euro brokers london" .

figi-ps:BAYL a owl:NamedIndividual .

figi-st:australian skos:prefLabel "australian" .

figi-ps:BAYL a figi-gii:PricingSource .

figi-ps:EBMX figi-gii:hasUniqueTextIdentifier "EBMX" .

figi-st:australian figi-gii:hasUniqueTextIdentifier "AUSTRALIAN" .

figi-ps:EBND a owl:NamedIndividual .

figi-ps:BAYL skos:prefLabel "bayernlb onlion" .

figi-ps:EBND a figi-gii:PricingSource .

figi-ps:AAUR a owl:NamedIndividual .

figi-ps:BAYL figi-gii:hasUniqueTextIdentifier "BAYL" .

figi-ps:EBND skos:prefLabel "bloomberg e-bond" .

figi-ps:BAYP a owl:NamedIndividual .

figi-ps:EBND figi-gii:hasUniqueTextIdentifier "EBND" .

figi-ps:AAUR a figi-gii:PricingSource .

figi-ps:BAYP a figi-gii:PricingSource .

figi-ps:EBS a owl:NamedIndividual .

figi-ps:AAUR skos:prefLabel "abn amro uruguay" .

figi-ps:BAYP skos:prefLabel "bayernlb pfandbriefe" .

figi-ps:EBS a figi-gii:PricingSource .

figi-ps:AAUR figi-gii:hasUniqueTextIdentifier "AAUR" .

figi-ps:BAYP figi-gii:hasUniqueTextIdentifier "BAYP" .

figi-ps:EBS skos:prefLabel "everbright securitie" .

figi-st:usIntBearCP a owl:NamedIndividual .

figi-ps:EBS figi-gii:hasUniqueTextIdentifier "EBS" .

figi-st:usIntBearCP a figi-gii:SecurityType .

figi-st:australianCD a owl:NamedIndividual .

figi-ps:EBUA a owl:NamedIndividual .

figi-st:australianCD a figi-gii:SecurityType .

figi-ps:EBUA a figi-gii:PricingSource .

figi-st:usIntBearCP skos:definition "Interest-Bearing Note. A note on which the issuer has agreed to pay the face value plus interest." .

figi-ps:EBUA skos:prefLabel "jsc erste bank" .

figi-st:usIntBearCP skos:prefLabel "u.s. int bear cp" .

figi-ps:EBUA figi-gii:hasUniqueTextIdentifier "EBUA" .

figi-st:usIntBearCP figi-gii:hasUniqueTextIdentifier "U.S. INT BEAR CP" .

figi-ps:ECCB a owl:NamedIndividual .

figi-st:australianCD skos:definition "Certificate of Deposit (CD). A debt instrument issued by a bank that will pay interest, periodically or at maturity (set by competitive forces in the marketplace), and principal when it reaches maturity. Maturities range from a few weeks to several years. It may have a fixed or floating rate of interest. Certificate of Deposit Rollover. An investment strategy used to defer taxes on income from a Certificate of Deposit. An individual who has purchased a certificate of deposit on margin expected to mature in the following year, can deduct the interest on the loan in the current year and move the income from the certificate to the up-coming year." .

figi-ps:ECCB a figi-gii:PricingSource .

figi-ps:BAYS a owl:NamedIndividual , figi-gii:PricingSource .

figi-ps:ECCB skos:prefLabel "elara capital plc" .

figi-ps:BAYS skos:prefLabel "bayernlb jumbos" .

figi-ps:ECCB figi-gii:hasUniqueTextIdentifier "ECCB" .

figi-ps:BAYS figi-gii:hasUniqueTextIdentifier "BAYS" .

figi-ps:ECKZ a owl:NamedIndividual .

figi-st:usNonDollar a owl:NamedIndividual .

figi-ps:ECKZ a figi-gii:PricingSource .

figi-st:usNonDollar a figi-gii:SecurityType .

figi-st:australianCD skos:prefLabel "australian cd" .

figi-ps:ECKZ skos:prefLabel "eurasian capital" .

figi-st:usNonDollar skos:definition "A US issuer issuing into the US domestic mkt in a currency other than US Dollars" .

figi-ps:ECKZ figi-gii:hasUniqueTextIdentifier "ECKZ" .

figi-st:usNonDollar skos:prefLabel "us non-dollar" .

figi-ps:ECM a owl:NamedIndividual .

figi-st:australianCD figi-gii:hasUniqueTextIdentifier "AUSTRALIAN CD" .

figi-ps:ECM a figi-gii:PricingSource .

figi-st:usNonDollar figi-gii:hasUniqueTextIdentifier "US NON-DOLLAR" .

figi-ps:ECM skos:prefLabel "exelion capital mgmt" .

figi-ps:BB a owl:NamedIndividual .

figi-ps:ECM figi-gii:hasUniqueTextIdentifier "ECM" .

figi-ps:AAUS a owl:NamedIndividual .

figi-ps:BB a figi-gii:PricingSource .

figi-ps:ECMB a owl:NamedIndividual .

figi-ps:AAUS a figi-gii:PricingSource .

figi-ps:ECMB a figi-gii:PricingSource .

figi-ps:BB skos:prefLabel "japan brokers broker" .

figi-ps:AAUS skos:prefLabel "abn amro - usa" .

figi-ps:ECMB skos:prefLabel "ecm libra" .

figi-ps:BB figi-gii:hasUniqueTextIdentifier "BB" .

figi-ps:AAUS figi-gii:hasUniqueTextIdentifier "AAUS" .

figi-ps:ECMB figi-gii:hasUniqueTextIdentifier "ECMB" .

figi-st:varRateDemObl a owl:NamedIndividual .

figi-st:australianCP a owl:NamedIndividual .

figi-st:varRateDemObl a figi-gii:SecurityType .

figi-ps:ECML a owl:NamedIndividual .

figi-st:australianCP a figi-gii:SecurityType .

figi-ps:ECML a figi-gii:PricingSource .

figi-st:varRateDemObl skos:definition "Variable Rate Demand Obligation, Municipal instrument with varying resets frequencies" .

figi-ps:ECML skos:prefLabel "european credit man" .

figi-st:varRateDemObl skos:prefLabel "var rate dem obl" .

figi-ps:ECML figi-gii:hasUniqueTextIdentifier "ECML" .

figi-st:australianCP skos:definition "Commercial Paper. An unsecured short-term promise to repay a fixed amount on a certain future date. Commercial paper usually matures from 2 to 270 days and is traded on a discount basis. This debt instrument, issued by banks, companies and other borrowers, use only their credit ratings to back the security. Commercial Paper House. A dealer who buys commercial paper at one price, then tries to sell it at another." .

figi-st:varRateDemObl figi-gii:hasUniqueTextIdentifier "VAR RATE DEM OBL" .

figi-ps:ECON a owl:NamedIndividual .

figi-st:australianCP skos:prefLabel "australian cp" .

figi-ps:BB3 a owl:NamedIndividual .

figi-ps:ECON a figi-gii:PricingSource .

figi-st:australianCP figi-gii:hasUniqueTextIdentifier "AUSTRALIAN CP" .

figi-ps:ECON skos:prefLabel "econoinvest" .

figi-ps:BB3 a figi-gii:PricingSource .

figi-ps:AAWH a owl:NamedIndividual .

figi-ps:ECON figi-gii:hasUniqueTextIdentifier "ECON" .

figi-ps:BB3 skos:prefLabel "brokers bkr 3pm prc" .

figi-ps:ECOP a owl:NamedIndividual .

figi-ps:BB3 figi-gii:hasUniqueTextIdentifier "BB3" .

figi-ps:AAWH a figi-gii:PricingSource .

figi-ps:ECOP a figi-gii:PricingSource .

figi-ps:BB3P a owl:NamedIndividual , figi-gii:PricingSource .

figi-ps:AAWH skos:prefLabel "abn amro wholesale" .

figi-ps:BB3P skos:prefLabel "brokers broker 3pm" .

figi-ps:ECOP skos:prefLabel "ebi sa grp ecobk frc" .

figi-ps:AAWH figi-gii:hasUniqueTextIdentifier "AAWH" .

figi-ps:ECOP figi-gii:hasUniqueTextIdentifier "ECOP" .

figi-st:austrianCrt a owl:NamedIndividual .

figi-ps:BB3P figi-gii:hasUniqueTextIdentifier "BB3P" .

figi-st:austrianCrt a figi-gii:SecurityType .

figi-ps:EDI a owl:NamedIndividual .

figi-st:variableAnnuity a owl:NamedIndividual .

figi-ps:EDI a figi-gii:PricingSource .

figi-st:austrianCrt skos:definition "Austrian Certificate: Depositary Receipt issued in Austria," .

figi-ps:EDI skos:prefLabel "edi financial inc" .

figi-st:variableAnnuity a figi-gii:SecurityType .

figi-st:austrianCrt skos:prefLabel "austrian crt" .

figi-ps:EDI figi-gii:hasUniqueTextIdentifier "EDI" .

figi-st:variableAnnuity skos:definition "An annuity contract which provides future payments to the holder (the annuitant), usually at retirement, the size of which depends on the performance of the portfolio's securities." .

figi-st:austrianCrt figi-gii:hasUniqueTextIdentifier "Austrian Crt" .

figi-st:variableAnnuity skos:prefLabel "variable annuity" .

figi-ps:AAXE a owl:NamedIndividual .

figi-ps:EDIS a owl:NamedIndividual .

figi-ps:AAXE a figi-gii:PricingSource .

figi-st:variableAnnuity figi-gii:hasUniqueTextIdentifier "Variable Annuity" .

figi-ps:EDIS a figi-gii:PricingSource .

figi-ps:AAXE skos:prefLabel "abn amro axes" .

figi-ps:BBAG a owl:NamedIndividual .

figi-ps:EDIS skos:prefLabel "edison spa" .

figi-ps:BBAG a figi-gii:PricingSource ;
	skos:prefLabel "blp agency composite" .

figi-ps:EDIS figi-gii:hasUniqueTextIdentifier "EDIS" .

figi-ps:BBAG figi-gii:hasUniqueTextIdentifier "BBAG" .

figi-ps:EDRA a owl:NamedIndividual .

figi-st:vatTrnch a owl:NamedIndividual .

figi-ps:AAXE figi-gii:hasUniqueTextIdentifier "AAXE" .

figi-ps:EDRA a figi-gii:PricingSource .

figi-st:vatTrnch a figi-gii:SecurityType .

figi-st:bankAcceptBill a owl:NamedIndividual .

figi-ps:EDRA skos:prefLabel "edmond de rothschild" .

figi-st:vatTrnch skos:definition "A facility a company is given as temporary reimbursement for a VAT credit it has with the state. The banks anticipate a credit that should be covered by the state." .

figi-ps:EDRA figi-gii:hasUniqueTextIdentifier "EDRA" .

figi-st:vatTrnch skos:prefLabel "vat-trnch" .

figi-ps:EF a owl:NamedIndividual .

figi-st:vatTrnch figi-gii:hasUniqueTextIdentifier "VAT-TRNCH" .

figi-ps:EF a figi-gii:PricingSource .

figi-st:bankAcceptBill a figi-gii:SecurityType .

figi-ps:BBAI a owl:NamedIndividual .

figi-ps:EF skos:prefLabel "efg-hermes uae ltd" .

figi-ps:BBAI a figi-gii:PricingSource .

figi-ps:EF figi-gii:hasUniqueTextIdentifier "EF" .

figi-ps:BBAI skos:prefLabel "bb alt inv demo db" .

figi-ps:EFD a owl:NamedIndividual .

figi-st:bankAcceptBill skos:definition "Banker's Acceptance. A draft drawn and accepted by banks that is based upon funds that will pay its face value at maturity. The security is traded at a discount. Because the accepting institution is obligated to pay for the bill, a banker's acceptance is considered less risky than commercial paper. Bloomberg abbreviates bankers acceptance as BA." .

figi-ps:EFD a figi-gii:PricingSource .

figi-ps:BBAI figi-gii:hasUniqueTextIdentifier "BBAI" .

figi-ps:EFD skos:prefLabel "e fund management co" .

figi-st:venezuelanCP a owl:NamedIndividual .

figi-ps:EFD figi-gii:hasUniqueTextIdentifier "EFD" .

figi-st:venezuelanCP a figi-gii:SecurityType .

figi-st:bankAcceptBill skos:prefLabel "bank accept bill" .

figi-st:venezuelanCP skos:definition "Venezuelan Commercial Paper" .

figi-ps:EFFE a owl:NamedIndividual .

figi-st:bankAcceptBill figi-gii:hasUniqueTextIdentifier "BANK ACCEPT BILL" .

figi-st:venezuelanCP skos:prefLabel "venezuelan cp" .

figi-ps:EFFE a figi-gii:PricingSource .

figi-ps:AB a owl:NamedIndividual .

figi-st:venezuelanCP figi-gii:hasUniqueTextIdentifier "VENEZUELAN CP" .

figi-ps:EFFE skos:prefLabel "effe gestioni sgr" .

figi-ps:BBAQ a owl:NamedIndividual .

figi-ps:EFFE figi-gii:hasUniqueTextIdentifier "EFFE" .

figi-ps:BBAQ a figi-gii:PricingSource .

figi-ps:AB a figi-gii:PricingSource .

figi-ps:EFG a owl:NamedIndividual .

figi-ps:BBAQ skos:prefLabel "bbac sal" .

figi-ps:EFG a figi-gii:PricingSource .

figi-ps:AB skos:prefLabel "db alex brown" .

figi-ps:BBAQ figi-gii:hasUniqueTextIdentifier "BBAQ" .

figi-ps:EFG skos:prefLabel "efg eurobank ergasia" .

figi-st:volatilityDerivative a owl:NamedIndividual .

figi-ps:EFG figi-gii:hasUniqueTextIdentifier "EFG" .

figi-st:volatilityDerivative a figi-gii:SecurityType .

figi-ps:AB figi-gii:hasUniqueTextIdentifier "AB" .

figi-ps:EFGA a owl:NamedIndividual .

figi-st:volatilityDerivative skos:definition "Volatility derivatives are a class of derivative securities." .

figi-ps:EFGA a figi-gii:PricingSource .

figi-ps:ABA1 a owl:NamedIndividual .

figi-st:volatilityDerivative skos:prefLabel "volatility derivative" .

figi-ps:EFGA skos:prefLabel "efg eurobank abs" .

figi-ps:ABA1 a figi-gii:PricingSource .

figi-st:volatilityDerivative figi-gii:hasUniqueTextIdentifier "VOLATILITY DERIVATIVE" .

figi-ps:EFGA figi-gii:hasUniqueTextIdentifier "EFGA" .

figi-ps:ABA1 skos:prefLabel "abax bank" .

figi-ps:EFGC a owl:NamedIndividual .

figi-ps:ABA1 figi-gii:hasUniqueTextIdentifier "ABA1" .

figi-ps:EFGC a figi-gii:PricingSource .

figi-ps:BBBG a owl:NamedIndividual .

figi-st:bankBill a owl:NamedIndividual .

figi-ps:EFGC skos:prefLabel "efg capital" .

figi-ps:BBBG a figi-gii:PricingSource .

figi-st:bankBill a figi-gii:SecurityType .

figi-ps:EFGC figi-gii:hasUniqueTextIdentifier "EFGC" .

figi-ps:BBBG skos:prefLabel "bbg do brasil" .

figi-ps:EFGD a owl:NamedIndividual .

figi-st:bankBill skos:definition "A bank bill is a short-term money market investment of which the acceptor and/or endorser is a bank." .

figi-ps:EFGD a figi-gii:PricingSource .

figi-ps:BBBG figi-gii:hasUniqueTextIdentifier "BBBG" .

figi-st:bankBill skos:prefLabel "bank bill" .

figi-st:warrant a owl:NamedIndividual .

figi-st:bankBill figi-gii:hasUniqueTextIdentifier "BANK BILL" .

figi-ps:EFGD skos:prefLabel "efg-hermes uae ltd" .

figi-st:warrant a figi-gii:SecurityType .

figi-ps:EFGD figi-gii:hasUniqueTextIdentifier "EFGD" .

figi-ps:ABAM a owl:NamedIndividual .

figi-ps:EFGH a owl:NamedIndividual .

figi-ps:ABAM a figi-gii:PricingSource .

figi-st:warrant skos:definition "Warrant. A company-issued certificate that represents an option to buy a certain number of stock shares at a specific price before a predetermined date. A warrant, because it has a value of its own, can be traded on the open market. Bloomberg abbreviates warrants as WRNTS or WT." .

figi-ps:ABAM skos:prefLabel "abn amro asset mgt" .

figi-ps:EFGH a figi-gii:PricingSource .

figi-st:warrant skos:prefLabel "warrant" .

figi-ps:EFGH skos:prefLabel "efg hermes asset mgt" .

figi-st:warrant figi-gii:hasUniqueTextIdentifier "WARRANT" .

figi-ps:EFGH figi-gii:hasUniqueTextIdentifier "EFGH" .

figi-ps:BBBI a owl:NamedIndividual .

figi-ps:ABAM figi-gii:hasUniqueTextIdentifier "ABAM" .

figi-ps:EFGM a owl:NamedIndividual .

figi-ps:BBBI a figi-gii:PricingSource .

figi-ps:EFGM a figi-gii:PricingSource .

figi-st:bankNote a owl:NamedIndividual .

figi-ps:BBBI skos:prefLabel "bradesco bbi" .

figi-ps:EFGM skos:prefLabel "efg eurobank trading" .

figi-st:bankNote a figi-gii:SecurityType .

figi-ps:EFGM figi-gii:hasUniqueTextIdentifier "EFGM" .

figi-ps:BBBI figi-gii:hasUniqueTextIdentifier "BBBI" .

figi-ps:EFGN a owl:NamedIndividual .

figi-st:bankNote skos:definition "Banker's Acceptance. A draft drawn and accepted by banks that is based upon funds that will pay its face value at maturity. The security is traded at a discount. Because the accepting institution is obligated to pay for the bill, a banker's acceptance is considered less risky than commercial paper. Bloomberg abbreviates bankers acceptance as BA." .

figi-ps:EFGN a figi-gii:PricingSource .

figi-st:whenIssued a owl:NamedIndividual , figi-gii:SecurityType .

figi-st:bankNote skos:prefLabel "bank note" .

figi-ps:EFGN skos:prefLabel "efg-hermes hld a mnt" .

figi-st:bankNote figi-gii:hasUniqueTextIdentifier "BANK NOTE" .

figi-ps:EFGN figi-gii:hasUniqueTextIdentifier "EFGN" .

figi-ps:ABAN a owl:NamedIndividual .

figi-ps:EFGT a owl:NamedIndividual .

figi-st:whenIssued skos:definition "When Issued. A security traded before it receives final trading authorization with the investor receiving the certificate only after the final approval is granted. The transaction would be canceled automatically if the security failed to receive approval." .

figi-ps:EFGT a figi-gii:PricingSource .

figi-st:whenIssued skos:prefLabel "when issued" .

figi-ps:ABAN a figi-gii:PricingSource .

figi-ps:EFGT skos:prefLabel "efg-hermes uae ltd" .

figi-ps:ABAN skos:prefLabel "alternatif bank" .

figi-ps:EFGT figi-gii:hasUniqueTextIdentifier "EFGT" .

figi-st:whenIssued figi-gii:hasUniqueTextIdentifier "WHEN ISSUED" .

figi-ps:EFGX a owl:NamedIndividual .

figi-ps:ABAN figi-gii:hasUniqueTextIdentifier "ABAN" .

figi-ps:BBBT a owl:NamedIndividual .

figi-ps:EFGX a figi-gii:PricingSource .

figi-ps:BBBT a figi-gii:PricingSource .

figi-ps:EFGX skos:prefLabel "efg eurobank trading" .

figi-ps:ABAS a owl:NamedIndividual .

figi-ps:BBBT skos:prefLabel "bangkok bk public co" .

figi-ps:EFGX figi-gii:hasUniqueTextIdentifier "EFGX" .

figi-ps:ABAS a figi-gii:PricingSource .

figi-ps:BBBT figi-gii:hasUniqueTextIdentifier "BBBT" .

figi-ps:EFIM a owl:NamedIndividual .

figi-ps:ABAS skos:prefLabel "abanka" .

figi-ps:EFIM a figi-gii:PricingSource .

figi-st:whenIssuedOid a owl:NamedIndividual .

figi-ps:ABAS figi-gii:hasUniqueTextIdentifier "ABAS" .

figi-ps:EFIM skos:prefLabel "evrofinance mosnarba" .

figi-st:bankersAccept a owl:NamedIndividual .

figi-ps:EFIM figi-gii:hasUniqueTextIdentifier "EFIM" .

figi-st:bankersAccept a figi-gii:SecurityType .

figi-st:whenIssuedOid a figi-gii:SecurityType .

figi-ps:EFSL a owl:NamedIndividual , figi-gii:PricingSource .

figi-st:bankersAccept skos:definition "Bankers Acceptances - a draft or bill of exchange drawn on a bank and accepted by it" .

figi-st:whenIssuedOid skos:definition "Indicates if the security does not have a firm settlement." .

figi-ps:EFSL skos:prefLabel "eurobank ad" .

figi-st:bankersAccept skos:prefLabel "bankers accept" .

figi-ps:EFSL figi-gii:hasUniqueTextIdentifier "EFSL" .

figi-st:bankersAccept figi-gii:hasUniqueTextIdentifier "BANKERS ACCEPT" .

figi-ps:EGAM a owl:NamedIndividual .

figi-ps:ABAV a owl:NamedIndividual .

figi-ps:EGAM a figi-gii:PricingSource .

figi-ps:ABAV a figi-gii:PricingSource .

figi-st:whenIssuedOid skos:prefLabel "when issued, oid" .

figi-ps:EGAM skos:prefLabel "egamo" .

figi-ps:ABAV skos:prefLabel "abaco" .

figi-ps:EGAM figi-gii:hasUniqueTextIdentifier "EGAM" .

figi-ps:ABAV figi-gii:hasUniqueTextIdentifier "ABAV" .

figi-ps:EGFI a owl:NamedIndividual .

figi-st:bankersAcceptance a owl:NamedIndividual .

figi-ps:EGFI a figi-gii:PricingSource .

figi-st:bankersAcceptance a figi-gii:SecurityType .

figi-st:whenIssuedOid figi-gii:hasUniqueTextIdentifier "WHEN ISSUED, OID" .

figi-ps:EGFI skos:prefLabel "gfi" .

figi-st:bankersAcceptance skos:definition "A draft drawn and accepted by banks that is based upon funds that will pay its face value at maturity. The security is traded at a discount." .

figi-ps:EGFI figi-gii:hasUniqueTextIdentifier "EGFI" .

figi-st:bankersAcceptance skos:prefLabel "bankers acceptance" .

figi-ps:EGIR a owl:NamedIndividual .

figi-st:bankersAcceptance figi-gii:hasUniqueTextIdentifier "BANKERS ACCEPTANCE" .

figi-ps:EGIR a figi-gii:PricingSource .

figi-ps:BBCA a owl:NamedIndividual .

figi-ps:EGIR skos:prefLabel "eiger trading" .

figi-ps:ABAX a owl:NamedIndividual .

figi-ps:BBCA a figi-gii:PricingSource .

figi-ps:EGIR figi-gii:hasUniqueTextIdentifier "EGIR" .

figi-ps:ABAX a figi-gii:PricingSource .

figi-ps:BBCA skos:prefLabel "bank central asia" .

figi-ps:EGRO a owl:NamedIndividual .

figi-ps:ABAX skos:prefLabel "abax bank" .

figi-ps:EGRO a figi-gii:PricingSource .

figi-ps:BBCA figi-gii:hasUniqueTextIdentifier "BBCA" .

figi-ps:ABAX figi-gii:hasUniqueTextIdentifier "ABAX" .

figi-ps:EGRO skos:prefLabel "emerging growth" .

figi-st:basisSwap a owl:NamedIndividual .

figi-ps:EGRO figi-gii:hasUniqueTextIdentifier "EGRO" .

figi-st:basisSwap a figi-gii:SecurityType .

figi-ps:EGX a owl:NamedIndividual .

figi-ps:BBCB a owl:NamedIndividual .

figi-ps:EGX a figi-gii:PricingSource .

figi-st:basisSwap skos:definition "Exchange of different floating indices in the same currency" .

figi-ps:EGX skos:prefLabel "egyptian exchange" .

figi-st:basisSwap skos:prefLabel "basis swap" .

figi-ps:EGX figi-gii:hasUniqueTextIdentifier "EGX" .

figi-st:basisSwap figi-gii:hasUniqueTextIdentifier "BASIS SWAP" .

figi-ps:EHCI a owl:NamedIndividual .

figi-ps:ABBA a owl:NamedIndividual , figi-gii:PricingSource .

figi-ps:EHCI a figi-gii:PricingSource .

figi-ps:BBCB a figi-gii:PricingSource .

figi-ps:ABBA skos:prefLabel "abax bank - internal" .

figi-ps:EHCI skos:prefLabel "estrada hinjosa and co" .

figi-ps:ABBA figi-gii:hasUniqueTextIdentifier "ABBA" .

figi-ps:EHCI figi-gii:hasUniqueTextIdentifier "EHCI" .

figi-st:basketWrt a owl:NamedIndividual .

figi-ps:EHCP a owl:NamedIndividual .

figi-st:basketWrt a figi-gii:SecurityType .

figi-ps:EHCP a figi-gii:PricingSource .

figi-ps:BBCB skos:prefLabel "bbva" .

figi-st:basketWrt skos:definition "A warrant over a group of securities, often within a sector." .

figi-ps:EHCP skos:prefLabel "eurohypo" .

figi-st:basketWrt skos:prefLabel "basket wrt" .

figi-ps:EHCP figi-gii:hasUniqueTextIdentifier "EHCP" .

figi-st:basketWrt figi-gii:hasUniqueTextIdentifier "Basket WRT" .

figi-ps:EIA a owl:NamedIndividual .

figi-ps:ABBK a owl:NamedIndividual .

figi-ps:EIA a figi-gii:PricingSource .

figi-ps:ABBK a figi-gii:PricingSource .

figi-ps:BBCB figi-gii:hasUniqueTextIdentifier "BBCB" .

figi-ps:ABBK skos:prefLabel "abn amro bk karachi" .

figi-ps:EIA skos:prefLabel "emirates investment" .

figi-ps:ABBK figi-gii:hasUniqueTextIdentifier "ABBK" .

figi-st:yankee a owl:NamedIndividual .

figi-ps:EIA figi-gii:hasUniqueTextIdentifier "EIA" .

figi-st:bdr a owl:NamedIndividual .

figi-st:yankee a figi-gii:SecurityType .

figi-st:bdr a figi-gii:SecurityType .

figi-ps:EIBC a owl:NamedIndividual , figi-gii:PricingSource ;
	skos:prefLabel "exim bank of china" ;
	figi-gii:hasUniqueTextIdentifier "EIBC" .

figi-st:bdr skos:definition "Brazilian Depositary Receipt: These are certificates that represent the stocks from a foreign company and that are issued in Brazil by a local financial institution based on the amount of shares the institution holds." .

figi-ps:EIBO a owl:NamedIndividual .

figi-st:bdr skos:prefLabel "bdr" .

figi-ps:EIBO a figi-gii:PricingSource .

figi-st:bdr figi-gii:hasUniqueTextIdentifier "BDR" .

figi-ps:EIBO skos:prefLabel "eibor market fixing" .

figi-ps:ABBR a owl:NamedIndividual .

figi-ps:EIBO figi-gii:hasUniqueTextIdentifier "EIBO" .

figi-ps:ABBR a figi-gii:PricingSource .

figi-ps:EIBV a owl:NamedIndividual .

figi-st:yankee skos:definition "Yankee Bond. A foreign bond denominated in U.S. dollars and registered with the Securities and Exchange Commission for sale in the United States." .

figi-ps:ABBR skos:prefLabel "arab bank" .

figi-ps:EIBV a figi-gii:PricingSource .

figi-st:yankee skos:prefLabel "yankee" .

figi-ps:ABBR figi-gii:hasUniqueTextIdentifier "ABBR" .

figi-ps:EIBV skos:prefLabel "euro invest bank ag" .

figi-st:bearerDepNote a owl:NamedIndividual .

figi-ps:EIBV figi-gii:hasUniqueTextIdentifier "EIBV" .

figi-st:bearerDepNote a figi-gii:SecurityType .

figi-ps:EIGR a owl:NamedIndividual .

figi-st:yankee figi-gii:hasUniqueTextIdentifier "YANKEE" .

figi-st:bearerDepNote skos:definition "Bearer Security. A negotiable security owned by the holder who is not registered upon the issuers books. Title to bearer securities is transferred by delivery." .

figi-ps:EIGR a figi-gii:PricingSource .

figi-ps:BBCH a owl:NamedIndividual .

figi-st:bearerDepNote skos:prefLabel "bearer dep note" .

figi-ps:EIGR skos:prefLabel "eiger trading" .

figi-st:bearerDepNote figi-gii:hasUniqueTextIdentifier "BEARER DEP NOTE" .

figi-ps:EIGR figi-gii:hasUniqueTextIdentifier "EIGR" .

figi-ps:ABBV a owl:NamedIndividual .

figi-ps:EIIB a owl:NamedIndividual .

figi-ps:ABBV a figi-gii:PricingSource .

figi-ps:EIIB a figi-gii:PricingSource .

figi-ps:BBCH a figi-gii:PricingSource .

figi-ps:ABBV skos:prefLabel "an binh stock bank" .

figi-ps:EIIB skos:prefLabel "islamic inv bank plc" .

figi-ps:BBCH skos:prefLabel "bbva chile" .

figi-ps:ABBV figi-gii:hasUniqueTextIdentifier "ABBV" .

figi-ps:EIIB figi-gii:hasUniqueTextIdentifier "EIIB" .

figi-st:belgiumCP a owl:NamedIndividual .

figi-ps:EJGB a owl:NamedIndividual .

figi-st:belgiumCP a figi-gii:SecurityType .

figi-ps:EJGB a figi-gii:PricingSource .

figi-ps:BBCH figi-gii:hasUniqueTextIdentifier "BBCH" .

figi-ps:EJGB skos:prefLabel "goldman sachs japan" .

figi-st:belgiumCP skos:definition "Belgium Domestic Commercial Paper - An unsecured short-term promise to repay a fixed amount on a certain future date. Commercial paper usually matures from 2 to 270 days and is traded on a discount basis. This debt instrument, issued by banks, companies and other borrowers, use only their credit ratings to back the security. Commercial Paper House. A dealer who buys commercial paper at one price, then tries to sell it at another" .

figi-ps:EJGB figi-gii:hasUniqueTextIdentifier "EJGB" .

figi-st:belgiumCP skos:prefLabel "belgium cp" .

figi-ps:EKAG a owl:NamedIndividual .

figi-st:belgiumCP figi-gii:hasUniqueTextIdentifier "BELGIUM CP" .

figi-ps:EKAG a figi-gii:PricingSource .

figi-ps:ABCB a owl:NamedIndividual .

figi-st:yankeeCD a owl:NamedIndividual .

figi-ps:ABCB a figi-gii:PricingSource .

figi-ps:EKAG skos:prefLabel "ek riley investments" .

figi-ps:ABCB skos:prefLabel "arab banking corp" .

figi-ps:EKAG figi-gii:hasUniqueTextIdentifier "EKAG" .

figi-ps:ABCB figi-gii:hasUniqueTextIdentifier "ABCB" .

figi-ps:EKCM a owl:NamedIndividual .

figi-st:belgiumCert a owl:NamedIndividual .

figi-st:yankeeCD a figi-gii:SecurityType .

figi-ps:EKCM a figi-gii:PricingSource .

figi-st:belgiumCert a figi-gii:SecurityType .

figi-ps:EKCM skos:prefLabel "ek riley inv corps" .

figi-st:yankeeCD skos:definition "Yankee Certificates of Deposit, issued by Foreign Banks via US Branch" .

figi-st:belgiumCert skos:definition "Belgium Certificate: Depositary Receipts issued in Belgium." .

figi-ps:EKCM figi-gii:hasUniqueTextIdentifier "EKCM" .

figi-st:belgiumCert skos:prefLabel "belgium cert" .

figi-ps:EKRC a owl:NamedIndividual .

figi-st:belgiumCert figi-gii:hasUniqueTextIdentifier "Belgium Cert" .

figi-ps:EKRC a figi-gii:PricingSource .

figi-ps:ABCI a owl:NamedIndividual .

figi-st:yankeeCD skos:prefLabel "yankee cd" .

figi-ps:EKRC skos:prefLabel "ek riley" .

figi-ps:ABCI a figi-gii:PricingSource .

figi-st:yankeeCD figi-gii:hasUniqueTextIdentifier "YANKEE CD" .

figi-ps:EKRC figi-gii:hasUniqueTextIdentifier "EKRC" .

figi-ps:ABCI skos:prefLabel "abc international bk" .

figi-ps:ELAP a owl:NamedIndividual .

figi-ps:ABCI figi-gii:hasUniqueTextIdentifier "ABCI" .

figi-ps:ELAP a figi-gii:PricingSource .

figi-ps:BBCN a owl:NamedIndividual .

figi-st:billOfExchange a owl:NamedIndividual .

figi-ps:ELAP skos:prefLabel "elana inc" .

figi-st:billOfExchange a figi-gii:SecurityType .

figi-ps:BBCN a figi-gii:PricingSource .

figi-ps:ELAP figi-gii:hasUniqueTextIdentifier "ELAP" .

figi-ps:BBCN skos:prefLabel "barcap us converts" .

figi-ps:ELEV a owl:NamedIndividual .

figi-st:billOfExchange skos:definition "Bill of Exchange. A short-term debt, the collateral for which is either a commodity or another product in the midst of transit. Papers that require the addressee to pay the bearer or anotherr person on demand." .

figi-ps:ELEV a figi-gii:PricingSource .

figi-ps:BBCN figi-gii:hasUniqueTextIdentifier "BBCN" .

figi-ps:ELEV skos:prefLabel "elevation, llc" .

figi-st:billOfExchange skos:prefLabel "bill of exchange" .

figi-ps:ELEV figi-gii:hasUniqueTextIdentifier "ELEV" .

figi-st:yenCD a owl:NamedIndividual .

figi-st:billOfExchange figi-gii:hasUniqueTextIdentifier "BILL OF EXCHANGE" .

figi-ps:ELID a owl:NamedIndividual .

figi-st:yenCD a figi-gii:SecurityType .

figi-ps:ELID a figi-gii:PricingSource .

figi-ps:ABCK a owl:NamedIndividual , figi-gii:PricingSource .

figi-ps:ELID skos:prefLabel "elidata" .

figi-ps:ABCK skos:prefLabel "africa bkng corp ltd" .

figi-ps:ELID figi-gii:hasUniqueTextIdentifier "ELID" .

figi-ps:ABCK figi-gii:hasUniqueTextIdentifier "ABCK" .

figi-ps:ELIX a owl:NamedIndividual .

figi-st:bond a owl:NamedIndividual .

figi-ps:ELIX a figi-gii:PricingSource .

figi-st:bond a figi-gii:SecurityType .

figi-ps:ELIX skos:prefLabel "elixir securities" .

figi-st:yenCD skos:definition "Japanese Yen Certificates of Deposit" .

figi-ps:ELIX figi-gii:hasUniqueTextIdentifier "ELIX" .

figi-st:bond skos:definition "Bond. A long-term debt security, issued by a corporation or government, with a stated interest rate and fixed due dates when interest and principal must be paid. Specific features are written into each bond's indenture, including whether the interest and principal will be paid to the person in whose name the security is registered, or if it will be payable to anyone presenting its coupons, in which case it is considered a bearer bond. Bondholders have a promise of repayment from the issuer but hold no ownership privileges as stockholders do." .

figi-ps:ELLT a owl:NamedIndividual .

figi-st:bond skos:prefLabel "bond" .

figi-ps:ELLT a figi-gii:PricingSource .

figi-st:bond figi-gii:hasUniqueTextIdentifier "Bond" .

figi-st:yenCD skos:prefLabel "yen cd" .

figi-ps:ABCL a owl:NamedIndividual .

figi-st:yenCD figi-gii:hasUniqueTextIdentifier "YEN CD" .

figi-ps:ABCL a figi-gii:PricingSource .

figi-ps:ELLT skos:prefLabel "elliott capital" .

figi-ps:ABCL skos:prefLabel "abc test firm london" .

figi-ps:BBCO a owl:NamedIndividual .

figi-ps:ELLT figi-gii:hasUniqueTextIdentifier "ELLT" .

figi-ps:ABCL figi-gii:hasUniqueTextIdentifier "ABCL" .

figi-ps:EMBA a owl:NamedIndividual .

figi-ps:ABCM a owl:NamedIndividual .

figi-ps:BBCO a figi-gii:PricingSource .

figi-ps:ABCM a figi-gii:PricingSource .

figi-ps:EMBA a figi-gii:PricingSource .

figi-ps:BBCO skos:prefLabel "banco bancolombia" .

figi-ps:ABCM skos:prefLabel "abn amro new york" .

figi-ps:EMBA skos:prefLabel "embatco" .

figi-ps:ABCM figi-gii:hasUniqueTextIdentifier "ABCM" .

figi-ps:EMBA figi-gii:hasUniqueTextIdentifier "EMBA" .

figi-st:brazilianCDi a owl:NamedIndividual .

figi-ps:EMCO a owl:NamedIndividual .

figi-st:brazilianCDi a figi-gii:SecurityType .

figi-ps:EMCO a figi-gii:PricingSource .

figi-ps:BBCO figi-gii:hasUniqueTextIdentifier "BBCO" .

figi-st:brazilianCDi skos:definition "Brazilian Mmkt instrument, interbank deposits or certificado de deposito interbanco (CDI)" .

figi-ps:EMCO skos:prefLabel "emcore" .

figi-st:brazilianCDi skos:prefLabel "brazilian cdi" .

figi-ps:EMCO figi-gii:hasUniqueTextIdentifier "EMCO" .

figi-st:brazilianCDi figi-gii:hasUniqueTextIdentifier "BRAZILIAN CDI" .

figi-ps:EMCT a owl:NamedIndividual .

figi-ps:ABCN a owl:NamedIndividual .

figi-ps:EMCT a figi-gii:PricingSource .

figi-ps:ABCN a figi-gii:PricingSource .

figi-st:yenCP a owl:NamedIndividual .

figi-ps:ABCN skos:prefLabel "cfif agri bank of ch" .

figi-st:yenCP a figi-gii:SecurityType .

figi-ps:ABCN figi-gii:hasUniqueTextIdentifier "ABCN" .

figi-ps:EMCT skos:prefLabel "citigroup" .

figi-ps:ABCO a owl:NamedIndividual .

figi-st:yenCP skos:definition "Japanese Yen Commercial Paper" .

figi-ps:EMCT figi-gii:hasUniqueTextIdentifier "EMCT" .

figi-ps:ABCO a figi-gii:PricingSource .

figi-st:yenCP skos:prefLabel "yen cp" .

figi-ps:ABCO skos:prefLabel "abn amro inc ny" .

figi-ps:EMDI a owl:NamedIndividual .

figi-st:yenCP figi-gii:hasUniqueTextIdentifier "YEN CP" .

figi-ps:EMDI a figi-gii:PricingSource .

figi-ps:ABCO figi-gii:hasUniqueTextIdentifier "ABCO" .

figi-ps:EMDI skos:prefLabel "jp morgan emdi" .

figi-st:bridge a owl:NamedIndividual .

figi-ps:EMDI figi-gii:hasUniqueTextIdentifier "EMDI" .

figi-st:bridge a figi-gii:SecurityType .

figi-ps:BBDC a owl:NamedIndividual .

figi-ps:EMEA a owl:NamedIndividual .

figi-ps:BBDC a figi-gii:PricingSource .

figi-ps:EMEA a figi-gii:PricingSource .

figi-st:bridge skos:definition "A loan, often event-driven, intended to provide finance for a short period of time until longer-term, permanent financing can be obtained. Bridge loans often contain significant fee and/or interest rate step up provisions which kick in after a short period (i.e. 12 months or less)" .

figi-ps:EMEA skos:prefLabel "aim demo - emea" .

figi-ps:BBDC skos:prefLabel "banco bradesco s.a." .

figi-ps:EMEA figi-gii:hasUniqueTextIdentifier "EMEA" .

figi-ps:BBDC figi-gii:hasUniqueTextIdentifier "BBDC" .

figi-ps:EMPO a owl:NamedIndividual .

figi-st:bridge skos:prefLabel "bridge" .

figi-ps:EMPO a figi-gii:PricingSource .

figi-st:yieldCurve a owl:NamedIndividual .

figi-ps:EMPO skos:prefLabel "emporiki bank" .

figi-st:bridge figi-gii:hasUniqueTextIdentifier "BRIDGE" .

figi-ps:EMPO figi-gii:hasUniqueTextIdentifier "EMPO" .

figi-ps:ABD a owl:NamedIndividual , figi-gii:PricingSource .

figi-st:yieldCurve a figi-gii:SecurityType .

figi-ps:EMTA a owl:NamedIndividual .

figi-ps:ABD skos:prefLabel "abd investment man" .

figi-ps:EMTA a figi-gii:PricingSource .

figi-ps:ABD figi-gii:hasUniqueTextIdentifier "ABD" .

figi-st:yieldCurve skos:definition "A chart consisting of the yields of bonds of the same quality but different maturities. This can be used as a gauge to evaluate the future of the interest rates. An upward trend with short-term rates lower than long-term rates is called a positive yield curve, while a down trend is a negative or inverted yield curve." .

figi-st:bridgeDelayDraw a owl:NamedIndividual .

figi-ps:EMTA skos:prefLabel "emrg mkts trdr assoc" .

figi-st:yieldCurve skos:prefLabel "yield curve" .

figi-st:bridgeDelayDraw a figi-gii:SecurityType .

figi-ps:EMTA figi-gii:hasUniqueTextIdentifier "EMTA" .

figi-st:yieldCurve figi-gii:hasUniqueTextIdentifier "Yield Curve" .

figi-st:bridgeDelayDraw skos:definition "Event-driven loan intended to provide finance for a short period of time until longer-term financing can be obtained. Borrower is allowed to draw down on the loan in one or more drawings within a specified time period after the signing date." .

figi-ps:EMTS a owl:NamedIndividual .

figi-ps:BBDI a owl:NamedIndividual .

figi-st:bridgeDelayDraw skos:prefLabel "bridge delay-draw" .

figi-ps:EMTS a figi-gii:PricingSource .

figi-st:bridgeDelayDraw figi-gii:hasUniqueTextIdentifier "BRIDGE DELAY-DRAW" .

figi-ps:EMTS skos:prefLabel "euro mts exchange" .

figi-ps:ABE a owl:NamedIndividual .

figi-ps:EMTS figi-gii:hasUniqueTextIdentifier "EMTS" .

figi-ps:ABE a figi-gii:PricingSource .

figi-ps:BBDI a figi-gii:PricingSource .

figi-ps:ABE skos:prefLabel "axa bank europe" .

figi-ps:BBDI skos:prefLabel "banco bradesco s-a" .

figi-ps:ENAM a owl:NamedIndividual .

figi-ps:BBDI figi-gii:hasUniqueTextIdentifier "BBDI" .

figi-ps:ABE figi-gii:hasUniqueTextIdentifier "ABE" .

figi-st:zeroCoupon a owl:NamedIndividual .

figi-ps:ENAM a figi-gii:PricingSource .

figi-st:zeroCoupon a figi-gii:SecurityType .

figi-ps:ENAM skos:prefLabel "euronext amsterdam" .

figi-ps:ABEL a owl:NamedIndividual .

figi-st:zeroCoupon skos:definition "Zero Coupon Bond. A bond sold at deep discount that pays no interest until maturity, at which time the holder receives the bond's face value plus all accrued interest. While holders receive no interest on the bond until maturity, they are responsible for paying taxes each year on the unpaid interest." .

figi-ps:ABEL a figi-gii:PricingSource .

figi-st:zeroCoupon skos:prefLabel "zero coupon" .

figi-ps:ENAM figi-gii:hasUniqueTextIdentifier "ENAM" .

figi-ps:ABEL skos:prefLabel "abel-noser" .

figi-st:zeroCoupon figi-gii:hasUniqueTextIdentifier "ZERO COUPON" .

figi-ps:ABEL figi-gii:hasUniqueTextIdentifier "ABEL" .

figi-ps:ENPR a owl:NamedIndividual .

figi-ps:BBDO a owl:NamedIndividual .

figi-ps:ABFX a owl:NamedIndividual .

figi-ps:ENPR a figi-gii:PricingSource .

figi-ps:ABFX a figi-gii:PricingSource .

figi-ps:BBDO a figi-gii:PricingSource .

figi-ps:ENPR skos:prefLabel "enlaces prebon" .

figi-ps:ABFX skos:prefLabel "axa banque" .

figi-ps:ENPR figi-gii:hasUniqueTextIdentifier "ENPR" .

figi-ps:BBDO skos:prefLabel "barcap us cdos" .

figi-ps:ABFX figi-gii:hasUniqueTextIdentifier "ABFX" .

figi-ps:BBDO figi-gii:hasUniqueTextIdentifier "BBDO" .

figi-st:zeroCouponOid a owl:NamedIndividual .

figi-ps:EON a owl:NamedIndividual .

figi-ps:ABGB a owl:NamedIndividual .

figi-st:zeroCouponOid a figi-gii:SecurityType .

figi-ps:EON a figi-gii:PricingSource .

figi-ps:ABGB a figi-gii:PricingSource .

figi-ps:EON skos:prefLabel "eon bank berhad" .

figi-ps:ABGB skos:prefLabel "abg sundal collier" .

figi-ps:EON figi-gii:hasUniqueTextIdentifier "EON" .

figi-st:zeroCouponOid skos:definition "Also called a Capital Appreciation Bond (CAB). The bond is sold at a deep discount, but on interest payments are made. The bondholder receives the full value (par amount) of the bond at maturity. The security is an Original Issue Discount" .

figi-ps:ABGB figi-gii:hasUniqueTextIdentifier "ABGB" .

figi-st:zeroCouponOid skos:prefLabel "zero coupon, oid" .

figi-ps:EPCI a owl:NamedIndividual .

figi-st:bridgeDelayDrawTerm a owl:NamedIndividual .

figi-st:zeroCouponOid figi-gii:hasUniqueTextIdentifier "ZERO COUPON, OID" .

figi-ps:EPCI a figi-gii:PricingSource .

figi-st:bridgeDelayDrawTerm a figi-gii:SecurityType .

figi-ps:EPCI skos:prefLabel "equitable-pci bank" .

figi-ps:BBES a owl:NamedIndividual .

figi-ps:EPCI figi-gii:hasUniqueTextIdentifier "EPCI" .

figi-st:bridgeDelayDrawTerm skos:definition "Event-driven loan intended to provide finance for a short period of time until longer-term financing can be obtained. Borrower is allowed to draw down on the loan in one or more drawings within a specified time period after the signing date." ;
	skos:prefLabel "bridge delay-draw term" .

figi-ps:EPCS a owl:NamedIndividual .

figi-ps:BBES a figi-gii:PricingSource .

figi-ps:EPCS a figi-gii:PricingSource .

figi-ps:BBES skos:prefLabel "barclays bk sing" .

figi-st:bridgeDelayDrawTerm figi-gii:hasUniqueTextIdentifier "BRIDGE DELAY-DRAW TERM" .

figi-ps:EPCS skos:prefLabel "goldman sachs (asia)" ;
	figi-gii:hasUniqueTextIdentifier "EPCS" .

figi-ps:ABGR a owl:NamedIndividual , figi-gii:PricingSource .

figi-ps:EPF a owl:NamedIndividual .

figi-ps:ABGR skos:prefLabel "alpha bank" .

figi-ps:EPF a figi-gii:PricingSource .

figi-ps:ABGR figi-gii:hasUniqueTextIdentifier "ABGR" .

figi-ps:EPF skos:prefLabel "employee provident f" .

figi-st:bridgeGuaranteeFac a owl:NamedIndividual .

figi-ps:EPF figi-gii:hasUniqueTextIdentifier "EPF" .

figi-st:bridgeGuaranteeFac a figi-gii:SecurityType .

figi-ps:EPFM a owl:NamedIndividual .

figi-st:bridgeGuaranteeFac skos:definition "Short-term financing issued by a bank to ensure/guarantee that an underlying project is completed." .

figi-ps:EPFM a figi-gii:PricingSource .

figi-ps:BBES figi-gii:hasUniqueTextIdentifier "BBES" .

figi-ps:EPFM skos:prefLabel "everbright pramerica" .

figi-st:bridgeGuaranteeFac skos:prefLabel "bridge guarantee fac" .

figi-ps:EPFM figi-gii:hasUniqueTextIdentifier "EPFM" .

figi-ps:BBET a owl:NamedIndividual .

figi-st:bridgeGuaranteeFac figi-gii:hasUniqueTextIdentifier "BRIDGE GUARANTEE FAC" .

figi-ps:EPS1 a owl:NamedIndividual .

figi-ps:BBET a figi-gii:PricingSource .

figi-ps:EPS1 a figi-gii:PricingSource .

figi-st:bridgeIslamic a owl:NamedIndividual .

figi-ps:BBET skos:prefLabel "bloomberg be test" .

figi-ps:EPS1 skos:prefLabel "eps internal test" .

figi-st:bridgeIslamic a figi-gii:SecurityType .

figi-ps:BBET figi-gii:hasUniqueTextIdentifier "BBET" .

figi-ps:EPS1 figi-gii:hasUniqueTextIdentifier "EPS1" .

figi-ps:BBGX a owl:NamedIndividual .

figi-ps:EQBK a owl:NamedIndividual .

figi-ps:BBGX a figi-gii:PricingSource .

figi-ps:EQBK a figi-gii:PricingSource .

figi-ps:BBGX skos:prefLabel "bbva exe" .

figi-ps:EQBK skos:prefLabel "equity bank ltd" .

figi-ps:BBGX figi-gii:hasUniqueTextIdentifier "BBGX" .

figi-ps:EQBK figi-gii:hasUniqueTextIdentifier "EQBK" .

figi-st:bridgeIslamic skos:definition "Event-driven loan intended to provide finance for a short period of time until longer-term financing can be obtained. Interest cannot be charged, complying with Islamic/sharpie law. Instead, the loan is structured using discounts, sale or lease, profit participation, or repurchase agreements." .

figi-ps:BBH a owl:NamedIndividual .

figi-ps:EQLN a owl:NamedIndividual .

figi-st:bridgeIslamic skos:prefLabel "bridge islamic" .

figi-ps:BBH a figi-gii:PricingSource .

figi-ps:EQLN a figi-gii:PricingSource .

figi-st:bridgeIslamic figi-gii:hasUniqueTextIdentifier "BRIDGE ISLAMIC" .

figi-ps:BBH skos:prefLabel "brown brothers" .

figi-ps:EQLN skos:prefLabel "ubs new york" .

figi-ps:ABHF a owl:NamedIndividual .

figi-ps:BBH figi-gii:hasUniqueTextIdentifier "BBH" .

figi-ps:ABHF a figi-gii:PricingSource .

figi-ps:BBHG a owl:NamedIndividual .

figi-ps:EQLN figi-gii:hasUniqueTextIdentifier "EQLN" .

figi-ps:ABHF skos:prefLabel "alliancebernstein lp" .

figi-ps:BBHG a figi-gii:PricingSource .

figi-ps:EQQB a owl:NamedIndividual .

figi-ps:BBHG skos:prefLabel "barcap spreads" .

figi-ps:ABHF figi-gii:hasUniqueTextIdentifier "ABHF" .

figi-ps:EQQB a figi-gii:PricingSource .

figi-ps:BBHG figi-gii:hasUniqueTextIdentifier "BBHG" .

figi-st:bridgeIslamicRev a owl:NamedIndividual .

figi-ps:BBI a owl:NamedIndividual .

figi-ps:EQQB skos:prefLabel "equity bank ltd" .

figi-ps:BBI a figi-gii:PricingSource .

figi-st:bridgeIslamicRev a figi-gii:SecurityType .

figi-ps:EQQB figi-gii:hasUniqueTextIdentifier "EQQB" .

figi-ps:BBI skos:prefLabel "bloomberg idx prime" .

figi-ps:EQUA a owl:NamedIndividual .

figi-ps:BBI figi-gii:hasUniqueTextIdentifier "BBI" .

figi-ps:EQUA a figi-gii:PricingSource ;
	skos:prefLabel "equitas america" .

figi-ps:BBIN a owl:NamedIndividual .

figi-st:bridgeIslamicRev skos:definition "Event-driven loan intended to provide finance for a short period of time until longer-term financing can be obtained. Interest cannot be charged, complying with Islamic/sharpie law. Instead, the loan is structured using discounts, sale or lease, profit participation, or repurchase agreements. Once borrowed funds are repaid they can be borrowed again." .

figi-ps:BBIN a figi-gii:PricingSource .

figi-ps:EQUA figi-gii:hasUniqueTextIdentifier "EQUA" .

figi-ps:BBIN skos:prefLabel "bberg bond index" .

figi-st:bridgeIslamicRev skos:prefLabel "bridge islamic rev" .

figi-ps:BBIN figi-gii:hasUniqueTextIdentifier "BBIN" .

figi-ps:ERBG a owl:NamedIndividual .

figi-ps:BBIX a owl:NamedIndividual .

figi-st:bridgeIslamicRev figi-gii:hasUniqueTextIdentifier "BRIDGE ISLAMIC REV" .

figi-ps:ERBG a figi-gii:PricingSource .

figi-ps:BBIX a figi-gii:PricingSource .

figi-ps:ABKL a owl:NamedIndividual .

figi-ps:BBIX skos:prefLabel "bloomberg bond index" .

figi-ps:ERBG skos:prefLabel "eurobank ergasias" .

figi-ps:ABKL a figi-gii:PricingSource .

figi-ps:BBIX figi-gii:hasUniqueTextIdentifier "BBIX" .

figi-ps:ERBG figi-gii:hasUniqueTextIdentifier "ERBG" .

figi-ps:ABKL skos:prefLabel "alliance bank berhad" .

figi-ps:BBKL a owl:NamedIndividual .

figi-ps:ERCF a owl:NamedIndividual .

figi-ps:BBKL a figi-gii:PricingSource .

figi-ps:ABKL figi-gii:hasUniqueTextIdentifier "ABKL" .

figi-ps:ERCF a figi-gii:PricingSource .

figi-ps:BBKL skos:prefLabel "bangkok bank berhad" .

figi-st:bridgeIslamicTerm a owl:NamedIndividual .

figi-ps:BBKL figi-gii:hasUniqueTextIdentifier "BBKL" .

figi-ps:ERCF skos:prefLabel "geam ltd." .

figi-ps:BBKR a owl:NamedIndividual .

figi-st:bridgeIslamicTerm a figi-gii:SecurityType .

figi-ps:ERCF figi-gii:hasUniqueTextIdentifier "ERCF" .

figi-ps:BBKR a figi-gii:PricingSource ;
	skos:prefLabel "bbk bahrain" .

figi-ps:EREX a owl:NamedIndividual .

figi-ps:BBKR figi-gii:hasUniqueTextIdentifier "BBKR" .

figi-ps:EREX a figi-gii:PricingSource .

figi-ps:BBKW a owl:NamedIndividual .

figi-st:bridgeIslamicTerm skos:definition "Event-driven loan intended to provide finance for a short period of time until longer-term financing can be obtained. Interest cannot be charged, complying with Islamic/sharpie law. Instead, the loan is structured using discounts, sale or lease, profit participation, or repurchase agreements. Once borrowed, cannot be re-borrowed." .

figi-ps:BBKW a figi-gii:PricingSource .

figi-ps:EREX skos:prefLabel "eurex bond prices" .

figi-st:bridgeIslamicTerm skos:prefLabel "bridge islamic term" .

figi-ps:BBKW skos:prefLabel "boubyan bank" .

figi-ps:EREX figi-gii:hasUniqueTextIdentifier "EREX" .

figi-st:bridgeIslamicTerm figi-gii:hasUniqueTextIdentifier "BRIDGE ISLAMIC TERM" .

figi-ps:BBKW figi-gii:hasUniqueTextIdentifier "BBKW" .

figi-ps:ERFN a owl:NamedIndividual .

figi-ps:ABMB a owl:NamedIndividual .

figi-ps:BBKZ a owl:NamedIndividual .

figi-ps:ERFN a figi-gii:PricingSource .

figi-ps:BBKZ a figi-gii:PricingSource .

figi-ps:ABMB a figi-gii:PricingSource .

figi-ps:ERFN skos:prefLabel "eurofin securities" .

figi-ps:BBKZ skos:prefLabel "bank bukopin" .

figi-ps:ABMB skos:prefLabel "amanah butler berhad" .

figi-ps:ERFN figi-gii:hasUniqueTextIdentifier "ERFN" .

figi-ps:BBKZ figi-gii:hasUniqueTextIdentifier "BBKZ" .

figi-ps:ABMB figi-gii:hasUniqueTextIdentifier "ABMB" .

figi-ps:ERFS a owl:NamedIndividual .

figi-ps:BBL a owl:NamedIndividual .

figi-st:bridgePik a owl:NamedIndividual .

figi-ps:ERFS a figi-gii:PricingSource .

figi-st:bridgePik a figi-gii:SecurityType .

figi-ps:BBL a figi-gii:PricingSource .

figi-ps:ERFS skos:prefLabel "e de rothschild" .

figi-ps:BBL skos:prefLabel "bb london demo sys" .

figi-ps:ERFS figi-gii:hasUniqueTextIdentifier "ERFS" .

figi-st:bridgePik skos:definition "Event-driven loan intended to provide finance for a short period of time until longer-term financing can be obtained. Interest may be capitalized and added to the principal amount of the loan, which is then compounded and due to lenders at maturity." .

figi-ps:BBL figi-gii:hasUniqueTextIdentifier "BBL" .

figi-ps:ERGB a owl:NamedIndividual .

figi-st:bridgePik skos:prefLabel "bridge pik" .

figi-ps:ERGB a figi-gii:PricingSource .

figi-ps:BBLO a owl:NamedIndividual .

figi-ps:ERGB skos:prefLabel "erste bank etrading" .

figi-ps:BBLO a figi-gii:PricingSource .

figi-ps:ERGB figi-gii:hasUniqueTextIdentifier "ERGB" .

figi-st:bridgePik figi-gii:hasUniqueTextIdentifier "BRIDGE PIK" .

figi-ps:BBLO skos:prefLabel "bolsa nacional block" .

figi-ps:ERGP a owl:NamedIndividual .

figi-ps:ABMV a owl:NamedIndividual .

figi-ps:ERGP a figi-gii:PricingSource .

figi-ps:ABMV a figi-gii:PricingSource .

figi-ps:ERGP skos:prefLabel "energy advice" ;
	figi-gii:hasUniqueTextIdentifier "ERGP" .

figi-ps:ABMV skos:prefLabel "abn amro bank mumbai" .

figi-ps:ERPL a owl:NamedIndividual .

figi-ps:BBLO figi-gii:hasUniqueTextIdentifier "BBLO" .

figi-ps:ERPL a figi-gii:PricingSource ;
	skos:prefLabel "erste hungary indic" .

figi-ps:BBLP a owl:NamedIndividual .

figi-ps:ERPL figi-gii:hasUniqueTextIdentifier "ERPL" .

figi-ps:BBLP a figi-gii:PricingSource .

figi-ps:ERS a owl:NamedIndividual .

figi-ps:ABMV figi-gii:hasUniqueTextIdentifier "ABMV" .

figi-ps:BBLP skos:prefLabel "demo lon portfolio" .

figi-ps:ERS a figi-gii:PricingSource .

figi-ps:BBLP figi-gii:hasUniqueTextIdentifier "BBLP" .

figi-ps:ERS skos:prefLabel "ers - texas" .

figi-st:bridgePikRev a owl:NamedIndividual .

figi-ps:ERS figi-gii:hasUniqueTextIdentifier "ERS" .

figi-ps:BBMM a owl:NamedIndividual .

figi-st:bridgePikRev a figi-gii:SecurityType .

figi-ps:BBMM a figi-gii:PricingSource .

figi-ps:ERST a owl:NamedIndividual , figi-gii:PricingSource .

figi-ps:BBMM skos:prefLabel "barc-mark to mrkt" .

figi-ps:ERST skos:prefLabel "erste bank" .

figi-ps:BBMM figi-gii:hasUniqueTextIdentifier "BBMM" .

figi-ps:ERST figi-gii:hasUniqueTextIdentifier "ERST" .

figi-st:bridgePikRev skos:definition "Event-driven loan intended to provide finance for a short period of time until longer-term financing can be obtained. Interest may be capitalized and added to the principal amount of the loan, which is then compounded and due to lenders at maturity. Once borrowed funds are repaid they can be borrowed again." .

figi-ps:ESAT a owl:NamedIndividual .

figi-ps:BBMS a owl:NamedIndividual .

figi-ps:ESAT a figi-gii:PricingSource .

figi-st:bridgePikRev skos:prefLabel "bridge pik rev" .

figi-ps:ESAT skos:prefLabel "earth satellite corp" .

figi-ps:BBMS a figi-gii:PricingSource .

figi-ps:ESAT figi-gii:hasUniqueTextIdentifier "ESAT" .

figi-st:bridgePikRev figi-gii:hasUniqueTextIdentifier "BRIDGE PIK REV" .

figi-ps:ESBH a owl:NamedIndividual .

figi-ps:BBMS skos:prefLabel "bloomberg mop feed" .

figi-ps:ESBH a figi-gii:PricingSource .

figi-ps:ABMX a owl:NamedIndividual .

figi-ps:ESBH skos:prefLabel "erste and steiermaerk" .

figi-ps:BBMS figi-gii:hasUniqueTextIdentifier "BBMS" .

figi-ps:ESBH figi-gii:hasUniqueTextIdentifier "ESBH" .

figi-ps:ABMX a figi-gii:PricingSource .

figi-ps:BBN a owl:NamedIndividual .

figi-ps:ESBK a owl:NamedIndividual .

figi-ps:ABMX skos:prefLabel "abn amro mex" .

figi-ps:ESBK a figi-gii:PricingSource .

figi-ps:BBN a figi-gii:PricingSource .

figi-ps:ESBK skos:prefLabel "e sun bank" .

figi-ps:ABMX figi-gii:hasUniqueTextIdentifier "ABMX" .

figi-ps:BBN skos:prefLabel "broadbill investment" .

figi-ps:ESBK figi-gii:hasUniqueTextIdentifier "ESBK" .

figi-st:bridgePikTerm a owl:NamedIndividual .

figi-ps:BBN figi-gii:hasUniqueTextIdentifier "BBN" .

figi-ps:ESIB a owl:NamedIndividual .

figi-st:bridgePikTerm a figi-gii:SecurityType .

figi-ps:ESIB a figi-gii:PricingSource .

figi-ps:BBNV a owl:NamedIndividual , figi-gii:PricingSource .

figi-ps:ESIB skos:prefLabel "bes investimento brl" ;
	figi-gii:hasUniqueTextIdentifier "ESIB" .

figi-ps:BBNV skos:prefLabel "bolsa nacional" .

figi-ps:ESIN a owl:NamedIndividual .

figi-st:bridgePikTerm skos:definition "Event-driven loan intended to provide finance for a short period of time until longer-term financing can be obtained. Interest may be capitalized and added to the principal amount of the loan, which is then compounded and due to lenders at maturity. Once borrowed, cannot be re-borrowed." .

figi-ps:ESIN a figi-gii:PricingSource .

figi-ps:BBNV figi-gii:hasUniqueTextIdentifier "BBNV" .

figi-ps:ESIN skos:prefLabel "espirito santo" .

figi-st:bridgePikTerm skos:prefLabel "bridge pik term" .

figi-ps:ESIN figi-gii:hasUniqueTextIdentifier "ESIN" .

figi-ps:BBNY a owl:NamedIndividual .

figi-st:bridgePikTerm figi-gii:hasUniqueTextIdentifier "BRIDGE PIK TERM" .

figi-ps:ESKM a owl:NamedIndividual .

figi-ps:BBNY a figi-gii:PricingSource .

figi-ps:ESKM a figi-gii:PricingSource .

figi-st:bridgeRev a owl:NamedIndividual .

figi-ps:BBNY skos:prefLabel "bbva securities" .

figi-ps:ESKM skos:prefLabel "eskom" .

figi-st:bridgeRev a figi-gii:SecurityType .

figi-ps:ESKM figi-gii:hasUniqueTextIdentifier "ESKM" .

figi-ps:BBNY figi-gii:hasUniqueTextIdentifier "BBNY" .

figi-ps:ESPI a owl:NamedIndividual , figi-gii:PricingSource ;
	skos:prefLabel "espirito santo inv" .

figi-ps:BBOA a owl:NamedIndividual .

figi-ps:ESPI figi-gii:hasUniqueTextIdentifier "ESPI" .

figi-st:bridgeRev skos:definition "Event-driven loan intended to provide finance for a short period of time until longer-term financing can be obtained. Once borrowed funds are repaid they can be borrowed again." .

figi-ps:BBOA a figi-gii:PricingSource .

figi-ps:ESSO a owl:NamedIndividual .

figi-st:bridgeRev skos:prefLabel "bridge rev" .

figi-ps:ESSO a figi-gii:PricingSource .

figi-ps:BBOA skos:prefLabel "bancofamerica-bronze" .

figi-st:bridgeRev figi-gii:hasUniqueTextIdentifier "BRIDGE REV" .

figi-ps:BBOA figi-gii:hasUniqueTextIdentifier "BBOA" .

figi-st:bridgeRevGuaranteeFac a owl:NamedIndividual .

figi-ps:BBOG a owl:NamedIndividual , figi-gii:PricingSource .

figi-ps:ESSO skos:prefLabel "esso (imperial oil)" .

figi-ps:BBOG skos:prefLabel "banco de bogota" .

figi-st:bridgeRevGuaranteeFac a figi-gii:SecurityType .

figi-ps:ESSO figi-gii:hasUniqueTextIdentifier "ESSO" .

figi-ps:BBOG figi-gii:hasUniqueTextIdentifier "BBOG" .

figi-st:bridgeRevGuaranteeFac skos:definition "Short-term financing issued by a bank to ensure/guarantee that an underlying project is completed. Once funds are borrowed, they can be borrowed again." .

figi-ps:ESTB a owl:NamedIndividual .

figi-ps:BBRL a owl:NamedIndividual .

figi-st:bridgeRevGuaranteeFac skos:prefLabel "bridge rev guarantee fac" .

figi-ps:BBRL a figi-gii:PricingSource .

figi-ps:ESTB a figi-gii:PricingSource .

figi-st:bridgeRevGuaranteeFac figi-gii:hasUniqueTextIdentifier "BRIDGE REV GUARANTEE FAC" .

figi-ps:BBRL skos:prefLabel "ing belgium" .

figi-ps:ESTB skos:prefLabel "erste bank vienna" .

figi-ps:ABMY a owl:NamedIndividual .

figi-ps:BBRL figi-gii:hasUniqueTextIdentifier "BBRL" .

figi-ps:ABMY a figi-gii:PricingSource .

figi-ps:ESTB figi-gii:hasUniqueTextIdentifier "ESTB" .

figi-ps:BBRT a owl:NamedIndividual , figi-gii:PricingSource .

figi-ps:ABMY skos:prefLabel "amanah butler kl" .

figi-ps:BBRT skos:prefLabel "brokers bkr minutely" .

figi-ps:ABMY figi-gii:hasUniqueTextIdentifier "ABMY" .

figi-ps:BBRT figi-gii:hasUniqueTextIdentifier "BBRT" .

figi-ps:ETBK a owl:NamedIndividual .

figi-st:bridgeTerm a owl:NamedIndividual .

figi-ps:ETBK a figi-gii:PricingSource .

figi-ps:BBRU a owl:NamedIndividual .

figi-st:bridgeTerm a figi-gii:SecurityType .

figi-ps:BBRU a figi-gii:PricingSource .

figi-ps:ETBK skos:prefLabel "etrade" .

figi-ps:BBRU skos:prefLabel "barclays capital mos" .

figi-ps:ETBK figi-gii:hasUniqueTextIdentifier "ETBK" .

figi-st:bridgeTerm skos:definition "Event-driven loan intended to provide finance for a short period of time until longer-term financing can be obtained. Once borrowed, cannot be re-borrowed." .

figi-ps:BBRU figi-gii:hasUniqueTextIdentifier "BBRU" .

figi-ps:ETER a owl:NamedIndividual .

figi-st:bridgeTerm skos:prefLabel "bridge term" .

figi-ps:ETER a figi-gii:PricingSource .

figi-ps:BBRV a owl:NamedIndividual .

figi-st:bridgeTerm figi-gii:hasUniqueTextIdentifier "BRIDGE TERM" .

figi-ps:ETER skos:prefLabel "etera mutual pension" .

figi-ps:BBRV a figi-gii:PricingSource .

figi-ps:ABN a owl:NamedIndividual .

figi-ps:BBRV skos:prefLabel "barclays moscow" .

figi-ps:ETER figi-gii:hasUniqueTextIdentifier "ETER" .

figi-ps:BBRV figi-gii:hasUniqueTextIdentifier "BBRV" .

figi-ps:ETHK a owl:NamedIndividual , figi-gii:PricingSource .

figi-ps:BBSE a owl:NamedIndividual .

figi-ps:ETHK skos:prefLabel "e*trade hong kong" .

figi-ps:BBSE a figi-gii:PricingSource .

figi-ps:ETHK figi-gii:hasUniqueTextIdentifier "ETHK" .

figi-ps:BBSE skos:prefLabel "barclays" .

figi-ps:ETIQ a owl:NamedIndividual .

figi-ps:BBSE figi-gii:hasUniqueTextIdentifier "BBSE" .

figi-ps:ETIQ a figi-gii:PricingSource .

figi-ps:BBSF a owl:NamedIndividual .

figi-ps:ETIQ skos:prefLabel "etiqa insurance bhd" .

figi-ps:BBSF a figi-gii:PricingSource .

figi-ps:ETIQ figi-gii:hasUniqueTextIdentifier "ETIQ" .

figi-ps:BBSF skos:prefLabel "blp san francisco" .

figi-ps:ETLX a owl:NamedIndividual .

figi-ps:BBSF figi-gii:hasUniqueTextIdentifier "BBSF" .

figi-ps:ETLX a figi-gii:PricingSource .

figi-ps:BBSL a owl:NamedIndividual .

figi-ps:ETLX skos:prefLabel "eurotlx markets" .

figi-ps:BBSL a figi-gii:PricingSource .

figi-ps:ETLX figi-gii:hasUniqueTextIdentifier "ETLX" .

figi-ps:BBSL skos:prefLabel "bb securities ltd" .

figi-ps:ETPX a owl:NamedIndividual .

figi-ps:BBSL figi-gii:hasUniqueTextIdentifier "BBSL" .

figi-ps:ETPX a figi-gii:PricingSource ;
	skos:prefLabel "e-trade capital mkts" .

figi-ps:BBSN a owl:NamedIndividual .

figi-ps:ETPX figi-gii:hasUniqueTextIdentifier "ETPX" .

figi-ps:BBSN a figi-gii:PricingSource .

figi-ps:ETT a owl:NamedIndividual .

figi-ps:BBSN skos:prefLabel "barc-structnote" .

figi-ps:ETT a figi-gii:PricingSource .

figi-ps:BBSN figi-gii:hasUniqueTextIdentifier "BBSN" .

figi-ps:ETT skos:prefLabel "et only test" .

figi-ps:BBSW a owl:NamedIndividual .

figi-ps:ETT figi-gii:hasUniqueTextIdentifier "ETT" .

figi-ps:BBSW a figi-gii:PricingSource .

figi-ps:EUEU a owl:NamedIndividual .

figi-ps:BBSW skos:prefLabel "bloomberg energy" .

figi-ps:EUEU a figi-gii:PricingSource .

figi-ps:BBSW figi-gii:hasUniqueTextIdentifier "BBSW" .

figi-ps:EUEU skos:prefLabel "european commision" .

figi-ps:BBSX a owl:NamedIndividual .

figi-ps:EUEU figi-gii:hasUniqueTextIdentifier "EUEU" .

figi-ps:BBSX a figi-gii:PricingSource .

figi-ps:EUKZ a owl:NamedIndividual .

figi-ps:BBSX skos:prefLabel "bb securities" .

figi-ps:EUKZ a figi-gii:PricingSource .

figi-ps:BBSX figi-gii:hasUniqueTextIdentifier "BBSX" .

figi-ps:EUKZ skos:prefLabel "eurasian bank" .

figi-ps:BBT a owl:NamedIndividual .

figi-ps:EUKZ figi-gii:hasUniqueTextIdentifier "EUKZ" .

figi-ps:BBT a figi-gii:PricingSource ;
	skos:prefLabel "bloomberg bondtrader" ;
	figi-gii:hasUniqueTextIdentifier "BBT" .

figi-ps:BBT3 a owl:NamedIndividual , figi-gii:PricingSource ;
	skos:prefLabel "cbbt - futures close" ;
	figi-gii:hasUniqueTextIdentifier "BBT3" .

figi-ps:ABN a figi-gii:PricingSource .

figi-ps:BBTB a owl:NamedIndividual , figi-gii:PricingSource .

figi-ps:ABN skos:prefLabel "abn amro bank" .

figi-ps:BBTB skos:prefLabel "barcap t-bills" .

figi-ps:ABN figi-gii:hasUniqueTextIdentifier "ABN" .

figi-ps:BBTB figi-gii:hasUniqueTextIdentifier "BBTB" .

figi-st:bridgeVatTrnch a owl:NamedIndividual .

figi-ps:BBTC a owl:NamedIndividual .

figi-st:bridgeVatTrnch a figi-gii:SecurityType .

figi-ps:BBTC a figi-gii:PricingSource ;
	skos:prefLabel "bbandt capital markets" .

figi-st:bridgeVatTrnch skos:definition "Event-driven loan intended to provide finance for a short period of time until longer-term financing can be obtained. Given as temporary reimbursement for a VAT credit it has with the state." .

figi-ps:BBTC figi-gii:hasUniqueTextIdentifier "BBTC" .

figi-st:bridgeVatTrnch skos:prefLabel "bridge vat-trnch" .

figi-ps:BBTD a owl:NamedIndividual .

figi-st:bridgeVatTrnch figi-gii:hasUniqueTextIdentifier "BRIDGE VAT-TRNCH" .

figi-ps:BBTD a figi-gii:PricingSource .

figi-ps:EULF a owl:NamedIndividual .

figi-ps:ABNA a owl:NamedIndividual .

figi-ps:BBTD skos:prefLabel "bb tokyo demo sys" .

figi-ps:EULF a figi-gii:PricingSource .

figi-ps:ABNA a figi-gii:PricingSource .

figi-ps:BBTD figi-gii:hasUniqueTextIdentifier "BBTD" .

figi-ps:EULF skos:prefLabel "euroland finance" .

figi-ps:BBTR a owl:NamedIndividual .

figi-ps:EULF figi-gii:hasUniqueTextIdentifier "EULF" .

figi-ps:ABNA skos:prefLabel "abn amro asia" .

figi-ps:EURB a owl:NamedIndividual .

figi-ps:ABNA figi-gii:hasUniqueTextIdentifier "ABNA" .

figi-ps:BBTR a figi-gii:PricingSource .

figi-ps:EURB a figi-gii:PricingSource .

figi-st:bulldog a owl:NamedIndividual .

figi-ps:BBTR skos:prefLabel "bloomb ts training" .

figi-ps:EURB skos:prefLabel "euronext brussels" .

figi-st:bulldog a figi-gii:SecurityType .

figi-ps:EURB figi-gii:hasUniqueTextIdentifier "EURB" .

figi-ps:BBTR figi-gii:hasUniqueTextIdentifier "BBTR" .

figi-ps:EURC a owl:NamedIndividual .

figi-ps:BBTS a owl:NamedIndividual .

figi-ps:EURC a figi-gii:PricingSource .

figi-ps:BBTS a figi-gii:PricingSource .

figi-st:bulldog skos:definition "Bulldog Securities. Foreign securities traded in the U.K. with face values and interest payments quoted in pounds sterling. As with Gilts, bulldogs follow an Actual/Actual day count convention." .

figi-ps:BBTS skos:prefLabel "bloomberg ts demo" .

figi-ps:EURC skos:prefLabel "euro contributor" .

figi-ps:BBTS figi-gii:hasUniqueTextIdentifier "BBTS" .

figi-st:bulldog skos:prefLabel "bulldog" .

figi-ps:EURC figi-gii:hasUniqueTextIdentifier "EURC" .

figi-ps:BBTT a owl:NamedIndividual .

figi-st:bulldog figi-gii:hasUniqueTextIdentifier "BULLDOG" .

figi-ps:EURO a owl:NamedIndividual .

figi-ps:BBTT a figi-gii:PricingSource .

figi-ps:ABNB a owl:NamedIndividual .

figi-ps:EURO a figi-gii:PricingSource .

figi-ps:BBTT skos:prefLabel "bbt trade prices" .

figi-ps:ABNB a figi-gii:PricingSource .

figi-ps:EURO skos:prefLabel "aim demo tier1 emea" .

figi-ps:BBTT figi-gii:hasUniqueTextIdentifier "BBTT" .

figi-ps:ABNB skos:prefLabel "abn amro romania" .

figi-ps:EURO figi-gii:hasUniqueTextIdentifier "EURO" .

figi-ps:BBTX a owl:NamedIndividual .

figi-ps:ABNB figi-gii:hasUniqueTextIdentifier "ABNB" .

figi-ps:BBTX a figi-gii:PricingSource .

figi-ps:EURV a owl:NamedIndividual .

figi-st:butterflySwap a owl:NamedIndividual .

figi-ps:BBTX skos:prefLabel "bloomberg tradebook" .

figi-st:butterflySwap a figi-gii:SecurityType .

figi-ps:BBTX figi-gii:hasUniqueTextIdentifier "BBTX" .

figi-ps:EURV a figi-gii:PricingSource .

figi-ps:BBTY a owl:NamedIndividual .

figi-st:butterflySwap skos:definition "Quoted in basis points, butterfly swaps take the spread between 3 different interest rate swaps." .

figi-ps:BBTY a figi-gii:PricingSource .

figi-ps:EURV skos:prefLabel "eurovest global secs" .

figi-st:butterflySwap skos:prefLabel "butterfly swap" .

figi-ps:BBTY skos:prefLabel "bloomberg tradebook2" .

figi-ps:EURV figi-gii:hasUniqueTextIdentifier "EURV" .

figi-st:butterflySwap figi-gii:hasUniqueTextIdentifier "BUTTERFLY SWAP" .

figi-ps:BBTY figi-gii:hasUniqueTextIdentifier "BBTY" .

figi-ps:EURX a owl:NamedIndividual .

figi-ps:ABNE a owl:NamedIndividual .

figi-ps:EURX a figi-gii:PricingSource .

figi-ps:BBTZ a owl:NamedIndividual .

figi-ps:ABNE a figi-gii:PricingSource .

figi-ps:BBTZ a figi-gii:PricingSource .

figi-ps:EURX skos:prefLabel "european exchange" .

figi-ps:ABNE skos:prefLabel "abn amro s. africa" .

figi-ps:BBTZ skos:prefLabel "bloomberg tradebook3" .

figi-ps:EURX figi-gii:hasUniqueTextIdentifier "EURX" .

figi-ps:ABNE figi-gii:hasUniqueTextIdentifier "ABNE" .

figi-ps:BBTZ figi-gii:hasUniqueTextIdentifier "BBTZ" .

figi-ps:EUWX a owl:NamedIndividual .

figi-st:cadIntBearCP a owl:NamedIndividual .

figi-ps:BBUJ a owl:NamedIndividual .

figi-st:cadIntBearCP a figi-gii:SecurityType .

figi-ps:BBUJ a figi-gii:PricingSource .

figi-st:cadIntBearCP skos:definition "Canadian Interest Bearing Commercial Paper" .

figi-ps:EUWX a figi-gii:PricingSource .

figi-ps:BBUJ skos:prefLabel "bank buana" .

figi-st:cadIntBearCP skos:prefLabel "cad int bear cp" .

figi-ps:BBUJ figi-gii:hasUniqueTextIdentifier "BBUJ" .

figi-ps:EUWX skos:prefLabel "euwax" .

figi-st:cadIntBearCP figi-gii:hasUniqueTextIdentifier "CAD INT BEAR CP" .

figi-ps:BBV a owl:NamedIndividual .

figi-ps:EUWX figi-gii:hasUniqueTextIdentifier "EUWX" .

figi-ps:BBV a figi-gii:PricingSource .

figi-ps:ABNH a owl:NamedIndividual .

figi-ps:EVAB a owl:NamedIndividual .

figi-ps:ABNH a figi-gii:PricingSource .

figi-ps:EVAB a figi-gii:PricingSource .

figi-ps:ABNH skos:prefLabel "abn amro vietnam" .

figi-ps:BBV skos:prefLabel "banco bilbao viz, ny" .

figi-ps:EVAB skos:prefLabel "evolution secs ltd" .

figi-ps:ABNH figi-gii:hasUniqueTextIdentifier "ABNH" .

figi-ps:BBV figi-gii:hasUniqueTextIdentifier "BBV" .

figi-ps:EVAB figi-gii:hasUniqueTextIdentifier "EVAB" .

figi-st:calendarSpreadOption a owl:NamedIndividual .

figi-ps:BBVA a owl:NamedIndividual .

figi-st:calendarSpreadOption a figi-gii:SecurityType .

figi-ps:BBVA a figi-gii:PricingSource .

figi-ps:EVER a owl:NamedIndividual .

figi-ps:BBVA skos:prefLabel "bbva" .

figi-ps:EVER a figi-gii:PricingSource .

figi-st:calendarSpreadOption skos:definition "Option on a Calendar Spreads which consists of two futures contracts within the same instrument group and with different maturity months." .

figi-ps:EVER skos:prefLabel "cfet everbright bank" .

figi-ps:BBVA figi-gii:hasUniqueTextIdentifier "BBVA" .

figi-st:calendarSpreadOption skos:prefLabel "calendar spread option" .

figi-ps:EVER figi-gii:hasUniqueTextIdentifier "EVER" .

figi-ps:BBVF a owl:NamedIndividual .

figi-st:calendarSpreadOption figi-gii:hasUniqueTextIdentifier "Calendar Spread Option" .

figi-ps:EVGB a owl:NamedIndividual .

figi-ps:BBVF a figi-gii:PricingSource .

figi-ps:EVGB a figi-gii:PricingSource .

figi-ps:ABNN a owl:NamedIndividual .

figi-ps:BBVF skos:prefLabel "banco bilbao vizcaya" .

figi-ps:ABNN a figi-gii:PricingSource .

figi-ps:EVGB skos:prefLabel "cfet evergrowing bk" .

figi-ps:BBVF figi-gii:hasUniqueTextIdentifier "BBVF" .

figi-ps:ABNN skos:prefLabel "abn amro mortgage" .

figi-ps:EVGB figi-gii:hasUniqueTextIdentifier "EVGB" .

figi-ps:BBVL a owl:NamedIndividual .

figi-ps:ABNN skos:prefLabel "rbs nv mortgage" .

figi-ps:EVM a owl:NamedIndividual .

figi-ps:BBVL a figi-gii:PricingSource .

figi-ps:ABNN figi-gii:hasUniqueTextIdentifier "ABNN" .

figi-ps:EVM a figi-gii:PricingSource .

figi-st:callLoans a owl:NamedIndividual .

figi-ps:EVM skos:prefLabel "eaton vance mgt" .

figi-st:callLoans a figi-gii:SecurityType .

figi-ps:EVM figi-gii:hasUniqueTextIdentifier "EVM" .

figi-ps:BBVL skos:prefLabel "bbva markets" .

figi-ps:EVMT a owl:NamedIndividual .

figi-ps:BBVL figi-gii:hasUniqueTextIdentifier "BBVL" .

figi-ps:EVMT a figi-gii:PricingSource .

figi-st:callLoans skos:definition "Call Loan. A loan usually made to a broker or specialist by a commercial bank with securities as collateral. Brokers may then loan the money to customers to finance margin activities. Most such loans can be terminated by either party on 24-hours notice and hence are said to involve call money. Also called Brokers'Loan." .

figi-ps:BBVM a owl:NamedIndividual .

figi-ps:EVMT skos:prefLabel "eaton vance mgmt" .

figi-ps:BBVM a figi-gii:PricingSource .

figi-st:callLoans skos:prefLabel "call loans" .

figi-ps:EVMT figi-gii:hasUniqueTextIdentifier "EVMT" .

figi-ps:BBVM skos:prefLabel "bbva credit trading" .

figi-st:callLoans figi-gii:hasUniqueTextIdentifier "CALL LOANS" .

figi-ps:EVOL a owl:NamedIndividual .

figi-ps:BBVM figi-gii:hasUniqueTextIdentifier "BBVM" .

figi-ps:EVOL a figi-gii:PricingSource .

figi-ps:ABNO a owl:NamedIndividual .

figi-ps:BBVP a owl:NamedIndividual .

figi-ps:ABNO a figi-gii:PricingSource .

figi-ps:EVOL skos:prefLabel "evolution markets" .

figi-ps:BBVP a figi-gii:PricingSource .

figi-ps:ABNO skos:prefLabel "abn amro bk, jakarta" .

figi-ps:EVOL figi-gii:hasUniqueTextIdentifier "EVOL" .

figi-ps:BBVP skos:prefLabel "bbva trading" .

figi-ps:ABNO figi-gii:hasUniqueTextIdentifier "ABNO" .

figi-ps:EVOS a owl:NamedIndividual .

figi-ps:BBVP figi-gii:hasUniqueTextIdentifier "BBVP" .

figi-ps:EVOS a figi-gii:PricingSource .

figi-st:callableCP a owl:NamedIndividual .

figi-ps:BBVS a owl:NamedIndividual .

figi-ps:EVOS skos:prefLabel "evolution securities" .

figi-ps:BBVS a figi-gii:PricingSource .

figi-ps:EVOS figi-gii:hasUniqueTextIdentifier "EVOS" .

figi-st:callableCP a figi-gii:SecurityType .

figi-ps:BBVS skos:prefLabel "bbv securities" .

figi-ps:EWB a owl:NamedIndividual .

figi-ps:BBVS figi-gii:hasUniqueTextIdentifier "BBVS" .

figi-ps:EWB a figi-gii:PricingSource ;
	skos:prefLabel "east west bk" .

figi-st:callableCP skos:definition "An unsecured short-term promise to repay a fixed amount on a certain future date. Commercial paper usually matures from 2 to 270 days and is traded on a discount basis. This debt instrument, issued by banks, companies and other borrowers, use only their credit ratings to back the security." .

figi-ps:EWB figi-gii:hasUniqueTextIdentifier "EWB" .

figi-st:callableCP skos:prefLabel "callable cp" ;
	figi-gii:hasUniqueTextIdentifier "CALLABLE CP" .

figi-ps:EWBC a owl:NamedIndividual .

figi-ps:BBWR a owl:NamedIndividual .

figi-ps:EWBC a figi-gii:PricingSource .

figi-ps:ABNP a owl:NamedIndividual .

figi-ps:BBWR a figi-gii:PricingSource .

figi-ps:EWBC skos:prefLabel "east west bank phils" .

figi-ps:ABNP a figi-gii:PricingSource .

figi-ps:BBWR skos:prefLabel "barclays cap ny" .

figi-ps:EWBC figi-gii:hasUniqueTextIdentifier "EWBC" .

figi-ps:ABNP skos:prefLabel "bnp paribas" .

figi-ps:BBWR figi-gii:hasUniqueTextIdentifier "BBWR" .

figi-ps:EWBM a owl:NamedIndividual .

figi-ps:ABNP figi-gii:hasUniqueTextIdentifier "ABNP" .

figi-ps:BBYF a owl:NamedIndividual .

figi-ps:EWBM a figi-gii:PricingSource .

figi-ps:BBYF a figi-gii:PricingSource .

figi-ps:ABNS a owl:NamedIndividual .

figi-ps:EWBM skos:prefLabel "east west bnk" .

figi-ps:BBYF skos:prefLabel "blp jp yen-bonds px" .

figi-ps:ABNS a figi-gii:PricingSource .

figi-ps:EWBM figi-gii:hasUniqueTextIdentifier "EWBM" .

figi-ps:BBYF figi-gii:hasUniqueTextIdentifier "BBYF" .

figi-ps:ABNS skos:prefLabel "abn amro pmi" .

figi-ps:EWBT a owl:NamedIndividual .

figi-ps:BBYY a owl:NamedIndividual .

figi-ps:ABNS figi-gii:hasUniqueTextIdentifier "ABNS" .

figi-ps:BBYY a figi-gii:PricingSource .

figi-ps:ABNT a owl:NamedIndividual .

figi-ps:EWBT a figi-gii:PricingSource .

figi-ps:BBYY skos:prefLabel "blp jp yen-bond yld" .

figi-ps:ABNT a figi-gii:PricingSource .

figi-ps:EWBT skos:prefLabel "east west bank trade" .

figi-ps:BBYY figi-gii:hasUniqueTextIdentifier "BBYY" .

figi-ps:ABNT skos:prefLabel "abn amro ldn test" .

figi-ps:EWBT figi-gii:hasUniqueTextIdentifier "EWBT" .

figi-ps:BCAF a owl:NamedIndividual .

figi-ps:ABNT figi-gii:hasUniqueTextIdentifier "ABNT" .

figi-ps:EX a owl:NamedIndividual .

figi-ps:BCAF a figi-gii:PricingSource .

figi-ps:EX a figi-gii:PricingSource .

figi-ps:ABNV a owl:NamedIndividual .

figi-ps:BCAF skos:prefLabel "banco davivienda" .

figi-ps:ABNV a figi-gii:PricingSource .

figi-ps:EX skos:prefLabel "exchange" .

figi-ps:BCAF figi-gii:hasUniqueTextIdentifier "BCAF" .

figi-ps:ABNV skos:prefLabel "abn amro london" .

figi-ps:EX figi-gii:hasUniqueTextIdentifier "EX" .

figi-ps:BCAN a owl:NamedIndividual .

figi-ps:ABNV figi-gii:hasUniqueTextIdentifier "ABNV" .

figi-ps:EXA a owl:NamedIndividual .

figi-ps:BCAN a figi-gii:PricingSource .

figi-ps:EXA a figi-gii:PricingSource .

figi-st:canadian a owl:NamedIndividual .

figi-ps:BCAN skos:prefLabel "barclays - boom" .

figi-st:canadian a figi-gii:SecurityType .

figi-ps:EXA skos:prefLabel "exane paris" .

figi-ps:BCAN figi-gii:hasUniqueTextIdentifier "BCAN" .

figi-ps:EXA figi-gii:hasUniqueTextIdentifier "EXA" .

figi-st:canadian skos:definition "Market issue type where the issue is a Canadian issuer issuing in CAD into the Canadian domestic market." .

figi-ps:BCAP a owl:NamedIndividual .

figi-ps:EXCA a owl:NamedIndividual .

figi-ps:BCAP a figi-gii:PricingSource .

figi-st:canadian skos:prefLabel "canadian" .

figi-ps:EXCA a figi-gii:PricingSource .

figi-ps:BCAP skos:prefLabel "barclays capital-ny" .

figi-st:canadian figi-gii:hasUniqueTextIdentifier "CANADIAN" .

figi-ps:EXCA skos:prefLabel "exclusive analysis" .

figi-ps:BCAP figi-gii:hasUniqueTextIdentifier "BCAP" .

figi-ps:ABNX a owl:NamedIndividual .

figi-ps:EXCA figi-gii:hasUniqueTextIdentifier "EXCA" .

figi-ps:BCAR a owl:NamedIndividual .

figi-ps:ABNX a figi-gii:PricingSource .

figi-ps:EXCH a owl:NamedIndividual .

figi-ps:BCAR a figi-gii:PricingSource .

figi-ps:ABNX skos:prefLabel "abn amro auto-ex ldn" .

figi-ps:EXCH a figi-gii:PricingSource .

figi-ps:BCAR skos:prefLabel "banco del caribe" .

figi-ps:ABNX figi-gii:hasUniqueTextIdentifier "ABNX" .

figi-ps:EXCH skos:prefLabel "exchange traded" .

figi-ps:BCAR figi-gii:hasUniqueTextIdentifier "BCAR" .

figi-st:canadianCD a owl:NamedIndividual .

figi-ps:EXCH figi-gii:hasUniqueTextIdentifier "EXCH" .

figi-st:canadianCD a figi-gii:SecurityType .

figi-ps:BCAT a owl:NamedIndividual .

figi-ps:EXEC a owl:NamedIndividual .

figi-ps:BCAT a figi-gii:PricingSource .

figi-ps:EXEC a figi-gii:PricingSource .

figi-ps:BCAT skos:prefLabel "barclays cap aex" .

figi-ps:EXEC skos:prefLabel "execution limited" .

figi-ps:BCAT figi-gii:hasUniqueTextIdentifier "BCAT" .

figi-ps:EXEC figi-gii:hasUniqueTextIdentifier "EXEC" .

figi-ps:BCBA a owl:NamedIndividual .

figi-ps:EXIN a owl:NamedIndividual .

figi-ps:BCBA a figi-gii:PricingSource .

figi-ps:EXIN a figi-gii:PricingSource .

figi-ps:BCBA skos:prefLabel "bofa cdo px" .

figi-st:canadianCD skos:definition "Canadian Certificate of Deposit - A debt instrument issued by a bank that will pay interest, periodically or at maturity (set by competitive forces in the marketplace), and principal when it reaches maturity. Maturities range from a few weeks to several years. It may have a fixed or floating rate of interest. Certificate of Deposit Rollover. An investment strategy used to defer taxes on income from a Certificate of Deposit. An individual who has purchased a certificate of deposit on margin expected to mature in the following year, can deduct the interest on the loan in the current year and move the income from the certificate to the up-coming year." .

figi-ps:BCBA figi-gii:hasUniqueTextIdentifier "BCBA" .

figi-ps:EXIN skos:prefLabel "export and industry" .

figi-st:canadianCD skos:prefLabel "canadian cd" .

figi-ps:BCBI a owl:NamedIndividual .

figi-ps:EXIN figi-gii:hasUniqueTextIdentifier "EXIN" .

figi-ps:BCBI a figi-gii:PricingSource .

figi-st:canadianCD figi-gii:hasUniqueTextIdentifier "CANADIAN CD" .

figi-ps:EXKR a owl:NamedIndividual .

figi-ps:BCBI skos:prefLabel "barclays cap corp" .

figi-ps:ABNZ a owl:NamedIndividual .

figi-ps:EXKR a figi-gii:PricingSource .

figi-ps:ABNZ a figi-gii:PricingSource .

figi-ps:EXKR skos:prefLabel "akb express-credit" .

figi-ps:ABNZ skos:prefLabel "abn amro zurich" .

figi-ps:BCBI figi-gii:hasUniqueTextIdentifier "BCBI" .

figi-ps:ABNZ figi-gii:hasUniqueTextIdentifier "ABNZ" .

figi-ps:EXKR figi-gii:hasUniqueTextIdentifier "EXKR" .

figi-ps:BCBL a owl:NamedIndividual .

figi-st:canadianCP a owl:NamedIndividual .

figi-ps:EXNI a owl:NamedIndividual .

figi-st:canadianCP a figi-gii:SecurityType .

figi-ps:BCBL a figi-gii:PricingSource .

figi-ps:EXNI a figi-gii:PricingSource .

figi-st:canadianCP skos:definition "Canadian Commercial Paper" .

figi-ps:BCBL skos:prefLabel "colombia exc bl" .

figi-ps:EXNI skos:prefLabel "exco nusantra indo" .

figi-ps:BCBL figi-gii:hasUniqueTextIdentifier "BCBL" .

figi-st:canadianCP skos:prefLabel "canadian cp" .

figi-ps:EXNI figi-gii:hasUniqueTextIdentifier "EXNI" .

figi-st:canadianCP figi-gii:hasUniqueTextIdentifier "CANADIAN CP" .

figi-ps:BCBM a owl:NamedIndividual .

figi-ps:EXOT a owl:NamedIndividual .

figi-ps:ABP a owl:NamedIndividual .

figi-ps:BCBM a figi-gii:PricingSource .

figi-ps:EXOT a figi-gii:PricingSource .

figi-ps:ABP a figi-gii:PricingSource .

figi-ps:BCBM skos:prefLabel "barclays, india" .

figi-ps:EXOT skos:prefLabel "exotix ltd" .

figi-ps:BCBM figi-gii:hasUniqueTextIdentifier "BCBM" .

figi-ps:ABP skos:prefLabel "allied banking corp" .

figi-ps:EXOT figi-gii:hasUniqueTextIdentifier "EXOT" .

figi-ps:BCBO a owl:NamedIndividual .

figi-ps:ABP figi-gii:hasUniqueTextIdentifier "ABP" .

figi-ps:BCBO a figi-gii:PricingSource .

figi-ps:EXPG a owl:NamedIndividual .

figi-st:capsAndFloors a owl:NamedIndividual .

figi-ps:BCBO skos:prefLabel "bco central bolivia" .

figi-st:capsAndFloors a figi-gii:SecurityType .

figi-ps:BCBO figi-gii:hasUniqueTextIdentifier "BCBO" .

figi-ps:EXPG a figi-gii:PricingSource .

figi-ps:BCBY a owl:NamedIndividual .

figi-st:capsAndFloors skos:definition "Series of vanilla call (Cap)/put ( floor) options on a floating index" .

figi-ps:BCBY a figi-gii:PricingSource .

figi-ps:EXPG skos:prefLabel "experian services" .

figi-st:capsAndFloors skos:prefLabel "caps and floors" .

figi-ps:BCBY skos:prefLabel "bvc mec bajo lote" .

figi-ps:EXPG figi-gii:hasUniqueTextIdentifier "EXPG" .

figi-st:capsAndFloors figi-gii:hasUniqueTextIdentifier "CAPS & FLOORS" .

figi-ps:BCBY figi-gii:hasUniqueTextIdentifier "BCBY" .

figi-ps:EXT a owl:NamedIndividual .

figi-ps:ABPE a owl:NamedIndividual .

figi-ps:BCC a owl:NamedIndividual .

figi-ps:EXT a figi-gii:PricingSource .

figi-ps:BCC a figi-gii:PricingSource .

figi-ps:ABPE a figi-gii:PricingSource .

figi-ps:EXT skos:prefLabel "extolia mgmt llc" .

figi-ps:BCC skos:prefLabel "bolsa de comm chile" .

figi-ps:ABPE skos:prefLabel "apg" .

figi-ps:EXT figi-gii:hasUniqueTextIdentifier "EXT" .

figi-ps:BCC figi-gii:hasUniqueTextIdentifier "BCC" .

figi-ps:ABPE figi-gii:hasUniqueTextIdentifier "ABPE" .

figi-ps:FABI a owl:NamedIndividual .

figi-ps:BCCB a owl:NamedIndividual .

figi-st:carForward a owl:NamedIndividual .

figi-ps:FABI a figi-gii:PricingSource .

figi-ps:BCCB a figi-gii:PricingSource .

figi-st:carForward a figi-gii:SecurityType .

figi-ps:FABI skos:prefLabel "flemming asset mgmt" .

figi-ps:BCCB skos:prefLabel "cfet bank of beijing" .

figi-ps:FABI figi-gii:hasUniqueTextIdentifier "FABI" .

figi-ps:BCCB figi-gii:hasUniqueTextIdentifier "BCCB" .

figi-ps:FAF a owl:NamedIndividual .

figi-ps:BCCI a owl:NamedIndividual .

figi-ps:FAF a figi-gii:PricingSource .

figi-ps:BCCI a figi-gii:PricingSource ;
	skos:prefLabel "barclays cap corps" .

figi-st:carForward skos:definition "Carry Forward. shares that show the accumulated and undivided profits of a corporation after provision has been made for dividends and reserves" .

figi-ps:BCCI figi-gii:hasUniqueTextIdentifier "BCCI" .

figi-st:carForward skos:prefLabel "car forward" .

figi-ps:BCCK a owl:NamedIndividual .

figi-st:carForward figi-gii:hasUniqueTextIdentifier "Car Forward" .

figi-ps:BCCK a figi-gii:PricingSource .

figi-st:cash a owl:NamedIndividual .

figi-ps:BCCK skos:prefLabel "bcc invest" .

figi-st:cash a figi-gii:SecurityType .

figi-ps:BCCK figi-gii:hasUniqueTextIdentifier "BCCK" .

figi-ps:FAF skos:prefLabel "first american finan" .

figi-ps:BCCN a owl:NamedIndividual .

figi-st:cash skos:definition "Legal tender or coins that can be used in exchange goods, debt, or services. Sometimes also including the value of assets that can be converted into cash immediately, as reported by a company." .

figi-ps:BCCN a figi-gii:PricingSource .

figi-ps:FAF figi-gii:hasUniqueTextIdentifier "FAF" .

figi-ps:BCCN skos:prefLabel "cnbond beijing bank" .

figi-ps:FALQ a owl:NamedIndividual .

figi-ps:BCCN figi-gii:hasUniqueTextIdentifier "BCCN" .

figi-ps:FALQ a figi-gii:PricingSource .

figi-ps:BCCR a owl:NamedIndividual .

figi-ps:FALQ skos:prefLabel "falcon square cpl" .

figi-ps:BCCR a figi-gii:PricingSource .

figi-st:cash skos:prefLabel "cash" .

figi-ps:BCCR skos:prefLabel "bco cent costa rica" .

figi-ps:FALQ figi-gii:hasUniqueTextIdentifier "FALQ" .

figi-st:cash figi-gii:hasUniqueTextIdentifier "CASH" .

figi-ps:BCCR figi-gii:hasUniqueTextIdentifier "BCCR" .

figi-ps:FANC a owl:NamedIndividual .

figi-st:cblo a owl:NamedIndividual .

figi-ps:BCCS a owl:NamedIndividual .

figi-ps:FANC a figi-gii:PricingSource .

figi-st:cblo a figi-gii:SecurityType .

figi-ps:BCCS a figi-gii:PricingSource .

figi-ps:FANC skos:prefLabel "finance 500, inc" .

figi-ps:BCCS skos:prefLabel "colombia exc sl" .

figi-ps:FANC figi-gii:hasUniqueTextIdentifier "FANC" .

figi-ps:BCCS figi-gii:hasUniqueTextIdentifier "BCCS" .

figi-ps:FATR a owl:NamedIndividual .

figi-ps:BCCY a owl:NamedIndividual .

figi-st:cblo skos:definition "A money market instrument that represents an obligation between a borrower and a lender as to the terms and conditions of the loan. Collateralized borrowing and lending obligations (CBLOs) are used by those who have been phased out of or heavily restricted in the interbank call money market." .

figi-ps:BCCY a figi-gii:PricingSource .

figi-st:cblo skos:prefLabel "cblo" .

figi-ps:FATR a figi-gii:PricingSource .

figi-ps:BCCY skos:prefLabel "bolsa comm chile yld" .

figi-st:cblo figi-gii:hasUniqueTextIdentifier "CBLO" .

figi-ps:FATR skos:prefLabel "fator doria atherino" .

figi-ps:BCCY figi-gii:hasUniqueTextIdentifier "BCCY" .

figi-ps:ABPI a owl:NamedIndividual .

figi-ps:FATR figi-gii:hasUniqueTextIdentifier "FATR" .

figi-ps:BCDC a owl:NamedIndividual .

figi-ps:ABPI a figi-gii:PricingSource .

figi-ps:FAYB a owl:NamedIndividual .

figi-ps:BCDC a figi-gii:PricingSource .

figi-ps:ABPI skos:prefLabel "apg asset mgmt us" .

figi-ps:FAYB a figi-gii:PricingSource .

figi-ps:BCDC skos:prefLabel "bcba cont dc" .

figi-ps:ABPI figi-gii:hasUniqueTextIdentifier "ABPI" .

figi-ps:BCDC figi-gii:hasUniqueTextIdentifier "BCDC" .

figi-ps:FAYB skos:prefLabel "faysal bank limited" .

figi-st:cd a owl:NamedIndividual .

figi-ps:BCE a owl:NamedIndividual .

figi-st:cd a figi-gii:SecurityType .

figi-ps:BCE a figi-gii:PricingSource .

figi-ps:FAYB figi-gii:hasUniqueTextIdentifier "FAYB" .

figi-ps:BCE skos:prefLabel "bimcor inc" .

figi-ps:FBA a owl:NamedIndividual .

figi-ps:BCE figi-gii:hasUniqueTextIdentifier "BCE" .

figi-ps:FBA a figi-gii:PricingSource ;
	skos:prefLabel "cs first boston sydn" .

figi-ps:BCEE a owl:NamedIndividual .

figi-ps:FBA figi-gii:hasUniqueTextIdentifier "FBA" .

figi-ps:BCEE a figi-gii:PricingSource .

figi-st:cd skos:definition "Certificate of Deposit (CD). A debt instrument issued by a bank that will pay interest, periodically or at maturity (set by competitive forces in the marketplace), and principal when it reaches maturity. Maturities range from a few weeks to several years. It may have a fixed or floating rate of interest. Certificate of Deposit Rollover. An investment strategy used to defer taxes on income from a Certificate of Deposit. An individual who has purchased a certificate of deposit on margin expected to mature in the following year, can deduct the interest on the loan in the current year and move the income from the certificate to the up-coming year." .

figi-ps:BCEE skos:prefLabel "bcee" .

figi-ps:FBC a owl:NamedIndividual .

figi-st:cd skos:prefLabel "cd" .

figi-ps:BCEE figi-gii:hasUniqueTextIdentifier "BCEE" .

figi-ps:FBC a figi-gii:PricingSource .

figi-st:cd figi-gii:hasUniqueTextIdentifier "CD" .

figi-ps:BCEI a owl:NamedIndividual .

figi-ps:FBC skos:prefLabel "credit suisse mtges" .

figi-ps:ABSA a owl:NamedIndividual .

figi-ps:FBC figi-gii:hasUniqueTextIdentifier "FBC" .

figi-ps:BCEI a figi-gii:PricingSource .

figi-ps:ABSA a figi-gii:PricingSource .

figi-ps:FBEN a owl:NamedIndividual .

figi-ps:BCEI skos:prefLabel "banco cred inversion" .

figi-ps:ABSA skos:prefLabel "absa corp and merc bk" .

figi-ps:FBEN a figi-gii:PricingSource .

figi-ps:BCEI figi-gii:hasUniqueTextIdentifier "BCEI" .

figi-ps:ABSA figi-gii:hasUniqueTextIdentifier "ABSA" .

figi-ps:FBEN skos:prefLabel "fubon bank, hk" .

figi-ps:BCEM a owl:NamedIndividual .

figi-st:cdi a owl:NamedIndividual .

figi-ps:BCEM a figi-gii:PricingSource .

figi-ps:FBEN figi-gii:hasUniqueTextIdentifier "FBEN" .

figi-st:cdi a figi-gii:SecurityType .

figi-ps:BCEM skos:prefLabel "barclays em internal" .

figi-ps:FBET a owl:NamedIndividual .

figi-st:cdi skos:definition "Chess Depositary Interest" .

figi-ps:BCEM figi-gii:hasUniqueTextIdentifier "BCEM" .

figi-ps:FBET a figi-gii:PricingSource .

figi-st:cdi skos:prefLabel "cdi" .

figi-ps:BCGE a owl:NamedIndividual .

figi-ps:FBET skos:prefLabel "csfb eurotrade" .

figi-st:cdi figi-gii:hasUniqueTextIdentifier "CDI" .

figi-ps:BCGE a figi-gii:PricingSource .

figi-ps:FBET figi-gii:hasUniqueTextIdentifier "FBET" .

figi-ps:BCGE skos:prefLabel "bk cantonale geneve" .

figi-ps:ABSB a owl:NamedIndividual .

figi-ps:FBIT a owl:NamedIndividual .

figi-ps:BCGE figi-gii:hasUniqueTextIdentifier "BCGE" .

figi-ps:FBIT a figi-gii:PricingSource .

figi-ps:ABSB a figi-gii:PricingSource .

figi-ps:BCIC a owl:NamedIndividual .

figi-ps:FBIT skos:prefLabel "finansbank as" .

figi-ps:ABSB skos:prefLabel "amanah butler malay" .

figi-ps:BCIC a figi-gii:PricingSource .

figi-ps:FBIT figi-gii:hasUniqueTextIdentifier "FBIT" .

figi-ps:ABSB figi-gii:hasUniqueTextIdentifier "ABSB" .

figi-ps:BCIC skos:prefLabel "bci-banco credito in" .

figi-ps:FBIY a owl:NamedIndividual .

figi-st:cdr a owl:NamedIndividual .

figi-ps:FBIY a figi-gii:PricingSource .

figi-ps:BCIC figi-gii:hasUniqueTextIdentifier "BCIC" .

figi-st:cdr a figi-gii:SecurityType .

figi-ps:FBIY skos:prefLabel "finansbank, turkey" .

figi-ps:BCIE a owl:NamedIndividual , figi-gii:PricingSource .

figi-ps:FBIY figi-gii:hasUniqueTextIdentifier "FBIY" .

figi-ps:BCIE skos:prefLabel "bcie" .

figi-st:cdr skos:definition "Continental Depositary Receipt: Certificates issued by the Amsterdam Depository Company NV representing a specific number of shares of a security traded on an exchange of another country." .

figi-ps:BCIE figi-gii:hasUniqueTextIdentifier "BCIE" .

figi-ps:FBLT a owl:NamedIndividual .

figi-st:cdr skos:prefLabel "cdr" .

figi-ps:BCII a owl:NamedIndividual .

figi-ps:FBLT a figi-gii:PricingSource .

figi-st:cdr figi-gii:hasUniqueTextIdentifier "CDR" .

figi-ps:FBLT skos:prefLabel "first ballantyne llc" .

figi-ps:BCII a figi-gii:PricingSource .

figi-ps:ABSE a owl:NamedIndividual .

figi-ps:FBLT figi-gii:hasUniqueTextIdentifier "FBLT" .

figi-ps:BCII skos:prefLabel "banca commerciale it" .

figi-ps:ABSE a figi-gii:PricingSource .

figi-ps:BCII figi-gii:hasUniqueTextIdentifier "BCII" .

figi-ps:FBND a owl:NamedIndividual .

figi-ps:ABSE skos:prefLabel "absa sa e-bond" .

figi-ps:FBND a figi-gii:PricingSource .

figi-ps:ABSE figi-gii:hasUniqueTextIdentifier "ABSE" .

figi-ps:BCJP a owl:NamedIndividual .

figi-ps:FBND skos:prefLabel "fortis bk nederland" .

figi-st:cdsIndex a owl:NamedIndividual .

figi-ps:BCJP a figi-gii:PricingSource .

figi-st:cdsIndex a figi-gii:SecurityType .

figi-ps:BCJP skos:prefLabel "barclays jp indictve" .

figi-ps:FBND figi-gii:hasUniqueTextIdentifier "FBND" .

figi-ps:BCJP figi-gii:hasUniqueTextIdentifier "BCJP" .

figi-ps:FBNK a owl:NamedIndividual .

figi-ps:BCJX a owl:NamedIndividual .

figi-st:cdsIndex skos:definition "Credit Default Swap (CDS) index, an example of an index is SPD34VL9" .

figi-ps:FBNK a figi-gii:PricingSource .

figi-ps:BCJX a figi-gii:PricingSource .

figi-ps:FBNK skos:prefLabel "finansbank" .

figi-st:cdsIndex skos:prefLabel "cds index" .

figi-ps:BCJX skos:prefLabel "bancaja valencia" .

figi-ps:FBNK figi-gii:hasUniqueTextIdentifier "FBNK" .

figi-st:cdsIndex figi-gii:hasUniqueTextIdentifier "CDS Index" .

figi-ps:BCJX figi-gii:hasUniqueTextIdentifier "BCJX" .

figi-ps:FBNL a owl:NamedIndividual .

figi-ps:ABSG a owl:NamedIndividual .

figi-ps:BCLB a owl:NamedIndividual .

figi-ps:ABSG a figi-gii:PricingSource .

figi-ps:FBNL a figi-gii:PricingSource .

figi-ps:BCLB a figi-gii:PricingSource .

figi-ps:ABSG skos:prefLabel "abn amro sg" .

figi-ps:FBNL skos:prefLabel "fortis bank nederlan" .

figi-ps:BCLB skos:prefLabel "bancolombia sa" .

figi-ps:ABSG figi-gii:hasUniqueTextIdentifier "ABSG" .

figi-ps:FBNL figi-gii:hasUniqueTextIdentifier "FBNL" .

figi-ps:BCLB figi-gii:hasUniqueTextIdentifier "BCLB" .

figi-st:cf a owl:NamedIndividual .

figi-ps:FBNQ a owl:NamedIndividual .

figi-ps:BCLM a owl:NamedIndividual .

figi-ps:FBNQ a figi-gii:PricingSource .

figi-st:cf a figi-gii:SecurityType .

figi-ps:BCLM a figi-gii:PricingSource .

figi-ps:FBNQ skos:prefLabel "fbn capital limited" .

figi-st:cf skos:definition "Cash Flow (Only for CDO,CLO,CBO securities)" .

figi-ps:BCLM skos:prefLabel "bancolombia" .

figi-st:cf skos:prefLabel "cf" .

figi-ps:FBNQ figi-gii:hasUniqueTextIdentifier "FBNQ" .

figi-ps:BCLM figi-gii:hasUniqueTextIdentifier "BCLM" .

figi-st:cf figi-gii:hasUniqueTextIdentifier "CF" .

figi-ps:FBR a owl:NamedIndividual .

figi-ps:BCLN a owl:NamedIndividual .

figi-ps:FBR a figi-gii:PricingSource .

figi-st:closedEndFund a owl:NamedIndividual .

figi-ps:BCLN a figi-gii:PricingSource .

figi-ps:FBR skos:prefLabel "fbr capital markets" .

figi-st:closedEndFund a figi-gii:SecurityType .

figi-ps:BCLN skos:prefLabel "barclays bacr float" .

figi-ps:FBR figi-gii:hasUniqueTextIdentifier "FBR" .

figi-ps:BCLN figi-gii:hasUniqueTextIdentifier "BCLN" .

figi-ps:FBRC a owl:NamedIndividual .

figi-ps:BCMH a owl:NamedIndividual .

figi-ps:FBRC a figi-gii:PricingSource .

figi-ps:BCMH a figi-gii:PricingSource .

figi-ps:FBRC skos:prefLabel "fbr and co, inc ny" .

figi-ps:BCMH skos:prefLabel "bk of communications" .

figi-ps:FBRC figi-gii:hasUniqueTextIdentifier "FBRC" .

figi-ps:BCMH figi-gii:hasUniqueTextIdentifier "BCMH" .

figi-st:closedEndFund skos:definition "A closed-end fund is a collective investment scheme with a limited number of shares. New shares are rarely issued after the fund is launched; shares are not normally redeemable for cash or securities until the fund liquidates. Typically an investor can acquire shares in a closed-end fund by buying shares on a secondary market from a broker, market maker, or other investor as opposed to an Open-end fund where all transactions eventually involve the fund company creating new shares on the fly (in exchange for either cash or securities) or redeeming shares (for cash or securities)." .

figi-ps:BCMN a owl:NamedIndividual .

figi-ps:FBRI a owl:NamedIndividual .

figi-st:closedEndFund skos:prefLabel "closed-end fund" .

figi-ps:FBRI a figi-gii:PricingSource .

figi-st:closedEndFund figi-gii:hasUniqueTextIdentifier "Closed-End Fund" .

figi-ps:FBRI skos:prefLabel "friedman billings" .

figi-ps:ABSL a owl:NamedIndividual .

figi-ps:FBRI figi-gii:hasUniqueTextIdentifier "FBRI" .

figi-ps:BCMN a figi-gii:PricingSource .

figi-ps:ABSL a figi-gii:PricingSource .

figi-ps:FBSD a owl:NamedIndividual , figi-gii:PricingSource .

figi-ps:ABSL skos:prefLabel "abn amro abs" .

figi-ps:FBSD skos:prefLabel "first brokers sec" .

figi-ps:ABSL figi-gii:hasUniqueTextIdentifier "ABSL" .

figi-ps:FBSD figi-gii:hasUniqueTextIdentifier "FBSD" .

figi-ps:ABSO a owl:NamedIndividual .

figi-ps:BCMN skos:prefLabel "cfet bk of communica" .

figi-ps:FBSL a owl:NamedIndividual .

figi-ps:ABSO a figi-gii:PricingSource .

figi-ps:FBSL a figi-gii:PricingSource .

figi-ps:BCMN figi-gii:hasUniqueTextIdentifier "BCMN" .

figi-ps:ABSO skos:prefLabel "absolut bank moscow" .

figi-ps:FBSL skos:prefLabel "first broker securit" .

figi-ps:BCMO a owl:NamedIndividual .

figi-ps:ABSO figi-gii:hasUniqueTextIdentifier "ABSO" .

figi-ps:FBSL figi-gii:hasUniqueTextIdentifier "FBSL" .

figi-ps:BCMO a figi-gii:PricingSource .

figi-st:cmbs a owl:NamedIndividual .

figi-ps:FBTR a owl:NamedIndividual .

figi-ps:BCMO skos:prefLabel "bear stearns" .

figi-ps:FBTR a figi-gii:PricingSource .

figi-st:cmbs a figi-gii:SecurityType .

figi-ps:BCMO skos:prefLabel "bear stearns*" .

figi-ps:FBTR skos:prefLabel "fortis bank istanbul" .

figi-ps:BCMO figi-gii:hasUniqueTextIdentifier "BCMO" .

figi-ps:FBTR figi-gii:hasUniqueTextIdentifier "FBTR" .

figi-st:cmbs skos:definition "Commercial Mortgage Backed Security: a mortgage backed by commercial property." .

figi-ps:BCMP a owl:NamedIndividual .

figi-ps:FCAP a owl:NamedIndividual .

figi-st:cmbs skos:prefLabel "cmbs" .

figi-ps:BCMP a figi-gii:PricingSource .

figi-ps:FCAP a figi-gii:PricingSource .

figi-st:cmbs figi-gii:hasUniqueTextIdentifier "CMBS" .

figi-ps:BCMP skos:prefLabel "bloomberg composite" .

figi-ps:FCAP skos:prefLabel "first capital" .

figi-ps:ABSW a owl:NamedIndividual .

figi-ps:BCMP figi-gii:hasUniqueTextIdentifier "BCMP" .

figi-ps:ABSW a figi-gii:PricingSource .

figi-ps:FCAP figi-gii:hasUniqueTextIdentifier "FCAP" .

figi-ps:BCMR a owl:NamedIndividual .

figi-ps:ABSW skos:prefLabel "absa bank" .

figi-ps:FCB a owl:NamedIndividual .

figi-ps:BCMR a figi-gii:PricingSource .

figi-ps:FCB a figi-gii:PricingSource .

figi-ps:ABSW figi-gii:hasUniqueTextIdentifier "ABSW" .

figi-ps:BCMR skos:prefLabel "bancomer s.a. de c.v" .

figi-ps:FCB skos:prefLabel "icap sa matched" .

figi-st:cmdtFutWrt a owl:NamedIndividual .

figi-ps:BCMR skos:prefLabel "bbva bancomer" .

figi-ps:FCB figi-gii:hasUniqueTextIdentifier "FCB" .

figi-st:cmdtFutWrt a figi-gii:SecurityType .

figi-ps:BCMR figi-gii:hasUniqueTextIdentifier "BCMR" .

figi-ps:FCBT a owl:NamedIndividual .

figi-st:cmdtFutWrt skos:definition "Commodity Future Warrant - Indicates that the underlying is a commodity future." .

figi-ps:FCBT a figi-gii:PricingSource .

figi-ps:BCMS a owl:NamedIndividual .

figi-st:cmdtFutWrt skos:prefLabel "cmdt fut wrt" .

figi-ps:FCBT skos:prefLabel "first citizens bank" .

figi-ps:BCMS a figi-gii:PricingSource .

figi-st:cmdtFutWrt figi-gii:hasUniqueTextIdentifier "Cmdt Fut WRT" .

figi-ps:FCBT figi-gii:hasUniqueTextIdentifier "FCBT" .

figi-ps:BCMS skos:prefLabel "colombia exc serial" .

figi-ps:ABSX a owl:NamedIndividual .

figi-ps:FCIB a owl:NamedIndividual .

figi-ps:BCMS figi-gii:hasUniqueTextIdentifier "BCMS" .

figi-ps:FCIB a figi-gii:PricingSource .

figi-ps:ABSX a figi-gii:PricingSource .

figi-ps:BCMX a owl:NamedIndividual .

figi-ps:FCIB skos:prefLabel "first caribbean intl" .

figi-ps:ABSX skos:prefLabel "hvb" .

figi-ps:BCMX a figi-gii:PricingSource .

figi-ps:FCIB figi-gii:hasUniqueTextIdentifier "FCIB" .

figi-ps:ABSX figi-gii:hasUniqueTextIdentifier "ABSX" .

figi-ps:BCMX skos:prefLabel "bancomer toms" .

figi-ps:FCML a owl:NamedIndividual .

figi-st:cmdtIdxWrt a owl:NamedIndividual .

figi-ps:BCMX figi-gii:hasUniqueTextIdentifier "BCMX" .

figi-st:cmdtIdxWrt a figi-gii:SecurityType .

figi-ps:FCML a figi-gii:PricingSource .

figi-ps:BCMZ a owl:NamedIndividual .

figi-ps:FCML skos:prefLabel "first capital mgt" .

figi-ps:BCMZ a figi-gii:PricingSource .

figi-ps:FCML figi-gii:hasUniqueTextIdentifier "FCML" .

figi-st:cmdtIdxWrt skos:definition "Commodity Index Warrant - Indicates that the underlying is a commodity index" .

figi-ps:BCMZ skos:prefLabel "bbva bancomer" .

figi-ps:FCMT a owl:NamedIndividual .

figi-st:cmdtIdxWrt skos:prefLabel "cmdt idx wrt" .

figi-ps:BCMZ figi-gii:hasUniqueTextIdentifier "BCMZ" .

figi-ps:FCMT a figi-gii:PricingSource .

figi-st:cmdtIdxWrt figi-gii:hasUniqueTextIdentifier "Cmdt Idx WRT" .

figi-ps:FCMT skos:prefLabel "fidelity capital mkt" .

figi-ps:BCNT a owl:NamedIndividual .

figi-ps:ABVN a owl:NamedIndividual .

figi-ps:FCMT figi-gii:hasUniqueTextIdentifier "FCMT" .

figi-ps:ABVN a figi-gii:PricingSource .

figi-ps:FCPT a owl:NamedIndividual .

figi-ps:BCNT a figi-gii:PricingSource .

figi-ps:FCPT a figi-gii:PricingSource .

figi-ps:ABVN skos:prefLabel "agri bk of vietnam" .

figi-ps:FCPT skos:prefLabel "first capital t" .

figi-ps:BCNT skos:prefLabel "biofuelsconnect" .

figi-ps:ABVN figi-gii:hasUniqueTextIdentifier "ABVN" .

figi-ps:FCPT figi-gii:hasUniqueTextIdentifier "FCPT" .

figi-ps:BCNT figi-gii:hasUniqueTextIdentifier "BCNT" .

figi-st:collatCallNote a owl:NamedIndividual .

figi-ps:FCRP a owl:NamedIndividual .

figi-ps:BCNV a owl:NamedIndividual .

figi-st:collatCallNote a figi-gii:SecurityType .

figi-ps:FCRP a figi-gii:PricingSource .

figi-ps:BCNV a figi-gii:PricingSource .

figi-st:collatCallNote skos:definition "Collateralized Call Notes" .

figi-ps:FCRP skos:prefLabel "financorp, san jose" .

figi-ps:BCNV skos:prefLabel "barclays capital inc" .

figi-st:collatCallNote skos:prefLabel "collat call note" .

figi-ps:FCRP figi-gii:hasUniqueTextIdentifier "FCRP" .

figi-ps:BCNV figi-gii:hasUniqueTextIdentifier "BCNV" .

figi-st:collatCallNote figi-gii:hasUniqueTextIdentifier "COLLAT CALL NOTE" .

figi-ps:FDCM a owl:NamedIndividual .

figi-ps:BCOB a owl:NamedIndividual .

figi-ps:ABYM a owl:NamedIndividual .

figi-ps:BCOB a figi-gii:PricingSource .

figi-ps:ABYM a figi-gii:PricingSource .

figi-ps:BCOB skos:prefLabel "barclays internal" .

figi-ps:FDCM a figi-gii:PricingSource .

figi-ps:ABYM skos:prefLabel "abn amro yield" .

figi-ps:BCOB figi-gii:hasUniqueTextIdentifier "BCOB" .

figi-ps:FDCM skos:prefLabel "fundamental cap mkts" .

figi-ps:ABYM figi-gii:hasUniqueTextIdentifier "ABYM" .

figi-ps:FDCM figi-gii:hasUniqueTextIdentifier "FDCM" .

figi-ps:BCOF a owl:NamedIndividual .

figi-st:commercialNote a owl:NamedIndividual .

figi-ps:FDR a owl:NamedIndividual .

figi-ps:BCOF a figi-gii:PricingSource .

figi-st:commercialNote a figi-gii:SecurityType .

figi-ps:FDR a figi-gii:PricingSource .

figi-ps:BCOF skos:prefLabel "barclays assetbacked" .

figi-st:commercialNote skos:definition "Commercial Notes" .

figi-ps:BCOF figi-gii:hasUniqueTextIdentifier "BCOF" .

figi-ps:FDR skos:prefLabel "fideuram" .

figi-st:commercialNote skos:prefLabel "commercial note" .

figi-ps:FDR figi-gii:hasUniqueTextIdentifier "FDR" .

figi-ps:BCOH a owl:NamedIndividual .

figi-st:commercialNote figi-gii:hasUniqueTextIdentifier "COMMERCIAL NOTE" .

figi-ps:BCOH a figi-gii:PricingSource .

figi-ps:FEDB a owl:NamedIndividual .

figi-ps:ABYQ a owl:NamedIndividual .

figi-ps:FEDB a figi-gii:PricingSource .

figi-ps:BCOH skos:prefLabel "bank of comm, china" .

figi-ps:ABYQ a figi-gii:PricingSource .

figi-ps:FEDB skos:prefLabel "federal bank" .

figi-ps:BCOH figi-gii:hasUniqueTextIdentifier "BCOH" .

figi-ps:ABYQ skos:prefLabel "abn amro yld quoted" .

figi-ps:FEDB figi-gii:hasUniqueTextIdentifier "FEDB" .

figi-ps:BCOM a owl:NamedIndividual .

figi-ps:ABYQ figi-gii:hasUniqueTextIdentifier "ABYQ" .

figi-ps:BCOM a figi-gii:PricingSource .

figi-ps:FEDE a owl:NamedIndividual .

figi-st:commercialPaper a owl:NamedIndividual .

figi-ps:FEDE a figi-gii:PricingSource .

figi-ps:BCOM skos:prefLabel "bank of comm 11:30" .

figi-st:commercialPaper a figi-gii:SecurityType .

figi-ps:FEDE skos:prefLabel "federated investors" .

figi-ps:BCOM figi-gii:hasUniqueTextIdentifier "BCOM" .

figi-ps:FEDE figi-gii:hasUniqueTextIdentifier "FEDE" .

figi-st:commercialPaper skos:definition "An unsecured short-term promise to repay a fixed amount on a certain future date. Commercial paper usually matures from 2 to 270 days and is traded on a discount basis. This debt instrument, issued by banks, companies and other borrowers, use only their credit ratings to back the security." .

figi-ps:FEFO a owl:NamedIndividual .

figi-ps:BCON a owl:NamedIndividual .

figi-st:commercialPaper skos:prefLabel "commercial paper" .

figi-ps:FEFO a figi-gii:PricingSource .

figi-ps:BCON a figi-gii:PricingSource .

figi-st:commercialPaper figi-gii:hasUniqueTextIdentifier "COMMERCIAL PAPER" .

figi-ps:FEFO skos:prefLabel "fearnley fonds as" .

figi-ps:BCON skos:prefLabel "bbv banco continent" .

figi-ps:ABYT a owl:NamedIndividual .

figi-ps:BCON figi-gii:hasUniqueTextIdentifier "BCON" .

figi-ps:FEFO figi-gii:hasUniqueTextIdentifier "FEFO" .

figi-ps:ABYT a figi-gii:PricingSource .

figi-ps:BCOP a owl:NamedIndividual .

figi-ps:FENI a owl:NamedIndividual .

figi-ps:ABYT skos:prefLabel "abn amro yield test" .

figi-ps:BCOP a figi-gii:PricingSource .

figi-ps:FENI a figi-gii:PricingSource .

figi-ps:ABYT figi-gii:hasUniqueTextIdentifier "ABYT" .

figi-ps:BCOP skos:prefLabel "bloomberg corp bond" .

figi-ps:FENI skos:prefLabel "fenice investimenti" .

figi-st:commonStock a owl:NamedIndividual .

figi-ps:BCOP figi-gii:hasUniqueTextIdentifier "BCOP" .

figi-ps:FENI figi-gii:hasUniqueTextIdentifier "FENI" .

figi-st:commonStock a figi-gii:SecurityType .

figi-ps:BCOR a owl:NamedIndividual .

figi-ps:FERL a owl:NamedIndividual .

figi-ps:BCOR a figi-gii:PricingSource .

figi-ps:FERL a figi-gii:PricingSource .

figi-ps:BCOR skos:prefLabel "banc of america bcor" .

figi-ps:FERL skos:prefLabel "fernandez laya sa" ;
	figi-gii:hasUniqueTextIdentifier "FERL" .

figi-ps:BCOR figi-gii:hasUniqueTextIdentifier "BCOR" .

figi-st:commonStock skos:definition "Common Stock. A unit of ownership in a public company for which the holder can vote on corporate matters and receive dividends fromthe company's growth. If the company is liquidated the claims of secured and unsecured creditors, bondholders and preferred stockholders take precedence over common stock holders. However, common stock has more potential for appreciation." .

figi-ps:FESB a owl:NamedIndividual .

figi-ps:BCP a owl:NamedIndividual .

figi-ps:FESB a figi-gii:PricingSource .

figi-st:commonStock skos:prefLabel "common stock" .

figi-ps:BCP a figi-gii:PricingSource .

figi-ps:FESB skos:prefLabel "forex berhad" .

figi-st:commonStock figi-gii:hasUniqueTextIdentifier "Common Stock" .

figi-ps:BCP skos:prefLabel "banco credito peru" .

figi-ps:FESB figi-gii:hasUniqueTextIdentifier "FESB" .

figi-ps:AC a owl:NamedIndividual .

figi-ps:BCP figi-gii:hasUniqueTextIdentifier "BCP" .

figi-ps:FESI a owl:NamedIndividual .

figi-ps:AC a figi-gii:PricingSource .

figi-ps:FESI a figi-gii:PricingSource .

figi-ps:BCPC a owl:NamedIndividual .

figi-ps:AC skos:prefLabel "air canada pension" .

figi-ps:FESI skos:prefLabel "first empire secs." .

figi-ps:BCPC a figi-gii:PricingSource .

figi-ps:AC figi-gii:hasUniqueTextIdentifier "AC" .

figi-ps:FESI figi-gii:hasUniqueTextIdentifier "FESI" .

figi-st:contractForDifference a owl:NamedIndividual , figi-gii:SecurityType .

figi-ps:BCPC skos:prefLabel "bcp securities llc" .

figi-ps:FFFF a owl:NamedIndividual .

figi-ps:BCPC figi-gii:hasUniqueTextIdentifier "BCPC" .

figi-ps:FFFF a figi-gii:PricingSource .

figi-ps:BCPG a owl:NamedIndividual .

figi-ps:FFFF skos:prefLabel "bad install on 342" .

figi-ps:BCPG a figi-gii:PricingSource .

figi-ps:FFFF figi-gii:hasUniqueTextIdentifier "FFFF" .

figi-ps:BCPG skos:prefLabel "bcp geneva" .

figi-st:contractForDifference skos:definition "Contract For Difference. An arrangement made in a futures contract whereby differences in settlement are made through cash payments, rather than the delivery of physical goods or securities." .

figi-ps:FG a owl:NamedIndividual .

figi-st:contractForDifference skos:prefLabel "contract for difference" .

figi-ps:FG a figi-gii:PricingSource .

figi-st:contractForDifference figi-gii:hasUniqueTextIdentifier "CONTRACT FOR DIFFERENCE" .

figi-ps:FG skos:prefLabel "fullgoal fund mgmt" .

figi-ps:ACAP a owl:NamedIndividual .

figi-ps:FG figi-gii:hasUniqueTextIdentifier "FG" .

figi-ps:ACAP a figi-gii:PricingSource ;
	skos:prefLabel "aladdin capital llc" ;
	figi-gii:hasUniqueTextIdentifier "ACAP" .

figi-st:contractFra a owl:NamedIndividual , figi-gii:SecurityType ;
	skos:definition "IMM FRAs, FRAs where the payment dates align with Eurodollar future contracts' expiration date" ;
	skos:prefLabel "contract fra" ;
	figi-gii:hasUniqueTextIdentifier "CONTRACT FRA" .

figi-ps:ACAV a owl:NamedIndividual , figi-gii:PricingSource ;
	skos:prefLabel "aca sa agencia valor" .

figi-ps:BCPG figi-gii:hasUniqueTextIdentifier "BCPG" .

figi-ps:FGCB a owl:NamedIndividual .

figi-ps:BCPL a owl:NamedIndividual , figi-gii:PricingSource ;
	skos:prefLabel "bcp securities" .

figi-ps:FGCB a figi-gii:PricingSource .

figi-ps:BCPL figi-gii:hasUniqueTextIdentifier "BCPL" .

figi-ps:FGCB skos:prefLabel "first global bank" .

figi-ps:BCPS a owl:NamedIndividual .

figi-ps:FGCB figi-gii:hasUniqueTextIdentifier "FGCB" .

figi-ps:BCPS a figi-gii:PricingSource .

figi-ps:ACAV figi-gii:hasUniqueTextIdentifier "ACAV" .

figi-ps:BCPS skos:prefLabel "bcp securities" .

figi-ps:FGCS a owl:NamedIndividual .

figi-ps:BCPS figi-gii:hasUniqueTextIdentifier "BCPS" .

figi-st:convBond a owl:NamedIndividual .

figi-ps:FGCS a figi-gii:PricingSource .

figi-ps:BCPT a owl:NamedIndividual .

figi-st:convBond a figi-gii:SecurityType .

figi-ps:FGCS skos:prefLabel "fgc securities llc" .

figi-ps:BCPT a figi-gii:PricingSource .

figi-ps:FGCS figi-gii:hasUniqueTextIdentifier "FGCS" .

figi-st:convBond skos:definition "Convertible Bond. A bond containing a provision that permits conversion to the issuer's common stock at some fixed exchange ratio." .

figi-ps:FGIC a owl:NamedIndividual .

figi-ps:BCPT skos:prefLabel "bcp securities, llc" .

figi-st:convBond skos:prefLabel "conv bond" .

figi-ps:FGIC a figi-gii:PricingSource .

figi-ps:BCPT figi-gii:hasUniqueTextIdentifier "BCPT" .

figi-st:convBond figi-gii:hasUniqueTextIdentifier "Conv Bond" .

figi-ps:BCPX a owl:NamedIndividual .

figi-ps:ACBS a owl:NamedIndividual .

figi-ps:BCPX a figi-gii:PricingSource .

figi-ps:ACBS a figi-gii:PricingSource .

figi-ps:FGIC skos:prefLabel "financial guaranty" .

figi-ps:BCPX skos:prefLabel "barclays inside1" .

figi-ps:FGIC figi-gii:hasUniqueTextIdentifier "FGIC" .

figi-ps:BCPX figi-gii:hasUniqueTextIdentifier "BCPX" .

figi-ps:FGSN a owl:NamedIndividual .

figi-ps:BCRD a owl:NamedIndividual .

figi-ps:FGSN a figi-gii:PricingSource .

figi-ps:BCRD a figi-gii:PricingSource .

figi-ps:ACBS skos:prefLabel "acb securities ltd" ;
	figi-gii:hasUniqueTextIdentifier "ACBS" .

figi-ps:FGSN skos:prefLabel "fagenson and co., inc" ;
	figi-gii:hasUniqueTextIdentifier "FGSN" .

figi-ps:FHBC a owl:NamedIndividual .

figi-ps:BCRD skos:prefLabel "banco central domrep" .

figi-st:convPrfd a owl:NamedIndividual .

figi-ps:FHBC a figi-gii:PricingSource .

figi-ps:BCRD figi-gii:hasUniqueTextIdentifier "BCRD" .

figi-st:convPrfd a figi-gii:SecurityType .

figi-ps:FHBC skos:prefLabel "fhb commercial bank" .

figi-ps:BCRI a owl:NamedIndividual .

figi-ps:FHBC figi-gii:hasUniqueTextIdentifier "FHBC" .

figi-ps:BCRI a figi-gii:PricingSource .

figi-st:convPrfd skos:definition "Convertible Preferred Stock. Preferred stock that includes an option for the holder to convert the preferred shares into a fixed number of common shares, usually anytime after a predetermined date." .

figi-ps:FIAA a owl:NamedIndividual .

figi-ps:BCRI skos:prefLabel "bank amer intrinsic" .

figi-st:convPrfd skos:prefLabel "conv prfd" .

figi-ps:FIAA a figi-gii:PricingSource .

figi-ps:BCRI figi-gii:hasUniqueTextIdentifier "BCRI" .

figi-st:convPrfd figi-gii:hasUniqueTextIdentifier "Conv Prfd" .

figi-ps:FIAA skos:prefLabel "abn kuala lumpur" .

figi-ps:BCRR a owl:NamedIndividual .

figi-ps:ACBV a owl:NamedIndividual .

figi-ps:FIAA figi-gii:hasUniqueTextIdentifier "FIAA" .

figi-ps:ACBV a figi-gii:PricingSource .

figi-ps:BCRR a figi-gii:PricingSource .

figi-ps:FIB a owl:NamedIndividual .

figi-ps:ACBV skos:prefLabel "asia commercial bank" .

figi-ps:FIB a figi-gii:PricingSource .

figi-ps:BCRR skos:prefLabel "banca intesa zao" .

figi-ps:ACBV figi-gii:hasUniqueTextIdentifier "ACBV" .

figi-ps:FIB skos:prefLabel "first independent bk" .

figi-ps:BCRR figi-gii:hasUniqueTextIdentifier "BCRR" .

figi-st:corpBndWrt a owl:NamedIndividual .

figi-ps:FIB figi-gii:hasUniqueTextIdentifier "FIB" .

figi-st:corpBndWrt a figi-gii:SecurityType .

figi-ps:BCRV a owl:NamedIndividual .

figi-ps:FIBK a owl:NamedIndividual .

figi-ps:BCRV a figi-gii:PricingSource .

figi-st:corpBndWrt skos:definition "Corporate Bond Warrant - Indicates that the underlying is a corporate bond" .

figi-ps:FIBK a figi-gii:PricingSource .

figi-ps:BCRV skos:prefLabel "banco de costa rica" .

figi-st:corpBndWrt skos:prefLabel "corp bnd wrt" .

figi-ps:FIBK skos:prefLabel "fibank" .

figi-ps:BCRV figi-gii:hasUniqueTextIdentifier "BCRV" .

figi-st:corpBndWrt figi-gii:hasUniqueTextIdentifier "Corp Bnd WRT" .

figi-ps:FIBK figi-gii:hasUniqueTextIdentifier "FIBK" .

figi-ps:BCSA a owl:NamedIndividual .

figi-ps:ACCB a owl:NamedIndividual .

figi-ps:FICU a owl:NamedIndividual .

figi-ps:BCSA a figi-gii:PricingSource .

figi-ps:ACCB a figi-gii:PricingSource .

figi-ps:FICU a figi-gii:PricingSource .

figi-ps:BCSA skos:prefLabel "barclays capital sa" .

figi-ps:ACCB skos:prefLabel "access bank" .

figi-ps:FICU skos:prefLabel "ficus capital" .

figi-ps:BCSA figi-gii:hasUniqueTextIdentifier "BCSA" .

figi-ps:ACCB figi-gii:hasUniqueTextIdentifier "ACCB" .

figi-ps:FICU figi-gii:hasUniqueTextIdentifier "FICU" .

figi-ps:BCSB a owl:NamedIndividual .

figi-st:cpLikeExtNote a owl:NamedIndividual .

figi-ps:FIDO a owl:NamedIndividual .

figi-st:cpLikeExtNote a figi-gii:SecurityType .

figi-ps:BCSB a figi-gii:PricingSource .

figi-ps:FIDO a figi-gii:PricingSource .

figi-st:cpLikeExtNote skos:definition "Extendible Notes issues off of Commercial Paper program prospectus" .

figi-ps:FIDO skos:prefLabel "fidelity mgmt" .

figi-ps:BCSB skos:prefLabel "barclays cap grp" .

figi-st:cpLikeExtNote skos:prefLabel "cp-like ext note" .

figi-ps:FIDO figi-gii:hasUniqueTextIdentifier "FIDO" .

figi-ps:BCSB figi-gii:hasUniqueTextIdentifier "BCSB" .

figi-st:cpLikeExtNote figi-gii:hasUniqueTextIdentifier "CP-LIKE EXT NOTE" .

figi-ps:FIET a owl:NamedIndividual .

figi-ps:BCSF a owl:NamedIndividual .

figi-ps:ACCR a owl:NamedIndividual .

figi-ps:FIET a figi-gii:PricingSource .

figi-ps:BCSF a figi-gii:PricingSource .

figi-ps:ACCR a figi-gii:PricingSource .

figi-ps:FIET skos:prefLabel "auto ex testing" .

figi-ps:BCSF skos:prefLabel "bocom schroder fm" .

figi-ps:ACCR skos:prefLabel "accionaria realtim" .

figi-ps:FIET figi-gii:hasUniqueTextIdentifier "FIET" .

figi-ps:ACCR figi-gii:hasUniqueTextIdentifier "ACCR" .

figi-ps:BCSF figi-gii:hasUniqueTextIdentifier "BCSF" .

figi-ps:FIGP a owl:NamedIndividual .

figi-ps:ACFB a owl:NamedIndividual .

figi-ps:BCSG a owl:NamedIndividual .

figi-ps:FIGP a figi-gii:PricingSource .

figi-ps:ACFB a figi-gii:PricingSource .

figi-ps:BCSG a figi-gii:PricingSource .

figi-ps:FIGP skos:prefLabel "first international" .

figi-ps:ACFB skos:prefLabel "ahorro corporacion" .

figi-ps:BCSG skos:prefLabel "barclays bank plc" .

figi-ps:FIGP figi-gii:hasUniqueTextIdentifier "FIGP" .

figi-ps:ACFB skos:prefLabel "ahorro corporation" .

figi-ps:BCSG figi-gii:hasUniqueTextIdentifier "BCSG" .

figi-ps:FIMD a owl:NamedIndividual .

figi-ps:ACFB figi-gii:hasUniqueTextIdentifier "ACFB" .

figi-ps:BCSP a owl:NamedIndividual .

figi-ps:FIMD a figi-gii:PricingSource .

figi-ps:BCSP a figi-gii:PricingSource .

figi-st:cpiLinked a owl:NamedIndividual .

figi-ps:FIMD skos:prefLabel "fixed in m-mkt dlrs" .

figi-ps:BCSP skos:prefLabel "barclays capital gcd" .

figi-st:cpiLinked a figi-gii:SecurityType .

figi-ps:FIMD figi-gii:hasUniqueTextIdentifier "FIMD" .

figi-ps:BCSP figi-gii:hasUniqueTextIdentifier "BCSP" .

figi-st:cpiLinked skos:definition "A special type of floating rate bond that is linked to the Consumer Price Index (CPI)" .

figi-ps:BCSR a owl:NamedIndividual .

figi-ps:FIME a owl:NamedIndividual .

figi-st:cpiLinked skos:prefLabel "cpi linked" .

figi-ps:FIME a figi-gii:PricingSource .

figi-st:cpiLinked figi-gii:hasUniqueTextIdentifier "CPI LINKED" .

figi-ps:FIME skos:prefLabel "fimat united states" .

figi-ps:ACIB a owl:NamedIndividual .

figi-ps:FIME figi-gii:hasUniqueTextIdentifier "FIME" .

figi-ps:BCSR a figi-gii:PricingSource .

figi-ps:FIMZ a owl:NamedIndividual .

figi-ps:BCSR skos:prefLabel "bkr credit services" .

figi-ps:ACIB a figi-gii:PricingSource .

figi-ps:FIMZ a figi-gii:PricingSource .

figi-ps:BCSR figi-gii:hasUniqueTextIdentifier "BCSR" .

figi-ps:ACIB skos:prefLabel "asociacion cibao" .

figi-ps:FIMZ skos:prefLabel "fi mmkt and der assc" .

figi-ps:BCSY a owl:NamedIndividual .

figi-ps:ACIB figi-gii:hasUniqueTextIdentifier "ACIB" .

figi-ps:FIMZ figi-gii:hasUniqueTextIdentifier "FIMZ" .

figi-ps:BCSY a figi-gii:PricingSource .

figi-st:cpiLinkedOid a owl:NamedIndividual .

figi-ps:FINA a owl:NamedIndividual .

figi-ps:BCSY skos:prefLabel "bvc mec sobre lote" .

figi-ps:FINA a figi-gii:PricingSource .

figi-st:cpiLinkedOid a figi-gii:SecurityType .

figi-ps:BCSY figi-gii:hasUniqueTextIdentifier "BCSY" .

figi-ps:FINA skos:prefLabel "finacorp securities" ;
	figi-gii:hasUniqueTextIdentifier "FINA" .

figi-ps:BCTI a owl:NamedIndividual .

figi-st:cpiLinkedOid skos:definition "A special type of floating rate bond that is linked to the Consumer Price Index (CPI). The security is an Original Issue Discount." .

figi-ps:FINB a owl:NamedIndividual .

figi-ps:BCTI a figi-gii:PricingSource .

figi-ps:FINB a figi-gii:PricingSource .

figi-st:cpiLinkedOid skos:prefLabel "cpi linked, oid" .

figi-ps:BCTI skos:prefLabel "bank chinatrust" .

figi-ps:FINB skos:prefLabel "finansbank" .

figi-st:cpiLinkedOid figi-gii:hasUniqueTextIdentifier "CPI LINKED, OID" .

figi-ps:BCTI figi-gii:hasUniqueTextIdentifier "BCTI" .

figi-ps:FINB figi-gii:hasUniqueTextIdentifier "FINB" .

figi-ps:ACIL a owl:NamedIndividual .

figi-ps:BCTK a owl:NamedIndividual .

figi-ps:FINR a owl:NamedIndividual .

figi-ps:BCTK a figi-gii:PricingSource .

figi-ps:FINR a figi-gii:PricingSource .

figi-ps:BCTK skos:prefLabel "barclays cap tokyo" .

figi-ps:ACIL a figi-gii:PricingSource .

figi-ps:BCTK skos:prefLabel "barclays cap. tokyo" .

figi-ps:FINR skos:prefLabel "finam investment co" .

figi-ps:BCTK figi-gii:hasUniqueTextIdentifier "BCTK" .

figi-ps:ACIL skos:prefLabel "agri commodities" .

figi-ps:BCTS a owl:NamedIndividual .

figi-ps:ACIL figi-gii:hasUniqueTextIdentifier "ACIL" .

figi-ps:BCTS a figi-gii:PricingSource .

figi-st:creditDefaultSwap a owl:NamedIndividual .

figi-ps:BCTS skos:prefLabel "barclays book" .

figi-ps:FINR figi-gii:hasUniqueTextIdentifier "FINR" .

figi-st:creditDefaultSwap a figi-gii:SecurityType .

figi-ps:BCTS figi-gii:hasUniqueTextIdentifier "BCTS" .

figi-ps:FINX a owl:NamedIndividual .

figi-ps:BCTT a owl:NamedIndividual .

figi-ps:FINX a figi-gii:PricingSource .

figi-ps:BCTT a figi-gii:PricingSource .

figi-ps:FINX skos:prefLabel "finex securities" .

figi-ps:BCTT skos:prefLabel "barcap actives" .

figi-st:creditDefaultSwap skos:definition "A credit derivative transaction in which two parties enter into an agreement, whereby one party pays the other a fixed periodic coupon for the specified life of the agreement. The other party makes no payments unless a credit event, relating to a predetermined reference asset, occurs. If such an event occurs, the party will then make a payment to the first party, and the swap will terminate." .

figi-ps:BCTT figi-gii:hasUniqueTextIdentifier "BCTT" .

figi-ps:FINX figi-gii:hasUniqueTextIdentifier "FINX" .

figi-st:creditDefaultSwap skos:prefLabel "credit default swap" .

figi-ps:BCTX a owl:NamedIndividual .

figi-ps:FISB a owl:NamedIndividual .

figi-ps:BCTX a figi-gii:PricingSource .

figi-st:creditDefaultSwap figi-gii:hasUniqueTextIdentifier "CREDIT DEFAULT SWAP" .

figi-ps:FISB a figi-gii:PricingSource .

figi-ps:BCTX skos:prefLabel "barc-tradeable axes" .

figi-ps:ACIM a owl:NamedIndividual .

figi-ps:FISB skos:prefLabel "fixed income sec" .

figi-ps:BCTX figi-gii:hasUniqueTextIdentifier "BCTX" .

figi-ps:ACIM a figi-gii:PricingSource .

figi-ps:FISB figi-gii:hasUniqueTextIdentifier "FISB" .

figi-ps:BCUS a owl:NamedIndividual .

figi-ps:ACIM skos:prefLabel "american century inv" .

figi-ps:BCUS a figi-gii:PricingSource .

figi-ps:FITB a owl:NamedIndividual .

figi-ps:ACIM figi-gii:hasUniqueTextIdentifier "ACIM" .

figi-ps:BCUS skos:prefLabel "bcba cont us" .

figi-ps:FITB a figi-gii:PricingSource .

figi-st:cross a owl:NamedIndividual .

figi-ps:BCUS figi-gii:hasUniqueTextIdentifier "BCUS" .

figi-st:cross a figi-gii:SecurityType .

figi-ps:FITB skos:prefLabel "fifth third secs" .

figi-ps:BCV a owl:NamedIndividual .

figi-st:cross skos:definition "Cross-rate: Currency against any other currency except US Dollar, eg EURCAD" .

figi-ps:BCV a figi-gii:PricingSource .

figi-ps:FITB figi-gii:hasUniqueTextIdentifier "FITB" .

figi-st:cross skos:prefLabel "cross" .

figi-ps:BCV skos:prefLabel "banco central de ven" .

figi-ps:FITQ a owl:NamedIndividual .

figi-st:cross figi-gii:hasUniqueTextIdentifier "CROSS" .

figi-ps:BCV figi-gii:hasUniqueTextIdentifier "BCV" .

figi-ps:FITQ a figi-gii:PricingSource .

figi-ps:ACLD a owl:NamedIndividual .

figi-ps:BCVA a owl:NamedIndividual .

figi-ps:FITQ skos:prefLabel "fit qa" .

figi-ps:ACLD a figi-gii:PricingSource .

figi-ps:BCVA a figi-gii:PricingSource .

figi-ps:FITQ figi-gii:hasUniqueTextIdentifier "FITQ" .

figi-ps:ACLD skos:prefLabel "arqaam capital" .

figi-ps:BCVA skos:prefLabel "cb venezuela highest" .

figi-ps:FIX a owl:NamedIndividual .

figi-ps:ACLD figi-gii:hasUniqueTextIdentifier "ACLD" .

figi-ps:BCVA figi-gii:hasUniqueTextIdentifier "BCVA" .

figi-ps:FIX a figi-gii:PricingSource .

figi-st:currencyFuture a owl:NamedIndividual .

figi-ps:BCVB a owl:NamedIndividual .

figi-ps:FIX skos:prefLabel "global fixing" .

figi-st:currencyFuture a figi-gii:SecurityType .

figi-ps:BCVB a figi-gii:PricingSource .

figi-ps:FIX figi-gii:hasUniqueTextIdentifier "FIX" .

figi-ps:BCVB skos:prefLabel "bcv" .

figi-ps:FIX1 a owl:NamedIndividual .

figi-ps:BCVB figi-gii:hasUniqueTextIdentifier "BCVB" .

figi-ps:FIX1 a figi-gii:PricingSource .

figi-ps:BCVE a owl:NamedIndividual .

figi-ps:FIX1 skos:prefLabel "fix cert 1" .

figi-ps:BCVE a figi-gii:PricingSource .

figi-ps:FIX1 figi-gii:hasUniqueTextIdentifier "FIX1" .

figi-ps:BCVE skos:prefLabel "cntrl bnk venezuela" ;
	figi-gii:hasUniqueTextIdentifier "BCVE" .

figi-ps:FIX3 a owl:NamedIndividual .

figi-ps:BCVI a owl:NamedIndividual .

figi-st:currencyFuture skos:definition "Currency Futures. Futures contracts on major currencies (e.g., the British pound, the German mark and the U.S. dollar) that are held by companies doing worldwide business in an effort to reduce their risks by hedging the value of their home country's currency." .

figi-ps:BCVI a figi-gii:PricingSource .

figi-st:currencyFuture skos:prefLabel "currency future." .

figi-ps:BCVI skos:prefLabel "cb venezuela lowest" .

figi-ps:FIX3 a figi-gii:PricingSource .

figi-st:currencyFuture figi-gii:hasUniqueTextIdentifier "Currency future." .

figi-ps:FIX3 skos:prefLabel "fix cert 3" .

figi-ps:ACM a owl:NamedIndividual .

figi-ps:BCVI figi-gii:hasUniqueTextIdentifier "BCVI" .

figi-ps:FIX3 figi-gii:hasUniqueTextIdentifier "FIX3" .

figi-ps:ACM a figi-gii:PricingSource .

figi-ps:BCVS a owl:NamedIndividual .

figi-ps:FLAH a owl:NamedIndividual .

figi-ps:ACM skos:prefLabel "artesian cptl mgmt" .

figi-ps:FLAH a figi-gii:PricingSource .

figi-ps:ACM figi-gii:hasUniqueTextIdentifier "ACM" .

figi-ps:FLAH skos:prefLabel "bank al-falah ltd" .

figi-ps:BCVS a figi-gii:PricingSource .

figi-st:currencyOption a owl:NamedIndividual .

figi-ps:FLAH figi-gii:hasUniqueTextIdentifier "FLAH" .

figi-st:currencyOption a figi-gii:SecurityType .

figi-ps:BCVS skos:prefLabel "banque cantonale vau" .

figi-ps:FLAR a owl:NamedIndividual .

figi-ps:BCVS figi-gii:hasUniqueTextIdentifier "BCVS" .

figi-ps:FLAR a figi-gii:PricingSource ;
	skos:prefLabel "flar" .

figi-ps:BCVZ a owl:NamedIndividual .

figi-ps:FLAR figi-gii:hasUniqueTextIdentifier "FLAR" .

figi-st:currencyOption skos:definition "Option. A contract that provides the right, but not the obligation, to buy or sell a specific amount of a specific security within a predetermined time period. A call option provides the right to buy 100 shares of the underlying security. A put option provides the right to sell 100 shares of the underlying security. The seller of the contracts is called the writer. Bloomberg abbreviates option as OPT." .

figi-ps:FLOW a owl:NamedIndividual , figi-gii:PricingSource .

figi-st:currencyOption skos:prefLabel "currency option." .

figi-ps:FLOW skos:prefLabel "internal do not del" .

figi-st:currencyOption figi-gii:hasUniqueTextIdentifier "Currency option." .

figi-ps:FLOW figi-gii:hasUniqueTextIdentifier "FLOW" .

figi-ps:BCVZ a figi-gii:PricingSource .

figi-ps:ACMI a owl:NamedIndividual .

figi-ps:FLTL a owl:NamedIndividual .

figi-ps:ACMI a figi-gii:PricingSource .

figi-ps:BCVZ skos:prefLabel "banco confederado" .

figi-ps:FLTL a figi-gii:PricingSource .

figi-ps:ACMI skos:prefLabel "asit c mehta invest" .

figi-ps:BCVZ figi-gii:hasUniqueTextIdentifier "BCVZ" .

figi-ps:FLTL skos:prefLabel "feltl and co" .

figi-ps:ACMI figi-gii:hasUniqueTextIdentifier "ACMI" .

figi-ps:BCWB a owl:NamedIndividual .

figi-ps:FLTL figi-gii:hasUniqueTextIdentifier "FLTL" .

figi-ps:BCWB a figi-gii:PricingSource .

figi-st:currencySpot a owl:NamedIndividual .

figi-ps:FLTS a owl:NamedIndividual .

figi-ps:BCWB skos:prefLabel "barclays white board" .

figi-ps:FLTS a figi-gii:PricingSource .

figi-st:currencySpot a figi-gii:SecurityType .

figi-ps:BCWB figi-gii:hasUniqueTextIdentifier "BCWB" .

figi-ps:FLTS skos:prefLabel "flow traders bv" .

figi-st:currencySpot skos:definition "A currency transaction where one leg is the USD" .

figi-ps:BCWM a owl:NamedIndividual .

figi-ps:FLTS figi-gii:hasUniqueTextIdentifier "FLTS" .

figi-ps:BCWM a figi-gii:PricingSource .

figi-st:currencySpot skos:prefLabel "currency spot." .

figi-ps:FLTT a owl:NamedIndividual .

figi-ps:BCWM skos:prefLabel "barclays bank suisse" .

figi-ps:FLTT a figi-gii:PricingSource .

figi-ps:BCWM figi-gii:hasUniqueTextIdentifier "BCWM" .

figi-ps:FLTT skos:prefLabel "flett futures" .

figi-st:currencySpot figi-gii:hasUniqueTextIdentifier "Currency spot." .

figi-ps:FLTT figi-gii:hasUniqueTextIdentifier "FLTT" .

figi-ps:BDAT a owl:NamedIndividual .

figi-ps:ACMP a owl:NamedIndividual .

figi-ps:FMA a owl:NamedIndividual .

figi-ps:BDAT a figi-gii:PricingSource .

figi-ps:ACMP a figi-gii:PricingSource .

figi-ps:FMA a figi-gii:PricingSource .

figi-ps:BDAT skos:prefLabel "banco de oro trust" .

figi-ps:ACMP skos:prefLabel "advent capital ny" .

figi-ps:FMA skos:prefLabel "first western" .

figi-ps:BDAT figi-gii:hasUniqueTextIdentifier "BDAT" .

figi-ps:ACMP figi-gii:hasUniqueTextIdentifier "ACMP" .

figi-ps:FMA figi-gii:hasUniqueTextIdentifier "FMA" .

figi-ps:BDCH a owl:NamedIndividual .

figi-ps:ACOB a owl:NamedIndividual .

figi-ps:FMDQ a owl:NamedIndividual .

figi-ps:ACOB a figi-gii:PricingSource .

figi-ps:FMDQ a figi-gii:PricingSource .

figi-ps:ACOB skos:prefLabel "acobo" .

figi-ps:BDCH a figi-gii:PricingSource .

figi-ps:ACOB figi-gii:hasUniqueTextIdentifier "ACOB" .

figi-ps:FMDQ skos:prefLabel "financial mrkt dl q" .

figi-st:currencyWrt a owl:NamedIndividual .

figi-ps:BDCH skos:prefLabel "banco de chile" .

figi-st:currencyWrt a figi-gii:SecurityType .

figi-ps:FMDQ figi-gii:hasUniqueTextIdentifier "FMDQ" .

figi-ps:BDCH figi-gii:hasUniqueTextIdentifier "BDCH" .

figi-st:currencyWrt skos:definition "Currency Warrant - Indicates that the underlying is a currency" .

figi-ps:FMEX a owl:NamedIndividual .

figi-st:currencyWrt skos:prefLabel "currency wrt" .

figi-ps:BDEG a owl:NamedIndividual .

figi-ps:FMEX a figi-gii:PricingSource .

figi-st:currencyWrt figi-gii:hasUniqueTextIdentifier "Currency WRT" .

figi-ps:BDEG a figi-gii:PricingSource .

figi-ps:FMEX skos:prefLabel "finamex" .

figi-ps:ACOF a owl:NamedIndividual .

figi-ps:BDEG skos:prefLabel "banque degroof (lux)" .

figi-ps:ACOF a figi-gii:PricingSource .

figi-ps:FMEX figi-gii:hasUniqueTextIdentifier "FMEX" .

figi-ps:ACOF skos:prefLabel "afp confia" .

figi-ps:BDEG figi-gii:hasUniqueTextIdentifier "BDEG" .

figi-ps:ACOF figi-gii:hasUniqueTextIdentifier "ACOF" .

figi-ps:FMI a owl:NamedIndividual .

figi-ps:BDF a owl:NamedIndividual .

figi-ps:FMI a figi-gii:PricingSource .

figi-ps:ACON a owl:NamedIndividual .

figi-ps:BDF a figi-gii:PricingSource .

figi-ps:ACON a figi-gii:PricingSource .

figi-ps:FMI skos:prefLabel "factory mutual insur" .

figi-ps:BDF skos:prefLabel "banque de france" .

figi-ps:FMI figi-gii:hasUniqueTextIdentifier "FMI" .

figi-ps:ACON skos:prefLabel "assoc conservateur" .

figi-ps:BDF figi-gii:hasUniqueTextIdentifier "BDF" .

figi-ps:ACON figi-gii:hasUniqueTextIdentifier "ACON" .

figi-ps:FMIC a owl:NamedIndividual .

figi-ps:BDFA a owl:NamedIndividual .

figi-ps:FMIC a figi-gii:PricingSource .

figi-ps:ACOP a owl:NamedIndividual .

figi-ps:BDFA a figi-gii:PricingSource .

figi-ps:ACOP a figi-gii:PricingSource .

figi-ps:FMIC skos:prefLabel "first metro inv" .

figi-ps:BDFA skos:prefLabel "bbg daily fixing aus" .

figi-ps:ACOP skos:prefLabel "agentes corredores" .

figi-ps:FMIC figi-gii:hasUniqueTextIdentifier "FMIC" .

figi-ps:ACOP figi-gii:hasUniqueTextIdentifier "ACOP" .

figi-ps:BDFA figi-gii:hasUniqueTextIdentifier "BDFA" .

figi-ps:FMPH a owl:NamedIndividual .

figi-ps:ACRS a owl:NamedIndividual .

figi-ps:BDG a owl:NamedIndividual .

figi-ps:FMPH a figi-gii:PricingSource .

figi-ps:BDG a figi-gii:PricingSource .

figi-ps:ACRS a figi-gii:PricingSource .

figi-ps:FMPH skos:prefLabel "fund mgr assoc phils" .

figi-ps:BDG skos:prefLabel "banca del gottardo" .

figi-ps:FMPH figi-gii:hasUniqueTextIdentifier "FMPH" .

figi-ps:ACRS skos:prefLabel "across investment" .

figi-ps:FMSI a owl:NamedIndividual .

figi-ps:BDG figi-gii:hasUniqueTextIdentifier "BDG" .

figi-ps:ACRS figi-gii:hasUniqueTextIdentifier "ACRS" .

figi-ps:FMSI a figi-gii:PricingSource .

figi-ps:BDIN a owl:NamedIndividual .

figi-ps:FMSI skos:prefLabel "fms bondscom" .

figi-ps:ACVA a owl:NamedIndividual .

figi-ps:BDIN a figi-gii:PricingSource .

figi-ps:ACVA a figi-gii:PricingSource .

figi-ps:BDIN skos:prefLabel "bk danamon indonesia" .

figi-ps:ACVA skos:prefLabel "acciones and valores" .

figi-ps:FMSI figi-gii:hasUniqueTextIdentifier "FMSI" .

figi-ps:BDIN figi-gii:hasUniqueTextIdentifier "BDIN" .

figi-ps:FMTS a owl:NamedIndividual .

figi-ps:ACVA figi-gii:hasUniqueTextIdentifier "ACVA" .

figi-ps:FMTS a figi-gii:PricingSource .

figi-ps:BDMN a owl:NamedIndividual .

figi-ps:FMTS skos:prefLabel "france mts" .

figi-st:delayDraw a owl:NamedIndividual .

figi-ps:FMTS figi-gii:hasUniqueTextIdentifier "FMTS" .

figi-ps:BDMN a figi-gii:PricingSource .

figi-st:delayDraw a figi-gii:SecurityType .

figi-ps:FNBL a owl:NamedIndividual .

figi-ps:BDMN skos:prefLabel "bank danamon" .

figi-ps:FNBL a figi-gii:PricingSource .

figi-ps:BDMN figi-gii:hasUniqueTextIdentifier "BDMN" .

figi-ps:FNBL skos:prefLabel "first national bank" ;
	figi-gii:hasUniqueTextIdentifier "FNBL" .

figi-ps:BDNI a owl:NamedIndividual , figi-gii:PricingSource .

figi-ps:FNBN a owl:NamedIndividual , figi-gii:PricingSource .

figi-ps:BDNI skos:prefLabel "bank danamon indnsia" .

figi-ps:FNBN skos:prefLabel "first bk of nigeria" .

figi-st:delayDraw skos:definition "Term loan where borrower is allowed to draw down on the loan in one or more drawings within a specified time period after the signing date. While the loan is technically effective from the signing date, availability is often subject to the completion of specific construction landmarks and/or the closing of a specific acquisition (note that this should not be confused with the Signed but not Effective status)." .

figi-ps:FNBN figi-gii:hasUniqueTextIdentifier "FNBN" .

figi-ps:BDNI figi-gii:hasUniqueTextIdentifier "BDNI" .

figi-st:delayDraw skos:prefLabel "delay-draw" .

figi-ps:FNBT a owl:NamedIndividual .

figi-ps:BDOB a owl:NamedIndividual .

figi-ps:FNBT a figi-gii:PricingSource .

figi-st:delayDraw figi-gii:hasUniqueTextIdentifier "DELAY-DRAW" .

figi-ps:FNBT skos:prefLabel "finarbit ag" .

figi-ps:BDOB a figi-gii:PricingSource .

figi-ps:FNBT figi-gii:hasUniqueTextIdentifier "FNBT" .

figi-ps:ACVZ a owl:NamedIndividual .

figi-ps:BDOB skos:prefLabel "banco do brasil" .

figi-ps:FNBW a owl:NamedIndividual .

figi-ps:ACVZ a figi-gii:PricingSource .

figi-ps:FNBW a figi-gii:PricingSource .

figi-ps:BDOB figi-gii:hasUniqueTextIdentifier "BDOB" .

figi-ps:ACVZ skos:prefLabel "activalores" .

figi-ps:FNBW skos:prefLabel "first national bank" .

figi-ps:BDOE a owl:NamedIndividual .

figi-ps:FNBW figi-gii:hasUniqueTextIdentifier "FNBW" .

figi-ps:BDOE a figi-gii:PricingSource .

figi-ps:FNCD a owl:NamedIndividual , figi-gii:PricingSource .

figi-ps:ACVZ figi-gii:hasUniqueTextIdentifier "ACVZ" .

figi-ps:BDOE skos:prefLabel "banco de oro - epci" .

figi-ps:AD a owl:NamedIndividual .

figi-ps:FNCD skos:prefLabel "financial northeastn" .

figi-ps:BDOE figi-gii:hasUniqueTextIdentifier "BDOE" .

figi-ps:FNCD figi-gii:hasUniqueTextIdentifier "FNCD" .

figi-ps:AD a figi-gii:PricingSource .

figi-ps:BDOP a owl:NamedIndividual .

figi-ps:FNY a owl:NamedIndividual .

figi-ps:AD skos:prefLabel "alphadyne" .

figi-ps:BDOP a figi-gii:PricingSource .

figi-ps:FNY a figi-gii:PricingSource .

figi-ps:AD figi-gii:hasUniqueTextIdentifier "AD" .

figi-ps:BDOP skos:prefLabel "banco de oro" .

figi-ps:FNY skos:prefLabel "fny aim" .

figi-st:delayDrawIslamic a owl:NamedIndividual .

figi-ps:FNY figi-gii:hasUniqueTextIdentifier "FNY" .

figi-ps:BDOP figi-gii:hasUniqueTextIdentifier "BDOP" .

figi-st:delayDrawIslamic a figi-gii:SecurityType .

figi-ps:FNY2 a owl:NamedIndividual .

figi-ps:BDOT a owl:NamedIndividual .

figi-ps:FNY2 a figi-gii:PricingSource .

figi-ps:BDOT a figi-gii:PricingSource .

figi-ps:FNY2 skos:prefLabel "fny aim equity" .

figi-ps:BDOT skos:prefLabel "bdo trust" .

figi-ps:FNY2 figi-gii:hasUniqueTextIdentifier "FNY2" .

figi-st:delayDrawIslamic skos:definition "Borrower is allowed to draw down on the loan in one or more drawings within a specified time period after the signing date. Interest cannot be charged, complying with Islamic/sharpie law." .

figi-ps:FNYP a owl:NamedIndividual .

figi-ps:BDOT figi-gii:hasUniqueTextIdentifier "BDOT" .

figi-st:delayDrawIslamic skos:prefLabel "delay-draw islamic" .

figi-ps:FNYP a figi-gii:PricingSource .

figi-ps:BDPC a owl:NamedIndividual .

figi-st:delayDrawIslamic figi-gii:hasUniqueTextIdentifier "DELAY-DRAW ISLAMIC" .

figi-ps:FNYP skos:prefLabel "first ny securities" .

figi-ps:BDPC a figi-gii:PricingSource .

figi-ps:ADAM a owl:NamedIndividual .

figi-ps:FNYP figi-gii:hasUniqueTextIdentifier "FNYP" .

figi-ps:ADAM a figi-gii:PricingSource .

figi-ps:FNYS a owl:NamedIndividual .

figi-ps:BDPC skos:prefLabel "broadpoint capital" .

figi-ps:FNYS a figi-gii:PricingSource .

figi-ps:ADAM skos:prefLabel "advisors asset mgmt" .

figi-ps:FNYS skos:prefLabel "first new york sec" .

figi-ps:BDPC figi-gii:hasUniqueTextIdentifier "BDPC" .

figi-ps:ADAM figi-gii:hasUniqueTextIdentifier "ADAM" .

figi-ps:FNYS figi-gii:hasUniqueTextIdentifier "FNYS" .

figi-ps:BDPR a owl:NamedIndividual .

figi-ps:FOBR a owl:NamedIndividual .

figi-st:delayDrawIslamicLoc a owl:NamedIndividual .

figi-ps:FOBR a figi-gii:PricingSource .

figi-ps:BDPR a figi-gii:PricingSource .

figi-ps:FOBR skos:prefLabel "fortis" .

figi-st:delayDrawIslamicLoc a figi-gii:SecurityType .

figi-ps:FOBR figi-gii:hasUniqueTextIdentifier "FOBR" .

figi-ps:BDPR skos:prefLabel "banco del progreso" .

figi-ps:FOIN a owl:NamedIndividual , figi-gii:PricingSource .

figi-ps:BDPR figi-gii:hasUniqueTextIdentifier "BDPR" .

figi-ps:FOIN skos:prefLabel "forest investment" ;
	figi-gii:hasUniqueTextIdentifier "FOIN" .

figi-ps:BDPT a owl:NamedIndividual .

figi-ps:FORU a owl:NamedIndividual .

figi-ps:BDPT a figi-gii:PricingSource .

figi-st:delayDrawIslamicLoc skos:definition "Borrower is allowed to draw down on the loan in one or more drawings within a specified time period after the signing date. Interest cannot be charged, complying with Islamic/sharpie law. Guaranteed by the lender(s) and used for purchase of goods, completion of construction projects, and/or general purposes." .

figi-ps:FORU a figi-gii:PricingSource .

figi-ps:BDPT skos:prefLabel "gleacher" .

figi-st:delayDrawIslamicLoc skos:prefLabel "delay-draw islamic loc" .

figi-ps:FORU skos:prefLabel "forum securities ltd" .

figi-ps:BDPT figi-gii:hasUniqueTextIdentifier "BDPT" .

figi-st:delayDrawIslamicLoc figi-gii:hasUniqueTextIdentifier "DELAY-DRAW ISLAMIC LOC" .

figi-ps:FORU figi-gii:hasUniqueTextIdentifier "FORU" .

figi-ps:BDS a owl:NamedIndividual .

figi-ps:ADB a owl:NamedIndividual .

figi-ps:FOXP a owl:NamedIndividual .

figi-ps:BDS a figi-gii:PricingSource .

figi-ps:ADB a figi-gii:PricingSource .

figi-ps:FOXP a figi-gii:PricingSource .

figi-ps:BDS skos:prefLabel "banca del sempione" .

figi-ps:ADB skos:prefLabel "asian dev bank" .

figi-ps:FOXP skos:prefLabel "fox-pitt,kelton,inc." .

figi-ps:BDS figi-gii:hasUniqueTextIdentifier "BDS" .

figi-ps:ADB figi-gii:hasUniqueTextIdentifier "ADB" .

figi-ps:FOXP figi-gii:hasUniqueTextIdentifier "FOXP" .

figi-st:delayDrawIslamicTerm a owl:NamedIndividual .

figi-ps:FOYL a owl:NamedIndividual .

figi-ps:BDSD a owl:NamedIndividual .

figi-st:delayDrawIslamicTerm a figi-gii:SecurityType .

figi-ps:FOYL a figi-gii:PricingSource .

figi-ps:BDSD a figi-gii:PricingSource .

figi-ps:FOYL skos:prefLabel "foyil securities" .

figi-ps:BDSD skos:prefLabel "bonds direct sec" .

figi-ps:FOYL figi-gii:hasUniqueTextIdentifier "FOYL" .

figi-ps:BDSD figi-gii:hasUniqueTextIdentifier "BDSD" .

figi-ps:FP0B a owl:NamedIndividual .

figi-st:delayDrawIslamicTerm skos:definition "Borrower is allowed to draw down on the loan in one or more drawings within a specified time period after the signing date. Interest cannot be charged, complying with Islamic/sharpie law. Once borrowed, cannot be re-borrowed." .

figi-ps:FP0B a figi-gii:PricingSource .

figi-ps:BDT a owl:NamedIndividual .

figi-st:delayDrawIslamicTerm skos:prefLabel "delay-draw islamic term" .

figi-ps:FP0B skos:prefLabel "bovespa gross sett" .

figi-ps:BDT a figi-gii:PricingSource .

figi-ps:FP0B figi-gii:hasUniqueTextIdentifier "FP0B" .

figi-st:delayDrawIslamicTerm figi-gii:hasUniqueTextIdentifier "DELAY-DRAW ISLAMIC TERM" .

figi-ps:FP0L a owl:NamedIndividual .

figi-ps:BDT skos:prefLabel "bdt investment man" .

figi-ps:FP0L a figi-gii:PricingSource .

figi-ps:ADBC a owl:NamedIndividual .

figi-ps:BDT figi-gii:hasUniqueTextIdentifier "BDT" .

figi-ps:FP0L skos:prefLabel "bovespa t+0 sett" .

figi-ps:ADBC a figi-gii:PricingSource .

figi-ps:FP0L figi-gii:hasUniqueTextIdentifier "FP0L" .

figi-ps:BEAH a owl:NamedIndividual .

figi-ps:ADBC skos:prefLabel "andbanc" .

figi-ps:BEAH a figi-gii:PricingSource .

figi-ps:FP1L a owl:NamedIndividual .

figi-ps:ADBC figi-gii:hasUniqueTextIdentifier "ADBC" .

figi-ps:BEAH skos:prefLabel "bank of east asia" .

figi-ps:FP1L a figi-gii:PricingSource .

figi-st:delayDrawPikTerm a owl:NamedIndividual .

figi-ps:FP1L skos:prefLabel "bovespa t+1 sett" .

figi-ps:BEAH figi-gii:hasUniqueTextIdentifier "BEAH" .

figi-st:delayDrawPikTerm a figi-gii:SecurityType .

figi-ps:FP1L figi-gii:hasUniqueTextIdentifier "FP1L" .

figi-ps:BEAP a owl:NamedIndividual , figi-gii:PricingSource .

figi-ps:FRAM a owl:NamedIndividual , figi-gii:PricingSource .

figi-ps:BEAP skos:prefLabel "bea 4:30" .

figi-ps:FRAM skos:prefLabel "fortis nl mortgages" .

figi-st:delayDrawPikTerm skos:definition "Borrower is allowed to draw down on the loan in one or more drawings within a specified time period after the signing date. Interest may be capitalized and added to the principal amount of the loan, which is then compounded and due to lenders at maturity. Once borrowed, cannot be re-borrowed." .

figi-ps:FRAM figi-gii:hasUniqueTextIdentifier "FRAM" .

figi-ps:BEAP figi-gii:hasUniqueTextIdentifier "BEAP" .

figi-ps:FRDM a owl:NamedIndividual .

figi-st:delayDrawPikTerm skos:prefLabel "delay-draw pik term" .

figi-ps:FRDM a figi-gii:PricingSource .

figi-ps:BEC a owl:NamedIndividual .

figi-st:delayDrawPikTerm figi-gii:hasUniqueTextIdentifier "DELAY-DRAW PIK TERM" .

figi-ps:BEC a figi-gii:PricingSource .

figi-ps:FRDM skos:prefLabel "freedom intl" .

figi-ps:ADCB a owl:NamedIndividual .

figi-ps:BEC skos:prefLabel "bolsa de elec chile" .

figi-ps:ADCB a figi-gii:PricingSource .

figi-ps:FRDM figi-gii:hasUniqueTextIdentifier "FRDM" .

figi-ps:BEC figi-gii:hasUniqueTextIdentifier "BEC" .

figi-ps:FREN a owl:NamedIndividual .

figi-ps:ADCB skos:prefLabel "abu dhabi commrl bk" .

figi-ps:FREN a figi-gii:PricingSource .

figi-ps:BECD a owl:NamedIndividual .

figi-ps:ADCB figi-gii:hasUniqueTextIdentifier "ADCB" .

figi-ps:FREN skos:prefLabel "fortis bank, hk" .

figi-ps:BECD a figi-gii:PricingSource .

figi-ps:FREN figi-gii:hasUniqueTextIdentifier "FREN" .

figi-st:delayDrawRev a owl:NamedIndividual .

figi-ps:BECD skos:prefLabel "barcap-eq link cds" .

figi-st:delayDrawRev a figi-gii:SecurityType .

figi-ps:FRNK a owl:NamedIndividual .

figi-ps:BECD figi-gii:hasUniqueTextIdentifier "BECD" .

figi-ps:FRNK a figi-gii:PricingSource .

figi-ps:BECH a owl:NamedIndividual .

figi-ps:FRNK skos:prefLabel "frankfurt exch" .

figi-ps:BECH a figi-gii:PricingSource .

figi-ps:FRNK figi-gii:hasUniqueTextIdentifier "FRNK" .

figi-ps:BECH skos:prefLabel "banco estado sa" .

figi-ps:FRST a owl:NamedIndividual .

figi-st:delayDrawRev skos:definition "Forward-start deal where borrower is allowed to draw down on the loan in one or more drawings within a specified time period after the signing date. While the loan is technically effective from the signing date, availability is often subject to the completion of specific construction landmarks and/or the closing of a specific acquisition (note that this should not be confused with the Signed but not Effective status)." .

figi-ps:FRST a figi-gii:PricingSource .

figi-ps:BECH figi-gii:hasUniqueTextIdentifier "BECH" .

figi-ps:FRST skos:prefLabel "first albany" .

figi-st:delayDrawRev skos:prefLabel "delay-draw rev" .

figi-ps:FRST figi-gii:hasUniqueTextIdentifier "FRST" .

figi-ps:BEIR a owl:NamedIndividual .

figi-st:delayDrawRev figi-gii:hasUniqueTextIdentifier "DELAY-DRAW REV" .

figi-ps:BEIR a figi-gii:PricingSource .

figi-ps:FRTB a owl:NamedIndividual .

figi-ps:ADCP a owl:NamedIndividual .

figi-ps:FRTB a figi-gii:PricingSource .

figi-ps:BEIR skos:prefLabel "beirut stock exch" .

figi-ps:ADCP a figi-gii:PricingSource .

figi-ps:FRTB skos:prefLabel "fortis bank" .

figi-ps:BEIR figi-gii:hasUniqueTextIdentifier "BEIR" .

figi-ps:FRTB figi-gii:hasUniqueTextIdentifier "FRTB" .

figi-ps:ADCP skos:prefLabel "adamant capital" .

figi-ps:BELC a owl:NamedIndividual .

figi-ps:FRTH a owl:NamedIndividual .

figi-ps:ADCP figi-gii:hasUniqueTextIdentifier "ADCP" .

figi-ps:FRTH a figi-gii:PricingSource .

figi-ps:BELC a figi-gii:PricingSource .

figi-ps:FRTH skos:prefLabel "fortis bank hk" .

figi-st:delayDrawStandbyTerm a owl:NamedIndividual , figi-gii:SecurityType .

figi-ps:BELC skos:prefLabel "barclays capital ny" .

figi-ps:FRTH figi-gii:hasUniqueTextIdentifier "FRTH" .

figi-ps:FRTK a owl:NamedIndividual , figi-gii:PricingSource ;
	skos:prefLabel "fortis bk hong kong" .

figi-st:delayDrawStandbyTerm skos:definition "Borrower is allowed to draw down on the loan in one or more drawings within a specified time period after the signing date. Issued on a stand-by basis and borrowed only if and when needed. Once borrowed, cannot be re-borrowed." .

figi-ps:FRTK figi-gii:hasUniqueTextIdentifier "FRTK" .

figi-ps:BELC figi-gii:hasUniqueTextIdentifier "BELC" .

figi-st:delayDrawStandbyTerm skos:prefLabel "delay-draw standby term" .

figi-ps:FRTM a owl:NamedIndividual .

figi-ps:BELE a owl:NamedIndividual .

figi-st:delayDrawStandbyTerm figi-gii:hasUniqueTextIdentifier "DELAY-DRAW STANDBY TERM" .

figi-ps:FRTM a figi-gii:PricingSource .

figi-ps:BELE a figi-gii:PricingSource .

figi-ps:FRTM skos:prefLabel "fortis bk" .

figi-ps:ADIX a owl:NamedIndividual .

figi-ps:BELE skos:prefLabel "bgc australia elec" .

figi-ps:FRTM figi-gii:hasUniqueTextIdentifier "FRTM" .

figi-ps:ADIX a figi-gii:PricingSource .

figi-ps:FRTN a owl:NamedIndividual .

figi-ps:BELE figi-gii:hasUniqueTextIdentifier "BELE" .

figi-ps:FRTN a figi-gii:PricingSource .

figi-ps:ADIX skos:prefLabel "adix" .

figi-ps:BELF a owl:NamedIndividual .

figi-ps:FRTN skos:prefLabel "fortis netherlands" .

figi-ps:ADIX figi-gii:hasUniqueTextIdentifier "ADIX" .

figi-ps:FRTN figi-gii:hasUniqueTextIdentifier "FRTN" .

figi-ps:BELF a figi-gii:PricingSource .

figi-st:delayDrawTerm a owl:NamedIndividual .

figi-ps:FRTZ a owl:NamedIndividual .

figi-ps:BELF skos:prefLabel "belfius bank" .

figi-ps:FRTZ a figi-gii:PricingSource .

figi-st:delayDrawTerm a figi-gii:SecurityType .

figi-ps:BELF figi-gii:hasUniqueTextIdentifier "BELF" .

figi-ps:FRTZ skos:prefLabel "fortis bank be" ;
	figi-gii:hasUniqueTextIdentifier "FRTZ" .

figi-ps:BELL a owl:NamedIndividual .

figi-ps:FS a owl:NamedIndividual .

figi-ps:BELL a figi-gii:PricingSource .

figi-ps:FS a figi-gii:PricingSource .

figi-st:delayDrawTerm skos:definition "Borrower is allowed to draw down on the loan in one or more drawings within a specified time period after the signing date. Once borrowed, cannot be re-borrowed." .

figi-ps:FS skos:prefLabel "first securities asa" .

figi-ps:BELL skos:prefLabel "belle haven" .

figi-ps:FS figi-gii:hasUniqueTextIdentifier "FS" .

figi-st:delayDrawTerm skos:prefLabel "delay-draw term" .

figi-ps:BELL figi-gii:hasUniqueTextIdentifier "BELL" .

figi-ps:FSA a owl:NamedIndividual .

figi-st:delayDrawTerm figi-gii:hasUniqueTextIdentifier "DELAY-DRAW TERM" .

figi-ps:FSA a figi-gii:PricingSource .

figi-ps:BELX a owl:NamedIndividual .

figi-ps:ADP a owl:NamedIndividual .

figi-ps:FSA skos:prefLabel "financial security a" .

figi-ps:BELX a figi-gii:PricingSource .

figi-ps:ADP a figi-gii:PricingSource .

figi-ps:FSA figi-gii:hasUniqueTextIdentifier "FSA" .

figi-ps:BELX skos:prefLabel "belgrade stock exch" .

figi-ps:ADP skos:prefLabel "adp" .

figi-ps:FSCA a owl:NamedIndividual .

figi-ps:BELX figi-gii:hasUniqueTextIdentifier "BELX" .

figi-ps:FSCA a figi-gii:PricingSource .

figi-ps:ADP figi-gii:hasUniqueTextIdentifier "ADP" .

figi-ps:BEMO a owl:NamedIndividual .

figi-ps:FSCA skos:prefLabel "first taisec sec" .

figi-st:delayDrawTermVatTrnch a owl:NamedIndividual .

figi-ps:BEMO a figi-gii:PricingSource .

figi-st:delayDrawTermVatTrnch a figi-gii:SecurityType .

figi-ps:BEMO skos:prefLabel "banque europeenne pl" ;
	figi-gii:hasUniqueTextIdentifier "BEMO" .

figi-st:delayDrawTermVatTrnch skos:definition "Borrower is allowed to draw down on the loan in one or more drawings within a specified time period after the signing date. Once borrowed, cannot be re-borrowed. Given as temporary reimbursement for a VAT credit it has with the state." .

figi-ps:BENG a owl:NamedIndividual , figi-gii:PricingSource .

figi-st:delayDrawTermVatTrnch skos:prefLabel "delay-draw term vat-trnch" .

figi-ps:FSCA figi-gii:hasUniqueTextIdentifier "FSCA" .

figi-ps:BENG skos:prefLabel "bengochea and co s.b." .

figi-st:delayDrawTermVatTrnch figi-gii:hasUniqueTextIdentifier "DELAY-DRAW TERM VAT-TRNCH" .

figi-ps:FSSS a owl:NamedIndividual .

figi-ps:BENG figi-gii:hasUniqueTextIdentifier "BENG" .

figi-ps:FSSS a figi-gii:PricingSource .

figi-ps:ADSS a owl:NamedIndividual .

figi-ps:BEPE a owl:NamedIndividual .

figi-ps:ADSS a figi-gii:PricingSource .

figi-ps:FSSS skos:prefLabel "fss spectrum" .

figi-ps:BEPE a figi-gii:PricingSource .

figi-ps:ADSS skos:prefLabel "ads securities llc" .

figi-ps:FSSS figi-gii:hasUniqueTextIdentifier "FSSS" .

figi-ps:BEPE skos:prefLabel "b-val internal pcs" .

figi-ps:ADSS figi-gii:hasUniqueTextIdentifier "ADSS" .

figi-ps:FSTB a owl:NamedIndividual .

figi-ps:BEPE figi-gii:hasUniqueTextIdentifier "BEPE" .

figi-ps:FSTB a figi-gii:PricingSource .

figi-st:delayDrawVatTrnch a owl:NamedIndividual .

figi-ps:BERB a owl:NamedIndividual .

figi-st:delayDrawVatTrnch a figi-gii:SecurityType .

figi-ps:FSTB skos:prefLabel "bd 2nd best" .

figi-st:delayDrawVatTrnch skos:definition "Delayed-draw VAT facility" .

figi-ps:BERB a figi-gii:PricingSource .

figi-ps:FSTB figi-gii:hasUniqueTextIdentifier "FSTB" .

figi-st:delayDrawVatTrnch skos:prefLabel "delay-draw vat-trnch" .

figi-ps:BERB skos:prefLabel "berenberg bank" .

figi-ps:FSW a owl:NamedIndividual .

figi-st:delayDrawVatTrnch figi-gii:hasUniqueTextIdentifier "DELAY-DRAW VAT-TRNCH" .

figi-ps:FSW a figi-gii:PricingSource .

figi-ps:BERB figi-gii:hasUniqueTextIdentifier "BERB" .

figi-st:deposit a owl:NamedIndividual .

figi-ps:FSW skos:prefLabel "first southwest co" .

figi-ps:BERM a owl:NamedIndividual .

figi-st:deposit a figi-gii:SecurityType .

figi-ps:FSW figi-gii:hasUniqueTextIdentifier "FSW" .

figi-ps:BERM a figi-gii:PricingSource .

figi-st:deposit skos:definition "The interest rate paid by financial institutions to deposit account holders" .

figi-ps:FTAZ a owl:NamedIndividual .

figi-ps:BERM skos:prefLabel "barcap em pricing" .

figi-st:deposit skos:prefLabel "deposit" .

figi-ps:FTAZ a figi-gii:PricingSource .

figi-ps:BERM figi-gii:hasUniqueTextIdentifier "BERM" .

figi-st:deposit figi-gii:hasUniqueTextIdentifier "DEPOSIT" .

figi-ps:FTAZ skos:prefLabel "first taz money" .

figi-ps:BES a owl:NamedIndividual .

figi-ps:ADV a owl:NamedIndividual .

figi-ps:FTAZ figi-gii:hasUniqueTextIdentifier "FTAZ" .

figi-ps:ADV a figi-gii:PricingSource .

figi-ps:FTFS a owl:NamedIndividual , figi-gii:PricingSource .

figi-ps:ADV skos:prefLabel "advantus capital" .

figi-ps:FTFS skos:prefLabel "financial services" .

figi-ps:ADV figi-gii:hasUniqueTextIdentifier "ADV" .

figi-ps:FTFS figi-gii:hasUniqueTextIdentifier "FTFS" .

figi-st:depositNote a owl:NamedIndividual .

figi-ps:FTID a owl:NamedIndividual .

figi-st:depositNote a figi-gii:SecurityType .

figi-ps:FTID a figi-gii:PricingSource ;
	skos:prefLabel "ft interactive data" ;
	figi-gii:hasUniqueTextIdentifier "FTID" .

figi-st:depositNote skos:definition "Deposit Note. Deposit Notes are securities issued by a financial institution using the deposits of the institution as collateral. These securities carry the FDIC insurance." .

figi-ps:FTIM a owl:NamedIndividual .

figi-st:depositNote skos:prefLabel "deposit note" .

figi-ps:FTIM a figi-gii:PricingSource .

figi-st:depositNote figi-gii:hasUniqueTextIdentifier "DEPOSIT NOTE" .

figi-ps:FTIM skos:prefLabel "ft interactive mtge" .

figi-ps:ADVA a owl:NamedIndividual .

figi-ps:FTIM figi-gii:hasUniqueTextIdentifier "FTIM" .

figi-ps:ADVA a figi-gii:PricingSource .

figi-ps:FTN a owl:NamedIndividual .

figi-ps:ADVA skos:prefLabel "advicorp plc" .

figi-ps:FTN a figi-gii:PricingSource .

figi-ps:ADVA figi-gii:hasUniqueTextIdentifier "ADVA" .

figi-ps:FTN skos:prefLabel "ftn fin'l" .

figi-st:dimSum a owl:NamedIndividual .

figi-ps:FTN figi-gii:hasUniqueTextIdentifier "FTN" .

figi-st:dimSum a figi-gii:SecurityType .

figi-ps:FTNF a owl:NamedIndividual , figi-gii:PricingSource ;
	skos:prefLabel "ftn financial" .

figi-st:dimSum skos:definition "Offshore lending facilities denominated in Renminbi (RMB) currency, the lending happens outside Mainland China, Dim Sum loans can be term or revolving loans." .

figi-ps:FTNF figi-gii:hasUniqueTextIdentifier "FTNF" .

figi-st:dimSum skos:prefLabel "dim sum" .

figi-ps:FTNN a owl:NamedIndividual .

figi-st:dimSum figi-gii:hasUniqueTextIdentifier "DIM SUM" .

figi-ps:FTNN a figi-gii:PricingSource .

figi-ps:ADVE a owl:NamedIndividual .

figi-ps:FTNN skos:prefLabel "ftn financial boom" .

figi-ps:ADVE a figi-gii:PricingSource .

figi-ps:FTNN figi-gii:hasUniqueTextIdentifier "FTNN" .

figi-ps:ADVE skos:prefLabel "advent capital" .

figi-ps:FTNT a owl:NamedIndividual .

figi-ps:ADVE figi-gii:hasUniqueTextIdentifier "ADVE" .

figi-ps:FTNT a figi-gii:PricingSource .

figi-st:dimSumBridgeTerm a owl:NamedIndividual .

figi-ps:FTNT skos:prefLabel "ftn financial" .

figi-st:dimSumBridgeTerm a figi-gii:SecurityType .

figi-ps:FTNT figi-gii:hasUniqueTextIdentifier "FTNT" .

figi-ps:FTRU a owl:NamedIndividual , figi-gii:PricingSource .

figi-st:dimSumBridgeTerm skos:definition "Event-driven loan intended to provide finance for a short period of time until longer-term financing can be obtained. Denominated in Renminbi (RMB) currency, the lending happens outside Mainland China. Once borrowed, cannot be re-borrowed." .

figi-ps:FTRU skos:prefLabel "first trust advisors" .

figi-st:dimSumBridgeTerm skos:prefLabel "dim sum bridge term" .

figi-ps:FTRU figi-gii:hasUniqueTextIdentifier "FTRU" .

figi-st:dimSumBridgeTerm figi-gii:hasUniqueTextIdentifier "DIM SUM BRIDGE TERM" .

figi-ps:FTW a owl:NamedIndividual , figi-gii:PricingSource .

figi-ps:ADVI a owl:NamedIndividual .

figi-ps:FTW skos:prefLabel "fort washington" .

figi-ps:ADVI a figi-gii:PricingSource .

figi-ps:FTW figi-gii:hasUniqueTextIdentifier "FTW" .

figi-ps:ADVI skos:prefLabel "advicorp" .

figi-ps:FUBK a owl:NamedIndividual .

figi-ps:ADVI figi-gii:hasUniqueTextIdentifier "ADVI" .

figi-ps:FUBK a figi-gii:PricingSource .

figi-ps:AELT a owl:NamedIndividual .

figi-ps:FUBK skos:prefLabel "fubon bank (hk) ltd" .

figi-ps:AELT a figi-gii:PricingSource .

figi-ps:FUBK figi-gii:hasUniqueTextIdentifier "FUBK" .

figi-ps:AELT skos:prefLabel "aeltus" .

figi-ps:FUBO a owl:NamedIndividual .

figi-ps:AELT figi-gii:hasUniqueTextIdentifier "AELT" .

figi-ps:FUBO a figi-gii:PricingSource .

figi-st:dimSumDelayDrawTerm a owl:NamedIndividual .

figi-ps:FUBO skos:prefLabel "fubon securities" .

figi-st:dimSumDelayDrawTerm a figi-gii:SecurityType .

figi-ps:FUBO figi-gii:hasUniqueTextIdentifier "FUBO" .

figi-ps:FUBP a owl:NamedIndividual , figi-gii:PricingSource .

figi-st:dimSumDelayDrawTerm skos:definition "Denominated in Renminbi (RMB) currency, the lending happens outside Mainland China. Borrower is allowed to draw down on the loan in one or more drawings within a specified time period after the signing date. Once borrowed, cannot be re-borrowed." .

figi-ps:FUBP skos:prefLabel "fubon bank tma 4pm" .

figi-st:dimSumDelayDrawTerm skos:prefLabel "dim sum delay-draw term" .

figi-ps:FUBP figi-gii:hasUniqueTextIdentifier "FUBP" .

figi-st:dimSumDelayDrawTerm figi-gii:hasUniqueTextIdentifier "DIM SUM DELAY-DRAW TERM" .

figi-ps:FUJZ a owl:NamedIndividual , figi-gii:PricingSource .

figi-ps:AEU1 a owl:NamedIndividual .

figi-ps:FUJZ skos:prefLabel "fuji bank zurich" .

figi-ps:AEU1 a figi-gii:PricingSource .

figi-ps:FUJZ figi-gii:hasUniqueTextIdentifier "FUJZ" .

figi-ps:AEU1 skos:prefLabel "efgam" .

figi-ps:FUNX a owl:NamedIndividual .

figi-ps:BES a figi-gii:PricingSource .

figi-ps:FUNX a figi-gii:PricingSource .

figi-ps:BES skos:prefLabel "banco espirito" .

figi-ps:AEU1 figi-gii:hasUniqueTextIdentifier "AEU1" .

figi-ps:FUNX skos:prefLabel "funnex asset mgmt" .

figi-ps:BES figi-gii:hasUniqueTextIdentifier "BES" .

figi-st:dimSumRev a owl:NamedIndividual .

figi-ps:FUNX figi-gii:hasUniqueTextIdentifier "FUNX" .

figi-ps:BESA a owl:NamedIndividual .

figi-st:dimSumRev a figi-gii:SecurityType .

figi-ps:BESA a figi-gii:PricingSource .

figi-ps:FURN a owl:NamedIndividual , figi-gii:PricingSource .

figi-ps:BESA skos:prefLabel "bloomberg average" .

figi-ps:FURN skos:prefLabel "furnoanddel castano" .

figi-ps:BESA figi-gii:hasUniqueTextIdentifier "BESA" .

figi-st:dimSumRev skos:definition "Event-driven loan intended to provide finance for a short period of time until longer-term financing can be obtained. Denominated in Renminbi (RMB) currency, the lending happens outside Mainland China. Once borrowed, can be borrowed again." .

figi-ps:BESB a owl:NamedIndividual .

figi-st:dimSumRev skos:prefLabel "dim sum rev" .

figi-ps:BESB a figi-gii:PricingSource .

figi-st:dimSumRev figi-gii:hasUniqueTextIdentifier "DIM SUM REV" .

figi-ps:BESB skos:prefLabel "banco espirito santo" .

figi-st:dimSumTerm a owl:NamedIndividual .

figi-ps:FURN figi-gii:hasUniqueTextIdentifier "FURN" .

figi-st:dimSumTerm a figi-gii:SecurityType .

figi-ps:FVLB a owl:NamedIndividual , figi-gii:PricingSource ;
	skos:prefLabel "f van lanschot bank" .

figi-st:dimSumTerm skos:definition "Denominated in Renminbi (RMB) currency, the lending happens outside Mainland China. Once borrowed, cannot be re-borrowed." .

figi-ps:FVLB figi-gii:hasUniqueTextIdentifier "FVLB" .

figi-st:dimSumTerm skos:prefLabel "dim sum term" .

figi-ps:FWCO a owl:NamedIndividual .

figi-st:dimSumTerm figi-gii:hasUniqueTextIdentifier "DIM SUM TERM" .

figi-ps:FWCO a figi-gii:PricingSource .

figi-ps:AEXB a owl:NamedIndividual .

figi-ps:FWCO skos:prefLabel "first washington" .

figi-ps:AEXB a figi-gii:PricingSource .

figi-ps:FWCO figi-gii:hasUniqueTextIdentifier "FWCO" .

figi-ps:AEXB skos:prefLabel "amex bank indonesia" .

figi-ps:FX0B a owl:NamedIndividual .

figi-ps:AEXB figi-gii:hasUniqueTextIdentifier "AEXB" .

figi-ps:FX0B a figi-gii:PricingSource .

figi-st:dip a owl:NamedIndividual .

figi-ps:FX0B skos:prefLabel "bovespa gross sett" .

figi-st:dip a figi-gii:SecurityType .

figi-ps:FX0B figi-gii:hasUniqueTextIdentifier "FX0B" .

figi-ps:FX0L a owl:NamedIndividual , figi-gii:PricingSource ;
	skos:prefLabel "bovespa t sett" ;
	figi-gii:hasUniqueTextIdentifier "FX0L" .

figi-ps:FX1L a owl:NamedIndividual , figi-gii:PricingSource ;
	skos:prefLabel "bovespa t+1 sett" ;
	figi-gii:hasUniqueTextIdentifier "FX1L" .

figi-st:dip skos:definition "Loans issued when a company is in bankruptcy. These have a ranking of Super Priority Secured unless stated otherwise." .

figi-ps:FXMY a owl:NamedIndividual .

figi-st:dip skos:prefLabel "dip" .

figi-ps:FXMY a figi-gii:PricingSource .

figi-st:dip figi-gii:hasUniqueTextIdentifier "DIP" .

figi-ps:FXMY skos:prefLabel "forex enterprise bhd" .

figi-ps:AFAP a owl:NamedIndividual .

figi-ps:FXMY figi-gii:hasUniqueTextIdentifier "FXMY" .

figi-ps:AFAP a figi-gii:PricingSource .

figi-ps:FY0B a owl:NamedIndividual .

figi-ps:AFAP skos:prefLabel "integracion afap" ;
	figi-gii:hasUniqueTextIdentifier "AFAP" .

figi-ps:FY0B a figi-gii:PricingSource .

figi-ps:AFCA a owl:NamedIndividual .

figi-ps:FY0B skos:prefLabel "bovespa gross sett" .

figi-ps:AFCA a figi-gii:PricingSource .

figi-ps:FY0B figi-gii:hasUniqueTextIdentifier "FY0B" .

figi-ps:AFCA skos:prefLabel "comm bank of africa" .

figi-ps:FY0L a owl:NamedIndividual .

figi-ps:AFCA figi-gii:hasUniqueTextIdentifier "AFCA" .

figi-ps:FY0L a figi-gii:PricingSource .

figi-st:dipDelayDrawIslamicTerm a owl:NamedIndividual .

figi-ps:FY0L skos:prefLabel "bovespa t+0 sett" .

figi-st:dipDelayDrawIslamicTerm a figi-gii:SecurityType .

figi-ps:FY0L figi-gii:hasUniqueTextIdentifier "FY0L" .

figi-ps:FY1L a owl:NamedIndividual .

figi-st:dipDelayDrawIslamicTerm skos:definition "Issued when a company is in bankruptcy. Once borrowed, cannot be re-borrowed. Interest cannot be charged, complying with Islamic/sharpie law." .

figi-ps:FY1L a figi-gii:PricingSource ;
	skos:prefLabel "bovespa t+1 sett" ;
	figi-gii:hasUniqueTextIdentifier "FY1L" .

figi-ps:FYNC a owl:NamedIndividual , figi-gii:PricingSource ;
	skos:prefLabel "fynsa international" ;
	figi-gii:hasUniqueTextIdentifier "FYNC" .

figi-ps:GAIA a owl:NamedIndividual , figi-gii:PricingSource ;
	skos:prefLabel "global absolute" ;
	figi-gii:hasUniqueTextIdentifier "GAIA" .

figi-st:dipDelayDrawIslamicTerm skos:prefLabel "dip delay-draw islamic term" .

figi-ps:GAIM a owl:NamedIndividual .

figi-st:dipDelayDrawIslamicTerm figi-gii:hasUniqueTextIdentifier "DIP DELAY-DRAW ISLAMIC TERM" .

figi-ps:GAIM a figi-gii:PricingSource .

figi-ps:AFCR a owl:NamedIndividual , figi-gii:PricingSource .

figi-ps:GAIM skos:prefLabel "gaim capital ltd" .

figi-ps:AFCR skos:prefLabel "arab finance corp" .

figi-ps:GAIM figi-gii:hasUniqueTextIdentifier "GAIM" .

figi-ps:AFCR figi-gii:hasUniqueTextIdentifier "AFCR" .

figi-ps:GAIN a owl:NamedIndividual .

figi-ps:BESB figi-gii:hasUniqueTextIdentifier "BESB" .

figi-st:dipDelayDrawPikTerm a owl:NamedIndividual .

figi-ps:GAIN a figi-gii:PricingSource .

figi-ps:BESI a owl:NamedIndividual .

figi-st:dipDelayDrawPikTerm a figi-gii:SecurityType .

figi-ps:BESI a figi-gii:PricingSource .

figi-ps:GAIN skos:prefLabel "gain capital" .

figi-ps:BESI skos:prefLabel "bes investimento br" .

figi-ps:GAIN figi-gii:hasUniqueTextIdentifier "GAIN" .

figi-st:dipDelayDrawPikTerm skos:definition "Issued when a company is in bankruptcy. Interest may be capitalized and added to the principal amount of the loan, which is then compounded and due to lenders at maturity. Once borrowed, cannot be re-borrowed." .

figi-ps:BESI figi-gii:hasUniqueTextIdentifier "BESI" .

figi-ps:GAL a owl:NamedIndividual .

figi-st:dipDelayDrawPikTerm skos:prefLabel "dip delay-draw pik term" .

figi-ps:BESP a owl:NamedIndividual .

figi-ps:GAL a figi-gii:PricingSource .

figi-st:dipDelayDrawPikTerm figi-gii:hasUniqueTextIdentifier "DIP DELAY-DRAW PIK TERM" .

figi-ps:GAL skos:prefLabel "galliard capital" .

figi-ps:AFI a owl:NamedIndividual .

figi-ps:BESP a figi-gii:PricingSource .

figi-ps:GAL figi-gii:hasUniqueTextIdentifier "GAL" .

figi-ps:AFI a figi-gii:PricingSource .

figi-ps:BESP skos:prefLabel "banco espirito santo" .

figi-ps:GALB a owl:NamedIndividual .

figi-ps:AFI skos:prefLabel "analistas financier" .

figi-ps:BESP figi-gii:hasUniqueTextIdentifier "BESP" .

figi-ps:GALB a figi-gii:PricingSource .

figi-ps:BETO a owl:NamedIndividual .

figi-ps:AFI figi-gii:hasUniqueTextIdentifier "AFI" .

figi-ps:BETO a figi-gii:PricingSource .

figi-ps:GALB skos:prefLabel "galbraiths" .

figi-ps:BETO skos:prefLabel "bets override" .

figi-ps:AFMA a owl:NamedIndividual .

figi-ps:GALB figi-gii:hasUniqueTextIdentifier "GALB" .

figi-ps:BETO figi-gii:hasUniqueTextIdentifier "BETO" .

figi-ps:AFMA a figi-gii:PricingSource .

figi-ps:GALF a owl:NamedIndividual .

figi-ps:BEVS a owl:NamedIndividual .

figi-ps:AFMA skos:prefLabel "australian fin mkts" .

figi-ps:BEVS a figi-gii:PricingSource .

figi-ps:GALF a figi-gii:PricingSource .

figi-ps:BEVS skos:prefLabel "bevsa" .

figi-ps:AFMA figi-gii:hasUniqueTextIdentifier "AFMA" .

figi-ps:BEVS figi-gii:hasUniqueTextIdentifier "BEVS" .

figi-ps:GALF skos:prefLabel "galfin soc. de bolsa" .

figi-ps:BEWS a owl:NamedIndividual .

figi-st:dipDelayDrawRev a owl:NamedIndividual .

figi-ps:BEWS a figi-gii:PricingSource .

figi-ps:GALF figi-gii:hasUniqueTextIdentifier "GALF" .

figi-st:dipDelayDrawRev a figi-gii:SecurityType .

figi-ps:BEWS skos:prefLabel "bloomberg energy- ws" .

figi-ps:GALI a owl:NamedIndividual .

figi-ps:BEWS figi-gii:hasUniqueTextIdentifier "BEWS" .

figi-ps:GALI a figi-gii:PricingSource .

figi-ps:BEXI a owl:NamedIndividual .

figi-ps:GALI skos:prefLabel "banco de galicia" .

figi-ps:BEXI a figi-gii:PricingSource .

figi-st:dipDelayDrawRev skos:definition "Issued when a company is in bankruptcy. Forward-start deal where borrower is allowed to draw down on the loan in one or more drawings within a specified time period after the signing date." .

figi-ps:BEXI skos:prefLabel "bank ekspor indonesi" .

figi-ps:GALI skos:prefLabel "banco galicia" .

figi-st:dipDelayDrawRev skos:prefLabel "dip delay-draw rev" .

figi-ps:BEXI figi-gii:hasUniqueTextIdentifier "BEXI" .

figi-ps:GALI figi-gii:hasUniqueTextIdentifier "GALI" .

figi-ps:BEXP a owl:NamedIndividual .

figi-st:dipDelayDrawRev figi-gii:hasUniqueTextIdentifier "DIP DELAY-DRAW REV" .

figi-ps:GALN a owl:NamedIndividual .

figi-ps:BEXP a figi-gii:PricingSource .

figi-ps:AFME a owl:NamedIndividual .

figi-ps:GALN a figi-gii:PricingSource .

figi-ps:AFME a figi-gii:PricingSource .

figi-ps:GALN skos:prefLabel "galleon asia" .

figi-ps:AFME skos:prefLabel "afma" .

figi-ps:GALN figi-gii:hasUniqueTextIdentifier "GALN" .

figi-ps:AFME figi-gii:hasUniqueTextIdentifier "AFME" .

figi-ps:GALT a owl:NamedIndividual .

figi-st:dipDelayDrawTerm a owl:NamedIndividual .

figi-ps:GALT a figi-gii:PricingSource .

figi-st:dipDelayDrawTerm a figi-gii:SecurityType .

figi-ps:GALT skos:prefLabel "galt and taggart" ;
	figi-gii:hasUniqueTextIdentifier "GALT" .

figi-st:dipDelayDrawTerm skos:definition "Issued when a company is in bankruptcy. Borrower is allowed to draw down on the loan in one or more drawings within a specified time period after the signing date. Once borrowed, cannot be re-borrowed." .

figi-ps:GAM a owl:NamedIndividual .

figi-st:dipDelayDrawTerm skos:prefLabel "dip delay-draw term" .

figi-ps:GAM a figi-gii:PricingSource .

figi-st:dipDelayDrawTerm figi-gii:hasUniqueTextIdentifier "DIP DELAY-DRAW TERM" .

figi-ps:GAM skos:prefLabel "gam" .

figi-st:dipLoc a owl:NamedIndividual .

figi-ps:GAM figi-gii:hasUniqueTextIdentifier "GAM" .

figi-st:dipLoc a figi-gii:SecurityType .

figi-ps:GAMJ a owl:NamedIndividual , figi-gii:PricingSource .

figi-st:dipLoc skos:definition "Issued when a company is in bankruptcy. Guaranteed by the lender(s) and used for purchase of goods, completion of construction projects, and/or general purposes." .

figi-ps:GAMJ skos:prefLabel "guardian life ltd" .

figi-st:dipLoc skos:prefLabel "dip loc" .

figi-ps:GAMJ figi-gii:hasUniqueTextIdentifier "GAMJ" .

figi-st:dipLoc figi-gii:hasUniqueTextIdentifier "DIP LOC" .

figi-ps:GARI a owl:NamedIndividual .

figi-ps:AFMY a owl:NamedIndividual .

figi-ps:GARI a figi-gii:PricingSource .

figi-ps:AFMY a figi-gii:PricingSource .

figi-ps:GARI skos:prefLabel "icap australia pty" .

figi-ps:AFMY skos:prefLabel "affin money brokers" .

figi-ps:GARI figi-gii:hasUniqueTextIdentifier "GARI" .

figi-ps:AFMY figi-gii:hasUniqueTextIdentifier "AFMY" .

figi-ps:GARL a owl:NamedIndividual .

figi-st:dipPikTerm a owl:NamedIndividual .

figi-ps:GARL a figi-gii:PricingSource .

figi-st:dipPikTerm a figi-gii:SecurityType .

figi-ps:GARL skos:prefLabel "global absolute rsch" .

figi-st:dipPikTerm skos:definition "Issued when a company is in bankruptcy. Interest may be capitalized and added to the principal amount of the loan, which is then compounded and due to lenders at maturity. Once borrowed, cannot be re-borrowed." .

figi-ps:GARL figi-gii:hasUniqueTextIdentifier "GARL" .

figi-st:dipPikTerm skos:prefLabel "dip pik term" ;
	figi-gii:hasUniqueTextIdentifier "DIP PIK TERM" .

figi-ps:GARV a owl:NamedIndividual .

figi-ps:BEXP skos:prefLabel "bond elec exch-price" .

figi-ps:AFSA a owl:NamedIndividual .

figi-ps:GARV a figi-gii:PricingSource .

figi-ps:BEXP figi-gii:hasUniqueTextIdentifier "BEXP" .

figi-ps:AFSA a figi-gii:PricingSource .

figi-ps:GARV skos:prefLabel "garvin info systems" .

figi-ps:BEXS a owl:NamedIndividual .

figi-ps:AFSA skos:prefLabel "afs interest" .

figi-ps:GARV figi-gii:hasUniqueTextIdentifier "GARV" .

figi-ps:BEXS a figi-gii:PricingSource .

figi-ps:AFSA figi-gii:hasUniqueTextIdentifier "AFSA" .

figi-ps:GATS a owl:NamedIndividual .

figi-ps:BEXS skos:prefLabel "belfius bank" .

figi-ps:AGCO a owl:NamedIndividual .

figi-ps:GATS a figi-gii:PricingSource .

figi-ps:AGCO a figi-gii:PricingSource .

figi-ps:BEXS figi-gii:hasUniqueTextIdentifier "BEXS" .

figi-ps:GATS skos:prefLabel "gates capital corp" .

figi-ps:AGCO skos:prefLabel "auerbach grayson inc" .

figi-ps:BEXT a owl:NamedIndividual .

figi-ps:GATS figi-gii:hasUniqueTextIdentifier "GATS" .

figi-ps:BEXT a figi-gii:PricingSource .

figi-ps:GAZP a owl:NamedIndividual .

figi-ps:BEXT skos:prefLabel "banco exterior" .

figi-ps:GAZP a figi-gii:PricingSource .

figi-ps:BEXT skos:prefLabel "belfius bank" .

figi-ps:GAZP skos:prefLabel "gazprom" ;
	figi-gii:hasUniqueTextIdentifier "GAZP" .

figi-ps:AGCO figi-gii:hasUniqueTextIdentifier "AGCO" .

figi-ps:GBAN a owl:NamedIndividual , figi-gii:PricingSource .

figi-st:dipRev a owl:NamedIndividual .

figi-ps:GBAN skos:prefLabel "icap gban treasuries" .

figi-ps:BEXT figi-gii:hasUniqueTextIdentifier "BEXT" .

figi-st:dipRev a figi-gii:SecurityType .

figi-ps:GBAN figi-gii:hasUniqueTextIdentifier "GBAN" .

figi-ps:BEXY a owl:NamedIndividual , figi-gii:PricingSource .

figi-ps:GBCL a owl:NamedIndividual .

figi-ps:BEXY skos:prefLabel "bond elec exch-yield" .

figi-st:dipRev skos:definition "Issued when a company is in bankruptcy. Once borrowed funds are repaid they can be borrowed again." .

figi-ps:GBCL a figi-gii:PricingSource .

figi-ps:BEXY figi-gii:hasUniqueTextIdentifier "BEXY" .

figi-ps:GBCL skos:prefLabel "global coal" .

figi-st:dipRev skos:prefLabel "dip rev" .

figi-ps:BFAA a owl:NamedIndividual .

figi-ps:GBCL figi-gii:hasUniqueTextIdentifier "GBCL" .

figi-ps:BFAA a figi-gii:PricingSource .

figi-st:dipRev figi-gii:hasUniqueTextIdentifier "DIP REV" .

figi-ps:GBEN a owl:NamedIndividual .

figi-ps:BFAA skos:prefLabel "banco fomento angola" .

figi-ps:GBEN a figi-gii:PricingSource .

figi-ps:AGI a owl:NamedIndividual .

figi-ps:BFAA figi-gii:hasUniqueTextIdentifier "BFAA" .

figi-ps:GBEN skos:prefLabel "gaston bengochea" .

figi-ps:AGI a figi-gii:PricingSource .

figi-ps:BFAT a owl:NamedIndividual .

figi-ps:GBEN figi-gii:hasUniqueTextIdentifier "GBEN" .

figi-ps:AGI skos:prefLabel "allianz gi asia pac" .

figi-ps:BFAT a figi-gii:PricingSource .

figi-ps:GBET a owl:NamedIndividual .

figi-ps:AGI skos:prefLabel "allianz global inv" .

figi-ps:BFAT skos:prefLabel "banco fator sa" .

figi-ps:AGI figi-gii:hasUniqueTextIdentifier "AGI" .

figi-ps:BFAT figi-gii:hasUniqueTextIdentifier "BFAT" .

figi-st:dipSynthLoc a owl:NamedIndividual .

figi-ps:GBET a figi-gii:PricingSource .

figi-ps:BFCV a owl:NamedIndividual .

figi-st:dipSynthLoc a figi-gii:SecurityType .

figi-ps:BFCV a figi-gii:PricingSource .

figi-ps:GBET skos:prefLabel "grant bettingen" .

figi-ps:BFCV skos:prefLabel "banco fondo comun" .

figi-ps:GBET figi-gii:hasUniqueTextIdentifier "GBET" .

figi-ps:BFCV figi-gii:hasUniqueTextIdentifier "BFCV" .

figi-st:dipSynthLoc skos:definition "Issued when a company is in bankruptcy. A letter of credit facility which is fully cash collateralized with proceeds of a term loan which has been issued by the same borrower, usually with the same amount and terms." .

figi-ps:GBI a owl:NamedIndividual .

figi-ps:BFDC a owl:NamedIndividual .

figi-ps:GBI a figi-gii:PricingSource .

figi-ps:BFDC a figi-gii:PricingSource .

figi-ps:GBI skos:prefLabel "gesmosa - gbi" .

figi-st:dipSynthLoc skos:prefLabel "dip synth loc" .

figi-ps:GBI figi-gii:hasUniqueTextIdentifier "GBI" .

figi-ps:BFDC skos:prefLabel "bcba floor dc" .

figi-st:dipSynthLoc figi-gii:hasUniqueTextIdentifier "DIP SYNTH LOC" .

figi-ps:BFDC figi-gii:hasUniqueTextIdentifier "BFDC" .

figi-ps:AGIC a owl:NamedIndividual .

figi-ps:BFER a owl:NamedIndividual .

figi-ps:AGIC a figi-gii:PricingSource .

figi-ps:BFER a figi-gii:PricingSource .

figi-ps:AGIC skos:prefLabel "agic-production" .

figi-ps:GBL a owl:NamedIndividual .

figi-ps:BFER skos:prefLabel "barclays loans" .

figi-ps:AGIC figi-gii:hasUniqueTextIdentifier "AGIC" .

figi-ps:BFER figi-gii:hasUniqueTextIdentifier "BFER" .

figi-ps:GBL a figi-gii:PricingSource .

figi-st:dipTerm a owl:NamedIndividual .

figi-ps:GBL skos:prefLabel "banca leonardo" .

figi-ps:BFIB a owl:NamedIndividual .

figi-st:dipTerm a figi-gii:SecurityType .

figi-ps:BFIB a figi-gii:PricingSource .

figi-ps:GBL figi-gii:hasUniqueTextIdentifier "GBL" .

figi-ps:BFIB skos:prefLabel "banco fibra" .

figi-st:dipTerm skos:definition "Issued when a company is in bankruptcy. Once borrowed, cannot be re-borrowed." .

figi-ps:GBLN a owl:NamedIndividual .

figi-ps:BFIB figi-gii:hasUniqueTextIdentifier "BFIB" .

figi-st:dipTerm skos:prefLabel "dip term" .

figi-ps:GBLN a figi-gii:PricingSource .

figi-ps:BFIS a owl:NamedIndividual .

figi-st:dipTerm figi-gii:hasUniqueTextIdentifier "DIP TERM" .

figi-ps:GBLN skos:prefLabel "banca leonardo" .

figi-ps:BFIS a figi-gii:PricingSource .

figi-ps:AGIT a owl:NamedIndividual .

figi-ps:GBLN figi-gii:hasUniqueTextIdentifier "GBLN" .

figi-ps:BFIS skos:prefLabel "bank for intl stlmnt" .

figi-ps:GBMI a owl:NamedIndividual .

figi-ps:BFIS figi-gii:hasUniqueTextIdentifier "BFIS" .

figi-ps:GBMI a figi-gii:PricingSource .

figi-ps:AGIT a figi-gii:PricingSource .

figi-ps:GBMI skos:prefLabel "gbm grupo bursatil" .

figi-ps:BFJP a owl:NamedIndividual .

figi-ps:GBMI figi-gii:hasUniqueTextIdentifier "GBMI" .

figi-ps:AGIT skos:prefLabel "agi parallel" .

figi-ps:BFJP a figi-gii:PricingSource .

figi-ps:GBMM a owl:NamedIndividual .

figi-ps:AGIT figi-gii:hasUniqueTextIdentifier "AGIT" .

figi-ps:GBMM a figi-gii:PricingSource .

figi-ps:BFJP skos:prefLabel "bfv japan 3pm px" .

figi-st:discountFixbis a owl:NamedIndividual .

figi-ps:BFJP figi-gii:hasUniqueTextIdentifier "BFJP" .

figi-ps:GBMM skos:prefLabel "gbm mexico" .

figi-st:discountFixbis a figi-gii:SecurityType .

figi-ps:BFMD a owl:NamedIndividual .

figi-ps:GBMM figi-gii:hasUniqueTextIdentifier "GBMM" .

figi-st:discountFixbis skos:definition "Bank of Intl Settlement Discount Notes / Discount Rate" .

figi-ps:BFMD a figi-gii:PricingSource .

figi-ps:GBOA a owl:NamedIndividual .

figi-st:discountFixbis skos:prefLabel "discount fixbis" .

figi-ps:BFMD skos:prefLabel "bvf india illiquid" .

figi-ps:GBOA a figi-gii:PricingSource .

figi-st:discountFixbis figi-gii:hasUniqueTextIdentifier "DISCOUNT FIXBIS" .

figi-ps:BFMD figi-gii:hasUniqueTextIdentifier "BFMD" .

figi-ps:GBOA skos:prefLabel "bancofamerica - gold" .

figi-ps:AGLA a owl:NamedIndividual .

figi-ps:BFRA a owl:NamedIndividual .

figi-ps:GBOA figi-gii:hasUniqueTextIdentifier "GBOA" .

figi-ps:AGLA a figi-gii:PricingSource .

figi-ps:BFRA a figi-gii:PricingSource .

figi-ps:GBUY a owl:NamedIndividual .

figi-ps:AGLA skos:prefLabel "agl energy ltd" .

figi-ps:BFRA skos:prefLabel "banco frances" .

figi-ps:GBUY a figi-gii:PricingSource .

figi-ps:AGLA figi-gii:hasUniqueTextIdentifier "AGLA" .

figi-ps:BFRA figi-gii:hasUniqueTextIdentifier "BFRA" .

figi-ps:GBUY skos:prefLabel "gbu soc de bolsa" .

figi-st:discountNotes a owl:NamedIndividual .

figi-ps:BFRU a owl:NamedIndividual .

figi-ps:GBUY figi-gii:hasUniqueTextIdentifier "GBUY" .

figi-ps:BFRU a figi-gii:PricingSource .

figi-st:discountNotes a figi-gii:SecurityType .

figi-ps:GC a owl:NamedIndividual .

figi-ps:BFRU skos:prefLabel "banco frances (usd)" .

figi-ps:GC a figi-gii:PricingSource .

figi-ps:BFRU figi-gii:hasUniqueTextIdentifier "BFRU" .

figi-ps:GC skos:prefLabel "gracie capital" .

figi-st:discountNotes skos:definition "Discount Notes - Short-term issues with no fixed offering schedule which are sold in $100,000 denominations with maturities of 30 to 270 days. Such notes are sold without government guarantees." .

figi-ps:BFSA a owl:NamedIndividual .

figi-ps:GC figi-gii:hasUniqueTextIdentifier "GC" .

figi-st:discountNotes skos:prefLabel "discount notes" .

figi-ps:BFSA a figi-gii:PricingSource .

figi-ps:GCAP a owl:NamedIndividual .

figi-st:discountNotes figi-gii:hasUniqueTextIdentifier "DISCOUNT NOTES" .

figi-ps:BFSA skos:prefLabel "business flyer" .

figi-ps:GCAP a figi-gii:PricingSource .

figi-ps:BFSA figi-gii:hasUniqueTextIdentifier "BFSA" .

figi-ps:AGOR a owl:NamedIndividual , figi-gii:PricingSource .

figi-ps:GCAP skos:prefLabel "greenwich cap" .

figi-ps:BFSU a owl:NamedIndividual .

figi-ps:AGOR skos:prefLabel "agora ctvm sa" .

figi-ps:BFSU a figi-gii:PricingSource .

figi-ps:AGOR figi-gii:hasUniqueTextIdentifier "AGOR" .

figi-ps:BFSU skos:prefLabel "banco finansur" .

figi-ps:GCAP figi-gii:hasUniqueTextIdentifier "GCAP" .

figi-st:dividendNeutralStockFuture a owl:NamedIndividual .

figi-ps:BFSU figi-gii:hasUniqueTextIdentifier "BFSU" .

figi-st:dividendNeutralStockFuture a figi-gii:SecurityType .

figi-ps:GCAT a owl:NamedIndividual .

figi-ps:BFUA a owl:NamedIndividual .

figi-ps:GCAT a figi-gii:PricingSource .

figi-ps:BFUA a figi-gii:PricingSource .

figi-ps:GCAT skos:prefLabel "comunidad autonoma" .

figi-ps:BFUA skos:prefLabel "bank forum" ;
	figi-gii:hasUniqueTextIdentifier "BFUA" .

figi-ps:GCAT figi-gii:hasUniqueTextIdentifier "GCAT" .

figi-st:dividendNeutralStockFuture skos:definition "Dividend Neutral Stock Futures (DNSF) are derivative instruments that give investors exposure to price movements of an underlying financial instrument (shares). A DNSF is a basket of two futures contracts, constructed from a Single Stock Futures Contract and a Dividend Futures Contract." .

figi-ps:BFUD a owl:NamedIndividual .

figi-ps:GCBF a owl:NamedIndividual .

figi-st:dividendNeutralStockFuture skos:prefLabel "dividend neutral stock future" .

figi-ps:GCBF a figi-gii:PricingSource .

figi-st:dividendNeutralStockFuture figi-gii:hasUniqueTextIdentifier "DIVIDEND NEUTRAL STOCK FUTURE" .

figi-ps:GCBF skos:prefLabel "holinger asset man." .

figi-ps:BFUD a figi-gii:PricingSource .

figi-ps:GCBF figi-gii:hasUniqueTextIdentifier "GCBF" .

figi-ps:AGRC a owl:NamedIndividual .

figi-ps:BFUD skos:prefLabel "finansur (us dollar)" .

figi-ps:GCCL a owl:NamedIndividual .

figi-ps:AGRC a figi-gii:PricingSource .

figi-ps:GCCL a figi-gii:PricingSource .

figi-ps:BFUD figi-gii:hasUniqueTextIdentifier "BFUD" .

figi-ps:AGRC skos:prefLabel "auerbach grayson" .

figi-ps:GCCL skos:prefLabel "global crown capital" .

figi-ps:BFUS a owl:NamedIndividual .

figi-ps:AGRC figi-gii:hasUniqueTextIdentifier "AGRC" .

figi-ps:GCCL figi-gii:hasUniqueTextIdentifier "GCCL" .

figi-ps:BFUS a figi-gii:PricingSource .

figi-st:domestcTimeDep a owl:NamedIndividual .

figi-ps:BFUS skos:prefLabel "bcba floor us" .

figi-ps:GCER a owl:NamedIndividual .

figi-st:domestcTimeDep a figi-gii:SecurityType .

figi-ps:GCER a figi-gii:PricingSource .

figi-ps:BFUS figi-gii:hasUniqueTextIdentifier "BFUS" .

figi-ps:GCER skos:prefLabel "gcr capital gmbh" ;
	figi-gii:hasUniqueTextIdentifier "GCER" .

figi-ps:BFV a owl:NamedIndividual , figi-gii:PricingSource .

figi-ps:GCHK a owl:NamedIndividual , figi-gii:PricingSource .

figi-ps:BFV skos:prefLabel "bloomberg fair value" .

figi-st:domestcTimeDep skos:definition "Time Deposit. A deposit in an interest-paying account that requires the money to remain on account for a specific length of time. While withdrawals can generally be made from a passbook account at any time, other time deposits, such as certificates of deposit, are penalized for early withdrawal." .

figi-ps:GCHK skos:prefLabel "grand cathay (hk)" ;
	figi-gii:hasUniqueTextIdentifier "GCHK" .

figi-st:domestcTimeDep skos:prefLabel "domestc time dep" .

figi-ps:GCM a owl:NamedIndividual , figi-gii:PricingSource .

figi-st:domestcTimeDep figi-gii:hasUniqueTextIdentifier "DOMESTC TIME DEP" .

figi-ps:GCM skos:prefLabel "greenwich cap mkts" .

figi-ps:BFV figi-gii:hasUniqueTextIdentifier "BFV" .

figi-ps:GCM figi-gii:hasUniqueTextIdentifier "GCM" .

figi-ps:AGRI a owl:NamedIndividual .

figi-ps:GCMA a owl:NamedIndividual .

figi-ps:BFVI a owl:NamedIndividual .

figi-ps:GCMA a figi-gii:PricingSource .

figi-ps:AGRI a figi-gii:PricingSource .

figi-ps:BFVI a figi-gii:PricingSource .

figi-ps:GCMA skos:prefLabel "greenwich cap mkts" .

figi-ps:AGRI skos:prefLabel "cfet agricultural bk" .

figi-ps:BFVI skos:prefLabel "bfv india" .

figi-ps:GCMA figi-gii:hasUniqueTextIdentifier "GCMA" .

figi-ps:BFVI figi-gii:hasUniqueTextIdentifier "BFVI" .

figi-ps:AGRI figi-gii:hasUniqueTextIdentifier "AGRI" .

figi-ps:GCMB a owl:NamedIndividual .

figi-ps:BFVJ a owl:NamedIndividual .

figi-ps:GCMB a figi-gii:PricingSource .

figi-ps:AGRN a owl:NamedIndividual .

figi-ps:BFVJ a figi-gii:PricingSource .

figi-ps:GCMB skos:prefLabel "greenwich cap mkts" .

figi-ps:AGRN a figi-gii:PricingSource .

figi-ps:BFVJ skos:prefLabel "bfv japan 3pm" .

figi-ps:GCMB skos:prefLabel "rbsmarketplace us" .

figi-ps:AGRN skos:prefLabel "cnbond aboc" .

figi-ps:BFVJ figi-gii:hasUniqueTextIdentifier "BFVJ" .

figi-ps:AGRN figi-gii:hasUniqueTextIdentifier "AGRN" .

figi-ps:BFVS a owl:NamedIndividual .

figi-ps:GCMB figi-gii:hasUniqueTextIdentifier "GCMB" .

figi-ps:BFVS a figi-gii:PricingSource .

figi-st:domestic a owl:NamedIndividual .

figi-ps:GCMT a owl:NamedIndividual .

figi-ps:BFVS skos:prefLabel "bfv singapore" .

figi-st:domestic a figi-gii:SecurityType .

figi-ps:GCMT a figi-gii:PricingSource .

figi-ps:BFVS figi-gii:hasUniqueTextIdentifier "BFVS" .

figi-ps:GCMT skos:prefLabel "greenwich capital mk" .

figi-st:domestic skos:definition "A security issued into a country's domestic market" .

figi-ps:BGC a owl:NamedIndividual .

figi-ps:GCMT figi-gii:hasUniqueTextIdentifier "GCMT" .

figi-st:domestic skos:prefLabel "domestic" .

figi-ps:GCNI a owl:NamedIndividual .

figi-st:domestic figi-gii:hasUniqueTextIdentifier "DOMESTIC" .

figi-ps:GCNI a figi-gii:PricingSource .

figi-ps:BGC a figi-gii:PricingSource .

figi-ps:GCNI skos:prefLabel "global crown cap" .

figi-ps:AGSC a owl:NamedIndividual .

figi-ps:GCNI figi-gii:hasUniqueTextIdentifier "GCNI" .

figi-ps:BGC skos:prefLabel "bgc capital markets" .

figi-ps:AGSC a figi-gii:PricingSource .

figi-ps:GCRC a owl:NamedIndividual .

figi-ps:BGC figi-gii:hasUniqueTextIdentifier "BGC" .

figi-ps:GCRC a figi-gii:PricingSource .

figi-ps:AGSC skos:prefLabel "ags capital markets" .

figi-ps:GCRC skos:prefLabel "gcr capital gmbh" .

figi-ps:BGCF a owl:NamedIndividual .

figi-ps:AGSC figi-gii:hasUniqueTextIdentifier "AGSC" .

figi-ps:GCRC figi-gii:hasUniqueTextIdentifier "GCRC" .

figi-ps:BGCF a figi-gii:PricingSource .

figi-st:domesticMtn a owl:NamedIndividual .

figi-ps:GCRE a owl:NamedIndividual .

figi-ps:BGCF skos:prefLabel "bgc financial lp" .

figi-ps:GCRE a figi-gii:PricingSource .

figi-st:domesticMtn a figi-gii:SecurityType .

figi-ps:BGCF figi-gii:hasUniqueTextIdentifier "BGCF" .

figi-ps:GCRE skos:prefLabel "general cologne re" .

figi-st:domesticMtn skos:definition "A medium term note issued into a country's domestic market." .

figi-ps:GCRE figi-gii:hasUniqueTextIdentifier "GCRE" .

figi-ps:BGCL a owl:NamedIndividual .

figi-st:domesticMtn skos:prefLabel "domestic mtn" .

figi-ps:GCS a owl:NamedIndividual .

figi-ps:BGCL a figi-gii:PricingSource .

figi-st:domesticMtn figi-gii:hasUniqueTextIdentifier "DOMESTIC MTN" .

figi-ps:GCS a figi-gii:PricingSource .

figi-ps:BGCL skos:prefLabel "birch grove capital" .

figi-ps:AGTT a owl:NamedIndividual .

figi-ps:GCS skos:prefLabel "grand cathay holding" .

figi-ps:BGCL figi-gii:hasUniqueTextIdentifier "BGCL" .

figi-ps:AGTT a figi-gii:PricingSource .

figi-ps:GCS figi-gii:hasUniqueTextIdentifier "GCS" .

figi-ps:BGCO a owl:NamedIndividual .

figi-ps:AGTT skos:prefLabel "agtradertalk" .

figi-ps:GCTB a owl:NamedIndividual .

figi-ps:BGCO a figi-gii:PricingSource .

figi-ps:AGTT figi-gii:hasUniqueTextIdentifier "AGTT" .

figi-ps:GCTB a figi-gii:PricingSource .

figi-ps:BGCO skos:prefLabel "bryan garnierandco ltd" .

figi-ps:AHLI a owl:NamedIndividual .

figi-ps:BGCO figi-gii:hasUniqueTextIdentifier "BGCO" .

figi-ps:AHLI a figi-gii:PricingSource .

figi-ps:BGCT a owl:NamedIndividual .

figi-ps:GCTB skos:prefLabel "greenwich capital mk" .

figi-ps:BGCT a figi-gii:PricingSource .

figi-ps:AHLI skos:prefLabel "al ahli bank" .

figi-ps:GCTB skos:prefLabel "rbs mtge" .

figi-ps:BGCT skos:prefLabel "bgc partner turkey" .

figi-ps:AHLI skos:prefLabel "al ahli bank qatar" .

figi-ps:GCTB figi-gii:hasUniqueTextIdentifier "GCTB" .

figi-ps:BGCT figi-gii:hasUniqueTextIdentifier "BGCT" .

figi-ps:AHLI figi-gii:hasUniqueTextIdentifier "AHLI" .

figi-ps:GDBK a owl:NamedIndividual .

figi-ps:BGDB a owl:NamedIndividual .

figi-st:dutchCP a owl:NamedIndividual .

figi-ps:GDBK a figi-gii:PricingSource .

figi-ps:BGDB a figi-gii:PricingSource .

figi-st:dutchCP a figi-gii:SecurityType .

figi-ps:GDBK skos:prefLabel "guangdong dvlpmnt bk" .

figi-ps:BGDB skos:prefLabel "banco ganadero" .

figi-ps:GDBK figi-gii:hasUniqueTextIdentifier "GDBK" .

figi-ps:BGDB figi-gii:hasUniqueTextIdentifier "BGDB" .

figi-ps:GDFS a owl:NamedIndividual .

figi-ps:BGEN a owl:NamedIndividual .

figi-ps:GDFS a figi-gii:PricingSource .

figi-ps:BGEN a figi-gii:PricingSource .

figi-ps:GDFS skos:prefLabel "gdf suez" .

figi-ps:BGEN skos:prefLabel "banco general" .

figi-st:dutchCP skos:definition "Commercial Paper. An unsecured short-term promise to repay a fixed amount on a certain future date. Commercial paper usually matures from 2 to 270 days and is traded on a discount basis. This debt instrument, issued by banks, companies and other borrowers, use only their credit ratings to back the security. Commercial Paper House. A dealer who buys commercial paper at one price, then tries to sell it at another. - DUTCH GUILDER" .

figi-ps:GDFS figi-gii:hasUniqueTextIdentifier "GDFS" .

figi-ps:BGEN figi-gii:hasUniqueTextIdentifier "BGEN" .

figi-st:dutchCP skos:prefLabel "dutch cp" .

figi-ps:GDMA a owl:NamedIndividual .

figi-ps:BGIS a owl:NamedIndividual .

figi-st:dutchCP figi-gii:hasUniqueTextIdentifier "DUTCH CP" .

figi-ps:GDMA a figi-gii:PricingSource .

figi-ps:BGIS a figi-gii:PricingSource .

figi-ps:AHS a owl:NamedIndividual .

figi-ps:GDMA skos:prefLabel "govt debt management" .

figi-ps:BGIS skos:prefLabel "blackrock exec srvcs" .

figi-ps:AHS a figi-gii:PricingSource .

figi-ps:GDMA figi-gii:hasUniqueTextIdentifier "GDMA" .

figi-ps:BGIS figi-gii:hasUniqueTextIdentifier "BGIS" .

figi-ps:AHS skos:prefLabel "adventist health sys" .

figi-ps:GDMS a owl:NamedIndividual .

figi-ps:BGIX a owl:NamedIndividual .

figi-ps:AHS figi-gii:hasUniqueTextIdentifier "AHS" .

figi-ps:BGIX a figi-gii:PricingSource .

figi-ps:GDMS a figi-gii:PricingSource .

figi-ps:AHWK a owl:NamedIndividual .

figi-ps:BGIX skos:prefLabel "bgi index" .

figi-ps:GDMS skos:prefLabel "goldman muni spread" .

figi-ps:AHWK a figi-gii:PricingSource .

figi-ps:BGIX figi-gii:hasUniqueTextIdentifier "BGIX" .

figi-ps:GDMS figi-gii:hasUniqueTextIdentifier "GDMS" .

figi-ps:AHWK skos:prefLabel "arrowhawk capital" .

figi-ps:BGJM a owl:NamedIndividual .

figi-ps:GDMY a owl:NamedIndividual .

figi-ps:AHWK figi-gii:hasUniqueTextIdentifier "AHWK" .

figi-ps:GDMY a figi-gii:PricingSource .

figi-ps:BGJM a figi-gii:PricingSource .

figi-st:dutchCert a owl:NamedIndividual .

figi-ps:GDMY skos:prefLabel "goldman s muni yield" .

figi-ps:BGJM skos:prefLabel "bgn mat jpn m-t-m" .

figi-st:dutchCert a figi-gii:SecurityType .

figi-ps:GDMY figi-gii:hasUniqueTextIdentifier "GDMY" .

figi-ps:BGJM figi-gii:hasUniqueTextIdentifier "BGJM" .

figi-ps:GDNR a owl:NamedIndividual , figi-gii:PricingSource .

figi-ps:BGJP a owl:NamedIndividual .

figi-ps:GDNR skos:prefLabel "gardner rich and co" .

figi-ps:BGJP a figi-gii:PricingSource .

figi-st:dutchCert skos:definition "Certificaten Van Aandelen. Netherland securities in the form of bearer certificates, issued by an administration office against the underlying original, mostly registered shares. The office acts as a trustee for the holders of the certificate and exercises voting rights on the shares." .

figi-ps:BGJP skos:prefLabel "bgn japan 5pm px" .

figi-ps:GDNR figi-gii:hasUniqueTextIdentifier "GDNR" .

figi-st:dutchCert skos:prefLabel "dutch cert" .

figi-ps:BGJP figi-gii:hasUniqueTextIdentifier "BGJP" .

figi-ps:GDPG a owl:NamedIndividual .

figi-st:dutchCert figi-gii:hasUniqueTextIdentifier "Dutch Cert" .

figi-ps:GDPG a figi-gii:PricingSource .

figi-ps:BGKR a owl:NamedIndividual .

figi-ps:AIAB a owl:NamedIndividual .

figi-ps:BGKR a figi-gii:PricingSource .

figi-ps:GDPG skos:prefLabel "gest di patrimoni" .

figi-ps:AIAB a figi-gii:PricingSource .

figi-ps:BGKR skos:prefLabel "bgc capital korea" .

figi-ps:GDPG figi-gii:hasUniqueTextIdentifier "GDPG" .

figi-ps:AIAB skos:prefLabel "aia co ltd" .

figi-ps:BGKR figi-gii:hasUniqueTextIdentifier "BGKR" .

figi-ps:AIAB figi-gii:hasUniqueTextIdentifier "AIAB" .

figi-ps:GDSB a owl:NamedIndividual .

figi-ps:BGL a owl:NamedIndividual .

figi-st:edr a owl:NamedIndividual .

figi-ps:GDSB a figi-gii:PricingSource .

figi-st:edr a figi-gii:SecurityType .

figi-ps:GDSB skos:prefLabel "aib" .

figi-ps:BGL a figi-gii:PricingSource .

figi-ps:GDSB figi-gii:hasUniqueTextIdentifier "GDSB" .

figi-ps:BGL skos:prefLabel "banq generale lux" ;
	figi-gii:hasUniqueTextIdentifier "BGL" .

figi-ps:GDSS a owl:NamedIndividual .

figi-st:edr skos:definition "European Depository Receipt. A document issued in place of stock shares that represents ownership of the shares, thus making it easier to deal in foreign securities because the actual stock certificates do not have to be physically transferred." .

figi-ps:GDSS a figi-gii:PricingSource .

figi-ps:BGLB a owl:NamedIndividual .

figi-st:edr skos:prefLabel "edr" .

figi-ps:BGLB a figi-gii:PricingSource .

figi-ps:GDSS skos:prefLabel "gateway demo-sseoms" .

figi-st:edr figi-gii:hasUniqueTextIdentifier "EDR" .

figi-ps:BGLB skos:prefLabel "bgl bnp paribas lux" .

figi-ps:AIAF a owl:NamedIndividual .

figi-ps:BGLB figi-gii:hasUniqueTextIdentifier "BGLB" .

figi-ps:AIAF a figi-gii:PricingSource .

figi-ps:BGLC a owl:NamedIndividual .

figi-ps:AIAF skos:prefLabel "aiaf" .

figi-ps:BGLC a figi-gii:PricingSource .

figi-ps:AIAF figi-gii:hasUniqueTextIdentifier "AIAF" .

figi-ps:GDSS figi-gii:hasUniqueTextIdentifier "GDSS" .

figi-ps:BGLC skos:prefLabel "bgc international" .

figi-ps:AIAP a owl:NamedIndividual .

figi-ps:GE a owl:NamedIndividual .

figi-ps:BGLC figi-gii:hasUniqueTextIdentifier "BGLC" .

figi-ps:AIAP a figi-gii:PricingSource .

figi-ps:GE a figi-gii:PricingSource .

figi-ps:BGLL a owl:NamedIndividual .

figi-ps:AIAP skos:prefLabel "aiaf bond (price)" .

figi-ps:BGLL a figi-gii:PricingSource .

figi-ps:GE skos:prefLabel "general electric" .

figi-ps:AIAP figi-gii:hasUniqueTextIdentifier "AIAP" .

figi-ps:BGLL skos:prefLabel "bgl societe anonyme" .

figi-ps:GE figi-gii:hasUniqueTextIdentifier "GE" .

figi-st:equityIndex a owl:NamedIndividual .

figi-ps:BGLL figi-gii:hasUniqueTextIdentifier "BGLL" .

figi-st:equityIndex a figi-gii:SecurityType .

figi-ps:GEBP a owl:NamedIndividual .

figi-ps:BGMA a owl:NamedIndividual .

figi-ps:GEBP a figi-gii:PricingSource .

figi-ps:BGMA a figi-gii:PricingSource .

figi-st:equityIndex skos:definition "Statistical movement of the stock market as represented by a basket of stocks." .

figi-ps:GEBP skos:prefLabel "gazenergoprombank" .

figi-ps:BGMA skos:prefLabel "bankhaus gebr.martin" .

figi-st:equityIndex skos:prefLabel "equity index" .

figi-ps:BGMA figi-gii:hasUniqueTextIdentifier "BGMA" .

figi-ps:GEBP figi-gii:hasUniqueTextIdentifier "GEBP" .

figi-st:equityIndex figi-gii:hasUniqueTextIdentifier "Equity Index" .

figi-ps:BGMP a owl:NamedIndividual .

figi-ps:AIBT a owl:NamedIndividual .

figi-ps:BGMP a figi-gii:PricingSource .

figi-ps:GEDD a owl:NamedIndividual .

figi-ps:AIBT a figi-gii:PricingSource .

figi-ps:BGMP skos:prefLabel "bgn jpn m-t-m px" .

figi-ps:AIBT skos:prefLabel "aib group treasury" .

figi-ps:BGMP figi-gii:hasUniqueTextIdentifier "BGMP" .

figi-ps:AIBT figi-gii:hasUniqueTextIdentifier "AIBT" .

figi-ps:BGN a owl:NamedIndividual .

figi-ps:AIDI a owl:NamedIndividual .

figi-ps:BGN a figi-gii:PricingSource .

figi-ps:AIDI a figi-gii:PricingSource .

figi-ps:BGN skos:prefLabel "bloomberg generic" .

figi-ps:GEDD a figi-gii:PricingSource .

figi-ps:AIDI skos:prefLabel "arab int'l dev corp" .

figi-ps:BGN figi-gii:hasUniqueTextIdentifier "BGN" .

figi-ps:AIDI figi-gii:hasUniqueTextIdentifier "AIDI" .

figi-ps:BGN3 a owl:NamedIndividual .

figi-st:equityOption a owl:NamedIndividual .

figi-ps:BGN3 a figi-gii:PricingSource .

figi-st:equityOption a figi-gii:SecurityType .

figi-ps:BGN3 skos:prefLabel "bgn 3pm close" .

figi-ps:GEDD skos:prefLabel "abn amro-rbs gedd" .

figi-st:equityOption skos:definition "Option. A contract that provides the right, but not the obligation, to buy or sell a specific amount of a specific security within a predetermined time period. A call option provides the right to buy 100 shares of the underlying security.A put option provides the right to sell 100 shares of theunderlying security. The seller of the contracts is called the writer. Bloomberg abbreviates option as OPT." .

figi-ps:BGN3 figi-gii:hasUniqueTextIdentifier "BGN3" .

figi-ps:GEDD figi-gii:hasUniqueTextIdentifier "GEDD" .

figi-st:equityOption skos:prefLabel "equity option" .

figi-ps:BGNC a owl:NamedIndividual .

figi-st:equityOption figi-gii:hasUniqueTextIdentifier "Equity Option" .

figi-ps:GEL a owl:NamedIndividual .

figi-ps:BGNC a figi-gii:PricingSource .

figi-ps:AIG a owl:NamedIndividual .

figi-ps:GEL a figi-gii:PricingSource .

figi-ps:AIG a figi-gii:PricingSource .

figi-ps:BGNC skos:prefLabel "bgn china" .

figi-ps:GEL skos:prefLabel "great eastern life" .

figi-ps:BGNC figi-gii:hasUniqueTextIdentifier "BGNC" .

figi-ps:AIG skos:prefLabel "aig global inv" .

figi-ps:GEL figi-gii:hasUniqueTextIdentifier "GEL" .

figi-ps:BGNI a owl:NamedIndividual .

figi-ps:AIG figi-gii:hasUniqueTextIdentifier "AIG" .

figi-ps:GEMB a owl:NamedIndividual .

figi-ps:BGNI a figi-gii:PricingSource .

figi-ps:AIGA a owl:NamedIndividual .

figi-ps:GEMB a figi-gii:PricingSource .

figi-ps:BGNI skos:prefLabel "bbrg generic india" .

figi-ps:AIGA a figi-gii:PricingSource .

figi-ps:GEMB skos:prefLabel "galloway emerging mk" .

figi-ps:BGNI figi-gii:hasUniqueTextIdentifier "BGNI" .

figi-ps:AIGA skos:prefLabel "aig-amb" .

figi-ps:GEMB figi-gii:hasUniqueTextIdentifier "GEMB" .

figi-ps:BGNJ a owl:NamedIndividual .

figi-ps:AIGA figi-gii:hasUniqueTextIdentifier "AIGA" .

figi-ps:BGNJ a figi-gii:PricingSource .

figi-ps:GEMM a owl:NamedIndividual .

figi-ps:BGNJ skos:prefLabel "bgn japan 3pm" .

figi-st:equityOtcOption a owl:NamedIndividual .

figi-ps:BGNJ figi-gii:hasUniqueTextIdentifier "BGNJ" .

figi-st:equityOtcOption a figi-gii:SecurityType .

figi-ps:GEMM a figi-gii:PricingSource .

figi-ps:BGNN a owl:NamedIndividual , figi-gii:PricingSource .

figi-ps:GEMM skos:prefLabel "dmo - gemma pricing" .

figi-ps:BGNN skos:prefLabel "bgn indonesia" .

figi-st:equityOtcOption skos:definition "Over The Counter Option on an Equity. Exchange-traded options (also called listed options) are a class of exchange-traded derivatives. Exchange traded options have standardized contracts, and are settled through a clearing house with fulfillment guaranteed by the credit of the exchange. Since the contracts are standardized, accurate pricing models are often available." .

figi-ps:BGNN figi-gii:hasUniqueTextIdentifier "BGNN" .

figi-ps:GEMM figi-gii:hasUniqueTextIdentifier "GEMM" .

figi-st:equityOtcOption skos:prefLabel "equity otc option" .

figi-ps:BGNS a owl:NamedIndividual .

figi-ps:GENE a owl:NamedIndividual .

figi-st:equityOtcOption figi-gii:hasUniqueTextIdentifier "Equity OTC Option" .

figi-ps:BGNS a figi-gii:PricingSource .

figi-ps:GENE a figi-gii:PricingSource .

figi-ps:AIGI a owl:NamedIndividual .

figi-ps:BGNS skos:prefLabel "bgn singapore" .

figi-ps:AIGI a figi-gii:PricingSource .

figi-ps:GENE skos:prefLabel "generali asset mgt" .

figi-ps:AIGI skos:prefLabel "aiggic (asia) ltd" .

figi-ps:BGNS figi-gii:hasUniqueTextIdentifier "BGNS" .

figi-ps:AIGI figi-gii:hasUniqueTextIdentifier "AIGI" .

figi-ps:GENE figi-gii:hasUniqueTextIdentifier "GENE" .

figi-ps:BGNT a owl:NamedIndividual .

figi-ps:AIGO a owl:NamedIndividual .

figi-ps:BGNT a figi-gii:PricingSource .

figi-ps:AIGO a figi-gii:PricingSource .

figi-ps:GENM a owl:NamedIndividual .

figi-ps:BGNT skos:prefLabel "bgn - test source" .

figi-ps:AIGO skos:prefLabel "banque aig" .

figi-ps:GENM a figi-gii:PricingSource .

figi-ps:AIGO figi-gii:hasUniqueTextIdentifier "AIGO" .

figi-ps:BGNT figi-gii:hasUniqueTextIdentifier "BGNT" .

figi-st:equityWrt a owl:NamedIndividual .

figi-ps:GENM skos:prefLabel "general motors accep" .

figi-ps:BGT2 a owl:NamedIndividual .

figi-st:equityWrt a figi-gii:SecurityType .

figi-ps:GENM figi-gii:hasUniqueTextIdentifier "GENM" .

figi-st:equityWrt skos:definition "Indicates that the underlying is an equity" .

figi-ps:BGT2 a figi-gii:PricingSource .

figi-ps:GEO a owl:NamedIndividual .

figi-st:equityWrt skos:prefLabel "equity wrt" .

figi-ps:BGT2 skos:prefLabel "bgc ust level 2" .

figi-st:equityWrt figi-gii:hasUniqueTextIdentifier "Equity WRT" .

figi-ps:GEO a figi-gii:PricingSource .

figi-ps:BGT2 figi-gii:hasUniqueTextIdentifier "BGT2" .

figi-st:etp a owl:NamedIndividual .

figi-ps:GEO skos:prefLabel "geologic resource" .

figi-ps:BGZW a owl:NamedIndividual .

figi-st:etp a figi-gii:SecurityType .

figi-ps:GEO figi-gii:hasUniqueTextIdentifier "GEO" .

figi-ps:BGZW a figi-gii:PricingSource .

figi-ps:GEPB a owl:NamedIndividual .

figi-ps:BGZW skos:prefLabel "bank gospodarki oddl" .

figi-st:etp skos:definition "Exchange Traded Product is a derivatively-priced security which trades intra-day on a national stock exchange. ETPs are typically benchmarked to indices, stocks, commodities, or may be actively managed." .

figi-ps:GEPB a figi-gii:PricingSource .

figi-st:etp skos:prefLabel "etp" .

figi-ps:BGZW figi-gii:hasUniqueTextIdentifier "BGZW" .

figi-st:etp figi-gii:hasUniqueTextIdentifier "ETP" .

figi-ps:GEPB skos:prefLabel "gazenergoprombank" .

figi-st:euroCD a owl:NamedIndividual .

figi-ps:BH a owl:NamedIndividual .

figi-st:euroCD a figi-gii:SecurityType .

figi-ps:GEPB figi-gii:hasUniqueTextIdentifier "GEPB" .

figi-ps:BH a figi-gii:PricingSource .

figi-st:euroCD skos:definition "Eurodollar Certificate of Deposit. A certificate of deposit issued by a bank outside the United States, with interest and principal paid in dollars." .

figi-ps:GERM a owl:NamedIndividual .

figi-ps:BH skos:prefLabel "butler securities" .

figi-ps:GERM a figi-gii:PricingSource .

figi-st:euroCD skos:prefLabel "euro cd" .

figi-ps:BH figi-gii:hasUniqueTextIdentifier "BH" .

figi-st:euroCD figi-gii:hasUniqueTextIdentifier "EURO CD" .

figi-ps:GERM skos:prefLabel "german exchange" .

figi-ps:BHCB a owl:NamedIndividual .

figi-st:euroCP a owl:NamedIndividual .

figi-ps:GERM figi-gii:hasUniqueTextIdentifier "GERM" .

figi-st:euroCP a figi-gii:SecurityType .

figi-ps:BHCB a figi-gii:PricingSource .

figi-st:euroCP skos:definition "Euro Commercial Paper" .

figi-ps:GES a owl:NamedIndividual .

figi-st:euroCP skos:prefLabel "euro cp" .

figi-ps:GES a figi-gii:PricingSource .

figi-st:euroCP figi-gii:hasUniqueTextIdentifier "EURO CP" .

figi-ps:GES skos:prefLabel "gestielle" .

figi-ps:AIGU a owl:NamedIndividual .

figi-ps:BHCB skos:prefLabel "boci securities" .

figi-ps:GES figi-gii:hasUniqueTextIdentifier "GES" .

figi-ps:AIGU a figi-gii:PricingSource .

figi-ps:BHCB figi-gii:hasUniqueTextIdentifier "BHCB" .

figi-ps:GES2 a owl:NamedIndividual .

figi-ps:AIGU skos:prefLabel "aig fin. securities" .

figi-ps:BHER a owl:NamedIndividual .

figi-ps:GES2 a figi-gii:PricingSource .

figi-ps:BHER a figi-gii:PricingSource .

figi-ps:AIGU figi-gii:hasUniqueTextIdentifier "AIGU" .

figi-ps:GES2 skos:prefLabel "gesmosa-gbi 2" .

figi-ps:BHER skos:prefLabel "banque heritage" .

figi-st:euroDollar a owl:NamedIndividual .

figi-ps:GES2 figi-gii:hasUniqueTextIdentifier "GES2" .

figi-ps:BHER figi-gii:hasUniqueTextIdentifier "BHER" .

figi-st:euroDollar a figi-gii:SecurityType .

figi-ps:GESM a owl:NamedIndividual .

figi-ps:BHFG a owl:NamedIndividual .

figi-ps:GESM a figi-gii:PricingSource .

figi-ps:BHFG a figi-gii:PricingSource .

figi-st:euroDollar skos:definition "Eurodollar Bonds. Bonds paying interest and principal in Eurodollars. Such bonds are not regulated by the Securities and Exchange Commission and can therefore be sold at interest rates that are lower than U.S. rates." .

figi-ps:GESM skos:prefLabel "gesmosa" .

figi-ps:BHFG skos:prefLabel "bhf-bank frankfurt" .

figi-ps:GESM figi-gii:hasUniqueTextIdentifier "GESM" .

figi-ps:BHFG figi-gii:hasUniqueTextIdentifier "BHFG" .

figi-st:euroDollar skos:prefLabel "euro-dollar" .

figi-ps:GESS a owl:NamedIndividual .

figi-ps:BHLX a owl:NamedIndividual .

figi-ps:GESS a figi-gii:PricingSource .

figi-st:euroDollar figi-gii:hasUniqueTextIdentifier "EURO-DOLLAR" .

figi-ps:BHLX a figi-gii:PricingSource .

figi-ps:GESS skos:prefLabel "gesmosa - gbi" .

figi-st:euroMtn a owl:NamedIndividual .

figi-ps:GESS figi-gii:hasUniqueTextIdentifier "GESS" .

figi-ps:BHLX skos:prefLabel "bankhaus lampe kg" .

figi-ps:GFAM a owl:NamedIndividual .

figi-st:euroMtn a figi-gii:SecurityType .

figi-ps:GFAM a figi-gii:PricingSource .

figi-ps:BHLX figi-gii:hasUniqueTextIdentifier "BHLX" .

figi-ps:GFAM skos:prefLabel "gf fund mgmt co" ;
	figi-gii:hasUniqueTextIdentifier "GFAM" .

figi-ps:BHTG a owl:NamedIndividual , figi-gii:PricingSource .

figi-ps:GFIC a owl:NamedIndividual .

figi-ps:BHTG skos:prefLabel "banque heritage" .

figi-ps:GFIC a figi-gii:PricingSource .

figi-ps:BHTG figi-gii:hasUniqueTextIdentifier "BHTG" .

figi-ps:GFIC skos:prefLabel "gfi group sydney" .

figi-st:euroMtn skos:definition "Euro Medium Term Note (EMTN). Continuously offered notes with maturities ranging from nine months to 40 years. Typically unsecured debt obligations, each euro medium term note issue (also known as a tranche) is a drawdown from a program (prospectus) level. EMTNs are flexible in structure and market timing because of this type of issuance (modeled from the commercial paper market). EMTNs are traded in the Euro market." .

figi-ps:GFIC figi-gii:hasUniqueTextIdentifier "GFIC" .

figi-ps:BHTM a owl:NamedIndividual .

figi-ps:GFIF a owl:NamedIndividual .

figi-st:euroMtn skos:prefLabel "euro mtn" .

figi-ps:GFIF a figi-gii:PricingSource .

figi-ps:BHTM a figi-gii:PricingSource .

figi-ps:GFIF skos:prefLabel "gfi group london" .

figi-st:euroMtn figi-gii:hasUniqueTextIdentifier "EURO MTN" .

figi-ps:GFIF figi-gii:hasUniqueTextIdentifier "GFIF" .

figi-ps:BHTM skos:prefLabel "bank of high tech" .

figi-ps:GFIH a owl:NamedIndividual .

figi-ps:AIM a owl:NamedIndividual .

figi-ps:GFIH a figi-gii:PricingSource .

figi-ps:BHTM figi-gii:hasUniqueTextIdentifier "BHTM" .

figi-ps:AIM a figi-gii:PricingSource .

figi-ps:GFIH skos:prefLabel "gfi group limited" .

figi-ps:AIM skos:prefLabel "amvescap" .

figi-ps:GFIH figi-gii:hasUniqueTextIdentifier "GFIH" .

figi-ps:BHWA a owl:NamedIndividual .

figi-ps:AIM figi-gii:hasUniqueTextIdentifier "AIM" .

figi-ps:GFIJ a owl:NamedIndividual .

figi-ps:BHWA a figi-gii:PricingSource .

figi-ps:GFIJ a figi-gii:PricingSource .

figi-st:euroNonDollar a owl:NamedIndividual .

figi-ps:GFIJ skos:prefLabel "gfi group inc london" .

figi-ps:BHWA skos:prefLabel "bank handlowy" .

figi-ps:GFIJ figi-gii:hasUniqueTextIdentifier "GFIJ" .

figi-st:euroNonDollar a figi-gii:SecurityType .

figi-ps:GFIS a owl:NamedIndividual .

figi-ps:BHWA figi-gii:hasUniqueTextIdentifier "BHWA" .

figi-ps:GFIS a figi-gii:PricingSource ;
	skos:prefLabel "gfi group inc" .

figi-st:euroNonDollar skos:definition "Euro Non-Dollar. Any security issued by a U.S. company in a foreign country in a currency other than U.S. dollars." .

figi-ps:BI a owl:NamedIndividual .

figi-ps:GFIS figi-gii:hasUniqueTextIdentifier "GFIS" .

figi-st:euroNonDollar skos:prefLabel "euro non-dollar" .

figi-ps:GFPL a owl:NamedIndividual .

figi-ps:BI a figi-gii:PricingSource .

figi-ps:GFPL a figi-gii:PricingSource .

figi-st:euroNonDollar figi-gii:hasUniqueTextIdentifier "EURO NON-DOLLAR" .

figi-ps:GFPL skos:prefLabel "global funding llc" .

figi-ps:BI skos:prefLabel "banco itau" .

figi-ps:GFPL figi-gii:hasUniqueTextIdentifier "GFPL" .

figi-ps:AIM7 a owl:NamedIndividual .

figi-ps:GHIL a owl:NamedIndividual .

figi-ps:BI figi-gii:hasUniqueTextIdentifier "BI" .

figi-ps:GHIL a figi-gii:PricingSource .

figi-ps:AIM7 a figi-gii:PricingSource .

figi-ps:GHIL skos:prefLabel "good hill master" .

figi-ps:BIA a owl:NamedIndividual .

figi-ps:GHIL figi-gii:hasUniqueTextIdentifier "GHIL" .

figi-ps:AIM7 skos:prefLabel "aim qa 7 day" .

figi-ps:GIC a owl:NamedIndividual .

figi-ps:BIA a figi-gii:PricingSource .

figi-ps:GIC a figi-gii:PricingSource .

figi-ps:AIM7 figi-gii:hasUniqueTextIdentifier "AIM7" .

figi-ps:BIA skos:prefLabel "bi asset management" .

figi-ps:GIC skos:prefLabel "gic, singapore" .

figi-st:euroStructrdLn a owl:NamedIndividual .

figi-ps:GIC figi-gii:hasUniqueTextIdentifier "GIC" .

figi-ps:BIA figi-gii:hasUniqueTextIdentifier "BIA" .

figi-st:euroStructrdLn a figi-gii:SecurityType .

figi-ps:GILL a owl:NamedIndividual .

figi-ps:BICB a owl:NamedIndividual .

figi-st:euroStructrdLn skos:definition "Euro Structured Loan Note" .

figi-ps:BICB a figi-gii:PricingSource .

figi-st:euroStructrdLn skos:prefLabel "euro structrd ln" .

figi-ps:BICB skos:prefLabel "bicbanco" ;
	figi-gii:hasUniqueTextIdentifier "BICB" .

figi-st:euroStructrdLn figi-gii:hasUniqueTextIdentifier "EURO STRUCTRD LN" .

figi-ps:BID a owl:NamedIndividual .

figi-ps:AIMD a owl:NamedIndividual , figi-gii:PricingSource .

figi-ps:GILL a figi-gii:PricingSource .

figi-ps:AIMD skos:prefLabel "aim qa2" .

figi-ps:BID a figi-gii:PricingSource .

figi-ps:GILL skos:prefLabel "gill capital" .

figi-ps:BID skos:prefLabel "bii indonesia" .

figi-ps:GILL figi-gii:hasUniqueTextIdentifier "GILL" .

figi-ps:AIMD figi-gii:hasUniqueTextIdentifier "AIMD" .

figi-ps:BID figi-gii:hasUniqueTextIdentifier "BID" .

figi-ps:GING a owl:NamedIndividual .

figi-st:euroTimeDepst a owl:NamedIndividual .

figi-ps:GING a figi-gii:PricingSource .

figi-ps:BIDS a owl:NamedIndividual .

figi-st:euroTimeDepst a figi-gii:SecurityType .

figi-ps:BIDS a figi-gii:PricingSource .

figi-st:euroTimeDepst skos:definition "Time Deposit / Euro Market" .

figi-ps:BIDS skos:prefLabel "bursa malaysia etp" .

figi-st:euroTimeDepst skos:prefLabel "euro time depst" .

figi-ps:GING skos:prefLabel "ginga petroleum" .

figi-ps:BIDS figi-gii:hasUniqueTextIdentifier "BIDS" .

figi-st:euroTimeDepst figi-gii:hasUniqueTextIdentifier "EURO TIME DEPST" .

figi-ps:GING figi-gii:hasUniqueTextIdentifier "GING" .

figi-ps:BIDV a owl:NamedIndividual .

figi-st:euroZone a owl:NamedIndividual .

figi-ps:GIRL a owl:NamedIndividual .

figi-ps:BIDV a figi-gii:PricingSource .

figi-ps:GIRL a figi-gii:PricingSource .

figi-ps:BIDV skos:prefLabel "bk invt and devpt" .

figi-ps:GIRL skos:prefLabel "kks securities" .

figi-ps:BIDV figi-gii:hasUniqueTextIdentifier "BIDV" .

figi-st:euroZone a figi-gii:SecurityType .

figi-ps:GIRL figi-gii:hasUniqueTextIdentifier "GIRL" .

figi-ps:BIDY a owl:NamedIndividual , figi-gii:PricingSource .

figi-ps:GISP a owl:NamedIndividual , figi-gii:PricingSource .

figi-ps:BIDY skos:prefLabel "bnegara fastbid yld" .

figi-st:euroZone skos:definition "Bonds issued by the countries that redenominated their debt from their legacy country to the Euro. Currency of the bond is in Euro." .

figi-ps:GISP skos:prefLabel "global investor serv" .

figi-ps:BIDY figi-gii:hasUniqueTextIdentifier "BIDY" .

figi-st:euroZone skos:prefLabel "euro-zone" .

figi-ps:GISP figi-gii:hasUniqueTextIdentifier "GISP" .

figi-ps:BIER a owl:NamedIndividual .

figi-st:euroZone figi-gii:hasUniqueTextIdentifier "EURO-ZONE" .

figi-ps:BIER a figi-gii:PricingSource .

figi-ps:GITB a owl:NamedIndividual , figi-gii:PricingSource .

figi-ps:BIER skos:prefLabel "berghoff and company" .

figi-ps:AIMF a owl:NamedIndividual .

figi-ps:GITB skos:prefLabel "garban info systems" .

figi-ps:BIER figi-gii:hasUniqueTextIdentifier "BIER" .

figi-ps:AIMF a figi-gii:PricingSource .

figi-ps:GITB figi-gii:hasUniqueTextIdentifier "GITB" .

figi-ps:BIEU a owl:NamedIndividual .

figi-ps:GJAL a owl:NamedIndividual .

figi-ps:AIMF skos:prefLabel "aim fix connectivity" .

figi-ps:GJAL a figi-gii:PricingSource .

figi-ps:BIEU a figi-gii:PricingSource .

figi-ps:AIMF figi-gii:hasUniqueTextIdentifier "AIMF" .

figi-ps:GJAL skos:prefLabel "guotai junan assets" .

figi-ps:BIEU skos:prefLabel "banco itau europa" .

figi-st:extendCommNote a owl:NamedIndividual .

figi-ps:GJAL figi-gii:hasUniqueTextIdentifier "GJAL" .

figi-st:extendCommNote a figi-gii:SecurityType .

figi-ps:GKBC a owl:NamedIndividual .

figi-st:extendCommNote skos:definition "Extendible Commercial Notes" .

figi-ps:BIEU figi-gii:hasUniqueTextIdentifier "BIEU" .

figi-ps:GKBC a figi-gii:PricingSource .

figi-st:extendCommNote skos:prefLabel "extend comm note" .

figi-ps:GKBC skos:prefLabel "george k baum and co" .

figi-ps:BIFI a owl:NamedIndividual .

figi-st:extendCommNote figi-gii:hasUniqueTextIdentifier "EXTEND COMM NOTE" .

figi-ps:BIFI a figi-gii:PricingSource .

figi-ps:GKBC figi-gii:hasUniqueTextIdentifier "GKBC" .

figi-ps:AIMQ a owl:NamedIndividual .

figi-ps:BIFI skos:prefLabel "banco itau brazil" .

figi-ps:GLBC a owl:NamedIndividual .

figi-ps:AIMQ a figi-gii:PricingSource .

figi-ps:BIFI figi-gii:hasUniqueTextIdentifier "BIFI" .

figi-ps:GLBC a figi-gii:PricingSource .

figi-ps:AIMQ skos:prefLabel "aim qa" .

figi-ps:GLBC skos:prefLabel "global bank corp." .

figi-ps:BIG1 a owl:NamedIndividual .

figi-ps:AIMQ figi-gii:hasUniqueTextIdentifier "AIMQ" .

figi-ps:BIG1 a figi-gii:PricingSource ;
	skos:prefLabel "banc investment grp" .

figi-st:extendNoteMtn a owl:NamedIndividual .

figi-ps:BIG1 figi-gii:hasUniqueTextIdentifier "BIG1" .

figi-st:extendNoteMtn a figi-gii:SecurityType .

figi-ps:BIG2 a owl:NamedIndividual .

figi-ps:GLBC figi-gii:hasUniqueTextIdentifier "GLBC" .

figi-st:extendNoteMtn skos:definition "Extendible Note issued off of MTN type prospectus" .

figi-ps:BIG2 a figi-gii:PricingSource .

figi-st:extendNoteMtn skos:prefLabel "extend. note mtn" .

figi-ps:GLBK a owl:NamedIndividual .

figi-st:extendNoteMtn figi-gii:hasUniqueTextIdentifier "EXTEND. NOTE MTN" .

figi-ps:BIG2 skos:prefLabel "brownstone internal2" .

figi-ps:GLBK a figi-gii:PricingSource .

figi-ps:AIQA a owl:NamedIndividual .

figi-ps:BIG2 figi-gii:hasUniqueTextIdentifier "BIG2" .

figi-ps:GLBK skos:prefLabel "glitnir" .

figi-ps:AIQA a figi-gii:PricingSource .

figi-ps:BIG3 a owl:NamedIndividual .

figi-ps:GLBK figi-gii:hasUniqueTextIdentifier "GLBK" .

figi-ps:BIG3 a figi-gii:PricingSource ;
	skos:prefLabel "brownstone internal3" .

figi-ps:GLBL a owl:NamedIndividual .

figi-ps:BIG3 figi-gii:hasUniqueTextIdentifier "BIG3" .

figi-ps:GLBL a figi-gii:PricingSource .

figi-ps:AIQA skos:prefLabel "bb aim qa" .

figi-ps:GLBL skos:prefLabel "global hunter" .

figi-ps:BIGG a owl:NamedIndividual .

figi-ps:AIQA figi-gii:hasUniqueTextIdentifier "AIQA" .

figi-ps:GLBL figi-gii:hasUniqueTextIdentifier "GLBL" .

figi-ps:BIGG a figi-gii:PricingSource .

figi-st:fdic a owl:NamedIndividual .

figi-ps:GLBM a owl:NamedIndividual .

figi-ps:BIGG skos:prefLabel "brownstone inv grp" .

figi-st:fdic a figi-gii:SecurityType .

figi-ps:GLBM a figi-gii:PricingSource .

figi-ps:BIGG figi-gii:hasUniqueTextIdentifier "BIGG" .

figi-ps:GLBM skos:prefLabel "az global" ;
	figi-gii:hasUniqueTextIdentifier "GLBM" .

figi-ps:BIGI a owl:NamedIndividual .

figi-ps:GLBT a owl:NamedIndividual .

figi-st:fdic skos:definition "Federal Deposit Insurance Corporation. A federal agency that insures deposits in member banks and thrifts up to $100,000." .

figi-ps:GLBT a figi-gii:PricingSource .

figi-ps:BIGI a figi-gii:PricingSource .

figi-ps:GLBT skos:prefLabel "global sec turkey" .

figi-st:fdic skos:prefLabel "fdic" .

figi-ps:GLBT figi-gii:hasUniqueTextIdentifier "GLBT" .

figi-ps:BIGI skos:prefLabel "brownstone internal" .

figi-ps:GLBX a owl:NamedIndividual .

figi-st:fdic figi-gii:hasUniqueTextIdentifier "FDIC" .

figi-ps:GLBX a figi-gii:PricingSource .

figi-ps:BIGI figi-gii:hasUniqueTextIdentifier "BIGI" .

figi-ps:GLBX skos:prefLabel "globex bank" .

figi-ps:AISM a owl:NamedIndividual .

figi-ps:BIGW a owl:NamedIndividual .

figi-ps:GLBX figi-gii:hasUniqueTextIdentifier "GLBX" .

figi-ps:AISM a figi-gii:PricingSource .

figi-ps:GLEN a owl:NamedIndividual .

figi-ps:BIGW a figi-gii:PricingSource .

figi-ps:GLEN a figi-gii:PricingSource .

figi-ps:AISM skos:prefLabel "aism" .

figi-ps:GLEN skos:prefLabel "glenwood capital" .

figi-ps:BIGW skos:prefLabel "bank millennium" .

figi-ps:GLEN figi-gii:hasUniqueTextIdentifier "GLEN" .

figi-ps:AISM figi-gii:hasUniqueTextIdentifier "AISM" .

figi-ps:GLG a owl:NamedIndividual .

figi-ps:BIGW figi-gii:hasUniqueTextIdentifier "BIGW" .

figi-st:fedFunds a owl:NamedIndividual .

figi-ps:GLG a figi-gii:PricingSource .

figi-st:fedFunds a figi-gii:SecurityType .

figi-ps:BIGZ a owl:NamedIndividual .

figi-ps:GLG skos:prefLabel "glg partners lp" .

figi-ps:BIGZ a figi-gii:PricingSource .

figi-ps:GLG figi-gii:hasUniqueTextIdentifier "GLG" .

figi-ps:BIGZ skos:prefLabel "blv fixed income" ;
	figi-gii:hasUniqueTextIdentifier "BIGZ" .

figi-ps:GLIC a owl:NamedIndividual .

figi-st:fedFunds skos:definition "The Fed Funds type is used by banks to track the overnight borrowing they partake in to meet bank reserve requirements. Banks needs to have certain amount of cash on hand at close of every day, if they are short they will borrow from another bank for the night. This program type was established to help the banks manage this process." .

figi-ps:GLIC a figi-gii:PricingSource .

figi-ps:BII a owl:NamedIndividual .

figi-st:fedFunds skos:prefLabel "fed funds" .

figi-ps:GLIC skos:prefLabel "guardian life ins" .

figi-ps:BII a figi-gii:PricingSource .

figi-st:fedFunds figi-gii:hasUniqueTextIdentifier "FED FUNDS" .

figi-ps:GLIC figi-gii:hasUniqueTextIdentifier "GLIC" .

figi-ps:BII skos:prefLabel "bank inter indonesia" .

figi-ps:AJL a owl:NamedIndividual .

figi-ps:GLLJ a owl:NamedIndividual .

figi-ps:BII figi-gii:hasUniqueTextIdentifier "BII" .

figi-ps:GLLJ a figi-gii:PricingSource .

figi-ps:AJL a figi-gii:PricingSource .

figi-ps:BIJK a owl:NamedIndividual .

figi-ps:GLLJ skos:prefLabel "guardian life ltd ja" .

figi-ps:BIJK a figi-gii:PricingSource .

figi-ps:AJL skos:prefLabel "ing (nz) ltd" .

figi-ps:GLLJ figi-gii:hasUniqueTextIdentifier "GLLJ" .

figi-ps:BIJK skos:prefLabel "bk indonesia" .

figi-ps:AJL figi-gii:hasUniqueTextIdentifier "AJL" .

figi-ps:GLLT a owl:NamedIndividual .

figi-ps:BIJK figi-gii:hasUniqueTextIdentifier "BIJK" .

figi-ps:GLLT a figi-gii:PricingSource .

figi-ps:AKBB a owl:NamedIndividual .

figi-ps:BILX a owl:NamedIndividual .

figi-ps:AKBB a figi-gii:PricingSource .

figi-ps:GLLT skos:prefLabel "guardian asset mgmt" .

figi-ps:BILX a figi-gii:PricingSource .

figi-ps:AKBB skos:prefLabel "akbars bank kazan" .

figi-ps:GLLT figi-gii:hasUniqueTextIdentifier "GLLT" .

figi-ps:AKBB figi-gii:hasUniqueTextIdentifier "AKBB" .

figi-ps:BILX skos:prefLabel "bil luxembourg" .

figi-ps:GLOS a owl:NamedIndividual .

figi-st:fedNoonBuyingRate a owl:NamedIndividual .

figi-ps:BILX figi-gii:hasUniqueTextIdentifier "BILX" .

figi-ps:GLOS a figi-gii:PricingSource .

figi-st:fedNoonBuyingRate a figi-gii:SecurityType .

figi-ps:BIM a owl:NamedIndividual .

figi-ps:GLOS skos:prefLabel "globalsec monaco" .

figi-ps:BIM a figi-gii:PricingSource .

figi-st:fedNoonBuyingRate skos:definition "12.00 noon buying FX rates from the Federal Reserve of New York" .

figi-ps:BIM skos:prefLabel "bim (uk) ltd" .

figi-ps:GLOS figi-gii:hasUniqueTextIdentifier "GLOS" .

figi-st:fedNoonBuyingRate skos:prefLabel "fed noon buying rate" .

figi-ps:BIM figi-gii:hasUniqueTextIdentifier "BIM" .

figi-ps:GLYN a owl:NamedIndividual .

figi-st:fedNoonBuyingRate figi-gii:hasUniqueTextIdentifier "FED NOON BUYING RATE" .

figi-ps:BIMC a owl:NamedIndividual .

figi-ps:GLYN a figi-gii:PricingSource .

figi-ps:BIMC a figi-gii:PricingSource .

figi-ps:AKBF a owl:NamedIndividual .

figi-ps:GLYN skos:prefLabel "glynn (j.a.) and co" .

figi-ps:AKBF a figi-gii:PricingSource .

figi-ps:BIMC skos:prefLabel "banco itau bz bonds" .

figi-ps:AKBF skos:prefLabel "ak bars finance" .

figi-ps:GLYN skos:prefLabel "glynn (ja) and co" .

figi-ps:AKBF figi-gii:hasUniqueTextIdentifier "AKBF" .

figi-ps:GLYN figi-gii:hasUniqueTextIdentifier "GLYN" .

figi-st:fidc a owl:NamedIndividual .

figi-ps:BIMC figi-gii:hasUniqueTextIdentifier "BIMC" .

figi-st:fidc a figi-gii:SecurityType .

figi-ps:GM a owl:NamedIndividual .

figi-ps:BIMI a owl:NamedIndividual .

figi-ps:GM a figi-gii:PricingSource .

figi-st:fidc skos:definition "This stands for Fundo De Investimento Em Direitos Creditorios in Portuguese" .

figi-ps:GM skos:prefLabel "gmimco" .

figi-st:fidc skos:prefLabel "fidc" .

figi-ps:BIMI a figi-gii:PricingSource .

figi-st:fidc figi-gii:hasUniqueTextIdentifier "FIDC" .

figi-ps:GM figi-gii:hasUniqueTextIdentifier "GM" .

figi-ps:BIMI skos:prefLabel "banca imi new york" .

figi-ps:AKBK a owl:NamedIndividual .

figi-ps:GMBS a owl:NamedIndividual .

figi-ps:BIMI figi-gii:hasUniqueTextIdentifier "BIMI" .

figi-ps:AKBK a figi-gii:PricingSource .

figi-ps:GMBS a figi-gii:PricingSource .

figi-ps:BINC a owl:NamedIndividual .

figi-ps:AKBK skos:prefLabel "akbank" .

figi-ps:GMBS skos:prefLabel "goldman sachs japan" .

figi-ps:BINC a figi-gii:PricingSource .

figi-ps:AKBK figi-gii:hasUniqueTextIdentifier "AKBK" .

figi-ps:BINC skos:prefLabel "binck bank nv" .

figi-ps:GMBS skos:prefLabel "goldman sacls japan" .

figi-st:financialCommodityFuture a owl:NamedIndividual .

figi-ps:BINC figi-gii:hasUniqueTextIdentifier "BINC" .

figi-ps:GMBS figi-gii:hasUniqueTextIdentifier "GMBS" .

figi-st:financialCommodityFuture a figi-gii:SecurityType .

figi-ps:BIND a owl:NamedIndividual .

figi-ps:GMGM a owl:NamedIndividual .

figi-ps:BIND a figi-gii:PricingSource .

figi-ps:GMGM a figi-gii:PricingSource .

figi-st:financialCommodityFuture skos:definition "Commodity Future. A contract to buy or sell a specific commodity at a specified price at a certain future date." .

figi-ps:GMGM skos:prefLabel "gmg brokers dubai" .

figi-ps:BIND skos:prefLabel "banco industrial" .

figi-ps:GMGM figi-gii:hasUniqueTextIdentifier "GMGM" .

figi-st:financialCommodityFuture skos:prefLabel "financial commodity future." .

figi-ps:BIND figi-gii:hasUniqueTextIdentifier "BIND" .

figi-st:financialCommodityFuture figi-gii:hasUniqueTextIdentifier "Financial commodity future." .

figi-ps:GMOP a owl:NamedIndividual .

figi-ps:BING a owl:NamedIndividual .

figi-ps:AKCA a owl:NamedIndividual .

figi-ps:BING a figi-gii:PricingSource .

figi-ps:GMOP a figi-gii:PricingSource .

figi-ps:AKCA a figi-gii:PricingSource .

figi-ps:BING skos:prefLabel "ing belgium - ingb" .

figi-ps:GMOP skos:prefLabel "goldman sachs uk mop" .

figi-ps:AKCA skos:prefLabel "ak capital" .

figi-ps:GMOP figi-gii:hasUniqueTextIdentifier "GMOP" .

figi-ps:AKCA figi-gii:hasUniqueTextIdentifier "AKCA" .

figi-ps:GMP a owl:NamedIndividual .

figi-ps:BING figi-gii:hasUniqueTextIdentifier "BING" .

figi-ps:GMP a figi-gii:PricingSource .

figi-st:financialCommodityGeneric a owl:NamedIndividual .

figi-ps:BIP a owl:NamedIndividual .

figi-ps:GMP skos:prefLabel "gmp investment mgmt" .

figi-ps:BIP a figi-gii:PricingSource .

figi-ps:GMP skos:prefLabel "gmp securities llc" .

figi-st:financialCommodityGeneric a figi-gii:SecurityType .

figi-ps:BIP skos:prefLabel "bberg indication prc" .

figi-ps:GMP figi-gii:hasUniqueTextIdentifier "GMP" .

figi-ps:BIP figi-gii:hasUniqueTextIdentifier "BIP" .

figi-st:financialCommodityGeneric skos:definition "Cash Settled (Financial) Generics on Commodity Futures. Generics are used to combine multiple futures contracts to build a generic history stream." .

figi-ps:BIS a owl:NamedIndividual .

figi-ps:GMPE a owl:NamedIndividual .

figi-ps:BIS a figi-gii:PricingSource .

figi-st:financialCommodityGeneric skos:prefLabel "financial commodity generic." .

figi-ps:GMPE a figi-gii:PricingSource .

figi-ps:BIS skos:prefLabel "bis" .

figi-st:financialCommodityGeneric figi-gii:hasUniqueTextIdentifier "Financial commodity generic." .

figi-ps:BIS figi-gii:hasUniqueTextIdentifier "BIS" .

figi-ps:GMPE skos:prefLabel "gmp europe" .

figi-ps:AKGM a owl:NamedIndividual .

figi-ps:GMPE figi-gii:hasUniqueTextIdentifier "GMPE" .

figi-ps:BISM a owl:NamedIndividual .

figi-ps:AKGM a figi-gii:PricingSource .

figi-ps:GMPN a owl:NamedIndividual .

figi-ps:BISM a figi-gii:PricingSource .

figi-ps:AKGM skos:prefLabel "ak bank" .

figi-ps:GMPN a figi-gii:PricingSource .

figi-ps:BISM skos:prefLabel "bank islam berhad" .

figi-ps:AKGM figi-gii:hasUniqueTextIdentifier "AKGM" .

figi-ps:GMPN skos:prefLabel "gmp securities" .

figi-ps:BISM figi-gii:hasUniqueTextIdentifier "BISM" .

figi-st:financialCommodityOption a owl:NamedIndividual .

figi-ps:GMPN figi-gii:hasUniqueTextIdentifier "GMPN" .

figi-st:financialCommodityOption a figi-gii:SecurityType .

figi-ps:BISP a owl:NamedIndividual .

figi-ps:GMS a owl:NamedIndividual .

figi-st:financialCommodityOption skos:definition "Cash Settled (Financial) Options on Commodity Futures." .

figi-ps:GMS a figi-gii:PricingSource .

figi-st:financialCommodityOption skos:prefLabel "financial commodity option." .

figi-ps:GMS skos:prefLabel "gms group" .

figi-st:financialCommodityOption figi-gii:hasUniqueTextIdentifier "Financial commodity option." .

figi-ps:GMS figi-gii:hasUniqueTextIdentifier "GMS" .

figi-ps:AKRO a owl:NamedIndividual .

figi-ps:BISP a figi-gii:PricingSource .

figi-ps:AKRO a figi-gii:PricingSource .

figi-ps:GMSC a owl:NamedIndividual .

figi-ps:BISP skos:prefLabel "bis parallel" .

figi-ps:AKRO skos:prefLabel "banca akros spa" .

figi-ps:GMSC a figi-gii:PricingSource .

figi-ps:BISP figi-gii:hasUniqueTextIdentifier "BISP" .

figi-ps:AKRO figi-gii:hasUniqueTextIdentifier "AKRO" .

figi-ps:GMSC skos:prefLabel "good morning secs" .

figi-ps:BJB a owl:NamedIndividual .

figi-st:financialCommoditySpot a owl:NamedIndividual .

figi-ps:BJB a figi-gii:PricingSource .

figi-st:financialCommoditySpot a figi-gii:SecurityType .

figi-ps:BJB skos:prefLabel "bank julius baer" .

figi-ps:GMSC figi-gii:hasUniqueTextIdentifier "GMSC" .

figi-ps:BJB figi-gii:hasUniqueTextIdentifier "BJB" .

figi-ps:GMSO a owl:NamedIndividual .

figi-st:financialCommoditySpot skos:definition "Cash Settled (Financial) Spot on Commodity Futures. The commodity will be delivered and settled immediately or in which a futures contract will expire in one month or less." .

figi-ps:GMSO a figi-gii:PricingSource .

figi-st:financialCommoditySpot skos:prefLabel "financial commodity spot." .

figi-ps:BJM a owl:NamedIndividual .

figi-ps:GMSO skos:prefLabel "gms group inc" .

figi-st:financialCommoditySpot figi-gii:hasUniqueTextIdentifier "Financial commodity spot." .

figi-ps:GMSO figi-gii:hasUniqueTextIdentifier "GMSO" .

figi-ps:AL a owl:NamedIndividual .

figi-ps:BJM a figi-gii:PricingSource .

figi-ps:GMSS a owl:NamedIndividual .

figi-ps:AL a figi-gii:PricingSource .

figi-ps:BJM skos:prefLabel "bjm" .

figi-ps:GMSS a figi-gii:PricingSource .

figi-ps:AL skos:prefLabel "alternative leaders" .

figi-ps:BJM figi-gii:hasUniqueTextIdentifier "BJM" .

figi-ps:GMSS skos:prefLabel "gm shinhan sec" .

figi-ps:AL figi-gii:hasUniqueTextIdentifier "AL" .

figi-ps:GMSS figi-gii:hasUniqueTextIdentifier "GMSS" .

figi-ps:BJME a owl:NamedIndividual .

figi-ps:ALAD a owl:NamedIndividual .

figi-ps:BJME a figi-gii:PricingSource .

figi-ps:GMTS a owl:NamedIndividual .

figi-ps:ALAD a figi-gii:PricingSource .

figi-ps:BJME skos:prefLabel "bjm holdings e-bond" .

figi-ps:GMTS a figi-gii:PricingSource .

figi-ps:ALAD skos:prefLabel "aladdin capital uk" .

figi-ps:BJME figi-gii:hasUniqueTextIdentifier "BJME" .

figi-ps:GMTS skos:prefLabel "germany mts" .

figi-ps:ALAD figi-gii:hasUniqueTextIdentifier "ALAD" .

figi-ps:GMTS figi-gii:hasUniqueTextIdentifier "GMTS" .

figi-ps:BKBJ a owl:NamedIndividual .

figi-st:financialIndexFuture a owl:NamedIndividual .

figi-ps:GNBW a owl:NamedIndividual .

figi-ps:BKBJ a figi-gii:PricingSource .

figi-st:financialIndexFuture a figi-gii:SecurityType .

figi-ps:BKBJ skos:prefLabel "bank of beijing" .

figi-ps:GNBW a figi-gii:PricingSource .

figi-ps:BKBJ figi-gii:hasUniqueTextIdentifier "BKBJ" .

figi-ps:GNBW skos:prefLabel "getin noble bank" ;
	figi-gii:hasUniqueTextIdentifier "GNBW" .

figi-ps:BKBK a owl:NamedIndividual .

figi-st:financialIndexFuture skos:definition "Futures contracts that use indices as their base and theoretically settle by delivery of the underlying securities or commodities that make up the indices." .

figi-ps:BKBK a figi-gii:PricingSource .

figi-ps:GNCP a owl:NamedIndividual .

figi-st:financialIndexFuture skos:prefLabel "financial index future." .

figi-ps:BKBK skos:prefLabel "bruell kallmus bank" .

figi-ps:GNCP a figi-gii:PricingSource .

figi-st:financialIndexFuture figi-gii:hasUniqueTextIdentifier "Financial index future." .

figi-ps:BKBK figi-gii:hasUniqueTextIdentifier "BKBK" .

figi-ps:GNCP skos:prefLabel "genghis capital ltd" .

figi-ps:ALB a owl:NamedIndividual .

figi-ps:BKBZ a owl:NamedIndividual .

figi-ps:GNCP figi-gii:hasUniqueTextIdentifier "GNCP" .

figi-ps:BKBZ a figi-gii:PricingSource .

figi-ps:GNLI a owl:NamedIndividual .

figi-ps:ALB a figi-gii:PricingSource .

figi-ps:GNLI a figi-gii:PricingSource .

figi-ps:BKBZ skos:prefLabel "banco de boston" .

figi-ps:ALB skos:prefLabel "alberta exchange" .

figi-ps:BKBZ figi-gii:hasUniqueTextIdentifier "BKBZ" .

figi-ps:GNLI skos:prefLabel "banca generali spa" .

figi-ps:ALB figi-gii:hasUniqueTextIdentifier "ALB" .

figi-ps:GNLI figi-gii:hasUniqueTextIdentifier "GNLI" .

figi-ps:BKC a owl:NamedIndividual .

figi-st:financialIndexGeneric a owl:NamedIndividual .

figi-ps:GNTC a owl:NamedIndividual .

figi-st:financialIndexGeneric a figi-gii:SecurityType .

figi-ps:GNTC a figi-gii:PricingSource .

figi-st:financialIndexGeneric skos:definition "Valid return for generic tickers." .

figi-ps:GNTC skos:prefLabel "grant capital" .

figi-st:financialIndexGeneric skos:prefLabel "financial index generic." .

figi-ps:BKC a figi-gii:PricingSource .

figi-ps:GNTC figi-gii:hasUniqueTextIdentifier "GNTC" .

figi-st:financialIndexGeneric figi-gii:hasUniqueTextIdentifier "Financial index generic." .

figi-ps:BKC skos:prefLabel "bank of commerce" .

figi-ps:GNWL a owl:NamedIndividual .

figi-ps:ALBG a owl:NamedIndividual .

figi-ps:BKC figi-gii:hasUniqueTextIdentifier "BKC" .

figi-ps:GNWL a figi-gii:PricingSource .

figi-ps:ALBG a figi-gii:PricingSource .

figi-ps:BKCM a owl:NamedIndividual .

figi-ps:GNWL skos:prefLabel "greenwich natwest" .

figi-ps:BKCM a figi-gii:PricingSource .

figi-ps:GNWL figi-gii:hasUniqueTextIdentifier "GNWL" .

figi-ps:BKCM skos:prefLabel "bny capital market" .

figi-ps:ALBG skos:prefLabel "al-baraka bank grp" .

figi-ps:BKCM figi-gii:hasUniqueTextIdentifier "BKCM" .

figi-ps:GNZS a owl:NamedIndividual .

figi-ps:ALBG figi-gii:hasUniqueTextIdentifier "ALBG" .

figi-ps:BKCO a owl:NamedIndividual .

figi-ps:GNZS a figi-gii:PricingSource .

figi-ps:BKCO a figi-gii:PricingSource .

figi-st:financialIndexOption a owl:NamedIndividual .

figi-ps:GNZS skos:prefLabel "guardians of nz sup" .

figi-ps:BKCO skos:prefLabel "cfif bk of communica" .

figi-st:financialIndexOption a figi-gii:SecurityType .

figi-ps:BKCO figi-gii:hasUniqueTextIdentifier "BKCO" .

figi-ps:GNZS figi-gii:hasUniqueTextIdentifier "GNZS" .

figi-ps:BKEA a owl:NamedIndividual .

figi-st:financialIndexOption skos:definition "An option that is based on a stock index (performance measure of a group of stocks). Such options enable investors to trade in a particular market or industry group without having to buy individual stocks. Index options are issued by the Options Clearing Corporation." .

figi-ps:BKEA a figi-gii:PricingSource .

figi-ps:GOAT a owl:NamedIndividual .

figi-st:financialIndexOption skos:prefLabel "financial index option." .

figi-ps:GOAT a figi-gii:PricingSource .

figi-st:financialIndexOption figi-gii:hasUniqueTextIdentifier "Financial index option." .

figi-ps:GOAT skos:prefLabel "global absolute" .

figi-ps:ALBR a owl:NamedIndividual .

figi-ps:GOAT figi-gii:hasUniqueTextIdentifier "GOAT" .

figi-ps:ALBR a figi-gii:PricingSource .

figi-ps:GOFH a owl:NamedIndividual .

figi-ps:ALBR skos:prefLabel "albaraka turk" .

figi-ps:GOFH a figi-gii:PricingSource .

figi-ps:ALBR figi-gii:hasUniqueTextIdentifier "ALBR" .

figi-ps:GOFH skos:prefLabel "genscape oil fulhist" .

figi-st:finnishCD a owl:NamedIndividual .

figi-ps:GOFH figi-gii:hasUniqueTextIdentifier "GOFH" .

figi-st:finnishCD a figi-gii:SecurityType .

figi-ps:GOLD a owl:NamedIndividual .

figi-st:finnishCD skos:definition "Finland Domestic Certificates of Deposit" .

figi-ps:GOLD a figi-gii:PricingSource .

figi-st:finnishCD skos:prefLabel "finnish cd" .

figi-ps:GOLD skos:prefLabel "goldman sachs" .

figi-st:finnishCD figi-gii:hasUniqueTextIdentifier "FINNISH CD" .

figi-ps:GOLD figi-gii:hasUniqueTextIdentifier "GOLD" .

figi-ps:ALC a owl:NamedIndividual .

figi-ps:GOLH a owl:NamedIndividual .

figi-ps:ALC a figi-gii:PricingSource .

figi-ps:GOLH a figi-gii:PricingSource .

figi-ps:ALC skos:prefLabel "alchemy special op l" .

figi-ps:GOLH skos:prefLabel "genscape oil limhist" .

figi-ps:ALC figi-gii:hasUniqueTextIdentifier "ALC" .

figi-ps:GOLH figi-gii:hasUniqueTextIdentifier "GOLH" .

figi-st:finnishCP a owl:NamedIndividual .

figi-ps:GOOG a owl:NamedIndividual .

figi-st:finnishCP a figi-gii:SecurityType .

figi-ps:GOOG a figi-gii:PricingSource ;
	skos:prefLabel "google" .

figi-st:finnishCP skos:definition "Finland Domestic Commercial Paper" .

figi-ps:GOOG figi-gii:hasUniqueTextIdentifier "GOOG" .

figi-st:finnishCP skos:prefLabel "finnish cp" .

figi-ps:GOQP a owl:NamedIndividual .

figi-st:finnishCP figi-gii:hasUniqueTextIdentifier "FINNISH CP" .

figi-ps:GOQP a figi-gii:PricingSource .

figi-ps:ALCE a owl:NamedIndividual .

figi-ps:GOQP skos:prefLabel "tpex otcquoteprice" .

figi-ps:ALCE a figi-gii:PricingSource .

figi-ps:GOQP figi-gii:hasUniqueTextIdentifier "GOQP" .

figi-ps:ALCE skos:prefLabel "alceda fund sa" .

figi-ps:GOQY a owl:NamedIndividual .

figi-ps:ALCE figi-gii:hasUniqueTextIdentifier "ALCE" .

figi-ps:GOQY a figi-gii:PricingSource .

figi-ps:BKEA skos:prefLabel "bea 11:30" .

figi-st:fixed a owl:NamedIndividual .

figi-ps:GOQY skos:prefLabel "tpex otcquoteyeild" .

figi-st:fixed a figi-gii:SecurityType .

figi-ps:BKEA figi-gii:hasUniqueTextIdentifier "BKEA" .

figi-st:fixed skos:definition "The coupon stays constant through maturity." .

figi-ps:GOQY figi-gii:hasUniqueTextIdentifier "GOQY" .

figi-st:fixed skos:prefLabel "fixed" .

figi-ps:BKIA a owl:NamedIndividual .

figi-st:fixed figi-gii:hasUniqueTextIdentifier "FIXED" .

figi-ps:GOVP a owl:NamedIndividual .

figi-ps:BKIA a figi-gii:PricingSource .

figi-ps:GOVP a figi-gii:PricingSource .

figi-ps:ALCH a owl:NamedIndividual .

figi-ps:BKIA skos:prefLabel "bankia" .

figi-ps:GOVP skos:prefLabel "govpx" .

figi-ps:ALCH a figi-gii:PricingSource .

figi-ps:BKIA figi-gii:hasUniqueTextIdentifier "BKIA" .

figi-ps:GOVP figi-gii:hasUniqueTextIdentifier "GOVP" .

figi-ps:ALCH skos:prefLabel "alchemy capital mgmt" .

figi-ps:BKIS a owl:NamedIndividual .

figi-ps:ALCH figi-gii:hasUniqueTextIdentifier "ALCH" .

figi-ps:GPB a owl:NamedIndividual .

figi-st:fixedOid a owl:NamedIndividual .

figi-ps:BKIS a figi-gii:PricingSource .

figi-ps:GPB a figi-gii:PricingSource .

figi-st:fixedOid a figi-gii:SecurityType .

figi-ps:BKIS skos:prefLabel "bank islam kl" .

figi-ps:GPB skos:prefLabel "gazprombank exec" .

figi-st:fixedOid skos:definition "The coupon stays constant through maturity. The security is an Original Issue Discount." .

figi-ps:BKIS figi-gii:hasUniqueTextIdentifier "BKIS" .

figi-st:fixedOid skos:prefLabel "fixed, oid" .

figi-ps:GPB figi-gii:hasUniqueTextIdentifier "GPB" .

figi-st:fixedOid figi-gii:hasUniqueTextIdentifier "FIXED, OID" .

figi-ps:BKME a owl:NamedIndividual .

figi-ps:GPBR a owl:NamedIndividual .

figi-ps:BKME a figi-gii:PricingSource .

figi-ps:ALDN a owl:NamedIndividual .

figi-ps:GPBR a figi-gii:PricingSource .

figi-ps:BKME skos:prefLabel "bank of lon and t m e" .

figi-ps:ALDN a figi-gii:PricingSource .

figi-ps:GPBR skos:prefLabel "gazprombank" .

figi-ps:ALDN skos:prefLabel "aladdin capital" .

figi-ps:BKME figi-gii:hasUniqueTextIdentifier "BKME" .

figi-ps:ALDN figi-gii:hasUniqueTextIdentifier "ALDN" .

figi-ps:GPBR figi-gii:hasUniqueTextIdentifier "GPBR" .

figi-ps:BKOC a owl:NamedIndividual .

figi-st:fixingRate a owl:NamedIndividual .

figi-ps:GPEM a owl:NamedIndividual .

figi-st:fixingRate a figi-gii:SecurityType .

figi-ps:BKOC a figi-gii:PricingSource .

figi-ps:GPEM a figi-gii:PricingSource .

figi-st:fixingRate skos:definition "The rate set at a specific time" .

figi-ps:BKOC skos:prefLabel "bank of commerce" .

figi-st:fixingRate skos:prefLabel "fixing rate" .

figi-ps:GPEM skos:prefLabel "global partners emkt" .

figi-st:fixingRate figi-gii:hasUniqueTextIdentifier "FIXING RATE" .

figi-ps:BKOC figi-gii:hasUniqueTextIdentifier "BKOC" .

figi-ps:ALEB a owl:NamedIndividual .

figi-ps:GPEM figi-gii:hasUniqueTextIdentifier "GPEM" .

figi-ps:ALEB a figi-gii:PricingSource .

figi-ps:BKRS a owl:NamedIndividual .

figi-ps:ALEB skos:prefLabel "banca aletti" .

figi-ps:GPF a owl:NamedIndividual .

figi-ps:ALEB figi-gii:hasUniqueTextIdentifier "ALEB" .

figi-ps:BKRS a figi-gii:PricingSource .

figi-ps:GPF a figi-gii:PricingSource .

figi-st:floating a owl:NamedIndividual .

figi-ps:BKRS skos:prefLabel "bank resona perdania" .

figi-st:floating a figi-gii:SecurityType .

figi-ps:GPF skos:prefLabel "governm pension fund" .

figi-ps:BKRS figi-gii:hasUniqueTextIdentifier "BKRS" .

figi-ps:GPF figi-gii:hasUniqueTextIdentifier "GPF" .

figi-st:floating skos:definition "The coupon is based off an index or benchmark, and changes in value as the index changes." .

figi-ps:BKSR a owl:NamedIndividual .

figi-ps:GPSS a owl:NamedIndividual .

figi-st:floating skos:prefLabel "floating" .

figi-ps:BKSR a figi-gii:PricingSource .

figi-ps:GPSS a figi-gii:PricingSource .

figi-st:floating figi-gii:hasUniqueTextIdentifier "FLOATING" .

figi-ps:BKSR skos:prefLabel "bookook securities" .

figi-ps:GPSS skos:prefLabel "gpssa" .

figi-ps:ALEM a owl:NamedIndividual .

figi-ps:BKSR figi-gii:hasUniqueTextIdentifier "BKSR" .

figi-ps:GPSS figi-gii:hasUniqueTextIdentifier "GPSS" .

figi-ps:ALEM a figi-gii:PricingSource .

figi-ps:BKWR a owl:NamedIndividual .

figi-ps:ALEM skos:prefLabel "banca aletti" .

figi-ps:GRAM a owl:NamedIndividual .

figi-ps:ALEM figi-gii:hasUniqueTextIdentifier "ALEM" .

figi-ps:BKWR a figi-gii:PricingSource .

figi-ps:GRAM a figi-gii:PricingSource .

figi-ps:ALET a owl:NamedIndividual .

figi-ps:BKWR skos:prefLabel "breakwater" .

figi-ps:GRAM skos:prefLabel "gramercy funds mgmt" .

figi-ps:ALET a figi-gii:PricingSource .

figi-ps:BKWR figi-gii:hasUniqueTextIdentifier "BKWR" .

figi-ps:GRAM figi-gii:hasUniqueTextIdentifier "GRAM" .

figi-ps:ALET skos:prefLabel "banca aletti 2" .

figi-ps:BKYO a owl:NamedIndividual .

figi-ps:ALET figi-gii:hasUniqueTextIdentifier "ALET" .

figi-ps:GRAZ a owl:NamedIndividual .

figi-ps:BKYO a figi-gii:PricingSource .

figi-st:floatingCP a owl:NamedIndividual .

figi-ps:GRAZ a figi-gii:PricingSource .

figi-st:floatingCP a figi-gii:SecurityType .

figi-ps:BKYO skos:prefLabel "bank of yokohama" .

figi-ps:GRAZ skos:prefLabel "capital bank" .

figi-st:floatingCP skos:definition "Floating Rate Commercial Paper" .

figi-ps:BKYO figi-gii:hasUniqueTextIdentifier "BKYO" .

figi-ps:GRAZ figi-gii:hasUniqueTextIdentifier "GRAZ" .

figi-st:floatingCP skos:prefLabel "floating cp" .

figi-ps:BL12 a owl:NamedIndividual .

figi-ps:GRET a owl:NamedIndividual .

figi-ps:BL12 a figi-gii:PricingSource .

figi-ps:GRET a figi-gii:PricingSource .

figi-ps:BL12 skos:prefLabel "bval london 12pm" .

figi-ps:GRET skos:prefLabel "gretai securities" .

figi-st:floatingCP figi-gii:hasUniqueTextIdentifier "FLOATING CP" .

figi-ps:GRET figi-gii:hasUniqueTextIdentifier "GRET" .

figi-ps:BL12 figi-gii:hasUniqueTextIdentifier "BL12" .

figi-ps:ALF a owl:NamedIndividual .

figi-ps:GS a owl:NamedIndividual .

figi-ps:BLCL a owl:NamedIndividual .

figi-ps:ALF a figi-gii:PricingSource .

figi-ps:GS a figi-gii:PricingSource .

figi-ps:BLCL a figi-gii:PricingSource .

figi-ps:ALF skos:prefLabel "alfa mutual insuranc" .

figi-ps:GS skos:prefLabel "goldman sachs london" .

figi-ps:ALF figi-gii:hasUniqueTextIdentifier "ALF" .

figi-ps:BLCL skos:prefLabel "blc bank sal" .

figi-ps:GS figi-gii:hasUniqueTextIdentifier "GS" .

figi-ps:ALFA a owl:NamedIndividual .

figi-ps:BLCL figi-gii:hasUniqueTextIdentifier "BLCL" .

figi-ps:GSAB a owl:NamedIndividual .

figi-ps:ALFA a figi-gii:PricingSource .

figi-ps:BLFI a owl:NamedIndividual .

figi-ps:GSAB a figi-gii:PricingSource .

figi-ps:ALFA skos:prefLabel "alfa" .

figi-ps:BLFI a figi-gii:PricingSource .

figi-ps:GSAB skos:prefLabel "goldman sachs asia" .

figi-ps:ALFA figi-gii:hasUniqueTextIdentifier "ALFA" .

figi-ps:BLFI skos:prefLabel "bloomberg fi" .

figi-ps:GSAB figi-gii:hasUniqueTextIdentifier "GSAB" .

figi-st:floatingOid a owl:NamedIndividual .

figi-ps:BLFI figi-gii:hasUniqueTextIdentifier "BLFI" .

figi-ps:GSAG a owl:NamedIndividual .

figi-st:floatingOid a figi-gii:SecurityType .

figi-ps:BLG1 a owl:NamedIndividual .

figi-ps:GSAG a figi-gii:PricingSource .

figi-ps:BLG1 a figi-gii:PricingSource .

figi-st:floatingOid skos:definition "The coupon is based off an index or benchmark, and changes in value as the index changes. The security is an Original Issue Discount." .

figi-ps:BLG1 skos:prefLabel "blp internal g1" .

figi-ps:GSAG skos:prefLabel "goldman sachs agcy" .

figi-st:floatingOid skos:prefLabel "floating, oid" .

figi-ps:BLG1 figi-gii:hasUniqueTextIdentifier "BLG1" .

figi-st:floatingOid figi-gii:hasUniqueTextIdentifier "FLOATING, OID" .

figi-ps:GSAG figi-gii:hasUniqueTextIdentifier "GSAG" .

figi-ps:BLG2 a owl:NamedIndividual .

figi-ps:ALFB a owl:NamedIndividual .

figi-ps:GSAM a owl:NamedIndividual .

figi-ps:BLG2 a figi-gii:PricingSource .

figi-ps:ALFB a figi-gii:PricingSource .

figi-ps:BLG2 skos:prefLabel "blp internal g2" .

figi-ps:GSAM a figi-gii:PricingSource .

figi-ps:BLG2 figi-gii:hasUniqueTextIdentifier "BLG2" .

figi-ps:ALFB skos:prefLabel "alfa bank" .

figi-ps:GSAM skos:prefLabel "goldman sachs ast mg" .

figi-ps:BLG3 a owl:NamedIndividual .

figi-ps:ALFB figi-gii:hasUniqueTextIdentifier "ALFB" .

figi-ps:BLG3 a figi-gii:PricingSource .

figi-ps:GSAM figi-gii:hasUniqueTextIdentifier "GSAM" .

figi-ps:BLG3 skos:prefLabel "blp internal g3" .

figi-st:foreignSh a owl:NamedIndividual .

figi-ps:BLG3 figi-gii:hasUniqueTextIdentifier "BLG3" .

figi-ps:GSAN a owl:NamedIndividual .

figi-st:foreignSh a figi-gii:SecurityType .

figi-ps:GSAN a figi-gii:PricingSource .

figi-ps:BLG4 a owl:NamedIndividual , figi-gii:PricingSource .

figi-ps:GSAN skos:prefLabel "greenwich cap boom" .

figi-ps:BLG4 skos:prefLabel "blp internal g4" .

figi-ps:GSAN figi-gii:hasUniqueTextIdentifier "GSAN" .

figi-ps:BLG4 figi-gii:hasUniqueTextIdentifier "BLG4" .

figi-st:foreignSh skos:definition "Foreign Share is a common stock, but it is the foreign line of the security and it trades on the foreign board. The foreign board was set up as an alternative board for foreign investors seeking direct ownership of securities" .

figi-ps:BLG5 a owl:NamedIndividual .

figi-ps:GSAX a owl:NamedIndividual .

figi-ps:BLG5 a figi-gii:PricingSource .

figi-st:foreignSh skos:prefLabel "foreign sh." .

figi-ps:BLG5 skos:prefLabel "bval internal icap" .

figi-ps:GSAX a figi-gii:PricingSource .

figi-st:foreignSh figi-gii:hasUniqueTextIdentifier "Foreign Sh." .

figi-ps:BLG5 figi-gii:hasUniqueTextIdentifier "BLG5" .

figi-ps:GSAX skos:prefLabel "gs japan eqd" .

figi-ps:ALFI a owl:NamedIndividual .

figi-ps:GSAX figi-gii:hasUniqueTextIdentifier "GSAX" .

figi-ps:BLIP a owl:NamedIndividual .

figi-ps:ALFI a figi-gii:PricingSource .

figi-ps:BLIP a figi-gii:PricingSource .

figi-ps:GSBT a owl:NamedIndividual .

figi-ps:BLIP skos:prefLabel "bank lippo" .

figi-ps:ALFI skos:prefLabel "alpha finance" .

figi-ps:GSBT a figi-gii:PricingSource .

figi-ps:BLIP figi-gii:hasUniqueTextIdentifier "BLIP" .

figi-ps:ALFI figi-gii:hasUniqueTextIdentifier "ALFI" .

figi-ps:GSBT skos:prefLabel "govt saving bank bkk" .

figi-ps:BLJC a owl:NamedIndividual .

figi-st:forward a owl:NamedIndividual .

figi-ps:BLJC a figi-gii:PricingSource .

figi-ps:GSBT figi-gii:hasUniqueTextIdentifier "GSBT" .

figi-st:forward a figi-gii:SecurityType .

figi-ps:BLJC skos:prefLabel "banco lj carregosa" .

figi-ps:GSCO a owl:NamedIndividual .

figi-ps:BLJC figi-gii:hasUniqueTextIdentifier "BLJC" .

figi-ps:GSCO a figi-gii:PricingSource .

figi-ps:BLKB a owl:NamedIndividual .

figi-ps:GSCO skos:prefLabel "goldman sachs ny spd" .

figi-st:forward skos:definition "Forward. A financial instrument an investor sells for future delivery. This act is in direct violation of federal securities laws." .

figi-ps:BLKB a figi-gii:PricingSource .

figi-ps:GSCO figi-gii:hasUniqueTextIdentifier "GSCO" .

figi-ps:BLKB skos:prefLabel "blackbird america" .

figi-st:forward skos:prefLabel "forward" .

figi-ps:BLKB figi-gii:hasUniqueTextIdentifier "BLKB" .

figi-ps:GSCT a owl:NamedIndividual .

figi-st:forward figi-gii:hasUniqueTextIdentifier "FORWARD" .

figi-ps:GSCT a figi-gii:PricingSource .

figi-ps:BLN a owl:NamedIndividual .

figi-ps:GSCT skos:prefLabel "goldman sachs" .

figi-ps:BLN a figi-gii:PricingSource .

figi-ps:GSCT figi-gii:hasUniqueTextIdentifier "GSCT" .

figi-ps:BLN skos:prefLabel "bln securities" .

figi-ps:GSCV a owl:NamedIndividual .

figi-ps:BLN figi-gii:hasUniqueTextIdentifier "BLN" .

figi-ps:GSCV a figi-gii:PricingSource .

figi-ps:BLN1 a owl:NamedIndividual , figi-gii:PricingSource .

figi-ps:GSCV skos:prefLabel "goldman sachs cvts" .

figi-ps:BLN1 skos:prefLabel "blp internal n1" .

figi-ps:GSCV figi-gii:hasUniqueTextIdentifier "GSCV" .

figi-ps:BLN1 figi-gii:hasUniqueTextIdentifier "BLN1" .

figi-ps:GSDN a owl:NamedIndividual .

figi-ps:BLN2 a owl:NamedIndividual .

figi-ps:GSDN a figi-gii:PricingSource .

figi-ps:BLN2 a figi-gii:PricingSource .

figi-ps:GSDN skos:prefLabel "goldman sachs boom" .

figi-ps:BLN2 skos:prefLabel "blp internal n2" .

figi-ps:GSDN figi-gii:hasUniqueTextIdentifier "GSDN" .

figi-ps:BLN2 figi-gii:hasUniqueTextIdentifier "BLN2" .

figi-ps:GSEB a owl:NamedIndividual .

figi-ps:BLN3 a owl:NamedIndividual .

figi-ps:GSEB a figi-gii:PricingSource .

figi-ps:BLN3 a figi-gii:PricingSource .

figi-ps:GSEB skos:prefLabel "goldman sachs credit" .

figi-ps:BLN3 skos:prefLabel "blp internal n3" .

figi-ps:GSEB figi-gii:hasUniqueTextIdentifier "GSEB" .

figi-ps:BLN3 figi-gii:hasUniqueTextIdentifier "BLN3" .

figi-ps:GSEC a owl:NamedIndividual .

figi-ps:BLOM a owl:NamedIndividual .

figi-ps:GSEC a figi-gii:PricingSource .

figi-ps:BLOM a figi-gii:PricingSource .

figi-ps:GSEC skos:prefLabel "goldman sachs credit" .

figi-ps:BLOM skos:prefLabel "blominvest bank sal" .

figi-ps:GSEC figi-gii:hasUniqueTextIdentifier "GSEC" .

figi-ps:BLOM figi-gii:hasUniqueTextIdentifier "BLOM" .

figi-ps:GSEF a owl:NamedIndividual .

figi-ps:BLOX a owl:NamedIndividual .

figi-ps:GSEF a figi-gii:PricingSource .

figi-ps:BLOX a figi-gii:PricingSource ;
	skos:prefLabel "bloxham" .

figi-ps:GSEF skos:prefLabel "goldman sachs corp" .

figi-ps:BLOX figi-gii:hasUniqueTextIdentifier "BLOX" .

figi-ps:GSEF figi-gii:hasUniqueTextIdentifier "GSEF" .

figi-ps:BLPP a owl:NamedIndividual , figi-gii:PricingSource .

figi-ps:GSEM a owl:NamedIndividual .

figi-ps:BLPP skos:prefLabel "bloomberg ts price" .

figi-ps:GSEM a figi-gii:PricingSource .

figi-ps:BLPP figi-gii:hasUniqueTextIdentifier "BLPP" .

figi-ps:GSEM skos:prefLabel "goldman sachs em" .

figi-ps:BLPY a owl:NamedIndividual , figi-gii:PricingSource .

figi-ps:GSEM skos:prefLabel "goldman sachs ny" .

figi-ps:BLPY skos:prefLabel "bloomberg ts yield" .

figi-ps:GSEM figi-gii:hasUniqueTextIdentifier "GSEM" .

figi-ps:BLPY figi-gii:hasUniqueTextIdentifier "BLPY" .

figi-ps:GSFH a owl:NamedIndividual .

figi-ps:BLR a owl:NamedIndividual .

figi-ps:GSFH a figi-gii:PricingSource .

figi-ps:BLR a figi-gii:PricingSource .

figi-ps:GSFH skos:prefLabel "guosen sec (hk)" .

figi-ps:BLR skos:prefLabel "blair,(william)andco" .

figi-ps:GSFH figi-gii:hasUniqueTextIdentifier "GSFH" .

figi-ps:BLR figi-gii:hasUniqueTextIdentifier "BLR" .

figi-ps:GSGL a owl:NamedIndividual .

figi-ps:BLRD a owl:NamedIndividual .

figi-ps:GSGL a figi-gii:PricingSource .

figi-ps:BLRD a figi-gii:PricingSource .

figi-ps:GSGL skos:prefLabel "gas strategies group" .

figi-ps:BLRD skos:prefLabel "banco leon" .

figi-ps:GSGL figi-gii:hasUniqueTextIdentifier "GSGL" .

figi-ps:BLRD figi-gii:hasUniqueTextIdentifier "BLRD" .

figi-ps:GSI a owl:NamedIndividual .

figi-ps:BLSE a owl:NamedIndividual .

figi-ps:GSI a figi-gii:PricingSource .

figi-ps:BLSE a figi-gii:PricingSource .

figi-ps:GSI skos:prefLabel "global strategic inv" .

figi-ps:BLSE skos:prefLabel "banja luka se" .

figi-ps:GSI figi-gii:hasUniqueTextIdentifier "GSI" .

figi-ps:BLSE figi-gii:hasUniqueTextIdentifier "BLSE" .

figi-ps:GSIM a owl:NamedIndividual .

figi-ps:ALFM a owl:NamedIndividual .

figi-ps:GSIM a figi-gii:PricingSource .

figi-ps:BLT a owl:NamedIndividual .

figi-ps:ALFM a figi-gii:PricingSource .

figi-ps:BLT a figi-gii:PricingSource .

figi-ps:GSIM skos:prefLabel "gatten sadowski inc" .

figi-ps:ALFM skos:prefLabel "alfa bank cjsc" .

figi-ps:BLT skos:prefLabel "comm bank baltikums" .

figi-ps:GSIM figi-gii:hasUniqueTextIdentifier "GSIM" .

figi-ps:ALFM figi-gii:hasUniqueTextIdentifier "ALFM" .

figi-ps:BLT figi-gii:hasUniqueTextIdentifier "BLT" .

figi-ps:GSIT a owl:NamedIndividual .

figi-st:forwardCross a owl:NamedIndividual .

figi-ps:GSIT a figi-gii:PricingSource .

figi-ps:BLTD a owl:NamedIndividual .

figi-st:forwardCross a figi-gii:SecurityType .

figi-ps:GSIT skos:prefLabel "global strategic inv" .

figi-ps:BLTD a figi-gii:PricingSource .

figi-ps:GSIT figi-gii:hasUniqueTextIdentifier "GSIT" .

figi-st:forwardCross skos:definition "Same as a forward but traded currencies do not follow spot conventions." .

figi-ps:BLTD skos:prefLabel "bourse securities" .

figi-ps:GSLP a owl:NamedIndividual .

figi-st:forwardCross skos:prefLabel "forward cross" .

figi-ps:GSLP a figi-gii:PricingSource .

figi-ps:BLTD figi-gii:hasUniqueTextIdentifier "BLTD" .

figi-ps:GSLP skos:prefLabel "global secs ltd" .

figi-st:forwardCross figi-gii:hasUniqueTextIdentifier "FORWARD CROSS" .

figi-ps:GSLP figi-gii:hasUniqueTextIdentifier "GSLP" .

figi-ps:BLTK a owl:NamedIndividual .

figi-ps:ALGO a owl:NamedIndividual .

figi-ps:GSLT a owl:NamedIndividual .

figi-ps:ALGO a figi-gii:PricingSource .

figi-ps:GSLT a figi-gii:PricingSource .

figi-ps:ALGO skos:prefLabel "inforalgo test" .

figi-ps:GSLT skos:prefLabel "gs em trading" .

figi-ps:ALGO figi-gii:hasUniqueTextIdentifier "ALGO" .

figi-ps:GSLT figi-gii:hasUniqueTextIdentifier "GSLT" .

figi-st:forwardCurve a owl:NamedIndividual .

figi-ps:GSM a owl:NamedIndividual .

figi-st:forwardCurve a figi-gii:SecurityType .

figi-ps:GSM a figi-gii:PricingSource .

figi-ps:BLTK a figi-gii:PricingSource .

figi-ps:GSM skos:prefLabel "gesmadrid" .

figi-ps:BLTK skos:prefLabel "bulltick llc" .

figi-ps:GSM figi-gii:hasUniqueTextIdentifier "GSM" .

figi-ps:BLTK figi-gii:hasUniqueTextIdentifier "BLTK" .

figi-st:forwardCurve skos:definition "The forward rates over different time periods" .

figi-ps:BLTN a owl:NamedIndividual .

figi-ps:GSMB a owl:NamedIndividual .

figi-ps:BLTN a figi-gii:PricingSource .

figi-st:forwardCurve skos:prefLabel "forward curve" .

figi-ps:GSMB a figi-gii:PricingSource .

figi-ps:BLTN skos:prefLabel "beltone financial" .

figi-st:forwardCurve figi-gii:hasUniqueTextIdentifier "FORWARD CURVE" .

figi-ps:ALI a owl:NamedIndividual , figi-gii:PricingSource ;
	skos:prefLabel "alico" ;
	figi-gii:hasUniqueTextIdentifier "ALI" .

figi-st:fra a owl:NamedIndividual , figi-gii:SecurityType ;
	skos:definition "Forward rate agreements are common OTC financial derivatives in which the buyer or seller will be compensated based upon the difference between an agreed upon future interest rate level and the realized interest rate. The contract will determine the rates to be used along with the termination date and notional value. On this type of agreement, it is only the differential that is paid on the notional amount of the contract." ;
	skos:prefLabel "fra" ;
	figi-gii:hasUniqueTextIdentifier "FRA" .

figi-ps:ALIC a owl:NamedIndividual , figi-gii:PricingSource ;
	skos:prefLabel "allstate life ins co" ;
	figi-gii:hasUniqueTextIdentifier "ALIC" .

figi-st:frenchCD a owl:NamedIndividual , figi-gii:SecurityType ;
	skos:definition "French Domestic Certificates of Deposit" ;
	skos:prefLabel "french cd" ;
	figi-gii:hasUniqueTextIdentifier "FRENCH CD" .

figi-st:frenchCP a owl:NamedIndividual , figi-gii:SecurityType ;
	skos:definition "French Domestic Commercial Paper" ;
	skos:prefLabel "french cp" ;
	figi-gii:hasUniqueTextIdentifier "FRENCH CP" .

figi-ps:GSMB skos:prefLabel "goldman sachs mtge" .

figi-ps:ALKN a owl:NamedIndividual .

figi-ps:GSMB figi-gii:hasUniqueTextIdentifier "GSMB" .

figi-ps:ALKN a figi-gii:PricingSource .

figi-ps:GSMS a owl:NamedIndividual , figi-gii:PricingSource ;
	skos:prefLabel "goldman sachs and co." ;
	figi-gii:hasUniqueTextIdentifier "GSMS" .

figi-ps:ALKN skos:prefLabel "alken asset mgmt" .

figi-ps:GSSB a owl:NamedIndividual .

figi-ps:ALKN figi-gii:hasUniqueTextIdentifier "ALKN" .

figi-ps:GSSB a figi-gii:PricingSource .

figi-st:frenchCert a owl:NamedIndividual .

figi-ps:GSSB skos:prefLabel "goldman sachs sb" .

figi-st:frenchCert a figi-gii:SecurityType .

figi-ps:GSSB figi-gii:hasUniqueTextIdentifier "GSSB" .

figi-st:frenchCert skos:definition "French Certificate - Depositary Receipt issued in France" ;
	skos:prefLabel "french cert" ;
	figi-gii:hasUniqueTextIdentifier "French Cert" .

figi-ps:GSSD a owl:NamedIndividual .

figi-ps:ALL a owl:NamedIndividual .

figi-ps:BLTN figi-gii:hasUniqueTextIdentifier "BLTN" .

figi-ps:GSSD a figi-gii:PricingSource .

figi-ps:ALL a figi-gii:PricingSource .

figi-ps:BLTR a owl:NamedIndividual .

figi-ps:GSSD skos:prefLabel "goldman sachs sd" .

figi-ps:ALL skos:prefLabel "allstate" .

figi-ps:BLTR a figi-gii:PricingSource .

figi-ps:GSSD figi-gii:hasUniqueTextIdentifier "GSSD" .

figi-ps:BLTR skos:prefLabel "bulltick argentina" .

figi-ps:ALL figi-gii:hasUniqueTextIdentifier "ALL" .

figi-ps:GSSN a owl:NamedIndividual .

figi-ps:BLTR figi-gii:hasUniqueTextIdentifier "BLTR" .

figi-ps:GSSN a figi-gii:PricingSource .

figi-st:fundOfFunds a owl:NamedIndividual .

figi-ps:GSSN skos:prefLabel "goldman sachs sn" .

figi-ps:BLTS a owl:NamedIndividual .

figi-st:fundOfFunds a figi-gii:SecurityType .

figi-ps:GSSN figi-gii:hasUniqueTextIdentifier "GSSN" .

figi-ps:BLTS a figi-gii:PricingSource .

figi-st:fundOfFunds skos:definition "A mutual fund that invests in other mutual funds." .

figi-ps:BLTS skos:prefLabel "bank baltikums" .

figi-ps:GSTY a owl:NamedIndividual .

figi-st:fundOfFunds skos:prefLabel "fund of funds" .

figi-ps:GSTY a figi-gii:PricingSource .

figi-ps:BLTS figi-gii:hasUniqueTextIdentifier "BLTS" .

figi-st:fundOfFunds figi-gii:hasUniqueTextIdentifier "Fund of Funds" .

figi-ps:GSTY skos:prefLabel "goldman sachs trsy" .

figi-ps:BLTU a owl:NamedIndividual .

figi-st:future a owl:NamedIndividual .

figi-ps:GSTY figi-gii:hasUniqueTextIdentifier "GSTY" .

figi-ps:BLTU a figi-gii:PricingSource .

figi-st:future a figi-gii:SecurityType .

figi-ps:GSUS a owl:NamedIndividual .

figi-ps:BLTU skos:prefLabel "bulltick" .

figi-ps:GSUS a figi-gii:PricingSource .

figi-ps:BLTU figi-gii:hasUniqueTextIdentifier "BLTU" .

figi-st:future skos:definition "An exchange-traded contract that obligates the buyer to purchase an asset at a pre-specified future date and price" .

figi-ps:GSUS skos:prefLabel "goldman sachs 144" .

figi-st:future skos:prefLabel "future" .

figi-ps:BLUE a owl:NamedIndividual .

figi-st:future figi-gii:hasUniqueTextIdentifier "FUTURE" .

figi-ps:BLUE a figi-gii:PricingSource .

figi-ps:ALLB a owl:NamedIndividual .

figi-ps:BLUE skos:prefLabel "blue edge advisors" .

figi-ps:ALLB a figi-gii:PricingSource .

figi-ps:BLUE figi-gii:hasUniqueTextIdentifier "BLUE" .

figi-ps:ALLB skos:prefLabel "allahabad bank" .

figi-ps:BLUK a owl:NamedIndividual .

figi-ps:ALLB figi-gii:hasUniqueTextIdentifier "ALLB" .

figi-ps:BLUK a figi-gii:PricingSource .

figi-st:fwdSwap a owl:NamedIndividual .

figi-ps:BLUK skos:prefLabel "bank leumi plc" .

figi-st:fwdSwap a figi-gii:SecurityType .

figi-ps:BLUK figi-gii:hasUniqueTextIdentifier "BLUK" .

figi-st:fwdSwap skos:definition "Forward starting swap, swap starting in a future date" .

figi-ps:BLUM a owl:NamedIndividual .

figi-ps:GSUS figi-gii:hasUniqueTextIdentifier "GSUS" .

figi-ps:BLUM a figi-gii:PricingSource .

figi-st:fwdSwap skos:prefLabel "fwd swap" .

figi-ps:GSVS a owl:NamedIndividual .

figi-ps:BLUM skos:prefLabel "blumont capital corp" .

figi-ps:GSVS a figi-gii:PricingSource .

figi-st:fwdSwap figi-gii:hasUniqueTextIdentifier "FWD SWAP" .

figi-ps:BLUM figi-gii:hasUniqueTextIdentifier "BLUM" .

figi-ps:GSVS skos:prefLabel "goldman sachs ny" .

figi-ps:BLUO a owl:NamedIndividual .

figi-ps:GSVS figi-gii:hasUniqueTextIdentifier "GSVS" .

figi-ps:GSWB a owl:NamedIndividual , figi-gii:PricingSource .

figi-ps:BLUO a figi-gii:PricingSource .

figi-ps:GSWB skos:prefLabel "goldman sachs wb" .

figi-ps:BLUO skos:prefLabel "blue oak capital" .

figi-ps:GSWB figi-gii:hasUniqueTextIdentifier "GSWB" .

figi-ps:BLUO figi-gii:hasUniqueTextIdentifier "BLUO" .

figi-ps:GSZT a owl:NamedIndividual .

figi-ps:BLUS a owl:NamedIndividual .

figi-ps:GSZT a figi-gii:PricingSource .

figi-ps:BLUS a figi-gii:PricingSource .

figi-ps:GSZT skos:prefLabel "goldman sachs tokyo" .

figi-ps:BLUS skos:prefLabel "bank leumi toms" .

figi-ps:GSZT figi-gii:hasUniqueTextIdentifier "GSZT" .

figi-ps:BLUS figi-gii:hasUniqueTextIdentifier "BLUS" .

figi-ps:GTAM a owl:NamedIndividual .

figi-ps:BLXB a owl:NamedIndividual .

figi-ps:GTAM a figi-gii:PricingSource .

figi-ps:BLXB a figi-gii:PricingSource .

figi-ps:GTAM skos:prefLabel "china guotai fund" .

figi-ps:BLXB skos:prefLabel "banque luxembourg" .

figi-ps:GTAM figi-gii:hasUniqueTextIdentifier "GTAM" .

figi-ps:BLXB figi-gii:hasUniqueTextIdentifier "BLXB" .

figi-ps:GTBN a owl:NamedIndividual .

figi-ps:BMA a owl:NamedIndividual .

figi-ps:GTBN a figi-gii:PricingSource .

figi-ps:BMA a figi-gii:PricingSource .

figi-ps:GTBN skos:prefLabel "guaranty trust bank" .

figi-ps:BMA skos:prefLabel "jse-besa exch" .

figi-ps:GTBN figi-gii:hasUniqueTextIdentifier "GTBN" .

figi-ps:BMA figi-gii:hasUniqueTextIdentifier "BMA" .

figi-ps:GTCB a owl:NamedIndividual , figi-gii:PricingSource .

figi-ps:BMAM a owl:NamedIndividual .

figi-ps:GTCB skos:prefLabel "global trading pte" .

figi-ps:BMAM a figi-gii:PricingSource .

figi-ps:GTCB figi-gii:hasUniqueTextIdentifier "GTCB" .

figi-ps:BMAM skos:prefLabel "bma capital mgt" ;
	figi-gii:hasUniqueTextIdentifier "BMAM" .

figi-ps:GTJA a owl:NamedIndividual .

figi-ps:BMAR a owl:NamedIndividual .

figi-ps:GTJA a figi-gii:PricingSource .

figi-ps:BMAR a figi-gii:PricingSource .

figi-ps:GTJA skos:prefLabel "cfet guotai junan se" .

figi-ps:BMAR skos:prefLabel "banco mariva" .

figi-ps:GTJA figi-gii:hasUniqueTextIdentifier "GTJA" .

figi-ps:BMAR figi-gii:hasUniqueTextIdentifier "BMAR" .

figi-ps:ALLG a owl:NamedIndividual .

figi-ps:GTJN a owl:NamedIndividual .

figi-ps:BMAS a owl:NamedIndividual .

figi-ps:ALLG a figi-gii:PricingSource .

figi-ps:GTJN a figi-gii:PricingSource .

figi-ps:BMAS a figi-gii:PricingSource .

figi-ps:ALLG skos:prefLabel "allegiant asset mgmt" .

figi-ps:GTJN skos:prefLabel "guotai junan hk ltd" .

figi-ps:ALLG figi-gii:hasUniqueTextIdentifier "ALLG" .

figi-ps:BMAS skos:prefLabel "bma securities" .

figi-ps:GTJN figi-gii:hasUniqueTextIdentifier "GTJN" .

figi-ps:BMAS figi-gii:hasUniqueTextIdentifier "BMAS" .

figi-ps:GTMD a owl:NamedIndividual .

figi-ps:BMBX a owl:NamedIndividual .

figi-ps:GTMD a figi-gii:PricingSource .

figi-ps:BMBX a figi-gii:PricingSource .

figi-ps:GTMD skos:prefLabel "gestimed" .

figi-ps:BMBX skos:prefLabel "banca mb" .

figi-ps:GTMD figi-gii:hasUniqueTextIdentifier "GTMD" .

figi-ps:BMBX figi-gii:hasUniqueTextIdentifier "BMBX" .

figi-ps:GTOP a owl:NamedIndividual .

figi-ps:BMCC a owl:NamedIndividual .

figi-ps:GTOP a figi-gii:PricingSource .

figi-ps:BMCC a figi-gii:PricingSource .

figi-ps:GTOP skos:prefLabel "gretai otcbond price" .

figi-ps:BMCC skos:prefLabel "brean murray, carret" .

figi-ps:GTOP skos:prefLabel "tpex otcbond price" .

figi-ps:BMCC figi-gii:hasUniqueTextIdentifier "BMCC" .

figi-ps:GTOP figi-gii:hasUniqueTextIdentifier "GTOP" .

figi-ps:BMCE a owl:NamedIndividual .

figi-ps:GTOY a owl:NamedIndividual .

figi-ps:BMCE a figi-gii:PricingSource .

figi-ps:GTOY a figi-gii:PricingSource .

figi-ps:BMCE skos:prefLabel "bmce capital" .

figi-ps:GTOY skos:prefLabel "gretai otcbond yield" .

figi-ps:BMCE figi-gii:hasUniqueTextIdentifier "BMCE" .

figi-ps:GTOY skos:prefLabel "tpex otcbond yield" .

figi-ps:BMCN a owl:NamedIndividual .

figi-ps:GTOY figi-gii:hasUniqueTextIdentifier "GTOY" .

figi-ps:BMCN a figi-gii:PricingSource .

figi-ps:GTQ1 a owl:NamedIndividual .

figi-ps:BMCN skos:prefLabel "bank of montreal chn" .

figi-ps:GTQ1 a figi-gii:PricingSource .

figi-ps:BMCN figi-gii:hasUniqueTextIdentifier "BMCN" .

figi-ps:GTQ1 skos:prefLabel "gtsm lstquote yield" .

figi-ps:BMEC a owl:NamedIndividual .

figi-ps:GTQ1 figi-gii:hasUniqueTextIdentifier "GTQ1" .

figi-ps:BMEC a figi-gii:PricingSource .

figi-ps:GTQ2 a owl:NamedIndividual .

figi-ps:BMEC skos:prefLabel "bolsa nacional mec" .

figi-ps:GTQ2 a figi-gii:PricingSource .

figi-ps:BMEC figi-gii:hasUniqueTextIdentifier "BMEC" .

figi-ps:GTQ2 skos:prefLabel "gtsm vwavg yield" .

figi-ps:BMF0 a owl:NamedIndividual .

figi-ps:GTQ2 figi-gii:hasUniqueTextIdentifier "GTQ2" .

figi-ps:BMF0 a figi-gii:PricingSource .

figi-ps:GTQ3 a owl:NamedIndividual .

figi-ps:BMF0 skos:prefLabel "bmf sisbex fwd 1d" .

figi-ps:GTQ3 a figi-gii:PricingSource .

figi-ps:BMF0 figi-gii:hasUniqueTextIdentifier "BMF0" .

figi-ps:GTQ3 skos:prefLabel "gtsm theory price" .

figi-ps:BMF1 a owl:NamedIndividual .

figi-ps:GTQ3 figi-gii:hasUniqueTextIdentifier "GTQ3" .

figi-ps:BMF1 a figi-gii:PricingSource .

figi-ps:GTQY a owl:NamedIndividual .

figi-st:fxDiscountNote a owl:NamedIndividual .

figi-ps:GTQY a figi-gii:PricingSource .

figi-st:fxDiscountNote a figi-gii:SecurityType ;
	skos:definition "Setup for Fixed Rate Agency Discount Notes" .

figi-ps:GTQY skos:prefLabel "gretai otcquoteyeild" .

figi-st:fxDiscountNote skos:prefLabel "fx discount note" .

figi-ps:GTQY figi-gii:hasUniqueTextIdentifier "GTQY" .

figi-ps:BMF1 skos:prefLabel "bmf sisbex fw 2-23d" .

figi-ps:GTRU a owl:NamedIndividual .

figi-ps:BMF1 figi-gii:hasUniqueTextIdentifier "BMF1" .

figi-ps:GTRU a figi-gii:PricingSource .

figi-st:fxDiscountNote figi-gii:hasUniqueTextIdentifier "FX DISCOUNT NOTE" .

figi-ps:GTRU skos:prefLabel "goldman sachs 144a" .

figi-ps:BMFR a owl:NamedIndividual .

figi-ps:GTRU figi-gii:hasUniqueTextIdentifier "GTRU" .

figi-ps:ALLI a owl:NamedIndividual .

figi-ps:GUAY a owl:NamedIndividual .

figi-ps:BMFR a figi-gii:PricingSource .

figi-ps:GUAY a figi-gii:PricingSource .

figi-ps:ALLI a figi-gii:PricingSource .

figi-ps:BMFR skos:prefLabel "bmf reference prices" .

figi-ps:GUAY skos:prefLabel "banco de guayaquil" .

figi-ps:ALLI skos:prefLabel "allianz asset mgmt" .

figi-ps:GUAY figi-gii:hasUniqueTextIdentifier "GUAY" .

figi-ps:ALLI figi-gii:hasUniqueTextIdentifier "ALLI" .

figi-ps:GUGG a owl:NamedIndividual .

figi-ps:BMFR figi-gii:hasUniqueTextIdentifier "BMFR" .

figi-ps:GUGG a figi-gii:PricingSource .

figi-ps:BMFZ a owl:NamedIndividual .

figi-st:gdr a owl:NamedIndividual .

figi-ps:BMFZ a figi-gii:PricingSource .

figi-st:gdr a figi-gii:SecurityType .

figi-ps:BMFZ skos:prefLabel "bmf sisbex cash" .

figi-ps:GUGG skos:prefLabel "guggenheim cap mkts" .

figi-ps:BMFZ figi-gii:hasUniqueTextIdentifier "BMFZ" .

figi-st:gdr skos:definition "Global Depository Receipts. (GDR) A negotiable certificate held in the bank of one country representing a specific number of shares of a stock traded on an exchange of another country." .

figi-ps:GUGG figi-gii:hasUniqueTextIdentifier "GUGG" .

figi-ps:BMIB a owl:NamedIndividual .

figi-st:gdr skos:prefLabel "gdr" .

figi-ps:GURT a owl:NamedIndividual .

figi-ps:BMIB a figi-gii:PricingSource .

figi-ps:GURT a figi-gii:PricingSource .

figi-ps:BMIB skos:prefLabel "bmi bank" .

figi-ps:GURT skos:prefLabel "gurtin fixed income" .

figi-ps:BMIB figi-gii:hasUniqueTextIdentifier "BMIB" .

figi-ps:GURT figi-gii:hasUniqueTextIdentifier "GURT" .

figi-ps:BMIC a owl:NamedIndividual .

figi-st:gdr figi-gii:hasUniqueTextIdentifier "GDR" .

figi-ps:BMIC a figi-gii:PricingSource .

figi-ps:GUYB a owl:NamedIndividual .

figi-st:genericCurrencyFuture a owl:NamedIndividual .

figi-ps:GUYB a figi-gii:PricingSource .

figi-ps:BMIC skos:prefLabel "biltmore internation" .

figi-st:genericCurrencyFuture a figi-gii:SecurityType .

figi-ps:GUYB skos:prefLabel "guy butler" .

figi-ps:BMIC figi-gii:hasUniqueTextIdentifier "BMIC" .

figi-st:genericCurrencyFuture skos:definition "Futures contracts on major currencies" .

figi-ps:GUYB figi-gii:hasUniqueTextIdentifier "GUYB" .

figi-ps:BMJA a owl:NamedIndividual .

figi-st:genericCurrencyFuture skos:prefLabel "generic currency future." .

figi-ps:BMJA a figi-gii:PricingSource .

figi-ps:GUYM a owl:NamedIndividual .

figi-st:genericCurrencyFuture figi-gii:hasUniqueTextIdentifier "Generic currency future." .

figi-ps:GUYM a figi-gii:PricingSource .

figi-ps:ALM a owl:NamedIndividual .

figi-ps:BMJA skos:prefLabel "bank mega" .

figi-ps:GUYM skos:prefLabel "guy butler - mtges" .

figi-ps:BMJA figi-gii:hasUniqueTextIdentifier "BMJA" .

figi-ps:ALM a figi-gii:PricingSource .

figi-ps:GUYM figi-gii:hasUniqueTextIdentifier "GUYM" .

figi-ps:ALM skos:prefLabel "alm brand" .

figi-ps:BMKS a owl:NamedIndividual , figi-gii:PricingSource .

figi-ps:ALM figi-gii:hasUniqueTextIdentifier "ALM" .

figi-ps:GVI a owl:NamedIndividual .

figi-ps:BMKS skos:prefLabel "benchmark securities" .

figi-st:genericIndexFuture a owl:NamedIndividual .

figi-ps:GVI a figi-gii:PricingSource .

figi-ps:BMKS figi-gii:hasUniqueTextIdentifier "BMKS" .

figi-st:genericIndexFuture a figi-gii:SecurityType .

figi-ps:GVI skos:prefLabel "global value inv." .

figi-ps:BML a owl:NamedIndividual .

figi-ps:GVI figi-gii:hasUniqueTextIdentifier "GVI" .

figi-ps:BML a figi-gii:PricingSource .

figi-st:genericIndexFuture skos:definition "Generics on Index Futures. Generics are used to combine multiple futures contracts to build a generic history stream." .

figi-ps:GVP3 a owl:NamedIndividual .

figi-ps:BML skos:prefLabel "banca mediolanum spa" .

figi-ps:GVP3 a figi-gii:PricingSource .

figi-st:genericIndexFuture skos:prefLabel "generic index future." .

figi-ps:BML figi-gii:hasUniqueTextIdentifier "BML" .

figi-ps:GVP3 skos:prefLabel "govpx 3pm end of day" .

figi-st:genericIndexFuture figi-gii:hasUniqueTextIdentifier "Generic index future." .

figi-ps:GVP3 figi-gii:hasUniqueTextIdentifier "GVP3" .

figi-ps:BMLA a owl:NamedIndividual .

figi-ps:GVP4 a owl:NamedIndividual .

figi-ps:ALMA a owl:NamedIndividual .

figi-ps:GVP4 a figi-gii:PricingSource .

figi-ps:ALMA a figi-gii:PricingSource .

figi-ps:GVP4 skos:prefLabel "govpx 4pm end of day" .

figi-ps:ALMA skos:prefLabel "al masah capital ltd" .

figi-ps:GVP4 figi-gii:hasUniqueTextIdentifier "GVP4" .

figi-ps:ALMA figi-gii:hasUniqueTextIdentifier "ALMA" .

figi-ps:BMLA a figi-gii:PricingSource .

figi-st:germanCP a owl:NamedIndividual .

figi-ps:BMLA skos:prefLabel "bofa merrill lynch" .

figi-ps:GVP5 a owl:NamedIndividual .

figi-st:germanCP a figi-gii:SecurityType .

figi-ps:BMLA figi-gii:hasUniqueTextIdentifier "BMLA" .

figi-ps:GVP5 a figi-gii:PricingSource .

figi-ps:BMLE a owl:NamedIndividual .

figi-st:germanCP skos:definition "German Domestic Commercial Paper" .

figi-ps:BMLE a figi-gii:PricingSource .

figi-st:germanCP skos:prefLabel "german cp" .

figi-ps:GVP5 skos:prefLabel "govpx 5pm end of day" .

figi-ps:BMLE skos:prefLabel "banco multiple leon" .

figi-st:germanCP figi-gii:hasUniqueTextIdentifier "GERMAN CP" .

figi-ps:GVP5 figi-gii:hasUniqueTextIdentifier "GVP5" .

figi-ps:BMLE figi-gii:hasUniqueTextIdentifier "BMLE" .

figi-ps:ALPH a owl:NamedIndividual .

figi-ps:GVRF a owl:NamedIndividual .

figi-ps:ALPH a figi-gii:PricingSource .

figi-ps:BMLL a owl:NamedIndividual .

figi-ps:GVRF a figi-gii:PricingSource .

figi-ps:ALPH skos:prefLabel "alpha bank a.e." .

figi-ps:BMLL a figi-gii:PricingSource .

figi-ps:GVRF skos:prefLabel "gvr company llc" .

figi-ps:ALPH figi-gii:hasUniqueTextIdentifier "ALPH" .

figi-ps:BMLL skos:prefLabel "bofa merrill lynch" .

figi-ps:GVRF figi-gii:hasUniqueTextIdentifier "GVRF" .

figi-ps:BMLL figi-gii:hasUniqueTextIdentifier "BMLL" .

figi-st:germanCert a owl:NamedIndividual .

figi-ps:GXC a owl:NamedIndividual .

figi-st:germanCert a figi-gii:SecurityType .

figi-ps:BMLU a owl:NamedIndividual .

figi-ps:GXC a figi-gii:PricingSource .

figi-ps:BMLU a figi-gii:PricingSource .

figi-ps:GXC skos:prefLabel "g x clarke" .

figi-ps:BMLU skos:prefLabel "bofa - baml" .

figi-st:germanCert skos:definition "Also known as Deutsches Zertifikat (German certificate). The DTZ identifies deposit receipts issued by German banks evidencing the ownership of foreign securities." .

figi-ps:GXC figi-gii:hasUniqueTextIdentifier "GXC" .

figi-st:germanCert skos:prefLabel "german cert" .

figi-ps:BMLU figi-gii:hasUniqueTextIdentifier "BMLU" .

figi-st:germanCert figi-gii:hasUniqueTextIdentifier "German Cert" .

figi-ps:GXCL a owl:NamedIndividual .

figi-ps:BMMM a owl:NamedIndividual .

figi-st:global a owl:NamedIndividual .

figi-ps:GXCL a figi-gii:PricingSource .

figi-ps:BMMM a figi-gii:PricingSource .

figi-st:global a figi-gii:SecurityType .

figi-ps:GXCL skos:prefLabel "gx clarke" .

figi-ps:BMMM skos:prefLabel "bmo cap mrkt ny" .

figi-ps:GXCL figi-gii:hasUniqueTextIdentifier "GXCL" .

figi-ps:BMMM figi-gii:hasUniqueTextIdentifier "BMMM" .

figi-ps:GXCM a owl:NamedIndividual .

figi-ps:BMMZ a owl:NamedIndividual .

figi-st:global skos:definition "Global Bond. A certificate representing the total debt of an issue. Such bonds are created to control the primary market distribution of an issue in compliance with selling restrictions in certain jurisdictions or because definitive bond certificates are not available. Also known as global certificate." .

figi-ps:GXCM a figi-gii:PricingSource .

figi-ps:BMMZ a figi-gii:PricingSource .

figi-st:global skos:prefLabel "global" .

figi-ps:GXCM skos:prefLabel "clarke (g.x.) and co." .

figi-ps:BMMZ skos:prefLabel "banque de mocambique" .

figi-st:global figi-gii:hasUniqueTextIdentifier "GLOBAL" .

figi-ps:GXCM skos:prefLabel "clarke (gx) and co" .

figi-ps:BMMZ figi-gii:hasUniqueTextIdentifier "BMMZ" .

figi-ps:ALPT a owl:NamedIndividual .

figi-ps:GXCM figi-gii:hasUniqueTextIdentifier "GXCM" .

figi-ps:BMNB a owl:NamedIndividual .

figi-ps:ALPT a figi-gii:PricingSource .

figi-ps:GYJJ a owl:NamedIndividual .

figi-ps:BMNB a figi-gii:PricingSource .

figi-ps:ALPT skos:prefLabel "alpha toronto" .

figi-ps:GYJJ a figi-gii:PricingSource .

figi-ps:BMNB skos:prefLabel "bmo capital markets" .

figi-ps:ALPT figi-gii:hasUniqueTextIdentifier "ALPT" .

figi-ps:BMNB figi-gii:hasUniqueTextIdentifier "BMNB" .

figi-ps:GYJJ skos:prefLabel "icbccs asset mgmt" .

figi-st:guaranteeFac a owl:NamedIndividual .

figi-ps:BMOB a owl:NamedIndividual .

figi-st:guaranteeFac a figi-gii:SecurityType .

figi-ps:GYJJ figi-gii:hasUniqueTextIdentifier "GYJJ" .

figi-ps:BMOB a figi-gii:PricingSource ;
	skos:prefLabel "bmo capital" .

figi-st:guaranteeFac skos:definition "Also known as a performance bond/guarantee, is a contingent liability which is issued by a bank to ensure/guarantee that an underlying project is completed. Similar to a letter of credit." .

figi-ps:BMOB figi-gii:hasUniqueTextIdentifier "BMOB" .

figi-st:guaranteeFac skos:prefLabel "guarantee fac" .

figi-ps:GZPC a owl:NamedIndividual .

figi-ps:BMOC a owl:NamedIndividual .

figi-st:guaranteeFac figi-gii:hasUniqueTextIdentifier "GUARANTEE FAC" .

figi-ps:BMOC a figi-gii:PricingSource .

figi-ps:GZPC a figi-gii:PricingSource .

figi-ps:ALPV a owl:NamedIndividual .

figi-ps:BMOC skos:prefLabel "bmo capital markets" .

figi-ps:ALPV a figi-gii:PricingSource .

figi-ps:GZPC skos:prefLabel "gazprombank" .

figi-ps:BMOC figi-gii:hasUniqueTextIdentifier "BMOC" .

figi-ps:ALPV skos:prefLabel "alpha toronto" .

figi-ps:GZPC figi-gii:hasUniqueTextIdentifier "GZPC" .

figi-ps:ALPV figi-gii:hasUniqueTextIdentifier "ALPV" .

figi-ps:BMOD a owl:NamedIndividual .

figi-ps:HA a owl:NamedIndividual .

figi-st:hb a owl:NamedIndividual .

figi-ps:BMOD a figi-gii:PricingSource .

figi-st:hb a figi-gii:SecurityType .

figi-ps:HA a figi-gii:PricingSource .

figi-ps:BMOD skos:prefLabel "bmo mrkt asset sw" .

figi-st:hb skos:definition "Hybrid (Only for CDO,CLO,CBO securities)" .

figi-ps:HA skos:prefLabel "hauck and aufhaeuser" .

figi-ps:BMOD figi-gii:hasUniqueTextIdentifier "BMOD" .

figi-ps:HA figi-gii:hasUniqueTextIdentifier "HA" .

figi-st:hb skos:prefLabel "hb" .

figi-ps:BMOM a owl:NamedIndividual .

figi-ps:HABU a owl:NamedIndividual .

figi-ps:BMOM a figi-gii:PricingSource .

figi-ps:HABU a figi-gii:PricingSource .

figi-ps:BMOM skos:prefLabel "bank montreal gkst" .

figi-st:hb figi-gii:hasUniqueTextIdentifier "HB" .

figi-ps:BMOM figi-gii:hasUniqueTextIdentifier "BMOM" .

figi-ps:ALRO a owl:NamedIndividual .

figi-ps:BMON a owl:NamedIndividual .

figi-ps:ALRO a figi-gii:PricingSource .

figi-ps:BMON a figi-gii:PricingSource .

figi-ps:ALRO skos:prefLabel "alpha bank" .

figi-ps:BMON skos:prefLabel "bank of montreal" .

figi-ps:ALRO figi-gii:hasUniqueTextIdentifier "ALRO" .

figi-ps:BMON figi-gii:hasUniqueTextIdentifier "BMON" .

figi-st:hdr a owl:NamedIndividual .

figi-ps:BMRU a owl:NamedIndividual .

figi-st:hdr a figi-gii:SecurityType .

figi-ps:BMRU a figi-gii:PricingSource .

figi-st:hdr skos:definition "Hong Kong Depository Receipt" .

figi-ps:HABU skos:prefLabel "habubank securities" .

figi-ps:BMRU skos:prefLabel "banco mariva (usd)" .

figi-st:hdr skos:prefLabel "hdr" .

figi-ps:HABU figi-gii:hasUniqueTextIdentifier "HABU" .

figi-ps:BMRU figi-gii:hasUniqueTextIdentifier "BMRU" .

figi-st:hdr figi-gii:hasUniqueTextIdentifier "HDR" .

figi-ps:HAFM a owl:NamedIndividual .

figi-ps:BMSG a owl:NamedIndividual .

figi-st:hedgeFund a owl:NamedIndividual .

figi-ps:HAFM a figi-gii:PricingSource .

figi-ps:BMSG a figi-gii:PricingSource .

figi-st:hedgeFund a figi-gii:SecurityType .

figi-ps:BMSG skos:prefLabel "bval internal msg" ;
	figi-gii:hasUniqueTextIdentifier "BMSG" .

figi-ps:BMTN a owl:NamedIndividual .

figi-st:hedgeFund skos:definition "A hedge fund is a loosely regulated investment pool, generally open only to high-net worth and institutional investors. Since hedge funds can utilize greater hedging, leveraging, and use of derivative instruments in their investments, they have developed investment techniques vastly different from traditional funds. Most hedge funds strive to achieve an absolute return, as opposed to a relative return based against a benchmark." .

figi-ps:BMTN a figi-gii:PricingSource .

figi-st:hedgeFund skos:prefLabel "hedge fund" .

figi-ps:BMTN skos:prefLabel "barclays capital" .

figi-st:hedgeFund figi-gii:hasUniqueTextIdentifier "Hedge Fund" .

figi-ps:BMTN figi-gii:hasUniqueTextIdentifier "BMTN" .

figi-ps:ALTA a owl:NamedIndividual .

figi-ps:BMTS a owl:NamedIndividual .

figi-ps:ALTA a figi-gii:PricingSource .

figi-ps:HAFM skos:prefLabel "hua an fund mgmt" .

figi-ps:ALTA skos:prefLabel "alta park capital" .

figi-ps:BMTS a figi-gii:PricingSource .

figi-ps:HAFM figi-gii:hasUniqueTextIdentifier "HAFM" .

figi-ps:ALTA figi-gii:hasUniqueTextIdentifier "ALTA" .

figi-ps:BMTS skos:prefLabel "belgium mts" .

figi-st:hongKongCD a owl:NamedIndividual .

figi-ps:BMTS figi-gii:hasUniqueTextIdentifier "BMTS" .

figi-st:hongKongCD a figi-gii:SecurityType .

figi-ps:HALE a owl:NamedIndividual .

figi-st:hongKongCD skos:definition "Hong Kong Certificates of Deposit" .

figi-ps:HALE a figi-gii:PricingSource ;
	skos:prefLabel "nathan hale" ;
	figi-gii:hasUniqueTextIdentifier "HALE" .

figi-st:hongKongCD skos:prefLabel "hong kong cd" .

figi-ps:HALL a owl:NamedIndividual .

figi-st:hongKongCD figi-gii:hasUniqueTextIdentifier "HONG KONG CD" .

figi-ps:HALL a figi-gii:PricingSource .

figi-ps:ALUA a owl:NamedIndividual .

figi-ps:HALL skos:prefLabel "hall commodity" ;
	figi-gii:hasUniqueTextIdentifier "HALL" .

figi-ps:HAMS a owl:NamedIndividual , figi-gii:PricingSource ;
	skos:prefLabel "hs bank ltd" ;
	figi-gii:hasUniqueTextIdentifier "HAMS" .

figi-ps:HAN a owl:NamedIndividual , figi-gii:PricingSource ;
	skos:prefLabel "hanoistockexch" ;
	figi-gii:hasUniqueTextIdentifier "HAN" .

figi-ps:ALUA a figi-gii:PricingSource .

figi-ps:HANP a owl:NamedIndividual .

figi-ps:ALUA skos:prefLabel "cjsc alfa bank" .

figi-ps:HANP a figi-gii:PricingSource .

figi-ps:ALUA figi-gii:hasUniqueTextIdentifier "ALUA" .

figi-st:idr a owl:NamedIndividual , figi-gii:SecurityType ;
	skos:definition "International Depository Receipt. A receipt given for a foreign corporation's share certificates." ;
	skos:prefLabel "idr" ;
	figi-gii:hasUniqueTextIdentifier "IDR" .

figi-ps:ALY a owl:NamedIndividual .

figi-ps:BMUR a owl:NamedIndividual .

figi-ps:ALY a figi-gii:PricingSource .

figi-ps:BMUR a figi-gii:PricingSource .

figi-ps:HANP skos:prefLabel "hanoistockexchneg" .

figi-ps:BMUR skos:prefLabel "brean murray, carret" ;
	figi-gii:hasUniqueTextIdentifier "BMUR" .

figi-ps:HANP figi-gii:hasUniqueTextIdentifier "HANP" .

figi-ps:BNAC a owl:NamedIndividual , figi-gii:PricingSource .

figi-ps:HANS a owl:NamedIndividual .

figi-ps:BNAC skos:prefLabel "banco nacional pan" .

figi-ps:HANS a figi-gii:PricingSource .

figi-ps:BNAC figi-gii:hasUniqueTextIdentifier "BNAC" .

figi-ps:HANS skos:prefLabel "hansabank estonia" .

figi-ps:BNAP a owl:NamedIndividual .

figi-ps:HANS figi-gii:hasUniqueTextIdentifier "HANS" .

figi-ps:BNAP a figi-gii:PricingSource .

figi-ps:HAPS a owl:NamedIndividual .

figi-ps:BNAP skos:prefLabel "banco de negocios" .

figi-ps:HAPS a figi-gii:PricingSource .

figi-ps:BNAP figi-gii:hasUniqueTextIdentifier "BNAP" .

figi-ps:HAPS skos:prefLabel "hapoalim secs usa" .

figi-ps:BNAU a owl:NamedIndividual .

figi-ps:HAPS figi-gii:hasUniqueTextIdentifier "HAPS" .

figi-ps:BNAU a figi-gii:PricingSource .

figi-ps:HARA a owl:NamedIndividual .

figi-ps:BNAU skos:prefLabel "bnp paribas sydney" .

figi-ps:HARA a figi-gii:PricingSource .

figi-ps:BNAU figi-gii:hasUniqueTextIdentifier "BNAU" .

figi-ps:HARA skos:prefLabel "hsbc - algorithmics" .

figi-ps:BNBF a owl:NamedIndividual .

figi-ps:HARA figi-gii:hasUniqueTextIdentifier "HARA" .

figi-ps:BNBF a figi-gii:PricingSource .

figi-ps:HARB a owl:NamedIndividual .

figi-ps:BNBF skos:prefLabel "bbg nz bond fixing" .

figi-ps:HARB a figi-gii:PricingSource .

figi-ps:BNBF figi-gii:hasUniqueTextIdentifier "BNBF" .

figi-ps:HARB skos:prefLabel "harbour asset mgmt" .

figi-ps:BNBN a owl:NamedIndividual .

figi-ps:HARB figi-gii:hasUniqueTextIdentifier "HARB" .

figi-ps:BNBN a figi-gii:PricingSource .

figi-ps:HARP a owl:NamedIndividual .

figi-ps:BNBN skos:prefLabel "bank niaga" .

figi-ps:HARP a figi-gii:PricingSource .

figi-ps:BNBN figi-gii:hasUniqueTextIdentifier "BNBN" .

figi-ps:HARP skos:prefLabel "harpoon capital man" .

figi-ps:BNBR a owl:NamedIndividual .

figi-ps:HARP figi-gii:hasUniqueTextIdentifier "HARP" .

figi-ps:BNBR a figi-gii:PricingSource .

figi-ps:HAUC a owl:NamedIndividual .

figi-ps:BNBR skos:prefLabel "bnp bahrain" .

figi-ps:HAUC a figi-gii:PricingSource .

figi-ps:BNBR figi-gii:hasUniqueTextIdentifier "BNBR" .

figi-ps:HAUC skos:prefLabel "hauck and aufhaeuser" .

figi-ps:BNC1 a owl:NamedIndividual .

figi-ps:HAUC figi-gii:hasUniqueTextIdentifier "HAUC" .

figi-ps:BNC1 a figi-gii:PricingSource .

figi-ps:HBAT a owl:NamedIndividual .

figi-ps:BNC1 skos:prefLabel "bank1" .

figi-ps:HBAT a figi-gii:PricingSource .

figi-ps:BNC1 figi-gii:hasUniqueTextIdentifier "BNC1" .

figi-ps:HBAT skos:prefLabel "hellenic bank" .

figi-ps:BNC2 a owl:NamedIndividual .

figi-ps:HBAT figi-gii:hasUniqueTextIdentifier "HBAT" .

figi-ps:BNC2 a figi-gii:PricingSource .

figi-ps:HBBZ a owl:NamedIndividual .

figi-ps:BNC2 skos:prefLabel "bank2" .

figi-ps:HBBZ a figi-gii:PricingSource .

figi-ps:BNC2 figi-gii:hasUniqueTextIdentifier "BNC2" .

figi-ps:HBBZ skos:prefLabel "hsbc bank brazil" .

figi-ps:BNCA a owl:NamedIndividual .

figi-ps:HBBZ figi-gii:hasUniqueTextIdentifier "HBBZ" .

figi-ps:BNCA a figi-gii:PricingSource .

figi-ps:HBC a owl:NamedIndividual .

figi-ps:BNCA skos:prefLabel "bnp paribas cad" .

figi-ps:HBC a figi-gii:PricingSource .

figi-ps:BNCA figi-gii:hasUniqueTextIdentifier "BNCA" .

figi-ps:HBC skos:prefLabel "hypo alpe-adria-bank" .

figi-ps:BNCC a owl:NamedIndividual .

figi-ps:HBC figi-gii:hasUniqueTextIdentifier "HBC" .

figi-ps:BNCC a figi-gii:PricingSource .

figi-ps:HBCY a owl:NamedIndividual .

figi-ps:BNCC skos:prefLabel "bank ncc" .

figi-ps:HBCY a figi-gii:PricingSource .

figi-ps:BNCC figi-gii:hasUniqueTextIdentifier "BNCC" .

figi-ps:HBCY skos:prefLabel "hellenic bank cyprus" .

figi-ps:BNCH a owl:NamedIndividual .

figi-ps:HBCY figi-gii:hasUniqueTextIdentifier "HBCY" .

figi-ps:BNCH a figi-gii:PricingSource .

figi-ps:HBEE a owl:NamedIndividual .

figi-ps:BNCH skos:prefLabel "benchmark securities" .

figi-ps:HBEE a figi-gii:PricingSource .

figi-ps:BNCH figi-gii:hasUniqueTextIdentifier "BNCH" .

figi-ps:HBEE skos:prefLabel "hansabank markets" .

figi-ps:BNCO a owl:NamedIndividual .

figi-ps:HBEE figi-gii:hasUniqueTextIdentifier "HBEE" .

figi-ps:BNCO a figi-gii:PricingSource .

figi-ps:HBGE a owl:NamedIndividual .

figi-ps:BNCO skos:prefLabel "banc one - pcs only" .

figi-ps:HBGE a figi-gii:PricingSource .

figi-ps:BNCO figi-gii:hasUniqueTextIdentifier "BNCO" .

figi-ps:HBGE skos:prefLabel "hsbc bnk georgia" .

figi-ps:BNCR a owl:NamedIndividual .

figi-ps:HBGE figi-gii:hasUniqueTextIdentifier "HBGE" .

figi-ps:BNCR a figi-gii:PricingSource .

figi-ps:HBIN a owl:NamedIndividual .

figi-ps:BNCR skos:prefLabel "bn valores puesto" .

figi-ps:HBIN a figi-gii:PricingSource .

figi-ps:BNCR figi-gii:hasUniqueTextIdentifier "BNCR" .

figi-ps:HBIN skos:prefLabel "hb international" .

figi-ps:BNCY a owl:NamedIndividual .

figi-ps:HBIN figi-gii:hasUniqueTextIdentifier "HBIN" .

figi-ps:BNCY a figi-gii:PricingSource .

figi-ps:HBK a owl:NamedIndividual .

figi-ps:BNCY skos:prefLabel "bn valores" .

figi-ps:HBK a figi-gii:PricingSource .

figi-ps:BNCY figi-gii:hasUniqueTextIdentifier "BNCY" .

figi-ps:HBK skos:prefLabel "hsbc brokerage usa" .

figi-ps:BNDB a owl:NamedIndividual .

figi-ps:HBK figi-gii:hasUniqueTextIdentifier "HBK" .

figi-ps:BNDB a figi-gii:PricingSource .

figi-ps:HBLP a owl:NamedIndividual .

figi-ps:BNDB skos:prefLabel "bawag intl bank cz" .

figi-ps:HBLP a figi-gii:PricingSource .

figi-ps:BNDB figi-gii:hasUniqueTextIdentifier "BNDB" .

figi-ps:HBLP skos:prefLabel "habib bank limited" .

figi-ps:BNDE a owl:NamedIndividual .

figi-ps:HBLP figi-gii:hasUniqueTextIdentifier "HBLP" .

figi-ps:BNDE a figi-gii:PricingSource .

figi-ps:HBLV a owl:NamedIndividual .

figi-ps:BNDE skos:prefLabel "bnp certs-warrants" .

figi-ps:HBLV a figi-gii:PricingSource .

figi-ps:BNDE figi-gii:hasUniqueTextIdentifier "BNDE" .

figi-ps:HBLV skos:prefLabel "hansabank" .

figi-ps:BNDR a owl:NamedIndividual .

figi-ps:HBLV figi-gii:hasUniqueTextIdentifier "HBLV" .

figi-ps:BNDR a figi-gii:PricingSource .

figi-ps:HBNK a owl:NamedIndividual .

figi-ps:BNDR skos:prefLabel "banesco banco mltple" .

figi-ps:HBNK a figi-gii:PricingSource ;
	skos:prefLabel "heritage bank" .

figi-ps:BNDR figi-gii:hasUniqueTextIdentifier "BNDR" .

figi-ps:HBNK figi-gii:hasUniqueTextIdentifier "HBNK" .

figi-ps:BNG a owl:NamedIndividual .

figi-ps:HBOS a owl:NamedIndividual .

figi-ps:BNG a figi-gii:PricingSource .

figi-ps:HBOS a figi-gii:PricingSource .

figi-ps:BNG skos:prefLabel "bng capital mngt" .

figi-ps:HBOS skos:prefLabel "hbos treasury" .

figi-ps:BNG figi-gii:hasUniqueTextIdentifier "BNG" .

figi-ps:HBOS figi-gii:hasUniqueTextIdentifier "HBOS" .

figi-ps:BNIJ a owl:NamedIndividual .

figi-ps:HBWH a owl:NamedIndividual .

figi-ps:BNIJ a figi-gii:PricingSource .

figi-ps:HBWH a figi-gii:PricingSource .

figi-ps:BNIJ skos:prefLabel "bank negara indones" .

figi-ps:HBWH skos:prefLabel "hbw express bank" .

figi-ps:BNIJ figi-gii:hasUniqueTextIdentifier "BNIJ" .

figi-ps:HBWH figi-gii:hasUniqueTextIdentifier "HBWH" .

figi-ps:BNIS a owl:NamedIndividual .

figi-ps:HCB a owl:NamedIndividual .

figi-ps:BNIS a figi-gii:PricingSource .

figi-ps:HCB a figi-gii:PricingSource .

figi-ps:BNIS skos:prefLabel "bni securities" .

figi-ps:HCB skos:prefLabel "hcb" .

figi-ps:ALY skos:prefLabel "alydar capital" .

figi-ps:BNIS figi-gii:hasUniqueTextIdentifier "BNIS" .

figi-ps:HCB figi-gii:hasUniqueTextIdentifier "HCB" .

figi-ps:ALY figi-gii:hasUniqueTextIdentifier "ALY" .

figi-ps:BNKS a owl:NamedIndividual .

figi-ps:HCBR a owl:NamedIndividual .

figi-st:immForward a owl:NamedIndividual .

figi-ps:BNKS a figi-gii:PricingSource .

figi-ps:HCBR a figi-gii:PricingSource .

figi-st:immForward a figi-gii:SecurityType .

figi-ps:BNKS skos:prefLabel "fig partners" .

figi-ps:HCBR skos:prefLabel "hsbc bahrain" .

figi-ps:BNKS figi-gii:hasUniqueTextIdentifier "BNKS" .

figi-st:immForward skos:definition "Represents an FX forward contract with a maturity on an IMM date" .

figi-ps:HCBR figi-gii:hasUniqueTextIdentifier "HCBR" .

figi-ps:BNLA a owl:NamedIndividual .

figi-st:immForward skos:prefLabel "imm forward" .

figi-ps:HCCB a owl:NamedIndividual .

figi-ps:BNLA a figi-gii:PricingSource .

figi-ps:HCCB a figi-gii:PricingSource .

figi-st:immForward figi-gii:hasUniqueTextIdentifier "IMM FORWARD" .

figi-ps:HCCB skos:prefLabel "k and h bank" .

figi-ps:BNLA skos:prefLabel "banca naz del lavoro" .

figi-st:immSwap a owl:NamedIndividual .

figi-ps:HCCB figi-gii:hasUniqueTextIdentifier "HCCB" .

figi-st:immSwap a figi-gii:SecurityType .

figi-ps:BNLA figi-gii:hasUniqueTextIdentifier "BNLA" .

figi-ps:HCFB a owl:NamedIndividual , figi-gii:PricingSource .

figi-st:immSwap skos:definition "Forward swap rates with payment dates that align with Eurodollar future contracts' expiration dates." .

figi-ps:HCFB skos:prefLabel "home credit finance" .

figi-st:immSwap skos:prefLabel "imm swap" .

figi-ps:HCFB figi-gii:hasUniqueTextIdentifier "HCFB" .

figi-st:immSwap figi-gii:hasUniqueTextIdentifier "IMM SWAP" .

figi-ps:HCGA a owl:NamedIndividual .

figi-ps:AM a owl:NamedIndividual .

figi-ps:HCGA a figi-gii:PricingSource .

figi-ps:AM a figi-gii:PricingSource .

figi-ps:HCGA skos:prefLabel "hcg advisors" .

figi-ps:AM skos:prefLabel "aim demo - americas" .

figi-ps:HCGA figi-gii:hasUniqueTextIdentifier "HCGA" .

figi-ps:AM figi-gii:hasUniqueTextIdentifier "AM" .

figi-ps:HCM a owl:NamedIndividual .

figi-st:index a owl:NamedIndividual .

figi-ps:HCM a figi-gii:PricingSource .

figi-st:index a figi-gii:SecurityType .

figi-ps:HCM skos:prefLabel "ho chi minh se" ;
	figi-gii:hasUniqueTextIdentifier "HCM" .

figi-st:index skos:definition "Index. A compilation of statistical data that tracks changes in the economy or in financial markets." .

figi-ps:HCMA a owl:NamedIndividual .

figi-st:index skos:prefLabel "index" .

figi-ps:HCMA a figi-gii:PricingSource ;
	skos:prefLabel "hobart capital marke" ;
	figi-gii:hasUniqueTextIdentifier "HCMA" .

figi-ps:HCML a owl:NamedIndividual .

figi-st:index figi-gii:hasUniqueTextIdentifier "Index" .

figi-ps:HCML a figi-gii:PricingSource ;
	skos:prefLabel "highland capital mgm" .

figi-ps:AMAT a owl:NamedIndividual .

figi-ps:HCML figi-gii:hasUniqueTextIdentifier "HCML" .

figi-ps:AMAT a figi-gii:PricingSource .

figi-ps:HCMS a owl:NamedIndividual .

figi-ps:AMAT skos:prefLabel "applied materials" .

figi-ps:HCMS a figi-gii:PricingSource .

figi-ps:AMAT figi-gii:hasUniqueTextIdentifier "AMAT" .

figi-ps:HCMS skos:prefLabel "hochiminh securities" .

figi-st:indexOption a owl:NamedIndividual .

figi-ps:HCMS figi-gii:hasUniqueTextIdentifier "HCMS" .

figi-st:indexOption a figi-gii:SecurityType .

figi-ps:HCMY a owl:NamedIndividual , figi-gii:PricingSource ;
	skos:prefLabel "hcm yield" ;
	figi-gii:hasUniqueTextIdentifier "HCMY" .

figi-ps:HCW a owl:NamedIndividual .

figi-ps:BNLR a owl:NamedIndividual .

figi-ps:HCW a figi-gii:PricingSource .

figi-ps:BNLR a figi-gii:PricingSource .

figi-ps:HCW skos:prefLabel "h.c. wainwright co." .

figi-ps:BNLR skos:prefLabel "bca naz del lavoro" .

figi-ps:HCW skos:prefLabel "hc wainwright co" .

figi-ps:BNLR figi-gii:hasUniqueTextIdentifier "BNLR" .

figi-ps:HCW figi-gii:hasUniqueTextIdentifier "HCW" .

figi-ps:BNLX a owl:NamedIndividual .

figi-ps:HDAT a owl:NamedIndividual , figi-gii:PricingSource .

figi-ps:BNLX a figi-gii:PricingSource .

figi-st:indexOption skos:definition "Option on Index Futures. Investors trading index options are essentially betting on the overall movement of the stock market as represented by a basket of stocks. Options on the S and P 500 are some of the most actively traded options in the world." .

figi-ps:BNLX skos:prefLabel "bnl spa" .

figi-ps:HDAT skos:prefLabel "bogr intraday" .

figi-st:indexOption skos:prefLabel "index option" .

figi-ps:HDAT figi-gii:hasUniqueTextIdentifier "HDAT" .

figi-ps:BNLX figi-gii:hasUniqueTextIdentifier "BNLX" .

figi-st:indexOption figi-gii:hasUniqueTextIdentifier "Index Option" .

figi-ps:HDBS a owl:NamedIndividual .

figi-ps:BNM a owl:NamedIndividual .

figi-ps:HDBS a figi-gii:PricingSource .

figi-st:indexOtcOption a owl:NamedIndividual .

figi-ps:BNM a figi-gii:PricingSource .

figi-ps:HDBS skos:prefLabel "hwang dbs asset mgt" .

figi-st:indexOtcOption a figi-gii:SecurityType .

figi-ps:BNM skos:prefLabel "bank negara malaysia" .

figi-ps:HDBS figi-gii:hasUniqueTextIdentifier "HDBS" .

figi-ps:BNM figi-gii:hasUniqueTextIdentifier "BNM" .

figi-ps:HDFC a owl:NamedIndividual .

figi-ps:BNMP a owl:NamedIndividual .

figi-ps:HDFC a figi-gii:PricingSource .

figi-ps:BNMP a figi-gii:PricingSource .

figi-st:indexOtcOption skos:definition "Options on a basket of the 100 most highly capitalized, unlisted securities, which will provide profit for investors who correctly gauge short-term, over-the-counter price movements. It also provides investors with a hedge against other over-the-counter securities in their portfolio." .

figi-ps:HDFC skos:prefLabel "hdfc bank" .

figi-ps:BNMP skos:prefLabel "bnp paribas mtge" .

figi-ps:HDFC figi-gii:hasUniqueTextIdentifier "HDFC" .

figi-st:indexOtcOption skos:prefLabel "index otc option" .

figi-ps:BNMP figi-gii:hasUniqueTextIdentifier "BNMP" .

figi-ps:HDSR a owl:NamedIndividual .

figi-st:indexOtcOption figi-gii:hasUniqueTextIdentifier "Index OTC Option" .

figi-ps:HDSR a figi-gii:PricingSource .

figi-ps:BNMX a owl:NamedIndividual .

figi-ps:AMB a owl:NamedIndividual .

figi-ps:HDSR skos:prefLabel "hyundai securities" .

figi-ps:AMB a figi-gii:PricingSource .

figi-ps:BNMX a figi-gii:PricingSource .

figi-ps:HDSR figi-gii:hasUniqueTextIdentifier "HDSR" .

figi-ps:AMB skos:prefLabel "ambac" .

figi-ps:BNMX skos:prefLabel "banco nacional mex" .

figi-ps:HEFL a owl:NamedIndividual .

figi-ps:AMB figi-gii:hasUniqueTextIdentifier "AMB" .

figi-ps:HEFL a figi-gii:PricingSource .

figi-ps:BNMX figi-gii:hasUniqueTextIdentifier "BNMX" .

figi-st:indexWrt a owl:NamedIndividual .

figi-ps:HEFL skos:prefLabel "heflin and co" .

figi-ps:BNP a owl:NamedIndividual .

figi-st:indexWrt a figi-gii:SecurityType .

figi-ps:HEFL figi-gii:hasUniqueTextIdentifier "HEFL" .

figi-ps:BNP a figi-gii:PricingSource .

figi-st:indexWrt skos:definition "Index Warrant - Indicates that the underlying is an index" .

figi-ps:HELA a owl:NamedIndividual .

figi-st:indexWrt skos:prefLabel "index wrt" .

figi-ps:HELA a figi-gii:PricingSource .

figi-st:indexWrt figi-gii:hasUniqueTextIdentifier "Index WRT" .

figi-ps:HELA skos:prefLabel "helaba auto ex" .

figi-ps:BNP skos:prefLabel "bnp capital markets" .

figi-ps:AMBK a owl:NamedIndividual .

figi-ps:HELA figi-gii:hasUniqueTextIdentifier "HELA" .

figi-ps:BNP figi-gii:hasUniqueTextIdentifier "BNP" .

figi-ps:AMBK a figi-gii:PricingSource .

figi-ps:HELB a owl:NamedIndividual .

figi-ps:BNPA a owl:NamedIndividual .

figi-ps:AMBK skos:prefLabel "amen bank" .

figi-ps:BNPA a figi-gii:PricingSource .

figi-ps:HELB a figi-gii:PricingSource .

figi-ps:AMBK figi-gii:hasUniqueTextIdentifier "AMBK" .

figi-ps:BNPA skos:prefLabel "bnp paribas - certs" .

figi-ps:HELB skos:prefLabel "helaba" .

figi-ps:AMBR a owl:NamedIndividual .

figi-ps:BNPA figi-gii:hasUniqueTextIdentifier "BNPA" .

figi-ps:HELB figi-gii:hasUniqueTextIdentifier "HELB" .

figi-ps:AMBR a figi-gii:PricingSource .

figi-ps:BNPB a owl:NamedIndividual .

figi-ps:HELD a owl:NamedIndividual .

figi-ps:AMBR skos:prefLabel "amber capital" .

figi-ps:BNPB a figi-gii:PricingSource .

figi-ps:HELD a figi-gii:PricingSource .

figi-ps:AMBR figi-gii:hasUniqueTextIdentifier "AMBR" .

figi-ps:BNPB skos:prefLabel "bnp fixed income" .

figi-ps:HELD skos:prefLabel "helaba et trading" .

figi-st:indianCD a owl:NamedIndividual .

figi-ps:BNPB figi-gii:hasUniqueTextIdentifier "BNPB" .

figi-ps:HELD figi-gii:hasUniqueTextIdentifier "HELD" .

figi-st:indianCD a figi-gii:SecurityType .

figi-ps:BNPC a owl:NamedIndividual .

figi-st:indianCD skos:definition "Indian Certificates of Deposit" .

figi-ps:BNPC a figi-gii:PricingSource .

figi-ps:HELF a owl:NamedIndividual .

figi-st:indianCD skos:prefLabel "indian cd" .

figi-ps:HELF a figi-gii:PricingSource .

figi-ps:BNPC skos:prefLabel "bnp paribas - ldn" .

figi-st:indianCD figi-gii:hasUniqueTextIdentifier "INDIAN CD" .

figi-ps:HELF skos:prefLabel "helaba f-rate notes" .

figi-ps:BNPC figi-gii:hasUniqueTextIdentifier "BNPC" .

figi-ps:AMBX a owl:NamedIndividual .

figi-ps:HELF figi-gii:hasUniqueTextIdentifier "HELF" .

figi-ps:AMBX a figi-gii:PricingSource .

figi-ps:BNPE a owl:NamedIndividual .

figi-ps:HELI a owl:NamedIndividual .

figi-ps:BNPE a figi-gii:PricingSource .

figi-ps:HELI a figi-gii:PricingSource .

figi-ps:BNPE skos:prefLabel "banco nacion" .

figi-ps:AMBX skos:prefLabel "ambank (m) bhd" .

figi-ps:BNPE figi-gii:hasUniqueTextIdentifier "BNPE" .

figi-ps:AMBX figi-gii:hasUniqueTextIdentifier "AMBX" .

figi-ps:BNPF a owl:NamedIndividual .

figi-ps:AMER a owl:NamedIndividual .

figi-ps:BNPF a figi-gii:PricingSource .

figi-ps:AMER a figi-gii:PricingSource .

figi-ps:HELI skos:prefLabel "helaba frn's" .

figi-ps:AMER skos:prefLabel "amerex futures ltd" .

figi-ps:BNPF skos:prefLabel "bnp paribas 4:30" .

figi-ps:HELI figi-gii:hasUniqueTextIdentifier "HELI" .

figi-ps:BNPF figi-gii:hasUniqueTextIdentifier "BNPF" .

figi-ps:AMER figi-gii:hasUniqueTextIdentifier "AMER" .

figi-ps:HELM a owl:NamedIndividual .

figi-ps:BNPG a owl:NamedIndividual .

figi-st:indianCP a owl:NamedIndividual .

figi-ps:HELM a figi-gii:PricingSource .

figi-ps:BNPG a figi-gii:PricingSource .

figi-st:indianCP a figi-gii:SecurityType .

figi-ps:HELM skos:prefLabel "helaba helm" .

figi-ps:BNPG skos:prefLabel "bnp frankfurt" .

figi-st:indianCP skos:definition "Indian Commercial Paper" .

figi-ps:HELM figi-gii:hasUniqueTextIdentifier "HELM" .

figi-ps:BNPG figi-gii:hasUniqueTextIdentifier "BNPG" .

figi-st:indianCP skos:prefLabel "indian cp" .

figi-ps:HELN a owl:NamedIndividual .

figi-ps:BNPH a owl:NamedIndividual .

figi-st:indianCP figi-gii:hasUniqueTextIdentifier "INDIAN CP" .

figi-ps:BNPH a figi-gii:PricingSource .

figi-ps:HELN a figi-gii:PricingSource .

figi-ps:AMEX a owl:NamedIndividual .

figi-ps:BNPH skos:prefLabel "bnp paribas,vietnam" .

figi-ps:AMEX a figi-gii:PricingSource .

figi-ps:HELN skos:prefLabel "helaba frn" .

figi-ps:BNPH figi-gii:hasUniqueTextIdentifier "BNPH" .

figi-ps:AMEX skos:prefLabel "nyse mkt llc" .

figi-ps:HELN figi-gii:hasUniqueTextIdentifier "HELN" .

figi-ps:AMEX figi-gii:hasUniqueTextIdentifier "AMEX" .

figi-ps:BNPJ a owl:NamedIndividual .

figi-ps:HELO a owl:NamedIndividual .

figi-ps:BNPJ a figi-gii:PricingSource .

figi-ps:HELO a figi-gii:PricingSource .

figi-ps:BNPJ skos:prefLabel "bnp securities japan" .

figi-ps:AMHE a owl:NamedIndividual .

figi-ps:HELO skos:prefLabel "helaba bank test" .

figi-ps:BNPJ figi-gii:hasUniqueTextIdentifier "BNPJ" .

figi-ps:AMHE a figi-gii:PricingSource .

figi-ps:HELO figi-gii:hasUniqueTextIdentifier "HELO" .

figi-ps:BNPM a owl:NamedIndividual .

figi-ps:AMHE skos:prefLabel "amherst securities" .

figi-ps:HELS a owl:NamedIndividual .

figi-ps:BNPM a figi-gii:PricingSource .

figi-ps:AMHE figi-gii:hasUniqueTextIdentifier "AMHE" .

figi-ps:HELS a figi-gii:PricingSource .

figi-ps:BNPM skos:prefLabel "bnp paribas metals" .

figi-st:indonesianCP a owl:NamedIndividual .

figi-ps:HELS skos:prefLabel "helsinki stk exch" .

figi-st:indonesianCP a figi-gii:SecurityType .

figi-ps:BNPM figi-gii:hasUniqueTextIdentifier "BNPM" .

figi-ps:HELS figi-gii:hasUniqueTextIdentifier "HELS" .

figi-st:indonesianCP skos:definition "Indonesian Commercial Paper" .

figi-ps:BNPP a owl:NamedIndividual .

figi-ps:HELT a owl:NamedIndividual .

figi-ps:BNPP a figi-gii:PricingSource .

figi-st:indonesianCP skos:prefLabel "indonesian cp" .

figi-ps:HELT a figi-gii:PricingSource .

figi-ps:BNPP skos:prefLabel "bnp paribas 11:30" .

figi-st:indonesianCP figi-gii:hasUniqueTextIdentifier "INDONESIAN CP" .

figi-ps:BNPP figi-gii:hasUniqueTextIdentifier "BNPP" .

figi-ps:HELT skos:prefLabel "helaba marketlink" .

figi-ps:AMIN a owl:NamedIndividual .

figi-ps:BNPR a owl:NamedIndividual .

figi-ps:HELT figi-gii:hasUniqueTextIdentifier "HELT" .

figi-ps:BNPR a figi-gii:PricingSource .

figi-ps:AMIN a figi-gii:PricingSource .

figi-ps:HELX a owl:NamedIndividual .

figi-ps:BNPR skos:prefLabel "bnp paribas equities" .

figi-ps:HELX a figi-gii:PricingSource .

figi-ps:BNPR figi-gii:hasUniqueTextIdentifier "BNPR" .

figi-ps:AMIN skos:prefLabel "aminvestment mgmt" .

figi-ps:BNPS a owl:NamedIndividual .

figi-ps:HELX skos:prefLabel "helaba internal mtm" .

figi-ps:BNPS a figi-gii:PricingSource .

figi-ps:AMIN figi-gii:hasUniqueTextIdentifier "AMIN" .

figi-ps:BNPS skos:prefLabel "bnp paribas" .

figi-ps:HELX figi-gii:hasUniqueTextIdentifier "HELX" .

figi-ps:BNPS figi-gii:hasUniqueTextIdentifier "BNPS" .

figi-st:indxFutWrt a owl:NamedIndividual .

figi-ps:BNPT a owl:NamedIndividual .

figi-st:indxFutWrt a figi-gii:SecurityType .

figi-ps:BNPT a figi-gii:PricingSource .

figi-st:indxFutWrt skos:definition "Indicates that the underlying is an index future" .

figi-ps:BNPT skos:prefLabel "bnp taiwan" .

figi-ps:HEND a owl:NamedIndividual .

figi-st:indxFutWrt skos:prefLabel "indx fut wrt" .

figi-ps:BNPT figi-gii:hasUniqueTextIdentifier "BNPT" .

figi-ps:HEND a figi-gii:PricingSource .

figi-st:indxFutWrt figi-gii:hasUniqueTextIdentifier "Indx Fut WRT" .

figi-ps:BNPY a owl:NamedIndividual .

figi-ps:HEND skos:prefLabel "henderson" .

figi-ps:AMM a owl:NamedIndividual .

figi-ps:BNPY a figi-gii:PricingSource .

figi-ps:AMM a figi-gii:PricingSource .

figi-ps:HEND figi-gii:hasUniqueTextIdentifier "HEND" .

figi-ps:BNPY skos:prefLabel "bnp paribas cairo" .

figi-ps:HERN a owl:NamedIndividual .

figi-ps:BNPY figi-gii:hasUniqueTextIdentifier "BNPY" .

figi-ps:HERN a figi-gii:PricingSource .

figi-ps:BNRT a owl:NamedIndividual .

figi-ps:HERN skos:prefLabel "heren energy" .

figi-ps:BNRT a figi-gii:PricingSource .

figi-ps:HERN figi-gii:hasUniqueTextIdentifier "HERN" .

figi-ps:BNRT skos:prefLabel "banorte" .

figi-ps:HERT a owl:NamedIndividual .

figi-ps:BNRT figi-gii:hasUniqueTextIdentifier "BNRT" .

figi-ps:AMM skos:prefLabel "american money mgmt" .

figi-ps:HERT a figi-gii:PricingSource .

figi-ps:AMM figi-gii:hasUniqueTextIdentifier "AMM" .

figi-ps:BNSC a owl:NamedIndividual .

figi-ps:AMMB a owl:NamedIndividual .

figi-ps:BNSC a figi-gii:PricingSource .

figi-ps:AMMB a figi-gii:PricingSource .

figi-ps:BNSC skos:prefLabel "banesco" .

figi-ps:AMMB skos:prefLabel "ambank group" ;
	figi-gii:hasUniqueTextIdentifier "AMMB" .

figi-ps:HERT skos:prefLabel "banque heritage" .

figi-st:inflationSwap a owl:NamedIndividual .

figi-ps:BNSC figi-gii:hasUniqueTextIdentifier "BNSC" .

figi-ps:HERT skos:prefLabel "heritage capital" .

figi-st:inflationSwap a figi-gii:SecurityType .

figi-ps:BNSJ a owl:NamedIndividual , figi-gii:PricingSource .

figi-st:inflationSwap skos:definition "A derivative used to transfer inflation risk from one party to another through an exchange of cash flows." .

figi-ps:BNSJ skos:prefLabel "bk of nova scot jama" .

figi-st:inflationSwap skos:prefLabel "inflation swap" .

figi-ps:HERT figi-gii:hasUniqueTextIdentifier "HERT" .

figi-st:inflationSwap figi-gii:hasUniqueTextIdentifier "INFLATION SWAP" .

figi-ps:BNSJ figi-gii:hasUniqueTextIdentifier "BNSJ" .

figi-ps:HETC a owl:NamedIndividual .

figi-ps:AMMC a owl:NamedIndividual .

figi-ps:BNSX a owl:NamedIndividual .

figi-ps:HETC a figi-gii:PricingSource .

figi-ps:AMMC a figi-gii:PricingSource .

figi-ps:BNSX a figi-gii:PricingSource .

figi-ps:HETC skos:prefLabel "hess energy" .

figi-ps:AMMC skos:prefLabel "amm invest" .

figi-ps:HETC figi-gii:hasUniqueTextIdentifier "HETC" .

figi-ps:AMMC figi-gii:hasUniqueTextIdentifier "AMMC" .

figi-ps:HEX a owl:NamedIndividual .

figi-ps:BNSX skos:prefLabel "bns europe" .

figi-ps:AMPF a owl:NamedIndividual .

figi-ps:HEX a figi-gii:PricingSource .

figi-ps:AMPF a figi-gii:PricingSource .

figi-ps:BNSX figi-gii:hasUniqueTextIdentifier "BNSX" .

figi-ps:HEX skos:prefLabel "hexagon securities" .

figi-ps:AMPF skos:prefLabel "ameriprise financial" .

figi-ps:BNTY a owl:NamedIndividual .

figi-ps:HEX figi-gii:hasUniqueTextIdentifier "HEX" .

figi-ps:BNTY a figi-gii:PricingSource .

figi-ps:AMPF figi-gii:hasUniqueTextIdentifier "AMPF" .

figi-ps:HEXM a owl:NamedIndividual , figi-gii:PricingSource .

figi-st:intBearFixbis a owl:NamedIndividual .

figi-ps:BNTY skos:prefLabel "bnp paribas - tsy" .

figi-st:intBearFixbis a figi-gii:SecurityType .

figi-ps:HEXM skos:prefLabel "hexam capital" .

figi-ps:BNTY figi-gii:hasUniqueTextIdentifier "BNTY" .

figi-st:intBearFixbis skos:definition "Bank of Intl Settlement Discount Notes / Interest Bearing Coupon Rate" .

figi-ps:BNUS a owl:NamedIndividual .

figi-st:intBearFixbis skos:prefLabel "int bear fixbis" .

figi-ps:BNUS a figi-gii:PricingSource .

figi-st:intBearFixbis figi-gii:hasUniqueTextIdentifier "INT BEAR FIXBIS" .

figi-ps:BNUS skos:prefLabel "bolsa nicaragua usd" .

figi-ps:AMPI a owl:NamedIndividual , figi-gii:PricingSource ;
	skos:prefLabel "amp investments nz" .

figi-ps:BNUS figi-gii:hasUniqueTextIdentifier "BNUS" .

figi-ps:AMPI figi-gii:hasUniqueTextIdentifier "AMPI" .

figi-ps:HEXM figi-gii:hasUniqueTextIdentifier "HEXM" .

figi-ps:AMPR a owl:NamedIndividual .

figi-ps:BNXX a owl:NamedIndividual .

figi-ps:AMPR a figi-gii:PricingSource .

figi-ps:HFFI a owl:NamedIndividual .

figi-ps:AMPR skos:prefLabel "american enterprise" .

figi-ps:BNXX a figi-gii:PricingSource .

figi-ps:HFFI a figi-gii:PricingSource .

figi-ps:AMPR figi-gii:hasUniqueTextIdentifier "AMPR" .

figi-ps:BNXX skos:prefLabel "bnp paribas hk" .

figi-ps:HFFI skos:prefLabel "housing financing fd" .

figi-st:intRtWrt a owl:NamedIndividual .

figi-ps:BNXX figi-gii:hasUniqueTextIdentifier "BNXX" .

figi-st:intRtWrt a figi-gii:SecurityType .

figi-ps:BNYA a owl:NamedIndividual .

figi-st:intRtWrt skos:definition "Interest Rate Warrant - Indicates that the underlying is an interest rate" .

figi-ps:BNYA a figi-gii:PricingSource .

figi-st:intRtWrt skos:prefLabel "int. rt. wrt" .

figi-ps:BNYA skos:prefLabel "bank of new york" .

figi-st:intRtWrt figi-gii:hasUniqueTextIdentifier "Int. Rt. WRT" .

figi-ps:BNYA figi-gii:hasUniqueTextIdentifier "BNYA" .

figi-ps:AMRB a owl:NamedIndividual .

figi-ps:HFFI figi-gii:hasUniqueTextIdentifier "HFFI" .

figi-ps:AMRB a figi-gii:PricingSource .

figi-ps:BNYC a owl:NamedIndividual .

figi-ps:AMRB skos:prefLabel "ameria bank" .

figi-ps:BNYC a figi-gii:PricingSource .

figi-ps:AMRB figi-gii:hasUniqueTextIdentifier "AMRB" .

figi-ps:BNYC skos:prefLabel "bnym capital markets" .

figi-ps:HFMC a owl:NamedIndividual .

figi-ps:AMRI a owl:NamedIndividual .

figi-ps:BNYC figi-gii:hasUniqueTextIdentifier "BNYC" .

figi-ps:AMRI a figi-gii:PricingSource .

figi-ps:HFMC a figi-gii:PricingSource .

figi-ps:BNZ a owl:NamedIndividual .

figi-ps:AMRI skos:prefLabel "abn amro n.v. dubai" .

figi-ps:BNZ a figi-gii:PricingSource .

figi-ps:HFMC skos:prefLabel "harvest fund mgt" .

figi-ps:AMRI figi-gii:hasUniqueTextIdentifier "AMRI" .

figi-ps:BNZ skos:prefLabel "bank of new zealand" .

figi-ps:HFMC figi-gii:hasUniqueTextIdentifier "HFMC" .

figi-st:interAppreciation a owl:NamedIndividual .

figi-ps:BNZ figi-gii:hasUniqueTextIdentifier "BNZ" .

figi-ps:HFMT a owl:NamedIndividual .

figi-st:interAppreciation a figi-gii:SecurityType .

figi-ps:HFMT a figi-gii:PricingSource ;
	skos:prefLabel "harvest fund test" .

figi-st:interAppreciation skos:definition "Also called Convertible Capital Appreciate Bonds. The bond starts as a Zero Coupon, then converts at some predetermined date to a fixed rate or current interest bond." .

figi-ps:HFMT figi-gii:hasUniqueTextIdentifier "HFMT" .

figi-ps:BOA a owl:NamedIndividual .

figi-st:interAppreciation skos:prefLabel "inter. appreciation" .

figi-ps:HFP a owl:NamedIndividual .

figi-ps:BOA a figi-gii:PricingSource .

figi-st:interAppreciation figi-gii:hasUniqueTextIdentifier "INTER. APPRECIATION" .

figi-ps:HFP a figi-gii:PricingSource .

figi-ps:BOA skos:prefLabel "bank of america cis" .

figi-ps:AMRX a owl:NamedIndividual .

figi-ps:HFP skos:prefLabel "hfp capital mkts llc" .

figi-ps:AMRX a figi-gii:PricingSource .

figi-ps:HFP figi-gii:hasUniqueTextIdentifier "HFP" .

figi-ps:AMRX skos:prefLabel "amerex futures ltd" .

figi-ps:BOA figi-gii:hasUniqueTextIdentifier "BOA" .

figi-ps:AMRX figi-gii:hasUniqueTextIdentifier "AMRX" .

figi-ps:HFT a owl:NamedIndividual .

figi-ps:AMSO a owl:NamedIndividual .

figi-ps:BOAA a owl:NamedIndividual .

figi-ps:HFT a figi-gii:PricingSource .

figi-ps:BOAA a figi-gii:PricingSource .

figi-ps:AMSO a figi-gii:PricingSource .

figi-ps:HFT skos:prefLabel "fortis haitong" .

figi-ps:BOAA skos:prefLabel "boa pricing" .

figi-ps:AMSO skos:prefLabel "amsouth bank" .

figi-ps:HFT figi-gii:hasUniqueTextIdentifier "HFT" .

figi-ps:AMSO figi-gii:hasUniqueTextIdentifier "AMSO" .

figi-ps:BOAA figi-gii:hasUniqueTextIdentifier "BOAA" .

figi-ps:HFVX a owl:NamedIndividual .

figi-st:interAppreciationOid a owl:NamedIndividual .

figi-ps:BOAF a owl:NamedIndividual .

figi-ps:HFVX a figi-gii:PricingSource .

figi-st:interAppreciationOid a figi-gii:SecurityType .

figi-ps:BOAF a figi-gii:PricingSource .

figi-ps:HFVX skos:prefLabel "hf securities" .

figi-st:interAppreciationOid skos:definition "Also called Convertible Capital Appreciate Bonds. The bond starts as a Zero Coupon, then converts at some predetermined date to a fixed rate or current interest bond." .

figi-ps:BOAF skos:prefLabel "bk of amer singapore" .

figi-st:interAppreciationOid skos:prefLabel "inter. appreciation, oid" .

figi-ps:BOAF figi-gii:hasUniqueTextIdentifier "BOAF" .

figi-ps:HFVX figi-gii:hasUniqueTextIdentifier "HFVX" .

figi-ps:BOAG a owl:NamedIndividual .

figi-st:interAppreciationOid figi-gii:hasUniqueTextIdentifier "INTER. APPRECIATION, OID" .

figi-ps:BOAG a figi-gii:PricingSource .

figi-ps:HGB a owl:NamedIndividual , figi-gii:PricingSource .

figi-ps:BOAG skos:prefLabel "boa gilt inside px" .

figi-ps:HGB skos:prefLabel "hsbc guyerzeller" .

figi-ps:BOAG figi-gii:hasUniqueTextIdentifier "BOAG" .

figi-ps:AMSP a owl:NamedIndividual .

figi-ps:HGB figi-gii:hasUniqueTextIdentifier "HGB" .

figi-ps:BOAM a owl:NamedIndividual .

figi-ps:AMSP a figi-gii:PricingSource .

figi-ps:BOAM a figi-gii:PricingSource .

figi-ps:HGFS a owl:NamedIndividual .

figi-ps:AMSP skos:prefLabel "amstel fin'l svs" .

figi-ps:BOAM skos:prefLabel "bank of america" .

figi-ps:HGFS a figi-gii:PricingSource .

figi-ps:BOAM skos:prefLabel "bank of america, mum" .

figi-ps:HGFS skos:prefLabel "hg factoring" .

figi-ps:BOAM figi-gii:hasUniqueTextIdentifier "BOAM" .

figi-ps:HGFS figi-gii:hasUniqueTextIdentifier "HGFS" .

figi-ps:AMSP figi-gii:hasUniqueTextIdentifier "AMSP" .

figi-ps:HHMI a owl:NamedIndividual .

figi-ps:BOAN a owl:NamedIndividual .

figi-ps:HHMI a figi-gii:PricingSource .

figi-ps:AMSS a owl:NamedIndividual .

figi-ps:BOAN a figi-gii:PricingSource .

figi-ps:HHMI skos:prefLabel "howard hughes med" .

figi-ps:AMSS a figi-gii:PricingSource .

figi-ps:BOAN skos:prefLabel "bancone cap boom" .

figi-ps:HHMI figi-gii:hasUniqueTextIdentifier "HHMI" .

figi-ps:BOAN figi-gii:hasUniqueTextIdentifier "BOAN" .

figi-ps:HIB a owl:NamedIndividual .

figi-ps:BOAP a owl:NamedIndividual .

figi-ps:HIB a figi-gii:PricingSource .

figi-ps:AMSS skos:prefLabel "amselsec. geneva" .

figi-ps:BOAP a figi-gii:PricingSource .

figi-ps:HIB skos:prefLabel "hypo investmentbank" .

figi-ps:AMSS figi-gii:hasUniqueTextIdentifier "AMSS" .

figi-ps:HIB figi-gii:hasUniqueTextIdentifier "HIB" .

figi-ps:BOAP skos:prefLabel "bk of america prime" .

figi-st:interbankOfferedRate a owl:NamedIndividual .

figi-ps:BOAP figi-gii:hasUniqueTextIdentifier "BOAP" .

figi-st:interbankOfferedRate a figi-gii:SecurityType .

figi-ps:BOAS a owl:NamedIndividual .

figi-ps:HIG a owl:NamedIndividual .

figi-ps:BOAS a figi-gii:PricingSource .

figi-st:interbankOfferedRate skos:definition "An interest rate at which banks can borrow funds from other banks, eg Libor" .

figi-ps:HIG a figi-gii:PricingSource .

figi-st:interbankOfferedRate skos:prefLabel "interbank offered rate" .

figi-ps:BOAS skos:prefLabel "bank of america" .

figi-st:interbankOfferedRate figi-gii:hasUniqueTextIdentifier "INTERBANK OFFERED RATE" .

figi-ps:HIG skos:prefLabel "hamon investment grp" .

figi-ps:BOAS figi-gii:hasUniqueTextIdentifier "BOAS" .

figi-ps:AMTB a owl:NamedIndividual .

figi-ps:HIG figi-gii:hasUniqueTextIdentifier "HIG" .

figi-ps:BOAX a owl:NamedIndividual .

figi-ps:AMTB a figi-gii:PricingSource .

figi-ps:BOAX a figi-gii:PricingSource .

figi-ps:HIGH a owl:NamedIndividual .

figi-ps:AMTB skos:prefLabel "amt bank llc" .

figi-ps:HIGH a figi-gii:PricingSource .

figi-ps:BOAX skos:prefLabel "boa testing px" .

figi-ps:AMTB figi-gii:hasUniqueTextIdentifier "AMTB" .

figi-ps:HIGH skos:prefLabel "highmark capital" .

figi-ps:BOAX figi-gii:hasUniqueTextIdentifier "BOAX" .

figi-ps:AMTR a owl:NamedIndividual .

figi-ps:HIGH figi-gii:hasUniqueTextIdentifier "HIGH" .

figi-ps:BOAY a owl:NamedIndividual .

figi-ps:AMTR a figi-gii:PricingSource .

figi-ps:BOAY a figi-gii:PricingSource .

figi-ps:AMTR skos:prefLabel "american technology" .

figi-ps:BOAY skos:prefLabel "bank of ayudhya bkk" .

figi-ps:AMTR figi-gii:hasUniqueTextIdentifier "AMTR" .

figi-ps:BOAY figi-gii:hasUniqueTextIdentifier "BOAY" .

figi-ps:HILL a owl:NamedIndividual .

figi-st:interestRateGuarantee a owl:NamedIndividual .

figi-ps:BOBE a owl:NamedIndividual .

figi-st:interestRateGuarantee a figi-gii:SecurityType .

figi-ps:BOBE a figi-gii:PricingSource .

figi-st:interestRateGuarantee skos:definition "An interest rate guarantee (IRG) is an option on a forward rate agreement (FRA) that is handled over-the-counter (OTC)." .

figi-ps:HILL a figi-gii:PricingSource .

figi-ps:BOBE skos:prefLabel "bank of beirut" .

figi-st:interestRateGuarantee skos:prefLabel "interest rate guarantee" .

figi-ps:HILL skos:prefLabel "hill, thompson, magi" .

figi-ps:BOBE figi-gii:hasUniqueTextIdentifier "BOBE" .

figi-st:interestRateGuarantee figi-gii:hasUniqueTextIdentifier "INTEREST RATE GUARANTEE" .

figi-ps:HILL skos:prefLabel "hillman company" .

figi-ps:BOBI a owl:NamedIndividual .

figi-ps:AMTS a owl:NamedIndividual .

figi-ps:HILL figi-gii:hasUniqueTextIdentifier "HILL" .

figi-ps:AMTS a figi-gii:PricingSource .

figi-ps:BOBI a figi-gii:PricingSource .

figi-ps:HIM a owl:NamedIndividual .

figi-ps:AMTS skos:prefLabel "amsterdam mts exch" .

figi-ps:HIM a figi-gii:PricingSource .

figi-ps:BOBI skos:prefLabel "bank of baroda" .

figi-ps:AMTS figi-gii:hasUniqueTextIdentifier "AMTS" .

figi-ps:HIM skos:prefLabel "harris investment" .

figi-ps:BOBI figi-gii:hasUniqueTextIdentifier "BOBI" .

figi-ps:HIM figi-gii:hasUniqueTextIdentifier "HIM" .

figi-ps:AMXI a owl:NamedIndividual .

figi-ps:BOBJ a owl:NamedIndividual .

figi-ps:HITO a owl:NamedIndividual .

figi-ps:BOBJ a figi-gii:PricingSource .

figi-ps:HITO a figi-gii:PricingSource .

figi-ps:BOBJ skos:prefLabel "bank of beijing" .

figi-ps:HITO skos:prefLabel "hipoteca total" .

figi-ps:BOBJ figi-gii:hasUniqueTextIdentifier "BOBJ" .

figi-ps:HITO figi-gii:hasUniqueTextIdentifier "HITO" .

figi-ps:BOBL a owl:NamedIndividual .

figi-ps:AMXI a figi-gii:PricingSource .

figi-ps:BOBL a figi-gii:PricingSource .

figi-ps:HITS a owl:NamedIndividual .

figi-ps:BOBL skos:prefLabel "bank of beirut bonds" .

figi-ps:HITS a figi-gii:PricingSource .

figi-ps:AMXI skos:prefLabel "american express bk" .

figi-ps:HITS skos:prefLabel "height analytics llc" .

figi-ps:BOBL figi-gii:hasUniqueTextIdentifier "BOBL" .

figi-ps:HITS figi-gii:hasUniqueTextIdentifier "HITS" .

figi-ps:BOC a owl:NamedIndividual .

figi-ps:HJSC a owl:NamedIndividual .

figi-ps:BOC a figi-gii:PricingSource .

figi-ps:HJSC a figi-gii:PricingSource .

figi-ps:AMXI figi-gii:hasUniqueTextIdentifier "AMXI" .

figi-ps:BOC skos:prefLabel "bank of china" .

figi-ps:HJSC skos:prefLabel "herbert j sims and co" .

figi-ps:BOC figi-gii:hasUniqueTextIdentifier "BOC" .

figi-ps:HJSC figi-gii:hasUniqueTextIdentifier "HJSC" .

figi-st:irFutWrt a owl:NamedIndividual .

figi-ps:BOCA a owl:NamedIndividual .

figi-ps:HKAM a owl:NamedIndividual .

figi-ps:BOCA a figi-gii:PricingSource .

figi-st:irFutWrt a figi-gii:SecurityType .

figi-ps:HKAM a figi-gii:PricingSource .

figi-ps:BOCA skos:prefLabel "bank of china ae" .

figi-ps:HKAM skos:prefLabel "haitong int'l am" .

figi-ps:BOCA skos:prefLabel "boc asset management" .

figi-st:irFutWrt skos:definition "Indicates that the underlying is an interest rate future" .

figi-ps:BOCA figi-gii:hasUniqueTextIdentifier "BOCA" .

figi-ps:HKAM figi-gii:hasUniqueTextIdentifier "HKAM" .

figi-st:irFutWrt skos:prefLabel "i.r. fut wrt" .

figi-ps:BOCB a owl:NamedIndividual .

figi-ps:HKBT a owl:NamedIndividual .

figi-st:irFutWrt figi-gii:hasUniqueTextIdentifier "I.R. Fut WRT" .

figi-ps:HKBT a figi-gii:PricingSource .

figi-ps:BOCB a figi-gii:PricingSource .

figi-ps:AMZS a owl:NamedIndividual .

figi-ps:HKBT skos:prefLabel "bloomberg t-s demo" .

figi-ps:BOCB skos:prefLabel "cfet bank of china" .

figi-ps:AMZS a figi-gii:PricingSource .

figi-ps:HKBT figi-gii:hasUniqueTextIdentifier "HKBT" .

figi-ps:BOCB figi-gii:hasUniqueTextIdentifier "BOCB" .

figi-ps:AMZS skos:prefLabel "amz securities" .

figi-ps:HKMA a owl:NamedIndividual .

figi-ps:BOCC a owl:NamedIndividual .

figi-ps:AMZS figi-gii:hasUniqueTextIdentifier "AMZS" .

figi-ps:HKMA a figi-gii:PricingSource .

figi-ps:BOCC a figi-gii:PricingSource .

figi-st:irSwpWrt a owl:NamedIndividual .

figi-ps:HKMA skos:prefLabel "hong kong mon auth" .

figi-st:irSwpWrt a figi-gii:SecurityType .

figi-ps:BOCC skos:prefLabel "banco occidente cali" .

figi-ps:HKMA figi-gii:hasUniqueTextIdentifier "HKMA" .

figi-st:irSwpWrt skos:definition "Indicates that the underlying is an interest rate swap" .

figi-ps:BOCC figi-gii:hasUniqueTextIdentifier "BOCC" .

figi-ps:HKMC a owl:NamedIndividual .

figi-st:irSwpWrt skos:prefLabel "i.r. swp wrt" .

figi-ps:HKMC a figi-gii:PricingSource .

figi-ps:BOCF a owl:NamedIndividual .

figi-st:irSwpWrt figi-gii:hasUniqueTextIdentifier "I.R. Swp WRT" .

figi-ps:HKMC skos:prefLabel "hong kong mtg corp" .

figi-ps:BOCF a figi-gii:PricingSource .

figi-ps:ANAD a owl:NamedIndividual .

figi-ps:HKMC figi-gii:hasUniqueTextIdentifier "HKMC" .

figi-ps:ANAD a figi-gii:PricingSource .

figi-ps:BOCF skos:prefLabel "cfif bank of china" .

figi-ps:XTKQ a owl:NamedIndividual .

figi-ps:ANAD skos:prefLabel "anadolubank" .

figi-ps:BOCF figi-gii:hasUniqueTextIdentifier "BOCF" .

figi-ps:XTKQ a figi-gii:PricingSource .

figi-ps:ANAD figi-gii:hasUniqueTextIdentifier "ANAD" .

figi-ps:BOCH a owl:NamedIndividual .

figi-ps:XTKQ skos:prefLabel "xtrakter quote price" .

figi-ps:ANAM a owl:NamedIndividual .

figi-ps:BOCH a figi-gii:PricingSource .

figi-ps:ANAM a figi-gii:PricingSource .

figi-ps:BOCH skos:prefLabel "bank of china" .

figi-ps:ANAM skos:prefLabel "allianz nederland" .

figi-ps:XTKQ figi-gii:hasUniqueTextIdentifier "XTKQ" .

figi-ps:BOCH figi-gii:hasUniqueTextIdentifier "BOCH" .

figi-ps:ANAM figi-gii:hasUniqueTextIdentifier "ANAM" .

figi-ps:HKSB a owl:NamedIndividual .

figi-st:islamic a owl:NamedIndividual .

figi-ps:BOCI a owl:NamedIndividual .

figi-ps:HKSB a figi-gii:PricingSource .

figi-st:islamic a figi-gii:SecurityType .

figi-ps:BOCI a figi-gii:PricingSource .

figi-ps:HKSB skos:prefLabel "hsbc india" .

figi-ps:BOCI skos:prefLabel "boc investment co" .

figi-ps:HKSB figi-gii:hasUniqueTextIdentifier "HKSB" .

figi-ps:BOCI figi-gii:hasUniqueTextIdentifier "BOCI" .

figi-ps:XTKT a owl:NamedIndividual .

figi-ps:BOCK a owl:NamedIndividual .

figi-st:islamic skos:definition "A type of loan that interest cannot be charged on, complying with Islamic/sharpie law. Instead, the loan is structured using discounts, sale or lease, profit participation, or repurchase agreements. Lenders are generally referred to as depositors. Islamic loans are further classified into sub-categories such as ljara, Murabaha, Mudarabah, etc." .

figi-ps:XTKT a figi-gii:PricingSource .

figi-ps:BOCK a figi-gii:PricingSource .

figi-st:islamic skos:prefLabel "islamic" .

figi-ps:XTKT skos:prefLabel "xtrakter trade price" .

figi-ps:BOCK skos:prefLabel "bochk" .

figi-st:islamic figi-gii:hasUniqueTextIdentifier "ISLAMIC" .

figi-ps:XTKT figi-gii:hasUniqueTextIdentifier "XTKT" .

figi-ps:BOCK figi-gii:hasUniqueTextIdentifier "BOCK" .

figi-ps:ANB a owl:NamedIndividual .

figi-ps:HKSE a owl:NamedIndividual .

figi-ps:BOCN a owl:NamedIndividual .

figi-ps:ANB a figi-gii:PricingSource .

figi-ps:BOCN a figi-gii:PricingSource .

figi-ps:HKSE a figi-gii:PricingSource .

figi-ps:ANB skos:prefLabel "anb financial, na" .

figi-ps:BOCN skos:prefLabel "cnbond boc" .

figi-ps:HKSE skos:prefLabel "hong kong stock exch" .

figi-ps:ANB figi-gii:hasUniqueTextIdentifier "ANB" .

figi-ps:BOCN figi-gii:hasUniqueTextIdentifier "BOCN" .

figi-ps:HKSE figi-gii:hasUniqueTextIdentifier "HKSE" .

figi-ps:ANBC a owl:NamedIndividual .

figi-ps:BOCO a owl:NamedIndividual .

figi-ps:ANBC a figi-gii:PricingSource .

figi-ps:BOCO a figi-gii:PricingSource .

figi-ps:XYZ a owl:NamedIndividual .

figi-ps:ANBC skos:prefLabel "andbank" .

figi-ps:BOCO skos:prefLabel "bank of comm 4:30" .

figi-ps:XYZ a figi-gii:PricingSource .

figi-ps:ANBC figi-gii:hasUniqueTextIdentifier "ANBC" .

figi-ps:BOCO figi-gii:hasUniqueTextIdentifier "BOCO" .

figi-ps:XYZ skos:prefLabel "aim-dart" .

figi-st:islamicBa a owl:NamedIndividual .

figi-ps:BOCP a owl:NamedIndividual .

figi-ps:XYZ figi-gii:hasUniqueTextIdentifier "XYZ" .

figi-ps:BOCP a figi-gii:PricingSource .

figi-ps:HKSG a owl:NamedIndividual .

figi-st:islamicBa a figi-gii:SecurityType .

figi-ps:BOCP skos:prefLabel "bank of china 4:30" .

figi-ps:HKSG a figi-gii:PricingSource .

figi-st:islamicBa skos:definition "Islamic Bankers Acceptances" .

figi-ps:BOCP figi-gii:hasUniqueTextIdentifier "BOCP" .

figi-ps:HKSG skos:prefLabel "sg securities hk ltd" .

figi-st:islamicBa skos:prefLabel "islamic ba" .

figi-ps:BOCS a owl:NamedIndividual .

figi-ps:HKSG figi-gii:hasUniqueTextIdentifier "HKSG" .

figi-ps:BOCS a figi-gii:PricingSource .

figi-st:islamicBa figi-gii:hasUniqueTextIdentifier "ISLAMIC BA" .

figi-ps:HLBS a owl:NamedIndividual .

figi-ps:BOCS skos:prefLabel "bank of china suisse" .

figi-ps:ANBD a owl:NamedIndividual .

figi-ps:HLBS a figi-gii:PricingSource .

figi-ps:ANBD a figi-gii:PricingSource .

figi-ps:BOCS figi-gii:hasUniqueTextIdentifier "BOCS" .

figi-ps:HLBS skos:prefLabel "hl bank singapore" .

figi-ps:ANBD skos:prefLabel "andbanc" .

figi-ps:BOCT a owl:NamedIndividual .

figi-ps:HLBS figi-gii:hasUniqueTextIdentifier "HLBS" .

figi-ps:ANBD figi-gii:hasUniqueTextIdentifier "ANBD" .

figi-ps:BOCT a figi-gii:PricingSource .

figi-ps:HMBG a owl:NamedIndividual .

figi-ps:ANBK a owl:NamedIndividual .

figi-ps:BOCT skos:prefLabel "bank of china 11:30" .

figi-ps:HMBG a figi-gii:PricingSource .

figi-ps:ANBK a figi-gii:PricingSource .

figi-ps:BOCT figi-gii:hasUniqueTextIdentifier "BOCT" .

figi-ps:HMBG skos:prefLabel "hamburg exchange" .

figi-ps:ANBK skos:prefLabel "arab national bank" .

figi-ps:BOCX a owl:NamedIndividual .

figi-ps:HMBG figi-gii:hasUniqueTextIdentifier "HMBG" .

figi-ps:ANBK figi-gii:hasUniqueTextIdentifier "ANBK" .

figi-ps:BOCX a figi-gii:PricingSource .

figi-ps:YBHT a owl:NamedIndividual .

figi-ps:ANCP a owl:NamedIndividual .

figi-ps:YBHT a figi-gii:PricingSource .

figi-ps:BOCX skos:prefLabel "bk of china beijing" .

figi-ps:ANCP a figi-gii:PricingSource .

figi-ps:YBHT skos:prefLabel "aig-huatai fund mgmt" .

figi-ps:BOCX figi-gii:hasUniqueTextIdentifier "BOCX" .

figi-ps:ANCP skos:prefLabel "antares capital" .

figi-ps:YBHT figi-gii:hasUniqueTextIdentifier "YBHT" .

figi-ps:ANCP figi-gii:hasUniqueTextIdentifier "ANCP" .

figi-ps:BOCY a owl:NamedIndividual .

figi-ps:HMBS a owl:NamedIndividual .

figi-ps:ANDA a owl:NamedIndividual .

figi-ps:BOCY a figi-gii:PricingSource .

figi-ps:HMBS a figi-gii:PricingSource .

figi-ps:ANDA a figi-gii:PricingSource .

figi-ps:BOCY skos:prefLabel "bank of cyprus" .

figi-ps:HMBS skos:prefLabel "hsbc internal mbs" .

figi-ps:ANDA skos:prefLabel "central bank r550" .

figi-ps:BOCY figi-gii:hasUniqueTextIdentifier "BOCY" .

figi-ps:HMBS figi-gii:hasUniqueTextIdentifier "HMBS" .

figi-ps:ANDA figi-gii:hasUniqueTextIdentifier "ANDA" .

figi-ps:BOEA a owl:NamedIndividual .

figi-ps:HMGI a owl:NamedIndividual .

figi-st:islamicCP a owl:NamedIndividual .

figi-ps:HMGI a figi-gii:PricingSource .

figi-ps:BOEA a figi-gii:PricingSource .

figi-st:islamicCP a figi-gii:SecurityType .

figi-ps:HMGI skos:prefLabel "harlow's and mgi" .

figi-ps:BOEA skos:prefLabel "bank of east asia" .

figi-st:islamicCP skos:definition "Islamic Commercial Paper" .

figi-ps:HMGI figi-gii:hasUniqueTextIdentifier "HMGI" .

figi-ps:BOEA figi-gii:hasUniqueTextIdentifier "BOEA" .

figi-st:islamicCP skos:prefLabel "islamic cp" .

figi-ps:YHZQ a owl:NamedIndividual .

figi-ps:BOFA a owl:NamedIndividual .

figi-st:islamicCP figi-gii:hasUniqueTextIdentifier "ISLAMIC CP" .

figi-ps:YHZQ a figi-gii:PricingSource .

figi-ps:BOFA a figi-gii:PricingSource .

figi-ps:ANDB a owl:NamedIndividual .

figi-ps:YHZQ skos:prefLabel "china galaxy sec" .

figi-ps:ANDB a figi-gii:PricingSource .

figi-ps:BOFA skos:prefLabel "bank of america" .

figi-ps:YHZQ figi-gii:hasUniqueTextIdentifier "YHZQ" .

figi-ps:ANDB skos:prefLabel "andhra bank" .

figi-ps:BOFA skos:prefLabel "barcap agencies" .

figi-ps:HMTC a owl:NamedIndividual .

figi-ps:ANDB figi-gii:hasUniqueTextIdentifier "ANDB" .

figi-ps:HMTC a figi-gii:PricingSource .

figi-ps:BOFA figi-gii:hasUniqueTextIdentifier "BOFA" .

figi-ps:ANDD a owl:NamedIndividual .

figi-ps:HMTC skos:prefLabel "hi-mtf convertibles" .

figi-ps:ANDD a figi-gii:PricingSource .

figi-ps:BOFC a owl:NamedIndividual .

figi-ps:HMTC figi-gii:hasUniqueTextIdentifier "HMTC" .

figi-ps:BOFC a figi-gii:PricingSource .

figi-ps:ANDD skos:prefLabel "andima debentures" .

figi-ps:YLDX a owl:NamedIndividual .

figi-ps:BOFC skos:prefLabel "barcap spreads" .

figi-ps:ANDD figi-gii:hasUniqueTextIdentifier "ANDD" .

figi-ps:BOFC figi-gii:hasUniqueTextIdentifier "BOFC" .

figi-st:islamicLoc a owl:NamedIndividual .

figi-ps:YLDX a figi-gii:PricingSource .

figi-st:islamicLoc a figi-gii:SecurityType .

figi-ps:BOFG a owl:NamedIndividual .

figi-ps:YLDX skos:prefLabel "jse centr ord book" .

figi-ps:BOFG a figi-gii:PricingSource .

figi-ps:YLDX figi-gii:hasUniqueTextIdentifier "YLDX" .

figi-ps:BOFG skos:prefLabel "barcap- tips" .

figi-st:islamicLoc skos:definition "Interest cannot be charged, complying with Islamic/sharpie law. Guaranteed by the lender(s) and used for purchase of goods, completion of construction projects, and/or general purposes." .

figi-ps:HMTF a owl:NamedIndividual .

figi-ps:BOFG figi-gii:hasUniqueTextIdentifier "BOFG" .

figi-st:islamicLoc skos:prefLabel "islamic loc" .

figi-ps:HMTF a figi-gii:PricingSource .

figi-ps:BOFX a owl:NamedIndividual .

figi-st:islamicLoc figi-gii:hasUniqueTextIdentifier "ISLAMIC LOC" .

figi-ps:BOFX a figi-gii:PricingSource .

figi-ps:HMTF skos:prefLabel "hi-mtf quote driven" .

figi-ps:ANDE a owl:NamedIndividual .

figi-ps:BOFX skos:prefLabel "barcap fx link notes" .

figi-ps:HMTF figi-gii:hasUniqueTextIdentifier "HMTF" .

figi-ps:ANDE a figi-gii:PricingSource .

figi-ps:BOFX figi-gii:hasUniqueTextIdentifier "BOFX" .

figi-ps:HMTS a owl:NamedIndividual .

figi-ps:ANDE skos:prefLabel "anbima yld reference" .

figi-ps:BOG a owl:NamedIndividual .

figi-ps:HMTS a figi-gii:PricingSource .

figi-ps:ANDE figi-gii:hasUniqueTextIdentifier "ANDE" .

figi-ps:BOG a figi-gii:PricingSource .

figi-ps:HMTS skos:prefLabel "finland mts" .

figi-st:islamicRev a owl:NamedIndividual .

figi-ps:BOG skos:prefLabel "bogr official" .

figi-ps:HMTS figi-gii:hasUniqueTextIdentifier "HMTS" .

figi-ps:BOG figi-gii:hasUniqueTextIdentifier "BOG" .

figi-ps:ZENT a owl:NamedIndividual .

figi-st:islamicRev a figi-gii:SecurityType .

figi-ps:ZENT a figi-gii:PricingSource .

figi-ps:BOGC a owl:NamedIndividual , figi-gii:PricingSource .

figi-ps:ZENT skos:prefLabel "bank zenit" .

figi-ps:BOGC skos:prefLabel "bg capital" .

figi-ps:ZENT figi-gii:hasUniqueTextIdentifier "ZENT" .

figi-st:islamicRev skos:definition "Interest cannot be charged, complying with Islamic/sharpie law. Instead, the loan is structured using discounts, sale or lease, profit participation, or repurchase agreements. Once borrowed funds are repaid they can be borrowed again." .

figi-ps:BOGC figi-gii:hasUniqueTextIdentifier "BOGC" .

figi-ps:HNBL a owl:NamedIndividual , figi-gii:PricingSource .

figi-ps:BOGE a owl:NamedIndividual .

figi-ps:HNBL skos:prefLabel "hnb securities ltd" .

figi-ps:BOGE a figi-gii:PricingSource .

figi-ps:HNBL figi-gii:hasUniqueTextIdentifier "HNBL" .

figi-ps:BOGE skos:prefLabel "bank of georgia" .

figi-ps:HNHK a owl:NamedIndividual .

figi-ps:BOGE figi-gii:hasUniqueTextIdentifier "BOGE" .

figi-ps:HNHK a figi-gii:PricingSource .

figi-ps:BOIZ a owl:NamedIndividual .

figi-st:islamicRev skos:prefLabel "islamic rev" .

figi-ps:HNHK skos:prefLabel "hua nan securities" .

figi-ps:BOIZ a figi-gii:PricingSource .

figi-st:islamicRev figi-gii:hasUniqueTextIdentifier "ISLAMIC REV" .

figi-ps:HNHK figi-gii:hasUniqueTextIdentifier "HNHK" .

figi-ps:BOIZ skos:prefLabel "bank of india" .

figi-ps:ANDI a owl:NamedIndividual .

figi-ps:BOIZ figi-gii:hasUniqueTextIdentifier "BOIZ" .

figi-ps:ANDI a figi-gii:PricingSource .

figi-ps:BOJ a owl:NamedIndividual .

figi-ps:ANDI skos:prefLabel "anbima minandmax yield" .

figi-ps:BOJ a figi-gii:PricingSource .

figi-ps:ZIEG a owl:NamedIndividual .

figi-ps:ANDI figi-gii:hasUniqueTextIdentifier "ANDI" .

figi-ps:ZIEG a figi-gii:PricingSource .

figi-ps:BOJ skos:prefLabel "bank of japan" .

figi-st:islamicStandby a owl:NamedIndividual .

figi-ps:ZIEG skos:prefLabel "bc ziegler and co" .

figi-st:islamicStandby a figi-gii:SecurityType .

figi-ps:BOJ figi-gii:hasUniqueTextIdentifier "BOJ" .

figi-ps:ZIEG figi-gii:hasUniqueTextIdentifier "ZIEG" .

figi-ps:BOK a owl:NamedIndividual , figi-gii:PricingSource .

figi-ps:HNNR a owl:NamedIndividual .

figi-ps:BOK skos:prefLabel "bank of korea" .

figi-st:islamicStandby skos:definition "Interest cannot be charged, complying with Islamic/sharpie law. Instead, the loan is structured using discounts, sale or lease, profit participation, or repurchase agreements. Issued on a stand-by basis and borrowed only if and when needed." .

figi-ps:HNNR a figi-gii:PricingSource .

figi-ps:BOK figi-gii:hasUniqueTextIdentifier "BOK" .

figi-st:islamicStandby skos:prefLabel "islamic standby" .

figi-ps:HNNR skos:prefLabel "kb investment sec co" .

figi-ps:BOMF a owl:NamedIndividual .

figi-st:islamicStandby figi-gii:hasUniqueTextIdentifier "ISLAMIC STANDBY" .

figi-ps:HNNR figi-gii:hasUniqueTextIdentifier "HNNR" .

figi-ps:BOMF a figi-gii:PricingSource .

figi-ps:ANDO a owl:NamedIndividual .

figi-ps:ZNTD a owl:NamedIndividual .

figi-ps:BOMF skos:prefLabel "bank of montreal" .

figi-ps:ANDO a figi-gii:PricingSource .

figi-ps:ZNTD a figi-gii:PricingSource .

figi-ps:BOMF figi-gii:hasUniqueTextIdentifier "BOMF" .

figi-ps:ANDO skos:prefLabel "credit andorra" .

figi-ps:ZNTD skos:prefLabel "bank zenit domestic" .

figi-ps:BOND a owl:NamedIndividual .

figi-ps:ANDO figi-gii:hasUniqueTextIdentifier "ANDO" .

figi-ps:BOND a figi-gii:PricingSource .

figi-ps:ZNTD figi-gii:hasUniqueTextIdentifier "ZNTD" .

figi-ps:ANOD a owl:NamedIndividual .

figi-ps:BOND skos:prefLabel "bondscom" .

figi-ps:HNVR a owl:NamedIndividual .

figi-ps:ANOD a figi-gii:PricingSource .

figi-ps:HNVR a figi-gii:PricingSource .

figi-ps:BOND figi-gii:hasUniqueTextIdentifier "BOND" .

figi-ps:ANOD skos:prefLabel "anod bank" .

figi-ps:HNVR skos:prefLabel "hanover exchange" .

figi-ps:BONP a owl:NamedIndividual .

figi-ps:ANOD figi-gii:hasUniqueTextIdentifier "ANOD" .

figi-ps:HNVR figi-gii:hasUniqueTextIdentifier "HNVR" .

figi-ps:BONP a figi-gii:PricingSource .

figi-st:islamicStandbyRev a owl:NamedIndividual .

figi-ps:HOOP a owl:NamedIndividual .

figi-st:islamicStandbyRev a figi-gii:SecurityType .

figi-ps:HOOP a figi-gii:PricingSource .

figi-ps:BONP skos:prefLabel "bondpartners sa" .

figi-ps:HOOP skos:prefLabel "hospitals of ontario" .

figi-ps:BONP figi-gii:hasUniqueTextIdentifier "BONP" .

figi-ps:HOOP figi-gii:hasUniqueTextIdentifier "HOOP" .

figi-st:islamicStandbyRev skos:definition "Interest cannot be charged, complying with Islamic/sharpie law. Instead, the loan is structured using discounts, sale or lease, profit participation, or repurchase agreements. Issued on a stand-by basis and borrowed only if and when needed. Once borrowed, cannot be borrowed again." .

figi-ps:ZXZQ a owl:NamedIndividual .

figi-ps:BONY a owl:NamedIndividual .

figi-ps:ZXZQ a figi-gii:PricingSource .

figi-st:islamicStandbyRev skos:prefLabel "islamic standby rev" .

figi-ps:BONY a figi-gii:PricingSource .

figi-ps:ZXZQ skos:prefLabel "citic securities" .

figi-st:islamicStandbyRev figi-gii:hasUniqueTextIdentifier "ISLAMIC STANDBY REV" .

figi-ps:ZXZQ figi-gii:hasUniqueTextIdentifier "ZXZQ" .

figi-ps:ANST a owl:NamedIndividual .

figi-ps:HOPL a owl:NamedIndividual .

figi-ps:ANST a figi-gii:PricingSource .

figi-ps:HOPL a figi-gii:PricingSource .

figi-ps:BONY skos:prefLabel "bank of new york" .

figi-ps:HOPL skos:prefLabel "hopwood lane trading" .

figi-ps:ANST skos:prefLabel "ansa merchant" .

figi-ps:HOPL figi-gii:hasUniqueTextIdentifier "HOPL" .

figi-ps:BONY figi-gii:hasUniqueTextIdentifier "BONY" .

figi-ps:HORI a owl:NamedIndividual .

figi-ps:BOOA a owl:NamedIndividual .

figi-ps:HORI a figi-gii:PricingSource .

figi-ps:BOOA a figi-gii:PricingSource .

figi-ps:ANST figi-gii:hasUniqueTextIdentifier "ANST" .

figi-ps:HORI skos:prefLabel "horizon" .

figi-ps:BOOA skos:prefLabel "boa pricing" .

figi-ps:HORI figi-gii:hasUniqueTextIdentifier "HORI" .

figi-ps:ANT a owl:NamedIndividual .

figi-ps:BOOA figi-gii:hasUniqueTextIdentifier "BOOA" .

figi-ps:BandB a owl:NamedIndividual .

figi-ps:ANT a figi-gii:PricingSource .

figi-ps:BandB a figi-gii:PricingSource .

figi-ps:BOPM a owl:NamedIndividual .

figi-ps:BandB skos:prefLabel "bradford and bingley" .

figi-ps:ANT skos:prefLabel "antonveneta" .

figi-ps:BOPM a figi-gii:PricingSource .

figi-ps:BandB figi-gii:hasUniqueTextIdentifier "B&B" .

figi-ps:ANT figi-gii:hasUniqueTextIdentifier "ANT" .

figi-ps:BOPM skos:prefLabel "bopi mart net 20%" .

figi-ps:HOWE a owl:NamedIndividual .

figi-st:islamicTerm a owl:NamedIndividual .

figi-ps:HOWE a figi-gii:PricingSource .

figi-ps:BOPM figi-gii:hasUniqueTextIdentifier "BOPM" .

figi-ps:HOWE skos:prefLabel "howe, barnes invest." .

figi-st:islamicTerm a figi-gii:SecurityType .

figi-ps:HOWE figi-gii:hasUniqueTextIdentifier "HOWE" .

figi-ps:BOPN a owl:NamedIndividual .

figi-ps:FandC a owl:NamedIndividual .

figi-ps:BOPN a figi-gii:PricingSource .

figi-ps:FandC a figi-gii:PricingSource .

figi-ps:BOPN skos:prefLabel "bopi mart 10%" .

figi-ps:FandC skos:prefLabel "f and c management" .

figi-st:islamicTerm skos:definition "Interest cannot be charged, complying with Islamic/sharpie law. Instead, the loan is structured using discounts, sale or lease, profit participation, or repurchase agreements. Once borrowed, cannot be borrowed again." .

figi-ps:FandC figi-gii:hasUniqueTextIdentifier "F&C" .

figi-ps:BOPN figi-gii:hasUniqueTextIdentifier "BOPN" .

figi-st:islamicTerm skos:prefLabel "islamic term" .

figi-ps:HPBZ a owl:NamedIndividual .

figi-ps:BOPU a owl:NamedIndividual .

figi-st:islamicTerm figi-gii:hasUniqueTextIdentifier "ISLAMIC TERM" .

figi-ps:HPBZ a figi-gii:PricingSource .

figi-ps:BOPU a figi-gii:PricingSource .

figi-ps:HPBZ skos:prefLabel "hrvatska post banka" .

figi-ps:ANTC a owl:NamedIndividual .

figi-ps:BOPU skos:prefLabel "bancpost sa" .

figi-ps:HPBZ figi-gii:hasUniqueTextIdentifier "HPBZ" .

figi-ps:ANTC a figi-gii:PricingSource .

figi-ps:BOPU figi-gii:hasUniqueTextIdentifier "BOPU" .

figi-ps:HPFB a owl:NamedIndividual .

figi-ps:ANTC skos:prefLabel "antanta capital" .

figi-ps:HPFB a figi-gii:PricingSource .

figi-ps:BORU a owl:NamedIndividual .

figi-ps:ANTC figi-gii:hasUniqueTextIdentifier "ANTC" .

figi-ps:BORU a figi-gii:PricingSource .

figi-ps:HPFB skos:prefLabel "hi asset management" .

figi-ps:ANZ a owl:NamedIndividual .

figi-ps:HPFB figi-gii:hasUniqueTextIdentifier "HPFB" .

figi-ps:BORU skos:prefLabel "bank of russia" .

figi-ps:ANZ a figi-gii:PricingSource .

figi-ps:KandS a owl:NamedIndividual .

figi-ps:BORU figi-gii:hasUniqueTextIdentifier "BORU" .

figi-ps:KandS a figi-gii:PricingSource .

figi-ps:ANZ skos:prefLabel "anz banking group" .

figi-ps:KandS skos:prefLabel "king and shaxson lnd" .

figi-ps:BOS a owl:NamedIndividual .

figi-ps:ANZ skos:prefLabel "anz securities" .

figi-ps:KandS figi-gii:hasUniqueTextIdentifier "K&S" .

figi-ps:BOS a figi-gii:PricingSource .

figi-ps:ANZ figi-gii:hasUniqueTextIdentifier "ANZ" .

figi-ps:HPFS a owl:NamedIndividual .

figi-ps:BOS skos:prefLabel "hbos" .

figi-ps:HPFS a figi-gii:PricingSource .

figi-st:jumboCD a owl:NamedIndividual .

figi-ps:BOS figi-gii:hasUniqueTextIdentifier "BOS" .

figi-ps:HPFS skos:prefLabel "hsbc pfs singapore" .

figi-st:jumboCD a figi-gii:SecurityType .

figi-ps:HPFS figi-gii:hasUniqueTextIdentifier "HPFS" .

figi-ps:BOSA a owl:NamedIndividual .

figi-ps:HPOR a owl:NamedIndividual .

figi-ps:BOSA a figi-gii:PricingSource .

figi-ps:HPOR a figi-gii:PricingSource .

figi-st:jumboCD skos:definition "Jumbo Certificate of Deposit. A certificate of deposit with a denomination of at least $100,000, usually purchased by institutional investors." .

figi-ps:BOSA skos:prefLabel "hbos tsy svcs plc" .

figi-ps:HPOR skos:prefLabel "havenport" .

figi-st:jumboCD skos:prefLabel "jumbo cd" .

figi-ps:BOSA figi-gii:hasUniqueTextIdentifier "BOSA" .

figi-ps:HPOR figi-gii:hasUniqueTextIdentifier "HPOR" .

figi-st:jumboCD figi-gii:hasUniqueTextIdentifier "JUMBO CD" .

figi-ps:BOSC a owl:NamedIndividual .

figi-ps:ANZB a owl:NamedIndividual .

figi-ps:HPWD a owl:NamedIndividual .

figi-ps:BOSC a figi-gii:PricingSource .

figi-ps:HPWD a figi-gii:PricingSource .

figi-ps:ANZB a figi-gii:PricingSource .

figi-ps:BOSC skos:prefLabel "bank oklahoma" .

figi-ps:ANZB skos:prefLabel "anz banking group" .

figi-ps:HPWD skos:prefLabel "hopwood lane trading" .

figi-ps:BOSC figi-gii:hasUniqueTextIdentifier "BOSC" .

figi-ps:ANZB figi-gii:hasUniqueTextIdentifier "ANZB" .

figi-ps:HPWD figi-gii:hasUniqueTextIdentifier "HPWD" .

figi-ps:BOSH a owl:NamedIndividual .

figi-ps:ANZE a owl:NamedIndividual .

figi-ps:BOSH a figi-gii:PricingSource .

figi-ps:HRBI a owl:NamedIndividual .

figi-ps:ANZE a figi-gii:PricingSource .

figi-ps:HRBI a figi-gii:PricingSource .

figi-ps:BOSH skos:prefLabel "cfif bk of shanghai" .

figi-ps:HRBI skos:prefLabel "hypo real estate ban" .

figi-ps:ANZE skos:prefLabel "anz banking corp" .

figi-ps:HRBI figi-gii:hasUniqueTextIdentifier "HRBI" .

figi-ps:BOSH figi-gii:hasUniqueTextIdentifier "BOSH" .

figi-ps:HRLF a owl:NamedIndividual .

figi-ps:ANZE figi-gii:hasUniqueTextIdentifier "ANZE" .

figi-ps:HRLF a figi-gii:PricingSource .

figi-ps:BOSK a owl:NamedIndividual .

figi-ps:HRLF skos:prefLabel "harel finance" .

figi-st:koreanCD a owl:NamedIndividual .

figi-ps:BOSK a figi-gii:PricingSource .

figi-ps:HRLF figi-gii:hasUniqueTextIdentifier "HRLF" .

figi-st:koreanCD a figi-gii:SecurityType .

figi-ps:BOSK skos:prefLabel "bankboston mexico" .

figi-ps:HS a owl:NamedIndividual .

figi-st:koreanCD skos:definition "Korean Certificates of Deposit" .

figi-ps:HS a figi-gii:PricingSource .

figi-ps:BOSK figi-gii:hasUniqueTextIdentifier "BOSK" .

figi-st:koreanCD skos:prefLabel "korean cd" .

figi-ps:HS skos:prefLabel "hsbc sec japan" .

figi-ps:BOTM a owl:NamedIndividual .

figi-ps:HS figi-gii:hasUniqueTextIdentifier "HS" .

figi-st:koreanCD figi-gii:hasUniqueTextIdentifier "KOREAN CD" .

figi-ps:BOTM a figi-gii:PricingSource .

figi-ps:HSAA a owl:NamedIndividual .

figi-ps:ANZI a owl:NamedIndividual .

figi-ps:HSAA a figi-gii:PricingSource .

figi-ps:BOTM skos:prefLabel "bureau of tsy manila" .

figi-ps:ANZI a figi-gii:PricingSource .

figi-ps:HSAA skos:prefLabel "hsbc argentina (usd)" .

figi-ps:BOTM figi-gii:hasUniqueTextIdentifier "BOTM" .

figi-ps:HSAA figi-gii:hasUniqueTextIdentifier "HSAA" .

figi-ps:ANZI skos:prefLabel "anz banking group" .

figi-ps:BOVB a owl:NamedIndividual .

figi-ps:HSAB a owl:NamedIndividual .

figi-ps:ANZI figi-gii:hasUniqueTextIdentifier "ANZI" .

figi-ps:HSAB a figi-gii:PricingSource .

figi-ps:BOVB a figi-gii:PricingSource .

figi-ps:HSAB skos:prefLabel "hsbc au" .

figi-ps:ANZS a owl:NamedIndividual .

figi-ps:HSAB figi-gii:hasUniqueTextIdentifier "HSAB" .

figi-ps:BOVB skos:prefLabel "colombia stock exch" .

figi-ps:ANZS a figi-gii:PricingSource .

figi-ps:HSAM a owl:NamedIndividual .

figi-ps:BOVB figi-gii:hasUniqueTextIdentifier "BOVB" .

figi-ps:ANZS skos:prefLabel "anz banking aust" .

figi-ps:HSAM a figi-gii:PricingSource .

figi-ps:BP a owl:NamedIndividual .

figi-ps:ANZS figi-gii:hasUniqueTextIdentifier "ANZS" .

figi-ps:BP a figi-gii:PricingSource .

figi-st:koreanCP a owl:NamedIndividual .

figi-ps:HSAM skos:prefLabel "hsbcam americas inc" .

figi-ps:BP skos:prefLabel "bp investment mgmt" .

figi-st:koreanCP a figi-gii:SecurityType .

figi-ps:HSAM figi-gii:hasUniqueTextIdentifier "HSAM" .

figi-ps:BP figi-gii:hasUniqueTextIdentifier "BP" .

figi-st:koreanCP skos:definition "Korean Commercial Paper" .

figi-ps:HSAP a owl:NamedIndividual .

figi-st:koreanCP skos:prefLabel "korean cp" .

figi-ps:BPAA a owl:NamedIndividual .

figi-ps:HSAP a figi-gii:PricingSource .

figi-st:koreanCP figi-gii:hasUniqueTextIdentifier "KOREAN CP" .

figi-ps:BPAA a figi-gii:PricingSource .

figi-ps:HSAP skos:prefLabel "hsbc access prod ind" .

figi-ps:ANZV a owl:NamedIndividual .

figi-ps:BPAA skos:prefLabel "banca pop dell'alto" .

figi-ps:ANZV a figi-gii:PricingSource .

figi-ps:HSAP figi-gii:hasUniqueTextIdentifier "HSAP" .

figi-ps:BPAA figi-gii:hasUniqueTextIdentifier "BPAA" .

figi-ps:ANZV skos:prefLabel "anz bank, vietnam" .

figi-ps:HSAR a owl:NamedIndividual .

figi-ps:BPAB a owl:NamedIndividual .

figi-ps:ANZV figi-gii:hasUniqueTextIdentifier "ANZV" .

figi-ps:HSAR a figi-gii:PricingSource .

figi-ps:BPAB a figi-gii:PricingSource .

figi-ps:ANZW a owl:NamedIndividual .

figi-ps:HSAR skos:prefLabel "hsbc bk argentina" .

figi-ps:ANZW a figi-gii:PricingSource .

figi-ps:BPAB skos:prefLabel "bnp paribas - mtges" .

figi-ps:HSAR figi-gii:hasUniqueTextIdentifier "HSAR" .

figi-ps:ANZW skos:prefLabel "anz wellington" .

figi-ps:BPAB figi-gii:hasUniqueTextIdentifier "BPAB" .

figi-ps:HSAS a owl:NamedIndividual .

figi-ps:ANZW figi-gii:hasUniqueTextIdentifier "ANZW" .

figi-ps:HSAS a figi-gii:PricingSource .

figi-ps:BPAG a owl:NamedIndividual .

figi-st:lebaneseCP a owl:NamedIndividual .

figi-ps:HSAS skos:prefLabel "hsbc asia" .

figi-ps:BPAG a figi-gii:PricingSource .

figi-st:lebaneseCP a figi-gii:SecurityType .

figi-ps:HSAS figi-gii:hasUniqueTextIdentifier "HSAS" .

figi-ps:BPAG skos:prefLabel "bnp paribas - ny" .

figi-st:lebaneseCP skos:definition "Lebanese Commercial Paper" .

figi-ps:HSAU a owl:NamedIndividual .

figi-ps:BPAG figi-gii:hasUniqueTextIdentifier "BPAG" .

figi-st:lebaneseCP skos:prefLabel "lebanese cp" .

figi-ps:HSAU a figi-gii:PricingSource .

figi-ps:BPAL a owl:NamedIndividual .

figi-st:lebaneseCP figi-gii:hasUniqueTextIdentifier "LEBANESE CP" .

figi-ps:BPAL a figi-gii:PricingSource .

figi-ps:HSAU skos:prefLabel "hsbc australia" .

figi-ps:ANZX a owl:NamedIndividual .

figi-ps:BPAL skos:prefLabel "bp alpha" .

figi-ps:ANZX a figi-gii:PricingSource .

figi-ps:HSAU figi-gii:hasUniqueTextIdentifier "HSAU" .

figi-ps:BPAL figi-gii:hasUniqueTextIdentifier "BPAL" .

figi-ps:ANZX skos:prefLabel "anz banking group" .

figi-ps:HSAY a owl:NamedIndividual .

figi-ps:BPAM a owl:NamedIndividual .

figi-ps:ANZX figi-gii:hasUniqueTextIdentifier "ANZX" .

figi-ps:HSAY a figi-gii:PricingSource .

figi-ps:BPAM a figi-gii:PricingSource .

figi-ps:AOIL a owl:NamedIndividual .

figi-ps:HSAY skos:prefLabel "hsbc securities usa" .

figi-ps:AOIL a figi-gii:PricingSource .

figi-ps:BPAM skos:prefLabel "boci-pru asset mgt" .

figi-ps:HSAY figi-gii:hasUniqueTextIdentifier "HSAY" .

figi-ps:AOIL skos:prefLabel "algorithm" .

figi-ps:BPAM figi-gii:hasUniqueTextIdentifier "BPAM" .

figi-ps:HSB a owl:NamedIndividual .

figi-ps:AOIL figi-gii:hasUniqueTextIdentifier "AOIL" .

figi-ps:HSB a figi-gii:PricingSource .

figi-ps:BPAP a owl:NamedIndividual .

figi-st:liquidityNote a owl:NamedIndividual .

figi-ps:BPAP a figi-gii:PricingSource .

figi-ps:HSB skos:prefLabel "hsbc bank usa" .

figi-st:liquidityNote a figi-gii:SecurityType .

figi-ps:BPAP skos:prefLabel "bnp paribas" .

figi-ps:HSB figi-gii:hasUniqueTextIdentifier "HSB" .

figi-st:liquidityNote skos:definition "Liquidity Note - asset backed, cp-like extendible instruments" .

figi-ps:BPAP figi-gii:hasUniqueTextIdentifier "BPAP" .

figi-ps:HSBB a owl:NamedIndividual .

figi-st:liquidityNote skos:prefLabel "liquidity note" .

figi-ps:HSBB a figi-gii:PricingSource .

figi-ps:BPAS a owl:NamedIndividual .

figi-st:liquidityNote figi-gii:hasUniqueTextIdentifier "LIQUIDITY NOTE" .

figi-ps:BPAS a figi-gii:PricingSource .

figi-ps:HSBB skos:prefLabel "hsbc 4:30" .

figi-ps:AONC a owl:NamedIndividual .

figi-ps:BPAS skos:prefLabel "bnp paribas pp" .

figi-ps:HSBB figi-gii:hasUniqueTextIdentifier "HSBB" .

figi-ps:AONC a figi-gii:PricingSource .

figi-ps:BPAS figi-gii:hasUniqueTextIdentifier "BPAS" .

figi-ps:HSBC a owl:NamedIndividual .

figi-ps:AONC skos:prefLabel "aon benfield securit" .

figi-ps:BPAV a owl:NamedIndividual .

figi-ps:HSBC a figi-gii:PricingSource .

figi-ps:AONC figi-gii:hasUniqueTextIdentifier "AONC" .

figi-ps:BPAV a figi-gii:PricingSource .

figi-ps:HSBC skos:prefLabel "hsbc tsy and cap mkts" .

figi-st:loc a owl:NamedIndividual .

figi-ps:BPAV skos:prefLabel "banca antoniana ven" .

figi-ps:HSBC figi-gii:hasUniqueTextIdentifier "HSBC" .

figi-st:loc a figi-gii:SecurityType .

figi-ps:BPAV figi-gii:hasUniqueTextIdentifier "BPAV" .

figi-ps:HSBE a owl:NamedIndividual , figi-gii:PricingSource .

figi-ps:BPAX a owl:NamedIndividual .

figi-ps:HSBE skos:prefLabel "hsbc sa e-bond" .

figi-ps:BPAX a figi-gii:PricingSource .

figi-ps:HSBE figi-gii:hasUniqueTextIdentifier "HSBE" .

figi-st:loc skos:definition "A financial obligation of the borrower which has been guaranteed by the lender(s). There are different types of Letters of Credit (L/Cs) used for various purposes. Trade and Commercial L/Cs are used for purchases of goods. Standby and Documentary L/Cs are used for the completion of construction projects and/or general purposes." .

figi-ps:BPAX skos:prefLabel "bnp paribas axes" .

figi-ps:HSBF a owl:NamedIndividual .

figi-st:loc skos:prefLabel "loc" .

figi-ps:BPAX figi-gii:hasUniqueTextIdentifier "BPAX" .

figi-st:loc figi-gii:hasUniqueTextIdentifier "LOC" .

figi-ps:BPBA a owl:NamedIndividual .

figi-ps:HSBF a figi-gii:PricingSource .

figi-ps:BPBA a figi-gii:PricingSource .

figi-ps:AP a owl:NamedIndividual .

figi-ps:HSBF skos:prefLabel "hsbc 11:30" .

figi-ps:BPBA skos:prefLabel "bco provincia bs as" .

figi-ps:AP a figi-gii:PricingSource .

figi-ps:HSBF figi-gii:hasUniqueTextIdentifier "HSBF" .

figi-ps:BPBA figi-gii:hasUniqueTextIdentifier "BPBA" .

figi-ps:AP skos:prefLabel "anaconda invest sa" .

figi-ps:HSBI a owl:NamedIndividual .

figi-ps:BPCW a owl:NamedIndividual .

figi-ps:AP figi-gii:hasUniqueTextIdentifier "AP" .

figi-ps:BPCW a figi-gii:PricingSource .

figi-st:locGuaranteeFac a owl:NamedIndividual .

figi-ps:HSBI a figi-gii:PricingSource .

figi-st:locGuaranteeFac a figi-gii:SecurityType .

figi-ps:BPCW skos:prefLabel "bnp paribas - corps" .

figi-ps:HSBI skos:prefLabel "hsbc london" .

figi-ps:BPCW figi-gii:hasUniqueTextIdentifier "BPCW" .

figi-ps:HSBI figi-gii:hasUniqueTextIdentifier "HSBI" .

figi-st:locGuaranteeFac skos:definition "A financial obligation of the borrower which has been guaranteed by the lender(s) to ensure a project is completed." .

figi-ps:BPDN a owl:NamedIndividual .

figi-ps:HSBK a owl:NamedIndividual .

figi-st:locGuaranteeFac skos:prefLabel "loc guarantee fac" .

figi-ps:BPDN a figi-gii:PricingSource .

figi-ps:HSBK a figi-gii:PricingSource .

figi-st:locGuaranteeFac figi-gii:hasUniqueTextIdentifier "LOC GUARANTEE FAC" .

figi-ps:BPDN skos:prefLabel "bnp paribas - boom" .

figi-ps:HSBK skos:prefLabel "halyk bk kazakhstan" .

figi-ps:AP4 a owl:NamedIndividual .

figi-ps:HSBK figi-gii:hasUniqueTextIdentifier "HSBK" .

figi-ps:BPDN figi-gii:hasUniqueTextIdentifier "BPDN" .

figi-ps:AP4 a figi-gii:PricingSource .

figi-ps:HSBL a owl:NamedIndividual .

figi-ps:BPDR a owl:NamedIndividual .

figi-ps:AP4 skos:prefLabel "fjarde ap-fonden" .

figi-ps:HSBL a figi-gii:PricingSource .

figi-ps:BPDR a figi-gii:PricingSource .

figi-ps:AP4 figi-gii:hasUniqueTextIdentifier "AP4" .

figi-ps:HSBL skos:prefLabel "hsbc" .

figi-ps:BPDR skos:prefLabel "banco popular,dr" .

figi-st:ltdPart a owl:NamedIndividual .

figi-ps:HSBL figi-gii:hasUniqueTextIdentifier "HSBL" .

figi-ps:BPDR figi-gii:hasUniqueTextIdentifier "BPDR" .

figi-st:ltdPart a figi-gii:SecurityType .

figi-ps:HSBM a owl:NamedIndividual .

figi-ps:BPEG a owl:NamedIndividual .

figi-ps:HSBM a figi-gii:PricingSource .

figi-ps:BPEG a figi-gii:PricingSource .

figi-st:ltdPart skos:definition "Limited Partnership. A partnership with at least one of the partners holding only a limited liability." .

figi-ps:HSBM skos:prefLabel "hsbc markets" .

figi-ps:BPEG skos:prefLabel "bnp paribas euro gov" .

figi-st:ltdPart skos:prefLabel "ltd part" .

figi-ps:HSBM figi-gii:hasUniqueTextIdentifier "HSBM" .

figi-ps:BPEG figi-gii:hasUniqueTextIdentifier "BPEG" .

figi-st:ltdPart figi-gii:hasUniqueTextIdentifier "Ltd Part" .

figi-ps:HSBP a owl:NamedIndividual .

figi-ps:BPEU a owl:NamedIndividual .

figi-ps:HSBP a figi-gii:PricingSource .

figi-ps:APCB a owl:NamedIndividual .

figi-ps:BPEU a figi-gii:PricingSource .

figi-ps:HSBP skos:prefLabel "hsbc prime" .

figi-ps:APCB a figi-gii:PricingSource .

figi-ps:BPEU skos:prefLabel "bp" .

figi-ps:HSBP figi-gii:hasUniqueTextIdentifier "HSBP" .

figi-ps:APCB skos:prefLabel "citibank apcb treas." .

figi-ps:BPEU figi-gii:hasUniqueTextIdentifier "BPEU" .

figi-ps:HSBQ a owl:NamedIndividual .

figi-ps:APCB figi-gii:hasUniqueTextIdentifier "APCB" .

figi-ps:BPEX a owl:NamedIndividual .

figi-ps:HSBQ a figi-gii:PricingSource .

figi-ps:BPEX a figi-gii:PricingSource .

figi-ps:APDR a owl:NamedIndividual .

figi-ps:HSBQ skos:prefLabel "hsbc internal" .

figi-ps:APDR a figi-gii:PricingSource .

figi-ps:BPEX skos:prefLabel "bnp paribas london" .

figi-ps:HSBQ figi-gii:hasUniqueTextIdentifier "HSBQ" .

figi-ps:APDR skos:prefLabel "asociacion popular" .

figi-ps:BPEX figi-gii:hasUniqueTextIdentifier "BPEX" .

figi-ps:HSBR a owl:NamedIndividual .

figi-ps:APDR figi-gii:hasUniqueTextIdentifier "APDR" .

figi-ps:HSBR a figi-gii:PricingSource .

figi-ps:BPGL a owl:NamedIndividual .

figi-st:malaysianCP a owl:NamedIndividual .

figi-ps:HSBR skos:prefLabel "hsbc bank plc, dubai" .

figi-ps:BPGL a figi-gii:PricingSource .

figi-st:malaysianCP a figi-gii:SecurityType .

figi-ps:HSBR figi-gii:hasUniqueTextIdentifier "HSBR" .

figi-st:malaysianCP skos:definition "Malaysian Commercial Paper" .

figi-ps:HSBS a owl:NamedIndividual .

figi-st:malaysianCP skos:prefLabel "malaysian cp" .

figi-ps:HSBS a figi-gii:PricingSource .

figi-st:malaysianCP figi-gii:hasUniqueTextIdentifier "MALAYSIAN CP" .

figi-ps:HSBS skos:prefLabel "hsbc brazil autoex" .

figi-ps:BPGL skos:prefLabel "bnp paribas london" .

figi-ps:APOC a owl:NamedIndividual .

figi-ps:HSBS figi-gii:hasUniqueTextIdentifier "HSBS" .

figi-ps:APOC a figi-gii:PricingSource .

figi-ps:BPGL figi-gii:hasUniqueTextIdentifier "BPGL" .

figi-ps:HSBT a owl:NamedIndividual .

figi-ps:APOC skos:prefLabel "alliance poc" .

figi-ps:HSBT a figi-gii:PricingSource .

figi-ps:BPGP a owl:NamedIndividual .

figi-ps:APOC figi-gii:hasUniqueTextIdentifier "APOC" .

figi-ps:HSBT skos:prefLabel "hsbc bank plc" .

figi-ps:BPGP a figi-gii:PricingSource .

figi-st:managedAccount a owl:NamedIndividual .

figi-ps:HSBT figi-gii:hasUniqueTextIdentifier "HSBT" .

figi-st:managedAccount a figi-gii:SecurityType .

figi-ps:BPGP skos:prefLabel "bnp paribas paris" .

figi-ps:HSBV a owl:NamedIndividual , figi-gii:PricingSource .

figi-ps:BPGP figi-gii:hasUniqueTextIdentifier "BPGP" .

figi-ps:HSBV skos:prefLabel "hsbc vietnam" .

figi-ps:BPHK a owl:NamedIndividual .

figi-ps:HSBV figi-gii:hasUniqueTextIdentifier "HSBV" .

figi-st:managedAccount skos:definition "An investment account that is owned by anindividual investorand looked after by a hired professional money manager. In contrast to mutual funds (which are professionally managed on behalf of many mutual-fund holders), managed accounts are personalizedinvestment portfolios tailored to the specific needs of the account holder." .

figi-ps:BPHK a figi-gii:PricingSource .

figi-ps:HSBW a owl:NamedIndividual .

figi-st:managedAccount skos:prefLabel "managed account" .

figi-ps:HSBW a figi-gii:PricingSource .

figi-ps:BPHK skos:prefLabel "bnp paribas hk gov" .

figi-st:managedAccount figi-gii:hasUniqueTextIdentifier "Managed Account" .

figi-ps:BPHK figi-gii:hasUniqueTextIdentifier "BPHK" .

figi-ps:APS a owl:NamedIndividual , figi-gii:PricingSource .

figi-ps:BPHX a owl:NamedIndividual .

figi-ps:APS skos:prefLabel "aps asset mgt" .

figi-ps:BPHX a figi-gii:PricingSource .

figi-ps:APS figi-gii:hasUniqueTextIdentifier "APS" .

figi-ps:BPHX skos:prefLabel "bank przemyslowo" .

figi-st:marginTermDep a owl:NamedIndividual .

figi-ps:BPHX figi-gii:hasUniqueTextIdentifier "BPHX" .

figi-st:marginTermDep a figi-gii:SecurityType .

figi-ps:BPI1 a owl:NamedIndividual .

figi-st:marginTermDep skos:definition "Margin Term Deposits" .

figi-ps:BPI1 a figi-gii:PricingSource .

figi-ps:HSBW skos:prefLabel "hsbc executable govt" .

figi-st:marginTermDep skos:prefLabel "margin term dep" .

figi-ps:BPI1 skos:prefLabel "bpi treasury" .

figi-ps:HSBW figi-gii:hasUniqueTextIdentifier "HSBW" .

figi-st:marginTermDep figi-gii:hasUniqueTextIdentifier "MARGIN TERM DEP" .

figi-ps:BPI1 figi-gii:hasUniqueTextIdentifier "BPI1" .

figi-ps:HSCB a owl:NamedIndividual .

figi-ps:ARAB a owl:NamedIndividual .

figi-ps:HSCB a figi-gii:PricingSource .

figi-ps:BPIB a owl:NamedIndividual .

figi-ps:ARAB a figi-gii:PricingSource .

figi-ps:HSCB skos:prefLabel "hsbc secs - corps" .

figi-ps:BPIB a figi-gii:PricingSource .

figi-ps:ARAB skos:prefLabel "arab bank" .

figi-ps:HSCB figi-gii:hasUniqueTextIdentifier "HSCB" .

figi-ps:BPIB skos:prefLabel "banco bpi sa" .

figi-ps:ARAB figi-gii:hasUniqueTextIdentifier "ARAB" .

figi-ps:HSCD a owl:NamedIndividual .

figi-ps:BPIB figi-gii:hasUniqueTextIdentifier "BPIB" .

figi-st:masterNotes a owl:NamedIndividual .

figi-ps:HSCD a figi-gii:PricingSource .

figi-st:masterNotes a figi-gii:SecurityType .

figi-ps:BPIC a owl:NamedIndividual .

figi-ps:HSCD skos:prefLabel "hsbc sec canada inc" .

figi-ps:BPIC a figi-gii:PricingSource .

figi-st:masterNotes skos:definition "MMKT instrument issued by large, creditworthy companies to banks." .

figi-ps:HSCD figi-gii:hasUniqueTextIdentifier "HSCD" .

figi-ps:BPIC skos:prefLabel "bpi manila" .

figi-st:masterNotes skos:prefLabel "master notes" .

figi-ps:HSCE a owl:NamedIndividual .

figi-ps:BPIC figi-gii:hasUniqueTextIdentifier "BPIC" .

figi-st:masterNotes figi-gii:hasUniqueTextIdentifier "MASTER NOTES" .

figi-ps:HSCE a figi-gii:PricingSource .

figi-ps:BPIL a owl:NamedIndividual .

figi-ps:ARAM a owl:NamedIndividual .

figi-ps:BPIL a figi-gii:PricingSource .

figi-ps:HSCE skos:prefLabel "hsbc sri lanka" .

figi-ps:ARAM a figi-gii:PricingSource .

figi-ps:BPIL skos:prefLabel "banco port de invst" .

figi-ps:HSCE figi-gii:hasUniqueTextIdentifier "HSCE" .

figi-ps:ARAM skos:prefLabel "ardevora" .

figi-ps:BPIL skos:prefLabel "banco port. de invst" .

figi-ps:HSCH a owl:NamedIndividual .

figi-ps:ARAM figi-gii:hasUniqueTextIdentifier "ARAM" .

figi-ps:HSCH a figi-gii:PricingSource .

figi-ps:BPIL figi-gii:hasUniqueTextIdentifier "BPIL" .

figi-st:mbs10yr a owl:NamedIndividual .

figi-ps:HSCH skos:prefLabel "hsbc bank usa chile" .

figi-st:mbs10yr a figi-gii:SecurityType .

figi-ps:BPIM a owl:NamedIndividual .

figi-ps:HSCH figi-gii:hasUniqueTextIdentifier "HSCH" .

figi-ps:BPIM a figi-gii:PricingSource .

figi-ps:HSCO a owl:NamedIndividual .

figi-ps:BPIM skos:prefLabel "banco portugues mtge" .

figi-ps:HSCO a figi-gii:PricingSource .

figi-st:mbs10yr skos:definition "Mortgage-Backed Security (MBS). A debt instrument with a pool of real estate loans as the underlying collateral. The mortgage payments of the individual real estate assets are used to pay interest and principal on the bonds. - 10 years" .

figi-ps:BPIM figi-gii:hasUniqueTextIdentifier "BPIM" .

figi-ps:HSCO skos:prefLabel "hsbc colombia" .

figi-st:mbs10yr skos:prefLabel "mbs 10yr" .

figi-ps:BPIP a owl:NamedIndividual .

figi-ps:HSCO figi-gii:hasUniqueTextIdentifier "HSCO" .

figi-st:mbs10yr figi-gii:hasUniqueTextIdentifier "MBS 10yr" .

figi-ps:BPIP a figi-gii:PricingSource .

figi-ps:HSCT a owl:NamedIndividual .

figi-ps:ARBJ a owl:NamedIndividual .

figi-ps:HSCT a figi-gii:PricingSource .

figi-ps:BPIP skos:prefLabel "bank phil islands" .

figi-ps:ARBJ a figi-gii:PricingSource .

figi-ps:HSCT skos:prefLabel "hsbc e trading" .

figi-ps:BPIP figi-gii:hasUniqueTextIdentifier "BPIP" .

figi-ps:ARBJ skos:prefLabel "arab bank plc" .

figi-ps:HSCT figi-gii:hasUniqueTextIdentifier "HSCT" .

figi-ps:BPIT a owl:NamedIndividual .

figi-ps:ARBJ figi-gii:hasUniqueTextIdentifier "ARBJ" .

figi-ps:BPIT a figi-gii:PricingSource .

figi-ps:HSDN a owl:NamedIndividual .

figi-st:mbs15yr a owl:NamedIndividual .

figi-ps:BPIT skos:prefLabel "bpi trust" .

figi-st:mbs15yr a figi-gii:SecurityType .

figi-ps:BPIT figi-gii:hasUniqueTextIdentifier "BPIT" .

figi-ps:HSDN a figi-gii:PricingSource .

figi-ps:BPJP a owl:NamedIndividual .

figi-ps:HSDN skos:prefLabel "hsbc boom" .

figi-ps:BPJP a figi-gii:PricingSource .

figi-st:mbs15yr skos:definition "Mortgage-Backed Security (MBS). A debt instrument with a pool of real estate loans as the underlying collateral. The mortgage payments of the individual real estate assets are used to pay interest and principal on the bonds. - 15 years" .

figi-ps:BPJP skos:prefLabel "bnp paribas eqty" .

figi-ps:HSDN figi-gii:hasUniqueTextIdentifier "HSDN" .

figi-st:mbs15yr skos:prefLabel "mbs 15yr" .

figi-ps:BPJP figi-gii:hasUniqueTextIdentifier "BPJP" .

figi-ps:HSDO a owl:NamedIndividual .

figi-st:mbs15yr figi-gii:hasUniqueTextIdentifier "MBS 15yr" .

figi-ps:HSDO a figi-gii:PricingSource .

figi-ps:BPLS a owl:NamedIndividual .

figi-ps:ARBQ a owl:NamedIndividual .

figi-ps:HSDO skos:prefLabel "hsbc secs - indic" .

figi-ps:ARBQ a figi-gii:PricingSource .

figi-ps:BPLS a figi-gii:PricingSource .

figi-ps:HSDO figi-gii:hasUniqueTextIdentifier "HSDO" .

figi-ps:ARBQ skos:prefLabel "arab bank plc qatar" .

figi-ps:BPLS skos:prefLabel "bond partners" .

figi-ps:HSEA a owl:NamedIndividual .

figi-ps:ARBQ figi-gii:hasUniqueTextIdentifier "ARBQ" .

figi-ps:HSEA a figi-gii:PricingSource .

figi-ps:BPLS figi-gii:hasUniqueTextIdentifier "BPLS" .

figi-st:mbs20yr a owl:NamedIndividual .

figi-ps:HSEA skos:prefLabel "hsbc equity asia" .

figi-st:mbs20yr a figi-gii:SecurityType .

figi-ps:BPLX a owl:NamedIndividual .

figi-ps:HSEA figi-gii:hasUniqueTextIdentifier "HSEA" .

figi-ps:BPLX a figi-gii:PricingSource .

figi-ps:HSEM a owl:NamedIndividual .

figi-ps:BPLX skos:prefLabel "bondpartners s.a." .

figi-ps:HSEM a figi-gii:PricingSource .

figi-st:mbs20yr skos:definition "Mortgage-Backed Security (MBS). A debt instrument with a pool of real estate loans as the underlying collateral. The mortgage payments of the individual real estate assets are used to pay interest and principal on the bonds. - 20 years" .

figi-ps:BPLX figi-gii:hasUniqueTextIdentifier "BPLX" .

figi-ps:HSEM skos:prefLabel "hsbc securities em" .

figi-st:mbs20yr skos:prefLabel "mbs 20yr" .

figi-ps:BPLZ a owl:NamedIndividual .

figi-ps:HSEM figi-gii:hasUniqueTextIdentifier "HSEM" .

figi-st:mbs20yr figi-gii:hasUniqueTextIdentifier "MBS 20yr" .

figi-ps:BPLZ a figi-gii:PricingSource .

figi-ps:HSEP a owl:NamedIndividual .

figi-ps:ARBR a owl:NamedIndividual .

figi-ps:BPLZ skos:prefLabel "banca popolare lazio" .

figi-ps:ARBR a figi-gii:PricingSource .

figi-ps:HSEP a figi-gii:PricingSource .

figi-ps:BPLZ figi-gii:hasUniqueTextIdentifier "BPLZ" .

figi-ps:ARBR skos:prefLabel "arbor researchandtrad" .

figi-ps:HSEP skos:prefLabel "hsbc egypt" .

figi-ps:BPMC a owl:NamedIndividual .

figi-ps:ARBR figi-gii:hasUniqueTextIdentifier "ARBR" .

figi-ps:BPMC a figi-gii:PricingSource .

figi-ps:HSEP figi-gii:hasUniqueTextIdentifier "HSEP" .

figi-st:mbs30yr a owl:NamedIndividual , figi-gii:SecurityType .

figi-ps:HSET a owl:NamedIndividual , figi-gii:PricingSource .

figi-ps:BPMC skos:prefLabel "bnp paribas ny" .

figi-ps:HSET skos:prefLabel "hsbc executable" .

figi-ps:BPMC figi-gii:hasUniqueTextIdentifier "BPMC" .

figi-ps:HSET figi-gii:hasUniqueTextIdentifier "HSET" .

figi-st:mbs30yr skos:definition "Mortgage-Backed Security (MBS). A debt instrument with a pool of real estate loans as the underlying collateral. The mortgage payments of the individual real estate assets are used to pay interest and principal on the bonds. - 30 years" .

figi-ps:BPMF a owl:NamedIndividual .

figi-ps:HSFD a owl:NamedIndividual .

figi-ps:BPMF a figi-gii:PricingSource .

figi-ps:HSFD a figi-gii:PricingSource ;
	skos:prefLabel "hsbc structured fund" .

figi-st:mbs30yr skos:prefLabel "mbs 30yr" .

figi-ps:HSFD figi-gii:hasUniqueTextIdentifier "HSFD" .

figi-ps:BPMF skos:prefLabel "baroda pioneer amc" .

figi-st:mbs30yr figi-gii:hasUniqueTextIdentifier "MBS 30yr" .

figi-ps:HSGC a owl:NamedIndividual .

figi-ps:BPMF figi-gii:hasUniqueTextIdentifier "BPMF" .

figi-ps:HSGC a figi-gii:PricingSource .

figi-ps:ARC a owl:NamedIndividual .

figi-ps:HSGC skos:prefLabel "hsbc" .

figi-ps:ARC a figi-gii:PricingSource .

figi-ps:BPMJ a owl:NamedIndividual .

figi-ps:HSGC figi-gii:hasUniqueTextIdentifier "HSGC" .

figi-ps:ARC skos:prefLabel "arc securities ltd" .

figi-ps:BPMJ a figi-gii:PricingSource .

figi-ps:HSH a owl:NamedIndividual .

figi-ps:ARC skos:prefLabel "arca sgr spa" .

figi-ps:HSH a figi-gii:PricingSource .

figi-ps:BPMJ skos:prefLabel "bnp paribas mbs" .

figi-ps:ARC figi-gii:hasUniqueTextIdentifier "ARC" .

figi-ps:HSH skos:prefLabel "hsh nordbank" .

figi-ps:BPMJ figi-gii:hasUniqueTextIdentifier "BPMJ" .

figi-st:mbsArm a owl:NamedIndividual .

figi-ps:HSH figi-gii:hasUniqueTextIdentifier "HSH" .

figi-ps:BPMM a owl:NamedIndividual .

figi-st:mbsArm a figi-gii:SecurityType .

figi-ps:HSHK a owl:NamedIndividual .

figi-ps:BPMM a figi-gii:PricingSource .

figi-ps:HSHK a figi-gii:PricingSource .

figi-ps:BPMM skos:prefLabel "banco popular" .

figi-ps:HSHK skos:prefLabel "hang seng bank" .

figi-st:mbsArm skos:definition "Mortgage-Backed Security (MBS). A debt instrument with a pool of real estate loans as the underlying collateral. The mortgage payments of the individual real estate assets are used to pay interest and principal on the bonds." .

figi-ps:HSHK figi-gii:hasUniqueTextIdentifier "HSHK" .

figi-ps:BPMM figi-gii:hasUniqueTextIdentifier "BPMM" .

figi-st:mbsArm skos:prefLabel "mbs arm" .

figi-ps:HSHT a owl:NamedIndividual .

figi-ps:BPMO a owl:NamedIndividual .

figi-st:mbsArm figi-gii:hasUniqueTextIdentifier "MBS ARM" .

figi-ps:HSHT a figi-gii:PricingSource .

figi-ps:BPMO a figi-gii:PricingSource .

figi-ps:ARCI a owl:NamedIndividual .

figi-ps:HSHT skos:prefLabel "hsh nordbank ag" .

figi-ps:BPMO skos:prefLabel "bnp paribas moscow" .

figi-ps:ARCI a figi-gii:PricingSource .

figi-ps:HSHT figi-gii:hasUniqueTextIdentifier "HSHT" .

figi-ps:BPMO figi-gii:hasUniqueTextIdentifier "BPMO" .

figi-ps:ARCI skos:prefLabel "arcis international" .

figi-ps:HSI a owl:NamedIndividual .

figi-ps:BPMP a owl:NamedIndividual .

figi-ps:ARCI figi-gii:hasUniqueTextIdentifier "ARCI" .

figi-ps:HSI a figi-gii:PricingSource .

figi-ps:BPMP a figi-gii:PricingSource .

figi-st:mbsBalloon a owl:NamedIndividual .

figi-ps:HSI skos:prefLabel "hsbc securities" .

figi-ps:BPMP skos:prefLabel "bpm ireland plc" .

figi-st:mbsBalloon a figi-gii:SecurityType .

figi-ps:HSI figi-gii:hasUniqueTextIdentifier "HSI" .

figi-ps:BPMP figi-gii:hasUniqueTextIdentifier "BPMP" .

figi-ps:HSIE a owl:NamedIndividual , figi-gii:PricingSource .

figi-ps:BPMT a owl:NamedIndividual .

figi-ps:HSIE skos:prefLabel "hsbc jakarta ebond" .

figi-st:mbsBalloon skos:definition "Balloon. The final payment on a loan or mortgage that is much larger than previous payments. Some debts are structured with balloon payments to account for events such as increased interest rates during the life of the loan." .

figi-ps:HSIE figi-gii:hasUniqueTextIdentifier "HSIE" .

figi-st:mbsBalloon skos:prefLabel "mbs balloon" .

figi-ps:BPMT a figi-gii:PricingSource .

figi-st:mbsBalloon figi-gii:hasUniqueTextIdentifier "MBS balloon" .

figi-ps:HSIP a owl:NamedIndividual .

figi-ps:BPMT skos:prefLabel "bank permata" .

figi-ps:HSIP a figi-gii:PricingSource .

figi-st:mbsOther a owl:NamedIndividual .

figi-ps:BPMT figi-gii:hasUniqueTextIdentifier "BPMT" .

figi-st:mbsOther a figi-gii:SecurityType .

figi-ps:HSIP skos:prefLabel "hsbc internal prices" .

figi-ps:BPNS a owl:NamedIndividual .

figi-ps:HSIP figi-gii:hasUniqueTextIdentifier "HSIP" .

figi-ps:BPNS a figi-gii:PricingSource .

figi-st:mbsOther skos:definition "Description for Agency Pools (Fannie, Freddie, Ginnie) that are unable to be mapped to a generic security." .

figi-ps:HSJC a owl:NamedIndividual .

figi-ps:BPNS skos:prefLabel "bnp paribas nyc" .

figi-st:mbsOther skos:prefLabel "mbs other" .

figi-ps:HSJC a figi-gii:PricingSource .

figi-ps:BPNS figi-gii:hasUniqueTextIdentifier "BPNS" .

figi-ps:HSJC skos:prefLabel "hsbc" .

figi-st:mbsOther figi-gii:hasUniqueTextIdentifier "MBS Other" .

figi-ps:BPNT a owl:NamedIndividual .

figi-ps:HSJC figi-gii:hasUniqueTextIdentifier "HSJC" .

figi-ps:BPNT a figi-gii:PricingSource .

figi-ps:AREC a owl:NamedIndividual .

figi-ps:BPNT skos:prefLabel "broadpoint capital" .

figi-ps:AREC a figi-gii:PricingSource .

figi-ps:HSLA a owl:NamedIndividual .

figi-ps:BPNT figi-gii:hasUniqueTextIdentifier "BPNT" .

figi-ps:AREC skos:prefLabel "armeconombank ojsc" .

figi-ps:HSLA a figi-gii:PricingSource .

figi-ps:BPNY a owl:NamedIndividual .

figi-ps:AREC figi-gii:hasUniqueTextIdentifier "AREC" .

figi-ps:HSLA skos:prefLabel "hsbc secs - usa" .

figi-ps:BPNY a figi-gii:PricingSource .

figi-st:medTermNote a owl:NamedIndividual .

figi-ps:HSLA figi-gii:hasUniqueTextIdentifier "HSLA" .

figi-st:medTermNote a figi-gii:SecurityType .

figi-ps:BPNY skos:prefLabel "bnp paribas ny" .

figi-ps:HSLB a owl:NamedIndividual .

figi-ps:BPNY figi-gii:hasUniqueTextIdentifier "BPNY" .

figi-ps:HSLB a figi-gii:PricingSource ;
	skos:prefLabel "hsbc tsy and cap mkts" .

figi-ps:BPPN a owl:NamedIndividual .

figi-ps:HSLB figi-gii:hasUniqueTextIdentifier "HSLB" .

figi-ps:BPPN a figi-gii:PricingSource .

figi-st:medTermNote skos:definition "Medium Term Note (MTN). Continuously offered notes with maturities ranging from nine months to 40 years. Typically unsecured debt obligations, each medium term note issue (also known as a tranche) is a drawdown from a program (prospectus) level. MTNs are flexible in structure and market timing because of this type of issuance (modeled from the commercial paper market)." .

figi-ps:BPPN skos:prefLabel "bnp private notes" .

figi-ps:HSLR a owl:NamedIndividual .

figi-st:medTermNote skos:prefLabel "med term note" .

figi-ps:BPPN figi-gii:hasUniqueTextIdentifier "BPPN" .

figi-ps:HSLR a figi-gii:PricingSource .

figi-st:medTermNote figi-gii:hasUniqueTextIdentifier "MED TERM NOTE" .

figi-ps:BPPR a owl:NamedIndividual .

figi-ps:HSLR skos:prefLabel "hsbc securities" .

figi-ps:BPPR a figi-gii:PricingSource .

figi-ps:ARES a owl:NamedIndividual .

figi-ps:HSLR figi-gii:hasUniqueTextIdentifier "HSLR" .

figi-ps:ARES a figi-gii:PricingSource .

figi-ps:BPPR skos:prefLabel "banco popular pr" .

figi-ps:HSLT a owl:NamedIndividual .

figi-ps:ARES skos:prefLabel "ares management" .

figi-ps:BPPR figi-gii:hasUniqueTextIdentifier "BPPR" .

figi-ps:ARES figi-gii:hasUniqueTextIdentifier "ARES" .

figi-ps:BPRX a owl:NamedIndividual .

figi-ps:HSLT a figi-gii:PricingSource .

figi-ps:BPRX a figi-gii:PricingSource .

figi-st:mediumTermCD a owl:NamedIndividual .

figi-ps:HSLT skos:prefLabel "hsbc loans" .

figi-st:mediumTermCD a figi-gii:SecurityType .

figi-ps:BPRX skos:prefLabel "bnp paribas etrading" .

figi-ps:HSLT figi-gii:hasUniqueTextIdentifier "HSLT" .

figi-ps:BPRX figi-gii:hasUniqueTextIdentifier "BPRX" .

figi-st:mediumTermCD skos:definition "Medium Term Certificates of Deposit - medium term maturities" .

figi-ps:HSMA a owl:NamedIndividual .

figi-ps:BPSC a owl:NamedIndividual .

figi-st:mediumTermCD skos:prefLabel "medium term cd" .

figi-ps:HSMA a figi-gii:PricingSource .

figi-ps:BPSC a figi-gii:PricingSource .

figi-st:mediumTermCD figi-gii:hasUniqueTextIdentifier "MEDIUM TERM CD" .

figi-ps:HSMA skos:prefLabel "hsbc phil" .

figi-ps:BPSC skos:prefLabel "bnp structured cred" .

figi-ps:ARGS a owl:NamedIndividual .

figi-ps:HSMA figi-gii:hasUniqueTextIdentifier "HSMA" .

figi-ps:ARGS a figi-gii:PricingSource .

figi-ps:BPSC figi-gii:hasUniqueTextIdentifier "BPSC" .

figi-ps:HSME a owl:NamedIndividual .

figi-ps:ARGS skos:prefLabel "argus media limited" .

figi-ps:HSME a figi-gii:PricingSource .

figi-ps:BPSG a owl:NamedIndividual .

figi-ps:ARGS figi-gii:hasUniqueTextIdentifier "ARGS" .

figi-ps:BPSG a figi-gii:PricingSource .

figi-ps:HSME skos:prefLabel "hsbc middle east" .

figi-st:mediumTermEcd a owl:NamedIndividual .

figi-ps:BPSG skos:prefLabel "bnp paribas sgp" .

figi-ps:HSME figi-gii:hasUniqueTextIdentifier "HSME" .

figi-st:mediumTermEcd a figi-gii:SecurityType .

figi-ps:BPSG figi-gii:hasUniqueTextIdentifier "BPSG" .

figi-ps:HSMN a owl:NamedIndividual , figi-gii:PricingSource .

figi-st:mediumTermEcd skos:definition "Medium Term Euro Certificates of Deposit - medium term maturities" .

figi-ps:HSMN skos:prefLabel "hsbc phil" .

figi-ps:BPSN a owl:NamedIndividual .

figi-st:mediumTermEcd skos:prefLabel "medium term ecd" .

figi-ps:HSMN figi-gii:hasUniqueTextIdentifier "HSMN" .

figi-ps:BPSN a figi-gii:PricingSource .

figi-st:mediumTermEcd figi-gii:hasUniqueTextIdentifier "MEDIUM TERM ECD" .

figi-ps:HSMT a owl:NamedIndividual .

figi-ps:BPSN skos:prefLabel "bnp mtn inventory" .

figi-ps:HSMT a figi-gii:PricingSource .

figi-st:mediumTermYcd a owl:NamedIndividual .

figi-ps:BPSN figi-gii:hasUniqueTextIdentifier "BPSN" .

figi-ps:HSMT skos:prefLabel "hsbc indicative" .

figi-st:mediumTermYcd a figi-gii:SecurityType .

figi-ps:BPSS a owl:NamedIndividual .

figi-ps:HSMT figi-gii:hasUniqueTextIdentifier "HSMT" .

figi-ps:BPSS a figi-gii:PricingSource .

figi-st:mediumTermYcd skos:definition "Medium Term Yankee Certificates of Deposit - medium term maturities" .

figi-ps:HSMX a owl:NamedIndividual .

figi-ps:BPSS skos:prefLabel "bps - sberbank" .

figi-ps:HSMX a figi-gii:PricingSource .

figi-st:mediumTermYcd skos:prefLabel "medium term ycd" .

figi-ps:BPSS figi-gii:hasUniqueTextIdentifier "BPSS" .

figi-ps:HSMX skos:prefLabel "hsbc bank mexico" .

figi-st:mediumTermYcd figi-gii:hasUniqueTextIdentifier "MEDIUM TERM YCD" .

figi-ps:BPTK a owl:NamedIndividual .

figi-ps:HSMX figi-gii:hasUniqueTextIdentifier "HSMX" .

figi-ps:BPTK a figi-gii:PricingSource .

figi-ps:ARIA a owl:NamedIndividual .

figi-ps:HSPH a owl:NamedIndividual .

figi-ps:ARIA a figi-gii:PricingSource .

figi-ps:BPTK skos:prefLabel "bnp paribas tky ust" .

figi-ps:HSPH a figi-gii:PricingSource .

figi-ps:ARIA skos:prefLabel "aria investment ltd" .

figi-ps:BPTK figi-gii:hasUniqueTextIdentifier "BPTK" .

figi-ps:HSPH skos:prefLabel "hsbc philippines" .

figi-ps:ARIA figi-gii:hasUniqueTextIdentifier "ARIA" .

figi-ps:BPTR a owl:NamedIndividual .

figi-ps:HSPH figi-gii:hasUniqueTextIdentifier "HSPH" .

figi-ps:BPTR a figi-gii:PricingSource .

figi-st:mexicanCP a owl:NamedIndividual .

figi-ps:HSPP a owl:NamedIndividual .

figi-st:mexicanCP a figi-gii:SecurityType .

figi-ps:BPTR skos:prefLabel "bankpozitif" .

figi-ps:HSPP a figi-gii:PricingSource .

figi-st:mexicanCP skos:definition "Mexican Commercial Paper" .

figi-ps:BPTR figi-gii:hasUniqueTextIdentifier "BPTR" .

figi-ps:HSPP skos:prefLabel "hsbc bank" .

figi-st:mexicanCP skos:prefLabel "mexican cp" .

figi-ps:BPXJ a owl:NamedIndividual .

figi-st:mexicanCP figi-gii:hasUniqueTextIdentifier "MEXICAN CP" .

figi-ps:BPXJ a figi-gii:PricingSource .

figi-ps:ARIG a owl:NamedIndividual .

figi-ps:BPXJ skos:prefLabel "bnp paribas - bpxj" .

figi-ps:ARIG a figi-gii:PricingSource .

figi-ps:BPXJ figi-gii:hasUniqueTextIdentifier "BPXJ" .

figi-ps:HSPP figi-gii:hasUniqueTextIdentifier "HSPP" .

figi-ps:ARIG skos:prefLabel "auriga usa llc" .

figi-ps:BPZH a owl:NamedIndividual .

figi-ps:HSPS a owl:NamedIndividual .

figi-ps:BPZH a figi-gii:PricingSource .

figi-ps:ARIG figi-gii:hasUniqueTextIdentifier "ARIG" .

figi-ps:HSPS a figi-gii:PricingSource .

figi-ps:BPZH skos:prefLabel "bnp paribas" .

figi-st:mexicanPagare a owl:NamedIndividual .

figi-ps:HSPS skos:prefLabel "hsbc - euro open" .

figi-st:mexicanPagare a figi-gii:SecurityType .

figi-ps:BPZH figi-gii:hasUniqueTextIdentifier "BPZH" .

figi-ps:HSPS figi-gii:hasUniqueTextIdentifier "HSPS" .

figi-st:mexicanPagare skos:definition "Mexican Short Term MMKT instrument" .

figi-ps:BQA1 a owl:NamedIndividual .

figi-ps:HSSC a owl:NamedIndividual .

figi-st:mexicanPagare skos:prefLabel "mexican pagare" .

figi-ps:BQA1 a figi-gii:PricingSource .

figi-ps:HSSC a figi-gii:PricingSource .

figi-st:mexicanPagare figi-gii:hasUniqueTextIdentifier "MEXICAN PAGARE" .

figi-ps:BQA1 skos:prefLabel "bloomberg msg1 qa" .

figi-ps:HSSC skos:prefLabel "hssc structured cred" .

figi-st:mlp a owl:NamedIndividual .

figi-ps:BQA1 figi-gii:hasUniqueTextIdentifier "BQA1" .

figi-st:mlp a figi-gii:SecurityType .

figi-ps:HSSC figi-gii:hasUniqueTextIdentifier "HSSC" .

figi-ps:BQA2 a owl:NamedIndividual , figi-gii:PricingSource .

figi-ps:HSSE a owl:NamedIndividual .

figi-ps:BQA2 skos:prefLabel "bloomberg sqa qa2" .

figi-ps:HSSE a figi-gii:PricingSource .

figi-ps:BQA2 figi-gii:hasUniqueTextIdentifier "BQA2" .

figi-ps:HSSE skos:prefLabel "hsbc structured rate" ;
	figi-gii:hasUniqueTextIdentifier "HSSE" .

figi-ps:BQCV a owl:NamedIndividual .

figi-st:mlp skos:definition "Master Limited Partnership: A type of limited partnership that is publicly traded. There are two types of partners in this type of partnership: The limited partner is the person or group that provides the capital to the MLP and receives periodic income distributions from the MLP's cash flow, whereas the general partner is the party responsible for managing the MLP's affairs and receives compensation that is linked to the performance of the venture." .

figi-ps:BQCV a figi-gii:PricingSource .

figi-st:mlp skos:prefLabel "mlp" .

figi-ps:HSSH a owl:NamedIndividual .

figi-st:mlp figi-gii:hasUniqueTextIdentifier "MLP" .

figi-ps:BQCV skos:prefLabel "banque cantonale" .

figi-ps:HSSH a figi-gii:PricingSource .

figi-ps:ARKA a owl:NamedIndividual .

figi-ps:HSSH skos:prefLabel "hsbc shanghai" .

figi-ps:BQCV figi-gii:hasUniqueTextIdentifier "BQCV" .

figi-ps:ARKA a figi-gii:PricingSource .

figi-ps:HSSH figi-gii:hasUniqueTextIdentifier "HSSH" .

figi-ps:BQDS a owl:NamedIndividual .

figi-ps:ARKA skos:prefLabel "casa bolsa arka" .

figi-ps:BQDS a figi-gii:PricingSource .

figi-ps:HSSI a owl:NamedIndividual .

figi-ps:ARKA figi-gii:hasUniqueTextIdentifier "ARKA" .

figi-ps:BQDS skos:prefLabel "bqds" .

figi-ps:HSSI a figi-gii:PricingSource .

figi-st:moneyMarketCall a owl:NamedIndividual .

figi-ps:BQDS figi-gii:hasUniqueTextIdentifier "BQDS" .

figi-ps:HSSI skos:prefLabel "hsbc structured" .

figi-st:moneyMarketCall a figi-gii:SecurityType .

figi-ps:BRAA a owl:NamedIndividual .

figi-ps:HSSI figi-gii:hasUniqueTextIdentifier "HSSI" .

figi-ps:BRAA a figi-gii:PricingSource .

figi-ps:HSSP a owl:NamedIndividual .

figi-ps:BRAA skos:prefLabel "abn amro brazil" .

figi-st:moneyMarketCall skos:definition "A short-term money market, which allows for large financial institutions, such as banks, mutual funds and corporations to borrow and lend money at interbank rates" .

figi-ps:HSSP a figi-gii:PricingSource .

figi-ps:BRAA figi-gii:hasUniqueTextIdentifier "BRAA" .

figi-st:moneyMarketCall skos:prefLabel "money market call" .

figi-ps:HSSP skos:prefLabel "hsbc eqty struct nts" .

figi-ps:BRAD a owl:NamedIndividual .

figi-st:moneyMarketCall figi-gii:hasUniqueTextIdentifier "MONEY MARKET CALL" .

figi-ps:HSSP figi-gii:hasUniqueTextIdentifier "HSSP" .

figi-ps:BRAD a figi-gii:PricingSource .

figi-ps:ARKE a owl:NamedIndividual .

figi-ps:HSTA a owl:NamedIndividual .

figi-ps:BRAD skos:prefLabel "bradesco" .

figi-ps:ARKE a figi-gii:PricingSource .

figi-ps:HSTA a figi-gii:PricingSource .

figi-ps:BRAD figi-gii:hasUniqueTextIdentifier "BRAD" .

figi-ps:ARKE skos:prefLabel "arkhe dtvm" .

figi-ps:HSTA skos:prefLabel "hsbc tel aviv" .

figi-ps:BRAI a owl:NamedIndividual .

figi-ps:ARKE figi-gii:hasUniqueTextIdentifier "ARKE" .

figi-ps:HSTA figi-gii:hasUniqueTextIdentifier "HSTA" .

figi-ps:BRAI a figi-gii:PricingSource .

figi-st:mtnSubordinated a owl:NamedIndividual .

figi-ps:HSTL a owl:NamedIndividual .

figi-ps:BRAI skos:prefLabel "bradesco" .

figi-st:mtnSubordinated a figi-gii:SecurityType .

figi-ps:HSTL a figi-gii:PricingSource .

figi-ps:BRAI skos:prefLabel "bradesco bbi" .

figi-st:mtnSubordinated skos:definition "Medium Term Notes with Subordinated Ranking" .

figi-ps:HSTL skos:prefLabel "hsbc turkey" .

figi-ps:BRAI figi-gii:hasUniqueTextIdentifier "BRAI" .

figi-ps:HSTL figi-gii:hasUniqueTextIdentifier "HSTL" .

figi-st:mtnSubordinated skos:prefLabel "mtn subordinated" .

figi-ps:HSTM a owl:NamedIndividual .

figi-st:mtnSubordinated figi-gii:hasUniqueTextIdentifier "MTN SUBORDINATED" .

figi-ps:BRAL a owl:NamedIndividual .

figi-ps:HSTM a figi-gii:PricingSource .

figi-st:muniCP a owl:NamedIndividual .

figi-ps:BRAL a figi-gii:PricingSource .

figi-ps:HSTM skos:prefLabel "hang seng bank 11:30" .

figi-st:muniCP a figi-gii:SecurityType .

figi-ps:HSTM figi-gii:hasUniqueTextIdentifier "HSTM" .

figi-ps:HSTP a owl:NamedIndividual , figi-gii:PricingSource ;
	skos:prefLabel "hang seng bank 4:30" ;
	figi-gii:hasUniqueTextIdentifier "HSTP" .

figi-st:muniCP skos:definition "Commercial Paper. An unsecured short-term promise to repay a fixed amount on a certain future date. Commercial paper usually matures from 2 to 270 days and is traded on a discount basis. This debt instrument, issued by banks, companies and other borrowers, use only their credit ratings to back the security. Commercial Paper House. A dealer who buys commercial paper at one price, then tries to sell it at another." .

figi-ps:HSTR a owl:NamedIndividual .

figi-st:muniCP skos:prefLabel "muni cp" .

figi-ps:BRAL skos:prefLabel "bradesco" .

figi-ps:HSTR a figi-gii:PricingSource .

figi-st:muniCP figi-gii:hasUniqueTextIdentifier "MUNI CP" .

figi-ps:BRAL figi-gii:hasUniqueTextIdentifier "BRAL" .

figi-ps:ARKH a owl:NamedIndividual , figi-gii:PricingSource .

figi-ps:BRAM a owl:NamedIndividual .

figi-ps:ARKH skos:prefLabel "icap brazil" .

figi-ps:BRAM a figi-gii:PricingSource .

figi-ps:ARKH figi-gii:hasUniqueTextIdentifier "ARKH" .

figi-ps:BRAM skos:prefLabel "black river asset" .

figi-ps:HSTR skos:prefLabel "hsbc ldn" .

figi-ps:BRAM figi-gii:hasUniqueTextIdentifier "BRAM" .

figi-st:muniIntBearCP a owl:NamedIndividual .

figi-ps:HSTR figi-gii:hasUniqueTextIdentifier "HSTR" .

figi-ps:BRAN a owl:NamedIndividual .

figi-st:muniIntBearCP a figi-gii:SecurityType .

figi-ps:BRAN a figi-gii:PricingSource .

figi-ps:HSTS a owl:NamedIndividual .

figi-st:muniIntBearCP skos:definition "Municipal Commercial Paper / Interest Bearing" .

figi-ps:BRAN skos:prefLabel "brandes fixed income" .

figi-st:muniIntBearCP skos:prefLabel "muni int bear cp" .

figi-ps:BRAN figi-gii:hasUniqueTextIdentifier "BRAN" .

figi-st:muniIntBearCP figi-gii:hasUniqueTextIdentifier "MUNI INT BEAR CP" .

figi-ps:ARME a owl:NamedIndividual .

figi-ps:BRAT a owl:NamedIndividual .

figi-ps:ARME a figi-gii:PricingSource .

figi-ps:HSTS a figi-gii:PricingSource .

figi-ps:ARME skos:prefLabel "armenia se" .

figi-ps:BRAT a figi-gii:PricingSource .

figi-ps:HSTS skos:prefLabel "hsbc securities-usa" .

figi-ps:ARME figi-gii:hasUniqueTextIdentifier "ARME" .

figi-ps:BRAT skos:prefLabel "bratislava stock ex" .

figi-ps:HSTS figi-gii:hasUniqueTextIdentifier "HSTS" .

figi-st:muniSwap a owl:NamedIndividual .

figi-ps:BRAT figi-gii:hasUniqueTextIdentifier "BRAT" .

figi-st:muniSwap a figi-gii:SecurityType .

figi-ps:HSTT a owl:NamedIndividual .

figi-ps:BRAV a owl:NamedIndividual .

figi-ps:HSTT a figi-gii:PricingSource .

figi-st:muniSwap skos:definition "A Municipal Swap is a swap that exchanges a municipal bond index with a funding leg" .

figi-ps:BRAV a figi-gii:PricingSource .

figi-ps:HSTT skos:prefLabel "hstt mop testing" .

figi-st:muniSwap skos:prefLabel "muni swap" .

figi-ps:BRAV skos:prefLabel "braver, stern, and co." .

figi-ps:HSTT figi-gii:hasUniqueTextIdentifier "HSTT" .

figi-ps:BRAV figi-gii:hasUniqueTextIdentifier "BRAV" .

figi-ps:HSTW a owl:NamedIndividual .

figi-ps:BRAZ a owl:NamedIndividual .

figi-ps:HSTW a figi-gii:PricingSource .

figi-ps:BRAZ a figi-gii:PricingSource .

figi-ps:HSTW skos:prefLabel "hsbc taiwan" .

figi-ps:BRAZ skos:prefLabel "abn amro inc" .

figi-ps:HSTW figi-gii:hasUniqueTextIdentifier "HSTW" .

figi-ps:BRAZ figi-gii:hasUniqueTextIdentifier "BRAZ" .

figi-ps:HSUY a owl:NamedIndividual .

figi-ps:BRBI a owl:NamedIndividual .

figi-st:muniSwap figi-gii:hasUniqueTextIdentifier "MUNI SWAP" .

figi-ps:HSUY a figi-gii:PricingSource .

figi-ps:BRBI a figi-gii:PricingSource .

figi-st:murabaha a owl:NamedIndividual .

figi-ps:BRBI skos:prefLabel "bbi" .

figi-st:murabaha a figi-gii:SecurityType .

figi-ps:HSUY skos:prefLabel "hsbc uruguay sa" .

figi-ps:BRBI figi-gii:hasUniqueTextIdentifier "BRBI" .

figi-ps:BRCA a owl:NamedIndividual , figi-gii:PricingSource .

figi-st:murabaha skos:definition "An Islamic financing structure, where an intermediary buys a property with free and clear title to it. The intermediary and prospective buyer then agree upon a sale price (including an agreed upon profit for the intermediary) that can be made through a series of installments, or as a lump sum payment." .

figi-ps:BRCA skos:prefLabel "barclays cap dev" .

figi-st:murabaha skos:prefLabel "murabaha" .

figi-ps:BRCA figi-gii:hasUniqueTextIdentifier "BRCA" .

figi-st:murabaha figi-gii:hasUniqueTextIdentifier "MURABAHA" .

figi-ps:HSUY figi-gii:hasUniqueTextIdentifier "HSUY" .

figi-ps:BRCN a owl:NamedIndividual .

figi-ps:ARQM a owl:NamedIndividual .

figi-ps:BRCN a figi-gii:PricingSource .

figi-ps:ARQM a figi-gii:PricingSource .

figi-ps:HTAS a owl:NamedIndividual .

figi-ps:BRCN skos:prefLabel "banco brascan" .

figi-ps:HTAS a figi-gii:PricingSource .

figi-ps:ARQM skos:prefLabel "arqaam capital" .

figi-ps:BRCN figi-gii:hasUniqueTextIdentifier "BRCN" .

figi-ps:HTAS skos:prefLabel "bmoc-bmo capital" .

figi-ps:ARQM figi-gii:hasUniqueTextIdentifier "ARQM" .

figi-ps:BRDB a owl:NamedIndividual .

figi-ps:HTAS figi-gii:hasUniqueTextIdentifier "HTAS" .

figi-st:mutualFund a owl:NamedIndividual .

figi-ps:BRDB a figi-gii:PricingSource .

figi-ps:HTSC a owl:NamedIndividual .

figi-st:mutualFund a figi-gii:SecurityType .

figi-ps:BRDB skos:prefLabel "bridge co uat" .

figi-ps:HTSC a figi-gii:PricingSource .

figi-ps:BRDB figi-gii:hasUniqueTextIdentifier "BRDB" .

figi-ps:HTSC skos:prefLabel "hua tai securities" .

figi-ps:BRDE a owl:NamedIndividual .

figi-ps:HTSC figi-gii:hasUniqueTextIdentifier "HTSC" .

figi-ps:BRDE a figi-gii:PricingSource .

figi-st:mutualFund skos:definition "Mutual Fund. An investment company that pools individual, institutional and other investors' money and invests it in a variety of securities or markets. Shares can be redeemed at Net Asset Value (NAV). The funds offer investors diversification and professional management for a yearly management fee." .

figi-ps:BRDE skos:prefLabel "brd romania" .

figi-ps:HUM a owl:NamedIndividual .

figi-st:mutualFund skos:prefLabel "mutual fund" .

figi-ps:BRDE figi-gii:hasUniqueTextIdentifier "BRDE" .

figi-ps:HUM a figi-gii:PricingSource .

figi-st:mutualFund figi-gii:hasUniqueTextIdentifier "Mutual Fund" .

figi-ps:BRDY a owl:NamedIndividual .

figi-ps:HUM skos:prefLabel "humana, inc" .

figi-ps:BRDY a figi-gii:PricingSource .

figi-ps:ART a owl:NamedIndividual .

figi-ps:HUM figi-gii:hasUniqueTextIdentifier "HUM" .

figi-ps:ART a figi-gii:PricingSource .

figi-ps:BRDY skos:prefLabel "brandywine asset mgt" .

figi-ps:HUNE a owl:NamedIndividual .

figi-ps:ART skos:prefLabel "artefact partners" .

figi-ps:HUNE a figi-gii:PricingSource .

figi-ps:ART figi-gii:hasUniqueTextIdentifier "ART" .

figi-ps:BRDY figi-gii:hasUniqueTextIdentifier "BRDY" .

figi-ps:HUNE skos:prefLabel "hungaria ertekpapir" .

figi-st:mv a owl:NamedIndividual .

figi-ps:BRE a owl:NamedIndividual .

figi-ps:HUNE figi-gii:hasUniqueTextIdentifier "HUNE" .

figi-ps:BRE a figi-gii:PricingSource .

figi-st:mv a figi-gii:SecurityType .

figi-ps:HUNT a owl:NamedIndividual .

figi-ps:BRE skos:prefLabel "bre bank" .

figi-ps:HUNT a figi-gii:PricingSource .

figi-st:mv skos:definition "Market Value (Only for CDO,CLO,CBO securities)" .

figi-ps:BRE figi-gii:hasUniqueTextIdentifier "BRE" .

figi-ps:HUNT skos:prefLabel "huntington invt co" .

figi-st:mv skos:prefLabel "mv" .

figi-ps:BREA a owl:NamedIndividual .

figi-ps:HUNT figi-gii:hasUniqueTextIdentifier "HUNT" .

figi-ps:BREA a figi-gii:PricingSource .

figi-st:mv figi-gii:hasUniqueTextIdentifier "MV" .

figi-ps:HVB a owl:NamedIndividual .

figi-ps:BREA skos:prefLabel "brean capital" .

figi-ps:HVB a figi-gii:PricingSource .

figi-st:mxCertBursatil a owl:NamedIndividual .

figi-ps:BREA figi-gii:hasUniqueTextIdentifier "BREA" .

figi-ps:HVB skos:prefLabel "hvb munich" .

figi-st:mxCertBursatil a figi-gii:SecurityType .

figi-ps:BREB a owl:NamedIndividual .

figi-ps:HVB figi-gii:hasUniqueTextIdentifier "HVB" .

figi-ps:BREB a figi-gii:PricingSource .

figi-st:mxCertBursatil skos:definition "Short term Mexican Mmkt instrument" .

figi-ps:HVBB a owl:NamedIndividual .

figi-ps:BREB skos:prefLabel "bre bank internal" .

figi-st:mxCertBursatil skos:prefLabel "mx cert bursatil" .

figi-ps:HVBB a figi-gii:PricingSource .

figi-ps:BREB figi-gii:hasUniqueTextIdentifier "BREB" .

figi-st:mxCertBursatil figi-gii:hasUniqueTextIdentifier "MX CERT BURSATIL" .

figi-ps:HVBB skos:prefLabel "hvb bk serbia and mont" .

figi-ps:BREN a owl:NamedIndividual .

figi-ps:ARTC a owl:NamedIndividual .

figi-ps:BREN a figi-gii:PricingSource .

figi-ps:HVBB figi-gii:hasUniqueTextIdentifier "HVBB" .

figi-ps:ARTC a figi-gii:PricingSource .

figi-ps:BREN skos:prefLabel "grupo brennand" .

figi-ps:HVBC a owl:NamedIndividual .

figi-ps:ARTC skos:prefLabel "artcapital" .

figi-ps:HVBC a figi-gii:PricingSource .

figi-ps:BREN figi-gii:hasUniqueTextIdentifier "BREN" .

figi-ps:ARTC figi-gii:hasUniqueTextIdentifier "ARTC" .

figi-ps:HVBC skos:prefLabel "hvb czech republic" .

figi-ps:BRID a owl:NamedIndividual .

figi-st:na a owl:NamedIndividual .

figi-ps:HVBC figi-gii:hasUniqueTextIdentifier "HVBC" .

figi-st:na a figi-gii:SecurityType .

figi-ps:BRID a figi-gii:PricingSource .

figi-ps:HVBI a owl:NamedIndividual .

figi-st:na skos:definition "Not used" .

figi-ps:BRID skos:prefLabel "bridport" .

figi-ps:HVBI a figi-gii:PricingSource .

figi-st:na skos:prefLabel "n.a." .

figi-ps:BRID figi-gii:hasUniqueTextIdentifier "BRID" .

figi-ps:HVBI skos:prefLabel "hvb munich internal" .

figi-st:na figi-gii:hasUniqueTextIdentifier "N.A." .

figi-ps:BRIJ a owl:NamedIndividual .

figi-ps:HVBI figi-gii:hasUniqueTextIdentifier "HVBI" .

figi-ps:BRIJ a figi-gii:PricingSource .

figi-ps:ARTE a owl:NamedIndividual .

figi-ps:HVBS a owl:NamedIndividual .

figi-ps:BRIJ skos:prefLabel "bank rakyat indo" .

figi-ps:ARTE a figi-gii:PricingSource .

figi-ps:HVBS a figi-gii:PricingSource .

figi-ps:BRIJ figi-gii:hasUniqueTextIdentifier "BRIJ" .

figi-ps:ARTE skos:prefLabel "artesia bk corp" .

figi-ps:HVBS skos:prefLabel "hvb bank slovakia as" .

figi-ps:BRIO a owl:NamedIndividual .

figi-ps:ARTE figi-gii:hasUniqueTextIdentifier "ARTE" .

figi-ps:HVBS figi-gii:hasUniqueTextIdentifier "HVBS" .

figi-ps:BRIO a figi-gii:PricingSource .

figi-st:ndfFixing a owl:NamedIndividual .

figi-ps:HVBT a owl:NamedIndividual .

figi-ps:BRIO skos:prefLabel "banco rio de la plat" .

figi-ps:HVBT a figi-gii:PricingSource .

figi-ps:BRIO figi-gii:hasUniqueTextIdentifier "BRIO" .

figi-ps:HVBT skos:prefLabel "hvb etrade" .

figi-ps:BRIV a owl:NamedIndividual .

figi-ps:HVBT figi-gii:hasUniqueTextIdentifier "HVBT" .

figi-ps:BRIV a figi-gii:PricingSource .

figi-st:ndfFixing a figi-gii:SecurityType .

figi-ps:HVBU a owl:NamedIndividual .

figi-ps:BRIV skos:prefLabel "black river am, uk" .

figi-ps:HVBU a figi-gii:PricingSource .

figi-st:ndfFixing skos:definition "The settlement rate for an NDF" .

figi-ps:BRIV figi-gii:hasUniqueTextIdentifier "BRIV" .

figi-ps:HVBU skos:prefLabel "hvb bank" .

figi-st:ndfFixing skos:prefLabel "ndf fixing" .

figi-ps:BRLA a owl:NamedIndividual .

figi-ps:HVBU figi-gii:hasUniqueTextIdentifier "HVBU" .

figi-ps:BRLA a figi-gii:PricingSource .

figi-st:ndfFixing figi-gii:hasUniqueTextIdentifier "NDF FIXING" .

figi-ps:HVCT a owl:NamedIndividual .

figi-ps:BRLA skos:prefLabel "bremer landesbank" .

figi-ps:HVCT a figi-gii:PricingSource .

figi-st:ndfSwap a owl:NamedIndividual .

figi-ps:BRLA figi-gii:hasUniqueTextIdentifier "BRLA" .

figi-ps:HVCT skos:prefLabel "hvb london" .

figi-st:ndfSwap a figi-gii:SecurityType .

figi-ps:BRLN a owl:NamedIndividual .

figi-ps:HVCT figi-gii:hasUniqueTextIdentifier "HVCT" .

figi-ps:BRLN a figi-gii:PricingSource .

figi-ps:HVSG a owl:NamedIndividual .

figi-ps:BRLN skos:prefLabel "berlin exchange" .

figi-ps:HVSG a figi-gii:PricingSource .

figi-ps:BRLN figi-gii:hasUniqueTextIdentifier "BRLN" .

figi-ps:HVSG skos:prefLabel "hvb singapore" .

figi-ps:BRMN a owl:NamedIndividual .

figi-ps:HVSG figi-gii:hasUniqueTextIdentifier "HVSG" .

figi-ps:BRMN a figi-gii:PricingSource ;
	skos:prefLabel "bremen exchange" .

figi-ps:HWLY a owl:NamedIndividual .

figi-ps:BRMN figi-gii:hasUniqueTextIdentifier "BRMN" .

figi-ps:HWLY a figi-gii:PricingSource .

figi-st:ndfSwap skos:definition "A swap that is similar to a non-deliverable forward, with the only difference being that settlement for both parties is done through a major currency. Non-deliverable swaps are used when the swap includes a major currency, such as the U.S. dollar, and a restricted currency, such as the Philippine peso or South Korean won." .

figi-ps:BRNP a owl:NamedIndividual .

figi-ps:HWLY skos:prefLabel "hotchkis and wiley cap" .

figi-st:ndfSwap skos:prefLabel "ndf swap" .

figi-ps:BRNP a figi-gii:PricingSource .

figi-ps:HWLY figi-gii:hasUniqueTextIdentifier "HWLY" .

figi-st:ndfSwap figi-gii:hasUniqueTextIdentifier "NDF SWAP" .

figi-ps:BRNP skos:prefLabel "bnp paribas brazil" .

figi-ps:ARTI a owl:NamedIndividual .

figi-ps:BRNP figi-gii:hasUniqueTextIdentifier "BRNP" .

figi-ps:ARTI a figi-gii:PricingSource .

figi-ps:BROS a owl:NamedIndividual .

figi-ps:ARTI skos:prefLabel "arta investments" .

figi-ps:BROS a figi-gii:PricingSource .

figi-ps:ARTI figi-gii:hasUniqueTextIdentifier "ARTI" .

figi-ps:BROS skos:prefLabel "bank rossiya" .

figi-st:negInstDeposit a owl:NamedIndividual .

figi-ps:BROS figi-gii:hasUniqueTextIdentifier "BROS" .

figi-st:negInstDeposit a figi-gii:SecurityType .

figi-ps:BRSE a owl:NamedIndividual , figi-gii:PricingSource .

figi-st:negInstDeposit skos:definition "Negotiable Institutional Deposit" .

figi-ps:HXBJ a owl:NamedIndividual .

figi-st:negInstDeposit skos:prefLabel "neg inst deposit" .

figi-ps:BRSE skos:prefLabel "bradesco securities" .

figi-ps:HXBJ a figi-gii:PricingSource .

figi-st:negInstDeposit figi-gii:hasUniqueTextIdentifier "NEG INST DEPOSIT" .

figi-ps:BRSE figi-gii:hasUniqueTextIdentifier "BRSE" .

figi-ps:HXBJ skos:prefLabel "hua xia bank" .

figi-ps:ARTU a owl:NamedIndividual .

figi-ps:BRSV a owl:NamedIndividual .

figi-ps:HXBJ figi-gii:hasUniqueTextIdentifier "HXBJ" .

figi-ps:ARTU a figi-gii:PricingSource .

figi-ps:BRSV a figi-gii:PricingSource .

figi-ps:HXBK a owl:NamedIndividual .

figi-ps:ARTU skos:prefLabel "astrum im" .

figi-ps:BRSV skos:prefLabel "banreservas" .

figi-ps:HXBK a figi-gii:PricingSource .

figi-ps:ARTU figi-gii:hasUniqueTextIdentifier "ARTU" .

figi-ps:BRSV figi-gii:hasUniqueTextIdentifier "BRSV" .

figi-ps:HXBK skos:prefLabel "hua xia bank" .

figi-st:negotiableCD a owl:NamedIndividual .

figi-ps:BRTP a owl:NamedIndividual .

figi-ps:HXBK figi-gii:hasUniqueTextIdentifier "HXBK" .

figi-st:negotiableCD a figi-gii:SecurityType .

figi-ps:BRTP a figi-gii:PricingSource ;
	skos:prefLabel "beirut se - pfd" ;
	figi-gii:hasUniqueTextIdentifier "BRTP" .

figi-st:negotiableCD skos:definition "Negotiable Certificate of Deposit. A negotiable money market instrument that trades on the open market with high returns and low risks. These instruments are typically large-dollar denominated and are held by large institutional investors. Alsoknown as jumbo CD's" .

figi-ps:BRTZ a owl:NamedIndividual .

figi-st:negotiableCD skos:prefLabel "negotiable cd" .

figi-ps:BRTZ a figi-gii:PricingSource .

figi-st:negotiableCD figi-gii:hasUniqueTextIdentifier "NEGOTIABLE CD" .

figi-ps:BRTZ skos:prefLabel "barz tanzania" .

figi-st:newZealandCP a owl:NamedIndividual .

figi-ps:BRTZ figi-gii:hasUniqueTextIdentifier "BRTZ" .

figi-st:newZealandCP a figi-gii:SecurityType .

figi-ps:BRWN a owl:NamedIndividual .

figi-st:newZealandCP skos:definition "New Zealand Commercial Paper" .

figi-ps:HYBA a owl:NamedIndividual .

figi-ps:BRWN a figi-gii:PricingSource .

figi-st:newZealandCP skos:prefLabel "new zealand cp" .

figi-ps:HYBA a figi-gii:PricingSource .

figi-ps:BRWN skos:prefLabel "brownstone invt grp" .

figi-st:newZealandCP figi-gii:hasUniqueTextIdentifier "NEW ZEALAND CP" .

figi-ps:HYBA skos:prefLabel "banc of america secs" .

figi-ps:BRWN figi-gii:hasUniqueTextIdentifier "BRWN" .

figi-ps:ASB a owl:NamedIndividual .

figi-ps:HYBA figi-gii:hasUniqueTextIdentifier "HYBA" .

figi-ps:ASB a figi-gii:PricingSource .

figi-ps:BS a owl:NamedIndividual .

figi-ps:HYBB a owl:NamedIndividual .

figi-ps:BS a figi-gii:PricingSource .

figi-ps:ASB skos:prefLabel "asb capital mgmt" .

figi-ps:HYBB a figi-gii:PricingSource .

figi-ps:BS skos:prefLabel "bear stearns ny" .

figi-ps:ASB figi-gii:hasUniqueTextIdentifier "ASB" .

figi-ps:HYBB skos:prefLabel "hypo bank burgenland" .

figi-ps:BS figi-gii:hasUniqueTextIdentifier "BS" .

figi-st:nonDeliverableForward a owl:NamedIndividual .

figi-ps:HYBB figi-gii:hasUniqueTextIdentifier "HYBB" .

figi-st:nonDeliverableForward a figi-gii:SecurityType .

figi-ps:BSAB a owl:NamedIndividual .

figi-ps:HYPO a owl:NamedIndividual .

figi-ps:BSAB a figi-gii:PricingSource .

figi-ps:HYPO a figi-gii:PricingSource .

figi-ps:BSAB skos:prefLabel "banco sabadell" .

figi-ps:HYPO skos:prefLabel "hypo capital mgmt" .

figi-ps:BSAB figi-gii:hasUniqueTextIdentifier "BSAB" .

figi-ps:HYPO figi-gii:hasUniqueTextIdentifier "HYPO" .

figi-st:nonDeliverableForward skos:definition "Non-deliverable forwards are a type of cash settled financial derivative. In the foreign exchange market, traders and investors will enter into an outright forward or futures contract where counterparties agree to settle based upon the difference between a strike price and the prevailing spot rate for a specified notional amount on a defined fixing date in the future." .

figi-ps:BSAC a owl:NamedIndividual .

figi-ps:HYPZ a owl:NamedIndividual .

figi-ps:BSAC a figi-gii:PricingSource .

figi-st:nonDeliverableForward skos:prefLabel "non-deliverable forward" .

figi-ps:HYPZ a figi-gii:PricingSource .

figi-ps:BSAC skos:prefLabel "banco santander-sant" .

figi-st:nonDeliverableForward figi-gii:hasUniqueTextIdentifier "NON-DELIVERABLE FORWARD" .

figi-ps:HYPZ skos:prefLabel "hyposwiss" .

figi-ps:BSAC figi-gii:hasUniqueTextIdentifier "BSAC" .

figi-ps:ASBA a owl:NamedIndividual .

figi-ps:HYPZ figi-gii:hasUniqueTextIdentifier "HYPZ" .

figi-ps:ASBA a figi-gii:PricingSource .

figi-ps:BSAN a owl:NamedIndividual .

figi-ps:HZCC a owl:NamedIndividual .

figi-ps:ASBA skos:prefLabel "asb bank limited" .

figi-ps:BSAN a figi-gii:PricingSource .

figi-ps:HZCC a figi-gii:PricingSource .

figi-ps:ASBA figi-gii:hasUniqueTextIdentifier "ASBA" .

figi-ps:BSAN skos:prefLabel "bco santander madrid" .

figi-ps:HZCC skos:prefLabel "cfet bk of hangzhou" .

figi-st:nonDeliverableIrsSwap a owl:NamedIndividual .

figi-ps:BSAN figi-gii:hasUniqueTextIdentifier "BSAN" .

figi-st:nonDeliverableIrsSwap a figi-gii:SecurityType .

figi-ps:HZCC figi-gii:hasUniqueTextIdentifier "HZCC" .

figi-ps:BSBG a owl:NamedIndividual , figi-gii:PricingSource .

figi-st:nonDeliverableIrsSwap skos:definition "Denominated in a currency on a non-deliverable basis, but settled in another currency that is deliverable" .

figi-ps:BSBG skos:prefLabel "basisbank" .

figi-ps:IAAC a owl:NamedIndividual .

figi-st:nonDeliverableIrsSwap skos:prefLabel "non-deliverable irs swap" .

figi-ps:BSBG figi-gii:hasUniqueTextIdentifier "BSBG" .

figi-ps:IAAC a figi-gii:PricingSource .

figi-st:nonDeliverableIrsSwap figi-gii:hasUniqueTextIdentifier "NON-DELIVERABLE IRS SWAP" .

figi-ps:BSBL a owl:NamedIndividual .

figi-ps:IAAC skos:prefLabel "intl assets advisory" .

figi-ps:BSBL a figi-gii:PricingSource .

figi-st:nonDeliverableOisSwap a owl:NamedIndividual .

figi-ps:IAAC figi-gii:hasUniqueTextIdentifier "IAAC" .

figi-st:nonDeliverableOisSwap a figi-gii:SecurityType .

figi-ps:BSBL skos:prefLabel "banco de sabadell" .

figi-ps:IAMG a owl:NamedIndividual , figi-gii:PricingSource .

figi-ps:BSBL figi-gii:hasUniqueTextIdentifier "BSBL" .

figi-st:nonDeliverableOisSwap skos:definition "Similar to an NDIRS, it is denominated in a currency on a non-deliverable basis, but settled in another currency that is deliverable however the index used on the floating leg is an Overnight Index" .

figi-ps:IAMG skos:prefLabel "intercontiental" .

figi-ps:BSBO a owl:NamedIndividual .

figi-st:nonDeliverableOisSwap skos:prefLabel "non-deliverable ois swap" .

figi-ps:BSBO a figi-gii:PricingSource .

figi-ps:IAMG figi-gii:hasUniqueTextIdentifier "IAMG" .

figi-st:nonDeliverableOisSwap figi-gii:hasUniqueTextIdentifier "NON-DELIVERABLE OIS SWAP" .

figi-ps:BSBO skos:prefLabel "banco santndr bogota" .

figi-ps:IAPD a owl:NamedIndividual .

figi-ps:ASBB a owl:NamedIndividual .

figi-ps:BSBO figi-gii:hasUniqueTextIdentifier "BSBO" .

figi-ps:IAPD a figi-gii:PricingSource .

figi-ps:ASBB a figi-gii:PricingSource .

figi-ps:IAPD skos:prefLabel "icap" .

figi-ps:BSBP a owl:NamedIndividual .

figi-ps:ASBB skos:prefLabel "al salam bank" .

figi-ps:BSBP a figi-gii:PricingSource .

figi-ps:IAPD figi-gii:hasUniqueTextIdentifier "IAPD" .

figi-ps:ASBB figi-gii:hasUniqueTextIdentifier "ASBB" .

figi-ps:BSBP skos:prefLabel "bnp paribas sg" .

figi-ps:IAPS a owl:NamedIndividual .

figi-st:nonEquityIndex a owl:NamedIndividual .

figi-ps:BSBP figi-gii:hasUniqueTextIdentifier "BSBP" .

figi-ps:IAPS a figi-gii:PricingSource .

figi-st:nonEquityIndex a figi-gii:SecurityType .

figi-ps:BSBR a owl:NamedIndividual .

figi-ps:IAPS skos:prefLabel "intercapital icap" .

figi-ps:BSBR a figi-gii:PricingSource .

figi-st:nonEquityIndex skos:definition "A basket of contracts whose underlying securities are instruments other than equities." .

figi-ps:IAPS figi-gii:hasUniqueTextIdentifier "IAPS" .

figi-ps:BSBR skos:prefLabel "british saudi bank" .

figi-st:nonEquityIndex skos:prefLabel "non-equity index" .

figi-ps:IBCA a owl:NamedIndividual .

figi-ps:BSBR figi-gii:hasUniqueTextIdentifier "BSBR" .

figi-ps:IBCA a figi-gii:PricingSource .

figi-st:nonEquityIndex figi-gii:hasUniqueTextIdentifier "Non-Equity Index" .

figi-ps:BSC a owl:NamedIndividual .

figi-ps:IBCA skos:prefLabel "interbono" .

figi-ps:BSC a figi-gii:PricingSource .

figi-ps:ASE a owl:NamedIndividual .

figi-ps:IBCA figi-gii:hasUniqueTextIdentifier "IBCA" .

figi-ps:ASE a figi-gii:PricingSource .

figi-ps:BSC skos:prefLabel "bear stearns n y" .

figi-ps:IBCC a owl:NamedIndividual .

figi-ps:ASE skos:prefLabel "athens stock exch" .

figi-ps:IBCC a figi-gii:PricingSource .

figi-ps:BSC figi-gii:hasUniqueTextIdentifier "BSC" .

figi-ps:ASE figi-gii:hasUniqueTextIdentifier "ASE" .

figi-ps:IBCC skos:prefLabel "iccrea banca" .

figi-ps:BSCB a owl:NamedIndividual .

figi-st:norwegianCD a owl:NamedIndividual .

figi-ps:IBCC figi-gii:hasUniqueTextIdentifier "IBCC" .

figi-st:norwegianCD a figi-gii:SecurityType .

figi-ps:IBCE a owl:NamedIndividual .

figi-ps:BSCB a figi-gii:PricingSource .

figi-st:norwegianCD skos:definition "Norwegian Certificates of Deposit" .

figi-ps:IBCE a figi-gii:PricingSource .

figi-ps:BSCB skos:prefLabel "bear stearns" .

figi-st:norwegianCD skos:prefLabel "norwegian cd" .

figi-ps:IBCE skos:prefLabel "ib corp investment" .

figi-ps:BSCB figi-gii:hasUniqueTextIdentifier "BSCB" .

figi-st:norwegianCD figi-gii:hasUniqueTextIdentifier "NORWEGIAN CD" .

figi-ps:IBCE figi-gii:hasUniqueTextIdentifier "IBCE" .

figi-ps:BSCE a owl:NamedIndividual .

figi-st:nvdr a owl:NamedIndividual .

figi-ps:IBCO a owl:NamedIndividual .

figi-st:nvdr a figi-gii:SecurityType .

figi-ps:IBCO a figi-gii:PricingSource .

figi-st:nvdr skos:definition "Thailand Non Voting Depositary Receipt." .

figi-ps:IBCO skos:prefLabel "interactive brokers" .

figi-st:nvdr skos:prefLabel "nvdr" .

figi-ps:IBCO figi-gii:hasUniqueTextIdentifier "IBCO" .

figi-st:nvdr figi-gii:hasUniqueTextIdentifier "NVDR" .

figi-ps:IBER a owl:NamedIndividual .

figi-ps:ASEC a owl:NamedIndividual .

figi-ps:IBER a figi-gii:PricingSource .

figi-ps:BSCE a figi-gii:PricingSource .

figi-ps:ASEC a figi-gii:PricingSource .

figi-ps:IBER skos:prefLabel "ibercaja gestion sg" .

figi-ps:BSCE skos:prefLabel "bear stearns eur cvt" .

figi-ps:ASEC skos:prefLabel "arctic securities" .

figi-ps:IBER figi-gii:hasUniqueTextIdentifier "IBER" .

figi-ps:BSCE figi-gii:hasUniqueTextIdentifier "BSCE" .

figi-ps:ASEC figi-gii:hasUniqueTextIdentifier "ASEC" .

figi-ps:IBFC a owl:NamedIndividual .

figi-ps:BSCH a owl:NamedIndividual .

figi-st:nyRegShrs a owl:NamedIndividual .

figi-ps:IBFC a figi-gii:PricingSource .

figi-ps:BSCH a figi-gii:PricingSource .

figi-st:nyRegShrs a figi-gii:SecurityType .

figi-ps:IBFC skos:prefLabel "int'l bills finance" .

figi-ps:BSCH skos:prefLabel "santander" .

figi-ps:IBFC figi-gii:hasUniqueTextIdentifier "IBFC" .

figi-st:nyRegShrs skos:definition "New York Registered Shares. A foreign company's shares that are registered through their home office in New York." .

figi-ps:BSCH figi-gii:hasUniqueTextIdentifier "BSCH" .

figi-ps:IBGN a owl:NamedIndividual .

figi-st:nyRegShrs skos:prefLabel "ny reg shrs" .

figi-ps:IBGN a figi-gii:PricingSource .

figi-ps:BSCM a owl:NamedIndividual .

figi-st:nyRegShrs figi-gii:hasUniqueTextIdentifier "NY Reg Shrs" .

figi-ps:BSCM a figi-gii:PricingSource .

figi-ps:IBGN skos:prefLabel "bloomberg generic" .

figi-st:oid a owl:NamedIndividual .

figi-ps:BSCM skos:prefLabel "santander" .

figi-st:oid a figi-gii:SecurityType .

figi-ps:BSCM figi-gii:hasUniqueTextIdentifier "BSCM" .

figi-ps:BSCO a owl:NamedIndividual , figi-gii:PricingSource ;
	skos:prefLabel "bear stearns" .

figi-st:oid skos:definition "Original Issue Discount (OID). A bond with its par value discounted at the time it is issued. The difference between the purchase price and the adjusted price is considered income in addition to any interest that may be paid. If held to maturity, no capital gains tax will be paid since the gain is considered interest." .

figi-ps:IBGN figi-gii:hasUniqueTextIdentifier "IBGN" .

figi-ps:BSCO figi-gii:hasUniqueTextIdentifier "BSCO" .

figi-st:oid skos:prefLabel "oid" .

figi-ps:IBII a owl:NamedIndividual .

figi-ps:BSCR a owl:NamedIndividual .

figi-st:oid figi-gii:hasUniqueTextIdentifier "OID" .

figi-ps:BSCR a figi-gii:PricingSource .

figi-ps:IBII a figi-gii:PricingSource .

figi-ps:ASEK a owl:NamedIndividual .

figi-ps:BSCR skos:prefLabel "bear stearns 144a" .

figi-ps:IBII skos:prefLabel "ibi group" .

figi-ps:ASEK a figi-gii:PricingSource .

figi-ps:BSCR figi-gii:hasUniqueTextIdentifier "BSCR" .

figi-ps:IBII figi-gii:hasUniqueTextIdentifier "IBII" .

figi-ps:ASEK skos:prefLabel "aaa securitas" .

figi-ps:BSCT a owl:NamedIndividual .

figi-ps:IBKR a owl:NamedIndividual .

figi-ps:ASEK figi-gii:hasUniqueTextIdentifier "ASEK" .

figi-ps:BSCT a figi-gii:PricingSource .

figi-ps:IBKR a figi-gii:PricingSource .

figi-st:onshoreForward a owl:NamedIndividual .

figi-ps:BSCT skos:prefLabel "barclays cap" .

figi-ps:IBKR skos:prefLabel "interactive brokers" .

figi-st:onshoreForward a figi-gii:SecurityType .

figi-ps:IBKR figi-gii:hasUniqueTextIdentifier "IBKR" .

figi-ps:BSCT skos:prefLabel "barclays cap." .

figi-ps:IBL a owl:NamedIndividual .

figi-ps:BSCT figi-gii:hasUniqueTextIdentifier "BSCT" .

figi-ps:IBL a figi-gii:PricingSource ;
	skos:prefLabel "indusind bank" .

figi-ps:BSCX a owl:NamedIndividual .

figi-st:onshoreForward skos:definition "Onshore forward foreign exchange transactions occur in controlled domestic markets and involve the purchase of a specified amount of one currency and selling of another on an agreed future date. Onshore forward rates are not necessarily determined by an arbitrage free relationship between the interest rates of the two currencies and the current spot rate." .

figi-ps:BSCX a figi-gii:PricingSource .

figi-st:onshoreForward skos:prefLabel "onshore forward" .

figi-ps:BSCX skos:prefLabel "grupo santander" .

figi-st:onshoreForward figi-gii:hasUniqueTextIdentifier "ONSHORE FORWARD" .

figi-ps:BSCX figi-gii:hasUniqueTextIdentifier "BSCX" .

figi-ps:ASG a owl:NamedIndividual .

figi-ps:BSE a owl:NamedIndividual .

figi-ps:IBL figi-gii:hasUniqueTextIdentifier "IBL" .

figi-ps:ASG a figi-gii:PricingSource .

figi-ps:BSE a figi-gii:PricingSource .

figi-ps:IBNM a owl:NamedIndividual .

figi-ps:ASG skos:prefLabel "amherst" .

figi-ps:BSE skos:prefLabel "bombay stock exch" .

figi-ps:IBNM a figi-gii:PricingSource .

figi-ps:ASG figi-gii:hasUniqueTextIdentifier "ASG" .

figi-ps:BSE figi-gii:hasUniqueTextIdentifier "BSE" .

figi-ps:IBNM skos:prefLabel "int exch bank manila" .

figi-st:onshoreSwap a owl:NamedIndividual .

figi-ps:BSEP a owl:NamedIndividual .

figi-st:onshoreSwap a figi-gii:SecurityType .

figi-ps:BSEP a figi-gii:PricingSource .

figi-ps:IBNM figi-gii:hasUniqueTextIdentifier "IBNM" .

figi-ps:BSEP skos:prefLabel "bear stearns eq" .

figi-st:onshoreSwap skos:definition "The Swap can only be traded in the local currency in the local market (ex: KRW onshore swaps)" .

figi-ps:BSEP figi-gii:hasUniqueTextIdentifier "BSEP" .

figi-ps:IBPA a owl:NamedIndividual .

figi-st:onshoreSwap skos:prefLabel "onshore swap" .

figi-ps:IBPA a figi-gii:PricingSource .

figi-ps:BSEY a owl:NamedIndividual .

figi-st:onshoreSwap figi-gii:hasUniqueTextIdentifier "ONSHORE SWAP" .

figi-ps:IBPA skos:prefLabel "ibpa (price)" .

figi-ps:BSEY a figi-gii:PricingSource .

figi-ps:ASGL a owl:NamedIndividual .

figi-ps:IBPA figi-gii:hasUniqueTextIdentifier "IBPA" .

figi-ps:ASGL a figi-gii:PricingSource .

figi-ps:BSEY skos:prefLabel "bse yield" .

figi-ps:IBTG a owl:NamedIndividual .

figi-ps:ASGL skos:prefLabel "amherst securities" .

figi-ps:IBTG a figi-gii:PricingSource .

figi-ps:BSEY figi-gii:hasUniqueTextIdentifier "BSEY" .

figi-ps:ASGL figi-gii:hasUniqueTextIdentifier "ASGL" .

figi-ps:IBTG skos:prefLabel "investbank" .

figi-ps:BSEZ a owl:NamedIndividual .

figi-st:openEndFund a owl:NamedIndividual .

figi-ps:IBTG figi-gii:hasUniqueTextIdentifier "IBTG" .

figi-ps:BSEZ a figi-gii:PricingSource .

figi-st:openEndFund a figi-gii:SecurityType .

figi-ps:ICAB a owl:NamedIndividual .

figi-ps:BSEZ skos:prefLabel "bombay stock exch" .

figi-ps:ICAB a figi-gii:PricingSource .

figi-st:openEndFund skos:definition "A fund that allows investors to buy and sell stock in it on an on-going basis since it has unlimited shares. It continuously issues and redeems shares so the number of shares issued and outstanding varies from day to day." .

figi-ps:ICAB skos:prefLabel "icap london" .

figi-ps:BSEZ figi-gii:hasUniqueTextIdentifier "BSEZ" .

figi-st:openEndFund skos:prefLabel "open-end fund" .

figi-ps:ICAB figi-gii:hasUniqueTextIdentifier "ICAB" .

figi-ps:BSFP a owl:NamedIndividual .

figi-st:openEndFund figi-gii:hasUniqueTextIdentifier "Open-End Fund" .

figi-ps:BSFP a figi-gii:PricingSource .

figi-ps:ICAG a owl:NamedIndividual .

figi-st:option a owl:NamedIndividual .

figi-ps:ICAG a figi-gii:PricingSource .

figi-ps:BSFP skos:prefLabel "bear stearns intl" .

figi-st:option a figi-gii:SecurityType .

figi-ps:ICAG skos:prefLabel "icap poland" .

figi-ps:BSFP figi-gii:hasUniqueTextIdentifier "BSFP" .

figi-ps:ICAG figi-gii:hasUniqueTextIdentifier "ICAG" .

figi-ps:BSFR a owl:NamedIndividual .

figi-ps:ICAK a owl:NamedIndividual .

figi-st:option skos:definition "A contract that provides the right, but not the obligation, to buy or sell a specific amount of a specific security within a predetermined time period." .

figi-ps:ICAK a figi-gii:PricingSource .

figi-st:option skos:prefLabel "option" .

figi-ps:BSFR a figi-gii:PricingSource .

figi-ps:ICAK skos:prefLabel "icbc (asia) ltd" .

figi-st:option figi-gii:hasUniqueTextIdentifier "OPTION" .

figi-ps:BSFR skos:prefLabel "banque saudi fransi" .

figi-ps:ICAK figi-gii:hasUniqueTextIdentifier "ICAK" .

figi-ps:BSFR figi-gii:hasUniqueTextIdentifier "BSFR" .

figi-ps:ICAP a owl:NamedIndividual .

figi-ps:BSGB a owl:NamedIndividual .

figi-ps:ICAP a figi-gii:PricingSource .

figi-ps:BSGB a figi-gii:PricingSource .

figi-ps:ASHI a owl:NamedIndividual .

figi-ps:ICAP skos:prefLabel "intercapital trading" .

figi-ps:BSGB skos:prefLabel "santander ex" .

figi-ps:ASHI a figi-gii:PricingSource .

figi-ps:BSGB figi-gii:hasUniqueTextIdentifier "BSGB" .

figi-ps:ASHI skos:prefLabel "ardshininvestbank cj" .

figi-ps:BSH a owl:NamedIndividual .

figi-ps:ASHI figi-gii:hasUniqueTextIdentifier "ASHI" .

figi-ps:BSH a figi-gii:PricingSource .

figi-st:optionVolatility a owl:NamedIndividual .

figi-ps:BSH skos:prefLabel "bosera asset mgmt" .

figi-st:optionVolatility a figi-gii:SecurityType .

figi-ps:BSH figi-gii:hasUniqueTextIdentifier "BSH" .

figi-ps:ICAP figi-gii:hasUniqueTextIdentifier "ICAP" .

figi-st:optionVolatility skos:definition "A measure of the variation of the price of the underlying asset" .

figi-ps:BSHA a owl:NamedIndividual .

figi-ps:ICAR a owl:NamedIndividual .

figi-st:optionVolatility skos:prefLabel "option volatility" .

figi-ps:BSHA a figi-gii:PricingSource .

figi-ps:ICAR a figi-gii:PricingSource .

figi-st:optionVolatility figi-gii:hasUniqueTextIdentifier "OPTION VOLATILITY" .

figi-ps:BSHA skos:prefLabel "cfet bk of shanghai" .

figi-ps:ICAR skos:prefLabel "icap north america" .

figi-ps:ASIA a owl:NamedIndividual .

figi-ps:BSHA figi-gii:hasUniqueTextIdentifier "BSHA" .

figi-ps:ASIA a figi-gii:PricingSource .

figi-ps:ICAR figi-gii:hasUniqueTextIdentifier "ICAR" .

figi-ps:BSI a owl:NamedIndividual .

figi-ps:ASIA skos:prefLabel "aim demo - asia" .

figi-ps:ICAS a owl:NamedIndividual .

figi-ps:BSI a figi-gii:PricingSource .

figi-ps:ASIA figi-gii:hasUniqueTextIdentifier "ASIA" .

figi-ps:ICAS a figi-gii:PricingSource .

figi-ps:BSI skos:prefLabel "boenning,scattergood" .

figi-st:otcOption a owl:NamedIndividual .

figi-ps:ICAS skos:prefLabel "icap energy" .

figi-ps:BSI figi-gii:hasUniqueTextIdentifier "BSI" .

figi-st:otcOption a figi-gii:SecurityType .

figi-ps:ICAS figi-gii:hasUniqueTextIdentifier "ICAS" .

figi-ps:BSIK a owl:NamedIndividual , figi-gii:PricingSource .

figi-ps:ICBB a owl:NamedIndividual .

figi-st:otcOption skos:definition "Over-The-Counter Option. An option with negotiated premium, striking price, and expiration date." .

figi-ps:ICBB a figi-gii:PricingSource .

figi-ps:BSIK skos:prefLabel "bankenes sikringsf" .

figi-st:otcOption skos:prefLabel "otc option" .

figi-ps:ICBB skos:prefLabel "cfif icbc" .

figi-ps:BSIK figi-gii:hasUniqueTextIdentifier "BSIK" .

figi-st:otcOption figi-gii:hasUniqueTextIdentifier "OTC Option" .

figi-ps:ICBB figi-gii:hasUniqueTextIdentifier "ICBB" .

figi-ps:BSIL a owl:NamedIndividual .

figi-ps:ASIM a owl:NamedIndividual .

figi-ps:BSIL a figi-gii:PricingSource .

figi-ps:ICBC a owl:NamedIndividual .

figi-ps:ASIM a figi-gii:PricingSource .

figi-ps:BSIL skos:prefLabel "bear stearns int ltd" .

figi-ps:ICBC a figi-gii:PricingSource .

figi-ps:ASIM skos:prefLabel "alliance sim" .

figi-ps:BSIL figi-gii:hasUniqueTextIdentifier "BSIL" .

figi-ps:ICBC skos:prefLabel "icbc" .

figi-ps:ASIM figi-gii:hasUniqueTextIdentifier "ASIM" .

figi-ps:BSJP a owl:NamedIndividual .

figi-ps:ICBC figi-gii:hasUniqueTextIdentifier "ICBC" .

figi-ps:BSJP a figi-gii:PricingSource .

figi-st:overNight a owl:NamedIndividual , figi-gii:SecurityType .

figi-ps:ICBN a owl:NamedIndividual .

figi-ps:BSJP skos:prefLabel "bear stearns japan" .

figi-ps:ICBN a figi-gii:PricingSource .

figi-ps:BSJP figi-gii:hasUniqueTextIdentifier "BSJP" .

figi-st:overNight skos:definition "Used for ticketing Overnight transactions" .

figi-ps:ICBN skos:prefLabel "icici bank" .

figi-ps:BSK a owl:NamedIndividual .

figi-st:overNight skos:prefLabel "over/night" .

figi-ps:BSK a figi-gii:PricingSource .

figi-ps:ICBN figi-gii:hasUniqueTextIdentifier "ICBN" .

figi-st:overNight figi-gii:hasUniqueTextIdentifier "OVER/NIGHT" .

figi-ps:BSK skos:prefLabel "basler kantonalbk" .

figi-ps:ICBP a owl:NamedIndividual .

figi-ps:ASRT a owl:NamedIndividual .

figi-ps:BSK figi-gii:hasUniqueTextIdentifier "BSK" .

figi-ps:ICBP a figi-gii:PricingSource .

figi-ps:ASRT a figi-gii:PricingSource .

figi-ps:BSKB a owl:NamedIndividual .

figi-ps:ICBP skos:prefLabel "icbc (asia) 4:30" .

figi-ps:ASRT skos:prefLabel "assurant, inc" .

figi-ps:BSKB a figi-gii:PricingSource .

figi-ps:ICBP figi-gii:hasUniqueTextIdentifier "ICBP" .

figi-ps:ASRT figi-gii:hasUniqueTextIdentifier "ASRT" .

figi-ps:BSKB skos:prefLabel "basler kantonalbank" .

figi-ps:ICBR a owl:NamedIndividual .

figi-ps:ASSD a owl:NamedIndividual .

figi-ps:BSKB figi-gii:hasUniqueTextIdentifier "BSKB" .

figi-ps:ICBR a figi-gii:PricingSource .

figi-ps:ASSD a figi-gii:PricingSource .

figi-ps:BSMG a owl:NamedIndividual .

figi-ps:ICBR skos:prefLabel "icbc (asia) 11:30" .

figi-ps:BSMG a figi-gii:PricingSource .

figi-ps:ASSD skos:prefLabel "bbg assessed pricing" .

figi-ps:ICBR figi-gii:hasUniqueTextIdentifier "ICBR" .

figi-ps:BSMG skos:prefLabel "bank syariah mega" .

figi-ps:ASSD figi-gii:hasUniqueTextIdentifier "ASSD" .

figi-ps:BSMG figi-gii:hasUniqueTextIdentifier "BSMG" .

figi-ps:ICBX a owl:NamedIndividual , figi-gii:PricingSource .

figi-st:overnightIndexedSwap a owl:NamedIndividual .

figi-ps:BSMM a owl:NamedIndividual .

figi-ps:ICBX skos:prefLabel "icbpi" .

figi-ps:BSMM a figi-gii:PricingSource .

figi-st:overnightIndexedSwap a figi-gii:SecurityType .

figi-ps:ICBX figi-gii:hasUniqueTextIdentifier "ICBX" .

figi-ps:BSMM skos:prefLabel "banco santander c h" ;
	figi-gii:hasUniqueTextIdentifier "BSMM" .

figi-ps:ICCH a owl:NamedIndividual .

figi-st:overnightIndexedSwap skos:definition "An overnight index swap uses an overnight rate index, such as the Federal Funds Rate, as the underlying for its floating leg." .

figi-ps:ICCH a figi-gii:PricingSource .

figi-ps:BSMP a owl:NamedIndividual .

figi-st:overnightIndexedSwap skos:prefLabel "overnight indexed swap" .

figi-ps:ICCH skos:prefLabel "iccrea holding" .

figi-ps:BSMP a figi-gii:PricingSource .

figi-st:overnightIndexedSwap figi-gii:hasUniqueTextIdentifier "OVERNIGHT INDEXED SWAP" .

figi-ps:ICCH figi-gii:hasUniqueTextIdentifier "ICCH" .

figi-ps:BSMP skos:prefLabel "bear stearns asia lt" .

figi-ps:ASTB a owl:NamedIndividual .

figi-ps:ICCR a owl:NamedIndividual .

figi-ps:BSMP figi-gii:hasUniqueTextIdentifier "BSMP" .

figi-ps:ASTB a figi-gii:PricingSource .

figi-ps:ICCR a figi-gii:PricingSource .

figi-ps:BSMS a owl:NamedIndividual .

figi-ps:ASTB skos:prefLabel "aston bond" .

figi-ps:ICCR skos:prefLabel "iccrea banca 2" .

figi-ps:BSMS a figi-gii:PricingSource .

figi-ps:ASTB figi-gii:hasUniqueTextIdentifier "ASTB" .

figi-ps:ICCR figi-gii:hasUniqueTextIdentifier "ICCR" .

figi-ps:BSMS skos:prefLabel "banca di san marino" ;
	figi-gii:hasUniqueTextIdentifier "BSMS" .

figi-st:philippineCP a owl:NamedIndividual .

figi-ps:ICCX a owl:NamedIndividual .

figi-ps:BSNY a owl:NamedIndividual .

figi-st:philippineCP a figi-gii:SecurityType .

figi-ps:ICCX a figi-gii:PricingSource .

figi-ps:BSNY a figi-gii:PricingSource .

figi-st:philippineCP skos:definition "Philippino Commercial Paper" .

figi-ps:ICCX skos:prefLabel "investors capital ny" .

figi-ps:BSNY skos:prefLabel "bradesco securities" .

figi-st:philippineCP skos:prefLabel "philippine cp" .

figi-ps:ICCX figi-gii:hasUniqueTextIdentifier "ICCX" .

figi-ps:BSNY figi-gii:hasUniqueTextIdentifier "BSNY" .

figi-st:philippineCP figi-gii:hasUniqueTextIdentifier "PHILIPPINE CP" .

figi-ps:ICEA a owl:NamedIndividual .

figi-ps:BSPA a owl:NamedIndividual .

figi-ps:ICEA a figi-gii:PricingSource .

figi-ps:ASTC a owl:NamedIndividual .

figi-ps:BSPA a figi-gii:PricingSource .

figi-ps:ICEA skos:prefLabel "icap australia" .

figi-ps:ASTC a figi-gii:PricingSource .

figi-ps:BSPA skos:prefLabel "bolsa val panama" .

figi-ps:ICEA figi-gii:hasUniqueTextIdentifier "ICEA" .

figi-ps:BSPA figi-gii:hasUniqueTextIdentifier "BSPA" .

figi-ps:ASTC skos:prefLabel "astra sociedad" .

figi-ps:ICEB a owl:NamedIndividual .

figi-ps:BSPH a owl:NamedIndividual .

figi-ps:ASTC figi-gii:hasUniqueTextIdentifier "ASTC" .

figi-ps:ICEB a figi-gii:PricingSource .

figi-ps:BSPH a figi-gii:PricingSource .

figi-ps:ASTO a owl:NamedIndividual .

figi-ps:ICEB skos:prefLabel "icap fixed income" .

figi-ps:BSPH skos:prefLabel "bank sinopac, hk" .

figi-ps:ASTO a figi-gii:PricingSource .

figi-ps:ICEB skos:prefLabel "icebank ltd." .

figi-ps:BSPH figi-gii:hasUniqueTextIdentifier "BSPH" .

figi-ps:ASTO skos:prefLabel "aston bank s.a." .

figi-ps:ICEB figi-gii:hasUniqueTextIdentifier "ICEB" .

figi-ps:BSPX a owl:NamedIndividual .

figi-ps:ASTO figi-gii:hasUniqueTextIdentifier "ASTO" .

figi-ps:BSPX a figi-gii:PricingSource .

figi-ps:ICEK a owl:NamedIndividual .

figi-ps:BSPX skos:prefLabel "bear stearns" .

figi-st:physicalCommodityForward a owl:NamedIndividual .

figi-ps:ICEK a figi-gii:PricingSource .

figi-ps:BSPX figi-gii:hasUniqueTextIdentifier "BSPX" .

figi-st:physicalCommodityForward a figi-gii:SecurityType .

figi-ps:ICEK skos:prefLabel "ic east capital" .

figi-ps:BSRX a owl:NamedIndividual .

figi-ps:ICEK figi-gii:hasUniqueTextIdentifier "ICEK" .

figi-ps:BSRX a figi-gii:PricingSource .

figi-ps:ICEN a owl:NamedIndividual .

figi-st:physicalCommodityForward skos:definition "The amount of a specified underlying asset of a contract that is physically delivered by the seller of the contract to the exchange, and by the exchange to the buyers of the contract." .

figi-ps:ICEN a figi-gii:PricingSource .

figi-st:physicalCommodityForward skos:prefLabel "physical commodity forward." .

figi-ps:BSRX skos:prefLabel "bear stearns intl." .

figi-ps:ICEN skos:prefLabel "icap us energy" .

figi-st:physicalCommodityForward figi-gii:hasUniqueTextIdentifier "Physical commodity forward." .

figi-ps:BSRX figi-gii:hasUniqueTextIdentifier "BSRX" .

figi-ps:ICEN figi-gii:hasUniqueTextIdentifier "ICEN" .

figi-ps:ASWI a owl:NamedIndividual .

figi-ps:BSSB a owl:NamedIndividual .

figi-ps:ASWI a figi-gii:PricingSource .

figi-ps:ICEX a owl:NamedIndividual .

figi-ps:BSSB a figi-gii:PricingSource .

figi-ps:ICEX a figi-gii:PricingSource .

figi-ps:ASWI skos:prefLabel "armswissbank cjsc" .

figi-ps:BSSB skos:prefLabel "bear stearns" .

figi-ps:ICEX skos:prefLabel "iceland stock exch" .

figi-ps:ASWI figi-gii:hasUniqueTextIdentifier "ASWI" .

figi-ps:BSSB figi-gii:hasUniqueTextIdentifier "BSSB" .

figi-ps:ICEX figi-gii:hasUniqueTextIdentifier "ICEX" .

figi-ps:ASX a owl:NamedIndividual .

figi-ps:BSTB a owl:NamedIndividual .

figi-ps:ASX a figi-gii:PricingSource .

figi-ps:ICHK a owl:NamedIndividual .

figi-ps:BSTB a figi-gii:PricingSource .

figi-ps:ICHK a figi-gii:PricingSource .

figi-ps:ASX skos:prefLabel "australian stk exch" .

figi-ps:BSTB skos:prefLabel "bearstearntba" .

figi-ps:ICHK skos:prefLabel "icap (hk) ltd" .

figi-ps:ASX figi-gii:hasUniqueTextIdentifier "ASX" .

figi-ps:BSTB figi-gii:hasUniqueTextIdentifier "BSTB" .

figi-ps:ICHK figi-gii:hasUniqueTextIdentifier "ICHK" .

figi-st:physicalCommodityFuture a owl:NamedIndividual .

figi-ps:BSTE a owl:NamedIndividual .

figi-ps:ICHS a owl:NamedIndividual .

figi-st:physicalCommodityFuture a figi-gii:SecurityType .

figi-ps:BSTE a figi-gii:PricingSource .

figi-ps:ICHS a figi-gii:PricingSource .

figi-ps:BSTE skos:prefLabel "banesto emisiones" .

figi-ps:ICHS skos:prefLabel "icap hong kong" .

figi-ps:BSTE figi-gii:hasUniqueTextIdentifier "BSTE" .

figi-st:physicalCommodityFuture skos:definition "Commodity Future. A contract to buy or sell a specific commodity a ta specified price at a certain future date." .

figi-ps:ICHS figi-gii:hasUniqueTextIdentifier "ICHS" .

figi-ps:BSTO a owl:NamedIndividual .

figi-st:physicalCommodityFuture skos:prefLabel "physical commodity future." .

figi-ps:ICIC a owl:NamedIndividual .

figi-ps:BSTO a figi-gii:PricingSource .

figi-ps:ICIC a figi-gii:PricingSource .

figi-st:physicalCommodityFuture figi-gii:hasUniqueTextIdentifier "Physical commodity future." .

figi-ps:BSTO skos:prefLabel "banesto" .

figi-ps:ICIC skos:prefLabel "icici securities" .

figi-ps:BSTO figi-gii:hasUniqueTextIdentifier "BSTO" .

figi-ps:ASXY a owl:NamedIndividual .

figi-ps:ICIC figi-gii:hasUniqueTextIdentifier "ICIC" .

figi-ps:BSTS a owl:NamedIndividual .

figi-ps:ASXY a figi-gii:PricingSource .

figi-ps:BSTS a figi-gii:PricingSource .

figi-ps:ICIN a owl:NamedIndividual .

figi-ps:ASXY skos:prefLabel "asx yield" .

figi-ps:BSTS skos:prefLabel "bear stearns sg" .

figi-ps:ICIN a figi-gii:PricingSource .

figi-ps:ASXY figi-gii:hasUniqueTextIdentifier "ASXY" .

figi-ps:BSTS figi-gii:hasUniqueTextIdentifier "BSTS" .

figi-ps:ICIN skos:prefLabel "icap india private" .

figi-ps:ASYA a owl:NamedIndividual .

figi-ps:BSTV a owl:NamedIndividual .

figi-ps:ICIN figi-gii:hasUniqueTextIdentifier "ICIN" .

figi-ps:ASYA a figi-gii:PricingSource .

figi-ps:BSTV a figi-gii:PricingSource .

figi-ps:ICJB a owl:NamedIndividual .

figi-ps:ASYA skos:prefLabel "asya katilim" .

figi-ps:BSTV skos:prefLabel "bestinver" .

figi-ps:ICJB a figi-gii:PricingSource .

figi-ps:ASYA figi-gii:hasUniqueTextIdentifier "ASYA" .

figi-ps:BSTV figi-gii:hasUniqueTextIdentifier "BSTV" .

figi-ps:ICJB skos:prefLabel "icap jgb" .

figi-st:physicalCommodityGeneric a owl:NamedIndividual .

figi-ps:BSUN a owl:NamedIndividual .

figi-ps:ICJB figi-gii:hasUniqueTextIdentifier "ICJB" .

figi-st:physicalCommodityGeneric a figi-gii:SecurityType .

figi-ps:BSUN a figi-gii:PricingSource .

figi-ps:ICJC a owl:NamedIndividual .

figi-ps:BSUN skos:prefLabel "birla sunlife amc" .

figi-ps:ICJC a figi-gii:PricingSource .

figi-ps:BSUN figi-gii:hasUniqueTextIdentifier "BSUN" .

figi-st:physicalCommodityGeneric skos:definition "Physically Deliverable (Physical) Generics on Commodity Futures. Generics are used to combine multiple futures contracts to build a generic history stream." .

figi-ps:ICJC skos:prefLabel "icap jgb closing" .

figi-ps:BSUP a owl:NamedIndividual .

figi-st:physicalCommodityGeneric skos:prefLabel "physical commodity generic." .

figi-ps:BSUP a figi-gii:PricingSource .

figi-ps:ICJC figi-gii:hasUniqueTextIdentifier "ICJC" .

figi-ps:BSUP skos:prefLabel "banco supervielle" .

figi-st:physicalCommodityGeneric figi-gii:hasUniqueTextIdentifier "Physical commodity generic." .

figi-ps:BSUP figi-gii:hasUniqueTextIdentifier "BSUP" .

figi-ps:ICJD a owl:NamedIndividual .

figi-ps:ASYL a owl:NamedIndividual .

figi-ps:ICJD a figi-gii:PricingSource .

figi-ps:ASYL a figi-gii:PricingSource .

figi-ps:ICJD skos:prefLabel "icap jgb delayed" .

figi-ps:BTAC a owl:NamedIndividual .

figi-ps:ICJD figi-gii:hasUniqueTextIdentifier "ICJD" .

figi-ps:ASYL skos:prefLabel "ao asyl-invest" .

figi-ps:BTAC a figi-gii:PricingSource .

figi-ps:ICJG a owl:NamedIndividual .

figi-ps:ASYL figi-gii:hasUniqueTextIdentifier "ASYL" .

figi-ps:ICJG a figi-gii:PricingSource .

figi-ps:BTAC skos:prefLabel "bta securities jsc" .

figi-ps:ICJG skos:prefLabel "icap jgb 15y" .

figi-st:physicalCommodityOption a owl:NamedIndividual .

figi-ps:BTAC figi-gii:hasUniqueTextIdentifier "BTAC" .

figi-ps:ICJG figi-gii:hasUniqueTextIdentifier "ICJG" .

figi-st:physicalCommodityOption a figi-gii:SecurityType .

figi-ps:BTBA a owl:NamedIndividual .

figi-ps:ICLG a owl:NamedIndividual .

figi-ps:BTBA a figi-gii:PricingSource .

figi-ps:ICLG a figi-gii:PricingSource .

figi-ps:BTBA skos:prefLabel "barclays mortgage" .

figi-st:physicalCommodityOption skos:definition "Physical Commodity. The actual, tangible commodity, such as corn or soybeans, which a seller delivers to the buyer of a commodities contract." .

figi-ps:ICLG skos:prefLabel "icon capital" .

figi-ps:BTBA figi-gii:hasUniqueTextIdentifier "BTBA" .

figi-st:physicalCommodityOption skos:prefLabel "physical commodity option." .

figi-ps:ICLG figi-gii:hasUniqueTextIdentifier "ICLG" .

figi-ps:BTCO a owl:NamedIndividual .

figi-st:physicalCommodityOption figi-gii:hasUniqueTextIdentifier "Physical commodity option." .

figi-ps:ICMA a owl:NamedIndividual .

figi-ps:BTCO a figi-gii:PricingSource .

figi-ps:ICMA a figi-gii:PricingSource .

figi-ps:ATEL a owl:NamedIndividual .

figi-ps:BTCO skos:prefLabel "banctrust and co" .

figi-ps:ATEL a figi-gii:PricingSource .

figi-ps:ICMA skos:prefLabel "harlows (malaysia)" .

figi-ps:BTCO figi-gii:hasUniqueTextIdentifier "BTCO" .

figi-ps:ATEL skos:prefLabel "amstel secs - london" .

figi-ps:ICMA figi-gii:hasUniqueTextIdentifier "ICMA" .

figi-ps:BTCW a owl:NamedIndividual .

figi-ps:ATEL figi-gii:hasUniqueTextIdentifier "ATEL" .

figi-ps:ICNG a owl:NamedIndividual .

figi-ps:BTCW a figi-gii:PricingSource .

figi-ps:ICNG a figi-gii:PricingSource .

figi-ps:ATEQ a owl:NamedIndividual .

figi-ps:BTCW skos:prefLabel "bahana tcw" .

figi-ps:ATEQ a figi-gii:PricingSource .

figi-ps:ICNG skos:prefLabel "icap new zealand" .

figi-ps:BTCW figi-gii:hasUniqueTextIdentifier "BTCW" .

figi-ps:ATEQ skos:prefLabel "atlantic equity llp" .

figi-ps:ICNG figi-gii:hasUniqueTextIdentifier "ICNG" .

figi-ps:BTEC a owl:NamedIndividual .

figi-ps:ATEQ figi-gii:hasUniqueTextIdentifier "ATEQ" .

figi-ps:BTEC a figi-gii:PricingSource .

figi-ps:ICP a owl:NamedIndividual .

figi-st:physicalCommoditySpot a owl:NamedIndividual .

figi-ps:BTEC skos:prefLabel "brokertec" .

figi-ps:ICP a figi-gii:PricingSource .

figi-st:physicalCommoditySpot a figi-gii:SecurityType .

figi-ps:BTEC figi-gii:hasUniqueTextIdentifier "BTEC" .

figi-ps:ICP skos:prefLabel "icp capital" ;
	figi-gii:hasUniqueTextIdentifier "ICP" .

figi-ps:BTES a owl:NamedIndividual .

figi-st:physicalCommoditySpot skos:definition "Physically Deliverable (Physical) Spot on Commodity Futures. Spot is the actual physical product on which a futures contract is based." .

figi-ps:ICPH a owl:NamedIndividual .

figi-ps:BTES a figi-gii:PricingSource .

figi-ps:ICPH a figi-gii:PricingSource .

figi-st:physicalCommoditySpot skos:prefLabel "physical commodity spot." .

figi-ps:BTES skos:prefLabel "bloomberg hk test" .

figi-ps:ICPH skos:prefLabel "icap philippines" .

figi-st:physicalCommoditySpot figi-gii:hasUniqueTextIdentifier "Physical commodity spot." .

figi-ps:BTES figi-gii:hasUniqueTextIdentifier "BTES" .

figi-ps:ICPH figi-gii:hasUniqueTextIdentifier "ICPH" .

figi-ps:ATFB a owl:NamedIndividual .

figi-ps:BTGA a owl:NamedIndividual .

figi-ps:ICPN a owl:NamedIndividual .

figi-ps:ATFB a figi-gii:PricingSource .

figi-ps:BTGA a figi-gii:PricingSource .

figi-ps:ICPN a figi-gii:PricingSource .

figi-ps:ATFB skos:prefLabel "atf bank" .

figi-ps:BTGA skos:prefLabel "bottega securities" .

figi-ps:ICPN skos:prefLabel "icap nz private" .

figi-ps:ATFB figi-gii:hasUniqueTextIdentifier "ATFB" .

figi-ps:BTGA figi-gii:hasUniqueTextIdentifier "BTGA" .

figi-ps:ICPN figi-gii:hasUniqueTextIdentifier "ICPN" .

figi-ps:ATHN a owl:NamedIndividual .

figi-ps:BTGE a owl:NamedIndividual .

figi-ps:ATHN a figi-gii:PricingSource .

figi-ps:ICPO a owl:NamedIndividual , figi-gii:PricingSource .

figi-ps:ATHN skos:prefLabel "athene asset mgt." .

figi-ps:ICPO skos:prefLabel "icap poland" .

figi-ps:ATHN figi-gii:hasUniqueTextIdentifier "ATHN" .

figi-ps:BTGE a figi-gii:PricingSource .

figi-ps:ICPO figi-gii:hasUniqueTextIdentifier "ICPO" .

figi-st:physicalIndexFuture a owl:NamedIndividual .

figi-ps:BTGE skos:prefLabel "bta bank" .

figi-st:physicalIndexFuture a figi-gii:SecurityType .

figi-ps:ICPR a owl:NamedIndividual .

figi-ps:BTGE figi-gii:hasUniqueTextIdentifier "BTGE" .

figi-ps:ICPR a figi-gii:PricingSource ;
	skos:prefLabel "icprc" .

figi-ps:BTHA a owl:NamedIndividual .

figi-st:physicalIndexFuture skos:definition "Stock Index Future. A futures contract that uses a stock index as its base, and which is settled by delivery of the underlying stocks." .

figi-ps:ICPR figi-gii:hasUniqueTextIdentifier "ICPR" .

figi-ps:BTHA a figi-gii:PricingSource .

figi-st:physicalIndexFuture skos:prefLabel "physical index future." .

figi-ps:ICSC a owl:NamedIndividual .

figi-ps:BTHA skos:prefLabel "bank of thailand" .

figi-ps:ICSC a figi-gii:PricingSource .

figi-st:physicalIndexFuture figi-gii:hasUniqueTextIdentifier "Physical index future." .

figi-ps:BTHA figi-gii:hasUniqueTextIdentifier "BTHA" .

figi-ps:ICSC skos:prefLabel "icap" .

figi-ps:ATIV a owl:NamedIndividual .

figi-ps:BTI a owl:NamedIndividual .

figi-ps:ATIV a figi-gii:PricingSource .

figi-ps:ICSC figi-gii:hasUniqueTextIdentifier "ICSC" .

figi-ps:BTI a figi-gii:PricingSource .

figi-ps:ATIV skos:prefLabel "ativa" .

figi-ps:ICSG a owl:NamedIndividual .

figi-ps:BTI skos:prefLabel "bankers trust istanb" .

figi-ps:ICSG a figi-gii:PricingSource .

figi-ps:ATIV figi-gii:hasUniqueTextIdentifier "ATIV" .

figi-ps:BTI figi-gii:hasUniqueTextIdentifier "BTI" .

figi-ps:ICSG skos:prefLabel "icap ap (singapore)" .

figi-ps:ATLA a owl:NamedIndividual .

figi-ps:BTIA a owl:NamedIndividual .

figi-ps:ATLA a figi-gii:PricingSource .

figi-ps:ICSG figi-gii:hasUniqueTextIdentifier "ICSG" .

figi-ps:BTIA a figi-gii:PricingSource .

figi-ps:ATLA skos:prefLabel "atlas one financial" .

figi-ps:ICSW a owl:NamedIndividual .

figi-ps:BTIA skos:prefLabel "btig singapore" .

figi-ps:ATLA figi-gii:hasUniqueTextIdentifier "ATLA" .

figi-ps:ICSW a figi-gii:PricingSource .

figi-ps:BTIA figi-gii:hasUniqueTextIdentifier "BTIA" .

figi-st:physicalIndexOption a owl:NamedIndividual .

figi-ps:ICSW skos:prefLabel "icap" .

figi-st:physicalIndexOption a figi-gii:SecurityType .

figi-ps:BTIG a owl:NamedIndividual .

figi-ps:ICSW figi-gii:hasUniqueTextIdentifier "ICSW" .

figi-ps:BTIG a figi-gii:PricingSource .

figi-ps:ICTE a owl:NamedIndividual .

figi-ps:BTIG skos:prefLabel "btig" .

figi-ps:ICTE a figi-gii:PricingSource .

figi-ps:BTIG figi-gii:hasUniqueTextIdentifier "BTIG" .

figi-ps:ICTE skos:prefLabel "cfets icap test" .

figi-st:physicalIndexOption skos:definition "Index Options. An option that is based on a stock index (performance measure of a group of stocks). Such options enable investors to trade in a particular market or industry group without having to buy individual stocks. Index options are issued by the Options Clearing Corporation." .

figi-ps:ICTE figi-gii:hasUniqueTextIdentifier "ICTE" .

figi-ps:BTIP a owl:NamedIndividual .

figi-st:physicalIndexOption skos:prefLabel "physical index option." .

figi-ps:ICTI a owl:NamedIndividual .

figi-ps:BTIP a figi-gii:PricingSource .

figi-ps:ICTI a figi-gii:PricingSource .

figi-st:physicalIndexOption figi-gii:hasUniqueTextIdentifier "Physical index option." .

figi-ps:BTIP skos:prefLabel "barclays tips" .

figi-ps:ICTI skos:prefLabel "ict" .

figi-ps:ATLS a owl:NamedIndividual .

figi-ps:BTIP figi-gii:hasUniqueTextIdentifier "BTIP" .

figi-ps:ATLS a figi-gii:PricingSource .

figi-ps:ICTI figi-gii:hasUniqueTextIdentifier "ICTI" .

figi-ps:BTMB a owl:NamedIndividual .

figi-ps:ATLS skos:prefLabel "atlas one financial" .

figi-ps:ICUA a owl:NamedIndividual .

figi-ps:BTMB a figi-gii:PricingSource .

figi-ps:ATLS figi-gii:hasUniqueTextIdentifier "ATLS" .

figi-ps:ICUA a figi-gii:PricingSource .

figi-ps:BTMB skos:prefLabel "btm training - buy" .

figi-st:pik a owl:NamedIndividual .

figi-ps:ICUA skos:prefLabel "inv capital ukraine" .

figi-st:pik a figi-gii:SecurityType .

figi-ps:BTMB figi-gii:hasUniqueTextIdentifier "BTMB" .

figi-ps:ICUA figi-gii:hasUniqueTextIdentifier "ICUA" .

figi-ps:BTMS a owl:NamedIndividual .

figi-ps:ICUB a owl:NamedIndividual .

figi-ps:BTMS a figi-gii:PricingSource .

figi-ps:ICUB a figi-gii:PricingSource .

figi-ps:BTMS skos:prefLabel "btm training - sell" .

figi-ps:ICUB skos:prefLabel "icubic ag" .

figi-ps:BTMS figi-gii:hasUniqueTextIdentifier "BTMS" .

figi-ps:ICUB figi-gii:hasUniqueTextIdentifier "ICUB" .

figi-ps:BTMU a owl:NamedIndividual .

figi-ps:ICVN a owl:NamedIndividual .

figi-st:pik skos:definition "A loan whereby interest may be capitalized and added to the principal amount of the loan, which is then compounded and the aggregated amount of which will be due to lenders at maturity. PIK loans are usually in the form of a term loan." .

figi-ps:BTMU a figi-gii:PricingSource .

figi-ps:ICVN a figi-gii:PricingSource .

figi-st:pik skos:prefLabel "pik" .

figi-ps:ICVN skos:prefLabel "incombank" .

figi-st:pik figi-gii:hasUniqueTextIdentifier "PIK" .

figi-ps:ICVN figi-gii:hasUniqueTextIdentifier "ICVN" .

figi-ps:ATOM a owl:NamedIndividual .

figi-ps:IDBC a owl:NamedIndividual .

figi-ps:ATOM a figi-gii:PricingSource .

figi-ps:IDBC a figi-gii:PricingSource .

figi-ps:BTMU skos:prefLabel "btmu" .

figi-ps:ATOM skos:prefLabel "aton llc" .

figi-ps:IDBC skos:prefLabel "idbi capital market" .

figi-ps:BTMU figi-gii:hasUniqueTextIdentifier "BTMU" .

figi-ps:ATOM figi-gii:hasUniqueTextIdentifier "ATOM" .

figi-ps:IDBC figi-gii:hasUniqueTextIdentifier "IDBC" .

figi-ps:BTTH a owl:NamedIndividual .

figi-ps:ATON a owl:NamedIndividual .

figi-ps:BTTH a figi-gii:PricingSource .

figi-ps:IDBE a owl:NamedIndividual .

figi-ps:ATON a figi-gii:PricingSource .

figi-ps:BTTH skos:prefLabel "bankthai public co" .

figi-ps:IDBE a figi-gii:PricingSource .

figi-ps:ATON skos:prefLabel "aton capital group" .

figi-ps:BTTH figi-gii:hasUniqueTextIdentifier "BTTH" .

figi-ps:IDBE skos:prefLabel "idb capital corp" .

figi-ps:ATON figi-gii:hasUniqueTextIdentifier "ATON" .

figi-ps:BUCK a owl:NamedIndividual .

figi-ps:IDBE figi-gii:hasUniqueTextIdentifier "IDBE" .

figi-ps:BUCK a figi-gii:PricingSource .

figi-st:pikRev a owl:NamedIndividual .

figi-ps:IDBI a owl:NamedIndividual .

figi-ps:BUCK skos:prefLabel "buckingham research" .

figi-st:pikRev a figi-gii:SecurityType .

figi-ps:IDBI a figi-gii:PricingSource .

figi-ps:BUCK figi-gii:hasUniqueTextIdentifier "BUCK" .

figi-ps:IDBI skos:prefLabel "idbi bank" .

figi-ps:BUDA a owl:NamedIndividual .

figi-ps:IDBI figi-gii:hasUniqueTextIdentifier "IDBI" .

figi-st:pikRev skos:definition "A loan whereby interest may be capitalized and added to the principal amount of the loan, which is then compounded and the aggregated amount of which will be due to lenders at maturity. Once borrowed, can be borrowed again." .

figi-ps:BUDA a figi-gii:PricingSource .

figi-ps:IDBK a owl:NamedIndividual .

figi-st:pikRev skos:prefLabel "pik rev" .

figi-ps:IDBK a figi-gii:PricingSource .

figi-ps:BUDA skos:prefLabel "budapest exchange" .

figi-st:pikRev figi-gii:hasUniqueTextIdentifier "PIK REV" .

figi-ps:IDBK skos:prefLabel "cfif industrial bank" .

figi-ps:BUDA figi-gii:hasUniqueTextIdentifier "BUDA" .

figi-ps:AUAT a owl:NamedIndividual .

figi-ps:IDBK figi-gii:hasUniqueTextIdentifier "IDBK" .

figi-ps:BUEP a owl:NamedIndividual .

figi-ps:AUAT a figi-gii:PricingSource .

figi-ps:BUEP a figi-gii:PricingSource .

figi-ps:IDBN a owl:NamedIndividual .

figi-ps:AUAT skos:prefLabel "ambank (m) bhd" .

figi-ps:BUEP skos:prefLabel "barclays us exotics" .

figi-ps:IDBN a figi-gii:PricingSource .

figi-ps:AUAT figi-gii:hasUniqueTextIdentifier "AUAT" .

figi-ps:BUEP figi-gii:hasUniqueTextIdentifier "BUEP" .

figi-ps:IDBN skos:prefLabel "israel discount bkny" .

figi-ps:AUB a owl:NamedIndividual .

figi-ps:IDBN figi-gii:hasUniqueTextIdentifier "IDBN" .

figi-ps:BULG a owl:NamedIndividual .

figi-ps:AUB a figi-gii:PricingSource .

figi-ps:IDBO a owl:NamedIndividual .

figi-ps:BULG a figi-gii:PricingSource .

figi-ps:AUB skos:prefLabel "asia united bk" .

figi-ps:IDBO a figi-gii:PricingSource .

figi-ps:BULG skos:prefLabel "bulgaria se" .

figi-ps:AUB figi-gii:hasUniqueTextIdentifier "AUB" .

figi-ps:IDBO skos:prefLabel "idbi bankxxxxxxxxxxx" .

figi-ps:BULG figi-gii:hasUniqueTextIdentifier "BULG" .

figi-st:pikStandbyTerm a owl:NamedIndividual .

figi-ps:IDBO figi-gii:hasUniqueTextIdentifier "IDBO" .

figi-ps:BULL a owl:NamedIndividual .

figi-st:pikStandbyTerm a figi-gii:SecurityType .

figi-ps:BULL a figi-gii:PricingSource .

figi-ps:IDC2 a owl:NamedIndividual .

figi-ps:BULL skos:prefLabel "bulltick llc" .

figi-ps:IDC2 a figi-gii:PricingSource .

figi-ps:BULL figi-gii:hasUniqueTextIdentifier "BULL" .

figi-ps:IDC2 skos:prefLabel "idc portfolio" .

figi-st:pikStandbyTerm skos:definition "A loan whereby interest may be capitalized and added to the principal amount of the loan, which is then compounded and the aggregated amount of which will be due to lenders at maturity. Issued on a stand-by basis and borrowed only if and when needed. Once borrowed, cannot be borrowed again." .

figi-ps:IDC2 figi-gii:hasUniqueTextIdentifier "IDC2" .

figi-ps:BULT a owl:NamedIndividual .

figi-st:pikStandbyTerm skos:prefLabel "pik standby term" .

figi-ps:IDCP a owl:NamedIndividual .

figi-ps:BULT a figi-gii:PricingSource .

figi-st:pikStandbyTerm figi-gii:hasUniqueTextIdentifier "PIK STANDBY TERM" .

figi-ps:IDCP a figi-gii:PricingSource .

figi-ps:BULT skos:prefLabel "burren capital advis" .

figi-ps:AUBE a owl:NamedIndividual .

figi-ps:IDCP skos:prefLabel "interactive data cp" .

figi-ps:AUBE a figi-gii:PricingSource .

figi-ps:BULT figi-gii:hasUniqueTextIdentifier "BULT" .

figi-ps:IDCP figi-gii:hasUniqueTextIdentifier "IDCP" .

figi-ps:AUBE skos:prefLabel "ahli united bank sae" .

figi-ps:BUMI a owl:NamedIndividual .

figi-ps:IDF a owl:NamedIndividual .

figi-ps:AUBE figi-gii:hasUniqueTextIdentifier "AUBE" .

figi-ps:IDF a figi-gii:PricingSource .

figi-ps:BUMI a figi-gii:PricingSource .

figi-st:pikSynthLoc a owl:NamedIndividual .

figi-ps:IDF skos:prefLabel "idfc asset managemen" .

figi-ps:BUMI skos:prefLabel "bumiputra commerce" .

figi-st:pikSynthLoc a figi-gii:SecurityType .

figi-ps:IDF figi-gii:hasUniqueTextIdentifier "IDF" .

figi-ps:BUMI figi-gii:hasUniqueTextIdentifier "BUMI" .

figi-ps:IDMA a owl:NamedIndividual .

figi-ps:BUR a owl:NamedIndividual .

figi-ps:IDMA a figi-gii:PricingSource .

figi-ps:BUR a figi-gii:PricingSource .

figi-ps:IDMA skos:prefLabel "inter dealer mkt ind" .

figi-st:pikSynthLoc skos:definition "A loan whereby interest may be capitalized and added to the principal amount of the loan, which is then compounded and the aggregated amount of which will be due to lenders at maturity. Fully cash collateralized with proceeds of a term loan which has been issued by the same borrower, usually with the same amount and terms." .

figi-ps:IDMA figi-gii:hasUniqueTextIdentifier "IDMA" .

figi-st:pikSynthLoc skos:prefLabel "pik synth loc" .

figi-ps:IDMF a owl:NamedIndividual .

figi-ps:BUR skos:prefLabel "bank burgenland" .

figi-ps:IDMF a figi-gii:PricingSource .

figi-st:pikSynthLoc figi-gii:hasUniqueTextIdentifier "PIK SYNTH LOC" .

figi-ps:BUR figi-gii:hasUniqueTextIdentifier "BUR" .

figi-ps:IDMF skos:prefLabel "inter dealer market" .

figi-ps:AUBR a owl:NamedIndividual .

figi-ps:IDMF figi-gii:hasUniqueTextIdentifier "IDMF" .

figi-ps:BURJ a owl:NamedIndividual .

figi-ps:AUBR a figi-gii:PricingSource .

figi-ps:BURJ a figi-gii:PricingSource .

figi-ps:IDSB a owl:NamedIndividual .

figi-ps:AUBR skos:prefLabel "ahli united bank" .

figi-ps:BURJ skos:prefLabel "burj bank limited" .

figi-ps:IDSB a figi-gii:PricingSource .

figi-ps:AUBR figi-gii:hasUniqueTextIdentifier "AUBR" .

figi-ps:BURJ figi-gii:hasUniqueTextIdentifier "BURJ" .

figi-ps:IDSB skos:prefLabel "bank dbs indonesia" .

figi-ps:AUDB a owl:NamedIndividual .

figi-ps:BVAC a owl:NamedIndividual .

figi-ps:AUDB a figi-gii:PricingSource .

figi-ps:IDSB figi-gii:hasUniqueTextIdentifier "IDSB" .

figi-ps:BVAC a figi-gii:PricingSource .

figi-ps:AUDB skos:prefLabel "banque audi" .

figi-ps:IEBI a owl:NamedIndividual .

figi-ps:BVAC skos:prefLabel "bbva colombia sa" .

figi-ps:AUDB figi-gii:hasUniqueTextIdentifier "AUDB" .

figi-ps:IEBI a figi-gii:PricingSource .

figi-ps:BVAC figi-gii:hasUniqueTextIdentifier "BVAC" .

figi-st:pikTerm a owl:NamedIndividual .

figi-ps:IEBI skos:prefLabel "ieb israel ltd" .

figi-ps:BVAL a owl:NamedIndividual .

figi-st:pikTerm a figi-gii:SecurityType .

figi-ps:IEBI figi-gii:hasUniqueTextIdentifier "IEBI" .

figi-ps:BVAL a figi-gii:PricingSource ;
	skos:prefLabel "bval" .

figi-ps:IEHY a owl:NamedIndividual .

figi-ps:BVAL figi-gii:hasUniqueTextIdentifier "BVAL" .

figi-st:pikTerm skos:definition "A loan whereby interest may be capitalized and added to the principal amount of the loan, which is then compounded and the aggregated amount of which will be due to lenders at maturity. Once borrowed, cannot be re-borrowed." .

figi-ps:IEHY a figi-gii:PricingSource .

figi-ps:BVAN a owl:NamedIndividual .

figi-st:pikTerm skos:prefLabel "pik term" .

figi-ps:IEHY skos:prefLabel "intl idx co (iboxx)" .

figi-ps:BVAN a figi-gii:PricingSource .

figi-st:pikTerm figi-gii:hasUniqueTextIdentifier "PIK TERM" .

figi-ps:IEHY figi-gii:hasUniqueTextIdentifier "IEHY" .

figi-ps:BVAN skos:prefLabel "banco venezuela" .

figi-ps:AUDD a owl:NamedIndividual .

figi-ps:IFCC a owl:NamedIndividual .

figi-ps:AUDD a figi-gii:PricingSource .

figi-ps:BVAN figi-gii:hasUniqueTextIdentifier "BVAN" .

figi-ps:IFCC a figi-gii:PricingSource .

figi-ps:AUDD skos:prefLabel "bank audi-audi group" .

figi-ps:BVC a owl:NamedIndividual .

figi-ps:IFCC skos:prefLabel "intl finance corp" .

figi-ps:AUDD figi-gii:hasUniqueTextIdentifier "AUDD" .

figi-ps:BVC a figi-gii:PricingSource .

figi-ps:IFCC figi-gii:hasUniqueTextIdentifier "IFCC" .

figi-ps:AUDE a owl:NamedIndividual .

figi-ps:BVC skos:prefLabel "caracas stock exch" .

figi-ps:IFEX a owl:NamedIndividual .

figi-ps:AUDE a figi-gii:PricingSource .

figi-ps:BVC figi-gii:hasUniqueTextIdentifier "BVC" .

figi-ps:IFEX a figi-gii:PricingSource .

figi-ps:AUDE skos:prefLabel "bank audi sae egypt" .

figi-ps:BVCM a owl:NamedIndividual .

figi-ps:IFEX skos:prefLabel "ifex-tass wp-hbank" .

figi-ps:BVCM a figi-gii:PricingSource .

figi-ps:AUDE figi-gii:hasUniqueTextIdentifier "AUDE" .

figi-ps:IFEX figi-gii:hasUniqueTextIdentifier "IFEX" .

figi-ps:BVCM skos:prefLabel "hvb america" .

figi-st:plazosFijos a owl:NamedIndividual .

figi-ps:IFGC a owl:NamedIndividual .

figi-ps:BVCM figi-gii:hasUniqueTextIdentifier "BVCM" .

figi-st:plazosFijos a figi-gii:SecurityType .

figi-ps:IFGC a figi-gii:PricingSource .

figi-ps:BVCO a owl:NamedIndividual .

figi-st:plazosFijos skos:definition "Argentinian MMkt instrument" .

figi-ps:BVCO a figi-gii:PricingSource .

figi-ps:IFGC skos:prefLabel "ifg continent" .

figi-ps:BVCO skos:prefLabel "bolsa de valores" .

figi-st:plazosFijos skos:prefLabel "plazos fijos" .

figi-ps:IFGC figi-gii:hasUniqueTextIdentifier "IFGC" .

figi-ps:BVCO figi-gii:hasUniqueTextIdentifier "BVCO" .

figi-st:plazosFijos figi-gii:hasUniqueTextIdentifier "PLAZOS FIJOS" .

figi-ps:IFP a owl:NamedIndividual .

figi-ps:BVDR a owl:NamedIndividual .

figi-ps:AUDI a owl:NamedIndividual .

figi-ps:IFP a figi-gii:PricingSource .

figi-ps:BVDR a figi-gii:PricingSource .

figi-ps:AUDI a figi-gii:PricingSource .

figi-ps:IFP skos:prefLabel "ifp services ltd" .

figi-ps:BVDR skos:prefLabel "bolsa de valores, dr" .

figi-ps:AUDI skos:prefLabel "bank audi sal" .

figi-ps:IFP figi-gii:hasUniqueTextIdentifier "IFP" .

figi-ps:BVDR figi-gii:hasUniqueTextIdentifier "BVDR" .

figi-ps:AUDI figi-gii:hasUniqueTextIdentifier "AUDI" .

figi-ps:IFPS a owl:NamedIndividual .

figi-ps:BVEN a owl:NamedIndividual .

figi-ps:IFPS a figi-gii:PricingSource .

figi-st:portugueseCP a owl:NamedIndividual .

figi-ps:BVEN a figi-gii:PricingSource .

figi-ps:IFPS skos:prefLabel "ifp switzerland" .

figi-ps:BVEN skos:prefLabel "banco venezuela" .

figi-st:portugueseCP a figi-gii:SecurityType .

figi-ps:IFPS figi-gii:hasUniqueTextIdentifier "IFPS" .

figi-ps:BVEN figi-gii:hasUniqueTextIdentifier "BVEN" .

figi-st:portugueseCP skos:definition "Portugal Domestic Commercial Paper" .

figi-ps:IGIM a owl:NamedIndividual .

figi-ps:BVES a owl:NamedIndividual .

figi-ps:IGIM a figi-gii:PricingSource .

figi-st:portugueseCP skos:prefLabel "portuguese cp" .

figi-ps:BVES a figi-gii:PricingSource .

figi-ps:IGIM skos:prefLabel "ig investment mgmt" .

figi-st:portugueseCP figi-gii:hasUniqueTextIdentifier "PORTUGUESE CP" .

figi-ps:BVES skos:prefLabel "bolsa el salvador" .

figi-ps:IGIM figi-gii:hasUniqueTextIdentifier "IGIM" .

figi-ps:AURA a owl:NamedIndividual .

figi-ps:BVES figi-gii:hasUniqueTextIdentifier "BVES" .

figi-ps:AURA a figi-gii:PricingSource .

figi-ps:IGLS a owl:NamedIndividual .

figi-ps:BVL3 a owl:NamedIndividual .

figi-ps:AURA skos:prefLabel "auriga global invest" .

figi-ps:IGLS a figi-gii:PricingSource .

figi-ps:BVL3 a figi-gii:PricingSource .

figi-ps:AURA figi-gii:hasUniqueTextIdentifier "AURA" .

figi-ps:IGLS skos:prefLabel "ingalls and snyder" .

figi-ps:BVL3 skos:prefLabel "bval london 3pm" .

figi-ps:AURG a owl:NamedIndividual .

figi-ps:IGLS figi-gii:hasUniqueTextIdentifier "IGLS" .

figi-ps:BVL3 figi-gii:hasUniqueTextIdentifier "BVL3" .

figi-ps:AURG a figi-gii:PricingSource .

figi-ps:IGNI a owl:NamedIndividual .

figi-ps:BVL4 a owl:NamedIndividual .

figi-ps:AURG skos:prefLabel "auriga securities" .

figi-ps:IGNI a figi-gii:PricingSource .

figi-ps:BVL4 a figi-gii:PricingSource .

figi-ps:AURG figi-gii:hasUniqueTextIdentifier "AURG" .

figi-ps:IGNI skos:prefLabel "cs-ignition" .

figi-ps:BVL4 skos:prefLabel "bval london 4pm" .

figi-st:preference a owl:NamedIndividual .

figi-ps:IGNI figi-gii:hasUniqueTextIdentifier "IGNI" .

figi-ps:BVL4 figi-gii:hasUniqueTextIdentifier "BVL4" .

figi-st:preference a figi-gii:SecurityType .

figi-ps:IGW a owl:NamedIndividual .

figi-ps:BVLM a owl:NamedIndividual .

figi-ps:IGW a figi-gii:PricingSource .

figi-ps:BVLM a figi-gii:PricingSource ;
	skos:prefLabel "bval malaysia" .

figi-ps:IGW skos:prefLabel "invesco greatwall" .

figi-st:preference skos:definition "Preference Stock. A special type of common stock that shares in the earnings of the company, has limited voting rights, and may have a dividend preference. Preference shares may also have liquidation preference." .

figi-ps:BVLM figi-gii:hasUniqueTextIdentifier "BVLM" .

figi-ps:IGW figi-gii:hasUniqueTextIdentifier "IGW" .

figi-st:preference skos:prefLabel "preference" .

figi-ps:BVLT a owl:NamedIndividual .

figi-ps:IIB a owl:NamedIndividual .

figi-st:preference figi-gii:hasUniqueTextIdentifier "Preference" .

figi-ps:IIB a figi-gii:PricingSource .

figi-ps:AURI a owl:NamedIndividual .

figi-ps:BVLT a figi-gii:PricingSource .

figi-ps:AURI a figi-gii:PricingSource .

figi-ps:IIB skos:prefLabel "ing insurance berhad" .

figi-ps:BVLT skos:prefLabel "b-val test pricing" .

figi-ps:AURI skos:prefLabel "auriga global invest" .

figi-ps:IIB figi-gii:hasUniqueTextIdentifier "IIB" .

figi-ps:BVLT figi-gii:hasUniqueTextIdentifier "BVLT" .

figi-ps:AURI figi-gii:hasUniqueTextIdentifier "AURI" .

figi-ps:IIFL a owl:NamedIndividual .

figi-ps:BVMO a owl:NamedIndividual .

figi-st:preferred a owl:NamedIndividual .

figi-ps:BVMO a figi-gii:PricingSource .

figi-st:preferred a figi-gii:SecurityType .

figi-ps:IIFL a figi-gii:PricingSource .

figi-ps:BVMO skos:prefLabel "bolsa de montevideo" ;
	figi-gii:hasUniqueTextIdentifier "BVMO" .

figi-st:preferred skos:definition "Preferred Stock. Stock shares that represent a portion of ownership in a company, with the shares normally carrying fixed dividends. Sometimes the shares have voting rights, but not generally." .

figi-ps:IIFL skos:prefLabel "india infoline asset" .

figi-ps:BVMT a owl:NamedIndividual .

figi-st:preferred skos:prefLabel "preferred" .

figi-ps:IIFL figi-gii:hasUniqueTextIdentifier "IIFL" .

figi-ps:BVMT a figi-gii:PricingSource .

figi-st:preferred figi-gii:hasUniqueTextIdentifier "Preferred" .

figi-ps:IILM a owl:NamedIndividual .

figi-ps:BVMT skos:prefLabel "bourse de tunis bond" .

figi-ps:AURO a owl:NamedIndividual .

figi-ps:IILM a figi-gii:PricingSource .

figi-ps:BVMT figi-gii:hasUniqueTextIdentifier "BVMT" .

figi-ps:AURO a figi-gii:PricingSource .

figi-ps:IILM skos:prefLabel "int'l islamic lqdty" .

figi-ps:BVN3 a owl:NamedIndividual .

figi-ps:AURO skos:prefLabel "aurora bank fsb" .

figi-ps:IILM figi-gii:hasUniqueTextIdentifier "IILM" .

figi-ps:BVN3 a figi-gii:PricingSource .

figi-ps:AURO figi-gii:hasUniqueTextIdentifier "AURO" .

figi-ps:IIME a owl:NamedIndividual .

figi-ps:BVN3 skos:prefLabel "bval new york 3pm" .

figi-st:pres a owl:NamedIndividual .

figi-ps:IIME a figi-gii:PricingSource .

figi-ps:BVN3 figi-gii:hasUniqueTextIdentifier "BVN3" .

figi-st:pres a figi-gii:SecurityType .

figi-ps:IIME skos:prefLabel "ing asset management" .

figi-st:pres skos:definition "Not used" .

figi-ps:BVN4 a owl:NamedIndividual .

figi-ps:IIME figi-gii:hasUniqueTextIdentifier "IIME" .

figi-ps:BVN4 a figi-gii:PricingSource .

figi-st:pres skos:prefLabel "pres" .

figi-ps:IIML a owl:NamedIndividual .

figi-ps:BVN4 skos:prefLabel "bval new york 4pm" .

figi-st:pres figi-gii:hasUniqueTextIdentifier "PRES" .

figi-ps:IIML a figi-gii:PricingSource .

figi-ps:BVN4 figi-gii:hasUniqueTextIdentifier "BVN4" .

figi-ps:AUTO a owl:NamedIndividual .

figi-ps:IIML skos:prefLabel "ing inv mgmt ltd" .

figi-ps:AUTO a figi-gii:PricingSource .

figi-ps:BVNI a owl:NamedIndividual .

figi-ps:IIML figi-gii:hasUniqueTextIdentifier "IIML" .

figi-ps:AUTO skos:prefLabel "aim automation" .

figi-ps:BVNI a figi-gii:PricingSource .

figi-ps:IING a owl:NamedIndividual .

figi-ps:AUTO figi-gii:hasUniqueTextIdentifier "AUTO" .

figi-ps:BVNI skos:prefLabel "bolsa nicaragua" .

figi-ps:IING a figi-gii:PricingSource .

figi-st:prfdWrt a owl:NamedIndividual .

figi-ps:BVNI figi-gii:hasUniqueTextIdentifier "BVNI" .

figi-ps:IING skos:prefLabel "ing bank ams" .

figi-st:prfdWrt a figi-gii:SecurityType .

figi-ps:BVPA a owl:NamedIndividual .

figi-ps:IING figi-gii:hasUniqueTextIdentifier "IING" .

figi-ps:BVPA a figi-gii:PricingSource .

figi-st:prfdWrt skos:definition "Indicates that the underlying is a preferred security" .

figi-ps:IJGP a owl:NamedIndividual .

figi-ps:BVPA skos:prefLabel "bolsa de panama" .

figi-st:prfdWrt skos:prefLabel "prfd wrt" .

figi-ps:IJGP a figi-gii:PricingSource .

figi-ps:BVPA figi-gii:hasUniqueTextIdentifier "BVPA" .

figi-st:prfdWrt figi-gii:hasUniqueTextIdentifier "Prfd WRT" .

figi-ps:IJGP skos:prefLabel "ijg securities (pty)" .

figi-ps:BVSA a owl:NamedIndividual .

figi-ps:AVA a owl:NamedIndividual .

figi-ps:IJGP figi-gii:hasUniqueTextIdentifier "IJGP" .

figi-ps:BVSA a figi-gii:PricingSource .

figi-ps:AVA a figi-gii:PricingSource .

figi-ps:IKB a owl:NamedIndividual .

figi-ps:BVSA skos:prefLabel "bovespa 3" .

figi-ps:AVA skos:prefLabel "avance asset mgmt" .

figi-ps:IKB a figi-gii:PricingSource .

figi-ps:BVSA figi-gii:hasUniqueTextIdentifier "BVSA" .

figi-ps:AVA figi-gii:hasUniqueTextIdentifier "AVA" .

figi-ps:IKB skos:prefLabel "ikb" .

figi-ps:BVSP a owl:NamedIndividual .

figi-st:privPlacement a owl:NamedIndividual .

figi-ps:IKB figi-gii:hasUniqueTextIdentifier "IKB" .

figi-ps:BVSP a figi-gii:PricingSource .

figi-st:privPlacement a figi-gii:SecurityType .

figi-ps:IKFO a owl:NamedIndividual .

figi-ps:BVSP skos:prefLabel "bovespa 1" .

figi-ps:IKFO a figi-gii:PricingSource .

figi-ps:BVSP figi-gii:hasUniqueTextIdentifier "BVSP" .

figi-ps:IKFO skos:prefLabel "ikano sa" .

figi-ps:BVSS a owl:NamedIndividual .

figi-st:privPlacement skos:definition "Private Placement. A large block of securities offered for sale to an institutional investor or a small number of investors through private negotiations, as opposed to the securities being acquired in a public offering. Such placements are not registered with the SEC." .

figi-ps:BVSS a figi-gii:PricingSource .

figi-st:privPlacement skos:prefLabel "priv placement" .

figi-ps:IKFO figi-gii:hasUniqueTextIdentifier "IKFO" .

figi-st:privPlacement figi-gii:hasUniqueTextIdentifier "PRIV PLACEMENT" .

figi-ps:BVSS skos:prefLabel "bovespa 2" .

figi-ps:IKL1 a owl:NamedIndividual .

figi-ps:AVCV a owl:NamedIndividual .

figi-ps:BVSS figi-gii:hasUniqueTextIdentifier "BVSS" .

figi-ps:IKL1 a figi-gii:PricingSource .

figi-ps:AVCV a figi-gii:PricingSource .

figi-ps:BVT3 a owl:NamedIndividual .

figi-ps:IKL1 skos:prefLabel "iseb large t+1 (prc)" .

figi-ps:BVT3 a figi-gii:PricingSource .

figi-ps:AVCV skos:prefLabel "avc valores" .

figi-ps:IKL1 figi-gii:hasUniqueTextIdentifier "IKL1" .

figi-ps:BVT3 skos:prefLabel "bval tokyo 3pm" .

figi-ps:AVCV figi-gii:hasUniqueTextIdentifier "AVCV" .

figi-ps:IKS a owl:NamedIndividual .

figi-ps:BVT3 figi-gii:hasUniqueTextIdentifier "BVT3" .

figi-ps:IKS a figi-gii:PricingSource .

figi-st:private a owl:NamedIndividual .

figi-ps:BVT4 a owl:NamedIndividual .

figi-ps:IKS skos:prefLabel "iks kb invest" .

figi-st:private a figi-gii:SecurityType .

figi-ps:BVT4 a figi-gii:PricingSource .

figi-ps:IKS figi-gii:hasUniqueTextIdentifier "IKS" .

figi-ps:BVT4 skos:prefLabel "bval tokyo 4pm" .

figi-ps:IKS1 a owl:NamedIndividual .

figi-ps:BVT4 figi-gii:hasUniqueTextIdentifier "BVT4" .

figi-ps:IKS1 a figi-gii:PricingSource .

figi-ps:BVUY a owl:NamedIndividual .

figi-ps:IKS1 skos:prefLabel "iseb small t+1 (prc)" .

figi-ps:BVUY a figi-gii:PricingSource .

figi-st:private skos:definition "a preferred security issued as a private placement (not registered with SEC). This also includes 144A securities that typically get exchanged into public securities once the company has the documentation ready for the SEC. 144A securities allow issuing entities to obtain their money be selling the securities and then typically have 90-180 days to file the correct documentation with the SEC." .

figi-ps:IKS1 figi-gii:hasUniqueTextIdentifier "IKS1" .

figi-ps:BVUY skos:prefLabel "bolsa de valores de" .

figi-st:private skos:prefLabel "private" .

figi-ps:ILME a owl:NamedIndividual .

figi-ps:BVUY figi-gii:hasUniqueTextIdentifier "BVUY" .

figi-st:private figi-gii:hasUniqueTextIdentifier "PRIVATE" .

figi-ps:ILME a figi-gii:PricingSource .

figi-ps:BXAB a owl:NamedIndividual .

figi-ps:AVHK a owl:NamedIndividual .

figi-ps:ILME skos:prefLabel "icap lme" .

figi-ps:BXAB a figi-gii:PricingSource .

figi-ps:AVHK a figi-gii:PricingSource .

figi-ps:ILME figi-gii:hasUniqueTextIdentifier "ILME" .

figi-ps:BXAB skos:prefLabel "barclays capital" .

figi-ps:AVHK skos:prefLabel "aviate global" .

figi-ps:ILQD a owl:NamedIndividual .

figi-ps:BXAB figi-gii:hasUniqueTextIdentifier "BXAB" .

figi-ps:AVHK figi-gii:hasUniqueTextIdentifier "AVHK" .

figi-ps:ILQD a figi-gii:PricingSource .

figi-ps:BXAC a owl:NamedIndividual .

figi-st:privateComp a owl:NamedIndividual .

figi-ps:ILQD skos:prefLabel "illiquidx" .

figi-ps:BXAC a figi-gii:PricingSource .

figi-st:privateComp a figi-gii:SecurityType .

figi-ps:ILQD figi-gii:hasUniqueTextIdentifier "ILQD" .

figi-ps:BXAC skos:prefLabel "barclays capital sg" .

figi-ps:ILSB a owl:NamedIndividual .

figi-ps:BXAC figi-gii:hasUniqueTextIdentifier "BXAC" .

figi-ps:ILSB a figi-gii:PricingSource .

figi-ps:BXAP a owl:NamedIndividual .

figi-ps:ILSB skos:prefLabel "ils brokers ltd" .

figi-ps:BXAP a figi-gii:PricingSource .

figi-st:privateComp skos:definition "Private Company: A company whose ownership is private. As a result, it does not need to meet the strict Securities and Exchange Commission filing requirements of public companies. Private companies may issue stock and have shareholders. However, their shares do not trade on public exchanges and are not issued through an initial public offering. In general, the shares of these businesses are less liquid and the values are difficult to determine." .

figi-ps:ILSB figi-gii:hasUniqueTextIdentifier "ILSB" .

figi-ps:BXAP skos:prefLabel "barclays sec japan" .

figi-st:privateComp skos:prefLabel "private comp" .

figi-ps:IMBM a owl:NamedIndividual .

figi-ps:BXAP figi-gii:hasUniqueTextIdentifier "BXAP" .

figi-st:privateComp figi-gii:hasUniqueTextIdentifier "Private Comp" .

figi-ps:IMBM a figi-gii:PricingSource .

figi-ps:BXCA a owl:NamedIndividual .

figi-st:privateEqty a owl:NamedIndividual .

figi-ps:IMBM skos:prefLabel "internl moscow bank" .

figi-ps:BXCA a figi-gii:PricingSource .

figi-st:privateEqty a figi-gii:SecurityType .

figi-ps:IMBM figi-gii:hasUniqueTextIdentifier "IMBM" .

figi-ps:BXCA skos:prefLabel "barclays capital ac" .

figi-ps:IMI a owl:NamedIndividual .

figi-ps:BXCA figi-gii:hasUniqueTextIdentifier "BXCA" .

figi-ps:IMI a figi-gii:PricingSource .

figi-ps:BXCE a owl:NamedIndividual .

figi-ps:IMI skos:prefLabel "banca imi" .

figi-ps:BXCE a figi-gii:PricingSource .

figi-ps:IMI figi-gii:hasUniqueTextIdentifier "IMI" .

figi-ps:BXCE skos:prefLabel "barclays bank" ;
	figi-gii:hasUniqueTextIdentifier "BXCE" .

figi-ps:IMIG a owl:NamedIndividual , figi-gii:PricingSource .

figi-ps:BXEC a owl:NamedIndividual .

figi-ps:IMIG skos:prefLabel "banca imi imig" .

figi-ps:BXEC a figi-gii:PricingSource .

figi-st:privateEqty skos:definition "Equity capital that is not quoted on a public exchange. Private equity consists of investors and funds that make investments directly into private companies or conduct buyouts of public companies that result in a delisting of public equity. Capital for private equity is raised from retail and institutional investors, and can be used to fund new technologies, expand working capital within an owned company, make acquisitions, or to strengthen a balance sheet. The majority of private equity consists of institutional investors and accredited investors who can commit large sums of money for long periods of time. Private equity investments often demand long holding periods to allow for a turnaround of a distressed company or a liquidity event such as an IPO or sale to a public company." .

figi-ps:BXEC skos:prefLabel "barclays bank plc" .

figi-ps:IMIG figi-gii:hasUniqueTextIdentifier "IMIG" .

figi-st:privateEqty skos:prefLabel "private eqty" .

figi-ps:BXEC figi-gii:hasUniqueTextIdentifier "BXEC" .

figi-ps:IMIJ a owl:NamedIndividual .

figi-st:privateEqty figi-gii:hasUniqueTextIdentifier "Private Eqty" .

figi-ps:IMIJ a figi-gii:PricingSource .

figi-ps:BXEM a owl:NamedIndividual .

figi-ps:AVON a owl:NamedIndividual .

figi-ps:BXEM a figi-gii:PricingSource .

figi-ps:IMIJ skos:prefLabel "bank imi cds" .

figi-ps:AVON a figi-gii:PricingSource .

figi-ps:BXEM skos:prefLabel "barclays bank em" .

figi-ps:IMIJ figi-gii:hasUniqueTextIdentifier "IMIJ" .

figi-ps:AVON skos:prefLabel "avondale partners" .

figi-ps:BXEM figi-gii:hasUniqueTextIdentifier "BXEM" .

figi-ps:IMIM a owl:NamedIndividual .

figi-ps:AVON figi-gii:hasUniqueTextIdentifier "AVON" .

figi-ps:IMIM a figi-gii:PricingSource .

figi-ps:BXEP a owl:NamedIndividual .

figi-st:promissoryNote a owl:NamedIndividual .

figi-ps:BXEP a figi-gii:PricingSource .

figi-st:promissoryNote a figi-gii:SecurityType .

figi-ps:IMIM skos:prefLabel "banca imi mortgage" .

figi-ps:BXEP skos:prefLabel "barclays capital ep" .

figi-ps:IMIM figi-gii:hasUniqueTextIdentifier "IMIM" .

figi-ps:BXEP figi-gii:hasUniqueTextIdentifier "BXEP" .

figi-st:promissoryNote skos:definition "Promissory Note. A written commitment to pay another party a specific amount of money by a specific date. A note, for example, is a promissory note." .

figi-ps:IMIR a owl:NamedIndividual .

figi-ps:BXEQ a owl:NamedIndividual .

figi-st:promissoryNote skos:prefLabel "promissory note" .

figi-ps:IMIR a figi-gii:PricingSource .

figi-ps:BXEQ a figi-gii:PricingSource .

figi-st:promissoryNote figi-gii:hasUniqueTextIdentifier "PROMISSORY NOTE" .

figi-ps:IMIR skos:prefLabel "banca imi pricing" .

figi-ps:BXEQ skos:prefLabel "barclays - equities" .

figi-ps:AXAC a owl:NamedIndividual .

figi-ps:IMIR figi-gii:hasUniqueTextIdentifier "IMIR" .

figi-ps:BXEQ figi-gii:hasUniqueTextIdentifier "BXEQ" .

figi-ps:AXAC a figi-gii:PricingSource .

figi-ps:IMIT a owl:NamedIndividual .

figi-ps:BXFR a owl:NamedIndividual .

figi-ps:AXAC skos:prefLabel "abn amro sgp" .

figi-ps:IMIT a figi-gii:PricingSource .

figi-ps:BXFR a figi-gii:PricingSource .

figi-ps:AXAC figi-gii:hasUniqueTextIdentifier "AXAC" .

figi-ps:IMIT skos:prefLabel "banca imi auto ex" .

figi-ps:BXFR skos:prefLabel "bxfr internal" .

figi-ps:AXCB a owl:NamedIndividual .

figi-ps:IMIT figi-gii:hasUniqueTextIdentifier "IMIT" .

figi-ps:BXFR figi-gii:hasUniqueTextIdentifier "BXFR" .

figi-ps:AXCB a figi-gii:PricingSource .

figi-ps:IMIX a owl:NamedIndividual .

figi-ps:BXIS a owl:NamedIndividual .

figi-ps:AXCB skos:prefLabel "abn amro bank london" .

figi-ps:IMIX a figi-gii:PricingSource .

figi-ps:BXIS a figi-gii:PricingSource .

figi-ps:AXCB skos:prefLabel "rbs nv london" .

figi-ps:IMIX skos:prefLabel "banca imi internal" .

figi-ps:BXIS skos:prefLabel "barclays inv sol" .

figi-ps:AXCB figi-gii:hasUniqueTextIdentifier "AXCB" .

figi-ps:IMIX figi-gii:hasUniqueTextIdentifier "IMIX" .

figi-ps:BXIS figi-gii:hasUniqueTextIdentifier "BXIS" .

figi-st:propertySwap a owl:NamedIndividual .

figi-ps:IMKL a owl:NamedIndividual .

figi-st:propertySwap a figi-gii:SecurityType .

figi-ps:BXJB a owl:NamedIndividual .

figi-ps:IMKL a figi-gii:PricingSource .

figi-ps:BXJB a figi-gii:PricingSource .

figi-st:propertySwap skos:definition "Exchange the return on a real estate index with a funding leg" .

figi-ps:IMKL skos:prefLabel "istanbul exch large" .

figi-ps:BXJB skos:prefLabel "barclays sec japan" .

figi-st:propertySwap skos:prefLabel "property swap" .

figi-ps:IMKL figi-gii:hasUniqueTextIdentifier "IMKL" .

figi-ps:BXJB figi-gii:hasUniqueTextIdentifier "BXJB" .

figi-st:propertySwap figi-gii:hasUniqueTextIdentifier "PROPERTY SWAP" .

figi-ps:IMKS a owl:NamedIndividual .

figi-ps:BXJP a owl:NamedIndividual .

figi-ps:AXGP a owl:NamedIndividual .

figi-ps:IMKS a figi-gii:PricingSource .

figi-ps:AXGP a figi-gii:PricingSource .

figi-ps:BXJP a figi-gii:PricingSource .

figi-ps:IMKS skos:prefLabel "istanbul exch small" .

figi-ps:AXGP skos:prefLabel "access securities" .

figi-ps:BXJP skos:prefLabel "barclays jgb bxjp" .

figi-ps:IMKS figi-gii:hasUniqueTextIdentifier "IMKS" .

figi-ps:AXGP figi-gii:hasUniqueTextIdentifier "AXGP" .

figi-ps:BXJP figi-gii:hasUniqueTextIdentifier "BXJP" .

figi-ps:IMPC a owl:NamedIndividual .

figi-st:provTBill a owl:NamedIndividual .

figi-ps:BXKB a owl:NamedIndividual .

figi-ps:IMPC a figi-gii:PricingSource .

figi-ps:BXKB a figi-gii:PricingSource .

figi-st:provTBill a figi-gii:SecurityType .

figi-ps:IMPC skos:prefLabel "imperial capital" .

figi-ps:BXKB skos:prefLabel "barclays krw bonds" .

figi-st:provTBill skos:definition "Commercial Paper issued by Canadian Provinces" .

figi-ps:IMPC figi-gii:hasUniqueTextIdentifier "IMPC" .

figi-ps:BXKB figi-gii:hasUniqueTextIdentifier "BXKB" .

figi-st:provTBill skos:prefLabel "prov t-bill" .

figi-ps:IMR1 a owl:NamedIndividual .

figi-ps:BXLN a owl:NamedIndividual .

figi-st:provTBill figi-gii:hasUniqueTextIdentifier "PROV T-BILL" .

figi-ps:IMR1 a figi-gii:PricingSource .

figi-ps:BXLN a figi-gii:PricingSource .

figi-ps:AXPG a owl:NamedIndividual .

figi-ps:IMR1 skos:prefLabel "imarex - $/bbl" .

figi-ps:AXPG a figi-gii:PricingSource .

figi-ps:BXLN skos:prefLabel "barclays loans" .

figi-ps:IMR1 figi-gii:hasUniqueTextIdentifier "IMR1" .

figi-ps:AXPG skos:prefLabel "abn amro pakistan" .

figi-ps:BXLN figi-gii:hasUniqueTextIdentifier "BXLN" .

figi-ps:IMR2 a owl:NamedIndividual .

figi-ps:AXPG figi-gii:hasUniqueTextIdentifier "AXPG" .

figi-ps:BXNT a owl:NamedIndividual .

figi-ps:IMR2 a figi-gii:PricingSource .

figi-ps:BXNT a figi-gii:PricingSource .

figi-st:prvtCmoFlt a owl:NamedIndividual .

figi-ps:IMR2 skos:prefLabel "imarex - $/day" .

figi-st:prvtCmoFlt a figi-gii:SecurityType .

figi-ps:BXNT skos:prefLabel "barcap struc. notes" .

figi-ps:IMR2 figi-gii:hasUniqueTextIdentifier "IMR2" .

figi-st:prvtCmoFlt skos:definition "Privately Issued CMO Floating Rate Security" .

figi-ps:BXNT figi-gii:hasUniqueTextIdentifier "BXNT" .

figi-ps:IMR3 a owl:NamedIndividual .

figi-st:prvtCmoFlt skos:prefLabel "prvt cmo flt" .

figi-ps:BXPM a owl:NamedIndividual .

figi-ps:IMR3 a figi-gii:PricingSource .

figi-st:prvtCmoFlt figi-gii:hasUniqueTextIdentifier "Prvt CMO FLT" .

figi-ps:BXPM a figi-gii:PricingSource .

figi-ps:IMR3 skos:prefLabel "imarex - ws" .

figi-ps:AXUS a owl:NamedIndividual .

figi-ps:BXPM skos:prefLabel "barcap metals" .

figi-ps:IMR3 figi-gii:hasUniqueTextIdentifier "IMR3" .

figi-ps:AXUS a figi-gii:PricingSource .

figi-ps:BXPM figi-gii:hasUniqueTextIdentifier "BXPM" .

figi-ps:IMRX a owl:NamedIndividual .

figi-ps:AXUS skos:prefLabel "abn amro ldn tsy" .

figi-ps:BXSA a owl:NamedIndividual .

figi-ps:IMRX a figi-gii:PricingSource .

figi-ps:BXSA a figi-gii:PricingSource .

figi-ps:AXUS figi-gii:hasUniqueTextIdentifier "AXUS" .

figi-ps:IMRX skos:prefLabel "imarex" .

figi-ps:BXSA skos:prefLabel "bond exch south afr" .

figi-st:prvtCmoInv a owl:NamedIndividual .

figi-ps:IMRX figi-gii:hasUniqueTextIdentifier "IMRX" .

figi-ps:BXSA figi-gii:hasUniqueTextIdentifier "BXSA" .

figi-st:prvtCmoInv a figi-gii:SecurityType .

figi-ps:IMTS a owl:NamedIndividual .

figi-ps:BXUC a owl:NamedIndividual .

figi-st:prvtCmoInv skos:definition "Privately Issued CMO Inverse Floating Rate Security" .

figi-ps:BXUC a figi-gii:PricingSource .

figi-st:prvtCmoInv skos:prefLabel "prvt cmo inv" .

figi-ps:IMTS a figi-gii:PricingSource .

figi-st:prvtCmoInv figi-gii:hasUniqueTextIdentifier "Prvt CMO INV" .

figi-ps:BXUC skos:prefLabel "bxuc barclays corps" .

figi-ps:IMTS skos:prefLabel "ireland mts" .

figi-ps:AZI a owl:NamedIndividual .

figi-ps:BXUC figi-gii:hasUniqueTextIdentifier "BXUC" .

figi-ps:IMTS figi-gii:hasUniqueTextIdentifier "IMTS" .

figi-ps:AZI a figi-gii:PricingSource .

figi-ps:BYBL a owl:NamedIndividual .

figi-ps:IMYL a owl:NamedIndividual .

figi-ps:BYBL a figi-gii:PricingSource .

figi-ps:AZI skos:prefLabel "azimut" .

figi-ps:IMYL a figi-gii:PricingSource .

figi-ps:BYBL skos:prefLabel "byblos bank sal" .

figi-ps:AZI figi-gii:hasUniqueTextIdentifier "AZI" .

figi-ps:IMYL skos:prefLabel "iseb large (yields)" .

figi-ps:BYBL figi-gii:hasUniqueTextIdentifier "BYBL" .

figi-st:prvtCmoIo a owl:NamedIndividual .

figi-ps:IMYL figi-gii:hasUniqueTextIdentifier "IMYL" .

figi-st:prvtCmoIo a figi-gii:SecurityType .

figi-ps:BYEM a owl:NamedIndividual .

figi-ps:IMYS a owl:NamedIndividual .

figi-ps:BYEM a figi-gii:PricingSource .

figi-st:prvtCmoIo skos:definition "Privately Issued CMO Interest Only Security" .

figi-ps:IMYS a figi-gii:PricingSource .

figi-ps:BYEM skos:prefLabel "barcap emrgmrkt" .

figi-st:prvtCmoIo skos:prefLabel "prvt cmo io" .

figi-ps:IMYS skos:prefLabel "iseb small (yields)" .

figi-ps:BYEM figi-gii:hasUniqueTextIdentifier "BYEM" .

figi-st:prvtCmoIo figi-gii:hasUniqueTextIdentifier "Prvt CMO IO" .

figi-ps:IMYS figi-gii:hasUniqueTextIdentifier "IMYS" .

figi-ps:BYRE a owl:NamedIndividual .

figi-ps:AZMF a owl:NamedIndividual .

figi-ps:BYRE a figi-gii:PricingSource .

figi-ps:AZMF a figi-gii:PricingSource .

figi-ps:INAU a owl:NamedIndividual .

figi-ps:BYRE skos:prefLabel "bolsaandrenta" .

figi-ps:AZMF skos:prefLabel "allianz zb doo" .

figi-ps:INAU a figi-gii:PricingSource .

figi-ps:BYRE figi-gii:hasUniqueTextIdentifier "BYRE" .

figi-ps:AZMF figi-gii:hasUniqueTextIdentifier "AZMF" .

figi-ps:INAU skos:prefLabel "ing investment manag" .

figi-ps:BZAS a owl:NamedIndividual .

figi-st:prvtCmoOther a owl:NamedIndividual .

figi-ps:INAU figi-gii:hasUniqueTextIdentifier "INAU" .

figi-ps:BZAS a figi-gii:PricingSource .

figi-st:prvtCmoOther a figi-gii:SecurityType .

figi-ps:INAX a owl:NamedIndividual .

figi-ps:BZAS skos:prefLabel "bzw asia ltd" .

figi-ps:INAX a figi-gii:PricingSource .

figi-st:prvtCmoOther skos:definition "Privately Issued CMO Other type (Less common type of security such as PAC or Sequential)" .

figi-ps:BZAS figi-gii:hasUniqueTextIdentifier "BZAS" .

figi-ps:INAX skos:prefLabel "ing bank belgium" .

figi-st:prvtCmoOther skos:prefLabel "prvt cmo other" .

figi-ps:CA a owl:NamedIndividual .

figi-ps:INAX figi-gii:hasUniqueTextIdentifier "INAX" .

figi-ps:CA a figi-gii:PricingSource .

figi-st:prvtCmoOther figi-gii:hasUniqueTextIdentifier "Prvt CMO Other" .

figi-ps:INBK a owl:NamedIndividual .

figi-ps:CA skos:prefLabel "camfunds" .

figi-ps:INBK a figi-gii:PricingSource .

figi-ps:AZOA a owl:NamedIndividual .

figi-ps:CA figi-gii:hasUniqueTextIdentifier "CA" .

figi-ps:INBK skos:prefLabel "interbank" .

figi-ps:AZOA a figi-gii:PricingSource .

figi-ps:CAAA a owl:NamedIndividual .

figi-ps:INBK figi-gii:hasUniqueTextIdentifier "INBK" .

figi-ps:AZOA skos:prefLabel "allianz of america" .

figi-ps:CAAA a figi-gii:PricingSource .

figi-ps:INBU a owl:NamedIndividual .

figi-ps:AZOA figi-gii:hasUniqueTextIdentifier "AZOA" .

figi-ps:CAAA skos:prefLabel "carnegie asa" .

figi-ps:INBU a figi-gii:PricingSource .

figi-ps:CAAA figi-gii:hasUniqueTextIdentifier "CAAA" .

figi-st:prvtCmoPo a owl:NamedIndividual .

figi-ps:INBU skos:prefLabel "ing bank bucharest" .

figi-st:prvtCmoPo a figi-gii:SecurityType .

figi-ps:CABG a owl:NamedIndividual .

figi-ps:INBU figi-gii:hasUniqueTextIdentifier "INBU" .

figi-ps:CABG a figi-gii:PricingSource .

figi-st:prvtCmoPo skos:definition "Privately Issued CMO Principal Only Security" .

figi-ps:INBZ a owl:NamedIndividual .

figi-ps:CABG skos:prefLabel "caboto-gruppo intesa" .

figi-st:prvtCmoPo skos:prefLabel "prvt cmo po" .

figi-ps:INBZ a figi-gii:PricingSource .

figi-ps:CABG figi-gii:hasUniqueTextIdentifier "CABG" .

figi-st:prvtCmoPo figi-gii:hasUniqueTextIdentifier "Prvt CMO PO" .

figi-ps:INBZ skos:prefLabel "ing bk" .

figi-ps:CABI a owl:NamedIndividual .

figi-ps:AZTO a owl:NamedIndividual .

figi-ps:INBZ figi-gii:hasUniqueTextIdentifier "INBZ" .

figi-ps:CABI a figi-gii:PricingSource .

figi-ps:AZTO a figi-gii:PricingSource .

figi-ps:INCA a owl:NamedIndividual .

figi-ps:CABI skos:prefLabel "caixa banco invest" .

figi-ps:AZTO skos:prefLabel "arizona st treasurer" .

figi-ps:INCA a figi-gii:PricingSource .

figi-ps:CABI figi-gii:hasUniqueTextIdentifier "CABI" .

figi-ps:AZTO figi-gii:hasUniqueTextIdentifier "AZTO" .

figi-ps:INCA skos:prefLabel "incapital" .

figi-ps:CABM a owl:NamedIndividual .

figi-st:prvtCmoZ a owl:NamedIndividual .

figi-ps:INCA figi-gii:hasUniqueTextIdentifier "INCA" .

figi-st:prvtCmoZ a figi-gii:SecurityType .

figi-ps:CABM a figi-gii:PricingSource .

figi-ps:INCB a owl:NamedIndividual .

figi-st:prvtCmoZ skos:definition "Privately Issued CMO Z (Accrual Bond)" .

figi-ps:CABM skos:prefLabel "caboto - emer mkts" .

figi-ps:INCB a figi-gii:PricingSource .

figi-st:prvtCmoZ skos:prefLabel "prvt cmo z" .

figi-ps:CABM figi-gii:hasUniqueTextIdentifier "CABM" .

figi-ps:INCB skos:prefLabel "incapital" .

figi-st:prvtCmoZ figi-gii:hasUniqueTextIdentifier "Prvt CMO Z" .

figi-ps:CABP a owl:NamedIndividual .

figi-ps:INCB figi-gii:hasUniqueTextIdentifier "INCB" .

figi-ps:CABP a figi-gii:PricingSource .

figi-ps:BA a owl:NamedIndividual .

figi-ps:INCE a owl:NamedIndividual .

figi-ps:CABP skos:prefLabel "caboto-cabp" .

figi-ps:BA a figi-gii:PricingSource .

figi-ps:INCE a figi-gii:PricingSource .

figi-ps:CABP figi-gii:hasUniqueTextIdentifier "CABP" .

figi-ps:BA skos:prefLabel "unicredit" .

figi-ps:INCE skos:prefLabel "incapital europe" .

figi-ps:CABR a owl:NamedIndividual .

figi-ps:BA figi-gii:hasUniqueTextIdentifier "BA" .

figi-ps:INCE figi-gii:hasUniqueTextIdentifier "INCE" .

figi-ps:CABR a figi-gii:PricingSource .

figi-st:public a owl:NamedIndividual .

figi-ps:INCH a owl:NamedIndividual .

figi-st:public a figi-gii:SecurityType .

figi-ps:CABR skos:prefLabel "cabrera capital mkts" .

figi-ps:INCH a figi-gii:PricingSource .

figi-st:public skos:definition "non private issue" .

figi-ps:CABR figi-gii:hasUniqueTextIdentifier "CABR" .

figi-ps:INCH skos:prefLabel "ing chb sec invt" .

figi-st:public skos:prefLabel "public" .

figi-ps:CABS a owl:NamedIndividual .

figi-ps:INCH figi-gii:hasUniqueTextIdentifier "INCH" .

figi-st:public figi-gii:hasUniqueTextIdentifier "PUBLIC" .

figi-ps:CABS a figi-gii:PricingSource .

figi-ps:INCO a owl:NamedIndividual .

figi-ps:CABS skos:prefLabel "cabrera llc" .

figi-ps:BAAB a owl:NamedIndividual .

figi-ps:INCO a figi-gii:PricingSource .

figi-ps:CABS figi-gii:hasUniqueTextIdentifier "CABS" .

figi-ps:BAAB a figi-gii:PricingSource .

figi-ps:INCO skos:prefLabel "interbolsa" .

figi-ps:CAC a owl:NamedIndividual .

figi-ps:BAAB skos:prefLabel "bank of america mtge" .

figi-ps:INCO figi-gii:hasUniqueTextIdentifier "INCO" .

figi-ps:CAC a figi-gii:PricingSource .

figi-ps:BAAB figi-gii:hasUniqueTextIdentifier "BAAB" .

figi-ps:INCX a owl:NamedIndividual .

figi-ps:CAC skos:prefLabel "caixa de catalunya" .

figi-ps:INCX a figi-gii:PricingSource .

figi-st:pvtEqtyFund a owl:NamedIndividual .

figi-ps:CAC figi-gii:hasUniqueTextIdentifier "CAC" .

figi-st:pvtEqtyFund a figi-gii:SecurityType .

figi-ps:INCX skos:prefLabel "intercontl exchange" .

figi-ps:CACB a owl:NamedIndividual , figi-gii:PricingSource .

figi-ps:INCX figi-gii:hasUniqueTextIdentifier "INCX" .

figi-ps:CACB skos:prefLabel "credit agricole cib" .

figi-ps:INDB a owl:NamedIndividual .

figi-ps:CACB figi-gii:hasUniqueTextIdentifier "CACB" .

figi-ps:INDB a figi-gii:PricingSource .

figi-ps:CACD a owl:NamedIndividual .

figi-ps:INDB skos:prefLabel "indusind bank" .

figi-ps:CACD a figi-gii:PricingSource .

figi-ps:INDB figi-gii:hasUniqueTextIdentifier "INDB" .

figi-ps:CACD skos:prefLabel "ca-cib mkt value cdo" .

figi-ps:INDC a owl:NamedIndividual .

figi-ps:CACD figi-gii:hasUniqueTextIdentifier "CACD" .

figi-ps:INDC a figi-gii:PricingSource .

figi-ps:CADE a owl:NamedIndividual .

figi-ps:INDC skos:prefLabel "industrial bank co" .

figi-ps:CADE a figi-gii:PricingSource .

figi-ps:INDC figi-gii:hasUniqueTextIdentifier "INDC" .

figi-ps:CADE skos:prefLabel "cec bank" ;
	figi-gii:hasUniqueTextIdentifier "CADE" .

figi-ps:INDI a owl:NamedIndividual .

figi-st:pvtEqtyFund skos:definition "A private equity fund is a collective investment scheme used for making investments in various equity (and to a lesser extent debt) securities according to one of the investment strategies associated with private equity. Private equity funds are typically limited partnerships with a fixed term of 10 years (often with annual extensions). At inception, institutional investors make an unfunded commitment to the limited partnership, which is then drawn over the term of the fund. From investors point of view funds can be traditional where all the investors invest with equal terms or asymmetric where different investors have different terms." .

figi-ps:CADO a owl:NamedIndividual .

figi-ps:INDI a figi-gii:PricingSource .

figi-st:pvtEqtyFund skos:prefLabel "pvt eqty fund" .

figi-ps:CADO a figi-gii:PricingSource .

figi-ps:INDI skos:prefLabel "exotix limited" .

figi-st:pvtEqtyFund figi-gii:hasUniqueTextIdentifier "Pvt Eqty Fund" .

figi-ps:CADO skos:prefLabel "ca-cib cdos" .

figi-ps:INDI figi-gii:hasUniqueTextIdentifier "INDI" .

figi-ps:BAAD a owl:NamedIndividual .

figi-ps:CADO figi-gii:hasUniqueTextIdentifier "CADO" .

figi-ps:BAAD a figi-gii:PricingSource .

figi-ps:INDN a owl:NamedIndividual .

figi-ps:CAED a owl:NamedIndividual .

figi-ps:BAAD skos:prefLabel "baader bank ag" .

figi-ps:INDN a figi-gii:PricingSource .

figi-ps:CAED a figi-gii:PricingSource .

figi-ps:BAAD figi-gii:hasUniqueTextIdentifier "BAAD" .

figi-ps:INDN skos:prefLabel "cnbond icbc" .

figi-ps:CAED skos:prefLabel "ca-cib eqty derivs" .

figi-st:quarterlySwap a owl:NamedIndividual .

figi-ps:INDN figi-gii:hasUniqueTextIdentifier "INDN" .

figi-ps:CAED figi-gii:hasUniqueTextIdentifier "CAED" .

figi-st:quarterlySwap a figi-gii:SecurityType .

figi-ps:INDS a owl:NamedIndividual .

figi-ps:CAEG a owl:NamedIndividual .

figi-ps:INDS a figi-gii:PricingSource .

figi-st:quarterlySwap skos:definition "Swap with a quarterly payment frequency" .

figi-ps:CAEG a figi-gii:PricingSource .

figi-ps:INDS skos:prefLabel "cfet industrial bank" .

figi-ps:CAEG skos:prefLabel "credit agricole" .

figi-st:quarterlySwap skos:prefLabel "quarterly swap" .

figi-ps:INDS figi-gii:hasUniqueTextIdentifier "INDS" .

figi-ps:CAEG figi-gii:hasUniqueTextIdentifier "CAEG" .

figi-st:quarterlySwap figi-gii:hasUniqueTextIdentifier "QUARTERLY SWAP" .

figi-ps:INDU a owl:NamedIndividual .

figi-ps:CAEI a owl:NamedIndividual .

figi-ps:INDU a figi-gii:PricingSource .

figi-ps:CAEI a figi-gii:PricingSource .

figi-ps:BAAM a owl:NamedIndividual .

figi-ps:INDU skos:prefLabel "cfet icbc" .

figi-ps:CAEI skos:prefLabel "credit agricole" .

figi-ps:BAAM a figi-gii:PricingSource .

figi-ps:INDU figi-gii:hasUniqueTextIdentifier "INDU" .

figi-ps:CAEI figi-gii:hasUniqueTextIdentifier "CAEI" .

figi-ps:BAAM skos:prefLabel "barep am" .

figi-ps:INDY a owl:NamedIndividual .

figi-ps:BAAM figi-gii:hasUniqueTextIdentifier "BAAM" .

figi-ps:CAEN a owl:NamedIndividual .

figi-ps:INDY a figi-gii:PricingSource .

figi-ps:CAEN a figi-gii:PricingSource .

figi-st:rdc a owl:NamedIndividual .

figi-ps:INDY skos:prefLabel "independent brokers" .

figi-st:rdc a figi-gii:SecurityType .

figi-ps:CAEN skos:prefLabel "credit agricole (hk)" .

figi-ps:INDY figi-gii:hasUniqueTextIdentifier "INDY" .

figi-ps:CAEN figi-gii:hasUniqueTextIdentifier "CAEN" .

figi-ps:INEM a owl:NamedIndividual .

figi-ps:CAF a owl:NamedIndividual .

figi-st:rdc skos:definition "Russian Depositary Certificate. The Russian Depositary Certificates represent fractional undivided interests in Sub-Trusts of the Russian Depositary." .

figi-ps:CAF a figi-gii:PricingSource .

figi-ps:INEM a figi-gii:PricingSource .

figi-ps:CAF skos:prefLabel "corporacion adina" .

figi-ps:INEM skos:prefLabel "ing financial market" .

figi-ps:CAF figi-gii:hasUniqueTextIdentifier "CAF" .

figi-ps:INEM figi-gii:hasUniqueTextIdentifier "INEM" .

figi-ps:CAGB a owl:NamedIndividual .

figi-ps:INFB a owl:NamedIndividual .

figi-st:rdc skos:prefLabel "rdc" .

figi-ps:CAGB a figi-gii:PricingSource .

figi-ps:INFB a figi-gii:PricingSource .

figi-st:rdc figi-gii:hasUniqueTextIdentifier "RDC" .

figi-ps:CAGB skos:prefLabel "ca-cib, hong kong" .

figi-ps:INFB skos:prefLabel "infa energy" .

figi-ps:BAAN a owl:NamedIndividual .

figi-ps:CAGB figi-gii:hasUniqueTextIdentifier "CAGB" .

figi-ps:INFB figi-gii:hasUniqueTextIdentifier "INFB" .

figi-ps:BAAN a figi-gii:PricingSource .

figi-ps:CAHK a owl:NamedIndividual .

figi-ps:INFG a owl:NamedIndividual .

figi-ps:CAHK a figi-gii:PricingSource .

figi-ps:BAAN skos:prefLabel "bank of america boom" .

figi-ps:INFG a figi-gii:PricingSource .

figi-ps:CAHK skos:prefLabel "ca-cib hk" .

figi-ps:BAAN figi-gii:hasUniqueTextIdentifier "BAAN" .

figi-ps:INFG skos:prefLabel "inforalgo toms" .

figi-ps:CAHK figi-gii:hasUniqueTextIdentifier "CAHK" .

figi-ps:BAAO a owl:NamedIndividual .

figi-ps:INFG figi-gii:hasUniqueTextIdentifier "INFG" .

figi-ps:BAAO a figi-gii:PricingSource .

figi-ps:CAIG a owl:NamedIndividual .

figi-ps:INFI a owl:NamedIndividual .

figi-ps:CAIG a figi-gii:PricingSource .

figi-ps:BAAO skos:prefLabel "boa-agency offerings" .

figi-ps:INFI a figi-gii:PricingSource .

figi-ps:CAIG skos:prefLabel "citigroup aig" .

figi-ps:BAAO figi-gii:hasUniqueTextIdentifier "BAAO" .

figi-ps:INFI skos:prefLabel "infinity cap mkts" .

figi-ps:CAIG figi-gii:hasUniqueTextIdentifier "CAIG" .

figi-st:receipt a owl:NamedIndividual .

figi-ps:INFI figi-gii:hasUniqueTextIdentifier "INFI" .

figi-st:receipt a figi-gii:SecurityType .

figi-ps:CAIN a owl:NamedIndividual .

figi-ps:INFL a owl:NamedIndividual .

figi-ps:CAIN a figi-gii:PricingSource .

figi-ps:INFL a figi-gii:PricingSource .

figi-st:receipt skos:definition "Certificates issued by a bank, representing shares held by the bank, usually by a branch or correspondent in the country of issue." .

figi-ps:CAIN skos:prefLabel "ca-cib - indicative" .

figi-ps:INFL skos:prefLabel "inflection asset mgt" .

figi-st:receipt skos:prefLabel "receipt" .

figi-ps:CAIN figi-gii:hasUniqueTextIdentifier "CAIN" .

figi-ps:INFL figi-gii:hasUniqueTextIdentifier "INFL" .

figi-st:receipt figi-gii:hasUniqueTextIdentifier "Receipt" .

figi-ps:CAIR a owl:NamedIndividual .

figi-ps:ING a owl:NamedIndividual .

figi-ps:BAAS a owl:NamedIndividual .

figi-ps:CAIR a figi-gii:PricingSource .

figi-ps:ING a figi-gii:PricingSource .

figi-ps:BAAS a figi-gii:PricingSource .

figi-ps:CAIR skos:prefLabel "calyon derivatives" .

figi-ps:ING skos:prefLabel "i n g bank" .

figi-ps:BAAS skos:prefLabel "bofaml asia" .

figi-ps:CAIR skos:prefLabel "caylon derivatives" .

figi-ps:ING skos:prefLabel "ing bank" .

figi-ps:BAAS figi-gii:hasUniqueTextIdentifier "BAAS" .

figi-ps:CAIR figi-gii:hasUniqueTextIdentifier "CAIR" .

figi-ps:ING figi-gii:hasUniqueTextIdentifier "ING" .

figi-st:reit a owl:NamedIndividual .

figi-ps:CAIX a owl:NamedIndividual .

figi-st:reit a figi-gii:SecurityType .

figi-ps:INGB a owl:NamedIndividual .

figi-ps:CAIX a figi-gii:PricingSource .

figi-ps:INGB a figi-gii:PricingSource .

figi-ps:CAIX skos:prefLabel "la caixa" .

figi-ps:INGB skos:prefLabel "ing bank sofia" .

figi-ps:CAIX figi-gii:hasUniqueTextIdentifier "CAIX" .

figi-ps:INGB figi-gii:hasUniqueTextIdentifier "INGB" .

figi-ps:CAJA a owl:NamedIndividual , figi-gii:PricingSource .

figi-ps:INGC a owl:NamedIndividual .

figi-ps:CAJA skos:prefLabel "caja de madrid" .

figi-ps:INGC a figi-gii:PricingSource .

figi-ps:CAJA figi-gii:hasUniqueTextIdentifier "CAJA" .

figi-ps:INGC skos:prefLabel "ing bank - new york" .

figi-ps:CAJM a owl:NamedIndividual .

figi-ps:INGC figi-gii:hasUniqueTextIdentifier "INGC" .

figi-ps:CAJM a figi-gii:PricingSource .

figi-st:reit skos:definition "Real Estate Investment Trust (REIT). A corporation or business trust which owns, manages and/or leases commercial real estate properties, and/or invests in Real Estate related securities, such as mortgaged-backed securities or whole loans and when meeting certain tax code requirements, is exempt at the entity level from corporate income tax. A creation of Congress, REIT legislation was initially passed in 1960 and was amended in 1986 to enhance and increase ownership and management focus on the underlying asset operations. REITs are exempt from federal (and usually state) corporate income taxation, subject to meeting certain IRS requirements for real estate investment and ownership, real estate income and dividend levels, i.e., dividend payout requirements for REITs require that 95% of taxable income be paid as a dividend." .

figi-ps:INGD a owl:NamedIndividual .

figi-ps:CAJM skos:prefLabel "caja madrid" .

figi-st:reit skos:prefLabel "reit" .

figi-ps:INGD a figi-gii:PricingSource .

figi-ps:CAJM figi-gii:hasUniqueTextIdentifier "CAJM" .

figi-st:reit figi-gii:hasUniqueTextIdentifier "REIT" .

figi-ps:INGD skos:prefLabel "ing direct" .

figi-ps:CALY a owl:NamedIndividual .

figi-ps:BABC a owl:NamedIndividual .

figi-ps:INGD figi-gii:hasUniqueTextIdentifier "INGD" .

figi-ps:CALY a figi-gii:PricingSource .

figi-ps:BABC a figi-gii:PricingSource .

figi-ps:INGE a owl:NamedIndividual .

figi-ps:CALY skos:prefLabel "credit agricole cib" .

figi-ps:BABC skos:prefLabel "babson capital mgmt" .

figi-ps:INGE a figi-gii:PricingSource .

figi-ps:CALY figi-gii:hasUniqueTextIdentifier "CALY" .

figi-ps:BABC skos:prefLabel "banco abc brasil" .

figi-ps:INGE skos:prefLabel "ing barings" .

figi-ps:CAMC a owl:NamedIndividual .

figi-ps:BABC figi-gii:hasUniqueTextIdentifier "BABC" .

figi-ps:CAMC a figi-gii:PricingSource .

figi-ps:INGE figi-gii:hasUniqueTextIdentifier "INGE" .

figi-st:repo a owl:NamedIndividual .

figi-ps:CAMC skos:prefLabel "china asset mgt" .

figi-st:repo a figi-gii:SecurityType .

figi-ps:INGF a owl:NamedIndividual .

figi-ps:CAMC figi-gii:hasUniqueTextIdentifier "CAMC" .

figi-ps:INGF a figi-gii:PricingSource .

figi-ps:CAMD a owl:NamedIndividual .

figi-ps:INGF skos:prefLabel "ing financial" .

figi-ps:CAMD a figi-gii:PricingSource .

figi-st:repo skos:definition "A form of short-term borrowing for dealers in government securities. The dealer sells the government securities to investors, usually on an overnight basis, and buys them back the following day." .

figi-ps:INGF figi-gii:hasUniqueTextIdentifier "INGF" .

figi-ps:CAMD skos:prefLabel "cicc asset manage" .

figi-st:repo skos:prefLabel "repo" .

figi-ps:INGG a owl:NamedIndividual .

figi-ps:CAMD figi-gii:hasUniqueTextIdentifier "CAMD" .

figi-st:repo figi-gii:hasUniqueTextIdentifier "REPO" .

figi-ps:INGG a figi-gii:PricingSource .

figi-ps:CAMI a owl:NamedIndividual .

figi-ps:BABR a owl:NamedIndividual .

figi-ps:INGG skos:prefLabel "ing bank govt" .

figi-ps:CAMI a figi-gii:PricingSource .

figi-ps:BABR a figi-gii:PricingSource .

figi-ps:INGG figi-gii:hasUniqueTextIdentifier "INGG" .

figi-ps:CAMI skos:prefLabel "banco caminos" .

figi-ps:BABR skos:prefLabel "banco barclays" .

figi-ps:INGH a owl:NamedIndividual .

figi-ps:CAMI figi-gii:hasUniqueTextIdentifier "CAMI" .

figi-ps:BABR figi-gii:hasUniqueTextIdentifier "BABR" .

figi-ps:INGH a figi-gii:PricingSource .

figi-ps:CAMJ a owl:NamedIndividual .

figi-st:restructurdDebt a owl:NamedIndividual .

figi-ps:CAMJ a figi-gii:PricingSource .

figi-ps:INGH skos:prefLabel "ing barings budapest" .

figi-st:restructurdDebt a figi-gii:SecurityType .

figi-ps:CAMJ skos:prefLabel "citi asset mgmt asia" .

figi-ps:INGH figi-gii:hasUniqueTextIdentifier "INGH" .

figi-ps:CAMJ figi-gii:hasUniqueTextIdentifier "CAMJ" .

figi-st:restructurdDebt skos:definition "Bonds that came out of the Brady plan in the 1980's that addressed the LDC debt crisis." .

figi-ps:CAML a owl:NamedIndividual .

figi-ps:INGI a owl:NamedIndividual .

figi-st:restructurdDebt skos:prefLabel "restructurd debt" .

figi-ps:CAML a figi-gii:PricingSource .

figi-ps:INGI a figi-gii:PricingSource .

figi-st:restructurdDebt figi-gii:hasUniqueTextIdentifier "RESTRUCTURD DEBT" .

figi-ps:CAML skos:prefLabel "camalia capital mrkt" .

figi-ps:INGI skos:prefLabel "ing invest mgnt prag" .

figi-ps:BABS a owl:NamedIndividual .

figi-ps:CAML figi-gii:hasUniqueTextIdentifier "CAML" .

figi-ps:INGI figi-gii:hasUniqueTextIdentifier "INGI" .

figi-ps:BABS a figi-gii:PricingSource .

figi-ps:CANA a owl:NamedIndividual .

figi-ps:INGK a owl:NamedIndividual .

figi-ps:BABS skos:prefLabel "barclays capital abs" .

figi-ps:CANA a figi-gii:PricingSource .

figi-ps:INGK a figi-gii:PricingSource .

figi-ps:BABS figi-gii:hasUniqueTextIdentifier "BABS" .

figi-ps:CANA skos:prefLabel "canara robeco amc" .

figi-ps:INGK skos:prefLabel "ing bank ukraine" .

figi-st:retailCD a owl:NamedIndividual .

figi-ps:CANA figi-gii:hasUniqueTextIdentifier "CANA" .

figi-ps:INGK figi-gii:hasUniqueTextIdentifier "INGK" .

figi-st:retailCD a figi-gii:SecurityType .

figi-ps:CANO a owl:NamedIndividual .

figi-ps:INGL a owl:NamedIndividual .

figi-ps:CANO a figi-gii:PricingSource .

figi-st:retailCD skos:definition "Certificates of Deposit sold to Retail customers" .

figi-ps:INGL a figi-gii:PricingSource .

figi-ps:CANO skos:prefLabel "caixanova" .

figi-st:retailCD skos:prefLabel "retail cd" .

figi-ps:INGL skos:prefLabel "ing bank milan" .

figi-ps:CANO figi-gii:hasUniqueTextIdentifier "CANO" .

figi-st:retailCD figi-gii:hasUniqueTextIdentifier "RETAIL CD" .

figi-ps:INGL figi-gii:hasUniqueTextIdentifier "INGL" .

figi-ps:CAP a owl:NamedIndividual .

figi-ps:BABU a owl:NamedIndividual .

figi-ps:CAP a figi-gii:PricingSource .

figi-ps:BABU a figi-gii:PricingSource .

figi-ps:INGM a owl:NamedIndividual .

figi-ps:CAP skos:prefLabel "capital group" .

figi-ps:BABU skos:prefLabel "hypo bank burgenland" .

figi-ps:INGM a figi-gii:PricingSource .

figi-ps:CAP figi-gii:hasUniqueTextIdentifier "CAP" .

figi-ps:BABU figi-gii:hasUniqueTextIdentifier "BABU" .

figi-ps:INGM skos:prefLabel "ing bank philippines" .

figi-ps:CAPB a owl:NamedIndividual .

figi-st:returnIdx a owl:NamedIndividual .

figi-ps:INGM skos:prefLabel "ing bank tst" .

figi-st:returnIdx a figi-gii:SecurityType .

figi-ps:CAPB a figi-gii:PricingSource .

figi-ps:INGM figi-gii:hasUniqueTextIdentifier "INGM" .

figi-st:returnIdx skos:definition "Not applicable to currencies" .

figi-ps:CAPB skos:prefLabel "cm capital markets" .

figi-ps:INGN a owl:NamedIndividual .

figi-st:returnIdx skos:prefLabel "return idx" .

figi-ps:CAPB figi-gii:hasUniqueTextIdentifier "CAPB" .

figi-ps:INGN a figi-gii:PricingSource .

figi-st:returnIdx figi-gii:hasUniqueTextIdentifier "RETURN IDX" .

figi-ps:CAPF a owl:NamedIndividual .

figi-ps:INGN skos:prefLabel "ing bank credits" .

figi-ps:CAPF a figi-gii:PricingSource .

figi-ps:BAC a owl:NamedIndividual .

figi-ps:INGN figi-gii:hasUniqueTextIdentifier "INGN" .

figi-ps:BAC a figi-gii:PricingSource .

figi-ps:CAPF skos:prefLabel "capitalfin" .

figi-ps:INGO a owl:NamedIndividual .

figi-ps:BAC skos:prefLabel "bank of america bbt" .

figi-ps:CAPF figi-gii:hasUniqueTextIdentifier "CAPF" .

figi-ps:INGO a figi-gii:PricingSource .

figi-ps:BAC figi-gii:hasUniqueTextIdentifier "BAC" .

figi-ps:CAPI a owl:NamedIndividual .

figi-ps:INGO skos:prefLabel "ing amsterdam-gov" .

figi-ps:CAPI a figi-gii:PricingSource .

figi-st:rev a owl:NamedIndividual .

figi-ps:INGO figi-gii:hasUniqueTextIdentifier "INGO" .

figi-st:rev a figi-gii:SecurityType .

figi-ps:CAPI skos:prefLabel "capitalgest sgr spa" .

figi-ps:INGP a owl:NamedIndividual .

figi-ps:CAPI figi-gii:hasUniqueTextIdentifier "CAPI" .

figi-ps:INGP a figi-gii:PricingSource .

figi-st:rev skos:definition "Funds may be borrowed, repaid, and then borrowed again throughout the life of the loan. (Resembles a credit card)." .

figi-ps:CAPJ a owl:NamedIndividual .

figi-ps:INGP skos:prefLabel "ing bank prague" .

figi-ps:CAPJ a figi-gii:PricingSource .

figi-st:rev skos:prefLabel "rev" .

figi-ps:INGP figi-gii:hasUniqueTextIdentifier "INGP" .

figi-ps:CAPJ skos:prefLabel "capital bk of jordan" .

figi-st:rev figi-gii:hasUniqueTextIdentifier "REV" .

figi-ps:INGQ a owl:NamedIndividual .

figi-ps:CAPJ figi-gii:hasUniqueTextIdentifier "CAPJ" .

figi-ps:INGQ a figi-gii:PricingSource .

figi-ps:BACG a owl:NamedIndividual .

figi-ps:CAPM a owl:NamedIndividual .

figi-ps:INGQ skos:prefLabel "ing bank" .

figi-ps:CAPM a figi-gii:PricingSource .

figi-ps:BACG a figi-gii:PricingSource .

figi-ps:INGQ figi-gii:hasUniqueTextIdentifier "INGQ" .

figi-ps:CAPM skos:prefLabel "capitol securities" .

figi-ps:BACG skos:prefLabel "barclays cap mkts" .

figi-ps:INGR a owl:NamedIndividual .

figi-ps:CAPM figi-gii:hasUniqueTextIdentifier "CAPM" .

figi-ps:BACG figi-gii:hasUniqueTextIdentifier "BACG" .

figi-ps:INGR a figi-gii:PricingSource .

figi-ps:CAPR a owl:NamedIndividual .

figi-st:revGuaranteeFac a owl:NamedIndividual .

figi-ps:INGR skos:prefLabel "ing bank eurasia" .

figi-ps:CAPR a figi-gii:PricingSource .

figi-st:revGuaranteeFac a figi-gii:SecurityType .

figi-ps:INGR figi-gii:hasUniqueTextIdentifier "INGR" .

figi-ps:CAPR skos:prefLabel "caprok capital llc" .

figi-ps:INGS a owl:NamedIndividual .

figi-ps:CAPR figi-gii:hasUniqueTextIdentifier "CAPR" .

figi-ps:INGS a figi-gii:PricingSource .

figi-st:revGuaranteeFac skos:definition "Funds may be borrowed, repaid, and then borrowed again throughout the life of the loan. Contingent liability which is issued by a bank to ensure/guarantee that an underlying project is completed." .

figi-ps:CAPS a owl:NamedIndividual .

figi-ps:INGS skos:prefLabel "ing" .

figi-st:revGuaranteeFac skos:prefLabel "rev guarantee fac" .

figi-ps:CAPS a figi-gii:PricingSource .

figi-st:revGuaranteeFac figi-gii:hasUniqueTextIdentifier "REV GUARANTEE FAC" .

figi-ps:CAPS skos:prefLabel "campisi, milan" .

figi-ps:INGS figi-gii:hasUniqueTextIdentifier "INGS" .

figi-ps:BACI a owl:NamedIndividual .

figi-ps:CAPS figi-gii:hasUniqueTextIdentifier "CAPS" .

figi-ps:BACI a figi-gii:PricingSource .

figi-ps:INGT a owl:NamedIndividual .

figi-ps:CARG a owl:NamedIndividual .

figi-ps:BACI skos:prefLabel "boa chicago - inside" .

figi-ps:INGT a figi-gii:PricingSource .

figi-ps:CARG a figi-gii:PricingSource .

figi-ps:BACI figi-gii:hasUniqueTextIdentifier "BACI" .

figi-ps:INGT skos:prefLabel "ing bank milan" .

figi-ps:CARG skos:prefLabel "carmignac gest" .

figi-st:revVatTrnch a owl:NamedIndividual .

figi-ps:INGT figi-gii:hasUniqueTextIdentifier "INGT" .

figi-st:revVatTrnch a figi-gii:SecurityType .

figi-ps:CARG figi-gii:hasUniqueTextIdentifier "CARG" .

figi-ps:INGU a owl:NamedIndividual , figi-gii:PricingSource .

figi-ps:CARM a owl:NamedIndividual .

figi-st:revVatTrnch skos:definition "Funds may be borrowed, repaid, and then borrowed again throughout the life of the loan. Given as temporary reimbursement for a VAT credit it has with the state." .

figi-ps:CARM a figi-gii:PricingSource .

figi-ps:INGU skos:prefLabel "ing bank nv" .

figi-st:revVatTrnch skos:prefLabel "rev vat-trnch" .

figi-ps:CARM skos:prefLabel "carmignac gestion" .

figi-ps:INGU figi-gii:hasUniqueTextIdentifier "INGU" .

figi-st:revVatTrnch figi-gii:hasUniqueTextIdentifier "REV VAT-TRNCH" .

figi-ps:CARM figi-gii:hasUniqueTextIdentifier "CARM" .

figi-ps:INGV a owl:NamedIndividual .

figi-ps:BACM a owl:NamedIndividual .

figi-ps:INGV a figi-gii:PricingSource .

figi-ps:CASA a owl:NamedIndividual .

figi-ps:BACM a figi-gii:PricingSource .

figi-ps:INGV skos:prefLabel "ing bank singapore" .

figi-ps:CASA a figi-gii:PricingSource .

figi-ps:BACM skos:prefLabel "bofa global cap mgmt" .

figi-ps:INGV figi-gii:hasUniqueTextIdentifier "INGV" .

figi-ps:CASA skos:prefLabel "casablanca se" .

figi-ps:BACM figi-gii:hasUniqueTextIdentifier "BACM" .

figi-ps:INGW a owl:NamedIndividual .

figi-ps:CASA figi-gii:hasUniqueTextIdentifier "CASA" .

figi-st:right a owl:NamedIndividual , figi-gii:SecurityType .

figi-ps:CASB a owl:NamedIndividual , figi-gii:PricingSource ;
	skos:prefLabel "ca-cib abs" ;
	figi-gii:hasUniqueTextIdentifier "CASB" .

figi-ps:INGW a figi-gii:PricingSource .

figi-st:right skos:definition "A security giving stockholders entitlement to purchase new shares issued by the corporation at a predetermined price (normally less than the current market price) in proportion to the number of shares already owned. Rights are issued only for a short period of time, after which they expire." .

figi-ps:CASL a owl:NamedIndividual .

figi-ps:INGW skos:prefLabel "ing bank slaski" .

figi-ps:CASL a figi-gii:PricingSource .

figi-ps:INGW figi-gii:hasUniqueTextIdentifier "INGW" .

figi-ps:CASL skos:prefLabel "castleoak securities" .

figi-ps:INGX a owl:NamedIndividual .

figi-st:right skos:prefLabel "right" .

figi-ps:CASL figi-gii:hasUniqueTextIdentifier "CASL" .

figi-ps:INGX a figi-gii:PricingSource .

figi-st:right figi-gii:hasUniqueTextIdentifier "Right" .

figi-ps:CASR a owl:NamedIndividual .

figi-ps:INGX skos:prefLabel "ing bank (mexico)" .

figi-ps:CASR a figi-gii:PricingSource .

figi-ps:BACO a owl:NamedIndividual .

figi-ps:INGX figi-gii:hasUniqueTextIdentifier "INGX" .

figi-ps:BACO a figi-gii:PricingSource .

figi-ps:CASR skos:prefLabel "credit agri srbija" .

figi-ps:INGY a owl:NamedIndividual .

figi-ps:BACO skos:prefLabel "banc one capital mkt" .

figi-ps:CASR figi-gii:hasUniqueTextIdentifier "CASR" .

figi-ps:INGY a figi-gii:PricingSource .

figi-ps:BACO figi-gii:hasUniqueTextIdentifier "BACO" .

figi-ps:CAST a owl:NamedIndividual .

figi-ps:INGY skos:prefLabel "inb-bbl brussels" .

figi-ps:CAST a figi-gii:PricingSource .

figi-ps:BACR a owl:NamedIndividual .

figi-ps:INGY figi-gii:hasUniqueTextIdentifier "INGY" .

figi-ps:BACR a figi-gii:PricingSource .

figi-ps:CAST skos:prefLabel "cai structured" .

figi-ps:INGZ a owl:NamedIndividual .

figi-ps:BACR skos:prefLabel "bofaml retail" .

figi-ps:CAST figi-gii:hasUniqueTextIdentifier "CAST" .

figi-ps:INGZ a figi-gii:PricingSource .

figi-ps:BACR figi-gii:hasUniqueTextIdentifier "BACR" .

figi-ps:CAT a owl:NamedIndividual .

figi-ps:INGZ skos:prefLabel "ing manila" .

figi-ps:CAT a figi-gii:PricingSource .

figi-st:royaltyTrst a owl:NamedIndividual .

figi-ps:INGZ figi-gii:hasUniqueTextIdentifier "INGZ" .

figi-st:royaltyTrst a figi-gii:SecurityType .

figi-ps:CAT skos:prefLabel "charter atlantic" .

figi-ps:INKA a owl:NamedIndividual .

figi-ps:CAT figi-gii:hasUniqueTextIdentifier "CAT" .

figi-ps:INKA a figi-gii:PricingSource .

figi-st:royaltyTrst skos:definition "Royalty Trust. An oil or gas company spins off property to its shareholders, which means it will not be taxed at the corporate level and will offer high returns to stockholders." .

figi-ps:CATE a owl:NamedIndividual .

figi-ps:INKA skos:prefLabel "intercap secs ltd" .

figi-ps:CATE a figi-gii:PricingSource .

figi-st:royaltyTrst skos:prefLabel "royalty trst" .

figi-ps:INKA figi-gii:hasUniqueTextIdentifier "INKA" .

figi-ps:CATE skos:prefLabel "catella fondforvaltn" .

figi-st:royaltyTrst figi-gii:hasUniqueTextIdentifier "Royalty Trst" .

figi-ps:INME a owl:NamedIndividual .

figi-ps:CATE figi-gii:hasUniqueTextIdentifier "CATE" .

figi-ps:INME a figi-gii:PricingSource .

figi-ps:BACS a owl:NamedIndividual .

figi-ps:CATW a owl:NamedIndividual .

figi-ps:INME skos:prefLabel "ing baring mexico" .

figi-ps:CATW a figi-gii:PricingSource .

figi-ps:BACS a figi-gii:PricingSource .

figi-ps:INME figi-gii:hasUniqueTextIdentifier "INME" .

figi-ps:CATW skos:prefLabel "calyon" .

figi-ps:BACS skos:prefLabel "bank austria credita" .

figi-ps:INMX a owl:NamedIndividual .

figi-ps:CATW figi-gii:hasUniqueTextIdentifier "CATW" .

figi-ps:BACS figi-gii:hasUniqueTextIdentifier "BACS" .

figi-ps:INMX a figi-gii:PricingSource .

figi-ps:CAU a owl:NamedIndividual .

figi-st:russianPn a owl:NamedIndividual .

figi-ps:INMX skos:prefLabel "ing mexico" .

figi-ps:CAU a figi-gii:PricingSource .

figi-st:russianPn a figi-gii:SecurityType .

figi-ps:INMX figi-gii:hasUniqueTextIdentifier "INMX" .

figi-ps:CAU skos:prefLabel "canaccord adams ltd" .

figi-st:russianPn skos:definition "Russian Promissory Note" .

figi-ps:INNS a owl:NamedIndividual .

figi-ps:CAU figi-gii:hasUniqueTextIdentifier "CAU" .

figi-st:russianPn skos:prefLabel "russian pn" .

figi-ps:INNS a figi-gii:PricingSource .

figi-ps:CAVE a owl:NamedIndividual .

figi-st:russianPn figi-gii:hasUniqueTextIdentifier "RUSSIAN PN" .

figi-ps:INNS skos:prefLabel "investindo nusantara" .

figi-ps:CAVE a figi-gii:PricingSource .

figi-ps:BADR a owl:NamedIndividual .

figi-ps:INNS figi-gii:hasUniqueTextIdentifier "INNS" .

figi-ps:CAVE skos:prefLabel "cavenagh capital" .

figi-ps:BADR a figi-gii:PricingSource .

figi-ps:INPL a owl:NamedIndividual .

figi-ps:CAVE figi-gii:hasUniqueTextIdentifier "CAVE" .

figi-ps:BADR skos:prefLabel "boa securities" .

figi-ps:INPL a figi-gii:PricingSource .

figi-ps:CAXP a owl:NamedIndividual .

figi-ps:BADR figi-gii:hasUniqueTextIdentifier "BADR" .

figi-ps:INPL skos:prefLabel "ing bank slaski sa" .

figi-ps:CAXP a figi-gii:PricingSource .

figi-st:sAMdTermYcd a owl:NamedIndividual .

figi-ps:INPL figi-gii:hasUniqueTextIdentifier "INPL" .

figi-st:sAMdTermYcd a figi-gii:SecurityType .

figi-ps:CAXP skos:prefLabel "caxton associates lp" .

figi-ps:INSG a owl:NamedIndividual .

figi-st:sAMdTermYcd skos:definition "Medium Term Yankee CD w/ semi-annual pay/compounding" .

figi-ps:INSG a figi-gii:PricingSource .

figi-ps:CAXP figi-gii:hasUniqueTextIdentifier "CAXP" .

figi-st:sAMdTermYcd skos:prefLabel "s/a md term ycd" .

figi-ps:INSG skos:prefLabel "insight invest mgtxx" .

figi-ps:CAXT a owl:NamedIndividual .

figi-st:sAMdTermYcd figi-gii:hasUniqueTextIdentifier "S/A MD TERM YCD" .

figi-ps:CAXT a figi-gii:PricingSource .

figi-ps:INSG figi-gii:hasUniqueTextIdentifier "INSG" .

figi-ps:BAE a owl:NamedIndividual .

figi-ps:CAXT skos:prefLabel "caxton associates" .

figi-ps:BAE a figi-gii:PricingSource .

figi-ps:INSK a owl:NamedIndividual .

figi-ps:CAXT figi-gii:hasUniqueTextIdentifier "CAXT" .

figi-ps:INSK a figi-gii:PricingSource .

figi-ps:BAE skos:prefLabel "bae systems pension" .

figi-ps:CAZ a owl:NamedIndividual .

figi-ps:INSK skos:prefLabel "ing bank, seoul" .

figi-ps:BAE figi-gii:hasUniqueTextIdentifier "BAE" .

figi-ps:CAZ a figi-gii:PricingSource .

figi-ps:INSK figi-gii:hasUniqueTextIdentifier "INSK" .

figi-st:samurai a owl:NamedIndividual .

figi-ps:CAZ skos:prefLabel "cazenove and co" .

figi-ps:INSN a owl:NamedIndividual .

figi-st:samurai a figi-gii:SecurityType .

figi-ps:CAZ figi-gii:hasUniqueTextIdentifier "CAZ" .

figi-ps:INSN a figi-gii:PricingSource ;
	skos:prefLabel "ingalls and snyder" .

figi-ps:CBA a owl:NamedIndividual .

figi-st:samurai skos:definition "Samurai Bond. A debt instrument denominated in Japanese yen, but not issued by a Japanese agency or company." .

figi-ps:CBA a figi-gii:PricingSource .

figi-ps:INSN figi-gii:hasUniqueTextIdentifier "INSN" .

figi-st:samurai skos:prefLabel "samurai" .

figi-ps:CBA skos:prefLabel "commonwealth bk aus" .

figi-ps:INSP a owl:NamedIndividual .

figi-st:samurai figi-gii:hasUniqueTextIdentifier "SAMURAI" .

figi-ps:CBA figi-gii:hasUniqueTextIdentifier "CBA" .

figi-ps:INSP a figi-gii:PricingSource .

figi-ps:BAEC a owl:NamedIndividual .

figi-ps:CBAA a owl:NamedIndividual .

figi-ps:INSP skos:prefLabel "ing singapore" .

figi-ps:BAEC a figi-gii:PricingSource .

figi-ps:CBAA a figi-gii:PricingSource .

figi-ps:INSP figi-gii:hasUniqueTextIdentifier "INSP" .

figi-ps:BAEC skos:prefLabel "bcba-cont (nominal)" .

figi-ps:CBAA skos:prefLabel "commonwealth bk aust" .

figi-ps:INSU a owl:NamedIndividual .

figi-ps:BAEC figi-gii:hasUniqueTextIdentifier "BAEC" .

figi-ps:CBAA figi-gii:hasUniqueTextIdentifier "CBAA" .

figi-ps:INSU a figi-gii:PricingSource .

figi-ps:BAEF a owl:NamedIndividual .

figi-ps:CBAB a owl:NamedIndividual .

figi-ps:INSU skos:prefLabel "la caja de canarias" .

figi-ps:CBAB a figi-gii:PricingSource .

figi-ps:BAEF a figi-gii:PricingSource .

figi-ps:INSU figi-gii:hasUniqueTextIdentifier "INSU" .

figi-ps:CBAB skos:prefLabel "cba inf linked bonds" .

figi-ps:BAEF skos:prefLabel "bcba-floor (nominal)" .

figi-ps:INSV a owl:NamedIndividual .

figi-ps:CBAB figi-gii:hasUniqueTextIdentifier "CBAB" .

figi-ps:BAEF figi-gii:hasUniqueTextIdentifier "BAEF" .

figi-ps:INSV a figi-gii:PricingSource .

figi-ps:CBAG a owl:NamedIndividual .

figi-st:savingsPlan a owl:NamedIndividual .

figi-ps:CBAG a figi-gii:PricingSource .

figi-ps:INSV skos:prefLabel "ins valores" .

figi-st:savingsPlan a figi-gii:SecurityType .

figi-ps:CBAG skos:prefLabel "commerzbank internal" .

figi-ps:INSV figi-gii:hasUniqueTextIdentifier "INSV" .

figi-ps:CBAG figi-gii:hasUniqueTextIdentifier "CBAG" .

figi-ps:INTE a owl:NamedIndividual .

figi-ps:CBAL a owl:NamedIndividual .

figi-st:savingsPlan skos:definition "Savings Plan is a general category which groups variable annuity, collective investment trusts and separately managed accounts. Securities categorized under collective investment trusts and separately managed accounts fund types are for Bloombergs internal use." .

figi-ps:CBAL a figi-gii:PricingSource .

figi-ps:INTE a figi-gii:PricingSource .

figi-st:savingsPlan skos:prefLabel "savings plan" .

figi-ps:CBAL skos:prefLabel "commonwealth bk aust" .

figi-ps:INTE skos:prefLabel "interbank" .

figi-st:savingsPlan figi-gii:hasUniqueTextIdentifier "Savings Plan" .

figi-ps:CBAL figi-gii:hasUniqueTextIdentifier "CBAL" .

figi-ps:INTE figi-gii:hasUniqueTextIdentifier "INTE" .

figi-ps:BAEG a owl:NamedIndividual .

figi-ps:CBAN a owl:NamedIndividual .

figi-ps:INTL a owl:NamedIndividual .

figi-ps:BAEG a figi-gii:PricingSource .

figi-ps:CBAN a figi-gii:PricingSource .

figi-ps:INTL a figi-gii:PricingSource .

figi-ps:BAEG skos:prefLabel "bank of america egov" .

figi-ps:CBAN skos:prefLabel "centrobanca" .

figi-ps:INTL skos:prefLabel "consilium inv mgmt" .

figi-ps:BAEG figi-gii:hasUniqueTextIdentifier "BAEG" .

figi-ps:CBAN figi-gii:hasUniqueTextIdentifier "CBAN" .

figi-ps:INTL figi-gii:hasUniqueTextIdentifier "INTL" .

figi-ps:CBAP a owl:NamedIndividual .

figi-ps:BAEI a owl:NamedIndividual .

figi-ps:INTT a owl:NamedIndividual .

figi-ps:CBAP a figi-gii:PricingSource .

figi-ps:BAEI a figi-gii:PricingSource .

figi-ps:INTT a figi-gii:PricingSource .

figi-ps:CBAP skos:prefLabel "commonwealth bank au" .

figi-ps:BAEI skos:prefLabel "boa london inside" .

figi-ps:INTT skos:prefLabel "intl trading" .

figi-ps:CBAP figi-gii:hasUniqueTextIdentifier "CBAP" .

figi-ps:BAEI figi-gii:hasUniqueTextIdentifier "BAEI" .

figi-ps:INTT figi-gii:hasUniqueTextIdentifier "INTT" .

figi-ps:CBAU a owl:NamedIndividual .

figi-st:sbaPool a owl:NamedIndividual .

figi-ps:CBAU a figi-gii:PricingSource .

figi-ps:INVB a owl:NamedIndividual .

figi-st:sbaPool a figi-gii:SecurityType .

figi-ps:CBAU skos:prefLabel "cba sydney" .

figi-ps:INVB a figi-gii:PricingSource .

figi-st:sbaPool skos:definition "Agency Pool issued by Small Business Association" .

figi-ps:CBAU skos:prefLabel "commonwealth bk aus" .

figi-ps:INVB skos:prefLabel "investec bank plc" .

figi-ps:CBAU figi-gii:hasUniqueTextIdentifier "CBAU" .

figi-st:sbaPool skos:prefLabel "sba pool" .

figi-ps:INVB figi-gii:hasUniqueTextIdentifier "INVB" .

figi-ps:CBAX a owl:NamedIndividual .

figi-st:sbaPool figi-gii:hasUniqueTextIdentifier "SBA Pool" .

figi-ps:CBAX a figi-gii:PricingSource .

figi-ps:BAEM a owl:NamedIndividual .

figi-ps:CBAX skos:prefLabel "cba london" .

figi-ps:BAEM a figi-gii:PricingSource .

figi-ps:CBAX figi-gii:hasUniqueTextIdentifier "CBAX" .

figi-ps:BAEM skos:prefLabel "bank of america em" .

figi-ps:CBB3 a owl:NamedIndividual .

figi-ps:BAEM figi-gii:hasUniqueTextIdentifier "BAEM" .

figi-ps:CBB3 a figi-gii:PricingSource .

figi-ps:INVE a owl:NamedIndividual .

figi-ps:CBB3 skos:prefLabel "cbbt - future close" .

figi-st:sdr a owl:NamedIndividual .

figi-ps:INVE a figi-gii:PricingSource .

figi-ps:CBB3 figi-gii:hasUniqueTextIdentifier "CBB3" .

figi-st:sdr a figi-gii:SecurityType .

figi-ps:INVE skos:prefLabel "investec sa e-bond" .

figi-ps:CBBR a owl:NamedIndividual .

figi-st:sdr skos:definition "Swedish Depository Receipt" .

figi-ps:INVE figi-gii:hasUniqueTextIdentifier "INVE" .

figi-ps:CBBR a figi-gii:PricingSource .

figi-st:sdr skos:prefLabel "sdr" .

figi-ps:INVH a owl:NamedIndividual .

figi-ps:CBBR skos:prefLabel "calyon bank bahrain" .

figi-ps:INVH a figi-gii:PricingSource .

figi-st:sdr figi-gii:hasUniqueTextIdentifier "SDR" .

figi-ps:CBBR figi-gii:hasUniqueTextIdentifier "CBBR" .

figi-ps:INVH skos:prefLabel "invesco" .

figi-ps:BAEO a owl:NamedIndividual .

figi-ps:CBBT a owl:NamedIndividual .

figi-ps:INVH figi-gii:hasUniqueTextIdentifier "INVH" .

figi-ps:BAEO a figi-gii:PricingSource .

figi-ps:CBBT a figi-gii:PricingSource .

figi-ps:INVR a owl:NamedIndividual .

figi-ps:BAEO skos:prefLabel "bank america sec uk" .

figi-ps:INVR a figi-gii:PricingSource .

figi-ps:CBBT skos:prefLabel "fit composite" .

figi-ps:BAEO figi-gii:hasUniqueTextIdentifier "BAEO" .

figi-ps:INVR skos:prefLabel "inverseguros madrid" .

figi-ps:CBBT figi-gii:hasUniqueTextIdentifier "CBBT" .

figi-ps:BAET a owl:NamedIndividual .

figi-ps:INVR figi-gii:hasUniqueTextIdentifier "INVR" .

figi-ps:CBC a owl:NamedIndividual .

figi-ps:BAET a figi-gii:PricingSource .

figi-ps:CBC a figi-gii:PricingSource .

figi-ps:INVX a owl:NamedIndividual .

figi-ps:BAET skos:prefLabel "bank of america uk" .

figi-ps:CBC skos:prefLabel "china banking corp" .

figi-ps:INVX a figi-gii:PricingSource .

figi-ps:BAET figi-gii:hasUniqueTextIdentifier "BAET" .

figi-ps:CBC figi-gii:hasUniqueTextIdentifier "CBC" .

figi-ps:INVX skos:prefLabel "invex" .

figi-st:secLending a owl:NamedIndividual .

figi-ps:CBCD a owl:NamedIndividual .

figi-st:secLending a figi-gii:SecurityType .

figi-ps:INVX figi-gii:hasUniqueTextIdentifier "INVX" .

figi-ps:CBCD a figi-gii:PricingSource .

figi-ps:INXS a owl:NamedIndividual .

figi-ps:CBCD skos:prefLabel "commerzbank cb" .

figi-ps:INXS a figi-gii:PricingSource .

figi-ps:CBCD figi-gii:hasUniqueTextIdentifier "CBCD" .

figi-ps:INXS skos:prefLabel "ing bank singapore" ;
	figi-gii:hasUniqueTextIdentifier "INXS" .

figi-ps:CBCF a owl:NamedIndividual , figi-gii:PricingSource .

figi-ps:IOBN a owl:NamedIndividual .

figi-st:secLending skos:definition "Security Lending. aka stock lending. Refers to the lending of securities by one party to another. The terms of the loan will be governed by a Securities Lending Agreement, which, under U.S. law, requires that the borrower provides the lender with collateral, in the form of cash, government securities, or a Letter of Credit of value equal to or greater than the loaned securities. As payment for the loan, the parties negotiate a fee, quoted as an annualized percentage of the value of the loaned securities. If the agreed form of collateral is cash, then the fee may be quoted as a rebate, meaning that the lender will earn all of the interest which accrues on the cash collateral, and will rebate an agreed rate of interest to the borrower." .

figi-ps:CBCF skos:prefLabel "commerzbank" .

figi-ps:IOBN a figi-gii:PricingSource .

figi-st:secLending skos:prefLabel "sec lending" .

figi-ps:CBCF figi-gii:hasUniqueTextIdentifier "CBCF" .

figi-ps:IOBN skos:prefLabel "indian overseas bank" .

figi-st:secLending figi-gii:hasUniqueTextIdentifier "Sec Lending" .

figi-ps:CBCO a owl:NamedIndividual .

figi-ps:IOBN figi-gii:hasUniqueTextIdentifier "IOBN" .

figi-ps:CBCO a figi-gii:PricingSource .

figi-ps:BAG3 a owl:NamedIndividual .

figi-ps:ION a owl:NamedIndividual .

figi-ps:CBCO skos:prefLabel "corpbanca colombia" .

figi-ps:ION a figi-gii:PricingSource .

figi-ps:BAG3 a figi-gii:PricingSource .

figi-ps:CBCO figi-gii:hasUniqueTextIdentifier "CBCO" .

figi-ps:ION skos:prefLabel "ion trading" .

figi-ps:CBCP a owl:NamedIndividual .

figi-ps:ION figi-gii:hasUniqueTextIdentifier "ION" .

figi-ps:CBCP a figi-gii:PricingSource .

figi-ps:IONA a owl:NamedIndividual .

figi-ps:CBCP skos:prefLabel "chinabond settle px" .

figi-ps:IONA a figi-gii:PricingSource .

figi-ps:BAG3 skos:prefLabel "blp agency 3pm close" .

figi-ps:CBCP figi-gii:hasUniqueTextIdentifier "CBCP" .

figi-ps:IONA skos:prefLabel "ion euro aep v5" .

figi-ps:BAG3 figi-gii:hasUniqueTextIdentifier "BAG3" .

figi-ps:CBDB a owl:NamedIndividual .

figi-ps:IONA figi-gii:hasUniqueTextIdentifier "IONA" .

figi-ps:BAGB a owl:NamedIndividual .

figi-ps:CBDB a figi-gii:PricingSource .

figi-ps:BAGB a figi-gii:PricingSource .

figi-ps:IONS a owl:NamedIndividual .

figi-ps:CBDB skos:prefLabel "deutsche securities" .

figi-ps:BAGB skos:prefLabel "boa lnd - gilts" .

figi-ps:IONS a figi-gii:PricingSource .

figi-ps:CBDB figi-gii:hasUniqueTextIdentifier "CBDB" .

figi-ps:BAGB figi-gii:hasUniqueTextIdentifier "BAGB" .

figi-ps:IONS skos:prefLabel "ion ny" .

figi-ps:CBED a owl:NamedIndividual .

figi-st:semiAnnualSwap a owl:NamedIndividual .

figi-ps:IONS figi-gii:hasUniqueTextIdentifier "IONS" .

figi-ps:CBED a figi-gii:PricingSource .

figi-st:semiAnnualSwap a figi-gii:SecurityType .

figi-ps:IOSH a owl:NamedIndividual .

figi-ps:CBED skos:prefLabel "commerzbank eq deriv" .

figi-ps:IOSH a figi-gii:PricingSource .

figi-st:semiAnnualSwap skos:definition "Swap with semi- annual payment frequency" .

figi-ps:CBED figi-gii:hasUniqueTextIdentifier "CBED" .

figi-ps:IOSH skos:prefLabel "interocean" .

figi-st:semiAnnualSwap skos:prefLabel "semi-annual swap" .

figi-ps:CBEG a owl:NamedIndividual .

figi-ps:IOSH figi-gii:hasUniqueTextIdentifier "IOSH" .

figi-st:semiAnnualSwap figi-gii:hasUniqueTextIdentifier "SEMI-ANNUAL SWAP" .

figi-ps:CBEG a figi-gii:PricingSource .

figi-ps:IPBM a owl:NamedIndividual .

figi-ps:BAGC a owl:NamedIndividual .

figi-ps:IPBM a figi-gii:PricingSource .

figi-ps:CBEG skos:prefLabel "central bank egypt" .

figi-ps:BAGC a figi-gii:PricingSource .

figi-ps:IPBM skos:prefLabel "interprombank" .

figi-ps:CBEG figi-gii:hasUniqueTextIdentifier "CBEG" .

figi-ps:BAGC skos:prefLabel "banco agricola" .

figi-ps:IPBM figi-gii:hasUniqueTextIdentifier "IPBM" .

figi-ps:CBEQ a owl:NamedIndividual .

figi-ps:BAGC figi-gii:hasUniqueTextIdentifier "BAGC" .

figi-ps:CBEQ a figi-gii:PricingSource .

figi-ps:IPC a owl:NamedIndividual .

figi-st:shogun a owl:NamedIndividual .

figi-ps:IPC a figi-gii:PricingSource .

figi-ps:CBEQ skos:prefLabel "commerzbank" .

figi-st:shogun a figi-gii:SecurityType .

figi-ps:IPC skos:prefLabel "ipc usa" .

figi-ps:CBEQ figi-gii:hasUniqueTextIdentifier "CBEQ" .

figi-ps:IPC figi-gii:hasUniqueTextIdentifier "IPC" .

figi-ps:CBFC a owl:NamedIndividual .

figi-st:shogun skos:definition "Shogun Security. A foreign corporation-issued, non-yen denominated security distributed in Japan. Also known as a geisha bond." .

figi-ps:CBFC a figi-gii:PricingSource .

figi-st:shogun skos:prefLabel "shogun" .

figi-ps:IPGC a owl:NamedIndividual .

figi-ps:CBFC skos:prefLabel "china bills finance" .

figi-ps:IPGC a figi-gii:PricingSource .

figi-ps:CBFC figi-gii:hasUniqueTextIdentifier "CBFC" .

figi-ps:IPGC skos:prefLabel "investment placement" .

figi-st:shogun figi-gii:hasUniqueTextIdentifier "SHOGUN" .

figi-ps:CBFT a owl:NamedIndividual .

figi-ps:IPGC figi-gii:hasUniqueTextIdentifier "IPGC" .

figi-ps:CBFT a figi-gii:PricingSource .

figi-ps:BAGJ a owl:NamedIndividual .

figi-ps:IPMB a owl:NamedIndividual .

figi-ps:CBFT skos:prefLabel "commerzbankfrankfurt" .

figi-ps:BAGJ a figi-gii:PricingSource .

figi-ps:IPMB a figi-gii:PricingSource .

figi-ps:CBFT figi-gii:hasUniqueTextIdentifier "CBFT" .

figi-ps:IPMB skos:prefLabel "inti prebon money br" .

figi-ps:CBGN a owl:NamedIndividual .

figi-ps:IPMB figi-gii:hasUniqueTextIdentifier "IPMB" .

figi-ps:CBGN a figi-gii:PricingSource .

figi-ps:IPOX a owl:NamedIndividual .

figi-ps:CBGN skos:prefLabel "corp bgn (internal)" .

figi-ps:IPOX a figi-gii:PricingSource .

figi-ps:CBGN figi-gii:hasUniqueTextIdentifier "CBGN" .

figi-ps:IPOX skos:prefLabel "ipox schuster" .

figi-ps:CBIJ a owl:NamedIndividual .

figi-ps:IPOX figi-gii:hasUniqueTextIdentifier "IPOX" .

figi-ps:CBIJ a figi-gii:PricingSource .

figi-ps:IPTB a owl:NamedIndividual .

figi-ps:CBIJ skos:prefLabel "citibank jakarta" .

figi-ps:IPTB a figi-gii:PricingSource .

figi-ps:CBIJ figi-gii:hasUniqueTextIdentifier "CBIJ" .

figi-ps:IPTB skos:prefLabel "ipopema securities" .

figi-ps:CBIR a owl:NamedIndividual .

figi-ps:IPTB figi-gii:hasUniqueTextIdentifier "IPTB" .

figi-ps:CBIR a figi-gii:PricingSource .

figi-ps:IROK a owl:NamedIndividual .

figi-ps:CBIR skos:prefLabel "central bank of irel" .

figi-ps:IROK a figi-gii:PricingSource .

figi-ps:CBIR figi-gii:hasUniqueTextIdentifier "CBIR" .

figi-ps:IROK skos:prefLabel "iroko securities" .

figi-ps:CBJU a owl:NamedIndividual .

figi-ps:IROK figi-gii:hasUniqueTextIdentifier "IROK" .

figi-ps:CBJU a figi-gii:PricingSource .

figi-ps:IRSE a owl:NamedIndividual .

figi-ps:CBJU skos:prefLabel "commerzbank jumbo" .

figi-ps:IRSE a figi-gii:PricingSource .

figi-ps:CBJU figi-gii:hasUniqueTextIdentifier "CBJU" .

figi-ps:IRSE skos:prefLabel "irish stock exch" .

figi-ps:CBK a owl:NamedIndividual .

figi-ps:IRSE figi-gii:hasUniqueTextIdentifier "IRSE" .

figi-ps:CBK a figi-gii:PricingSource .

figi-ps:IRVN a owl:NamedIndividual .

figi-ps:CBK skos:prefLabel "commerzbank ag group" .

figi-ps:IRVN a figi-gii:PricingSource .

figi-ps:CBK figi-gii:hasUniqueTextIdentifier "CBK" .

figi-ps:IRVN skos:prefLabel "irevna" .

figi-ps:CBKF a owl:NamedIndividual .

figi-ps:IRVN figi-gii:hasUniqueTextIdentifier "IRVN" .

figi-ps:CBKF a figi-gii:PricingSource .

figi-ps:ISBB a owl:NamedIndividual .

figi-ps:CBKF skos:prefLabel "commerz bk financial" .

figi-ps:ISBB a figi-gii:PricingSource .

figi-ps:CBKF figi-gii:hasUniqueTextIdentifier "CBKF" .

figi-ps:ISBB skos:prefLabel "israel discount bk" .

figi-ps:CBKG a owl:NamedIndividual .

figi-ps:ISBB figi-gii:hasUniqueTextIdentifier "ISBB" .

figi-ps:CBKG a figi-gii:PricingSource ;
	skos:prefLabel "commerzbank" .

figi-ps:ISEL a owl:NamedIndividual .

figi-ps:CBKG figi-gii:hasUniqueTextIdentifier "CBKG" .

figi-ps:ISEL a figi-gii:PricingSource .

figi-ps:CBKI a owl:NamedIndividual .

figi-ps:ISEL skos:prefLabel "ise large market" .

figi-ps:CBKI a figi-gii:PricingSource .

figi-ps:ISEL figi-gii:hasUniqueTextIdentifier "ISEL" .

figi-ps:CBKI skos:prefLabel "commerzbank priv bk" .

figi-ps:ISGR a owl:NamedIndividual .

figi-ps:CBKI figi-gii:hasUniqueTextIdentifier "CBKI" .

figi-ps:ISGR a figi-gii:PricingSource .

figi-ps:CBKM a owl:NamedIndividual .

figi-ps:ISGR skos:prefLabel "investment standard" .

figi-ps:CBKM a figi-gii:PricingSource .

figi-ps:ISGR figi-gii:hasUniqueTextIdentifier "ISGR" .

figi-ps:CBKM skos:prefLabel "commerzbank london" .

figi-ps:ISIG a owl:NamedIndividual .

figi-ps:CBKM figi-gii:hasUniqueTextIdentifier "CBKM" .

figi-ps:ISIG a figi-gii:PricingSource .

figi-ps:CBKT a owl:NamedIndividual .

figi-ps:ISIG skos:prefLabel "isi group" .

figi-ps:CBKT a figi-gii:PricingSource .

figi-ps:ISIG figi-gii:hasUniqueTextIdentifier "ISIG" .

figi-ps:CBKT skos:prefLabel "commerzbank ffrt" .

figi-ps:ISL0 a owl:NamedIndividual .

figi-ps:CBKT figi-gii:hasUniqueTextIdentifier "CBKT" .

figi-ps:ISL0 a figi-gii:PricingSource .

figi-ps:CBKV a owl:NamedIndividual .

figi-ps:ISL0 skos:prefLabel "ise large market t0" .

figi-ps:CBKV a figi-gii:PricingSource .

figi-ps:ISL0 figi-gii:hasUniqueTextIdentifier "ISL0" .

figi-ps:CBKV skos:prefLabel "citibank venezuela" .

figi-ps:ISL1 a owl:NamedIndividual .

figi-ps:CBKV figi-gii:hasUniqueTextIdentifier "CBKV" .

figi-ps:ISL1 a figi-gii:PricingSource .

figi-ps:CBLD a owl:NamedIndividual .

figi-ps:ISL1 skos:prefLabel "ise large market t1" .

figi-ps:CBLD a figi-gii:PricingSource .

figi-ps:ISL1 figi-gii:hasUniqueTextIdentifier "ISL1" .

figi-ps:CBLD skos:prefLabel "commerzbank ag ldn" .

figi-ps:ISPX a owl:NamedIndividual .

figi-ps:CBLD figi-gii:hasUniqueTextIdentifier "CBLD" .

figi-ps:ISPX a figi-gii:PricingSource .

figi-ps:CBMA a owl:NamedIndividual .

figi-ps:ISPX skos:prefLabel "icap new issues" .

figi-ps:CBMA a figi-gii:PricingSource .

figi-ps:ISPX figi-gii:hasUniqueTextIdentifier "ISPX" .

figi-ps:CBMA skos:prefLabel "central bank malta" .

figi-ps:ISR0 a owl:NamedIndividual .

figi-ps:CBMA figi-gii:hasUniqueTextIdentifier "CBMA" .

figi-ps:ISR0 a figi-gii:PricingSource .

figi-ps:CBMI a owl:NamedIndividual .

figi-ps:ISR0 skos:prefLabel "ise retailt+0lge" .

figi-ps:CBMI a figi-gii:PricingSource .

figi-ps:ISR0 figi-gii:hasUniqueTextIdentifier "ISR0" .

figi-ps:CBMI skos:prefLabel "corp bank india" .

figi-ps:ISR1 a owl:NamedIndividual .

figi-ps:CBMI figi-gii:hasUniqueTextIdentifier "CBMI" .

figi-ps:ISR1 a figi-gii:PricingSource .

figi-ps:CBMN a owl:NamedIndividual .

figi-ps:ISR1 skos:prefLabel "ise retailt+1lge" .

figi-ps:CBMN a figi-gii:PricingSource .

figi-ps:ISR1 figi-gii:hasUniqueTextIdentifier "ISR1" .

figi-ps:CBMN skos:prefLabel "capital bank" .

figi-ps:ISS0 a owl:NamedIndividual .

figi-ps:CBMN figi-gii:hasUniqueTextIdentifier "CBMN" .

figi-ps:ISS0 a figi-gii:PricingSource .

figi-ps:CBNK a owl:NamedIndividual .

figi-ps:ISS0 skos:prefLabel "ise small market t0" .

figi-ps:CBNK a figi-gii:PricingSource .

figi-ps:ISS0 figi-gii:hasUniqueTextIdentifier "ISS0" .

figi-ps:CBNK skos:prefLabel "compass bank" .

figi-ps:ISTA a owl:NamedIndividual .

figi-ps:CBNK figi-gii:hasUniqueTextIdentifier "CBNK" .

figi-ps:ISTA a figi-gii:PricingSource .

figi-ps:CBOA a owl:NamedIndividual .

figi-ps:ISTA skos:prefLabel "istrobanka" .

figi-ps:CBOA a figi-gii:PricingSource .

figi-ps:ISTA figi-gii:hasUniqueTextIdentifier "ISTA" .

figi-ps:CBOA skos:prefLabel "central bank armenia" .

figi-ps:ISTR a owl:NamedIndividual .

figi-ps:CBOA figi-gii:hasUniqueTextIdentifier "CBOA" .

figi-ps:ISTR a figi-gii:PricingSource .

figi-ps:CBOD a owl:NamedIndividual .

figi-ps:ISTR skos:prefLabel "isbankasi" .

figi-ps:CBOD a figi-gii:PricingSource .

figi-ps:ISTR figi-gii:hasUniqueTextIdentifier "ISTR" .

figi-ps:CBOD skos:prefLabel "com bank of dubai" .

figi-ps:ISW0 a owl:NamedIndividual .

figi-ps:CBOD figi-gii:hasUniqueTextIdentifier "CBOD" .

figi-ps:ISW0 a figi-gii:PricingSource .

figi-ps:CBOI a owl:NamedIndividual .

figi-ps:ISW0 skos:prefLabel "ise wholesalet+0lge" .

figi-ps:CBOI a figi-gii:PricingSource .

figi-ps:ISW0 figi-gii:hasUniqueTextIdentifier "ISW0" .

figi-ps:CBOI skos:prefLabel "central bank india" .

figi-ps:ISW1 a owl:NamedIndividual .

figi-ps:CBOI figi-gii:hasUniqueTextIdentifier "CBOI" .

figi-ps:ISW1 a figi-gii:PricingSource .

figi-ps:CBOM a owl:NamedIndividual .

figi-ps:ISW1 skos:prefLabel "ise wholesalet+1lge" .

figi-ps:CBOM a figi-gii:PricingSource .

figi-ps:ISW1 figi-gii:hasUniqueTextIdentifier "ISW1" .

figi-ps:CBOM skos:prefLabel "bank al maghrib" ;
	figi-gii:hasUniqueTextIdentifier "CBOM" .

figi-ps:ISYA a owl:NamedIndividual , figi-gii:PricingSource .

figi-ps:CBPM a owl:NamedIndividual , figi-gii:PricingSource .

figi-ps:ISYA skos:prefLabel "is yatirim" .

figi-ps:CBPM skos:prefLabel "commercebank na" .

figi-ps:ISYA figi-gii:hasUniqueTextIdentifier "ISYA" .

figi-ps:CBPM figi-gii:hasUniqueTextIdentifier "CBPM" .

figi-ps:ITAS a owl:NamedIndividual .

figi-ps:CBQQ a owl:NamedIndividual .

figi-ps:ITAS a figi-gii:PricingSource .

figi-ps:CBQQ a figi-gii:PricingSource .

figi-ps:ITAS skos:prefLabel "itau securities" .

figi-ps:CBQQ skos:prefLabel "commercial bk qatar" .

figi-ps:ITAS figi-gii:hasUniqueTextIdentifier "ITAS" .

figi-ps:CBQQ figi-gii:hasUniqueTextIdentifier "CBQQ" .

figi-ps:ITAU a owl:NamedIndividual , figi-gii:PricingSource .

figi-ps:CBRI a owl:NamedIndividual .

figi-ps:ITAU skos:prefLabel "banco itau" .

figi-ps:CBRI a figi-gii:PricingSource .

figi-ps:ITAU skos:prefLabel "banco itau-buen ayre" .

figi-ps:CBRI skos:prefLabel "citizens bank of ri" .

figi-ps:ITAU figi-gii:hasUniqueTextIdentifier "ITAU" .

figi-ps:CBRI figi-gii:hasUniqueTextIdentifier "CBRI" .

figi-ps:ITHA a owl:NamedIndividual .

figi-ps:CBRO a owl:NamedIndividual .

figi-ps:ITHA a figi-gii:PricingSource .

figi-ps:CBRO a figi-gii:PricingSource .

figi-ps:ITHA skos:prefLabel "icap thailand" .

figi-ps:CBRO skos:prefLabel "cain brothers" .

figi-ps:ITHA figi-gii:hasUniqueTextIdentifier "ITHA" .

figi-ps:CBRO figi-gii:hasUniqueTextIdentifier "CBRO" .

figi-ps:IVC a owl:NamedIndividual .

figi-ps:CBSB a owl:NamedIndividual .

figi-ps:IVC a figi-gii:PricingSource .

figi-ps:CBSB a figi-gii:PricingSource .

figi-ps:IVC skos:prefLabel "iv capital" .

figi-ps:CBSB skos:prefLabel "cbseydler ffm" .

figi-ps:IVC figi-gii:hasUniqueTextIdentifier "IVC" .

figi-ps:CBSB figi-gii:hasUniqueTextIdentifier "CBSB" .

figi-ps:IVCP a owl:NamedIndividual .

figi-ps:CBSL a owl:NamedIndividual .

figi-ps:IVCP a figi-gii:PricingSource .

figi-ps:CBSL a figi-gii:PricingSource .

figi-ps:IVCP skos:prefLabel "invest capital and sec" .

figi-ps:CBSL skos:prefLabel "central bk srilanka" .

figi-ps:IVCP figi-gii:hasUniqueTextIdentifier "IVCP" .

figi-ps:CBSL figi-gii:hasUniqueTextIdentifier "CBSL" .

figi-ps:IVET a owl:NamedIndividual .

figi-ps:CBTK a owl:NamedIndividual .

figi-ps:IVET a figi-gii:PricingSource .

figi-ps:CBTK a figi-gii:PricingSource .

figi-ps:IVET skos:prefLabel "investec bk et" .

figi-ps:CBTK skos:prefLabel "commerz secs" .

figi-ps:IVET figi-gii:hasUniqueTextIdentifier "IVET" .

figi-ps:CBTK figi-gii:hasUniqueTextIdentifier "CBTK" .

figi-ps:IVEX a owl:NamedIndividual .

figi-ps:CBTS a owl:NamedIndividual .

figi-ps:IVEX a figi-gii:PricingSource .

figi-ps:CBTS a figi-gii:PricingSource .

figi-ps:IVEX skos:prefLabel "invex" .

figi-ps:CBTS skos:prefLabel "cboa" .

figi-ps:IVEX figi-gii:hasUniqueTextIdentifier "IVEX" .

figi-ps:CBTS figi-gii:hasUniqueTextIdentifier "CBTS" .

figi-ps:IVSS a owl:NamedIndividual .

figi-ps:CBTU a owl:NamedIndividual .

figi-ps:IVSS a figi-gii:PricingSource .

figi-ps:CBTU a figi-gii:PricingSource .

figi-ps:IVSS skos:prefLabel "investec bank (uk)" .

figi-ps:CBTU skos:prefLabel "central bank tunisia" .

figi-ps:IVSS figi-gii:hasUniqueTextIdentifier "IVSS" .

figi-ps:CBTU figi-gii:hasUniqueTextIdentifier "CBTU" .

figi-ps:IWB a owl:NamedIndividual .

figi-ps:CBTW a owl:NamedIndividual .

figi-ps:IWB a figi-gii:PricingSource .

figi-ps:CBTW a figi-gii:PricingSource .

figi-ps:IWB skos:prefLabel "iw bank" .

figi-ps:CBTW skos:prefLabel "citibank tw" .

figi-ps:IWB figi-gii:hasUniqueTextIdentifier "IWB" .

figi-ps:CBTW figi-gii:hasUniqueTextIdentifier "CBTW" .

figi-ps:IXE a owl:NamedIndividual .

figi-ps:CBUN a owl:NamedIndividual .

figi-ps:IXE a figi-gii:PricingSource .

figi-ps:CBUN a figi-gii:PricingSource .

figi-ps:IXE skos:prefLabel "ixe casa de bolsa" .

figi-ps:CBUN skos:prefLabel "central banco univer" .

figi-ps:IXE figi-gii:hasUniqueTextIdentifier "IXE" .

figi-ps:CBUN figi-gii:hasUniqueTextIdentifier "CBUN" .

figi-ps:IXEC a owl:NamedIndividual .

figi-ps:CCAM a owl:NamedIndividual .

figi-ps:IXEC a figi-gii:PricingSource .

figi-ps:CCAM a figi-gii:PricingSource .

figi-ps:IXEC skos:prefLabel "iboxx-euro coll" .

figi-ps:CCAM skos:prefLabel "conning and co" .

figi-ps:IXEC figi-gii:hasUniqueTextIdentifier "IXEC" .

figi-ps:CCAM figi-gii:hasUniqueTextIdentifier "CCAM" .

figi-ps:IXEF a owl:NamedIndividual .

figi-ps:CCAX a owl:NamedIndividual .

figi-ps:IXEF a figi-gii:PricingSource .

figi-ps:CCAX a figi-gii:PricingSource .

figi-ps:IXEF skos:prefLabel "ixe financial group" .

figi-ps:CCAX skos:prefLabel "la caixa" .

figi-ps:IXEF figi-gii:hasUniqueTextIdentifier "IXEF" .

figi-ps:CCAX figi-gii:hasUniqueTextIdentifier "CCAX" .

figi-ps:IXEP a owl:NamedIndividual .

figi-ps:CCB a owl:NamedIndividual .

figi-ps:IXEP a figi-gii:PricingSource .

figi-ps:CCB a figi-gii:PricingSource .

figi-ps:IXEP skos:prefLabel "iboxx-euro corp cons" .

figi-ps:CCB skos:prefLabel "china construct bk" .

figi-ps:IXEP figi-gii:hasUniqueTextIdentifier "IXEP" .

figi-ps:CCB figi-gii:hasUniqueTextIdentifier "CCB" .

figi-ps:IXES a owl:NamedIndividual .

figi-ps:CCBB a owl:NamedIndividual .

figi-ps:IXES a figi-gii:PricingSource .

figi-ps:CCBB a figi-gii:PricingSource .

figi-ps:IXES skos:prefLabel "iboxx-euro sovereign" .

figi-ps:CCBB skos:prefLabel "cfif ch cnstructn bk" .

figi-ps:IXES figi-gii:hasUniqueTextIdentifier "IXES" .

figi-ps:CCBB figi-gii:hasUniqueTextIdentifier "CCBB" .

figi-ps:IXEV a owl:NamedIndividual .

figi-ps:CCBD a owl:NamedIndividual .

figi-ps:IXEV a figi-gii:PricingSource .

figi-ps:CCBD a figi-gii:PricingSource .

figi-ps:IXEV skos:prefLabel "iboxx-euro sub-sov" .

figi-ps:CCBD skos:prefLabel "cfet construction bk" .

figi-ps:IXEV figi-gii:hasUniqueTextIdentifier "IXEV" .

figi-ps:CCBD figi-gii:hasUniqueTextIdentifier "CCBD" .

figi-ps:IXPI a owl:NamedIndividual .

figi-ps:CCBH a owl:NamedIndividual .

figi-ps:IXPI a figi-gii:PricingSource .

figi-ps:CCBH a figi-gii:PricingSource .

figi-ps:IXPI skos:prefLabel "ic banche popolari" .

figi-ps:CCBH skos:prefLabel "ccbchk" .

figi-ps:IXPI figi-gii:hasUniqueTextIdentifier "IXPI" .

figi-ps:CCBH figi-gii:hasUniqueTextIdentifier "CCBH" .

figi-ps:IXSC a owl:NamedIndividual .

figi-ps:CCBK a owl:NamedIndividual .

figi-ps:IXSC a figi-gii:PricingSource .

figi-ps:CCBK a figi-gii:PricingSource .

figi-ps:IXSC skos:prefLabel "iboxx-ster coll" .

figi-ps:CCBK skos:prefLabel "ccb 11:30" .

figi-ps:IXSC figi-gii:hasUniqueTextIdentifier "IXSC" .

figi-ps:CCBK figi-gii:hasUniqueTextIdentifier "CCBK" .

figi-ps:IXSP a owl:NamedIndividual .

figi-ps:CCBN a owl:NamedIndividual .

figi-ps:IXSP a figi-gii:PricingSource .

figi-ps:CCBN a figi-gii:PricingSource .

figi-ps:IXSP skos:prefLabel "iboxx-ster corp cons" .

figi-ps:CCBN skos:prefLabel "cnbond cbc" .

figi-ps:IXSP figi-gii:hasUniqueTextIdentifier "IXSP" .

figi-ps:CCBN figi-gii:hasUniqueTextIdentifier "CCBN" .

figi-ps:IXSS a owl:NamedIndividual .

figi-ps:CCBP a owl:NamedIndividual .

figi-ps:IXSS a figi-gii:PricingSource .

figi-ps:CCBP a figi-gii:PricingSource .

figi-ps:IXSS skos:prefLabel "iboxx-ster sovereign" .

figi-ps:CCBP skos:prefLabel "ccb 4:30" .

figi-ps:IXSS figi-gii:hasUniqueTextIdentifier "IXSS" .

figi-ps:CCBP figi-gii:hasUniqueTextIdentifier "CCBP" .

figi-ps:IXSV a owl:NamedIndividual .

figi-ps:CCBS a owl:NamedIndividual .

figi-ps:IXSV a figi-gii:PricingSource .

figi-ps:CCBS a figi-gii:PricingSource .

figi-ps:IXSV skos:prefLabel "iboxx-ster sub-sov" .

figi-ps:CCBS skos:prefLabel "central cooperative" .

figi-ps:IXSV figi-gii:hasUniqueTextIdentifier "IXSV" .

figi-ps:CCBS figi-gii:hasUniqueTextIdentifier "CCBS" .

figi-ps:IYL1 a owl:NamedIndividual .

figi-ps:CCC a owl:NamedIndividual .

figi-ps:IYL1 a figi-gii:PricingSource .

figi-ps:CCC a figi-gii:PricingSource .

figi-ps:IYL1 skos:prefLabel "iseb large t+1 (yld)" .

figi-ps:CCC skos:prefLabel "climate change cap" .

figi-ps:IYL1 figi-gii:hasUniqueTextIdentifier "IYL1" .

figi-ps:CCC figi-gii:hasUniqueTextIdentifier "CCC" .

figi-ps:IYM a owl:NamedIndividual .

figi-ps:CCCM a owl:NamedIndividual .

figi-ps:IYM a figi-gii:PricingSource .

figi-ps:CCCM a figi-gii:PricingSource .

figi-ps:IYM skos:prefLabel "is investment" .

figi-ps:CCCM skos:prefLabel "caroline capital" .

figi-ps:IYM figi-gii:hasUniqueTextIdentifier "IYM" .

figi-ps:CCCM figi-gii:hasUniqueTextIdentifier "CCCM" .

figi-ps:IYS1 a owl:NamedIndividual .

figi-ps:CCDO a owl:NamedIndividual .

figi-ps:IYS1 a figi-gii:PricingSource .

figi-ps:CCDO a figi-gii:PricingSource .

figi-ps:IYS1 skos:prefLabel "iseb small t+1 (yld)" .

figi-ps:CCDO skos:prefLabel "citigroup syn cdo" .

figi-ps:IYS1 figi-gii:hasUniqueTextIdentifier "IYS1" .

figi-ps:CCDO figi-gii:hasUniqueTextIdentifier "CCDO" .

figi-ps:JABS a owl:NamedIndividual .

figi-ps:CCG a owl:NamedIndividual .

figi-ps:JABS a figi-gii:PricingSource .

figi-ps:CCG a figi-gii:PricingSource .

figi-ps:JABS skos:prefLabel "jp morgan uk abs" .

figi-ps:CCG skos:prefLabel "caixa cataluna gesti" .

figi-ps:JABS figi-gii:hasUniqueTextIdentifier "JABS" .

figi-ps:CCG figi-gii:hasUniqueTextIdentifier "CCG" .

figi-ps:JADW a owl:NamedIndividual .

figi-ps:CCI a owl:NamedIndividual .

figi-ps:JADW a figi-gii:PricingSource .

figi-ps:CCI a figi-gii:PricingSource .

figi-ps:JADW skos:prefLabel "jadwa investment" .

figi-ps:CCI skos:prefLabel "credit capital inv" .

figi-ps:JADW figi-gii:hasUniqueTextIdentifier "JADW" .

figi-ps:CCI figi-gii:hasUniqueTextIdentifier "CCI" .

figi-ps:JAGN a owl:NamedIndividual .

figi-ps:CCL a owl:NamedIndividual .

figi-ps:JAGN a figi-gii:PricingSource .

figi-ps:CCL a figi-gii:PricingSource .

figi-ps:JAGN skos:prefLabel "jefferies agencies" .

figi-ps:CCL skos:prefLabel "constellation cap" .

figi-ps:JAGN figi-gii:hasUniqueTextIdentifier "JAGN" .

figi-ps:CCL figi-gii:hasUniqueTextIdentifier "CCL" .

figi-ps:JAMX a owl:NamedIndividual .

figi-ps:CCM a owl:NamedIndividual .

figi-ps:JAMX a figi-gii:PricingSource .

figi-ps:CCM a figi-gii:PricingSource .

figi-ps:JAMX skos:prefLabel "jp morg mexico aex" .

figi-ps:CCM skos:prefLabel "continental capital" .

figi-ps:JAMX figi-gii:hasUniqueTextIdentifier "JAMX" .

figi-ps:CCM figi-gii:hasUniqueTextIdentifier "CCM" .

figi-ps:JANC a owl:NamedIndividual .

figi-ps:CCMB a owl:NamedIndividual .

figi-ps:JANC a figi-gii:PricingSource .

figi-ps:CCMB a figi-gii:PricingSource .

figi-ps:JANC skos:prefLabel "janco partners, inc." .

figi-ps:CCMB skos:prefLabel "capital credit merch" .

figi-ps:JANC figi-gii:hasUniqueTextIdentifier "JANC" .

figi-ps:CCMB figi-gii:hasUniqueTextIdentifier "CCMB" .

figi-ps:JANE a owl:NamedIndividual .

figi-ps:CCME a owl:NamedIndividual .

figi-ps:JANE a figi-gii:PricingSource .

figi-ps:CCME a figi-gii:PricingSource .

figi-ps:JANE skos:prefLabel "jane street capital" .

figi-ps:CCME skos:prefLabel "commerzbank capital" .

figi-ps:JANE figi-gii:hasUniqueTextIdentifier "JANE" .

figi-ps:CCME figi-gii:hasUniqueTextIdentifier "CCME" .

figi-ps:JARG a owl:NamedIndividual .

figi-ps:CCMI a owl:NamedIndividual .

figi-ps:JARG a figi-gii:PricingSource .

figi-ps:CCMI a figi-gii:PricingSource .

figi-ps:JARG skos:prefLabel "jpm argentina" .

figi-ps:CCMI skos:prefLabel "commerce capital mkt" .

figi-ps:JARG figi-gii:hasUniqueTextIdentifier "JARG" .

figi-ps:CCMI figi-gii:hasUniqueTextIdentifier "CCMI" .

figi-ps:JBCM a owl:NamedIndividual , figi-gii:PricingSource .

figi-ps:CCMK a owl:NamedIndividual .

figi-ps:JBCM skos:prefLabel "jb capital markets" .

figi-ps:CCMK a figi-gii:PricingSource .

figi-ps:JBCM figi-gii:hasUniqueTextIdentifier "JBCM" .

figi-ps:CCMK skos:prefLabel "conticap indicative" .

figi-ps:JBFI a owl:NamedIndividual .

figi-ps:CCMK figi-gii:hasUniqueTextIdentifier "CCMK" .

figi-ps:JBFI a figi-gii:PricingSource .

figi-ps:CCMQ a owl:NamedIndividual .

figi-ps:JBFI skos:prefLabel "banco jp morgan sa" .

figi-ps:CCMQ a figi-gii:PricingSource .

figi-ps:JBFI figi-gii:hasUniqueTextIdentifier "JBFI" .

figi-ps:CCMQ skos:prefLabel "carolina capital" .

figi-ps:JBI a owl:NamedIndividual .

figi-ps:CCMQ figi-gii:hasUniqueTextIdentifier "CCMQ" .

figi-ps:JBI a figi-gii:PricingSource .

figi-ps:CCMS a owl:NamedIndividual .

figi-ps:JBI skos:prefLabel "jp local bond assoc" .

figi-ps:CCMS a figi-gii:PricingSource .

figi-ps:JBI figi-gii:hasUniqueTextIdentifier "JBI" .

figi-ps:CCMS skos:prefLabel "continental cap mrkt" .

figi-ps:JBM a owl:NamedIndividual .

figi-ps:CCMS figi-gii:hasUniqueTextIdentifier "CCMS" .

figi-ps:JBM a figi-gii:PricingSource .

figi-ps:CCMX a owl:NamedIndividual .

figi-ps:JBM skos:prefLabel "joint baltic market" .

figi-ps:CCMX a figi-gii:PricingSource .

figi-ps:JBM figi-gii:hasUniqueTextIdentifier "JBM" .

figi-ps:CCMX skos:prefLabel "conduit cap mkts" .

figi-ps:JBON a owl:NamedIndividual .

figi-ps:CCMX figi-gii:hasUniqueTextIdentifier "CCMX" .

figi-ps:JBON a figi-gii:PricingSource .

figi-ps:CCMZ a owl:NamedIndividual .

figi-ps:JBON skos:prefLabel "jbond securities" .

figi-ps:CCMZ a figi-gii:PricingSource .

figi-ps:JBON figi-gii:hasUniqueTextIdentifier "JBON" .

figi-ps:CCMZ skos:prefLabel "continental capital" .

figi-ps:JBRL a owl:NamedIndividual .

figi-ps:CCMZ figi-gii:hasUniqueTextIdentifier "CCMZ" .

figi-ps:JBRL a figi-gii:PricingSource ;
	skos:prefLabel "jpmorgan ldn" .

figi-ps:CCOM a owl:NamedIndividual .

figi-ps:JBRL figi-gii:hasUniqueTextIdentifier "JBRL" .

figi-ps:CCOM a figi-gii:PricingSource .

figi-ps:JBST a owl:NamedIndividual .

figi-ps:CCOM skos:prefLabel "commerzbank certs" .

figi-ps:JBST a figi-gii:PricingSource .

figi-ps:CCOM figi-gii:hasUniqueTextIdentifier "CCOM" .

figi-ps:JBST skos:prefLabel "julius baer" .

figi-ps:CCP a owl:NamedIndividual .

figi-ps:JBST figi-gii:hasUniqueTextIdentifier "JBST" .

figi-ps:CCP a figi-gii:PricingSource .

figi-ps:JBWA a owl:NamedIndividual .

figi-ps:CCP skos:prefLabel "chapdelaine credit" .

figi-ps:JBWA a figi-gii:PricingSource .

figi-ps:CCP figi-gii:hasUniqueTextIdentifier "CCP" .

figi-ps:JBWA skos:prefLabel "jb were" .

figi-ps:CCSJ a owl:NamedIndividual .

figi-ps:JBWA figi-gii:hasUniqueTextIdentifier "JBWA" .

figi-ps:CCSJ a figi-gii:PricingSource .

figi-ps:JCAG a owl:NamedIndividual .

figi-ps:CCSJ skos:prefLabel "capital credit" .

figi-ps:JCAG a figi-gii:PricingSource .

figi-ps:CCSJ figi-gii:hasUniqueTextIdentifier "CCSJ" .

figi-ps:JCAG skos:prefLabel "jefferies agencies" .

figi-ps:CDBC a owl:NamedIndividual .

figi-ps:JCAG figi-gii:hasUniqueTextIdentifier "JCAG" .

figi-ps:CDBC a figi-gii:PricingSource .

figi-ps:JCDO a owl:NamedIndividual .

figi-ps:CDBC skos:prefLabel "china development bk" .

figi-ps:JCDO a figi-gii:PricingSource .

figi-ps:CDBC figi-gii:hasUniqueTextIdentifier "CDBC" .

figi-ps:JCDO skos:prefLabel "jpmorgan jcdo" .

figi-ps:CDBH a owl:NamedIndividual .

figi-ps:JCDO figi-gii:hasUniqueTextIdentifier "JCDO" .

figi-ps:CDBH a figi-gii:PricingSource .

figi-ps:JCEF a owl:NamedIndividual .

figi-ps:CDBH skos:prefLabel "chinadevelopmentbank" .

figi-ps:JCEF a figi-gii:PricingSource .

figi-ps:CDBH figi-gii:hasUniqueTextIdentifier "CDBH" .

figi-ps:JCEF skos:prefLabel "jefferies funds" .

figi-ps:CDBI a owl:NamedIndividual .

figi-ps:JCEF figi-gii:hasUniqueTextIdentifier "JCEF" .

figi-ps:CDBI a figi-gii:PricingSource .

figi-ps:JCEM a owl:NamedIndividual .

figi-ps:CDBI skos:prefLabel "china dev bk fin mkt" .

figi-ps:JCEM a figi-gii:PricingSource .

figi-ps:CDBI figi-gii:hasUniqueTextIdentifier "CDBI" .

figi-ps:JCEM skos:prefLabel "jefferies internal" .

figi-ps:CDBN a owl:NamedIndividual .

figi-ps:JCEM figi-gii:hasUniqueTextIdentifier "JCEM" .

figi-ps:CDBN a figi-gii:PricingSource .

figi-ps:JCMO a owl:NamedIndividual .

figi-ps:CDBN skos:prefLabel "china dev bk indicat" .

figi-ps:JCMO a figi-gii:PricingSource .

figi-ps:CDBN figi-gii:hasUniqueTextIdentifier "CDBN" .

figi-ps:JCMO skos:prefLabel "jp morgan ny abs" .

figi-ps:CDBQ a owl:NamedIndividual .

figi-ps:JCMO figi-gii:hasUniqueTextIdentifier "JCMO" .

figi-ps:CDBQ a figi-gii:PricingSource .

figi-ps:JCOR a owl:NamedIndividual .

figi-ps:CDBQ skos:prefLabel "cfif china dev bank" .

figi-ps:JCOR a figi-gii:PricingSource .

figi-ps:CDBQ figi-gii:hasUniqueTextIdentifier "CDBQ" .

figi-ps:JCOR skos:prefLabel "jefferies pricing" .

figi-ps:CDBS a owl:NamedIndividual .

figi-ps:JCOR figi-gii:hasUniqueTextIdentifier "JCOR" .

figi-ps:CDBS a figi-gii:PricingSource .

figi-ps:JCPC a owl:NamedIndividual .

figi-ps:CDBS skos:prefLabel "bear stearns nyc" .

figi-ps:JCPC a figi-gii:PricingSource .

figi-ps:CDBS figi-gii:hasUniqueTextIdentifier "CDBS" .

figi-ps:JCPC skos:prefLabel "jermyn cap ptnrs pl" .

figi-ps:CDCC a owl:NamedIndividual .

figi-ps:JCPC figi-gii:hasUniqueTextIdentifier "JCPC" .

figi-ps:CDCC a figi-gii:PricingSource .

figi-ps:JCR1 a owl:NamedIndividual .

figi-ps:CDCC skos:prefLabel "chinabond-cdc clean" .

figi-ps:JCR1 a figi-gii:PricingSource .

figi-ps:CDCC figi-gii:hasUniqueTextIdentifier "CDCC" .

figi-ps:JCR1 skos:prefLabel "jefferies b" .

figi-ps:CDCD a owl:NamedIndividual .

figi-ps:JCR1 figi-gii:hasUniqueTextIdentifier "JCR1" .

figi-ps:CDCD a figi-gii:PricingSource .

figi-ps:JCR3 a owl:NamedIndividual .

figi-ps:CDCD skos:prefLabel "chinabond-cdc dirty" .

figi-ps:JCR3 a figi-gii:PricingSource .

figi-ps:CDCD figi-gii:hasUniqueTextIdentifier "CDCD" .

figi-ps:JCR3 skos:prefLabel "jefferies c" .

figi-ps:CDCE a owl:NamedIndividual .

figi-ps:JCR3 figi-gii:hasUniqueTextIdentifier "JCR3" .

figi-ps:CDCE a figi-gii:PricingSource .

figi-ps:JEF a owl:NamedIndividual .

figi-ps:CDCE skos:prefLabel "caisse des depots" .

figi-ps:JEF a figi-gii:PricingSource .

figi-ps:CDCE figi-gii:hasUniqueTextIdentifier "CDCE" .

figi-ps:JEF skos:prefLabel "jefferies-bd" .

figi-ps:CDES a owl:NamedIndividual .

figi-ps:JEF figi-gii:hasUniqueTextIdentifier "JEF" .

figi-ps:CDES a figi-gii:PricingSource .

figi-ps:JEFX a owl:NamedIndividual .

figi-ps:CDES skos:prefLabel "citadel" .

figi-ps:JEFX a figi-gii:PricingSource .

figi-ps:CDES figi-gii:hasUniqueTextIdentifier "CDES" .

figi-ps:JEFX skos:prefLabel "jefferies intl" .

figi-ps:CDP a owl:NamedIndividual .

figi-ps:JEFX figi-gii:hasUniqueTextIdentifier "JEFX" .

figi-ps:CDP a figi-gii:PricingSource .

figi-ps:JESP a owl:NamedIndividual .

figi-ps:CDP skos:prefLabel "caisse de depot" .

figi-ps:JESP a figi-gii:PricingSource .

figi-ps:CDP figi-gii:hasUniqueTextIdentifier "CDP" .

figi-ps:JESP skos:prefLabel "jesup and lamont" .

figi-ps:CDQA a owl:NamedIndividual .

figi-ps:JESP figi-gii:hasUniqueTextIdentifier "JESP" .

figi-ps:CDQA a figi-gii:PricingSource .

figi-ps:JFED a owl:NamedIndividual .

figi-ps:CDQA skos:prefLabel "codestreet qa" .

figi-ps:JFED a figi-gii:PricingSource .

figi-ps:CDQA figi-gii:hasUniqueTextIdentifier "CDQA" .

figi-ps:JFED skos:prefLabel "jefferies structured" .

figi-ps:CDST a owl:NamedIndividual .

figi-ps:JFED figi-gii:hasUniqueTextIdentifier "JFED" .

figi-ps:CDST a figi-gii:PricingSource .

figi-ps:JFLO a owl:NamedIndividual .

figi-ps:CDST skos:prefLabel "codestreet" .

figi-ps:JFLO a figi-gii:PricingSource .

figi-ps:CDST figi-gii:hasUniqueTextIdentifier "CDST" .

figi-ps:JFLO skos:prefLabel "jefferies int ltd" .

figi-ps:CDZE a owl:NamedIndividual .

figi-ps:JFLO figi-gii:hasUniqueTextIdentifier "JFLO" .

figi-ps:CDZE a figi-gii:PricingSource .

figi-ps:JFRX a owl:NamedIndividual .

figi-ps:CDZE skos:prefLabel "cadiz sa e-bond" .

figi-ps:JFRX a figi-gii:PricingSource .

figi-ps:CDZE figi-gii:hasUniqueTextIdentifier "CDZE" .

figi-ps:JFRX skos:prefLabel "jefferies c" .

figi-ps:CEBA a owl:NamedIndividual .

figi-ps:JFRX figi-gii:hasUniqueTextIdentifier "JFRX" .

figi-ps:CEBA a figi-gii:PricingSource .

figi-ps:JFUA a owl:NamedIndividual .

figi-ps:CEBA skos:prefLabel "credit europe bank" .

figi-ps:JFUA a figi-gii:PricingSource .

figi-ps:CEBA figi-gii:hasUniqueTextIdentifier "CEBA" .

figi-ps:JFUA skos:prefLabel "jefferies and co inc" .

figi-ps:CEBK a owl:NamedIndividual .

figi-ps:JFUA figi-gii:hasUniqueTextIdentifier "JFUA" .

figi-ps:CEBK a figi-gii:PricingSource .

figi-ps:JGBA a owl:NamedIndividual .

figi-ps:CEBK skos:prefLabel "china everbright bk" .

figi-ps:JGBA a figi-gii:PricingSource .

figi-ps:CEBK figi-gii:hasUniqueTextIdentifier "CEBK" .

figi-ps:JGBA skos:prefLabel "central tanshi tokyo" .

figi-ps:CEC a owl:NamedIndividual .

figi-ps:JGBA figi-gii:hasUniqueTextIdentifier "JGBA" .

figi-ps:CEC a figi-gii:PricingSource .

figi-ps:JHSC a owl:NamedIndividual .

figi-ps:CEC skos:prefLabel "ceca madrid - abs" .

figi-ps:JHSC a figi-gii:PricingSource .

figi-ps:CEC figi-gii:hasUniqueTextIdentifier "CEC" .

figi-ps:JHSC skos:prefLabel "jhs capital advisors" .

figi-ps:CECA a owl:NamedIndividual .

figi-ps:JHSC figi-gii:hasUniqueTextIdentifier "JHSC" .

figi-ps:CECA a figi-gii:PricingSource .

figi-ps:JIBK a owl:NamedIndividual .

figi-ps:CECA skos:prefLabel "cecabank" .

figi-ps:JIBK a figi-gii:PricingSource .

figi-ps:CECA figi-gii:hasUniqueTextIdentifier "CECA" .

figi-ps:JIBK skos:prefLabel "jordan intl bank" .

figi-ps:CEEM a owl:NamedIndividual .

figi-ps:JIBK figi-gii:hasUniqueTextIdentifier "JIBK" .

figi-ps:CEEM a figi-gii:PricingSource .

figi-ps:JIFI a owl:NamedIndividual .

figi-ps:CEEM skos:prefLabel "cs emerging markets" .

figi-ps:JIFI a figi-gii:PricingSource .

figi-ps:CEEM figi-gii:hasUniqueTextIdentifier "CEEM" .

figi-ps:JIFI skos:prefLabel "jefferies intl" .

figi-ps:CELA a owl:NamedIndividual .

figi-ps:JIFI figi-gii:hasUniqueTextIdentifier "JIFI" .

figi-ps:CELA a figi-gii:PricingSource .

figi-ps:JINT a owl:NamedIndividual .

figi-ps:CELA skos:prefLabel "celfin capital asset" .

figi-ps:JINT a figi-gii:PricingSource .

figi-ps:CELA figi-gii:hasUniqueTextIdentifier "CELA" .

figi-ps:JINT skos:prefLabel "jp morgan intrinsic" .

figi-ps:CELE a owl:NamedIndividual .

figi-ps:JINT figi-gii:hasUniqueTextIdentifier "JINT" .

figi-ps:CELE a figi-gii:PricingSource .

figi-ps:JIPB a owl:NamedIndividual .

figi-ps:CELE skos:prefLabel "celfin capital" .

figi-ps:JIPB a figi-gii:PricingSource .

figi-ps:CELE figi-gii:hasUniqueTextIdentifier "CELE" .

figi-ps:JIPB skos:prefLabel "jp morgan ipb" .

figi-ps:CELF a owl:NamedIndividual .

figi-ps:JIPB figi-gii:hasUniqueTextIdentifier "JIPB" .

figi-ps:CELF a figi-gii:PricingSource .

figi-ps:JJ a owl:NamedIndividual .

figi-ps:CELF skos:prefLabel "celfin capital" .

figi-ps:JJ a figi-gii:PricingSource .

figi-ps:CELF figi-gii:hasUniqueTextIdentifier "CELF" .

figi-ps:JJ skos:prefLabel "jj kenny drake" .

figi-ps:CEM a owl:NamedIndividual .

figi-ps:JJ figi-gii:hasUniqueTextIdentifier "JJ" .

figi-ps:CEM a figi-gii:PricingSource .

figi-ps:JJEY a owl:NamedIndividual .

figi-ps:CEM skos:prefLabel "cantor co2e" .

figi-ps:JJEY a figi-gii:PricingSource .

figi-ps:CEM figi-gii:hasUniqueTextIdentifier "CEM" .

figi-ps:JJEY skos:prefLabel "jefferies" .

figi-ps:CEMM a owl:NamedIndividual .

figi-ps:JJEY figi-gii:hasUniqueTextIdentifier "JJEY" .

figi-ps:CEMM a figi-gii:PricingSource .

figi-ps:JKBK a owl:NamedIndividual .

figi-ps:CEMM skos:prefLabel "credem" .

figi-ps:JKBK a figi-gii:PricingSource .

figi-ps:CEMM figi-gii:hasUniqueTextIdentifier "CEMM" .

figi-ps:JKBK skos:prefLabel "jammu and kashmir bk" .

figi-ps:CENT a owl:NamedIndividual .

figi-ps:JKBK figi-gii:hasUniqueTextIdentifier "JKBK" .

figi-ps:CENT a figi-gii:PricingSource .

figi-ps:JKM a owl:NamedIndividual .

figi-ps:CENT skos:prefLabel "centrica" .

figi-ps:JKM a figi-gii:PricingSource .

figi-ps:CENT figi-gii:hasUniqueTextIdentifier "CENT" .

figi-ps:JKM skos:prefLabel "jkmilne asset mngt" .

figi-ps:CEPE a owl:NamedIndividual .

figi-ps:JKM figi-gii:hasUniqueTextIdentifier "JKM" .

figi-ps:CEPE a figi-gii:PricingSource .

figi-ps:JLAM a owl:NamedIndividual .

figi-ps:CEPE skos:prefLabel "caixa penedes" .

figi-ps:JLAM a figi-gii:PricingSource .

figi-ps:CEPE figi-gii:hasUniqueTextIdentifier "CEPE" .

figi-ps:JLAM skos:prefLabel "jpmorgan chase bank" ;
	figi-gii:hasUniqueTextIdentifier "JLAM" .

figi-ps:CERO a owl:NamedIndividual .

figi-ps:JLBI a owl:NamedIndividual .

figi-ps:CERO a figi-gii:PricingSource .

figi-ps:JLBI a figi-gii:PricingSource .

figi-ps:CERO skos:prefLabel "credit europe bk" .

figi-ps:JLBI skos:prefLabel "jbi" .

figi-ps:CERO figi-gii:hasUniqueTextIdentifier "CERO" .

figi-ps:JLBI figi-gii:hasUniqueTextIdentifier "JLBI" .

figi-ps:CESA a owl:NamedIndividual .

figi-ps:JLCM a owl:NamedIndividual .

figi-ps:CESA a figi-gii:PricingSource .

figi-ps:JLCM a figi-gii:PricingSource .

figi-ps:CESA skos:prefLabel "celfin sa" .

figi-ps:JLCM skos:prefLabel "jesup and lamont" .

figi-ps:CESA figi-gii:hasUniqueTextIdentifier "CESA" .

figi-ps:JLCM figi-gii:hasUniqueTextIdentifier "JLCM" .

figi-ps:CEY a owl:NamedIndividual .

figi-ps:JLTA a owl:NamedIndividual .

figi-ps:CEY a figi-gii:PricingSource .

figi-ps:JLTA a figi-gii:PricingSource .

figi-ps:CEY skos:prefLabel "bank of ceylon" .

figi-ps:JLTA skos:prefLabel "jpmorgan latam" .

figi-ps:CEY figi-gii:hasUniqueTextIdentifier "CEY" .

figi-ps:JLTA figi-gii:hasUniqueTextIdentifier "JLTA" .

figi-ps:CEYB a owl:NamedIndividual .

figi-ps:JMBB a owl:NamedIndividual .

figi-ps:CEYB a figi-gii:PricingSource .

figi-ps:JMBB a figi-gii:PricingSource .

figi-ps:CEYB skos:prefLabel "bank of ceylon ltd" .

figi-ps:JMBB skos:prefLabel "jamaica money market" .

figi-ps:CEYB figi-gii:hasUniqueTextIdentifier "CEYB" .

figi-ps:JMBB figi-gii:hasUniqueTextIdentifier "JMBB" .

figi-ps:CEYL a owl:NamedIndividual .

figi-ps:JMBS a owl:NamedIndividual .

figi-ps:CEYL a figi-gii:PricingSource .

figi-ps:JMBS a figi-gii:PricingSource .

figi-ps:CEYL skos:prefLabel "entrust limited" .

figi-ps:JMBS skos:prefLabel "jefferies mortgages" .

figi-ps:CEYL figi-gii:hasUniqueTextIdentifier "CEYL" .

figi-ps:JMBS figi-gii:hasUniqueTextIdentifier "JMBS" .

figi-ps:CFAG a owl:NamedIndividual .

figi-ps:JMCB a owl:NamedIndividual .

figi-ps:CFAG a figi-gii:PricingSource .

figi-ps:JMCB a figi-gii:PricingSource .

figi-ps:CFAG skos:prefLabel "cantorfitz-agencies" .

figi-ps:JMCB skos:prefLabel "jpmorgan asia" .

figi-ps:CFAG figi-gii:hasUniqueTextIdentifier "CFAG" .

figi-ps:JMCB figi-gii:hasUniqueTextIdentifier "JMCB" .

figi-ps:CFBN a owl:NamedIndividual .

figi-ps:JMCH a owl:NamedIndividual .

figi-ps:CFBN a figi-gii:PricingSource .

figi-ps:JMCH a figi-gii:PricingSource .

figi-ps:CFBN skos:prefLabel "citigroup, hong kong" .

figi-ps:JMCH skos:prefLabel "cfet jp morgan china" .

figi-ps:CFBN figi-gii:hasUniqueTextIdentifier "CFBN" .

figi-ps:JMCH figi-gii:hasUniqueTextIdentifier "JMCH" .

figi-ps:CFCA a owl:NamedIndividual .

figi-ps:JMET a owl:NamedIndividual .

figi-ps:CFCA a figi-gii:PricingSource .

figi-ps:JMET a figi-gii:PricingSource .

figi-ps:CFCA skos:prefLabel "cantor agency inside" .

figi-ps:JMET skos:prefLabel "jp morgan asia" .

figi-ps:CFCA figi-gii:hasUniqueTextIdentifier "CFCA" .

figi-ps:JMET figi-gii:hasUniqueTextIdentifier "JMET" .

figi-ps:CFCC a owl:NamedIndividual .

figi-ps:JMMB a owl:NamedIndividual .

figi-ps:CFCC a figi-gii:PricingSource .

figi-ps:JMMB a figi-gii:PricingSource .

figi-ps:CFCC skos:prefLabel "cantorfitz-insidepx" .

figi-ps:JMMB skos:prefLabel "jamaica money market" .

figi-ps:CFCC figi-gii:hasUniqueTextIdentifier "CFCC" .

figi-ps:JMMB figi-gii:hasUniqueTextIdentifier "JMMB" .

figi-ps:CFEB a owl:NamedIndividual .

figi-ps:JMMS a owl:NamedIndividual .

figi-ps:CFEB a figi-gii:PricingSource .

figi-ps:JMMS a figi-gii:PricingSource .

figi-ps:CFEB skos:prefLabel "cantor fitzgerald hk" .

figi-ps:JMMS skos:prefLabel "j.m. morgan stanley" .

figi-ps:CFEB figi-gii:hasUniqueTextIdentifier "CFEB" .

figi-ps:JMMS figi-gii:hasUniqueTextIdentifier "JMMS" .

figi-ps:CFEM a owl:NamedIndividual .

figi-ps:JMPD a owl:NamedIndividual .

figi-ps:CFEM a figi-gii:PricingSource .

figi-ps:JMPD a figi-gii:PricingSource .

figi-ps:CFEM skos:prefLabel "cantor-emergingmrkts" .

figi-ps:JMPD skos:prefLabel "jm financial product" .

figi-ps:CFEM figi-gii:hasUniqueTextIdentifier "CFEM" .

figi-ps:JMPD figi-gii:hasUniqueTextIdentifier "JMPD" .

figi-ps:CFET a owl:NamedIndividual .

figi-ps:JMS a owl:NamedIndividual .

figi-ps:CFET a figi-gii:PricingSource .

figi-ps:JMS a figi-gii:PricingSource .

figi-ps:CFET skos:prefLabel "cfet outright repo" .

figi-ps:JMS skos:prefLabel "janney montgomery" .

figi-ps:CFET figi-gii:hasUniqueTextIdentifier "CFET" .

figi-ps:JMS figi-gii:hasUniqueTextIdentifier "JMS" .

figi-ps:CFFB a owl:NamedIndividual .

figi-ps:JNAT a owl:NamedIndividual .

figi-ps:CFFB a figi-gii:PricingSource .

figi-ps:JNAT a figi-gii:PricingSource .

figi-ps:CFFB skos:prefLabel "credit suisse japan" .

figi-ps:JNAT skos:prefLabel "jamaica national bld" .

figi-ps:CFFB figi-gii:hasUniqueTextIdentifier "CFFB" .

figi-ps:CFGT a owl:NamedIndividual , figi-gii:PricingSource ;
	skos:prefLabel "cf global trading" ;
	figi-gii:hasUniqueTextIdentifier "CFGT" .

figi-ps:CFH a owl:NamedIndividual , figi-gii:PricingSource ;
	skos:prefLabel "cathay holdings" .

figi-ps:JNAT figi-gii:hasUniqueTextIdentifier "JNAT" .

figi-ps:CFH figi-gii:hasUniqueTextIdentifier "CFH" .

figi-ps:JNBS a owl:NamedIndividual .

figi-ps:CFHC a owl:NamedIndividual .

figi-ps:JNBS a figi-gii:PricingSource .

figi-ps:CFHC a figi-gii:PricingSource .

figi-ps:JNBS skos:prefLabel "jamaican national bs" .

figi-ps:CFHC skos:prefLabel "cathay financial" .

figi-ps:JNBS figi-gii:hasUniqueTextIdentifier "JNBS" .

figi-ps:CFHC figi-gii:hasUniqueTextIdentifier "CFHC" .

figi-ps:JNES a owl:NamedIndividual .

figi-ps:CFIM a owl:NamedIndividual .

figi-ps:JNES a figi-gii:PricingSource .

figi-ps:CFIM a figi-gii:PricingSource .

figi-ps:JNES skos:prefLabel "jonestrading" .

figi-ps:CFIM skos:prefLabel "commerzbank, london" .

figi-ps:JNES figi-gii:hasUniqueTextIdentifier "JNES" .

figi-ps:CFIM figi-gii:hasUniqueTextIdentifier "CFIM" .

figi-ps:JOEX a owl:NamedIndividual .

figi-ps:CFIY a owl:NamedIndividual .

figi-ps:JOEX a figi-gii:PricingSource .

figi-ps:CFIY a figi-gii:PricingSource .

figi-ps:JOEX skos:prefLabel "amman stock exchange" .

figi-ps:CFIY skos:prefLabel "cfets-icap yield" .

figi-ps:JOEX figi-gii:hasUniqueTextIdentifier "JOEX" .

figi-ps:CFIY figi-gii:hasUniqueTextIdentifier "CFIY" .

figi-ps:JOHC a owl:NamedIndividual .

figi-ps:CFMI a owl:NamedIndividual .

figi-ps:JOHC a figi-gii:PricingSource .

figi-ps:CFMI a figi-gii:PricingSource .

figi-ps:JOHC skos:prefLabel "jo hambro capital" .

figi-ps:CFMI skos:prefLabel "ceat financial" ;
	figi-gii:hasUniqueTextIdentifier "CFMI" .

figi-ps:CFNY a owl:NamedIndividual , figi-gii:PricingSource ;
	skos:prefLabel "cantor fitzgerald" .

figi-ps:JOHC figi-gii:hasUniqueTextIdentifier "JOHC" .

figi-ps:CFNY figi-gii:hasUniqueTextIdentifier "CFNY" .

figi-ps:JONE a owl:NamedIndividual .

figi-ps:CFRN a owl:NamedIndividual .

figi-ps:JONE a figi-gii:PricingSource .

figi-ps:CFRN a figi-gii:PricingSource .

figi-ps:JONE skos:prefLabel "jonestrading inst" .

figi-ps:CFRN skos:prefLabel "bgc partners ldn" .

figi-ps:JONE figi-gii:hasUniqueTextIdentifier "JONE" .

figi-ps:CFRN figi-gii:hasUniqueTextIdentifier "CFRN" .

figi-ps:JPAA a owl:NamedIndividual .

figi-ps:CG a owl:NamedIndividual .

figi-ps:JPAA a figi-gii:PricingSource .

figi-ps:CG a figi-gii:PricingSource ;
	skos:prefLabel "citigroup" ;
	figi-gii:hasUniqueTextIdentifier "CG" .

figi-ps:CGA a owl:NamedIndividual , figi-gii:PricingSource ;
	skos:prefLabel "cibc asset uat" ;
	figi-gii:hasUniqueTextIdentifier "CGA" .

figi-ps:CGAB a owl:NamedIndividual , figi-gii:PricingSource ;
	skos:prefLabel "citigroup gl markets" ;
	figi-gii:hasUniqueTextIdentifier "CGAB" .

figi-ps:CGAE a owl:NamedIndividual , figi-gii:PricingSource ;
	skos:prefLabel "citigroup us agency" ;
	figi-gii:hasUniqueTextIdentifier "CGAE" .

figi-ps:JPAA skos:prefLabel "jp morgan japan eqd" .

figi-ps:CGAG a owl:NamedIndividual , figi-gii:PricingSource .

figi-ps:JPAA figi-gii:hasUniqueTextIdentifier "JPAA" .

figi-ps:CGAG skos:prefLabel "citi - agencies" .

figi-ps:JPAB a owl:NamedIndividual .

figi-ps:CGAG figi-gii:hasUniqueTextIdentifier "CGAG" .

figi-ps:JPAB a figi-gii:PricingSource .

figi-ps:CGAP a owl:NamedIndividual .

figi-ps:JPAB skos:prefLabel "jpmorgan abs" .

figi-ps:CGAP a figi-gii:PricingSource .

figi-ps:JPAB figi-gii:hasUniqueTextIdentifier "JPAB" .

figi-ps:CGAP skos:prefLabel "citigroup mrkts asia" .

figi-ps:JPAE a owl:NamedIndividual .

figi-ps:CGAP figi-gii:hasUniqueTextIdentifier "CGAP" .

figi-ps:JPAE a figi-gii:PricingSource .

figi-ps:CGAU a owl:NamedIndividual .

figi-ps:JPAE skos:prefLabel "jp morgan aust etf" .

figi-ps:CGAU a figi-gii:PricingSource .

figi-ps:JPAE figi-gii:hasUniqueTextIdentifier "JPAE" .

figi-ps:CGAU skos:prefLabel "citigroup gm aus" .

figi-ps:JPAP a owl:NamedIndividual , figi-gii:PricingSource .

figi-ps:CGAU figi-gii:hasUniqueTextIdentifier "CGAU" .

figi-ps:JPAP skos:prefLabel "jp morgan asia" .

figi-ps:CGAX a owl:NamedIndividual .

figi-ps:JPAP figi-gii:hasUniqueTextIdentifier "JPAP" .

figi-ps:CGAX a figi-gii:PricingSource .

figi-ps:JPAR a owl:NamedIndividual .

figi-ps:CGAX skos:prefLabel "citigroup spreads" .

figi-ps:JPAR a figi-gii:PricingSource .

figi-ps:CGAX figi-gii:hasUniqueTextIdentifier "CGAX" .

figi-ps:JPAR skos:prefLabel "jp morgan argentina" .

figi-ps:CGBH a owl:NamedIndividual .

figi-ps:JPAR figi-gii:hasUniqueTextIdentifier "JPAR" .

figi-ps:CGBH a figi-gii:PricingSource .

figi-ps:JPAU a owl:NamedIndividual .

figi-ps:CGBH skos:prefLabel "china guangfa bank" .

figi-ps:JPAU a figi-gii:PricingSource .

figi-ps:CGBH figi-gii:hasUniqueTextIdentifier "CGBH" .

figi-ps:JPAU skos:prefLabel "jp morgan australia" .

figi-ps:CGC a owl:NamedIndividual .

figi-ps:JPAU figi-gii:hasUniqueTextIdentifier "JPAU" .

figi-ps:CGC a figi-gii:PricingSource .

figi-ps:JPAX a owl:NamedIndividual .

figi-ps:CGC skos:prefLabel "citigroup credit" .

figi-ps:JPAX a figi-gii:PricingSource .

figi-ps:CGC figi-gii:hasUniqueTextIdentifier "CGC" .

figi-ps:JPAX skos:prefLabel "jp morgan - eu govts" .

figi-ps:CGCB a owl:NamedIndividual .

figi-ps:JPAX figi-gii:hasUniqueTextIdentifier "JPAX" .

figi-ps:CGCB a figi-gii:PricingSource .

figi-ps:JPB2 a owl:NamedIndividual .

figi-ps:CGCB skos:prefLabel "citigroup axcb" .

figi-ps:JPB2 a figi-gii:PricingSource .

figi-ps:CGCB figi-gii:hasUniqueTextIdentifier "CGCB" .

figi-ps:JPB2 skos:prefLabel "jp morgan ipb uat" .

figi-ps:CGCH a owl:NamedIndividual .

figi-ps:JPB2 figi-gii:hasUniqueTextIdentifier "JPB2" .

figi-ps:CGCH a figi-gii:PricingSource .

figi-ps:JPBA a owl:NamedIndividual .

figi-ps:CGCH skos:prefLabel "citigroup suisse" .

figi-ps:JPBA a figi-gii:PricingSource .

figi-ps:CGCH figi-gii:hasUniqueTextIdentifier "CGCH" .

figi-ps:JPBA skos:prefLabel "jp morgan ldn abs" .

figi-ps:CGDO a owl:NamedIndividual .

figi-ps:JPBA figi-gii:hasUniqueTextIdentifier "JPBA" .

figi-ps:CGDO a figi-gii:PricingSource .

figi-ps:JPBI a owl:NamedIndividual .

figi-ps:CGDO skos:prefLabel "citigroup delta one" .

figi-ps:JPBI a figi-gii:PricingSource .

figi-ps:CGDO figi-gii:hasUniqueTextIdentifier "CGDO" .

figi-ps:JPBI skos:prefLabel "jp morgan tokyo" .

figi-ps:CGDX a owl:NamedIndividual .

figi-ps:JPBI figi-gii:hasUniqueTextIdentifier "JPBI" .

figi-ps:CGDX a figi-gii:PricingSource .

figi-ps:JPCA a owl:NamedIndividual .

figi-ps:CGDX skos:prefLabel "caixa geral de dep" .

figi-ps:JPCA a figi-gii:PricingSource .

figi-ps:CGDX figi-gii:hasUniqueTextIdentifier "CGDX" .

figi-ps:JPCA skos:prefLabel "jpmorgan catastrophe" .

figi-ps:CGEM a owl:NamedIndividual .

figi-ps:JPCA figi-gii:hasUniqueTextIdentifier "JPCA" .

figi-ps:CGEM a figi-gii:PricingSource .

figi-ps:JPCD a owl:NamedIndividual .

figi-ps:CGEM skos:prefLabel "citgroup em" .

figi-ps:JPCD a figi-gii:PricingSource .

figi-ps:CGEM skos:prefLabel "citigroup em" .

figi-ps:JPCD skos:prefLabel "jp morgan canada" .

figi-ps:CGEM figi-gii:hasUniqueTextIdentifier "CGEM" .

figi-ps:JPCD figi-gii:hasUniqueTextIdentifier "JPCD" .

figi-ps:CGIL a owl:NamedIndividual .

figi-ps:JPCM a owl:NamedIndividual .

figi-ps:CGIL a figi-gii:PricingSource .

figi-ps:JPCM a figi-gii:PricingSource .

figi-ps:CGIL skos:prefLabel "citigroup inflation" .

figi-ps:JPCM skos:prefLabel "jpmorgan chase" .

figi-ps:CGIL figi-gii:hasUniqueTextIdentifier "CGIL" .

figi-ps:JPCM figi-gii:hasUniqueTextIdentifier "JPCM" .

figi-ps:CGIS a owl:NamedIndividual .

figi-ps:JPDN a owl:NamedIndividual .

figi-ps:CGIS a figi-gii:PricingSource .

figi-ps:JPDN a figi-gii:PricingSource .

figi-ps:CGIS skos:prefLabel "citibank tel-aviv" .

figi-ps:JPDN skos:prefLabel "jp morgan boom" .

figi-ps:CGIS figi-gii:hasUniqueTextIdentifier "CGIS" .

figi-ps:JPDN figi-gii:hasUniqueTextIdentifier "JPDN" .

figi-ps:CGJ a owl:NamedIndividual .

figi-ps:JPDP a owl:NamedIndividual .

figi-ps:CGJ a figi-gii:PricingSource .

figi-ps:JPDP a figi-gii:PricingSource .

figi-ps:CGJ skos:prefLabel "citigroup auto-ex" .

figi-ps:JPDP skos:prefLabel "jp morgan drvs" .

figi-ps:CGJ figi-gii:hasUniqueTextIdentifier "CGJ" .

figi-ps:JPDP figi-gii:hasUniqueTextIdentifier "JPDP" .

figi-ps:CGLD a owl:NamedIndividual .

figi-ps:JPE a owl:NamedIndividual .

figi-ps:CGLD a figi-gii:PricingSource .

figi-ps:JPE a figi-gii:PricingSource .

figi-ps:CGLD skos:prefLabel "citi structured note" .

figi-ps:JPE skos:prefLabel "jpmorgan ldn autoex" .

figi-ps:CGLD figi-gii:hasUniqueTextIdentifier "CGLD" .

figi-ps:JPE figi-gii:hasUniqueTextIdentifier "JPE" .

figi-ps:CGLM a owl:NamedIndividual .

figi-ps:JPED a owl:NamedIndividual .

figi-ps:CGLM a figi-gii:PricingSource .

figi-ps:JPED a figi-gii:PricingSource .

figi-ps:CGLM skos:prefLabel "citigroup lm" .

figi-ps:JPED skos:prefLabel "jp morgan secs" .

figi-ps:CGLM figi-gii:hasUniqueTextIdentifier "CGLM" .

figi-ps:JPED figi-gii:hasUniqueTextIdentifier "JPED" .

figi-ps:CGLO a owl:NamedIndividual .

figi-ps:JPEM a owl:NamedIndividual .

figi-ps:CGLO a figi-gii:PricingSource .

figi-ps:JPEM a figi-gii:PricingSource .

figi-ps:CGLO skos:prefLabel "citigroup loans" .

figi-ps:JPEM skos:prefLabel "jpmorgan ny autoex" .

figi-ps:CGLO figi-gii:hasUniqueTextIdentifier "CGLO" .

figi-ps:JPEM figi-gii:hasUniqueTextIdentifier "JPEM" .

figi-ps:CGMA a owl:NamedIndividual .

figi-ps:JPEP a owl:NamedIndividual .

figi-ps:CGMA a figi-gii:PricingSource .

figi-ps:JPEP a figi-gii:PricingSource .

figi-ps:CGMA skos:prefLabel "citigroup global mrk" .

figi-ps:JPEP skos:prefLabel "jpm asia e-trading" .

figi-ps:CGMA figi-gii:hasUniqueTextIdentifier "CGMA" .

figi-ps:JPEP figi-gii:hasUniqueTextIdentifier "JPEP" .

figi-ps:CGMP a owl:NamedIndividual .

figi-ps:JPEX a owl:NamedIndividual .

figi-ps:CGMP a figi-gii:PricingSource .

figi-ps:JPEX a figi-gii:PricingSource .

figi-ps:CGMP skos:prefLabel "citi parallel prod" .

figi-ps:JPEX skos:prefLabel "jp morgan ldn autoex" .

figi-ps:CGMP figi-gii:hasUniqueTextIdentifier "CGMP" .

figi-ps:JPEX figi-gii:hasUniqueTextIdentifier "JPEX" .

figi-ps:CGMT a owl:NamedIndividual .

figi-ps:JPFD a owl:NamedIndividual .

figi-ps:CGMT a figi-gii:PricingSource .

figi-ps:JPFD a figi-gii:PricingSource .

figi-ps:CGMT skos:prefLabel "citigroup mbs" .

figi-ps:JPFD skos:prefLabel "jefferies and co" .

figi-ps:CGMT figi-gii:hasUniqueTextIdentifier "CGMT" .

figi-ps:JPFD figi-gii:hasUniqueTextIdentifier "JPFD" .

figi-ps:CGOV a owl:NamedIndividual .

figi-ps:JPFT a owl:NamedIndividual .

figi-ps:CGOV a figi-gii:PricingSource .

figi-ps:JPFT a figi-gii:PricingSource .

figi-ps:CGOV skos:prefLabel "caboto governments" .

figi-ps:JPFT skos:prefLabel "jpmorgan pp" .

figi-ps:CGOV figi-gii:hasUniqueTextIdentifier "CGOV" .

figi-ps:JPFT figi-gii:hasUniqueTextIdentifier "JPFT" .

figi-ps:CGPP a owl:NamedIndividual , figi-gii:PricingSource .

figi-ps:JPGM a owl:NamedIndividual .

figi-ps:CGPP skos:prefLabel "citigroup highgrade" .

figi-ps:JPGM a figi-gii:PricingSource .

figi-ps:CGPP figi-gii:hasUniqueTextIdentifier "CGPP" .

figi-ps:JPGM skos:prefLabel "jpmorgan gem" .

figi-ps:CGR a owl:NamedIndividual .

figi-ps:JPGM figi-gii:hasUniqueTextIdentifier "JPGM" .

figi-ps:CGR a figi-gii:PricingSource .

figi-ps:JPGN a owl:NamedIndividual .

figi-ps:CGR skos:prefLabel "citigroup" .

figi-ps:JPGN a figi-gii:PricingSource .

figi-ps:CGR figi-gii:hasUniqueTextIdentifier "CGR" .

figi-ps:JPGN skos:prefLabel "jpmorgan generic" .

figi-ps:CGRP a owl:NamedIndividual .

figi-ps:JPGN figi-gii:hasUniqueTextIdentifier "JPGN" .

figi-ps:CGRP a figi-gii:PricingSource .

figi-ps:JPGV a owl:NamedIndividual .

figi-ps:CGRP skos:prefLabel "cambridge group" .

figi-ps:JPGV a figi-gii:PricingSource .

figi-ps:CGRP figi-gii:hasUniqueTextIdentifier "CGRP" .

figi-ps:JPGV skos:prefLabel "jpmorgan e-trading" .

figi-ps:CGRT a owl:NamedIndividual .

figi-ps:JPGV figi-gii:hasUniqueTextIdentifier "JPGV" .

figi-ps:CGRT a figi-gii:PricingSource .

figi-ps:JPGX a owl:NamedIndividual .

figi-ps:CGRT skos:prefLabel "citigroup - retail" .

figi-ps:JPGX a figi-gii:PricingSource .

figi-ps:CGRT figi-gii:hasUniqueTextIdentifier "CGRT" .

figi-ps:JPGX skos:prefLabel "jp morgan london gov" .

figi-ps:CGTT a owl:NamedIndividual .

figi-ps:JPGX figi-gii:hasUniqueTextIdentifier "JPGX" .

figi-ps:CGTT a figi-gii:PricingSource .

figi-ps:JPGY a owl:NamedIndividual .

figi-ps:CGTT skos:prefLabel "citifx" .

figi-ps:JPGY a figi-gii:PricingSource .

figi-ps:CGTT figi-gii:hasUniqueTextIdentifier "CGTT" .

figi-ps:JPGY skos:prefLabel "jp morgan london gov" .

figi-ps:CGUD a owl:NamedIndividual .

figi-ps:JPGY figi-gii:hasUniqueTextIdentifier "JPGY" .

figi-ps:CGUD a figi-gii:PricingSource .

figi-ps:JPGZ a owl:NamedIndividual .

figi-ps:CGUD skos:prefLabel "citigroup us corpdbt" .

figi-ps:JPGZ a figi-gii:PricingSource .

figi-ps:CGUD figi-gii:hasUniqueTextIdentifier "CGUD" .

figi-ps:JPGZ skos:prefLabel "jpmorgan e-tradingz" .

figi-ps:CGUS a owl:NamedIndividual .

figi-ps:JPGZ figi-gii:hasUniqueTextIdentifier "JPGZ" .

figi-ps:CGUS a figi-gii:PricingSource .

figi-ps:JPHF a owl:NamedIndividual .

figi-ps:CGUS skos:prefLabel "citi structured prod" .

figi-ps:JPHF a figi-gii:PricingSource .

figi-ps:CGUS figi-gii:hasUniqueTextIdentifier "CGUS" .

figi-ps:JPHF skos:prefLabel "jpmorgan intrnl huf" .

figi-ps:CGX a owl:NamedIndividual .

figi-ps:JPHF figi-gii:hasUniqueTextIdentifier "JPHF" .

figi-ps:CGX a figi-gii:PricingSource .

figi-ps:JPHK a owl:NamedIndividual .

figi-ps:CGX skos:prefLabel "citigroup" .

figi-ps:JPHK a figi-gii:PricingSource .

figi-ps:CGX figi-gii:hasUniqueTextIdentifier "CGX" .

figi-ps:JPHK skos:prefLabel "jpmorgan securities" .

figi-ps:CGXI a owl:NamedIndividual .

figi-ps:JPHK figi-gii:hasUniqueTextIdentifier "JPHK" .

figi-ps:CGXI a figi-gii:PricingSource .

figi-ps:JPIN a owl:NamedIndividual .

figi-ps:CGXI skos:prefLabel "citigroup, london" .

figi-ps:JPIN a figi-gii:PricingSource .

figi-ps:CGXI figi-gii:hasUniqueTextIdentifier "CGXI" .

figi-ps:JPIN skos:prefLabel "jp morgan (internal)" .

figi-ps:CGZE a owl:NamedIndividual .

figi-ps:JPIN figi-gii:hasUniqueTextIdentifier "JPIN" .

figi-ps:CGZE a figi-gii:PricingSource .

figi-ps:JPIS a owl:NamedIndividual , figi-gii:PricingSource ;
	skos:prefLabel "jpmorgan infl swaps" .

figi-ps:CGZE skos:prefLabel "citibank sa e-bond" .

figi-ps:JPIS figi-gii:hasUniqueTextIdentifier "JPIS" .

figi-ps:JPJX a owl:NamedIndividual .

figi-ps:CGZE figi-gii:hasUniqueTextIdentifier "CGZE" .

figi-ps:JPJX a figi-gii:PricingSource ;
	skos:prefLabel "jpmorgan london" .

figi-ps:CHAP a owl:NamedIndividual .

figi-ps:JPJX figi-gii:hasUniqueTextIdentifier "JPJX" .

figi-ps:CHAP a figi-gii:PricingSource .

figi-ps:JPLM a owl:NamedIndividual , figi-gii:PricingSource .

figi-ps:CHAP skos:prefLabel "chapdelaine corp" .

figi-ps:JPLM skos:prefLabel "jpmorgan gem" .

figi-ps:CHAP figi-gii:hasUniqueTextIdentifier "CHAP" .

figi-ps:JPLM figi-gii:hasUniqueTextIdentifier "JPLM" .

figi-ps:CHBE a owl:NamedIndividual .

figi-ps:JPLU a owl:NamedIndividual .

figi-ps:CHBE a figi-gii:PricingSource .

figi-ps:JPLU a figi-gii:PricingSource .

figi-ps:CHBE skos:prefLabel "cfets executable prx" .

figi-ps:JPLU skos:prefLabel "jpmorgan aplus" .

figi-ps:CHBE figi-gii:hasUniqueTextIdentifier "CHBE" .

figi-ps:JPLU figi-gii:hasUniqueTextIdentifier "JPLU" .

figi-ps:CHBK a owl:NamedIndividual .

figi-ps:JPM a owl:NamedIndividual .

figi-ps:CHBK a figi-gii:PricingSource .

figi-ps:JPM a figi-gii:PricingSource .

figi-ps:CHBK skos:prefLabel "cfets trade price" .

figi-ps:JPM skos:prefLabel "jp morgan wm" .

figi-ps:CHBK figi-gii:hasUniqueTextIdentifier "CHBK" .

figi-ps:JPM figi-gii:hasUniqueTextIdentifier "JPM" .

figi-ps:CHBQ a owl:NamedIndividual .

figi-ps:JPMA a owl:NamedIndividual .

figi-ps:CHBQ a figi-gii:PricingSource .

figi-ps:JPMA a figi-gii:PricingSource .

figi-ps:CHBQ skos:prefLabel "cfets price quote" .

figi-ps:JPMA skos:prefLabel "jp morgan" .

figi-ps:CHBQ figi-gii:hasUniqueTextIdentifier "CHBQ" .

figi-ps:JPMA figi-gii:hasUniqueTextIdentifier "JPMA" .

figi-ps:CHCN a owl:NamedIndividual .

figi-ps:JPMC a owl:NamedIndividual .

figi-ps:CHCN a figi-gii:PricingSource .

figi-ps:JPMC a figi-gii:PricingSource .

figi-ps:CHCN skos:prefLabel "chemconnect" .

figi-ps:JPMC skos:prefLabel "jp morgan chase" .

figi-ps:CHCN figi-gii:hasUniqueTextIdentifier "CHCN" .

figi-ps:JPMC figi-gii:hasUniqueTextIdentifier "JPMC" .

figi-ps:CHDN a owl:NamedIndividual .

figi-ps:JPMD a owl:NamedIndividual .

figi-ps:CHDN a figi-gii:PricingSource .

figi-ps:JPMD a figi-gii:PricingSource .

figi-ps:CHDN skos:prefLabel "chardan capital mkts" .

figi-ps:JPMD skos:prefLabel "jp morgan securities" .

figi-ps:CHDN figi-gii:hasUniqueTextIdentifier "CHDN" .

figi-ps:JPMD figi-gii:hasUniqueTextIdentifier "JPMD" .

figi-ps:CHEM a owl:NamedIndividual .

figi-ps:JPME a owl:NamedIndividual .

figi-ps:CHEM a figi-gii:PricingSource .

figi-ps:JPME a figi-gii:PricingSource .

figi-ps:CHEM skos:prefLabel "jp morgan london" .

figi-ps:JPME skos:prefLabel "jp morgan ba" ;
	figi-gii:hasUniqueTextIdentifier "JPME" .

figi-ps:CHEM figi-gii:hasUniqueTextIdentifier "CHEM" .

figi-ps:JPMG a owl:NamedIndividual , figi-gii:PricingSource .

figi-ps:CHGC a owl:NamedIndividual .

figi-ps:JPMG skos:prefLabel "jpmorgan mtge" .

figi-ps:CHGC a figi-gii:PricingSource .

figi-ps:JPMG figi-gii:hasUniqueTextIdentifier "JPMG" .

figi-ps:CHGC skos:prefLabel "chg" .

figi-ps:JPMI a owl:NamedIndividual , figi-gii:PricingSource .

figi-ps:CHGC figi-gii:hasUniqueTextIdentifier "CHGC" .

figi-ps:JPMI skos:prefLabel "jp morgan (internal)" .

figi-ps:CHIC a owl:NamedIndividual .

figi-ps:JPMI figi-gii:hasUniqueTextIdentifier "JPMI" .

figi-ps:JPML a owl:NamedIndividual .

figi-ps:CHIC a figi-gii:PricingSource .

figi-ps:JPML a figi-gii:PricingSource .

figi-ps:CHIC skos:prefLabel "cfet ch intl cap crp" .

figi-ps:JPML skos:prefLabel "jp morgan london pmi" .

figi-ps:CHIC figi-gii:hasUniqueTextIdentifier "CHIC" .

figi-ps:JPML figi-gii:hasUniqueTextIdentifier "JPML" .

figi-ps:CHIN a owl:NamedIndividual .

figi-ps:JPMM a owl:NamedIndividual .

figi-ps:CHIN a figi-gii:PricingSource .

figi-ps:JPMM a figi-gii:PricingSource ;
	skos:prefLabel "jp morgan money mkt" .

figi-ps:CHIN skos:prefLabel "chase manhattan" .

figi-ps:JPMM figi-gii:hasUniqueTextIdentifier "JPMM" .

figi-ps:CHIN figi-gii:hasUniqueTextIdentifier "CHIN" .

figi-ps:JPMO a owl:NamedIndividual , figi-gii:PricingSource .

figi-ps:CHKE a owl:NamedIndividual .

figi-ps:JPMO skos:prefLabel "jp morgan secs tokyo" .

figi-ps:CHKE a figi-gii:PricingSource .

figi-ps:JPMO figi-gii:hasUniqueTextIdentifier "JPMO" .

figi-ps:CHKE skos:prefLabel "chase bank (k) ltd" .

figi-ps:JPMS a owl:NamedIndividual , figi-gii:PricingSource .

figi-ps:CHKE figi-gii:hasUniqueTextIdentifier "CHKE" .

figi-ps:JPMS skos:prefLabel "jpmorgan ny" .

figi-ps:CHKH a owl:NamedIndividual .

figi-ps:JPMS figi-gii:hasUniqueTextIdentifier "JPMS" .

figi-ps:CHKH a figi-gii:PricingSource .

figi-ps:JPMT a owl:NamedIndividual , figi-gii:PricingSource .

figi-ps:CHKH skos:prefLabel "chinggis khaan bank" .

figi-ps:JPMT skos:prefLabel "jpmorgan sec tokyo" .

figi-ps:CHKH figi-gii:hasUniqueTextIdentifier "CHKH" .

figi-ps:JPMT figi-gii:hasUniqueTextIdentifier "JPMT" .

figi-ps:CHLK a owl:NamedIndividual .

figi-ps:JPMW a owl:NamedIndividual .

figi-ps:CHLK a figi-gii:PricingSource .

figi-ps:JPMW a figi-gii:PricingSource .

figi-ps:CHLK skos:prefLabel "chalkhill partners" .

figi-ps:JPMW skos:prefLabel "jp morgan warrants" .

figi-ps:CHLK figi-gii:hasUniqueTextIdentifier "CHLK" .

figi-ps:JPMW figi-gii:hasUniqueTextIdentifier "JPMW" .

figi-ps:CHLM a owl:NamedIndividual .

figi-ps:JPNG a owl:NamedIndividual .

figi-ps:CHLM a figi-gii:PricingSource .

figi-ps:JPNG a figi-gii:PricingSource .

figi-ps:CHLM skos:prefLabel "craig hallum capital" .

figi-ps:JPNG skos:prefLabel "jpmorgan london 2" .

figi-ps:CHLM figi-gii:hasUniqueTextIdentifier "CHLM" .

figi-ps:CHLP a owl:NamedIndividual .

figi-ps:JPNG figi-gii:hasUniqueTextIdentifier "JPNG" .

figi-ps:CHLP a figi-gii:PricingSource ;
	skos:prefLabel "chalkhill partners" .

figi-ps:JPNT a owl:NamedIndividual .

figi-ps:CHLP figi-gii:hasUniqueTextIdentifier "CHLP" .

figi-ps:JPNT a figi-gii:PricingSource .

figi-ps:CHNT a owl:NamedIndividual , figi-gii:PricingSource .

figi-ps:JPNT skos:prefLabel "jp morgan securities" .

figi-ps:CHNT skos:prefLabel "chinatrust cmrcl bk" .

figi-ps:JPNT figi-gii:hasUniqueTextIdentifier "JPNT" .

figi-ps:CHNT figi-gii:hasUniqueTextIdentifier "CHNT" .

figi-ps:JPNY a owl:NamedIndividual .

figi-ps:CHQF a owl:NamedIndividual .

figi-ps:JPNY a figi-gii:PricingSource .

figi-ps:CHQF a figi-gii:PricingSource .

figi-ps:JPNY skos:prefLabel "jp morgan ny auto-ex" .

figi-ps:CHQF skos:prefLabel "ing qfii" .

figi-ps:JPNY figi-gii:hasUniqueTextIdentifier "JPNY" .

figi-ps:CHQF figi-gii:hasUniqueTextIdentifier "CHQF" .

figi-ps:JPOG a owl:NamedIndividual .

figi-ps:CHSI a owl:NamedIndividual .

figi-ps:JPOG a figi-gii:PricingSource .

figi-ps:CHSI a figi-gii:PricingSource .

figi-ps:JPOG skos:prefLabel "jp morgan mumbai" .

figi-ps:CHSI skos:prefLabel "chase mnhtn istanbul" .

figi-ps:JPOG figi-gii:hasUniqueTextIdentifier "JPOG" .

figi-ps:CHSI figi-gii:hasUniqueTextIdentifier "CHSI" .

figi-ps:JPOX a owl:NamedIndividual .

figi-ps:CI a owl:NamedIndividual .

figi-ps:JPOX a figi-gii:PricingSource .

figi-ps:CI a figi-gii:PricingSource .

figi-ps:JPOX skos:prefLabel "japan off-exch cb" .

figi-ps:CI skos:prefLabel "cominvest" .

figi-ps:JPOX figi-gii:hasUniqueTextIdentifier "JPOX" .

figi-ps:CI figi-gii:hasUniqueTextIdentifier "CI" .

figi-ps:JPPX a owl:NamedIndividual .

figi-ps:CIAM a owl:NamedIndividual .

figi-ps:JPPX a figi-gii:PricingSource .

figi-ps:CIAM a figi-gii:PricingSource .

figi-ps:JPPX skos:prefLabel "jp morgan chase bank" .

figi-ps:CIAM skos:prefLabel "ciam" .

figi-ps:JPPX figi-gii:hasUniqueTextIdentifier "JPPX" .

figi-ps:CIAM figi-gii:hasUniqueTextIdentifier "CIAM" .

figi-ps:JPS1 a owl:NamedIndividual .

figi-ps:CIAN a owl:NamedIndividual .

figi-ps:JPS1 a figi-gii:PricingSource .

figi-ps:CIAN a figi-gii:PricingSource .

figi-ps:JPS1 skos:prefLabel "jp morgan - level 1" .

figi-ps:CIAN skos:prefLabel "citigrp global boom" .

figi-ps:JPS1 figi-gii:hasUniqueTextIdentifier "JPS1" .

figi-ps:CIAN figi-gii:hasUniqueTextIdentifier "CIAN" .

figi-ps:JPS2 a owl:NamedIndividual .

figi-ps:CIAR a owl:NamedIndividual .

figi-ps:JPS2 a figi-gii:PricingSource .

figi-ps:CIAR a figi-gii:PricingSource .

figi-ps:JPS2 skos:prefLabel "jp morgan - level 2" .

figi-ps:CIAR skos:prefLabel "citibank baires" .

figi-ps:JPS2 figi-gii:hasUniqueTextIdentifier "JPS2" .

figi-ps:CIAR figi-gii:hasUniqueTextIdentifier "CIAR" .

figi-ps:JPS3 a owl:NamedIndividual .

figi-ps:CIBA a owl:NamedIndividual .

figi-ps:JPS3 a figi-gii:PricingSource .

figi-ps:CIBA a figi-gii:PricingSource .

figi-ps:JPS3 skos:prefLabel "jp morgan inside 3" .

figi-ps:CIBA skos:prefLabel "citibank arg (usd)" .

figi-ps:JPS3 figi-gii:hasUniqueTextIdentifier "JPS3" .

figi-ps:CIBA figi-gii:hasUniqueTextIdentifier "CIBA" .

figi-ps:JPS4 a owl:NamedIndividual .

figi-ps:CIBC a owl:NamedIndividual .

figi-ps:JPS4 a figi-gii:PricingSource .

figi-ps:CIBC a figi-gii:PricingSource .

figi-ps:JPS4 skos:prefLabel "jp morgan inside 4" .

figi-ps:CIBC skos:prefLabel "cibc world mkts ny" .

figi-ps:JPS4 figi-gii:hasUniqueTextIdentifier "JPS4" .

figi-ps:CIBC figi-gii:hasUniqueTextIdentifier "CIBC" .

figi-ps:JPSE a owl:NamedIndividual .

figi-ps:CIBH a owl:NamedIndividual .

figi-ps:JPSE a figi-gii:PricingSource .

figi-ps:CIBH a figi-gii:PricingSource .

figi-ps:JPSE skos:prefLabel "jpmorgan sp" .

figi-ps:CIBH skos:prefLabel "central european int" .

figi-ps:JPSE figi-gii:hasUniqueTextIdentifier "JPSE" .

figi-ps:CIBH figi-gii:hasUniqueTextIdentifier "CIBH" .

figi-ps:JPSI a owl:NamedIndividual .

figi-ps:CIBM a owl:NamedIndividual .

figi-ps:JPSI a figi-gii:PricingSource .

figi-ps:CIBM a figi-gii:PricingSource .

figi-ps:JPSI skos:prefLabel "jp morgan inside prx" .

figi-ps:CIBM skos:prefLabel "cibc world mkts" .

figi-ps:JPSI figi-gii:hasUniqueTextIdentifier "JPSI" .

figi-ps:CIBM figi-gii:hasUniqueTextIdentifier "CIBM" .

figi-ps:JPSR a owl:NamedIndividual .

figi-ps:CIBN a owl:NamedIndividual .

figi-ps:JPSR a figi-gii:PricingSource .

figi-ps:CIBN a figi-gii:PricingSource .

figi-ps:JPSR skos:prefLabel "jpmorgan" .

figi-ps:CIBN skos:prefLabel "cibc world notes" .

figi-ps:JPSR figi-gii:hasUniqueTextIdentifier "JPSR" .

figi-ps:CIBN figi-gii:hasUniqueTextIdentifier "CIBN" .

figi-ps:JPSX a owl:NamedIndividual .

figi-ps:CIBR a owl:NamedIndividual .

figi-ps:JPSX a figi-gii:PricingSource .

figi-ps:CIBR a figi-gii:PricingSource .

figi-ps:JPSX skos:prefLabel "jp morgan sgp autoex" .

figi-ps:CIBR skos:prefLabel "banco citibank sa" .

figi-ps:JPSX figi-gii:hasUniqueTextIdentifier "JPSX" .

figi-ps:CIBR figi-gii:hasUniqueTextIdentifier "CIBR" .

figi-ps:JPTR a owl:NamedIndividual .

figi-ps:CIBU a owl:NamedIndividual .

figi-ps:JPTR a figi-gii:PricingSource .

figi-ps:CIBU a figi-gii:PricingSource .

figi-ps:JPTR skos:prefLabel "jp morgan - ts" .

figi-ps:CIBU skos:prefLabel "citigroup sofia" .

figi-ps:JPTR figi-gii:hasUniqueTextIdentifier "JPTR" .

figi-ps:CIBU figi-gii:hasUniqueTextIdentifier "CIBU" .

figi-ps:JPTT a owl:NamedIndividual .

figi-ps:CIBX a owl:NamedIndividual .

figi-ps:JPTT a figi-gii:PricingSource .

figi-ps:CIBX a figi-gii:PricingSource .

figi-ps:JPTT skos:prefLabel "jp morgan, turkey" .

figi-ps:CIBX skos:prefLabel "cibc world mkts" .

figi-ps:JPTT figi-gii:hasUniqueTextIdentifier "JPTT" .

figi-ps:CIBX figi-gii:hasUniqueTextIdentifier "CIBX" .

figi-ps:JPTU a owl:NamedIndividual .

figi-ps:CIBZ a owl:NamedIndividual .

figi-ps:JPTU a figi-gii:PricingSource .

figi-ps:CIBZ a figi-gii:PricingSource .

figi-ps:JPTU skos:prefLabel "jp morgan, istanbul" .

figi-ps:CIBZ skos:prefLabel "cibc world markets" .

figi-ps:JPTU figi-gii:hasUniqueTextIdentifier "JPTU" .

figi-ps:CIBZ figi-gii:hasUniqueTextIdentifier "CIBZ" .

figi-ps:JPTX a owl:NamedIndividual .

figi-ps:CIC a owl:NamedIndividual .

figi-ps:JPTX a figi-gii:PricingSource .

figi-ps:CIC a figi-gii:PricingSource .

figi-ps:JPTX skos:prefLabel "jpmorgan ap internal" .

figi-ps:CIC skos:prefLabel "china investment co" .

figi-ps:JPTX figi-gii:hasUniqueTextIdentifier "JPTX" .

figi-ps:CIC figi-gii:hasUniqueTextIdentifier "CIC" .

figi-ps:JPTY a owl:NamedIndividual .

figi-ps:CICC a owl:NamedIndividual .

figi-ps:JPTY a figi-gii:PricingSource .

figi-ps:CICC a figi-gii:PricingSource .

figi-ps:JPTY skos:prefLabel "jp morgan treasuries" .

figi-ps:CICC skos:prefLabel "cicc fp" .

figi-ps:JPTY figi-gii:hasUniqueTextIdentifier "JPTY" .

figi-ps:CICC figi-gii:hasUniqueTextIdentifier "CICC" .

figi-ps:JPWM a owl:NamedIndividual , figi-gii:PricingSource ;
	skos:prefLabel "jp morgan s africa" ;
	figi-gii:hasUniqueTextIdentifier "JPWM" .

figi-ps:JPXM a owl:NamedIndividual .

figi-ps:CICF a owl:NamedIndividual .

figi-ps:JPXM a figi-gii:PricingSource .

figi-ps:CICF a figi-gii:PricingSource .

figi-ps:JPXM skos:prefLabel "jpmorgan autoex(test" .

figi-ps:CICF skos:prefLabel "cic (cial)" .

figi-ps:JPXM figi-gii:hasUniqueTextIdentifier "JPXM" .

figi-ps:CICF figi-gii:hasUniqueTextIdentifier "CICF" .

figi-ps:JPZA a owl:NamedIndividual .

figi-ps:CICM a owl:NamedIndividual .

figi-ps:JPZA a figi-gii:PricingSource .

figi-ps:CICM a figi-gii:PricingSource .

figi-ps:JPZA skos:prefLabel "jpmorgan so africa" .

figi-ps:CICM skos:prefLabel "cic" .

figi-ps:JPZA figi-gii:hasUniqueTextIdentifier "JPZA" .

figi-ps:CICM figi-gii:hasUniqueTextIdentifier "CICM" .

figi-ps:JPZE a owl:NamedIndividual .

figi-ps:CICO a owl:NamedIndividual .

figi-ps:JPZE a figi-gii:PricingSource .

figi-ps:CICO a figi-gii:PricingSource .

figi-ps:JPZE skos:prefLabel "jp morgan sa e-bond" .

figi-ps:CICO skos:prefLabel "citibank costa rica" .

figi-ps:JPZE figi-gii:hasUniqueTextIdentifier "JPZE" .

figi-ps:CICO figi-gii:hasUniqueTextIdentifier "CICO" .

figi-ps:JQ a owl:NamedIndividual .

figi-ps:CICT a owl:NamedIndividual .

figi-ps:JQ a figi-gii:PricingSource .

figi-ps:CICT a figi-gii:PricingSource .

figi-ps:JQ skos:prefLabel "japan dealers quote" .

figi-ps:CICT skos:prefLabel "cic test" .

figi-ps:JQ figi-gii:hasUniqueTextIdentifier "JQ" .

figi-ps:CICT figi-gii:hasUniqueTextIdentifier "CICT" .

figi-ps:JSBP a owl:NamedIndividual .

figi-ps:CIDR a owl:NamedIndividual .

figi-ps:JSBP a figi-gii:PricingSource .

figi-ps:CIDR a figi-gii:PricingSource .

figi-ps:JSBP skos:prefLabel "js bank" .

figi-ps:CIDR skos:prefLabel "citibank dr" .

figi-ps:JSBP figi-gii:hasUniqueTextIdentifier "JSBP" .

figi-ps:CIDR figi-gii:hasUniqueTextIdentifier "CIDR" .

figi-ps:JSCL a owl:NamedIndividual .

figi-ps:CIDU a owl:NamedIndividual .

figi-ps:JSCL a figi-gii:PricingSource .

figi-ps:CIDU a figi-gii:PricingSource .

figi-ps:JSCL skos:prefLabel "js global capitalltd" .

figi-ps:CIDU skos:prefLabel "citibank dubai" .

figi-ps:JSCL figi-gii:hasUniqueTextIdentifier "JSCL" .

figi-ps:CIDU figi-gii:hasUniqueTextIdentifier "CIDU" .

figi-ps:JSDA a owl:NamedIndividual .

figi-ps:CIEG a owl:NamedIndividual .

figi-ps:JSDA a figi-gii:PricingSource .

figi-ps:CIEG a figi-gii:PricingSource .

figi-ps:JSDA skos:prefLabel "japan sec dealers" .

figi-ps:CIEG skos:prefLabel "citibank cairo" .

figi-ps:JSDA figi-gii:hasUniqueTextIdentifier "JSDA" .

figi-ps:CIEG figi-gii:hasUniqueTextIdentifier "CIEG" .

figi-ps:JSDM a owl:NamedIndividual .

figi-ps:CIEU a owl:NamedIndividual .

figi-ps:JSDM a figi-gii:PricingSource .

figi-ps:CIEU a figi-gii:PricingSource .

figi-ps:JSDM skos:prefLabel "japan secs matrix" .

figi-ps:CIEU skos:prefLabel "creditsuisse pricing" .

figi-ps:JSDM figi-gii:hasUniqueTextIdentifier "JSDM" .

figi-ps:CIEU figi-gii:hasUniqueTextIdentifier "CIEU" .

figi-ps:JSDP a owl:NamedIndividual .

figi-ps:CIFL a owl:NamedIndividual .

figi-ps:JSDP a figi-gii:PricingSource .

figi-ps:CIFL a figi-gii:PricingSource .

figi-ps:JSDP skos:prefLabel "japan sec dealer" .

figi-ps:CIFL skos:prefLabel "cs inflationswap" .

figi-ps:JSDP skos:prefLabel "jsda - price" .

figi-ps:CIFL figi-gii:hasUniqueTextIdentifier "CIFL" .

figi-ps:JSDP figi-gii:hasUniqueTextIdentifier "JSDP" .

figi-ps:CIGI a owl:NamedIndividual .

figi-ps:JSDQ a owl:NamedIndividual .

figi-ps:CIGI a figi-gii:PricingSource .

figi-ps:JSDQ a figi-gii:PricingSource .

figi-ps:CIGI skos:prefLabel "citadel investment" .

figi-ps:JSDQ skos:prefLabel "jasdaq" .

figi-ps:CIGI figi-gii:hasUniqueTextIdentifier "CIGI" .

figi-ps:JSDQ figi-gii:hasUniqueTextIdentifier "JSDQ" .

figi-ps:CIGK a owl:NamedIndividual .

figi-ps:JSE a owl:NamedIndividual .

figi-ps:CIGK a figi-gii:PricingSource .

figi-ps:JSE a figi-gii:PricingSource .

figi-ps:CIGK skos:prefLabel "cimb-gk securities" .

figi-ps:JSE skos:prefLabel "johannesburg exch" .

figi-ps:CIGK figi-gii:hasUniqueTextIdentifier "CIGK" .

figi-ps:JSE figi-gii:hasUniqueTextIdentifier "JSE" .

figi-ps:CIGM a owl:NamedIndividual .

figi-ps:JSHK a owl:NamedIndividual .

figi-ps:CIGM a figi-gii:PricingSource .

figi-ps:JSHK a figi-gii:PricingSource .

figi-ps:CIGM skos:prefLabel "citigroup global mar" .

figi-ps:JSHK skos:prefLabel "js cresvale intl ltd" .

figi-ps:CIGM figi-gii:hasUniqueTextIdentifier "CIGM" .

figi-ps:JSHK figi-gii:hasUniqueTextIdentifier "JSHK" .

figi-ps:CIHK a owl:NamedIndividual .

figi-ps:JSPR a owl:NamedIndividual .

figi-ps:CIHK a figi-gii:PricingSource .

figi-ps:JSPR a figi-gii:PricingSource .

figi-ps:CIHK skos:prefLabel "citibank na" .

figi-ps:JSPR skos:prefLabel "js price" .

figi-ps:CIHK figi-gii:hasUniqueTextIdentifier "CIHK" .

figi-ps:JSPR figi-gii:hasUniqueTextIdentifier "JSPR" .

figi-ps:CIIJ a owl:NamedIndividual .

figi-ps:JSSF a owl:NamedIndividual .

figi-ps:CIIJ a figi-gii:PricingSource .

figi-ps:JSSF a figi-gii:PricingSource .

figi-ps:CIIJ skos:prefLabel "israel bond trading" .

figi-ps:JSSF skos:prefLabel "jmp securities" .

figi-ps:CIIJ figi-gii:hasUniqueTextIdentifier "CIIJ" .

figi-ps:JSSF figi-gii:hasUniqueTextIdentifier "JSSF" .

figi-ps:CIMB a owl:NamedIndividual .

figi-ps:JSUN a owl:NamedIndividual .

figi-ps:CIMB a figi-gii:PricingSource .

figi-ps:JSUN a figi-gii:PricingSource .

figi-ps:CIMB skos:prefLabel "cimb kl" .

figi-ps:JSUN skos:prefLabel "jih sun securities" .

figi-ps:CIMB figi-gii:hasUniqueTextIdentifier "CIMB" .

figi-ps:JSUN figi-gii:hasUniqueTextIdentifier "JSUN" .

figi-ps:CIMD a owl:NamedIndividual .

figi-ps:JSUP a owl:NamedIndividual .

figi-ps:CIMD a figi-gii:PricingSource .

figi-ps:JSUP a figi-gii:PricingSource .

figi-ps:CIMD skos:prefLabel "cimd madrid" .

figi-ps:JSUP skos:prefLabel "jesup and lamont corp" .

figi-ps:CIMD figi-gii:hasUniqueTextIdentifier "CIMD" .

figi-ps:JSUP figi-gii:hasUniqueTextIdentifier "JSUP" .

figi-ps:CIME a owl:NamedIndividual .

figi-ps:JTBA a owl:NamedIndividual .

figi-ps:CIME a figi-gii:PricingSource .

figi-ps:JTBA a figi-gii:PricingSource .

figi-ps:CIME skos:prefLabel "cimd spanish power" .

figi-ps:JTBA skos:prefLabel "jandt banka prague" .

figi-ps:CIME figi-gii:hasUniqueTextIdentifier "CIME" .

figi-ps:JTBA figi-gii:hasUniqueTextIdentifier "JTBA" .

figi-ps:CIMR a owl:NamedIndividual .

figi-ps:JTS1 a owl:NamedIndividual .

figi-ps:CIMR a figi-gii:PricingSource .

figi-ps:JTS1 a figi-gii:PricingSource .

figi-ps:CIMR skos:prefLabel "cimb bank bhd" .

figi-ps:JTS1 skos:prefLabel "jp morgan test lvl 1" .

figi-ps:CIMR figi-gii:hasUniqueTextIdentifier "CIMR" .

figi-ps:JTS1 figi-gii:hasUniqueTextIdentifier "JTS1" .

figi-ps:CIMS a owl:NamedIndividual .

figi-ps:JTS2 a owl:NamedIndividual .

figi-ps:CIMS a figi-gii:PricingSource .

figi-ps:JTS2 a figi-gii:PricingSource .

figi-ps:CIMS skos:prefLabel "cimb group (sg)" .

figi-ps:JTS2 skos:prefLabel "jp morgan test lvl 2" .

figi-ps:CIMS figi-gii:hasUniqueTextIdentifier "CIMS" .

figi-ps:JTS2 figi-gii:hasUniqueTextIdentifier "JTS2" .

figi-ps:CINF a owl:NamedIndividual .

figi-ps:JTS3 a owl:NamedIndividual .

figi-ps:CINF a figi-gii:PricingSource .

figi-ps:JTS3 a figi-gii:PricingSource .

figi-ps:CINF skos:prefLabel "cincinnati financial" .

figi-ps:JTS3 skos:prefLabel "jp morgan test lvl 3" .

figi-ps:CINF figi-gii:hasUniqueTextIdentifier "CINF" .

figi-ps:JTS3 figi-gii:hasUniqueTextIdentifier "JTS3" .

figi-ps:CINO a owl:NamedIndividual .

figi-ps:JTSI a owl:NamedIndividual .

figi-ps:CINO a figi-gii:PricingSource .

figi-ps:JTSI a figi-gii:PricingSource .

figi-ps:CINO skos:prefLabel "chinabond val inbk n" .

figi-ps:JTSI skos:prefLabel "jp morgan corp test" .

figi-ps:CINO figi-gii:hasUniqueTextIdentifier "CINO" .

figi-ps:JTSI figi-gii:hasUniqueTextIdentifier "JTSI" .

figi-ps:CINT a owl:NamedIndividual .

figi-ps:JUBA a owl:NamedIndividual .

figi-ps:CINT a figi-gii:PricingSource .

figi-ps:JUBA a figi-gii:PricingSource .

figi-ps:CINT skos:prefLabel "citicorp intl sec jp" .

figi-ps:JUBA skos:prefLabel "julius baer" .

figi-ps:CINT figi-gii:hasUniqueTextIdentifier "CINT" .

figi-ps:JUBA figi-gii:hasUniqueTextIdentifier "JUBA" .

figi-ps:CIOP a owl:NamedIndividual .

figi-ps:JVB a owl:NamedIndividual .

figi-ps:CIOP a figi-gii:PricingSource .

figi-ps:JVB a figi-gii:PricingSource .

figi-ps:CIOP skos:prefLabel "chinabond val inbk o" .

figi-ps:JVB skos:prefLabel "jvb" .

figi-ps:CIOP figi-gii:hasUniqueTextIdentifier "CIOP" .

figi-ps:JVB figi-gii:hasUniqueTextIdentifier "JVB" .

figi-ps:CIPA a owl:NamedIndividual .

figi-ps:JVBG a owl:NamedIndividual .

figi-ps:CIPA a figi-gii:PricingSource .

figi-ps:JVBG a figi-gii:PricingSource .

figi-ps:CIPA skos:prefLabel "citibank panama" .

figi-ps:JVBG skos:prefLabel "jvb financial" .

figi-ps:CIPA figi-gii:hasUniqueTextIdentifier "CIPA" .

figi-ps:JVBG skos:prefLabel "jvb financial llc" .

figi-ps:CIPB a owl:NamedIndividual .

figi-ps:JVBG figi-gii:hasUniqueTextIdentifier "JVBG" .

figi-ps:CIPB a figi-gii:PricingSource .

figi-ps:JYSB a owl:NamedIndividual .

figi-ps:CIPB skos:prefLabel "cicc pte banking" .

figi-ps:JYSB a figi-gii:PricingSource .

figi-ps:CIPB figi-gii:hasUniqueTextIdentifier "CIPB" .

figi-ps:JYSB skos:prefLabel "jyske bank" .

figi-ps:CIPH a owl:NamedIndividual .

figi-ps:JYSB figi-gii:hasUniqueTextIdentifier "JYSB" .

figi-ps:CIPH a figi-gii:PricingSource .

figi-ps:JYSG a owl:NamedIndividual .

figi-ps:CIPH skos:prefLabel "citibank na" .

figi-ps:JYSG a figi-gii:PricingSource .

figi-ps:CIPH figi-gii:hasUniqueTextIdentifier "CIPH" .

figi-ps:JYSG skos:prefLabel "jyskebank silkeborg" .

figi-ps:CIR a owl:NamedIndividual .

figi-ps:JYSG figi-gii:hasUniqueTextIdentifier "JYSG" .

figi-ps:CIR a figi-gii:PricingSource .

figi-ps:KAAT a owl:NamedIndividual .

figi-ps:CIR skos:prefLabel "cundill inv research" .

figi-ps:KAAT a figi-gii:PricingSource .

figi-ps:CIR figi-gii:hasUniqueTextIdentifier "CIR" .

figi-ps:KAAT skos:prefLabel "kommunalkredit aus" .

figi-ps:CISE a owl:NamedIndividual .

figi-ps:KAAT figi-gii:hasUniqueTextIdentifier "KAAT" .

figi-ps:CISE a figi-gii:PricingSource .

figi-ps:KABA a owl:NamedIndividual .

figi-ps:CISE skos:prefLabel "cfet citic securitie" .

figi-ps:KABA a figi-gii:PricingSource .

figi-ps:CISE figi-gii:hasUniqueTextIdentifier "CISE" .

figi-ps:KABA skos:prefLabel "capitron bank" .

figi-ps:CISL a owl:NamedIndividual .

figi-ps:KABA figi-gii:hasUniqueTextIdentifier "KABA" .

figi-ps:CISL a figi-gii:PricingSource .

figi-ps:KAFD a owl:NamedIndividual .

figi-ps:CISL skos:prefLabel "citibank, colombo" .

figi-ps:KAFD a figi-gii:PricingSource .

figi-ps:CISL figi-gii:hasUniqueTextIdentifier "CISL" .

figi-ps:KAFD skos:prefLabel "kaf discount berhad" .

figi-ps:CISM a owl:NamedIndividual .

figi-ps:KAFD figi-gii:hasUniqueTextIdentifier "KAFD" .

figi-ps:CISM a figi-gii:PricingSource .

figi-ps:KAGE a owl:NamedIndividual .

figi-ps:CISM skos:prefLabel "centreinvest sec" .

figi-ps:KAGE a figi-gii:PricingSource .

figi-ps:CISM figi-gii:hasUniqueTextIdentifier "CISM" .

figi-ps:KAGE skos:prefLabel "kagiso e-bond" .

figi-ps:CIST a owl:NamedIndividual .

figi-ps:KAGE figi-gii:hasUniqueTextIdentifier "KAGE" .

figi-ps:CIST a figi-gii:PricingSource .

figi-ps:KAMC a owl:NamedIndividual .

figi-ps:CIST skos:prefLabel "capital institutiona" .

figi-ps:KAMC a figi-gii:PricingSource .

figi-ps:CIST figi-gii:hasUniqueTextIdentifier "CIST" .

figi-ps:KAMC skos:prefLabel "kuwait invest proj" .

figi-ps:CIT a owl:NamedIndividual .

figi-ps:KAMC figi-gii:hasUniqueTextIdentifier "KAMC" .

figi-ps:CIT a figi-gii:PricingSource .

figi-ps:KAPG a owl:NamedIndividual .

figi-ps:CIT skos:prefLabel "citibank (phils)" .

figi-ps:KAPG a figi-gii:PricingSource .

figi-ps:CIT figi-gii:hasUniqueTextIdentifier "CIT" .

figi-ps:KAPG skos:prefLabel "kapital inv. group" .

figi-ps:CITA a owl:NamedIndividual .

figi-ps:KAPG figi-gii:hasUniqueTextIdentifier "KAPG" .

figi-ps:CITA a figi-gii:PricingSource .

figi-ps:KARB a owl:NamedIndividual .

figi-ps:CITA skos:prefLabel "citigroup asia" .

figi-ps:KARB a figi-gii:PricingSource .

figi-ps:CITA figi-gii:hasUniqueTextIdentifier "CITA" .

figi-ps:KARB skos:prefLabel "karnataka bank" .

figi-ps:CITB a owl:NamedIndividual .

figi-ps:KARB figi-gii:hasUniqueTextIdentifier "KARB" .

figi-ps:CITB a figi-gii:PricingSource .

figi-ps:KAUP a owl:NamedIndividual .

figi-ps:CITB skos:prefLabel "citibank slovakia" .

figi-ps:KAUP a figi-gii:PricingSource .

figi-ps:CITB figi-gii:hasUniqueTextIdentifier "CITB" .

figi-ps:KAUP skos:prefLabel "kaupthing bank" .

figi-ps:CITC a owl:NamedIndividual .

figi-ps:KAUP figi-gii:hasUniqueTextIdentifier "KAUP" .

figi-ps:CITC a figi-gii:PricingSource .

figi-ps:KAZA a owl:NamedIndividual .

figi-ps:CITC skos:prefLabel "china citic bank" .

figi-ps:KAZA a figi-gii:PricingSource .

figi-ps:CITC figi-gii:hasUniqueTextIdentifier "CITC" .

figi-ps:KAZA skos:prefLabel "kazakhstan exchange" .

figi-ps:CITF a owl:NamedIndividual .

figi-ps:KAZA figi-gii:hasUniqueTextIdentifier "KAZA" .

figi-ps:CITF a figi-gii:PricingSource .

figi-ps:KBBL a owl:NamedIndividual .

figi-ps:CITF skos:prefLabel "cit finance (ojsc)" .

figi-ps:KBBL a figi-gii:PricingSource .

figi-ps:CITF figi-gii:hasUniqueTextIdentifier "CITF" .

figi-ps:KBBL skos:prefLabel "basellandschaftl kb" .

figi-ps:CITI a owl:NamedIndividual .

figi-ps:KBBL figi-gii:hasUniqueTextIdentifier "KBBL" .

figi-ps:CITI a figi-gii:PricingSource .

figi-ps:KBC a owl:NamedIndividual .

figi-ps:CITI skos:prefLabel "citibank intl plc." .

figi-ps:KBC a figi-gii:PricingSource .

figi-ps:CITI figi-gii:hasUniqueTextIdentifier "CITI" .

figi-ps:KBC skos:prefLabel "kbc bank nv" .

figi-ps:CITJ a owl:NamedIndividual .

figi-ps:KBC figi-gii:hasUniqueTextIdentifier "KBC" .

figi-ps:CITJ a figi-gii:PricingSource .

figi-ps:KBCC a owl:NamedIndividual .

figi-ps:CITJ skos:prefLabel "citi, jamaica" .

figi-ps:KBCC a figi-gii:PricingSource .

figi-ps:CITJ figi-gii:hasUniqueTextIdentifier "CITJ" .

figi-ps:KBCC skos:prefLabel "kbc exploitatie nv" .

figi-ps:CITL a owl:NamedIndividual .

figi-ps:KBCC figi-gii:hasUniqueTextIdentifier "KBCC" .

figi-ps:CITL a figi-gii:PricingSource .

figi-ps:KBCG a owl:NamedIndividual .

figi-ps:CITL skos:prefLabel "citibank bombay" .

figi-ps:KBCG a figi-gii:PricingSource .

figi-ps:CITL figi-gii:hasUniqueTextIdentifier "CITL" .

figi-ps:KBCG skos:prefLabel "kbc financial group" .

figi-ps:CITM a owl:NamedIndividual .

figi-ps:KBCG figi-gii:hasUniqueTextIdentifier "KBCG" .

figi-ps:CITM a figi-gii:PricingSource .

figi-ps:KBCM a owl:NamedIndividual .

figi-ps:CITM skos:prefLabel "citibank moscow" .

figi-ps:KBCM a figi-gii:PricingSource .

figi-ps:CITM figi-gii:hasUniqueTextIdentifier "CITM" .

figi-ps:KBCM skos:prefLabel "keybanc capital mkts" .

figi-ps:CITS a owl:NamedIndividual .

figi-ps:KBCM figi-gii:hasUniqueTextIdentifier "KBCM" .

figi-ps:CITS a figi-gii:PricingSource .

figi-ps:KBCP a owl:NamedIndividual .

figi-ps:CITS skos:prefLabel "citigroup asia - int" .

figi-ps:KBCP a figi-gii:PricingSource .

figi-ps:CITS figi-gii:hasUniqueTextIdentifier "CITS" .

figi-ps:KBCP skos:prefLabel "kbc bk belgium" .

figi-ps:CITT a owl:NamedIndividual .

figi-ps:KBCP figi-gii:hasUniqueTextIdentifier "KBCP" .

figi-ps:CITT a figi-gii:PricingSource .

figi-ps:KBCT a owl:NamedIndividual .

figi-ps:CITT skos:prefLabel "citibank na dubai" .

figi-ps:KBCT a figi-gii:PricingSource .

figi-ps:CITT figi-gii:hasUniqueTextIdentifier "CITT" .

figi-ps:KBCT skos:prefLabel "kbc bank belg" .

figi-ps:CIUA a owl:NamedIndividual .

figi-ps:KBCT figi-gii:hasUniqueTextIdentifier "KBCT" .

figi-ps:CIUA a figi-gii:PricingSource .

figi-ps:KBFP a owl:NamedIndividual .

figi-ps:CIUA skos:prefLabel "citibank ukraine" .

figi-ps:KBFP a figi-gii:PricingSource .

figi-ps:CIUA figi-gii:hasUniqueTextIdentifier "CIUA" .

figi-ps:KBFP skos:prefLabel "kbc financial" .

figi-ps:CIUY a owl:NamedIndividual .

figi-ps:KBFP figi-gii:hasUniqueTextIdentifier "KBFP" .

figi-ps:CIUY a figi-gii:PricingSource .

figi-ps:KBIS a owl:NamedIndividual .

figi-ps:CIUY skos:prefLabel "citibank uruguay" .

figi-ps:KBIS a figi-gii:PricingSource .

figi-ps:CIUY figi-gii:hasUniqueTextIdentifier "CIUY" .

figi-ps:KBIS skos:prefLabel "kb investment sec" .

figi-ps:CIX a owl:NamedIndividual .

figi-ps:KBIS figi-gii:hasUniqueTextIdentifier "KBIS" .

figi-ps:CIX a figi-gii:PricingSource .

figi-ps:KBL a owl:NamedIndividual .

figi-ps:CIX skos:prefLabel "cix composite" .

figi-ps:KBL a figi-gii:PricingSource .

figi-ps:CIX figi-gii:hasUniqueTextIdentifier "CIX" .

figi-ps:KBL skos:prefLabel "kreditbank sa luxemb" .

figi-ps:CIXE a owl:NamedIndividual .

figi-ps:KBL figi-gii:hasUniqueTextIdentifier "KBL" .

figi-ps:CIXE a figi-gii:PricingSource .

figi-ps:KBLS a owl:NamedIndividual .

figi-ps:CIXE skos:prefLabel "casa de bolsa ixe" .

figi-ps:KBLS a figi-gii:PricingSource .

figi-ps:CIXE figi-gii:hasUniqueTextIdentifier "CIXE" .

figi-ps:KBLS skos:prefLabel "kbl struct products" .

figi-ps:CJCA a owl:NamedIndividual .

figi-ps:KBLS figi-gii:hasUniqueTextIdentifier "KBLS" .

figi-ps:CJCA a figi-gii:PricingSource .

figi-ps:KBLU a owl:NamedIndividual .

figi-ps:CJCA skos:prefLabel "caja caracas" .

figi-ps:KBLU a figi-gii:PricingSource .

figi-ps:CJCA figi-gii:hasUniqueTextIdentifier "CJCA" .

figi-ps:KBLU skos:prefLabel "kredietbank lux" .

figi-ps:CKCC a owl:NamedIndividual .

figi-ps:KBLU figi-gii:hasUniqueTextIdentifier "KBLU" .

figi-ps:CKCC a figi-gii:PricingSource .

figi-ps:KBNK a owl:NamedIndividual .

figi-ps:CKCC skos:prefLabel "ck cooper" .

figi-ps:KBNK a figi-gii:PricingSource .

figi-ps:CKCC figi-gii:hasUniqueTextIdentifier "CKCC" .

figi-ps:KBNK skos:prefLabel "kasikornbank" .

figi-ps:CKLX a owl:NamedIndividual .

figi-ps:KBNK figi-gii:hasUniqueTextIdentifier "KBNK" .

figi-ps:CKLX a figi-gii:PricingSource .

figi-ps:KBNP a owl:NamedIndividual .

figi-ps:CKLX skos:prefLabel "carl kliem" .

figi-ps:KBNP a figi-gii:PricingSource .

figi-ps:CKLX figi-gii:hasUniqueTextIdentifier "CKLX" .

figi-ps:KBNP skos:prefLabel "kbpm and npri average" .

figi-ps:CKWP a owl:NamedIndividual .

figi-ps:KBNP figi-gii:hasUniqueTextIdentifier "KBNP" .

figi-ps:CKWP a figi-gii:PricingSource .

figi-ps:KBNY a owl:NamedIndividual .

figi-ps:CKWP skos:prefLabel "citic ka wah 4:30" .

figi-ps:KBNY a figi-gii:PricingSource .

figi-ps:CKWP figi-gii:hasUniqueTextIdentifier "CKWP" .

figi-ps:KBNY skos:prefLabel "kbc ny convertibles" .

figi-ps:CKWT a owl:NamedIndividual .

figi-ps:KBNY figi-gii:hasUniqueTextIdentifier "KBNY" .

figi-ps:CKWT a figi-gii:PricingSource .

figi-ps:KBPL a owl:NamedIndividual .

figi-ps:CKWT skos:prefLabel "citic ka wah 11:30" .

figi-ps:KBPL a figi-gii:PricingSource .

figi-ps:CKWT figi-gii:hasUniqueTextIdentifier "CKWT" .

figi-ps:KBPL skos:prefLabel "kredyt bank sa" .

figi-ps:CL a owl:NamedIndividual .

figi-ps:KBPL figi-gii:hasUniqueTextIdentifier "KBPL" .

figi-ps:CL a figi-gii:PricingSource .

figi-ps:KBPM a owl:NamedIndividual .

figi-ps:CL skos:prefLabel "ca-cib paris" .

figi-ps:KBPM a figi-gii:PricingSource .

figi-ps:CL figi-gii:hasUniqueTextIdentifier "CL" .

figi-ps:KBPM skos:prefLabel "kbp and kmcc ii" .

figi-ps:CLA a owl:NamedIndividual .

figi-ps:KBPM figi-gii:hasUniqueTextIdentifier "KBPM" .

figi-ps:CLA a figi-gii:PricingSource .

figi-ps:KBPY a owl:NamedIndividual .

figi-ps:CLA skos:prefLabel "claymore securities" .

figi-ps:KBPY a figi-gii:PricingSource .

figi-ps:CLA figi-gii:hasUniqueTextIdentifier "CLA" .

figi-ps:KBPY skos:prefLabel "kbpm - yield" .

figi-ps:CLBK a owl:NamedIndividual .

figi-ps:KBPY figi-gii:hasUniqueTextIdentifier "KBPY" .

figi-ps:CLBK a figi-gii:PricingSource .

figi-ps:KBRO a owl:NamedIndividual .

figi-ps:CLBK skos:prefLabel "comm bank ceylon" .

figi-ps:KBRO a figi-gii:PricingSource .

figi-ps:CLBK figi-gii:hasUniqueTextIdentifier "CLBK" .

figi-ps:KBRO skos:prefLabel "kaufman bros., l.p." .

figi-ps:CLEU a owl:NamedIndividual .

figi-ps:KBRO figi-gii:hasUniqueTextIdentifier "KBRO" .

figi-ps:CLEU a figi-gii:PricingSource .

figi-ps:KBRU a owl:NamedIndividual .

figi-ps:CLEU skos:prefLabel "clariden leu" .

figi-ps:KBRU a figi-gii:PricingSource .

figi-ps:CLEU figi-gii:hasUniqueTextIdentifier "CLEU" .

figi-ps:KBRU skos:prefLabel "bank bcc-moscow" .

figi-ps:CLFF a owl:NamedIndividual .

figi-ps:KBRU figi-gii:hasUniqueTextIdentifier "KBRU" .

figi-ps:CLFF a figi-gii:PricingSource .

figi-ps:KBW a owl:NamedIndividual .

figi-ps:CLFF skos:prefLabel "clarkson secs user b" .

figi-ps:KBW a figi-gii:PricingSource .

figi-ps:CLFF figi-gii:hasUniqueTextIdentifier "CLFF" .

figi-ps:KBW skos:prefLabel "keefe, bruyette and wo" .

figi-ps:CLI a owl:NamedIndividual .

figi-ps:KBW skos:prefLabel "keefe; bruyette and wo" .

figi-ps:CLI a figi-gii:PricingSource .

figi-ps:KBW figi-gii:hasUniqueTextIdentifier "KBW" .

figi-ps:CLI skos:prefLabel "cathay life insur" .

figi-ps:KCIC a owl:NamedIndividual .

figi-ps:CLI figi-gii:hasUniqueTextIdentifier "CLI" .

figi-ps:KCIC a figi-gii:PricingSource .

figi-ps:CLIB a owl:NamedIndividual .

figi-ps:KCIC skos:prefLabel "kuwait china inv co" .

figi-ps:CLIB a figi-gii:PricingSource .

figi-ps:KCIC figi-gii:hasUniqueTextIdentifier "KCIC" .

figi-ps:CLIB skos:prefLabel "credit libanais sal" .

figi-ps:KCM a owl:NamedIndividual .

figi-ps:CLIB figi-gii:hasUniqueTextIdentifier "CLIB" .

figi-ps:KCM a figi-gii:PricingSource .

figi-ps:CLK a owl:NamedIndividual .

figi-ps:KCM skos:prefLabel "knighthead cap mgmt" .

figi-ps:CLK a figi-gii:PricingSource .

figi-ps:KCM figi-gii:hasUniqueTextIdentifier "KCM" .

figi-ps:CLK skos:prefLabel "cl king" .

figi-ps:KCMP a owl:NamedIndividual .

figi-ps:CLK figi-gii:hasUniqueTextIdentifier "CLK" .

figi-ps:KCMP a figi-gii:PricingSource .

figi-ps:CLLN a owl:NamedIndividual .

figi-ps:KCMP skos:prefLabel "korean composite" .

figi-ps:CLLN a figi-gii:PricingSource .

figi-ps:KCMP figi-gii:hasUniqueTextIdentifier "KCMP" .

figi-ps:CLLN skos:prefLabel "credit lyonnais sec" .

figi-ps:KDB a owl:NamedIndividual .

figi-ps:CLLN figi-gii:hasUniqueTextIdentifier "CLLN" .

figi-ps:KDB a figi-gii:PricingSource .

figi-ps:CLM a owl:NamedIndividual .

figi-ps:KDB skos:prefLabel "korea development bk" .

figi-ps:CLM a figi-gii:PricingSource .

figi-ps:KDB figi-gii:hasUniqueTextIdentifier "KDB" .

figi-ps:CLM skos:prefLabel "chasm lake mgmt" .

figi-ps:KDBB a owl:NamedIndividual .

figi-ps:CLM figi-gii:hasUniqueTextIdentifier "CLM" .

figi-ps:KDBB a figi-gii:PricingSource .

figi-ps:CLMI a owl:NamedIndividual .

figi-ps:KDBB skos:prefLabel "banco kdb s.a." .

figi-ps:CLMI a figi-gii:PricingSource .

figi-ps:KDBB figi-gii:hasUniqueTextIdentifier "KDBB" .

figi-ps:CLMI skos:prefLabel "ca-cib bank" .

figi-ps:KDBL a owl:NamedIndividual , figi-gii:PricingSource .

figi-ps:CLMI figi-gii:hasUniqueTextIdentifier "CLMI" .

figi-ps:KDBL skos:prefLabel "korea devlop. bank" .

figi-ps:CLNY a owl:NamedIndividual .

figi-ps:KDBL figi-gii:hasUniqueTextIdentifier "KDBL" .

figi-ps:CLNY a figi-gii:PricingSource .

figi-ps:KDBS a owl:NamedIndividual .

figi-ps:CLNY skos:prefLabel "credit lyonnais" .

figi-ps:KDBS a figi-gii:PricingSource .

figi-ps:CLNY figi-gii:hasUniqueTextIdentifier "CLNY" .

figi-ps:KDBS skos:prefLabel "korea devpt bank sg" .

figi-ps:CLOM a owl:NamedIndividual .

figi-ps:KDBS figi-gii:hasUniqueTextIdentifier "KDBS" .

figi-ps:CLOM a figi-gii:PricingSource .

figi-ps:KDHL a owl:NamedIndividual .

figi-ps:CLOM skos:prefLabel "cassa lombarda milan" .

figi-ps:KDHL a figi-gii:PricingSource .

figi-ps:CLOM figi-gii:hasUniqueTextIdentifier "CLOM" .

figi-ps:KDHL skos:prefLabel "kakawa" .

figi-ps:CLRD a owl:NamedIndividual .

figi-ps:KDHL figi-gii:hasUniqueTextIdentifier "KDHL" .

figi-ps:CLRD a figi-gii:PricingSource .

figi-ps:KDP a owl:NamedIndividual .

figi-ps:CLRD skos:prefLabel "claren road asset" .

figi-ps:KDP a figi-gii:PricingSource .

figi-ps:CLRD figi-gii:hasUniqueTextIdentifier "CLRD" .

figi-ps:KDP skos:prefLabel "kdp investment" .

figi-ps:CLRF a owl:NamedIndividual .

figi-ps:KDP figi-gii:hasUniqueTextIdentifier "KDP" .

figi-ps:CLRF a figi-gii:PricingSource .

figi-ps:KEAT a owl:NamedIndividual .

figi-ps:CLRF skos:prefLabel "clarkson securities" .

figi-ps:KEAT a figi-gii:PricingSource .

figi-ps:CLRF figi-gii:hasUniqueTextIdentifier "CLRF" .

figi-ps:KEAT skos:prefLabel "kim eng asset mgmt" .

figi-ps:CLSC a owl:NamedIndividual .

figi-ps:KEAT figi-gii:hasUniqueTextIdentifier "KEAT" .

figi-ps:CLSC a figi-gii:PricingSource .

figi-ps:KEET a owl:NamedIndividual .

figi-ps:CLSC skos:prefLabel "central securities" .

figi-ps:KEET a figi-gii:PricingSource .

figi-ps:CLSC figi-gii:hasUniqueTextIdentifier "CLSC" .

figi-ps:KEET skos:prefLabel "kommunalkredit aus" .

figi-ps:CLST a owl:NamedIndividual .

figi-ps:KEET figi-gii:hasUniqueTextIdentifier "KEET" .

figi-ps:CLST a figi-gii:PricingSource .

figi-ps:KEJK a owl:NamedIndividual .

figi-ps:CLST skos:prefLabel "canaccord genuity" .

figi-ps:KEJK a figi-gii:PricingSource .

figi-ps:CLST figi-gii:hasUniqueTextIdentifier "CLST" .

figi-ps:KEJK skos:prefLabel "kim eng securities" .

figi-ps:CMAM a owl:NamedIndividual .

figi-ps:KEJK figi-gii:hasUniqueTextIdentifier "KEJK" .

figi-ps:CMAM a figi-gii:PricingSource .

figi-ps:KEMP a owl:NamedIndividual .

figi-ps:CMAM skos:prefLabel "cm-cic am" .

figi-ps:KEMP a figi-gii:PricingSource .

figi-ps:CMAM figi-gii:hasUniqueTextIdentifier "CMAM" .

figi-ps:KEMP skos:prefLabel "kempen and co" .

figi-ps:CMAR a owl:NamedIndividual .

figi-ps:KEMP figi-gii:hasUniqueTextIdentifier "KEMP" .

figi-ps:CMAR a figi-gii:PricingSource .

figi-ps:KENT a owl:NamedIndividual .

figi-ps:CMAR skos:prefLabel "credit mutuel arkea" .

figi-ps:KENT a figi-gii:PricingSource .

figi-ps:CMAR figi-gii:hasUniqueTextIdentifier "CMAR" .

figi-ps:KENT skos:prefLabel "kentbank" .

figi-ps:CMB a owl:NamedIndividual .

figi-ps:KENT figi-gii:hasUniqueTextIdentifier "KENT" .

figi-ps:CMB a figi-gii:PricingSource .

figi-ps:KFHB a owl:NamedIndividual .

figi-ps:CMB skos:prefLabel "china merchants bank" .

figi-ps:KFHB a figi-gii:PricingSource .

figi-ps:CMB figi-gii:hasUniqueTextIdentifier "CMB" .

figi-ps:KFHB skos:prefLabel "kfh malaysia" .

figi-ps:CMBC a owl:NamedIndividual .

figi-ps:KFHB figi-gii:hasUniqueTextIdentifier "KFHB" .

figi-ps:CMBC a figi-gii:PricingSource .

figi-ps:KFHD a owl:NamedIndividual .

figi-ps:CMBC skos:prefLabel "china minsheng bank" .

figi-ps:KFHD a figi-gii:PricingSource .

figi-ps:CMBC figi-gii:hasUniqueTextIdentifier "CMBC" .

figi-ps:KFHD skos:prefLabel "kuwait finance" .

figi-ps:CMBR a owl:NamedIndividual .

figi-ps:KFHD figi-gii:hasUniqueTextIdentifier "KFHD" .

figi-ps:CMBR a figi-gii:PricingSource .

figi-ps:KFHM a owl:NamedIndividual .

figi-ps:CMBR skos:prefLabel "cm capital mkts" .

figi-ps:KFHM a figi-gii:PricingSource .

figi-ps:CMBR figi-gii:hasUniqueTextIdentifier "CMBR" .

figi-ps:KFHM skos:prefLabel "kuwait finance house" .

figi-ps:CMBS a owl:NamedIndividual .

figi-ps:KFHM figi-gii:hasUniqueTextIdentifier "KFHM" .

figi-ps:CMBS a figi-gii:PricingSource .

figi-ps:KFIM a owl:NamedIndividual .

figi-ps:CMBS skos:prefLabel "cfets abs-mbs" .

figi-ps:KFIM a figi-gii:PricingSource .

figi-ps:CMBS figi-gii:hasUniqueTextIdentifier "CMBS" .

figi-ps:KFIM skos:prefLabel "keijser capital" .

figi-ps:CMCA a owl:NamedIndividual .

figi-ps:KFIM figi-gii:hasUniqueTextIdentifier "KFIM" .

figi-ps:CMCA a figi-gii:PricingSource .

figi-ps:KGIS a owl:NamedIndividual .

figi-ps:CMCA skos:prefLabel "comerica equity" .

figi-ps:KGIS a figi-gii:PricingSource .

figi-ps:CMCA figi-gii:hasUniqueTextIdentifier "CMCA" .

figi-ps:KGIS skos:prefLabel "kgi securities, th" .

figi-ps:CMCM a owl:NamedIndividual .

figi-ps:KGIS figi-gii:hasUniqueTextIdentifier "KGIS" .

figi-ps:CMCM a figi-gii:PricingSource .

figi-ps:KGIT a owl:NamedIndividual .

figi-ps:CMCM skos:prefLabel "cm capital mrkts" .

figi-ps:KGIT a figi-gii:PricingSource .

figi-ps:CMCM figi-gii:hasUniqueTextIdentifier "CMCM" .

figi-ps:KGIT skos:prefLabel "kgi securities,tw" .

figi-ps:CMDN a owl:NamedIndividual .

figi-ps:KGIT figi-gii:hasUniqueTextIdentifier "KGIT" .

figi-ps:CMDN a figi-gii:PricingSource .

figi-ps:KGS a owl:NamedIndividual .

figi-ps:CMDN skos:prefLabel "camden asset mgmt" .

figi-ps:KGS a figi-gii:PricingSource .

figi-ps:CMDN figi-gii:hasUniqueTextIdentifier "CMDN" .

figi-ps:KGS skos:prefLabel "kgs-alpha" .

figi-ps:CMEN a owl:NamedIndividual .

figi-ps:KGS figi-gii:hasUniqueTextIdentifier "KGS" .

figi-ps:CMEN a figi-gii:PricingSource .

figi-ps:KHAD a owl:NamedIndividual .

figi-ps:CMEN skos:prefLabel "cnbond cn merch bk" .

figi-ps:KHAD a figi-gii:PricingSource .

figi-ps:CMEN figi-gii:hasUniqueTextIdentifier "CMEN" .

figi-ps:KHAD skos:prefLabel "kasb securities" .

figi-ps:CMER a owl:NamedIndividual .

figi-ps:KHAD figi-gii:hasUniqueTextIdentifier "KHAD" .

figi-ps:CMER a figi-gii:PricingSource .

figi-ps:KHBM a owl:NamedIndividual , figi-gii:PricingSource .

figi-ps:CMER skos:prefLabel "cfet ch merchants bk" .

figi-ps:KHBM skos:prefLabel "khan bank" .

figi-ps:CMER figi-gii:hasUniqueTextIdentifier "CMER" .

figi-ps:KHBM figi-gii:hasUniqueTextIdentifier "KHBM" .

figi-ps:CMF a owl:NamedIndividual .

figi-ps:KHDS a owl:NamedIndividual .

figi-ps:CMF a figi-gii:PricingSource .

figi-ps:KHDS a figi-gii:PricingSource .

figi-ps:CMF skos:prefLabel "china merchants fund" .

figi-ps:KHDS skos:prefLabel "khandwala secs ltd" .

figi-ps:CMF figi-gii:hasUniqueTextIdentifier "CMF" .

figi-ps:KHDS figi-gii:hasUniqueTextIdentifier "KHDS" .

figi-ps:CMGL a owl:NamedIndividual .

figi-ps:KHL2 a owl:NamedIndividual .

figi-ps:CMGL a figi-gii:PricingSource .

figi-ps:KHL2 a figi-gii:PricingSource .

figi-ps:CMGL skos:prefLabel "blp commingled" .

figi-ps:KHL2 skos:prefLabel "al khalij comm bank" .

figi-ps:CMGL figi-gii:hasUniqueTextIdentifier "CMGL" .

figi-ps:KHL2 figi-gii:hasUniqueTextIdentifier "KHL2" .

figi-ps:CMGS a owl:NamedIndividual .

figi-ps:KHLJ a owl:NamedIndividual .

figi-ps:CMGS a figi-gii:PricingSource .

figi-ps:KHLJ a figi-gii:PricingSource .

figi-ps:CMGS skos:prefLabel "cibc mellon global" .

figi-ps:KHLJ skos:prefLabel "al khalij comm bank" .

figi-ps:CMGS figi-gii:hasUniqueTextIdentifier "CMGS" .

figi-ps:KHLJ figi-gii:hasUniqueTextIdentifier "KHLJ" .

figi-ps:CMIB a owl:NamedIndividual .

figi-ps:KIBK a owl:NamedIndividual .

figi-ps:CMIB a figi-gii:PricingSource .

figi-ps:KIBK a figi-gii:PricingSource .

figi-ps:CMIB skos:prefLabel "commercial int'l bk" .

figi-ps:KIBK skos:prefLabel "kuwait intl bank" .

figi-ps:CMIB figi-gii:hasUniqueTextIdentifier "CMIB" .

figi-ps:KIBK figi-gii:hasUniqueTextIdentifier "KIBK" .

figi-ps:CMMB a owl:NamedIndividual .

figi-ps:KIC a owl:NamedIndividual .

figi-ps:CMMB a figi-gii:PricingSource .

figi-ps:KIC a figi-gii:PricingSource .

figi-ps:CMMB skos:prefLabel "caribbean mmkt brkrs" .

figi-ps:KIC skos:prefLabel "korea invest corp" .

figi-ps:CMMB skos:prefLabel "first citizens" .

figi-ps:KIC figi-gii:hasUniqueTextIdentifier "KIC" .

figi-ps:CMMB figi-gii:hasUniqueTextIdentifier "CMMB" .

figi-ps:KIDB a owl:NamedIndividual .

figi-ps:CMOS a owl:NamedIndividual .

figi-ps:KIDB a figi-gii:PricingSource .

figi-ps:CMOS a figi-gii:PricingSource .

figi-ps:KIDB skos:prefLabel "korea inter dealer" .

figi-ps:CMOS skos:prefLabel "jvb financial" .

figi-ps:KIDB figi-gii:hasUniqueTextIdentifier "KIDB" .

figi-ps:CMOS figi-gii:hasUniqueTextIdentifier "CMOS" .

figi-ps:KILE a owl:NamedIndividual , figi-gii:PricingSource ;
	skos:prefLabel "kiley partners, inc" ;
	figi-gii:hasUniqueTextIdentifier "KILE" .

figi-ps:CMPS a owl:NamedIndividual .

figi-ps:KILO a owl:NamedIndividual , figi-gii:PricingSource .

figi-ps:CMPS a figi-gii:PricingSource .

figi-ps:KILO skos:prefLabel "kilometre capital" .

figi-ps:CMPS skos:prefLabel "campisi and c. sim spa" .

figi-ps:KILO figi-gii:hasUniqueTextIdentifier "KILO" .

figi-ps:CMPS figi-gii:hasUniqueTextIdentifier "CMPS" .

figi-ps:KING a owl:NamedIndividual .

figi-ps:CMRC a owl:NamedIndividual .

figi-ps:KING a figi-gii:PricingSource .

figi-ps:CMRC a figi-gii:PricingSource .

figi-ps:KING skos:prefLabel "cl king and associat" .

figi-ps:CMRC skos:prefLabel "commerce group" .

figi-ps:KING figi-gii:hasUniqueTextIdentifier "KING" .

figi-ps:CMRC figi-gii:hasUniqueTextIdentifier "CMRC" .

figi-ps:KISK a owl:NamedIndividual .

figi-ps:CMSB a owl:NamedIndividual .

figi-ps:KISK a figi-gii:PricingSource .

figi-ps:CMSB a figi-gii:PricingSource .

figi-ps:KISK skos:prefLabel "korea investor svc" .

figi-ps:CMSB skos:prefLabel "cfet ch minsheng bk" .

figi-ps:KISK figi-gii:hasUniqueTextIdentifier "KISK" .

figi-ps:CMSB figi-gii:hasUniqueTextIdentifier "CMSB" .

figi-ps:KISP a owl:NamedIndividual .

figi-ps:CMSC a owl:NamedIndividual .

figi-ps:KISP a figi-gii:PricingSource .

figi-ps:CMSC a figi-gii:PricingSource .

figi-ps:KISP skos:prefLabel "kis pricing (yield)" .

figi-ps:CMSC skos:prefLabel "china merchants sec" .

figi-ps:KISP figi-gii:hasUniqueTextIdentifier "KISP" .

figi-ps:CMSC figi-gii:hasUniqueTextIdentifier "CMSC" .

figi-ps:KIWB a owl:NamedIndividual .

figi-ps:CMSN a owl:NamedIndividual .

figi-ps:KIWB a figi-gii:PricingSource .

figi-ps:CMSN a figi-gii:PricingSource .

figi-ps:KIWB skos:prefLabel "kiwi bank ltd" .

figi-ps:CMSN skos:prefLabel "cnbond minsheng bk" .

figi-ps:KIWB figi-gii:hasUniqueTextIdentifier "KIWB" .

figi-ps:CMSN figi-gii:hasUniqueTextIdentifier "CMSN" .

figi-ps:KIWI a owl:NamedIndividual .

figi-ps:CMSS a owl:NamedIndividual .

figi-ps:KIWI a figi-gii:PricingSource .

figi-ps:CMSS a figi-gii:PricingSource .

figi-ps:KIWI skos:prefLabel "kiwi bank limited" .

figi-ps:CMSS skos:prefLabel "compass group" .

figi-ps:KIWI figi-gii:hasUniqueTextIdentifier "KIWI" .

figi-ps:CMSS figi-gii:hasUniqueTextIdentifier "CMSS" .

figi-ps:KIWO a owl:NamedIndividual .

figi-ps:CMTS a owl:NamedIndividual .

figi-ps:KIWO a figi-gii:PricingSource .

figi-ps:CMTS a figi-gii:PricingSource .

figi-ps:KIWO skos:prefLabel "kiwoomcom" .

figi-ps:CMTS skos:prefLabel "eurocredit mts" .

figi-ps:KIWO figi-gii:hasUniqueTextIdentifier "KIWO" .

figi-ps:CMTS figi-gii:hasUniqueTextIdentifier "CMTS" .

figi-ps:KLI a owl:NamedIndividual .

figi-ps:CNA a owl:NamedIndividual .

figi-ps:KLI a figi-gii:PricingSource .

figi-ps:CNA a figi-gii:PricingSource .

figi-ps:KLI skos:prefLabel "knight libertas intl" .

figi-ps:CNA skos:prefLabel "cna financial corp" .

figi-ps:KLI figi-gii:hasUniqueTextIdentifier "KLI" .

figi-ps:CNA figi-gii:hasUniqueTextIdentifier "CNA" .

figi-ps:KLS a owl:NamedIndividual .

figi-ps:CNB a owl:NamedIndividual .

figi-ps:KLS a figi-gii:PricingSource .

figi-ps:CNB a figi-gii:PricingSource .

figi-ps:KLS skos:prefLabel "kls diversified" .

figi-ps:CNB skos:prefLabel "city national bank" .

figi-ps:KLS figi-gii:hasUniqueTextIdentifier "KLS" .

figi-ps:CNB figi-gii:hasUniqueTextIdentifier "CNB" .

figi-ps:KLSD a owl:NamedIndividual .

figi-ps:CNBK a owl:NamedIndividual .

figi-ps:KLSD a figi-gii:PricingSource .

figi-ps:CNBK a figi-gii:PricingSource .

figi-ps:KLSD skos:prefLabel "kis diversified" .

figi-ps:CNBK skos:prefLabel "canara bank" .

figi-ps:KLSD skos:prefLabel "kls diversified" .

figi-ps:CNBK figi-gii:hasUniqueTextIdentifier "CNBK" .

figi-ps:KLSD figi-gii:hasUniqueTextIdentifier "KLSD" .

figi-ps:CNMB a owl:NamedIndividual .

figi-ps:KLSE a owl:NamedIndividual .

figi-ps:CNMB a figi-gii:PricingSource .

figi-ps:KLSE a figi-gii:PricingSource .

figi-ps:CNMB skos:prefLabel "cfif ch merchants bk" .

figi-ps:KLSE skos:prefLabel "bursa malaysia" .

figi-ps:CNMB figi-gii:hasUniqueTextIdentifier "CNMB" .

figi-ps:KLSE figi-gii:hasUniqueTextIdentifier "KLSE" .

figi-ps:CNPT a owl:NamedIndividual .

figi-ps:KMBL a owl:NamedIndividual .

figi-ps:CNPT a figi-gii:PricingSource .

figi-ps:KMBL a figi-gii:PricingSource .

figi-ps:CNPT skos:prefLabel "cn pension trust" .

figi-ps:KMBL skos:prefLabel "kotak mahindra bank" .

figi-ps:CNPT figi-gii:hasUniqueTextIdentifier "CNPT" .

figi-ps:KMBL figi-gii:hasUniqueTextIdentifier "KMBL" .

figi-ps:CNST a owl:NamedIndividual .

figi-ps:KMBS a owl:NamedIndividual .

figi-ps:CNST a figi-gii:PricingSource .

figi-ps:KMBS a figi-gii:PricingSource .

figi-ps:CNST skos:prefLabel "consultinvest sgr" .

figi-ps:KMBS skos:prefLabel "kookmin bk-intl fin" .

figi-ps:CNST figi-gii:hasUniqueTextIdentifier "CNST" .

figi-ps:KMBS figi-gii:hasUniqueTextIdentifier "KMBS" .

figi-ps:CNTF a owl:NamedIndividual .

figi-ps:KMGB a owl:NamedIndividual .

figi-ps:CNTF a figi-gii:PricingSource .

figi-ps:KMGB a figi-gii:PricingSource .

figi-ps:CNTF skos:prefLabel "cantor fitzgerald lp" .

figi-ps:KMGB skos:prefLabel "kmg holding ag" .

figi-ps:CNTF figi-gii:hasUniqueTextIdentifier "CNTF" .

figi-ps:KMGB figi-gii:hasUniqueTextIdentifier "KMGB" .

figi-ps:CNTR a owl:NamedIndividual .

figi-ps:KMUK a owl:NamedIndividual .

figi-ps:CNTR a figi-gii:PricingSource .

figi-ps:KMUK a figi-gii:PricingSource .

figi-ps:CNTR skos:prefLabel "bgc market data" .

figi-ps:KMUK skos:prefLabel "kotak mahindra (uk)" .

figi-ps:CNTR figi-gii:hasUniqueTextIdentifier "CNTR" .

figi-ps:KMUK figi-gii:hasUniqueTextIdentifier "KMUK" .

figi-ps:CNTS a owl:NamedIndividual .

figi-ps:KND a owl:NamedIndividual .

figi-ps:CNTS a figi-gii:PricingSource .

figi-ps:KND a figi-gii:PricingSource .

figi-ps:CNTS skos:prefLabel "centras securities" .

figi-ps:KND skos:prefLabel "kinsell newcomb and de" .

figi-ps:CNTS figi-gii:hasUniqueTextIdentifier "CNTS" .

figi-ps:KND figi-gii:hasUniqueTextIdentifier "KND" .

figi-ps:CNVC a owl:NamedIndividual .

figi-ps:KNGK a owl:NamedIndividual .

figi-ps:CNVC a figi-gii:PricingSource .

figi-ps:KNGK a figi-gii:PricingSource .

figi-ps:CNVC skos:prefLabel "convencao" .

figi-ps:KNGK skos:prefLabel "kingdom securities" .

figi-ps:CNVC figi-gii:hasUniqueTextIdentifier "CNVC" .

figi-ps:KNGK figi-gii:hasUniqueTextIdentifier "KNGK" .

figi-ps:COAK a owl:NamedIndividual .

figi-ps:KNGS a owl:NamedIndividual .

figi-ps:COAK a figi-gii:PricingSource .

figi-ps:KNGS a figi-gii:PricingSource .

figi-ps:COAK skos:prefLabel "castleoak securities" .

figi-ps:KNGS skos:prefLabel "kng securities" .

figi-ps:COAK figi-gii:hasUniqueTextIdentifier "COAK" .

figi-ps:KNGS figi-gii:hasUniqueTextIdentifier "KNGS" .

figi-ps:COAS a owl:NamedIndividual .

figi-ps:KOFC a owl:NamedIndividual .

figi-ps:COAS a figi-gii:PricingSource .

figi-ps:KOFC a figi-gii:PricingSource .

figi-ps:COAS skos:prefLabel "corredores asociados" .

figi-ps:KOFC skos:prefLabel "knights of columbus" .

figi-ps:COAS figi-gii:hasUniqueTextIdentifier "COAS" .

figi-ps:KOFC figi-gii:hasUniqueTextIdentifier "KOFC" .

figi-ps:COBA a owl:NamedIndividual .

figi-ps:KOMB a owl:NamedIndividual .

figi-ps:COBA a figi-gii:PricingSource .

figi-ps:KOMB a figi-gii:PricingSource .

figi-ps:COBA skos:prefLabel "commerzbnkstructpdts" .

figi-ps:KOMB skos:prefLabel "komercni banka" .

figi-ps:COBA figi-gii:hasUniqueTextIdentifier "COBA" .

figi-ps:KOMB figi-gii:hasUniqueTextIdentifier "KOMB" .

figi-ps:COF a owl:NamedIndividual .

figi-ps:KPAR a owl:NamedIndividual .

figi-ps:COF a figi-gii:PricingSource .

figi-ps:KPAR a figi-gii:PricingSource .

figi-ps:COF skos:prefLabel "capital one financia" .

figi-ps:KPAR skos:prefLabel "kellogg partners" .

figi-ps:COF figi-gii:hasUniqueTextIdentifier "COF" .

figi-ps:KPAR figi-gii:hasUniqueTextIdentifier "KPAR" .

figi-ps:COFI a owl:NamedIndividual .

figi-ps:KPEC a owl:NamedIndividual .

figi-ps:COFI a figi-gii:PricingSource .

figi-ps:KPEC a figi-gii:PricingSource .

figi-ps:COFI skos:prefLabel "cofide" .

figi-ps:KPEC skos:prefLabel "kepler cm" .

figi-ps:COFI figi-gii:hasUniqueTextIdentifier "COFI" .

figi-ps:KPEC figi-gii:hasUniqueTextIdentifier "KPEC" .

figi-ps:COHE a owl:NamedIndividual .

figi-ps:KPEM a owl:NamedIndividual .

figi-ps:COHE a figi-gii:PricingSource .

figi-ps:KPEM a figi-gii:PricingSource .

figi-ps:COHE skos:prefLabel "cohen bros and co" .

figi-ps:KPEM skos:prefLabel "kepler equities sz" .

figi-ps:COHE figi-gii:hasUniqueTextIdentifier "COHE" .

figi-ps:KPEM figi-gii:hasUniqueTextIdentifier "KPEM" .

figi-ps:COJP a owl:NamedIndividual .

figi-ps:KPIX a owl:NamedIndividual .

figi-ps:COJP a figi-gii:PricingSource .

figi-ps:KPIX a figi-gii:PricingSource .

figi-ps:COJP skos:prefLabel "jp morgan bogota" .

figi-ps:KPIX skos:prefLabel "kiley partners, inc" .

figi-ps:COJP figi-gii:hasUniqueTextIdentifier "COJP" .

figi-ps:KPIX figi-gii:hasUniqueTextIdentifier "KPIX" .

figi-ps:COL a owl:NamedIndividual .

figi-ps:KPM a owl:NamedIndividual .

figi-ps:COL a figi-gii:PricingSource .

figi-ps:KPM a figi-gii:PricingSource .

figi-ps:COL skos:prefLabel "colonial first" .

figi-ps:KPM skos:prefLabel "kdp investment inc" .

figi-ps:COL figi-gii:hasUniqueTextIdentifier "COL" .

figi-ps:KPM figi-gii:hasUniqueTextIdentifier "KPM" .

figi-ps:COMC a owl:NamedIndividual .

figi-ps:KRBN a owl:NamedIndividual .

figi-ps:COMC a figi-gii:PricingSource .

figi-ps:KRBN a figi-gii:PricingSource .

figi-ps:COMC skos:prefLabel "commerce bank kc" .

figi-ps:KRBN skos:prefLabel "karbone inc" .

figi-ps:COMC figi-gii:hasUniqueTextIdentifier "COMC" .

figi-ps:KRBN figi-gii:hasUniqueTextIdentifier "KRBN" .

figi-ps:COMM a owl:NamedIndividual .

figi-ps:KRDB a owl:NamedIndividual .

figi-ps:COMM a figi-gii:PricingSource .

figi-ps:KRDB a figi-gii:PricingSource .

figi-ps:COMM skos:prefLabel "commercial b. ceylon" .

figi-ps:KRDB skos:prefLabel "korea development ba" .

figi-ps:COMM figi-gii:hasUniqueTextIdentifier "COMM" .

figi-ps:KRDB figi-gii:hasUniqueTextIdentifier "KRDB" .

figi-ps:COMS a owl:NamedIndividual .

figi-ps:KRES a owl:NamedIndividual .

figi-ps:COMS a figi-gii:PricingSource .

figi-ps:KRES a figi-gii:PricingSource .

figi-ps:COMS skos:prefLabel "comerica securities" .

figi-ps:KRES skos:prefLabel "kresna securities" .

figi-ps:COMS figi-gii:hasUniqueTextIdentifier "COMS" .

figi-ps:KRES figi-gii:hasUniqueTextIdentifier "KRES" .

figi-ps:CON a owl:NamedIndividual .

figi-ps:KRFZ a owl:NamedIndividual .

figi-ps:CON a figi-gii:PricingSource .

figi-ps:KRFZ a figi-gii:PricingSource .

figi-ps:CON skos:prefLabel "conning and co." .

figi-ps:KRFZ skos:prefLabel "korfezbank" .

figi-ps:CON figi-gii:hasUniqueTextIdentifier "CON" .

figi-ps:KRFZ figi-gii:hasUniqueTextIdentifier "KRFZ" .

figi-ps:CONF a owl:NamedIndividual .

figi-ps:KRTH a owl:NamedIndividual .

figi-ps:CONF a figi-gii:PricingSource .

figi-ps:KRTH a figi-gii:PricingSource .

figi-ps:CONF skos:prefLabel "aim - conference" .

figi-ps:KRTH skos:prefLabel "jw korth and co" .

figi-ps:CONF figi-gii:hasUniqueTextIdentifier "CONF" .

figi-ps:KRTH figi-gii:hasUniqueTextIdentifier "KRTH" .

figi-ps:CONN a owl:NamedIndividual .

figi-ps:KSAM a owl:NamedIndividual .

figi-ps:CONN a figi-gii:PricingSource .

figi-ps:KSAM a figi-gii:PricingSource .

figi-ps:CONN skos:prefLabel "conning" .

figi-ps:KSAM skos:prefLabel "ksam" .

figi-ps:CONN figi-gii:hasUniqueTextIdentifier "CONN" .

figi-ps:KSAM figi-gii:hasUniqueTextIdentifier "KSAM" .

figi-ps:CONO a owl:NamedIndividual .

figi-ps:KSBB a owl:NamedIndividual .

figi-ps:CONO a figi-gii:PricingSource .

figi-ps:KSBB a figi-gii:PricingSource .

figi-ps:CONO skos:prefLabel "chinabond val othe n" .

figi-ps:KSBB skos:prefLabel "king and shaxson" .

figi-ps:CONO figi-gii:hasUniqueTextIdentifier "CONO" .

figi-ps:KSBB figi-gii:hasUniqueTextIdentifier "KSBB" .

figi-ps:CONQ a owl:NamedIndividual .

figi-ps:KSBE a owl:NamedIndividual .

figi-ps:CONQ a figi-gii:PricingSource .

figi-ps:KSBE a figi-gii:PricingSource .

figi-ps:CONQ skos:prefLabel "conquest capital" .

figi-ps:KSBE skos:prefLabel "king and shaxson" .

figi-ps:CONQ figi-gii:hasUniqueTextIdentifier "CONQ" .

figi-ps:KSBE figi-gii:hasUniqueTextIdentifier "KSBE" .

figi-ps:CONR a owl:NamedIndividual .

figi-ps:KSBM a owl:NamedIndividual .

figi-ps:CONR a figi-gii:PricingSource .

figi-ps:KSBM a figi-gii:PricingSource .

figi-ps:CONR skos:prefLabel "concorde capital" .

figi-ps:KSBM skos:prefLabel "bloomberg ksbm mtrix" .

figi-ps:CONR figi-gii:hasUniqueTextIdentifier "CONR" .

figi-ps:KSBM figi-gii:hasUniqueTextIdentifier "KSBM" .

figi-ps:CONS a owl:NamedIndividual .

figi-ps:KSDA a owl:NamedIndividual .

figi-ps:CONS a figi-gii:PricingSource .

figi-ps:KSDA a figi-gii:PricingSource .

figi-ps:CONS skos:prefLabel "consensus pmi" .

figi-ps:KSDA skos:prefLabel "korean sec dealers" .

figi-ps:CONS figi-gii:hasUniqueTextIdentifier "CONS" .

figi-ps:KSDA figi-gii:hasUniqueTextIdentifier "KSDA" .

figi-ps:CONT a owl:NamedIndividual .

figi-ps:KSDP a owl:NamedIndividual .

figi-ps:CONT a figi-gii:PricingSource .

figi-ps:KSDP a figi-gii:PricingSource .

figi-ps:CONT skos:prefLabel "constanta bank" .

figi-ps:KSDP skos:prefLabel "ksda otc price quote" ;
	figi-gii:hasUniqueTextIdentifier "KSDP" .

figi-ps:KSDY a owl:NamedIndividual , figi-gii:PricingSource ;
	skos:prefLabel "ksda otc yield quote" ;
	figi-gii:hasUniqueTextIdentifier "KSDY" .

figi-ps:KSEC a owl:NamedIndividual , figi-gii:PricingSource ;
	skos:prefLabel "korea stock exchange" ;
	figi-gii:hasUniqueTextIdentifier "KSEC" .

figi-ps:CONT figi-gii:hasUniqueTextIdentifier "CONT" .

figi-ps:KSEI a owl:NamedIndividual .

figi-ps:COOP a owl:NamedIndividual .

figi-ps:KSEI a figi-gii:PricingSource .

figi-ps:COOP a figi-gii:PricingSource .

figi-ps:KSEI skos:prefLabel "ksei" .

figi-ps:COOP skos:prefLabel "chinabond val othe o" .

figi-ps:KSEI figi-gii:hasUniqueTextIdentifier "KSEI" .

figi-ps:COOP figi-gii:hasUniqueTextIdentifier "COOP" .

figi-ps:KSEP a owl:NamedIndividual .

figi-ps:COPE a owl:NamedIndividual .

figi-ps:KSEP a figi-gii:PricingSource .

figi-ps:COPE a figi-gii:PricingSource .

figi-ps:KSEP skos:prefLabel "korea stk exch-price" .

figi-ps:COPE skos:prefLabel "copenhagen exchange" .

figi-ps:KSEP figi-gii:hasUniqueTextIdentifier "KSEP" .

figi-ps:COPE figi-gii:hasUniqueTextIdentifier "COPE" .

figi-ps:KSTB a owl:NamedIndividual .

figi-ps:COPS a owl:NamedIndividual .

figi-ps:KSTB a figi-gii:PricingSource .

figi-ps:COPS a figi-gii:PricingSource .

figi-ps:KSTB skos:prefLabel "kor standard bank" .

figi-ps:COPS skos:prefLabel "citi 144a" .

figi-ps:KSTB figi-gii:hasUniqueTextIdentifier "KSTB" .

figi-ps:COPS figi-gii:hasUniqueTextIdentifier "COPS" .

figi-ps:KTB a owl:NamedIndividual .

figi-ps:CORA a owl:NamedIndividual .

figi-ps:KTB a figi-gii:PricingSource .

figi-ps:CORA a figi-gii:PricingSource .

figi-ps:KTB skos:prefLabel "krung thai bank plc" .

figi-ps:CORA skos:prefLabel "corredores asociados" .

figi-ps:KTB figi-gii:hasUniqueTextIdentifier "KTB" .

figi-ps:CORA figi-gii:hasUniqueTextIdentifier "CORA" .

figi-ps:KTBI a owl:NamedIndividual .

figi-ps:CORB a owl:NamedIndividual .

figi-ps:KTBI a figi-gii:PricingSource .

figi-ps:CORB a figi-gii:PricingSource .

figi-ps:KTBI skos:prefLabel "krung thai bank" .

figi-ps:CORB skos:prefLabel "corpbanca" .

figi-ps:KTBI figi-gii:hasUniqueTextIdentifier "KTBI" .

figi-ps:CORB figi-gii:hasUniqueTextIdentifier "CORB" .

figi-ps:KTBT a owl:NamedIndividual .

figi-ps:CORF a owl:NamedIndividual .

figi-ps:KTBT a figi-gii:PricingSource .

figi-ps:CORF a figi-gii:PricingSource .

figi-ps:KTBT skos:prefLabel "krung thai bank" .

figi-ps:CORF skos:prefLabel "corficolombiana" .

figi-ps:KTBT figi-gii:hasUniqueTextIdentifier "KTBT" .

figi-ps:CORF figi-gii:hasUniqueTextIdentifier "CORF" .

figi-ps:KTFB a owl:NamedIndividual .

figi-ps:CORT a owl:NamedIndividual .

figi-ps:KTFB a figi-gii:PricingSource .

figi-ps:CORT a figi-gii:PricingSource .

figi-ps:KTFB skos:prefLabel "kit finance invest" .

figi-ps:CORT skos:prefLabel "cortview capital" .

figi-ps:KTFB figi-gii:hasUniqueTextIdentifier "KTFB" .

figi-ps:CORT figi-gii:hasUniqueTextIdentifier "CORT" .

figi-ps:KUWT a owl:NamedIndividual .

figi-ps:COSF a owl:NamedIndividual .

figi-ps:KUWT a figi-gii:PricingSource .

figi-ps:COSF a figi-gii:PricingSource .

figi-ps:KUWT skos:prefLabel "kuwait finance house" .

figi-ps:COSF skos:prefLabel "cosford capital" .

figi-ps:KUWT figi-gii:hasUniqueTextIdentifier "KUWT" .

figi-ps:COSF figi-gii:hasUniqueTextIdentifier "COSF" .

figi-ps:KWBK a owl:NamedIndividual .

figi-ps:COTS a owl:NamedIndividual .

figi-ps:KWBK a figi-gii:PricingSource .

figi-ps:COTS a figi-gii:PricingSource .

figi-ps:KWBK skos:prefLabel "citic ka wah bank" .

figi-ps:COTS skos:prefLabel "dresdner coba" .

figi-ps:KWBK figi-gii:hasUniqueTextIdentifier "KWBK" .

figi-ps:COTS figi-gii:hasUniqueTextIdentifier "COTS" .

figi-ps:KWFH a owl:NamedIndividual .

figi-ps:COUN a owl:NamedIndividual .

figi-ps:KWFH a figi-gii:PricingSource .

figi-ps:COUN a figi-gii:PricingSource .

figi-ps:KWFH skos:prefLabel "kuwait finance house" .

figi-ps:COUN skos:prefLabel "abu dhabi inv counc" .

figi-ps:KWFH figi-gii:hasUniqueTextIdentifier "KWFH" .

figi-ps:COUN figi-gii:hasUniqueTextIdentifier "COUN" .

figi-ps:KYOB a owl:NamedIndividual .

figi-ps:COWE a owl:NamedIndividual .

figi-ps:KYOB a figi-gii:PricingSource .

figi-ps:COWE a figi-gii:PricingSource .

figi-ps:KYOB skos:prefLabel "kyobo securities" .

figi-ps:COWE skos:prefLabel "cowen and company" .

figi-ps:KYOB figi-gii:hasUniqueTextIdentifier "KYOB" .

figi-ps:COWE figi-gii:hasUniqueTextIdentifier "COWE" .

figi-ps:KYSC a owl:NamedIndividual .

figi-ps:COWN a owl:NamedIndividual .

figi-ps:KYSC a figi-gii:PricingSource .

figi-ps:COWN a figi-gii:PricingSource .

figi-ps:KYSC skos:prefLabel "kyobo securities co" .

figi-ps:COWN skos:prefLabel "crosswind invmts llc" .

figi-ps:KYSC figi-gii:hasUniqueTextIdentifier "KYSC" .

figi-ps:COWN figi-gii:hasUniqueTextIdentifier "COWN" .

figi-ps:LBBJ a owl:NamedIndividual .

figi-ps:CP14 a owl:NamedIndividual .

figi-ps:LBBJ a figi-gii:PricingSource .

figi-ps:CP14 a figi-gii:PricingSource .

figi-ps:LBBJ skos:prefLabel "jumbo lbbw stuttgart" .

figi-ps:CP14 skos:prefLabel "cfets 14d bnd fwd pr" .

figi-ps:LBBJ figi-gii:hasUniqueTextIdentifier "LBBJ" .

figi-ps:CP14 figi-gii:hasUniqueTextIdentifier "CP14" .

figi-ps:LBWX a owl:NamedIndividual .

figi-ps:CP1M a owl:NamedIndividual .

figi-ps:LBWX a figi-gii:PricingSource .

figi-ps:CP1M a figi-gii:PricingSource .

figi-ps:LBWX skos:prefLabel "lbbw abs" .

figi-ps:CP1M skos:prefLabel "cfets 1m bnd fwd prx" .

figi-ps:LBWX figi-gii:hasUniqueTextIdentifier "LBWX" .

figi-ps:CP1M figi-gii:hasUniqueTextIdentifier "CP1M" .

figi-ps:LCPR a owl:NamedIndividual .

figi-ps:CP1Y a owl:NamedIndividual .

figi-ps:LCPR a figi-gii:PricingSource .

figi-ps:CP1Y a figi-gii:PricingSource .

figi-ps:LCPR skos:prefLabel "asia last price" .

figi-ps:CP1Y skos:prefLabel "cfets 1y bnd fwd prx" .

figi-ps:LCPR figi-gii:hasUniqueTextIdentifier "LCPR" .

figi-ps:CP1Y figi-gii:hasUniqueTextIdentifier "CP1Y" .

figi-ps:LEHM a owl:NamedIndividual .

figi-ps:CP21 a owl:NamedIndividual .

figi-ps:LEHM a figi-gii:PricingSource .

figi-ps:CP21 a figi-gii:PricingSource .

figi-ps:LEHM skos:prefLabel "barclays wealth amer" .

figi-ps:CP21 skos:prefLabel "cfets 21d bnd fwd pr" .

figi-ps:LEHM figi-gii:hasUniqueTextIdentifier "LEHM" .

figi-ps:CP21 figi-gii:hasUniqueTextIdentifier "CP21" .

figi-ps:LEU a owl:NamedIndividual .

figi-ps:CP2M a owl:NamedIndividual .

figi-ps:LEU a figi-gii:PricingSource .

figi-ps:CP2M a figi-gii:PricingSource .

figi-ps:LEU skos:prefLabel "bank leu" .

figi-ps:CP2M skos:prefLabel "cfets 2m bnd fwd prx" .

figi-ps:LEU figi-gii:hasUniqueTextIdentifier "LEU" .

figi-ps:CP2M figi-gii:hasUniqueTextIdentifier "CP2M" .

figi-ps:LEUM a owl:NamedIndividual .

figi-ps:CP3M a owl:NamedIndividual .

figi-ps:LEUM a figi-gii:PricingSource .

figi-ps:CP3M a figi-gii:PricingSource .

figi-ps:LEUM skos:prefLabel "bank leumi zurich" .

figi-ps:CP3M skos:prefLabel "cfets 3m bnd fwd prx" .

figi-ps:LEUM figi-gii:hasUniqueTextIdentifier "LEUM" .

figi-ps:CP3M figi-gii:hasUniqueTextIdentifier "CP3M" .

figi-ps:LFBP a owl:NamedIndividual .

figi-ps:CP4M a owl:NamedIndividual .

figi-ps:LFBP a figi-gii:PricingSource .

figi-ps:CP4M a figi-gii:PricingSource .

figi-ps:LFBP skos:prefLabel "la francaise" .

figi-ps:CP4M skos:prefLabel "cfets 4m bnd fwd prx" .

figi-ps:LFBP figi-gii:hasUniqueTextIdentifier "LFBP" .

figi-ps:CP4M figi-gii:hasUniqueTextIdentifier "CP4M" .

figi-ps:LIBE a owl:NamedIndividual .

figi-ps:CP6M a owl:NamedIndividual .

figi-ps:LIBE a figi-gii:PricingSource .

figi-ps:CP6M a figi-gii:PricingSource .

figi-ps:LIBE skos:prefLabel "knight fixed income" .

figi-ps:CP6M skos:prefLabel "cfets 6m bnd fwd prx" .

figi-ps:LIBE figi-gii:hasUniqueTextIdentifier "LIBE" .

figi-ps:CP6M figi-gii:hasUniqueTextIdentifier "CP6M" .

figi-ps:LIET a owl:NamedIndividual .

figi-ps:CP7D a owl:NamedIndividual .

figi-ps:LIET a figi-gii:PricingSource .

figi-ps:CP7D a figi-gii:PricingSource .

figi-ps:LIET skos:prefLabel "ab hansabankas" .

figi-ps:CP7D skos:prefLabel "cfets 7d bnd fwd prx" .

figi-ps:LIET figi-gii:hasUniqueTextIdentifier "LIET" .

figi-ps:CP7D figi-gii:hasUniqueTextIdentifier "CP7D" .

figi-ps:LINK a owl:NamedIndividual .

figi-ps:CP9M a owl:NamedIndividual .

figi-ps:LINK a figi-gii:PricingSource .

figi-ps:CP9M a figi-gii:PricingSource .

figi-ps:LINK skos:prefLabel "guggenheim cap mkts" .

figi-ps:CP9M skos:prefLabel "cfets 9m bnd fwd prx" .

figi-ps:LINK figi-gii:hasUniqueTextIdentifier "LINK" .

figi-ps:CP9M figi-gii:hasUniqueTextIdentifier "CP9M" .

figi-ps:LLEU a owl:NamedIndividual .

figi-ps:CPA a owl:NamedIndividual .

figi-ps:LLEU a figi-gii:PricingSource .

figi-ps:CPA a figi-gii:PricingSource .

figi-ps:LLEU skos:prefLabel "lloyds tsb ldn" .

figi-ps:CPA skos:prefLabel "capital alliance ltd" .

figi-ps:LLEU figi-gii:hasUniqueTextIdentifier "LLEU" .

figi-ps:CPA figi-gii:hasUniqueTextIdentifier "CPA" .

figi-ps:LLFI a owl:NamedIndividual .

figi-ps:CPAL a owl:NamedIndividual .

figi-ps:LLFI a figi-gii:PricingSource .

figi-ps:CPAL a figi-gii:PricingSource .

figi-ps:LLFI skos:prefLabel "lloyds tsb" .

figi-ps:CPAL skos:prefLabel "capital alliance" .

figi-ps:LLFI figi-gii:hasUniqueTextIdentifier "LLFI" .

figi-ps:CPAL figi-gii:hasUniqueTextIdentifier "CPAL" .

figi-ps:LNKS a owl:NamedIndividual .

figi-ps:CPB a owl:NamedIndividual .

figi-ps:LNKS a figi-gii:PricingSource .

figi-ps:CPB a figi-gii:PricingSource .

figi-ps:LNKS skos:prefLabel "guggenheim" .

figi-ps:CPB skos:prefLabel "citi private banking" .

figi-ps:LNKS figi-gii:hasUniqueTextIdentifier "LNKS" .

figi-ps:CPB figi-gii:hasUniqueTextIdentifier "CPB" .

figi-ps:LOMB a owl:NamedIndividual .

figi-ps:CPIC a owl:NamedIndividual .

figi-ps:LOMB a figi-gii:PricingSource .

figi-ps:CPIC a figi-gii:PricingSource .

figi-ps:LOMB skos:prefLabel "cassa lombarda" .

figi-ps:CPIC skos:prefLabel "cinda plunkett intl" .

figi-ps:LOMB figi-gii:hasUniqueTextIdentifier "LOMB" .

figi-ps:CPIC figi-gii:hasUniqueTextIdentifier "CPIC" .

figi-ps:LUX a owl:NamedIndividual .

figi-ps:CPIS a owl:NamedIndividual .

figi-ps:LUX a figi-gii:PricingSource .

figi-ps:CPIS a figi-gii:PricingSource .

figi-ps:LUX skos:prefLabel "luxembourg exchange" .

figi-ps:CPIS skos:prefLabel "capis" .

figi-ps:LUX figi-gii:hasUniqueTextIdentifier "LUX" .

figi-ps:CPIS figi-gii:hasUniqueTextIdentifier "CPIS" .

figi-ps:LYON a owl:NamedIndividual .

figi-ps:CPL a owl:NamedIndividual .

figi-ps:LYON a figi-gii:PricingSource .

figi-ps:CPL a figi-gii:PricingSource .

figi-ps:LYON skos:prefLabel "calyon securities" .

figi-ps:CPL skos:prefLabel "cambridge place ltd" .

figi-ps:LYON figi-gii:hasUniqueTextIdentifier "LYON" .

figi-ps:CPL figi-gii:hasUniqueTextIdentifier "CPL" .

figi-ps:MABS a owl:NamedIndividual .

figi-ps:CPOJ a owl:NamedIndividual .

figi-ps:MABS a figi-gii:PricingSource .

figi-ps:CPOJ a figi-gii:PricingSource .

figi-ps:MABS skos:prefLabel "boa merrill lynch" .

figi-ps:CPOJ skos:prefLabel "ceska pojistovna" .

figi-ps:MABS figi-gii:hasUniqueTextIdentifier "MABS" .

figi-ps:CPOJ figi-gii:hasUniqueTextIdentifier "CPOJ" .

figi-ps:MALA a owl:NamedIndividual .

figi-ps:CPP a owl:NamedIndividual .

figi-ps:MALA a figi-gii:PricingSource .

figi-ps:CPP a figi-gii:PricingSource .

figi-ps:MALA skos:prefLabel "jehangir, rustom" .

figi-ps:CPP skos:prefLabel "cpp investment board" .

figi-ps:MALA figi-gii:hasUniqueTextIdentifier "MALA" .

figi-ps:CPP figi-gii:hasUniqueTextIdentifier "CPP" .

figi-ps:MAND a owl:NamedIndividual .

figi-ps:CPRT a owl:NamedIndividual .

figi-ps:MAND a figi-gii:PricingSource .

figi-ps:CPRT a figi-gii:PricingSource .

figi-ps:MAND skos:prefLabel "bnk mandiri" .

figi-ps:CPRT skos:prefLabel "compass point randt" .

figi-ps:MAND figi-gii:hasUniqueTextIdentifier "MAND" .

figi-ps:CPRT figi-gii:hasUniqueTextIdentifier "CPRT" .

figi-ps:MARC a owl:NamedIndividual .

figi-ps:CPS a owl:NamedIndividual .

figi-ps:MARC a figi-gii:PricingSource .

figi-ps:CPS a figi-gii:PricingSource .

figi-ps:MARC skos:prefLabel "bbrg mart corp bond" .

figi-ps:CPS skos:prefLabel "capis" .

figi-ps:MARC figi-gii:hasUniqueTextIdentifier "MARC" .

figi-ps:CPS figi-gii:hasUniqueTextIdentifier "CPS" .

figi-ps:MART a owl:NamedIndividual .

figi-ps:CPTS a owl:NamedIndividual .

figi-ps:MART a figi-gii:PricingSource .

figi-ps:CPTS a figi-gii:PricingSource .

figi-ps:MART skos:prefLabel "bloomberg mart comp" .

figi-ps:CPTS skos:prefLabel "capital securities" .

figi-ps:MART figi-gii:hasUniqueTextIdentifier "MART" .

figi-ps:CPTS figi-gii:hasUniqueTextIdentifier "CPTS" .

figi-ps:MASS a owl:NamedIndividual .

figi-ps:CPTW a owl:NamedIndividual .

figi-ps:MASS a figi-gii:PricingSource .

figi-ps:CPTW a figi-gii:PricingSource .

figi-ps:MASS skos:prefLabel "babson capital" .

figi-ps:CPTW skos:prefLabel "capital securities" .

figi-ps:MASS figi-gii:hasUniqueTextIdentifier "MASS" .

figi-ps:CPTW figi-gii:hasUniqueTextIdentifier "CPTW" .

figi-ps:MAST a owl:NamedIndividual .

figi-ps:CQUA a owl:NamedIndividual .

figi-ps:MAST a figi-gii:PricingSource .

figi-ps:CQUA a figi-gii:PricingSource .

figi-ps:MAST skos:prefLabel "amstel securities nv" .

figi-ps:CQUA skos:prefLabel "c-quadrat" .

figi-ps:MAST figi-gii:hasUniqueTextIdentifier "MAST" .

figi-ps:CQUA figi-gii:hasUniqueTextIdentifier "CQUA" .

figi-ps:MATH a owl:NamedIndividual .

figi-ps:CRBK a owl:NamedIndividual .

figi-ps:MATH a figi-gii:PricingSource .

figi-ps:CRBK a figi-gii:PricingSource .

figi-ps:MATH skos:prefLabel "insinger de beaufort" .

figi-ps:CRBK skos:prefLabel "credit bank" .

figi-ps:MATH figi-gii:hasUniqueTextIdentifier "MATH" .

figi-ps:CRBK figi-gii:hasUniqueTextIdentifier "CRBK" .

figi-ps:MAXI a owl:NamedIndividual .

figi-ps:CRBN a owl:NamedIndividual .

figi-ps:MAXI a figi-gii:PricingSource .

figi-ps:CRBN a figi-gii:PricingSource .

figi-ps:MAXI skos:prefLabel "banco maxima" .

figi-ps:CRBN skos:prefLabel "bnp paribas credit" .

figi-ps:MAXI figi-gii:hasUniqueTextIdentifier "MAXI" .

figi-ps:CRBN figi-gii:hasUniqueTextIdentifier "CRBN" .

figi-ps:MAXM a owl:NamedIndividual .

figi-ps:CRDA a owl:NamedIndividual .

figi-ps:MAXM a figi-gii:PricingSource .

figi-ps:CRDA a figi-gii:PricingSource .

figi-ps:MAXM skos:prefLabel "maxim group" .

figi-ps:CRDA skos:prefLabel "crd analytics llc" .

figi-ps:MAXM figi-gii:hasUniqueTextIdentifier "MAXM" .

figi-ps:CRDA figi-gii:hasUniqueTextIdentifier "CRDA" .

figi-ps:MBMX a owl:NamedIndividual .

figi-ps:CRDC a owl:NamedIndividual .

figi-ps:MBMX a figi-gii:PricingSource .

figi-ps:CRDC a figi-gii:PricingSource .

figi-ps:MBMX skos:prefLabel "banca mb" .

figi-ps:CRDC skos:prefLabel "credicorp securities" .

figi-ps:MBMX figi-gii:hasUniqueTextIdentifier "MBMX" .

figi-ps:CRDC figi-gii:hasUniqueTextIdentifier "CRDC" .

figi-ps:MCRB a owl:NamedIndividual .

figi-ps:CREM a owl:NamedIndividual .

figi-ps:MCRB a figi-gii:PricingSource .

figi-ps:CREM a figi-gii:PricingSource .

figi-ps:MCRB skos:prefLabel "creditbank of moscow" .

figi-ps:CREM skos:prefLabel "citi em and intl" .

figi-ps:MCRB figi-gii:hasUniqueTextIdentifier "MCRB" .

figi-ps:CREM skos:prefLabel "credem" .

figi-ps:MDRI a owl:NamedIndividual .

figi-ps:CREM figi-gii:hasUniqueTextIdentifier "CREM" .

figi-ps:MDRI a figi-gii:PricingSource .

figi-ps:CRES a owl:NamedIndividual .

figi-ps:MDRI skos:prefLabel "bank mandiri" .

figi-ps:CRES a figi-gii:PricingSource .

figi-ps:MDRI figi-gii:hasUniqueTextIdentifier "MDRI" .

figi-ps:CRES skos:prefLabel "crescent advisor grp" .

figi-ps:MEDX a owl:NamedIndividual .

figi-ps:CRES figi-gii:hasUniqueTextIdentifier "CRES" .

figi-ps:MEDX a figi-gii:PricingSource .

figi-ps:CRET a owl:NamedIndividual .

figi-ps:MEDX skos:prefLabel "mediobanca spa" .

figi-ps:CRET a figi-gii:PricingSource .

figi-ps:MEDX figi-gii:hasUniqueTextIdentifier "MEDX" .

figi-ps:CRET skos:prefLabel "citigroup retail" .

figi-ps:MELI a owl:NamedIndividual .

figi-ps:CRET figi-gii:hasUniqueTextIdentifier "CRET" .

figi-ps:MELI a figi-gii:PricingSource .

figi-ps:CRIS a owl:NamedIndividual .

figi-ps:MELI skos:prefLabel "bper-meliorbanca" .

figi-ps:CRIS a figi-gii:PricingSource .

figi-ps:MELI figi-gii:hasUniqueTextIdentifier "MELI" .

figi-ps:CRIS skos:prefLabel "caris and company" .

figi-ps:MESA a owl:NamedIndividual .

figi-ps:CRIS figi-gii:hasUniqueTextIdentifier "CRIS" .

figi-ps:MESA a figi-gii:PricingSource .

figi-ps:CRMO a owl:NamedIndividual .

figi-ps:MESA skos:prefLabel "aim demo - mesa" .

figi-ps:CRMO a figi-gii:PricingSource .

figi-ps:MESA figi-gii:hasUniqueTextIdentifier "MESA" .

figi-ps:CRMO skos:prefLabel "credit - moscow bank" .

figi-ps:METS a owl:NamedIndividual .

figi-ps:CRMO figi-gii:hasUniqueTextIdentifier "CRMO" .

figi-ps:METS a figi-gii:PricingSource .

figi-ps:CROM a owl:NamedIndividual .

figi-ps:METS skos:prefLabel "aim demo - metrd" .

figi-ps:CROM a figi-gii:PricingSource .

figi-ps:METS figi-gii:hasUniqueTextIdentifier "METS" .

figi-ps:CROM skos:prefLabel "citibank romania" .

figi-ps:METX a owl:NamedIndividual .

figi-ps:CROM figi-gii:hasUniqueTextIdentifier "CROM" .

figi-ps:METX a figi-gii:PricingSource .

figi-ps:CROS a owl:NamedIndividual .

figi-ps:METX skos:prefLabel "meteorlogix llc" .

figi-ps:CROS a figi-gii:PricingSource .

figi-ps:METX figi-gii:hasUniqueTextIdentifier "METX" .

figi-ps:CROS skos:prefLabel "crosby advisors" .

figi-ps:MFI a owl:NamedIndividual .

figi-ps:CROS figi-gii:hasUniqueTextIdentifier "CROS" .

figi-ps:MFI a figi-gii:PricingSource .

figi-ps:CRRV a owl:NamedIndividual .

figi-ps:MFI skos:prefLabel "mesirow" .

figi-ps:CRRV a figi-gii:PricingSource .

figi-ps:MFI figi-gii:hasUniqueTextIdentifier "MFI" .

figi-ps:CRRV skos:prefLabel "correval sa" .

figi-ps:MHI a owl:NamedIndividual .

figi-ps:CRRV figi-gii:hasUniqueTextIdentifier "CRRV" .

figi-ps:MHI a figi-gii:PricingSource .

figi-ps:CRSA a owl:NamedIndividual .

figi-ps:MHI skos:prefLabel "mizuho international" .

figi-ps:CRSA a figi-gii:PricingSource .

figi-ps:MHI figi-gii:hasUniqueTextIdentifier "MHI" .

figi-ps:CRSA skos:prefLabel "credit agricole sa" .

figi-ps:MHIT a owl:NamedIndividual .

figi-ps:CRSA figi-gii:hasUniqueTextIdentifier "CRSA" .

figi-ps:MHIT a figi-gii:PricingSource .

figi-ps:CRSP a owl:NamedIndividual .

figi-ps:MHIT skos:prefLabel "mizuho international" .

figi-ps:CRSP a figi-gii:PricingSource .

figi-ps:MHIT figi-gii:hasUniqueTextIdentifier "MHIT" .

figi-ps:CRSP skos:prefLabel "citigroup hk" .

figi-ps:MICB a owl:NamedIndividual .

figi-ps:CRSP figi-gii:hasUniqueTextIdentifier "CRSP" .

figi-ps:MICB a figi-gii:PricingSource .

figi-ps:CRT a owl:NamedIndividual .

figi-ps:MICB skos:prefLabel "micex corp bonds" .

figi-ps:CRT a figi-gii:PricingSource .

figi-ps:MICB figi-gii:hasUniqueTextIdentifier "MICB" .

figi-ps:CRT skos:prefLabel "crt capital group" .

figi-ps:MILA a owl:NamedIndividual .

figi-ps:CRT figi-gii:hasUniqueTextIdentifier "CRT" .

figi-ps:MILA a figi-gii:PricingSource .

figi-ps:CRTB a owl:NamedIndividual .

figi-ps:MILA skos:prefLabel "milan exch" .

figi-ps:CRTB a figi-gii:PricingSource .

figi-ps:MILA figi-gii:hasUniqueTextIdentifier "MILA" .

figi-ps:CRTB skos:prefLabel "cartu bank" .

figi-ps:MILW a owl:NamedIndividual .

figi-ps:CRTB figi-gii:hasUniqueTextIdentifier "CRTB" .

figi-ps:MILW a figi-gii:PricingSource .

figi-ps:CRTC a owl:NamedIndividual .

figi-ps:MILW skos:prefLabel "bank millennium" .

figi-ps:CRTC a figi-gii:PricingSource .

figi-ps:MILW figi-gii:hasUniqueTextIdentifier "MILW" .

figi-ps:CRTC skos:prefLabel "crt capital group" .

figi-ps:MITM a owl:NamedIndividual .

figi-ps:CRTC figi-gii:hasUniqueTextIdentifier "CRTC" .

figi-ps:MITM a figi-gii:PricingSource .

figi-ps:CRTT a owl:NamedIndividual .

figi-ps:MITM skos:prefLabel "mitsubishi ufj sec" .

figi-ps:CRTT a figi-gii:PricingSource .

figi-ps:MITM figi-gii:hasUniqueTextIdentifier "MITM" .

figi-ps:CRTT skos:prefLabel "crt group toms px" .

figi-ps:MIYF a owl:NamedIndividual .

figi-ps:CRTT figi-gii:hasUniqueTextIdentifier "CRTT" .

figi-ps:MIYF a figi-gii:PricingSource .

figi-ps:CRTY a owl:NamedIndividual .

figi-ps:MIYF skos:prefLabel "mitsubishi yen bonds" .

figi-ps:CRTY a figi-gii:PricingSource .

figi-ps:MIYF figi-gii:hasUniqueTextIdentifier "MIYF" .

figi-ps:CRTY skos:prefLabel "carty and co" .

figi-ps:MIZM a owl:NamedIndividual .

figi-ps:CRTY figi-gii:hasUniqueTextIdentifier "CRTY" .

figi-ps:MIZM a figi-gii:PricingSource .

figi-ps:CRWN a owl:NamedIndividual .

figi-ps:MIZM skos:prefLabel "mizuho intl plc" .

figi-ps:CRWN a figi-gii:PricingSource .

figi-ps:MIZM figi-gii:hasUniqueTextIdentifier "MIZM" .

figi-ps:CRWN skos:prefLabel "crosswind invmts llc" .

figi-ps:MLAX a owl:NamedIndividual .

figi-ps:CRWN figi-gii:hasUniqueTextIdentifier "CRWN" .

figi-ps:MLAX a figi-gii:PricingSource .

figi-ps:CS a owl:NamedIndividual .

figi-ps:MLAX skos:prefLabel "bofa-ml treasury axe" .

figi-ps:CS a figi-gii:PricingSource .

figi-ps:MLAX figi-gii:hasUniqueTextIdentifier "MLAX" .

figi-ps:CS skos:prefLabel "creditsuisse" .

figi-ps:MLBP a owl:NamedIndividual .

figi-ps:CS figi-gii:hasUniqueTextIdentifier "CS" .

figi-ps:MLBP a figi-gii:PricingSource .

figi-ps:CSAB a owl:NamedIndividual .

figi-ps:MLBP skos:prefLabel "malbec partners-fi" .

figi-ps:CSAB a figi-gii:PricingSource .

figi-ps:MLBP figi-gii:hasUniqueTextIdentifier "MLBP" .

figi-ps:CSAB skos:prefLabel "credit suisse mtge" .

figi-ps:MLCL a owl:NamedIndividual .

figi-ps:CSAB skos:prefLabel "cs mortgages-abs" .

figi-ps:MLCL a figi-gii:PricingSource .

figi-ps:CSAB figi-gii:hasUniqueTextIdentifier "CSAB" .

figi-ps:MLCL skos:prefLabel "bofa ml london" .

figi-ps:CSAM a owl:NamedIndividual .

figi-ps:MLCL figi-gii:hasUniqueTextIdentifier "MLCL" .

figi-ps:CSAM a figi-gii:PricingSource .

figi-ps:MLIL a owl:NamedIndividual .

figi-ps:CSAM skos:prefLabel "csam zurich" .

figi-ps:MLIL a figi-gii:PricingSource .

figi-ps:CSAM figi-gii:hasUniqueTextIdentifier "CSAM" .

figi-ps:MLIL skos:prefLabel "bofa merrill lynch" .

figi-ps:CSAN a owl:NamedIndividual .

figi-ps:MLIL figi-gii:hasUniqueTextIdentifier "MLIL" .

figi-ps:CSAN a figi-gii:PricingSource .

figi-ps:MLIN a owl:NamedIndividual .

figi-ps:CSAN skos:prefLabel "cs first boston boom" .

figi-ps:MLIN a figi-gii:PricingSource .

figi-ps:CSAN figi-gii:hasUniqueTextIdentifier "CSAN" .

figi-ps:MLIN skos:prefLabel "merrill lynch" .

figi-ps:CSAS a owl:NamedIndividual .

figi-ps:MLIN figi-gii:hasUniqueTextIdentifier "MLIN" .

figi-ps:CSAS a figi-gii:PricingSource .

figi-ps:MLIX a owl:NamedIndividual .

figi-ps:CSAS skos:prefLabel "credit suisse sing" .

figi-ps:MLIX a figi-gii:PricingSource .

figi-ps:CSAS figi-gii:hasUniqueTextIdentifier "CSAS" .

figi-ps:MLIX skos:prefLabel "merrill lynch fi idx" .

figi-ps:CSAT a owl:NamedIndividual .

figi-ps:MLIX figi-gii:hasUniqueTextIdentifier "MLIX" .

figi-ps:CSAT a figi-gii:PricingSource .

figi-ps:MLJ a owl:NamedIndividual .

figi-ps:CSAT skos:prefLabel "cs latam bonds" .

figi-ps:MLJ a figi-gii:PricingSource .

figi-ps:CSAT figi-gii:hasUniqueTextIdentifier "CSAT" .

figi-ps:MLJ skos:prefLabel "bofa merrill lynch" .

figi-ps:CSAU a owl:NamedIndividual .

figi-ps:MLJ figi-gii:hasUniqueTextIdentifier "MLJ" .

figi-ps:CSAU a figi-gii:PricingSource .

figi-ps:MLJM a owl:NamedIndividual .

figi-ps:CSAU skos:prefLabel "credit suisse ltd" .

figi-ps:MLJM a figi-gii:PricingSource .

figi-ps:CSAU figi-gii:hasUniqueTextIdentifier "CSAU" .

figi-ps:MLJM skos:prefLabel "merrill lynch jp" .

figi-ps:CSBR a owl:NamedIndividual .

figi-ps:MLJM figi-gii:hasUniqueTextIdentifier "MLJM" .

figi-ps:CSBR a figi-gii:PricingSource .

figi-ps:MLNM a owl:NamedIndividual .

figi-ps:CSBR skos:prefLabel "credit suisse brazil" .

figi-ps:MLNM a figi-gii:PricingSource .

figi-ps:CSBR figi-gii:hasUniqueTextIdentifier "CSBR" .

figi-ps:MLNM skos:prefLabel "merrill lynch tba" .

figi-ps:CSBZ a owl:NamedIndividual , figi-gii:PricingSource .

figi-ps:MLNM figi-gii:hasUniqueTextIdentifier "MLNM" .

figi-ps:CSBZ skos:prefLabel "credit suisse brazil" .

figi-ps:MLO1 a owl:NamedIndividual .

figi-ps:CSBZ figi-gii:hasUniqueTextIdentifier "CSBZ" .

figi-ps:MLO1 a figi-gii:PricingSource .

figi-ps:CSCB a owl:NamedIndividual .

figi-ps:MLO1 skos:prefLabel "merrill lynch ldn" .

figi-ps:CSCB a figi-gii:PricingSource .

figi-ps:MLO1 figi-gii:hasUniqueTextIdentifier "MLO1" .

figi-ps:CSCB skos:prefLabel "cr suisse 1st boston" .

figi-ps:MLPL a owl:NamedIndividual .

figi-ps:CSCB figi-gii:hasUniqueTextIdentifier "CSCB" .

figi-ps:MLPL a figi-gii:PricingSource .

figi-ps:CSCC a owl:NamedIndividual .

figi-ps:MLPL skos:prefLabel "bank millennium sa" .

figi-ps:CSCC a figi-gii:PricingSource .

figi-ps:MLPL figi-gii:hasUniqueTextIdentifier "MLPL" .

figi-ps:CSCC skos:prefLabel "china securities" .

figi-ps:MLPS a owl:NamedIndividual .

figi-ps:CSCC figi-gii:hasUniqueTextIdentifier "CSCC" .

figi-ps:MLPS a figi-gii:PricingSource .

figi-ps:CSCM a owl:NamedIndividual .

figi-ps:MLPS skos:prefLabel "bofa-ml pricing svc" .

figi-ps:CSCM a figi-gii:PricingSource .

figi-ps:MLPS figi-gii:hasUniqueTextIdentifier "MLPS" .

figi-ps:CSCM skos:prefLabel "cs first boston mtge" .

figi-ps:MLSC a owl:NamedIndividual .

figi-ps:CSCM figi-gii:hasUniqueTextIdentifier "CSCM" .

figi-ps:MLSC a figi-gii:PricingSource .

figi-ps:CSD a owl:NamedIndividual .

figi-ps:MLSC skos:prefLabel "mi new york" .

figi-ps:CSD a figi-gii:PricingSource .

figi-ps:MLSC figi-gii:hasUniqueTextIdentifier "MLSC" .

figi-ps:CSD skos:prefLabel "county of san diego" .

figi-ps:MLST a owl:NamedIndividual .

figi-ps:CSD figi-gii:hasUniqueTextIdentifier "CSD" .

figi-ps:MLST a figi-gii:PricingSource .

figi-ps:CSDS a owl:NamedIndividual .

figi-ps:MLST skos:prefLabel "merrill lynch; lond" .

figi-ps:CSDS a figi-gii:PricingSource .

figi-ps:MLST figi-gii:hasUniqueTextIdentifier "MLST" .

figi-ps:CSDS skos:prefLabel "cs, london cds" .

figi-ps:MLTB a owl:NamedIndividual .

figi-ps:CSDS figi-gii:hasUniqueTextIdentifier "CSDS" .

figi-ps:MLTB a figi-gii:PricingSource .

figi-ps:CSE a owl:NamedIndividual .

figi-ps:MLTB skos:prefLabel "merrill lynch tbas" .

figi-ps:CSE a figi-gii:PricingSource .

figi-ps:MLTB figi-gii:hasUniqueTextIdentifier "MLTB" .

figi-ps:CSE skos:prefLabel "cyprus stock exch" .

figi-ps:MMBM a owl:NamedIndividual .

figi-ps:CSE figi-gii:hasUniqueTextIdentifier "CSE" .

figi-ps:MMBM a figi-gii:PricingSource .

figi-ps:CSEB a owl:NamedIndividual .

figi-ps:MMBM skos:prefLabel "bank of moscow" .

figi-ps:CSEB a figi-gii:PricingSource .

figi-ps:MMBM figi-gii:hasUniqueTextIdentifier "MMBM" .

figi-ps:CSEB skos:prefLabel "credit suisse ldn" .

figi-ps:MPOI a owl:NamedIndividual .

figi-ps:CSEB figi-gii:hasUniqueTextIdentifier "CSEB" .

figi-ps:MPOI a figi-gii:PricingSource .

figi-ps:CSEC a owl:NamedIndividual .

figi-ps:MPOI skos:prefLabel "bloomberg palm oil" .

figi-ps:CSEC a figi-gii:PricingSource .

figi-ps:MPOI figi-gii:hasUniqueTextIdentifier "MPOI" .

figi-ps:CSEC skos:prefLabel "citic securities hk" .

figi-ps:MPSA a owl:NamedIndividual .

figi-ps:CSEC figi-gii:hasUniqueTextIdentifier "CSEC" .

figi-ps:MPSA a figi-gii:PricingSource .

figi-ps:CSEG a owl:NamedIndividual .

figi-ps:MPSA skos:prefLabel "mps capital services" .

figi-ps:CSEG a figi-gii:PricingSource .

figi-ps:MPSA figi-gii:hasUniqueTextIdentifier "MPSA" .

figi-ps:CSEG skos:prefLabel "cs london" .

figi-ps:MQAU a owl:NamedIndividual .

figi-ps:CSEG figi-gii:hasUniqueTextIdentifier "CSEG" .

figi-ps:MQAU a figi-gii:PricingSource .

figi-ps:CSEM a owl:NamedIndividual .

figi-ps:MQAU skos:prefLabel "macquarie bank" .

figi-ps:CSEM a figi-gii:PricingSource .

figi-ps:MQAU figi-gii:hasUniqueTextIdentifier "MQAU" .

figi-ps:CSEM skos:prefLabel "credit suisse em" .

figi-ps:MSDQ a owl:NamedIndividual .

figi-ps:CSEM figi-gii:hasUniqueTextIdentifier "CSEM" .

figi-ps:MSDQ a figi-gii:PricingSource .

figi-ps:CSER a owl:NamedIndividual .

figi-ps:MSDQ skos:prefLabel "f-i inventory" .

figi-ps:CSER a figi-gii:PricingSource .

figi-ps:MSDQ figi-gii:hasUniqueTextIdentifier "MSDQ" .

figi-ps:CSER skos:prefLabel "countryserv" .

figi-ps:MSFI a owl:NamedIndividual .

figi-ps:CSER figi-gii:hasUniqueTextIdentifier "CSER" .

figi-ps:MSFI a figi-gii:PricingSource .

figi-ps:CSET a owl:NamedIndividual .

figi-ps:MSFI skos:prefLabel "morgan stanley ldn" .

figi-ps:CSET a figi-gii:PricingSource .

figi-ps:MSFI figi-gii:hasUniqueTextIdentifier "MSFI" .

figi-ps:CSET skos:prefLabel "credit suisse em" .

figi-ps:MSG1 a owl:NamedIndividual .

figi-ps:CSET figi-gii:hasUniqueTextIdentifier "CSET" .

figi-ps:MSG1 a figi-gii:PricingSource .

figi-ps:CSEZ a owl:NamedIndividual .

figi-ps:MSG1 skos:prefLabel "msg quotes" .

figi-ps:CSEZ a figi-gii:PricingSource .

figi-ps:MSG1 figi-gii:hasUniqueTextIdentifier "MSG1" .

figi-ps:CSEZ skos:prefLabel "cs zurich credit" .

figi-ps:MSGH a owl:NamedIndividual .

figi-ps:CSEZ figi-gii:hasUniqueTextIdentifier "CSEZ" .

figi-ps:MSGH a figi-gii:PricingSource .

figi-ps:CSFB a owl:NamedIndividual .

figi-ps:MSGH skos:prefLabel "morgan stanley mufj" .

figi-ps:CSFB a figi-gii:PricingSource .

figi-ps:MSGH figi-gii:hasUniqueTextIdentifier "MSGH" .

figi-ps:CSFB skos:prefLabel "credit suisse ny" .

figi-ps:MSGQ a owl:NamedIndividual .

figi-ps:CSFB figi-gii:hasUniqueTextIdentifier "CSFB" .

figi-ps:MSGQ a figi-gii:PricingSource .

figi-ps:CSFC a owl:NamedIndividual .

figi-ps:MSGQ skos:prefLabel "msg scraping qa" .

figi-ps:CSFC a figi-gii:PricingSource .

figi-ps:MSGQ figi-gii:hasUniqueTextIdentifier "MSGQ" .

figi-ps:CSFC skos:prefLabel "chang sheng" .

figi-ps:MSIG a owl:NamedIndividual .

figi-ps:CSFC figi-gii:hasUniqueTextIdentifier "CSFC" .

figi-ps:MSIG a figi-gii:PricingSource .

figi-ps:CSFI a owl:NamedIndividual .

figi-ps:MSIG skos:prefLabel "morgan stanley" .

figi-ps:CSFI a figi-gii:PricingSource .

figi-ps:MSIG figi-gii:hasUniqueTextIdentifier "MSIG" .

figi-ps:CSFI skos:prefLabel "credit suisse govts" .

figi-ps:MSPX a owl:NamedIndividual .

figi-ps:CSFI figi-gii:hasUniqueTextIdentifier "CSFI" .

figi-ps:MSPX a figi-gii:PricingSource .

figi-ps:CSFJ a owl:NamedIndividual .

figi-ps:MSPX skos:prefLabel "morgan stanley" .

figi-ps:CSFJ a figi-gii:PricingSource .

figi-ps:MSPX figi-gii:hasUniqueTextIdentifier "MSPX" .

figi-ps:CSFJ skos:prefLabel "csfb, japan" .

figi-ps:MSRB a owl:NamedIndividual .

figi-ps:CSFJ figi-gii:hasUniqueTextIdentifier "CSFJ" .

figi-ps:MSRB a figi-gii:PricingSource .

figi-ps:CSFM a owl:NamedIndividual .

figi-ps:MSRB skos:prefLabel "muni sec rulemaking" .

figi-ps:CSFM a figi-gii:PricingSource .

figi-ps:MSRB figi-gii:hasUniqueTextIdentifier "MSRB" .

figi-ps:CSFM skos:prefLabel "china southern fund" .

figi-ps:MSTA a owl:NamedIndividual .

figi-ps:CSFM figi-gii:hasUniqueTextIdentifier "CSFM" .

figi-ps:MSTA a figi-gii:PricingSource .

figi-ps:CSGC a owl:NamedIndividual .

figi-ps:MSTA skos:prefLabel "morningstar inc" .

figi-ps:CSGC a figi-gii:PricingSource .

figi-ps:MSTA figi-gii:hasUniqueTextIdentifier "MSTA" .

figi-ps:CSGC skos:prefLabel "credit suisse-ny" .

figi-ps:MSTB a owl:NamedIndividual .

figi-ps:CSGC figi-gii:hasUniqueTextIdentifier "CSGC" .

figi-ps:MSTB a figi-gii:PricingSource .

figi-ps:CSGD a owl:NamedIndividual .

figi-ps:MSTB skos:prefLabel "morgan stanley max" .

figi-ps:CSGD a figi-gii:PricingSource .

figi-ps:MSTB figi-gii:hasUniqueTextIdentifier "MSTB" .

figi-ps:CSGD skos:prefLabel "credit suisse sg" .

figi-ps:MSXP a owl:NamedIndividual .

figi-ps:CSGD figi-gii:hasUniqueTextIdentifier "CSGD" .

figi-ps:MSXP a figi-gii:PricingSource .

figi-ps:CSGN a owl:NamedIndividual .

figi-ps:MSXP skos:prefLabel "morgan stanley" .

figi-ps:CSGN a figi-gii:PricingSource .

figi-ps:MSXP figi-gii:hasUniqueTextIdentifier "MSXP" .

figi-ps:CSGN skos:prefLabel "credit suisse 144a" .

figi-ps:MTJK a owl:NamedIndividual .

figi-ps:CSGN figi-gii:hasUniqueTextIdentifier "CSGN" .

figi-ps:MTJK a figi-gii:PricingSource .

figi-ps:CSHK a owl:NamedIndividual .

figi-ps:MTJK skos:prefLabel "emco transforex" .

figi-ps:CSHK a figi-gii:PricingSource .

figi-ps:MTJK figi-gii:hasUniqueTextIdentifier "MTJK" .

figi-ps:CSHK skos:prefLabel "credit suisse hk" .

figi-ps:MTRF a owl:NamedIndividual .

figi-ps:CSHK figi-gii:hasUniqueTextIdentifier "CSHK" .

figi-ps:MTRF a figi-gii:PricingSource .

figi-ps:CSHL a owl:NamedIndividual .

figi-ps:MTRF skos:prefLabel "ifc metropol" .

figi-ps:CSHL a figi-gii:PricingSource .

figi-ps:MTRF figi-gii:hasUniqueTextIdentifier "MTRF" .

figi-ps:CSHL skos:prefLabel "credit suisse asia" .

figi-ps:MTS a owl:NamedIndividual .

figi-ps:CSHL figi-gii:hasUniqueTextIdentifier "CSHL" .

figi-ps:MTS a figi-gii:PricingSource .

figi-ps:CSI a owl:NamedIndividual .

figi-ps:MTS skos:prefLabel "mts spa" .

figi-ps:CSI a figi-gii:PricingSource .

figi-ps:MTS figi-gii:hasUniqueTextIdentifier "MTS" .

figi-ps:CSI skos:prefLabel "jp morgan" .

figi-ps:MTSA a owl:NamedIndividual .

figi-ps:CSI figi-gii:hasUniqueTextIdentifier "CSI" .

figi-ps:MTSA a figi-gii:PricingSource .

figi-ps:CSIL a owl:NamedIndividual .

figi-ps:MTSA skos:prefLabel "austria mts" .

figi-ps:CSIL a figi-gii:PricingSource .

figi-ps:MTSA figi-gii:hasUniqueTextIdentifier "MTSA" .

figi-ps:CSIL skos:prefLabel "citic securities hk" .

figi-ps:MXBA a owl:NamedIndividual .

figi-ps:CSIL figi-gii:hasUniqueTextIdentifier "CSIL" .

figi-ps:MXBA a figi-gii:PricingSource .

figi-ps:CSIM a owl:NamedIndividual .

figi-ps:MXBA skos:prefLabel "bank of america mx" .

figi-ps:CSIM a figi-gii:PricingSource .

figi-ps:MXBA figi-gii:hasUniqueTextIdentifier "MXBA" .

figi-ps:CSIM skos:prefLabel "centrosim" .

figi-ps:MZHC a owl:NamedIndividual .

figi-ps:CSIM figi-gii:hasUniqueTextIdentifier "CSIM" .

figi-ps:MZHC a figi-gii:PricingSource .

figi-ps:CSIT a owl:NamedIndividual .

figi-ps:MZHC skos:prefLabel "mizuho secs cdos" .

figi-ps:CSIT a figi-gii:PricingSource .

figi-ps:MZHC figi-gii:hasUniqueTextIdentifier "MZHC" .

figi-ps:CSIT skos:prefLabel "china securites inv" .

figi-ps:MZPT a owl:NamedIndividual .

figi-ps:CSIT figi-gii:hasUniqueTextIdentifier "CSIT" .

figi-ps:MZPT a figi-gii:PricingSource .

figi-ps:CSJC a owl:NamedIndividual .

figi-ps:MZPT skos:prefLabel "mizuho tba pricing" .

figi-ps:CSJC a figi-gii:PricingSource .

figi-ps:MZPT figi-gii:hasUniqueTextIdentifier "MZPT" .

figi-ps:CSJC skos:prefLabel "cs japan" .

figi-ps:MZSR a owl:NamedIndividual .

figi-ps:CSJC figi-gii:hasUniqueTextIdentifier "CSJC" .

figi-ps:MZSR a figi-gii:PricingSource .

figi-ps:CSJD a owl:NamedIndividual .

figi-ps:MZSR skos:prefLabel "mizuho sec" .

figi-ps:CSJD a figi-gii:PricingSource .

figi-ps:MZSR figi-gii:hasUniqueTextIdentifier "MZSR" .

figi-ps:CSJD skos:prefLabel "cs, japan eqd" .

figi-ps:MZYF a owl:NamedIndividual .

figi-ps:CSJD figi-gii:hasUniqueTextIdentifier "CSJD" .

figi-ps:MZYF a figi-gii:PricingSource .

figi-ps:CSL a owl:NamedIndividual .

figi-ps:MZYF skos:prefLabel "mizuho sec yen bonds" .

figi-ps:CSL a figi-gii:PricingSource .

figi-ps:MZYF figi-gii:hasUniqueTextIdentifier "MZYF" .

figi-ps:CSL skos:prefLabel "collins stewart" .

figi-ps:NABS a owl:NamedIndividual .

figi-ps:CSL figi-gii:hasUniqueTextIdentifier "CSL" .

figi-ps:NABS a figi-gii:PricingSource .

figi-ps:CSLB a owl:NamedIndividual .

figi-ps:NABS skos:prefLabel "natl bk australia" .

figi-ps:CSLB a figi-gii:PricingSource .

figi-ps:NABS figi-gii:hasUniqueTextIdentifier "NABS" .

figi-ps:CSLB skos:prefLabel "crdsuisse latam bnds" .

figi-ps:NBDD a owl:NamedIndividual .

figi-ps:CSLB figi-gii:hasUniqueTextIdentifier "CSLB" .

figi-ps:NBDD a figi-gii:PricingSource .

figi-ps:CSLC a owl:NamedIndividual .

figi-ps:NBDD skos:prefLabel "emirates nbd" .

figi-ps:CSLC a figi-gii:PricingSource .

figi-ps:NBDD figi-gii:hasUniqueTextIdentifier "NBDD" .

figi-ps:CSLC skos:prefLabel "credit suisse fb llc" .

figi-ps:NBKZ a owl:NamedIndividual .

figi-ps:CSLC figi-gii:hasUniqueTextIdentifier "CSLC" .

figi-ps:NBKZ a figi-gii:PricingSource .

figi-ps:CSLI a owl:NamedIndividual .

figi-ps:NBKZ skos:prefLabel "kaz natbank fixing" .

figi-ps:CSLI a figi-gii:PricingSource .

figi-ps:NBKZ figi-gii:hasUniqueTextIdentifier "NBKZ" .

figi-ps:CSLI skos:prefLabel "crdt suisse fi indx" .

figi-ps:NBPC a owl:NamedIndividual .

figi-ps:CSLI figi-gii:hasUniqueTextIdentifier "CSLI" .

figi-ps:NBPC a figi-gii:PricingSource .

figi-ps:CSLL a owl:NamedIndividual .

figi-ps:NBPC skos:prefLabel "nomura bpi cleanprx" .

figi-ps:CSLL a figi-gii:PricingSource .

figi-ps:NBPC figi-gii:hasUniqueTextIdentifier "NBPC" .

figi-ps:CSLL skos:prefLabel "cs loans desk" .

figi-ps:NBSA a owl:NamedIndividual .

figi-ps:CSLL figi-gii:hasUniqueTextIdentifier "CSLL" .

figi-ps:NBSA a figi-gii:PricingSource .

figi-ps:CSLM a owl:NamedIndividual .

figi-ps:NBSA skos:prefLabel "national bk serbia" .

figi-ps:CSLM a figi-gii:PricingSource .

figi-ps:NBSA figi-gii:hasUniqueTextIdentifier "NBSA" .

figi-ps:CSLM skos:prefLabel "credit suisse metals" .

figi-ps:NBSI a owl:NamedIndividual .

figi-ps:CSLM figi-gii:hasUniqueTextIdentifier "CSLM" .

figi-ps:NBSI a figi-gii:PricingSource .

figi-ps:CSLN a owl:NamedIndividual .

figi-ps:NBSI skos:prefLabel "bmo capital markets" .

figi-ps:CSLN a figi-gii:PricingSource .

figi-ps:NBSI figi-gii:hasUniqueTextIdentifier "NBSI" .

figi-ps:CSLN skos:prefLabel "cs first boston eur" .

figi-ps:NCAP a owl:NamedIndividual .

figi-ps:CSLN figi-gii:hasUniqueTextIdentifier "CSLN" .

figi-ps:NCAP a figi-gii:PricingSource .

figi-ps:CSLP a owl:NamedIndividual .

figi-ps:NCAP skos:prefLabel "isis am" .

figi-ps:CSLP a figi-gii:PricingSource .

figi-ps:NCAP figi-gii:hasUniqueTextIdentifier "NCAP" .

figi-ps:CSLP skos:prefLabel "coastal securities" .

figi-ps:NCCB a owl:NamedIndividual .

figi-ps:CSLP figi-gii:hasUniqueTextIdentifier "CSLP" .

figi-ps:NCCB a figi-gii:PricingSource .

figi-ps:CSLZ a owl:NamedIndividual .

figi-ps:NCCB skos:prefLabel "cfet bank of nanjing" .

figi-ps:CSLZ a figi-gii:PricingSource .

figi-ps:NCCB figi-gii:hasUniqueTextIdentifier "NCCB" .

figi-ps:CSLZ skos:prefLabel "cs eurobonds london" .

figi-ps:NCCN a owl:NamedIndividual .

figi-ps:CSLZ figi-gii:hasUniqueTextIdentifier "CSLZ" .

figi-ps:NCCN a figi-gii:PricingSource .

figi-ps:CSMI a owl:NamedIndividual .

figi-ps:NCCN skos:prefLabel "cnbond nanjing bank" .

figi-ps:CSMI a figi-gii:PricingSource .

figi-ps:NCCN figi-gii:hasUniqueTextIdentifier "NCCN" .

figi-ps:CSMI skos:prefLabel "credit suisse mtge's" .

figi-ps:NCG a owl:NamedIndividual .

figi-ps:CSMI figi-gii:hasUniqueTextIdentifier "CSMI" .

figi-ps:NCG a figi-gii:PricingSource .

figi-ps:CSMS a owl:NamedIndividual .

figi-ps:NCG skos:prefLabel "caixanova" .

figi-ps:CSMS a figi-gii:PricingSource .

figi-ps:NCG figi-gii:hasUniqueTextIdentifier "NCG" .

figi-ps:CSMS skos:prefLabel "credit suisse" .

figi-ps:NCLO a owl:NamedIndividual .

figi-ps:CSMS skos:prefLabel "credit suisse mtge" .

figi-ps:NCLO a figi-gii:PricingSource .

figi-ps:CSMS figi-gii:hasUniqueTextIdentifier "CSMS" .

figi-ps:NCLO skos:prefLabel "nikko citigroup jp" .

figi-ps:CSMX a owl:NamedIndividual .

figi-ps:NCLO figi-gii:hasUniqueTextIdentifier "NCLO" .

figi-ps:CSMX a figi-gii:PricingSource .

figi-ps:NCSI a owl:NamedIndividual .

figi-ps:CSMX skos:prefLabel "credit suisse mex" .

figi-ps:NCSI a figi-gii:PricingSource .

figi-ps:CSMX figi-gii:hasUniqueTextIdentifier "CSMX" .

figi-ps:NCSI skos:prefLabel "nikko cordial sec" .

figi-ps:CSNO a owl:NamedIndividual .

figi-ps:NCSI figi-gii:hasUniqueTextIdentifier "NCSI" .

figi-ps:CSNO a figi-gii:PricingSource .

figi-ps:NCZT a owl:NamedIndividual .

figi-ps:CSNO skos:prefLabel "chinabond val shse n" .

figi-ps:NCZT a figi-gii:PricingSource .

figi-ps:CSNO figi-gii:hasUniqueTextIdentifier "CSNO" .

figi-ps:NCZT skos:prefLabel "citigroup jp" .

figi-ps:CSOB a owl:NamedIndividual .

figi-ps:NCZT figi-gii:hasUniqueTextIdentifier "NCZT" .

figi-ps:CSOB a figi-gii:PricingSource .

figi-ps:NDSO a owl:NamedIndividual .

figi-ps:CSOB skos:prefLabel "csob prague" .

figi-ps:NDSO a figi-gii:PricingSource ;
	skos:prefLabel "india rbi odd lot" .

figi-ps:CSOB figi-gii:hasUniqueTextIdentifier "CSOB" .

figi-ps:NDSO figi-gii:hasUniqueTextIdentifier "NDSO" .

figi-ps:CSOF a owl:NamedIndividual .

figi-ps:NDSW a owl:NamedIndividual .

figi-ps:CSOF a figi-gii:PricingSource .

figi-ps:NDSW a figi-gii:PricingSource .

figi-ps:CSOF skos:prefLabel "credit suisse sp" .

figi-ps:NDSW skos:prefLabel "india rbi whis" .

figi-ps:CSOF figi-gii:hasUniqueTextIdentifier "CSOF" .

figi-ps:NDSW figi-gii:hasUniqueTextIdentifier "NDSW" .

figi-ps:CSOG a owl:NamedIndividual .

figi-ps:NECL a owl:NamedIndividual .

figi-ps:CSOG a figi-gii:PricingSource .

figi-ps:NECL a figi-gii:PricingSource .

figi-ps:CSOG skos:prefLabel "credit suisse sp2" .

figi-ps:NECL skos:prefLabel "nedbank capital" .

figi-ps:CSOG figi-gii:hasUniqueTextIdentifier "CSOG" .

figi-ps:NECL figi-gii:hasUniqueTextIdentifier "NECL" .

figi-ps:CSOP a owl:NamedIndividual .

figi-ps:NEWB a owl:NamedIndividual .

figi-ps:CSOP a figi-gii:PricingSource .

figi-ps:NEWB a figi-gii:PricingSource .

figi-ps:CSOP skos:prefLabel "chinabond val shse o" .

figi-ps:NEWB skos:prefLabel "newbridge securites" .

figi-ps:CSOP figi-gii:hasUniqueTextIdentifier "CSOP" .

figi-ps:NEWB figi-gii:hasUniqueTextIdentifier "NEWB" .

figi-ps:CSOS a owl:NamedIndividual .

figi-ps:NFBK a owl:NamedIndividual .

figi-ps:CSOS a figi-gii:PricingSource .

figi-ps:NFBK a figi-gii:PricingSource .

figi-ps:CSOS skos:prefLabel "cesko obchodni banka" .

figi-ps:NFBK skos:prefLabel "jsc nfbk capital" .

figi-ps:CSOS figi-gii:hasUniqueTextIdentifier "CSOS" .

figi-ps:NFBK figi-gii:hasUniqueTextIdentifier "NFBK" .

figi-ps:CSPF a owl:NamedIndividual .

figi-ps:NIBB a owl:NamedIndividual .

figi-ps:CSPF a figi-gii:PricingSource .

figi-ps:NIBB a figi-gii:PricingSource .

figi-ps:CSPF skos:prefLabel "credit suisse london" .

figi-ps:NIBB skos:prefLabel "nibc bank nv" .

figi-ps:CSPF figi-gii:hasUniqueTextIdentifier "CSPF" .

figi-ps:NIBB figi-gii:hasUniqueTextIdentifier "NIBB" .

figi-ps:CSPG a owl:NamedIndividual .

figi-ps:NISP a owl:NamedIndividual .

figi-ps:CSPG a figi-gii:PricingSource .

figi-ps:NISP a figi-gii:PricingSource .

figi-ps:CSPG skos:prefLabel "ceska sporitelna" .

figi-ps:NISP skos:prefLabel "bank nisp" .

figi-ps:CSPG figi-gii:hasUniqueTextIdentifier "CSPG" .

figi-ps:NISP figi-gii:hasUniqueTextIdentifier "NISP" .

figi-ps:CSPX a owl:NamedIndividual .

figi-ps:NISX a owl:NamedIndividual .

figi-ps:CSPX a figi-gii:PricingSource .

figi-ps:NISX a figi-gii:PricingSource .

figi-ps:CSPX skos:prefLabel "ceska sporitelna ind" .

figi-ps:NISX skos:prefLabel "bk nisp" .

figi-ps:CSPX figi-gii:hasUniqueTextIdentifier "CSPX" .

figi-ps:NISX figi-gii:hasUniqueTextIdentifier "NISX" .

figi-ps:CSQ a owl:NamedIndividual .

figi-ps:NITE a owl:NamedIndividual .

figi-ps:CSQ a figi-gii:PricingSource .

figi-ps:NITE a figi-gii:PricingSource .

figi-ps:CSQ skos:prefLabel "conseq im" .

figi-ps:NITE skos:prefLabel "knight equity mkts" .

figi-ps:CSQ figi-gii:hasUniqueTextIdentifier "CSQ" .

figi-ps:NITE figi-gii:hasUniqueTextIdentifier "NITE" .

figi-ps:CSRU a owl:NamedIndividual .

figi-ps:NJEF a owl:NamedIndividual .

figi-ps:CSRU a figi-gii:PricingSource .

figi-ps:NJEF a figi-gii:PricingSource .

figi-ps:CSRU skos:prefLabel "credit suisse moscow" .

figi-ps:NJEF skos:prefLabel "jefferies and co." .

figi-ps:CSRU figi-gii:hasUniqueTextIdentifier "CSRU" .

figi-ps:NJEF figi-gii:hasUniqueTextIdentifier "NJEF" .

figi-ps:CSSA a owl:NamedIndividual .

figi-ps:NMGH a owl:NamedIndividual .

figi-ps:CSSA a figi-gii:PricingSource .

figi-ps:NMGH a figi-gii:PricingSource .

figi-ps:CSSA skos:prefLabel "credit suisse sg" .

figi-ps:NMGH skos:prefLabel "nomura securities" .

figi-ps:CSSA figi-gii:hasUniqueTextIdentifier "CSSA" .

figi-ps:NMGH figi-gii:hasUniqueTextIdentifier "NMGH" .

figi-ps:CSSC a owl:NamedIndividual .

figi-ps:NORM a owl:NamedIndividual .

figi-ps:CSSC a figi-gii:PricingSource .

figi-ps:NORM a figi-gii:PricingSource .

figi-ps:CSSC skos:prefLabel "credit suisse" .

figi-ps:NORM skos:prefLabel "norddeutsche mtge" .

figi-ps:CSSC figi-gii:hasUniqueTextIdentifier "CSSC" .

figi-ps:NORM figi-gii:hasUniqueTextIdentifier "NORM" .

figi-ps:NOVA a owl:NamedIndividual .

figi-ps:CSSD a owl:NamedIndividual .

figi-ps:NOVA a figi-gii:PricingSource .

figi-ps:CSSD a figi-gii:PricingSource .

figi-ps:NOVA skos:prefLabel "bank of nova scotia" .

figi-ps:CSSD skos:prefLabel "credit suisse - mtge" .

figi-ps:NOVA figi-gii:hasUniqueTextIdentifier "NOVA" .

figi-ps:CSSD figi-gii:hasUniqueTextIdentifier "CSSD" .

figi-ps:NOYS a owl:NamedIndividual .

figi-ps:CSSL a owl:NamedIndividual .

figi-ps:NOYS a figi-gii:PricingSource .

figi-ps:CSSL a figi-gii:PricingSource .

figi-ps:NOYS skos:prefLabel "david a. noyes co." .

figi-ps:CSSL skos:prefLabel "credit suisse sec ln" .

figi-ps:NOYS figi-gii:hasUniqueTextIdentifier "NOYS" .

figi-ps:CSSL figi-gii:hasUniqueTextIdentifier "CSSL" .

figi-ps:NPRI a owl:NamedIndividual .

figi-ps:CSSN a owl:NamedIndividual .

figi-ps:NPRI a figi-gii:PricingSource .

figi-ps:CSSN a figi-gii:PricingSource .

figi-ps:NPRI skos:prefLabel "nice pricing - price" .

figi-ps:CSSN skos:prefLabel "credit suisse - cssn" .

figi-ps:NPRI figi-gii:hasUniqueTextIdentifier "NPRI" .

figi-ps:CSSN figi-gii:hasUniqueTextIdentifier "CSSN" .

figi-ps:NPSB a owl:NamedIndividual .

figi-ps:CSSP a owl:NamedIndividual , figi-gii:PricingSource .

figi-ps:NPSB a figi-gii:PricingSource .

figi-ps:CSSP skos:prefLabel "credit suisse" .

figi-ps:NPSB skos:prefLabel "nice pricing service" .

figi-ps:CSSP figi-gii:hasUniqueTextIdentifier "CSSP" .

figi-ps:NPSB figi-gii:hasUniqueTextIdentifier "NPSB" .

figi-ps:CSSS a owl:NamedIndividual .

figi-ps:NSHL a owl:NamedIndividual .

figi-ps:CSSS a figi-gii:PricingSource .

figi-ps:NSHL a figi-gii:PricingSource .

figi-ps:CSSS skos:prefLabel "credit suisse - csss" .

figi-ps:NSHL skos:prefLabel "citgroup japan" .

figi-ps:CSSS figi-gii:hasUniqueTextIdentifier "CSSS" .

figi-ps:NSHL skos:prefLabel "citigroup japan" .

figi-ps:CSST a owl:NamedIndividual .

figi-ps:NSHL figi-gii:hasUniqueTextIdentifier "NSHL" .

figi-ps:CSST a figi-gii:PricingSource .

figi-ps:NSPR a owl:NamedIndividual .

figi-ps:CSST skos:prefLabel "credit suisse sgp" .

figi-ps:NSPR a figi-gii:PricingSource .

figi-ps:CSST figi-gii:hasUniqueTextIdentifier "CSST" .

figi-ps:NSPR skos:prefLabel "insparo asset mang" .

figi-ps:CSTB a owl:NamedIndividual .

figi-ps:NSPR figi-gii:hasUniqueTextIdentifier "NSPR" .

figi-ps:CSTB a figi-gii:PricingSource .

figi-ps:NSYF a owl:NamedIndividual .

figi-ps:CSTB skos:prefLabel "credit suisse - ny" .

figi-ps:NSYF a figi-gii:PricingSource .

figi-ps:CSTB figi-gii:hasUniqueTextIdentifier "CSTB" .

figi-ps:NSYF skos:prefLabel "nikko citi yen bonds" .

figi-ps:CSTI a owl:NamedIndividual .

figi-ps:NSYF figi-gii:hasUniqueTextIdentifier "NSYF" .

figi-ps:CSTI a figi-gii:PricingSource .

figi-ps:NVCS a owl:NamedIndividual .

figi-ps:CSTI skos:prefLabel "canaccord genuity" .

figi-ps:NVCS a figi-gii:PricingSource .

figi-ps:CSTI figi-gii:hasUniqueTextIdentifier "CSTI" .

figi-ps:NVCS skos:prefLabel "bnk of nova scotia" .

figi-ps:CSTL a owl:NamedIndividual .

figi-ps:NVCS figi-gii:hasUniqueTextIdentifier "NVCS" .

figi-ps:CSTL a figi-gii:PricingSource .

figi-ps:NXAB a owl:NamedIndividual .

figi-ps:CSTL skos:prefLabel "citibank secs taiwan" .

figi-ps:NXAB a figi-gii:PricingSource .

figi-ps:CSTL figi-gii:hasUniqueTextIdentifier "CSTL" .

figi-ps:NXAB skos:prefLabel "natixis abs mbs" .

figi-ps:CSTR a owl:NamedIndividual .

figi-ps:NXAB figi-gii:hasUniqueTextIdentifier "NXAB" .

figi-ps:CSTR a figi-gii:PricingSource .

figi-ps:NXIC a owl:NamedIndividual .

figi-ps:CSTR skos:prefLabel "calstrs" .

figi-ps:NXIC a figi-gii:PricingSource .

figi-ps:CSTR figi-gii:hasUniqueTextIdentifier "CSTR" .

figi-ps:NXIC skos:prefLabel "natixis" .

figi-ps:CSTT a owl:NamedIndividual .

figi-ps:NXIC figi-gii:hasUniqueTextIdentifier "NXIC" .

figi-ps:CSTT a figi-gii:PricingSource .

figi-ps:NZNG a owl:NamedIndividual .

figi-ps:CSTT skos:prefLabel "christopher street" .

figi-ps:NZNG a figi-gii:PricingSource .

figi-ps:CSTT skos:prefLabel "cs tier testing" .

figi-ps:NZNG skos:prefLabel "nzfm bond fixings" .

figi-ps:CSTT figi-gii:hasUniqueTextIdentifier "CSTT" .

figi-ps:NZNG figi-gii:hasUniqueTextIdentifier "NZNG" .

figi-ps:CSUC a owl:NamedIndividual .

figi-ps:NZSA a owl:NamedIndividual .

figi-ps:CSUC a figi-gii:PricingSource .

figi-ps:NZSA a figi-gii:PricingSource .

figi-ps:CSUC skos:prefLabel "credsu - carnegie" .

figi-ps:NZSA skos:prefLabel "abn nzswapclose" .

figi-ps:CSUC figi-gii:hasUniqueTextIdentifier "CSUC" .

figi-ps:NZSA figi-gii:hasUniqueTextIdentifier "NZSA" .

figi-ps:CSUK a owl:NamedIndividual .

figi-ps:NZSB a owl:NamedIndividual .

figi-ps:CSUK a figi-gii:PricingSource .

figi-ps:NZSB a figi-gii:PricingSource .

figi-ps:CSUK skos:prefLabel "credit suisse d1" .

figi-ps:NZSB skos:prefLabel "anz nzswapclose" .

figi-ps:CSUK skos:prefLabel "credit suisse ldn" .

figi-ps:NZSB figi-gii:hasUniqueTextIdentifier "NZSB" .

figi-ps:CSUK figi-gii:hasUniqueTextIdentifier "CSUK" .

figi-ps:NZSC a owl:NamedIndividual .

figi-ps:CSUX a owl:NamedIndividual .

figi-ps:NZSC a figi-gii:PricingSource .

figi-ps:CSUX a figi-gii:PricingSource .

figi-ps:NZSC skos:prefLabel "asb nzswapclose" .

figi-ps:CSUX skos:prefLabel "credit suisse ldn" .

figi-ps:NZSC figi-gii:hasUniqueTextIdentifier "NZSC" .

figi-ps:CSUX figi-gii:hasUniqueTextIdentifier "CSUX" .

figi-ps:NZSD a owl:NamedIndividual .

figi-ps:CSZB a owl:NamedIndividual .

figi-ps:NZSD a figi-gii:PricingSource .

figi-ps:CSZB a figi-gii:PricingSource .

figi-ps:NZSD skos:prefLabel "bnp nzswapclose" .

figi-ps:CSZB skos:prefLabel "cs zurich high grade" .

figi-ps:NZSD figi-gii:hasUniqueTextIdentifier "NZSD" .

figi-ps:CSZB figi-gii:hasUniqueTextIdentifier "CSZB" .

figi-ps:NZSF a owl:NamedIndividual .

figi-ps:CSZC a owl:NamedIndividual .

figi-ps:NZSF a figi-gii:PricingSource .

figi-ps:CSZC a figi-gii:PricingSource .

figi-ps:NZSF skos:prefLabel "cba nzswapclose" .

figi-ps:CSZC skos:prefLabel "credit suisse zurich" .

figi-ps:NZSF figi-gii:hasUniqueTextIdentifier "NZSF" .

figi-ps:CSZC figi-gii:hasUniqueTextIdentifier "CSZC" .

figi-ps:NZSG a owl:NamedIndividual .

figi-ps:CSZE a owl:NamedIndividual .

figi-ps:NZSG a figi-gii:PricingSource .

figi-ps:CSZE a figi-gii:PricingSource .

figi-ps:NZSG skos:prefLabel "citi nzswapclose" .

figi-ps:CSZE skos:prefLabel "cs zurich" .

figi-ps:NZSG figi-gii:hasUniqueTextIdentifier "NZSG" .

figi-ps:CSZE figi-gii:hasUniqueTextIdentifier "CSZE" .

figi-ps:NZSH a owl:NamedIndividual .

figi-ps:CSZH a owl:NamedIndividual .

figi-ps:NZSH a figi-gii:PricingSource .

figi-ps:CSZH a figi-gii:PricingSource .

figi-ps:NZSH skos:prefLabel "cs nzswapclose" .

figi-ps:CSZH skos:prefLabel "credit suisse swiss" .

figi-ps:NZSH figi-gii:hasUniqueTextIdentifier "NZSH" .

figi-ps:CSZH figi-gii:hasUniqueTextIdentifier "CSZH" .

figi-ps:NZSI a owl:NamedIndividual .

figi-ps:CSZZ a owl:NamedIndividual , figi-gii:PricingSource .

figi-ps:NZSI a figi-gii:PricingSource .

figi-ps:CSZZ skos:prefLabel "cs zurich em" .

figi-ps:NZSI skos:prefLabel "db nzswapclose" .

figi-ps:CSZZ figi-gii:hasUniqueTextIdentifier "CSZZ" .

figi-ps:NZSI figi-gii:hasUniqueTextIdentifier "NZSI" .

figi-ps:CTAP a owl:NamedIndividual , figi-gii:PricingSource .

figi-ps:NZSJ a owl:NamedIndividual , figi-gii:PricingSource .

figi-ps:CTAP skos:prefLabel "citibank asia" .

figi-ps:NZSJ skos:prefLabel "hsbc nzswapclose" .

figi-ps:CTAP figi-gii:hasUniqueTextIdentifier "CTAP" .

figi-ps:NZSJ figi-gii:hasUniqueTextIdentifier "NZSJ" .

figi-ps:CTBA a owl:NamedIndividual .

figi-ps:NZSK a owl:NamedIndividual .

figi-ps:CTBA a figi-gii:PricingSource .

figi-ps:NZSK a figi-gii:PricingSource .

figi-ps:CTBA skos:prefLabel "citigroup" .

figi-ps:NZSK skos:prefLabel "jp swapclose" .

figi-ps:CTBA figi-gii:hasUniqueTextIdentifier "CTBA" .

figi-ps:NZSK skos:prefLabel "sg nzswapclose" .

figi-ps:CTBD a owl:NamedIndividual .

figi-ps:NZSK figi-gii:hasUniqueTextIdentifier "NZSK" .

figi-ps:CTBD a figi-gii:PricingSource ;
	skos:prefLabel "citic securities" .

figi-ps:NZSN a owl:NamedIndividual .

figi-ps:CTBD figi-gii:hasUniqueTextIdentifier "CTBD" .

figi-ps:CTBK a owl:NamedIndividual .

figi-ps:NZSN a figi-gii:PricingSource .

figi-ps:CTBK a figi-gii:PricingSource .

figi-ps:NZSN skos:prefLabel "bnz nzswapclose" .

figi-ps:CTBK skos:prefLabel "citic bank" .

figi-ps:NZSN figi-gii:hasUniqueTextIdentifier "NZSN" .

figi-ps:CTBK figi-gii:hasUniqueTextIdentifier "CTBK" .

figi-ps:NZSW a owl:NamedIndividual .

figi-ps:CTBO a owl:NamedIndividual .

figi-ps:NZSW a figi-gii:PricingSource .

figi-ps:CTBO a figi-gii:PricingSource .

figi-ps:NZSW skos:prefLabel "avg nzswapclose" .

figi-ps:CTBO skos:prefLabel "citibank colombia" .

figi-ps:NZSW figi-gii:hasUniqueTextIdentifier "NZSW" .

figi-ps:CTBO figi-gii:hasUniqueTextIdentifier "CTBO" .

figi-ps:OBGN a owl:NamedIndividual .

figi-ps:CTBR a owl:NamedIndividual .

figi-ps:OBGN a figi-gii:PricingSource .

figi-ps:CTBR a figi-gii:PricingSource .

figi-ps:OBGN skos:prefLabel "internal bb generic" .

figi-ps:CTBR skos:prefLabel "banco citibank" .

figi-ps:OBGN figi-gii:hasUniqueTextIdentifier "OBGN" .

figi-ps:CTBR figi-gii:hasUniqueTextIdentifier "CTBR" .

figi-ps:OBNK a owl:NamedIndividual .

figi-ps:CTBT a owl:NamedIndividual .

figi-ps:OBNK a figi-gii:PricingSource .

figi-ps:CTBT a figi-gii:PricingSource .

figi-ps:OBNK skos:prefLabel "bank fuer oberoester" .

figi-ps:CTBT skos:prefLabel "citibank bangkok" .

figi-ps:OBNK figi-gii:hasUniqueTextIdentifier "OBNK" .

figi-ps:CTBT figi-gii:hasUniqueTextIdentifier "CTBT" .

figi-ps:OCCI a owl:NamedIndividual .

figi-ps:CTC a owl:NamedIndividual .

figi-ps:OCCI a figi-gii:PricingSource .

figi-ps:CTC a figi-gii:PricingSource .

figi-ps:OCCI skos:prefLabel "banco de occidente" .

figi-ps:CTC skos:prefLabel "chinatrust phil" .

figi-ps:OCCI figi-gii:hasUniqueTextIdentifier "OCCI" .

figi-ps:CTC figi-gii:hasUniqueTextIdentifier "CTC" .

figi-ps:ODFI a owl:NamedIndividual .

figi-ps:CTCB a owl:NamedIndividual .

figi-ps:ODFI a figi-gii:PricingSource .

figi-ps:CTCB a figi-gii:PricingSource .

figi-ps:ODFI skos:prefLabel "oddo and cie" .

figi-ps:CTCB skos:prefLabel "chinatrust, taiwan" .

figi-ps:ODFI figi-gii:hasUniqueTextIdentifier "ODFI" .

figi-ps:CTCB figi-gii:hasUniqueTextIdentifier "CTCB" .

figi-ps:CTCH a owl:NamedIndividual .

figi-ps:OECM a owl:NamedIndividual .

figi-ps:CTCH a figi-gii:PricingSource .

figi-ps:OECM a figi-gii:PricingSource .

figi-ps:CTCH skos:prefLabel "cfet citibank china" .

figi-ps:OECM skos:prefLabel "bloomberg otc energy" .

figi-ps:CTCH figi-gii:hasUniqueTextIdentifier "CTCH" .

figi-ps:OECM figi-gii:hasUniqueTextIdentifier "OECM" .

figi-ps:CTCM a owl:NamedIndividual .

figi-ps:OHM a owl:NamedIndividual .

figi-ps:CTCM a figi-gii:PricingSource .

figi-ps:OHM a figi-gii:PricingSource .

figi-ps:CTCM skos:prefLabel "c12 capital manageme" .

figi-ps:OHM skos:prefLabel "e ohman j:or ab" .

figi-ps:CTCM figi-gii:hasUniqueTextIdentifier "CTCM" .

figi-ps:OHM figi-gii:hasUniqueTextIdentifier "OHM" .

figi-ps:CTCN a owl:NamedIndividual .

figi-ps:OPCO a owl:NamedIndividual .

figi-ps:CTCN a figi-gii:PricingSource .

figi-ps:OPCO a figi-gii:PricingSource .

figi-ps:CTCN skos:prefLabel "citibank china" .

figi-ps:OPCO skos:prefLabel "oppenheimer and co" .

figi-ps:CTCN figi-gii:hasUniqueTextIdentifier "CTCN" .

figi-ps:OPCO figi-gii:hasUniqueTextIdentifier "OPCO" .

figi-ps:CTDL a owl:NamedIndividual .

figi-ps:OSBC a owl:NamedIndividual .

figi-ps:CTDL a figi-gii:PricingSource .

figi-ps:OSBC a figi-gii:PricingSource .

figi-ps:CTDL skos:prefLabel "citadel securities" .

figi-ps:OSBC skos:prefLabel "overseas-chinese bnk" .

figi-ps:CTDL figi-gii:hasUniqueTextIdentifier "CTDL" .

figi-ps:OSBC figi-gii:hasUniqueTextIdentifier "OSBC" .

figi-ps:CTER a owl:NamedIndividual .

figi-ps:PABG a owl:NamedIndividual .

figi-ps:CTER a figi-gii:PricingSource .

figi-ps:PABG a figi-gii:PricingSource .

figi-ps:CTER skos:prefLabel "citigroup japan" .

figi-ps:PABG skos:prefLabel "banco general sa" .

figi-ps:CTER figi-gii:hasUniqueTextIdentifier "CTER" .

figi-ps:PABG figi-gii:hasUniqueTextIdentifier "PABG" .

figi-ps:CTFC a owl:NamedIndividual .

figi-ps:PACT a owl:NamedIndividual .

figi-ps:CTFC a figi-gii:PricingSource .

figi-ps:PACT a figi-gii:PricingSource .

figi-ps:CTFC skos:prefLabel "chinatrust (phils)" .

figi-ps:PACT skos:prefLabel "btg" .

figi-ps:CTFC figi-gii:hasUniqueTextIdentifier "CTFC" .

figi-ps:PACT figi-gii:hasUniqueTextIdentifier "PACT" .

figi-ps:CTFI a owl:NamedIndividual .

figi-ps:PARI a owl:NamedIndividual .

figi-ps:CTFI a figi-gii:PricingSource .

figi-ps:PARI a figi-gii:PricingSource .

figi-ps:CTFI skos:prefLabel "cantor fitzgerald" .

figi-ps:PARI skos:prefLabel "bnp paribas" .

figi-ps:CTFI figi-gii:hasUniqueTextIdentifier "CTFI" .

figi-ps:PARI figi-gii:hasUniqueTextIdentifier "PARI" .

figi-ps:CTGM a owl:NamedIndividual .

figi-ps:PARS a owl:NamedIndividual .

figi-ps:CTGM a figi-gii:PricingSource .

figi-ps:PARS a figi-gii:PricingSource .

figi-ps:CTGM skos:prefLabel "citibank guatemala" .

figi-ps:PARS skos:prefLabel "bnp paribas" .

figi-ps:CTGM figi-gii:hasUniqueTextIdentifier "CTGM" .

figi-ps:PARS figi-gii:hasUniqueTextIdentifier "PARS" .

figi-ps:CTIC a owl:NamedIndividual .

figi-ps:PARU a owl:NamedIndividual .

figi-ps:CTIC a figi-gii:PricingSource .

figi-ps:PARU a figi-gii:PricingSource .

figi-ps:CTIC skos:prefLabel "cfet china citic bk" .

figi-ps:PARU skos:prefLabel "bolsa de valores de asuncion (paraguay) usd price" .

figi-ps:CTIC figi-gii:hasUniqueTextIdentifier "CTIC" .

figi-ps:PARU figi-gii:hasUniqueTextIdentifier "PARU" .

figi-ps:CTKN a owl:NamedIndividual .

figi-ps:PATA a owl:NamedIndividual .

figi-ps:CTKN a figi-gii:PricingSource .

figi-ps:PATA a figi-gii:PricingSource .

figi-ps:CTKN skos:prefLabel "citibank kuala lumpu" .

figi-ps:PATA skos:prefLabel "banco patagonia" .

figi-ps:CTKN figi-gii:hasUniqueTextIdentifier "CTKN" .

figi-ps:PATA figi-gii:hasUniqueTextIdentifier "PATA" .

figi-ps:CTKP a owl:NamedIndividual .

figi-ps:PBGM a owl:NamedIndividual .

figi-ps:CTKP a figi-gii:PricingSource .

figi-ps:PBGM a figi-gii:PricingSource .

figi-ps:CTKP skos:prefLabel "citibank peru" .

figi-ps:PBGM skos:prefLabel "piraeus bank abs" .

figi-ps:CTKP figi-gii:hasUniqueTextIdentifier "CTKP" .

figi-ps:PBGM figi-gii:hasUniqueTextIdentifier "PBGM" .

figi-ps:CTNK a owl:NamedIndividual .

figi-ps:PCDB a owl:NamedIndividual .

figi-ps:CTNK a figi-gii:PricingSource .

figi-ps:PCDB a figi-gii:PricingSource .

figi-ps:CTNK skos:prefLabel "citibank na, karachi" .

figi-ps:PCDB skos:prefLabel "banco bilbao vizcaya" .

figi-ps:CTNK figi-gii:hasUniqueTextIdentifier "CTNK" .

figi-ps:PCDB figi-gii:hasUniqueTextIdentifier "PCDB" .

figi-ps:CTNL a owl:NamedIndividual .

figi-ps:PCER a owl:NamedIndividual .

figi-ps:CTNL a figi-gii:PricingSource .

figi-ps:PCER a figi-gii:PricingSource .

figi-ps:CTNL skos:prefLabel "citi nigeria" .

figi-ps:PCER skos:prefLabel "citigroup hong kong" .

figi-ps:CTNL figi-gii:hasUniqueTextIdentifier "CTNL" .

figi-ps:PCER figi-gii:hasUniqueTextIdentifier "PCER" .

figi-ps:CTNN a owl:NamedIndividual .

figi-ps:PCTF a owl:NamedIndividual .

figi-ps:CTNN a figi-gii:PricingSource .

figi-ps:PCTF a figi-gii:PricingSource .

figi-ps:CTNN skos:prefLabel "citibank nigeria ltd" .

figi-ps:PCTF skos:prefLabel "btg pactual autoex" .

figi-ps:CTNN figi-gii:hasUniqueTextIdentifier "CTNN" .

figi-ps:PCTF figi-gii:hasUniqueTextIdentifier "PCTF" .

figi-ps:CTNO a owl:NamedIndividual .

figi-ps:PCTX a owl:NamedIndividual .

figi-ps:CTNO a figi-gii:PricingSource .

figi-ps:PCTX a figi-gii:PricingSource .

figi-ps:CTNO skos:prefLabel "chinabond val otc n" .

figi-ps:PCTX skos:prefLabel "banco ubs pactual" .

figi-ps:CTNO figi-gii:hasUniqueTextIdentifier "CTNO" .

figi-ps:PCTX figi-gii:hasUniqueTextIdentifier "PCTX" .

figi-ps:CTOP a owl:NamedIndividual .

figi-ps:PFS a owl:NamedIndividual .

figi-ps:CTOP a figi-gii:PricingSource .

figi-ps:PFS a figi-gii:PricingSource .

figi-ps:CTOP skos:prefLabel "chinabond val otc o" .

figi-ps:PFS skos:prefLabel "dt postbank fin serv" .

figi-ps:CTOP figi-gii:hasUniqueTextIdentifier "CTOP" .

figi-ps:PFS figi-gii:hasUniqueTextIdentifier "PFS" .

figi-ps:CTPE a owl:NamedIndividual .

figi-ps:PIPJ a owl:NamedIndividual .

figi-ps:CTPE a figi-gii:PricingSource .

figi-ps:PIPJ a figi-gii:PricingSource .

figi-ps:CTPE skos:prefLabel "citibank taiwan" .

figi-ps:PIPJ skos:prefLabel "piper jaffray" .

figi-ps:CTPE figi-gii:hasUniqueTextIdentifier "CTPE" .

figi-ps:PIPJ figi-gii:hasUniqueTextIdentifier "PIPJ" .

figi-ps:CTPR a owl:NamedIndividual .

figi-ps:PIPN a owl:NamedIndividual .

figi-ps:CTPR a figi-gii:PricingSource .

figi-ps:PIPN a figi-gii:PricingSource .

figi-ps:CTPR skos:prefLabel "citibank czech rep" .

figi-ps:PIPN skos:prefLabel "abn priv inv prod" .

figi-ps:CTPR figi-gii:hasUniqueTextIdentifier "CTPR" .

figi-ps:PIPN figi-gii:hasUniqueTextIdentifier "PIPN" .

figi-ps:CTRC a owl:NamedIndividual .

figi-ps:PIPU a owl:NamedIndividual .

figi-ps:CTRC a figi-gii:PricingSource .

figi-ps:PIPU a figi-gii:PricingSource .

figi-ps:CTRC skos:prefLabel "citibank na sgp" .

figi-ps:PIPU skos:prefLabel "bank indonesia" .

figi-ps:CTRC figi-gii:hasUniqueTextIdentifier "CTRC" .

figi-ps:PIPU figi-gii:hasUniqueTextIdentifier "PIPU" .

figi-ps:CTRG a owl:NamedIndividual .

figi-ps:PIVD a owl:NamedIndividual .

figi-ps:CTRG a figi-gii:PricingSource .

figi-ps:PIVD a figi-gii:PricingSource .

figi-ps:CTRG skos:prefLabel "citigroup mortgage" .

figi-ps:PIVD skos:prefLabel "bank pivdennyi" .

figi-ps:CTRG skos:prefLabel "citigroup mortgages" .

figi-ps:PIVD figi-gii:hasUniqueTextIdentifier "PIVD" .

figi-ps:CTRG figi-gii:hasUniqueTextIdentifier "CTRG" .

figi-ps:PKEO a owl:NamedIndividual .

figi-ps:CTSE a owl:NamedIndividual .

figi-ps:PKEO a figi-gii:PricingSource .

figi-ps:CTSE a figi-gii:PricingSource .

figi-ps:PKEO skos:prefLabel "bank pekao internal" .

figi-ps:CTSE skos:prefLabel "citic securities" .

figi-ps:PKEO figi-gii:hasUniqueTextIdentifier "PKEO" .

figi-ps:CTSE figi-gii:hasUniqueTextIdentifier "CTSE" .

figi-ps:PKIB a owl:NamedIndividual .

figi-ps:CTSG a owl:NamedIndividual .

figi-ps:PKIB a figi-gii:PricingSource .

figi-ps:CTSG a figi-gii:PricingSource .

figi-ps:PKIB skos:prefLabel "financial mrkt assoc" ;
	figi-gii:hasUniqueTextIdentifier "PKIB" .

figi-ps:CTSG skos:prefLabel "citibank inv bk (sg)" .

figi-ps:PLKD a owl:NamedIndividual , figi-gii:PricingSource .

figi-ps:CTSG figi-gii:hasUniqueTextIdentifier "CTSG" .

figi-ps:PLKD skos:prefLabel "bank polska" .

figi-ps:CTSH a owl:NamedIndividual .

figi-ps:PLKD figi-gii:hasUniqueTextIdentifier "PLKD" .

figi-ps:CTSH a figi-gii:PricingSource .

figi-ps:PMG a owl:NamedIndividual .

figi-ps:CTSH skos:prefLabel "cfif citibank shangh" .

figi-ps:PMG a figi-gii:PricingSource .

figi-ps:CTSH figi-gii:hasUniqueTextIdentifier "CTSH" .

figi-ps:PMG skos:prefLabel "aetna" .

figi-ps:CTSM a owl:NamedIndividual .

figi-ps:PMG figi-gii:hasUniqueTextIdentifier "PMG" .

figi-ps:CTSM a figi-gii:PricingSource .

figi-ps:PMPL a owl:NamedIndividual .

figi-ps:CTSM skos:prefLabel "centrosim spa" .

figi-ps:PMPL a figi-gii:PricingSource .

figi-ps:CTSM figi-gii:hasUniqueTextIdentifier "CTSM" .

figi-ps:PMPL skos:prefLabel "bim (uk) ltd" .

figi-ps:CTT a owl:NamedIndividual .

figi-ps:PMPL figi-gii:hasUniqueTextIdentifier "PMPL" .

figi-ps:CTT a figi-gii:PricingSource .

figi-ps:PNBP a owl:NamedIndividual .

figi-ps:CTT skos:prefLabel "citigroup treasury" .

figi-ps:PNBP a figi-gii:PricingSource .

figi-ps:CTT figi-gii:hasUniqueTextIdentifier "CTT" .

figi-ps:PNBP skos:prefLabel "bnp paribas poland" .

figi-ps:CTVN a owl:NamedIndividual .

figi-ps:PNBP figi-gii:hasUniqueTextIdentifier "PNBP" .

figi-ps:CTVN a figi-gii:PricingSource .

figi-ps:PNCS a owl:NamedIndividual .

figi-ps:CTVN skos:prefLabel "citibank vietnam" .

figi-ps:PNCS a figi-gii:PricingSource .

figi-ps:CTVN figi-gii:hasUniqueTextIdentifier "CTVN" .

figi-ps:PNCS skos:prefLabel "pnc cap markets" .

figi-ps:CUAD a owl:NamedIndividual .

figi-ps:PNCS figi-gii:hasUniqueTextIdentifier "PNCS" .

figi-ps:CUAD a figi-gii:PricingSource .

figi-ps:POBA a owl:NamedIndividual .

figi-ps:CUAD skos:prefLabel "cuadra y degwitz" .

figi-ps:POBA a figi-gii:PricingSource .

figi-ps:CUAD figi-gii:hasUniqueTextIdentifier "CUAD" .

figi-ps:POBA skos:prefLabel "banca popolare bari" .

figi-ps:CUAM a owl:NamedIndividual .

figi-ps:POBA figi-gii:hasUniqueTextIdentifier "POBA" .

figi-ps:CUAM a figi-gii:PricingSource .

figi-ps:POST a owl:NamedIndividual .

figi-ps:CUAM skos:prefLabel "china universal" .

figi-ps:POST a figi-gii:PricingSource .

figi-ps:CUAM figi-gii:hasUniqueTextIdentifier "CUAM" .

figi-ps:CUGS a owl:NamedIndividual , figi-gii:PricingSource ;
	skos:prefLabel "cuttone and co" ;
	figi-gii:hasUniqueTextIdentifier "CUGS" .

figi-ps:POST skos:prefLabel "bancoposta" .

figi-ps:CURZ a owl:NamedIndividual , figi-gii:PricingSource .

figi-ps:POST figi-gii:hasUniqueTextIdentifier "POST" .

figi-ps:CURZ skos:prefLabel "curzon securities" .

figi-ps:PPFM a owl:NamedIndividual , figi-gii:PricingSource .

figi-ps:CURZ figi-gii:hasUniqueTextIdentifier "CURZ" .

figi-ps:PPFM skos:prefLabel "ppf banka" .

figi-ps:CUST a owl:NamedIndividual .

figi-ps:PPFM figi-gii:hasUniqueTextIdentifier "PPFM" .

figi-ps:CUST a figi-gii:PricingSource .

figi-ps:PRIV a owl:NamedIndividual .

figi-ps:CUST skos:prefLabel "customer testing" .

figi-ps:PRIV a figi-gii:PricingSource .

figi-ps:CUST figi-gii:hasUniqueTextIdentifier "CUST" .

figi-ps:PRIV skos:prefLabel "bdo - private bank" .

figi-ps:CUT a owl:NamedIndividual .

figi-ps:PRIV figi-gii:hasUniqueTextIdentifier "PRIV" .

figi-ps:CUT a figi-gii:PricingSource .

figi-ps:PRMN a owl:NamedIndividual .

figi-ps:CUT skos:prefLabel "cutwater investor" .

figi-ps:PRMN a figi-gii:PricingSource .

figi-ps:CUT figi-gii:hasUniqueTextIdentifier "CUT" .

figi-ps:PRMN skos:prefLabel "banca promos spa" .

figi-ps:CVE a owl:NamedIndividual .

figi-ps:PRMN figi-gii:hasUniqueTextIdentifier "PRMN" .

figi-ps:CVE a figi-gii:PricingSource .

figi-ps:PROM a owl:NamedIndividual .

figi-ps:CVE skos:prefLabel "canadian venture" .

figi-ps:PROM a figi-gii:PricingSource .

figi-ps:CVE figi-gii:hasUniqueTextIdentifier "CVE" .

figi-ps:PROM skos:prefLabel "banca profilo" .

figi-ps:CVMB a owl:NamedIndividual .

figi-ps:PROM figi-gii:hasUniqueTextIdentifier "PROM" .

figi-ps:CVMB a figi-gii:PricingSource .

figi-ps:PROZ a owl:NamedIndividual .

figi-ps:CVMB skos:prefLabel "capiton value mgmt" .

figi-ps:PROZ a figi-gii:PricingSource .

figi-ps:CVMB figi-gii:hasUniqueTextIdentifier "CVMB" .

figi-ps:PROZ skos:prefLabel "banca profilo" .

figi-ps:CWAY a owl:NamedIndividual .

figi-ps:PROZ figi-gii:hasUniqueTextIdentifier "PROZ" .

figi-ps:CWAY a figi-gii:PricingSource .

figi-ps:PRTG a owl:NamedIndividual .

figi-ps:CWAY skos:prefLabel "causeway capital" .

figi-ps:PRTG a figi-gii:PricingSource .

figi-ps:CWAY figi-gii:hasUniqueTextIdentifier "CWAY" .

figi-ps:PRTG skos:prefLabel "proton bank athens" .

figi-ps:CWB a owl:NamedIndividual .

figi-ps:PRTG figi-gii:hasUniqueTextIdentifier "PRTG" .

figi-ps:CWB a figi-gii:PricingSource .

figi-ps:PRUD a owl:NamedIndividual .

figi-ps:CWB skos:prefLabel "internal do not del" .

figi-ps:PRUD a figi-gii:PricingSource .

figi-ps:CWB figi-gii:hasUniqueTextIdentifier "CWB" .

figi-ps:PRUD skos:prefLabel "dresdner bank" .

figi-ps:CWMC a owl:NamedIndividual .

figi-ps:PRUD figi-gii:hasUniqueTextIdentifier "PRUD" .

figi-ps:CWMC a figi-gii:PricingSource .

figi-ps:PRUP a owl:NamedIndividual .

figi-ps:CWMC skos:prefLabel "china wealth mgmt" .

figi-ps:PRUP a figi-gii:PricingSource .

figi-ps:CWMC figi-gii:hasUniqueTextIdentifier "CWMC" .

figi-ps:PRUP skos:prefLabel "commerzbank pp" .

figi-ps:CWTH a owl:NamedIndividual , figi-gii:PricingSource .

figi-ps:PRUP figi-gii:hasUniqueTextIdentifier "PRUP" .

figi-ps:CWTH skos:prefLabel "customweather" .

figi-ps:PSRB a owl:NamedIndividual .

figi-ps:CWTH figi-gii:hasUniqueTextIdentifier "CWTH" .

figi-ps:PSRB a figi-gii:PricingSource .

figi-ps:CXAM a owl:NamedIndividual .

figi-ps:PSRB skos:prefLabel "cfif ch postal savng" .

figi-ps:CXAM a figi-gii:PricingSource .

figi-ps:PSRB figi-gii:hasUniqueTextIdentifier "PSRB" .

figi-ps:CXAM skos:prefLabel "chang xin asset mgmt" .

figi-ps:PSRP a owl:NamedIndividual .

figi-ps:CXAM figi-gii:hasUniqueTextIdentifier "CXAM" .

figi-ps:PSRP a figi-gii:PricingSource .

figi-ps:CXBI a owl:NamedIndividual .

figi-ps:PSRP skos:prefLabel "abn amro struc rates" .

figi-ps:CXBI a figi-gii:PricingSource .

figi-ps:PSRP figi-gii:hasUniqueTextIdentifier "PSRP" .

figi-ps:CXBI skos:prefLabel "caixa banco invest." .

figi-ps:Q11 a owl:NamedIndividual .

figi-ps:CXBI figi-gii:hasUniqueTextIdentifier "CXBI" .

figi-ps:Q11 a figi-gii:PricingSource .

figi-ps:CY14 a owl:NamedIndividual .

figi-ps:Q11 skos:prefLabel "bloomberg b2b #1" .

figi-ps:CY14 a figi-gii:PricingSource .

figi-ps:Q11 figi-gii:hasUniqueTextIdentifier "Q11" .

figi-ps:CY14 skos:prefLabel "cfets 14d bnd fwd yd" .

figi-ps:Q12 a owl:NamedIndividual , figi-gii:PricingSource .

figi-ps:CY14 figi-gii:hasUniqueTextIdentifier "CY14" .

figi-ps:Q12 skos:prefLabel "bloomberg b2b #2" .

figi-ps:CY1M a owl:NamedIndividual .

figi-ps:Q12 figi-gii:hasUniqueTextIdentifier "Q12" .

figi-ps:CY1M a figi-gii:PricingSource .

figi-ps:QAGI a owl:NamedIndividual .

figi-ps:CY1M skos:prefLabel "cfets 1m bnd fwd yld" .

figi-ps:QAGI a figi-gii:PricingSource .

figi-ps:CY1M figi-gii:hasUniqueTextIdentifier "CY1M" .

figi-ps:QAGI skos:prefLabel "agic-parallel" .

figi-ps:CY1Y a owl:NamedIndividual .

figi-ps:QAGI figi-gii:hasUniqueTextIdentifier "QAGI" .

figi-ps:CY1Y a figi-gii:PricingSource .

figi-ps:RAB0 a owl:NamedIndividual .

figi-ps:CY1Y skos:prefLabel "cfets 1y bnd fwd yld" .

figi-ps:RAB0 a figi-gii:PricingSource .

figi-ps:CY1Y figi-gii:hasUniqueTextIdentifier "CY1Y" .

figi-ps:RAB0 skos:prefLabel "rabobank internation" .

figi-ps:CY21 a owl:NamedIndividual .

figi-ps:RAB0 figi-gii:hasUniqueTextIdentifier "RAB0" .

figi-ps:CY21 a figi-gii:PricingSource .

figi-ps:RABO a owl:NamedIndividual .

figi-ps:CY21 skos:prefLabel "cfets 21d bnd fwd yd" .

figi-ps:RABO a figi-gii:PricingSource .

figi-ps:CY21 figi-gii:hasUniqueTextIdentifier "CY21" .

figi-ps:RABO skos:prefLabel "rabobank auto ex" .

figi-ps:CY2M a owl:NamedIndividual .

figi-ps:RABO figi-gii:hasUniqueTextIdentifier "RABO" .

figi-ps:CY2M a figi-gii:PricingSource .

figi-ps:RBBT a owl:NamedIndividual .

figi-ps:CY2M skos:prefLabel "cfets 2m bnd fwd yld" .

figi-ps:RBBT a figi-gii:PricingSource .

figi-ps:CY2M figi-gii:hasUniqueTextIdentifier "CY2M" .

figi-ps:RBBT skos:prefLabel "abn amro, incorp." .

figi-ps:CY3M a owl:NamedIndividual , figi-gii:PricingSource ;
	skos:prefLabel "cfets 3m bnd fwd yld" ;
	figi-gii:hasUniqueTextIdentifier "CY3M" .

figi-ps:CY4M a owl:NamedIndividual , figi-gii:PricingSource ;
	skos:prefLabel "cfets 4m bnd fwd yld" .

figi-ps:RBBT figi-gii:hasUniqueTextIdentifier "RBBT" .

figi-ps:CY4M figi-gii:hasUniqueTextIdentifier "CY4M" .

figi-ps:RBCL a owl:NamedIndividual .

figi-ps:CY6M a owl:NamedIndividual .

figi-ps:RBCL a figi-gii:PricingSource .

figi-ps:CY6M a figi-gii:PricingSource .

figi-ps:RBCL skos:prefLabel "rbc london" .

figi-ps:CY6M skos:prefLabel "cfets 6m bnd fwd yld" .

figi-ps:RBCL figi-gii:hasUniqueTextIdentifier "RBCL" .

figi-ps:CY6M figi-gii:hasUniqueTextIdentifier "CY6M" .

figi-ps:RBCR a owl:NamedIndividual .

figi-ps:CY7D a owl:NamedIndividual .

figi-ps:RBCR a figi-gii:PricingSource .

figi-ps:CY7D a figi-gii:PricingSource .

figi-ps:RBCR skos:prefLabel "rbc captial market" .

figi-ps:CY7D skos:prefLabel "cfets 7d bnd fwd yld" .

figi-ps:RBCR figi-gii:hasUniqueTextIdentifier "RBCR" .

figi-ps:CY7D figi-gii:hasUniqueTextIdentifier "CY7D" .

figi-ps:RBDE a owl:NamedIndividual .

figi-ps:CY9M a owl:NamedIndividual .

figi-ps:RBDE a figi-gii:PricingSource .

figi-ps:CY9M a figi-gii:PricingSource .

figi-ps:RBDE skos:prefLabel "inv. services madrid" .

figi-ps:CY9M skos:prefLabel "cfets 9m bnd fwd yld" .

figi-ps:RBDE figi-gii:hasUniqueTextIdentifier "RBDE" .

figi-ps:CY9M figi-gii:hasUniqueTextIdentifier "CY9M" .

figi-ps:RBMT a owl:NamedIndividual .

figi-ps:CYBE a owl:NamedIndividual .

figi-ps:RBMT a figi-gii:PricingSource .

figi-ps:CYBE a figi-gii:PricingSource .

figi-ps:RBMT skos:prefLabel "rbc toms mortgages" .

figi-ps:CYBE skos:prefLabel "cfets executable yld" .

figi-ps:RBMT figi-gii:hasUniqueTextIdentifier "RBMT" .

figi-ps:CYBE figi-gii:hasUniqueTextIdentifier "CYBE" .

figi-ps:RBNV a owl:NamedIndividual .

figi-ps:CYBK a owl:NamedIndividual .

figi-ps:RBNV a figi-gii:PricingSource .

figi-ps:CYBK a figi-gii:PricingSource .

figi-ps:RBNV skos:prefLabel "rbsnvlon" .

figi-ps:CYBK skos:prefLabel "cfets trade yield" .

figi-ps:RBNV figi-gii:hasUniqueTextIdentifier "RBNV" .

figi-ps:CYBK figi-gii:hasUniqueTextIdentifier "CYBK" .

figi-ps:RBOS a owl:NamedIndividual .

figi-ps:CYBQ a owl:NamedIndividual .

figi-ps:RBOS a figi-gii:PricingSource .

figi-ps:CYBQ a figi-gii:PricingSource .

figi-ps:RBOS skos:prefLabel "rbs financial mkts" .

figi-ps:CYBQ skos:prefLabel "cfets yield quote" .

figi-ps:RBOS figi-gii:hasUniqueTextIdentifier "RBOS" .

figi-ps:CYBQ figi-gii:hasUniqueTextIdentifier "CYBQ" .

figi-ps:RBSE a owl:NamedIndividual .

figi-ps:CYDB a owl:NamedIndividual .

figi-ps:RBSE a figi-gii:PricingSource .

figi-ps:CYDB a figi-gii:PricingSource .

figi-ps:RBSE skos:prefLabel "bucharest stock exch" .

figi-ps:CYDB skos:prefLabel "cyprus dev bank" .

figi-ps:RBSE figi-gii:hasUniqueTextIdentifier "RBSE" .

figi-ps:CYDB skos:prefLabel "cyprus development b" .

figi-ps:RBSI a owl:NamedIndividual .

figi-ps:CYDB figi-gii:hasUniqueTextIdentifier "CYDB" .

figi-ps:RBSI a figi-gii:PricingSource .

figi-ps:CZAB a owl:NamedIndividual .

figi-ps:RBSI skos:prefLabel "rbs" .

figi-ps:CZAB a figi-gii:PricingSource .

figi-ps:RBSI figi-gii:hasUniqueTextIdentifier "RBSI" .

figi-ps:CZAB skos:prefLabel "commerzbank, london" .

figi-ps:RBSL a owl:NamedIndividual .

figi-ps:CZAB skos:prefLabel "commerzbank; london" .

figi-ps:RBSL a figi-gii:PricingSource .

figi-ps:CZAB figi-gii:hasUniqueTextIdentifier "CZAB" .

figi-ps:RBSL skos:prefLabel "royal bk of scotland" .

figi-ps:CZBK a owl:NamedIndividual .

figi-ps:RBSL figi-gii:hasUniqueTextIdentifier "RBSL" .

figi-ps:CZBK a figi-gii:PricingSource .

figi-ps:RCMH a owl:NamedIndividual .

figi-ps:CZBK skos:prefLabel "commerzbank abs" .

figi-ps:RCMH a figi-gii:PricingSource .

figi-ps:CZBK figi-gii:hasUniqueTextIdentifier "CZBK" .

figi-ps:RCMH skos:prefLabel "rbc capital hk" .

figi-ps:CZNO a owl:NamedIndividual .

figi-ps:RCMH figi-gii:hasUniqueTextIdentifier "RCMH" .

figi-ps:CZNO a figi-gii:PricingSource .

figi-ps:REPK a owl:NamedIndividual .

figi-ps:CZNO skos:prefLabel "chinabond val szse n" .

figi-ps:REPK a figi-gii:PricingSource .

figi-ps:CZNO figi-gii:hasUniqueTextIdentifier "CZNO" .

figi-ps:REPK skos:prefLabel "jsc bank republic sg" .

figi-ps:CZOP a owl:NamedIndividual .

figi-ps:REPK figi-gii:hasUniqueTextIdentifier "REPK" .

figi-ps:CZOP a figi-gii:PricingSource .

figi-ps:RETL a owl:NamedIndividual .

figi-ps:CZOP skos:prefLabel "chinabond val szse o" .

figi-ps:RETL a figi-gii:PricingSource .

figi-ps:CZOP figi-gii:hasUniqueTextIdentifier "CZOP" .

figi-ps:RETL skos:prefLabel "bofa internal retail" .

figi-ps:DAB a owl:NamedIndividual .

figi-ps:RETL figi-gii:hasUniqueTextIdentifier "RETL" .

figi-ps:DAB a figi-gii:PricingSource .

figi-ps:REVO a owl:NamedIndividual , figi-gii:PricingSource .

figi-ps:DAB skos:prefLabel "deutsche bk-dab" .

figi-ps:REVO skos:prefLabel "drkw test feed" .

figi-ps:DAB figi-gii:hasUniqueTextIdentifier "DAB" .

figi-ps:REVO figi-gii:hasUniqueTextIdentifier "REVO" .

figi-ps:DABC a owl:NamedIndividual .

figi-ps:RFC a owl:NamedIndividual .

figi-ps:DABC a figi-gii:PricingSource .

figi-ps:RFC a figi-gii:PricingSource .

figi-ps:DABC skos:prefLabel "deutsche bank-credit" .

figi-ps:RFC skos:prefLabel "ally securities llc" .

figi-ps:DABC figi-gii:hasUniqueTextIdentifier "DABC" .

figi-ps:RFC figi-gii:hasUniqueTextIdentifier "RFC" .

figi-ps:DABR a owl:NamedIndividual .

figi-ps:RFCC a owl:NamedIndividual .

figi-ps:DABR a figi-gii:PricingSource .

figi-ps:RFCC a figi-gii:PricingSource .

figi-ps:DABR skos:prefLabel "deutsche bank-rates" .

figi-ps:RFCC skos:prefLabel "residential funding" .

figi-ps:DABR figi-gii:hasUniqueTextIdentifier "DABR" .

figi-ps:RFCC figi-gii:hasUniqueTextIdentifier "RFCC" .

figi-ps:DADA a owl:NamedIndividual .

figi-ps:RFCO a owl:NamedIndividual .

figi-ps:DADA a figi-gii:PricingSource .

figi-ps:RFCO a figi-gii:PricingSource .

figi-ps:DADA skos:prefLabel "da davidson" .

figi-ps:RFCO skos:prefLabel "gmac rfc securities" .

figi-ps:DADA figi-gii:hasUniqueTextIdentifier "DADA" .

figi-ps:RFCO figi-gii:hasUniqueTextIdentifier "RFCO" .

figi-ps:DAH a owl:NamedIndividual .

figi-ps:RIKZ a owl:NamedIndividual .

figi-ps:DAH a figi-gii:PricingSource .

figi-ps:RIKZ a figi-gii:PricingSource .

figi-ps:DAH skos:prefLabel "dah sing bank" .

figi-ps:RIKZ skos:prefLabel "fc real-invest" .

figi-ps:DAH figi-gii:hasUniqueTextIdentifier "DAH" .

figi-ps:RIKZ figi-gii:hasUniqueTextIdentifier "RIKZ" .

figi-ps:DAI1 a owl:NamedIndividual .

figi-ps:RILY a owl:NamedIndividual .

figi-ps:DAI1 a figi-gii:PricingSource .

figi-ps:RILY a figi-gii:PricingSource .

figi-ps:DAI1 skos:prefLabel "dai-ichi mutual life" .

figi-ps:RILY skos:prefLabel "b riley and company" .

figi-ps:DAI1 figi-gii:hasUniqueTextIdentifier "DAI1" .

figi-ps:RILY figi-gii:hasUniqueTextIdentifier "RILY" .

figi-ps:DAIE a owl:NamedIndividual .

figi-ps:RIOD a owl:NamedIndividual .

figi-ps:DAIE a figi-gii:PricingSource .

figi-ps:RIOD a figi-gii:PricingSource .

figi-ps:DAIE skos:prefLabel "daiwa cap markets" .

figi-ps:RIOD skos:prefLabel "banco rio (usd)" .

figi-ps:DAIE figi-gii:hasUniqueTextIdentifier "DAIE" .

figi-ps:RIOD figi-gii:hasUniqueTextIdentifier "RIOD" .

figi-ps:DAIM a owl:NamedIndividual .

figi-ps:RLBL a owl:NamedIndividual .

figi-ps:DAIM a figi-gii:PricingSource .

figi-ps:RLBL a figi-gii:PricingSource .

figi-ps:DAIM skos:prefLabel "daiwa cm" .

figi-ps:RLBL skos:prefLabel "kepler-fonds kag" .

figi-ps:DAIM figi-gii:hasUniqueTextIdentifier "DAIM" .

figi-ps:RLBL figi-gii:hasUniqueTextIdentifier "RLBL" .

figi-ps:DAIW a owl:NamedIndividual .

figi-ps:RMBE a owl:NamedIndividual .

figi-ps:DAIW a figi-gii:PricingSource .

figi-ps:RMBE a figi-gii:PricingSource .

figi-ps:DAIW skos:prefLabel "daiwa capmkts am" .

figi-ps:RMBE skos:prefLabel "firstrand sa e-bond" .

figi-ps:DAIW figi-gii:hasUniqueTextIdentifier "DAIW" .

figi-ps:RMBE figi-gii:hasUniqueTextIdentifier "RMBE" .

figi-ps:DALE a owl:NamedIndividual .

figi-ps:ROBA a owl:NamedIndividual .

figi-ps:DALE a figi-gii:PricingSource .

figi-ps:ROBA a figi-gii:PricingSource .

figi-ps:DALE skos:prefLabel "ancora adv" .

figi-ps:ROBA skos:prefLabel "robeco bank holding" .

figi-ps:DALE figi-gii:hasUniqueTextIdentifier "DALE" .

figi-ps:ROBA figi-gii:hasUniqueTextIdentifier "ROBA" .

figi-ps:DAM a owl:NamedIndividual .

figi-ps:ROMB a owl:NamedIndividual .

figi-ps:DAM a figi-gii:PricingSource .

figi-ps:ROMB a figi-gii:PricingSource .

figi-ps:DAM skos:prefLabel "delaware management" .

figi-ps:ROMB skos:prefLabel "banca romaneasca" .

figi-ps:DAM figi-gii:hasUniqueTextIdentifier "DAM" .

figi-ps:ROMB figi-gii:hasUniqueTextIdentifier "ROMB" .

figi-ps:DAMA a owl:NamedIndividual .

figi-ps:ROSA a owl:NamedIndividual .

figi-ps:DAMA a figi-gii:PricingSource .

figi-ps:ROSA a figi-gii:PricingSource .

figi-ps:DAMA skos:prefLabel "daman securities" .

figi-ps:ROSA skos:prefLabel "ej de la rosa" .

figi-ps:DAMA figi-gii:hasUniqueTextIdentifier "DAMA" .

figi-ps:ROSA figi-gii:hasUniqueTextIdentifier "ROSA" .

figi-ps:DAMS a owl:NamedIndividual .

figi-ps:ROSE a owl:NamedIndividual .

figi-ps:DAMS a figi-gii:PricingSource .

figi-ps:ROSE a figi-gii:PricingSource .

figi-ps:DAMS skos:prefLabel "daiwa smbc muni sprd" .

figi-ps:ROSE skos:prefLabel "dahlman rose weiss" .

figi-ps:DAMS figi-gii:hasUniqueTextIdentifier "DAMS" .

figi-ps:ROSE figi-gii:hasUniqueTextIdentifier "ROSE" .

figi-ps:DAMY a owl:NamedIndividual .

figi-ps:RTAM a owl:NamedIndividual .

figi-ps:DAMY a figi-gii:PricingSource .

figi-ps:RTAM a figi-gii:PricingSource .

figi-ps:DAMY skos:prefLabel "daiwa smbc muni yld" .

figi-ps:RTAM skos:prefLabel "gia partners" .

figi-ps:DAMY figi-gii:hasUniqueTextIdentifier "DAMY" .

figi-ps:RTAM figi-gii:hasUniqueTextIdentifier "RTAM" .

figi-ps:DAPR a owl:NamedIndividual .

figi-ps:RURL a owl:NamedIndividual .

figi-ps:DAPR a figi-gii:PricingSource .

figi-ps:RURL a figi-gii:PricingSource .

figi-ps:DAPR skos:prefLabel "dyer and blair inv b" .

figi-ps:RURL skos:prefLabel "caja rural castellon" .

figi-ps:DAPR figi-gii:hasUniqueTextIdentifier "DAPR" .

figi-ps:RURL figi-gii:hasUniqueTextIdentifier "RURL" .

figi-ps:DAPT a owl:NamedIndividual .

figi-ps:RZB a owl:NamedIndividual .

figi-ps:DAPT a figi-gii:PricingSource .

figi-ps:RZB a figi-gii:PricingSource .

figi-ps:DAPT skos:prefLabel "daiwa smbc gpt hk" .

figi-ps:RZB skos:prefLabel "rzb austria ii" .

figi-ps:DAPT figi-gii:hasUniqueTextIdentifier "DAPT" .

figi-ps:RZB figi-gii:hasUniqueTextIdentifier "RZB" .

figi-ps:DAR2 a owl:NamedIndividual .

figi-ps:RZBA a owl:NamedIndividual .

figi-ps:DAR2 a figi-gii:PricingSource .

figi-ps:RZBA a figi-gii:PricingSource .

figi-ps:DAR2 skos:prefLabel "aimdart2" .

figi-ps:RZBA skos:prefLabel "rzb austria" .

figi-ps:DAR2 figi-gii:hasUniqueTextIdentifier "DAR2" .

figi-ps:RZBA figi-gii:hasUniqueTextIdentifier "RZBA" .

figi-ps:DAR3 a owl:NamedIndividual .

figi-ps:SABA a owl:NamedIndividual .

figi-ps:DAR3 a figi-gii:PricingSource .

figi-ps:SABA a figi-gii:PricingSource .

figi-ps:DAR3 skos:prefLabel "aimdart3" .

figi-ps:SABA skos:prefLabel "banco santander sa" .

figi-ps:DAR3 figi-gii:hasUniqueTextIdentifier "DAR3" .

figi-ps:SABA figi-gii:hasUniqueTextIdentifier "SABA" .

figi-ps:DAR4 a owl:NamedIndividual .

figi-ps:SABB a owl:NamedIndividual .

figi-ps:DAR4 a figi-gii:PricingSource .

figi-ps:SABB a figi-gii:PricingSource ;
	skos:prefLabel "banco sabadell" .

figi-ps:DAR4 skos:prefLabel "aimdart4" .

figi-ps:SABB figi-gii:hasUniqueTextIdentifier "SABB" .

figi-ps:DAR4 figi-gii:hasUniqueTextIdentifier "DAR4" .

figi-ps:SABL a owl:NamedIndividual , figi-gii:PricingSource .

figi-ps:DARS a owl:NamedIndividual .

figi-ps:SABL skos:prefLabel "caja sabadell" .

figi-ps:DARS a figi-gii:PricingSource .

figi-ps:SABL figi-gii:hasUniqueTextIdentifier "SABL" .

figi-ps:DARS skos:prefLabel "daiwa smbc sec hk" .

figi-ps:SAFR a owl:NamedIndividual , figi-gii:PricingSource .

figi-ps:DARS figi-gii:hasUniqueTextIdentifier "DARS" .

figi-ps:SAFR skos:prefLabel "banco safra" ;
	figi-gii:hasUniqueTextIdentifier "SAFR" .

figi-ps:DART a owl:NamedIndividual .

figi-ps:SAL a owl:NamedIndividual .

figi-ps:DART a figi-gii:PricingSource .

figi-ps:SAL a figi-gii:PricingSource ;
	skos:prefLabel "citigroup 1" .

figi-ps:DART skos:prefLabel "aim dart demo" .

figi-ps:SAL figi-gii:hasUniqueTextIdentifier "SAL" .

figi-ps:DART figi-gii:hasUniqueTextIdentifier "DART" .

figi-ps:SALI a owl:NamedIndividual , figi-gii:PricingSource .

figi-ps:DARW a owl:NamedIndividual .

figi-ps:SALI skos:prefLabel "sterne; agee and leach" .

figi-ps:DARW a figi-gii:PricingSource .

figi-ps:SALI figi-gii:hasUniqueTextIdentifier "SALI" .

figi-ps:DARW skos:prefLabel "darwin financial" .

figi-ps:SAMB a owl:NamedIndividual , figi-gii:PricingSource .

figi-ps:DARW figi-gii:hasUniqueTextIdentifier "DARW" .

figi-ps:SAMB skos:prefLabel "sampo mtge" .

figi-ps:DASG a owl:NamedIndividual .

figi-ps:SAMB figi-gii:hasUniqueTextIdentifier "SAMB" .

figi-ps:DASG a figi-gii:PricingSource .

figi-ps:SANM a owl:NamedIndividual , figi-gii:PricingSource .

figi-ps:DASG skos:prefLabel "daiwa capital s'pore" .

figi-ps:SANM skos:prefLabel "banco santander" .

figi-ps:DASG figi-gii:hasUniqueTextIdentifier "DASG" .

figi-ps:SANM figi-gii:hasUniqueTextIdentifier "SANM" .

figi-ps:SAPX a owl:NamedIndividual .

figi-ps:DASJ a owl:NamedIndividual .

figi-ps:SAPX a figi-gii:PricingSource .

figi-ps:DASJ a figi-gii:PricingSource .

figi-ps:SAPX skos:prefLabel "bloomberg server api" ;
	figi-gii:hasUniqueTextIdentifier "SAPX" .

figi-ps:DASJ skos:prefLabel "daiwa sec cm" .

figi-ps:SARA a owl:NamedIndividual .

figi-ps:DASJ figi-gii:hasUniqueTextIdentifier "DASJ" .

figi-ps:SARA a figi-gii:PricingSource .

figi-ps:DAV a owl:NamedIndividual .

figi-ps:SARA skos:prefLabel "bank sarasin" .

figi-ps:DAV a figi-gii:PricingSource .

figi-ps:SARA figi-gii:hasUniqueTextIdentifier "SARA" .

figi-ps:SBFT a owl:NamedIndividual .

figi-ps:DAV skos:prefLabel "davy" .

figi-ps:SBFT a figi-gii:PricingSource .

figi-ps:DAV figi-gii:hasUniqueTextIdentifier "DAV" .

figi-ps:SBFT skos:prefLabel "citigroup frankfurt" .

figi-ps:DAVB a owl:NamedIndividual .

figi-ps:SBFT figi-gii:hasUniqueTextIdentifier "SBFT" .

figi-ps:DAVB a figi-gii:PricingSource .

figi-ps:SBLL a owl:NamedIndividual , figi-gii:PricingSource .

figi-ps:DAVB skos:prefLabel "davy" .

figi-ps:SBLL skos:prefLabel "standard bank london" ;
	figi-gii:hasUniqueTextIdentifier "SBLL" .

figi-ps:DAVB figi-gii:hasUniqueTextIdentifier "DAVB" .

figi-ps:SBLN a owl:NamedIndividual , figi-gii:PricingSource .

figi-ps:DAVI a owl:NamedIndividual .

figi-ps:SBLN skos:prefLabel "standard bank ln" .

figi-ps:DAVI a figi-gii:PricingSource .

figi-ps:SBLN figi-gii:hasUniqueTextIdentifier "SBLN" .

figi-ps:SBOA a owl:NamedIndividual .

figi-ps:DAVI skos:prefLabel "banco davivienda sa" .

figi-ps:SBOA a figi-gii:PricingSource ;
	skos:prefLabel "bancofamerica-silver" .

figi-ps:DAVI figi-gii:hasUniqueTextIdentifier "DAVI" .

figi-ps:SBOA figi-gii:hasUniqueTextIdentifier "SBOA" .

figi-ps:SBSH a owl:NamedIndividual .

figi-ps:DAVW a owl:NamedIndividual .

figi-ps:SBSH a figi-gii:PricingSource .

figi-ps:DAVW a figi-gii:PricingSource .

figi-ps:SBSH skos:prefLabel "citigroup global" ;
	figi-gii:hasUniqueTextIdentifier "SBSH" .

figi-ps:DAVW skos:prefLabel "david william sec" .

figi-ps:SBSI a owl:NamedIndividual , figi-gii:PricingSource .

figi-ps:DAVW skos:prefLabel "david william sec's" .

figi-ps:SBSI skos:prefLabel "citigroup special st" .

figi-ps:DAVW figi-gii:hasUniqueTextIdentifier "DAVW" .

figi-ps:SBSI figi-gii:hasUniqueTextIdentifier "SBSI" .

figi-ps:DAVY a owl:NamedIndividual .

figi-ps:SCBX a owl:NamedIndividual .

figi-ps:DAVY a figi-gii:PricingSource .

figi-ps:SCBX a figi-gii:PricingSource .

figi-ps:DAVY skos:prefLabel "davy" .

figi-ps:SCBX skos:prefLabel "standard chartered" .

figi-ps:DAVY figi-gii:hasUniqueTextIdentifier "DAVY" .

figi-ps:SCBX figi-gii:hasUniqueTextIdentifier "SCBX" .

figi-ps:DAWA a owl:NamedIndividual .

figi-ps:SCCC a owl:NamedIndividual .

figi-ps:DAWA a figi-gii:PricingSource .

figi-ps:SCCC a figi-gii:PricingSource ;
	skos:prefLabel "bank of nova scotia" .

figi-ps:DAWA skos:prefLabel "daiwa europe ltd" .

figi-ps:SCCC figi-gii:hasUniqueTextIdentifier "SCCC" .

figi-ps:DAWA figi-gii:hasUniqueTextIdentifier "DAWA" .

figi-ps:SCDR a owl:NamedIndividual , figi-gii:PricingSource ;
	skos:prefLabel "banco santa cruz" .

figi-ps:DAWT a owl:NamedIndividual .

figi-ps:SCDR figi-gii:hasUniqueTextIdentifier "SCDR" .

figi-ps:DAWT a figi-gii:PricingSource .

figi-ps:SCRP a owl:NamedIndividual , figi-gii:PricingSource .

figi-ps:DAWT skos:prefLabel "daiwasecs ion test" .

figi-ps:SCRP skos:prefLabel "blp mscr internal" .

figi-ps:DAWT figi-gii:hasUniqueTextIdentifier "DAWT" .

figi-ps:SCRP figi-gii:hasUniqueTextIdentifier "SCRP" .

figi-ps:DAYC a owl:NamedIndividual , figi-gii:PricingSource .

figi-ps:SCUD a owl:NamedIndividual .

figi-ps:DAYC skos:prefLabel "banco daycoval" .

figi-ps:SCUD a figi-gii:PricingSource .

figi-ps:DAYC figi-gii:hasUniqueTextIdentifier "DAYC" .

figi-ps:SCUD skos:prefLabel "dbam zurich" .

figi-ps:DAYF a owl:NamedIndividual .

figi-ps:SCUD figi-gii:hasUniqueTextIdentifier "SCUD" .

figi-ps:DAYF a figi-gii:PricingSource .

figi-ps:SDBK a owl:NamedIndividual .

figi-ps:DAYF skos:prefLabel "daiwa sec cm yen bds" .

figi-ps:SDBK a figi-gii:PricingSource .

figi-ps:DAYF figi-gii:hasUniqueTextIdentifier "DAYF" .

figi-ps:SDBK skos:prefLabel "cfif shenzhen dev bk" .

figi-ps:DB a owl:NamedIndividual .

figi-ps:SDBK figi-gii:hasUniqueTextIdentifier "SDBK" .

figi-ps:DB a figi-gii:PricingSource .

figi-ps:SDEL a owl:NamedIndividual .

figi-ps:DB skos:prefLabel "deutsche bank group" .

figi-ps:SDEL a figi-gii:PricingSource .

figi-ps:DB figi-gii:hasUniqueTextIdentifier "DB" .

figi-ps:SDEL skos:prefLabel "grupo banco sabadell" .

figi-ps:DBA a owl:NamedIndividual .

figi-ps:SDEL figi-gii:hasUniqueTextIdentifier "SDEL" .

figi-ps:DBA a figi-gii:PricingSource .

figi-ps:SEBM a owl:NamedIndividual .

figi-ps:DBA skos:prefLabel "deutsche bank asia" .

figi-ps:SEBM a figi-gii:PricingSource .

figi-ps:DBA figi-gii:hasUniqueTextIdentifier "DBA" .

figi-ps:SEBM skos:prefLabel "seb london mtge" .

figi-ps:DBAB a owl:NamedIndividual .

figi-ps:SEBM figi-gii:hasUniqueTextIdentifier "SEBM" .

figi-ps:DBAB a figi-gii:PricingSource .

figi-ps:SEBP a owl:NamedIndividual .

figi-ps:DBAB skos:prefLabel "deutsche bank prop" .

figi-ps:SEBP a figi-gii:PricingSource .

figi-ps:DBAB figi-gii:hasUniqueTextIdentifier "DBAB" .

figi-ps:SEBP skos:prefLabel "seb stockholm" .

figi-ps:DBAE a owl:NamedIndividual .

figi-ps:SEBP figi-gii:hasUniqueTextIdentifier "SEBP" .

figi-ps:DBAE a figi-gii:PricingSource .

figi-ps:SEBS a owl:NamedIndividual .

figi-ps:DBAE skos:prefLabel "deutsche bk auto ex" .

figi-ps:SEBS a figi-gii:PricingSource .

figi-ps:DBAE figi-gii:hasUniqueTextIdentifier "DBAE" .

figi-ps:SEBS skos:prefLabel "seb merchant banking" .

figi-ps:DBAN a owl:NamedIndividual .

figi-ps:SEBS figi-gii:hasUniqueTextIdentifier "SEBS" .

figi-ps:DBAN a figi-gii:PricingSource ;
	skos:prefLabel "deutsche bank - boom" ;
	figi-gii:hasUniqueTextIdentifier "DBAN" .

figi-ps:SEBZ a owl:NamedIndividual .

figi-ps:DBAP a owl:NamedIndividual .

figi-ps:SEBZ a figi-gii:PricingSource .

figi-ps:DBAP a figi-gii:PricingSource .

figi-ps:SEBZ skos:prefLabel "seb stockholm" .

figi-ps:DBAP skos:prefLabel "deutsche asia pac" .

figi-ps:SEBZ figi-gii:hasUniqueTextIdentifier "SEBZ" .

figi-ps:DBAP figi-gii:hasUniqueTextIdentifier "DBAP" .

figi-ps:SEDL a owl:NamedIndividual .

figi-ps:DBAS a owl:NamedIndividual .

figi-ps:SEDL a figi-gii:PricingSource .

figi-ps:DBAS a figi-gii:PricingSource .

figi-ps:SEDL skos:prefLabel "centrl bk of iceland" .

figi-ps:DBAS skos:prefLabel "deutsche bank sing" .

figi-ps:SEDL figi-gii:hasUniqueTextIdentifier "SEDL" .

figi-ps:SEEL a owl:NamedIndividual , figi-gii:PricingSource ;
	skos:prefLabel "seelaus and co" ;
	figi-gii:hasUniqueTextIdentifier "SEEL" .

figi-ps:SEID a owl:NamedIndividual , figi-gii:PricingSource .

figi-ps:DBAS figi-gii:hasUniqueTextIdentifier "DBAS" .

figi-ps:SEID skos:prefLabel "david william sec's" .

figi-ps:DBAU a owl:NamedIndividual .

figi-ps:SEID figi-gii:hasUniqueTextIdentifier "SEID" .

figi-ps:DBAU a figi-gii:PricingSource .

figi-ps:SETA a owl:NamedIndividual .

figi-ps:DBAU skos:prefLabel "deut. bank australia" .

figi-ps:SETA a figi-gii:PricingSource .

figi-ps:DBAU figi-gii:hasUniqueTextIdentifier "DBAU" .

figi-ps:SETA skos:prefLabel "santander auto-ex ny" .

figi-ps:DBAX a owl:NamedIndividual .

figi-ps:SETA figi-gii:hasUniqueTextIdentifier "SETA" .

figi-ps:DBAX a figi-gii:PricingSource .

figi-ps:SFB a owl:NamedIndividual .

figi-ps:DBAX skos:prefLabel "deutsche bank kl" .

figi-ps:SFB a figi-gii:PricingSource .

figi-ps:DBAX figi-gii:hasUniqueTextIdentifier "DBAX" .

figi-ps:SFB skos:prefLabel "cordares" .

figi-ps:DBBY a owl:NamedIndividual .

figi-ps:SFB figi-gii:hasUniqueTextIdentifier "SFB" .

figi-ps:DBBY a figi-gii:PricingSource .

figi-ps:SGAR a owl:NamedIndividual .

figi-ps:DBBY skos:prefLabel "deutsche bank india" .

figi-ps:SGAR a figi-gii:PricingSource .

figi-ps:DBBY figi-gii:hasUniqueTextIdentifier "DBBY" .

figi-ps:SGAR skos:prefLabel "societe gen reval" .

figi-ps:DBBZ a owl:NamedIndividual .

figi-ps:SGAR figi-gii:hasUniqueTextIdentifier "SGAR" .

figi-ps:DBBZ a figi-gii:PricingSource .

figi-ps:SGAU a owl:NamedIndividual .

figi-ps:DBBZ skos:prefLabel "deutsche brazil" .

figi-ps:SGAU a figi-gii:PricingSource .

figi-ps:DBBZ figi-gii:hasUniqueTextIdentifier "DBBZ" .

figi-ps:SGAU skos:prefLabel "sg australia" .

figi-ps:DBCE a owl:NamedIndividual .

figi-ps:SGAU figi-gii:hasUniqueTextIdentifier "SGAU" .

figi-ps:DBCE a figi-gii:PricingSource .

figi-ps:SGEX a owl:NamedIndividual .

figi-ps:DBCE skos:prefLabel "db structured notes" .

figi-ps:SGEX a figi-gii:PricingSource .

figi-ps:DBCE figi-gii:hasUniqueTextIdentifier "DBCE" .

figi-ps:SGEX skos:prefLabel "singapore stock exch" .

figi-ps:DBCH a owl:NamedIndividual .

figi-ps:SGEX figi-gii:hasUniqueTextIdentifier "SGEX" .

figi-ps:DBCH a figi-gii:PricingSource .

figi-ps:SGIN a owl:NamedIndividual .

figi-ps:DBCH skos:prefLabel "deutsche bk chile" .

figi-ps:SGIN a figi-gii:PricingSource .

figi-ps:DBCH figi-gii:hasUniqueTextIdentifier "DBCH" .

figi-ps:SGIN skos:prefLabel "socgen cap mkts" .

figi-ps:DBCN a owl:NamedIndividual .

figi-ps:SGIN figi-gii:hasUniqueTextIdentifier "SGIN" .

figi-ps:DBCN a figi-gii:PricingSource .

figi-ps:SGOZ a owl:NamedIndividual .

figi-ps:DBCN skos:prefLabel "deutsche bank canada" .

figi-ps:SGOZ a figi-gii:PricingSource .

figi-ps:DBCN figi-gii:hasUniqueTextIdentifier "DBCN" .

figi-ps:SGOZ skos:prefLabel "sg australia limited" .

figi-ps:DBDK a owl:NamedIndividual .

figi-ps:SGOZ figi-gii:hasUniqueTextIdentifier "SGOZ" .

figi-ps:DBDK a figi-gii:PricingSource .

figi-ps:SHCA a owl:NamedIndividual .

figi-ps:DBDK skos:prefLabel "danske bank" .

figi-ps:SHCA a figi-gii:PricingSource .

figi-ps:DBDK figi-gii:hasUniqueTextIdentifier "DBDK" .

figi-ps:SHCA skos:prefLabel "icbc (macau) limited" .

figi-ps:DBEA a owl:NamedIndividual .

figi-ps:SHCA figi-gii:hasUniqueTextIdentifier "SHCA" .

figi-ps:DBEA a figi-gii:PricingSource .

figi-ps:SHIS a owl:NamedIndividual .

figi-ps:DBEA skos:prefLabel "deutsche secs tokyo" .

figi-ps:SHIS a figi-gii:PricingSource .

figi-ps:DBEA figi-gii:hasUniqueTextIdentifier "DBEA" .

figi-ps:SHIS skos:prefLabel "shinsei secs" .

figi-ps:DBEN a owl:NamedIndividual .

figi-ps:SHIS figi-gii:hasUniqueTextIdentifier "SHIS" .

figi-ps:DBEN a figi-gii:PricingSource .

figi-ps:SINE a owl:NamedIndividual .

figi-ps:DBEN skos:prefLabel "deutsche bank" .

figi-ps:SINE a figi-gii:PricingSource .

figi-ps:DBEN figi-gii:hasUniqueTextIdentifier "DBEN" .

figi-ps:SINE skos:prefLabel "national alliance" .

figi-ps:DBES a owl:NamedIndividual .

figi-ps:SINE figi-gii:hasUniqueTextIdentifier "SINE" .

figi-ps:DBES a figi-gii:PricingSource .

figi-ps:SINV a owl:NamedIndividual .

figi-ps:DBES skos:prefLabel "deutsche bank pp" .

figi-ps:SINV a figi-gii:PricingSource .

figi-ps:DBES figi-gii:hasUniqueTextIdentifier "DBES" .

figi-ps:SINV skos:prefLabel "banco santander mex" .

figi-ps:DBEX a owl:NamedIndividual .

figi-ps:SINV figi-gii:hasUniqueTextIdentifier "SINV" .

figi-ps:DBEX a figi-gii:PricingSource .

figi-ps:SLBZ a owl:NamedIndividual .

figi-ps:DBEX skos:prefLabel "danske bk" .

figi-ps:SLBZ a figi-gii:PricingSource .

figi-ps:DBEX figi-gii:hasUniqueTextIdentifier "DBEX" .

figi-ps:SLBZ skos:prefLabel "banco standard bz" .

figi-ps:DBGN a owl:NamedIndividual .

figi-ps:SLBZ figi-gii:hasUniqueTextIdentifier "SLBZ" .

figi-ps:DBGN a figi-gii:PricingSource .

figi-ps:SLSP a owl:NamedIndividual .

figi-ps:DBGN skos:prefLabel "deutsche bank - dbgn" .

figi-ps:SLSP a figi-gii:PricingSource .

figi-ps:DBGN figi-gii:hasUniqueTextIdentifier "DBGN" .

figi-ps:DBI a owl:NamedIndividual , figi-gii:PricingSource ;
	skos:prefLabel "deutsche bank intern" .

figi-ps:SLSP skos:prefLabel "asset mgmt slsp" .

figi-ps:DBI figi-gii:hasUniqueTextIdentifier "DBI" .

figi-ps:SLSP figi-gii:hasUniqueTextIdentifier "SLSP" .

figi-ps:SN a owl:NamedIndividual .

figi-ps:DBIA a owl:NamedIndividual .

figi-ps:SN a figi-gii:PricingSource .

figi-ps:DBIA a figi-gii:PricingSource .

figi-ps:SN skos:prefLabel "stifel nicolaus" .

figi-ps:DBIA skos:prefLabel "db asia internal" .

figi-ps:SN figi-gii:hasUniqueTextIdentifier "SN" .

figi-ps:DBIA figi-gii:hasUniqueTextIdentifier "DBIA" .

figi-ps:SNKS a owl:NamedIndividual .

figi-ps:DBIN a owl:NamedIndividual .

figi-ps:SNKS a figi-gii:PricingSource .

figi-ps:DBIN a figi-gii:PricingSource .

figi-ps:SNKS skos:prefLabel "shinko sec tokyo" .

figi-ps:DBIN skos:prefLabel "db intern (wkn)" .

figi-ps:SNKS figi-gii:hasUniqueTextIdentifier "SNKS" .

figi-ps:DBIN figi-gii:hasUniqueTextIdentifier "DBIN" .

figi-ps:SNY a owl:NamedIndividual .

figi-ps:DBIS a owl:NamedIndividual .

figi-ps:SNY a figi-gii:PricingSource .

figi-ps:DBIS a figi-gii:PricingSource .

figi-ps:SNY skos:prefLabel "stone and youngberg" .

figi-ps:DBIS skos:prefLabel "db intern (isin)" .

figi-ps:SNY figi-gii:hasUniqueTextIdentifier "SNY" .

figi-ps:DBIS figi-gii:hasUniqueTextIdentifier "DBIS" .

figi-ps:DBIX a owl:NamedIndividual .

figi-ps:SPDB a owl:NamedIndividual .

figi-ps:DBIX a figi-gii:PricingSource .

figi-ps:SPDB a figi-gii:PricingSource .

figi-ps:DBIX skos:prefLabel "deutsche bank iboxx" .

figi-ps:SPDB skos:prefLabel "cfets sh pudg dev bk" .

figi-ps:DBIX figi-gii:hasUniqueTextIdentifier "DBIX" .

figi-ps:SPDB figi-gii:hasUniqueTextIdentifier "SPDB" .

figi-ps:DBJA a owl:NamedIndividual .

figi-ps:SPDV a owl:NamedIndividual .

figi-ps:DBJA a figi-gii:PricingSource .

figi-ps:SPDV a figi-gii:PricingSource .

figi-ps:DBJA skos:prefLabel "deutsche sec japan" .

figi-ps:SPDV skos:prefLabel "cfet sh pudong dv bk" .

figi-ps:DBJA figi-gii:hasUniqueTextIdentifier "DBJA" .

figi-ps:SPDV figi-gii:hasUniqueTextIdentifier "SPDV" .

figi-ps:DBJB a owl:NamedIndividual .

figi-ps:SPEX a owl:NamedIndividual , figi-gii:PricingSource .

figi-ps:DBJB a figi-gii:PricingSource .

figi-ps:SPEX skos:prefLabel "bloomberg spex" .

figi-ps:DBJB skos:prefLabel "deutsche jo'burg" .

figi-ps:SPEX figi-gii:hasUniqueTextIdentifier "SPEX" .

figi-ps:DBJB figi-gii:hasUniqueTextIdentifier "DBJB" .

figi-ps:SPRI a owl:NamedIndividual .

figi-ps:DBJE a owl:NamedIndividual .

figi-ps:SPRI a figi-gii:PricingSource .

figi-ps:DBJE a figi-gii:PricingSource .

figi-ps:SPRI skos:prefLabel "ing amsterdam" .

figi-ps:DBJE skos:prefLabel "deutsche bank sa" .

figi-ps:SPRI figi-gii:hasUniqueTextIdentifier "SPRI" .

figi-ps:DBJE figi-gii:hasUniqueTextIdentifier "DBJE" .

figi-ps:SPS a owl:NamedIndividual .

figi-ps:DBKL a owl:NamedIndividual .

figi-ps:SPS a figi-gii:PricingSource .

figi-ps:DBKL a figi-gii:PricingSource .

figi-ps:SPS skos:prefLabel "street software" .

figi-ps:DBKL skos:prefLabel "deutsche axes" .

figi-ps:SPS figi-gii:hasUniqueTextIdentifier "SPS" .

figi-ps:DBKL figi-gii:hasUniqueTextIdentifier "DBKL" .

figi-ps:SPSE a owl:NamedIndividual .

figi-ps:DBLO a owl:NamedIndividual .

figi-ps:SPSE a figi-gii:PricingSource .

figi-ps:DBLO a figi-gii:PricingSource .

figi-ps:SPSE skos:prefLabel "standard and poor's" .

figi-ps:DBLO skos:prefLabel "deutsche bank loans" .

figi-ps:SPSE figi-gii:hasUniqueTextIdentifier "SPSE" .

figi-ps:DBLO figi-gii:hasUniqueTextIdentifier "DBLO" .

figi-ps:SPSP a owl:NamedIndividual .

figi-ps:DBMM a owl:NamedIndividual .

figi-ps:SPSP a figi-gii:PricingSource .

figi-ps:DBMM a figi-gii:PricingSource .

figi-ps:SPSP skos:prefLabel "sandp-client portfolio" .

figi-ps:DBMM skos:prefLabel "deutsche bk msc mtge" .

figi-ps:SPSP figi-gii:hasUniqueTextIdentifier "SPSP" .

figi-ps:DBMM figi-gii:hasUniqueTextIdentifier "DBMM" .

figi-ps:SSBA a owl:NamedIndividual .

figi-ps:DBMN a owl:NamedIndividual .

figi-ps:SSBA a figi-gii:PricingSource .

figi-ps:DBMN a figi-gii:PricingSource .

figi-ps:SSBA skos:prefLabel "citigroup australia" .

figi-ps:DBMN skos:prefLabel "deutsche bank mnl" .

figi-ps:SSBA figi-gii:hasUniqueTextIdentifier "SSBA" .

figi-ps:DBMN figi-gii:hasUniqueTextIdentifier "DBMN" .

figi-ps:SSBH a owl:NamedIndividual .

figi-ps:DBMO a owl:NamedIndividual .

figi-ps:SSBH a figi-gii:PricingSource .

figi-ps:DBMO a figi-gii:PricingSource .

figi-ps:SSBH skos:prefLabel "citigroup global mkt" .

figi-ps:DBMO skos:prefLabel "deutsche bank moscow" .

figi-ps:SSBH figi-gii:hasUniqueTextIdentifier "SSBH" .

figi-ps:DBMO figi-gii:hasUniqueTextIdentifier "DBMO" .

figi-ps:SSBM a owl:NamedIndividual .

figi-ps:DBMX a owl:NamedIndividual .

figi-ps:SSBM a figi-gii:PricingSource .

figi-ps:DBMX a figi-gii:PricingSource .

figi-ps:SSBM skos:prefLabel "citigroup london" .

figi-ps:DBMX skos:prefLabel "deutsche mexico" .

figi-ps:SSBM figi-gii:hasUniqueTextIdentifier "SSBM" .

figi-ps:DBMX figi-gii:hasUniqueTextIdentifier "DBMX" .

figi-ps:SSBQ a owl:NamedIndividual .

figi-ps:DBNA a owl:NamedIndividual .

figi-ps:SSBQ a figi-gii:PricingSource .

figi-ps:DBNA a figi-gii:PricingSource .

figi-ps:SSBQ skos:prefLabel "citigroup 2" .

figi-ps:DBNA skos:prefLabel "deutsche bank na" .

figi-ps:SSBQ figi-gii:hasUniqueTextIdentifier "SSBQ" .

figi-ps:DBNA figi-gii:hasUniqueTextIdentifier "DBNA" .

figi-ps:SSDP a owl:NamedIndividual .

figi-ps:DBNN a owl:NamedIndividual .

figi-ps:SSDP a figi-gii:PricingSource .

figi-ps:DBNN a figi-gii:PricingSource .

figi-ps:SSDP skos:prefLabel "citigroup 3" .

figi-ps:DBNN skos:prefLabel "deutsche bank corps" .

figi-ps:SSDP figi-gii:hasUniqueTextIdentifier "SSDP" .

figi-ps:DBNN figi-gii:hasUniqueTextIdentifier "DBNN" .

figi-ps:SSEI a owl:NamedIndividual .

figi-ps:DBNY a owl:NamedIndividual .

figi-ps:SSEI a figi-gii:PricingSource .

figi-ps:DBNY a figi-gii:PricingSource .

figi-ps:SSEI skos:prefLabel "indonesia stock exch" .

figi-ps:DBNY skos:prefLabel "deutsche bank ny" .

figi-ps:SSEI figi-gii:hasUniqueTextIdentifier "SSEI" .

figi-ps:DBNY figi-gii:hasUniqueTextIdentifier "DBNY" .

figi-ps:SSFT a owl:NamedIndividual .

figi-ps:DBNZ a owl:NamedIndividual .

figi-ps:SSFT a figi-gii:PricingSource .

figi-ps:DBNZ a figi-gii:PricingSource .

figi-ps:SSFT skos:prefLabel "street software" .

figi-ps:DBNZ skos:prefLabel "deutsche bank nz" .

figi-ps:SSFT figi-gii:hasUniqueTextIdentifier "SSFT" .

figi-ps:DBNZ figi-gii:hasUniqueTextIdentifier "DBNZ" .

figi-ps:SSMB a owl:NamedIndividual .

figi-ps:DBON a owl:NamedIndividual .

figi-ps:SSMB a figi-gii:PricingSource .

figi-ps:DBON a figi-gii:PricingSource .

figi-ps:SSMB skos:prefLabel "citigroup new york" .

figi-ps:DBON skos:prefLabel "deutsche bk shanghai" .

figi-ps:SSMB figi-gii:hasUniqueTextIdentifier "SSMB" .

figi-ps:DBON figi-gii:hasUniqueTextIdentifier "DBON" .

figi-ps:STAG a owl:NamedIndividual .

figi-ps:DBP a owl:NamedIndividual .

figi-ps:STAG a figi-gii:PricingSource .

figi-ps:DBP a figi-gii:PricingSource .

figi-ps:STAG skos:prefLabel "aim staging database" .

figi-ps:DBP skos:prefLabel "devt bk of the phils" .

figi-ps:STAG figi-gii:hasUniqueTextIdentifier "STAG" .

figi-ps:DBP figi-gii:hasUniqueTextIdentifier "DBP" .

figi-ps:STCO a owl:NamedIndividual .

figi-ps:DBPE a owl:NamedIndividual .

figi-ps:STCO a figi-gii:PricingSource .

figi-ps:DBPE a figi-gii:PricingSource .

figi-ps:STCO skos:prefLabel "suntrust cap mkts" .

figi-ps:DBPE skos:prefLabel "deutsche bank peru" .

figi-ps:STCO figi-gii:hasUniqueTextIdentifier "STCO" .

figi-ps:DBPE figi-gii:hasUniqueTextIdentifier "DBPE" .

figi-ps:STPH a owl:NamedIndividual .

figi-ps:DBPK a owl:NamedIndividual .

figi-ps:STPH a figi-gii:PricingSource .

figi-ps:DBPK a figi-gii:PricingSource .

figi-ps:STPH skos:prefLabel "stephens inc" .

figi-ps:DBPK skos:prefLabel "deutsche bank, pk" .

figi-ps:STPH figi-gii:hasUniqueTextIdentifier "STPH" .

figi-ps:DBPK figi-gii:hasUniqueTextIdentifier "DBPK" .

figi-ps:STUR a owl:NamedIndividual .

figi-ps:DBPM a owl:NamedIndividual .

figi-ps:STUR a figi-gii:PricingSource .

figi-ps:DBPM a figi-gii:PricingSource .

figi-ps:STUR skos:prefLabel "e i sturdza" .

figi-ps:DBPM skos:prefLabel "deutsche bank metals" .

figi-ps:STUR figi-gii:hasUniqueTextIdentifier "STUR" .

figi-ps:DBPM figi-gii:hasUniqueTextIdentifier "DBPM" .

figi-ps:SUSA a owl:NamedIndividual .

figi-ps:DBPP a owl:NamedIndividual .

figi-ps:SUSA a figi-gii:PricingSource .

figi-ps:DBPP a figi-gii:PricingSource .

figi-ps:SUSA skos:prefLabel "stephens inc - mtge" .

figi-ps:DBPP skos:prefLabel "deutsche bk privates" .

figi-ps:SUSA figi-gii:hasUniqueTextIdentifier "SUSA" .

figi-ps:DBPP figi-gii:hasUniqueTextIdentifier "DBPP" .

figi-ps:SWFZ a owl:NamedIndividual .

figi-ps:DBPU a owl:NamedIndividual .

figi-ps:SWFZ a figi-gii:PricingSource .

figi-ps:DBPU a figi-gii:PricingSource .

figi-ps:SWFZ skos:prefLabel "banque pasche sa" .

figi-ps:DBPU skos:prefLabel "deutsche public prc" .

figi-ps:SWFZ figi-gii:hasUniqueTextIdentifier "SWFZ" .

figi-ps:DBPU figi-gii:hasUniqueTextIdentifier "DBPU" .

figi-ps:SWXQ a owl:NamedIndividual .

figi-ps:DBPX a owl:NamedIndividual .

figi-ps:SWXQ a figi-gii:PricingSource .

figi-ps:DBPX a figi-gii:PricingSource .

figi-ps:SWXQ skos:prefLabel "alex-swx quotematch" .

figi-ps:DBPX skos:prefLabel "deutsche pricing" .

figi-ps:SWXQ figi-gii:hasUniqueTextIdentifier "SWXQ" .

figi-ps:DBPX figi-gii:hasUniqueTextIdentifier "DBPX" .

figi-ps:SYNF a owl:NamedIndividual .

figi-ps:DBRV a owl:NamedIndividual .

figi-ps:SYNF a figi-gii:PricingSource .

figi-ps:DBRV a figi-gii:PricingSource .

figi-ps:SYNF skos:prefLabel "synesis finance sa" .

figi-ps:DBRV skos:prefLabel "deutsche bank london" .

figi-ps:SYNF figi-gii:hasUniqueTextIdentifier "SYNF" .

figi-ps:DBRV figi-gii:hasUniqueTextIdentifier "DBRV" .

figi-ps:SYZ a owl:NamedIndividual .

figi-ps:DBS a owl:NamedIndividual .

figi-ps:SYZ a figi-gii:PricingSource .

figi-ps:DBS a figi-gii:PricingSource .

figi-ps:SYZ skos:prefLabel "banque syz" ;
	figi-gii:hasUniqueTextIdentifier "SYZ" .

figi-ps:DBS skos:prefLabel "dbs bank ltd" .

figi-ps:T998 a owl:NamedIndividual .

figi-ps:DBS figi-gii:hasUniqueTextIdentifier "DBS" .

figi-ps:T998 a figi-gii:PricingSource .

figi-ps:DBSA a owl:NamedIndividual .

figi-ps:T998 skos:prefLabel "bb buy-side demo" .

figi-ps:DBSA a figi-gii:PricingSource .

figi-ps:T998 figi-gii:hasUniqueTextIdentifier "T998" .

figi-ps:DBSA skos:prefLabel "dbs asset management" .

figi-ps:T999 a owl:NamedIndividual .

figi-ps:DBSA figi-gii:hasUniqueTextIdentifier "DBSA" .

figi-ps:T999 a figi-gii:PricingSource .

figi-ps:DBSB a owl:NamedIndividual .

figi-ps:T999 skos:prefLabel "bb sell-side demo" .

figi-ps:DBSB a figi-gii:PricingSource .

figi-ps:T999 figi-gii:hasUniqueTextIdentifier "T999" .

figi-ps:DBSB skos:prefLabel "dbs bk hk ltd 11:30" .

figi-ps:TAIC a owl:NamedIndividual .

figi-ps:DBSB figi-gii:hasUniqueTextIdentifier "DBSB" .

figi-ps:TAIC a figi-gii:PricingSource .

figi-ps:DBSD a owl:NamedIndividual .

figi-ps:TAIC skos:prefLabel "arab investment" .

figi-ps:DBSD a figi-gii:PricingSource .

figi-ps:TAIC figi-gii:hasUniqueTextIdentifier "TAIC" .

figi-ps:DBSD skos:prefLabel "dbs bank" .

figi-ps:TAPS a owl:NamedIndividual .

figi-ps:DBSD figi-gii:hasUniqueTextIdentifier "DBSD" .

figi-ps:TAPS a figi-gii:PricingSource .

figi-ps:DBSH a owl:NamedIndividual .

figi-ps:TAPS skos:prefLabel "fed home loan bank" .

figi-ps:DBSH a figi-gii:PricingSource .

figi-ps:TAPS figi-gii:hasUniqueTextIdentifier "TAPS" .

figi-ps:TASM a owl:NamedIndividual .

figi-ps:DBSH skos:prefLabel "dbs bank (hk) ltd" .

figi-ps:TASM a figi-gii:PricingSource .

figi-ps:DBSH figi-gii:hasUniqueTextIdentifier "DBSH" .

figi-ps:TASM skos:prefLabel "tass mtge abs" .

figi-ps:DBSM a owl:NamedIndividual .

figi-ps:TASM skos:prefLabel "tass wp-handelsbank" .

figi-ps:DBSM a figi-gii:PricingSource .

figi-ps:TASM figi-gii:hasUniqueTextIdentifier "TASM" .

figi-ps:DBSM skos:prefLabel "bank of seast asia" ;
	figi-gii:hasUniqueTextIdentifier "DBSM" .

figi-ps:TBDL a owl:NamedIndividual .

figi-ps:DBSP a owl:NamedIndividual .

figi-ps:TBDL a figi-gii:PricingSource .

figi-ps:DBSP a figi-gii:PricingSource .

figi-ps:TBDL skos:prefLabel "bloomberg-trbk-demo" .

figi-ps:DBSP skos:prefLabel "dbs bk hk ltd 4:30" .

figi-ps:TBDL figi-gii:hasUniqueTextIdentifier "TBDL" .

figi-ps:DBSP figi-gii:hasUniqueTextIdentifier "DBSP" .

figi-ps:TDSX a owl:NamedIndividual .

figi-ps:DBSU a owl:NamedIndividual .

figi-ps:TDSX a figi-gii:PricingSource .

figi-ps:DBSU a figi-gii:PricingSource .

figi-ps:TDSX skos:prefLabel "toronto dominion tom" .

figi-ps:DBSU skos:prefLabel "deutsche bank suisse" .

figi-ps:TDSX figi-gii:hasUniqueTextIdentifier "TDSX" .

figi-ps:DBSU figi-gii:hasUniqueTextIdentifier "DBSU" .

figi-ps:TEBA a owl:NamedIndividual .

figi-ps:DBTB a owl:NamedIndividual .

figi-ps:TEBA a figi-gii:PricingSource .

figi-ps:DBTB a figi-gii:PricingSource .

figi-ps:TEBA skos:prefLabel "economy bank" .

figi-ps:DBTB skos:prefLabel "deutsche aud toms" .

figi-ps:TEBA figi-gii:hasUniqueTextIdentifier "TEBA" .

figi-ps:DBTB figi-gii:hasUniqueTextIdentifier "DBTB" .

figi-ps:TIJI a owl:NamedIndividual .

figi-ps:DBTP a owl:NamedIndividual .

figi-ps:TIJI a figi-gii:PricingSource .

figi-ps:DBTP a figi-gii:PricingSource .

figi-ps:TIJI skos:prefLabel "cfif bank of tianjin" .

figi-ps:DBTP skos:prefLabel "deutsche bank tips" .

figi-ps:TIJI figi-gii:hasUniqueTextIdentifier "TIJI" .

figi-ps:DBTP figi-gii:hasUniqueTextIdentifier "DBTP" .

figi-ps:TIMS a owl:NamedIndividual .

figi-ps:DBTR a owl:NamedIndividual .

figi-ps:TIMS a figi-gii:PricingSource .

figi-ps:DBTR a figi-gii:PricingSource .

figi-ps:TIMS skos:prefLabel "ing inv mgt parallel" .

figi-ps:DBTR skos:prefLabel "deutsche bk turkey" .

figi-ps:TIMS figi-gii:hasUniqueTextIdentifier "TIMS" .

figi-ps:DBTR figi-gii:hasUniqueTextIdentifier "DBTR" .

figi-ps:TING a owl:NamedIndividual .

figi-ps:DBTW a owl:NamedIndividual .

figi-ps:TING a figi-gii:PricingSource .

figi-ps:DBTW a figi-gii:PricingSource .

figi-ps:TING skos:prefLabel "ing turkey" .

figi-ps:DBTW skos:prefLabel "deutsche bk,taiwan" .

figi-ps:TING figi-gii:hasUniqueTextIdentifier "TING" .

figi-ps:DBTW figi-gii:hasUniqueTextIdentifier "DBTW" .

figi-ps:TITU a owl:NamedIndividual .

figi-ps:DBUY a owl:NamedIndividual .

figi-ps:TITU a figi-gii:PricingSource .

figi-ps:DBUY a figi-gii:PricingSource .

figi-ps:TITU skos:prefLabel "titularizadora colom" .

figi-ps:DBUY skos:prefLabel "discount bank urugua" .

figi-ps:TITU figi-gii:hasUniqueTextIdentifier "TITU" .

figi-ps:DBUY figi-gii:hasUniqueTextIdentifier "DBUY" .

figi-ps:TM21 a owl:NamedIndividual .

figi-ps:DBWA a owl:NamedIndividual .

figi-ps:TM21 a figi-gii:PricingSource .

figi-ps:DBWA a figi-gii:PricingSource .

figi-ps:TM21 skos:prefLabel "fms bonds inc" .

figi-ps:DBWA skos:prefLabel "deutsche secs asia" .

figi-ps:TM21 figi-gii:hasUniqueTextIdentifier "TM21" .

figi-ps:DBWA figi-gii:hasUniqueTextIdentifier "DBWA" .

figi-ps:TMBK a owl:NamedIndividual .

figi-ps:DBXM a owl:NamedIndividual .

figi-ps:TMBK a figi-gii:PricingSource .

figi-ps:DBXM a figi-gii:PricingSource .

figi-ps:TMBK skos:prefLabel "enter name here" .

figi-ps:DBXM skos:prefLabel "deutsche bk" .

figi-ps:TMBK figi-gii:hasUniqueTextIdentifier "TMBK" .

figi-ps:DBXM figi-gii:hasUniqueTextIdentifier "DBXM" .

figi-ps:TMH a owl:NamedIndividual .

figi-ps:DBZ a owl:NamedIndividual .

figi-ps:TMH a figi-gii:PricingSource .

figi-ps:DBZ a figi-gii:PricingSource .

figi-ps:TMH skos:prefLabel "botm ufj hong kong" .

figi-ps:DBZ skos:prefLabel "d.b. zwirn and co. lp" .

figi-ps:TMH figi-gii:hasUniqueTextIdentifier "TMH" .

figi-ps:DBZ figi-gii:hasUniqueTextIdentifier "DBZ" .

figi-ps:TMI a owl:NamedIndividual , figi-gii:PricingSource .

figi-ps:DCAP a owl:NamedIndividual .

figi-ps:TMI skos:prefLabel "botm ufj indonesia" .

figi-ps:DCAP a figi-gii:PricingSource .

figi-ps:TMI figi-gii:hasUniqueTextIdentifier "TMI" .

figi-ps:DCAP skos:prefLabel "derivium capital" .

figi-ps:TMIM a owl:NamedIndividual .

figi-ps:DCAP figi-gii:hasUniqueTextIdentifier "DCAP" .

figi-ps:TMIM a figi-gii:PricingSource .

figi-ps:DCBI a owl:NamedIndividual .

figi-ps:TMIM skos:prefLabel "tokyo-mitsubishi plc" .

figi-ps:DCBI a figi-gii:PricingSource .

figi-ps:TMIM figi-gii:hasUniqueTextIdentifier "TMIM" .

figi-ps:DCBI skos:prefLabel "development credit" .

figi-ps:TMIX a owl:NamedIndividual .

figi-ps:DCBI figi-gii:hasUniqueTextIdentifier "DCBI" .

figi-ps:TMIX a figi-gii:PricingSource .

figi-ps:DCFM a owl:NamedIndividual .

figi-ps:TMIX skos:prefLabel "mitsubishi ufj sec" .

figi-ps:DCFM a figi-gii:PricingSource .

figi-ps:TMIX figi-gii:hasUniqueTextIdentifier "TMIX" .

figi-ps:DCFM skos:prefLabel "da cheng fund mgmt" .

figi-ps:TMSG a owl:NamedIndividual .

figi-ps:DCFM figi-gii:hasUniqueTextIdentifier "DCFM" .

figi-ps:TMSG a figi-gii:PricingSource .

figi-ps:DCHY a owl:NamedIndividual .

figi-ps:TMSG skos:prefLabel "botm ufj singapore" .

figi-ps:DCHY a figi-gii:PricingSource .

figi-ps:TMSG figi-gii:hasUniqueTextIdentifier "TMSG" .

figi-ps:DCHY skos:prefLabel "deutsche bank - dchy" .

figi-ps:TMSL a owl:NamedIndividual .

figi-ps:DCHY figi-gii:hasUniqueTextIdentifier "DCHY" .

figi-ps:TMSL a figi-gii:PricingSource .

figi-ps:DCM a owl:NamedIndividual .

figi-ps:TMSL skos:prefLabel "bank of tokyo mits" .

figi-ps:DCM a figi-gii:PricingSource .

figi-ps:TMSL figi-gii:hasUniqueTextIdentifier "TMSL" .

figi-ps:DCM skos:prefLabel "dellacamera capital" .

figi-ps:TMT a owl:NamedIndividual .

figi-ps:DCM figi-gii:hasUniqueTextIdentifier "DCM" .

figi-ps:TMT a figi-gii:PricingSource .

figi-ps:DCMX a owl:NamedIndividual .

figi-ps:TMT skos:prefLabel "btmu tokyo" .

figi-ps:DCMX a figi-gii:PricingSource .

figi-ps:TMT figi-gii:hasUniqueTextIdentifier "TMT" .

figi-ps:DCMX skos:prefLabel "daiwa capmkts europe" .

figi-ps:TMT2 a owl:NamedIndividual .

figi-ps:DCMX figi-gii:hasUniqueTextIdentifier "DCMX" .

figi-ps:TMT2 a figi-gii:PricingSource .

figi-ps:DDBM a owl:NamedIndividual .

figi-ps:TMT2 skos:prefLabel "btmu tokyo 2" .

figi-ps:DDBM a figi-gii:PricingSource .

figi-ps:TMT2 figi-gii:hasUniqueTextIdentifier "TMT2" .

figi-ps:DDBM skos:prefLabel "danske bank - ddbm" .

figi-ps:TMTL a owl:NamedIndividual .

figi-ps:DDBM figi-gii:hasUniqueTextIdentifier "DDBM" .

figi-ps:TMTL a figi-gii:PricingSource .

figi-ps:DDMN a owl:NamedIndividual .

figi-ps:TMTL skos:prefLabel "bk of tky-mitsubishi" .

figi-ps:DDMN a figi-gii:PricingSource .

figi-ps:TMTL figi-gii:hasUniqueTextIdentifier "TMTL" .

figi-ps:DDMN skos:prefLabel "ddm italy non ton" .

figi-ps:TMZA a owl:NamedIndividual .

figi-ps:DDMN figi-gii:hasUniqueTextIdentifier "DDMN" .

figi-ps:TMZA a figi-gii:PricingSource .

figi-ps:DDMT a owl:NamedIndividual .

figi-ps:TMZA skos:prefLabel "bank of tokyo-mits" .

figi-ps:DDMT a figi-gii:PricingSource .

figi-ps:TMZA figi-gii:hasUniqueTextIdentifier "TMZA" .

figi-ps:DDMT skos:prefLabel "ddm italy ton trades" ;
	figi-gii:hasUniqueTextIdentifier "DDMT" .

figi-ps:TOMO a owl:NamedIndividual .

figi-ps:DEBA a owl:NamedIndividual .

figi-ps:TOMO a figi-gii:PricingSource .

figi-ps:DEBA a figi-gii:PricingSource .

figi-ps:TOMO skos:prefLabel "etoms - beta / qa" .

figi-ps:DEBA skos:prefLabel "deutsche bank, sgp" .

figi-ps:TOMO figi-gii:hasUniqueTextIdentifier "TOMO" .

figi-ps:DEBA figi-gii:hasUniqueTextIdentifier "DEBA" .

figi-ps:TOMS a owl:NamedIndividual , figi-gii:PricingSource .

figi-ps:DEKA a owl:NamedIndividual .

figi-ps:TOMS skos:prefLabel "gib toms" .

figi-ps:DEKA a figi-gii:PricingSource .

figi-ps:TOMS figi-gii:hasUniqueTextIdentifier "TOMS" .

figi-ps:DEKA skos:prefLabel "dekabank" .

figi-ps:TPOM a owl:NamedIndividual , figi-gii:PricingSource .

figi-ps:DEKA figi-gii:hasUniqueTextIdentifier "DEKA" .

figi-ps:TPOM skos:prefLabel "aim us enterprise" .

figi-ps:DEMO a owl:NamedIndividual .

figi-ps:TPOM figi-gii:hasUniqueTextIdentifier "TPOM" .

figi-ps:DEMO a figi-gii:PricingSource .

figi-ps:TRAC a owl:NamedIndividual , figi-gii:PricingSource .

figi-ps:DEMO skos:prefLabel "demo portfolio" .

figi-ps:TRAC skos:prefLabel "finra - trace" .

figi-ps:DEMO figi-gii:hasUniqueTextIdentifier "DEMO" .

figi-ps:TRAC figi-gii:hasUniqueTextIdentifier "TRAC" .

figi-ps:TRBB a owl:NamedIndividual .

figi-ps:DEND a owl:NamedIndividual .

figi-ps:TRBB a figi-gii:PricingSource .

figi-ps:DEND a figi-gii:PricingSource .

figi-ps:TRBB skos:prefLabel "abs test inside" ;
	figi-gii:hasUniqueTextIdentifier "TRBB" .

figi-ps:DEND skos:prefLabel "den danske pmi" .

figi-ps:TRCM a owl:NamedIndividual , figi-gii:PricingSource .

figi-ps:DEND figi-gii:hasUniqueTextIdentifier "DEND" .

figi-ps:TRCM skos:prefLabel "finra trac 1mm+/5mm+" .

figi-ps:DENJ a owl:NamedIndividual .

figi-ps:TRCM figi-gii:hasUniqueTextIdentifier "TRCM" .

figi-ps:DENJ a figi-gii:PricingSource .

figi-ps:TREP a owl:NamedIndividual , figi-gii:PricingSource .

figi-ps:DENJ skos:prefLabel "denjoy capital" .

figi-ps:TREP skos:prefLabel "trepp llc" ;
	figi-gii:hasUniqueTextIdentifier "TREP" .

figi-ps:DENJ figi-gii:hasUniqueTextIdentifier "DENJ" .

figi-ps:TRL1 a owl:NamedIndividual , figi-gii:PricingSource .

figi-ps:DEPF a owl:NamedIndividual .

figi-ps:TRL1 skos:prefLabel "finra trace (>=1mm)" .

figi-ps:DEPF a figi-gii:PricingSource .

figi-ps:TRL1 figi-gii:hasUniqueTextIdentifier "TRL1" .

figi-ps:TRL5 a owl:NamedIndividual .

figi-ps:DEPF skos:prefLabel "depfa-fac" .

figi-ps:TRL5 a figi-gii:PricingSource ;
	skos:prefLabel "finra trace (>5mm)" .

figi-ps:DEPF figi-gii:hasUniqueTextIdentifier "DEPF" .

figi-ps:TRL5 figi-gii:hasUniqueTextIdentifier "TRL5" .

figi-ps:TRMT a owl:NamedIndividual .

figi-ps:DEPS a owl:NamedIndividual .

figi-ps:TRMT a figi-gii:PricingSource .

figi-ps:DEPS a figi-gii:PricingSource .

figi-ps:TRMT skos:prefLabel "finra trace (>=250m)" ;
	figi-gii:hasUniqueTextIdentifier "TRMT" .

figi-ps:DEPS skos:prefLabel "depfa" .

figi-ps:TRNK a owl:NamedIndividual , figi-gii:PricingSource .

figi-ps:DEPS figi-gii:hasUniqueTextIdentifier "DEPS" .

figi-ps:TRNK skos:prefLabel "hsbc trinkaus" .

figi-ps:DERI a owl:NamedIndividual .

figi-ps:TRNK figi-gii:hasUniqueTextIdentifier "TRNK" .

figi-ps:DERI a figi-gii:PricingSource .

figi-ps:TRST a owl:NamedIndividual , figi-gii:PricingSource .

figi-ps:DERI skos:prefLabel "deripartners" .

figi-ps:TRST skos:prefLabel "finra trace" .

figi-ps:DERI figi-gii:hasUniqueTextIdentifier "DERI" .

figi-ps:TRST figi-gii:hasUniqueTextIdentifier "TRST" .

figi-ps:DERR a owl:NamedIndividual .

figi-ps:TRYN a owl:NamedIndividual .

figi-ps:DERR a figi-gii:PricingSource .

figi-ps:TRYN a figi-gii:PricingSource ;
	skos:prefLabel "first tryon sec" .

figi-ps:DERR skos:prefLabel "derivation software" .

figi-ps:TRYN figi-gii:hasUniqueTextIdentifier "TRYN" .

figi-ps:TSLV a owl:NamedIndividual .

figi-ps:DERR figi-gii:hasUniqueTextIdentifier "DERR" .

figi-ps:TSLV a figi-gii:PricingSource .

figi-ps:DERZ a owl:NamedIndividual .

figi-ps:TSLV skos:prefLabel "banca transilvania" .

figi-ps:DERZ a figi-gii:PricingSource .

figi-ps:TSLV figi-gii:hasUniqueTextIdentifier "TSLV" .

figi-ps:TSNY a owl:NamedIndividual .

figi-ps:DERZ skos:prefLabel "bank derzhava" .

figi-ps:TSNY a figi-gii:PricingSource ;
	skos:prefLabel "bberg toms demo-test" .

figi-ps:DERZ figi-gii:hasUniqueTextIdentifier "DERZ" .

figi-ps:TSNY figi-gii:hasUniqueTextIdentifier "TSNY" .

figi-ps:DEUV a owl:NamedIndividual .

figi-ps:TSOF a owl:NamedIndividual .

figi-ps:DEUV a figi-gii:PricingSource .

figi-ps:TSOF a figi-gii:PricingSource .

figi-ps:DEUV skos:prefLabel "deutsche bk vietnam" .

figi-ps:TSOF skos:prefLabel "credit suisse t1" .

figi-ps:DEUV figi-gii:hasUniqueTextIdentifier "DEUV" .

figi-ps:TSOF figi-gii:hasUniqueTextIdentifier "TSOF" .

figi-ps:DEXB a owl:NamedIndividual .

figi-ps:TSOG a owl:NamedIndividual .

figi-ps:DEXB a figi-gii:PricingSource .

figi-ps:TSOG a figi-gii:PricingSource ;
	skos:prefLabel "credit suisse t2" .

figi-ps:DEXB skos:prefLabel "dexia bank brussels" .

figi-ps:TSOG figi-gii:hasUniqueTextIdentifier "TSOG" .

figi-ps:TSOH a owl:NamedIndividual .

figi-ps:DEXB skos:prefLabel "dexia capital mkts" .

figi-ps:TSOH a figi-gii:PricingSource .

figi-ps:DEXB figi-gii:hasUniqueTextIdentifier "DEXB" .

figi-ps:TSOH skos:prefLabel "credit suisse t3" ;
	figi-gii:hasUniqueTextIdentifier "TSOH" .

figi-ps:DEXG a owl:NamedIndividual .

figi-ps:TUNE a owl:NamedIndividual .

figi-ps:DEXG a figi-gii:PricingSource .

figi-ps:TUNE a figi-gii:PricingSource ;
	skos:prefLabel "anbima tunnel" .

figi-ps:DEXG skos:prefLabel "dexia group" .

figi-ps:TUNE figi-gii:hasUniqueTextIdentifier "TUNE" .

figi-ps:DEXG figi-gii:hasUniqueTextIdentifier "DEXG" .

figi-ps:TURK a owl:NamedIndividual , figi-gii:PricingSource .

figi-ps:DEXL a owl:NamedIndividual .

figi-ps:TURK skos:prefLabel "cs emerging markets" .

figi-ps:DEXL a figi-gii:PricingSource .

figi-ps:TURK figi-gii:hasUniqueTextIdentifier "TURK" .

figi-ps:DEXL skos:prefLabel "dexia bank brussels" .

figi-ps:UABS a owl:NamedIndividual , figi-gii:PricingSource .

figi-ps:DEXL skos:prefLabel "dexia bil luxembourg" .

figi-ps:UABS skos:prefLabel "ubs ny - mortgages" .

figi-ps:DEXL figi-gii:hasUniqueTextIdentifier "DEXL" .

figi-ps:UABS figi-gii:hasUniqueTextIdentifier "UABS" .

figi-ps:DEXM a owl:NamedIndividual .

figi-ps:UAT a owl:NamedIndividual .

figi-ps:DEXM a figi-gii:PricingSource .

figi-ps:UAT a figi-gii:PricingSource ;
	skos:prefLabel "anz banking uat" .

figi-ps:DEXM skos:prefLabel "dexia bank belg" .

figi-ps:UAT figi-gii:hasUniqueTextIdentifier "UAT" .

figi-ps:UBAB a owl:NamedIndividual .

figi-ps:DEXM figi-gii:hasUniqueTextIdentifier "DEXM" .

figi-ps:UBAB a figi-gii:PricingSource .

figi-ps:DEXP a owl:NamedIndividual .

figi-ps:UBAB skos:prefLabel "united bank africa" .

figi-ps:DEXP a figi-gii:PricingSource .

figi-ps:UBAB figi-gii:hasUniqueTextIdentifier "UBAB" .

figi-ps:UBAN a owl:NamedIndividual .

figi-ps:DEXP skos:prefLabel "belfius technical" .

figi-ps:UBAN a figi-gii:PricingSource .

figi-ps:DEXP figi-gii:hasUniqueTextIdentifier "DEXP" .

figi-ps:DEXS a owl:NamedIndividual .

figi-ps:UBAN skos:prefLabel "united bk of africa" .

figi-ps:DEXS a figi-gii:PricingSource .

figi-ps:UBAN figi-gii:hasUniqueTextIdentifier "UBAN" .

figi-ps:DEXS skos:prefLabel "dexia bnk brussels" ;
	figi-gii:hasUniqueTextIdentifier "DEXS" .

figi-ps:DEXT a owl:NamedIndividual .

figi-ps:UBIZ a owl:NamedIndividual .

figi-ps:DEXT a figi-gii:PricingSource .

figi-ps:UBIZ a figi-gii:PricingSource .

figi-ps:DEXT skos:prefLabel "dexia capital mkts" .

figi-ps:UBIZ skos:prefLabel "centrobanca" .

figi-ps:DEXT figi-gii:hasUniqueTextIdentifier "DEXT" .

figi-ps:UBIZ figi-gii:hasUniqueTextIdentifier "UBIZ" .

figi-ps:DEZE a owl:NamedIndividual .

figi-ps:UBMX a owl:NamedIndividual .

figi-ps:DEZE a figi-gii:PricingSource .

figi-ps:UBMX a figi-gii:PricingSource .

figi-ps:DEZE skos:prefLabel "dezelna bnk slovenia" .

figi-ps:UBMX skos:prefLabel "hvb milan branch" .

figi-ps:DEZE figi-gii:hasUniqueTextIdentifier "DEZE" .

figi-ps:UBMX figi-gii:hasUniqueTextIdentifier "UBMX" .

figi-ps:DFHI a owl:NamedIndividual .

figi-ps:UBSB a owl:NamedIndividual .

figi-ps:DFHI a figi-gii:PricingSource .

figi-ps:UBSB a figi-gii:PricingSource .

figi-ps:DFHI skos:prefLabel "discount and fin house" .

figi-ps:UBSB skos:prefLabel "ubs auto-ex bbt aust" .

figi-ps:DFHI figi-gii:hasUniqueTextIdentifier "DFHI" .

figi-ps:UBSB figi-gii:hasUniqueTextIdentifier "UBSB" .

figi-ps:DFM a owl:NamedIndividual .

figi-ps:UBSX a owl:NamedIndividual .

figi-ps:DFM a figi-gii:PricingSource .

figi-ps:UBSX a figi-gii:PricingSource .

figi-ps:DFM skos:prefLabel "dubai financial mrkt" .

figi-ps:UBSX skos:prefLabel "ubs investment bk" .

figi-ps:DFM figi-gii:hasUniqueTextIdentifier "DFM" .

figi-ps:UBSX figi-gii:hasUniqueTextIdentifier "UBSX" .

figi-ps:DFMJ a owl:NamedIndividual .

figi-ps:UBZA a owl:NamedIndividual .

figi-ps:DFMJ a figi-gii:PricingSource .

figi-ps:UBZA a figi-gii:PricingSource .

figi-ps:DFMJ skos:prefLabel "danareksa securities" .

figi-ps:UBZA skos:prefLabel "ubs secs japan ltd" .

figi-ps:DFMJ figi-gii:hasUniqueTextIdentifier "DFMJ" .

figi-ps:UBZA figi-gii:hasUniqueTextIdentifier "UBZA" .

figi-ps:DGEF a owl:NamedIndividual .

figi-ps:UCBM a owl:NamedIndividual .

figi-ps:DGEF a figi-gii:PricingSource .

figi-ps:UCBM a figi-gii:PricingSource .

figi-ps:DGEF skos:prefLabel "daiwa capital hk" .

figi-ps:UCBM skos:prefLabel "aton llc" .

figi-ps:DGEF figi-gii:hasUniqueTextIdentifier "DGEF" .

figi-ps:UCBM figi-gii:hasUniqueTextIdentifier "UCBM" .

figi-ps:DGI a owl:NamedIndividual .

figi-ps:UGBR a owl:NamedIndividual .

figi-ps:DGI a figi-gii:PricingSource .

figi-ps:UGBR a figi-gii:PricingSource .

figi-ps:DGI skos:prefLabel "degroof gestion inst" .

figi-ps:UGBR skos:prefLabel "garantibank" .

figi-ps:DGI figi-gii:hasUniqueTextIdentifier "DGI" .

figi-ps:UGBR figi-gii:hasUniqueTextIdentifier "UGBR" .

figi-ps:DIA a owl:NamedIndividual .

figi-ps:UHIS a owl:NamedIndividual .

figi-ps:DIA a figi-gii:PricingSource .

figi-ps:UHIS a figi-gii:PricingSource .

figi-ps:DIA skos:prefLabel "denver inv advisers" .

figi-ps:UHIS skos:prefLabel "eesti uhispank" .

figi-ps:DIA figi-gii:hasUniqueTextIdentifier "DIA" .

figi-ps:UHIS figi-gii:hasUniqueTextIdentifier "UHIS" .

figi-ps:DIBD a owl:NamedIndividual .

figi-ps:UMBB a owl:NamedIndividual .

figi-ps:DIBD a figi-gii:PricingSource .

figi-ps:UMBB a figi-gii:PricingSource .

figi-ps:DIBD skos:prefLabel "dubai islamic bank" .

figi-ps:UMBB skos:prefLabel "umb bank" .

figi-ps:DIBD figi-gii:hasUniqueTextIdentifier "DIBD" .

figi-ps:UMBB figi-gii:hasUniqueTextIdentifier "UMBB" .

figi-ps:DIET a owl:NamedIndividual .

figi-ps:UMBM a owl:NamedIndividual .

figi-ps:DIET a figi-gii:PricingSource .

figi-ps:UMBM a figi-gii:PricingSource .

figi-ps:DIET skos:prefLabel "diethniki s.a." .

figi-ps:UMBM skos:prefLabel "umb mortgages" .

figi-ps:DIET figi-gii:hasUniqueTextIdentifier "DIET" .

figi-ps:UMBM figi-gii:hasUniqueTextIdentifier "UMBM" .

figi-ps:DING a owl:NamedIndividual .

figi-ps:UMBS a owl:NamedIndividual .

figi-ps:DING a figi-gii:PricingSource .

figi-ps:UMBS a figi-gii:PricingSource .

figi-ps:DING skos:prefLabel "ing value" .

figi-ps:UMBS skos:prefLabel "ubs tokyo mbs" .

figi-ps:DING figi-gii:hasUniqueTextIdentifier "DING" .

figi-ps:UMBS figi-gii:hasUniqueTextIdentifier "UMBS" .

figi-ps:DINO a owl:NamedIndividual .

figi-ps:VALE a owl:NamedIndividual .

figi-ps:DINO a figi-gii:PricingSource .

figi-ps:VALE a figi-gii:PricingSource .

figi-ps:DINO skos:prefLabel "dinosaur securities" .

figi-ps:VALE skos:prefLabel "valero energy" .

figi-ps:DINO figi-gii:hasUniqueTextIdentifier "DINO" .

figi-ps:VALE figi-gii:hasUniqueTextIdentifier "VALE" .

figi-ps:DISA a owl:NamedIndividual .

figi-ps:VBNC a owl:NamedIndividual .

figi-ps:DISA a figi-gii:PricingSource .

figi-ps:VBNC a figi-gii:PricingSource .

figi-ps:DISA skos:prefLabel "dfmc" .

figi-ps:VBNC skos:prefLabel "banco nac de credito" .

figi-ps:DISA figi-gii:hasUniqueTextIdentifier "DISA" .

figi-ps:VBNC figi-gii:hasUniqueTextIdentifier "VBNC" .

figi-ps:DKBI a owl:NamedIndividual .

figi-ps:VBOD a owl:NamedIndividual .

figi-ps:DKBI a figi-gii:PricingSource .

figi-ps:VBOD a figi-gii:PricingSource .

figi-ps:DKBI skos:prefLabel "dkb international" .

figi-ps:VBOD skos:prefLabel "banco occidental" .

figi-ps:DKBI figi-gii:hasUniqueTextIdentifier "DKBI" .

figi-ps:VBOD figi-gii:hasUniqueTextIdentifier "VBOD" .

figi-ps:DKBS a owl:NamedIndividual .

figi-ps:VENT a owl:NamedIndividual .

figi-ps:DKBS a figi-gii:PricingSource .

figi-ps:VENT a figi-gii:PricingSource .

figi-ps:DKBS skos:prefLabel "dkb securities" .

figi-ps:VENT skos:prefLabel "venture finanzas" .

figi-ps:DKBS figi-gii:hasUniqueTextIdentifier "DKBS" .

figi-ps:VENT figi-gii:hasUniqueTextIdentifier "VENT" .

figi-ps:DKCB a owl:NamedIndividual .

figi-ps:VIPR a owl:NamedIndividual .

figi-ps:DKCB a figi-gii:PricingSource .

figi-ps:VIPR a figi-gii:PricingSource .

figi-ps:DKCB skos:prefLabel "dresdner kleinwort" .

figi-ps:VIPR skos:prefLabel "bbg appliance test" .

figi-ps:DKCB figi-gii:hasUniqueTextIdentifier "DKCB" .

figi-ps:VIPR figi-gii:hasUniqueTextIdentifier "VIPR" .

figi-ps:DKFI a owl:NamedIndividual .

figi-ps:VISB a owl:NamedIndividual .

figi-ps:DKFI a figi-gii:PricingSource .

figi-ps:VISB a figi-gii:PricingSource .

figi-ps:DKFI skos:prefLabel "deka bank" .

figi-ps:VISB skos:prefLabel "ing vysya bank" .

figi-ps:DKFI figi-gii:hasUniqueTextIdentifier "DKFI" .

figi-ps:VISB figi-gii:hasUniqueTextIdentifier "VISB" .

figi-ps:DKST a owl:NamedIndividual .

figi-ps:VLB a owl:NamedIndividual .

figi-ps:DKST a figi-gii:PricingSource .

figi-ps:VLB a figi-gii:PricingSource .

figi-ps:DKST skos:prefLabel "dkst dresdner klein" .

figi-ps:VLB skos:prefLabel "f van lanschot bank" .

figi-ps:DKST figi-gii:hasUniqueTextIdentifier "DKST" .

figi-ps:VLB figi-gii:hasUniqueTextIdentifier "VLB" .

figi-ps:DL a owl:NamedIndividual .

figi-ps:VMD a owl:NamedIndividual .

figi-ps:DL a figi-gii:PricingSource .

figi-ps:VMD a figi-gii:PricingSource .

figi-ps:DL skos:prefLabel "doubleline" .

figi-ps:VMD skos:prefLabel "desjardins sec" .

figi-ps:DL figi-gii:hasUniqueTextIdentifier "DL" .

figi-ps:VMD figi-gii:hasUniqueTextIdentifier "VMD" .

figi-ps:DLA a owl:NamedIndividual .

figi-ps:VONT a owl:NamedIndividual .

figi-ps:DLA a figi-gii:PricingSource .

figi-ps:VONT a figi-gii:PricingSource .

figi-ps:DLA skos:prefLabel "david lerner assoc" .

figi-ps:VONT skos:prefLabel "bank vontobel ag" .

figi-ps:DLA figi-gii:hasUniqueTextIdentifier "DLA" .

figi-ps:VONT figi-gii:hasUniqueTextIdentifier "VONT" .

figi-ps:DLAM a owl:NamedIndividual .

figi-ps:VOT a owl:NamedIndividual , figi-gii:PricingSource ;
	skos:prefLabel "banco votorantim sa" ;
	figi-gii:hasUniqueTextIdentifier "VOT" .

figi-ps:VOTD a owl:NamedIndividual , figi-gii:PricingSource ;
	skos:prefLabel "bco votorantim" ;
	figi-gii:hasUniqueTextIdentifier "VOTD" .

figi-ps:VOTO a owl:NamedIndividual , figi-gii:PricingSource ;
	skos:prefLabel "banco votorantim" ;
	figi-gii:hasUniqueTextIdentifier "VOTO" .

figi-ps:VTBI a owl:NamedIndividual , figi-gii:PricingSource ;
	skos:prefLabel "vtb capital plc" ;
	figi-gii:hasUniqueTextIdentifier "VTBI" .

figi-ps:VTBX a owl:NamedIndividual , figi-gii:PricingSource ;
	skos:prefLabel "vtb capital plc" ;
	figi-gii:hasUniqueTextIdentifier "VTBX" .

figi-ps:VTRR a owl:NamedIndividual , figi-gii:PricingSource ;
	skos:prefLabel "bank vtb24" ;
	figi-gii:hasUniqueTextIdentifier "VTRR" .

figi-ps:WABS a owl:NamedIndividual , figi-gii:PricingSource ;
	skos:prefLabel "wachovia wabs" ;
	figi-gii:hasUniqueTextIdentifier "WABS" .

figi-ps:WBKP a owl:NamedIndividual , figi-gii:PricingSource ;
	skos:prefLabel "bank zachodni wbk" ;
	figi-gii:hasUniqueTextIdentifier "WBKP" .

figi-ps:WBNP a owl:NamedIndividual , figi-gii:PricingSource ;
	skos:prefLabel "bnp paribas bangkok" ;
	figi-gii:hasUniqueTextIdentifier "WBNP" .

figi-ps:WCCB a owl:NamedIndividual , figi-gii:PricingSource ;
	skos:prefLabel "cfet hankou bank" ;
	figi-gii:hasUniqueTextIdentifier "WCCB" .

figi-ps:WDRC a owl:NamedIndividual , figi-gii:PricingSource ;
	skos:prefLabel "ubs stamford" ;
	figi-gii:hasUniqueTextIdentifier "WDRC" .

figi-ps:WDRL a owl:NamedIndividual , figi-gii:PricingSource ;
	skos:prefLabel "ubs london" ;
	figi-gii:hasUniqueTextIdentifier "WDRL" .

figi-ps:WGD a owl:NamedIndividual , figi-gii:PricingSource ;
	skos:prefLabel "cibc world mkts-can" ;
	figi-gii:hasUniqueTextIdentifier "WGD" .

figi-ps:WGSW a owl:NamedIndividual , figi-gii:PricingSource ;
	skos:prefLabel "cibc world markets" ;
	figi-gii:hasUniqueTextIdentifier "WGSW" .

figi-ps:WHSL a owl:NamedIndividual , figi-gii:PricingSource ;
	skos:prefLabel "hanson westhouse" ;
	figi-gii:hasUniqueTextIdentifier "WHSL" .

figi-ps:WLBI a owl:NamedIndividual , figi-gii:PricingSource ;
	skos:prefLabel "west lb london" ;
	figi-gii:hasUniqueTextIdentifier "WLBI" .

figi-ps:WLBT a owl:NamedIndividual , figi-gii:PricingSource ;
	skos:prefLabel "west lb ag" ;
	figi-gii:hasUniqueTextIdentifier "WLBT" .

figi-ps:WMBS a owl:NamedIndividual , figi-gii:PricingSource ;
	skos:prefLabel "wachovia cmbs" ;
	figi-gii:hasUniqueTextIdentifier "WMBS" .

figi-ps:WOLF a owl:NamedIndividual , figi-gii:PricingSource ;
	skos:prefLabel "armored wolf, llc" ;
	figi-gii:hasUniqueTextIdentifier "WOLF" .

figi-ps:WOTC a owl:NamedIndividual , figi-gii:PricingSource ;
	skos:prefLabel "gretai sec market" ;
	figi-gii:hasUniqueTextIdentifier "WOTC" .

figi-ps:WSPL a owl:NamedIndividual , figi-gii:PricingSource ;
	skos:prefLabel "wachovia pools" ;
	figi-gii:hasUniqueTextIdentifier "WSPL" .

figi-ps:XBBT a owl:NamedIndividual , figi-gii:PricingSource ;
	skos:prefLabel "cbbt internal comp" ;
	figi-gii:hasUniqueTextIdentifier "XBBT" .

figi-ps:XNES a owl:NamedIndividual , figi-gii:PricingSource ;
	skos:prefLabel "excellence nessuah" ;
	figi-gii:hasUniqueTextIdentifier "XNES" .

_:node1fqlq18m7x1 a owl:Restriction ;
	owl:onProperty figi-gii:hasUniqueTextIdentifier ;
	owl:qualifiedCardinality "1"^^xsd:nonNegativeInteger ;
	owl:onDataRange xsd:string .

_:node1fqlq18m7x10 rdf:first _:node1fqlq18m7x9 ;
	rdf:rest _:node1fqlq18m7x12 .

_:node1fqlq18m7x11 a owl:Restriction ;
	owl:onProperty figi-gii:isClassifiedBy ;
	owl:onClass figi-gii:SecurityType ;
	owl:minQualifiedCardinality "1"^^xsd:nonNegativeInteger .

_:node1fqlq18m7x12 rdf:first _:node1fqlq18m7x11 ;
	rdf:rest _:node1fqlq18m7x14 .

_:node1fqlq18m7x13 a owl:Restriction ;
	owl:onProperty figi-gii:isIdentifiedBy ;
	owl:onClass figi-gii:FinancialInstrumentName ;
	owl:minQualifiedCardinality "1"^^xsd:nonNegativeInteger .

_:node1fqlq18m7x14 rdf:first _:node1fqlq18m7x13 ;
	rdf:rest _:node1fqlq18m7x16 .

_:node1fqlq18m7x15 a owl:Restriction .
