# baseURI: http://finregont.com/fro/cfr/Code_Federal_Regulations.ttl
# imports: http://finregont.com/fro/ref/US_LegalReference.ttl
# prefix: fro-cfr

@prefix : <http://finregont.com/fro/cfr/Code_Federal_Regulations.ttl#> .
@prefix dct: <http://purl.org/dc/terms/> .
@prefix fro-cfr: <http://finregont.com/fro/cfr/Code_Federal_Regulations.ttl#> .
@prefix fro-leg-ref: <http://finregont.com/fro/ref/LegalReference.ttl#> .
@prefix lkif-action: <http://www.estrellaproject.org/lkif-core/action.owl#> .
@prefix lkif-expr: <http://www.estrellaproject.org/lkif-core/expression.owl#> .
@prefix lkif-mereo: <http://www.estrellaproject.org/lkif-core/mereology.owl#> .
@prefix lkif-norm: <http://www.estrellaproject.org/lkif-core/norm.owl#> .
@prefix lkif-proc: <http://www.estrellaproject.org/lkif-core/process.owl#> .
@prefix lkif-top: <http://www.estrellaproject.org/lkif-core/lkif-top.owl#> .
@prefix owl: <http://www.w3.org/2002/07/owl#> .
@prefix rdf: <http://www.w3.org/1999/02/22-rdf-syntax-ns#> .
@prefix rdfs: <http://www.w3.org/2000/01/rdf-schema#> .
@prefix skos: <http://www.w3.org/2004/02/skos/core#> .
@prefix sm: <http://www.omg.org/techprocess/ab/SpecificationMetadata/> .
@prefix spinmap: <http://spinrdf.org/spinmap#> .
@prefix xml: <http://www.w3.org/XML/1998/namespace> .
@prefix xsd: <http://www.w3.org/2001/XMLSchema#> .

<http://finregont.com/fro/cfr/Code_Federal_Regulations.ttl>
  rdf:type owl:Ontology ;
  dct:license "https://opensource.org/licenses/GPL-3.0" ;
  sm:author "Jurgen Ziemer" ;
  sm:copyright "Jayzed Data Models Inc." ;
  rdfs:comment "The ontology model for the US Code of Federal Regulations. It has the ontology target classes for Part, Volume, Title, Section, Chapter,  and Paragraph." ;
  rdfs:label "Financial Regulation Ontology: Code of Federal Regulations module" ;
  owl:imports <http://finregont.com/fro/ref/US_LegalReference.ttl> ;
  owl:versionInfo "Created with TopBraid Composer" ;
.
fro-cfr:CFR_Annual_Edition_2016_Title_12
  rdf:type fro-cfr:CFR_Edition ;
  rdf:type owl:NamedIndividual ;
  fro-leg-ref:hasEditionText "CFR Annual Edition Title 12" ;
  lkif-expr:bears fro-cfr:Definitional_Expression_US_Dodd_Frank_Act ;
  rdfs:label "CFR Annual Edition Title 12 (2016)" ;
.
fro-cfr:CFR_Annual_Edition_2016_Title_17
  rdf:type fro-cfr:CFR_Edition ;
  rdf:type owl:NamedIndividual ;
  fro-leg-ref:hasEditionText "fro-cfr:CFR_Title-17" ;
  lkif-expr:bears fro-cfr:Definitional_Expression_US_Investment_Adviser_Regulation ;
  lkif-mereo:member fro-cfr:CFR_Title-17 ;
  rdfs:label "CFR Annual Edition 2016 Title 17" ;
.
fro-cfr:CFR_Chapter
  rdf:type owl:Class ;
  sm:author "Jurgen Ziemer" ;
  sm:copyright "Jayzed Data Models Inc." ;
  rdfs:label "CFR Chapter" ;
  rdfs:subClassOf fro-cfr:CFR_Component ;
  rdfs:subClassOf [
      rdf:type owl:Restriction ;
      owl:onProperty fro-leg-ref:divides ;
      owl:someValuesFrom fro-cfr:CFR_Title ;
    ] ;
  skos:definition "Each CFR title is divided into chapters, which usually bear the name of the issuing agency." ;
.
fro-cfr:CFR_Component
  rdf:type owl:Class ;
  rdfs:label "CFR Component" ;
  rdfs:subClassOf fro-cfr:CodeFederalRegulations ;
  skos:definition "A superclass for CFR components: Chapter, Paragraph, Part, Section, Title and Volume" ;
.
fro-cfr:CFR_Edition
  rdf:type owl:Class ;
  sm:author "Jurgen Ziemer" ;
  sm:copyright "Jayzed Data Models Inc." ;
  rdfs:comment "A collection class for CFR sections and paragraphs. This is to differentiate CFR from other regulations. E.g. the European Alternative Investment Fund Managers Directive will be a sibling to this class." ;
  rdfs:isDefinedBy <https://www.gpo.gov/fdsys/browse/collectionCfr.action?collectionCode=CFR> ;
  rdfs:label "CFR Edition" ;
  rdfs:seeAlso <https://www.gpo.gov/help/index.html#about_code_of_federal_regulations.htm> ;
  rdfs:subClassOf fro-cfr:CodeFederalRegulations ;
  rdfs:subClassOf [
      rdf:type owl:Restriction ;
      owl:onProperty fro-leg-ref:hasEditionText ;
      owl:someValuesFrom xsd:string ;
    ] ;
  skos:definition "The Code of Federal Regulations (CFR) annual edition is the codification of the general and permanent rules published in the Federal Register by the departments and agencies of the Federal Government" ;
.
fro-cfr:CFR_Note
  rdf:type owl:Class ;
  rdfs:isDefinedBy <https://www.gpo.gov/fdsys/bulkdata/CFR/resources/CFRMergedXML.xsd> ;
  rdfs:label "CFR Note" ;
  rdfs:subClassOf fro-cfr:CFR_Component ;
  rdfs:subClassOf [
      rdf:type owl:Restriction ;
      owl:onProperty fro-cfr:hasNoteText ;
      owl:someValuesFrom xsd:string ;
    ] ;
  skos:definition """Used for smalltype \"Note:\" entries. [annex, appendix, attach, 
    ar, cgcindex, enclo, exhibit, extract, figure, guide, part, 
    ptcindex, redes, regtext, sched, section, sfar, subchap, 
    subpart, supple, table, text, toc, tscindex]""" ;
.
fro-cfr:CFR_Parapraph
  rdf:type owl:Class ;
  rdfs:label "CFR Paragraph" ;
  rdfs:subClassOf fro-cfr:CFR_Component ;
  rdfs:subClassOf [
      rdf:type owl:Restriction ;
      owl:onProperty fro-leg-ref:divides ;
      owl:someValuesFrom fro-cfr:CFR_Section ;
    ] ;
  skos:definition "Paragraph is the atomic piece of text in the CFR document. It is not divided any further." ;
.
fro-cfr:CFR_Part
  rdf:type owl:Class ;
  sm:author "Jurgen Ziemer" ;
  sm:copyright "Jayzed Data Models Inc." ;
  rdfs:label "CFR Part" ;
  rdfs:subClassOf fro-cfr:CFR_Component ;
  rdfs:subClassOf [
      rdf:type owl:Restriction ;
      owl:onProperty fro-leg-ref:divides ;
      owl:someValuesFrom fro-cfr:CFR_Chapter ;
    ] ;
  skos:definition "Part is a major division within Chapters and Subchapters. " ;
.
fro-cfr:CFR_Section
  rdf:type owl:Class ;
  rdfs:label "CFR Section" ;
  rdfs:subClassOf fro-cfr:CFR_Component ;
  rdfs:subClassOf [
      rdf:type owl:Restriction ;
      owl:onProperty fro-leg-ref:divides ;
      owl:someValuesFrom fro-cfr:CFR_Part ;
    ] ;
  skos:definition "CFR document are organized in sections. A section contains group or container tag for search and retrieval purposes." ;
.
fro-cfr:CFR_Title
  rdf:type owl:Class ;
  sm:author "Jurgen Ziemer" ;
  sm:copyright "Jayzed Data Models Inc." ;
  rdfs:label "CFR Title" ;
  rdfs:subClassOf fro-cfr:CFR_Component ;
  rdfs:subClassOf [
      rdf:type owl:Restriction ;
      owl:onProperty lkif-mereo:member_of ;
      owl:someValuesFrom fro-leg-ref:DocumentEdition ;
    ] ;
  skos:definition "The Code of Federal Regulations is divided into 50 titles that represent broad areas subject to Federal regulation." ;
.
fro-cfr:CFR_Title-12
  rdf:type fro-cfr:CFR_Title ;
  fro-leg-ref:hasTitleText "BANKS and BANKING" ;
  lkif-expr:bears fro-leg-ref:Definitional_Expression_US_AdvisorRegulation ;
  lkif-mereo:member_of fro-cfr:CFR_Annual_Edition_2016_Title_12 ;
  rdfs:label "BANKS and BANKING" ;
.
fro-cfr:CFR_Title-12_Chapter-2
  rdf:type fro-cfr:CFR_Chapter ;
  rdf:type owl:NamedIndividual ;
  fro-cfr:hasChapterText "Chapter II - FEDERAL RESERVE SYSTEM" ;
  fro-leg-ref:divides fro-cfr:CFR_Title-12 ;
  rdfs:label "Chapter II - FEDERAL RESERVE SYSTEM" ;
.
fro-cfr:CFR_Title-12_Part-217
  rdf:type fro-cfr:CFR_Part ;
  rdf:type owl:NamedIndividual ;
  fro-cfr:hasPartText "12 CFR 217 - CAPITAL ADEQUACY OF BOARD-REGULATED INSTITUTIONS" ;
  fro-leg-ref:divides fro-cfr:CFR_Title-12_Chapter-2 ;
  rdfs:label "12 CFR 217 - CAPITAL ADEQUACY OF BOARD-REGULATED INSTITUTIONS" ;
.
fro-cfr:CFR_Title-12_Part-225
  rdf:type fro-cfr:CFR_Part ;
  rdf:type owl:NamedIndividual ;
  fro-cfr:hasPartText "12 CFR Part 225 - BANK HOLDING COMPANIES AND CHANGE IN BANK CONTROL (REGULATION Y)" ;
  fro-leg-ref:divides fro-cfr:CFR_Title-12_Chapter-2 ;
  rdfs:label "Part 225 - BANK HOLDING COMPANIES AND CHANGE IN BANK CONTROL (REGULATION Y)" ;
.
fro-cfr:CFR_Title-12_Part-252
  rdf:type fro-cfr:CFR_Part ;
  rdf:type owl:NamedIndividual ;
  fro-cfr:hasPartText "Part 252 - ENHANCED PRUDENTIAL STANDARDS (REGULATION YY)" ;
  fro-leg-ref:divides fro-cfr:CFR_Title-12_Chapter-2 ;
  rdfs:label "Part 252 - ENHANCED PRUDENTIAL STANDARDS (REGULATION YY)" ;
.
fro-cfr:CFR_Title-17
  rdf:type fro-cfr:CFR_Title ;
  fro-leg-ref:hasTitleText "RULES AND REGULATIONS, INVESTMENT ADVISERS ACT OF 1940" ;
  lkif-expr:bears fro-leg-ref:Definitional_Expression_US_AdvisorRegulation ;
  lkif-mereo:member_of fro-cfr:CFR_Annual_Edition_2016_Title_17 ;
  rdfs:label "CFR Title: RULES AND REGULATIONS, INVESTMENT ADVISERS ACT OF 1940" ;
.
fro-cfr:CFR_Title-17_Chapter-2
  rdf:type fro-cfr:CFR_Chapter ;
  rdf:type owl:NamedIndividual ;
  fro-cfr:hasChapterText "Chapter II - SECURITIES AND EXCHANGE COMMISSION (CONTINUED) (Parts 200 - 399)" ;
  fro-leg-ref:divides fro-cfr:CFR_Title-17 ;
  rdfs:label "Chapter II - SECURITIES AND EXCHANGE COMMISSION" ;
.
fro-cfr:CFR_Title-17_Part-275
  rdf:type fro-cfr:CFR_Part ;
  rdf:type owl:NamedIndividual ;
  fro-cfr:hasPartText "Part 275 - RULES AND REGULATIONS, INVESTMENT ADVISERS ACT OF 1940" ;
  fro-leg-ref:divides fro-cfr:CFR_Title-17_Chapter-2 ;
  rdfs:label "Part 275 - RULES AND REGULATIONS, INVESTMENT ADVISERS ACT OF 1940" ;
.
fro-cfr:CFR_Volume
  rdf:type owl:Class ;
  sm:author "Jurgen Ziemer" ;
  sm:copyright "Jayzed Data Models Inc." ;
  rdfs:label "CFR Volume" ;
  rdfs:subClassOf fro-cfr:CFR_Component ;
  skos:definition "The 50 subject matter titles contain one or more individual volumes, which are updated once each calendar year, on a staggered basis." ;
.
fro-cfr:CFR_Volume-3
  rdf:type fro-cfr:CFR_Volume ;
  rdf:type owl:NamedIndividual ;
  fro-cfr:hasVolumeText "CFR Title 17 Volume 3" ;
  lkif-mereo:component_of fro-cfr:CFR_Title-17 ;
  rdfs:label "CFR Title 17 Volume 3" ;
.
fro-cfr:CodeFederalRegulations
  rdf:type owl:Class ;
  rdfs:label "Code of Federal Regulations" ;
  rdfs:subClassOf lkif-norm:Regulation ;
  skos:definition "A collection class for CFR Edition and Components." ;
.
fro-cfr:Definitional_Expression_US_Dodd_Frank_Act
  rdf:type lkif-norm:Definitional_Expression ;
  rdf:type owl:NamedIndividual ;
  lkif-expr:medium fro-cfr:CFR_Annual_Edition_2016_Title_12 ;
  lkif-proc:created_by fro-leg-ref:Rulemaking_IAA_Amended_2012 ;
  rdfs:label "Definitional expression for Investment Adviser Regulation" ;
.
fro-cfr:Definitional_Expression_US_Investment_Adviser_Regulation
  rdf:type lkif-norm:Definitional_Expression ;
  rdf:type owl:NamedIndividual ;
  lkif-expr:medium fro-cfr:CFR_Annual_Edition_2016_Title_17 ;
  lkif-proc:created_by fro-leg-ref:Rulemaking_IAA_Amended_2012 ;
  rdfs:label "Definitional expression for Investment Adviser Regulation" ;
.
fro-cfr:hasAuthorizationText
  rdf:type owl:DatatypeProperty ;
  rdfs:domain fro-cfr:CFR_Component ;
  rdfs:label "Authorization Text" ;
  rdfs:range xsd:string ;
  rdfs:subPropertyOf fro-leg-ref:hasComponentText ;
  skos:definition "A text property with legal authorization for the regulation. Typically references to United States Code." ;
  skos:example "<\"15 U.S.C. 80b-2(a)(11)(G), 80b-2(a)(11)(H), 80b-2(a)(17), 80b-3, 80b-4, 80b-4a, 80b-6(4), 80b-6a, and 80b-11, unless otherwise noted.\"> (for CFR Part 275)" ;
.
fro-cfr:hasCFR_ComponentText
  rdf:type owl:DatatypeProperty ;
  rdfs:domain fro-cfr:CFR_Component ;
  rdfs:label "Component Text" ;
  rdfs:range xsd:string ;
  rdfs:subPropertyOf fro-leg-ref:hasComponentText ;
  skos:definition "The text of a CFR component. This a the actual text of the CFR Paragraph, Note etc." ;
.
fro-cfr:hasChapterText
  rdf:type owl:DatatypeProperty ;
  rdfs:domain fro-cfr:CFR_Chapter ;
  rdfs:label "Chapter Text" ;
  rdfs:range xsd:string ;
  rdfs:subPropertyOf fro-leg-ref:hasComponentName ;
  skos:definition "The text of a CFR Chapter." ;
.
fro-cfr:hasNoteText
  rdf:type owl:DatatypeProperty ;
  rdfs:domain fro-cfr:CFR_Component ;
  rdfs:label "Note Text" ;
  rdfs:range xsd:string ;
  rdfs:subPropertyOf fro-leg-ref:hasComponentText ;
  skos:definition "The text of a CFR Note." ;
.
fro-cfr:hasParagraphEnumText
  rdf:type owl:DatatypeProperty ;
  rdfs:comment "CFR ontology denomalized the USLM Enum into this data property." ;
  rdfs:domain fro-cfr:CFR_Parapraph ;
  rdfs:label "Paragraph Enum Text" ;
  rdfs:range xsd:string ;
  rdfs:subPropertyOf fro-leg-ref:hasComponentText ;
  skos:definition "The text of a CFR Paragraph Enumeration. " ;
.
fro-cfr:hasParagraphText
  rdf:type owl:DatatypeProperty ;
  rdfs:domain fro-cfr:CFR_Parapraph ;
  rdfs:label "Paragraph Text" ;
  rdfs:range xsd:string ;
  rdfs:subPropertyOf fro-leg-ref:hasComponentText ;
  skos:definition "The text of the CFR paragraph" ;
.
fro-cfr:hasPartText
  rdf:type owl:DatatypeProperty ;
  rdfs:domain fro-cfr:CFR_Part ;
  rdfs:label "PartText" ;
  rdfs:range xsd:string ;
  rdfs:subPropertyOf fro-leg-ref:hasComponentName ;
  skos:definition "The text of the CFR Part, usually a short name or description." ;
.
fro-cfr:hasRuleText
  rdf:type owl:DatatypeProperty ;
  rdfs:label "Rule Text" ;
  rdfs:range xsd:string ;
  skos:definition "The text of the CFR rule." ;
.
fro-cfr:hasSectionCitation
  rdf:type owl:DatatypeProperty ;
  rdfs:comment "The Code of Federal Regulations (CFR) ontology denomalizes the USLM class into this data property." ;
  rdfs:domain fro-cfr:CFR_Section ;
  rdfs:label "Section Citation" ;
  rdfs:range xsd:string ;
  skos:definition "The text of the CFR citation, usually for a CFR Section" ;
.
fro-cfr:hasSectionNumber
  rdf:type owl:DatatypeProperty ;
  rdfs:domain fro-cfr:CFR_Section ;
  rdfs:label "Section Number" ;
  rdfs:range xsd:string ;
  skos:definition "The section munber is derived from the United States Legilative Model NUM element." ;
  skos:example "ยง 275.0-4" ;
.
fro-cfr:hasSectionSubject
  rdf:type owl:DatatypeProperty ;
  rdfs:domain fro-cfr:CFR_Section ;
  rdfs:label "Section Subject" ;
  rdfs:range xsd:string ;
  rdfs:subPropertyOf fro-leg-ref:hasComponentName ;
  skos:definition "The subject of the section. A short heading/name." ;
  skos:example "\"References to rules and regulations.\"" ;
.
fro-cfr:hasVolumeText
  rdf:type owl:DatatypeProperty ;
  rdfs:domain fro-cfr:CFR_Volume ;
  rdfs:label "Volume Text" ;
  rdfs:range xsd:string ;
  rdfs:subPropertyOf fro-leg-ref:hasComponentName ;
  skos:definition "A short textual description for the CFR volume." ;
.
fro-leg-ref:divided_by
  owl:inverseOf fro-leg-ref:divides ;
.
lkif-expr:utterer
  lkif-expr:utterer fro-leg-ref:RegulatoryAuthority_SecuritiesAndExchangeCommission ;
.
