# baseURI: https://spec.edmcouncil.org/fibo/ontology/master/2021Q4/SEC/Securities/SecuritiesRestrictions/
# imports: https://spec.edmcouncil.org/fibo/ontology/master/2021Q4/BE/GovernmentEntities/NorthAmericanJurisdiction/USGovernmentEntitiesAndJurisdictions/
# imports: https://spec.edmcouncil.org/fibo/ontology/master/2021Q4/BE/LegalEntities/LegalPersons/
# imports: https://spec.edmcouncil.org/fibo/ontology/master/2021Q4/BE/OwnershipAndControl/OwnershipParties/
# imports: https://spec.edmcouncil.org/fibo/ontology/master/2021Q4/FBC/FinancialInstruments/FinancialInstruments/
# imports: https://spec.edmcouncil.org/fibo/ontology/master/2021Q4/FBC/FunctionalEntities/RegulatoryAgencies/
# imports: https://spec.edmcouncil.org/fibo/ontology/master/2021Q4/FND/AgentsAndPeople/People/
# imports: https://spec.edmcouncil.org/fibo/ontology/master/2021Q4/FND/Agreements/Contracts/
# imports: https://spec.edmcouncil.org/fibo/ontology/master/2021Q4/FND/DatesAndTimes/FinancialDates/
# imports: https://spec.edmcouncil.org/fibo/ontology/master/2021Q4/FND/Law/Jurisdiction/
# imports: https://spec.edmcouncil.org/fibo/ontology/master/2021Q4/FND/Law/LegalCapacity/
# imports: https://spec.edmcouncil.org/fibo/ontology/master/2021Q4/FND/Law/LegalCore/
# imports: https://spec.edmcouncil.org/fibo/ontology/master/2021Q4/FND/Organizations/FormalOrganizations/
# imports: https://spec.edmcouncil.org/fibo/ontology/master/2021Q4/FND/Relations/Relations/
# imports: https://spec.edmcouncil.org/fibo/ontology/master/2021Q4/FND/Utilities/AnnotationVocabulary/
# imports: https://spec.edmcouncil.org/fibo/ontology/master/2021Q4/SEC/Securities/SecuritiesListings/
# imports: https://www.omg.org/spec/LCC/Countries/CountryRepresentation/
# imports: https://www.omg.org/spec/LCC/Languages/LanguageRepresentation/

@base <https://spec.edmcouncil.org/fibo/ontology/master/2021Q4/SEC/Securities/SecuritiesRestrictions/> .
@prefix dct: <http://purl.org/dc/terms/> .
@prefix fibo-be-ge-usj: <https://spec.edmcouncil.org/fibo/ontology/BE/GovernmentEntities/NorthAmericanJurisdiction/USGovernmentEntitiesAndJurisdictions/> .
@prefix fibo-be-le-lp: <https://spec.edmcouncil.org/fibo/ontology/BE/LegalEntities/LegalPersons/> .
@prefix fibo-be-oac-opty: <https://spec.edmcouncil.org/fibo/ontology/BE/OwnershipAndControl/OwnershipParties/> .
@prefix fibo-fbc-fi-fi: <https://spec.edmcouncil.org/fibo/ontology/FBC/FinancialInstruments/FinancialInstruments/> .
@prefix fibo-fnd-agr-ctr: <https://spec.edmcouncil.org/fibo/ontology/FND/Agreements/Contracts/> .
@prefix fibo-fnd-dt-fd: <https://spec.edmcouncil.org/fibo/ontology/FND/DatesAndTimes/FinancialDates/> .
@prefix fibo-fnd-law-jur: <https://spec.edmcouncil.org/fibo/ontology/FND/Law/Jurisdiction/> .
@prefix fibo-fnd-law-lcap: <https://spec.edmcouncil.org/fibo/ontology/FND/Law/LegalCapacity/> .
@prefix fibo-fnd-org-fm: <https://spec.edmcouncil.org/fibo/ontology/FND/Organizations/FormalOrganizations/> .
@prefix fibo-fnd-rel-rel: <https://spec.edmcouncil.org/fibo/ontology/FND/Relations/Relations/> .
@prefix fibo-fnd-utl-av: <https://spec.edmcouncil.org/fibo/ontology/FND/Utilities/AnnotationVocabulary/> .
@prefix fibo-sec-sec-lst: <https://spec.edmcouncil.org/fibo/ontology/SEC/Securities/SecuritiesListings/> .
@prefix fibo-sec-sec-rst: <https://spec.edmcouncil.org/fibo/ontology/SEC/Securities/SecuritiesRestrictions/> .
@prefix lcc-cr: <https://www.omg.org/spec/LCC/Countries/CountryRepresentation/> .
@prefix lcc-lr: <https://www.omg.org/spec/LCC/Languages/LanguageRepresentation/> .
@prefix owl: <http://www.w3.org/2002/07/owl#> .
@prefix rdf: <http://www.w3.org/1999/02/22-rdf-syntax-ns#> .
@prefix rdfs: <http://www.w3.org/2000/01/rdf-schema#> .
@prefix skos: <http://www.w3.org/2004/02/skos/core#> .
@prefix sm: <http://www.omg.org/techprocess/ab/SpecificationMetadata/> .
@prefix xsd: <http://www.w3.org/2001/XMLSchema#> .

<https://spec.edmcouncil.org/fibo/ontology/SEC/Securities/SecuritiesRestrictions/>
	a owl:Ontology ;
	rdfs:label "Securities Restrictions Ontology" ;
	dct:abstract "This ontology defines the concepts related to restrictions on finanicial instruments, securities and listings." ;
	dct:license "http://opensource.org/licenses/MIT"^^xsd:anyURI ;
	sm:contentLanguage "https://www.w3.org/TR/owl2-quick-reference/"^^xsd:anyURI ;
	sm:copyright
		"Copyright (c) 2016-2021 EDM Council, Inc." ,
		"Copyright (c) 2018-2021 Object Management Group, Inc."
		;
	sm:dependsOn
		"https://spec.edmcouncil.org/fibo/ontology/BE/"^^xsd:anyURI ,
		"https://spec.edmcouncil.org/fibo/ontology/FBC/"^^xsd:anyURI ,
		"https://spec.edmcouncil.org/fibo/ontology/FND/"^^xsd:anyURI ,
		"https://www.omg.org/spec/LCC/"^^xsd:anyURI
		;
	sm:fileAbbreviation "fibo-sec-sec-rst" ;
	sm:filename "SecuritiesRestrictions.rdf" ;
	owl:imports
		<https://spec.edmcouncil.org/fibo/ontology/master/2021Q4/BE/GovernmentEntities/NorthAmericanJurisdiction/USGovernmentEntitiesAndJurisdictions/> ,
		<https://spec.edmcouncil.org/fibo/ontology/master/2021Q4/BE/LegalEntities/LegalPersons/> ,
		<https://spec.edmcouncil.org/fibo/ontology/master/2021Q4/BE/OwnershipAndControl/OwnershipParties/> ,
		<https://spec.edmcouncil.org/fibo/ontology/master/2021Q4/FBC/FinancialInstruments/FinancialInstruments/> ,
		<https://spec.edmcouncil.org/fibo/ontology/master/2021Q4/FBC/FunctionalEntities/RegulatoryAgencies/> ,
		<https://spec.edmcouncil.org/fibo/ontology/master/2021Q4/FND/AgentsAndPeople/People/> ,
		<https://spec.edmcouncil.org/fibo/ontology/master/2021Q4/FND/Agreements/Contracts/> ,
		<https://spec.edmcouncil.org/fibo/ontology/master/2021Q4/FND/DatesAndTimes/FinancialDates/> ,
		<https://spec.edmcouncil.org/fibo/ontology/master/2021Q4/FND/Law/Jurisdiction/> ,
		<https://spec.edmcouncil.org/fibo/ontology/master/2021Q4/FND/Law/LegalCapacity/> ,
		<https://spec.edmcouncil.org/fibo/ontology/master/2021Q4/FND/Law/LegalCore/> ,
		<https://spec.edmcouncil.org/fibo/ontology/master/2021Q4/FND/Organizations/FormalOrganizations/> ,
		<https://spec.edmcouncil.org/fibo/ontology/master/2021Q4/FND/Relations/Relations/> ,
		<https://spec.edmcouncil.org/fibo/ontology/master/2021Q4/FND/Utilities/AnnotationVocabulary/> ,
		<https://spec.edmcouncil.org/fibo/ontology/master/2021Q4/SEC/Securities/SecuritiesListings/> ,
		<https://www.omg.org/spec/LCC/Countries/CountryRepresentation/> ,
		<https://www.omg.org/spec/LCC/Languages/LanguageRepresentation/>
		;
	owl:versionIRI <https://spec.edmcouncil.org/fibo/ontology/master/2021Q4/SEC/Securities/SecuritiesRestrictions/> ;
	skos:changeNote
		"The https://spec.edmcouncil.org/fibo/ontology/SEC/Securities/SecuritiesRestrictions.rdf version of the ontology was modified to eliminate an unused ontology import and to augment the information associated with references needed to define depositary receipts." ,
		"The https://spec.edmcouncil.org/fibo/ontology/SEC/Securities/SecuritiesRestrictions.rdf version of the ontology was modified to eliminate duplication of concepts in LCC." ,
		"The https://spec.edmcouncil.org/fibo/ontology/SEC/Securities/SecuritiesRestrictions.rdf version of the ontology was modified to fix spelling errors." ,
		"The https://spec.edmcouncil.org/fibo/ontology/SEC/Securities/SecuritiesRestrictions.rdf version of the ontology was modified to reflect the change in representation of a listing." ,
		"The https://spec.edmcouncil.org/fibo/ontology/SEC/Securities/SecuritiesRestrictions.rdf version of the ontology was modified to simplify the hierarchy with respect to regulatory requirements and eliminate deprecated elements."
		;
	fibo-fnd-utl-av:hasMaturityLevel fibo-fnd-utl-av:Release ;
	.

fibo-fbc-fi-fi:FinancialInstrument
	a owl:Class ;
	rdfs:subClassOf [
		a owl:Restriction ;
		owl:onProperty fibo-sec-sec-rst:hasRestriction ;
		owl:onClass fibo-sec-sec-rst:SecuritiesRestriction ;
		owl:minQualifiedCardinality "0"^^xsd:nonNegativeInteger ;
	] ;
	.

fibo-sec-sec-lst:Listing
	a owl:Class ;
	rdfs:subClassOf [
		a owl:Restriction ;
		owl:onProperty fibo-sec-sec-rst:hasRestriction ;
		owl:onClass fibo-sec-sec-rst:SecuritiesRestriction ;
		owl:minQualifiedCardinality "0"^^xsd:nonNegativeInteger ;
	] ;
	.

fibo-sec-sec-rst:BlueSkyLaw
	a owl:Class ;
	rdfs:subClassOf fibo-sec-sec-rst:SecuritiesRegulation ;
	rdfs:label "Blue-Sky law" ;
	rdfs:isDefinedBy <https://spec.edmcouncil.org/fibo/ontology/SEC/Securities/SecuritiesRestrictions/> ;
	skos:definition "securities regulation passed by various states, designed to protect investors against securities fraud by requiring sellers of new issues to register their offerings and provide financial details" ;
	fibo-fnd-utl-av:explanatoryNote "This allows investors to base their judgments on trustworthy data." ;
	.

fibo-sec-sec-rst:ContractualRestriction
	a owl:Class ;
	rdfs:subClassOf
		fibo-fnd-agr-ctr:ContractualCommitment ,
		fibo-sec-sec-rst:SecuritiesRestriction ,
		[
			a owl:Restriction ;
			owl:onProperty fibo-fnd-rel-rel:isMandatedBy ;
			owl:allValuesFrom fibo-fnd-agr-ctr:Contract ;
		]
		;
	rdfs:label "contractual restriction" ;
	rdfs:isDefinedBy <https://spec.edmcouncil.org/fibo/ontology/SEC/Securities/SecuritiesRestrictions/> ;
	skos:definition "contract terms setting out restrictions on either the holder or the issuer of the security, as specified in the terms of the instrument itself" ;
	.

fibo-sec-sec-rst:IndividualInvestor
	a owl:Class ;
	rdfs:subClassOf
		fibo-be-oac-opty:Investor ,
		[
			a owl:Restriction ;
			owl:onProperty fibo-fnd-rel-rel:hasIdentity ;
			owl:allValuesFrom fibo-be-le-lp:LegallyCompetentNaturalPerson ;
		]
		;
	rdfs:label "individual investor" ;
	rdfs:isDefinedBy <https://spec.edmcouncil.org/fibo/ontology/SEC/Securities/SecuritiesRestrictions/> ;
	skos:definition "investor that is a person, rather than an organization, who may or may not be considered a qualified investor from a legal perspective" ;
	.

fibo-sec-sec-rst:InstitutionalInvestor
	a owl:Class ;
	rdfs:subClassOf
		fibo-be-oac-opty:Investor ,
		[
			a owl:Restriction ;
			owl:onProperty fibo-fnd-rel-rel:hasIdentity ;
			owl:allValuesFrom fibo-fnd-org-fm:FormalOrganization ;
		]
		;
	rdfs:label "institutional investor" ;
	rdfs:isDefinedBy <https://spec.edmcouncil.org/fibo/ontology/SEC/Securities/SecuritiesRestrictions/> ;
	skos:definition "investor that is an organization that trades large volumes of securities" ;
	skos:example "Example institutional investors include banks, insurance companies, mutual funds, pension funds, and other similar large funds." ;
	fibo-fnd-utl-av:explanatoryNote "Typically more than 70 percent of the daily trading on the New York Stock Exchange is conducted on behalf of institutional investors." ;
	.

fibo-sec-sec-rst:InvestorsDomicileRestriction
	a owl:Class ;
	rdfs:subClassOf fibo-sec-sec-rst:LegalHoldingRestriction ;
	rdfs:label "investors' domicile restriction" ;
	rdfs:isDefinedBy <https://spec.edmcouncil.org/fibo/ontology/SEC/Securities/SecuritiesRestrictions/> ;
	skos:definition "legal holding restriction that specifies where holders of a security may be domiciled" ;
	.

fibo-sec-sec-rst:LegalHoldingRestriction
	a owl:Class ;
	rdfs:subClassOf fibo-sec-sec-rst:SecuritiesRestriction ;
	rdfs:label "legal holding restriction" ;
	rdfs:isDefinedBy <https://spec.edmcouncil.org/fibo/ontology/SEC/Securities/SecuritiesRestrictions/> ;
	skos:definition "security restriction applicable to holding the security" ;
	.

fibo-sec-sec-rst:QualifiedInvestorRestriction
	a owl:Class ;
	rdfs:subClassOf
		fibo-sec-sec-rst:LegalHoldingRestriction ,
		[
			a owl:Restriction ;
			owl:onProperty fibo-sec-sec-rst:hasHoldingPeriod ;
			owl:allValuesFrom fibo-fnd-dt-fd:DatePeriod ;
		]
		;
	rdfs:label "qualified investor restriction" ;
	rdfs:isDefinedBy <https://spec.edmcouncil.org/fibo/ontology/SEC/Securities/SecuritiesRestrictions/> ;
	skos:definition "legal holding restriction that defines the concept of a qualified investor for a given purpose and specifies that only such qualified investors may hold the security" ;
	fibo-fnd-utl-av:explanatoryNote "If a holding period is not defined, then the period for which the restriction applies is indefinite." ;
	.

fibo-sec-sec-rst:RegulationS
	a owl:Class ;
	rdfs:subClassOf
		fibo-sec-sec-rst:InvestorsDomicileRestriction ,
		fibo-sec-sec-rst:QualifiedInvestorRestriction ,
		fibo-sec-sec-rst:SecuritiesRegulation ,
		[
			a owl:Restriction ;
			owl:onProperty fibo-fnd-law-jur:appliesIn ;
			owl:hasValue fibo-be-ge-usj:UnitedStatesJurisdiction ;
		]
		;
	rdfs:label "Regulation S" ;
	rdfs:isDefinedBy <https://spec.edmcouncil.org/fibo/ontology/SEC/Securities/SecuritiesRestrictions/> ;
	rdfs:seeAlso
		<https://www.law.cornell.edu/cfr/text/17/230.902> ,
		<https://www.sec.gov/divisions/corpfin/ecfrlinks.shtml>
		;
	skos:definition "securities regulation defining an exemption through which corporations can issue unregistered securities to qualified foreign investors and foreign institutions" ;
	fibo-fnd-utl-av:explanatoryNote "Regulation S covers rules governing offers and sales made outside the United States without registration under the Securities Act of 1933. Created in 1990, this regulation was intended to encourage foreign investors to purchase American stocks in order to increase the liquidity of American markets." ;
	.

fibo-sec-sec-rst:Restriction144A
	a owl:Class ;
	rdfs:subClassOf
		fibo-sec-sec-rst:LegalHoldingRestriction ,
		[
			a owl:Restriction ;
			owl:onProperty fibo-sec-sec-rst:hasHoldingPeriod ;
			owl:allValuesFrom fibo-fnd-dt-fd:DatePeriod ;
		] ,
		[
			a owl:Restriction ;
			owl:onProperty fibo-fnd-law-jur:appliesIn ;
			owl:hasValue fibo-be-ge-usj:UnitedStatesJurisdiction ;
		]
		;
	rdfs:label "Restriction 144-A" ;
	rdfs:isDefinedBy <https://spec.edmcouncil.org/fibo/ontology/SEC/Securities/SecuritiesRestrictions/> ;
	rdfs:seeAlso
		<https://www.law.cornell.edu/cfr/text/17/230.144> ,
		<https://www.sec.gov/divisions/corpfin/ecfrlinks.shtml>
		;
	skos:definition "Securities & Exchange Commission rule that establishes specific criteria for determining whether a person is not engaged in a distribution and creates a safe harbor from the Section 2(a)(11) definition of 'underwriter'; section A modifies holding period requirements on privately placed securities to permit qualified institutional buyers to trade these positions among themselves" ;
	.

fibo-sec-sec-rst:SecuritiesRegulation
	a owl:Class ;
	rdfs:subClassOf
		fibo-fnd-law-lcap:Regulation ,
		[
			a owl:Restriction ;
			owl:onProperty fibo-fnd-rel-rel:defines ;
			owl:allValuesFrom fibo-sec-sec-rst:SecuritiesRestriction ;
		] ,
		[
			a owl:Restriction ;
			owl:onProperty fibo-fnd-rel-rel:isConferredBy ;
			owl:someValuesFrom fibo-fnd-law-jur:StatuteLaw ;
		]
		;
	rdfs:label "securities regulation" ;
	rdfs:isDefinedBy <https://spec.edmcouncil.org/fibo/ontology/SEC/Securities/SecuritiesRestrictions/> ;
	skos:definition "regulation codified in law specific to securities and investments" ;
	.

fibo-sec-sec-rst:SecuritiesRestriction
	a owl:Class ;
	rdfs:subClassOf
		fibo-fnd-law-lcap:LegalObligation ,
		[
			a owl:Restriction ;
			owl:onProperty fibo-fnd-rel-rel:appliesTo ;
			owl:allValuesFrom [
				a owl:Class ;
				owl:unionOf (
					fibo-fbc-fi-fi:FinancialInstrument
					fibo-sec-sec-lst:Listing
				) ;
			] ;
		] ,
		[
			a owl:Restriction ;
			owl:onProperty fibo-fnd-rel-rel:isMandatedBy ;
			owl:allValuesFrom [
				a owl:Class ;
				owl:unionOf (
					fibo-fnd-law-jur:StatuteLaw
					fibo-sec-sec-rst:SecuritiesRegulation
					fibo-fnd-agr-ctr:Contract
				) ;
			] ;
		]
		;
	rdfs:label "securities restriction" ;
	rdfs:isDefinedBy <https://spec.edmcouncil.org/fibo/ontology/SEC/Securities/SecuritiesRestrictions/> ;
	skos:definition "legal obligation that is applicable to a financial instrument or listing as mandated in a law or by contract" ;
	.

fibo-sec-sec-rst:TradingRestriction
	a owl:Class ;
	rdfs:subClassOf fibo-sec-sec-rst:SecuritiesRestriction ;
	rdfs:label "trading restriction" ;
	rdfs:isDefinedBy <https://spec.edmcouncil.org/fibo/ontology/SEC/Securities/SecuritiesRestrictions/> ;
	skos:definition "restriction that limits trading in some manner, typically summarized on term sheets or in other documentation, including but not limited to restrictions on day trading" ;
	.

fibo-sec-sec-rst:hasHoldingPeriod
	a owl:ObjectProperty ;
	rdfs:subPropertyOf fibo-fnd-dt-fd:hasDatePeriod ;
	rdfs:label "has holding period" ;
	rdfs:isDefinedBy <https://spec.edmcouncil.org/fibo/ontology/SEC/Securities/SecuritiesRestrictions/> ;
	rdfs:range fibo-fnd-dt-fd:DatePeriod ;
	skos:definition "identifies a holding period applicable to some financial asset" ;
	.

fibo-sec-sec-rst:hasRestriction
	a owl:ObjectProperty ;
	rdfs:subPropertyOf lcc-lr:has ;
	rdfs:label "has restriction" ;
	rdfs:isDefinedBy <https://spec.edmcouncil.org/fibo/ontology/SEC/Securities/SecuritiesRestrictions/> ;
	rdfs:range fibo-sec-sec-rst:SecuritiesRestriction ;
	skos:definition "identifies a restriction applicable to a given financial instrument or listing" ;
	.

fibo-sec-sec-rst:isNotClearedIn
	a owl:ObjectProperty ;
	rdfs:label "is not cleared in" ;
	rdfs:domain fibo-sec-sec-rst:BlueSkyLaw ;
	rdfs:isDefinedBy <https://spec.edmcouncil.org/fibo/ontology/SEC/Securities/SecuritiesRestrictions/> ;
	rdfs:range lcc-cr:GeographicRegion ;
	skos:definition "identifies a country subdivision, such as a US state or territory, where an issue is NOT cleared under Blue Sky Restrictions" ;
	skos:editorialNote "This requires review -- shouldn't this be a ternary relation between the regulation, the security and the location?" ;
	.

