# baseURI: https://spec.edmcouncil.org/fibo/ontology/master/2021Q4/FND/Agreements/Agreements/
# imports: https://spec.edmcouncil.org/fibo/ontology/master/2021Q4/FND/Parties/Parties/
# imports: https://spec.edmcouncil.org/fibo/ontology/master/2021Q4/FND/Parties/Roles/
# imports: https://spec.edmcouncil.org/fibo/ontology/master/2021Q4/FND/Relations/Relations/
# imports: https://spec.edmcouncil.org/fibo/ontology/master/2021Q4/FND/Utilities/AnnotationVocabulary/

@base <https://spec.edmcouncil.org/fibo/ontology/master/2021Q4/FND/Agreements/Agreements/> .
@prefix dct: <http://purl.org/dc/terms/> .
@prefix fibo-fnd-agr-agr: <https://spec.edmcouncil.org/fibo/ontology/FND/Agreements/Agreements/> .
@prefix fibo-fnd-pty-pty: <https://spec.edmcouncil.org/fibo/ontology/FND/Parties/Parties/> .
@prefix fibo-fnd-pty-rl: <https://spec.edmcouncil.org/fibo/ontology/FND/Parties/Roles/> .
@prefix fibo-fnd-rel-rel: <https://spec.edmcouncil.org/fibo/ontology/FND/Relations/Relations/> .
@prefix fibo-fnd-utl-av: <https://spec.edmcouncil.org/fibo/ontology/FND/Utilities/AnnotationVocabulary/> .
@prefix lcc-lr: <https://www.omg.org/spec/LCC/Languages/LanguageRepresentation/> .
@prefix owl: <http://www.w3.org/2002/07/owl#> .
@prefix rdf: <http://www.w3.org/1999/02/22-rdf-syntax-ns#> .
@prefix rdfs: <http://www.w3.org/2000/01/rdf-schema#> .
@prefix skos: <http://www.w3.org/2004/02/skos/core#> .
@prefix sm: <http://www.omg.org/techprocess/ab/SpecificationMetadata/> .
@prefix xsd: <http://www.w3.org/2001/XMLSchema#> .

<https://spec.edmcouncil.org/fibo/ontology/FND/Agreements/Agreements/>
	a owl:Ontology ;
	rdfs:label "Agreements Ontology" ;
	dct:abstract "This ontology defines concepts for agreements, for use in other ontology elements. Agreements as defined here are the actual agreements between parties, and this ontology is intended to be referred to in conjunction with the contracts ontology which defines the actual contracts which formalize such agreements. The concepts of agreement and contract are intended to be kept distinct in the FIBO ontologies, that is neither is intended to be regarded as a sub type of the other." ;
	dct:license "http://opensource.org/licenses/MIT"^^xsd:anyURI ;
	sm:contentLanguage "http://www.w3.org/standards/techs/owl#w3c_all"^^xsd:anyURI ;
	sm:copyright
		"Copyright (c) 2013-2020 EDM Council, Inc." ,
		"Copyright (c) 2013-2020 Object Management Group, Inc."
		;
	sm:dependsOn
		"https://spec.edmcouncil.org/fibo/ontology/FND/Parties/Parties/"^^xsd:anyURI ,
		"https://spec.edmcouncil.org/fibo/ontology/FND/Parties/Roles/"^^xsd:anyURI ,
		"https://spec.edmcouncil.org/fibo/ontology/FND/Relations/Relations/"^^xsd:anyURI ,
		"https://spec.edmcouncil.org/fibo/ontology/FND/Utilities/AnnotationVocabulary/"^^xsd:anyURI ,
		"https://www.omg.org/spec/LCC/"^^xsd:anyURI
		;
	sm:fileAbbreviation "fibo-fnd-agr-agr" ;
	sm:filename "Agreements.rdf" ;
	owl:imports
		<https://spec.edmcouncil.org/fibo/ontology/master/2021Q4/FND/Parties/Parties/> ,
		<https://spec.edmcouncil.org/fibo/ontology/master/2021Q4/FND/Parties/Roles/> ,
		<https://spec.edmcouncil.org/fibo/ontology/master/2021Q4/FND/Relations/Relations/> ,
		<https://spec.edmcouncil.org/fibo/ontology/master/2021Q4/FND/Utilities/AnnotationVocabulary/>
		;
	owl:versionIRI <https://spec.edmcouncil.org/fibo/ontology/master/2021Q4/FND/Agreements/Agreements/> ;
	skos:changeNote
		"""The http://www.omg.org/spec/FIBO/Foundations/20130601/Agreements/Agreements.owl version of the ontology was revised in advance of the September 2013 New Brunswick, NJ meeting, as follows:
   (1) to use slash style URI/IRIss (also called 303 URIs, vs. hash style) as required to support server side processing 
   (2) to use version-independent IRIs for all definitions internally as opposed to version-specific IRIs
   (3) to change the file suffix from .owl to .rdf to increase usability in RDF tools
   (4) to use 4-level abbreviations and corresponding namespace prefixes for all FIBO ontologies, reflecting a family/specification/module/ontology structure
   (5) to incorporate changes to the specification metadata to support documentation at the family, specification, module, and ontology level, similar to the abbreviations.
   (6) to revise a few of the definitions based on more formal sources.""" ,
		"The https://spec.edmcouncil.org/fibo/ontology/FND/Agreements/Agreement.rdf version of the ontology was modified per FIBO 2.0 RFC to add general concepts including obligor, obligee, and beneficiary in support of other FIBO domain areas." ,
		"The https://spec.edmcouncil.org/fibo/ontology/FND/Agreements/Agreement.rdf version of the ontology was modified per the issue resolutions identified in the FIBO FND 1.0 FTF report and in https://spec.edmcouncil.org/fibo/ontology/FND/1.0/AboutFND-1.0/." ,
		"The https://spec.edmcouncil.org/fibo/ontology/FND/Agreements/Agreement.rdf version of the ontology was modified per the issue resolutions identified in the FIBO FND 1.1 RTF report and in https://spec.edmcouncil.org/fibo/ontology/FND/1.1/AboutFND-1.1/." ,
		"The https://spec.edmcouncil.org/fibo/ontology/FND/Agreements/Agreement.rdf version of the ontology was modified to eliminate duplication of concepts in LCC."
		;
	fibo-fnd-utl-av:hasMaturityLevel fibo-fnd-utl-av:Release ;
	.

fibo-fnd-agr-agr:Agreement
	a owl:Class ;
	rdfs:subClassOf
		[
			a owl:Restriction ;
			owl:onProperty fibo-fnd-pty-pty:hasPartyInRole ;
			owl:onClass fibo-fnd-pty-pty:PartyInRole ;
			owl:minQualifiedCardinality "2"^^xsd:nonNegativeInteger ;
		] ,
		[
			a owl:Restriction ;
			owl:onProperty fibo-fnd-rel-rel:confers ;
			owl:someValuesFrom fibo-fnd-agr-agr:Commitment ;
		]
		;
	rdfs:label "agreement"@en ;
	rdfs:isDefinedBy <https://spec.edmcouncil.org/fibo/ontology/FND/Agreements/Agreements/> ;
	skos:definition "a negotiated understanding between two or more parties, reflecting the offer and acceptance of commitments on the part of either party" ;
	.

fibo-fnd-agr-agr:Beneficiary
	a owl:Class ;
	rdfs:subClassOf
		fibo-fnd-pty-pty:PartyInRole ,
		[
			a owl:Restriction ;
			owl:onProperty fibo-fnd-pty-rl:isPlayedBy ;
			owl:someValuesFrom [
				a owl:Restriction ;
				owl:onProperty fibo-fnd-pty-pty:isAPartyTo ;
				owl:onClass fibo-fnd-agr-agr:Agreement ;
				owl:minQualifiedCardinality "0"^^xsd:nonNegativeInteger ;
			] ;
		]
		;
	rdfs:label "beneficiary" ;
	rdfs:isDefinedBy <https://spec.edmcouncil.org/fibo/ontology/FND/Agreements/Agreements/> ;
	skos:definition "a party that receives some benefit or advantage or profits from something" ;
	.

fibo-fnd-agr-agr:Commitment
	a owl:Class ;
	rdfs:label "commitment"@en ;
	rdfs:isDefinedBy <https://spec.edmcouncil.org/fibo/ontology/FND/Agreements/Agreements/> ;
	skos:definition "A legal construct which represents the undertaking on the part of some party to act or refrain from acting in some manner." ;
	skos:editorialNote "The undertaking by some party to act or refrain from acting results in an obligation on the part of that party, and usually results in the existence of some corresponding right on the party of some other party, in the event that the commitment is to such party. Thus Obligations and Rights are considered as reciprocal aspects of this Commitment concept." ;
	.

fibo-fnd-agr-agr:CommitmentAtLarge
	a owl:Class ;
	rdfs:subClassOf fibo-fnd-agr-agr:UnilateralCommitment ;
	rdfs:label "commitment at large" ;
	rdfs:isDefinedBy <https://spec.edmcouncil.org/fibo/ontology/FND/Agreements/Agreements/> ;
	skos:definition "a commitment made by some party without direct involvement from the potential beneficiaries of that commitment" ;
	skos:scopeNote "Forms the basis for negotiable securities including transferable contracts and potentially other types of agreement such as software licenses." ;
	.

fibo-fnd-agr-agr:IndividualUnilateralCommitment
	a owl:Class ;
	rdfs:subClassOf fibo-fnd-agr-agr:UnilateralCommitment ;
	rdfs:label "individual unilateral commitment" ;
	rdfs:isDefinedBy <https://spec.edmcouncil.org/fibo/ontology/FND/Agreements/Agreements/> ;
	skos:definition "a commitment made by some party unilaterally to another specific party" ;
	.

fibo-fnd-agr-agr:MutualAgreement
	a owl:Class ;
	rdfs:subClassOf
		fibo-fnd-agr-agr:Agreement ,
		[
			a owl:Restriction ;
			owl:onProperty fibo-fnd-rel-rel:confers ;
			owl:someValuesFrom fibo-fnd-agr-agr:MutualCommitment ;
		]
		;
	rdfs:label "mutual agreement" ;
	rdfs:isDefinedBy <https://spec.edmcouncil.org/fibo/ontology/FND/Agreements/Agreements/> ;
	skos:definition "an agreement between two or more specific named parties. The rights and obligations pertaining to either party cannot be transferred to another party without prior agreement" ;
	skos:scopeNote "This may or may not be a contractual agreement - it also forms the basis of REA transaction models which may or may not refer to contractual agreements, since REA is also used to frame transactions internal to an individual organization." ;
	.

fibo-fnd-agr-agr:MutualCommitment
	a owl:Class ;
	rdfs:subClassOf fibo-fnd-agr-agr:Commitment ;
	rdfs:label "mutual commitment" ;
	rdfs:isDefinedBy <https://spec.edmcouncil.org/fibo/ontology/FND/Agreements/Agreements/> ;
	skos:definition "A commitment between two or more parties" ;
	.

fibo-fnd-agr-agr:Obligee
	a owl:Class ;
	rdfs:subClassOf
		fibo-fnd-pty-pty:PartyInRole ,
		[
			a owl:Restriction ;
			owl:onProperty fibo-fnd-pty-rl:isPlayedBy ;
			owl:someValuesFrom [
				a owl:Restriction ;
				owl:onProperty fibo-fnd-pty-pty:isAPartyTo ;
				owl:onClass fibo-fnd-agr-agr:Agreement ;
				owl:minQualifiedCardinality "0"^^xsd:nonNegativeInteger ;
			] ;
		]
		;
	rdfs:label "obligee" ;
	rdfs:isDefinedBy <https://spec.edmcouncil.org/fibo/ontology/FND/Agreements/Agreements/> ;
	skos:definition "a party to whom some commitment or obligation is owed, either legally or per the terms of an agreement" ;
	.

fibo-fnd-agr-agr:Obligor
	a owl:Class ;
	rdfs:subClassOf
		fibo-fnd-pty-pty:PartyInRole ,
		[
			a owl:Restriction ;
			owl:onProperty fibo-fnd-agr-agr:hasObligation ;
			owl:someValuesFrom fibo-fnd-agr-agr:Commitment ;
		] ,
		[
			a owl:Restriction ;
			owl:onProperty fibo-fnd-pty-rl:isPlayedBy ;
			owl:someValuesFrom [
				a owl:Restriction ;
				owl:onProperty fibo-fnd-pty-pty:isAPartyTo ;
				owl:onClass fibo-fnd-agr-agr:Agreement ;
				owl:minQualifiedCardinality "0"^^xsd:nonNegativeInteger ;
			] ;
		]
		;
	rdfs:label "obligor" ;
	rdfs:isDefinedBy <https://spec.edmcouncil.org/fibo/ontology/FND/Agreements/Agreements/> ;
	skos:definition "a party that is bound legally or by agreement to repay a debt, make a payment, do something, or refrain from doing something" ;
	fibo-fnd-utl-av:synonym
		"obligated party" ,
		"obligator"
		;
	.

fibo-fnd-agr-agr:UnilateralCommitment
	a owl:Class ;
	rdfs:subClassOf fibo-fnd-agr-agr:Commitment ;
	rdfs:label "unilateral commitment" ;
	rdfs:isDefinedBy <https://spec.edmcouncil.org/fibo/ontology/FND/Agreements/Agreements/> ;
	skos:definition "A commitment made by one party without reference to the party to which the commitment is made." ;
	.

fibo-fnd-agr-agr:hasObligation
	a owl:ObjectProperty ;
	rdfs:subPropertyOf lcc-lr:has ;
	rdfs:label "has obligation" ;
	rdfs:domain fibo-fnd-agr-agr:Obligor ;
	rdfs:isDefinedBy <https://spec.edmcouncil.org/fibo/ontology/FND/Agreements/Agreements/> ;
	owl:inverseOf fibo-fnd-agr-agr:isObligationOf ;
	skos:definition "identifies a duty or obligation that a given party has taken on" ;
	.

fibo-fnd-agr-agr:isObligationOf
	a owl:ObjectProperty ;
	rdfs:label "is obligation of" ;
	rdfs:isDefinedBy <https://spec.edmcouncil.org/fibo/ontology/FND/Agreements/Agreements/> ;
	rdfs:range fibo-fnd-agr-agr:Obligor ;
	skos:definition "identifies a party that has a given obligation" ;
	.

